@prefix dc: <http://purl.org/dc/elements/1.1/> .
@prefix foaf: <http://xmlns.com/foaf/0.1/> .
@prefix status: <http://www.w3.org/2003/06/sw-vocab-status/ns#> .
@prefix wo: <http://purl.org/ontology/wo/core#> .
@prefix vann: <http://purl.org/vocab/vann/> .
@prefix dcterms: <http://purl.org/dc/terms/> .
@prefix rdfs: <http://www.w3.org/2000/01/rdf-schema#> .
@prefix time: <http://www.w3.org/2006/time#> .
@prefix ao: <http://purl.org/ontology/ao/core#> .
@prefix cco: <http://purl.org/ontology/cco/core#> .
@prefix event: <http://purl.org/NET/c4dm/event.owl#> .
@prefix xsd: <http://www.w3.org/2001/XMLSchema#> .
@prefix owl: <http://www.w3.org/2002/07/owl#> .
@prefix rdf: <http://www.w3.org/1999/02/22-rdf-syntax-ns#> .
@prefix scovo: <http://purl.org/NET/scovo#> .

<http://purl.org/ontology/cco/core#> a owl:Ontology ;
	dc:creator <http://tobyinkster.co.uk/#i> , "Yan Wang"^^xsd:string , <http://foaf.me/zazi#me> , <http://swordfish.rdfweb.org/people/libby/rdfweb/webwho.xrdf#me> , <http://sw.deri.org/~sheila/foaf.rdf#me> , <http://www.johnbreslin.com/foaf/foaf.rdf#me> , "Yi Zeng"^^xsd:string , "Danica Damljanovic"^^xsd:string , <http://danbri.org/foaf.rdf#danbri> , "Zhisheng Huang"^^xsd:string ;
	dc:date "2010-09-16T10:39:52+01:00"^^xsd:dateTime ;
	dc:description "A vocabulary for describing cognitive pattern within contexts, their temporal dynamics and their origins"@en ;
	dc:title "Cognitive Characteristics Ontology"@en ;
	vann:preferredNamespacePrefix "cco" ;
	vann:preferredNamespaceUri "http://purl.org/ontology/cco/core#" ;
	owl:imports <http://purl.org/NET/scovo> , <http://purl.org/ontology/wo/core> , <http://purl.org/dc/terms/> , <http://purl.org/dc/elements/1.1/> , <http://purl.org/vocab/vann/> , <http://www.w3.org/2006/time> , <http://purl.org/NET/c4dm/event.owl> , <http://www.w3.org/2003/06/sw-vocab-status/ns> , <http://xmlns.com/foaf/0.1/> , <http://purl.org/ontology/ao/core> ;
	owl:versionInfo "0.1"^^xsd:decimal .

cco:CharacteristicDynamics a rdfs:Class , owl:Class ;
	rdfs:comment "An event concept for describing dynamics of characteristics, e.g. weight changes, periods of interest."@en ;
	rdfs:isDefinedBy <http://purl.org/ontology/cco/core#> ;
	rdfs:label "Characteristic Dynamics"@en ;
	rdfs:subClassOf wo:Weight ;
	status:term_status "testing"@en .

cco:CognitiveCharacteristic a owl:Class , rdfs:Class ;
	rdfs:comment "A cognitive characteristic object, which also can have weightings and characteristic dynamics etc. for describing a cognitive pattern."@en ;
	rdfs:isDefinedBy <http://purl.org/ontology/cco/core#> ;
	rdfs:label "Cognitive Characteristic"@en ;
	rdfs:subClassOf scovo:Item ;
	status:term_status "unstable"@en .

cco:ExplicitMining a scovo:Dimension ;
	rdfs:isDefinedBy <http://purl.org/ontology/cco/core#> ;
	dc:description "An explicitly mined cognitive pattern"@en ;
	dc:title "Explicit Mining"@en ;
	status:term_status "testing"@en .

cco:ImplicitMining a scovo:Dimension ;
	rdfs:isDefinedBy <http://purl.org/ontology/cco/core#> ;
	dc:description "An implicitly mined cognitive pattern"@en ;
	dc:title "Implicit Mining"@en ;
	status:term_status "testing"@en .

cco:activity a owl:ObjectProperty , rdf:Property ;
	rdfs:comment "An activity, which is related to a topic of a cognitive charateristic description, e.g. if the topic is football a related activity can be playing or watching."@en ;
	rdfs:domain cco:CognitiveCharacteristic ;
	rdfs:isDefinedBy <http://purl.org/ontology/cco/core#> ;
	rdfs:label "has activity"@en ;
	rdfs:subPropertyOf ao:activity , event:factor ;
	status:term_status "testing"@en .

cco:agent a rdf:Property , owl:ObjectProperty ;
	rdfs:comment "A link from a mined cognitive characteristic to the related person"@en ;
	rdfs:domain cco:CognitiveCharacteristic ;
	rdfs:isDefinedBy <http://purl.org/ontology/cco/core#> ;
	rdfs:label "has agent"@en ;
	rdfs:range foaf:Agent ;
	owl:inverseOf cco:habit ;
	status:term_status "testing"@en .

cco:appear_time a owl:ObjectProperty , rdf:Property ;
	rdfs:comment "The time when the cognitive pattern appears in a certain kind of scenario."@en .

_:node171cnk2ikx1 a owl:Class .

_:node171cnk2ikx2 rdf:first cco:CognitiveCharacteristic ;
	rdf:rest _:node171cnk2ikx3 .

_:node171cnk2ikx3 rdf:first cco:CharacteristicDynamics ;
	rdf:rest rdf:nil .

_:node171cnk2ikx1 owl:unionOf _:node171cnk2ikx2 .

cco:appear_time rdfs:domain _:node171cnk2ikx1 ;
	rdfs:isDefinedBy <http://purl.org/ontology/cco/core#> ;
	rdfs:label "has appear time"@en ;
	rdfs:subPropertyOf event:time ;
	status:term_status "testing"@en .

cco:attention_duration a rdf:Property , owl:ObjectProperty ;
	rdfs:comment "An interval of attention for a cognitive pattern."@en ;
	rdfs:domain cco:CognitiveCharacteristic ;
	rdfs:isDefinedBy <http://purl.org/ontology/cco/core#> ;
	rdfs:label "has attention duration"@en ;
	rdfs:range time:Interval ;
	rdfs:subPropertyOf scovo:dimension , event:time ;
	status:term_status "testing"@en .

cco:belief a owl:ObjectProperty , rdf:Property ;
	rdfs:comment "An uncertain relation for competence representation. That means beliefs, persuasions or opinions, which can also be misconceptions."@en ;
	rdfs:isDefinedBy <http://purl.org/ontology/cco/core#> ;
	rdfs:label "has belief"@en ;
	rdfs:subPropertyOf cco:competence ;
	status:term_status "testing"@en .

cco:characteristic_dynamics a owl:ObjectProperty , rdf:Property ;
	rdfs:comment "To relate a cognitive characteristic to its temporal dynamics."@en ;
	rdfs:domain cco:CognitiveCharacteristic ;
	rdfs:isDefinedBy <http://purl.org/ontology/cco/core#> ;
	rdfs:label "has characteristic dynamics"@en ;
	rdfs:range cco:CharacteristicDynamics ;
	rdfs:subPropertyOf event:sub_event ;
	status:term_status "testing"@en .

cco:cognitive_characteristic a rdf:Property , owl:ObjectProperty ;
	rdfs:comment "This is the super property to describe cognitive characteristics of the user of the cognitive pattern dimension, e.g. interests, skills, or expertise."@en ;
	rdfs:domain foaf:Agent ;
	rdfs:isDefinedBy <http://purl.org/ontology/cco/core#> ;
	rdfs:label "has cognitive characteristic"@en ;
	rdfs:range owl:Thing .

_:node171cnk2ikx4 rdf:first cco:habit ;
	rdf:rest _:node171cnk2ikx5 .

_:node171cnk2ikx5 rdf:first cco:topic ;
	rdf:rest rdf:nil .

cco:cognitive_characteristic owl:propertyChainAxiom _:node171cnk2ikx4 ;
	status:term_status "testing"@en .

cco:competence a owl:ObjectProperty , rdf:Property ;
	rdfs:comment "The competence to (be able to) do or know something. That means abilities, skills, knowledge, expertise, beliefs etc."@en ;
	rdfs:isDefinedBy <http://purl.org/ontology/cco/core#> ;
	rdfs:label "has competence"@en ;
	rdfs:subPropertyOf cco:cognitive_characteristic ;
	status:term_status "testing"@en .

cco:evidence a rdf:Property , owl:ObjectProperty ;
	rdfs:comment "A link between a context and evidence supporting the interpretation of habits in a context"@en .

_:node171cnk2ikx6 a owl:Class .

_:node171cnk2ikx7 rdf:first cco:CognitiveCharacteristic ;
	rdf:rest _:node171cnk2ikx8 .

_:node171cnk2ikx8 rdf:first cco:CharacteristicDynamics ;
	rdf:rest rdf:nil .

_:node171cnk2ikx6 owl:unionOf _:node171cnk2ikx7 .

cco:evidence rdfs:domain _:node171cnk2ikx6 ;
	rdfs:isDefinedBy <http://purl.org/ontology/cco/core#> ;
	rdfs:label "has evidence"@en ;
	rdfs:subPropertyOf event:factor ;
	status:term_status "unstable"@en .

cco:expertise a owl:ObjectProperty , rdf:Property ;
	rdfs:comment "The knowledge or expertise in a certain domain or specific topic, e.g. football, programming languages or music."@en ;
	rdfs:isDefinedBy <http://purl.org/ontology/cco/core#> ;
	rdfs:label "has expertise"@en ;
	rdfs:subPropertyOf cco:competence ;
	status:term_status "testing"@en .

cco:habit a owl:ObjectProperty , rdf:Property ;
	rdfs:comment "A link between an agent and a cognitive characteristic description"@en ;
	rdfs:domain foaf:Agent ;
	rdfs:isDefinedBy <http://purl.org/ontology/cco/core#> ;
	rdfs:label "has habit"@en ;
	rdfs:range cco:CognitiveCharacteristic ;
	status:term_status "unstable"@en .

cco:interest a owl:ObjectProperty , rdf:Property ;
	rdfs:comment "This property relates a certain area of interest or preference to an agent. That means this agent likes this topic somehow."@en ;
	rdfs:isDefinedBy <http://purl.org/ontology/cco/core#> ;
	rdfs:label "has interest"@en ;
	rdfs:subPropertyOf cco:cognitive_characteristic ;
	owl:equivalentProperty foaf:topic_interest ;
	status:term_status "testing"@en .

cco:longest_duration a owl:ObjectProperty , rdf:Property ;
	rdfs:comment "The longest continuous interval of attention for a cognitive pattern, e.g. for an interest, if it appears in the following years: 1990, 1991, 1995, 1996, 1997, 1998, 2001, then the longest duration is 4 years."@en ;
	rdfs:isDefinedBy <http://purl.org/ontology/cco/core#> ;
	rdfs:label "has longest duration"@en ;
	rdfs:subPropertyOf cco:attention_duration ;
	status:term_status "testing"@en .

cco:not_interested_in a rdf:Property , owl:ObjectProperty ;
	rdfs:comment "A link between an agent and a topic of no interest to them"@en ;
	rdfs:domain foaf:Agent ;
	rdfs:isDefinedBy <http://purl.org/ontology/cco/core#> ;
	rdfs:label "is not interested in"@en ;
	rdfs:range owl:Thing ;
	status:term_status "unstable"@en .

cco:overall_weight a owl:ObjectProperty , owl:FunctionalProperty , rdf:Property ;
	rdfs:comment "This weight reflects the overall interest in a topic and should be different from the actual weight of a cognitive characteristic."@en ;
	rdfs:domain cco:CognitiveCharacteristic ;
	rdfs:isDefinedBy <http://purl.org/ontology/cco/core#> ;
	rdfs:label "has overall weight"@en ;
	rdfs:subPropertyOf scovo:dimension , wo:weight ;
	status:term_status "testing"@en .

cco:setting a owl:ObjectProperty , rdf:Property ;
	rdfs:comment "A certain setting or preference. Often re. a specific environment, e.g. an application."@en ;
	rdfs:isDefinedBy <http://purl.org/ontology/cco/core#> ;
	rdfs:label "has setting"@en ;
	rdfs:subPropertyOf cco:cognitive_characteristic ;
	status:term_status "testing"@en .

cco:skill a owl:ObjectProperty , rdf:Property ;
	rdfs:comment "The ability or skill to (be able to) do something, e.g. to walk, to play the piano or to work in a team."@en ;
	rdfs:isDefinedBy <http://purl.org/ontology/cco/core#> ;
	rdfs:label "has skill"@en ;
	rdfs:subPropertyOf cco:competence ;
	status:term_status "testing"@en .

cco:statistical_item a rdf:Property , owl:ObjectProperty ;
	rdfs:comment "A link from a cognitive characteristic to statistics about itself"@en ;
	rdfs:domain cco:CognitiveCharacteristic ;
	rdfs:isDefinedBy <http://purl.org/ontology/cco/core#> ;
	rdfs:label "has statistical item"@en ;
	rdfs:range scovo:Item ;
	status:term_status "testing"@en .

cco:topic a owl:ObjectProperty , rdf:Property ;
	rdfs:comment "A topic of the cognitive characteristic."@en ;
	rdfs:domain cco:CognitiveCharacteristic ;
	rdfs:isDefinedBy <http://purl.org/ontology/cco/core#> ;
	rdfs:label "has topic"@en ;
	rdfs:range owl:Thing ;
	rdfs:subPropertyOf dcterms:subject ;
	status:term_status "unstable"@en .

cco:ultimative_duration a rdf:Property , owl:ObjectProperty ;
	rdfs:comment "The overall duration of attention for a cognitive pattern, e.g. for an interest, if it appears in the following years: 1990, 1991, 1995, 1996, 1997, 1998, 2001, then the longest duration is 7 years."@en ;
	rdfs:isDefinedBy <http://purl.org/ontology/cco/core#> ;
	rdfs:label "has ultimative duration"@en ;
	rdfs:subPropertyOf cco:attention_duration ;
	status:term_status "testing"@en .

_:node171cnk2ikx9 a owl:Class .

_:node171cnk2ikx10 rdf:first cco:CognitiveCharacteristic ;
	rdf:rest _:node171cnk2ikx11 .

_:node171cnk2ikx11 rdf:first cco:CharacteristicDynamics ;
	rdf:rest rdf:nil .

_:node171cnk2ikx9 owl:unionOf _:node171cnk2ikx10 .

cco:appear_time rdfs:domain _:node171cnk2ikx9 .

_:node171cnk2ikx12 rdf:first cco:habit ;
	rdf:rest _:node171cnk2ikx13 .

_:node171cnk2ikx13 rdf:first cco:topic ;
	rdf:rest rdf:nil .

cco:cognitive_characteristic owl:propertyChainAxiom _:node171cnk2ikx12 .

_:node171cnk2ikx14 a owl:Class .

_:node171cnk2ikx15 rdf:first cco:CognitiveCharacteristic ;
	rdf:rest _:node171cnk2ikx16 .

_:node171cnk2ikx16 rdf:first cco:CharacteristicDynamics ;
	rdf:rest rdf:nil .

_:node171cnk2ikx14 owl:unionOf _:node171cnk2ikx15 .

cco:evidence rdfs:domain _:node171cnk2ikx14 .
