@prefix accpol: <http://purl.org/cld/accpol/> .
@prefix dc: <http://purl.org/dc/elements/1.1/> .
@prefix cld: <http://purl.org/cld/terms/> .
@prefix rdfs: <http://www.w3.org/2000/01/rdf-schema#> .
@prefix cdtype: <http://purl.org/cld/cdtype/> .
@prefix freq: <http://purl.org/cld/freq/> .
@prefix dcmitype: <http://purl.org/dc/dcmitype/> .
@prefix rdf: <http://www.w3.org/1999/02/22-rdf-syntax-ns#> .
@prefix dcam: <http://purl.org/dc/dcam/> .
@prefix accmeth: <http://purl.org/cld/accmeth/> .
@prefix skos: <http://www.w3.org/2004/02/skos/core#> .
@prefix dcterms: <http://purl.org/dc/terms/> .

<http://purl.org/cld/terms/> dcterms:title "The Collection Description Terms"@en ;
	dcterms:creator _:node181bqvakpx2 .

_:node181bqvakpx2 rdfs:label "Dublin Core Collection Description Working Group" .

<http://purl.org/cld/terms/> dcterms:modified "2013-06-26"^^dcterms:W3CDTF .

cld:itemType a rdf:Property ;
	rdfs:label "Item Type"@en ;
	rdfs:comment "The nature or genre of the content of one or more items within the collection."@en ;
	rdfs:domain dcmitype:Collection ;
	rdfs:isDefinedBy <http://purl.org/cld/terms/> .

cld:itemFormat a rdf:Property ;
	rdfs:label "Item Format"@en ;
	rdfs:comment "The media type, physical or digital, of one or more items within the collection."@en ;
	rdfs:domain dcmitype:Collection ;
	rdfs:isDefinedBy <http://purl.org/cld/terms/> .

cld:dateItemsCreated a rdf:Property ;
	rdfs:label "Date Items Created"@en ;
	rdfs:comment "A range of dates over which the individual items within the collection were created."@en ;
	rdfs:domain dcmitype:Collection ;
	rdfs:subPropertyOf dc:date ;
	rdfs:isDefinedBy <http://purl.org/cld/terms/> .

cld:isLocatedAt a rdf:Property ;
	rdfs:label "Is Located At"@en ;
	rdfs:comment "A location where the collection is held."@en ;
	rdfs:domain dcmitype:Collection ;
	rdfs:subPropertyOf dc:relation ;
	rdfs:isDefinedBy <http://purl.org/cld/terms/> .

cld:isAccessedVia a rdf:Property ;
	rdfs:label "Is Accessed Via"@en ;
	rdfs:comment "A service that provides access to the items within the collection."@en ;
	rdfs:domain dcmitype:Collection ;
	rdfs:range dcmitype:Service ;
	rdfs:subPropertyOf dc:relation ;
	rdfs:isDefinedBy <http://purl.org/cld/terms/> .

cld:catalogueOrIndex a rdf:Property ;
	rdfs:label "Catalogue or Index"@en ;
	rdfs:comment "A catalogue for, or index of, the collection."@en ;
	rdfs:domain dcmitype:Collection ;
	rdfs:range dcmitype:Collection , cdtype:CatalogueOrIndex ;
	rdfs:subPropertyOf dc:description ;
	rdfs:isDefinedBy <http://purl.org/cld/terms/> .

cld:associatedCollection a rdf:Property ;
	rdfs:label "Associated Collection"@en ;
	rdfs:comment "A second collection that is associated with the current collection."@en ;
	rdfs:domain dcmitype:Collection ;
	rdfs:range dcmitype:Collection ;
	rdfs:subPropertyOf dc:relation ;
	rdfs:isDefinedBy <http://purl.org/cld/terms/> .

cld:describedCollection a rdf:Property ;
	rdfs:label "Described Collection"@en ;
	rdfs:comment "A collection that is described by the current collection."@en ;
	rdfs:domain dcmitype:Collection , cdtype:CatalogueOrIndex ;
	rdfs:range dcmitype:Collection ;
	rdfs:subPropertyOf dc:relation ;
	rdfs:isDefinedBy <http://purl.org/cld/terms/> .

cld:AccrualMethod a dcam:VocabularyEncodingScheme , skos:ConceptScheme ;
	rdfs:label "Collection Description Accrual Method Vocabulary"@en ;
	rdfs:comment "A set of methods by which items are added to a collection."@en ;
	rdfs:seeAlso <http://purl.org/cld/accmeth/> , <http://dublincore.org/groups/collections/accrual-method/> ;
	rdfs:isDefinedBy <http://purl.org/cld/terms/> .

cld:Frequency a dcam:VocabularyEncodingScheme , skos:ConceptScheme ;
	rdfs:label "Collection Description Frequency Vocabulary"@en ;
	rdfs:comment "A set of frequencies with which a repeatable event occurs.."@en ;
	dc:description "The Collection Description Frequency Vocabulary is based on the set of codes used for publication frequency in the MARC 21 Concise Format for Holdings Data."@en ;
	rdfs:seeAlso <http://purl.org/cld/freq/> , <http://dublincore.org/groups/collections/frequency/> , <http://www.loc.gov/marc/holdings/echdcapt.html> ;
	rdfs:isDefinedBy <http://purl.org/cld/terms/> .

cld:AccrualPolicy a dcam:VocabularyEncodingScheme , skos:ConceptScheme ;
	rdfs:label "Collection Description Accrual Policy Vocabulary"@en ;
	rdfs:comment "A set of policies governing the addition of items are added to a collection."@en ;
	rdfs:seeAlso <http://purl.org/cld/accpol/> , <http://dublincore.org/groups/collections/accrual-policy/> ;
	rdfs:isDefinedBy <http://purl.org/cld/terms/> .

cld:RKMS-ISO8601 rdfs:label "Recordkeeping Metadata Schema Extension to ISO8601"@en ;
	rdfs:comment "Instances of this datatype are dates or periods of time represented as literals according to the rules specified in Recordkeeping Metadata Schema Extension to ISO8601."@en ;
	rdfs:seeAlso <http://www.sims.monash.edu.au/research/rcrg/research/spirt/deliver/schemes.html#rkmsextension> ;
	rdfs:isDefinedBy <http://purl.org/cld/terms/> .
