@prefix dc:    <http://purl.org/dc/elements/1.1/> .
@prefix rdfs:  <http://www.w3.org/2000/01/rdf-schema#> .
@prefix foaf:  <http://xmlns.com/foaf/0.1/> .
@prefix fea:   <http://vocab.data.gov/def/fea#> .
@prefix owl:   <http://www.w3.org/2002/07/owl#> .
@prefix xsd:   <http://www.w3.org/2001/XMLSchema#> .
@prefix rdf:   <http://www.w3.org/1999/02/22-rdf-syntax-ns#> .
@prefix vann:  <http://purl.org/vocab/vann/> .

fea:CivilServant  a       owl:Class , rdfs:Class ;
        rdfs:comment      "An employee of the US Government" ;
        rdfs:isDefinedBy  <http://vocab.data.gov/def/fea> ;
        rdfs:label        "Civil Servant" ;
        rdfs:subClassOf   fea:Party .

fea:isPartOf  a           rdf:Property ;
        rdfs:comment      "used to describe part of relationships, such as, for example, the fact that one organization is part of another (departmental hierarchy)." ;
        rdfs:isDefinedBy  <http://vocab.data.gov/def/fea> ;
        rdfs:label        "is part of" .

fea:isComprisedOf  a      rdf:Property ;
        rdfs:isDefinedBy  <http://vocab.data.gov/def/fea> ;
        rdfs:label        "isComprisedOf" .

fea:Technology  a         owl:Class , rdfs:Class ;
        rdfs:comment      "Technology means Information Technology" ;
        rdfs:isDefinedBy  <http://vocab.data.gov/def/fea> ;
        rdfs:label        "Technology" ;
        rdfs:subClassOf   fea:ValuePoint , fea:FEA_TechnologyConcept .

fea:GovernmentBody  a     owl:Class , rdfs:Class ;
        rdfs:comment      "Any US government organization" ;
        rdfs:isDefinedBy  <http://vocab.data.gov/def/fea> ;
        rdfs:label        "Government Body" ;
        rdfs:subClassOf   fea:OrganizationEntity .

fea:FEA_Model  a          owl:Class , rdfs:Class ;
        rdfs:comment      "1, the FEA is being constructed through a collection of interrelated\n“reference models” designed to facilitate cross-agency analysis and the identification of duplicative investments, gaps, and opportunities for collaboration within and across Federal Agencies." ;
        rdfs:isDefinedBy  <http://vocab.data.gov/def/fea> ;
        rdfs:label        "FEA Model" ;
        rdfs:subClassOf   fea:FEA_ArchitectureConcept .

fea:IndustryBody  a       owl:Class , rdfs:Class ;
        rdfs:comment      "Any non government organization" ;
        rdfs:isDefinedBy  <http://vocab.data.gov/def/fea> ;
        rdfs:label        "Industry Body" ;
        rdfs:subClassOf   fea:OrganizationEntity .

fea:StrategicOutcome  a   owl:Class , rdfs:Class ;
        rdfs:comment      "Strategic Outcomes represent broad, policy priorities that drive the direction of government (such as to Secure the Homeland or Expand E-Government).\nPRM volume 1, p.13" ;
        rdfs:isDefinedBy  <http://vocab.data.gov/def/fea> ;
        rdfs:label        "Strategic Outcome" ;
        rdfs:subClassOf   fea:ValuePoint .

fea:Board  a              owl:Class , rdfs:Class ;
        rdfs:comment      "US government board" ;
        rdfs:isDefinedBy  <http://vocab.data.gov/def/fea> ;
        rdfs:label        "Board" ;
        rdfs:subClassOf   fea:GovernmentBody .

fea:hasIntent  a          owl:FunctionalProperty , rdf:Property ;
        rdfs:domain       fea:OrganizationEntity ;
        rdfs:isDefinedBy  <http://vocab.data.gov/def/fea> ;
        rdfs:label        "hasIntent" ;
        rdfs:range        fea:Mission .

fea:date  a               owl:FunctionalProperty , owl:DatatypeProperty , rdf:Property ;
        rdfs:isDefinedBy  <http://vocab.data.gov/def/fea> ;
        rdfs:label        "date" ;
        rdfs:range        xsd:date .

fea:intentOf  a           owl:InverseFunctionalProperty , rdf:Property ;
        rdfs:domain       fea:Mission ;
        rdfs:isDefinedBy  <http://vocab.data.gov/def/fea> ;
        rdfs:label        "intentOf" ;
        rdfs:range        fea:OrganizationEntity .

fea:Partition  a          owl:Class , rdfs:Class ;
        rdfs:comment      "Each reference model has an extensional  property based on partitioning. This reveals implicit semantics in each reference model.\n" ;
        rdfs:isDefinedBy  <http://vocab.data.gov/def/fea> ;
        rdfs:label        "Partition" ;
        rdfs:subClassOf   fea:FEA_ArchitectureConcept .

fea:HumanResource  a      owl:Class , rdfs:Class ;
        rdfs:comment      "This class refers to the workforce" ;
        rdfs:isDefinedBy  <http://vocab.data.gov/def/fea> ;
        rdfs:label        "Human Resource" ;
        rdfs:subClassOf   fea:Resource .

fea:supportedBy  a        rdf:Property ;
        rdfs:isDefinedBy  <http://vocab.data.gov/def/fea> ;
        rdfs:label        "supportedBy" .

fea:Agency  a             owl:Class , rdfs:Class ;
        rdfs:comment      "An agency of the US government" ;
        rdfs:isDefinedBy  <http://vocab.data.gov/def/fea> ;
        rdfs:label        "Agency" ;
        rdfs:subClassOf   fea:ValuePoint , fea:GovernmentBody .

fea:Council  a            owl:Class , rdfs:Class ;
        rdfs:comment      "US Government council" ;
        rdfs:isDefinedBy  <http://vocab.data.gov/def/fea> ;
        rdfs:label        "Council" ;
        rdfs:subClassOf   fea:GovernmentBody .

fea:Process  a            owl:Class , rdfs:Class ;
        rdfs:comment      "The BRM includes a Mode of Delivery Business Area that is designed to identify at a very high level the process that is being used to achieve an intended purpose.\nPRM volume 1, p.16" ;
        rdfs:isDefinedBy  <http://vocab.data.gov/def/fea> ;
        rdfs:label        "Process" ;
        rdfs:subClassOf   fea:ValuePoint .

fea:FEA_Concept  a        owl:Class , rdfs:Class ;
        rdfs:isDefinedBy  <http://vocab.data.gov/def/fea> ;
        rdfs:label        "FEA Concept" .

fea:Party  a              owl:Class , rdfs:Class ;
        rdfs:isDefinedBy  <http://vocab.data.gov/def/fea> ;
        rdfs:label        "Party" ;
        rdfs:subClassOf   fea:FEA_EnterpriseConcept , fea:Customer .

fea:undertakenBy  a       rdf:Property ;
        rdfs:domain       fea:IT_Initiative ;
        rdfs:isDefinedBy  <http://vocab.data.gov/def/fea> ;
        rdfs:label        "undertakenBy" ;
        rdfs:range        fea:Agency .

fea:FEA_ArchitectureConcept
        a                 owl:Class , rdfs:Class ;
        rdfs:isDefinedBy  <http://vocab.data.gov/def/fea> ;
        rdfs:label        "FEA Architecture Concept" ;
        rdfs:subClassOf   fea:FEA_Concept .

<http://vocab.data.gov/def/fea>
        a                              owl:Ontology ;
        dc:creator                     fea: ;
        dc:modified                    "2014-11-21"^^xsd:date ;
        dc:title                       "FEA Vocabulary" ;
        vann:preferredNamespacePrefix  "fea" ;
        vann:preferredNamespaceUri     "http://vocab.data.gov/def/fea#" ;
        foaf:page                      <http://vocab.data.gov/def/fea.html> .

fea:Company  a            owl:Class , rdfs:Class ;
        rdfs:comment      "A commercial organization" ;
        rdfs:isDefinedBy  <http://vocab.data.gov/def/fea> ;
        rdfs:label        "Company" ;
        rdfs:subClassOf   fea:IndustryBody .

fea:description  a        owl:FunctionalProperty , owl:DatatypeProperty , rdf:Property ;
        rdfs:domain       fea:FEA_Concept ;
        rdfs:isDefinedBy  <http://vocab.data.gov/def/fea> ;
        rdfs:label        "description" ;
        rdfs:range        xsd:string .

fea:Mission  a            owl:Class , rdfs:Class ;
        rdfs:comment      "Missions are carried out by the organizational entities" ;
        rdfs:isDefinedBy  <http://vocab.data.gov/def/fea> ;
        rdfs:label        "Mission" ;
        rdfs:subClassOf   fea:FEA_EnterpriseConcept .

fea:IndependentAgency
        a                 owl:Class , rdfs:Class ;
        rdfs:comment      "Independent Agency of the US government" ;
        rdfs:isDefinedBy  <http://vocab.data.gov/def/fea> ;
        rdfs:label        "Independent Agency" ;
        rdfs:subClassOf   fea:Agency .

fea:QuasiOfficialAgency
        a                 owl:Class , rdfs:Class ;
        rdfs:comment      "Quasi Official Agency of the US government" ;
        rdfs:isDefinedBy  <http://vocab.data.gov/def/fea> ;
        rdfs:label        "Quasi Official Agency" ;
        rdfs:subClassOf   fea:Agency .

fea:OrganizationEntity
        a                 owl:Class , rdfs:Class ;
        rdfs:isDefinedBy  <http://vocab.data.gov/def/fea> ;
        rdfs:label        "Organization Entity" ;
        rdfs:subClassOf   fea:Party .

fea:Customer  a           owl:Class , rdfs:Class ;
        rdfs:comment      "The diverse nature of federal programs means that there are many customers spanning the citizen, business, other government, and internal categories.  Some customers\nreceive direct government services, such as veterans receiving health care from the Veterans Health Administration. Other “customers” are those subject to regulatory activities, such as large businesses conforming to safety regulations administered by the Occupational Safety and Health Administration. Importantly, the citizen is generally considered to be the ultimate “customer” of government activities regardless of the nature of the customer relationship.\nPRM volume 1, p.14" ;
        rdfs:isDefinedBy  <http://vocab.data.gov/def/fea> ;
        rdfs:label        "Customer" ;
        rdfs:subClassOf   fea:ValuePoint .

fea:Budget  a             owl:Class , rdfs:Class ;
        rdfs:isDefinedBy  <http://vocab.data.gov/def/fea> ;
        rdfs:label        "Budget" ;
        rdfs:subClassOf   fea:FEA_EnterpriseConcept .

fea:ValuePoint  a         owl:Class , rdfs:Class ;
        rdfs:comment      "The point at which value is measured." ;
        rdfs:isDefinedBy  <http://vocab.data.gov/def/fea> ;
        rdfs:label        "ValuePoint" ;
        rdfs:subClassOf   fea:FEA_EnterpriseConcept .

fea:FEA_EnterpriseConcept
        a                 owl:Class , rdfs:Class ;
        rdfs:isDefinedBy  <http://vocab.data.gov/def/fea> ;
        rdfs:label        "FEA Enterprise Concept" ;
        rdfs:subClassOf   fea:FEA_Concept .

fea:dependsOn  a          rdf:Property ;
        rdfs:domain       fea:Partition ;
        rdfs:isDefinedBy  <http://vocab.data.gov/def/fea> ;
        rdfs:label        "dependsOn" ;
        rdfs:range        fea:Partition .

fea:    a       foaf:Person .

fea:FEA_TechnologyConcept
        a                 owl:Class , rdfs:Class ;
        rdfs:isDefinedBy  <http://vocab.data.gov/def/fea> ;
        rdfs:label        "FEA Technology Concept" ;
        rdfs:subClassOf   fea:FEA_Concept .

fea:Commission  a         owl:Class , rdfs:Class ;
        rdfs:comment      "Us government commission" ;
        rdfs:isDefinedBy  <http://vocab.data.gov/def/fea> ;
        rdfs:label        "Commission" ;
        rdfs:subClassOf   fea:GovernmentBody .

fea:ExecutiveAgency  a    owl:Class , rdfs:Class ;
        rdfs:comment      "Executive Agency of the US government" ;
        rdfs:isDefinedBy  <http://vocab.data.gov/def/fea> ;
        rdfs:label        "Executive Agency" ;
        rdfs:subClassOf   fea:Agency .

fea:IT_Initiative  a      owl:Class , rdfs:Class ;
        rdfs:comment      "A program of work that implements information technology based capabilities." ;
        rdfs:isDefinedBy  <http://vocab.data.gov/def/fea> ;
        rdfs:label        "IT Initiative" ;
        rdfs:subClassOf   fea:FEA_EnterpriseConcept .

fea:FederalEnterpriseArchitecture
        a                 owl:Class , rdfs:Class ;
        rdfs:comment      "To facilitate efforts to transform the Federal Government to one that is citizen-centered, results-oriented, and market-based, the Office of Management and Budget (OMB) is developing the Federal Enterprise Architecture (FEA), a business-based framework for Governmentwide improvement." ;
        rdfs:isDefinedBy  <http://vocab.data.gov/def/fea> ;
        rdfs:label        "Federal Enterprise Architecture" ;
        rdfs:subClassOf   fea:FEA_ArchitectureConcept .

fea:undertakes  a         rdf:Property ;
        rdfs:domain       fea:Agency ;
        rdfs:isDefinedBy  <http://vocab.data.gov/def/fea> ;
        rdfs:label        "undertakes" ;
        rdfs:range        fea:IT_Initiative .

fea:Resource  a           owl:Class , rdfs:Class ;
        rdfs:isDefinedBy  <http://vocab.data.gov/def/fea> ;
        rdfs:label        "Resource" ;
        rdfs:subClassOf   fea:ValuePoint .

fea:Standard  a           owl:Class , rdfs:Class ;
        rdfs:comment      "Technology standard" ;
        rdfs:isDefinedBy  <http://vocab.data.gov/def/fea> ;
        rdfs:label        "Standard" ;
        rdfs:subClassOf   fea:FEA_TechnologyConcept .

fea:OtherFixedAsset  a    owl:Class , rdfs:Class ;
        rdfs:comment      "This class includes any fixed assets such as vehicle fleets, facilities and other equipment." ;
        rdfs:isDefinedBy  <http://vocab.data.gov/def/fea> ;
        rdfs:label        "Other Fixed Asset" ;
        rdfs:subClassOf   fea:Resource .

fea:buildsOn  a           rdf:Property ;
        rdfs:domain       fea:Partition ;
        rdfs:isDefinedBy  <http://vocab.data.gov/def/fea> ;
        rdfs:label        "buildsOn" ;
        rdfs:range        fea:Partition .

fea:Office  a             owl:Class , rdfs:Class ;
        rdfs:comment      "US government office" ;
        rdfs:isDefinedBy  <http://vocab.data.gov/def/fea> ;
        rdfs:label        "Office" ;
        rdfs:subClassOf   fea:GovernmentBody .

fea:Citizen  a            owl:Class , rdfs:Class ;
        rdfs:comment      "Citizen of the United States of Americe" ;
        rdfs:isDefinedBy  <http://vocab.data.gov/def/fea> ;
        rdfs:label        "Citizen" ;
        rdfs:subClassOf   fea:Party .

fea:drawsUpon  a          rdf:Property ;
        rdfs:domain       fea:FEA_Model ;
        rdfs:isDefinedBy  <http://vocab.data.gov/def/fea> ;
        rdfs:label        "drawsUpon" ;
        rdfs:range        fea:FEA_Model .

fea:comprises  a          rdf:Property ;
        rdfs:isDefinedBy  <http://vocab.data.gov/def/fea> ;
        rdfs:label        "comprises" .

fea:allignedWith  a       rdf:Property ;
        rdfs:isDefinedBy  <http://vocab.data.gov/def/fea> ;
        rdfs:label        "allignedWith" .

fea:mnemonic  a           owl:DatatypeProperty , rdf:Property ;
        rdfs:domain       fea:FEA_Concept ;
        rdfs:isDefinedBy  <http://vocab.data.gov/def/fea> ;
        rdfs:label        "mnemonic" ;
        rdfs:range        xsd:string .
