@prefix dc: <http://purl.org/dc/elements/1.1/> .
@prefix rdfs: <http://www.w3.org/2000/01/rdf-schema#> .
@prefix owl: <http://www.w3.org/2002/07/owl#> .
@prefix rdf: <http://www.w3.org/1999/02/22-rdf-syntax-ns#> .
@prefix gold: <http://purl.org/linguistics/gold/> .
@prefix bibliography: <http://www.linguistics-ontology.org/bibliography/bibliography.owl#> .

_:node172f9vp6jx1 a owl:Ontology ;
	dc:identifier "http://purl.org/linguistics/gold" ;
	owl:versionInfo "2008" ;
	dc:title "Genderal Ontology for Linguistic Description" ;
	dc:description "This is the General Ontology for Linguistic Description (GOLD) described using the Web Ontology Language. This ontology was created primarily for applications involving descriptive linguistics." , "" ;
	dc:creator "Scott Farrar" , "D. Terence Langendoen" ;
	dc:contributor "Anthony Aristar" , "Helen Aristar-Dry" , "Dunstan Brown" , "Greville Corbett" , "Anna Kibort" , "William D. Lewis" , "Steven Moran" , "Gary Simons" .

gold:acousticRealization a owl:ObjectProperty ;
	rdfs:label "acousticRealization"@eng ;
	rdfs:subPropertyOf gold:realization ;
	rdfs:isDefinedBy "http://purl.org/linguistics/gold"^^<http://www.w3.org/2001/XMLSchema#anyURI> ;
	rdfs:comment "The relation between some linguistic unit and its corresponding spoken expression."@eng ;
	rdfs:domain gold:LinguisticUnit ;
	rdfs:range gold:SpokenLinguisticExpression .

gold:adjunct a owl:ObjectProperty ;
	rdfs:label "adjunct"@eng ;
	rdfs:subPropertyOf gold:hasSyntacticConstituent ;
	rdfs:isDefinedBy "http://purl.org/linguistics/gold"^^<http://www.w3.org/2001/XMLSchema#anyURI> .

gold:agent a owl:ObjectProperty ;
	rdfs:label "agent"@eng ;
	rdfs:subPropertyOf gold:semanticRole ;
	rdfs:isDefinedBy "http://purl.org/linguistics/gold"^^<http://www.w3.org/2001/XMLSchema#anyURI> .

gold:agrees a owl:ObjectProperty ;
	rdfs:label "agrees"@eng ;
	rdfs:isDefinedBy "http://purl.org/linguistics/gold"^^<http://www.w3.org/2001/XMLSchema#anyURI> ;
	rdfs:comment "A relation holding between syntactic units, often manifesting itself in shared form features. NOTE: this could be better defined once syntactic roles and relations are developed."@eng .

gold:allomorph a owl:ObjectProperty ;
	rdfs:label "allomorph"@eng ;
	rdfs:isDefinedBy "http://purl.org/linguistics/gold"^^<http://www.w3.org/2001/XMLSchema#anyURI> ;
	rdfs:comment "The relation that holds between a morpheme and one of its morphs, an occurrence of a morpheme in context."@eng .

gold:allophone a owl:ObjectProperty ;
	rdfs:label "allophone"@eng ;
	rdfs:isDefinedBy "http://purl.org/linguistics/gold"^^<http://www.w3.org/2001/XMLSchema#anyURI> ;
	rdfs:comment "The relation that holds between a phoneme and one of its phones, an occurrence of a phoneme in context."@eng .

gold:ancestorVariety a owl:ObjectProperty ;
	rdfs:label "ancestorVariety"@eng ;
	rdfs:isDefinedBy "http://purl.org/linguistics/gold"^^<http://www.w3.org/2001/XMLSchema#anyURI> ;
	rdfs:comment "ancestorVariety is the predicate expressing the basic diachronic relationship  between a language variety that existed some time in the past and a variety existing at a later time  such that the  former has evolved into the latter through regular language change."@eng ;
	rdfs:domain gold:HumanLanguageVariety ;
	rdfs:range gold:HumanLanguageVariety .

gold:antonym a owl:ObjectProperty ;
	rdfs:label "antonym"@eng ;
	rdfs:subPropertyOf gold:lexicalRelation ;
	rdfs:isDefinedBy "http://purl.org/linguistics/gold"^^<http://www.w3.org/2001/XMLSchema#anyURI> ;
	rdfs:comment "antonym"@eng .

gold:argument a owl:ObjectProperty ;
	rdfs:label "argument"@eng ;
	rdfs:subPropertyOf gold:syntacticRole ;
	rdfs:isDefinedBy "http://purl.org/linguistics/gold"^^<http://www.w3.org/2001/XMLSchema#anyURI> ;
	rdfs:comment "The syntactic entity about which something is predicated."@eng ;
	rdfs:range gold:Clause .

gold:circumscribes a owl:ObjectProperty ;
	rdfs:label "circumscribes"@eng ;
	rdfs:subPropertyOf gold:morphologicalRelation ;
	rdfs:isDefinedBy "http://purl.org/linguistics/gold"^^<http://www.w3.org/2001/XMLSchema#anyURI> ;
	rdfs:comment "NOTE: still lacks development. This relation holds between two form units and represents the notion of circumscription in a morphosyntactic system. That is, (circumscribes A B) means that part of A comes before B and part of A comes after B, in the linearization of the units of a language."@eng .

gold:coda a owl:ObjectProperty ;
	rdfs:label "coda"@eng ;
	rdfs:isDefinedBy "http://purl.org/linguistics/gold"^^<http://www.w3.org/2001/XMLSchema#anyURI> ;
	rdfs:comment "The closing segment of a syllable."@eng .

gold:complement a owl:ObjectProperty ;
	rdfs:label "complement"@eng ;
	rdfs:subPropertyOf gold:hasSyntacticConstituent ;
	rdfs:isDefinedBy "http://purl.org/linguistics/gold"^^<http://www.w3.org/2001/XMLSchema#anyURI> .

gold:constituents a owl:ObjectProperty ;
	rdfs:label "constituents"@eng ;
	rdfs:isDefinedBy "http://purl.org/linguistics/gold"^^<http://www.w3.org/2001/XMLSchema#anyURI> ;
	rdfs:comment "The relation holding between a linguistic unit and a list (rdf:Seq) of its constituents."@eng ;
	rdfs:domain gold:LinguisticUnit .

gold:dataStructureRelation a owl:ObjectProperty ;
	rdfs:label "dataStructureRelation"@eng ;
	rdfs:isDefinedBy "http://purl.org/linguistics/gold"^^<http://www.w3.org/2001/XMLSchema#anyURI> ;
	rdfs:comment "This subsumes all structuring relations used for LinguisticDataStructures. As a naming convention to distinguish relations in data structure from other relations, all names of dataStructuringRelations begin with 'has-'."@eng ;
	rdfs:domain gold:LinguisticDataStructure .

gold:derivedForm a owl:ObjectProperty ;
	rdfs:label "derivedForm"@eng ;
	rdfs:isDefinedBy "http://purl.org/linguistics/gold"^^<http://www.w3.org/2001/XMLSchema#anyURI> ;
	rdfs:domain gold:Stem .

gold:directObject a owl:ObjectProperty ;
	rdfs:label "directObject"@eng ;
	rdfs:subPropertyOf gold:object ;
	rdfs:isDefinedBy "http://purl.org/linguistics/gold"^^<http://www.w3.org/2001/XMLSchema#anyURI> ;
	rdfs:comment "A direct object is a grammatical relation that exhibits a combination of certain independent syntactic properties, such as the following:  the usual grammatical characteristics of the patient of typically  transitive verbs; particular case marking; a particular clause  position; the conditioning of an agreement  affix on the verb; the capability of becoming the clause subject in  passivization; the capability of reflexivization. The identification of the direct object relation may be further confirmed by finding significant overlap with similar direct object relations previously established in other languages. This may be done by analyzing correspondence between  translation equivalents [Crystal 1985, 94; Hartmann and Stork 1972, 155; Comrie 1989, 66; Andrews 1985, 68,120,126; Comrie 1985, 337]."@eng .

gold:entailedBy a owl:ObjectProperty ;
	rdfs:label "entailedBy"@eng ;
	rdfs:isDefinedBy "http://purl.org/linguistics/gold"^^<http://www.w3.org/2001/XMLSchema#anyURI> .

gold:entails a owl:ObjectProperty ;
	rdfs:label "entails"@eng ;
	rdfs:isDefinedBy "http://purl.org/linguistics/gold"^^<http://www.w3.org/2001/XMLSchema#anyURI> .

gold:feature a owl:ObjectProperty ;
	rdfs:label "feature"@eng ;
	rdfs:isDefinedBy "http://purl.org/linguistics/gold"^^<http://www.w3.org/2001/XMLSchema#anyURI> ;
	rdfs:comment "The relation between a linguistic unit and a linguistic feature. A feature inheres in its host. NOTE: this relation is distinct from the hasFeature which pertains to data structures."@eng ;
	rdfs:range gold:LinguisticProperty .

gold:follows a owl:ObjectProperty ;
	rdfs:label "follows"@eng ;
	rdfs:subPropertyOf gold:orderingRelation ;
	rdfs:isDefinedBy "http://purl.org/linguistics/gold"^^<http://www.w3.org/2001/XMLSchema#anyURI> ;
	rdfs:comment "This relation holds between two linguistic units and represents the inverse of 'precedes'. That is, (follows A B) means that A comes after B in the linearization of the realization of linguistic signs. The inverse of this relation is 'precedes'."@eng .

gold:freeTranslation a owl:ObjectProperty ;
	rdfs:label "freeTranslation"@eng ;
	rdfs:subPropertyOf gold:translation ;
	rdfs:isDefinedBy "http://purl.org/linguistics/gold"^^<http://www.w3.org/2001/XMLSchema#anyURI> ;
	rdfs:comment "The relation between an orthographic expression in one language and some orthographic expression in another such that both expressions have exactly the same meaning. The words in the translation may not correspond to the those in the source expression."@eng .

gold:geneticallyRelated a owl:ObjectProperty ;
	rdfs:label "geneticallyRelated"@eng ;
	rdfs:isDefinedBy "http://purl.org/linguistics/gold"^^<http://www.w3.org/2001/XMLSchema#anyURI> ;
	rdfs:comment "geneticallyRelated is the basic kinship relation between languages varieties. If two language varieties are genetically related, then this implies that both  varieties are derived from a common  proto-language."@eng ;
	rdfs:domain gold:HumanLanguageVariety ;
	rdfs:range gold:HumanLanguageVariety .

gold:goal a owl:ObjectProperty ;
	rdfs:label "goal"@eng ;
	rdfs:subPropertyOf gold:semanticRole ;
	rdfs:isDefinedBy "http://purl.org/linguistics/gold"^^<http://www.w3.org/2001/XMLSchema#anyURI> .

gold:hasComplexValue a owl:ObjectProperty ;
	rdfs:label "hasComplexValue"@eng ;
	rdfs:subPropertyOf gold:dataStructureRelation ;
	rdfs:isDefinedBy "http://purl.org/linguistics/gold"^^<http://www.w3.org/2001/XMLSchema#anyURI> ;
	rdfs:comment "This relates a ComplexSpecification to a FeatureStructure, thus giving a FeatureStructure its recursive properties."@eng ;
	rdfs:domain gold:ComplexSpecification ;
	rdfs:range gold:FeatureStructure .

gold:hasConstituent a owl:ObjectProperty ;
	rdfs:label "hasConstituent"@eng ;
	rdfs:isDefinedBy "http://purl.org/linguistics/gold"^^<http://www.w3.org/2001/XMLSchema#anyURI> ;
	rdfs:comment "The relation hasConstituent is an abstract partial ordering relation that expresses dominance between two linguistic units. This relation is meant to cover all possible types of linguistic constituency: phonological, morphological, syntactic, etc. constituency."@eng ;
	rdfs:domain gold:LinguisticUnit ;
	rdfs:range gold:LinguisticUnit .

gold:hasConstraint a owl:ObjectProperty ;
	rdfs:label "hasConstraint"@eng ;
	rdfs:subPropertyOf gold:dataStructureRelation ;
	rdfs:isDefinedBy "http://purl.org/linguistics/gold"^^<http://www.w3.org/2001/XMLSchema#anyURI> ;
	rdfs:comment "This relates a FeatureSystem to a FeatureContraint."@eng ;
	rdfs:domain gold:FeatureSystem ;
	rdfs:range gold:FeatureConstraint .

gold:hasFeature a owl:ObjectProperty ;
	rdfs:label "hasFeature"@eng ;
	rdfs:subPropertyOf gold:dataStructureRelation ;
	rdfs:isDefinedBy "http://purl.org/linguistics/gold"^^<http://www.w3.org/2001/XMLSchema#anyURI> ;
	rdfs:comment "This relates a FeatureSpecification to a type of LinguisticProperty."@eng ;
	rdfs:domain gold:FeatureSpecification .

gold:hasForm a owl:ObjectProperty ;
	rdfs:label "hasForm"@eng ;
	rdfs:isDefinedBy "http://purl.org/linguistics/gold"^^<http://www.w3.org/2001/XMLSchema#anyURI> ;
	rdfs:comment "The relation that associates some LinguisticSign with its FormUnit."@eng ;
	rdfs:domain gold:LinguisticSign ;
	rdfs:range gold:FormUnit .

gold:hasGlosses a owl:ObjectProperty ;
	rdfs:label "hasGlosses"@eng ;
	rdfs:subPropertyOf gold:dataStructureRelation ;
	rdfs:isDefinedBy "http://purl.org/linguistics/gold"^^<http://www.w3.org/2001/XMLSchema#anyURI> ;
	rdfs:comment "The binary relation holding between an instance of interlinear glossed text (IGT) and a sequence of labels or 'grams' used to describe the morphemes of the IGT."@eng .

gold:hasGrammar a owl:ObjectProperty ;
	rdfs:label "hasGrammar"@eng ;
	rdfs:isDefinedBy "http://purl.org/linguistics/gold"^^<http://www.w3.org/2001/XMLSchema#anyURI> ;
	rdfs:comment "The relation that holds between a LinguisticSign and a GrammaticalUnit."@eng ;
	rdfs:domain gold:LinguisticSign ;
	rdfs:range gold:GrammarUnit .

gold:hasLexicalItem a owl:ObjectProperty ;
	rdfs:label "hasLexicalItem"@eng ;
	rdfs:subPropertyOf gold:dataStructureRelation ;
	rdfs:isDefinedBy "http://purl.org/linguistics/gold"^^<http://www.w3.org/2001/XMLSchema#anyURI> ;
	rdfs:comment "The relation between a Lexicon and its contents, instances of LexicalItem. NOTE: this could probably be replaced by the memberOf relation from set theory."@eng ;
	rdfs:domain gold:Lexicon ;
	rdfs:range gold:LexicalItem .

gold:hasLexicalUnit a owl:ObjectProperty ;
	rdfs:label "hasLexicalUnit"@eng ;
	rdfs:subPropertyOf gold:dataStructureRelation ;
	rdfs:isDefinedBy "http://purl.org/linguistics/gold"^^<http://www.w3.org/2001/XMLSchema#anyURI> ;
	rdfs:comment "This relates a LexicalItem to a LexicalUnit, those elements commonly represented in a dictionary."@eng ;
	rdfs:domain gold:LexicalItem .

gold:hasMeaning a owl:ObjectProperty ;
	rdfs:label "hasMeaning"@eng ;
	rdfs:isDefinedBy "http://purl.org/linguistics/gold"^^<http://www.w3.org/2001/XMLSchema#anyURI> ;
	rdfs:comment "The relation that associates some LinguisticSign with a SemanticUnit."@eng ;
	rdfs:domain gold:LinguisticSign ;
	rdfs:range gold:SemanticUnit .

gold:hasMorphologicalConstituent a owl:ObjectProperty ;
	rdfs:label "hasMorphologicalConstituent"@eng ;
	rdfs:subPropertyOf gold:hasConstituent ;
	rdfs:isDefinedBy "http://purl.org/linguistics/gold"^^<http://www.w3.org/2001/XMLSchema#anyURI> ;
	rdfs:comment "The relation hasMorphologicalConstituent is an abstract partial ordering relation that expresses dominance between two morphological units. This relation is meant to cover all possible types of morphological constituency."@eng ;
	rdfs:domain gold:MorphologicalUnit ;
	rdfs:range gold:MorphologicalUnit .

gold:hasProperty a owl:ObjectProperty ;
	rdfs:label "hasProperty"@eng ;
	rdfs:isDefinedBy "http://purl.org/linguistics/gold"^^<http://www.w3.org/2001/XMLSchema#anyURI> ;
	rdfs:comment "The relation between a linguistic unit and a linguistic property, e.g., (m1 hasProperty AllativeCase) where m1 is an instance of Morpheme."@eng ;
	rdfs:domain gold:LinguisticSign ;
	rdfs:range gold:LinguisticProperty .

gold:hasSourceLine a owl:ObjectProperty ;
	rdfs:label "hasSourceLine"@eng ;
	rdfs:subPropertyOf gold:dataStructureRelation ;
	rdfs:isDefinedBy "http://purl.org/linguistics/gold"^^<http://www.w3.org/2001/XMLSchema#anyURI> ;
	rdfs:comment "The binary relation holding between an instance of interlinear glossed text and a linguistic unit (clause, phrase, etc.) from the source language."@eng .

gold:hasSpecification a owl:ObjectProperty ;
	rdfs:label "hasSpecification"@eng ;
	rdfs:subPropertyOf gold:dataStructureRelation ;
	rdfs:isDefinedBy "http://purl.org/linguistics/gold"^^<http://www.w3.org/2001/XMLSchema#anyURI> ;
	rdfs:comment "This relates a FeatureStructure to a FeatureSpecification."@eng ;
	rdfs:domain gold:FeatureStructure ;
	rdfs:range gold:FeatureSpecification .

gold:hasSyntacticConstituent a owl:ObjectProperty ;
	rdfs:label "hasSyntacticConstituent"@eng ;
	rdfs:subPropertyOf gold:hasConstituent ;
	rdfs:isDefinedBy "http://purl.org/linguistics/gold"^^<http://www.w3.org/2001/XMLSchema#anyURI> ;
	rdfs:comment "The relation hasSyntacticConstituent is an abstract partial ordering relation that expresses dominance between two syntactic units. This relation is meant to cover all possible types of syntactic constituency."@eng ;
	rdfs:domain gold:SyntacticUnit ;
	rdfs:range gold:SyntacticUnit .

gold:hasTerm a owl:ObjectProperty ;
	rdfs:label "hasTerm"@eng ;
	rdfs:isDefinedBy "http://purl.org/linguistics/gold"^^<http://www.w3.org/2001/XMLSchema#anyURI> ;
	rdfs:comment "The relation between some Termset and a Term."@eng ;
	rdfs:domain gold:Termset ;
	rdfs:range gold:Term .

gold:hasTranslationLine a owl:ObjectProperty ;
	rdfs:label "hasTranslationLine"@eng ;
	rdfs:subPropertyOf gold:dataStructureRelation ;
	rdfs:isDefinedBy "http://purl.org/linguistics/gold"^^<http://www.w3.org/2001/XMLSchema#anyURI> ;
	rdfs:comment "The binary relation holding between an instance of interlinear glossed text and a linguistic unit (clause, phrase, etc.) acting as a free translation of the source text from the IGT instance."@eng .

gold:hasType a owl:ObjectProperty ;
	rdfs:label "hasType"@eng ;
	rdfs:subPropertyOf gold:dataStructureRelation ;
	rdfs:isDefinedBy "http://purl.org/linguistics/gold"^^<http://www.w3.org/2001/XMLSchema#anyURI> ;
	rdfs:comment "This relates either a FeatureStructure or a FeatureConstraint to its type, expressed by an instance of PartOfSpeech."@eng ;
	rdfs:domain gold:FeatureStructure .

gold:head a owl:ObjectProperty ;
	rdfs:label "head"@eng ;
	rdfs:subPropertyOf gold:hasSyntacticConstituent ;
	rdfs:isDefinedBy "http://purl.org/linguistics/gold"^^<http://www.w3.org/2001/XMLSchema#anyURI> ;
	rdfs:range gold:Phrase .

gold:hypernym a owl:ObjectProperty ;
	rdfs:label "hypernym"@eng ;
	rdfs:subPropertyOf gold:lexicalRelation ;
	rdfs:isDefinedBy "http://purl.org/linguistics/gold"^^<http://www.w3.org/2001/XMLSchema#anyURI> ;
	rdfs:comment "hypernym"@eng .

gold:inLanguage a owl:ObjectProperty ;
	rdfs:label "inLanguage"@eng ;
	rdfs:isDefinedBy "http://purl.org/linguistics/gold"^^<http://www.w3.org/2001/XMLSchema#anyURI> ;
	rdfs:comment "The relation that holds between a LinguisticSign and a Language. The sign is said to be a member or part of that language."@eng ;
	rdfs:domain gold:LinguisticUnit ;
	rdfs:range gold:HumanLanguageVariety .

gold:indirectObject a owl:ObjectProperty ;
	rdfs:label "indirectObject"@eng ;
	rdfs:subPropertyOf gold:object ;
	rdfs:isDefinedBy "http://purl.org/linguistics/gold"^^<http://www.w3.org/2001/XMLSchema#anyURI> .

gold:infixedIn a owl:ObjectProperty ;
	rdfs:label "infixedIn"@eng ;
	rdfs:subPropertyOf gold:morphologicalRelation ;
	rdfs:isDefinedBy "http://purl.org/linguistics/gold"^^<http://www.w3.org/2001/XMLSchema#anyURI> ;
	rdfs:comment "infixedIn is the relation between a Lexical- or SublexicalUnit and a Root. The Root is realized as discontinuous, surrounding the inserted Lexical- or SublexicalUnit [Hartmann and Stork 1972, 111]."@eng .

gold:inflectedForm a owl:ObjectProperty ;
	rdfs:label "inflectedForm"@eng ;
	rdfs:isDefinedBy "http://purl.org/linguistics/gold"^^<http://www.w3.org/2001/XMLSchema#anyURI> ;
	rdfs:domain gold:Stem .

gold:labels a owl:ObjectProperty ;
	rdfs:label "labels"@eng ;
	rdfs:isDefinedBy "http://purl.org/linguistics/gold"^^<http://www.w3.org/2001/XMLSchema#anyURI> ;
	rdfs:comment "This relation names or simply associates some SymbolicString with any Entity."@eng .

gold:lexicalRelation a owl:ObjectProperty ;
	rdfs:label "lexicalRelation"@eng ;
	rdfs:isDefinedBy "http://purl.org/linguistics/gold"^^<http://www.w3.org/2001/XMLSchema#anyURI> ;
	rdfs:comment "This is the superclass of common lexical relatations such as synonym, antonym, etc. NOTE: this needs work. Such relations really pertain to meaning and not form units."@eng .

gold:literalTranslation a owl:ObjectProperty ;
	rdfs:label "literalTranslation"@eng ;
	rdfs:subPropertyOf gold:translation ;
	rdfs:isDefinedBy "http://purl.org/linguistics/gold"^^<http://www.w3.org/2001/XMLSchema#anyURI> ;
	rdfs:comment "The relation between an orthographic expression in one language and some orthographic expression in another such that the translation is done on a word by word, or morpheme by morpheme, basis without regard for idiomatic usage."@eng .

gold:meronym a owl:ObjectProperty ;
	rdfs:label "meronym"@eng ;
	rdfs:subPropertyOf gold:lexicalRelation ;
	rdfs:isDefinedBy "http://purl.org/linguistics/gold"^^<http://www.w3.org/2001/XMLSchema#anyURI> ;
	rdfs:comment "meronym"@eng .

gold:morphologicalRelation a owl:ObjectProperty ;
	rdfs:label "morphologicalRelation"@eng ;
	rdfs:isDefinedBy "http://purl.org/linguistics/gold"^^<http://www.w3.org/2001/XMLSchema#anyURI> ;
	rdfs:comment "A relation holding between morphological units."@eng ;
	rdfs:domain gold:MorphologicalUnit ;
	rdfs:range gold:MorphologicalUnit .

gold:mutuallyIntelligible a owl:ObjectProperty ;
	rdfs:label "mutuallyIntelligible"@eng ;
	rdfs:isDefinedBy "http://purl.org/linguistics/gold"^^<http://www.w3.org/2001/XMLSchema#anyURI> ;
	rdfs:comment "mutuallyIntelligible is the binary, symmetric relation holding between two language varieties such that speakers of the first variety can communicate with members of the second with relative ease, and vice versa."@eng ;
	rdfs:domain gold:HumanLanguageVariety ;
	rdfs:range gold:HumanLanguageVariety .

gold:names a owl:ObjectProperty ;
	rdfs:label "names"@eng ;
	rdfs:isDefinedBy "http://purl.org/linguistics/gold"^^<http://www.w3.org/2001/XMLSchema#anyURI> ;
	rdfs:comment "This semiotic relation associates some OrthographicExpression with some Entity. It differs from 'labels' in that a name is usually considered part of the orthographic system, where a label is not."@eng ;
	rdfs:domain gold:WrittenLinguisticExpression .

gold:nucleus a owl:ObjectProperty ;
	rdfs:label "nucleus"@eng ;
	rdfs:isDefinedBy "http://purl.org/linguistics/gold"^^<http://www.w3.org/2001/XMLSchema#anyURI> ;
	rdfs:comment "The central segment of a syllable."@eng .

gold:object a owl:ObjectProperty ;
	rdfs:label "object"@eng ;
	rdfs:subPropertyOf gold:argument ;
	rdfs:isDefinedBy "http://purl.org/linguistics/gold"^^<http://www.w3.org/2001/XMLSchema#anyURI> ;
	rdfs:comment "An object, traditionally defined, is either a direct object or an indirect object.An object, in some usages, is any  grammatical relation other than subject [Crystal 1985, 211; Hartmann and Stork 1972, 155-156; Comrie 1989, 66]."@eng .

gold:onset a owl:ObjectProperty ;
	rdfs:label "onset"@eng ;
	rdfs:isDefinedBy "http://purl.org/linguistics/gold"^^<http://www.w3.org/2001/XMLSchema#anyURI> ;
	rdfs:comment "The initial segment of a syllable."@eng .

gold:orderingRelation a owl:ObjectProperty ;
	rdfs:label "orderingRelation"@eng ;
	rdfs:isDefinedBy "http://purl.org/linguistics/gold"^^<http://www.w3.org/2001/XMLSchema#anyURI> ;
	rdfs:comment "Any relation that establishes a linear ordering of linguistic units."@eng .

gold:parentVariety a owl:ObjectProperty ;
	rdfs:label "parentVariety"@eng ;
	rdfs:isDefinedBy "http://purl.org/linguistics/gold"^^<http://www.w3.org/2001/XMLSchema#anyURI> ;
	rdfs:comment "parentVariety is the  relation of direct genetic relatedness, where there are  no intermediate ancestors between the ancestor and descendant. For example, Old English is the parent variety of Middle English."@eng ;
	rdfs:domain gold:HumanLanguageVariety ;
	rdfs:range gold:HumanLanguageVariety .

gold:patient a owl:ObjectProperty ;
	rdfs:label "patient"@eng ;
	rdfs:subPropertyOf gold:semanticRole ;
	rdfs:isDefinedBy "http://purl.org/linguistics/gold"^^<http://www.w3.org/2001/XMLSchema#anyURI> .

gold:precedes a owl:ObjectProperty ;
	rdfs:label "precedes"@eng ;
	rdfs:subPropertyOf gold:orderingRelation ;
	rdfs:isDefinedBy "http://purl.org/linguistics/gold"^^<http://www.w3.org/2001/XMLSchema#anyURI> ;
	rdfs:comment "This relation holds between two linguistic units and represents the notion of precedence in a language. That is, (precedes A B) means that A comes before B in the linearization of the realization of linguistic signs. This inverse of this relation is 'follows'."@eng .

gold:predicate a owl:ObjectProperty ;
	rdfs:label "predicate"@eng ;
	rdfs:subPropertyOf gold:syntacticRole ;
	rdfs:isDefinedBy "http://purl.org/linguistics/gold"^^<http://www.w3.org/2001/XMLSchema#anyURI> ;
	rdfs:comment "The predicate is the relation between the Clause and a portion of a  clause, excluding the subject, that expresses something about the subject [Crystal 1980, 280; Hartmann and Stork 1972, 182; Pei and Gaynor 1954, 173; Pike and Pike 1982, 40; Crystal 1985, 241-242]."@eng ;
	rdfs:range gold:Clause .

gold:prefix a owl:ObjectProperty ;
	rdfs:label "prefix"@eng ;
	rdfs:subPropertyOf gold:morphologicalRelation ;
	rdfs:isDefinedBy "http://purl.org/linguistics/gold"^^<http://www.w3.org/2001/XMLSchema#anyURI> ;
	rdfs:comment "The relation between a morphological unit and the  lexical unit to which it is attached. The LexicalUnit is usually a Root or Stem. The inverse of prefix is suffix [Crystal 1980, 281; Hartmann and Stork 1972, 182]."@eng .

gold:realization a owl:ObjectProperty ;
	rdfs:label "realization"@eng ;
	rdfs:isDefinedBy "http://purl.org/linguistics/gold"^^<http://www.w3.org/2001/XMLSchema#anyURI> ;
	rdfs:comment "The relation holding between a linguistic unit and its physical form, either a spoken, written or signed expression."@eng ;
	rdfs:domain gold:LinguisticUnit ;
	rdfs:range gold:LinguisticExpression .

gold:rhyme a owl:ObjectProperty ;
	rdfs:label "rhyme"@eng ;
	rdfs:isDefinedBy "http://purl.org/linguistics/gold"^^<http://www.w3.org/2001/XMLSchema#anyURI> ;
	rdfs:comment "The core of a syllable, consisting of a nucleus and coda."@eng .

gold:semanticRole a owl:ObjectProperty ;
	rdfs:label "semanticRole"@eng ;
	rdfs:isDefinedBy "http://purl.org/linguistics/gold"^^<http://www.w3.org/2001/XMLSchema#anyURI> .

gold:signedRealization a owl:ObjectProperty ;
	rdfs:label "signedRealization"@eng ;
	rdfs:subPropertyOf gold:realization ;
	rdfs:isDefinedBy "http://purl.org/linguistics/gold"^^<http://www.w3.org/2001/XMLSchema#anyURI> ;
	rdfs:comment "The relation between some linguistic unit and its corresponding signed expression."@eng ;
	rdfs:domain gold:LinguisticUnit ;
	rdfs:range gold:SignedLinguisticExpression .

gold:specifier a owl:ObjectProperty ;
	rdfs:label "specifier"@eng ;
	rdfs:subPropertyOf gold:hasSyntacticConstituent ;
	rdfs:isDefinedBy "http://purl.org/linguistics/gold"^^<http://www.w3.org/2001/XMLSchema#anyURI> .

gold:subject a owl:ObjectProperty ;
	rdfs:label "subject"@eng ;
	rdfs:subPropertyOf gold:argument ;
	rdfs:isDefinedBy "http://purl.org/linguistics/gold"^^<http://www.w3.org/2001/XMLSchema#anyURI> .

gold:suffix a owl:ObjectProperty ;
	rdfs:label "suffix"@eng ;
	rdfs:subPropertyOf gold:morphologicalRelation ;
	rdfs:isDefinedBy "http://purl.org/linguistics/gold"^^<http://www.w3.org/2001/XMLSchema#anyURI> ;
	rdfs:comment "The relation between a morphological unit and the  lexical unit to which it is attached. The LexicalUnit is usually a Root or Stem. The inverse of suffix is 'prefix' [Crystal 1980, 340; Hartmann and Stork 1972, 226]."@eng .

gold:synonym a owl:ObjectProperty ;
	rdfs:label "synonym"@eng ;
	rdfs:subPropertyOf gold:lexicalRelation ;
	rdfs:isDefinedBy "http://purl.org/linguistics/gold"^^<http://www.w3.org/2001/XMLSchema#anyURI> ;
	rdfs:comment "synonym"@eng .

gold:syntacticRole a owl:ObjectProperty ;
	rdfs:label "syntacticRole"@eng ;
	rdfs:isDefinedBy "http://purl.org/linguistics/gold"^^<http://www.w3.org/2001/XMLSchema#anyURI> ;
	rdfs:comment """A general category subsuming relations relevant at the level of the Clause, such as predicate and subject. 
A grammatical relation is a role of a phrase or  complement clause that determines syntactic behaviors such as the following: word position in a clause; verb agreement; participation and behavior in such operations as  passivization [Comrie 1989, 65-66; Andrews 1985, 66]."""@eng .

gold:translation a owl:ObjectProperty ;
	rdfs:label "translation"@eng ;
	rdfs:isDefinedBy "http://purl.org/linguistics/gold"^^<http://www.w3.org/2001/XMLSchema#anyURI> ;
	rdfs:comment "The relation between an orthographic expression in one language and some orthographic expression in another such that both expressions have the same or roughly the same meaning."@eng .

gold:writtenRealization a owl:ObjectProperty ;
	rdfs:label "writtenRealization"@eng ;
	rdfs:subPropertyOf gold:realization ;
	rdfs:isDefinedBy "http://purl.org/linguistics/gold"^^<http://www.w3.org/2001/XMLSchema#anyURI> ;
	rdfs:comment "The relation between some linguistic unit and its corresponding written expression."@eng ;
	rdfs:domain gold:LinguisticUnit ;
	rdfs:range gold:WrittenLinguisticExpression .

bibliography:hasCitation a owl:ObjectProperty ;
	rdfs:label "hasCitation"@eng ;
	rdfs:isDefinedBy "http://purl.org/linguistics/gold"^^<http://www.w3.org/2001/XMLSchema#anyURI> .

bibliography:hasEntry a owl:ObjectProperty ;
	rdfs:label "hasEntry"@eng ;
	rdfs:isDefinedBy "http://purl.org/linguistics/gold"^^<http://www.w3.org/2001/XMLSchema#anyURI> .

gold:abbreviation a owl:DatatypeProperty ;
	rdfs:label "abbreviation"@eng ;
	rdfs:isDefinedBy "http://purl.org/linguistics/gold"^^<http://www.w3.org/2001/XMLSchema#anyURI> ;
	rdfs:comment "The abbreviated form representing a scientific term, e.g., ACC, 2, CL."@eng .

gold:hasExample a owl:DatatypeProperty ;
	rdfs:label "hasExample"@eng ;
	rdfs:isDefinedBy "http://purl.org/linguistics/gold"^^<http://www.w3.org/2001/XMLSchema#anyURI> .

gold:orthographicRep a owl:DatatypeProperty ;
	rdfs:label "orthographicRep"@eng ;
	rdfs:subPropertyOf gold:stringRep ;
	rdfs:isDefinedBy "http://purl.org/linguistics/gold"^^<http://www.w3.org/2001/XMLSchema#anyURI> .

gold:phonemicRep a owl:DatatypeProperty ;
	rdfs:label "phonemicRep"@eng ;
	rdfs:subPropertyOf gold:stringRep ;
	rdfs:isDefinedBy "http://purl.org/linguistics/gold"^^<http://www.w3.org/2001/XMLSchema#anyURI> .

gold:phoneticRep a owl:DatatypeProperty ;
	rdfs:label "phoneticRep"@eng ;
	rdfs:subPropertyOf gold:stringRep ;
	rdfs:isDefinedBy "http://purl.org/linguistics/gold"^^<http://www.w3.org/2001/XMLSchema#anyURI> .

gold:stringRep a owl:DatatypeProperty ;
	rdfs:label "stringRep"@eng ;
	rdfs:isDefinedBy "http://purl.org/linguistics/gold"^^<http://www.w3.org/2001/XMLSchema#anyURI> ;
	rdfs:domain gold:LinguisticUnit ;
	rdfs:range <http://www.w3.org/2001/XMLSchema#string> .

bibliography:hasPageInformation a owl:DatatypeProperty ;
	rdfs:label "hasPageInformation"@eng ;
	rdfs:isDefinedBy "http://purl.org/linguistics/gold"^^<http://www.w3.org/2001/XMLSchema#anyURI> .

owl:Ontology a owl:Class ;
	rdfs:label "Ontology"@eng ;
	rdfs:isDefinedBy "http://purl.org/linguistics/gold"^^<http://www.w3.org/2001/XMLSchema#anyURI> .

owl:AnnotationProperty a owl:Class ;
	rdfs:label "AnnotationProperty"@eng ;
	rdfs:isDefinedBy "http://purl.org/linguistics/gold"^^<http://www.w3.org/2001/XMLSchema#anyURI> .

owl:ObjectProperty a owl:Class ;
	rdfs:label "ObjectProperty"@eng ;
	rdfs:isDefinedBy "http://purl.org/linguistics/gold"^^<http://www.w3.org/2001/XMLSchema#anyURI> .

owl:TransitiveProperty a owl:Class ;
	rdfs:label "TransitiveProperty"@eng ;
	rdfs:isDefinedBy "http://purl.org/linguistics/gold"^^<http://www.w3.org/2001/XMLSchema#anyURI> .

owl:SymmetricProperty a owl:Class ;
	rdfs:label "SymmetricProperty"@eng ;
	rdfs:isDefinedBy "http://purl.org/linguistics/gold"^^<http://www.w3.org/2001/XMLSchema#anyURI> .

owl:InverseFunctionalProperty a owl:Class ;
	rdfs:label "InverseFunctionalProperty"@eng ;
	rdfs:isDefinedBy "http://purl.org/linguistics/gold"^^<http://www.w3.org/2001/XMLSchema#anyURI> .

owl:DatatypeProperty a owl:Class ;
	rdfs:label "DatatypeProperty"@eng ;
	rdfs:isDefinedBy "http://purl.org/linguistics/gold"^^<http://www.w3.org/2001/XMLSchema#anyURI> .

owl:Class a owl:Class ;
	rdfs:label "Class"@eng ;
	rdfs:isDefinedBy "http://purl.org/linguistics/gold"^^<http://www.w3.org/2001/XMLSchema#anyURI> .

bibliography:Citation a owl:Class ;
	rdfs:label "Citation"@eng ;
	rdfs:isDefinedBy "http://purl.org/linguistics/gold"^^<http://www.w3.org/2001/XMLSchema#anyURI> .

gold:CaseProperty a owl:Class ;
	rdfs:label "CaseProperty"@eng ;
	rdfs:subClassOf gold:MorphosyntacticProperty ;
	rdfs:isDefinedBy "http://purl.org/linguistics/gold"^^<http://www.w3.org/2001/XMLSchema#anyURI> ;
	rdfs:comment "CaseProperty is the class of properties that concern the grammatical encoding of a noun's relationship (syntactic or semantic) to some other element in the sentence, such as a verb, noun, pronoun, or adposition [Pei and Gaynor 1954, 35; Crystal 1980, 53-54; Anderson 1985, 179-180; Andrews 1985, 7172; Kuno 1973, 45; Blake 2001]."@eng .

gold:ModalityProperty a owl:Class ;
	rdfs:label "ModalityProperty"@eng ;
	rdfs:subClassOf gold:MorphosyntacticProperty ;
	rdfs:isDefinedBy "http://purl.org/linguistics/gold"^^<http://www.w3.org/2001/XMLSchema#anyURI> ;
	rdfs:comment "ModalityProperty is the class of properties that concern the grammatical encoding of the status of the proposition itself, and not of the event to which the proposition refers, cf. AspectProperty [Palmer 2001, 1].  As a grammatical property, it represents those dimensions in the domains of knowledge (epistemic modality), social relations (deontic modality) and ability (abilitative modality), and possibly others."@eng .

gold:VoiceProperty a owl:Class ;
	rdfs:label "VoiceProperty"@eng ;
	rdfs:subClassOf gold:MorphosyntacticProperty ;
	rdfs:isDefinedBy "http://purl.org/linguistics/gold"^^<http://www.w3.org/2001/XMLSchema#anyURI> ;
	rdfs:comment "VoiceProperty is the class of properties that concern the grammatical encoding of the relationship between the verb and the nominals in a subject-predicate configuration. It selects a grammatically prominent syntactic constituent--subject--from the underlying semantic functions. In accusative language, the basic strategy is to select an agent as a subject [Shibatani 1988, 3]. It can be said that all voice systems mark the affectedness/nonaffectedness of sentential subjects [Klaiman 1988, 30]. Voice is also known as diathesis [Klaiman 1991,323]."@eng .

gold:PhoneticProperty a owl:Class ;
	rdfs:label "PhoneticProperty"@eng ;
	rdfs:subClassOf gold:LinguisticProperty ;
	rdfs:isDefinedBy "http://purl.org/linguistics/gold"^^<http://www.w3.org/2001/XMLSchema#anyURI> ;
	rdfs:comment "The class of properties used to describe speech sounds. The properties given here are more or less taken directly from Ladefoged's later works, in particular, the taxonomies of [Ladefoged  1997]."@eng .

gold:ForceProperty a owl:Class ;
	rdfs:label "ForceProperty"@eng ;
	rdfs:subClassOf gold:MorphosyntacticProperty ;
	rdfs:isDefinedBy "http://purl.org/linguistics/gold"^^<http://www.w3.org/2001/XMLSchema#anyURI> ;
	rdfs:comment "ForceProperty is the class of properties that concern the grammatical encoding of the speech act associated with a proposition. Among the traditionally defined values are Declarative, Imperative and Interrogative. Force is here distinguished from Mood, but there is a close association of Mood with Force values, e.g. between IndicativeMood and DeclarativeForce."@eng .

gold:Predicator a owl:Class ;
	rdfs:label "Predicator"@eng ;
	rdfs:subClassOf gold:PartOfSpeechProperty ;
	rdfs:isDefinedBy "http://purl.org/linguistics/gold"^^<http://www.w3.org/2001/XMLSchema#anyURI> ;
	rdfs:comment "Predicator is the class of syntactic words that are fundamentally relation inducing. That is, predicators license argument structure [Anderson 1997, 14]. Verbs are quintessential predicators, though other categories, such as determiners and some nouns, are also predicative in nature."@eng .

gold:Phrase a owl:Class ;
	rdfs:label "Phrase"@eng ;
	rdfs:subClassOf gold:SyntacticConstruction ;
	rdfs:isDefinedBy "http://purl.org/linguistics/gold"^^<http://www.w3.org/2001/XMLSchema#anyURI> ;
	rdfs:comment "Phrase is the class of syntactic constructions that consist of one or more syntactic words, but lack the subject-predicate organization of a clause. Phrases get their grammatical characteristics according to what word occupies the head position; thus, all phrases have heads [Crystal 1980, 232-233;  Pei and Gaynor 1954, 169; Pike and Pike 1982, 453]."@eng .

gold:SubordinateClause a owl:Class ;
	rdfs:label "SubordinateClause"@eng ;
	rdfs:subClassOf gold:Clause ;
	rdfs:isDefinedBy "http://purl.org/linguistics/gold"^^<http://www.w3.org/2001/XMLSchema#anyURI> ;
	rdfs:comment "SubordinateClause is the class of clauses that cannot stand on their own as sentences.  A matrix clause combined with a subordinate clause form a main clause. In the sentence 'John thinks that Mary is sick', 'Mary is sick' is the subordinate clause."@eng .

gold:Functor a owl:Class ;
	rdfs:label "Functor"@eng ;
	rdfs:subClassOf gold:PartOfSpeechProperty ;
	rdfs:isDefinedBy "http://purl.org/linguistics/gold"^^<http://www.w3.org/2001/XMLSchema#anyURI> ;
	rdfs:comment "Functor is the class of syntactic word whose members are neither relation- nor argument-like non-relational [Anderson 1997, 20]. Typical functors include adpositions, subordinators, and complementizers."@eng .

gold:SubordinatingConnective a owl:Class ;
	rdfs:label "SubordinatingConnective"@eng ;
	rdfs:subClassOf gold:Connective ;
	rdfs:isDefinedBy "http://purl.org/linguistics/gold"^^<http://www.w3.org/2001/XMLSchema#anyURI> ;
	rdfs:comment "A subordinating connective is a connective that links constructions by making one of them a constituent of another. The subordinating conjunction typically marks the incorporated constituent [Crystal 1997, 370]."@eng .

gold:MorphologicalUnit a owl:Class ;
	rdfs:label "MorphologicalUnit"@eng ;
	rdfs:subClassOf gold:GrammarUnit ;
	rdfs:isDefinedBy "http://purl.org/linguistics/gold"^^<http://www.w3.org/2001/XMLSchema#anyURI> ;
	rdfs:comment "MorphologicalUnit subsumes all grammatical units below the level of the syntactic word. Only a morphological unit may be a constituent of another morphological unit."@eng .

gold:ArticulatoryProperty a owl:Class ;
	rdfs:label "ArticulatoryProperty"@eng ;
	rdfs:subClassOf gold:PhoneticProperty ;
	rdfs:isDefinedBy "http://purl.org/linguistics/gold"^^<http://www.w3.org/2001/XMLSchema#anyURI> ;
	rdfs:comment "The class of properties concerning how sounds are produced in the mouth."@eng .

gold:AnteriorProperty a owl:Class ;
	rdfs:label "AnteriorProperty"@eng ;
	rdfs:subClassOf gold:CoronalProperty ;
	rdfs:isDefinedBy "http://purl.org/linguistics/gold"^^<http://www.w3.org/2001/XMLSchema#anyURI> ;
	rdfs:comment "Properties characterized by focusing on the upper passive articulator on the roof of the mouth [Ladefoged 1997, 597]."@eng .

gold:GenderProperty a owl:Class ;
	rdfs:label "GenderProperty"@eng ;
	rdfs:subClassOf gold:MorphosyntacticProperty ;
	rdfs:isDefinedBy "http://purl.org/linguistics/gold"^^<http://www.w3.org/2001/XMLSchema#anyURI> ;
	rdfs:comment "GenderProperty is the class of properties that are assigned to nouns on the basis of their inherent properties by an AssignmentSystem and required by the syntax to appear on the target in an AgreementSystem. Gender may but need not be assigned on the basis of sex [Corbett 1991]."@eng .

gold:CoronalProperty a owl:Class ;
	rdfs:label "CoronalProperty"@eng ;
	rdfs:subClassOf gold:BuccalProperty ;
	rdfs:isDefinedBy "http://purl.org/linguistics/gold"^^<http://www.w3.org/2001/XMLSchema#anyURI> ;
	rdfs:comment "Properties of sounds produced with passive articulators lying on the coronal axis."@eng .

gold:ApicalityProperty a owl:Class ;
	rdfs:label "ApicalityProperty"@eng ;
	rdfs:subClassOf gold:CoronalProperty ;
	rdfs:isDefinedBy "http://purl.org/linguistics/gold"^^<http://www.w3.org/2001/XMLSchema#anyURI> ;
	rdfs:comment "Properties characterized by focusing on the action of the lower, active articulator, ie which part of the tounge is used in articulation [Ladefoged 1997, 597]."@eng .

gold:StrictureProperty a owl:Class ;
	rdfs:label "StrictureProperty"@eng ;
	rdfs:subClassOf gold:MannerProperty ;
	rdfs:isDefinedBy "http://purl.org/linguistics/gold"^^<http://www.w3.org/2001/XMLSchema#anyURI> ;
	rdfs:comment "Property of sounds produced by stricture of the vocal tract."@eng .

gold:Determiner a owl:Class ;
	rdfs:label "Determiner"@eng ;
	rdfs:subClassOf gold:PartOfSpeechProperty ;
	rdfs:isDefinedBy "http://purl.org/linguistics/gold"^^<http://www.w3.org/2001/XMLSchema#anyURI> ;
	rdfs:comment "A Determiner is a part of speech whose members belong to a class of noun modifiers and express the reference, including  quantity, of a noun [Crystal 1997,112]."@eng .

gold:MorphosemanticProperty a owl:Class ;
	rdfs:label "MorphosemanticProperty"@eng ;
	rdfs:subClassOf gold:LinguisticProperty ;
	rdfs:isDefinedBy "http://purl.org/linguistics/gold"^^<http://www.w3.org/2001/XMLSchema#anyURI> ;
	rdfs:comment "Linguistic properties having a semantic component."@eng .

gold:GlottalTimingProperty a owl:Class ;
	rdfs:label "GlottalTimingProperty"@eng ;
	rdfs:subClassOf gold:LaryngealProperty ;
	rdfs:isDefinedBy "http://purl.org/linguistics/gold"^^<http://www.w3.org/2001/XMLSchema#anyURI> ;
	rdfs:comment "[Need a definition.]"@eng .

gold:EvidentialityProperty a owl:Class ;
	rdfs:label "EvidentialityProperty"@eng ;
	rdfs:subClassOf gold:MorphosyntacticProperty ;
	rdfs:isDefinedBy "http://purl.org/linguistics/gold"^^<http://www.w3.org/2001/XMLSchema#anyURI> ;
	rdfs:comment "EvidentialFeature is the class of properties that concern the grammatical encoding of the speaker's belief in what they say. It is closely related to mood, some of whose values indicate the strength of the agent's belief."@eng .

gold:HumanLanguageVariety a owl:Class ;
	rdfs:label "HumanLanguageVariety"@eng ;
	rdfs:subClassOf gold:LinguisticSystem ;
	rdfs:isDefinedBy "http://purl.org/linguistics/gold"^^<http://www.w3.org/2001/XMLSchema#anyURI> ;
	rdfs:comment "Human language variety is the class of all discrete entities (as identified by a linguist) that are considered systems of signs in their own right, emerge gradually as a cultural artifact, and are used by a particular community for communication."@eng .

gold:SizeProperty a owl:Class ;
	rdfs:label "SizeProperty"@eng ;
	rdfs:subClassOf gold:MorphosyntacticProperty ;
	rdfs:isDefinedBy "http://purl.org/linguistics/gold"^^<http://www.w3.org/2001/XMLSchema#anyURI> ;
	rdfs:comment "SizeProperty is the class of properties that concern the grammatical encoding of relative size. Currently only Diminutive and Augmentative defined as possible properties. Typically, size is specified \"derivationally\" rather than by inflection."@eng .

gold:Verbal a owl:Class ;
	rdfs:label "Verbal"@eng ;
	rdfs:subClassOf gold:Predicator ;
	rdfs:isDefinedBy "http://purl.org/linguistics/gold"^^<http://www.w3.org/2001/XMLSchema#anyURI> ;
	rdfs:comment "A Verbal is a part of speech whose members typically signal events and actions; constitute, singly or in a phrase, a minimal  predicate in a  clause; govern the number and types of other constituents which may occur in the clause; and, in inflectional languages, may be inflected for tense, aspect, voice, modality, or agreement with other constituents in person, number, or grammatical gender  [Crystal 1997, 409; Givon 1984, 52; Payne 1997, 47]."@eng .

gold:BacknessProperty a owl:Class ;
	rdfs:label "BacknessProperty"@eng ;
	rdfs:subClassOf gold:DorsalProperty ;
	rdfs:isDefinedBy "http://purl.org/linguistics/gold"^^<http://www.w3.org/2001/XMLSchema#anyURI> ;
	rdfs:comment "The class of properties describing sounds based on the relative horizontal position of the tongue. Note, Ladefoged refers to this property as Back."@eng .

gold:DorsalProperty a owl:Class ;
	rdfs:label "DorsalProperty"@eng ;
	rdfs:subClassOf gold:BuccalProperty ;
	rdfs:isDefinedBy "http://purl.org/linguistics/gold"^^<http://www.w3.org/2001/XMLSchema#anyURI> ;
	rdfs:comment "The class of properties associated with sounds made with the body of the tongue [Ladefoged 1997, 601]. Almost all vowels can be described using subclasses of this property."@eng .

gold:GlottalStrictureProperty a owl:Class ;
	rdfs:label "GlottalStrictureProperty"@eng ;
	rdfs:subClassOf gold:LaryngealProperty ;
	rdfs:isDefinedBy "http://purl.org/linguistics/gold"^^<http://www.w3.org/2001/XMLSchema#anyURI> ;
	rdfs:comment "[Need a definition.]"@eng .

gold:PlaceProperty a owl:Class ;
	rdfs:label "PlaceProperty"@eng ;
	rdfs:subClassOf gold:SupraLaryngealProperty ;
	rdfs:isDefinedBy "http://purl.org/linguistics/gold"^^<http://www.w3.org/2001/XMLSchema#anyURI> ;
	rdfs:comment "The superclass of properties that specify the location of the articulators [Ladefoged 1997, 594]."@eng .

gold:Numeral a owl:Class ;
	rdfs:label "Numeral"@eng ;
	rdfs:subClassOf gold:Quantifier ;
	rdfs:isDefinedBy "http://purl.org/linguistics/gold"^^<http://www.w3.org/2001/XMLSchema#anyURI> ;
	rdfs:comment "A numeral is a partOfSpeech whose members function most typically as adjectives or pronouns and express a number, or relation to the number, such as one of the following: quantity, sequence, frequency, fraction [Hartmann and Stork 1972,155; Pei and Gaynor 1954,149]."@eng .

gold:MorphosyntacticProperty a owl:Class ;
	rdfs:label "MorphosyntacticProperty"@eng ;
	rdfs:subClassOf gold:LinguisticProperty ;
	rdfs:isDefinedBy "http://purl.org/linguistics/gold"^^<http://www.w3.org/2001/XMLSchema#anyURI> ;
	rdfs:comment "MorphosyntacticFeature is the class of linguistic features that govern the grammatical behavior of morphosyntactic units. E.g., two morphosyntactic units can agree according to shared morphosyntactic features. Morphosyntactic features are also called grammatical categories. This class is intended to represent only the formal aspects of morphosyntax; that is, there is no notional component. In a grammatical system, such features occur in contrast to one another other, and are typically expressed in the same fashion [Crystal 1985, 43-44; Hopper, P. 1992, 81; Bybee 1985, 191]."@eng .

gold:DerivationalUnit a owl:Class ;
	rdfs:label "DerivationalUnit"@eng ;
	rdfs:subClassOf gold:FunctionalUnit ;
	rdfs:isDefinedBy "http://purl.org/linguistics/gold"^^<http://www.w3.org/2001/XMLSchema#anyURI> ;
	rdfs:comment "DerivationalUnit is the class of functional units whose members function to derive a new lexical unit from an existing one, by systematically changing the meaning and possibly altering the part of speech feature of the root or stem it attaches to [Hartmann and Stork 1972,62; Crystal 1985,89; Bybee 1985,81-82, 99]."@eng .

gold:LateralProperty a owl:Class ;
	rdfs:label "LateralProperty"@eng ;
	rdfs:subClassOf gold:BuccalProperty ;
	rdfs:isDefinedBy "http://purl.org/linguistics/gold"^^<http://www.w3.org/2001/XMLSchema#anyURI> ;
	rdfs:comment "Characterizing sounds involving air released through side of the mouth."@eng .

gold:Abstract a owl:Class ;
	rdfs:label "Abstract"@eng ;
	rdfs:subClassOf owl:Thing ;
	rdfs:isDefinedBy "http://purl.org/linguistics/gold"^^<http://www.w3.org/2001/XMLSchema#anyURI> ;
	rdfs:comment "Any entity that does not occupy a position in space and  time. See SUMO for a detailed explanation."@eng .

gold:PartOfSpeechProperty a owl:Class ;
	rdfs:label "PartOfSpeechProperty"@eng ;
	rdfs:subClassOf gold:LinguisticProperty ;
	rdfs:isDefinedBy "http://purl.org/linguistics/gold"^^<http://www.w3.org/2001/XMLSchema#anyURI> ;
	rdfs:comment "PartOfSpeechProperty is the class of all kind of parts of speech."@eng .

gold:SyntacticConstruction a owl:Class ;
	rdfs:label "SyntacticConstruction"@eng ;
	rdfs:subClassOf gold:SyntacticUnit ;
	rdfs:isDefinedBy "http://purl.org/linguistics/gold"^^<http://www.w3.org/2001/XMLSchema#anyURI> ;
	rdfs:comment "SyntacticConstruction is the class of grammar units that have syntactic structure, i.e., consisting of more than one syntactic word or construction in a syntactic configuration. [Crystal 1980, 85-86]."@eng .

gold:TenseProperty a owl:Class ;
	rdfs:label "TenseProperty"@eng ;
	rdfs:subClassOf gold:MorphosemanticProperty ;
	rdfs:isDefinedBy "http://purl.org/linguistics/gold"^^<http://www.w3.org/2001/XMLSchema#anyURI> ;
	rdfs:comment """Following [Comrie 1985, vii], we take tense to be the grammaticalisation of location in time.  Tense Property is assigned to clauses on the basis of semantics: a tense value is selected for the clause from the range of tense values available in the given language. Tense Property is typically realised on the verb, but it may be found expressed multiply on different elements in the same clause. For example, tense may be found on more than one element of the verbal complex (e.g. in Kayardild [Evans 2003] or  Paamese [Crowley 2002, 68], or on verbs as well as on certain spatial and temporal adverbs and certain prepositions in the same clause (e.g. in Malagasy [Randriamasimanana 1981, 355-367],  [Keenan and Polinsky 1998, 566-567].

In the given language, the values of the Tense Property are assigned to the designated elements as a consequence of semantic choice, and all the available options of particular tense values expressing particular tense meanings can be described with a Tense Assignment System for that language. Since no languages have been found for which tense values are assigned by a Tense Distribution System (i.e. contextually, through agreement or government), Tense Property is not a Morphosyntactic Property. Instead, it is a Morphosemantic Property only."""@eng .

gold:Noun a owl:Class ;
	rdfs:label "Noun"@eng ;
	rdfs:subClassOf gold:PartOfSpeechProperty ;
	rdfs:isDefinedBy "http://purl.org/linguistics/gold"^^<http://www.w3.org/2001/XMLSchema#anyURI> ;
	rdfs:comment "A noun is a broad classification of parts of speech usually identifying time-stable concept [Crystal 1997,371]."@eng .

gold:Adjectival a owl:Class ;
	rdfs:label "Adjectival"@eng ;
	rdfs:subClassOf gold:Predicator ;
	rdfs:isDefinedBy "http://purl.org/linguistics/gold"^^<http://www.w3.org/2001/XMLSchema#anyURI> ;
	rdfs:comment "An adjectival, or 'adjective', is a part of speech whose members modify nouns. An adjectival specifies the attributes of a noun referent. Note: this is one case among many. Adjectivals are a class of modifiers. An adjectival may be inflected as comparitive or superlative [Crystal 1997,8; Payne 1997,63]."@eng .

gold:AspectProperty a owl:Class ;
	rdfs:label "AspectProperty"@eng ;
	rdfs:subClassOf gold:MorphosemanticProperty ;
	rdfs:isDefinedBy "http://purl.org/linguistics/gold"^^<http://www.w3.org/2001/XMLSchema#anyURI> ;
	rdfs:comment """The term 'aspect'; designates the perspective taken on the internal temporal organisation of the event, and different values of the Aspect Feature distinguish different ways of viewing the internal temporal constituency of the same event [Comrie 1976, 3ff], after [Holt 1943, 6; Bybee 2003, 157]. The 'event is understood here as a general term covering any situation type (a state, activity, accomplishment, achievement, etc.) as expressed by the verb phrase of the construction. Unlike Tense Feature, which expresses event-external time and is deictic, Aspect Feature is event-internal and non-deictic, as it is not concerned with relating the time of the event to any other time point.

Aspect Property is assigned to clauses on the basis of semantics: an aspect value is selected for the clause from the range of aspect values available in the given language. Aspect Property is typically realised on the verb, but it may be found expressed multiply on different elements in the same clause. It may be found on more than one element of the verbal complex, or on verbs as well as certain adverbs in the same clause.

In the given language, the values of the Aspect Property are assigned to the designated elements as a consequence of semantic choice, and all the available options of particular aspect values expressing particular aspect meanings can be described with an Aspect Assignment System for that language. Since no languages have been found for which aspect values are assigned by an Aspect Distribution System (i.e. contextually, through agreement or government), Aspect Feature is not a Morphosyntactic Property.  Instead, it is a Morphosemantic Property only.

NOTE: Although the semantic basis for the Aspect Property are the distinctions identified in the internal temporal constituency of an event, aspect meanings frequently combine with tense, modal or other meanings expressing actionality distinctions. Hence, markers expressing aspect values are frequently portmanteaux realising combined TAM values."""@eng .

gold:FeatureSpecification a owl:Class ;
	rdfs:label "FeatureSpecification"@eng ;
	rdfs:subClassOf gold:LinguisticDataStructure ;
	rdfs:isDefinedBy "http://purl.org/linguistics/gold"^^<http://www.w3.org/2001/XMLSchema#anyURI> ;
	rdfs:comment "A FeatureSpecification is a data structure that groups together a linguistic feature with a value [Maxwell, Simons, and Hayashi 2000]."@eng .

gold:LabialProperty a owl:Class ;
	rdfs:label "LabialProperty"@eng ;
	rdfs:subClassOf gold:PlaceProperty ;
	rdfs:isDefinedBy "http://purl.org/linguistics/gold"^^<http://www.w3.org/2001/XMLSchema#anyURI> ;
	rdfs:comment "The class of properties associated with characteristics of labial articulations [Ladefoged 1997, 594]."@eng .

gold:CoordinatingConnective a owl:Class ;
	rdfs:label "CoordinatingConnective"@eng ;
	rdfs:subClassOf gold:Connective ;
	rdfs:isDefinedBy "http://purl.org/linguistics/gold"^^<http://www.w3.org/2001/XMLSchema#anyURI> ;
	rdfs:comment "A coordinating connective is a connective that links constituents without syntactically subordinating one to the other [Crystal 1997,93]."@eng .

gold:Segment a owl:Class ;
	rdfs:label "Segment"@eng ;
	rdfs:subClassOf gold:FormUnit ;
	rdfs:isDefinedBy "http://purl.org/linguistics/gold"^^<http://www.w3.org/2001/XMLSchema#anyURI> .

gold:LinguisticTaxon a owl:Class ;
	rdfs:label "LinguisticTaxon"@eng ;
	rdfs:subClassOf gold:Taxon ;
	rdfs:isDefinedBy "http://purl.org/linguistics/gold"^^<http://www.w3.org/2001/XMLSchema#anyURI> ;
	rdfs:comment "LinguisticTaxon is the class of  Taxons whose instances are used in the scientific classification language varieties. That is, instances of LinguisticTaxon have instances that are human language varieties."@eng .

gold:Connective a owl:Class ;
	rdfs:label "Connective"@eng ;
	rdfs:subClassOf gold:Functor ;
	rdfs:isDefinedBy "http://purl.org/linguistics/gold"^^<http://www.w3.org/2001/XMLSchema#anyURI> ;
	rdfs:comment "Also known as a conjunction, a Connective is a class of parts of speech whose members syntactically link words or larger  constituents, and expresses a semantic relationship between them. A conjunction is positionally fixed relative to one or more of the elements related by it, thus distinguishing it from constituents such as English conjunctive adverbs [Crystal 1997, 81]."@eng .

gold:BuccalProperty a owl:Class ;
	rdfs:label "BuccalProperty"@eng ;
	rdfs:subClassOf gold:PlaceProperty ;
	rdfs:isDefinedBy "http://purl.org/linguistics/gold"^^<http://www.w3.org/2001/XMLSchema#anyURI> ;
	rdfs:comment "A subclass of place Properties roughly referring to positions inside the mouth [Ladefoged 1997, 606]."@eng .

gold:Article a owl:Class ;
	rdfs:label "Article"@eng ;
	rdfs:subClassOf gold:Determiner ;
	rdfs:isDefinedBy "http://purl.org/linguistics/gold"^^<http://www.w3.org/2001/XMLSchema#anyURI> ;
	rdfs:comment "An article is a member of a small class of determiners that identify a noun's definite or indefinite reference, and new or given status [Crystal 1997,26]."@eng .

gold:Pronominal a owl:Class ;
	rdfs:label "Pronominal"@eng ;
	rdfs:subClassOf gold:ProForm ;
	rdfs:isDefinedBy "http://purl.org/linguistics/gold"^^<http://www.w3.org/2001/XMLSchema#anyURI> ;
	rdfs:comment "A Pronoun is a ProForm which functions like a noun and substitutes for a noun or  noun phrase [Crystal 1997,312]."@eng .

gold:FunctionalUnit a owl:Class ;
	rdfs:label "FunctionalUnit"@eng ;
	rdfs:subClassOf gold:MorphologicalUnit ;
	rdfs:isDefinedBy "http://purl.org/linguistics/gold"^^<http://www.w3.org/2001/XMLSchema#anyURI> ;
	rdfs:comment "FunctionalUnit is the class of units that includes inflectional and derivational units. Functional units attach to roots and stems and can be used to form morphological paradigms in a grammatical description."@eng .

gold:OrthographicPart a owl:Class ;
	rdfs:label "OrthographicPart"@eng ;
	rdfs:subClassOf gold:WrittenLinguisticExpression ;
	rdfs:isDefinedBy "http://purl.org/linguistics/gold"^^<http://www.w3.org/2001/XMLSchema#anyURI> ;
	rdfs:comment "An OrthographicPart is a unit of an orthography that is not orthographically independent, that is, not necessarily able to stand alone as an orthographic word set off by whitespace. In the printed instance of the word 'conceive', 'eive' is an instance of orthographic part. Note that an orthographic part is not the same as a single glyph, although, some orthogrpaphic parts are single glyphs."@eng .

gold:GeneticTaxon a owl:Class ;
	rdfs:label "GeneticTaxon"@eng ;
	rdfs:subClassOf gold:LinguisticTaxon ;
	rdfs:isDefinedBy "http://purl.org/linguistics/gold"^^<http://www.w3.org/2001/XMLSchema#anyURI> ;
	rdfs:comment "GeneticTaxon is the class of all taxons whose members are based on genetic relatedness."@eng .

gold:LinguisticProperty a owl:Class ;
	rdfs:label "LinguisticProperty"@eng ;
	rdfs:subClassOf gold:Abstract ;
	rdfs:isDefinedBy "http://purl.org/linguistics/gold"^^<http://www.w3.org/2001/XMLSchema#anyURI> ;
	rdfs:comment "LinguisticProperty is the class  of properties that pertain to linguistic units. A unit's properties determine its behavior  in a grammatical system. Specific kinds of propertiess are relevant to certain types of units. In some language, for example, tense properties may be relevant for verbs. See also Feature and FeatureValue for the corresponding data structure for properties."@eng .

gold:LinguisticUnit a owl:Class ;
	rdfs:label "LinguisticUnit"@eng ;
	rdfs:subClassOf gold:Abstract ;
	rdfs:isDefinedBy "http://purl.org/linguistics/gold"^^<http://www.w3.org/2001/XMLSchema#anyURI> ;
	rdfs:comment "The class of all kinds of units, defined according to the particular level of linguistic analysis."@eng .

gold:TertiaryPredicator a owl:Class ;
	rdfs:label "TertiaryPredicator"@eng ;
	rdfs:subClassOf gold:Predicator ;
	rdfs:isDefinedBy "http://purl.org/linguistics/gold"^^<http://www.w3.org/2001/XMLSchema#anyURI> ;
	rdfs:comment "TertiaryPredicator is the class of syntactic words that take three required arguments."@eng .

gold:NumberProperty a owl:Class ;
	rdfs:label "NumberProperty"@eng ;
	rdfs:subClassOf gold:MorphosyntacticProperty ;
	rdfs:isDefinedBy "http://purl.org/linguistics/gold"^^<http://www.w3.org/2001/XMLSchema#anyURI> ;
	rdfs:comment "NumberProperty is the class of properties that concern the grammatical encoding of quantity. It is often found on nouns, pronouns, and verbs and expresses count distinctions--such as 'one' or 'more than one'. The count distinctions typically, but not always, correspond to the actual count of the referents of the marked noun or Pronoun [Crystal 1980, 245; Hartmann and Stork 1972, 155]."@eng .

gold:MoodProperty a owl:Class ;
	rdfs:label "MoodProperty"@eng ;
	rdfs:subClassOf gold:MorphosemanticProperty ;
	rdfs:isDefinedBy "http://purl.org/linguistics/gold"^^<http://www.w3.org/2001/XMLSchema#anyURI> ;
	rdfs:comment "MoodProperty is the class of properties that concern the grammatical encoding of mood or force of a proposition. Among the traditionally defined properties are Declarative, Imperative and Interrogative. These are a somewhat mixed bag of attitude (e.g. optative, volitive, subjunctive) and speech-act (e.g. imperative, commissive) values."@eng .

gold:Clitic a owl:Class ;
	rdfs:label "Clitic"@eng ;
	rdfs:subClassOf gold:MorphologicalUnit ;
	rdfs:isDefinedBy "http://purl.org/linguistics/gold"^^<http://www.w3.org/2001/XMLSchema#anyURI> ;
	rdfs:comment "Clitic is the class of units which members exhibit syntactic characteristics of a lexical unit, but show evidence of being morphologically bound to another lexical unit, the host, by being unstressed or subject to word-level phonological rules [Crystal 1980, 64; Hartmann and Stork 1972, 38; Anderson 1985, 158; Klavans 1982, xi-xiv, 74-76,83,93-95,100-101; Zwicky 1977,5]."@eng .

gold:FeatureDistributionSystem a owl:Class ;
	rdfs:label "FeatureDistributionSystem"@eng ;
	rdfs:subClassOf gold:LinguisticDataStructure ;
	rdfs:isDefinedBy "http://purl.org/linguistics/gold"^^<http://www.w3.org/2001/XMLSchema#anyURI> ;
	rdfs:comment "In a given language, the system according to which feature values (of a particular feature) are determined contextually for elements, through agreement or government.  FeatureDistributionSystem can have one or two main components: FeatureAgreementSystem, and FeatureGovernmentSystem."@eng .

gold:LinguisticDataStructure a owl:Class ;
	rdfs:label "LinguisticDataStructure"@eng ;
	rdfs:subClassOf gold:Abstract ;
	rdfs:isDefinedBy "http://purl.org/linguistics/gold"^^<http://www.w3.org/2001/XMLSchema#anyURI> ;
	rdfs:comment "A linguistic data structure is an abstract container for grouping together instances of linguistic data, usually to suit a particular theory or computational implementation. Examples include: feature structures, lexical entries, and paradigms."@eng .

gold:PersonProperty a owl:Class ;
	rdfs:label "PersonProperty"@eng ;
	rdfs:subClassOf gold:MorphosyntacticProperty ;
	rdfs:isDefinedBy "http://purl.org/linguistics/gold"^^<http://www.w3.org/2001/XMLSchema#anyURI> ;
	rdfs:comment "PersonProperty is the class of properties  with a deictic dimension, interpreted relative to the speaker, encoding the participants in a speech situation. Usually a three-way contrast is found: firstPerson (speaker), secondPerson (addressee), and thirdPerson (neither speaker nor addressee). Other distinctions within this feature include: inclusive/exclusive and proximative/obviative."@eng .

gold:FormUnit a owl:Class ;
	rdfs:label "FormUnit"@eng ;
	rdfs:subClassOf gold:LinguisticUnit ;
	rdfs:isDefinedBy "http://purl.org/linguistics/gold"^^<http://www.w3.org/2001/XMLSchema#anyURI> ;
	rdfs:comment "A FormUnit is any unit of linguistic form; the abstract form component of a linguistic sign. Subclasses include various phonology units such as Phoneme, Mora, PhonologicalWord, etc."@eng .

gold:FeatureAssignmentSystem a owl:Class ;
	rdfs:label "FeatureAssignmentSystem"@eng ;
	rdfs:subClassOf gold:LinguisticDataStructure ;
	rdfs:isDefinedBy "http://purl.org/linguistics/gold"^^<http://www.w3.org/2001/XMLSchema#anyURI> ;
	rdfs:comment "In a given language, the system according to which feature values (of a particular feature) are assigned inherently to elements, based on the elements' inherent formal or semantic properties."@eng .

gold:LaryngealProperty a owl:Class ;
	rdfs:label "LaryngealProperty"@eng ;
	rdfs:subClassOf gold:ArticulatoryProperty ;
	rdfs:isDefinedBy "http://purl.org/linguistics/gold"^^<http://www.w3.org/2001/XMLSchema#anyURI> ;
	rdfs:comment "[Need a definition.]"@eng .

gold:HeightProperty a owl:Class ;
	rdfs:label "HeightProperty"@eng ;
	rdfs:subClassOf gold:DorsalProperty ;
	rdfs:isDefinedBy "http://purl.org/linguistics/gold"^^<http://www.w3.org/2001/XMLSchema#anyURI> ;
	rdfs:comment "The class of features describing sounds based on the relative vertical position of the tongue. Note, Ladefoged refers to this feature as High."@eng .

gold:LinguisticSystem a owl:Class ;
	rdfs:label "LinguisticSystem"@eng ;
	rdfs:subClassOf gold:Abstract ;
	rdfs:isDefinedBy "http://purl.org/linguistics/gold"^^<http://www.w3.org/2001/XMLSchema#anyURI> ;
	rdfs:comment "LinguisticSystem is the class of languages, broadly construed. It includes human, animal, and computer language. Furthermore, it includes natural and constructed varieties as well as written, signed, and spoken varieties."@eng .

gold:Affix a owl:Class ;
	rdfs:label "Affix"@eng ;
	rdfs:subClassOf gold:MorphologicalUnit ;
	rdfs:isDefinedBy "http://purl.org/linguistics/gold"^^<http://www.w3.org/2001/XMLSchema#anyURI> .

gold:ProForm a owl:Class ;
	rdfs:label "ProForm"@eng ;
	rdfs:subClassOf gold:PartOfSpeechProperty ;
	rdfs:isDefinedBy "http://purl.org/linguistics/gold"^^<http://www.w3.org/2001/XMLSchema#anyURI> ;
	rdfs:comment "A ProForm is a partOfSpeech whose members usually substitute for other constituents, including phrases, clauses, or sentences, and whose meaning is recoverable from the linguistic or extralinguistic context [Schachter 1985,24-25; Crystal 1997,310]."@eng .

gold:UnaryPredicator a owl:Class ;
	rdfs:label "UnaryPredicator"@eng ;
	rdfs:subClassOf gold:Predicator ;
	rdfs:isDefinedBy "http://purl.org/linguistics/gold"^^<http://www.w3.org/2001/XMLSchema#anyURI> ;
	rdfs:comment "UnaryPredicator is the class of syntactic words that take only one required argument."@eng .

gold:CategoryChanger a owl:Class ;
	rdfs:label "CategoryChanger"@eng ;
	rdfs:subClassOf gold:DerivationalUnit ;
	rdfs:isDefinedBy "http://purl.org/linguistics/gold"^^<http://www.w3.org/2001/XMLSchema#anyURI> ;
	rdfs:comment "CategoryChanger is a cover class for all derivational units that change the syntactic category of the root to which they are attached."@eng .

gold:SemanticUnit a owl:Class ;
	rdfs:label "SemanticUnit"@eng ;
	rdfs:subClassOf gold:LinguisticUnit ;
	rdfs:isDefinedBy "http://purl.org/linguistics/gold"^^<http://www.w3.org/2001/XMLSchema#anyURI> ;
	rdfs:comment "A SemanticUnit is the class of semantics elements, or units of semantic structure (sometimes called a sememe). Semantic units serve as the meaning component of linguistic signs. A semantic unit is intended for linguistic description and no particular logical representation is implied."@eng .

gold:Glyph a owl:Class ;
	rdfs:label "Glyph"@eng ;
	rdfs:subClassOf gold:OrthographicPart ;
	rdfs:isDefinedBy "http://purl.org/linguistics/gold"^^<http://www.w3.org/2001/XMLSchema#anyURI> ;
	rdfs:comment "A Glyph is a symbol used in a writing system to represent some kind of linguistic unit, such as a single sound, a  phoneme or an entire word. Glyphs are concatenated in a writing system to form orthographic parts and orthographic words. Consider the printed word 'apple'. This word contains two instances of the 'p' glyph, which is a subclass of Glyph. Instances of a Glyph share a similar shape and can be called 'shapemes'. The class Glyph is not the same as Grapheme. A Grapheme is a contrastive unit within a particular writing system. The notion of a glyph is relevant across writing systems. For instance, consider the symbol 'р' used in a printed instance of a Russian word 'русский'. Now consider the symbol 'p' used in the printed instance of an English word 'pickle'. Both symbols are instances of the same Glyph. They share the same general shape, but do not have the same phonemic value."@eng .

gold:Object a owl:Class ;
	rdfs:label "Object"@eng ;
	rdfs:subClassOf owl:Thing ;
	rdfs:isDefinedBy "http://purl.org/linguistics/gold"^^<http://www.w3.org/2001/XMLSchema#anyURI> ;
	rdfs:comment "Any entity that is stable throughout time and has other objects as parts. At any point in time, an object is wholly present. See SUMO for a detailed explanation."@eng .

gold:Taxon a owl:Class ;
	rdfs:label "Taxon"@eng ;
	rdfs:subClassOf gold:Abstract ;
	rdfs:isDefinedBy "http://purl.org/linguistics/gold"^^<http://www.w3.org/2001/XMLSchema#anyURI> ;
	rdfs:comment "Taxon is the class of scientific categories used to create a taxonomy and determined according to scientific principles in a given domain, e.g., Biology or Linguistics."@eng .

gold:Clause a owl:Class ;
	rdfs:label "Clause"@eng ;
	rdfs:subClassOf gold:SyntacticConstruction ;
	rdfs:isDefinedBy "http://purl.org/linguistics/gold"^^<http://www.w3.org/2001/XMLSchema#anyURI> ;
	rdfs:comment "Clause is the class of constructions that form minimal sentential units. They must  include a predicate, all arguments of the predicate, and all modifiers of the predicate and the arguments."@eng .

gold:SupraLaryngealProperty a owl:Class ;
	rdfs:label "SupraLaryngealProperty"@eng ;
	rdfs:subClassOf gold:ArticulatoryProperty ;
	rdfs:isDefinedBy "http://purl.org/linguistics/gold"^^<http://www.w3.org/2001/XMLSchema#anyURI> ;
	rdfs:comment "Property of sounds characterized by focusing on the active articulator."@eng .

gold:RadicalProperty a owl:Class ;
	rdfs:label "RadicalProperty"@eng ;
	rdfs:subClassOf gold:PlaceProperty ;
	rdfs:isDefinedBy "http://purl.org/linguistics/gold"^^<http://www.w3.org/2001/XMLSchema#anyURI> ;
	rdfs:comment "The class of place  properties used to classifiy articulatory gestures made with the root of the tongue [Ladefoged 1997, 603]."@eng .

gold:VelaricProperty a owl:Class ;
	rdfs:label "VelaricProperty"@eng ;
	rdfs:subClassOf gold:AirstreamProperty ;
	rdfs:isDefinedBy "http://purl.org/linguistics/gold"^^<http://www.w3.org/2001/XMLSchema#anyURI> ;
	rdfs:comment "[Need a definition.]"@eng .

gold:PulmonicProperty a owl:Class ;
	rdfs:label "PulmonicProperty"@eng ;
	rdfs:subClassOf gold:AirstreamProperty ;
	rdfs:isDefinedBy "http://purl.org/linguistics/gold"^^<http://www.w3.org/2001/XMLSchema#anyURI> ;
	rdfs:comment "[Need a definition.]"@eng .

gold:NasalityProperty a owl:Class ;
	rdfs:label "NasalityProperty"@eng ;
	rdfs:subClassOf gold:SupraLaryngealProperty ;
	rdfs:isDefinedBy "http://purl.org/linguistics/gold"^^<http://www.w3.org/2001/XMLSchema#anyURI> ;
	rdfs:comment "The class of properties  used to characterize the degree to which air  escapes through the nose."@eng .

gold:GrammarUnit a owl:Class ;
	rdfs:label "GrammarUnit"@eng ;
	rdfs:subClassOf gold:LinguisticUnit ;
	rdfs:isDefinedBy "http://purl.org/linguistics/gold"^^<http://www.w3.org/2001/XMLSchema#anyURI> ;
	rdfs:comment "A GrammarUnit is the structural component of the linguistic sign and includes notions such as morpheme, syntactic word, and construction. Grammar units are classified according to their mereology (part-whole and complexity),  morphosyntactic function, and whether they exist in a bound or free forms."@eng .

gold:PolarityProperty a owl:Class ;
	rdfs:label "PolarityProperty"@eng ;
	rdfs:subClassOf gold:MorphosyntacticProperty ;
	rdfs:isDefinedBy "http://purl.org/linguistics/gold"^^<http://www.w3.org/2001/XMLSchema#anyURI> ;
	rdfs:comment "PolarityProperty is the class of properties that concern the grammatical encoding of negation. As a morphosyntactic property, generally only Negative is marked, i.e. associated with a linguistic expression."@eng .

gold:Classifier a owl:Class ;
	rdfs:label "Classifier"@eng ;
	rdfs:subClassOf gold:PartOfSpeechProperty ;
	rdfs:isDefinedBy "http://purl.org/linguistics/gold"^^<http://www.w3.org/2001/XMLSchema#anyURI> ;
	rdfs:comment "Classifier is a kind of operator used to indicate the syntactic class of some word."@eng .

gold:Particle a owl:Class ;
	rdfs:label "Particle"@eng ;
	rdfs:subClassOf gold:PartOfSpeechProperty ;
	rdfs:isDefinedBy "http://purl.org/linguistics/gold"^^<http://www.w3.org/2001/XMLSchema#anyURI> ;
	rdfs:comment "A particle is a part of speech whose members do not belong to one of the main classes of words, is invariable, and can have grammatical or semantic significance."@eng .

gold:Quantifier a owl:Class ;
	rdfs:label "Quantifier"@eng ;
	rdfs:subClassOf gold:Determiner ;
	rdfs:isDefinedBy "http://purl.org/linguistics/gold"^^<http://www.w3.org/2001/XMLSchema#anyURI> ;
	rdfs:comment "A quantifier is a determiner that expresses a referent's definite or indefinite  number or amount. A quantifier functions as a modifier of a noun, or a pronoun [Crystal 1997, 317]."@eng .

gold:WrittenLinguisticExpression a owl:Class ;
	rdfs:label "WrittenLinguisticExpression"@eng ;
	rdfs:subClassOf gold:LinguisticExpression ;
	rdfs:isDefinedBy "http://purl.org/linguistics/gold"^^<http://www.w3.org/2001/XMLSchema#anyURI> ;
	rdfs:comment "A WrittenLinguisticExpression is the written physical form of language as distinct from either signed or spoken expressions. A written expression is the physical product of the writing process."@eng .

gold:OrthographicPhrase a owl:Class ;
	rdfs:label "OrthographicPhrase"@eng ;
	rdfs:subClassOf gold:WrittenLinguisticExpression ;
	rdfs:isDefinedBy "http://purl.org/linguistics/gold"^^<http://www.w3.org/2001/XMLSchema#anyURI> ;
	rdfs:comment "An OrthographicPhrase is a sequence of orthographic words."@eng .

gold:EvaluativeProperty a owl:Class ;
	rdfs:label "EvaluativeProperty"@eng ;
	rdfs:subClassOf gold:MorphosyntacticProperty ;
	rdfs:isDefinedBy "http://purl.org/linguistics/gold"^^<http://www.w3.org/2001/XMLSchema#anyURI> ;
	rdfs:comment "EvaluativeProperty is the class of properties that concern the grammatical encoding of judged value. These properties are associated with nominals that generally indicate that the referent is viewed favorably or unfavorably by the speaker."@eng .

gold:Adposition a owl:Class ;
	rdfs:label "Adposition"@eng ;
	rdfs:subClassOf gold:Functor ;
	rdfs:isDefinedBy "http://purl.org/linguistics/gold"^^<http://www.w3.org/2001/XMLSchema#anyURI> ;
	rdfs:comment "An adposition is a part of speech whose members are of a closed set and occur before or after a complement composed of a noun phrase, noun, pronoun, or clause that functions as a noun phrase and forms a single structure with the complement to express its grammatical and semantic relation to another unit within a clause [Comrie 1989,91; Crystal 1997, 305; Payne 1997,86]."@eng .

gold:AirstreamProperty a owl:Class ;
	rdfs:label "AirstreamProperty"@eng ;
	rdfs:subClassOf gold:ArticulatoryProperty ;
	rdfs:isDefinedBy "http://purl.org/linguistics/gold"^^<http://www.w3.org/2001/XMLSchema#anyURI> ;
	rdfs:comment "[Need a definition.]"@eng .

gold:DiscourseProperty a owl:Class ;
	rdfs:label "DiscourseProperty"@eng ;
	rdfs:subClassOf gold:LinguisticProperty ;
	rdfs:isDefinedBy "http://purl.org/linguistics/gold"^^<http://www.w3.org/2001/XMLSchema#anyURI> .

gold:LinguisticExpression a owl:Class ;
	rdfs:label "LinguisticExpression"@eng ;
	rdfs:subClassOf gold:Object ;
	rdfs:isDefinedBy "http://purl.org/linguistics/gold"^^<http://www.w3.org/2001/XMLSchema#anyURI> ;
	rdfs:comment "A LinguisticExpression is any physical form (sound, visual image or sequence thereof) used to represent a linguistic unit. A linguistic expression may be spoken, written, or signed. A linguistic expression is distinct form the actual proces (speaking, writing, signing) that produces the expression."@eng .

gold:MannerProperty a owl:Class ;
	rdfs:label "MannerProperty"@eng ;
	rdfs:subClassOf gold:SupraLaryngealProperty ;
	rdfs:isDefinedBy "http://purl.org/linguistics/gold"^^<http://www.w3.org/2001/XMLSchema#anyURI> ;
	rdfs:comment "A property of sounds that focuses on the active articulator and how the airstream is obstructed."@eng .

gold:SyntacticUnit a owl:Class ;
	rdfs:label "SyntacticUnit"@eng ;
	rdfs:subClassOf gold:GrammarUnit ;
	rdfs:isDefinedBy "http://purl.org/linguistics/gold"^^<http://www.w3.org/2001/XMLSchema#anyURI> ;
	rdfs:comment "SyntacticUnit is the class of grammatical units whose members make up the constituents of syntactic constructions. They are the product of syntactic analysis. Syntactic units participate in syntactic relations, e.g.,  constituency or syntactic function relations."@eng .

gold:TrillProperty a owl:Class ;
	rdfs:label "TrillProperty"@eng ;
	rdfs:subClassOf gold:MannerProperty ;
	rdfs:isDefinedBy "http://purl.org/linguistics/gold"^^<http://www.w3.org/2001/XMLSchema#anyURI> ;
	rdfs:comment "A subclass of MannerFeature used to distinguish the various types of trills."@eng .

gold:BinaryPredicator a owl:Class ;
	rdfs:label "BinaryPredicator"@eng ;
	rdfs:subClassOf gold:Predicator ;
	rdfs:isDefinedBy "http://purl.org/linguistics/gold"^^<http://www.w3.org/2001/XMLSchema#anyURI> ;
	rdfs:comment "BinaryPredicator is the class of syntactic words that take two required arguments."@eng .

gold:VoicingProperty a owl:Class ;
	rdfs:label "VoicingProperty"@eng ;
	rdfs:subClassOf gold:LaryngealProperty ;
	rdfs:isDefinedBy "http://purl.org/linguistics/gold"^^<http://www.w3.org/2001/XMLSchema#anyURI> ;
	rdfs:comment "[Need a definition.]"@eng .

gold:AbessiveCase a owl:Class ;
	rdfs:label "AbessiveCase"@eng ;
	rdfs:subClassOf gold:CaseProperty ;
	rdfs:isDefinedBy "http://purl.org/linguistics/gold"^^<http://www.w3.org/2001/XMLSchema#anyURI> ;
	rdfs:comment "AbessiveCase expresses the lack or absence of the referent of the noun it marks. It has the meaning of the English preposition 'without' [Pei and Gaynor 1954, 3, 35]."@eng .

gold:AbilitativeModality a owl:Class ;
	rdfs:label "AbilitativeModality"@eng ;
	rdfs:subClassOf gold:ModalityProperty ;
	rdfs:isDefinedBy "http://purl.org/linguistics/gold"^^<http://www.w3.org/2001/XMLSchema#anyURI> ;
	rdfs:comment "AbilitativeModality indicates the capacity of an agent to perform some action, regardless of type or condition. This is also known as the abilitive."@eng .

gold:AblativeCase a owl:Class ;
	rdfs:label "AblativeCase"@eng ;
	rdfs:subClassOf gold:CaseProperty ;
	rdfs:isDefinedBy "http://purl.org/linguistics/gold"^^<http://www.w3.org/2001/XMLSchema#anyURI> ;
	rdfs:comment "AblativeCase expresses that  the referent of the noun it marks is the location from which another referent is moving. It has the meaning 'from'."@eng .

gold:AbsolutiveAntipassiveVoice a owl:Class ;
	rdfs:label "AbsolutiveAntipassiveVoice"@eng ;
	rdfs:subClassOf gold:VoiceProperty ;
	rdfs:isDefinedBy "http://purl.org/linguistics/gold"^^<http://www.w3.org/2001/XMLSchema#anyURI> ;
	rdfs:comment "An Antipassive in which the P or logical object is suppressed or overtly absent. [Klaiman 1991,232]"@eng .

gold:AbsolutiveCase a owl:Class ;
	rdfs:label "AbsolutiveCase"@eng ;
	rdfs:subClassOf gold:CaseProperty ;
	rdfs:isDefinedBy "http://purl.org/linguistics/gold"^^<http://www.w3.org/2001/XMLSchema#anyURI> ;
	rdfs:comment "AbsolutiveCase in ergative-absolutive languages mark referents that would generally be the subjects of intransitive verbs or the objects of transitive verbs in the translational equivalents of nominative-accusative languages [Anderson 1985, 181; Crystal 1985, 1; Andrews 1985, 138]."@eng .

gold:AccusativeCase a owl:Class ;
	rdfs:label "AccusativeCase"@eng ;
	rdfs:subClassOf gold:CaseProperty ;
	rdfs:isDefinedBy "http://purl.org/linguistics/gold"^^<http://www.w3.org/2001/XMLSchema#anyURI> ;
	rdfs:comment "AccusativeCase in nominative-accusative languages marks certain syntactic functions, usually direct objects [Hartmann and Stork 1972, 3,156; Crystal 1980, 11,246; Andrews 1985, 75; Anderson 1985, 181]."@eng .

gold:AcousticProperty a owl:Class ;
	rdfs:label "AcousticProperty"@eng ;
	rdfs:subClassOf gold:PhoneticProperty ;
	rdfs:isDefinedBy "http://purl.org/linguistics/gold"^^<http://www.w3.org/2001/XMLSchema#anyURI> ;
	rdfs:comment "The class of properties concerning the acoustic nature of speech sounds."@eng .

gold:ActionalForce a owl:Class ;
	rdfs:label "ActionalForce"@eng ;
	rdfs:subClassOf gold:ForceProperty ;
	rdfs:isDefinedBy "http://purl.org/linguistics/gold"^^<http://www.w3.org/2001/XMLSchema#anyURI> ;
	rdfs:comment "ActionalForce indicates that the speaker or hearer is to undertake some action. Subsumes Imperative, Commissive and Hortatory."@eng .

gold:ActiveVoice a owl:Class ;
	rdfs:label "ActiveVoice"@eng ;
	rdfs:subClassOf gold:VoiceProperty ;
	rdfs:isDefinedBy "http://purl.org/linguistics/gold"^^<http://www.w3.org/2001/XMLSchema#anyURI> ;
	rdfs:comment """Associated with transitivity, when the action is performed by an agent (subject) on another participant (object), or with intransitivity [McIntosh 1984, 108]. Refers to the category of underived verb forms associated with the basic diathesis: Diathesis=D0:(X=SUBabs/nom) (Y=DIROBacc)
[Shibatani 1995, 7]"""@eng .

gold:AdessiveCase a owl:Class ;
	rdfs:label "AdessiveCase"@eng ;
	rdfs:subClassOf gold:CaseProperty ;
	rdfs:isDefinedBy "http://purl.org/linguistics/gold"^^<http://www.w3.org/2001/XMLSchema#anyURI> ;
	rdfs:comment "AdessiveCase expresses that  the referent of the noun it marks is the location near/at which another referent exists. It has the meaning of 'at' or 'near' [Crystal 1997, 8]."@eng .

gold:AdjectivePhrase a owl:Class ;
	rdfs:label "AdjectivePhrase"@eng ;
	rdfs:subClassOf gold:Phrase ;
	rdfs:isDefinedBy "http://purl.org/linguistics/gold"^^<http://www.w3.org/2001/XMLSchema#anyURI> ;
	rdfs:comment "AdjectivePhrase is the class of phrases that have adjectives as heads."@eng .

gold:AdjunctSubordinate a owl:Class ;
	rdfs:label "AdjunctSubordinate"@eng ;
	rdfs:subClassOf gold:SubordinateClause ;
	rdfs:isDefinedBy "http://purl.org/linguistics/gold"^^<http://www.w3.org/2001/XMLSchema#anyURI> ;
	rdfs:comment "suggested at E-MELD  (no documentation yet)"@eng .

gold:Adverbial a owl:Class ;
	rdfs:label "Adverbial"@eng ;
	rdfs:subClassOf gold:Predicator ;
	rdfs:isDefinedBy "http://purl.org/linguistics/gold"^^<http://www.w3.org/2001/XMLSchema#anyURI> ;
	rdfs:comment "An adverbial, or 'adverb', narrowly defined, is a part of speech whose members modify verbs for such categories as time, manner, place, or direction. An adverbal, broadly defined, is a part of speech whose members modify any constituent class of words other than nouns, such as  verbs, adjectives, adverbs, phrases, clauses, or sentences. Under this definition, the possible type of modification depends on the class of the constituent being modified [Crystal 1997,11; Payne 1997,69]."@eng .

gold:Adverbializer a owl:Class ;
	rdfs:label "Adverbializer"@eng ;
	rdfs:subClassOf gold:SubordinatingConnective ;
	rdfs:isDefinedBy "http://purl.org/linguistics/gold"^^<http://www.w3.org/2001/XMLSchema#anyURI> ;
	rdfs:comment "An adverbializer is a subordinating connective that links a subordinate clause  to a main clause, and indicates that the subordinate clause has an adverbial or interpropositional relation  to the main clause, indicating purpose, condition, time, and location."@eng .

gold:AgentDeletionPassiveVoice a owl:Class ;
	rdfs:label "AgentDeletionPassiveVoice"@eng ;
	rdfs:subClassOf gold:VoiceProperty ;
	rdfs:isDefinedBy "http://purl.org/linguistics/gold"^^<http://www.w3.org/2001/XMLSchema#anyURI> ;
	rdfs:comment """The object of the active retains its old case-marking in the passive, the subject of the active cannot appear in the passive clause, and the passive tends to be semantically active.
[Givon 1988,419]"""@eng .

gold:AllativeCase a owl:Class ;
	rdfs:label "AllativeCase"@eng ;
	rdfs:subClassOf gold:CaseProperty ;
	rdfs:isDefinedBy "http://purl.org/linguistics/gold"^^<http://www.w3.org/2001/XMLSchema#anyURI> ;
	rdfs:comment "AllativeCase expresses motion to or toward the referent of the noun it marks [Pei and Gaynor 1954, 6,9,216; Lyons 1968, 299; Crystal 1985, 1213]."@eng .

gold:Alveolar a owl:Class ;
	rdfs:label "Alveolar"@eng ;
	rdfs:subClassOf gold:AnteriorProperty ;
	rdfs:isDefinedBy "http://purl.org/linguistics/gold"^^<http://www.w3.org/2001/XMLSchema#anyURI> ;
	rdfs:comment "Characterizing sounds produced with the alveolar ridge as the passive articulator [Ladefoged 1997, 598]."@eng .

gold:AnimateGender a owl:Class ;
	rdfs:label "AnimateGender"@eng ;
	rdfs:subClassOf gold:GenderProperty ;
	rdfs:isDefinedBy "http://purl.org/linguistics/gold"^^<http://www.w3.org/2001/XMLSchema#anyURI> ;
	rdfs:comment "A grammatical gender  property assigned to a class of nouns with animate denotation. In a given language it may include larger or smaller numbers of nouns which do not meet this semantic criterion. The animate gender may occur in a two-gender system, with the other gender being labelled inanimate. However, the animate gender may also occur in larger inventories (i.e. greater than two values). Examples of these larger systems are found in Bantu languages (where nouns denoting humans are included in the animate gender) and in languages of Daghestan (where the animate gender is typically for non-human animates) [Corbett 1991, 20-32].@en"@eng .

gold:AntiCausativeVoice a owl:Class ;
	rdfs:label "AntiCausativeVoice"@eng ;
	rdfs:subClassOf gold:VoiceProperty ;
	rdfs:isDefinedBy "http://purl.org/linguistics/gold"^^<http://www.w3.org/2001/XMLSchema#anyURI> ;
	rdfs:comment """An intransitive verb is derived from a basically transitive one with the direct object of the transitive verb corresponding to the subject of the intransitive.
[Siewierska 1988,267]"""@eng , """An intransitive verb is derived from a basically transitive one with the direct object of the transitive verb corresponding to the subject of the intransitive.
[Siewierska 1988,267]@en"""@eng .

gold:AntiPassiveVoice a owl:Class ;
	rdfs:label "AntiPassiveVoice"@eng ;
	rdfs:subClassOf gold:VoiceProperty ;
	rdfs:isDefinedBy "http://purl.org/linguistics/gold"^^<http://www.w3.org/2001/XMLSchema#anyURI> ;
	rdfs:comment "Derives an intransitive verb from a transitive stem whereby the original agent (only) is cross-referrenced by the absolutive markers on the verb and the original patient, if it appears, is in an oblique phrase. [England 1983,110]"@eng .

gold:Apical a owl:Class ;
	rdfs:label "Apical"@eng ;
	rdfs:subClassOf gold:ApicalityProperty ;
	rdfs:isDefinedBy "http://purl.org/linguistics/gold"^^<http://www.w3.org/2001/XMLSchema#anyURI> ;
	rdfs:comment "Characterizing sounds produced by the tip of the tongue [Ladefoged 1997, 596]."@eng .

gold:ApplicativeVoice a owl:Class ;
	rdfs:label "ApplicativeVoice"@eng ;
	rdfs:subClassOf gold:VoiceProperty ;
	rdfs:isDefinedBy "http://purl.org/linguistics/gold"^^<http://www.w3.org/2001/XMLSchema#anyURI> ;
	rdfs:comment "painted the door green"@eng .

gold:Approximant a owl:Class ;
	rdfs:label "Approximant"@eng ;
	rdfs:subClassOf gold:StrictureProperty ;
	rdfs:isDefinedBy "http://purl.org/linguistics/gold"^^<http://www.w3.org/2001/XMLSchema#anyURI> ;
	rdfs:comment "[Need comment]"@eng .

gold:ArabicNumeralGender a owl:Class ;
	rdfs:label "ArabicNumeralGender"@eng ;
	rdfs:subClassOf gold:GenderProperty ;
	rdfs:isDefinedBy "http://purl.org/linguistics/gold"^^<http://www.w3.org/2001/XMLSchema#anyURI> ;
	rdfs:comment "[Need comment]"@eng .

gold:Aspirated a owl:Class ;
	rdfs:label "Aspirated"@eng ;
	rdfs:subClassOf gold:GlottalTimingProperty ;
	rdfs:isDefinedBy "http://purl.org/linguistics/gold"^^<http://www.w3.org/2001/XMLSchema#anyURI> ;
	rdfs:comment "[Need comment]"@eng .

gold:AssumptiveEvidentiality a owl:Class ;
	rdfs:label "AssumptiveEvidentiality"@eng ;
	rdfs:subClassOf gold:EvidentialityProperty ;
	rdfs:isDefinedBy "http://purl.org/linguistics/gold"^^<http://www.w3.org/2001/XMLSchema#anyURI> ;
	rdfs:comment "AssumptiveEvidentiality encodes the fact that the speaker came to believe the content of the expression through a possibly unsound inference procedure. That is, it is at least reasonalbe [Palmer 2001, 6-8]."@eng .

gold:AttestedVariety a owl:Class ;
	rdfs:label "AttestedVariety"@eng ;
	rdfs:subClassOf gold:HumanLanguageVariety ;
	rdfs:isDefinedBy "http://purl.org/linguistics/gold"^^<http://www.w3.org/2001/XMLSchema#anyURI> ;
	rdfs:comment "AttestedVariety is the class of human language varieties that have been observed by a linguist, and for which there is at least some record and/or data. Examples of attested varieties include all of the language varieties mentioned in the Ethnologue."@eng .

gold:AuditoryEvidentiality a owl:Class ;
	rdfs:label "AuditoryEvidentiality"@eng ;
	rdfs:subClassOf gold:EvidentialityProperty ;
	rdfs:isDefinedBy "http://purl.org/linguistics/gold"^^<http://www.w3.org/2001/XMLSchema#anyURI> ;
	rdfs:comment "AuditoryEvidentiality encodes the fact that the speaker came to believe the content of the expression through direct auditory experience; they heard it. This does not include spoken reported accounts, but only direct sensory evidence, such as the situation of 'hearing a tree fall' [Palmer 2001, 38]."@eng .

gold:AugmentativeSize a owl:Class ;
	rdfs:label "AugmentativeSize"@eng ;
	rdfs:subClassOf gold:SizeProperty ;
	rdfs:isDefinedBy "http://purl.org/linguistics/gold"^^<http://www.w3.org/2001/XMLSchema#anyURI> ;
	rdfs:comment "A special form of a noun that signals that the object being referred to is large relative to the usual size of such an object [Crystal 1980, 34]."@eng .

gold:Auxiliary a owl:Class ;
	rdfs:label "Auxiliary"@eng ;
	rdfs:subClassOf gold:Verbal ;
	rdfs:isDefinedBy "http://purl.org/linguistics/gold"^^<http://www.w3.org/2001/XMLSchema#anyURI> .

gold:AversiveCase a owl:Class ;
	rdfs:label "AversiveCase"@eng ;
	rdfs:subClassOf gold:CaseProperty ;
	rdfs:isDefinedBy "http://purl.org/linguistics/gold"^^<http://www.w3.org/2001/XMLSchema#anyURI> ;
	rdfs:comment "AversiveCase expresses fear or is literally translated as 'turning from' in some languages [Blake 2001, 156]."@eng .

gold:Back a owl:Class ;
	rdfs:label "Back"@eng ;
	rdfs:subClassOf gold:BacknessProperty ;
	rdfs:isDefinedBy "http://purl.org/linguistics/gold"^^<http://www.w3.org/2001/XMLSchema#anyURI> ;
	rdfs:comment "Characterizing sounds produced with the tongue  near the back of the mouth."@eng .

gold:BenefactiveCase a owl:Class ;
	rdfs:label "BenefactiveCase"@eng ;
	rdfs:subClassOf gold:CaseProperty ;
	rdfs:isDefinedBy "http://purl.org/linguistics/gold"^^<http://www.w3.org/2001/XMLSchema#anyURI> ;
	rdfs:comment "BenefactiveCase expresses that the referent of the noun it marks receives the benefit of the situation expressed by the clause [Crystal 1980, 43]."@eng .

gold:Breathy a owl:Class ;
	rdfs:label "Breathy"@eng ;
	rdfs:subClassOf gold:GlottalStrictureProperty ;
	rdfs:isDefinedBy "http://purl.org/linguistics/gold"^^<http://www.w3.org/2001/XMLSchema#anyURI> ;
	rdfs:comment "[Need comment]"@eng .

gold:CardinalNumeral a owl:Class ;
	rdfs:label "CardinalNumeral"@eng ;
	rdfs:subClassOf gold:Numeral ;
	rdfs:isDefinedBy "http://purl.org/linguistics/gold"^^<http://www.w3.org/2001/XMLSchema#anyURI> ;
	rdfs:comment "A cardinal numeral is a numeral of the class whose members are considered basic in form, are used in counting, and are used in expressing how many objects are referred to [Crystal 1997,52]."@eng .

gold:CausativeVoice a owl:Class ;
	rdfs:label "CausativeVoice"@eng ;
	rdfs:subClassOf gold:VoiceProperty ;
	rdfs:isDefinedBy "http://purl.org/linguistics/gold"^^<http://www.w3.org/2001/XMLSchema#anyURI> ;
	rdfs:comment "Expressing the causation of an action."@eng .

gold:Central a owl:Class ;
	rdfs:label "Central"@eng ;
	rdfs:subClassOf gold:BacknessProperty ;
	rdfs:isDefinedBy "http://purl.org/linguistics/gold"^^<http://www.w3.org/2001/XMLSchema#anyURI> ;
	rdfs:comment "Characterizing sounds produced with the tongue  near the center of the mouth (along the front-back dimension)."@eng .

gold:CentralEscape a owl:Class ;
	rdfs:label "CentralEscape"@eng ;
	rdfs:subClassOf gold:LateralProperty ;
	rdfs:isDefinedBy "http://purl.org/linguistics/gold"^^<http://www.w3.org/2001/XMLSchema#anyURI> ;
	rdfs:comment "Characterizing sounds produced with a release of air through the center of the mouth. (Note, [Ladefoged 1997] refers to this value as central.)"@eng .

gold:Character a owl:Class ;
	rdfs:label "Character"@eng ;
	rdfs:subClassOf gold:Abstract ;
	rdfs:isDefinedBy "http://purl.org/linguistics/gold"^^<http://www.w3.org/2001/XMLSchema#anyURI> ;
	rdfs:comment "A Character is the computational equivalent of a grapheme. For instance, a Unicode code point represents an instance of a character, such as LATIN CAPITAL LETTER A."@eng .

gold:CloseFutureTense a owl:Class ;
	rdfs:label "CloseFutureTense"@eng ;
	rdfs:subClassOf gold:TenseProperty ;
	rdfs:isDefinedBy "http://purl.org/linguistics/gold"^^<http://www.w3.org/2001/XMLSchema#anyURI> ;
	rdfs:comment ""@eng , "@en"@eng .

gold:Closed a owl:Class ;
	rdfs:label "Closed"@eng ;
	rdfs:subClassOf gold:GlottalStrictureProperty ;
	rdfs:isDefinedBy "http://purl.org/linguistics/gold"^^<http://www.w3.org/2001/XMLSchema#anyURI> ;
	rdfs:comment "[Need comment]"@eng .

gold:CoVerb a owl:Class ;
	rdfs:label "CoVerb"@eng ;
	rdfs:subClassOf gold:Verbal ;
	rdfs:isDefinedBy "http://purl.org/linguistics/gold"^^<http://www.w3.org/2001/XMLSchema#anyURI> .

gold:ComitativeCase a owl:Class ;
	rdfs:label "ComitativeCase"@eng ;
	rdfs:subClassOf gold:CaseProperty ;
	rdfs:isDefinedBy "http://purl.org/linguistics/gold"^^<http://www.w3.org/2001/XMLSchema#anyURI> ;
	rdfs:comment "ComitativeCase expresses accompaniment. It carries the meaning 'with' or 'accompanied by' [Anderson 1985, 186; Pei and Gaynor 1954, 42; Dixon, R. 1972, 12]."@eng .

gold:CommissiveForce a owl:Class ;
	rdfs:label "CommissiveForce"@eng ;
	rdfs:subClassOf gold:ForceProperty ;
	rdfs:isDefinedBy "http://purl.org/linguistics/gold"^^<http://www.w3.org/2001/XMLSchema#anyURI> ;
	rdfs:comment "CommisiveForce indicates that the speaker promises or threatens to perform some action [Palmer 2001, 10, 72]."@eng .

gold:CommonNoun a owl:Class ;
	rdfs:label "CommonNoun"@eng ;
	rdfs:subClassOf gold:Noun ;
	rdfs:isDefinedBy "http://purl.org/linguistics/gold"^^<http://www.w3.org/2001/XMLSchema#anyURI> ;
	rdfs:comment "no documentation yet"@eng .

gold:ComparativeAdjective a owl:Class ;
	rdfs:label "ComparativeAdjective"@eng ;
	rdfs:subClassOf gold:Adjectival ;
	rdfs:isDefinedBy "http://purl.org/linguistics/gold"^^<http://www.w3.org/2001/XMLSchema#anyURI> ;
	rdfs:comment "suggested at E-MELD  (no documentation yet)"@eng .

gold:ComplementSubordinate a owl:Class ;
	rdfs:label "ComplementSubordinate"@eng ;
	rdfs:subClassOf gold:SubordinateClause ;
	rdfs:isDefinedBy "http://purl.org/linguistics/gold"^^<http://www.w3.org/2001/XMLSchema#anyURI> ;
	rdfs:comment "suggested at E-MELD  (no documentation yet)"@eng .

gold:Complementizer a owl:Class ;
	rdfs:label "Complementizer"@eng ;
	rdfs:subClassOf gold:SubordinatingConnective ;
	rdfs:isDefinedBy "http://purl.org/linguistics/gold"^^<http://www.w3.org/2001/XMLSchema#anyURI> ;
	rdfs:comment "A complementizer is a connective which marks a complement clause [Crystal 1997,75]."@eng .

gold:CompletiveAspect a owl:Class ;
	rdfs:label "CompletiveAspect"@eng ;
	rdfs:subClassOf gold:AspectProperty ;
	rdfs:isDefinedBy "http://purl.org/linguistics/gold"^^<http://www.w3.org/2001/XMLSchema#anyURI> ;
	rdfs:comment "[Bybee, Perkins and Pagliuca, 1984]"@eng , "CompletiveAspect"@eng .

gold:ComplexSpecification a owl:Class ;
	rdfs:label "ComplexSpecification"@eng ;
	rdfs:subClassOf gold:FeatureSpecification ;
	rdfs:isDefinedBy "http://purl.org/linguistics/gold"^^<http://www.w3.org/2001/XMLSchema#anyURI> ;
	rdfs:comment "A ComplexSpecification is a kind of FeatureSpecification whose value must be a FeatureStructure. This class gives a feature system its recursive properites [Maxwell, Simons, and Hayashi 2000]."@eng .

gold:Compound a owl:Class ;
	rdfs:label "Compound"@eng ;
	rdfs:subClassOf gold:MorphologicalUnit ;
	rdfs:isDefinedBy "http://purl.org/linguistics/gold"^^<http://www.w3.org/2001/XMLSchema#anyURI> ;
	rdfs:comment "Compound is the class of complex units whose members are composed of at least two roots."@eng .

gold:Compressed a owl:Class ;
	rdfs:label "Compressed"@eng ;
	rdfs:subClassOf gold:LabialProperty ;
	rdfs:isDefinedBy "http://purl.org/linguistics/gold"^^<http://www.w3.org/2001/XMLSchema#anyURI> ;
	rdfs:comment "One of the three types of Labial that can be associated with sounds involving lip compression involving the vertical movement of one lip towards the other. Such a property is associated with a normal bilabial stop."@eng .

gold:ConVerb a owl:Class ;
	rdfs:label "ConVerb"@eng ;
	rdfs:subClassOf gold:Verbal ;
	rdfs:isDefinedBy "http://purl.org/linguistics/gold"^^<http://www.w3.org/2001/XMLSchema#anyURI> .

gold:ConditionalModality a owl:Class ;
	rdfs:label "ConditionalModality"@eng ;
	rdfs:subClassOf gold:ModalityProperty ;
	rdfs:isDefinedBy "http://purl.org/linguistics/gold"^^<http://www.w3.org/2001/XMLSchema#anyURI> ;
	rdfs:comment "ConditionalModality"@eng .

gold:ConditionalPhysicalAbilitiveModality a owl:Class ;
	rdfs:label "ConditionalPhysicalAbilitiveModality"@eng ;
	rdfs:subClassOf gold:ModalityProperty ;
	rdfs:isDefinedBy "http://purl.org/linguistics/gold"^^<http://www.w3.org/2001/XMLSchema#anyURI> ;
	rdfs:comment "ConditionalPhysicalAbilitiveModality indicates ability of an agent to perform some action, requiring the presence of conditions external to the agent [Bybee, Perkins, and Pagliuca 1994, 177; Palmer 2001, 76]"@eng .

gold:Conjunction a owl:Class ;
	rdfs:label "Conjunction"@eng ;
	rdfs:subClassOf gold:CoordinatingConnective ;
	rdfs:isDefinedBy "http://purl.org/linguistics/gold"^^<http://www.w3.org/2001/XMLSchema#anyURI> ;
	rdfs:comment "no documentation yet"@eng .

gold:Consonant a owl:Class ;
	rdfs:label "Consonant"@eng ;
	rdfs:subClassOf gold:Segment ;
	rdfs:isDefinedBy "http://purl.org/linguistics/gold"^^<http://www.w3.org/2001/XMLSchema#anyURI> .

gold:ContablativeCase a owl:Class ;
	rdfs:label "ContablativeCase"@eng ;
	rdfs:subClassOf gold:CaseProperty ;
	rdfs:isDefinedBy "http://purl.org/linguistics/gold"^^<http://www.w3.org/2001/XMLSchema#anyURI> ;
	rdfs:comment "ContablativeCase expresses that  the referent of the noun it marks is the location 'from near' which another referent is moving. It has the meaning 'from near'."@eng .

gold:ContallativeCase a owl:Class ;
	rdfs:label "ContallativeCase"@eng ;
	rdfs:subClassOf gold:CaseProperty ;
	rdfs:isDefinedBy "http://purl.org/linguistics/gold"^^<http://www.w3.org/2001/XMLSchema#anyURI> ;
	rdfs:comment "ContallativeCase expresses that  something is moving toward the vicinity of the referent of the noun it marks. It has the meaning  'towards the vicinity of'."@eng .

gold:ConterminativeCase a owl:Class ;
	rdfs:label "ConterminativeCase"@eng ;
	rdfs:subClassOf gold:CaseProperty ;
	rdfs:isDefinedBy "http://purl.org/linguistics/gold"^^<http://www.w3.org/2001/XMLSchema#anyURI> ;
	rdfs:comment "ConterminativeCase expresses the notion of something moving into the vicinity of the referent of the noun it marks, but not through that region. It has the meaning 'moving into the vicinity of'."@eng .

gold:ContextOfUseTaxon a owl:Class ;
	rdfs:label "ContextOfUseTaxon"@eng ;
	rdfs:subClassOf gold:LinguisticTaxon ;
	rdfs:isDefinedBy "http://purl.org/linguistics/gold"^^<http://www.w3.org/2001/XMLSchema#anyURI> ;
	rdfs:comment "ContextOfUseTaxon is the class of taxons whose instances  classify language varieties according to how they are primarly used."@eng .

gold:ContinuousAspect a owl:Class ;
	rdfs:label "ContinuousAspect"@eng ;
	rdfs:subClassOf gold:AspectProperty ;
	rdfs:isDefinedBy "http://purl.org/linguistics/gold"^^<http://www.w3.org/2001/XMLSchema#anyURI> ;
	rdfs:comment """A value of Aspect Property assigned to the designated element in the clause when the meaning selected for the clause is that which indicates that the situation spoken about has internal temporal structure, but the situation cannot be regarded as habitual (i.e. it cannot be regarded as a characteristic feature of a whole period). Hence, continuousness can be defined negatively as imperfectivity that is not habituality [Comrie 1976, 26-32], and it can be regarded as a sub-type of imperfectivity.

Typically, for an aspect value to be labelled as Continuous, the aspectual meaning has to minimally express continuousness, although it may additionally express other temporal, aspectual, or modal meanings, or actionality distinctions.

Continuous aspectual meaning can be further subdivided into two types: progressive meaning and nonprogressive meaning. These two aspectual meanings may or may not be grammaticalised as separate aspect values."""@eng .

gold:ContlativeCase a owl:Class ;
	rdfs:label "ContlativeCase"@eng ;
	rdfs:subClassOf gold:CaseProperty ;
	rdfs:isDefinedBy "http://purl.org/linguistics/gold"^^<http://www.w3.org/2001/XMLSchema#anyURI> ;
	rdfs:comment "ContlativeCase expresses that  the referent of the noun it marks is the location in the vicinity of which another referent is moving. It has the meaning 'in the vicinity of'."@eng .

gold:Copula a owl:Class ;
	rdfs:label "Copula"@eng ;
	rdfs:subClassOf gold:Verbal ;
	rdfs:isDefinedBy "http://purl.org/linguistics/gold"^^<http://www.w3.org/2001/XMLSchema#anyURI> .

gold:Copulative a owl:Class ;
	rdfs:label "Copulative"@eng ;
	rdfs:subClassOf gold:Verbal ;
	rdfs:isDefinedBy "http://purl.org/linguistics/gold"^^<http://www.w3.org/2001/XMLSchema#anyURI> ;
	rdfs:comment "A type of Verb, e.g., 'seem' and 'appear'."@eng .

gold:CorrelativeConnective a owl:Class ;
	rdfs:label "CorrelativeConnective"@eng ;
	rdfs:subClassOf gold:CoordinatingConnective ;
	rdfs:isDefinedBy "http://purl.org/linguistics/gold"^^<http://www.w3.org/2001/XMLSchema#anyURI> ;
	rdfs:comment "A correlative connective is either of a pair of  coordinating conjunctions (connectives) used in ordered fashion. Typically, one is used immediately before each member of a pair of constituents [Crystal 1997,96]."@eng .

gold:Creaky a owl:Class ;
	rdfs:label "Creaky"@eng ;
	rdfs:subClassOf gold:GlottalStrictureProperty ;
	rdfs:isDefinedBy "http://purl.org/linguistics/gold"^^<http://www.w3.org/2001/XMLSchema#anyURI> ;
	rdfs:comment "[Need comment]"@eng .

gold:DativeCase a owl:Class ;
	rdfs:label "DativeCase"@eng ;
	rdfs:subClassOf gold:CaseProperty ;
	rdfs:isDefinedBy "http://purl.org/linguistics/gold"^^<http://www.w3.org/2001/XMLSchema#anyURI> ;
	rdfs:comment "DativeCase marks 1) Indirect objects (for languages in which they are held to exist) or 2) nouns having the role of recipient (as of things given), beneficiary of an action, or possessor of an item [Crystal 1980, 102]."@eng .

gold:DeclarativeForce a owl:Class ;
	rdfs:label "DeclarativeForce"@eng ;
	rdfs:subClassOf gold:ForceProperty ;
	rdfs:isDefinedBy "http://purl.org/linguistics/gold"^^<http://www.w3.org/2001/XMLSchema#anyURI> ;
	rdfs:comment "DeclarativeForce indicates that the speaker is informing the hearer about the content of what is said."@eng .

gold:DeductiveEvidentiality a owl:Class ;
	rdfs:label "DeductiveEvidentiality"@eng ;
	rdfs:subClassOf gold:EvidentialityProperty ;
	rdfs:isDefinedBy "http://purl.org/linguistics/gold"^^<http://www.w3.org/2001/XMLSchema#anyURI> ;
	rdfs:comment "DeductiveEvidentiality encodes the fact that the speaker came to believe the content of the expression through a sound inference procedure. [Palmer 2001, 6-8]."@eng .

gold:DefiniteArticle a owl:Class ;
	rdfs:label "DefiniteArticle"@eng ;
	rdfs:subClassOf gold:Article ;
	rdfs:isDefinedBy "http://purl.org/linguistics/gold"^^<http://www.w3.org/2001/XMLSchema#anyURI> ;
	rdfs:comment "An definite article is a part of speech whose members refer to a specific, identifiable entity (or class of entities) [Crystal 1997,107]."@eng .

gold:DelativeCase a owl:Class ;
	rdfs:label "DelativeCase"@eng ;
	rdfs:subClassOf gold:CaseProperty ;
	rdfs:isDefinedBy "http://purl.org/linguistics/gold"^^<http://www.w3.org/2001/XMLSchema#anyURI> ;
	rdfs:comment "DelativeCase expresses motion downward from the referent of the noun it marks [Pei and Gaynor 1954, 53]."@eng .

gold:Demonstrative a owl:Class ;
	rdfs:label "Demonstrative"@eng ;
	rdfs:subClassOf gold:Pronominal ;
	rdfs:isDefinedBy "http://purl.org/linguistics/gold"^^<http://www.w3.org/2001/XMLSchema#anyURI> ;
	rdfs:comment "A demonstrative is a determiner that is used deictically to indicate a referent's spatial, temporal, or discourse location. A demonstrative functions as a modifier of a noun, or a pronoun [Crystal 1997,312]."@eng .

gold:Dental a owl:Class ;
	rdfs:label "Dental"@eng ;
	rdfs:subClassOf gold:AnteriorProperty ;
	rdfs:isDefinedBy "http://purl.org/linguistics/gold"^^<http://www.w3.org/2001/XMLSchema#anyURI> ;
	rdfs:comment "Characterizing sounds produced with the area behind the teeth but in front of the center of the alveolar ridge as the passive articulator [Ladefoged 1997, 597]."@eng .

gold:DeonticModality a owl:Class ;
	rdfs:label "DeonticModality"@eng ;
	rdfs:subClassOf gold:ModalityProperty ;
	rdfs:isDefinedBy "http://purl.org/linguistics/gold"^^<http://www.w3.org/2001/XMLSchema#anyURI> ;
	rdfs:comment "DeonticModality indicates that an agent has permission or is under an obligation to perform some action."@eng .

gold:DeponentMiddleVoice a owl:Class ;
	rdfs:label "DeponentMiddleVoice"@eng ;
	rdfs:subClassOf gold:VoiceProperty ;
	rdfs:isDefinedBy "http://purl.org/linguistics/gold"^^<http://www.w3.org/2001/XMLSchema#anyURI> ;
	rdfs:comment "Action denotes physical/mental disposition of subject. [Siewierska 1988,257]"@eng .

gold:DescribedVariety a owl:Class ;
	rdfs:label "DescribedVariety"@eng ;
	rdfs:subClassOf gold:HumanLanguageVariety ;
	rdfs:isDefinedBy "http://purl.org/linguistics/gold"^^<http://www.w3.org/2001/XMLSchema#anyURI> ;
	rdfs:comment "DescribedVariety is the class of  distinct human languages or language varieties as recognized by a linguist or a particular linguistic community, but not necessarily recognized by the ISO 639-3 standard. This category allows a language to be described even though it is not (yet) included in ISO 639-3."@eng .

gold:Diacritic a owl:Class ;
	rdfs:label "Diacritic"@eng ;
	rdfs:subClassOf gold:OrthographicPart ;
	rdfs:isDefinedBy "http://purl.org/linguistics/gold"^^<http://www.w3.org/2001/XMLSchema#anyURI> ;
	rdfs:comment "A Diacritic is a small mark added to a glyph (usually above or below) used to indicate stress, tone, or some kind of change in the quality of the segment represented by the glyph. Diacritics are used extensively in some writing systems, such as in French, Hebrew, or Arabic, and in transcription systems such as the International Phonetic Alphabet."@eng .

gold:Dialect a owl:Class ;
	rdfs:label "Dialect"@eng ;
	rdfs:subClassOf gold:GeneticTaxon ;
	rdfs:isDefinedBy "http://purl.org/linguistics/gold"^^<http://www.w3.org/2001/XMLSchema#anyURI> ;
	rdfs:comment """\"A Dialect is a GeneticTaxon, such that: (a) there is at least one other dialect to which the particular instance of dialect is compared, (b) the two dialects are mutually intelligible, and (c) there is a language such that the two dialects are
dialects of some language."""@eng .

gold:Digraph a owl:Class ;
	rdfs:label "Digraph"@eng ;
	rdfs:subClassOf gold:OrthographicPart ;
	rdfs:isDefinedBy "http://purl.org/linguistics/gold"^^<http://www.w3.org/2001/XMLSchema#anyURI> ;
	rdfs:comment "A Digraph is a sequence of glyphs used in some writing systems to represent a single phoneme. For instance, 'ng' is used to represent the velar nasal in several Germanic languages."@eng .

gold:DiminuativeSize a owl:Class ;
	rdfs:label "DiminuativeSize"@eng ;
	rdfs:subClassOf gold:SizeProperty ;
	rdfs:isDefinedBy "http://purl.org/linguistics/gold"^^<http://www.w3.org/2001/XMLSchema#anyURI> ;
	rdfs:comment "A special form of a noun that signals that the object being referred to is small relative to the usual size of such an object.  In some cases it may be used as a term of endearment [Crystal 1980, 116]."@eng .

gold:DirectEvidentiality a owl:Class ;
	rdfs:label "DirectEvidentiality"@eng ;
	rdfs:subClassOf gold:EvidentialityProperty ;
	rdfs:isDefinedBy "http://purl.org/linguistics/gold"^^<http://www.w3.org/2001/XMLSchema#anyURI> ;
	rdfs:comment "DirectEvidential, also called sensory, encodes the fact that the speaker came to believe the content of the expression by having direct sensory experience of some situation; this does not include hearing about it from someone else [Palmer 2001, 35-36]."@eng .

gold:DirectVoice a owl:Class ;
	rdfs:label "DirectVoice"@eng ;
	rdfs:subClassOf gold:VoiceProperty ;
	rdfs:isDefinedBy "http://purl.org/linguistics/gold"^^<http://www.w3.org/2001/XMLSchema#anyURI> .

gold:DiscourseUnit a owl:Class ;
	rdfs:label "DiscourseUnit"@eng ;
	rdfs:subClassOf gold:LinguisticUnit ;
	rdfs:isDefinedBy "http://purl.org/linguistics/gold"^^<http://www.w3.org/2001/XMLSchema#anyURI> ;
	rdfs:comment "The most general unit at the level of discourse. [This domain needs work.]"@eng .

gold:Disjunction a owl:Class ;
	rdfs:label "Disjunction"@eng ;
	rdfs:subClassOf gold:CoordinatingConnective ;
	rdfs:isDefinedBy "http://purl.org/linguistics/gold"^^<http://www.w3.org/2001/XMLSchema#anyURI> ;
	rdfs:comment "no documentation yet"@eng .

gold:DistributiveAspect a owl:Class ;
	rdfs:label "DistributiveAspect"@eng ;
	rdfs:subClassOf gold:AspectProperty ;
	rdfs:isDefinedBy "http://purl.org/linguistics/gold"^^<http://www.w3.org/2001/XMLSchema#anyURI> ;
	rdfs:comment "[Pei and Gaynor 1954, 59; Comrie 1985, 344]"@eng , "DistributiveAspect"@eng .

gold:DistributiveNumeral a owl:Class ;
	rdfs:label "DistributiveNumeral"@eng ;
	rdfs:subClassOf gold:Numeral ;
	rdfs:isDefinedBy "http://purl.org/linguistics/gold"^^<http://www.w3.org/2001/XMLSchema#anyURI> ;
	rdfs:comment "A distributive numeral is a numeral which expresses a group of the number specified."@eng .

gold:DitransitiveVerb a owl:Class ;
	rdfs:label "DitransitiveVerb"@eng ;
	rdfs:subClassOf gold:TertiaryPredicator ;
	rdfs:isDefinedBy "http://purl.org/linguistics/gold"^^<http://www.w3.org/2001/XMLSchema#anyURI> ;
	rdfs:comment "A ditransitive verb is a verb that takes two objects [Crystal 1997,397]."@eng .

gold:DualNumber a owl:Class ;
	rdfs:label "DualNumber"@eng ;
	rdfs:subClassOf gold:NumberProperty ;
	rdfs:isDefinedBy "http://purl.org/linguistics/gold"^^<http://www.w3.org/2001/XMLSchema#anyURI> ;
	rdfs:comment "\"http://purl.org/linguistics/gold-bibliography;Corbett2000_2595\"^^anyURI"@eng .

gold:DubitiveMood a owl:Class ;
	rdfs:label "DubitiveMood"@eng ;
	rdfs:subClassOf gold:MoodProperty ;
	rdfs:isDefinedBy "http://purl.org/linguistics/gold"^^<http://www.w3.org/2001/XMLSchema#anyURI> ;
	rdfs:comment "DubitiveMood indicates a speaker's doubt or uncertainty about a proposition [Palmer 2001]."@eng .

gold:DurativeAspect a owl:Class ;
	rdfs:label "DurativeAspect"@eng ;
	rdfs:subClassOf gold:AspectProperty ;
	rdfs:isDefinedBy "http://purl.org/linguistics/gold"^^<http://www.w3.org/2001/XMLSchema#anyURI> ;
	rdfs:comment "Events which involve some duration [Bhat 1999, 58]."@eng .

gold:ElativeCase a owl:Class ;
	rdfs:label "ElativeCase"@eng ;
	rdfs:subClassOf gold:CaseProperty ;
	rdfs:isDefinedBy "http://purl.org/linguistics/gold"^^<http://www.w3.org/2001/XMLSchema#anyURI> ;
	rdfs:comment "ElativeCase expresses that  the referent of the noun it marks is the location out of which another referent is moving. It has the meaning 'out of' [Lyons 1968, 299; Pei and Gaynor 1954, 64; Crystal 1985, 106]."@eng .

gold:Enclitic a owl:Class ;
	rdfs:label "Enclitic"@eng ;
	rdfs:subClassOf gold:Clitic ;
	rdfs:isDefinedBy "http://purl.org/linguistics/gold"^^<http://www.w3.org/2001/XMLSchema#anyURI> ;
	rdfs:comment "An enclitic is a clitic that is phonologically joined at the end of a preceding lexical unit to form a single phonological unit [Crystal 1980,64; Pei and Gaynor 1954,65]."@eng .

gold:EndangermentTaxon a owl:Class ;
	rdfs:label "EndangermentTaxon"@eng ;
	rdfs:subClassOf gold:LinguisticTaxon ;
	rdfs:isDefinedBy "http://purl.org/linguistics/gold"^^<http://www.w3.org/2001/XMLSchema#anyURI> ;
	rdfs:comment "EndangermentTaxon is a class of taxons based on the robustness of its members. Endangerment is based on a number of criteria including the number of speakers, the average age of the native-speaker population, etc."@eng .

gold:EpistemicModality a owl:Class ;
	rdfs:label "EpistemicModality"@eng ;
	rdfs:subClassOf gold:ModalityProperty ;
	rdfs:isDefinedBy "http://purl.org/linguistics/gold"^^<http://www.w3.org/2001/XMLSchema#anyURI> ;
	rdfs:comment "EpistemicModality indicates that a state of affairs is known to be possible or certain (necessary)."@eng .

gold:EpistemicNecessityModality a owl:Class ;
	rdfs:label "EpistemicNecessityModality"@eng ;
	rdfs:subClassOf gold:ModalityProperty ;
	rdfs:isDefinedBy "http://purl.org/linguistics/gold"^^<http://www.w3.org/2001/XMLSchema#anyURI> ;
	rdfs:comment "EpistemicNecessityModality indicates that the expressed proposition is known to be true. Also known as CategoricalModality [Palmer 2001, 37, 68-69]."@eng .

gold:EpistemicPossibilityModality a owl:Class ;
	rdfs:label "EpistemicPossibilityModality"@eng ;
	rdfs:subClassOf gold:ModalityProperty ;
	rdfs:isDefinedBy "http://purl.org/linguistics/gold"^^<http://www.w3.org/2001/XMLSchema#anyURI> ;
	rdfs:comment "EpistemicPossibilityModality indicates that the designated state of affairs is not known not to be true."@eng .

gold:ErgativeCase a owl:Class ;
	rdfs:label "ErgativeCase"@eng ;
	rdfs:subClassOf gold:CaseProperty ;
	rdfs:isDefinedBy "http://purl.org/linguistics/gold"^^<http://www.w3.org/2001/XMLSchema#anyURI> ;
	rdfs:comment "ErgativeCase in ergative-absolutive languages generally identifies the subject of transitive verbs in the translation equivalents of nominative-accusative Languages such as English [Crystal 1980, 134; Hartmann and Stork 1972, 78; Pei and Gaynor 1954, 67; Andrews 1985, 138]."@eng .

gold:EssiveCase a owl:Class ;
	rdfs:label "EssiveCase"@eng ;
	rdfs:subClassOf gold:CaseProperty ;
	rdfs:isDefinedBy "http://purl.org/linguistics/gold"^^<http://www.w3.org/2001/XMLSchema#anyURI> ;
	rdfs:comment "EssiveCase expresses that  the referent of the noun it marks is the location at which another referent exists [Lyons 1968, 299,301; Crystal 1985, 112; Blake 2001]."@eng .

gold:ExistentialMarker a owl:Class ;
	rdfs:label "ExistentialMarker"@eng ;
	rdfs:subClassOf gold:Verbal ;
	rdfs:isDefinedBy "http://purl.org/linguistics/gold"^^<http://www.w3.org/2001/XMLSchema#anyURI> ;
	rdfs:comment "An existential marker is a syntactic category whose members are found in distinct clause types and which mark a referent's existence [Crystal 1997,142]."@eng .

gold:Expletive a owl:Class ;
	rdfs:label "Expletive"@eng ;
	rdfs:subClassOf gold:PartOfSpeechProperty ;
	rdfs:isDefinedBy "http://purl.org/linguistics/gold"^^<http://www.w3.org/2001/XMLSchema#anyURI> ;
	rdfs:comment "An expletive (also known as a dummy word) is a part of speech whose members have no meaning, but complete a sentence to make it grammatical [Crystal 1997,127;]."@eng .

gold:ExtinctVariety a owl:Class ;
	rdfs:label "ExtinctVariety"@eng ;
	rdfs:subClassOf gold:HumanLanguageVariety ;
	rdfs:isDefinedBy "http://purl.org/linguistics/gold"^^<http://www.w3.org/2001/XMLSchema#anyURI> ;
	rdfs:comment "ExtinctVariety is the class of human language varieties that no longer have native speakers, e.g., Frankish or Mozarabic."@eng .

gold:FeatureAgreementSystem a owl:Class ;
	rdfs:label "FeatureAgreementSystem"@eng ;
	rdfs:subClassOf gold:FeatureDistributionSystem ;
	rdfs:isDefinedBy "http://purl.org/linguistics/gold"^^<http://www.w3.org/2001/XMLSchema#anyURI> ;
	rdfs:comment "A type of FeatureDistributionSystem; in a given language, it is the system according to which feature values (of a particular feature) are determined for elements through agreement (i.e. where the form of the element is determined by the presence of another element)."@eng .

gold:FeatureConstraint a owl:Class ;
	rdfs:label "FeatureConstraint"@eng ;
	rdfs:subClassOf gold:LinguisticDataStructure ;
	rdfs:isDefinedBy "http://purl.org/linguistics/gold"^^<http://www.w3.org/2001/XMLSchema#anyURI> ;
	rdfs:comment "A FeatureConstraint is a LinguisticDataStructure which groups a part of speech value with a set of features. Within a FeatureSystem of some language, it indicates which Features may be associated with a particular linguistic unit based on the unit's part of speech."@eng .

gold:FeatureGovernmentSystem a owl:Class ;
	rdfs:label "FeatureGovernmentSystem"@eng ;
	rdfs:subClassOf gold:FeatureDistributionSystem ;
	rdfs:isDefinedBy "http://purl.org/linguistics/gold"^^<http://www.w3.org/2001/XMLSchema#anyURI> ;
	rdfs:comment "A type of FeatureDistributionSystem; in a given language, it is the system according to which feature values (of a particular feature) are determined for elements through government (i.e. where the form of the element is determined by the presence of another element)."@eng .

gold:FeatureStructure a owl:Class ;
	rdfs:label "FeatureStructure"@eng ;
	rdfs:subClassOf gold:LinguisticDataStructure ;
	rdfs:isDefinedBy "http://purl.org/linguistics/gold"^^<http://www.w3.org/2001/XMLSchema#anyURI> ;
	rdfs:comment "A FeatureStructure is a set of one or more FeatureSpecifications. A FeatureStructure is a kind of information structure, a container or data structure, used to group together qualities or features of some object. In a grammatical feature system, a FeatureStructure holds the grammatical information associated with some linguistic unit. In a typed feature system, a FeatureStructure has an associated type, usually a PartOfSpeech. [Shieber 1986; Maxwell, Simons, and Hayashi 2000]."@eng .

gold:FeatureSystem a owl:Class ;
	rdfs:label "FeatureSystem"@eng ;
	rdfs:subClassOf gold:LinguisticDataStructure ;
	rdfs:isDefinedBy "http://purl.org/linguistics/gold"^^<http://www.w3.org/2001/XMLSchema#anyURI> ;
	rdfs:comment "A 3-tuple: (1) a set of FeatureValues, (2) the particular FeatureAssignmentSystem according to which the values are assigned inherently to elements in the given language, and (3) the particular FeatureDistributionSystem according to which the values are determined contextually for elements in the given language. The class of grammatical opposition sets relevant for a specific domain (tense, aspect, number, etc.) in a given language."@eng .

gold:FeminineGender a owl:Class ;
	rdfs:label "FeminineGender"@eng ;
	rdfs:subClassOf gold:GenderProperty ;
	rdfs:isDefinedBy "http://purl.org/linguistics/gold"^^<http://www.w3.org/2001/XMLSchema#anyURI> ;
	rdfs:comment "A gender property established on the basis of agreement, to which nouns may be assigned if 1) they inherently denote females. Additionally, but not necessarily, nouns may be assigned this value if: 2) their formal properties (morphological or phonological) lead them to be assigned to the same agreement pattern as other nouns within the language that have female denotation. 3) they are arbitrarily assigned to the same agreement pattern as other nouns in the language that have female denotation [Corbett 1991].@en"@eng .

gold:FirstPerson a owl:Class ;
	rdfs:label "FirstPerson"@eng ;
	rdfs:subClassOf gold:PersonProperty ;
	rdfs:isDefinedBy "http://purl.org/linguistics/gold"^^<http://www.w3.org/2001/XMLSchema#anyURI> ;
	rdfs:comment "First is a  person property that refers minimally to the speaker. It may also refer to the speaker combined with either the addressee or the non-participant or both, allowing for the following subdivisions: a) first person b) first person inclusive c) first person exclusive [Cysouw 2003]."@eng .

gold:FirstPersonExclusive a owl:Class ;
	rdfs:label "FirstPersonExclusive"@eng ;
	rdfs:subClassOf gold:PersonProperty ;
	rdfs:isDefinedBy "http://purl.org/linguistics/gold"^^<http://www.w3.org/2001/XMLSchema#anyURI> .

gold:FirstPersonInclusive a owl:Class ;
	rdfs:label "FirstPersonInclusive"@eng ;
	rdfs:subClassOf gold:PersonProperty ;
	rdfs:isDefinedBy "http://purl.org/linguistics/gold"^^<http://www.w3.org/2001/XMLSchema#anyURI> .

gold:FocusAntipassiveVoice a owl:Class ;
	rdfs:label "FocusAntipassiveVoice"@eng ;
	rdfs:subClassOf gold:VoiceProperty ;
	rdfs:isDefinedBy "http://purl.org/linguistics/gold"^^<http://www.w3.org/2001/XMLSchema#anyURI> ;
	rdfs:comment """Blocks the P or logical object (basic absolutive) nominal from being assigned Focus salience.  Topic salience is available for assignment to various arguments, including the P, but Focus salience is always assigned to A, and is therefore inaccessible to P or any other nominal.
[Klaiman 1991, 236]"""@eng .

gold:FolkloreEvidentiality a owl:Class ;
	rdfs:label "FolkloreEvidentiality"@eng ;
	rdfs:subClassOf gold:EvidentialityProperty ;
	rdfs:isDefinedBy "http://purl.org/linguistics/gold"^^<http://www.w3.org/2001/XMLSchema#anyURI> ;
	rdfs:comment "FolkloreEvidentiality encodes the fact that the speaker came to believe the content of the expression through legend, folklore or some other established tradition [Palmer 2001, 40]."@eng .

gold:Foot a owl:Class ;
	rdfs:label "Foot"@eng ;
	rdfs:subClassOf gold:FormUnit ;
	rdfs:isDefinedBy "http://purl.org/linguistics/gold"^^<http://www.w3.org/2001/XMLSchema#anyURI> .

gold:FormalAssignmentSystem a owl:Class ;
	rdfs:label "FormalAssignmentSystem"@eng ;
	rdfs:subClassOf gold:FeatureAssignmentSystem ;
	rdfs:isDefinedBy "http://purl.org/linguistics/gold"^^<http://www.w3.org/2001/XMLSchema#anyURI> .

gold:FreeUnit a owl:Class ;
	rdfs:label "FreeUnit"@eng ;
	rdfs:subClassOf gold:MorphologicalUnit ;
	rdfs:isDefinedBy "http://purl.org/linguistics/gold"^^<http://www.w3.org/2001/XMLSchema#anyURI> ;
	rdfs:comment "FreeUnit is the class of  morphological units that can exist on their own without being a constituent of  another morphological unit. Note that free units can also be syntactic units, namely syntactic words, at the level of the syntactic construction."@eng .

gold:FrequentiveAspect a owl:Class ;
	rdfs:label "FrequentiveAspect"@eng ;
	rdfs:subClassOf gold:AspectProperty ;
	rdfs:isDefinedBy "http://purl.org/linguistics/gold"^^<http://www.w3.org/2001/XMLSchema#anyURI> ;
	rdfs:comment "Events which are frequently repeated, differs from habitual in that it can only be based upon the observation of several occurrences of the event concerned, whereas habitual can be based upon the observation of a single occurrence [Bhat 1999, 53]."@eng .

gold:Fricative a owl:Class ;
	rdfs:label "Fricative"@eng ;
	rdfs:subClassOf gold:StrictureProperty ;
	rdfs:isDefinedBy "http://purl.org/linguistics/gold"^^<http://www.w3.org/2001/XMLSchema#anyURI> ;
	rdfs:comment "[Need comment]"@eng .

gold:Front a owl:Class ;
	rdfs:label "Front"@eng ;
	rdfs:subClassOf gold:BacknessProperty ;
	rdfs:isDefinedBy "http://purl.org/linguistics/gold"^^<http://www.w3.org/2001/XMLSchema#anyURI> ;
	rdfs:comment "Characterizing sounds produced with the tongue  near the front of the mouth."@eng .

gold:FutureInFutureTense a owl:Class ;
	rdfs:label "FutureInFutureTense"@eng ;
	rdfs:subClassOf gold:TenseProperty ;
	rdfs:isDefinedBy "http://purl.org/linguistics/gold"^^<http://www.w3.org/2001/XMLSchema#anyURI> ;
	rdfs:comment "FutureInFutureTense locates the situation in question in the future, relative to a temporal reference point that itself is located in the future relative to the moment of utterance [Comrie 1985, 128]."@eng .

gold:FutureInPastTense a owl:Class ;
	rdfs:label "FutureInPastTense"@eng ;
	rdfs:subClassOf gold:TenseProperty ;
	rdfs:isDefinedBy "http://purl.org/linguistics/gold"^^<http://www.w3.org/2001/XMLSchema#anyURI> ;
	rdfs:comment "FutureInPastTense locates the situation in question in the future, relative to a contextually determined temporal reference point that itself must be located in the past relative to the moment of utterance [Comrie 1985, 128]."@eng .

gold:FuturePerfectTense a owl:Class ;
	rdfs:label "FuturePerfectTense"@eng ;
	rdfs:subClassOf gold:TenseProperty ;
	rdfs:isDefinedBy "http://purl.org/linguistics/gold"^^<http://www.w3.org/2001/XMLSchema#anyURI> ;
	rdfs:comment "Describes an event that occurs after the time of speaking but before some reference point in time which also occurs after the time of speaking. This is also known as PastInFutureTense. [Comrie 1985, 126]"@eng .

gold:FutureTense a owl:Class ;
	rdfs:label "FutureTense"@eng ;
	rdfs:subClassOf gold:TenseProperty ;
	rdfs:isDefinedBy "http://purl.org/linguistics/gold"^^<http://www.w3.org/2001/XMLSchema#anyURI> ;
	rdfs:comment """A value of Tense Property assigned to the designated element in the clause when the meaning selected for the clause is that intended to locate the event spoken about as posterior to the deictic centre of the utterance. Most commonly, this tense meaning is referred to as 'future', because in absolute tense systems the deictic centre is the moment of speech. However, in relative tense systems, where the deictic centre can be moved to any point on the time line, it is more appropriate to refer to this temporal relation as 'posterior'.

The posterior temporal relation may obtain either in 'simple' or 'perfect' contexts.  Modelling of this distinction originates from [Reichenbach  1947], who suggested using a third point in time, 'reference point', to capture all possible tense distinctions. In all 'simple' temporal relations, the reference point coincides with the location of the event spoken about.  'Perfect' tense meanings are created when the reference point is separated and moved away from the event time, thus altering the viewing of the temporal location of the event even though the event's actual location with respect to the deictic centre remains the same.

Posterior temporal relationships obtaining in a 'perfect' context occur when the reference point is moved away from the event time. There are various logical possibilities for locating the reference point with respect to the other two points, though none of them seem to be typically grammaticalised as separate tenses.

Typically, for a tense value to be labelled as Future Tense, the tense meaning has to minimally express the posterior temporal relationship, although it may additionally express other temporal, aspectual, or modal meanings."""@eng .

gold:GeneralNumber a owl:Class ;
	rdfs:label "GeneralNumber"@eng ;
	rdfs:subClassOf gold:NumberProperty ;
	rdfs:isDefinedBy "http://purl.org/linguistics/gold"^^<http://www.w3.org/2001/XMLSchema#anyURI> .

gold:GenitiveCase a owl:Class ;
	rdfs:label "GenitiveCase"@eng ;
	rdfs:subClassOf gold:CaseProperty ;
	rdfs:isDefinedBy "http://purl.org/linguistics/gold"^^<http://www.w3.org/2001/XMLSchema#anyURI> ;
	rdfs:comment "GenitiveCase is used to mark the noun whose referent is the possessor of the referent of another noun [Crystal 1980, 161; Hartmann and Stork 1972, 9495,180; Pei and Gaynor 1954, 82,172; Anderson 1985, 185; Fleming 1988, 10]."@eng .

gold:GeographicTaxon a owl:Class ;
	rdfs:label "GeographicTaxon"@eng ;
	rdfs:subClassOf gold:LinguisticTaxon ;
	rdfs:isDefinedBy "http://purl.org/linguistics/gold"^^<http://www.w3.org/2001/XMLSchema#anyURI> ;
	rdfs:comment "GeographicTaxon is the class of linguistic taxons whose instances are groupings based on where, in general, the language varieties are used, e.g., AustralianLanguage."@eng .

gold:Gerund a owl:Class ;
	rdfs:label "Gerund"@eng ;
	rdfs:subClassOf gold:Noun ;
	rdfs:isDefinedBy "http://purl.org/linguistics/gold"^^<http://www.w3.org/2001/XMLSchema#anyURI> ;
	rdfs:comment "A part of speech derived from a verb and used as a noun, usually restricted to non-finite forms of the verb [Crystal 1997, 279]."@eng .

gold:GlottalMovementProperty a owl:Class ;
	rdfs:label "GlottalMovementProperty"@eng ;
	rdfs:subClassOf gold:LaryngealProperty ;
	rdfs:isDefinedBy "http://purl.org/linguistics/gold"^^<http://www.w3.org/2001/XMLSchema#anyURI> ;
	rdfs:comment "[Need a definition.]"@eng .

gold:Grapheme a owl:Class ;
	rdfs:label "Grapheme"@eng ;
	rdfs:subClassOf gold:FormUnit ;
	rdfs:isDefinedBy "http://purl.org/linguistics/gold"^^<http://www.w3.org/2001/XMLSchema#anyURI> ;
	rdfs:comment "A Grapheme is the smallest meaningful contrastive unit in a writing system. A grapheme is an abstraction over a set of like glyphs, the actual images on the   page. That is, a particular grapheme is realized by particular glyphs. More than one glyph can realize the same grapheme. For instance, the letter A  and its cursive equivalent are each realizations of the grapheme Latin Captial Letter A."@eng .

gold:GreaterPaucalNumber a owl:Class ;
	rdfs:label "GreaterPaucalNumber"@eng ;
	rdfs:subClassOf gold:NumberProperty ;
	rdfs:isDefinedBy "http://purl.org/linguistics/gold"^^<http://www.w3.org/2001/XMLSchema#anyURI> ;
	rdfs:comment "GreaterPaucal is a number property that quantifies the denotation of the nominal element so that it specifies that there are a small number of distinct entities, greater than paucalNumber but less than pluralNumber (so semantically similar to 'several' in English). Ln An example of greaterPaucalNumber is found in Sursurunga (sgz): Ln Gamhat til main gam han suri tártár Ln 2.GRPAU from here 2.PL go PURPOSE chop Ln on á kakau káián Himaul viles, honin Ln it TOPIC cacao its Himaul village today Ln dilhat má lu tangkabin sirai má ... Ln 3.GRPAU EMPHATIC HABITUAL begin selling now Ln \"You all from here (i.e. from this village) went to slash (for burning then planting) Himaul village's cacao, which already they (i.e. people from Himaul) have begun to sell ...\" Hutchisson uses the term 'quadral' for Greater Paucal; see the terminology notes for a comment on this [Corbett 2000: 28]."@eng .

gold:GreaterPlural a owl:Class ;
	rdfs:label "GreaterPlural"@eng ;
	rdfs:subClassOf gold:NumberProperty ;
	rdfs:isDefinedBy "http://purl.org/linguistics/gold"^^<http://www.w3.org/2001/XMLSchema#anyURI> ;
	rdfs:comment "GreaterPlural"@eng .

gold:GreaterPluralNumber a owl:Class ;
	rdfs:label "GreaterPluralNumber"@eng ;
	rdfs:subClassOf gold:NumberProperty ;
	rdfs:isDefinedBy "http://purl.org/linguistics/gold"^^<http://www.w3.org/2001/XMLSchema#anyURI> ;
	rdfs:comment "GreaterPlural is a number property that expresses (a) the fact that there is an excessive number of events or entities denoted by the noun or nominal element, or (b) the fact that the noun or nominal denotes all possible instances."@eng .

gold:Group a owl:Class ;
	rdfs:label "Group"@eng ;
	rdfs:subClassOf gold:SyntacticConstruction ;
	rdfs:isDefinedBy "http://purl.org/linguistics/gold"^^<http://www.w3.org/2001/XMLSchema#anyURI> ;
	rdfs:comment "Group is the class of syntactic constructions intermediate between the level of word and phrase."@eng .

gold:HabitualAspect a owl:Class ;
	rdfs:label "HabitualAspect"@eng ;
	rdfs:subClassOf gold:AspectProperty ;
	rdfs:isDefinedBy "http://purl.org/linguistics/gold"^^<http://www.w3.org/2001/XMLSchema#anyURI> ;
	rdfs:comment """A value of Aspect Property assigned to the designated element in the clause when the meaning selected for the clause is that which indicates that the situation spoken about is characteristic of an extended period of time --- so extended that the situation is viewed as characteristic of the whole period. The decision that a situation is characteristic of an extended period of time is not in itself linguistic, but once it has been made, an explicitly habitual form can be used to describe it. Note that the classification of a situation as characteristic of a period of time is not derived directly from the comparison of their length or frequency; hence, the situation may be objectively either long or short, and either frequent or infrequent, with respect to the period it characterises. This is because the way we choose to characterise can ivolve a component which is objectively small in relation to the whole.

Typically, for an aspect value to be labelled as Habitual, the aspectual meaning has to minimally express habituality, although it may additionally express other temporal, aspectual, or modal meanings, or actionality distinctions. Habituality can in principle be combined with any other semantic aspectual values appropriate to situations that can be protracted in time or iterated [Comrie 1976, 26-32]. Since habituality is concerned with the internal temporal structure of the (extended) event, it can be regarded as a sub-type of imperfectivity."""@eng .

gold:HearsayEvidentiality a owl:Class ;
	rdfs:label "HearsayEvidentiality"@eng ;
	rdfs:subClassOf gold:EvidentialityProperty ;
	rdfs:isDefinedBy "http://purl.org/linguistics/gold"^^<http://www.w3.org/2001/XMLSchema#anyURI> ;
	rdfs:comment "HearsayEvidentiality, also called third hand, encodes the fact that the speaker came to believe the content of the expression from a source generally considered less reliable than with a SecondHandEvidential [Palmer 2001, 40]."@eng .

gold:HesternalPastTense a owl:Class ;
	rdfs:label "HesternalPastTense"@eng ;
	rdfs:subClassOf gold:TenseProperty ;
	rdfs:isDefinedBy "http://purl.org/linguistics/gold"^^<http://www.w3.org/2001/XMLSchema#anyURI> ;
	rdfs:comment "HesternalPastTense locates the situation in question somewhere in the span beginning with the period defined culturally as 'yesterday' and extends back through some period that is considered nonremote [Comrie 1985,87-88; Dahl 1985,126]."@eng .

gold:High a owl:Class ;
	rdfs:label "High"@eng ;
	rdfs:subClassOf gold:HeightProperty ;
	rdfs:isDefinedBy "http://purl.org/linguistics/gold"^^<http://www.w3.org/2001/XMLSchema#anyURI> ;
	rdfs:comment "Characterizing sounds produced with the tongue  near the top of the mouth."@eng .

gold:HodiernalFutureTense a owl:Class ;
	rdfs:label "HodiernalFutureTense"@eng ;
	rdfs:subClassOf gold:TenseProperty ;
	rdfs:isDefinedBy "http://purl.org/linguistics/gold"^^<http://www.w3.org/2001/XMLSchema#anyURI> ;
	rdfs:comment "HodiernalFutureTense locates the situation in question after the moment of utterance within the span culturally defined as 'today' [Comrie 1985, 86; Bybee, Perkins and Pagliuca 1994, 247]."@eng .

gold:HodiernalPastTense a owl:Class ;
	rdfs:label "HodiernalPastTense"@eng ;
	rdfs:subClassOf gold:TenseProperty ;
	rdfs:isDefinedBy "http://purl.org/linguistics/gold"^^<http://www.w3.org/2001/XMLSchema#anyURI> ;
	rdfs:comment "HodiernalPastTense locates the situation in question before the moment of utterance within the span culturally defined as 'today' [Comrie 1985,87; Dahl 1985,125-126]. Contrasts with PreHodiernalPastTense."@eng .

gold:HortatoryForce a owl:Class ;
	rdfs:label "HortatoryForce"@eng ;
	rdfs:subClassOf gold:ForceProperty ;
	rdfs:isDefinedBy "http://purl.org/linguistics/gold"^^<http://www.w3.org/2001/XMLSchema#anyURI> ;
	rdfs:comment "HortatoryForce indicates that the hearer, possibly together with speaker, is admonished or to allow others to take action."@eng .

gold:HumanGender a owl:Class ;
	rdfs:label "HumanGender"@eng ;
	rdfs:subClassOf gold:GenderProperty ;
	rdfs:isDefinedBy "http://purl.org/linguistics/gold"^^<http://www.w3.org/2001/XMLSchema#anyURI> ;
	rdfs:comment "[Need comment]"@eng .

gold:IllativeCase a owl:Class ;
	rdfs:label "IllativeCase"@eng ;
	rdfs:subClassOf gold:CaseProperty ;
	rdfs:isDefinedBy "http://purl.org/linguistics/gold"^^<http://www.w3.org/2001/XMLSchema#anyURI> ;
	rdfs:comment "IllativeCase expresses that  the referent of the noun it marks is the location into which another referent is moving. It has the meaning 'into' [Lyons 1968, 299; Crystal 1985, 152]."@eng .

gold:ImmediateFutureTense a owl:Class ;
	rdfs:label "ImmediateFutureTense"@eng ;
	rdfs:subClassOf gold:TenseProperty ;
	rdfs:isDefinedBy "http://purl.org/linguistics/gold"^^<http://www.w3.org/2001/XMLSchema#anyURI> ;
	rdfs:comment "ImmediateFutureTense, also called 'close future', locates the situation in question shortly after the moment of utterance [Dahl 1985,121; Comrie 1985,94; Bybee, Perkins, and Pagliuca 1994, 244-245)."@eng .

gold:ImmediatePastTense a owl:Class ;
	rdfs:label "ImmediatePastTense"@eng ;
	rdfs:subClassOf gold:TenseProperty ;
	rdfs:isDefinedBy "http://purl.org/linguistics/gold"^^<http://www.w3.org/2001/XMLSchema#anyURI> ;
	rdfs:comment "ImmediatePastTense locates the situation in question at a time considered very recent in relation to the moment of utterance [Comrie 1985, 87]."@eng .

gold:ImperativeForce a owl:Class ;
	rdfs:label "ImperativeForce"@eng ;
	rdfs:subClassOf gold:ForceProperty ;
	rdfs:isDefinedBy "http://purl.org/linguistics/gold"^^<http://www.w3.org/2001/XMLSchema#anyURI> ;
	rdfs:comment "[Need comment]"@eng .

gold:ImperfectiveAspect a owl:Class ;
	rdfs:label "ImperfectiveAspect"@eng ;
	rdfs:subClassOf gold:AspectProperty ;
	rdfs:isDefinedBy "http://purl.org/linguistics/gold"^^<http://www.w3.org/2001/XMLSchema#anyURI> ;
	rdfs:comment """A value of Aspect Property assigned to the designated element in the clause when the meaning selected for the clause is that which indicates that the event spoken about is to be looked at from inside, from within its temporal boundaries; imperfective aspect is crucially concerned with the internal temporal structure of the event [Comrie 1976, 16ff].

Typically, for an aspect value to be labelled as Imperfective, the aspectual meaning has to minimally express the imperfective viewpoint, although it may additionally express other temporal, aspectual, or modal meanings, or actionality distinctions.

Imperfective aspectual meaning can be further subdivided into two types: habitual meaning and continuous meaning. These two aspectual meanings may or may not be grammaticalised as separate aspect values."""@eng .

gold:ImpersonalPassiveVoice a owl:Class ;
	rdfs:label "ImpersonalPassiveVoice"@eng ;
	rdfs:subClassOf gold:VoiceProperty ;
	rdfs:isDefinedBy "http://purl.org/linguistics/gold"^^<http://www.w3.org/2001/XMLSchema#anyURI> ;
	rdfs:comment "A Passive that alters the mapping of a nominal to the Subject relation in a basic intransitive structure [Klaiman 1991,23]"@eng .

gold:InablativeCase a owl:Class ;
	rdfs:label "InablativeCase"@eng ;
	rdfs:subClassOf gold:CaseProperty ;
	rdfs:isDefinedBy "http://purl.org/linguistics/gold"^^<http://www.w3.org/2001/XMLSchema#anyURI> ;
	rdfs:comment "InablativeCase expresses that  the referent of the noun it marks is the location from within which another referent is moving. It has the meaning 'from within'."@eng .

gold:InallativeCase a owl:Class ;
	rdfs:label "InallativeCase"@eng ;
	rdfs:subClassOf gold:CaseProperty ;
	rdfs:isDefinedBy "http://purl.org/linguistics/gold"^^<http://www.w3.org/2001/XMLSchema#anyURI> ;
	rdfs:comment "InallativeCase expresses that  something is moving toward the region that is inside the referent of the noun it marks. It has the meaning  'towards in(side)'."@eng .

gold:InanimateGender a owl:Class ;
	rdfs:label "InanimateGender"@eng ;
	rdfs:subClassOf gold:GenderProperty ;
	rdfs:isDefinedBy "http://purl.org/linguistics/gold"^^<http://www.w3.org/2001/XMLSchema#anyURI> ;
	rdfs:comment "A grammatical gender property such that membership in the inanimate grammatical class is largely based on meaning, in that non-living things, such as objects of manufacture and natural 'non-living' things are included in it.  For example, one of the two grammatical genders, or noun classes, of Nishnaabemwin, the other being animate  [Valentine 2001, 114]."@eng .

gold:InceptiveAspect a owl:Class ;
	rdfs:label "InceptiveAspect"@eng ;
	rdfs:subClassOf gold:AspectProperty ;
	rdfs:isDefinedBy "http://purl.org/linguistics/gold"^^<http://www.w3.org/2001/XMLSchema#anyURI> ;
	rdfs:comment "InceptiveAspect, also called the ingressive, encodes the beginning portion of some event [Bybee 1985, 147, 149; Payne 1997, 240; Bhat 1999,176]."@eng .

gold:IncorporatingAntipassiveVoice a owl:Class ;
	rdfs:label "IncorporatingAntipassiveVoice"@eng ;
	rdfs:subClassOf gold:VoiceProperty ;
	rdfs:isDefinedBy "http://purl.org/linguistics/gold"^^<http://www.w3.org/2001/XMLSchema#anyURI> ;
	rdfs:comment "Blocks the P or logical object (basic absolutive) nominal from being assigned Focus salience. This correlates with the P's morphosyntactic downgrading, whereby it becomes insusceptible to any informational salience assignment. [Klaiman 1991,236]"@eng .

gold:IndefiniteArticle a owl:Class ;
	rdfs:label "IndefiniteArticle"@eng ;
	rdfs:subClassOf gold:Article ;
	rdfs:isDefinedBy "http://purl.org/linguistics/gold"^^<http://www.w3.org/2001/XMLSchema#anyURI> ;
	rdfs:comment "An article is a part of speech whose members are used to refer to an entity (or class of entities) which is not capable of specific identification [Crystal 1997, 193]."@eng .

gold:IndefinitePronoun a owl:Class ;
	rdfs:label "IndefinitePronoun"@eng ;
	rdfs:subClassOf gold:Pronominal ;
	rdfs:isDefinedBy "http://purl.org/linguistics/gold"^^<http://www.w3.org/2001/XMLSchema#anyURI> ;
	rdfs:comment "An indefinite pronoun is a pronoun that belongs to a class whose members indicate  indefinite reference [Crystal 1997, 312]."@eng .

gold:IndicativeMood a owl:Class ;
	rdfs:label "IndicativeMood"@eng ;
	rdfs:subClassOf gold:MoodProperty ;
	rdfs:isDefinedBy "http://purl.org/linguistics/gold"^^<http://www.w3.org/2001/XMLSchema#anyURI> ;
	rdfs:comment "IndicativeMood indicates that the speaker believes the expression to be true."@eng .

gold:IndirectEvidentiality a owl:Class ;
	rdfs:label "IndirectEvidentiality"@eng ;
	rdfs:subClassOf gold:EvidentialityProperty ;
	rdfs:isDefinedBy "http://purl.org/linguistics/gold"^^<http://www.w3.org/2001/XMLSchema#anyURI> ;
	rdfs:comment "IndirectEvidentiality, also called reported, encodes the fact that the speaker came to believe the content of the expression from a source other than by experiencing the situation directly [Palmer 2001, 40]."@eng .

gold:InessiveCase a owl:Class ;
	rdfs:label "InessiveCase"@eng ;
	rdfs:subClassOf gold:CaseProperty ;
	rdfs:isDefinedBy "http://purl.org/linguistics/gold"^^<http://www.w3.org/2001/XMLSchema#anyURI> ;
	rdfs:comment "InessiveCase expresses that  the referent of the noun it marks is the location within which another referent exists. It has the meaning of 'within' or 'inside' [Lyons 1968, 299; Crystal 1985, 156]. X in Y."@eng .

gold:InferentialEvidentiality a owl:Class ;
	rdfs:label "InferentialEvidentiality"@eng ;
	rdfs:subClassOf gold:EvidentialityProperty ;
	rdfs:isDefinedBy "http://purl.org/linguistics/gold"^^<http://www.w3.org/2001/XMLSchema#anyURI> ;
	rdfs:comment "InferentialEvidentiality encodes the fact that the speaker came to believe the content of the expression through some kind of internal inference procedure, e.g., deduction, abduction, induction [Palmer 2001, 6-8]."@eng .

gold:Infix a owl:Class ;
	rdfs:label "Infix"@eng ;
	rdfs:subClassOf gold:Affix ;
	rdfs:isDefinedBy "http://purl.org/linguistics/gold"^^<http://www.w3.org/2001/XMLSchema#anyURI> .

gold:InflectionalUnit a owl:Class ;
	rdfs:label "InflectionalUnit"@eng ;
	rdfs:subClassOf gold:FunctionalUnit ;
	rdfs:isDefinedBy "http://purl.org/linguistics/gold"^^<http://www.w3.org/2001/XMLSchema#anyURI> ;
	rdfs:comment "InflectionalUnit is the class of functional units whose members designate such grammatical categories as tense, aspect, mood etc. The various forms of an InflectionalUnit plus the stem forms a grammatical paradigm and express a grammatical contrast that is obligatory for its stem's part of speech in some given grammatical context. An inflectional unit does not alter the part of speech feature of the root or stem it attaches to. It is typically located farther from its Root than a derivational unit and  produces a predictable, nonidiosyncratic change of meaning [Crystal 1980,184; Hartmann and Stork 1972,112; Bybee 1985,2, 99]."@eng .

gold:InformationalForce a owl:Class ;
	rdfs:label "InformationalForce"@eng ;
	rdfs:subClassOf gold:ForceProperty ;
	rdfs:isDefinedBy "http://purl.org/linguistics/gold"^^<http://www.w3.org/2001/XMLSchema#anyURI> ;
	rdfs:comment "InformationalForce indicates that the hearer is to relate to the informational content of what is expressed. Subsumes Declarative, Speculative and Interrogative."@eng .

gold:InstrumentalCase a owl:Class ;
	rdfs:label "InstrumentalCase"@eng ;
	rdfs:subClassOf gold:CaseProperty ;
	rdfs:isDefinedBy "http://purl.org/linguistics/gold"^^<http://www.w3.org/2001/XMLSchema#anyURI> ;
	rdfs:comment "InstrumentalCase indicates that the referent of the noun it marks is the means of the accomplishment of the action expressed by the clause [Crystal 1980, 187; Hartmann and Stork 1972, 114]."@eng .

gold:InterablativeCase a owl:Class ;
	rdfs:label "InterablativeCase"@eng ;
	rdfs:subClassOf gold:CaseProperty ;
	rdfs:isDefinedBy "http://purl.org/linguistics/gold"^^<http://www.w3.org/2001/XMLSchema#anyURI> ;
	rdfs:comment "InterablativeCase expresses that  the referent of the noun it marks is the location from between which another referent is moving. It has the meaning 'from in between'."@eng .

gold:InterallativeCase a owl:Class ;
	rdfs:label "InterallativeCase"@eng ;
	rdfs:subClassOf gold:CaseProperty ;
	rdfs:isDefinedBy "http://purl.org/linguistics/gold"^^<http://www.w3.org/2001/XMLSchema#anyURI> ;
	rdfs:comment "InterallativeCase expresses that  something is moving toward the region that is in the middle of the referent of the noun it marks. It has the meaning  'towards the middle of'."@eng .

gold:InteressiveCase a owl:Class ;
	rdfs:label "InteressiveCase"@eng ;
	rdfs:subClassOf gold:CaseProperty ;
	rdfs:isDefinedBy "http://purl.org/linguistics/gold"^^<http://www.w3.org/2001/XMLSchema#anyURI> ;
	rdfs:comment "InteressiveCase expresses that  the referent of the noun it marks is the location between which another referent exists. It has the meaning of 'between'."@eng .

gold:Interjection a owl:Class ;
	rdfs:label "Interjection"@eng ;
	rdfs:subClassOf gold:PartOfSpeechProperty ;
	rdfs:isDefinedBy "http://purl.org/linguistics/gold"^^<http://www.w3.org/2001/XMLSchema#anyURI> ;
	rdfs:comment "An interjection is a part of speech, typically brief in form, such as one syllable or word, whose members are used most often as exclamations or parts of an exclamation. An interjection, typically expressing an emotional reaction, often with respect to an accompanying sentence, is not syntactically related to other accompanying expressions, and may include a combination of sounds not otherwise found in the language [Crystal 1997,200]."@eng .

gold:InterlativeCase a owl:Class ;
	rdfs:label "InterlativeCase"@eng ;
	rdfs:subClassOf gold:CaseProperty ;
	rdfs:isDefinedBy "http://purl.org/linguistics/gold"^^<http://www.w3.org/2001/XMLSchema#anyURI> ;
	rdfs:comment "InterlativeCase expresses that  the referent of the noun it marks is the location between which another referent is moving. It has the meaning 'to the middle of'."@eng .

gold:InterlinearGlossedText a owl:Class ;
	rdfs:label "InterlinearGlossedText"@eng ;
	rdfs:subClassOf gold:LinguisticDataStructure ;
	rdfs:isDefinedBy "http://purl.org/linguistics/gold"^^<http://www.w3.org/2001/XMLSchema#anyURI> ;
	rdfs:comment "Interlinear glossed text (IGT) is a linguistic data structure meant to display morphosyntactic structure: morphemes, morpheme boundaries, morpheme types (clitics, prefixes, reduplicated forms), morphosyntactic features/values and part of speech information. At a minimum, an instance of IGT includes a single line of source language followed by a translation line.  Often, a second gloss line is included to show detailed morphosyntactic structure using both words and phrases from the target language and various labels, or 'grams', that indicate morphosyntactic features/values, etc. It is possible to include separate lines for the orthographic form, phonetic form, and phonological form. Standards for IGT include the Leipzig Glossing Rules."@eng .

gold:InterminativeCase a owl:Class ;
	rdfs:label "InterminativeCase"@eng ;
	rdfs:subClassOf gold:CaseProperty ;
	rdfs:isDefinedBy "http://purl.org/linguistics/gold"^^<http://www.w3.org/2001/XMLSchema#anyURI> ;
	rdfs:comment "'into in(side of)'."@eng .

gold:InterrogativeForce a owl:Class ;
	rdfs:label "InterrogativeForce"@eng ;
	rdfs:subClassOf gold:ForceProperty ;
	rdfs:isDefinedBy "http://purl.org/linguistics/gold"^^<http://www.w3.org/2001/XMLSchema#anyURI> ;
	rdfs:comment "[Need comment]"@eng .

gold:InterrogativeOperator a owl:Class ;
	rdfs:label "InterrogativeOperator"@eng ;
	rdfs:subClassOf gold:PartOfSpeechProperty ;
	rdfs:isDefinedBy "http://purl.org/linguistics/gold"^^<http://www.w3.org/2001/XMLSchema#anyURI> ;
	rdfs:comment "Also referred to as a 'question particle', an interrogative operator is a category whose members signal a yes/no question [Payne 1997, 296]."@eng .

gold:InterrogativeProform a owl:Class ;
	rdfs:label "InterrogativeProform"@eng ;
	rdfs:subClassOf gold:ProForm ;
	rdfs:isDefinedBy "http://purl.org/linguistics/gold"^^<http://www.w3.org/2001/XMLSchema#anyURI> ;
	rdfs:comment "An InterrogativeProform is a Proform that is used in questions to stand for the item questioned."@eng .

gold:InterterminativeCase a owl:Class ;
	rdfs:label "InterterminativeCase"@eng ;
	rdfs:subClassOf gold:CaseProperty ;
	rdfs:isDefinedBy "http://purl.org/linguistics/gold"^^<http://www.w3.org/2001/XMLSchema#anyURI> ;
	rdfs:comment "InterterminativeCase expresses the notion of something moving into the middle of the referent of the noun it marks, but not through it. It has the meaning 'into the middle of'."@eng .

gold:IntertranslativeCase a owl:Class ;
	rdfs:label "IntertranslativeCase"@eng ;
	rdfs:subClassOf gold:CaseProperty ;
	rdfs:isDefinedBy "http://purl.org/linguistics/gold"^^<http://www.w3.org/2001/XMLSchema#anyURI> ;
	rdfs:comment "IntertranslativeCase expresses the notion of something moving along a trajectory between the referent of the noun it marks. It has the meaning 'along the in between'."@eng .

gold:IntransitiveVerb a owl:Class ;
	rdfs:label "IntransitiveVerb"@eng ;
	rdfs:subClassOf gold:UnaryPredicator ;
	rdfs:isDefinedBy "http://purl.org/linguistics/gold"^^<http://www.w3.org/2001/XMLSchema#anyURI> ;
	rdfs:comment "An intransitive verb is a verb that cannot take a direct object, and describes a property, state, or situation involving only one participant [Crystal 1997,397; Payne 1997,171]."@eng .

gold:Intransitivizer a owl:Class ;
	rdfs:label "Intransitivizer"@eng ;
	rdfs:subClassOf gold:CategoryChanger ;
	rdfs:isDefinedBy "http://purl.org/linguistics/gold"^^<http://www.w3.org/2001/XMLSchema#anyURI> ;
	rdfs:comment "A derivational unit that derives intransitive verbs from adjectives or other categories."@eng .

gold:IntranslativeCase a owl:Class ;
	rdfs:label "IntranslativeCase"@eng ;
	rdfs:subClassOf gold:CaseProperty ;
	rdfs:isDefinedBy "http://purl.org/linguistics/gold"^^<http://www.w3.org/2001/XMLSchema#anyURI> ;
	rdfs:comment "IntranslativeCase expresses the notion of something moving through the referent of the noun it marks. It has the meaning 'along through'."@eng .

gold:InverseVoice a owl:Class ;
	rdfs:label "InverseVoice"@eng ;
	rdfs:subClassOf gold:VoiceProperty ;
	rdfs:isDefinedBy "http://purl.org/linguistics/gold"^^<http://www.w3.org/2001/XMLSchema#anyURI> .

gold:IrrealisMood a owl:Class ;
	rdfs:label "IrrealisMood"@eng ;
	rdfs:subClassOf gold:MoodProperty ;
	rdfs:isDefinedBy "http://purl.org/linguistics/gold"^^<http://www.w3.org/2001/XMLSchema#anyURI> ;
	rdfs:comment "A mood that indicates possible or conditional truth."@eng , "IrrealisMood"@eng .

gold:Isolate a owl:Class ;
	rdfs:label "Isolate"@eng ;
	rdfs:subClassOf gold:GeneticTaxon ;
	rdfs:isDefinedBy "http://purl.org/linguistics/gold"^^<http://www.w3.org/2001/XMLSchema#anyURI> ;
	rdfs:comment "Isolate is the class of human language varieties such that there are no other varieties that are genetically related."@eng .

gold:IterativeAspect a owl:Class ;
	rdfs:label "IterativeAspect"@eng ;
	rdfs:subClassOf gold:AspectProperty ;
	rdfs:isDefinedBy "http://purl.org/linguistics/gold"^^<http://www.w3.org/2001/XMLSchema#anyURI> ;
	rdfs:comment "IterativeAspect, also called repetitives, encodes a number of events of the same type that are repeated on a particular occasion. The time interval which is relevant to the iterative is relatively shorter than in the case of the habitual [Bybee 1985, 150; Bybee, Perkins and Pagliuca 1994, 127]. Portrays events repeated on the same occasion (like the iterative knocking on the door) [Bhat 1999, 53]"@eng .

gold:JussiveForce a owl:Class ;
	rdfs:label "JussiveForce"@eng ;
	rdfs:subClassOf gold:ForceProperty ;
	rdfs:isDefinedBy "http://purl.org/linguistics/gold"^^<http://www.w3.org/2001/XMLSchema#anyURI> ;
	rdfs:comment "JussiveForce indicates a request for permission to take action."@eng .

gold:Laminal a owl:Class ;
	rdfs:label "Laminal"@eng ;
	rdfs:subClassOf gold:ApicalityProperty ;
	rdfs:isDefinedBy "http://purl.org/linguistics/gold"^^<http://www.w3.org/2001/XMLSchema#anyURI> ;
	rdfs:comment "Characterizing sounds produced by the blade of the tongue  [Ladefoged 1997, 596]."@eng .

gold:Language a owl:Class ;
	rdfs:label "Language"@eng ;
	rdfs:subClassOf gold:GeneticTaxon ;
	rdfs:isDefinedBy "http://purl.org/linguistics/gold"^^<http://www.w3.org/2001/XMLSchema#anyURI> ;
	rdfs:comment "The concept of a language is very difficult to define axiomatically. Here, we say that a language is a subclass of GeneticTaxon above the level of dialect. Language, in this sense, is often defined according to mutual intelligibility among its speakers, when the speakers of the language are located in the same general location, the sharing of a common writing system, or the sharing of a common literature."@eng .

gold:LanguageFamily a owl:Class ;
	rdfs:label "LanguageFamily"@eng ;
	rdfs:subClassOf gold:GeneticTaxon ;
	rdfs:isDefinedBy "http://purl.org/linguistics/gold"^^<http://www.w3.org/2001/XMLSchema#anyURI> ;
	rdfs:comment "LanguageFamily is a relatively broad grouping of languages. In a given language family, all languages are genetically related."@eng .

gold:LanguageStock a owl:Class ;
	rdfs:label "LanguageStock"@eng ;
	rdfs:subClassOf gold:GeneticTaxon ;
	rdfs:isDefinedBy "http://purl.org/linguistics/gold"^^<http://www.w3.org/2001/XMLSchema#anyURI> ;
	rdfs:comment "LanguageStock is a wide grouping of languages based on genetic affiliation and at a higher level than a LanguageFamily. LanguageStock is defined according to the existence of language families."@eng .

gold:LanguageSubfamily a owl:Class ;
	rdfs:label "LanguageSubfamily"@eng ;
	rdfs:subClassOf gold:GeneticTaxon ;
	rdfs:isDefinedBy "http://purl.org/linguistics/gold"^^<http://www.w3.org/2001/XMLSchema#anyURI> ;
	rdfs:comment "LanguageSubfamily is a grouping of languages defined more narrowly than a LanguageFamily. In a given Subfamily, all languages are genetically related and are instances of the same LanguageFamily. For there to be a subfamily, there must be a family."@eng .

gold:LateralEscape a owl:Class ;
	rdfs:label "LateralEscape"@eng ;
	rdfs:subClassOf gold:LateralProperty ;
	rdfs:isDefinedBy "http://purl.org/linguistics/gold"^^<http://www.w3.org/2001/XMLSchema#anyURI> ;
	rdfs:comment "Characterizing sounds produced with a release of air through the sides of the mouth. (Note, [Ladefoged 1997] refers to this as lateral.)"@eng .

gold:LativeCase a owl:Class ;
	rdfs:label "LativeCase"@eng ;
	rdfs:subClassOf gold:CaseProperty ;
	rdfs:isDefinedBy "http://purl.org/linguistics/gold"^^<http://www.w3.org/2001/XMLSchema#anyURI> ;
	rdfs:comment "LativeCase expresses 'motion up to the location of,' or 'as far as' the referent of the noun it marks [Pei and Gaynor 1954, 121]."@eng .

gold:LexicalItem a owl:Class ;
	rdfs:label "LexicalItem"@eng ;
	rdfs:subClassOf gold:LinguisticDataStructure ;
	rdfs:isDefinedBy "http://purl.org/linguistics/gold"^^<http://www.w3.org/2001/XMLSchema#anyURI> ;
	rdfs:comment "The information structure used to encode all the information associated with an entry in a dictionary."@eng .

gold:LexicalizedConcept a owl:Class ;
	rdfs:label "LexicalizedConcept"@eng ;
	rdfs:subClassOf gold:SemanticUnit ;
	rdfs:isDefinedBy "http://purl.org/linguistics/gold"^^<http://www.w3.org/2001/XMLSchema#anyURI> ;
	rdfs:comment "LexicalizedConcept is the class of semantic units that are expressed as grammatical atoms in a language."@eng .

gold:Lexicon a owl:Class ;
	rdfs:label "Lexicon"@eng ;
	rdfs:subClassOf gold:LinguisticDataStructure ;
	rdfs:isDefinedBy "http://purl.org/linguistics/gold"^^<http://www.w3.org/2001/XMLSchema#anyURI> ;
	rdfs:comment "A collection of LexicalItems."@eng .

gold:Ligature a owl:Class ;
	rdfs:label "Ligature"@eng ;
	rdfs:subClassOf gold:Glyph ;
	rdfs:isDefinedBy "http://purl.org/linguistics/gold"^^<http://www.w3.org/2001/XMLSchema#anyURI> ;
	rdfs:comment "A Ligature is a special type of glyph composed by two or more basic glyphs fused together as a single symbol."@eng .

gold:LinguisticSign a owl:Class ;
	rdfs:label "LinguisticSign"@eng ;
	rdfs:subClassOf gold:Abstract ;
	rdfs:isDefinedBy "http://purl.org/linguistics/gold"^^<http://www.w3.org/2001/XMLSchema#anyURI> ;
	rdfs:comment "A linguistic sign is an abstract structure whose instances participate in a linguistic system, or language. By definition, a linguistic sign must have a form component (whose elements are phonological units), a grammatical component (whose elements are grammatical units), and a meaning component (whose elements are semantic units). The formal structure of a linguistic sign is determined by the grammar of a language. The information value of a linguistic sign, its meaning, is not fixed, but determined by the conventions of the language. The relation of form to meaning is largely arbitrary within a semiotic system. Signs are classified primarily according to what kinds of formal relations they participate in, and, secondly, according to their complexity (whether they are atomic or composed of other signs). Signs range from morphological and syntactic constructions to whole discourse segments [de Saussure 1983; Hervey 1979; Pollard and Sag 1994]."@eng .

gold:LivingVariety a owl:Class ;
	rdfs:label "LivingVariety"@eng ;
	rdfs:subClassOf gold:HumanLanguageVariety ;
	rdfs:isDefinedBy "http://purl.org/linguistics/gold"^^<http://www.w3.org/2001/XMLSchema#anyURI> ;
	rdfs:comment "LivingVariety is the class of human language varieties that are currently in use and have native speakers."@eng .

gold:LocativeCase a owl:Class ;
	rdfs:label "LocativeCase"@eng ;
	rdfs:subClassOf gold:CaseProperty ;
	rdfs:isDefinedBy "http://purl.org/linguistics/gold"^^<http://www.w3.org/2001/XMLSchema#anyURI> ;
	rdfs:comment "Category of case that denotes that the referent of the noun it marks is a location."@eng .

gold:LocativePassiveVoice a owl:Class ;
	rdfs:label "LocativePassiveVoice"@eng ;
	rdfs:subClassOf gold:VoiceProperty ;
	rdfs:isDefinedBy "http://purl.org/linguistics/gold"^^<http://www.w3.org/2001/XMLSchema#anyURI> ;
	rdfs:comment """An oblique locative nominal assumes the subject relation.
[Klaiman 1991,17]"""@eng .

gold:Low a owl:Class ;
	rdfs:label "Low"@eng ;
	rdfs:subClassOf gold:HeightProperty ;
	rdfs:isDefinedBy "http://purl.org/linguistics/gold"^^<http://www.w3.org/2001/XMLSchema#anyURI> ;
	rdfs:comment "Characterizing sounds produced with the tongue  near the bottom of the mouth."@eng .

gold:MainClause a owl:Class ;
	rdfs:label "MainClause"@eng ;
	rdfs:subClassOf gold:Clause ;
	rdfs:isDefinedBy "http://purl.org/linguistics/gold"^^<http://www.w3.org/2001/XMLSchema#anyURI> ;
	rdfs:comment "MainClause is the class of clauses that can stand on their own as a  full, independent sentence.  If a sentence contains any embedded clauses, the main clause is understood as the matrix plus the embedded clauses. In the sentence 'John thinks that Mary is sick', 'John thinks that Mary is sick' is the main clause [Crystal 2001, 231]."@eng .

gold:MalefactiveCase a owl:Class ;
	rdfs:label "MalefactiveCase"@eng ;
	rdfs:subClassOf gold:CaseProperty ;
	rdfs:isDefinedBy "http://purl.org/linguistics/gold"^^<http://www.w3.org/2001/XMLSchema#anyURI> ;
	rdfs:comment "Opposite of BenefactiveCase; used when the marked noun is negatively affected in the clause."@eng .

gold:MasculineGender a owl:Class ;
	rdfs:label "MasculineGender"@eng ;
	rdfs:subClassOf gold:GenderProperty ;
	rdfs:isDefinedBy "http://purl.org/linguistics/gold"^^<http://www.w3.org/2001/XMLSchema#anyURI> .

gold:MentalAbilitiveModality a owl:Class ;
	rdfs:label "MentalAbilitiveModality"@eng ;
	rdfs:subClassOf gold:ModalityProperty ;
	rdfs:isDefinedBy "http://purl.org/linguistics/gold"^^<http://www.w3.org/2001/XMLSchema#anyURI> ;
	rdfs:comment "MentalAbilitiveModality indicates that an agent has the  capacity to perform some mental action [Bybee, Perkins, and Pagliuca 1994, 192; Palmer 2001, 77]."@eng .

gold:Mid a owl:Class ;
	rdfs:label "Mid"@eng ;
	rdfs:subClassOf gold:HeightProperty ;
	rdfs:isDefinedBy "http://purl.org/linguistics/gold"^^<http://www.w3.org/2001/XMLSchema#anyURI> ;
	rdfs:comment "[Need comment]"@eng .

gold:MinusATR a owl:Class ;
	rdfs:label "MinusATR"@eng ;
	rdfs:subClassOf gold:RadicalProperty ;
	rdfs:isDefinedBy "http://purl.org/linguistics/gold"^^<http://www.w3.org/2001/XMLSchema#anyURI> ;
	rdfs:comment "Characterizing sounds made with the tongue root in the neutral position."@eng .

gold:MinusClick a owl:Class ;
	rdfs:label "MinusClick"@eng ;
	rdfs:subClassOf gold:VelaricProperty ;
	rdfs:isDefinedBy "http://purl.org/linguistics/gold"^^<http://www.w3.org/2001/XMLSchema#anyURI> ;
	rdfs:comment "[Need comment]"@eng .

gold:MinusFortis a owl:Class ;
	rdfs:label "MinusFortis"@eng ;
	rdfs:subClassOf gold:PulmonicProperty ;
	rdfs:isDefinedBy "http://purl.org/linguistics/gold"^^<http://www.w3.org/2001/XMLSchema#anyURI> ;
	rdfs:comment "[Need comment]"@eng .

gold:MinusNasal a owl:Class ;
	rdfs:label "MinusNasal"@eng ;
	rdfs:subClassOf gold:NasalityProperty ;
	rdfs:isDefinedBy "http://purl.org/linguistics/gold"^^<http://www.w3.org/2001/XMLSchema#anyURI> ;
	rdfs:comment "Characterizing sounds produced with no air escaping through the nose."@eng .

gold:Modal a owl:Class ;
	rdfs:label "Modal"@eng ;
	rdfs:subClassOf gold:PartOfSpeechProperty ;
	rdfs:isDefinedBy "http://purl.org/linguistics/gold"^^<http://www.w3.org/2001/XMLSchema#anyURI> ;
	rdfs:comment "no documentation yet"@eng .

gold:ModalVoice a owl:Class ;
	rdfs:label "ModalVoice"@eng ;
	rdfs:subClassOf gold:GlottalStrictureProperty ;
	rdfs:isDefinedBy "http://purl.org/linguistics/gold"^^<http://www.w3.org/2001/XMLSchema#anyURI> ;
	rdfs:comment "[Need comment]"@eng .

gold:Mora a owl:Class ;
	rdfs:label "Mora"@eng ;
	rdfs:subClassOf gold:FormUnit ;
	rdfs:isDefinedBy "http://purl.org/linguistics/gold"^^<http://www.w3.org/2001/XMLSchema#anyURI> .

gold:MultalNumber a owl:Class ;
	rdfs:label "MultalNumber"@eng ;
	rdfs:subClassOf gold:NumberProperty ;
	rdfs:isDefinedBy "http://purl.org/linguistics/gold"^^<http://www.w3.org/2001/XMLSchema#anyURI> ;
	rdfs:comment "Multal is a number property that refers to a large number of individuals."@eng .

gold:MultiplicativeNumeral a owl:Class ;
	rdfs:label "MultiplicativeNumeral"@eng ;
	rdfs:subClassOf gold:Numeral ;
	rdfs:isDefinedBy "http://purl.org/linguistics/gold"^^<http://www.w3.org/2001/XMLSchema#anyURI> ;
	rdfs:comment "A multiplicative numeral is a numeral that expresses how many fold or how many times [Pei and Gaynor 1954,149; Hartmann and Stork 1972,147]."@eng .

gold:NearFutureTense a owl:Class ;
	rdfs:label "NearFutureTense"@eng ;
	rdfs:subClassOf gold:TenseProperty ;
	rdfs:isDefinedBy "http://purl.org/linguistics/gold"^^<http://www.w3.org/2001/XMLSchema#anyURI> ;
	rdfs:comment ""@eng , "@en"@eng .

gold:NearlyExtinctVariety a owl:Class ;
	rdfs:label "NearlyExtinctVariety"@eng ;
	rdfs:subClassOf gold:HumanLanguageVariety ;
	rdfs:isDefinedBy "http://purl.org/linguistics/gold"^^<http://www.w3.org/2001/XMLSchema#anyURI> ;
	rdfs:comment "The class of languages that have relatively few native speakers. A nearly extinct variety is expected to become extrinct in a short time period, e.g., Jebero or Wichita."@eng .

gold:NecessitativePassiveVoice a owl:Class ;
	rdfs:label "NecessitativePassiveVoice"@eng ;
	rdfs:subClassOf gold:VoiceProperty ;
	rdfs:isDefinedBy "http://purl.org/linguistics/gold"^^<http://www.w3.org/2001/XMLSchema#anyURI> ;
	rdfs:comment "A passive in Irish in which the preposition \"with\" is used, and a semantic meaning of necessity is added. [Noonan 1994,280]"@eng .

gold:NecessityModality a owl:Class ;
	rdfs:label "NecessityModality"@eng ;
	rdfs:subClassOf gold:ModalityProperty ;
	rdfs:isDefinedBy "http://purl.org/linguistics/gold"^^<http://www.w3.org/2001/XMLSchema#anyURI> ;
	rdfs:comment "NecessityModality indicates that the described state of affairs is necessary, either directly, or because of a requirement on the part of an agent."@eng .

gold:NegationOperator a owl:Class ;
	rdfs:label "NegationOperator"@eng ;
	rdfs:subClassOf gold:PartOfSpeechProperty ;
	rdfs:isDefinedBy "http://purl.org/linguistics/gold"^^<http://www.w3.org/2001/XMLSchema#anyURI> ;
	rdfs:comment "no documentation yet"@eng .

gold:NegativePolarity a owl:Class ;
	rdfs:label "NegativePolarity"@eng ;
	rdfs:subClassOf gold:PolarityProperty ;
	rdfs:isDefinedBy "http://purl.org/linguistics/gold"^^<http://www.w3.org/2001/XMLSchema#anyURI> ;
	rdfs:comment "A construction that expresses the contradiction of some or all of a proposition [Crystal 1980,  257]. Note: this value is not to be confused with the notion \"Negative Polarity Item\", which is an expression that occurs in the scope of Negation (i.e. Negative Polarity)."@eng .

gold:NeuterGender a owl:Class ;
	rdfs:label "NeuterGender"@eng ;
	rdfs:subClassOf gold:GenderProperty ;
	rdfs:isDefinedBy "http://purl.org/linguistics/gold"^^<http://www.w3.org/2001/XMLSchema#anyURI> ;
	rdfs:comment "A gender property established on the basis of agreement, to which nouns may be assigned, either by a semantic rule, if they belong to the semantic residue of the assignment system, or by a formal rule, if assignment depends on inflectional class membership. Typically, this means that the neuter gender may cover some inanimates and possibly some portion of lower order animates. Note: Although in familiar Indo-European languages the term neuter gender may be part of a system with three or less values, it can be used for systems containing more than three gender values (e.g. Bininj Gunwok)."@eng , "NeuterGender"@eng .

gold:Nominal a owl:Class ;
	rdfs:label "Nominal"@eng ;
	rdfs:subClassOf gold:PartOfSpeechProperty ;
	rdfs:isDefinedBy "http://purl.org/linguistics/gold"^^<http://www.w3.org/2001/XMLSchema#anyURI> ;
	rdfs:comment "A nominal is a partOfSpeech whose members differ grammatically from a substantive but which functions as one [Crystal 1997, 260]."@eng .

gold:NominalClassifier a owl:Class ;
	rdfs:label "NominalClassifier"@eng ;
	rdfs:subClassOf gold:Classifier ;
	rdfs:isDefinedBy "http://purl.org/linguistics/gold"^^<http://www.w3.org/2001/XMLSchema#anyURI> ;
	rdfs:comment "suggested at E-MELD  (no documentation yet)"@eng .

gold:NominalParticle a owl:Class ;
	rdfs:label "NominalParticle"@eng ;
	rdfs:subClassOf gold:Particle ;
	rdfs:isDefinedBy "http://purl.org/linguistics/gold"^^<http://www.w3.org/2001/XMLSchema#anyURI> ;
	rdfs:comment "A nominal particle is a member of a closed class of particles that co-occur with nouns."@eng .

gold:Nominalizer a owl:Class ;
	rdfs:label "Nominalizer"@eng ;
	rdfs:subClassOf gold:CategoryChanger ;
	rdfs:isDefinedBy "http://purl.org/linguistics/gold"^^<http://www.w3.org/2001/XMLSchema#anyURI> ;
	rdfs:comment "Nominalizer is the class of category changing units that change a verb or verb phrase to a corresponding nominal."@eng .

gold:NominativeCase a owl:Class ;
	rdfs:label "NominativeCase"@eng ;
	rdfs:subClassOf gold:CaseProperty ;
	rdfs:isDefinedBy "http://purl.org/linguistics/gold"^^<http://www.w3.org/2001/XMLSchema#anyURI> ;
	rdfs:comment "NominativeCase identifies clause subjects in nominative-accusative languages. It is usually the unmarked case. Nouns used in isolation often have this case [Crystal 1980, 242; Pei and Gaynor 1954, 147; Hartmann and Stork 1972, 224]."@eng .

gold:NonAbsolutiveAntipassiveVoice a owl:Class ;
	rdfs:label "NonAbsolutiveAntipassiveVoice"@eng ;
	rdfs:subClassOf gold:VoiceProperty ;
	rdfs:isDefinedBy "http://purl.org/linguistics/gold"^^<http://www.w3.org/2001/XMLSchema#anyURI> ;
	rdfs:comment "An Antipassive in which the P or logical object is overtly downgraded.  [Klaiman 1991,232]"@eng .

gold:NonFutureTense a owl:Class ;
	rdfs:label "NonFutureTense"@eng ;
	rdfs:subClassOf gold:TenseProperty ;
	rdfs:isDefinedBy "http://purl.org/linguistics/gold"^^<http://www.w3.org/2001/XMLSchema#anyURI> ;
	rdfs:comment "NonFutureTense locates the situation in question at or before the moment of utterance, and contrasts with a FutureTense [Comrie 1985, 49]."@eng .

gold:NonPastTense a owl:Class ;
	rdfs:label "NonPastTense"@eng ;
	rdfs:subClassOf gold:TenseProperty ;
	rdfs:isDefinedBy "http://purl.org/linguistics/gold"^^<http://www.w3.org/2001/XMLSchema#anyURI> ;
	rdfs:comment "NonPastTense locates the situation in question at or after the moment of utterance, and contrasts with a past tense [Comrie 1985,48-49]."@eng .

gold:NonProgressiveAspect a owl:Class ;
	rdfs:label "NonProgressiveAspect"@eng ;
	rdfs:subClassOf gold:AspectProperty ;
	rdfs:isDefinedBy "http://purl.org/linguistics/gold"^^<http://www.w3.org/2001/XMLSchema#anyURI> ;
	rdfs:comment """A value of Aspect Property (also stative aspect) assigned to the designated element in the clause when the meaning selected for the clause is that which indicates that the situation spoken about has internal temporal structure, it cannot be regarded as habitual, but is regarded as a continuing state.  Hence, Nonprogressive Aspect can be regarded as a sub-type of continuousness (which, in turn, is a sub-type of imperfectivity). Since languages have different criteria for classifying predicates as stative or not, they may have different rules for determining when explicitly nonprogressive (i.e. explicitly stative) forms can be used.

Typically, for an aspect value to be labelled as Nonprogressive, the aspectual meaning has to minimally express nonprogressiveness, although it may additionally express other temporal, aspectual, or modal meanings, or actionality distinctions."""@eng , """A value of Aspect Property (also stative aspect) assigned to the designated element in the clause when the meaning selected for the clause is that which indicates that the situation spoken about has internal temporal structure, it cannot be regarded as habitual, but is regarded as a continuing state.  Hence, Nonprogressive Aspect can be regarded as a sub-type of continuousness (which, in turn, is a sub-type of imperfectivity). Since languages have different criteria for classifying predicates as stative or not, they may have different rules for determining when explicitly nonprogressive (i.e. explicitly stative) forms can be used.

Typically, for an aspect value to be labelled as Nonprogressive, the aspectual meaning has to minimally express nonprogressiveness, although it may additionally express other temporal, aspectual, or modal meanings, or actionality distinctions.@en"""@eng .

gold:NonPromotionalInverseVoice a owl:Class ;
	rdfs:label "NonPromotionalInverseVoice"@eng ;
	rdfs:subClassOf gold:VoiceProperty ;
	rdfs:isDefinedBy "http://purl.org/linguistics/gold"^^<http://www.w3.org/2001/XMLSchema#anyURI> ;
	rdfs:comment "Involves demotion of the non-topical obviate-agent from subjecthood. [Givon 1994,24]"@eng .

gold:NounClassifier a owl:Class ;
	rdfs:label "NounClassifier"@eng ;
	rdfs:subClassOf gold:Classifier ;
	rdfs:isDefinedBy "http://purl.org/linguistics/gold"^^<http://www.w3.org/2001/XMLSchema#anyURI> ;
	rdfs:comment "A classifier is a partOfSpeech whose members express the classification of a noun [Crystal 1997,61; Payne 1997,107]."@eng .

gold:NounPhrase a owl:Class ;
	rdfs:label "NounPhrase"@eng ;
	rdfs:subClassOf gold:Phrase ;
	rdfs:isDefinedBy "http://purl.org/linguistics/gold"^^<http://www.w3.org/2001/XMLSchema#anyURI> ;
	rdfs:comment "NounPhrase is the class of phrases that have nouns as heads. They can play the role of subject in a main clause."@eng .

gold:NucleonicMiddleVoice a owl:Class ;
	rdfs:label "NucleonicMiddleVoice"@eng ;
	rdfs:subClassOf gold:VoiceProperty ;
	rdfs:isDefinedBy "http://purl.org/linguistics/gold"^^<http://www.w3.org/2001/XMLSchema#anyURI> ;
	rdfs:comment """Object of action belongs to. Moves into, or moves from sphere of subject.
[Siewierska 1988,257]"""@eng .

gold:NumeralClassifier a owl:Class ;
	rdfs:label "NumeralClassifier"@eng ;
	rdfs:subClassOf gold:Classifier ;
	rdfs:isDefinedBy "http://purl.org/linguistics/gold"^^<http://www.w3.org/2001/XMLSchema#anyURI> ;
	rdfs:comment "suggested at E-MELD  (no documentation yet)"@eng .

gold:ObligativeModality a owl:Class ;
	rdfs:label "ObligativeModality"@eng ;
	rdfs:subClassOf gold:ModalityProperty ;
	rdfs:isDefinedBy "http://purl.org/linguistics/gold"^^<http://www.w3.org/2001/XMLSchema#anyURI> ;
	rdfs:comment "ObligativeModality indicates that an agent is required to perform the action expressed by the predicate [Bybee, Perkins, and Pagliuca 1994, 177; Palmer 2001, 71]."@eng .

gold:ObliqueCase a owl:Class ;
	rdfs:label "ObliqueCase"@eng ;
	rdfs:subClassOf gold:CaseProperty ;
	rdfs:isDefinedBy "http://purl.org/linguistics/gold"^^<http://www.w3.org/2001/XMLSchema#anyURI> ;
	rdfs:comment "ObliqueCase"@eng .

gold:ObliquePassiveVoice a owl:Class ;
	rdfs:label "ObliquePassiveVoice"@eng ;
	rdfs:subClassOf gold:VoiceProperty ;
	rdfs:isDefinedBy "http://purl.org/linguistics/gold"^^<http://www.w3.org/2001/XMLSchema#anyURI> ;
	rdfs:comment "A Passive in which a basic Oblique nominal assumes the Subject relation in a corresponding nonbasic configuration.  Can include locative passives, benefactive passives and instrumental passives. [Klaiman 1991,23]"@eng .

gold:OptativeMood a owl:Class ;
	rdfs:label "OptativeMood"@eng ;
	rdfs:subClassOf gold:MoodProperty ;
	rdfs:isDefinedBy "http://purl.org/linguistics/gold"^^<http://www.w3.org/2001/XMLSchema#anyURI> ;
	rdfs:comment "Optative indicates that the speaker wishes or hopes that the expressed proposition be the case [Bybee, Perkins, and Pagliuca 1994, 179; Palmer 2001, 204]."@eng .

gold:OrdinalNumeral a owl:Class ;
	rdfs:label "OrdinalNumeral"@eng ;
	rdfs:subClassOf gold:Numeral ;
	rdfs:isDefinedBy "http://purl.org/linguistics/gold"^^<http://www.w3.org/2001/XMLSchema#anyURI> ;
	rdfs:comment "An ordinal numeral is a numeral belonging to a class whose members designate positions in a sequence [Crystal 1997,272]."@eng .

gold:OrthographicSentence a owl:Class ;
	rdfs:label "OrthographicSentence"@eng ;
	rdfs:subClassOf gold:OrthographicPhrase ;
	rdfs:isDefinedBy "http://purl.org/linguistics/gold"^^<http://www.w3.org/2001/XMLSchema#anyURI> ;
	rdfs:comment "An OrthographicSentence is a special type of orthographic phrase, usually representing a clause. In Western writing systems, an orthographic sentence is set off by white space on the left edge and some kind of puncuation, such as a period or question mark, on the right."@eng .

gold:OrthographicSystem a owl:Class ;
	rdfs:label "OrthographicSystem"@eng ;
	rdfs:subClassOf gold:Abstract ;
	rdfs:isDefinedBy "http://purl.org/linguistics/gold"^^<http://www.w3.org/2001/XMLSchema#anyURI> .

gold:OrthographicWord a owl:Class ;
	rdfs:label "OrthographicWord"@eng ;
	rdfs:subClassOf gold:WrittenLinguisticExpression ;
	rdfs:isDefinedBy "http://purl.org/linguistics/gold"^^<http://www.w3.org/2001/XMLSchema#anyURI> ;
	rdfs:comment "An OrthographicWord is a fundamental unit of an orthography, usually set off by white space and dependent on the rules of a writing system."@eng .

gold:OtherSourceEvidentiality a owl:Class ;
	rdfs:label "OtherSourceEvidentiality"@eng ;
	rdfs:subClassOf gold:EvidentialityProperty ;
	rdfs:isDefinedBy "http://purl.org/linguistics/gold"^^<http://www.w3.org/2001/XMLSchema#anyURI> ;
	rdfs:comment "OtherSourceEvidentiality indicates that the agent relies on another source for theirbelief in what they say."@eng .

gold:OtherThanVisualEvidentiality a owl:Class ;
	rdfs:label "OtherThanVisualEvidentiality"@eng ;
	rdfs:subClassOf gold:EvidentialityProperty ;
	rdfs:isDefinedBy "http://purl.org/linguistics/gold"^^<http://www.w3.org/2001/XMLSchema#anyURI> ;
	rdfs:comment "OtherThanVisualEvidentiality encodes the fact that the speaker came to believe the content of the expression directly in a way other than through visual experience; they heard it, smelled it, tasted it, etc. [Palmer 2001, 36, 57]."@eng .

gold:Paragraph a owl:Class ;
	rdfs:label "Paragraph"@eng ;
	rdfs:subClassOf gold:WrittenLinguisticExpression ;
	rdfs:isDefinedBy "http://purl.org/linguistics/gold"^^<http://www.w3.org/2001/XMLSchema#anyURI> ;
	rdfs:comment "A Paragraph is a self contained unit in written language composed of a sequence of orthographic sentences. Paragraphs are set off by vertical spacing, indentation or other conventions."@eng .

gold:Participle a owl:Class ;
	rdfs:label "Participle"@eng ;
	rdfs:subClassOf gold:PartOfSpeechProperty ;
	rdfs:isDefinedBy "http://purl.org/linguistics/gold"^^<http://www.w3.org/2001/XMLSchema#anyURI> ;
	rdfs:comment "no documentation yet"@eng .

gold:PartitiveCase a owl:Class ;
	rdfs:label "PartitiveCase"@eng ;
	rdfs:subClassOf gold:CaseProperty ;
	rdfs:isDefinedBy "http://purl.org/linguistics/gold"^^<http://www.w3.org/2001/XMLSchema#anyURI> ;
	rdfs:comment "PartitiveCase expresses the partial nature of the referent of the noun it marks, as opposed to expressing the whole unit or class of which the referent is a part. This case may be found in items such as the following: existential clauses, nouns that are accompanied by numerals or units of measure, or predications of material from which something is made. It often has a meaning similar to the English word 'some' [Pei and Gaynor 1954, 161; Richards, Platt, and Weber 1985, 208; Quirk, et al. 1985, 249; Sebeok 1946, 1214]."@eng .

gold:PartitiveNumeral a owl:Class ;
	rdfs:label "PartitiveNumeral"@eng ;
	rdfs:subClassOf gold:Numeral ;
	rdfs:isDefinedBy "http://purl.org/linguistics/gold"^^<http://www.w3.org/2001/XMLSchema#anyURI> ;
	rdfs:comment "A partitive numeral is a numeral that expresses a fraction [Pei and Gaynor 1954, 149; Hartmann and Stork 1972, 165]."@eng .

gold:PassiveVoice a owl:Class ;
	rdfs:label "PassiveVoice"@eng ;
	rdfs:subClassOf gold:VoiceProperty ;
	rdfs:isDefinedBy "http://purl.org/linguistics/gold"^^<http://www.w3.org/2001/XMLSchema#anyURI> ;
	rdfs:comment """Associated with actions performed on the subject by an unspecified agent.
[McIntosh 1984,108] Refers to the category of verb forms, typically identifies with a specific morphological marking, that encode the derived diatheses in which the agent role is not linked with a subject noun phrase: Diatheis: D1=(X=AgOb)(Y+SUBabs/nom) [Shibatani 1995,7]"""@eng .

gold:PastInPastTense a owl:Class ;
	rdfs:label "PastInPastTense"@eng ;
	rdfs:subClassOf gold:TenseProperty ;
	rdfs:isDefinedBy "http://purl.org/linguistics/gold"^^<http://www.w3.org/2001/XMLSchema#anyURI> ;
	rdfs:comment "Locates the situation in question prior to a reference time in the past before the time of the speaking event. This is also known as the PluperfectTense [Comrie 1985, 125]."@eng .

gold:PastPerfectTense a owl:Class ;
	rdfs:label "PastPerfectTense"@eng ;
	rdfs:subClassOf gold:TenseProperty ;
	rdfs:isDefinedBy "http://purl.org/linguistics/gold"^^<http://www.w3.org/2001/XMLSchema#anyURI> ;
	rdfs:comment "Locates the situation in question in the future, prior to a reference time in the future. Also called PastInPast tense."@eng .

gold:PastTense a owl:Class ;
	rdfs:label "PastTense"@eng ;
	rdfs:subClassOf gold:TenseProperty ;
	rdfs:isDefinedBy "http://purl.org/linguistics/gold"^^<http://www.w3.org/2001/XMLSchema#anyURI> ;
	rdfs:comment """A value of Tense Property assigned to the designated element in the clause when the meaning selected for the clause is that intended to locate the event spoken about as anterior to the deictic centre of the utterance. Most commonly, this tense meaning is referred to as 'past', because in absolute tense systems the deictic centre is the moment of speech. However, in relative tense systems, where the deictic centre can be moved to any point on the time line, it is more appropriate to refer to this temporal relation as 'anterior'.

The anterior temporal relation may obtain either in 'simple' or 'perfect' contexts. Modelling of this distinction originates from [Reichenbach 1947], who suggested using a third point in time, 'reference point', to capture all possible tense distinctions. In all 'simple' temporal relations, the reference point coincides with the location of the event spoken about. 'Perfect' tense meanings are created when the reference point is separated and moved away from the event time, thus altering the viewing of the temporal location of the event even though the event's actual location with respect to the deictic centre remains the same. 

A common instance of an anterior temporal relationship obtaining in a 'perfect' context occurs when the reference point is moved away from the event time and located instead at the moment of speech. The event time is still anterior to the moment of speech, but it is viewed against a stretch of time which began at the event and continues up to the moment of speech --- e.g. the English I have read this book, I have seen John --- hence the interpretation that the event has an effect or is in some way still relevant at the moment of speech. In some languages (e.g. English) this tense meaning is labelled as (one of the uses of the) Present Perfect, in others (e.g. Polish) this meaning may be collapsed with the 'simple' anterior meaning and labelled simply as Past.

Typically, for a tense value to be labelled as Past Tense, the tense meaning has to minimally express the anterior temporal relationship, although it may additionally express other temporal relationships or aspectual and/or modal meanings. For example, when the usage of the Past Tense value is restricted to a semantically defined domain, it is conventional to add a further qualification to the label of the Past Tense value (e.g. Past Imperfective --- when the anterior temporal relationship is necessarily combined with an aspectual meaning of the Imperfective Aspect value, and grammaticalised as a single TAM category in the language)."""@eng .

gold:PaucalNumber a owl:Class ;
	rdfs:label "PaucalNumber"@eng ;
	rdfs:subClassOf gold:NumberProperty ;
	rdfs:isDefinedBy "http://purl.org/linguistics/gold"^^<http://www.w3.org/2001/XMLSchema#anyURI> .

gold:PejorativeEvaluative a owl:Class ;
	rdfs:label "PejorativeEvaluative"@eng ;
	rdfs:subClassOf gold:EvaluativeProperty ;
	rdfs:isDefinedBy "http://purl.org/linguistics/gold"^^<http://www.w3.org/2001/XMLSchema#anyURI> ;
	rdfs:comment "An evaluative property of a noun that indicates the speaker regards the person or object being referred to with distaste, contempt, or displeasure [Valentine 2001,  190-193]."@eng .

gold:PerfectTense a owl:Class ;
	rdfs:label "PerfectTense"@eng ;
	rdfs:subClassOf gold:TenseProperty ;
	rdfs:isDefinedBy "http://purl.org/linguistics/gold"^^<http://www.w3.org/2001/XMLSchema#anyURI> ;
	rdfs:comment """A value of Tense Feature assigned to the designated element in the clause when the meaning selected for the clause is that intended to locate the event spoken about as anterior, simultaneous, or posterior to the deictic centre of the utterance, and additionally the reference point from which this event is viewed is separated and moved away from the event time. This alters the viewing of the temporal location of the event even though the event's actual location with respect to the deictic centre remains the same. 'Perfect' temporal relations contrast with 'simple' temporal relations in which the reference point coincides with the location of the event spoken about. Modelling of this distinction originates from [Reichenbach 1947].

There are two types of 'perfect' context which may lead to separate tense values:

(1) The first type occurs when the reference point is moved away from the event time and instead located after the event time. A common example occurs with an anterior temporal relationship, when the reference point is moved from the event time to the moment of speech. The event time is anterior to the moment of speech, but it is viewed against a stretch of time which began at the event and continues up to the moment of speech --- e.g. the English I have read this book, I have seen John --- hence the interpretation that the event has an effect or is in
some way still relevant at the moment of speech. [Note that in some languages (e.g. English) this tense meaning is labelled as (one of the uses of the) Present Perfect, in others (e.g. Polish) this meaning may be collapsed with the 'simple' anterior meaning and labelled simply as
Past.] The interpretation of this type of the perfect often includes at least two related but distinguishable uses: the resultative perfect (Someone has stolen my purse) and the experiential perfect (I have read this book before) [Dahl and Velupillai 2005,271].

(2) The second type occurs when the reference point is moved away from the event time and instead located before the event time. A common example occurs with a simultaneous temporal relationship, when the reference point is moved from the event time and located before the moment of speech. The event time is still simultaneous with the moment of speech, but it is viewed against a stretch of time which began at the reference point and continues up to the moment of speech --- e.g. the English I have lived here [for ten years] --- hence the interpretation that the event which began in the past extends up to the moment of speech. [Note that in some languages (e.g. English) this tense meaning is labelled as (one of the uses of the) Present Perfect, in others (e.g. Polish) this meaning may be collapsed with the 'simple' simultaneous meaning and labelled simply as Present.] The interpretation of this type of the perfect is often referred to as the universal perfect or perfect of persistent situation.

Typically, for a tense value to be labelled as Perfect Tense, the tense meaning has to minimally express the meaning resulting from the separation of the reference point from the event time, although it may additionally express other temporal, aspectual, or modal meanings."""@eng .

gold:PerfectiveAspect a owl:Class ;
	rdfs:label "PerfectiveAspect"@eng ;
	rdfs:subClassOf gold:AspectProperty ;
	rdfs:isDefinedBy "http://purl.org/linguistics/gold"^^<http://www.w3.org/2001/XMLSchema#anyURI> ;
	rdfs:comment """A value of Aspect Property assigned to the designated element in the clause when the meaning selected for the clause is that which indicates that the event spoken about is to be viewed as a bounded whole, looked at from outside, without necessarily distinguishing any of its internal structure [Comrie 1976,16ff).

Typically, for an aspect value to be labeled as Perfective, the aspectual meaning has to minimally express the perfective viewpoint, although it may additionally express other temporal, aspectual, or modal meanings, or actionality distinctions."""@eng , """A value of Aspect Property assigned to the designated element in the clause when the meaning selected for the clause is that which indicates that the event spoken about is to be viewed as a bounded whole, looked at from outside, without necessarily distinguishing any of its internal structure [Comrie 1976,16ff).

Typically, for an aspect value to be labeled as Perfective, the aspectual meaning has to minimally express the perfective viewpoint, although it may additionally express other temporal, aspectual, or modal meanings, or actionality distinctions.@en"""@eng .

gold:PerlativeCase a owl:Class ;
	rdfs:label "PerlativeCase"@eng ;
	rdfs:subClassOf gold:CaseProperty ;
	rdfs:isDefinedBy "http://purl.org/linguistics/gold"^^<http://www.w3.org/2001/XMLSchema#anyURI> ;
	rdfs:comment "PerlativeCase expresses that something moved 'through','across', or 'along' the referent of the noun that is marked [Blake 2001]."@eng .

gold:PermissiveModality a owl:Class ;
	rdfs:label "PermissiveModality"@eng ;
	rdfs:subClassOf gold:ModalityProperty ;
	rdfs:isDefinedBy "http://purl.org/linguistics/gold"^^<http://www.w3.org/2001/XMLSchema#anyURI> ;
	rdfs:comment "PermissiveModality indicates that an agent has permission to perform the action expressed by the predicate [Palmer 2001, 10, 71]."@eng .

gold:PersonalPassiveVoice a owl:Class ;
	rdfs:label "PersonalPassiveVoice"@eng ;
	rdfs:subClassOf gold:VoiceProperty ;
	rdfs:isDefinedBy "http://purl.org/linguistics/gold"^^<http://www.w3.org/2001/XMLSchema#anyURI> ;
	rdfs:comment "A Passive in which the argument mapped to Object in a basic structural configuration assumes the Subject relation in a corresponding nonbasic configuration. [Klaiman 1991, 23]"@eng .

gold:PersonalPronoun a owl:Class ;
	rdfs:label "PersonalPronoun"@eng ;
	rdfs:subClassOf gold:Pronominal ;
	rdfs:isDefinedBy "http://purl.org/linguistics/gold"^^<http://www.w3.org/2001/XMLSchema#anyURI> ;
	rdfs:comment "A personal pronoun is a pronoun that expresses a distinction of person deixis."@eng .

gold:PhasalAspect a owl:Class ;
	rdfs:label "PhasalAspect"@eng ;
	rdfs:subClassOf gold:AspectProperty ;
	rdfs:isDefinedBy "http://purl.org/linguistics/gold"^^<http://www.w3.org/2001/XMLSchema#anyURI> ;
	rdfs:comment "A set of aspectual distinctions involving relations between a background situation (the reference situation) and a situation located relative to the reference situation (the denoted situation). In English, phasal distinctions are expressed by auxiliary-headed constructions, like the inceptive, progressive, and perfect constructions, whose head verbs express the aspectual class of the denoted situation. The aspectual class of the denoted situation differs from that of the reference situation [Michaelis 1998,xv]. An event may have a beginning and an end, a middle portion (continuing or changing), and also an ensuing result or an altered state. These are considered to be the various \"phases\" of an event. A speaker may talk about an event from the point of view of any of these individual phases, and his language may have inflectional (or other type of) markers for representing these distinctions. Since such markers indicate distinctions in the temporal structure of an event, we may regard them as belonging to the category of aspect. It has been suggested [Dik 1989, 186] that these may be grouped under a subcategory (or \"level\") of aspect called \"phasal aspect\". [Bhat 1999,49]"@eng .

gold:Phoneme a owl:Class ;
	rdfs:label "Phoneme"@eng ;
	rdfs:subClassOf gold:FormUnit ;
	rdfs:isDefinedBy "http://purl.org/linguistics/gold"^^<http://www.w3.org/2001/XMLSchema#anyURI> .

gold:PhonologicalProperty a owl:Class ;
	rdfs:label "PhonologicalProperty"@eng ;
	rdfs:subClassOf gold:LinguisticProperty ;
	rdfs:isDefinedBy "http://purl.org/linguistics/gold"^^<http://www.w3.org/2001/XMLSchema#anyURI> ;
	rdfs:comment "The class of linguistic properties that pertain to phonological units."@eng .

gold:PhonologicalSystem a owl:Class ;
	rdfs:label "PhonologicalSystem"@eng ;
	rdfs:subClassOf gold:Abstract ;
	rdfs:isDefinedBy "http://purl.org/linguistics/gold"^^<http://www.w3.org/2001/XMLSchema#anyURI> .

gold:PhysicalAbilitiveModality a owl:Class ;
	rdfs:label "PhysicalAbilitiveModality"@eng ;
	rdfs:subClassOf gold:ModalityProperty ;
	rdfs:isDefinedBy "http://purl.org/linguistics/gold"^^<http://www.w3.org/2001/XMLSchema#anyURI> .

gold:PlainAdjective a owl:Class ;
	rdfs:label "PlainAdjective"@eng ;
	rdfs:subClassOf gold:Adjectival ;
	rdfs:isDefinedBy "http://purl.org/linguistics/gold"^^<http://www.w3.org/2001/XMLSchema#anyURI> ;
	rdfs:comment "suggested at E-MELD  (no documentation yet)"@eng .

gold:PlainMiddleVoice a owl:Class ;
	rdfs:label "PlainMiddleVoice"@eng ;
	rdfs:subClassOf gold:VoiceProperty ;
	rdfs:isDefinedBy "http://purl.org/linguistics/gold"^^<http://www.w3.org/2001/XMLSchema#anyURI> ;
	rdfs:comment """Results of action occur to subject.
[Siewierska 1988,257]"""@eng .

gold:PluralNumber a owl:Class ;
	rdfs:label "PluralNumber"@eng ;
	rdfs:subClassOf gold:NumberProperty ;
	rdfs:isDefinedBy "http://purl.org/linguistics/gold"^^<http://www.w3.org/2001/XMLSchema#anyURI> ;
	rdfs:comment """PluralNumber is a number property that quantifies the denotation of the nominal element so that: 1) it specifies that there are more than one. In this English example below, plural is shown by both the noun and the verb in (2): 

(1) my dog watches television 
(2) my dogs watch television 

[Corbett 2000: 5] 

2) additionally, but not necessarily, pluralNumber may be assigned on the basis of formal properties (e.g. pluralia tantum, or measles / *measle). 3) if pluralNumber functions as generalNumber, it may specify a lack of commitment with regard to quantification ([Corbett 2000,17] notes this system does not exist in pure form, that is, no language employs it as the normal case).

Some Cushitic languages, generalNumber can be the same as singularNumber for some nouns, but the same as pluralNumber for other nouns. For example, in Arbore (arv), generalNumber may contrast with the singular in the absence of a distinct plural form: Ln Singular Ln tiis-in 'a maize cob' Ln lasa-n 'a loaf' 

nebel-in 'a cock ostrich' ln General ln tíise 'maize cob(s)' ln lássa 'bread' ln nebel 'ostrich(es)' ln [Corbett 2000: 17-18]"""@eng .

gold:PlusATR a owl:Class ;
	rdfs:label "PlusATR"@eng ;
	rdfs:subClassOf gold:RadicalProperty ;
	rdfs:isDefinedBy "http://purl.org/linguistics/gold"^^<http://www.w3.org/2001/XMLSchema#anyURI> ;
	rdfs:comment "Characterizing sounds made with advanced tongue root."@eng .

gold:PlusClick a owl:Class ;
	rdfs:label "PlusClick"@eng ;
	rdfs:subClassOf gold:VelaricProperty ;
	rdfs:isDefinedBy "http://purl.org/linguistics/gold"^^<http://www.w3.org/2001/XMLSchema#anyURI> ;
	rdfs:comment "[Need comment]"@eng .

gold:PlusFortis a owl:Class ;
	rdfs:label "PlusFortis"@eng ;
	rdfs:subClassOf gold:PulmonicProperty ;
	rdfs:isDefinedBy "http://purl.org/linguistics/gold"^^<http://www.w3.org/2001/XMLSchema#anyURI> ;
	rdfs:comment "[Need comment]"@eng .

gold:PlusNasal a owl:Class ;
	rdfs:label "PlusNasal"@eng ;
	rdfs:subClassOf gold:NasalityProperty ;
	rdfs:isDefinedBy "http://purl.org/linguistics/gold"^^<http://www.w3.org/2001/XMLSchema#anyURI> ;
	rdfs:comment "Characterizing sounds produced with air escaping through the nose."@eng , "PlusNasal"@eng .

gold:PoliticalTaxon a owl:Class ;
	rdfs:label "PoliticalTaxon"@eng ;
	rdfs:subClassOf gold:LinguisticTaxon ;
	rdfs:isDefinedBy "http://purl.org/linguistics/gold"^^<http://www.w3.org/2001/XMLSchema#anyURI> ;
	rdfs:comment "PoliticalTaxon is the class of taxons whose instances are groupings based on political entities such as states or countries or larger politically defined entities, e.g., CameroonianLanguage."@eng .

gold:PositivePolarity a owl:Class ;
	rdfs:label "PositivePolarity"@eng ;
	rdfs:subClassOf gold:PolarityProperty ;
	rdfs:isDefinedBy "http://purl.org/linguistics/gold"^^<http://www.w3.org/2001/XMLSchema#anyURI> ;
	rdfs:comment "In general, positive polarity refers to an assertion that contains no marker of negation [Crystal 1980,  299]."@eng .

gold:PossessedCase a owl:Class ;
	rdfs:label "PossessedCase"@eng ;
	rdfs:subClassOf gold:CaseProperty ;
	rdfs:isDefinedBy "http://purl.org/linguistics/gold"^^<http://www.w3.org/2001/XMLSchema#anyURI> ;
	rdfs:comment "PossessedCase is used to mark the noun whose referent is possessed by the referent of another noun."@eng .

gold:PossessivePronoun a owl:Class ;
	rdfs:label "PossessivePronoun"@eng ;
	rdfs:subClassOf gold:Pronominal ;
	rdfs:isDefinedBy "http://purl.org/linguistics/gold"^^<http://www.w3.org/2001/XMLSchema#anyURI> ;
	rdfs:comment "A possessive pronoun is a pronoun that expresses ownership and relationships like ownership, such as kinship, and other forms of association [Crystal 1997,312]."@eng .

gold:PossibilityModality a owl:Class ;
	rdfs:label "PossibilityModality"@eng ;
	rdfs:subClassOf gold:ModalityProperty ;
	rdfs:isDefinedBy "http://purl.org/linguistics/gold"^^<http://www.w3.org/2001/XMLSchema#anyURI> ;
	rdfs:comment "PossibilityModality indicates that the designated state of affairs is possible, either directly, or because an agent has the ability or permission to carry it out."@eng .

gold:PostHodiernalFutureTense a owl:Class ;
	rdfs:label "PostHodiernalFutureTense"@eng ;
	rdfs:subClassOf gold:TenseProperty ;
	rdfs:isDefinedBy "http://purl.org/linguistics/gold"^^<http://www.w3.org/2001/XMLSchema#anyURI> ;
	rdfs:comment "PostHodiernalFutureTense locates the situation in question after the span that is culturally defined as 'today' [Bybee, Perkins, and Pagliuca 1994, 247]."@eng .

gold:Postalveolar a owl:Class ;
	rdfs:label "Postalveolar"@eng ;
	rdfs:subClassOf gold:AnteriorProperty ;
	rdfs:isDefinedBy "http://purl.org/linguistics/gold"^^<http://www.w3.org/2001/XMLSchema#anyURI> ;
	rdfs:comment "Characterizing sounds produced with the area just behind the center of the alveolar ridge as the passive articulator [Ladefoged 1997, 597]."@eng .

gold:Postposition a owl:Class ;
	rdfs:label "Postposition"@eng ;
	rdfs:subClassOf gold:Adposition ;
	rdfs:isDefinedBy "http://purl.org/linguistics/gold"^^<http://www.w3.org/2001/XMLSchema#anyURI> ;
	rdfs:comment "A postposition is an adposition that occurs after its complement [Crystal 1997,300; Payne 1997,86]."@eng .

gold:PragmaticInverseVoice a owl:Class ;
	rdfs:label "PragmaticInverseVoice"@eng ;
	rdfs:subClassOf gold:VoiceProperty ;
	rdfs:isDefinedBy "http://purl.org/linguistics/gold"^^<http://www.w3.org/2001/XMLSchema#anyURI> ;
	rdfs:comment "If the agent is more topical than the patient, the direct-active clause is used.  If norm is reversed and the patient is more topical, the inverse clause is used. [Givon 1994,23]"@eng .

gold:PreHodiernalPastTense a owl:Class ;
	rdfs:label "PreHodiernalPastTense"@eng ;
	rdfs:subClassOf gold:TenseProperty ;
	rdfs:isDefinedBy "http://purl.org/linguistics/gold"^^<http://www.w3.org/2001/XMLSchema#anyURI> ;
	rdfs:comment "PreHodiernalPastTense locates the situation in question before that of a contrasting HodiernalPastTense. According to Bybee, Perkins, Pagliuca 1994, 98. this category must be defined relative to a HodiernalPastTense."@eng .

gold:Predicative a owl:Class ;
	rdfs:label "Predicative"@eng ;
	rdfs:subClassOf gold:Predicator ;
	rdfs:isDefinedBy "http://purl.org/linguistics/gold"^^<http://www.w3.org/2001/XMLSchema#anyURI> .

gold:PreferredEvaluative a owl:Class ;
	rdfs:label "PreferredEvaluative"@eng ;
	rdfs:subClassOf gold:EvaluativeProperty ;
	rdfs:isDefinedBy "http://purl.org/linguistics/gold"^^<http://www.w3.org/2001/XMLSchema#anyURI> ;
	rdfs:comment "An evaluative property  of a noun that indicates the speaker regards the person or object being referred to with favor or admiration."@eng .

gold:Prefix a owl:Class ;
	rdfs:label "Prefix"@eng ;
	rdfs:subClassOf gold:Affix ;
	rdfs:isDefinedBy "http://purl.org/linguistics/gold"^^<http://www.w3.org/2001/XMLSchema#anyURI> .

gold:Prenoun a owl:Class ;
	rdfs:label "Prenoun"@eng ;
	rdfs:subClassOf gold:PartOfSpeechProperty ;
	rdfs:isDefinedBy "http://purl.org/linguistics/gold"^^<http://www.w3.org/2001/XMLSchema#anyURI> ;
	rdfs:comment "An element which may be compounded to the front of a noun to signal information such as size, color, etc. [Valentine 2001,  152-154]."@eng .

gold:Preposition a owl:Class ;
	rdfs:label "Preposition"@eng ;
	rdfs:subClassOf gold:Adposition ;
	rdfs:isDefinedBy "http://purl.org/linguistics/gold"^^<http://www.w3.org/2001/XMLSchema#anyURI> ;
	rdfs:comment "A preposition is an adposition that occurs before its complement [Crystal 1997, 305; Payne 1997, 86]."@eng .

gold:PresentPerfectTense a owl:Class ;
	rdfs:label "PresentPerfectTense"@eng ;
	rdfs:subClassOf gold:TenseProperty ;
	rdfs:isDefinedBy "http://purl.org/linguistics/gold"^^<http://www.w3.org/2001/XMLSchema#anyURI> ;
	rdfs:comment """The simultaneous temporal relation may obtain either in 'simple' or 'perfect' contexts.  Modelling of this distinction originates from [Reichenbach 1947], who suggested using a third point in time, 'reference point', to capture all possible tense distinctions. In all 'simple' temporal relations, the reference point coincides with the location of the event spoken about.  'Perfect' tense meanings are created when the reference point is separated and moved away from the event time, thus altering the viewing of the temporal location of the event even though the event's actual location with respect to the deictic centre remains the same.

A common instance of a simultaneous temporal relationship obtaining in a 'perfect' context occurs when the reference point is moved away from the event time and located instead before the moment of speech. The event time is still simultaneous with the moment of speech, but it is viewed against a stretch of time which began at the reference point and continues up to the moment of speech --- e.g. the English I have lived here [for ten years] --- hence the interpretation that the event which began in the past extends up to the moment of speech. In some languages (e.g. English) this tense meaning is labelled as (one of the uses of the) Present Perfect, in others (e.g. Polish) this meaning may be collapsed with the 'simple' simultaneous meaning and labelled simply as Present."""@eng .

gold:PresentTense a owl:Class ;
	rdfs:label "PresentTense"@eng ;
	rdfs:subClassOf gold:TenseProperty ;
	rdfs:isDefinedBy "http://purl.org/linguistics/gold"^^<http://www.w3.org/2001/XMLSchema#anyURI> ;
	rdfs:comment """A value of Tense Property assigned to the designated element in the clause when the meaning selected for the clause is that intended to locate the event spoken about as simultaneous with the deictic centre of the utterance. Most commonly, this tense meaning is referred to as 'present', because in absolute tense systems the deictic centre is the moment of speech.  However, in relative tense systems, where the deictic centre can be moved to any point on the time line, it is more appropriate to refer to this temporal relation as 'simultaneous'.

It is important to note --- for all tense values, but in particular for the Present Tense --- that the 'times' which are used to locate the event, the deictic centre, and the reference point, may or may not be 'points' on the time line. Conventionally, these concepts are considered neutral with regard to whether they are points or intervals of time longer than a point. In a formal model of tense meanings they could, for example, be represented as sets (of points): in order to capture temporal distinctions, the notion of an event being 'simultaneous with the moment of speech', may be understood as (the set of) event time (points) and (the set of) speech time (points) having a non-empty intersection. Hence, this semantic model of the Present Tense value may include the interpretation of the present as 'universal' or 'generic'.

The simultaneous temporal relation may obtain either in 'simple' or 'perfect' contexts. Modelling of this distinction originates from [Reichenbach  1947], who suggested using a third point in time, 'reference point', to capture all possible tense distinctions. In all 'simple' temporal relations, the reference point coincides with the location of the event spoken about. 'Perfect' tense meanings are created when the reference point is separated and moved away from the event time, thus altering the viewing of the temporal location of the event even though the event's actual location with respect to the deictic centre remains the same.

A common instance of a simultaneous temporal relationship obtaining in a 'perfect' context occurs when the reference point is moved away from the event time and located instead before the moment of speech. The event time is still simultaneous with the moment of speech, but it is viewed against a stretch of time which began at the reference point and continues up to the moment of speech --- e.g. the English I have lived here [for ten years] ---
hence the interpretation that the event which began in the past extends up to the moment of speech. In some languages (e.g. English) this tense meaning is labelled as (one of the uses of the) Present Perfect, in others (e.g. Polish) this meaning may be collapsed with the 'simple' simultaneous meaning and labelled simply as Present.

Typically, for a tense value to be labelled as Present Tense, the tense meaning has to minimally express the simultaneous temporal relationship, although it may additionally express other temporal, aspectual, or modal meanings."""@eng .

gold:Preverb a owl:Class ;
	rdfs:label "Preverb"@eng ;
	rdfs:subClassOf gold:PartOfSpeechProperty ;
	rdfs:isDefinedBy "http://purl.org/linguistics/gold"^^<http://www.w3.org/2001/XMLSchema#anyURI> ;
	rdfs:comment "An element which may be compounded to the front of a verb, to signal information such as tense, direction, etc. [Valentine 2001,  154-158]."@eng .

gold:Proadjective a owl:Class ;
	rdfs:label "Proadjective"@eng ;
	rdfs:subClassOf gold:ProForm ;
	rdfs:isDefinedBy "http://purl.org/linguistics/gold"^^<http://www.w3.org/2001/XMLSchema#anyURI> ;
	rdfs:comment "A Proadjective is a proForm that substitutes for an adjective or adjective phrase."@eng .

gold:Proadverb a owl:Class ;
	rdfs:label "Proadverb"@eng ;
	rdfs:subClassOf gold:ProForm ;
	rdfs:isDefinedBy "http://purl.org/linguistics/gold"^^<http://www.w3.org/2001/XMLSchema#anyURI> ;
	rdfs:comment "A Proadverb is a Proform that substitutes for an adverb or other expression having an adverbial function."@eng .

gold:Process a owl:Class ;
	rdfs:label "Process"@eng ;
	rdfs:subClassOf owl:Thing ;
	rdfs:isDefinedBy "http://purl.org/linguistics/gold"^^<http://www.w3.org/2001/XMLSchema#anyURI> ;
	rdfs:comment "Any entity that is relatively time unstable and has other processes as parts. See SUMO for a detailed explanation."@eng .

gold:Processive a owl:Class ;
	rdfs:label "Processive"@eng ;
	rdfs:subClassOf gold:DerivationalUnit ;
	rdfs:isDefinedBy "http://purl.org/linguistics/gold"^^<http://www.w3.org/2001/XMLSchema#anyURI> ;
	rdfs:comment "A derivational unit that derives transitives from other transitives or intransitive verb (stems)."@eng .

gold:Proclitic a owl:Class ;
	rdfs:label "Proclitic"@eng ;
	rdfs:subClassOf gold:Clitic ;
	rdfs:isDefinedBy "http://purl.org/linguistics/gold"^^<http://www.w3.org/2001/XMLSchema#anyURI> ;
	rdfs:comment "A proclitic is a clitic that precedes the lexical unit to which it is phonologically joined [Crystal 1980,64; Hartmann and Stork 1972,185; Pei and Gaynor 1954,176]."@eng .

gold:ProgressiveAspect a owl:Class ;
	rdfs:label "ProgressiveAspect"@eng ;
	rdfs:subClassOf gold:AspectProperty ;
	rdfs:isDefinedBy "http://purl.org/linguistics/gold"^^<http://www.w3.org/2001/XMLSchema#anyURI> ;
	rdfs:comment """A value of Aspect Property (also called Nonstative aspect) assigned to the designated element in the clause when the meaning selected for the clause is that which indicates that the situation spoken about has internal temporal structure, it cannot be regarded as habitual, and reference is made to this situation in progress. Hence, progressiveness can be defined as the combination of progressive meaning with nonstative meaning, and it can be regarded as a sub-type of continuousness (which, in turn, is a sub-type of imperfectivity). Since languages have different criteria for classifying predicates as stative or not, they may have different rules for determining when explicitly progressive forms can be used.

Typically, for an aspect value to be labelled as Progressive, the aspectual meaning has to minimally express progressiveness, although it may additionally express other temporal, aspectual, or modal meanings, or actionality distinctions."""@eng , """A value of Aspect Property (also called Nonstative aspect) assigned to the designated element in the clause when the meaning selected for the clause is that which indicates that the situation spoken about has internal temporal structure, it cannot be regarded as habitual, and reference is made to this situation in progress. Hence, progressiveness can be defined as the combination of progressive meaning with nonstative meaning, and it can be regarded as a sub-type of continuousness (which, in turn, is a sub-type of imperfectivity). Since languages have different criteria for classifying predicates as stative or not, they may have different rules for determining when explicitly progressive forms can be used.

Typically, for an aspect value to be labelled as Progressive, the aspectual meaning has to minimally express progressiveness, although it may additionally express other temporal, aspectual, or modal meanings, or actionality distinctions.@en"""@eng .

gold:ProgressivePassiveVoice a owl:Class ;
	rdfs:label "ProgressivePassiveVoice"@eng ;
	rdfs:subClassOf gold:VoiceProperty ;
	rdfs:isDefinedBy "http://purl.org/linguistics/gold"^^<http://www.w3.org/2001/XMLSchema#anyURI> ;
	rdfs:comment "A passive in Irish  in which the preposition \"at\" is used, and a semantic meaning of progressive tense is found [Noonan 1994,280]"@eng .

gold:ProhibitiveMood a owl:Class ;
	rdfs:label "ProhibitiveMood"@eng ;
	rdfs:subClassOf gold:MoodProperty ;
	rdfs:isDefinedBy "http://purl.org/linguistics/gold"^^<http://www.w3.org/2001/XMLSchema#anyURI> ;
	rdfs:comment "Used to issue warnings."@eng , "ProhibitiveMood"@eng .

gold:PromotionalInverseVoice a owl:Class ;
	rdfs:label "PromotionalInverseVoice"@eng ;
	rdfs:subClassOf gold:VoiceProperty ;
	rdfs:isDefinedBy "http://purl.org/linguistics/gold"^^<http://www.w3.org/2001/XMLSchema#anyURI> ;
	rdfs:comment "Involves promotion of the topical proximate-patient to subjecthood. [Givon 1994,24]"@eng .

gold:ProperNoun a owl:Class ;
	rdfs:label "ProperNoun"@eng ;
	rdfs:subClassOf gold:Noun ;
	rdfs:isDefinedBy "http://purl.org/linguistics/gold"^^<http://www.w3.org/2001/XMLSchema#anyURI> ;
	rdfs:comment "ProperNoun, also referred to as proper names, is the class of nouns that are used to address particular persons or culturally significant personages or places. They refer to specific entities and are not usually with articles, modifiers, possessors [Payne 1997, 39]."@eng .

gold:Protruded a owl:Class ;
	rdfs:label "Protruded"@eng ;
	rdfs:subClassOf gold:LabialProperty ;
	rdfs:isDefinedBy "http://purl.org/linguistics/gold"^^<http://www.w3.org/2001/XMLSchema#anyURI> ;
	rdfs:comment "[Need comment]"@eng .

gold:Proverb a owl:Class ;
	rdfs:label "Proverb"@eng ;
	rdfs:subClassOf gold:Verbal ;
	rdfs:isDefinedBy "http://purl.org/linguistics/gold"^^<http://www.w3.org/2001/XMLSchema#anyURI> ;
	rdfs:comment "no documentation yet"@eng .

gold:QuantificationalAspect a owl:Class ;
	rdfs:label "QuantificationalAspect"@eng ;
	rdfs:subClassOf gold:AspectProperty ;
	rdfs:isDefinedBy "http://purl.org/linguistics/gold"^^<http://www.w3.org/2001/XMLSchema#anyURI> .

gold:RealisMood a owl:Class ;
	rdfs:label "RealisMood"@eng ;
	rdfs:subClassOf gold:MoodProperty ;
	rdfs:isDefinedBy "http://purl.org/linguistics/gold"^^<http://www.w3.org/2001/XMLSchema#anyURI> ;
	rdfs:comment "Same as Indicative mood."@eng , "ReallisModality"@eng .

gold:RecentPastTense a owl:Class ;
	rdfs:label "RecentPastTense"@eng ;
	rdfs:subClassOf gold:TenseProperty ;
	rdfs:isDefinedBy "http://purl.org/linguistics/gold"^^<http://www.w3.org/2001/XMLSchema#anyURI> ;
	rdfs:comment "RecentPastTense locates the situation in question prior to the present moment, but by culturally and situationally defined criteria, usually within the span ranging from yesterday to a week or a few months previous [Comrie 1985,87; Dahl 1985,121-122]."@eng .

gold:RecentTense a owl:Class ;
	rdfs:label "RecentTense"@eng ;
	rdfs:subClassOf gold:TenseProperty ;
	rdfs:isDefinedBy "http://purl.org/linguistics/gold"^^<http://www.w3.org/2001/XMLSchema#anyURI> ;
	rdfs:comment "RecentTense"@eng .

gold:ReciprocalMiddleVoice a owl:Class ;
	rdfs:label "ReciprocalMiddleVoice"@eng ;
	rdfs:subClassOf gold:VoiceProperty ;
	rdfs:isDefinedBy "http://purl.org/linguistics/gold"^^<http://www.w3.org/2001/XMLSchema#anyURI> ;
	rdfs:comment "Referents of plural subject do action to one another. [Siewierska 1988, 257]"@eng .

gold:ReciprocalPronoun a owl:Class ;
	rdfs:label "ReciprocalPronoun"@eng ;
	rdfs:subClassOf gold:Pronominal ;
	rdfs:isDefinedBy "http://purl.org/linguistics/gold"^^<http://www.w3.org/2001/XMLSchema#anyURI> ;
	rdfs:comment "A reciprocal pronoun is a pronoun that expresses a mutual feeling or action among the referents of a plural subject [Crystal 1997,323]."@eng .

gold:ReferentialVoice a owl:Class ;
	rdfs:label "ReferentialVoice"@eng ;
	rdfs:subClassOf gold:VoiceProperty ;
	rdfs:isDefinedBy "http://purl.org/linguistics/gold"^^<http://www.w3.org/2001/XMLSchema#anyURI> .

gold:ReflexiveMiddleVoice a owl:Class ;
	rdfs:label "ReflexiveMiddleVoice"@eng ;
	rdfs:subClassOf gold:VoiceProperty ;
	rdfs:isDefinedBy "http://purl.org/linguistics/gold"^^<http://www.w3.org/2001/XMLSchema#anyURI> ;
	rdfs:comment "Subjects perform action to self. [Siewierska 1988,257]"@eng .

gold:ReflexivePassiveVoice a owl:Class ;
	rdfs:label "ReflexivePassiveVoice"@eng ;
	rdfs:subClassOf gold:VoiceProperty ;
	rdfs:isDefinedBy "http://purl.org/linguistics/gold"^^<http://www.w3.org/2001/XMLSchema#anyURI> ;
	rdfs:comment "A Passive construction which contains reflexive markings. [Siewierska 1988,257]"@eng .

gold:ReflexivePronoun a owl:Class ;
	rdfs:label "ReflexivePronoun"@eng ;
	rdfs:subClassOf gold:Pronominal ;
	rdfs:isDefinedBy "http://purl.org/linguistics/gold"^^<http://www.w3.org/2001/XMLSchema#anyURI> ;
	rdfs:comment "A reflexive pronoun is a pronoun that has coreference with the subject."@eng .

gold:RelativeFutureTense a owl:Class ;
	rdfs:label "RelativeFutureTense"@eng ;
	rdfs:subClassOf gold:TenseProperty ;
	rdfs:isDefinedBy "http://purl.org/linguistics/gold"^^<http://www.w3.org/2001/XMLSchema#anyURI> ;
	rdfs:comment "RelativeFutureTense locates the situation in question after a contextually determined temporal reference point, regardless of the latter's relation to the moment of utterance. Also called FuturePerfectTense [Comrie 1985, 69-71]."@eng .

gold:RelativePastTense a owl:Class ;
	rdfs:label "RelativePastTense"@eng ;
	rdfs:subClassOf gold:TenseProperty ;
	rdfs:isDefinedBy "http://purl.org/linguistics/gold"^^<http://www.w3.org/2001/XMLSchema#anyURI> ;
	rdfs:comment "RelativePastTense locates the situation in question before that of a contextually determined temporal reference point [Comrie 1985, 104]. Also called PastPerfectTense."@eng .

gold:RelativePresentTense a owl:Class ;
	rdfs:label "RelativePresentTense"@eng ;
	rdfs:subClassOf gold:TenseProperty ;
	rdfs:isDefinedBy "http://purl.org/linguistics/gold"^^<http://www.w3.org/2001/XMLSchema#anyURI> ;
	rdfs:comment "RelativePresentTense locates the situation in question simultaneously with some contextually determined temporal reference point."@eng .

gold:RelativePronoun a owl:Class ;
	rdfs:label "RelativePronoun"@eng ;
	rdfs:subClassOf gold:Pronominal ;
	rdfs:isDefinedBy "http://purl.org/linguistics/gold"^^<http://www.w3.org/2001/XMLSchema#anyURI> ;
	rdfs:comment "A relative pronoun is a pronoun that marks a relative clause, functions grammatically within the relative clause, and is coreferential to the word modified by the relative clause [Crystal 1997,329]."@eng .

gold:Relativizer a owl:Class ;
	rdfs:label "Relativizer"@eng ;
	rdfs:subClassOf gold:SubordinatingConnective ;
	rdfs:isDefinedBy "http://purl.org/linguistics/gold"^^<http://www.w3.org/2001/XMLSchema#anyURI> ;
	rdfs:comment "A relativizer is a subordinating connective that links a relative clause to its head  noun. It is distinguishable from a relative pronoun in that it does not have a nominal function within the relative clause [Payne1997, 332]."@eng .

gold:RemoteFutureTense a owl:Class ;
	rdfs:label "RemoteFutureTense"@eng ;
	rdfs:subClassOf gold:TenseProperty ;
	rdfs:isDefinedBy "http://purl.org/linguistics/gold"^^<http://www.w3.org/2001/XMLSchema#anyURI> ;
	rdfs:comment "RemoteFutureTense locates the situation in question at a time that is considered relatively distant. It is characteristically after the span of time culturally defined as 'tomorrow' [Dahl 1985,121; Comrie 1985,94]."@eng .

gold:RemotePastTense a owl:Class ;
	rdfs:label "RemotePastTense"@eng ;
	rdfs:subClassOf gold:TenseProperty ;
	rdfs:isDefinedBy "http://purl.org/linguistics/gold"^^<http://www.w3.org/2001/XMLSchema#anyURI> ;
	rdfs:comment "RemotePastTense locates the situation in question prior to the present moment, usually more than a few days ago [Dahl 1985,121; Comrie 1985,88]. Subsumes notion of PreHesternalPast tense, which locates the situation in question before that of an opposing hesternal past tense. [Bybee, Perkins, Pagliuca 1994, 98]."@eng .

gold:Repetitive a owl:Class ;
	rdfs:label "Repetitive"@eng ;
	rdfs:subClassOf gold:DerivationalUnit ;
	rdfs:isDefinedBy "http://purl.org/linguistics/gold"^^<http://www.w3.org/2001/XMLSchema#anyURI> ;
	rdfs:comment "A derivational unit that derives transitives from other transitive or intransitive stems adding the meaning of repitition to the resulting form."@eng .

gold:Retracted a owl:Class ;
	rdfs:label "Retracted"@eng ;
	rdfs:subClassOf gold:LabialProperty ;
	rdfs:isDefinedBy "http://purl.org/linguistics/gold"^^<http://www.w3.org/2001/XMLSchema#anyURI> ;
	rdfs:comment "Characterizing sounds involving compression without necessarily drawing the corners of the lips forward."@eng .

gold:RomanNumeralGender a owl:Class ;
	rdfs:label "RomanNumeralGender"@eng ;
	rdfs:subClassOf gold:GenderProperty ;
	rdfs:isDefinedBy "http://purl.org/linguistics/gold"^^<http://www.w3.org/2001/XMLSchema#anyURI> .

gold:Root a owl:Class ;
	rdfs:label "Root"@eng ;
	rdfs:subClassOf gold:MorphologicalUnit ;
	rdfs:isDefinedBy "http://purl.org/linguistics/gold"^^<http://www.w3.org/2001/XMLSchema#anyURI> ;
	rdfs:comment "Root is the class of morphologically simple units that are not further analyzable into meaningful elements, being morphologically simple. Roots  have a lexicalized meaning and designate the principle portion of meaning of the unit to which it belongs. They are the grammatical units to which derivational and inflectional material are added."@eng .

gold:SaliencePropety a owl:Class ;
	rdfs:label "SaliencePropety"@eng ;
	rdfs:subClassOf gold:DiscourseProperty ;
	rdfs:isDefinedBy "http://purl.org/linguistics/gold"^^<http://www.w3.org/2001/XMLSchema#anyURI> .

gold:SecondHandEvidentiality a owl:Class ;
	rdfs:label "SecondHandEvidentiality"@eng ;
	rdfs:subClassOf gold:EvidentialityProperty ;
	rdfs:isDefinedBy "http://purl.org/linguistics/gold"^^<http://www.w3.org/2001/XMLSchema#anyURI> ;
	rdfs:comment "SecondHandEvidentiality, also called the quotative, encodes the fact that the speaker came to believe the content of the expression from communicating with someone else [Palmer 2001, 40]."@eng .

gold:SecondLanguageOnlyVariety a owl:Class ;
	rdfs:label "SecondLanguageOnlyVariety"@eng ;
	rdfs:subClassOf gold:HumanLanguageVariety ;
	rdfs:isDefinedBy "http://purl.org/linguistics/gold"^^<http://www.w3.org/2001/XMLSchema#anyURI> ;
	rdfs:comment "A class of language varieties with no native speakers, i.e., only spoken by those that learned the variety after childhood."@eng .

gold:SecondPerson a owl:Class ;
	rdfs:label "SecondPerson"@eng ;
	rdfs:subClassOf gold:PersonProperty ;
	rdfs:isDefinedBy "http://purl.org/linguistics/gold"^^<http://www.w3.org/2001/XMLSchema#anyURI> ;
	rdfs:comment "SecondPerson is a person property that refers minimally to the addressee [Crystal 1997, 285; Cysouw 2003, 75]."@eng .

gold:SemanticAssignmentSystem a owl:Class ;
	rdfs:label "SemanticAssignmentSystem"@eng ;
	rdfs:subClassOf gold:FeatureAssignmentSystem ;
	rdfs:isDefinedBy "http://purl.org/linguistics/gold"^^<http://www.w3.org/2001/XMLSchema#anyURI> .

gold:SemanticInverseVoice a owl:Class ;
	rdfs:label "SemanticInverseVoice"@eng ;
	rdfs:subClassOf gold:VoiceProperty ;
	rdfs:isDefinedBy "http://purl.org/linguistics/gold"^^<http://www.w3.org/2001/XMLSchema#anyURI> ;
	rdfs:comment "If the agent outranks the patient on the relevant generic topic hierarchy, the direct-active clause is used.  If the relevant norm is reversed and the patient outranks the agent on the relevant hierarchy, the inverse clause is used. [Givon 1994,23]"@eng .

gold:SemanticProperty a owl:Class ;
	rdfs:label "SemanticProperty"@eng ;
	rdfs:subClassOf gold:LinguisticProperty ;
	rdfs:isDefinedBy "http://purl.org/linguistics/gold"^^<http://www.w3.org/2001/XMLSchema#anyURI> ;
	rdfs:comment "The class of linguistic properties that pertain to semantic units."@eng .

gold:SemelfactiveAspect a owl:Class ;
	rdfs:label "SemelfactiveAspect"@eng ;
	rdfs:subClassOf gold:AspectProperty ;
	rdfs:isDefinedBy "http://purl.org/linguistics/gold"^^<http://www.w3.org/2001/XMLSchema#anyURI> ;
	rdfs:comment "Momentaneous, without an inherent end-point, as sneeze [Michaelis 1998,xvi]."@eng .

gold:SeveralNumber a owl:Class ;
	rdfs:label "SeveralNumber"@eng ;
	rdfs:subClassOf gold:NumberProperty ;
	rdfs:isDefinedBy "http://purl.org/linguistics/gold"^^<http://www.w3.org/2001/XMLSchema#anyURI> ;
	rdfs:comment "Several is used in a system together with Singular and LargePlural or Multal to refer to a small, non-singular number of individuals."@eng .

gold:SignedLanguage a owl:Class ;
	rdfs:label "SignedLanguage"@eng ;
	rdfs:subClassOf gold:HumanLanguageVariety ;
	rdfs:isDefinedBy "http://purl.org/linguistics/gold"^^<http://www.w3.org/2001/XMLSchema#anyURI> ;
	rdfs:comment "SignedLanguage is the class of linguistic systems which instances are expressed using a system of (primarily manual) gestures."@eng .

gold:SignedLinguisticExpression a owl:Class ;
	rdfs:label "SignedLinguisticExpression"@eng ;
	rdfs:subClassOf gold:LinguisticExpression ;
	rdfs:isDefinedBy "http://purl.org/linguistics/gold"^^<http://www.w3.org/2001/XMLSchema#anyURI> ;
	rdfs:comment "A SignedLinguisticExpression is the signed physical form of language as distinct from either written or spoken expressions. Signed expressions are the primary means in which sign languages are tranmitted. A signed expression is  the image sequence that is produced (and perceived) during a signing event."@eng .

gold:SimpleFutureTense a owl:Class ;
	rdfs:label "SimpleFutureTense"@eng ;
	rdfs:subClassOf gold:TenseProperty ;
	rdfs:isDefinedBy "http://purl.org/linguistics/gold"^^<http://www.w3.org/2001/XMLSchema#anyURI> ;
	rdfs:comment "The posterior temporal relation may obtain either in 'simple' or 'perfect' contexts.  Modelling of this distinction originates from [Reichenbach  1947], who suggested using a third point in time, 'reference point', to capture all possible tense distinctions. In all 'simple' temporal relations, the reference point coincides with the location of the event spoken about."@eng .

gold:SimplePastTense a owl:Class ;
	rdfs:label "SimplePastTense"@eng ;
	rdfs:subClassOf gold:TenseProperty ;
	rdfs:isDefinedBy "http://purl.org/linguistics/gold"^^<http://www.w3.org/2001/XMLSchema#anyURI> ;
	rdfs:comment "The anterior temporal relation may obtain either in 'simple' or 'perfect' contexts. Modelling of this distinction originates from [Reichenbach  1947], who suggested using a third point in time, 'reference point', to capture all possible tense distinctions. In all 'simple' temporal relations, the reference point coincides with the location of the event spoken about."@eng .

gold:SimplePresentTense a owl:Class ;
	rdfs:label "SimplePresentTense"@eng ;
	rdfs:subClassOf gold:TenseProperty ;
	rdfs:isDefinedBy "http://purl.org/linguistics/gold"^^<http://www.w3.org/2001/XMLSchema#anyURI> ;
	rdfs:comment "The simultaneous temporal relation may obtain either in 'simple' or 'perfect' contexts.  Modelling of this distinction originates from [Reichenbach  1947], who suggested using a third point in time, 'reference point', to capture all possible tense distinctions. In all 'simple' temporal relations, the reference point coincides with the location of the event spoken about."@eng .

gold:SimpleSpecification a owl:Class ;
	rdfs:label "SimpleSpecification"@eng ;
	rdfs:subClassOf gold:FeatureSpecification ;
	rdfs:isDefinedBy "http://purl.org/linguistics/gold"^^<http://www.w3.org/2001/XMLSchema#anyURI> ;
	rdfs:comment "A SimpleSpecification is a kind of FeatureSpecification whose value must be a simple linguistic attribute [Maxwell, Simons, and Hayashi 2000]."@eng .

gold:SimultaneousAspect a owl:Class ;
	rdfs:label "SimultaneousAspect"@eng ;
	rdfs:subClassOf gold:AspectProperty ;
	rdfs:isDefinedBy "http://purl.org/linguistics/gold"^^<http://www.w3.org/2001/XMLSchema#anyURI> ;
	rdfs:comment "SimultaneousAspect"@eng .

gold:SingularNumber a owl:Class ;
	rdfs:label "SingularNumber"@eng ;
	rdfs:subClassOf gold:NumberProperty ;
	rdfs:isDefinedBy "http://purl.org/linguistics/gold"^^<http://www.w3.org/2001/XMLSchema#anyURI> .

gold:SmallPaucalNumber a owl:Class ;
	rdfs:label "SmallPaucalNumber"@eng ;
	rdfs:subClassOf gold:NumberProperty ;
	rdfs:isDefinedBy "http://purl.org/linguistics/gold"^^<http://www.w3.org/2001/XMLSchema#anyURI> ;
	rdfs:comment "SmallPaucal is a number property that occurs in a number system together with LargePlural, referring to a very small number of individuals. It core:entails Paucal and is entailed by both Singular and Dual."@eng .

gold:SpeculativeForce a owl:Class ;
	rdfs:label "SpeculativeForce"@eng ;
	rdfs:subClassOf gold:ForceProperty ;
	rdfs:isDefinedBy "http://purl.org/linguistics/gold"^^<http://www.w3.org/2001/XMLSchema#anyURI> ;
	rdfs:comment "SpeculativeForce indicates that the speaker considers, or 'entertains', the content of the expression. That is, it is in the realm of possibility, though the speaker does not necessarilty believe it [Palmer 2001, 6-8, 25]."@eng .

gold:SpokenLanguage a owl:Class ;
	rdfs:label "SpokenLanguage"@eng ;
	rdfs:subClassOf gold:HumanLanguageVariety ;
	rdfs:isDefinedBy "http://purl.org/linguistics/gold"^^<http://www.w3.org/2001/XMLSchema#anyURI> ;
	rdfs:comment "SpokenLanguage is the class of linguistic systems whose instances are expressed in speech. For every spoken language, there exists a phonological system in which the language is expressed."@eng .

gold:SpokenLinguisticExpression a owl:Class ;
	rdfs:label "SpokenLinguisticExpression"@eng ;
	rdfs:subClassOf gold:LinguisticExpression ;
	rdfs:isDefinedBy "http://purl.org/linguistics/gold"^^<http://www.w3.org/2001/XMLSchema#anyURI> ;
	rdfs:comment "A SpokenLinguisticExpression is the physical sound form of language as distinct from either signed or spoken expressions. A spoken expression is the sound that is produced (and perceived) during a speaking event."@eng .

gold:Stem a owl:Class ;
	rdfs:label "Stem"@eng ;
	rdfs:subClassOf gold:MorphologicalUnit ;
	rdfs:isDefinedBy "http://purl.org/linguistics/gold"^^<http://www.w3.org/2001/XMLSchema#anyURI> ;
	rdfs:comment "Stem is the class of  morphological units that are analyzable into a root and possibly one or more derivational units. Stems can occur alone and are the basis for adding inflectional units."@eng .

gold:StillTense a owl:Class ;
	rdfs:label "StillTense"@eng ;
	rdfs:subClassOf gold:TenseProperty ;
	rdfs:isDefinedBy "http://purl.org/linguistics/gold"^^<http://www.w3.org/2001/XMLSchema#anyURI> ;
	rdfs:comment "StillPresentTense is similar to PresentTense but carries the presupposition that an event or state held before the moment of utterance. In positive declarative clauses, still present tense asserts that the event or state holds at the moment of utterance [Comrie 1985, 54]."@eng .

gold:Stop a owl:Class ;
	rdfs:label "Stop"@eng ;
	rdfs:subClassOf gold:StrictureProperty ;
	rdfs:isDefinedBy "http://purl.org/linguistics/gold"^^<http://www.w3.org/2001/XMLSchema#anyURI> ;
	rdfs:comment "The property of sounds produced by stopping the airflow in the vocal tract."@eng .

gold:StructuralDescription a owl:Class ;
	rdfs:label "StructuralDescription"@eng ;
	rdfs:subClassOf gold:LinguisticDataStructure ;
	rdfs:isDefinedBy "http://purl.org/linguistics/gold"^^<http://www.w3.org/2001/XMLSchema#anyURI> ;
	rdfs:comment "This is a data structure commonly associated with morphosyntactic analysis. It is usually represented graphically as a tree."@eng .

gold:SubablativeCase a owl:Class ;
	rdfs:label "SubablativeCase"@eng ;
	rdfs:subClassOf gold:CaseProperty ;
	rdfs:isDefinedBy "http://purl.org/linguistics/gold"^^<http://www.w3.org/2001/XMLSchema#anyURI> ;
	rdfs:comment "SubablativeCase expresses that  the referent of the noun it marks is the location from under which another referent is moving. It has the meaning 'from under'."@eng .

gold:SuballativeCase a owl:Class ;
	rdfs:label "SuballativeCase"@eng ;
	rdfs:subClassOf gold:CaseProperty ;
	rdfs:isDefinedBy "http://purl.org/linguistics/gold"^^<http://www.w3.org/2001/XMLSchema#anyURI> ;
	rdfs:comment "SuballativeCase expresses that  something is moving toward the region that is under the referent of the noun it marks. It has the meaning 'towards the region that is under'."@eng .

gold:SubessiveCase a owl:Class ;
	rdfs:label "SubessiveCase"@eng ;
	rdfs:subClassOf gold:CaseProperty ;
	rdfs:isDefinedBy "http://purl.org/linguistics/gold"^^<http://www.w3.org/2001/XMLSchema#anyURI> ;
	rdfs:comment "SubessiveCase expresses that  the referent of the noun it marks is the location under which another referent exists. It has the meaning of 'under' or 'beneath'."@eng .

gold:SubjunctiveMood a owl:Class ;
	rdfs:label "SubjunctiveMood"@eng ;
	rdfs:subClassOf gold:MoodProperty ;
	rdfs:isDefinedBy "http://purl.org/linguistics/gold"^^<http://www.w3.org/2001/XMLSchema#anyURI> ;
	rdfs:comment "SubjunctiveMood indicates that the expression is  not believed to be true."@eng .

gold:Sublaminal a owl:Class ;
	rdfs:label "Sublaminal"@eng ;
	rdfs:subClassOf gold:ApicalityProperty ;
	rdfs:isDefinedBy "http://purl.org/linguistics/gold"^^<http://www.w3.org/2001/XMLSchema#anyURI> ;
	rdfs:comment "Characterizing sounds produced by the underside of the tip of the tongue  [Ladefoged 1997, 596]."@eng .

gold:SublativeCase a owl:Class ;
	rdfs:label "SublativeCase"@eng ;
	rdfs:subClassOf gold:CaseProperty ;
	rdfs:isDefinedBy "http://purl.org/linguistics/gold"^^<http://www.w3.org/2001/XMLSchema#anyURI> ;
	rdfs:comment "SublativeCase expresses that  the referent of the noun it marks is the location under which another referent is moving toward. It has the meaning 'towards the underneath of'."@eng .

gold:Substantive a owl:Class ;
	rdfs:label "Substantive"@eng ;
	rdfs:subClassOf gold:PartOfSpeechProperty ;
	rdfs:isDefinedBy "http://purl.org/linguistics/gold"^^<http://www.w3.org/2001/XMLSchema#anyURI> ;
	rdfs:comment "A substantive is a member of the syntactic class in which the names of physical, concrete, relatively unchanging experiences are most typically found whose members may act as subjects and  objects, and most of whose members have inherently determined grammatical  gender (in languages which inflect for gender) [Crystal 1997,264; Givon 1984,51-52; Payne 1997,33]."@eng .

gold:SubterminativeCase a owl:Class ;
	rdfs:label "SubterminativeCase"@eng ;
	rdfs:subClassOf gold:CaseProperty ;
	rdfs:isDefinedBy "http://purl.org/linguistics/gold"^^<http://www.w3.org/2001/XMLSchema#anyURI> ;
	rdfs:comment "SubterminativeCase expresses the notion of something moving into the region under the referent of the noun it marks, but not through that region. It has the meaning 'into the region under'."@eng .

gold:SubtranslativeCase a owl:Class ;
	rdfs:label "SubtranslativeCase"@eng ;
	rdfs:subClassOf gold:CaseProperty ;
	rdfs:isDefinedBy "http://purl.org/linguistics/gold"^^<http://www.w3.org/2001/XMLSchema#anyURI> ;
	rdfs:comment "SubtranslativeCase expresses the notion of something moving along a trajectory underneath the referent of the noun it marks. It has the meaning 'along the region underneath'. Unfortunate name clash with 'Superlative' as a feature of adjectives."@eng .

gold:Suffix a owl:Class ;
	rdfs:label "Suffix"@eng ;
	rdfs:subClassOf gold:Affix ;
	rdfs:isDefinedBy "http://purl.org/linguistics/gold"^^<http://www.w3.org/2001/XMLSchema#anyURI> .

gold:SuperablativeCase a owl:Class ;
	rdfs:label "SuperablativeCase"@eng ;
	rdfs:subClassOf gold:CaseProperty ;
	rdfs:isDefinedBy "http://purl.org/linguistics/gold"^^<http://www.w3.org/2001/XMLSchema#anyURI> ;
	rdfs:comment "Superablative expresses that  the referent of the noun it marks is the location from over which another referent is moving. It has the meaning 'from over'."@eng .

gold:SuperallativeCase a owl:Class ;
	rdfs:label "SuperallativeCase"@eng ;
	rdfs:subClassOf gold:CaseProperty ;
	rdfs:isDefinedBy "http://purl.org/linguistics/gold"^^<http://www.w3.org/2001/XMLSchema#anyURI> ;
	rdfs:comment "SuperallativeCase expresses that  something is moving toward the region that is above the referent of the noun it marks. It has the meaning 'towards the region that is over'."@eng .

gold:SuperessiveCase a owl:Class ;
	rdfs:label "SuperessiveCase"@eng ;
	rdfs:subClassOf gold:CaseProperty ;
	rdfs:isDefinedBy "http://purl.org/linguistics/gold"^^<http://www.w3.org/2001/XMLSchema#anyURI> ;
	rdfs:comment "SuperessiveCase expresses that  the referent of the noun it marks is the location on which another referent exists. It has the meaning of 'on' or 'upon'. [Pei and Gaynor 1954, 207]."@eng .

gold:SuperlativeAdjective a owl:Class ;
	rdfs:label "SuperlativeAdjective"@eng ;
	rdfs:subClassOf gold:Adjectival ;
	rdfs:isDefinedBy "http://purl.org/linguistics/gold"^^<http://www.w3.org/2001/XMLSchema#anyURI> ;
	rdfs:comment "suggested at E-MELD  (no documentation yet)"@eng .

gold:SuperlativeCase a owl:Class ;
	rdfs:label "SuperlativeCase"@eng ;
	rdfs:subClassOf gold:CaseProperty ;
	rdfs:isDefinedBy "http://purl.org/linguistics/gold"^^<http://www.w3.org/2001/XMLSchema#anyURI> ;
	rdfs:comment "SuperlativeCase expresses that  the referent of the noun it marks is the location onto which another referent is moving. It has the meaning of 'onto'. Unfortunate name clash with 'Superlative' as a property of adjectives."@eng .

gold:SuperterminativeCase a owl:Class ;
	rdfs:label "SuperterminativeCase"@eng ;
	rdfs:subClassOf gold:CaseProperty ;
	rdfs:isDefinedBy "http://purl.org/linguistics/gold"^^<http://www.w3.org/2001/XMLSchema#anyURI> ;
	rdfs:comment "SuperterminativeCase expresses the notion of something moving into the region over the referent of the noun it marks, but not through that region. It has the meaning 'into the region over'."@eng .

gold:SupertranslativeCase a owl:Class ;
	rdfs:label "SupertranslativeCase"@eng ;
	rdfs:subClassOf gold:CaseProperty ;
	rdfs:isDefinedBy "http://purl.org/linguistics/gold"^^<http://www.w3.org/2001/XMLSchema#anyURI> ;
	rdfs:comment "SupertranslativeCase expresses the notion of something moving along a trajectory above the referent of the noun it marks. It has the meaning 'along the region over'."@eng .

gold:Suprasegmental a owl:Class ;
	rdfs:label "Suprasegmental"@eng ;
	rdfs:subClassOf gold:FormUnit ;
	rdfs:isDefinedBy "http://purl.org/linguistics/gold"^^<http://www.w3.org/2001/XMLSchema#anyURI> .

gold:Syllable a owl:Class ;
	rdfs:label "Syllable"@eng ;
	rdfs:subClassOf gold:FormUnit ;
	rdfs:isDefinedBy "http://purl.org/linguistics/gold"^^<http://www.w3.org/2001/XMLSchema#anyURI> .

gold:SyntacticArgument a owl:Class ;
	rdfs:label "SyntacticArgument"@eng ;
	rdfs:subClassOf gold:PartOfSpeechProperty ;
	rdfs:isDefinedBy "http://purl.org/linguistics/gold"^^<http://www.w3.org/2001/XMLSchema#anyURI> ;
	rdfs:comment "SyntacticArgument is the class of syntactic words that are fundamentally referable and  non-relational [Anderson 1997, 15]. Proper names are the quintessential arguments, though pronouns and nouns possess  argument properties."@eng .

gold:SyntacticWord a owl:Class ;
	rdfs:label "SyntacticWord"@eng ;
	rdfs:subClassOf gold:SyntacticUnit ;
	rdfs:isDefinedBy "http://purl.org/linguistics/gold"^^<http://www.w3.org/2001/XMLSchema#anyURI> ;
	rdfs:comment "SyntacticWord is the class of syntactic units occupying the lowest position in a syntactic construction.  They are the largest units resistant to insertion of new constituents within their boundaries; or they are the smallest constituents that can be moved within a sentence without making the sentence ungrammatical."@eng .

gold:Tap a owl:Class ;
	rdfs:label "Tap"@eng ;
	rdfs:subClassOf gold:TrillProperty ;
	rdfs:isDefinedBy "http://purl.org/linguistics/gold"^^<http://www.w3.org/2001/XMLSchema#anyURI> ;
	rdfs:comment "Also known as a flap, the property of sounds produced when one articulator is forced against another."@eng .

gold:Term a owl:Class ;
	rdfs:label "Term"@eng ;
	rdfs:subClassOf gold:LinguisticDataStructure ;
	rdfs:isDefinedBy "http://purl.org/linguistics/gold"^^<http://www.w3.org/2001/XMLSchema#anyURI> ;
	rdfs:comment "A specific string representing an entity within some scientific domain."@eng .

gold:TerminativeAspect a owl:Class ;
	rdfs:label "TerminativeAspect"@eng ;
	rdfs:subClassOf gold:AspectProperty ;
	rdfs:isDefinedBy "http://purl.org/linguistics/gold"^^<http://www.w3.org/2001/XMLSchema#anyURI> ;
	rdfs:comment "Denotes the termination of an event [Bhat 1999, 92]."@eng .

gold:TerminativeCase a owl:Class ;
	rdfs:label "TerminativeCase"@eng ;
	rdfs:subClassOf gold:CaseProperty ;
	rdfs:isDefinedBy "http://purl.org/linguistics/gold"^^<http://www.w3.org/2001/XMLSchema#anyURI> ;
	rdfs:comment "[Need comment]"@eng .

gold:Termset a owl:Class ;
	rdfs:label "Termset"@eng ;
	rdfs:subClassOf gold:LinguisticDataStructure ;
	rdfs:isDefinedBy "http://purl.org/linguistics/gold"^^<http://www.w3.org/2001/XMLSchema#anyURI> ;
	rdfs:comment "A set of scientific terms used as part of an annotation system, usually the standard terms from a particular linguistic theory."@eng .

gold:ThirdPerson a owl:Class ;
	rdfs:label "ThirdPerson"@eng ;
	rdfs:subClassOf gold:PersonProperty ;
	rdfs:isDefinedBy "http://purl.org/linguistics/gold"^^<http://www.w3.org/2001/XMLSchema#anyURI> ;
	rdfs:comment "Third Person is a person property that refers to the non-participant (other than the speaker and the addressee) [Crystal 1997, 285]."@eng .

gold:ThirdPersonObviative a owl:Class ;
	rdfs:label "ThirdPersonObviative"@eng ;
	rdfs:subClassOf gold:PersonProperty ;
	rdfs:isDefinedBy "http://purl.org/linguistics/gold"^^<http://www.w3.org/2001/XMLSchema#anyURI> ;
	rdfs:comment "ThirdPersonObviative is a person property that  refers to one or more non-participants that are in some way further removed from the speaker than other non-particpants. Contrasts with thirdPersonProximative."@eng .

gold:ThirdPersonProximative a owl:Class ;
	rdfs:label "ThirdPersonProximative"@eng ;
	rdfs:subClassOf gold:PersonProperty ;
	rdfs:isDefinedBy "http://purl.org/linguistics/gold"^^<http://www.w3.org/2001/XMLSchema#anyURI> .

gold:TimitiveMood a owl:Class ;
	rdfs:label "TimitiveMood"@eng ;
	rdfs:subClassOf gold:MoodProperty ;
	rdfs:isDefinedBy "http://purl.org/linguistics/gold"^^<http://www.w3.org/2001/XMLSchema#anyURI> ;
	rdfs:comment "TimitiveMood encodes that the speaker fears something expressed in what is said [Palmer 2001, 13, 22]."@eng .

gold:Toneme a owl:Class ;
	rdfs:label "Toneme"@eng ;
	rdfs:subClassOf gold:FormUnit ;
	rdfs:isDefinedBy "http://purl.org/linguistics/gold"^^<http://www.w3.org/2001/XMLSchema#anyURI> ;
	rdfs:comment "[No definition yet.]"@eng .

gold:TransitiveVerb a owl:Class ;
	rdfs:label "TransitiveVerb"@eng ;
	rdfs:subClassOf gold:BinaryPredicator ;
	rdfs:isDefinedBy "http://purl.org/linguistics/gold"^^<http://www.w3.org/2001/XMLSchema#anyURI> ;
	rdfs:comment "A transitive verb is a verb that takes a direct object, and describes a relation between two participants [Crystal 1997,397; Payne 1997,171]."@eng .

gold:Transitivizer a owl:Class ;
	rdfs:label "Transitivizer"@eng ;
	rdfs:subClassOf gold:DerivationalUnit ;
	rdfs:isDefinedBy "http://purl.org/linguistics/gold"^^<http://www.w3.org/2001/XMLSchema#anyURI> ;
	rdfs:comment "A derivational unit that derives transitive verbs from intransitive verb (stems)."@eng .

gold:TranslativeCase a owl:Class ;
	rdfs:label "TranslativeCase"@eng ;
	rdfs:subClassOf gold:CaseProperty ;
	rdfs:isDefinedBy "http://purl.org/linguistics/gold"^^<http://www.w3.org/2001/XMLSchema#anyURI> ;
	rdfs:comment "TranslativeCase expresses that the referent of the noun, or the quality of the adjective, that it marks is the result of a process of change [Lyons 1968, 299-301; Sebeok 1946, 17; Hakulinen 1961, 70]. X along, across Y."@eng .

gold:TrialNumber a owl:Class ;
	rdfs:label "TrialNumber"@eng ;
	rdfs:subClassOf gold:NumberProperty ;
	rdfs:isDefinedBy "http://purl.org/linguistics/gold"^^<http://www.w3.org/2001/XMLSchema#anyURI> ;
	rdfs:comment "Trial is a number property that quantifies the denotation of the nominal element so that it specifies that there are exactly three. In this example from Larike (alo), trialNumber is expressed on the pronoun: Ln Duma hima aridu naʔa Ln house that 1.TRIAL.EXCL own.it Ln 'We three own that house' Ln [Corbett 2000, 21]"@eng .

gold:Trill a owl:Class ;
	rdfs:label "Trill"@eng ;
	rdfs:subClassOf gold:TrillProperty ;
	rdfs:isDefinedBy "http://purl.org/linguistics/gold"^^<http://www.w3.org/2001/XMLSchema#anyURI> ;
	rdfs:comment "The property associated with sounds caused from vibrations of the active and passive articulators as a result of air being forced between them."@eng .

gold:Unaspirated a owl:Class ;
	rdfs:label "Unaspirated"@eng ;
	rdfs:subClassOf gold:GlottalTimingProperty ;
	rdfs:isDefinedBy "http://purl.org/linguistics/gold"^^<http://www.w3.org/2001/XMLSchema#anyURI> ;
	rdfs:comment "[Need comment]"@eng .

gold:UnattestedVariety a owl:Class ;
	rdfs:label "UnattestedVariety"@eng ;
	rdfs:subClassOf gold:HumanLanguageVariety ;
	rdfs:isDefinedBy "http://purl.org/linguistics/gold"^^<http://www.w3.org/2001/XMLSchema#anyURI> ;
	rdfs:comment "UnattestedVariety is the class of language varieties that are posited to exist or to have existed. Examples include reconstructed languages, such as Proto-Indo-European."@eng .

gold:VegetableGender a owl:Class ;
	rdfs:label "VegetableGender"@eng ;
	rdfs:subClassOf gold:GenderProperty ;
	rdfs:isDefinedBy "http://purl.org/linguistics/gold"^^<http://www.w3.org/2001/XMLSchema#anyURI> ;
	rdfs:comment "Vegetable gender refers to inanimates and exists in some four-way gender systems, e.g., masculine, feminine, neuter, and vegetable as in Bininj Gun-wok [Evans 2003, 202]."@eng .

gold:VerbPhrase a owl:Class ;
	rdfs:label "VerbPhrase"@eng ;
	rdfs:subClassOf gold:Phrase ;
	rdfs:isDefinedBy "http://purl.org/linguistics/gold"^^<http://www.w3.org/2001/XMLSchema#anyURI> ;
	rdfs:comment "VerbPhrase is the class of phrases that have verbs as heads. They can play the role of predicate in a main clause."@eng .

gold:VerbalAdjective a owl:Class ;
	rdfs:label "VerbalAdjective"@eng ;
	rdfs:subClassOf gold:Adjectival ;
	rdfs:isDefinedBy "http://purl.org/linguistics/gold"^^<http://www.w3.org/2001/XMLSchema#anyURI> ;
	rdfs:comment "suggested at E-MELD  (no documentation yet)"@eng .

gold:VerbalParticle a owl:Class ;
	rdfs:label "VerbalParticle"@eng ;
	rdfs:subClassOf gold:Particle ;
	rdfs:isDefinedBy "http://purl.org/linguistics/gold"^^<http://www.w3.org/2001/XMLSchema#anyURI> ;
	rdfs:comment "A verbal particle is a member of a closed class of particles which co-occur with some verbs to form phrasal verbs. In some languages, verbal particles are identical to certain adpositions."@eng .

gold:Verbalizer a owl:Class ;
	rdfs:label "Verbalizer"@eng ;
	rdfs:subClassOf gold:CategoryChanger ;
	rdfs:isDefinedBy "http://purl.org/linguistics/gold"^^<http://www.w3.org/2001/XMLSchema#anyURI> ;
	rdfs:comment "Verbalizer is the class of category changing units that change nouns into verbs."@eng .

gold:Versive a owl:Class ;
	rdfs:label "Versive"@eng ;
	rdfs:subClassOf gold:CategoryChanger ;
	rdfs:isDefinedBy "http://purl.org/linguistics/gold"^^<http://www.w3.org/2001/XMLSchema#anyURI> ;
	rdfs:comment "A derivational unit that derives intransitive stems from adjectives, with the meaning of becoming or taking on the quality of the adjective."@eng .

gold:VisualEvidentiality a owl:Class ;
	rdfs:label "VisualEvidentiality"@eng ;
	rdfs:subClassOf gold:EvidentialityProperty ;
	rdfs:isDefinedBy "http://purl.org/linguistics/gold"^^<http://www.w3.org/2001/XMLSchema#anyURI> ;
	rdfs:comment "VisualEvidentiality encodes the fact that the speaker came to believe the content of the expression through direct visual experience; they saw it [Palmer 2001, 57]."@eng .

gold:VocativeCase a owl:Class ;
	rdfs:label "VocativeCase"@eng ;
	rdfs:subClassOf gold:CaseProperty ;
	rdfs:isDefinedBy "http://purl.org/linguistics/gold"^^<http://www.w3.org/2001/XMLSchema#anyURI> ;
	rdfs:comment "VocativeCase marks a noun whose referent is being addressed [Crystal 1980, 377; Hartmann and Stork 1972, 251; Pei and Gaynor 1954, 228]."@eng .

gold:Voiced a owl:Class ;
	rdfs:label "Voiced"@eng ;
	rdfs:subClassOf gold:VoicingProperty ;
	rdfs:isDefinedBy "http://purl.org/linguistics/gold"^^<http://www.w3.org/2001/XMLSchema#anyURI> .

gold:Voiceless a owl:Class ;
	rdfs:label "Voiceless"@eng ;
	rdfs:subClassOf gold:VoicingProperty ;
	rdfs:isDefinedBy "http://purl.org/linguistics/gold"^^<http://www.w3.org/2001/XMLSchema#anyURI> .

gold:VolitiveForce a owl:Class ;
	rdfs:label "VolitiveForce"@eng ;
	rdfs:subClassOf gold:ForceProperty ;
	rdfs:isDefinedBy "http://purl.org/linguistics/gold"^^<http://www.w3.org/2001/XMLSchema#anyURI> ;
	rdfs:comment "VolitiveForce indicates that the speaker is willing to perform some action [Palmer 2001, 76]."@eng .

gold:Vowel a owl:Class ;
	rdfs:label "Vowel"@eng ;
	rdfs:subClassOf gold:Segment ;
	rdfs:isDefinedBy "http://purl.org/linguistics/gold"^^<http://www.w3.org/2001/XMLSchema#anyURI> .

gold:WeakObligativeModality a owl:Class ;
	rdfs:label "WeakObligativeModality"@eng ;
	rdfs:subClassOf gold:ModalityProperty ;
	rdfs:isDefinedBy "http://purl.org/linguistics/gold"^^<http://www.w3.org/2001/XMLSchema#anyURI> ;
	rdfs:comment "WeakObligativeModality indicates that an agent is under a moral obligation to perform the action expressed by the predicate [Bybee, Perkins, and Pagliuca 1994, 186-187]."@eng .

gold:WrittenLanguage a owl:Class ;
	rdfs:label "WrittenLanguage"@eng ;
	rdfs:subClassOf gold:HumanLanguageVariety ;
	rdfs:isDefinedBy "http://purl.org/linguistics/gold"^^<http://www.w3.org/2001/XMLSchema#anyURI> ;
	rdfs:comment "WrittenLanguage is the class of linguistic systems whose instance are expressed using a written, time-stable form. For every written language, there exists an orthographic system in which the language is expressed."@eng .

gold:ZeroPlacePredicator a owl:Class ;
	rdfs:label "ZeroPlacePredicator"@eng ;
	rdfs:subClassOf gold:Predicator ;
	rdfs:isDefinedBy "http://purl.org/linguistics/gold"^^<http://www.w3.org/2001/XMLSchema#anyURI> ;
	rdfs:comment "ZeroPlacePredicator is the class of syntactic words that need not take any arguments, but act as predicators nevertheless."@eng .

_:node172f9vp6jx2 a owl:Ontology ;
	dc:identifier "http://purl.org/linguistics/gold" ;
	owl:versionInfo "2008" ;
	dc:title "Genderal Ontology for Linguistic Description" ;
	dc:description "This is the General Ontology for Linguistic Description (GOLD) described using the Web Ontology Language. This ontology was created primarily for applications involving descriptive linguistics." , "" ;
	dc:creator "Scott Farrar" , "D. Terence Langendoen" ;
	dc:contributor "Anthony Aristar" , "Helen Aristar-Dry" , "Dunstan Brown" , "Greville Corbett" , "Anna Kibort" , "William D. Lewis" , "Steven Moran" , "Gary Simons" .
