@prefix dc: <http://purl.org/dc/elements/1.1/> .
@prefix voaf: <http://purl.org/vocommons/voaf#> .
@prefix rdfs: <http://www.w3.org/2000/01/rdf-schema#> .
@prefix dct: <http://purl.org/dc/terms/> .
@prefix xsd: <http://www.w3.org/2001/XMLSchema#> .
@prefix owl: <http://www.w3.org/2002/07/owl#> .
@prefix vann: <http://purl.org/vocab/vann/> .
@prefix rdf: <http://www.w3.org/1999/02/22-rdf-syntax-ns#> .
@prefix h2o: <http://def.seegrid.csiro.au/isotc211/iso19150/-2/2012/basic#> .
@prefix skos: <http://www.w3.org/2004/02/skos/core#> .
@prefix prov-dc: <http://www.w3.org/ns/prov-dc#> .

<http://def.seegrid.csiro.au/isotc211/iso19150/-2/2012/basic> a voaf:Vocabulary , owl:Ontology ;
	dc:contributor "ISO/TC 211 Project Team 19150-2"^^xsd:string ;
	dc:creator """Simon J D COX
CSIRO Australia"""^^xsd:string ;
	dc:description "This ontology establishes classes corresponding to stereotypes used in ISO-conformant models, as used in the rules for conversion of the ISO TC 211 Harmonized Model from the UML to OWL representations"^^xsd:string ;
	dc:rights "Copyright Â© 2012-2013 CSIRO"^^xsd:string ;
	dc:title "Ontology elements required for conversion of ISO/TC 211 Harmonized Model to OWL"^^xsd:string ;
	dct:created "2012-06-04T00:00:00"^^xsd:dateTime ;
	dct:hasPart h2o:ISOClassName , h2o:TaggedValue , h2o:constraint , h2o:isAbstract , h2o:isStereotype , h2o:tag , h2o:ttag , h2o:tvalue ;
	dct:license <http://creativecommons.org/licenses/by/3.0/> ;
	dct:modified "2014-01-07T00:00:00"^^xsd:dateTime ;
	vann:preferredNamespacePrefix "h2o"^^xsd:string ;
	vann:preferredNamespaceUri <http://def.seegrid.csiro.au/isotc211/iso19150/-2/2012/basic#> ;
	rdfs:comment """This ontology establishes classes corresponding to stereotypes used in ISO-conformant models, as used in the rules for conversion of the ISO TC 211 Harmonized Model from the UML to OWL representations. 

This vocabulary is provisional, pending finalization of ISO 19150-2.

The URI stem http://def.seegrid.csiro.au/isotc211/ is temporary. The vocabulary is expected to be ultimately published in the domain http://def.isotc211.org/ ."""^^xsd:string ;
	owl:imports <http://purl.org/dc/elements/1.1/> ;
	owl:priorVersion <https://www.seegrid.csiro.au/subversion/xmml/ontologies/tags/201305/ISOTC211/HM/hm2owl.rdf> ;
	owl:versionIRI <https://www.seegrid.csiro.au/subversion/xmml/ontologies/tags/201311/ISOTC211/HM/iso19150/-2/2012/basic.rdf> .

h2o:ISOClassName a rdfs:Datatype ;
	rdfs:comment "A datatype for skos:notation annotations, used to indicate the original UML class name"^^xsd:string ;
	rdfs:isDefinedBy <http://def.seegrid.csiro.au/isotc211/iso19150/-2/2012/basic> ;
	rdfs:label "ISO Class name"^^xsd:string .

_:node18qof2jatx1 a rdfs:Datatype ;
	owl:onDataType xsd:string .

_:node18qof2jatx2 xsd:pattern "^[A-Z]\\w*"^^xsd:string .

_:node18qof2jatx3 rdf:first _:node18qof2jatx2 ;
	rdf:rest rdf:nil .

_:node18qof2jatx1 owl:withRestrictions _:node18qof2jatx3 .

h2o:ISOClassName owl:equivalentClass _:node18qof2jatx1 .

h2o:TaggedValue a owl:Class ;
	rdfs:comment "Class for UML tagged values"^^xsd:string ;
	rdfs:isDefinedBy <http://def.seegrid.csiro.au/isotc211/iso19150/-2/2012/basic> ;
	rdfs:label "UML tagged value structure"^^xsd:string .

_:node18qof2jatx4 a owl:Restriction ;
	owl:cardinality "1"^^xsd:nonNegativeInteger ;
	owl:onProperty h2o:ttag .

h2o:TaggedValue rdfs:subClassOf _:node18qof2jatx4 .

_:node18qof2jatx5 a owl:Restriction ;
	owl:cardinality "1"^^xsd:nonNegativeInteger ;
	owl:onProperty h2o:tvalue .

h2o:TaggedValue rdfs:subClassOf _:node18qof2jatx5 .

h2o:constraint a owl:AnnotationProperty ;
	rdfs:isDefinedBy <http://def.seegrid.csiro.au/isotc211/iso19150/-2/2012/basic> ;
	rdfs:label "UML constraint"^^xsd:string ;
	rdfs:range xsd:string .

h2o:isAbstract a owl:AnnotationProperty ;
	rdfs:comment "This property indicates whether the class was flagged 'abstract' in the UML model. Abstract classes cannot be instantiated directly. Concrete subclasses may be instantiated."^^xsd:string ;
	rdfs:isDefinedBy <http://def.seegrid.csiro.au/isotc211/iso19150/-2/2012/basic> ;
	rdfs:label "UML abstract class"^^xsd:string ;
	rdfs:range xsd:boolean .

h2o:isStereotype a owl:AnnotationProperty ;
	rdfs:comment "This property indicates if the class corresponds to a UML stereotype"^^xsd:string ;
	rdfs:isDefinedBy <http://def.seegrid.csiro.au/isotc211/iso19150/-2/2012/basic> ;
	rdfs:label "ISO stereotype flag"^^xsd:string ;
	rdfs:range xsd:boolean .

h2o:tag a owl:AnnotationProperty ;
	rdfs:comment "OWL property that links to a tagged value"^^xsd:string ;
	rdfs:isDefinedBy <http://def.seegrid.csiro.au/isotc211/iso19150/-2/2012/basic> ;
	rdfs:label "UML tagged value"^^xsd:string ;
	rdfs:range h2o:TaggedValue .

h2o:ttag a owl:DatatypeProperty ;
	rdfs:domain h2o:TaggedValue ;
	rdfs:isDefinedBy <http://def.seegrid.csiro.au/isotc211/iso19150/-2/2012/basic> ;
	rdfs:label "UML tagged value tag"^^xsd:string ;
	rdfs:range xsd:string .

h2o:tvalue a owl:DatatypeProperty ;
	rdfs:domain h2o:TaggedValue ;
	rdfs:isDefinedBy <http://def.seegrid.csiro.au/isotc211/iso19150/-2/2012/basic> ;
	rdfs:label "UML tagged value value"^^xsd:string ;
	rdfs:range xsd:string .

h2o:valueAssignment a owl:ObjectProperty ;
	rdfs:comment "property that can be attached to any statement to support a link to the evidence for the value"^^xsd:string ;
	rdfs:domain rdf:Statement ;
	rdfs:label "value assignment method"^^xsd:string .

_:node18qof2jatx6 a rdfs:Datatype ;
	owl:onDataType xsd:string .

_:node18qof2jatx7 xsd:pattern "^[A-Z]\\w*"^^xsd:string .

_:node18qof2jatx8 rdf:first _:node18qof2jatx7 ;
	rdf:rest rdf:nil .

_:node18qof2jatx6 owl:withRestrictions _:node18qof2jatx8 .

h2o:ISOClassName owl:equivalentClass _:node18qof2jatx6 .

_:node18qof2jatx9 a owl:Restriction ;
	owl:cardinality "1"^^xsd:nonNegativeInteger ;
	owl:onProperty h2o:ttag .

h2o:TaggedValue rdfs:subClassOf _:node18qof2jatx9 .

_:node18qof2jatx10 a owl:Restriction ;
	owl:cardinality "1"^^xsd:nonNegativeInteger ;
	owl:onProperty h2o:tvalue .

h2o:TaggedValue rdfs:subClassOf _:node18qof2jatx10 .
