@prefix dc: <http://purl.org/dc/elements/1.1/> .
@prefix rdfs: <http://www.w3.org/2000/01/rdf-schema#> .
@prefix foaf: <http://xmlns.com/foaf/0.1/> .
@prefix owl: <http://www.w3.org/2002/07/owl#> .
@prefix rdf: <http://www.w3.org/1999/02/22-rdf-syntax-ns#> .
@prefix vann: <http://purl.org/vocab/vann/> .
@prefix label: <http://purl.org/net/vocab/2004/03/label#> .
@prefix cc: <http://web.resource.org/cc/> .
@prefix dcterms: <http://purl.org/dc/terms/> .

<http://purl.org/net/vocab/2004/03/label> a owl:Ontology ;
	rdfs:label "label"@en ;
	rdfs:comment "Term definitions for singular and plural label properties, and their inverses, for RDF terms"@en , "Definitioner for relationer mellem en term, dens inverse, og dens navn i entals- og flertalsform"@da , "Definiciones de etiquetas plurales y singulares de términos RDF"@es ;
	owl:imports <http://www.w3.org/2000/01/rdf-schema> , <http://www.w3.org/2002/07/owl> ;
	foaf:maker _:node17168lt0mx2 .

_:node17168lt0mx2 a foaf:Person ;
	foaf:name "Morten Høybye Frederiksen" ;
	foaf:mbox_sha1sum "65b983bb397fb71849da910996741752ace8369b" ;
	foaf:homepage <http://www.wasab.dk/morten/> .

<http://purl.org/net/vocab/2004/03/label> dcterms:created "2004-03-28"@en ;
	a cc:Work ;
	cc:license <http://creativecommons.org/licenses/by/1.0/> .

label:singular a owl:AnnotationProperty ;
	rdfs:label "singular"@en ;
	label:singular "singular form"@en ;
	label:plural "singular forms"@en ;
	rdfs:comment "A relation between a term and its label in literal singular form"@en ;
	rdfs:label "ental"@da ;
	label:singular "entalsform"@da ;
	label:plural "entalsformer"@da ;
	rdfs:comment "En relation mellem en term og dens navn i entalsform"@da ;
	rdfs:label "singular"@es ;
	label:singular "forma singular"@es ;
	label:plural "formas singulares"@es ;
	rdfs:comment "Una relación entre un término y su etiqueta en forma singular"@es ;
	rdfs:subPropertyOf rdfs:label ;
	rdfs:isDefinedBy <http://purl.org/net/vocab/2004/03/label> .

label:plural a owl:AnnotationProperty ;
	rdfs:label "plural"@en ;
	label:singular "plural form"@en ;
	label:plural "plural forms"@en ;
	rdfs:comment "A relation between a term and its label in literal plural form"@en ;
	rdfs:label "flertal"@da ;
	label:singular "flertalsform"@da ;
	label:plural "flertalsformer"@da ;
	rdfs:comment "En relation mellem en term og dens navn i flertalsform"@da ;
	rdfs:label "plural"@es ;
	label:singular "forma plural"@es ;
	label:plural "formas plurales"@es ;
	rdfs:comment "Una relación entre un término y su etiqueta en forma plural"@es ;
	rdfs:subPropertyOf rdfs:label ;
	rdfs:isDefinedBy <http://purl.org/net/vocab/2004/03/label> .

label:inverseSingular a owl:AnnotationProperty ;
	rdfs:label "inverse singular"@en ;
	label:singular "singular form of inverse"@en ;
	label:plural "singular forms of inverses"@en ;
	rdfs:comment "A relation between a term and the label of its inverse in literal singular form"@en ;
	rdfs:label "inverst ental"@da ;
	label:singular "entalsform for invers"@da ;
	label:plural "entalsformer for inverse"@da ;
	rdfs:comment "En relation mellem en term og dens inverses navn i entalsform"@da ;
	rdfs:subPropertyOf rdfs:label ;
	rdfs:isDefinedBy <http://purl.org/net/vocab/2004/03/label> .

label:inversePlural a owl:AnnotationProperty ;
	rdfs:label "inverse plural"@en ;
	label:singular "plural form of inverse"@en ;
	label:plural "plural forms of inverses"@en ;
	rdfs:comment "A relation between a term and the label of its inverse in literal plural form"@en ;
	rdfs:label "inverst flertal"@da ;
	label:singular "flertalsform for invers"@da ;
	label:plural "flertalsformer for inverse"@da ;
	rdfs:comment "En relation mellem en term og dens inverses navn i flertalsform"@da ;
	rdfs:subPropertyOf rdfs:label ;
	rdfs:isDefinedBy <http://purl.org/net/vocab/2004/03/label> .
