@prefix dc: <http://purl.org/dc/elements/1.1#> .
@prefix rdfs: <http://www.w3.org/2000/01/rdf-schema#> .
@prefix foaf: <http://xmlns.com/foaf/0.1#> .
@prefix owl: <http://www.w3.org/2002/07/owl#> .
@prefix vann: <http://purl.org/vocab/vann#> .
@prefix rdf: <http://www.w3.org/1999/02/22-rdf-syntax-ns#> .
@prefix skos: <http://www.w3.org/2004/02/skos/core#> .
@prefix dcterms: <http://purl.org/dc/terms#> .

<http://purl.org/limo-ontology/limo/> a owl:Ontology ;
	dcterms:title "Linked Statistical Models Vocabulary (limo)" ;
	dcterms:description "This document introduces an RDF vocabulary that enables the publishing of descriptions of predictive models into the Linked Data Web and establishes links to other resources such as datasets, other models, academic articles and studies. This is an early draft. Feedback and discussion are welcomed." ;
	dcterms:modified "2013-09-23"^^<http://www.w3.org/2001/XMLSchema#date> ;
	vann:preferredNamespaceUri "http://purl.org/limo-ontology/limo#" ;
	vann:preferredNamespacePrefix "limo" ;
	foaf:homepage <http://purl.org/limo-ontology/limo/limo.html> ;
	dcterms:created "2013-09-23"^^<http://www.w3.org/2001/XMLSchema#date> ;
	dcterms:publisher "http://purl.org/limo-ontology/limo/limo#Information%20Systems%20Lab%20%28ISLab%29" ;
	dcterms:partOf <http://195.251.218.39:8181/vocab> ;
	dcterms:type <http://purl.org/adms/assettype/Ontology> ;
	dcterms:status <http://purl.org/adms/status/UnderDevelopment> ;
	dc:creator <http://purl.org/limo-ontology/limo#akarm> , <http://purl.org/limo-ontology/limo#ekal> , <http://purl.org/limo-ontology/limo#kat> , <http://purl.org/limo-ontology/limo#tambouris> .

<http://purl.org/limo-ontology/limo#ttl> dcterms:FileFormat "" .

<http://purl.org/limo-ontology/limo#rdf> dcterms:FileFormat "" .

<http://purl.org/limo-ontology/limo#akarm> a foaf:Person ;
	foaf:name "Areti Karamanou" ;
	foaf:homepage "" ;
	foaf:mbox <mailto:akarm@uom.gr> .

<http://purl.org/limo-ontology/limo#Information%20Systems%20Lab%20%28ISLab%29> a dcterms:Agent ;
	foaf:member <http://purl.org/limo-ontology/limo#akarm> , <http://purl.org/limo-ontology/limo#ekal> , <http://purl.org/limo-ontology/limo#kat> , <http://purl.org/limo-ontology/limo#tambouris> ;
	foaf:name "Information Systems Lab (ISLab)" ;
	foaf:homepage <http://islab.uom.gr/> .

<http://purl.org/limo-ontology/limo#ekal> a foaf:Person ;
	foaf:name "Evangelos Kalampokis" ;
	foaf:homepage "" ;
	foaf:mbox <mailto:ekal@uom.gr> .

<http://purl.org/limo-ontology/limo#kat> a foaf:Person ;
	foaf:name "Konstantinos Tarabanis" ;
	foaf:homepage "" ;
	foaf:mbox <mailto:kat@uom.gr> .

<http://purl.org/limo-ontology/limo#tambouris> a foaf:Person ;
	foaf:name "Eythimios Tambouris" ;
	foaf:homepage "" ;
	foaf:mbox <mailto:tambouris@uom.gr> .

<http://purl.org/limo-ontology/limo#Model> a rdfs:Class , owl:Class ;
	rdfs:label "limo:Model" ;
	rdfs:comment "The actual predictive model that is described by the vocabulary." .

<http://purl.org/limo-ontology/limo#Variable> a rdfs:Class , owl:Class ;
	rdfs:label "limo:Variable" ;
	rdfs:comment "Represents the variables that are included in the predictive model." .

<http://purl.org/limo-ontology/limo#Method> a rdfs:Class , owl:Class ;
	rdfs:label "limo:Method" ;
	rdfs:subClassOf skos:Concept .

skos:Concept a rdfs:Class .

<http://purl.org/limo-ontology/limo#Method> rdfs:comment "Describes a statistical or data mining method used for creating a model. We assume that this class uses a set of predefined concepts such as linear regression, logistic regression, markov models, support vector machine, random forest, neural networks etc." .

<http://purl.org/limo-ontology/limo#Power> a rdfs:Class , owl:Class ;
	rdfs:label "limo:Power" ;
	rdfs:comment "Describes the predictive power of a model." .

<http://purl.org/limo-ontology/limo#File> a rdfs:Class , owl:Class ;
	rdfs:label "limo:File" ;
	rdfs:comment "Describes a file that can be imported in a particular platform such as R or SAS and execute the model. This could also be a PMML-XML file." .

<http://purl.org/limo-ontology/limo#data> a rdf:Property ;
	rdfs:label "limo:data" ;
	rdfs:comment "Connects a model to the dataset that contains the actual data that have been used for the development of the model." ;
	rdfs:domain <http://purl.org/limo-ontology/limo/limo#Model> ;
	rdfs:range <http://purl.org/linked-data/cube#Dataset> .

<http://purl.org/limo-ontology/limo#power> a rdf:Property ;
	rdfs:label "limo:power" ;
	rdfs:comment "Connects a model to its predictive power." ;
	rdfs:domain <http://purl.org/limo-ontology/limo#Model> ;
	rdfs:range <http://purl.org/limo-ontology/limo#Power> .

<http://purl.org/limo-ontology/limo#creator> a rdf:Property ;
	rdfs:label "dct:creator" ;
	rdfs:comment "The person or organization that actually builds the model." ;
	rdfs:domain <http://purl.org/limo-ontology/limo#Model> ;
	rdfs:range <http://xmlns.com/foaf/0.1/Agent> .

<http://purl.org/limo-ontology/limo#method> a rdf:Property ;
	rdfs:label "limo:method" ;
	rdfs:comment "Connects a model with its statistical or data mining method." ;
	rdfs:domain <http://purl.org/limo-ontology/limo#Model> ;
	rdfs:range <http://purl.org/limo-ontology/limo#Method> .

<http://purl.org/limo-ontology/limo#variable> a rdf:Property ;
	rdfs:label "limo:variable" ;
	rdfs:comment "Connects a model to one of its variables." ;
	rdfs:domain <http://purl.org/limo-ontology/limo#Model> ;
	rdfs:range <http://purl.org/limo-ontology/limo#Variable> .

<http://purl.org/limo-ontology/limo#theme> a rdf:Property ;
	rdfs:label "limo:theme" ;
	rdfs:comment "Connects a variable to its concept theme." ;
	rdfs:domain <http://purl.org/limo-ontology/limo#Variable> ;
	rdfs:range skos:Concept .

<http://purl.org/limo-ontology/limo#file> a rdf:Property ;
	rdfs:label "limo:file" ;
	rdfs:comment "Connects a model with a relative file." ;
	rdfs:domain <http://purl.org/limo-ontology/limo#Model> ;
	rdfs:range <http://purl.org/limo-ontology/limo#File> .

<http://purl.org/limo-ontology/limo#publishedIn> a rdf:Property ;
	rdfs:label "limo:publishedIn" ;
	rdfs:comment "Connects a model with the bibliographic resource it is published." ;
	rdfs:domain <http://purl.org/limo-ontology/limo#Model> ;
	rdfs:range dcterms:BibliographicResource .

<http://purl.org/limo-ontology/limo#baseline> a rdf:Property ;
	rdfs:label "limo:baseline" ;
	rdfs:comment "Explicitly denotes that the predictive power of a model has been evaluated against the power of another model." ;
	rdfs:domain <http://purl.org/limo-ontology/limo#Model> ;
	rdfs:range <http://purl.org/limo-ontology/limo#Model> .

<http://purl.org/limo-ontology/limo#evaluationData> a rdf:Property ;
	rdfs:label "limo:evaluationData" ;
	rdfs:comment "Connects a model to the dataset that represents its evaluation data." ;
	rdfs:subPropertyOf <http://purl.org/limo-ontology/limo#data> .

<http://purl.org/limo-ontology/limo#validationData> a rdf:Property ;
	rdfs:label "limo:validationData" ;
	rdfs:comment "Connects a model to a qb:DataSet that represents data that was used for the validation of the model." ;
	rdfs:subPropertyOf <http://purl.org/limo-ontology/limo#data> .

<http://purl.org/limo-ontology/limo#trainingData> a rdf:Property ;
	rdfs:label "limo:trainingData" ;
	rdfs:comment "Connects a model to a qb:DataSet that represents data that was used for the training of the model." ;
	rdfs:subPropertyOf <http://purl.org/limo-ontology/limo#data> .

<http://purl.org/limo-ontology/limo#rawData> a rdf:Property ;
	rdfs:label "limo:rawData" ;
	rdfs:comment "Connects a model with it's dataset." ;
	rdfs:domain <http://purl.org/limo-ontology/limo#Model> ;
	rdfs:range <http://purl.org/dc/dcmitype#Dataset> .

<http://purl.org/limo-ontology/limo#evaluationMethod> a rdf:Property ;
	rdfs:label "limo:evaluationMethod" ;
	rdfs:comment "mpla mpla" ;
	rdfs:domain <http://purl.org/limo-ontology/limo#Power> .

<http://purl.org/limo-ontology/limo#outcome> a rdf:Property ;
	rdfs:label "limo:outcome" ;
	rdfs:comment "" ;
	rdfs:domain <http://purl.org/limo-ontology/limo#Power> .

<http://purl.org/limo-ontology/limo#accessURL> a rdf:Property ;
	rdfs:label "limo:accessURL" ;
	rdfs:comment "The URL that the file can be accessed from." ;
	rdfs:domain <http://purl.org/limo-ontology/limo#File> .

dcterms:title a rdf:Property ;
	rdfs:label "dct:title" ;
	rdfs:comment "A name given to the model." ;
	rdfs:domain <http://purl.org/limo-ontology/limo#Model> ;
	rdfs:range rdfs:Literal ;
	rdfs:comment "A name given to the variable or model." ;
	rdfs:domain <http://purl.org/limo-ontology/limo#Variable> .

dcterms:description a rdf:Property ;
	rdfs:label "dct:description" ;
	rdfs:comment "A small text to describe what the variable or model is about." ;
	rdfs:domain <http://purl.org/limo-ontology/limo#Variable> ;
	rdfs:range rdfs:Literal ;
	rdfs:domain <http://purl.org/limo-ontology/limo#Model> .

<http://purl.org/limo-ontology/limo#variableType> a rdf:Property ;
	rdfs:label "limo:variableType" ;
	rdfs:comment "Denotes whether the variable is continuous, categorical or ordinal." ;
	rdfs:domain <http://purl.org/limo-ontology/limo#Variable> .

<http://purl.org/limo-ontology/limo#usageType> a rdf:Property ;
	rdfs:label "limo:usageType" ;
	rdfs:comment "Denotes whether the variable is the response of the model or one of the predictors." ;
	rdfs:domain <http://purl.org/limo-ontology/limo#Variable> .

dcterms:issued a rdf:Property ;
	rdfs:label "dct:issued" ;
	rdfs:comment "Defines the actual date that the model has been created." ;
	rdfs:domain <http://purl.org/limo-ontology/limo#Model> .

<http://purl.org/limo-ontology/limo#spatial> a rdf:Property ;
	rdfs:label "limo:spatial" ;
	rdfs:comment "Dexcribes the spatial dimension of the model. The spatial dimension is derived from the actual data that has been employed." ;
	rdfs:domain <http://purl.org/limo-ontology/limo#Model> ;
	rdfs:range dcterms:Location .

<http://purl.org/limo-ontology/limo#temporal> a rdf:Property ;
	rdfs:label "limo:temporal" ;
	rdfs:comment "Describes the time period that the model covers. The time period reflects the period that is described in the actual data that have been used for the development of the model." ;
	rdfs:domain <http://purl.org/limo-ontology/limo#Model> ;
	rdfs:range dcterms:PeriodOfTime .

<http://purl.org/limo-ontology/limo#modelType> a rdf:Property ;
	rdfs:label "limo:modelType" ;
	rdfs:comment "Describes the main categories of the model that can be developed, namely classification, regression, clustering and dimension reduction." ;
	rdfs:domain <http://purl.org/limo-ontology/limo#Model> .

<http://purl.org/limo-ontology/limo#evaluationMethod> rdfs:comment "Is used to infer the predictive power of the model. The evaluation methods include out-of-sample evaluation with statistics such as Predicted Residual Sums of Squares, Root Mean Square Error or cross-validation techniques." .

<http://purl.org/limo-ontology/limo#outcome> rdfs:comment "The actual value that the evaluation method produces." .
