@prefix prv: <http://purl.org/net/provenance/ns#> .
@prefix rdfs: <http://www.w3.org/2000/01/rdf-schema#> .
@prefix foaf: <http://xmlns.com/foaf/0.1/> .
@prefix dcterm: <http://purl.org/dc/terms/> .
@prefix rdf: <http://www.w3.org/1999/02/22-rdf-syntax-ns#> .
@prefix xhv: <http://www.w3.org/1999/xhtml/vocab#> .

<http://observedchange.com/moac/ns/> a foaf:Document ;
	dcterm:title "Management of a Crisis (MOAC) Vocabulary Specification"@en ;
	xhv:stylesheet <http://observedchange.com/tisc/ns/main.css> ;
	rdfs:label "Document that defines the Management of a Crisis Vocabulary"@en ;
	foaf:primaryTopic <http://www.observedchange.com/moac/ns#> .

<http://www.observedchange.com/moac/ns#> a prv:DataItem , <http://www.w3.org/2002/07/owl#Ontology> ;
	dcterm:title "Management of a Crisis Vocabulary namespace"@en ;
	prv:createdBy _:node172hmq1dux1 .

_:node172hmq1dux1 a prv:DataCreation ;
	prv:performedBy <http://kauppinen.net/tomi#me> ;
	prv:performedAt "2012-01-29T20:30:00Z"^^<http://www.w3.org/2001/XMLSchema#dateTime> .

<http://www.observedchange.com/moac/ns#> dcterm:creator <http://kauppinen.net/tomi#me> ;
	dcterm:created "2012-01-29T20:30:00Z"^^<http://www.w3.org/2001/XMLSchema#dateTime> .

<http://kauppinen.net/tomi#me> a foaf:Person ;
	foaf:homepage <http://kauppinen.net/tomi> ;
	foaf:name "Tomi Kauppinen"@en .

<http://observedchange.com/moac/ns/> dcterm:conformsTo <http://www.w3.org/TR/rdfa-syntax> .

<http://observedchange.com/moac/ns#> dcterm:description "MOAC, the Management of a Crisis Vocabulary, is a lightweight vocabulary aiming to provide terms to enable practitioners to relate different \"things\" in crisis management activities together as Linked Data. The initial MOAC terms originated from the Inter Agency Standing Committee (IASC), Emergency Shelter Cluster in Haiti, UNOCHA 3W Who What Where Contact Database and"@en .

<http://observedchange.com/moac/ns/> dcterm:description "Efforts have been made to involve a number of international humanitarian and crowdsourcing volunteering communities to authenticate MOAC usability, functionality and structures. Since, the vocabulary is still evolving, necessary changes based on expert recommendations will be carefully documented and necessary changes will be continuously updated in the same platform."@en , ""@en .

<http://observedchange.com/moac/ns#WhoWhatWhere3W> a <http://www.w3.org/2002/07/owl#Class> ;
	rdfs:isDefinedBy <http://observedchange.com/moac/ns#WhoWhatWhereSection> ;
	rdfs:label "WaterShortage"@en ;
	rdfs:comment "Abstract term to describe the collection of which agency is doing what activities and where."@en .

<http://observedchange.com/moac/ns#Who3W> a <http://www.w3.org/2002/07/owl#Class> ;
	rdfs:isDefinedBy <http://observedchange.com/moac/ns#WhoWhatWhereSection> ;
	rdfs:label "Who3W"@en ;
	rdfs:comment "Specific agency or Organisation humanitarian response information."@en .

<http://observedchange.com/moac/ns#What3W> a <http://www.w3.org/2002/07/owl#Class> ;
	rdfs:isDefinedBy <http://observedchange.com/moac/ns#WhoWhatWhereSection> ;
	rdfs:label "What3W"@en ;
	rdfs:comment "Specific activities in relation to humanitarian response."@en .

<http://observedchange.com/moac/ns#Where3W> a <http://www.w3.org/2002/07/owl#Class> ;
	rdfs:isDefinedBy <http://observedchange.com/moac/ns#WhoWhatWhereSection> ;
	rdfs:label "Where3W"@en ;
	rdfs:comment "Specific location(s) in relation to humanitarian response."@en .

<http://observedchange.com/moac/ns#When3W> a <http://www.w3.org/2002/07/owl#Class> ;
	rdfs:isDefinedBy <http://observedchange.com/moac/ns#WhoWhatWhereSection> ;
	rdfs:label "When3W"@en ;
	rdfs:comment "Specific time in relation to humanitarian response."@en .

<http://observedchange.com/moac/ns#NeedsResponse3W> a <http://www.w3.org/2002/07/owl#Class> ;
	rdfs:isDefinedBy <http://observedchange.com/moac/ns#WhoWhatWhereSection> ;
	rdfs:label "NeedsResponse3W"@en ;
	rdfs:comment "Humanitarian needs and response related activities."@en .

<http://observedchange.com/moac/ns#Response3W> a <http://www.w3.org/2002/07/owl#Class> ;
	rdfs:isDefinedBy <http://observedchange.com/moac/ns#WhoWhatWhereSection> ;
	rdfs:label "Response3W"@en ;
	rdfs:comment "Cluster Specific humanitarian response information."@en .

<http://observedchange.com/moac/ns#Needs3W> a <http://www.w3.org/2002/07/owl#Class> ;
	rdfs:isDefinedBy <http://observedchange.com/moac/ns#WhoWhatWhereSection> ;
	rdfs:label "Needs3W"@en ;
	rdfs:comment "Cluster Specific humanitarian response information."@en .

<http://observedchange.com/moac/ns#IASCCluster> a <http://www.w3.org/2002/07/owl#Class> ;
	rdfs:isDefinedBy <http://observedchange.com/moac/ns#IASCClusterSection> ;
	rdfs:label "IASCCluster"@en ;
	rdfs:comment "Humanitarian sectors and categories of population for achieving more strategic responses and better prioritization of available resources by clarifying the division of labour among organizations, better defining the roles and responsibilities of humanitarian organizations within the sectors, and providing the Humanitarian Coordinator with both a first point of call and a provider of last resort in all the key sectors or areas of activity."@en .

<http://observedchange.com/moac/ns#Cluster1Shelter> a <http://www.w3.org/2002/07/owl#Class> ;
	rdfs:isDefinedBy <http://observedchange.com/moac/ns#IASCClusterSection> ;
	rdfs:label "Cluster1Shelter"@en ;
	rdfs:comment "Inter Agency Standing Committee Emergency Shelter related agency specific activities. The Shelter Cluster is co-chaired by IFRC and UNHCR at the global level. IFRC is convener of the Emergency Shelter Cluster in disaster situations while UNHCR leads the Emergency Shelter Cluster in the area of conflict generated IDPs (Internally Displaced Persons). In addition to IFRC and UNHCR, participants in the Global Shelter Cluster include: ACTED, Archi-Urgent, Article 25, Care UK, CHF, CRS, DFID, Habitat for Humanity, IOM, Medair, NRC, OFDA, Oxfam GB, ProAct, ProVention, RedR, Relief International, RICS, Save The Children UK, Shelter Centre, SKAT, UN Habitat, UN OCHA, UNRWA and World Vision. (source: sheltercluster.org, accessed on 12 Feb 2012)"@en .

<http://observedchange.com/moac/ns#Cluster2Food> a <http://www.w3.org/2002/07/owl#Class> ;
	rdfs:isDefinedBy <http://observedchange.com/moac/ns#IASCClusterSection> ;
	rdfs:label "Cluster2Food"@en ;
	rdfs:comment "Inter Agency Standing Committee Emergency Food related agency specific activities. World Food Programme (WFP) is the global cluster lead for Food."@en .

<http://observedchange.com/moac/ns#Cluster3WASH> a <http://www.w3.org/2002/07/owl#Class> ;
	rdfs:isDefinedBy <http://observedchange.com/moac/ns#IASCClusterSection> ;
	rdfs:label "Cluster3WASH"@en ;
	rdfs:comment "Inter Agency Standing Committee Emergency Water Sanitation and Hygine related agency specific activities. UNICEF is the global cluster lead for WASH."@en .

<http://observedchange.com/moac/ns#ShelterAgency> a <http://www.w3.org/2002/07/owl#Class> ;
	rdfs:isDefinedBy <http://observedchange.com/moac/ns#IASCClusterSection> ;
	rdfs:label "ShelterAgency"@en ;
	rdfs:comment "ShelterAgency is a Shelter Cluster related humanitarian partner or a specific organization involved in shelter related humanitarian response."@en .

<http://observedchange.com/moac/ns#ShelterActivity> a <http://www.w3.org/2002/07/owl#Class> ;
	rdfs:isDefinedBy <http://observedchange.com/moac/ns#IASCClusterSection> ;
	rdfs:label "ShelterActivity"@en ;
	rdfs:comment "ShelterActivity is a term that describes Shelter Cluster related humanitarian response."@en .

<http://observedchange.com/moac/ns#ShelterNFIItems> a <http://www.w3.org/2002/07/owl#Class> ;
	rdfs:isDefinedBy <http://observedchange.com/moac/ns#IASCClusterSection> ;
	rdfs:label "ShelterNFIItems"@en ;
	rdfs:comment "ShelterNFIItems define Shelter Cluster related humanitarian relief items (e.g. tents, tarpulins)."@en .

<http://observedchange.com/moac/ns#ShelterItems> a <http://www.w3.org/2002/07/owl#Class> ;
	rdfs:isDefinedBy <http://observedchange.com/moac/ns#IASCClusterSection> ;
	rdfs:label "ShelterItems"@en ;
	rdfs:comment "ShelterItems include, but are not limited to, tents, tarpulins distributed or stocked by shelter response humanitarian agencies."@en .

<http://observedchange.com/moac/ns#NFIItems> a <http://www.w3.org/2002/07/owl#Class> ;
	rdfs:isDefinedBy <http://observedchange.com/moac/ns#IASCClusterSection> ;
	rdfs:label "NFIItems"@en ;
	rdfs:comment "NFIItems also known as Non Food Items include, but are not limited to, jerry cans, kots, mats distributed or stocked by shelter response humanitarian agencies."@en .

<http://observedchange.com/moac/ns#ShelterResponse> a <http://www.w3.org/2002/07/owl#Class> ;
	rdfs:isDefinedBy <http://observedchange.com/moac/ns#IASCClusterSection> ;
	rdfs:label "ShelterResponse"@en ;
	rdfs:comment "ShelterResponse is related to activities defining Shelter Clusters' humanitarian response in an emergency."@en .

<http://observedchange.com/moac/ns#ShelterOffered> a <http://www.w3.org/2002/07/owl#Class> ;
	rdfs:isDefinedBy <http://observedchange.com/moac/ns#IASCClusterSection> ;
	rdfs:label "ShelterOffered"@en ;
	rdfs:comment "ShelterOffered relates shelter activities when a humanitarian relief agencies provide shelter (e.g. tents, tarps) materials as a part of a relief distribution."@en .

<http://observedchange.com/moac/ns#ShelterNeeded> a <http://www.w3.org/2002/07/owl#Class> ;
	rdfs:isDefinedBy <http://observedchange.com/moac/ns#IASCClusterSection> ;
	rdfs:label "ShelterNeeded"@en ;
	rdfs:comment "ShelterNeeded records information regarding additional shelter needs as a part of planned relief distribution processes."@en .

<http://observedchange.com/moac/ns#ShelterDistributionPoint> a <http://www.w3.org/2002/07/owl#Class> ;
	rdfs:isDefinedBy <http://observedchange.com/moac/ns#IASCClusterSection> ;
	rdfs:label "ShelterDistributionPoint"@en ;
	rdfs:comment "ShelterDistributionPoint is a specific location where humanitarian relief agencies provide shelter assistances as a part of relief distribution."@en .

<http://observedchange.com/moac/ns#belongsToCluster> a <http://www.w3.org/2002/07/owl#DataProperty> ;
	rdfs:isDefinedBy <http://observedchange.com/moac/ns> ;
	rdfs:label "belongsToCluster"@en ;
	rdfs:comment "belongsToCluster indicates the organisation which belongs to a specific IASC cluster for example, emergency Shelter cluster or Food Cluster."@en ;
	rdfs:range <http://observedchange.com/moac/ns#moac:Who3W> , <http://observedchange.com/moac/ns#IASCCluster> .

<http://observedchange.com/moac/ns#affectedby> a <http://www.w3.org/2002/07/owl#DataProperty> ;
	rdfs:isDefinedBy <http://observedchange.com/moac/ns> ;
	rdfs:label "affectedby"@en ;
	rdfs:comment "affectedby indicates the relation of people being affected by certain disaster."@en ;
	rdfs:range <http://observedchange.com/moac/ns#ShelterOffered> , <http://observedchange.com/moac/ns#NaturalHazards> .

<http://observedchange.com/moac/ns#countOfAffectedPopulation> a <http://www.w3.org/2002/07/owl#DataProperty> ;
	rdfs:isDefinedBy <http://observedchange.com/moac/ns> ;
	rdfs:label "countOfAffectedPopulation"@en ;
	rdfs:comment "countOfAffectedPopulation indicates the total number of people affected by a certain disaster."@en ;
	rdfs:range <http://observedchange.com/moac/ns#AffectedPopulation> , rdfs:int .

<http://observedchange.com/moac/ns#countofAffectedHH> a <http://www.w3.org/2002/07/owl#DataProperty> ;
	rdfs:isDefinedBy <http://observedchange.com/moac/ns> ;
	rdfs:label "countofAffectedHH"@en ;
	rdfs:comment "countofAffectedHH indicates total number of House Holds affected by a certain disaster."@en ;
	rdfs:range <http://observedchange.com/moac/ns#AffectedPopulation> , rdfs:int .

<http://observedchange.com/moac/ns#clusterActivity> a <http://www.w3.org/2002/07/owl#DataProperty> ;
	rdfs:isDefinedBy <http://observedchange.com/moac/ns> ;
	rdfs:label "atLocation"@en ;
	rdfs:comment "clusterActivity is a property to relate humanitarian Clusters with ongoing humanitarian response to meet the needs of affected population."@en ;
	rdfs:domain <http://observedchange.com/moac/ns#IASCCluster> , <http://observedchange.com/moac/ns#NeedsResponse3W> .

<http://observedchange.com/moac/ns#countInStock> a <http://www.w3.org/2002/07/owl#DataProperty> ;
	rdfs:isDefinedBy <http://observedchange.com/moac/ns> ;
	rdfs:label "countInStock"@en ;
	rdfs:comment "countInStock indicates the number of items currently stockpiled either at a store or at a distribution location."@en ;
	rdfs:range <http://observedchange.com/moac/ns#ShelterNFIItems> , rdfs:int .

<http://observedchange.com/moac/ns#countInPipeline> a <http://www.w3.org/2002/07/owl#DataProperty> ;
	rdfs:isDefinedBy <http://observedchange.com/moac/ns> ;
	rdfs:label "countInPipeline"@en ;
	rdfs:comment "countInPipeline indicates the number of relief items that are \"in the process\" of arriving from a different location."@en ;
	rdfs:range <http://observedchange.com/moac/ns#ShelterNFIItems> , rdfs:int .

<http://observedchange.com/moac/ns#dateOfDistbn> a <http://www.w3.org/2002/07/owl#DataProperty> ;
	rdfs:isDefinedBy <http://observedchange.com/moac/ns> ;
	rdfs:label "dateOfDistbn"@en ;
	rdfs:comment "dateOfDistbn indicates a particular date when shelter/NFI items are distributed."@en ;
	rdfs:range <http://observedchange.com/moac/ns#When3W> , <http://purl.org/dc/elements/1.1/date> .

<http://observedchange.com/moac/ns#distributingPartner> a <http://www.w3.org/2002/07/owl#DataProperty> ;
	rdfs:isDefinedBy <http://observedchange.com/moac/ns> ;
	rdfs:label "distributingPartner"@en ;
	rdfs:comment "distributingPartner indicates the name of an organisation that is responsible to distribute relief items in a disaster."@en ;
	rdfs:range <http://observedchange.com/moac/ns#ShelterAgency> , rdfs:Literal .

<http://observedchange.com/moac/ns#has3Wcomponent> a <http://www.w3.org/2002/07/owl#DataProperty> ;
	rdfs:isDefinedBy <http://observedchange.com/moac/ns> ;
	rdfs:label "has3Wcomponent"@en ;
	rdfs:comment "has3Wcomponent indicates the four saparate components of 3W i.e Who What Where and When."@en ;
	rdfs:range <http://observedchange.com/moac/ns#WhoWhatWhere3W> .

<http://observedchange.com/moac/ns#hasOrganisationID> a <http://www.w3.org/2002/07/owl#DataProperty> ;
	rdfs:isDefinedBy <http://observedchange.com/moac/ns> ;
	rdfs:label "hasOrganisationID"@en ;
	rdfs:comment "hasOrganisationID is a unique identification number given to relief agency."@en ;
	rdfs:range <http://observedchange.com/moac/ns#moac:Who3W> , <http://observedchange.com/moac/ns#ShelterAgency> , <http://www.w3.org/2001/XMLSchema#string> .

<http://observedchange.com/moac/ns#hasShelterItems> a <http://www.w3.org/2002/07/owl#DataProperty> ;
	rdfs:isDefinedBy <http://observedchange.com/moac/ns> ;
	rdfs:label "hasShelterItems"@en ;
	rdfs:comment "hasShelterItems indicates the name or a type of shelter related items."@en ;
	rdfs:range <http://observedchange.com/moac/ns#ShelterItems> , rdfs:string .

<http://observedchange.com/moac/ns#hasNFIItems> a <http://www.w3.org/2002/07/owl#DataProperty> ;
	rdfs:isDefinedBy <http://observedchange.com/moac/ns> ;
	rdfs:label "hasNFIItems"@en ;
	rdfs:comment "hasNFIItems indicates the name or a type of Non Food Items."@en ;
	rdfs:range <http://observedchange.com/moac/ns#NFIItems> , rdfs:string .

<http://observedchange.com/moac/ns#involvedIn> a <http://www.w3.org/2002/07/owl#DataProperty> ;
	rdfs:isDefinedBy <http://observedchange.com/moac/ns> ;
	rdfs:label "involvedIn"@en ;
	rdfs:comment "involvedIn indicates the agency that is involved with humanitarian activities/response in a disaster."@en ;
	rdfs:range <http://observedchange.com/moac/ns#ShelterAgency> , <http://observedchange.com/moac/ns#ShelterActivity> , <http://observedchange.com/moac/ns#ShelterResponse> .

<http://observedchange.com/moac/ns#NFINeededAt> a <http://www.w3.org/2002/07/owl#DataProperty> ;
	rdfs:isDefinedBy <http://observedchange.com/moac/ns> ;
	rdfs:label "NFINeededAt"@en ;
	rdfs:comment "NFINeededAt relates \"where\" Non Food Items response might be necessary."@en ;
	rdfs:range <http://observedchange.com/moac/ns#AffectedPopulation> , <http://observedchange.com/moac/ns#Where3W> , dcterm:Location .

<http://observedchange.com/moac/ns#organizationName> a <http://www.w3.org/2002/07/owl#DataProperty> ;
	rdfs:isDefinedBy <http://observedchange.com/moac/ns> ;
	rdfs:label "organizationName"@en ;
	rdfs:comment "organizationName indicates the name of the organisation for a specific IASC cluster like emergency Shelter cluster or Food Cluster."@en ;
	rdfs:range <http://observedchange.com/moac/ns#Who3W> , <http://observedchange.com/moac/ns#ShelterAgency> , <http://observedchange.com/moac/ns#IASCCluster> .

<http://observedchange.com/moac/ns#shelterOfferedAt> a <http://www.w3.org/2002/07/owl#DataProperty> ;
	rdfs:isDefinedBy <http://observedchange.com/moac/ns> ;
	rdfs:label "shelterOfferedAt"@en ;
	rdfs:comment "shelterOfferedAt relates \"where\" shelter relief agencies provided relief items."@en ;
	rdfs:range <http://observedchange.com/moac/ns#ShelterAgency> , <http://observedchange.com/moac/ns#Where3W> , dcterm:Location .

<http://observedchange.com/moac/ns#shelterNeededAt> a <http://www.w3.org/2002/07/owl#DataProperty> ;
	rdfs:isDefinedBy <http://observedchange.com/moac/ns> ;
	rdfs:label "shelterNeededAt"@en ;
	rdfs:comment "shelterNeededAt relates \"where\" shelter response might be necessary."@en ;
	rdfs:range <http://observedchange.com/moac/ns#AffectedPopulation> , <http://observedchange.com/moac/ns#Where3W> , dcterm:Location .

<http://observedchange.com/moac/ns#supplyingAgency> a <http://www.w3.org/2002/07/owl#DataProperty> ;
	rdfs:isDefinedBy <http://observedchange.com/moac/ns> ;
	rdfs:label "supplyingAgency"@en ;
	rdfs:comment "supplyingAgency indicates the name of an organisation that is responsible to provide humanitarian relief items."@en ;
	rdfs:range <http://observedchange.com/moac/ns#moac:Who3W> , <http://observedchange.com/moac/ns#ShelterAgency> , <http://www.w3.org/2001/XMLSchema#string> .

<http://observedchange.com/moac/ns#tentDistbn> a <http://www.w3.org/2002/07/owl#DataProperty> ;
	rdfs:isDefinedBy <http://observedchange.com/moac/ns> ;
	rdfs:label "tentDistbn"@en ;
	rdfs:comment "tentDistbn relates the amount (count) of shelter items being offered."@en ;
	rdfs:range <http://observedchange.com/moac/ns#ShelterOffered> , rdfs:int .

<http://observedchange.com/moac/ns#AffectedPopulation> a <http://www.w3.org/2002/07/owl#Class> ;
	rdfs:isDefinedBy <http://observedchange.com/moac/ns> ;
	rdfs:label "AffectedPopulation"@en ;
	rdfs:comment "AffectedPopulation is a group of disaster affecgted people in need of humanitarian support."@en .

<http://observedchange.com/moac/ns#Agency> a <http://www.w3.org/2002/07/owl#Class> ;
	rdfs:isDefinedBy <http://observedchange.com/moac/ns> ;
	rdfs:label "Agency"@en ;
	rdfs:comment "Agency is an organization that aims to manage a crisis."@en .

<http://observedchange.com/moac/ns#AidManipulation> a <http://www.w3.org/2002/07/owl#Class> ;
	rdfs:isDefinedBy <http://observedchange.com/moac/ns> ;
	rdfs:label "AidManipulation"@en ;
	rdfs:comment "AidManipulation."@en .

<http://observedchange.com/moac/ns#AnimalIllnessOrDeath> a <http://www.w3.org/2002/07/owl#Class> ;
	rdfs:isDefinedBy <http://observedchange.com/moac/ns> ;
	rdfs:label "AnimalIllnessOrDeath"@en ;
	rdfs:comment "AnimalIllnessOrDeath refers to the illness or death of animals caused by a disaster highlighting the possibility of spread of disease because of direct or indirect contamination."@en .

<http://observedchange.com/moac/ns#AskingToFowardAMessage> a <http://www.w3.org/2002/07/owl#Class> ;
	rdfs:isDefinedBy <http://observedchange.com/moac/ns> ;
	rdfs:label "AskingToFowardAMessage"@en ;
	rdfs:comment "AskingToFowardAMessage is the term used to forward certain community directed messages using third party sources."@en .

<http://observedchange.com/moac/ns#ChronicCareNeeds> a <http://www.w3.org/2002/07/owl#Class> ;
	rdfs:isDefinedBy <http://observedchange.com/moac/ns> ;
	rdfs:label "ChronicCareNeeds"@en ;
	rdfs:comment "ChronicCareNeeds refers to the requirement of medical care which addresses preexisting or long term illness."@en .

<http://observedchange.com/moac/ns#CollapsedStructure> a <http://www.w3.org/2002/07/owl#Class> ;
	rdfs:isDefinedBy <http://observedchange.com/moac/ns> ;
	rdfs:label "CollapsedStructure"@en ;
	rdfs:comment "A CollapsedStructure is a term that defines a totally damaged state of a structure resulting from human or natural phenomenon."@en .

<http://observedchange.com/moac/ns#CommunicationLinesDown> a <http://www.w3.org/2002/07/owl#Class> ;
	rdfs:isDefinedBy <http://observedchange.com/moac/ns> ;
	rdfs:label "CommunicationLinesDown"@en ;
	rdfs:comment "CommunicationLinesDown indicates that a mobile or a landline phone in ceratain area will not work because of the problem in the communication wired poles."@en .

<http://observedchange.com/moac/ns#CompromisedBridge> a <http://www.w3.org/2002/07/owl#Class> ;
	rdfs:isDefinedBy <http://observedchange.com/moac/ns> ;
	rdfs:label "CompromisedBridge"@en ;
	rdfs:comment "CompromisedBridge is a partially or completely damaged bridge that can no longer be used for transporting people or relief materials."@en .

<http://observedchange.com/moac/ns#ContaminatedWater> a <http://www.w3.org/2002/07/owl#Class> ;
	rdfs:isDefinedBy <http://observedchange.com/moac/ns> ;
	rdfs:label "ContaminatedWater"@en ;
	rdfs:comment "Undrinkable Water is water that is regarded unfit/unhealthy to drink for both humans and animals."@en .

<http://observedchange.com/moac/ns#ContaminatedWaterSupply> a <http://www.w3.org/2002/07/owl#Class> ;
	rdfs:isDefinedBy <http://observedchange.com/moac/ns> ;
	rdfs:label "ContaminatedWaterSupply"@en ;
	rdfs:comment "The source and delivery system provides water but polluted. It could result in outbreaks of diseases and other health realted issues."@en .

<http://observedchange.com/moac/ns#Deaths> a <http://www.w3.org/2002/07/owl#Class> ;
	rdfs:isDefinedBy <http://observedchange.com/moac/ns> ;
	rdfs:label "Deaths"@en ;
	rdfs:comment "Deaths are the termination of the biological functions that sustain a living organism."@en .

<http://observedchange.com/moac/ns#EarthquakeAndAftershock> a <http://www.w3.org/2002/07/owl#Class> ;
	rdfs:isDefinedBy <http://observedchange.com/moac/ns> ;
	rdfs:label "EarthquakeAndAftershock"@en ;
	rdfs:comment "An earthquake is the result of a sudden release of energy in the Earth's crust that creates seismic waves, and an aftershock is an earthquake that occurs after a previous earthquake, the mainshock."@en .

<http://observedchange.com/moac/ns#Emergency> a <http://www.w3.org/2002/07/owl#Class> ;
	rdfs:isDefinedBy <http://observedchange.com/moac/ns> ;
	rdfs:label "Emergency"@en ;
	rdfs:comment "Emergency is a situation that poses an immediate crisis to human, life, health, property or environment."@en .

<http://observedchange.com/moac/ns#FeedingCentersAvailable> a <http://www.w3.org/2002/07/owl#Class> ;
	rdfs:isDefinedBy <http://observedchange.com/moac/ns> ;
	rdfs:label "FeedingCentersAvailable"@en ;
	rdfs:comment "FeedingCentersAvailable is a term that defines a location of a facility which supports providing basic life saving foods to infants and lactating mothers."@en .

<http://observedchange.com/moac/ns#FinancialServicesAvailable> a <http://www.w3.org/2002/07/owl#Class> ;
	rdfs:isDefinedBy <http://observedchange.com/moac/ns> ;
	rdfs:label "FinancialServicesAvailable"@en ;
	rdfs:comment "FinancialServicesAvailabe refers to services provided by the certain Non Government Organizations or finance industry as a part of recovery packages to the disaster affected communities."@en .

<http://observedchange.com/moac/ns#Fire> a <http://www.w3.org/2002/07/owl#Class> ;
	rdfs:isDefinedBy <http://observedchange.com/moac/ns> ;
	rdfs:label "Fire"@en ;
	rdfs:comment "Fire is an uncontrolled burning that has the potential to cause physical damage on human life, health, property or ecology."@en .

<http://observedchange.com/moac/ns#Floods> a <http://www.w3.org/2002/07/owl#Class> ;
	rdfs:isDefinedBy <http://observedchange.com/moac/ns> ;
	rdfs:label "Floods"@en ;
	rdfs:comment "A flood is an overflow of an expanse of water that submerges land."@en .

<http://observedchange.com/moac/ns#FoodDistributionPoint> a <http://www.w3.org/2002/07/owl#Class> ;
	rdfs:isDefinedBy <http://observedchange.com/moac/ns> ;
	rdfs:label "FoodDistributionPoint"@en ;
	rdfs:comment "FoodDistributionPoint is a pre-identified location for distributing or transporting food or drink to the affected communities."@en .

<http://observedchange.com/moac/ns#FoodShortage> a <http://www.w3.org/2002/07/owl#Class> ;
	rdfs:isDefinedBy <http://observedchange.com/moac/ns> ;
	rdfs:label "FoodShortage"@en ;
	rdfs:comment "FoodShortage is a widespread scarcity of food that may apply to any faunal species."@en .

<http://observedchange.com/moac/ns#FuelShortage> a <http://www.w3.org/2002/07/owl#Class> ;
	rdfs:isDefinedBy <http://observedchange.com/moac/ns> ;
	rdfs:label "FuelShortage"@en ;
	rdfs:comment "FuelShortage is a lack of minimal cooking or other fuel that a person need on a daily basis."@en .

<http://observedchange.com/moac/ns#GroupViolence> a <http://www.w3.org/2002/07/owl#Class> ;
	rdfs:isDefinedBy <http://observedchange.com/moac/ns> ;
	rdfs:label "GroupViolence"@en ;
	rdfs:comment "GroupViolence is a term used to describe more than one individual engaging in some form of criminal activities."@en .

<http://observedchange.com/moac/ns#HealthOfWomen> a <http://www.w3.org/2002/07/owl#Class> ;
	rdfs:isDefinedBy <http://observedchange.com/moac/ns> ;
	rdfs:label "HealthOfWomen"@en ;
	rdfs:comment "HealthOfWomen is a term used to include all the health issues related to female gender."@en .

<http://observedchange.com/moac/ns#HighlyVulnerable> a <http://www.w3.org/2002/07/owl#Class> ;
	rdfs:isDefinedBy <http://observedchange.com/moac/ns> ;
	rdfs:label "MedicalEmergency"@en ;
	rdfs:comment "High possibility of loss resulting from the occurrence of the phenomenon."@en .

<http://observedchange.com/moac/ns#HospitalOperating> a <http://www.w3.org/2002/07/owl#Class> ;
	rdfs:isDefinedBy <http://observedchange.com/moac/ns> ;
	rdfs:label "HospitalOperating"@en ;
	rdfs:comment "HospitalOperating describes still functioning hospital after a disaster."@en .

<http://observedchange.com/moac/ns#HumanRemainsManagement> a <http://www.w3.org/2002/07/owl#Class> ;
	rdfs:isDefinedBy <http://observedchange.com/moac/ns> ;
	rdfs:label "HumanRemainsManagement"@en ;
	rdfs:comment "HumanRemainsManagement is an abstract term used to define morgues or other locations where dead bodies can be properlay managed."@en .

<http://observedchange.com/moac/ns#IDPConcentration> a <http://www.w3.org/2002/07/owl#Class> ;
	rdfs:isDefinedBy <http://observedchange.com/moac/ns> ;
	rdfs:label "IDPConcentration"@en ;
	rdfs:comment "IDPConcentration refers to the act of internally displaced people gathering in a certain location, which could eventually turn into an IDP camp."@en .

<http://observedchange.com/moac/ns#Incident> a <http://www.w3.org/2002/07/owl#Class> ;
	rdfs:isDefinedBy <http://observedchange.com/moac/ns> ;
	rdfs:label "Incident"@en ;
	rdfs:comment "Incident is a distinct or definite event."@en .

<http://observedchange.com/moac/ns#InfectiousHumanDisease> a <http://www.w3.org/2002/07/owl#Class> ;
	rdfs:isDefinedBy <http://observedchange.com/moac/ns> ;
	rdfs:label "InfectiousHumanDisease"@en ;
	rdfs:comment "InfectiousHumanDisease comprise of clinically evident illness resulting from the infection, presence and growth of pathogenic biological agents in an individual host organism that could also infect others."@en .

<http://observedchange.com/moac/ns#InfrastructureDamage> a <http://www.w3.org/2002/07/owl#Class> ;
	rdfs:isDefinedBy <http://observedchange.com/moac/ns> ;
	rdfs:label "InfrastructureDamage"@en ;
	rdfs:comment "InfrastureDamage is about the damage of physically existing basic facilities, services, and installations needed for the functioning of a community or society."@en .

<http://observedchange.com/moac/ns#InternetAccess> a <http://www.w3.org/2002/07/owl#Class> ;
	rdfs:isDefinedBy <http://observedchange.com/moac/ns> ;
	rdfs:label "InternetAccess"@en ;
	rdfs:comment "InternetAccess refers to certain place that can provide internet services."@en .

<http://observedchange.com/moac/ns#Landslides> a <http://www.w3.org/2002/07/owl#Class> ;
	rdfs:isDefinedBy <http://observedchange.com/moac/ns> ;
	rdfs:label "Landslides"@en ;
	rdfs:comment "A landslide is a geological phenomenon which includes a wide range of ground movement."@en .

<http://observedchange.com/moac/ns#Looting> a <http://www.w3.org/2002/07/owl#Class> ;
	rdfs:isDefinedBy <http://observedchange.com/moac/ns> ;
	rdfs:label "Looting"@en ;
	rdfs:comment "Looting is term that indicate a form of criminal activity when disaster affected people forcefully take away the relief distribution materials."@en .

<http://observedchange.com/moac/ns#MedicalEmergency> a <http://www.w3.org/2002/07/owl#Class> ;
	rdfs:isDefinedBy <http://observedchange.com/moac/ns> ;
	rdfs:label "MedicalEmergency"@en ;
	rdfs:comment "A medical emergency is an injury that is acute and poses an immediate risk to a person's life or long term health."@en .

<http://observedchange.com/moac/ns#MedicalEquipmentAndSupplyNeeds> a <http://www.w3.org/2002/07/owl#Class> ;
	rdfs:isDefinedBy <http://observedchange.com/moac/ns> ;
	rdfs:label "MedicalEquipmentAndSupplyNeeds"@en ;
	rdfs:comment "MedicalEquipmentAndSupplyNeeds is a term describe the demand for Medical Equipment and Supplies."@en .

<http://observedchange.com/moac/ns#Menaces> a <http://www.w3.org/2002/07/owl#Class> ;
	rdfs:isDefinedBy <http://observedchange.com/moac/ns> ;
	rdfs:label "Menaces"@en ;
	rdfs:comment "A Menace is a threat or danger that causes intimidation."@en .

<http://observedchange.com/moac/ns#MissingPersons> a <http://www.w3.org/2002/07/owl#Class> ;
	rdfs:isDefinedBy <http://observedchange.com/moac/ns> ;
	rdfs:label "MissingPersons"@en ;
	rdfs:comment "MissingPersons are persons whose whereabouts are unknown after sudden onset of disaster."@en .

<http://observedchange.com/moac/ns#NaturalHazards> a <http://www.w3.org/2002/07/owl#Class> ;
	rdfs:isDefinedBy <http://observedchange.com/moac/ns> ;
	rdfs:label "NaturalHazards"@en ;
	rdfs:comment "NaturalHazards is a term represent a threat of a naturally occurring event that will have a negative effect on people or the environment ."@en .

<http://observedchange.com/moac/ns#NonfoodAidDistributionPoint> a <http://www.w3.org/2002/07/owl#Class> ;
	rdfs:isDefinedBy <http://observedchange.com/moac/ns> ;
	rdfs:label "NonfoodAidDistributionPoint"@en ;
	rdfs:comment "NonfoodAidDistributionPoint is a location for distributing or transporting life saving Non Food Item other than food items, also known as NFIs in humaniatarian sphere."@en .

<http://observedchange.com/moac/ns#Others> a <http://www.w3.org/2002/07/owl#Class> ;
	rdfs:isDefinedBy <http://observedchange.com/moac/ns> ;
	rdfs:label "Others"@en ;
	rdfs:comment "Others is the class that is used when certain instance does not fit any of the classes. (Source:Ushahidi Haiti)"@en .

<http://observedchange.com/moac/ns#PeopleTrapped> a <http://www.w3.org/2002/07/owl#Class> ;
	rdfs:isDefinedBy <http://observedchange.com/moac/ns> ;
	rdfs:label "PeopleTrapped"@en ;
	rdfs:comment "People found in dangerous stituation might not be able to escape from the place they are."@en .

<http://observedchange.com/moac/ns#PersonsNews> a <http://www.w3.org/2002/07/owl#Class> ;
	rdfs:isDefinedBy <http://observedchange.com/moac/ns> ;
	rdfs:label "PersonsNews"@en ;
	rdfs:comment "PersonNews is the information about a person's status, e.g. death, injured, alive etc."@en .

<http://observedchange.com/moac/ns#PortOpen> a <http://www.w3.org/2002/07/owl#Class> ;
	rdfs:isDefinedBy <http://observedchange.com/moac/ns> ;
	rdfs:label "PortOpen"@en ;
	rdfs:comment "PortOpen is the term that indicate a port opening of regular business for receiving humanitarian relief materials."@en .

<http://observedchange.com/moac/ns#PowerOutage> a <http://www.w3.org/2002/07/owl#Class> ;
	rdfs:isDefinedBy <http://observedchange.com/moac/ns> ;
	rdfs:label "PowerOutage"@en ;
	rdfs:comment "A PowerOutage is a term which refers to electrical power failure, which means a short- or long-term loss of the electric power to an area."@en .

<http://observedchange.com/moac/ns#PriceGouging> a <http://www.w3.org/2002/07/owl#Class> ;
	rdfs:isDefinedBy <http://observedchange.com/moac/ns> ;
	rdfs:label "PriceGouging"@en ;
	rdfs:comment "PriceGouging is a pejorative term referring to a situation in which a seller prices goods or commodities much higher than is considered reasonable or fair."@en .

<http://observedchange.com/moac/ns#PsychiatricNeed> a <http://www.w3.org/2002/07/owl#Class> ;
	rdfs:isDefinedBy <http://observedchange.com/moac/ns> ;
	rdfs:label "PsychiatricNeed"@en ;
	rdfs:comment "PsychiatricNeed is a term indicate that people need medical care for mental disorders."@en .

<http://observedchange.com/moac/ns#PublicHealth> a <http://www.w3.org/2002/07/owl#Class> ;
	rdfs:isDefinedBy <http://observedchange.com/moac/ns> ;
	rdfs:label "PublicHealth"@en ;
	rdfs:comment "PublicHealth is a term that deals with overall health related issues, conerns and initiatives for or in a community ."@en .

<http://observedchange.com/moac/ns#Riot> a <http://www.w3.org/2002/07/owl#Class> ;
	rdfs:isDefinedBy <http://observedchange.com/moac/ns> ;
	rdfs:label "Riot"@en ;
	rdfs:comment "A riot is a form of civil disorder characterized often by disorganized groups lashing out in a sudden and intense rash of violence against authority, property or people."@en .

<http://observedchange.com/moac/ns#RoadBlocked> a <http://www.w3.org/2002/07/owl#Class> ;
	rdfs:isDefinedBy <http://observedchange.com/moac/ns> ;
	rdfs:label "RoadBlocked"@en ;
	rdfs:comment "RoadBlocked indicate a road is blocked by a barricade caused by natural disaster or set up by human."@en .

<http://observedchange.com/moac/ns#RubbleRemoval> a <http://www.w3.org/2002/07/owl#Class> ;
	rdfs:isDefinedBy <http://observedchange.com/moac/ns> ;
	rdfs:label "RubbleRemoval"@en ;
	rdfs:comment "RubbleRemoval is a term about the agreed upon and systamatic disopsal of of broken stone, of irregular size, shape and texture from a locaktion with totally damaged or partially damaged infrastructures."@en .

<http://observedchange.com/moac/ns#SearchAndRescue> a <http://www.w3.org/2002/07/owl#Class> ;
	rdfs:isDefinedBy <http://observedchange.com/moac/ns> ;
	rdfs:label "SearchAndRescue"@en ;
	rdfs:comment "SearchAndRescue is a part of humanitarian relief effort on the immediate on set of disaster where a team of experts try and locate missing persons."@en .

<http://observedchange.com/moac/ns#SecurityConcern> a <http://www.w3.org/2002/07/owl#Class> ;
	rdfs:isDefinedBy <http://observedchange.com/moac/ns> ;
	rdfs:label "SecurityConcern"@en ;
	rdfs:comment "SecurityConcern is a abstract term related to the worries of protection against danger, damage, loss, and criminal activity."@en .

<http://observedchange.com/moac/ns#ServiceAvailable> a <http://www.w3.org/2002/07/owl#Class> ;
	rdfs:isDefinedBy <http://observedchange.com/moac/ns> ;
	rdfs:label "ServiceAvailable"@en ;
	rdfs:comment "ServiceAvailable is an abstract term that indicates availability of different life saving and sustaining services in a disaster struck location/place."@en .

<http://observedchange.com/moac/ns#ShelterNeeded> rdfs:isDefinedBy <http://observedchange.com/moac/ns> ;
	rdfs:comment "ShelterNeeded is a term used to indicate number of emergency life saving basic structures like tents and tarpaulins."@en .

<http://observedchange.com/moac/ns#ShelterOffered> rdfs:isDefinedBy <http://observedchange.com/moac/ns> ;
	rdfs:comment "ShelterOffered indicates a location where internally displace people have been offered termporary/transitional shelters."@en .

<http://observedchange.com/moac/ns#TheftOfAid> a <http://www.w3.org/2002/07/owl#Class> ;
	rdfs:isDefinedBy <http://observedchange.com/moac/ns> ;
	rdfs:label "TheftOfAid"@en ;
	rdfs:comment "TheftOfAid is a term that indicate a form of criminal activity when unknown person(s) steal the relief distribution materials either from gowdown or relief distribution points."@en .

<http://observedchange.com/moac/ns#UnstableStructure> a <http://www.w3.org/2002/07/owl#Class> ;
	rdfs:isDefinedBy <http://observedchange.com/moac/ns> ;
	rdfs:label "UnstableStructure"@en ;
	rdfs:comment "UnstableStructure is a term that describe a partially damaged bulidings/structures which is still standing but uninhabitable."@en .

<http://observedchange.com/moac/ns#UshahidiReport> a <http://www.w3.org/2002/07/owl#Class> ;
	rdfs:isDefinedBy <http://observedchange.com/moac/ns> ;
	rdfs:label "UshahidiReport"@en ;
	rdfs:comment "UshahidiReport is a report from Ushahidi, contains simultaneously temporal and geospatial archive of events, based on the local observers' reports."@en .

<http://observedchange.com/moac/ns#VitalLines> a <http://www.w3.org/2002/07/owl#Class> ;
	rdfs:isDefinedBy <http://observedchange.com/moac/ns> ;
	rdfs:label "VitalLines"@en ;
	rdfs:comment "Vitallines is an abstract term that refer to particulars that could directly impact human lives."@en .

<http://observedchange.com/moac/ns#WaterSanitationAndHygienePromotion> a <http://www.w3.org/2002/07/owl#Class> ;
	rdfs:isDefinedBy <http://observedchange.com/moac/ns> ;
	rdfs:label "WaterSanitationAndHygienePromotion"@en ;
	rdfs:comment "WaterSanitationAndHygienePromotion is a term refers to a concept that improving access to safe water and sanitation facilities leads to healthier families and communities. (UNICEF)"@en .

<http://observedchange.com/moac/ns#WaterShortage> a <http://www.w3.org/2002/07/owl#Class> ;
	rdfs:isDefinedBy <http://observedchange.com/moac/ns> ;
	rdfs:label "WaterShortage"@en ;
	rdfs:comment "Watershortage is a term used to refer to the situations that water resources can not meet human demand."@en .

<http://observedchange.com/moac/ns#WaterDistributionPoint> a <http://www.w3.org/2002/07/owl#Class> ;
	rdfs:isDefinedBy <http://observedchange.com/moac/ns> ;
	rdfs:label "WaterDistributionPoint"@en ;
	rdfs:comment "WaterDistributionPoint is a location for distributing or transporting daily water to the disaster affected communities."@en .

<http://observedchange.com/moac/ns#affectedby> rdfs:comment "affectedby indicates disaster which has influence on population."@en ;
	rdfs:range <http://observedchange.com/moac/ns#AffectedPopulation> , <http://observedchange.com/moac/ns#NaturalHazard> .

<http://observedchange.com/moac/ns#approved> a <http://www.w3.org/2002/07/owl#DataProperty> ;
	rdfs:isDefinedBy <http://observedchange.com/moac/ns> ;
	rdfs:label "approved"@en ;
	rdfs:comment "approved is a data property to attest a event or incident or document is true or not."@en ;
	rdfs:domain <http://observedchange.com/moac/ns#Agency> ;
	rdfs:range <http://www.w3.org/2001/XMLSchema#boolean> .

<http://observedchange.com/moac/ns#atLocation> a <http://www.w3.org/2002/07/owl#DataProperty> ;
	rdfs:isDefinedBy <http://observedchange.com/moac/ns> ;
	rdfs:label "atLocation"@en ;
	rdfs:comment "atLocation is a data property to attest agency to a certain location."@en ;
	rdfs:domain <http://observedchange.com/moac/ns#Who3W> ;
	rdfs:range <http://www.w3.org/2001/XMLSchema#string> .

<http://observedchange.com/moac/ns#atGeoLocationLatitude> a <http://www.w3.org/2002/07/owl#DataProperty> ;
	rdfs:isDefinedBy <http://observedchange.com/moac/ns> ;
	rdfs:label "atLocation"@en ;
	rdfs:comment "atGeoLocationLatitude is a data property used to link location or \"Where\" with specific latitude in the form of decimal degree."@en ;
	rdfs:domain <http://observedchange.com/moac/ns#Where3W> ;
	rdfs:range <http://www.w3.org/2001/XMLSchema#float> .

<http://observedchange.com/moac/ns#atGeoLocationLongitude> a <http://www.w3.org/2002/07/owl#DataProperty> ;
	rdfs:isDefinedBy <http://observedchange.com/moac/ns> ;
	rdfs:label "atLocation"@en ;
	rdfs:comment "GeoLocationLatitude is a data property used to link location or \"Where\" with specific longitude in the form of decimal degree."@en ;
	rdfs:domain <http://observedchange.com/moac/ns#Where3W> ;
	rdfs:range <http://www.w3.org/2001/XMLSchema#float> .

<http://observedchange.com/moac/ns#category> a <http://www.w3.org/2002/07/owl#DataProperty> ;
	rdfs:isDefinedBy <http://observedchange.com/moac/ns> ;
	rdfs:label "title"@en ;
	rdfs:comment "category is about the sort of an incident."@en ;
	rdfs:domain <http://observedchange.com/moac/ns#Incident> ;
	rdfs:range <http://www.w3.org/2001/XMLSchema#string> .

<http://observedchange.com/moac/ns#date> a <http://www.w3.org/2002/07/owl#DataProperty> ;
	rdfs:isDefinedBy <http://observedchange.com/moac/ns> ;
	rdfs:label "date"@en ;
	rdfs:comment "date indicates a particular date."@en ;
	rdfs:range <http://purl.org/dc/elements/1.1/date> .

<http://observedchange.com/moac/ns#description> a <http://www.w3.org/2002/07/owl#DataProperty> ;
	rdfs:isDefinedBy <http://observedchange.com/moac/ns> ;
	rdfs:label "title"@en ;
	rdfs:comment "description is about the content of an incident."@en ;
	rdfs:domain <http://observedchange.com/moac/ns#Incident> ;
	rdfs:range <http://www.w3.org/2001/XMLSchema#string> .

<http://observedchange.com/moac/ns#impact> a <http://www.w3.org/2002/07/owl#DataProperty> ;
	rdfs:isDefinedBy <http://observedchange.com/moac/ns> ;
	rdfs:label "impact"@en ;
	rdfs:comment "Impact is the effect or impression of disaster on population or infrastructure"@en ;
	rdfs:range <http://observedchange.com/moac/ns#NaturalHazard> , <http://observedchange.com/moac/ns#AffectedPopulation> , <http://observedchange.com/moac/ns#InfrastructureDamage> .

<http://observedchange.com/moac/ns#title> a <http://www.w3.org/2002/07/owl#DataProperty> ;
	rdfs:isDefinedBy <http://observedchange.com/moac/ns> ;
	rdfs:label "title"@en ;
	rdfs:comment "Title is an identifying name given to an incident."@en ;
	rdfs:domain <http://observedchange.com/moac/ns#Incident> ;
	rdfs:range <http://www.w3.org/2001/XMLSchema#string> .

<http://observedchange.com/moac/ns#verified> a <http://www.w3.org/2002/07/owl#DataProperty> ;
	rdfs:isDefinedBy <http://observedchange.com/moac/ns> ;
	rdfs:label "verified"@en ;
	rdfs:comment "verified is a property used in describing if certain information/data has been checked with more than one sources."@en ;
	rdfs:domain <http://observedchange.com/moac/ns#Agency> ;
	rdfs:range <http://www.w3.org/2001/XMLSchema#boolean> .

<http://www.observedchange.com/moac/ns#> prv:createdBy _:node172hmq1dux2 .

_:node172hmq1dux2 a prv:DataCreation ;
	prv:performedBy <http://kauppinen.net/tomi#me> ;
	prv:performedAt "2012-01-29T20:30:00Z"^^<http://www.w3.org/2001/XMLSchema#dateTime> .
