@prefix dc: <http://purl.org/dc/elements/1.1/> .
@prefix dat: <http://contextus.net/ontology/ontomedia/misc/date#> .
@prefix rdfs: <http://www.w3.org/2000/01/rdf-schema#> .
@prefix dct: <http://purl.org/dc/terms/> .
@prefix xsd: <http://www.w3.org/2001/XMLSchema#> .
@prefix owl: <http://www.w3.org/2002/07/owl#> .
@prefix rdf: <http://www.w3.org/1999/02/22-rdf-syntax-ns#> .
@prefix locspec: <http://contextus.net/ontology/ontomedia/misc/locspec#> .

<http://contextus.net/ontology/ontomedia/core/expression#> a owl:Ontology ;
	rdfs:label "OntoMedia Core" ;
	dc:title "OntoMedia Core"@en ;
	dc:description "OntoMedia (Ontology for Media) has been designed to describe the interactions occurring in multimedia."@en ;
	dc:creator "Michael O. Jewell (mailto:moj@ecs.soton.ac.uk)" , "K Faith Lawrence (mailto:kf03r@ecs.soton.ac.uk)" , "Mischa M Tuffield (mailto:mmt04r@ecs.soton.ac.uk)" ;
	dct:created "2005-05-03" ;
	owl:versionInfo "0.32" .

<http://contextus.net/ontology/ontomedia/core/expression#Expression> a owl:Class ;
	rdfs:label "Expression" ;
	rdfs:comment "This class represents a piece of information conveyed through a media" .

<http://contextus.net/ontology/ontomedia/core/expression#is-linked-to> a owl:ObjectProperty ;
	rdfs:label "Is Linked To" ;
	rdfs:comment "This property indicates that there is some type of link between the named Expressions" ;
	owl:inverseOf <http://contextus.net/ontology/ontomedia/core/expression#is-not-linked-to> ;
	rdfs:domain <http://contextus.net/ontology/ontomedia/core/expression#Expression> ;
	rdfs:range <http://contextus.net/ontology/ontomedia/core/expression#Expression> .

<http://contextus.net/ontology/ontomedia/core/expression#is-not-linked-to> a owl:ObjectProperty ;
	rdfs:label "Is Not Linked To" ;
	rdfs:comment "This property indicates that there is some no link between the named Expressions" ;
	owl:inverseOf <http://contextus.net/ontology/ontomedia/core/expression#is-linked-to> ;
	rdfs:domain <http://contextus.net/ontology/ontomedia/core/expression#Expression> ;
	rdfs:range <http://contextus.net/ontology/ontomedia/core/expression#Expression> .

<http://contextus.net/ontology/ontomedia/core/expression#contains> a owl:ObjectProperty ;
	rdfs:label "Contains" ;
	rdfs:comment "This property indicates that one expression contains the other" ;
	owl:inverseOf <http://contextus.net/ontology/ontomedia/core/expression#contained-by> ;
	rdfs:subPropertyOf <http://contextus.net/ontology/ontomedia/core/expression#is-linked-to> ;
	rdfs:range <http://contextus.net/ontology/ontomedia/core/expression#Expression> ;
	rdfs:domain <http://contextus.net/ontology/ontomedia/core/expression#Expression> .

<http://contextus.net/ontology/ontomedia/core/expression#contained-by> a owl:ObjectProperty ;
	rdfs:label "Contained By" ;
	rdfs:comment "This property indicates that one expression is contained by the other" ;
	owl:inverseOf <http://contextus.net/ontology/ontomedia/core/expression#contains> ;
	rdfs:subPropertyOf <http://contextus.net/ontology/ontomedia/core/expression#is-linked-to> ;
	rdfs:range <http://contextus.net/ontology/ontomedia/core/expression#Expression> ;
	rdfs:domain <http://contextus.net/ontology/ontomedia/core/expression#Expression> .

<http://contextus.net/ontology/ontomedia/core/expression#is> a owl:ObjectProperty ;
	rdfs:label "Is" ;
	rdfs:comment "This property indicates that the expression is exactly the same as another" ;
	rdfs:subPropertyOf <http://contextus.net/ontology/ontomedia/core/expression#is-linked-to> ;
	owl:inverseOf <http://contextus.net/ontology/ontomedia/core/expression#is> ;
	rdfs:domain <http://contextus.net/ontology/ontomedia/core/expression#Expression> ;
	rdfs:range <http://contextus.net/ontology/ontomedia/core/expression#Expression> .

<http://contextus.net/ontology/ontomedia/core/expression#is-not> a owl:ObjectProperty ;
	rdfs:label "Is Not" ;
	rdfs:comment "This property indicates that the expression is entirely different to another" ;
	rdfs:subPropertyOf <http://contextus.net/ontology/ontomedia/core/expression#is-not-linked-to> ;
	owl:inverseOf <http://contextus.net/ontology/ontomedia/core/expression#is-not> ;
	rdfs:domain <http://contextus.net/ontology/ontomedia/core/expression#Expression> ;
	rdfs:range <http://contextus.net/ontology/ontomedia/core/expression#Expression> .

<http://contextus.net/ontology/ontomedia/core/expression#has-variant> a owl:ObjectProperty ;
	rdfs:label "Has Variant" ;
	rdfs:comment "This property indicates that the expression is a variation of another" ;
	rdfs:subPropertyOf <http://contextus.net/ontology/ontomedia/core/expression#is-linked-to> ;
	owl:inverseOf <http://contextus.net/ontology/ontomedia/core/has-variant> ;
	rdfs:range <http://contextus.net/ontology/ontomedia/core/expression#Expression> ;
	rdfs:domain <http://contextus.net/ontology/ontomedia/core/expression#Expression> .

<http://contextus.net/ontology/ontomedia/core/expression#has-shadow> a owl:ObjectProperty ;
	rdfs:label "Has Shadow" ;
	rdfs:comment "This property indicates that the expression is a variation on another, very similar but not exactly the same. For example the different interpretations of the same character" ;
	rdfs:subPropertyOf <http://contextus.net/ontology/ontomedia/core/expression#has-variant> ;
	owl:inverseOf <http://contextus.net/ontology/ontomedia/core/expression#is-shadow-of> ;
	rdfs:range <http://contextus.net/ontology/ontomedia/core/expression#Expression> ;
	rdfs:domain <http://contextus.net/ontology/ontomedia/core/expression#Expression> .

<http://contextus.net/ontology/ontomedia/core/expression#is-shadow-of> a owl:ObjectProperty ;
	rdfs:label "Is Shadow Of" ;
	rdfs:comment "This property indicates that the expression is a variation on another, very similar but not exactly the same. For example the different interpretations of the same character" ;
	rdfs:subPropertyOf <http://contextus.net/ontology/ontomedia/core/expression#has-variant> ;
	owl:inverseOf <http://contextus.net/ontology/ontomedia/core/expression#has-shadow> ;
	rdfs:range <http://contextus.net/ontology/ontomedia/core/expression#Expression> ;
	rdfs:domain <http://contextus.net/ontology/ontomedia/core/expression#Expression> .

<http://contextus.net/ontology/ontomedia/core/expression#has-spin-off> a owl:ObjectProperty ;
	rdfs:label "Has Spin Off" ;
	rdfs:comment "This property indicates that the expression has developed from another" ;
	rdfs:subPropertyOf <http://contextus.net/ontology/ontomedia/core/expression#has-variant> ;
	owl:inverseOf <http://contextus.net/ontology/ontomedia/core/expression#is-spin-off-of> ;
	rdfs:domain <http://contextus.net/ontology/ontomedia/core/expression#Item> ;
	rdfs:range <http://contextus.net/ontology/ontomedia/core/expression#Item> .

<http://contextus.net/ontology/ontomedia/core/expression#is-spin-off-of> a owl:ObjectProperty ;
	rdfs:label "Is Spin Off Of" ;
	rdfs:comment "This property indicates that the expression has developed from another" ;
	rdfs:subPropertyOf <http://contextus.net/ontology/ontomedia/core/expression#has-variant> ;
	owl:inverseOf <http://contextus.net/ontology/ontomedia/core/expression#has-spin-off> ;
	rdfs:domain <http://contextus.net/ontology/ontomedia/core/expression#Item> ;
	rdfs:range <http://contextus.net/ontology/ontomedia/core/expression#Item> .

<http://contextus.net/ontology/ontomedia/core/expression#inspired-by> a owl:ObjectProperty ;
	rdfs:label "Inspired By" ;
	rdfs:comment "This property indicates that the expression was inspired by another" ;
	rdfs:subPropertyOf <http://contextus.net/ontology/ontomedia/core/expression#has-variant> ;
	owl:inverseOf <http://contextus.net/ontology/ontomedia/core/expression#inspired> ;
	rdfs:domain <http://contextus.net/ontology/ontomedia/core/expression#Expression> ;
	rdfs:range <http://contextus.net/ontology/ontomedia/core/expression#Expression> .

<http://contextus.net/ontology/ontomedia/core/expression#inspired> a owl:ObjectProperty ;
	rdfs:label "Inspired" ;
	rdfs:comment "This property indicates that the expression inspired another" ;
	rdfs:subPropertyOf <http://contextus.net/ontology/ontomedia/core/expression#has-variant> ;
	owl:inverseOf <http://contextus.net/ontology/ontomedia/core/expression#inspired-by> ;
	rdfs:domain <http://contextus.net/ontology/ontomedia/core/expression#Expression> ;
	rdfs:range <http://contextus.net/ontology/ontomedia/core/expression#Expression> .

<http://contextus.net/ontology/ontomedia/core/expression#is-potentially> a owl:ObjectProperty ;
	rdfs:label "Is Potentially" ;
	rdfs:subPropertyOf <http://contextus.net/ontology/ontomedia/core/expression#has-variant> ;
	rdfs:range <http://contextus.net/ontology/ontomedia/core/expression#Expression> ;
	rdfs:domain <http://contextus.net/ontology/ontomedia/core/expression#Expression> ;
	rdfs:comment "This property indicates that the expression is potentially another. For example, it may be a possible future version" .

<http://contextus.net/ontology/ontomedia/core/expression#refers-to> a owl:ObjectProperty ;
	rdfs:label "Refers To" ;
	rdfs:range <http://contextus.net/ontology/ontomedia/core/expression#Expression> ;
	rdfs:domain <http://contextus.net/ontology/ontomedia/core/expression#Expression> ;
	owl:inverseOf <http://contextus.net/ontology/ontomedia/core/expression#referenced-by> ;
	rdfs:comment "This property indicates that the expression refers to another expression. This may be an event referring to a location, or a character refering to an event, etc." .

<http://contextus.net/ontology/ontomedia/core/expression#referenced-by> a owl:ObjectProperty ;
	rdfs:label "Refers To" ;
	rdfs:range <http://contextus.net/ontology/ontomedia/core/expression#Expression> ;
	rdfs:domain <http://contextus.net/ontology/ontomedia/core/expression#Expression> ;
	owl:inverseOf <http://contextus.net/ontology/ontomedia/core/expression#refers-to> ;
	rdfs:comment "This property indicates that the expression is refered to by another expression." .

<http://contextus.net/ontology/ontomedia/core/expression#Entity> a owl:Class ;
	rdfs:label "Entity" ;
	rdfs:comment "A thing" ;
	rdfs:subClassOf <http://contextus.net/ontology/ontomedia/core/expression#Expression> .

<http://contextus.net/ontology/ontomedia/core/expression#Item> a owl:Class ;
	rdfs:comment "This class represents an entity which may participate in an event within the media. An Item may be abstract or physical" ;
	rdfs:label "Item" ;
	rdfs:subClassOf <http://contextus.net/ontology/ontomedia/core/expression#Entity> .

<http://contextus.net/ontology/ontomedia/core/expression#Physical-Item> a owl:Class ;
	rdfs:comment "This class represents a physical entity which may participate in an event within the media" ;
	rdfs:label "Physical Item" ;
	rdfs:subClassOf <http://contextus.net/ontology/ontomedia/core/expression#Item> , <http://contextus.net/ontology/ontomedia/core/expression#Collection> .

<http://contextus.net/ontology/ontomedia/core/expression#Abstract-Item> a owl:Class ;
	rdfs:comment "This class represents an abstract entity which may participate in an event within the media" ;
	rdfs:label "Abstract Item" ;
	rdfs:subClassOf <http://contextus.net/ontology/ontomedia/core/expression#Item> .

<http://contextus.net/ontology/ontomedia/core/expression#Context> a owl:Class ;
	rdfs:comment "This class represents the context in which an event or entity exists" ;
	rdfs:label "Context" ;
	rdfs:subClassOf <http://contextus.net/ontology/ontomedia/core/expression#Abstract-Item> .

<http://contextus.net/ontology/ontomedia/core/expression#Collection> a owl:Class ;
	rdfs:comment "This class represents a collection of entities" ;
	rdfs:label "Collection" ;
	rdfs:subClassOf <http://contextus.net/ontology/ontomedia/core/expression#Abstract-Item> .

<http://contextus.net/ontology/ontomedia/core/expression#allows-existence-of> a owl:ObjectProperty ;
	rdfs:comment "This class represents that the desired expression may exist within the context" ;
	rdfs:label "Allows Existence Of" ;
	rdfs:domain <http://contextus.net/ontology/ontomedia/core/expression#Context> ;
	owl:inverseOf <http://contextus.net/ontology/ontomedia/core/expression#exists-in> ;
	rdfs:range <http://contextus.net/ontology/ontomedia/core/expression#Expression> .

<http://contextus.net/ontology/ontomedia/core/expression#exists-in> a owl:ObjectProperty ;
	rdfs:comment "This class represents that the expression exists within the related context" ;
	rdfs:label "Exists In" ;
	rdfs:domain <http://contextus.net/ontology/ontomedia/core/expression#Expression> ;
	owl:inverseOf <http://contextus.net/ontology/ontomedia/core/expression#allows-existence-of> ;
	rdfs:range <http://contextus.net/ontology/ontomedia/core/expression#Context> .

<http://contextus.net/ontology/ontomedia/core/expression#has-number-of-parts> a owl:ObjectProperty ;
	rdfs:label "Has Number Of Parts" ;
	rdfs:comment "This property specifies the number of parts contained by the collection" ;
	rdfs:domain <http://contextus.net/ontology/ontomedia/core/expression#Collection> ;
	rdfs:range rdfs:Literal .

<http://contextus.net/ontology/ontomedia/core/expression#has-max-number-of-parts> a owl:ObjectProperty ;
	rdfs:label "Has Maximum Number Of Parts" ;
	rdfs:comment "This property specifies the maximum number of parts that can be contained by the collection" ;
	rdfs:domain <http://contextus.net/ontology/ontomedia/core/expression#Collection> ;
	rdfs:range rdfs:Literal .

<http://contextus.net/ontology/ontomedia/core/expression#has-min-number-of-parts> a owl:ObjectProperty ;
	rdfs:label "Has Minimum Number Of Parts" ;
	rdfs:comment "This property specifies the minimum number of parts that can be contained by the collection" ;
	rdfs:domain <http://contextus.net/ontology/ontomedia/core/expression#Collection> ;
	rdfs:range rdfs:Literal .

<http://contextus.net/ontology/ontomedia/core/expression#Timeline> a owl:Class ;
	rdfs:comment "This class contains a sequence of occurring events" ;
	rdfs:label "Timeline" ;
	rdfs:subClassOf <http://contextus.net/ontology/ontomedia/core/expression#Entity> .

<http://contextus.net/ontology/ontomedia/core/expression#Occurrence> a owl:Class ;
	rdfs:comment "This class represents a single occurrence of an event, placing it at a position in a timeline" ;
	rdfs:label "Occurrence" ;
	rdfs:subClassOf <http://contextus.net/ontology/ontomedia/core/expression#Entity> .

<http://contextus.net/ontology/ontomedia/core/expression#timeline-ref> a owl:ObjectProperty ;
	rdfs:label "Timeline Reference" ;
	rdfs:comment "Reference to the Timeline that the Occurrence exists on" ;
	rdfs:range <http://contextus.net/ontology/ontomedia/core/expression#Timeline> ;
	rdfs:domain <http://contextus.net/ontology/ontomedia/core/expression#Occurrence> .

<http://contextus.net/ontology/ontomedia/core/expression#occurrence-of> a owl:ObjectProperty ;
	rdfs:label "Occurrence Of" ;
	rdfs:comment "This property defines any the event that the occurrence relates to" ;
	owl:inverseOf <http://contextus.net/ontology/ontomedia/core/expression#has-occurrence> ;
	rdfs:domain <http://contextus.net/ontology/ontomedia/core/expression#Occurrence> ;
	rdfs:range <http://contextus.net/ontology/ontomedia/core/expression#Event> .

<http://contextus.net/ontology/ontomedia/core/expression#precedes> a owl:ObjectProperty ;
	rdfs:label "Precedes" ;
	rdfs:comment "This property defines the occurrence which immediately follows this occurrence" ;
	rdfs:range <http://contextus.net/ontology/ontomedia/core/expression#Occurrence> ;
	rdfs:domain <http://contextus.net/ontology/ontomedia/core/expression#Occurrence> ;
	owl:inverseOf <http://contextus.net/ontology/ontomedia/core/expression#follows> .

<http://contextus.net/ontology/ontomedia/core/expression#follows> a owl:ObjectProperty ;
	rdfs:label "Follows" ;
	rdfs:comment "Follows specifies the occurrence that happens after the referencing occurrence" ;
	rdfs:range <http://contextus.net/ontology/ontomedia/core/expression#Occurrence> ;
	rdfs:domain <http://contextus.net/ontology/ontomedia/core/expression#Occurrence> ;
	owl:inverseOf <http://contextus.net/ontology/ontomedia/core/expression#precedes> .

<http://contextus.net/ontology/ontomedia/core/expression#TAQ> a owl:ObjectProperty ;
	rdfs:label "Period Terminal Limit" ;
	rdfs:comment "Terminus Ante Quem (Limit Before Which): The latest date that the period the event covers could have happened" ;
	rdfs:domain <http://contextus.net/ontology/ontomedia/core/expression#Occurrence> ;
	rdfs:range dat:Date .

<http://contextus.net/ontology/ontomedia/core/expression#TPQ> a owl:ObjectProperty ;
	rdfs:label "Temporal Start" ;
	rdfs:comment "The time/date/temporal reference for the start of the event" ;
	rdfs:range dat:Date ;
	rdfs:domain <http://contextus.net/ontology/ontomedia/core/expression#Occurrence> .

<http://contextus.net/ontology/ontomedia/core/expression#StartTime> a owl:ObjectProperty ;
	rdfs:label "Temporal End" ;
	rdfs:comment "The time/date/temporal reference for the start of the event" ;
	rdfs:domain <http://contextus.net/ontology/ontomedia/core/expression#Occurrence> ;
	rdfs:range dat:Date .

<http://contextus.net/ontology/ontomedia/core/expression#EndTime> a owl:ObjectProperty ;
	rdfs:label "Period Initial Limit" ;
	rdfs:comment "The time/date/temporal reference for the end of the event" ;
	rdfs:range dat:Date ;
	rdfs:domain <http://contextus.net/ontology/ontomedia/core/expression#Occurrence> .

<http://contextus.net/ontology/ontomedia/core/expression#DiscreteTime> a owl:ObjectProperty ;
	rdfs:label "Time/Date" ;
	rdfs:comment "The time/date/temporal reference for the the event" ;
	rdfs:domain <http://contextus.net/ontology/ontomedia/core/expression#Occurrence> ;
	rdfs:range dat:Date .

<http://contextus.net/ontology/ontomedia/core/expression#occurs> a owl:FunctionalProperty ;
	rdfs:label "Occurs" ;
	rdfs:comment "This property specifies the region of media in when an event occurrence happens" ;
	rdfs:range locspec:LocSpec ;
	rdfs:domain <http://contextus.net/ontology/ontomedia/core/expression#Occurrence> .

<http://contextus.net/ontology/ontomedia/core/expression#start-point> a owl:FunctionalProperty ;
	rdfs:label "Start point in Media" ;
	rdfs:comment "This property specifies the point in the media at which the event occurrence starts happening" ;
	rdfs:domain <http://contextus.net/ontology/ontomedia/core/expression#Occurrence> ;
	rdfs:range locspec:LocSpec .

<http://contextus.net/ontology/ontomedia/core/expression#has-duration> a owl:FunctionalProperty ;
	rdfs:label "Duration of Occurrence" ;
	rdfs:comment "This property specifies the duration of the occurrence" ;
	rdfs:domain <http://contextus.net/ontology/ontomedia/core/expression#Occurrence> ;
	rdfs:range _:node17168lu6gx22 .

_:node17168lu6gx22 a owl:Class ;
	owl:unionOf _:node17168lu6gx23 .

_:node17168lu6gx23 rdf:first locspec:LocSpec .

locspec:LocSpec a owl:Class .

_:node17168lu6gx23 rdf:rest _:node17168lu6gx24 .

_:node17168lu6gx24 rdf:first <http://contextus.net/ontology/ontomedia/ext/common/trait#Dimension> .

<http://contextus.net/ontology/ontomedia/ext/common/trait#Dimension> a owl:Class .

_:node17168lu6gx24 rdf:rest rdf:nil .

<http://contextus.net/ontology/ontomedia/core/expression#end-point> a owl:ObjectProperty ;
	rdfs:label "End Point in Media" ;
	rdfs:comment "This property specifies the point in the media at which the event occurrence stops happening" ;
	rdfs:range locspec:LocSpec ;
	rdfs:domain <http://contextus.net/ontology/ontomedia/core/expression#Occurrence> .

<http://contextus.net/ontology/ontomedia/core/expression#MediaTPQ> a owl:ObjectProperty ;
	rdfs:label "Media Start Period Limit" ;
	rdfs:comment "This property specifies the earliest point in the media at which the event occurrence could have happened" ;
	rdfs:range locspec:LocSpec ;
	rdfs:comment "Terminus Post Quem (Limit After Which): The earliest point that the period the event covers could be said to be happening" ;
	rdfs:domain <http://contextus.net/ontology/ontomedia/core/expression#Occurrence> .

<http://contextus.net/ontology/ontomedia/core/expression#MediaTAQ> a owl:ObjectProperty ;
	rdfs:label "Media End Period Limit" ;
	rdfs:comment "Terminus Ante Quem (Limit Before Which): The latest point that the period the event covers could have happened" ;
	rdfs:domain <http://contextus.net/ontology/ontomedia/core/expression#Occurrence> ;
	rdfs:range locspec:LocSpec .

<http://contextus.net/ontology/ontomedia/core/expression#Event> a owl:Class ;
	rdfs:label "Event" ;
	rdfs:comment "This property defines an event" ;
	rdfs:subClassOf <http://contextus.net/ontology/ontomedia/core/expression#Expression> .

<http://contextus.net/ontology/ontomedia/core/expression#final-event> a owl:ObjectProperty ;
	rdfs:domain <http://contextus.net/ontology/ontomedia/core/expression#Event> ;
	rdfs:range <http://contextus.net/ontology/ontomedia/core/expression#Event> .

<http://contextus.net/ontology/ontomedia/core/expression#initial-event> a owl:ObjectProperty ;
	rdfs:comment "the first event which begins this sequence" ;
	rdfs:domain <http://contextus.net/ontology/ontomedia/core/expression#Event> ;
	rdfs:range <http://contextus.net/ontology/ontomedia/core/expression#Event> .

<http://contextus.net/ontology/ontomedia/core/expression#has-subject-entity> a owl:ObjectProperty ;
	rdfs:label "Has Subject Entity" ;
	rdfs:comment "This property specifies the entity which carries out the aim of the event" ;
	rdfs:domain <http://contextus.net/ontology/ontomedia/core/expression#Event> ;
	rdfs:range <http://contextus.net/ontology/ontomedia/core/expression#Entity> .

<http://contextus.net/ontology/ontomedia/core/expression#has-object-entity> a owl:ObjectProperty ;
	rdfs:label "Has Object Entity" ;
	rdfs:comment "This property specifies the entity which is the target of the event" ;
	rdfs:range <http://contextus.net/ontology/ontomedia/core/expression#Entity> ;
	rdfs:domain <http://contextus.net/ontology/ontomedia/core/expression#Event> .

<http://contextus.net/ontology/ontomedia/core/expression#has-occurrence> a owl:ObjectProperty ;
	rdfs:label "Has occurrence" ;
	rdfs:comment "This property defines any occurrences of this event" ;
	rdfs:range <http://contextus.net/ontology/ontomedia/core/expression#Occurrence> ;
	rdfs:domain <http://contextus.net/ontology/ontomedia/core/expression#Event> ;
	owl:inverseOf <http://contextus.net/ontology/ontomedia/core/expression#occurrence-of> .

<http://contextus.net/ontology/ontomedia/core/expression#summary> a owl:FunctionalProperty ;
	rdfs:label "Summary" ;
	rdfs:domain <http://contextus.net/ontology/ontomedia/core/expression#Event> ;
	rdfs:range rdfs:Literal ;
	rdfs:comment "This property is a plain-text summery of what occurs in the event" .

<http://contextus.net/ontology/ontomedia/core/expression#precondition> a owl:ObjectProperty ;
	rdfs:label "Precondition" ;
	rdfs:comment "This property is a state that must exist before the event can occur" ;
	rdfs:range _:node17168lu6gx25 .

_:node17168lu6gx25 a owl:Class ;
	owl:unionOf _:node17168lu6gx26 .

_:node17168lu6gx26 rdf:first <http://contextus.net/ontology/ontomedia/core/expression#Entity> ;
	rdf:rest _:node17168lu6gx27 .

_:node17168lu6gx27 rdf:first <http://contextus.net/ontology/ontomedia/core/expression#Event> ;
	rdf:rest rdf:nil .

<http://contextus.net/ontology/ontomedia/core/expression#precondition> rdfs:domain <http://contextus.net/ontology/ontomedia/core/expression#Event> .

<http://contextus.net/ontology/ontomedia/core/expression#postcondition> a owl:ObjectProperty ;
	rdfs:label "Postcondition" ;
	rdfs:range _:node17168lu6gx28 .

_:node17168lu6gx28 a owl:Class ;
	owl:unionOf _:node17168lu6gx29 .

_:node17168lu6gx29 rdf:first <http://contextus.net/ontology/ontomedia/core/expression#Entity> ;
	rdf:rest _:node17168lu6gx30 .

_:node17168lu6gx30 rdf:first <http://contextus.net/ontology/ontomedia/core/expression#Event> ;
	rdf:rest rdf:nil .

<http://contextus.net/ontology/ontomedia/core/expression#postcondition> rdfs:comment "This property contains the state which should occur as a consequence of this event" ;
	rdfs:domain <http://contextus.net/ontology/ontomedia/core/expression#Event> .

<http://contextus.net/ontology/ontomedia/core/expression#involves> a owl:ObjectProperty ;
	rdfs:label "Involves" ;
	rdfs:comment "This property specifies the entities involved in this event. Note that this includes the subject and object." ;
	rdfs:range <http://contextus.net/ontology/ontomedia/core/expression#Entity> ;
	rdfs:domain <http://contextus.net/ontology/ontomedia/core/expression#Event> ;
	owl:inverseOf <http://contextus.net/ontology/ontomedia/core/expression#involved-in> .

<http://contextus.net/ontology/ontomedia/core/expression#involved-in> a owl:ObjectProperty ;
	rdfs:label "Involves" ;
	rdfs:comment "This property specifies the events involved in by this entity. Note that this includes the subject and object." ;
	rdfs:range <http://contextus.net/ontology/ontomedia/core/expression#Event> ;
	rdfs:domain <http://contextus.net/ontology/ontomedia/core/expression#Entity> ;
	owl:inverseOf <http://contextus.net/ontology/ontomedia/core/expression#involves> .

<http://contextus.net/ontology/ontomedia/core/expression#causes> a owl:ObjectProperty ;
	rdfs:label "Causes" ;
	rdfs:comment "This property indicates the instigating factor of an event, whether it be an item, event, or collection." ;
	rdfs:range _:node17168lu6gx31 .

_:node17168lu6gx31 a owl:Class ;
	owl:unionOf _:node17168lu6gx32 .

_:node17168lu6gx32 rdf:first <http://contextus.net/ontology/ontomedia/core/expression#Event> ;
	rdf:rest _:node17168lu6gx33 .

_:node17168lu6gx33 rdf:first <http://contextus.net/ontology/ontomedia/core/expression#Entity> ;
	rdf:rest rdf:nil .

<http://contextus.net/ontology/ontomedia/core/expression#causes> rdfs:domain _:node17168lu6gx34 .

_:node17168lu6gx34 a owl:Class ;
	owl:unionOf _:node17168lu6gx35 .

_:node17168lu6gx35 rdf:first <http://contextus.net/ontology/ontomedia/core/expression#Event> ;
	rdf:rest _:node17168lu6gx36 .

_:node17168lu6gx36 rdf:first <http://contextus.net/ontology/ontomedia/core/expression#Entity> ;
	rdf:rest rdf:nil .

<http://contextus.net/ontology/ontomedia/core/expression#causes> owl:inverseOf <http://contextus.net/ontology/ontomedia/core/expression#caused-by> .

<http://contextus.net/ontology/ontomedia/core/expression#caused-by> a owl:ObjectProperty ;
	rdfs:label "Caused By" ;
	rdfs:comment "This property indicates the instigating factor of an event, whether it be an item, event, or collection." ;
	rdfs:range _:node17168lu6gx37 .

_:node17168lu6gx37 a owl:Class ;
	owl:unionOf _:node17168lu6gx38 .

_:node17168lu6gx38 rdf:first <http://contextus.net/ontology/ontomedia/core/expression#Event> ;
	rdf:rest _:node17168lu6gx39 .

_:node17168lu6gx39 rdf:first <http://contextus.net/ontology/ontomedia/core/expression#Entity> ;
	rdf:rest rdf:nil .

<http://contextus.net/ontology/ontomedia/core/expression#caused-by> rdfs:domain _:node17168lu6gx40 .

_:node17168lu6gx40 a owl:Class ;
	owl:unionOf _:node17168lu6gx41 .

_:node17168lu6gx41 rdf:first <http://contextus.net/ontology/ontomedia/core/expression#Event> ;
	rdf:rest _:node17168lu6gx42 .

_:node17168lu6gx42 rdf:first <http://contextus.net/ontology/ontomedia/core/expression#Entity> ;
	rdf:rest rdf:nil .

<http://contextus.net/ontology/ontomedia/core/expression#caused-by> owl:inverseOf <http://contextus.net/ontology/ontomedia/core/expression#causes> .

<http://contextus.net/ontology/ontomedia/core/expression#Gain> a owl:Class ;
	rdfs:label "Gain" ;
	rdfs:subClassOf <http://contextus.net/ontology/ontomedia/core/expression#Event> ;
	rdfs:comment "This event class results in an overall increase of the entities related to the primary subject or subjects of the event" .

<http://contextus.net/ontology/ontomedia/core/expression#Introduction> a owl:Class ;
	rdfs:label "Introduction" ;
	rdfs:comment "This event class denotes the introduction of an entity to the media" ;
	rdfs:subClassOf <http://contextus.net/ontology/ontomedia/core/expression#Event> .

<http://contextus.net/ontology/ontomedia/core/expression#Loss> a owl:Class ;
	rdfs:label "Loss" ;
	rdfs:comment "This event class results in an overall reduction of the entities related to the primary subject or subjects of the event" ;
	rdfs:subClassOf <http://contextus.net/ontology/ontomedia/core/expression#Event> .

<http://contextus.net/ontology/ontomedia/core/expression#Transformation> a owl:Class ;
	rdfs:comment "This event class results in no gain or loss of attributes or entities, merely alteration" ;
	rdfs:label "Transformation" ;
	rdfs:subClassOf <http://contextus.net/ontology/ontomedia/core/expression#Event> .

<http://contextus.net/ontology/ontomedia/core/expression#Action> a owl:Class ;
	rdfs:comment "This event class describes an action sequence (ie no plot)" ;
	rdfs:label "Action" ;
	rdfs:subClassOf <http://contextus.net/ontology/ontomedia/core/expression#Event> .

<http://contextus.net/ontology/ontomedia/core/expression#Social> a owl:Class ;
	rdfs:comment "This event class describes a sequence focusing on social, interpersonal and personal emotional elements" ;
	rdfs:label "Social" ;
	rdfs:subClassOf <http://contextus.net/ontology/ontomedia/core/expression#Event> .

<http://contextus.net/ontology/ontomedia/core/expression#from> a owl:ObjectProperty ;
	rdfs:label "From" ;
	rdfs:comment "This property specifies the entity which is being transformed" ;
	rdfs:range <http://contextus.net/ontology/ontomedia/core/expression#Entity> ;
	rdfs:domain <http://contextus.net/ontology/ontomedia/core/expression#Transformation> .

<http://contextus.net/ontology/ontomedia/core/expression#to> a owl:ObjectProperty ;
	rdfs:label "To" ;
	rdfs:comment "This property specifies the resultant entity" ;
	rdfs:range <http://contextus.net/ontology/ontomedia/core/expression#Entity> ;
	rdfs:domain <http://contextus.net/ontology/ontomedia/core/expression#Transformation> .
