@prefix rev: <http://purl.org/stuff/rev#> .
@prefix foaf: <http://xmlns.com/foaf/0.1/> .
@prefix frbr: <http://purl.org/vocab/frbr/core#> .
@prefix vann: <http://purl.org/vocab/vann/> .
@prefix org: <http://www.w3.org/ns/org#> .
@prefix odapps: <http://semweb.mmlab.be/ns/odapps#> .
@prefix rdfs: <http://www.w3.org/2000/01/rdf-schema#> .
@prefix dcat: <http://www.w3.org/ns/dcat#> .
@prefix dct: <http://purl.org/dc/terms/> .
@prefix owl: <http://www.w3.org/2002/07/owl#> .
@prefix xsd: <http://www.w3.org/2001/XMLSchema#> .
@prefix rdf: <http://www.w3.org/1999/02/22-rdf-syntax-ns#> .
@prefix dvia: <http://purl.org/ontology/dvia#> .
@prefix cc: <http://creativecommons.org/ns#> .

<http://semweb.mmlab.be/ns/odapps> a owl:Ontology ;
	rdfs:comment "odapps is an RDF vocabulary defined to facilitate the description of Open-Data-based ideas and applications published on the Web."@en ;
	dct:title "The vocabulary for (L)OD ideas and applications"@en ;
	dct:issued "2013-05-10"^^xsd:date ;
	dct:modified "2014-01-14"^^xsd:date .

_:node18qipo0qvx1 foaf:mbox "Anastasia.Dimou@UGent.be" ;
	foaf:name "Anastasia Dimou" .

<http://semweb.mmlab.be/ns/odapps> dct:creator _:node18qipo0qvx1 .

_:node18qipo0qvx2 foaf:mbox "Pieter.Colpaert@UGent.be" ;
	foaf:name "Pieter Colpaert" .

<http://semweb.mmlab.be/ns/odapps> dct:creator _:node18qipo0qvx2 .

_:node18qipo0qvx3 foaf:mbox "rtroncy@eurecom.fr" ;
	foaf:name "Raphael Troncy" .

<http://semweb.mmlab.be/ns/odapps> dct:contributor _:node18qipo0qvx3 .

_:node18qipo0qvx4 foaf:mbox "atemezin@eurecom.fr" ;
	foaf:name "Ghislain Auguste Atemezing" .

<http://semweb.mmlab.be/ns/odapps> dct:contributor _:node18qipo0qvx4 ;
	cc:license <http://creativecommons.org/licenses/by/3.0/> ;
	vann:preferredNamespacePrefix "odapps" ;
	owl:versionInfo "1.1 - 2014-01-14" .

odapps:AppConcept a rdfs:Class ;
	rdfs:label "Application Concept"@en ;
	rdfs:comment "An App Concept describes an idea for an application (a digital work) which refers to Open Data."@en ;
	rdfs:subClassOf frbr:Work ;
	rdfs:isDefinedBy <http://semweb.mmlab.be/ns/odapps> .

dvia:Application rdfs:subClassOf odapps:Application .

odapps:Application a rdfs:Class ;
	rdfs:label "Application"@en ;
	rdfs:comment "An App Concept implementation." ;
	rdfs:isDefinedBy <http://semweb.mmlab.be/ns/odapps> .

dvia:VisualTool rdfs:subClassOf odapps:Tool .

odapps:Tool a rdfs:Class ;
	rdfs:comment "The tool or library used to build the application."@en ;
	rdfs:isDefinedBy <http://semweb.mmlab.be/ns/odapps> ;
	rdfs:label "Tool."@en .

odapps:conceived a rdf:Property ;
	rdfs:label "conceived by" ;
	rdfs:comment "The Agent which conceived the idea about the App Concept" ;
	rdfs:range foaf:Agent .

dvia:consumes rdfs:SubClassOf odapps:consumes .

odapps:consumes a rdf:Property , owl:ObjectProperty ;
	rdfs:comment "links to the dataset used to make the application, and could be of different types or formats" ;
	rdfs:domain odapps:Application , odapps:AppConcept ;
	rdfs:isDefinedBy <http://semweb.mmlab.be/ns/odapps> ;
	rdfs:label "consumes"@en ;
	rdfs:range dcat:Dataset , xsd:string .

odapps:comment a rdf:Property , owl:ObjectProperty ;
	rdfs:comment "comment on the application and the Concept" ;
	rdfs:domain odapps:Application , odapps:AppConcept ;
	rdfs:isDefinedBy <http://semweb.mmlab.be/ns/odapps> ;
	rdfs:label "comment"@en ;
	rdfs:range odapps:AppConcept , odapps:Application .

odapps:demoUri a rdf:Property , owl:ObjectProperty ;
	rdfs:comment "Property for a given demo of the application and/or the Concept."@en ;
	rdfs:domain odapps:AppConcept , odapps:Application ;
	rdfs:isDefinedBy <http://semweb.mmlab.be/ns/odapps> ;
	rdfs:label "demo uri"@en .

odapps:description a rdf:Property , owl:ObjectProperty ;
	rdfs:comment "Property for a given descriptive informations of the concept and/or the application."@en ;
	rdfs:domain odapps:AppConcept , odapps:Application ;
	rdfs:isDefinedBy <http://semweb.mmlab.be/ns/odapps> ;
	rdfs:label "Concept and/or Application description"@en .

odapps:datasetDescription a rdf:Property , owl:ObjectProperty ;
	rdfs:comment "Property for a given descriptive informations of the datasets used for making the application. It could be used when no more details are given on the datasets like URL, formats, etc."@en ;
	rdfs:domain odapps:AppConcept , odapps:Application ;
	rdfs:isDefinedBy <http://semweb.mmlab.be/ns/odapps> ;
	rdfs:label "dataset description"@en .

dvia:downloadUrl rdfs:subClassOf odapps:downloadUrl .

odapps:downloadUrl a rdf:Property ;
	rdfs:comment "This property links to the application"@en ;
	rdfs:domain odapps:Application ;
	rdfs:isDefinedBy <http://semweb.mmlab.be/ns/odapps> ;
	rdfs:label "download url"@en ;
	rdfs:range xsd:anyURI .

dvia:keyword rdfs:subPropertyOf odapps:keyword .

odapps:keyword a rdf:Property , owl:ObjectProperty ;
	rdfs:comment "The keywords of the Application."@en ;
	rdfs:domain odapps:AppConcept , odapps:Application ;
	rdfs:isDefinedBy <http://semweb.mmlab.be/ns/odapps> ;
	rdfs:label "dataset description"@en .

dvia:hasLicense rdfs:subPropertyOf odapps:license .

odapps:license a rdf:Property , owl:DatatypeProperty ;
	rdfs:comment "This property links to the license of the application" ;
	rdfs:domain odapps:Application ;
	rdfs:isDefinedBy <http://semweb.mmlab.be/ns/odapps> ;
	rdfs:label "has license"@en ;
	rdfs:range xsd:anyURI .

odapps:instigator a rdf:Property , owl:ObjectProperty ;
	rdfs:label "instigator"@en ;
	rdfs:comment "The Agent which conceived the idea about the App Concept (the instigator/initiator)."@en ;
	rdfs:isDefinedBy <http://semweb.mmlab.be/ns/odapps> ;
	rdfs:domain odapps:AppConcept ;
	rdfs:range foaf:Agent .

odapps:implements a rdf:Property , owl:ObjectProperty ;
	rdfs:label "implements"@en ;
	rdfs:comment "The App Concept that this application implements"@en ;
	rdfs:isDefinedBy <http://semweb.mmlab.be/ns/odapps> ;
	rdfs:domain odapps:Application ;
	rdfs:range odapps:AppConcept .

odapps:revision a rdf:Property ;
	rdfs:label "revision of" ;
	rdfs:comment "An App concept which was revised and re-posed / extended. " ;
	rdfs:isDefinedBy <http://semweb.mmlab.be/ns/odapps> ;
	rdfs:domain odapps:AppConcept ;
	rdfs:range odapps:AppConcept .

odapps:revised a rdf:Property , owl:ObjectProperty ;
	rdfs:label "revised"@en ;
	rdfs:comment "The Agent which revised / extended the idea about the App Concept."@en ;
	rdfs:isDefinedBy <http://semweb.mmlab.be/ns/odapps> ;
	rdfs:domain odapps:AppConcept ;
	rdfs:range foaf:Agent .

dvia:usesTool rdfs:subClassOf odapps:usesTool .

odapps:usesTool a rdf:Property ;
	rdfs:comment "This property links to the tools or libraries used for the application"@en ;
	rdfs:domain odapps:Application ;
	rdfs:isDefinedBy <http://semweb.mmlab.be/ns/odapps> ;
	rdfs:label "usesTool"@en ;
	rdfs:range odapps:Tool .

dvia:url rdfs:subClassOf odapps:url .

odapps:url a rdf:Property ;
	rdfs:comment "This property links to the application"@en ;
	rdfs:domain odapps:Application ;
	rdfs:isDefinedBy <http://semweb.mmlab.be/ns/odapps> ;
	rdfs:label "url"@en ;
	rdfs:range xsd:anyURI .

_:node18qipo0qvx5 foaf:mbox "Anastasia.Dimou@UGent.be" ;
	foaf:name "Anastasia Dimou" .

<http://semweb.mmlab.be/ns/odapps> dct:creator _:node18qipo0qvx5 .

_:node18qipo0qvx6 foaf:mbox "Pieter.Colpaert@UGent.be" ;
	foaf:name "Pieter Colpaert" .

<http://semweb.mmlab.be/ns/odapps> dct:creator _:node18qipo0qvx6 .

_:node18qipo0qvx7 foaf:mbox "rtroncy@eurecom.fr" ;
	foaf:name "Raphael Troncy" .

<http://semweb.mmlab.be/ns/odapps> dct:contributor _:node18qipo0qvx7 .

_:node18qipo0qvx8 foaf:mbox "atemezin@eurecom.fr" ;
	foaf:name "Ghislain Auguste Atemezing" .

<http://semweb.mmlab.be/ns/odapps> dct:contributor _:node18qipo0qvx8 .
