@prefix :      <http://lsdis.cs.uga.edu/projects/semdis/opus#> .
@prefix dc:    <http://purl.org/dc/elements/1.1/> .
@prefix rdfs:  <http://www.w3.org/2000/01/rdf-schema#> .
@prefix owl:   <http://www.w3.org/2002/07/owl#> .
@prefix rdf:   <http://www.w3.org/1999/02/22-rdf-syntax-ns#> .
@prefix opus:  <http://lsdis.cs.uga.edu/projects/semdis/opus#> .

opus:gMonth  a        owl:DatatypeProperty ;
        rdfs:comment  "The month part of the date of a foaf:Document represented as xsd:gMonth value" ;
        rdfs:domain   <http://xmlns.com/foaf/0.1/Document> ;
        rdfs:label    "gMonth" ;
        rdfs:range    <http://www.w3.org/2001/XMLSchema#gMonth> .

<http://purl.org/net/nknouf/ns/bibtex#hasISBN>
        a       owl:DatatypeProperty .

opus:Journal  a              owl:Class ;
        rdfs:comment         "A periodical presenting articles on a particular subject." ;
        rdfs:label           "Journal" ;
        rdfs:subClassOf      opus:Serial_Publication ;
        owl:equivalentClass  <http://sw-portal.deri.org/ontologies/swportal#Journal> , <http://www.aktors.org/ontology/portal#Journal> .

opus:Serial_Publication
        a                owl:Class ;
        rdfs:comment     "A periodical that appears at scheduled times." ;
        rdfs:label       "Serial Publication" ;
        rdfs:subClassOf  opus:Publication .

opus:in_series  a     owl:ObjectProperty ;
        rdfs:comment  "Indicates that a Publication is part of a Publication Series." ;
        rdfs:domain   opus:Publication ;
        rdfs:label    "In Series" ;
        rdfs:range    opus:Series .

<http://swrc.ontoware.org/ontology#affiliation>
        a       owl:ObjectProperty .

opus:chapter_of  a    owl:ObjectProperty ;
        rdfs:comment  "Indicates that a book chapter belongs to a specific book. It is debateable whether this should be subclass of Collection." ;
        rdfs:domain   opus:Book_Chapter ;
        rdfs:label    "Chapter Of" ;
        rdfs:range    opus:Edited_Book .

opus:isbn  a                    owl:DatatypeProperty ;
        rdfs:comment            "The ISBN of a publication." ;
        rdfs:domain             opus:Publication ;
        rdfs:label              "isbn" ;
        rdfs:range              <http://www.w3.org/2001/XMLSchema#string> ;
        owl:equivalentProperty  <http://purl.org/net/nknouf/ns/bibtex#hasISBN> , <http://swrc.ontoware.org/ontology#isbn> .

opus:Webpage  a          owl:Class ;
        rdfs:comment     "A webpage, it is subclass of Document because we want to emphasize that the URL of the webpage is used the URI." ;
        rdfs:label       "Webpage" ;
        rdfs:subClassOf  <http://xmlns.com/foaf/0.1/Document> .

opus:affiliation  a             owl:ObjectProperty ;
        rdfs:comment            "Indicates that a person is affiliated to a specific organization." ;
        rdfs:domain             <http://xmlns.com/foaf/0.1/Person> ;
        rdfs:label              "Affiliation" ;
        rdfs:range              <http://xmlns.com/foaf/0.1/Organization> ;
        owl:equivalentProperty  <http://www.aktors.org/ontology/portal#has-affiliation> , <http://swrc.ontoware.org/ontology#affiliation> .

opus:Article_in_Proceedings
        a                    owl:Class ;
        rdfs:comment         "An article in the proceedings of a meeting, such as a conference, workhshop and symposium." ;
        rdfs:label           "Article in Proceedings" ;
        rdfs:subClassOf      opus:Publication ;
        owl:equivalentClass  <http://purl.org/net/nknouf/ns/bibtex#Inproceedings> , <http://sw-portal.deri.org/ontologies/swportal#Inproceedings> .

opus:coeditor  a      owl:ObjectProperty ;
        rdfs:comment  "Indicates that a person is co-editor with another person" ;
        rdfs:domain   <http://xmlns.com/foaf/0.1/Person> ;
        rdfs:label    "coeditor" ;
        rdfs:range    <http://xmlns.com/foaf/0.1/Person> .

opus:Series  a        owl:Class ;
        rdfs:comment  "Publication Series, such as LNCS, WEUR Workshops, etc. (at this time debatable whether this should be subclassof Publication)" ;
        rdfs:label    "Series" .

<http://purl.org/net/nknouf/ns/bibtex#hasJournal>
        a       owl:DatatypeProperty .

<http://purl.org/net/nknouf/ns/bibtex#hasMonth>
        a       owl:DatatypeProperty .

opus:Edited_Publication
        a                owl:Class ;
        rdfs:comment     "An edited publication, that is, it has one or more editors (edited books, etc)" ;
        rdfs:label       "Edited Publication" ;
        rdfs:subClassOf  opus:Publication .

opus:number  a                  owl:DatatypeProperty ;
        rdfs:comment            "The Number part of citation of a publication." ;
        rdfs:domain             opus:Publication ;
        rdfs:label              "number" ;
        rdfs:range              <http://www.w3.org/2001/XMLSchema#string> ;
        owl:equivalentProperty  <http://purl.org/net/nknouf/ns/bibtex#hasNumber> .

<http://swrc.ontoware.org/ontology#month>
        a       owl:DatatypeProperty .

opus:sameAffiliation  a  owl:ObjectProperty ;
        rdfs:comment  "Indicates that a person has same affiliation than another person (this is not necessarily transitive)" ;
        rdfs:domain   <http://xmlns.com/foaf/0.1/Person> ;
        rdfs:label    "sameAffiliation" ;
        rdfs:range    <http://xmlns.com/foaf/0.1/Person> .

opus:University  a           owl:Class ;
        rdfs:comment         "An institution for higher learning with teaching and research facilities constituting a graduate school and professional schools that award master's degrees and doctorates and an undergraduate division that awards bachelor's degrees." ;
        rdfs:label           "University" ;
        rdfs:subClassOf      opus:School ;
        owl:equivalentClass  <http://sw-portal.deri.org/ontologies/swportal#University> , <http://www.aktors.org/ontology/portal#University> , <http://swrc.ontoware.org/ontology#University> , <http://knowledgeweb.semanticweb.org/semanticportal/OWL/Organization_Ontology.owl#University> .

opus:Book_Chapter  a         owl:Class ;
        rdfs:comment         "A part of a book, such as a chapter (or section/preface) and/or a range of pages." ;
        rdfs:label           "Book Chapter" ;
        rdfs:subClassOf      opus:Publication ;
        owl:equivalentClass  <http://purl.org/net/nknouf/ns/bibtex#Inbook> , <http://knowledgeweb.semanticweb.org/semanticportal/OWL/Documentation_Ontology.owl#Article_in_Book> .

opus:   a                owl:Ontology ;
        rdfs:comment     "This file specifies in RDF Schema format the classes and properties for SwetoDblp.\n    These classes and properties are based on the internal LSDIS Library portal engine.\n    Contact Person is Boanerges Aleman-Meza (baleman at uga dot edu).\n    " ;
        rdfs:label       "SwetoDblp Ontology" ;
        dc:creator       "Boanerges Aleman-Meza" ;
        owl:versionInfo  "2007-05-01" .

<http://www.aktors.org/ontology/portal#has-page-numbers>
        a       owl:DatatypeProperty .

<http://purl.org/net/nknouf/ns/bibtex#hasBooktitle>
        a       owl:DatatypeProperty .

<http://swrc.ontoware.org/ontology#year>
        a       owl:DatatypeProperty .

opus:Thesis  a               owl:Class ;
        rdfs:comment         "A treatise advancing a new point of view resulting from research; usually a requirement for an advanced academic degree." ;
        rdfs:label           "Thesis" ;
        rdfs:subClassOf      opus:Publication ;
        owl:equivalentClass  <http://sw-portal.deri.org/ontologies/swportal#Thesis> , <http://swrc.ontoware.org/ontology#Thesis> , <http://knowledgeweb.semanticweb.org/semanticportal/OWL/Documentation_Ontology.owl#Thesis> .

opus:journal_name  a            owl:DatatypeProperty ;
        rdfs:comment            "The name of a Journal, such as where an article appears" ;
        rdfs:domain             opus:Journal ;
        rdfs:label              "journal name" ;
        rdfs:range              <http://www.w3.org/2001/XMLSchema#string> ;
        owl:equivalentProperty  <http://purl.org/net/nknouf/ns/bibtex#hasJournal> .

opus:last_modified_date
        a             owl:DatatypeProperty ;
        rdfs:comment  "The last modified date of a document." ;
        rdfs:domain   <http://xmlns.com/foaf/0.1/Document> ;
        rdfs:label    "last modified date" ;
        rdfs:range    <http://www.w3.org/2001/XMLSchema#string> .

opus:coauthor  a      owl:ObjectProperty ;
        rdfs:comment  "Indicates that a person is co-author with another person" ;
        rdfs:domain   <http://xmlns.com/foaf/0.1/Person> ;
        rdfs:label    "coauthor" ;
        rdfs:range    <http://xmlns.com/foaf/0.1/Person> .

opus:chapter  a                 owl:DatatypeProperty ;
        rdfs:comment            "The chapter number of a publication" ;
        rdfs:domain             opus:Book_Chapter ;
        rdfs:label              "chapter" ;
        rdfs:range              <http://www.w3.org/2001/XMLSchema#string> ;
        owl:equivalentProperty  <http://swrc.ontoware.org/ontology#chapter> , <http://knowledgeweb.semanticweb.org/semanticportal/OWL/Documentation_Ontology.owl#Chapter> .

opus:month  a                   owl:DatatypeProperty ;
        rdfs:comment            "The month part of the date of a foaf:Document." ;
        rdfs:domain             <http://xmlns.com/foaf/0.1/Document> ;
        rdfs:label              "month" ;
        rdfs:range              <http://www.w3.org/2001/XMLSchema#string> ;
        owl:equivalentProperty  <http://purl.org/net/nknouf/ns/bibtex#hasMonth> , <http://swrc.ontoware.org/ontology#month> .

opus:Article  a              owl:Class ;
        rdfs:comment         "An article from a journal or magazine." ;
        rdfs:label           "Article" ;
        rdfs:subClassOf      opus:Publication ;
        owl:equivalentClass  <http://purl.org/net/nknouf/ns/bibtex#Article> , <http://sw-portal.deri.org/ontologies/swportal#Article> , <http://knowledgeweb.semanticweb.org/semanticportal/OWL/Documentation_Ontology.owl#Article_in_Journal> .

<http://knowledgeweb.semanticweb.org/semanticportal/OWL/Documentation_Ontology.owl#Chapter>
        a       owl:DatatypeProperty .

<http://www.aktors.org/ontology/portal#has-affiliation>
        a       owl:ObjectProperty .

opus:editor  a        owl:ObjectProperty ;
        rdfs:comment  "Indicates that a publication has a specific editor(s)." ;
        rdfs:domain   opus:Edited_Publication ;
        rdfs:label    "Editor" ;
        rdfs:range    rdf:Seq .

opus:Edited_Book  a          owl:Class ;
        rdfs:comment         "An edited book with an explicit publisher." ;
        rdfs:label           "Edited Book" ;
        rdfs:subClassOf      opus:Book , opus:Edited_Publication ;
        owl:equivalentClass  <http://www.aktors.org/ontology/portal#Edited-Book> .

opus:book_title  a              owl:DatatypeProperty ;
        rdfs:comment            "An alternative Book Title or the Book Title where an article appears, such as title of proceedings." ;
        rdfs:domain             opus:Publication ;
        rdfs:label              "book title" ;
        rdfs:range              <http://www.w3.org/2001/XMLSchema#string> ;
        owl:equivalentProperty  <http://purl.org/net/nknouf/ns/bibtex#hasBooktitle> , <http://swrc.ontoware.org/ontology#booktitle> .

<http://purl.org/net/nknouf/ns/bibtex#hasNumber>
        a       owl:DatatypeProperty .

<http://swrc.ontoware.org/ontology#pages>
        a       owl:DatatypeProperty .

opus:School  a           owl:Class ;
        rdfs:comment     "An organization where individuals receive education." ;
        rdfs:label       "School" ;
        rdfs:subClassOf  <http://xmlns.com/foaf/0.1/Organization> .

opus:eepresentation  a  owl:DatatypeProperty ;
        rdfs:comment  "The Electronic Edition of a Presentation of a publication" ;
        rdfs:domain   opus:Publication ;
        rdfs:label    "presentation" ;
        rdfs:range    <http://www.w3.org/2001/XMLSchema#string> .

opus:at_organization  a  owl:ObjectProperty ;
        rdfs:comment  "Indicates that a publication originates or is related to a specific Organization." ;
        rdfs:domain   opus:Publication ;
        rdfs:label    "at organization" ;
        rdfs:range    <http://xmlns.com/foaf/0.1/Organization> .

<http://swrc.ontoware.org/ontology#isbn>
        a       owl:DatatypeProperty .

opus:Doctoral_Dissertation
        a                    owl:Class ;
        rdfs:comment         "A dissertation written to receive a PhD." ;
        rdfs:label           "Doctoral Dissertation" ;
        rdfs:subClassOf      opus:Thesis ;
        owl:equivalentClass  <http://purl.org/net/nknouf/ns/bibtex#Phdthesis> , <http://sw-portal.deri.org/ontologies/swportal#PhDThesis> , <http://swrc.ontoware.org/ontology#PhDThesis> , <http://knowledgeweb.semanticweb.org/semanticportal/OWL/Documentation_Ontology.owl#PhD_Thesis> .

opus:cdrom  a         owl:DatatypeProperty ;
        rdfs:comment  "The CDROM location of a Publication, as used by the ACM SIGMOD Anthology." ;
        rdfs:domain   opus:Publication ;
        rdfs:label    "cdrom" ;
        rdfs:range    <http://www.w3.org/2001/XMLSchema#string> .

opus:Book  a                 owl:Class ;
        rdfs:comment         "A book with an explicit publisher." ;
        rdfs:label           "Book" ;
        rdfs:subClassOf      opus:Publication ;
        owl:equivalentClass  <http://purl.org/net/nknouf/ns/bibtex#Book> , <http://www.aktors.org/ontology/portal#Book> , <http://swrc.ontoware.org/ontology#Book> , <http://knowledgeweb.semanticweb.org/semanticportal/OWL/Documentation_Ontology.owl#Book> , <http://www.marcont.org/ontology/marcont.owl#Book> .

opus:isIncludedIn  a            owl:ObjectProperty ;
        rdfs:comment            "Indicates that a publication is included in a specific proceedings publication." ;
        rdfs:domain             opus:Article_in_Proceedings ;
        rdfs:label              "is Included in Proceedings" ;
        rdfs:range              opus:Proceedings ;
        owl:equivalentProperty  <http://sw-portal.deri.org/ontologies/swportal#containedInProceedings> .

opus:Publishing_Organization
        a                    owl:Class ;
        rdfs:comment         "An organization that, among other things, creates publishing periodicals, books or music." ;
        rdfs:label           "Publisher" ;
        rdfs:subClassOf      <http://xmlns.com/foaf/0.1/Organization> ;
        owl:equivalentClass  <http://www.aktors.org/ontology/portal#Publishing-House> .

opus:volume  a                  owl:DatatypeProperty ;
        rdfs:comment            "The Volume part of citation of a publication." ;
        rdfs:domain             opus:Publication ;
        rdfs:label              "volume" ;
        rdfs:range              <http://www.w3.org/2001/XMLSchema#string> ;
        owl:equivalentProperty  <http://swrc.ontoware.org/ontology#volume> .

<http://swrc.ontoware.org/ontology#chapter>
        a       owl:DatatypeProperty .

<http://swrc.ontoware.org/ontology#volume>
        a       owl:DatatypeProperty .

opus:cites  a                   owl:ObjectProperty ;
        rdfs:comment            "Indicates that a publication cites another publication." ;
        rdfs:domain             opus:Publication ;
        rdfs:label              "Cites" ;
        owl:equivalentProperty  <http://swrc.ontoware.org/ontology#cite> .

opus:author  a        owl:ObjectProperty ;
        rdfs:comment  "Indicates that a publication is authored by a specific person(s)." ;
        rdfs:domain   opus:Publication ;
        rdfs:label    "Author" ;
        rdfs:range    rdf:Seq .

<http://swrc.ontoware.org/ontology#booktitle>
        a       owl:DatatypeProperty .

opus:Publication  a          owl:Class ;
        rdfs:comment         "Individual documents and collections of documents such as series, journals, etc." ;
        rdfs:label           "Publication" ;
        rdfs:subClassOf      <http://xmlns.com/foaf/0.1/Document> ;
        owl:equivalentClass  <http://sw-portal.deri.org/ontologies/swportal#Publication> , <http://www.aktors.org/ontology/portal#Publication> , <http://swrc.ontoware.org/ontology#Publication> , <http://knowledgeweb.semanticweb.org/semanticportal/OWL/Documentation_Ontology.owl#Publication> .

opus:year  a                    owl:DatatypeProperty ;
        rdfs:comment            "The year part of the date of a foaf:Document." ;
        rdfs:domain             <http://xmlns.com/foaf/0.1/Document> ;
        rdfs:label              "year" ;
        rdfs:range              <http://www.w3.org/2001/XMLSchema#gYear> ;
        owl:equivalentProperty  <http://swrc.ontoware.org/ontology#year> .

opus:ee  a            owl:DatatypeProperty ;
        rdfs:comment  "The Electronic Edition of a publication" ;
        rdfs:domain   opus:Publication ;
        rdfs:label    "ee" ;
        rdfs:range    <http://www.w3.org/2001/XMLSchema#string> .

<http://purl.org/net/nknouf/ns/bibtex#hasPages>
        a       owl:DatatypeProperty .

opus:Masters_Thesis  a       owl:Class ;
        rdfs:comment         "A thesis written to receive a Master's degree." ;
        rdfs:label           "Masters Thesis" ;
        rdfs:subClassOf      opus:Thesis ;
        owl:equivalentClass  <http://purl.org/net/nknouf/ns/bibtex#Mastersthesis> , <http://sw-portal.deri.org/ontologies/swportal#MasterThesis> , <http://swrc.ontoware.org/ontology#MasterThesis> , <http://knowledgeweb.semanticweb.org/semanticportal/OWL/Documentation_Ontology.owl#Master_Thesis> .

<http://swrc.ontoware.org/ontology#cite>
        a       owl:ObjectProperty .

opus:Proceedings  a          owl:Class ;
        rdfs:comment         "A written account of what transpired at a meeting." ;
        rdfs:label           "Proceedings" ;
        rdfs:subClassOf      opus:Publication ;
        owl:equivalentClass  <http://purl.org/net/nknouf/ns/bibtex#Proceedings> , <http://sw-portal.deri.org/ontologies/swportal#Proceedings> , <http://swrc.ontoware.org/ontology#Proceedings> .

opus:abstract  a      owl:DatatypeProperty ;
        rdfs:comment  "The abstract of a document" ;
        rdfs:domain   <http://xmlns.com/foaf/0.1/Document> ;
        rdfs:label    "abstract" ;
        rdfs:range    <http://www.w3.org/2001/XMLSchema#string> .

opus:pages  a                   owl:DatatypeProperty ;
        rdfs:comment            "The Pages part of citation of a publication." ;
        rdfs:domain             opus:Publication ;
        rdfs:label              "pages" ;
        rdfs:range              <http://www.w3.org/2001/XMLSchema#string> ;
        owl:equivalentProperty  <http://purl.org/net/nknouf/ns/bibtex#hasPages> , <http://www.aktors.org/ontology/portal#has-page-numbers> , <http://swrc.ontoware.org/ontology#pages> .

opus:at_university  a  owl:ObjectProperty ;
        rdfs:comment  "Indicates that a publication originates or is related to a specific University." ;
        rdfs:domain   opus:Publication ;
        rdfs:label    "at university" ;
        rdfs:range    opus:University .

<http://sw-portal.deri.org/ontologies/swportal#containedInProceedings>
        a       owl:ObjectProperty .
