@prefix adms:  <http://www.w3.org/ns/adms#> .
@prefix dc:    <http://purl.org/dc/elements/1.1/> .
@prefix rdfs:  <http://www.w3.org/2000/01/rdf-schema#> .
@prefix foaf:  <http://xmlns.com/foaf/0.1/> .
@prefix owl:   <http://www.w3.org/2002/07/owl#> .
@prefix xsd:   <http://www.w3.org/2001/XMLSchema#> .
@prefix rdf:   <http://www.w3.org/1999/02/22-rdf-syntax-ns#> .
@prefix vann:  <http://purl.org/vocab/vann/> .
@prefix dcterms: <http://purl.org/dc/terms/> .
@prefix pdo:   <http://ontologies.smile.deri.ie/pdo#> .

<http://vocab.deri.ie/pdo>
        a                              owl:Ontology , adms:SemanticAsset ;
        dc:creator                     <http://vocab.deri.ie/pdo#pravar> ;
        dcterms:created                "2010-07-09"^^xsd:date ;
        dcterms:description            "The Project Documents Ontology, described using W3C RDF Schema and the Web Ontology Language, models the inherent structure and concepts of various documents in a project-specific setting, like meeting minutes, status reports etc." ;
        dcterms:modified               "2010-07-09"^^xsd:date ;
        dcterms:partOf                 <http://vocab.deri.ie> ;
        dcterms:publisher              "http://vocab.deri.ie/pdo#DERI%2C%20NUI%20Galway" ;
        dcterms:status                 <http://purl.org/adms/status/UnderDevelopment> ;
        dcterms:title                  "Project Documents Ontology" ;
        dcterms:type                   <http://purl.org/adms/assettype/Ontology> ;
        vann:preferredNamespacePrefix  "pdo" ;
        vann:preferredNamespaceUri     "http://ontologies.smile.deri.ie/pdo#" ;
        foaf:homepage                  <http://vocab.deri.ie/pdo.html> .

pdo:hasStartTime  a  owl:DatatypeProperty , rdf:Property ;
        rdfs:domain  pdo:ActionItem ;
        rdfs:label   "hasStartTime" ;
        rdfs:range   xsd:dateTime .

<http://vocab.deri.ie/pdo#rdf>
        a                   adms:SemanticDistribution ;
        dcterms:FileFormat  <http://vocab.deri.ie/pdo> ;
        adms:accessURL      "http://vocab.deri.ie/pdo.rdf" ;
        adms:status         <http://purl.org/adms/status/Completed> .

pdo:Scribe  a            owl:Class , rdfs:Class ;
        rdfs:comment     "Models the scribe role of a person in a meeting context." ;
        rdfs:label       "Scribe" ;
        rdfs:subClassOf  pdo:PersonRole .

pdo:Absentee  a          owl:Class , rdfs:Class ;
        rdfs:comment     "Models the absentee role of a person in a meeting context." ;
        rdfs:label       "Absentee" ;
        rdfs:subClassOf  pdo:PersonRole .

pdo:Poll  a              owl:Class , rdfs:Class ;
        rdfs:comment     "Subclasses pdo:Artifact and models the structure of a poll" ;
        rdfs:label       "Poll" ;
        rdfs:subClassOf  pdo:Artefact .

pdo:isAssignedTo  a   rdf:Property ;
        rdfs:comment  "This property links a pdo:ActionItem object to a foaf:Person object who is reponsible for the action item" ;
        rdfs:domain   pdo:ActionItem ;
        rdfs:label    "isAssignedTo" ;
        rdfs:range    foaf:Person .

pdo:Presenter  a         owl:Class , rdfs:Class ;
        rdfs:comment     "Models the presenter role of a person in the context of an agenda item." ;
        rdfs:label       "Presenter" ;
        rdfs:subClassOf  pdo:PersonRole .

pdo:Reporter  a          owl:Class , rdfs:Class ;
        rdfs:comment     "Models the reporting role of a person in a status reporting context." ;
        rdfs:label       "Reporter" ;
        rdfs:subClassOf  pdo:PersonRole .

<http://vocab.deri.ie/pdo#ttl>
        a                   adms:SemanticDistribution ;
        dcterms:FileFormat  <http://vocab.deri.ie/pdo> ;
        adms:accessURL      "http://vocab.deri.ie/pdo.ttl" ;
        adms:status         <http://purl.org/adms/status/Completed> .

pdo:hasDescription  a  owl:DatatypeProperty , rdf:Property ;
        rdfs:domain  pdo:ActionItem ;
        rdfs:label   "hasDescription" ;
        rdfs:range   rdf:XMLLiteral .

pdo:hasAlias  a       owl:DatatypeProperty , rdf:Property ;
        rdfs:comment  "A way to store different alias names of objects (used internally by the application)" ;
        rdfs:domain   owl:Thing ;
        rdfs:label    "hasAlias" ;
        rdfs:range    xsd:string .

pdo:Publication  a       owl:Class , rdfs:Class ;
        rdfs:comment     "Subclasses pdo:Artifact and uses bibliography ontology to model the structure of a publication" ;
        rdfs:label       "Publication" ;
        rdfs:subClassOf  pdo:Artefact .

pdo:Artefact  a       owl:Class , rdfs:Class ;
        rdfs:comment  "An abstract class for  any kind of information artifact which can be structured according to its sematics." ;
        rdfs:label    "Artefact" .

pdo:ActionItem  a        owl:Class , rdfs:Class ;
        rdfs:comment     "Subclasses pdo:Artifact and models the structure of an action item/task" ;
        rdfs:label       "ActionItem" ;
        rdfs:subClassOf  pdo:Artefact .

pdo:Meeting  a        owl:Class , rdfs:Class ;
        rdfs:comment  "The class modelling the actual meeting which is the subject of a particular minutes document." ;
        rdfs:label    "Meeting" .

pdo:mentions  a       rdf:Property ;
        rdfs:comment  "The property which links an artefact (for example, an agenda item , an action item, a travle report, etc ) to the document in which it is mentioned." ;
        rdfs:domain   pdo:Document , pdo:Comment , pdo:Artefact ;
        rdfs:label    "mentions" ;
        rdfs:range    rdf:Resource .

pdo:StatusReport  a      owl:Class , rdfs:Class ;
        rdfs:comment     "The class modelling the structure and content of an electronic version of a status reports document" ;
        rdfs:label       "Report" ;
        rdfs:subClassOf  pdo:Document .

pdo:AgendaItem  a        owl:Class , rdfs:Class ;
        rdfs:comment     "Subclasses pdo:Artifact and models the structure of an agenda item" ;
        rdfs:label       "AgendaItem" ;
        rdfs:subClassOf  pdo:Artefact .

pdo:LeaveReport  a       owl:Class , rdfs:Class ;
        rdfs:comment     "Subclasses pdo:Artefact and models the structure of a leave report" ;
        rdfs:label       "LeaveReport" ;
        rdfs:subClassOf  pdo:Report , pdo:LeaveReport .

pdo:Comment  a        owl:Class , rdfs:Class ;
        rdfs:comment  "Models a comment made by a person" ;
        rdfs:label    "Comment" .

pdo:MeetingMinutes  a    owl:Class , rdfs:Class ;
        rdfs:comment     "The class modelling the structure and cotent of an electronic version of the minutes of a meetintg." ;
        rdfs:label       "Minutes" ;
        rdfs:subClassOf  pdo:Document .

pdo:hasCreationTime  a  owl:DatatypeProperty , rdf:Property ;
        rdfs:domain  pdo:ActionItem ;
        rdfs:label   "hasCreationTime" ;
        rdfs:range   xsd:dateTime .

pdo:Chair  a             owl:Class , rdfs:Class ;
        rdfs:comment     "Models the chair role of a person in a meeting context." ;
        rdfs:label       "Chair" ;
        rdfs:subClassOf  pdo:PersonRole .

pdo:hasStatus  a     owl:DatatypeProperty , rdf:Property ;
        rdfs:domain  pdo:ActionItem ;
        rdfs:label   "hasStatus" ;
        rdfs:range   rdf:XMLLiteral .

pdo:hasEndTime  a    owl:DatatypeProperty , rdf:Property ;
        rdfs:domain  pdo:ActionItem ;
        rdfs:label   "hadEndTime" ;
        rdfs:range   xsd:dateTime .

pdo:PollOption  a     owl:Class , rdfs:Class ;
        rdfs:comment  "Models an option in a poll. Each option is linked to a list of people who selected the option during the poll" ;
        rdfs:label    "PollOption" .

pdo:Report  a            owl:Class , rdfs:Class ;
        rdfs:comment     "Subclasses pdo:Artefact and models the structure of a travel report" ;
        rdfs:label       "TravelReport" ;
        rdfs:subClassOf  pdo:Artefact .

pdo:Document  a          owl:Class , rdfs:Class ;
        rdfs:comment     "The base class for all kinds of electronic documents in a project-specific setting." ;
        rdfs:label       "Document" ;
        rdfs:subClassOf  foaf:Document .

<http://vocab.deri.ie/pdo#pravar>
        a              foaf:Person ;
        foaf:homepage  <http://vocab.deri.ie/pdo> ;
        foaf:mbox      <mailto:pradeep.varma@deri.org> ;
        foaf:name      "Pradeep Varma" .

pdo:Attendee  a          owl:Class , rdfs:Class ;
        rdfs:comment     "Models the attendee role of a person in a meeting context." ;
        rdfs:label       "Attendee" ;
        rdfs:subClassOf  pdo:PersonRole .

pdo:contains  a       rdf:Property ;
        rdfs:comment  "The property which links an artefact (for example, an agenda item , an action item, a travle report, etc ) to the document in which it is mentioned." ;
        rdfs:domain   pdo:Document ;
        rdfs:label    "contains" ;
        rdfs:range    pdo:Artefact .

pdo:TravelReport  a      owl:Class , rdfs:Class ;
        rdfs:comment     "Subclasses pdo:Artefact and models the structure of a travel report" ;
        rdfs:label       "TravelReport" ;
        rdfs:subClassOf  pdo:Report .

pdo:PersonRole  a     owl:Class , rdfs:Class ;
        rdfs:comment  "The abstract class modelling various roles taken by individuals during a particular context ( for example, the attendees, scribe etc in a meeting or the reporter in a status report.)" ;
        rdfs:label    "PersonRole" .

<http://vocab.deri.ie/pdo#DERI%2C%20NUI%20Galway>
        a              dcterms:Agent ;
        foaf:homepage  <http://deri.ie/> ;
        foaf:member    <http://vocab.deri.ie/pdo#pravar> ;
        foaf:name      "DERI, NUI Galway" .
