@prefix rdfs: <http://www.w3.org/2000/01/rdf-schema#> .
@prefix foaf: <http://xmlns.com/foaf/0.1/> .
@prefix event: <http://purl.org/NET/c4dm/event.owl#> .
@prefix xsd: <http://www.w3.org/2001/XMLSchema#> .
@prefix owl: <http://www.w3.org/2002/07/owl#> .
@prefix pns: <http://data.press.net/ontology/stuff/> .
@prefix rdf: <http://www.w3.org/1999/02/22-rdf-syntax-ns#> .
@prefix pnc: <http://data.press.net/ontology/classification/> .
@prefix vs: <http://www.w3.org/2003/06/sw-vocab-status/ns#> .
@prefix pne: <http://data.press.net/ontology/event/> .
@prefix dcterms: <http://purl.org/dc/terms/> .

<http://uk.linkedin.com/in/jarredmcginnis> a foaf:Person ;
	foaf:name "Jarred McGinnis" .

<http://uk.linkedin.com/in/pauliharman> a foaf:Person ;
	foaf:name "Paul Harman" .

<http://uk.linkedin.com/in/paulwilton> a foaf:Person ;
	foaf:name "Paul Wilton" .

<http://data.press.net/ontology/event/> a owl:Ontology ;
	dcterms:title "SNaP Event Ontology"@en ;
	dcterms:created "2011-07-28"^^xsd:date ;
	dcterms:modified "2012-04-20"^^xsd:date ;
	dcterms:license <http://creativecommons.org/licenses/by-nd/3.0/> ;
	rdfs:comment "The Event Ontology models news-worthy events and their relationship to news assets and stuff (simple entities) in the world."@en ;
	foaf:maker <http://uk.linkedin.com/in/jarredmcginnis> , <http://uk.linkedin.com/in/paulwilton> , <http://uk.linkedin.com/in/pauliharman> ;
	owl:versionInfo "0.5.0"^^xsd:string .

pne:Event a owl:Class ;
	rdfs:subClassOf event:Event , pns:Stuff ;
	rdfs:label "Generic Event Class"@en ;
	rdfs:comment "Generic Event Class, a subclass of event:Event. The Event class also subclasses pnt:Stuff as it is a Compound domain entity, this inheritance means news assets can be tagged with Events"@en ;
	rdfs:isDefinedBy <http://data.press.net/ontology/event/> ;
	vs:term_status "testing" .

pne:subEventOf a owl:TransitiveProperty ;
	rdfs:domain pne:Event ;
	rdfs:range pne:Event ;
	rdfs:label "Transitive Property defining a parent-child relationship between events"@en ;
	rdfs:comment "Transitive Property defining a parent-child relationship between events. Event Y is a sub event of Event X"@en ;
	rdfs:isDefinedBy <http://data.press.net/ontology/event/> ;
	vs:term_status "testing" .

pne:title a owl:DatatypeProperty ;
	rdfs:subPropertyOf dcterms:title , pns:label ;
	rdfs:domain pne:Event ;
	rdfs:range xsd:string ;
	rdfs:label "An Event title"@en ;
	rdfs:comment "Property for expressing an event title. Datatype is String"@en ;
	rdfs:isDefinedBy <http://data.press.net/ontology/event/> ;
	vs:term_status "testing" .

pne:summary a owl:DatatypeProperty ;
	rdfs:subPropertyOf dcterms:abstract , pns:comment ;
	rdfs:domain pne:Event ;
	rdfs:range xsd:string ;
	rdfs:label "An Event summary"@en ;
	rdfs:comment "Property for expressing an event summary. Datatype is String"@en ;
	rdfs:isDefinedBy <http://data.press.net/ontology/event/> ;
	vs:term_status "testing" .

pne:theme a owl:ObjectProperty ;
	rdfs:subPropertyOf pns:notablyAssociatedWith ;
	rdfs:domain pne:Event ;
	rdfs:range pns:Intangible ;
	rdfs:label "Associates an Event with an intangible theme"@en ;
	rdfs:comment "Property for expressing the theme of an event, its range is pns:Intangible"@en ;
	rdfs:isDefinedBy <http://data.press.net/ontology/event/> ;
	vs:term_status "testing" .
