@prefix rdfs: <http://www.w3.org/2000/01/rdf-schema#> .
@prefix foaf: <http://xmlns.com/foaf/0.1/> .
@prefix pni: <http://data.press.net/ontology/identifier/> .
@prefix owl: <http://www.w3.org/2002/07/owl#> .
@prefix xsd: <http://www.w3.org/2001/XMLSchema#> .
@prefix rdf: <http://www.w3.org/1999/02/22-rdf-syntax-ns#> .
@prefix vs: <http://www.w3.org/2003/06/sw-vocab-status/ns#> .
@prefix dcterms: <http://purl.org/dc/terms/> .

<http://data.press.net/ontology/identifier/> a owl:Ontology ;
	dcterms:title "SNaP Identifier Ontology"@en ;
	dcterms:created "2012-03-21"^^xsd:date ;
	dcterms:modified "2012-03-21"^^xsd:date ;
	dcterms:license <http://creativecommons.org/licenses/by-nd/3.0/> ;
	rdfs:comment "The Identifier Ontology models non-RDF based Identifiers for resources. The enables us to maintain a mapping between RDF resources identifiers and their equivalent IDs in an alternate, non-RDF based domain."@en ;
	foaf:maker <http://uk.linkedin.com/in/paulwilton> .

<http://uk.linkedin.com/in/paulwilton> a foaf:Person ;
	foaf:name "Paul Wilton" .

<http://data.press.net/ontology/identifier/> foaf:maker <http://www.linkedin.com/pub/matt-nathan/33/44a/68a> .

<http://www.linkedin.com/pub/matt-nathan/33/44a/68a> a foaf:Person ;
	foaf:name "Matt Nathan" .

<http://data.press.net/ontology/identifier/> foaf:maker <http://uk.linkedin.com/in/pauliharman> .

<http://uk.linkedin.com/in/pauliharman> a foaf:Person ;
	foaf:name "Paul Harman" .

<http://data.press.net/ontology/identifier/> foaf:maker <http://uk.linkedin.com/in/jarredmcginnis> .

<http://uk.linkedin.com/in/jarredmcginnis> a foaf:Person ;
	foaf:name "Jarred McGinnis" .

<http://data.press.net/ontology/identifier/> owl:versionInfo "0.3.0"^^xsd:string .

pni:Identifier a owl:Class ;
	rdfs:label "An Identifier for a resource"@en ;
	rdfs:comment "An ID for a given resource. For example a literal ID from a legacy system"@en ;
	rdfs:isDefinedBy <http://data.press.net/ontology/identifier/> ;
	vs:term_status "testing" .

pni:hasIdentifier a owl:ObjectProperty ;
	rdfs:domain pni:Identifiable .

pni:Identifiable a owl:Class ;
	rdfs:label "An Identifiable resource type"@en ;
	rdfs:comment "An instance that is Identifiable can have an Identifier associated with it."@en ;
	rdfs:isDefinedBy <http://data.press.net/ontology/identifier/> ;
	vs:term_status "testing" .

pni:hasIdentifier rdfs:range pni:Identifier ;
	rdfs:label "Associates an Identifier to an Identifiable thing"@en ;
	rdfs:comment "Associates an Identifier to an Identifiable thing"@en ;
	rdfs:isDefinedBy <http://data.press.net/ontology/identifier/> ;
	vs:term_status "testing" .

pni:value a owl:DatatypeProperty ;
	rdfs:domain pni:Identifier ;
	rdfs:range rdfs:Literal ;
	rdfs:label "the value of the Identifier"@en ;
	rdfs:comment "Property indicating the literal value of the Identifier"@en ;
	rdfs:isDefinedBy <http://data.press.net/ontology/identifier/> ;
	vs:term_status "testing" .

pni:authority a owl:ObjectProperty ;
	rdfs:domain pni:Identifier ;
	rdfs:range pni:Authority .

pni:Authority a owl:Class ;
	rdfs:label "The Authority for an Identifier"@en ;
	rdfs:comment "The Authority for an Identifier, for example the domain or namespace within which an ID is contained"@en ;
	rdfs:isDefinedBy <http://data.press.net/ontology/identifier/> ;
	vs:term_status "testing" .

pni:authority rdfs:label "Indicates the ID Authority of an Identifier"@en ;
	rdfs:comment "Property defining the containing authority of an Identifier"@en ;
	rdfs:isDefinedBy <http://data.press.net/ontology/identifier/> ;
	vs:term_status "testing" .
