@prefix tags: <http://www.holygoat.co.uk/owl/redwood/0.1/tags/> .
@prefix : <http://purl.org/ontology/po/> .
@prefix dc: <http://purl.org/dc/elements/1.1/> .
@prefix tl: <http://purl.org/NET/c4dm/timeline.owl#> .
@prefix geo: <http://www.w3.org/2003/01/geo/wgs84_pos#> .
@prefix mo: <http://purl.org/ontology/mo/> .
@prefix foaf: <http://xmlns.com/foaf/0.1/> .
@prefix frbr: <http://purl.org/vocab/frbr/core#> .
@prefix vs: <http://www.w3.org/2003/06/sw-vocab-status/ns#> .
@prefix dcterms: <http://purl.org/dc/terms/> .
@prefix provenance: <http://www.bbc.co.uk/ontologies/provenance/> .
@prefix rdfs: <http://www.w3.org/2000/01/rdf-schema#> .
@prefix event: <http://purl.org/NET/c4dm/event.owl#> .
@prefix xsd: <http://www.w3.org/2001/XMLSchema#> .
@prefix owl: <http://www.w3.org/2002/07/owl#> .
@prefix rdf: <http://www.w3.org/1999/02/22-rdf-syntax-ns#> .
@prefix skos: <http://www.w3.org/2004/02/skos/core#> .

<http://purl.org/ontology/po/> a provenance:Ontology , owl:Ontology ;
	rdfs:comment """
		A vocabulary for programme data.
		It defines concepts such as brands, series, episodes, but
		also defined broadcasting events.
	""" ;
	rdfs:isDefinedBy <http://purl.org/ontology/po/> ;
	rdfs:label "Programmes ontology" ;
	dc:creator <http://moustaki.org/foaf.rdf#moustaki> ;
	dc:date "$Date: 2007/11/19 15:25:11 $" ;
	dcterms:license <http://creativecommons.org/licenses/by/4.0#id> ;
	provenance:canonicalLocation "https://repo.dev.bbc.co.uk/services/linked-data/ontologies/domain/programmes"^^xsd:string ;
	provenance:changeReason "Added fist meta"@en-gb ;
	provenance:public "true"^^xsd:boolean ;
	provenance:slug "po"^^xsd:string ;
	provenance:version "0.1"^^xsd:double ;
	owl:versionIRI <http://purl.org/ontology/po/0.1> ;
	owl:versionInfo "0.1" .

:AudioDescribedVersion a owl:Class ;
	rdfs:comment """
		A version holding an audio description.
	""" ;
	rdfs:isDefinedBy <http://purl.org/ontology/po/> ;
	rdfs:label "Audio description" ;
	rdfs:subClassOf :Version ;
	vs:term_status "testing" .

:Brand a owl:Class ;
	rdfs:comment """
		A brand, eg. `Flight of the Conchords'
	""" ;
	rdfs:isDefinedBy <http://purl.org/ontology/po/> ;
	rdfs:label "Brand" ;
	rdfs:subClassOf :Programme ;
	owl:disjointWith :Episode , :Series ;
	vs:term_status "testing" .

:Broadcast a owl:Class ;
	rdfs:comment """
		A broadcast event.
		Subsumes the event concept defined in
		the event ontology.
		A broadcast is associated to a service, and to a
		particular version of an episode.
	""" ;
	rdfs:isDefinedBy <http://purl.org/ontology/po/> ;
	rdfs:label "Broadcast" ;
	rdfs:subClassOf event:Event ;
	vs:term_status "testing" .

:Episode a owl:Class ;
	rdfs:comment """
		A particular episode, eg. `Flight of the Conchords, first episode of the first season'
	""" ;
	rdfs:isDefinedBy <http://purl.org/ontology/po/> ;
	rdfs:label "Episode" ;
	rdfs:subClassOf :Programme ;
	owl:disjointWith :Series ;
	vs:term_status "testing" .

:FirstBroadcast a owl:Class ;
	rdfs:comment """
		Specifies a broadcast as being the 
		first one of a particular version.
	 """ ;
	rdfs:isDefinedBy <http://purl.org/ontology/po/> ;
	rdfs:label "First broadcast" ;
	rdfs:subClassOf :Broadcast ;
	owl:disjointWith :RepeatBroadcast ;
	vs:term_status "unstable" .

:Format a owl:Class ;
	rdfs:comment """
		The format of a particular version (should be of the episode, btw).
		Instances of this concept include documentaries, talk shows, animation, etc.
	""" ;
	rdfs:isDefinedBy <http://purl.org/ontology/po/> ;
	rdfs:label "Format" ;
	vs:term_status "testing" .

:Genre a skos:ConceptScheme ;
	rdfs:comment """
		A concept scheme for a genre taxonomy for programmes,
		organised using SKOS (Simple Knowledge Organisation System).
	""" ;
	rdfs:isDefinedBy <http://purl.org/ontology/po/> ;
	rdfs:label "Genre" ;
	vs:term_status "testing" .

:LocalRadio a owl:Class ;
	rdfs:comment """
		Radio services aiming at a local coverage.
	""" ;
	rdfs:isDefinedBy <http://purl.org/ontology/po/> ;
	rdfs:label "Local radio" ;
	rdfs:subClassOf :Radio ;
	owl:disjointWith :NationalRadio , :RegionalRadio ;
	vs:term_status "testing" .

:NationalRadio a owl:Class ;
	rdfs:comment """
		Radio services aiming at a national coverage.
	""" ;
	rdfs:isDefinedBy <http://purl.org/ontology/po/> ;
	rdfs:label "National radio" ;
	rdfs:subClassOf :Radio ;
	vs:term_status "testing" .

:OriginalVersion a owl:Class ;
	rdfs:comment """
		An `original' version, the legacy version of
		a particular episode.
	""" ;
	rdfs:isDefinedBy <http://purl.org/ontology/po/> ;
	rdfs:label "Original version" ;
	rdfs:subClassOf :Version ;
	vs:term_status "testing" .

:Programme a owl:Class ;
	rdfs:comment """
		A programme, can either be a brand, a series or an episode
	""" ;
	rdfs:isDefinedBy <http://purl.org/ontology/po/> ;
	rdfs:label "Programme" ;
	vs:term_status "testing" .

:Radio a owl:Class ;
	rdfs:comment """
		Services that use a radio medium.
	""" ;
	rdfs:isDefinedBy <http://purl.org/ontology/po/> ;
	rdfs:label "Radio" ;
	rdfs:subClassOf :Service ;
	owl:disjointWith :TV , :Web ;
	vs:term_status "testing" .

:RegionalRadio a owl:Class ;
	rdfs:comment """
		Radio services aiming at a regional coverage.
	""" ;
	rdfs:isDefinedBy <http://purl.org/ontology/po/> ;
	rdfs:label "Regional radio" ;
	rdfs:subClassOf :Radio ;
	owl:disjointWith :NationalRadio ;
	vs:term_status "testing" .

:RepeatBroadcast a owl:Class ;
	rdfs:comment """
		Specifies a broadcast as being a 
		repeat.
	""" ;
	rdfs:isDefinedBy <http://purl.org/ontology/po/> ;
	rdfs:label "Repeat" ;
	rdfs:subClassOf :Broadcast ;
	owl:disjointWith :FirstBroadcast ;
	vs:term_status "unstable" .

:Series a owl:Class ;
	rdfs:comment """
		A serie, eg. `Flight of the Conchors, first season'
	""" ;
	rdfs:isDefinedBy <http://purl.org/ontology/po/> ;
	rdfs:label "Serie" ;
	rdfs:subClassOf :Programme ;
	vs:term_status "testing" .

:Service a owl:Class ;
	rdfs:comment """
		A service is a particular channel on which a broadcast occurrs.
		Instances of this concept include BBC Radio Wales, BBC Radio 4, BBC News, etc.
	""" ;
	rdfs:isDefinedBy <http://purl.org/ontology/po/> ;
	rdfs:label "Service" ;
	vs:term_status "testing" .

:ShortenedVersion a owl:Class ;
	rdfs:comment """
		A shortened version.
	""" ;
	rdfs:isDefinedBy <http://purl.org/ontology/po/> ;
	rdfs:label "Shortened version" ;
	rdfs:subClassOf :Version ;
	owl:disjointWith :OriginalVersion ;
	vs:term_status "testing" .

:SignedVersion a owl:Class ;
	rdfs:comment """
		A version holding sign language.
	""" ;
	rdfs:isDefinedBy <http://purl.org/ontology/po/> ;
	rdfs:label "Sign language" ;
	rdfs:subClassOf :Version ;
	vs:term_status "testing" .

:Subtitle a owl:Class ;
	rdfs:comment """
		Subtitles associated to a particular version.
	""" ;
	rdfs:isDefinedBy <http://purl.org/ontology/po/> ;
	rdfs:label "Subtitle" ;
	vs:term_status "testing" .

:TV a owl:Class ;
	rdfs:comment """
		Services that use a television medium.
	""" ;
	rdfs:isDefinedBy <http://purl.org/ontology/po/> ;
	rdfs:label "TV" ;
	rdfs:subClassOf :Service ;
	owl:disjointWith :Web ;
	vs:term_status "testing" .

:Version a owl:Class ;
	rdfs:comment """
		A particular version of an episode.
		Such versions include shortened ones, audio described ones
		or ones that holds sign language.
	""" ;
	rdfs:isDefinedBy <http://purl.org/ontology/po/> ;
	rdfs:label "Version" ;
	vs:term_status "testing" .

:Web a owl:Class ;
	rdfs:comment """
		Services that use a Web medium.
	""" ;
	rdfs:isDefinedBy <http://purl.org/ontology/po/> ;
	rdfs:label "Web" ;
	rdfs:subClassOf :Service ;
	vs:term_status "testing" .

:aspect_ratio a owl:DatatypeProperty ;
	rdfs:comment """
		The aspect ration of a particular version.
	""" ;
	rdfs:domain :Version ;
	rdfs:isDefinedBy <http://purl.org/ontology/po/> ;
	rdfs:label "aspect ratio" ;
	rdfs:range xsd:string ;
	rdfs:subPropertyOf dc:format ;
	vs:term_status "testing" .

:broadcast_of a owl:ObjectProperty ;
	rdfs:comment """
		Relates a particular broadcast to the version being broadcasted.
		Sub-property of the event:factor one.
	""" ;
	rdfs:domain :Broadcast ;
	rdfs:isDefinedBy <http://purl.org/ontology/po/> ;
	rdfs:label "broadcast of" ;
	rdfs:range :Version ;
	rdfs:subPropertyOf event:factor ;
	vs:term_status "testing" .

:broadcasted_on a owl:ObjectProperty ;
	rdfs:comment """
		Relates a particular broadcast to the service on which it was on.
		Sub-property of the event:factor one.
	""" ;
	rdfs:domain :Broadcast ;
	rdfs:isDefinedBy <http://purl.org/ontology/po/> ;
	rdfs:label "broadcasted on" ;
	rdfs:range :Service ;
	rdfs:subPropertyOf event:factor ;
	vs:term_status "testing" .

:creation_date a owl:DatatypeProperty ;
	rdfs:comment "\n                The creation date of a thing.\n                Sub-property of dc:date.\n        " ;
	rdfs:isDefinedBy <http://purl.org/ontology/po/> ;
	rdfs:label "creation date" ;
	rdfs:range xsd:dateTime ;
	rdfs:subPropertyOf dc:date ;
	vs:term_status "testing" .

:duration a owl:DatatypeProperty ;
	rdfs:comment "The duration, in seconds. Sub-property of mo:duration." ;
	rdfs:isDefinedBy <http://purl.org/ontology/po/> ;
	rdfs:label "duration" ;
	rdfs:range xsd:int ;
	rdfs:subPropertyOf mo:duration ;
	vs:term_status "testing" .

:episode a owl:InverseFunctionalProperty , owl:ObjectProperty ;
	rdfs:comment """
		Associates a brand or a series to an episode constituting it.
	""" ;
	rdfs:isDefinedBy <http://purl.org/ontology/po/> ;
	rdfs:label "episode" ;
	rdfs:range :Episode ;
	rdfs:subPropertyOf dcterms:hasPart ;
	vs:term_status "testing" .

:format a owl:ObjectProperty ;
	rdfs:comment """
		Relates a version to a particular format (eg. `Animation', `Documentary', etc.).
	""" ;
	rdfs:domain :Version ;
	rdfs:isDefinedBy <http://purl.org/ontology/po/> ;
	rdfs:label "format" ;
	rdfs:range :Format ;
	vs:term_status "testing" .

:genre a owl:ObjectProperty ;
	rdfs:comment """
		Relates an episode to a corresponding genre in a SKOS taxonomy.
	""" ;
	rdfs:domain :Programme ;
	rdfs:isDefinedBy <http://purl.org/ontology/po/> ;
	rdfs:label "genre" ;
	rdfs:range :Genre ;
	vs:term_status "testing" .

:letter a owl:DatatypeProperty ;
	rdfs:comment "Just a letter, aiming at sorting a set of resources" ;
	rdfs:isDefinedBy <http://purl.org/ontology/po/> ;
	rdfs:label "sort letter" ;
	rdfs:range xsd:string ;
	vs:term_status "testing" .

:location a owl:ObjectProperty ;
	rdfs:comment """
		Associates a radio service to a geographic location, 
		aiming at capturing what this service aims at covering.
	""" ;
	rdfs:domain :Radio ;
	rdfs:isDefinedBy <http://purl.org/ontology/po/> ;
	rdfs:label "location" ;
	rdfs:range geo:SpatialThing ;
	rdfs:subPropertyOf foaf:based_near ;
	vs:term_status "testing" .

:long_synopsis a owl:DatatypeProperty ;
	rdfs:comment """
		A long synopsis of a serie, brand or episode.
		Sub-property of po:synopsis.
	""" ;
	rdfs:isDefinedBy <http://purl.org/ontology/po/> ;
	rdfs:label "long synopsis" ;
	rdfs:subPropertyOf :synopsis ;
	vs:term_status "testing" .

:medium_synopsis a owl:DatatypeProperty ;
	rdfs:comment """
		A medium synopsis of a serie, brand or episode.
		Sub-property of po:synopsis.
	""" ;
	rdfs:isDefinedBy <http://purl.org/ontology/po/> ;
	rdfs:label "medium synopsis" ;
	rdfs:subPropertyOf :synopsis ;
	vs:term_status "testing" .

:parent_series a owl:ObjectProperty , owl:TransitiveProperty ;
	rdfs:comment """
		Relates a series to a series constituting it (eg. `Waking the dead').
	""" ;
	rdfs:domain :Serie ;
	rdfs:isDefinedBy <http://purl.org/ontology/po/> ;
	rdfs:label "parent serie" ;
	rdfs:range :Serie ;
	rdfs:subPropertyOf dcterms:isPartOf ;
	vs:term_status "testing" .

:parent_service a owl:ObjectProperty , owl:TransitiveProperty ;
	rdfs:comment """
		Relates a service to another service encapsulating it (eg. `BBC One' and `BBC One South')
	""" ;
	rdfs:domain :Service ;
	rdfs:isDefinedBy <http://purl.org/ontology/po/> ;
	rdfs:label "parent service" ;
	rdfs:range :Service ;
	rdfs:subPropertyOf dcterms:isPartOf ;
	vs:term_status "testing" .

:pid a owl:DatatypeProperty ;
	rdfs:comment "Just a BBC internal identifier - should be removed" ;
	rdfs:domain :Brand ;
	rdfs:isDefinedBy <http://purl.org/ontology/po/> ;
	rdfs:label "pid" ;
	rdfs:range xsd:string ;
	vs:term_status "unstable" .

:pid_imi a owl:DatatypeProperty ;
	rdfs:comment "Just a BBC internal identifier - should be removed" ;
	rdfs:domain :Broadcast ;
	rdfs:isDefinedBy <http://purl.org/ontology/po/> ;
	rdfs:label "pid imi" ;
	rdfs:range xsd:string ;
	vs:term_status "unstable" .

:position a owl:DatatypeProperty ;
	rdfs:comment "The position of a particular series or episode within its containing programme" ;
	rdfs:isDefinedBy <http://purl.org/ontology/po/> ;
	rdfs:label "position" ;
	rdfs:range xsd:int ;
	vs:term_status "testing" .

:schedule_date a owl:DatatypeProperty ;
	rdfs:comment """
		The schedule date of a broadcast event.
		Sub-property of dc:date.
	""" ;
	rdfs:domain :Broadcast ;
	rdfs:isDefinedBy <http://purl.org/ontology/po/> ;
	rdfs:label "schedule date" ;
	rdfs:range xsd:date ;
	rdfs:subPropertyOf dc:date ;
	vs:term_status "testing" .

:series a owl:InverseFunctionalProperty , owl:ObjectProperty , owl:TransitiveProperty ;
	rdfs:comment """
		Associates a brand or a series to a series constituting it.
	""" ;
	rdfs:isDefinedBy <http://purl.org/ontology/po/> ;
	rdfs:label "series" ;
	rdfs:range :Series ;
	rdfs:subPropertyOf dcterms:hasPart ;
	vs:term_status "testing" .

:service a owl:FunctionalProperty , owl:ObjectProperty ;
	rdfs:comment """
		Associate a brand, series or episode to the master brand service.
	""" ;
	rdfs:domain :Programme ;
	rdfs:isDefinedBy <http://purl.org/ontology/po/> ;
	rdfs:label "service" ;
	rdfs:range :Service ;
	vs:term_status "testing" .

:short_synopsis a owl:DatatypeProperty ;
	rdfs:comment """
		A short synopsis of a serie, brand or episode.
		Sub-property of po:synopsis.
	""" ;
	rdfs:isDefinedBy <http://purl.org/ontology/po/> ;
	rdfs:label "short synopsis" ;
	rdfs:subPropertyOf :synopsis ;
	vs:term_status "testing" .

:slice_title a owl:DatatypeProperty ;
	rdfs:isDefinedBy <http://purl.org/ontology/po/> ;
	rdfs:label "A sliced literal title" ;
	rdfs:range xsd:string ;
	rdfs:subPropertyOf dc:title ;
	vs:term_status "testing" .

:sort_title a owl:DatatypeProperty ;
	rdfs:comment "A literal title, aiming at being sorted on" ;
	rdfs:isDefinedBy <http://purl.org/ontology/po/> ;
	rdfs:label "sort title" ;
	rdfs:range xsd:string ;
	rdfs:subPropertyOf dc:title ;
	vs:term_status "testing" .

:sound_format a owl:DatatypeProperty ;
	rdfs:comment """
		The sound format of a particular version.
	""" ;
	rdfs:domain :Version ;
	rdfs:isDefinedBy <http://purl.org/ontology/po/> ;
	rdfs:label "sound format" ;
	rdfs:range xsd:string ;
	rdfs:subPropertyOf dc:format ;
	vs:term_status "testing" .

:subtitle a owl:ObjectProperty ;
	rdfs:comment "Relates a version to a subtitle" ;
	rdfs:domain :Version ;
	rdfs:isDefinedBy <http://purl.org/ontology/po/> ;
	rdfs:label "subtitle" ;
	rdfs:range :Subtitle ;
	vs:term_status "testing" .

:subtitle_language a owl:DatatypeProperty ;
	rdfs:comment "Language of a subtitle" ;
	rdfs:domain :Subtitle ;
	rdfs:isDefinedBy <http://purl.org/ontology/po/> ;
	rdfs:label "subtitle language" ;
	rdfs:range xsd:string ;
	vs:term_status "testing" .

:subtitle_supplemental a owl:DatatypeProperty ;
	rdfs:comment "Supplemental of a subtitle" ;
	rdfs:domain :Subtitle ;
	rdfs:isDefinedBy <http://purl.org/ontology/po/> ;
	rdfs:label "subtitle supplemental" ;
	rdfs:range xsd:string ;
	vs:term_status "unstable" .

:subtitle_type a owl:DatatypeProperty ;
	rdfs:comment "The type of a subtitle (open or closed)" ;
	rdfs:domain :Subtitle ;
	rdfs:isDefinedBy <http://purl.org/ontology/po/> ;
	rdfs:label "subtitle type" ;
	rdfs:range xsd:string ;
	vs:term_status "unstable" .

:synopsis a owl:DatatypeProperty ;
	rdfs:comment """
		The synopsis of a serie, brand or episode.
		This is a subproperty of dc:description.
	""" ;
	rdfs:domain :Programme ;
	rdfs:isDefinedBy <http://purl.org/ontology/po/> ;
	rdfs:label "synopsis" ;
	rdfs:range xsd:string ;
	rdfs:subPropertyOf dc:description ;
	vs:term_status "testing" .

:update_date a owl:DatatypeProperty ;
	rdfs:comment """
		The update date of a thing (last update).
		Sub-property of dc:date
	""" ;
	rdfs:isDefinedBy <http://purl.org/ontology/po/> ;
	rdfs:label "update date" ;
	rdfs:range xsd:dateTime ;
	rdfs:subPropertyOf dc:date ;
	vs:term_status "testing" .

:version a owl:InverseFunctionalProperty , owl:ObjectProperty ;
	rdfs:comment """
		Associate an episode to a version of it.
		Different versions of a same episode can exist (shortened version, version
		designed for the hearing impaired, etc.). 
	""" ;
	rdfs:domain :Episode ;
	rdfs:isDefinedBy <http://purl.org/ontology/po/> ;
	rdfs:label "version" ;
	rdfs:range :Version ;
	vs:term_status "testing" .
