@prefix : <http://www.w3.org/ns/radion#> .
@prefix wdrs: <http://www.w3.org/2007/05/powder-s#> .
@prefix foaf: <http://xmlns.com/foaf/0.1/> .
@prefix vann: <http://purl.org/vocab/vann/> .
@prefix dcterms: <http://purl.org/dc/terms/> .
@prefix sioc: <http://rdfs.org/sioc/ns#> .
@prefix schema: <http://schema.org/> .
@prefix rdfs: <http://www.w3.org/2000/01/rdf-schema#> .
@prefix dcat: <http://www.w3.org/ns/dcat#> .
@prefix xsd: <http://www.w3.org/2001/XMLSchema#> .
@prefix owl: <http://www.w3.org/2002/07/owl#> .
@prefix rdf: <http://www.w3.org/1999/02/22-rdf-syntax-ns#> .
@prefix xhv: <http://www.w3.org/1999/xhtml/vocab#> .
@prefix skos: <http://www.w3.org/2004/02/skos/core#> .
@prefix cc: <http://creativecommons.org/ns#> .

<http://www.w3.org/ns/radion#> a owl:Ontology ;
	rdfs:label "Repository Asset Distribution (RADion)"@en ;
	rdfs:comment "This file specifies the set of RDF classes and properties used in RADion"@en ;
	owl:versionInfo "Version 1.2 11 October 2012"@en ;
	dcterms:modified "2012-10-11"^^xsd:date ;
	xhv:last <http://www.w3.org/ns/radion#> ;
	vann:preferredNamespaceUri "http://www.w3.org/ns/radion#"@en ;
	vann:preferredNamespacePrefix "radion"@en ;
	dcterms:creator _:node17k1l9dmux1 .

_:node17k1l9dmux1 rdfs:seeAlso <http://makxdekkers.com/makxdekkers.rdf#me> ;
	foaf:name "Makx Dekkers"@en ;
	foaf:homepage <http://makxdekkers.com/> .

<http://www.w3.org/ns/radion#> dcterms:creator _:node17k1l9dmux2 .

_:node17k1l9dmux2 rdfs:seeAlso <http://andrea-perego.name/foaf/#me> ;
	foaf:name "Andrea Perego"@en ;
	foaf:homepage <http://andrea-perego.name/> ;
	schema:affiliation _:node17k1l9dmux3 .

_:node17k1l9dmux3 foaf:name "European Commission, JRC-IES"@en .

<http://www.w3.org/ns/radion#> dcterms:creator _:node17k1l9dmux4 .

_:node17k1l9dmux4 rdfs:seeAlso <http://philarcher.org/foaf.rdf#me> ;
	foaf:name "Phil Archer"@en ;
	foaf:homepage <http://philarcher.org/> ;
	schema:affiliation _:node17k1l9dmux5 .

_:node17k1l9dmux5 foaf:name "W3C/ERCIM"@en .

<http://www.w3.org/ns/radion#> foaf:maker _:node17k1l9dmux6 .

_:node17k1l9dmux6 foaf:name "ADMS Working Group"@en ;
	foaf:page <http://joinup.ec.europa.eu/asset/adms/home> .

<http://www.w3.org/ns/radion#> dcterms:description """<p xmlns=\"http://www.w3.org/ns/radion#\">The Repository Asset Distribution (RADion) was developed under the European 
          Commission's <a href=\"http://ec.europa.eu/isa/\">ISA Programme</a>. More information is available from the European Commission's
          <a href=\"http://joinup.ec.europa.eu/asset/radion/description\">Joinup portal</a>. This includes background information,
          use cases, the conceptual model and full definitions for all terms used.</p> 
    """^^rdf:XMLLiteral ;
	dcterms:abstract """RADion, and the higher level vocabularies that build upon it, are 
    intended as a model that facilitates federation 
    and co-operation. It is not the primary intention that repository owners 
    redesign or convert their current systems and data to conform to RADion, but 
    rather that it acts as a common layer among repositories that want to 
    exchange data."""@en ;
	wdrs:describedby <https://joinup.ec.europa.eu/asset/radion/description> .

<https://joinup.ec.europa.eu/asset/radion/description> dcterms:title "RADion RDF Schema"@en .

<http://www.w3.org/ns/radion#> dcterms:conformsTo <https://joinup.ec.europa.eu/elibrary/document/isa-deliverable-process-and-methodology-developing-core-vocabularies> .

<https://joinup.ec.europa.eu/elibrary/document/isa-deliverable-process-and-methodology-developing-core-vocabularies> dcterms:title "Process and Methodology for Developing Core Vocabularies"@en .

<http://www.w3.org/ns/radion#> dcterms:relation <http://joinup.ec.europa.eu/asset/radion/forum/all> .

<http://joinup.ec.europa.eu/asset/radion/forum/all> a sioc:Forum ;
	dcterms:title "Public comments on RADion"@en .

<http://www.w3.org/ns/radion#> dcterms:rights "Copyright Â© 2012 European Commission."@en ;
	dcterms:license <https://joinup.ec.europa.eu/category/licence/isa-open-metadata-licence-v11> .

<https://joinup.ec.europa.eu/category/licence/isa-open-metadata-licence-v11> dcterms:title "ISA Open Metadata Licence v1.1"@en ;
	cc:attributionName "European Commission"@en ;
	cc:attributionURL <http://ec.europa.eu/> .

<http://www.w3.org/ns/radion#> cc:attributionName "European Commission"@en ;
	cc:attributionURL <http://ec.europa.eu/> .

:Repository a rdfs:Class ;
	rdfs:label "Repository"@en ;
	rdfs:comment """A Repository is a system or service that provides facilities for storage and 
    maintenance of descriptions of Assets and Distributions. A Repository will typically contain descriptions 
    of several Assets and functionality that allows users to search and access these descriptions. The 
    Distributions - the actual files themselves - will typically be available from the Repository or 
    elsewhere on the World Wide Web."""@en ;
	rdfs:isDefinedBy <https://joinup.ec.europa.eu/asset/radion/description> ;
	dcterms:identifier "rad:Repository"@en .

:Asset rdfs:label "Asset"@en ;
	rdfs:comment """An Asset represents the conceptual content of a resource. A particular 
    Asset may have zero or more Distributions in different formats."""@en ;
	rdfs:isDefinedBy <https://joinup.ec.europa.eu/asset/radion/description> ;
	dcterms:identifier "rad:Asset"@en .

:Distribution a rdfs:Class ;
	rdfs:label "Distribution"@en ;
	rdfs:comment """A Distribution is a particular representation or concretisation of an 
    Asset in the form of a downloadable computer file that implements the intellectual content of an 
    Asset. A particular Distribution is typically associated with one Asset."""@en ;
	rdfs:isDefinedBy <https://joinup.ec.europa.eu/asset/radion/description> ;
	dcterms:identifier "rad:Distribution"@en .

dcterms:Agent rdfs:label "Agent"@en ;
	rdfs:comment "A resource that acts or has the power to act."@en ;
	vann:usageNote "The dcterms:Agent class (or a sub class of it) is used in RADion to represent the publisher of a Repository or its components."@en ;
	rdfs:isDefinedBy <http://purl.org/dc/terms/> ;
	dcterms:identifier "dcterms:Agent"@en .

dcterms:Location rdfs:label "Location"@en ;
	rdfs:comment "The dcterms:Location class fully represents the RADion class of Geographic Coverage."@en ;
	vann:usageNote "The <a href=\"https://joinup.ec.europa.eu/asset/core_location/description\" xmlns=\"http://www.w3.org/ns/radion#\">Location Core Vocabulary</a> also uses dcterms:Location."^^rdf:XMLLiteral ;
	rdfs:isDefinedBy <http://www.w3.org/ns/dublincore.org/documents/dcmi-terms/> ;
	dcterms:identifier "dcterms:Location"@en .

dcterms:LinguisticSystem rdfs:label "Language"@en ;
	rdfs:comment "The dcterms:LinguisticSystem class fully represents the RADion concept of Language."@en ;
	vann:usageNote "Used in RADion to provide the language of textual information within an Asset, e.g. the language of the terms in a controlled vocabulary (ideally the set of tags defined by RFC 3066 ) or the language that a specification is written in."@en ;
	rdfs:isDefinedBy <http://purl.org/dc/terms/> ;
	dcterms:identifier "dcterms:LinguisticSystem"@en .

dcterms:FileFormat rdfs:label "File Format"@en ;
	rdfs:comment "The dcterms:FileFormat class fully represents the RADion concept of a file format."@en ;
	vann:usageNote "Used in RADion to provide the technical format that a Distribution is available in, e.g. PDF for a document, XML for a schema."@en ;
	rdfs:isDefinedBy <http://purl.org/dc/terms/> ;
	dcterms:identifier "dcterms:FileFormat"@en .

dcterms:LicenseDocument rdfs:label "License"@en ;
	rdfs:comment "The dcterms:LicenseDocument class fully represents the RADion concept of a Licence"@en ;
	vann:usageNote "Used in RADion to provide the conditions or restrictions that apply to the use of a Distribution, e.g. whether it is in the public domain, or that some restrictions apply like in cases attribution is required, or the Asset can only be used for non-commercial purposes etc."@en ;
	rdfs:isDefinedBy <http://purl.org/dc/terms/> ;
	dcterms:identifier "dcterms:LicenseDocument"@en .

rdfs:Literal rdfs:label "string, URI, dateTime, text"@en ;
	rdfs:comment """At the conceptual level, the rdfs:Literal datatype fully represents the RADion datatypes of 
    a string (an untyped literal) and text (string plus language tag). The RADion datatype of 
    dateTime is also served since that requires a string conformant with ISO 8601:2004 which is 
    true of all relevant xsd datatypes. Likewise a Literal datatyped as xsd:anyURI will fulfil 
    the needs of RADion's URI data type."""@en ;
	rdfs:isDefinedBy <http://www.w3.org/2000/01/rdf-schema#> ;
	dcterms:identifier "rdfs:Literal"@en .

skos:Concept rdfs:label "Code"@en ;
	rdfs:comment """<p xmlns=\"http://www.w3.org/ns/radion#\">The Conceptual Model includes a 'Code' datatype that 
      is used by several classes. This is expressed using the <a href=\"http://www.w3.org/TR/skos-primer/\">SKOS vocabulary</a> with
      a particular 'code' usually being a skos:Concept that is part of a scheme. 
      The intention is that the skos:Concept class be used as follows;</p><ul>
      <li>for the content property, use skos:notation</li>
      <li>the 'list' property will be taken care of by means of the skos:inScheme property;</li>
      <li>the list agency property is likely to be applied to the scheme as a whole for which dcterms:creator is appropriate;</li>
      <li>the list version property can be fulfilled using schema:version (see <a href=\"http://schema.org/CreativeWork\">http://schema.org/CreativeWork</a>)</li></ul>
    """^^rdf:XMLLiteral ;
	rdfs:isDefinedBy <http://www.w3.org/TR/skos-primer/> ;
	dcterms:identifier "skos:Concept"@en .

dcterms:alternative rdfs:label "alternative name"@en ;
	rdfs:comment "The dcterms:alternative property fully represents the RADion property of Alternative Name."@en ;
	vann:usageNote "Used in RADion to provide an alternative name for the Asset: this information may be used to provide additional access points, e.g. allowing indexing of any acronyms, nicknames, shorthand notations or other identifying information that a user might expect to find the Asset under.  The range of dcterms:alternative is rdfs:Literal"@en ;
	rdfs:isDefinedBy <http://purl.org/dc/terms/> ;
	dcterms:identifier "dcterms:alternative"@en .

xhv:last rdfs:label "current version"@en ;
	rdfs:comment "The xhv:last property fully represents the RADion relationship of Current version"@en ;
	rdfs:isDefinedBy <http://www.w3.org/1999/xhtml/vocab#> ;
	vann:usageNote "RADion uses the XHTML 'last' property to link an Asset to the most recent (i.e. current) version."@en ;
	dcterms:identifier "xhv:last"@en .

dcterms:created rdfs:label "date created"@en ;
	rdfs:comment "The dcterms:created property fully represents the RADion property of Date of Creation."@en ;
	vann:usageNote "RADion uses this to provide the creation date of this version of the Repository, Asset or Distribution. RADion expects a datatyped value and for it to be conformant with ISO 8601, preferably using an xsd data type."@en ;
	rdfs:isDefinedBy <http://purl.org/dc/terms/> ;
	dcterms:identifier "dcterms:created"@en .

dcterms:modified rdfs:label "date modified"@en ;
	rdfs:comment "The dcterms:modified property fully represents the RADion property Date of Last Modification."@en ;
	vann:usageNote "RADion uses this to provide the date of latest update of the Repository, Asset or Distribution. RADion expects a datatyped value and for it to be conformant with ISO 8601, preferably using an xsd data type."@en ;
	rdfs:isDefinedBy <http://purl.org/dc/terms/> ;
	dcterms:identifier "dcterms:modified"@en .

dcterms:description rdfs:label "description"@en ;
	rdfs:comment "The dcterms:description property fully covers the RADion property of the same name."@en ;
	vann:usageNote "Used in RADion to provide descriptive text for the Repository, Asset or Distribution."@en ;
	rdfs:isDefinedBy <http://purl.org/dc/terms/> ;
	dcterms:identifier "dcterms:description"@en .

:distribution a rdf:Property ;
	rdfs:label "distribution"@en ;
	rdfs:comment "The distribution relationship associates an Asset (its domain) with a Distribution (its range). It is the inverse of distributionOf"@en ;
	rdfs:isDefinedBy <https://joinup.ec.europa.eu/asset/radion/description> ;
	rdfs:domain :Asset ;
	rdfs:range :Distribution ;
	dcterms:identifier "rad:distribution"@en .

:distributionOf a rdf:Property ;
	rdfs:label "distributionOf"@en ;
	rdfs:comment "The distributionOf relationship associates a Distribution (its domain) with the Asset (its range) of which it is a Distribution. It is the inverse of distribution"@en ;
	rdfs:isDefinedBy <https://joinup.ec.europa.eu/asset/radion/description> ;
	rdfs:domain :Distribution ;
	rdfs:range :Asset ;
	dcterms:identifier "rad:distributionOf"@en .

dcterms:format rdfs:label "format"@en ;
	rdfs:comment "The dcterms:format property fully represents the RADion relationship of the same name"@en ;
	vann:usageNote "Used in RADion to link to the format that the Distribution is available in (e.g. PDF, XML, RDF/XML, HTML) which is provided as a property of dcterms:FileFormat"@en ;
	rdfs:isDefinedBy <http://purl.org/dc/terms/> ;
	dcterms:identifier "dcterms:format"@en .

dcterms:hasPart rdfs:label "includes"@en ;
	rdfs:comment "The dcterms:hasPart property fully represents the RADion relationship of includes."@en ;
	vann:usageNote "RADion uses dcterms:hasPart to link a Repository to an Asset."@en ;
	rdfs:isDefinedBy <http://purl.org/dc/terms/> ;
	dcterms:identifier "dcterms:hasPart"@en .

:keyword a rdf:Property ;
	rdfs:label "keyword"@en ;
	rdfs:comment "A word or phrase used to succinctly descibe the Asset"@en ;
	rdfs:isDefinedBy <https://joinup.ec.europa.eu/asset/radion/description> ;
	rdfs:range rdfs:Literal ;
	dcterms:identifier "rad:keyword"@en .

rdfs:label rdfs:label "label or name"@en ;
	rdfs:comment "The rdfs:label property fully represents the RADion properties of name and label."@en ;
	vann:usageNote "RADion uses this to provide the name or label of any class."@en ;
	rdfs:isDefinedBy <http://www.w3.org/2000/01/rdf-schema#> ;
	dcterms:identifier "rdfs:label"@en .

dcterms:language rdfs:label "language"@en ;
	rdfs:comment "The dcterms:language property fully represents the RADion property of the same name."@en ;
	vann:usageNote "RADion uses this to provide the language of the Asset."@en ;
	rdfs:isDefinedBy <http://purl.org/dc/terms/> ;
	dcterms:identifier "dcterms:language"@en .

dcterms:license rdfs:label "license"@en ;
	rdfs:comment "The dcterms:license property fully represents the RADion relationship of the same name."@en ;
	vann:usageNote "Used in RADion to link to the conditions or restrictions for (re-use) of the Distribution. Note that the range is dcterms:LicenseDocument"@en ;
	rdfs:isDefinedBy <http://purl.org/dc/terms/> ;
	dcterms:identifier "dcterms:license"@en .

xhv:next rdfs:label "next version"@en ;
	rdfs:comment "The xhv:next property fully represents the RADion relationship of Next version"@en ;
	rdfs:isDefinedBy <http://www.w3.org/1999/xhtml/vocab#> ;
	vann:usageNote "RADion uses the XHTML 'next' property to link an Asset to the next most recent version."@en ;
	dcterms:identifier "xhv:next"@en .

xhv:prev rdfs:label "previous version"@en ;
	rdfs:comment "The xhv:prev property fully represents the RADion relationship of Previous version"@en ;
	rdfs:isDefinedBy <http://www.w3.org/1999/xhtml/vocab#> ;
	vann:usageNote "RADion uses the XHTML 'previous' property to link an Asset to the previous version."@en ;
	dcterms:identifier "xhv:prev"@en .

dcterms:publisher rdfs:label "publisher"@en ;
	rdfs:comment "The dcterms:publisher property fully represents the RADion relationship of the same name"@en ;
	vann:usageNote "Used in RADion to link to the organisation responsible for the publication of the Asset, Repository or Distribution. Note that the range is dcterms:Agent."@en ;
	rdfs:isDefinedBy <http://purl.org/dc/terms/> ;
	dcterms:identifier "dcterms:publisher"@en .

dcterms:relation rdfs:label "relation"@en ;
	rdfs:comment "The dcterms:relation property fully represents the RADion related asset property."@en ;
	vann:usageNote "Used in RADion to link any Asset to any other related Asset. RADion expects the object to be of type rad:Asset."@en ;
	rdfs:isDefinedBy <http://purl.org/dc/terms/> ;
	dcterms:identifier "dcterms:relation"@en .

dcterms:isPartOf rdfs:label "repository origin"@en ;
	rdfs:comment "The dcterms:isPartOf property fully represents the RADion relationship of repository origin.."@en ;
	vann:usageNote "RADion uses dcterms:isPartOf to link an Asset to a Repository."@en ;
	rdfs:isDefinedBy <http://purl.org/dc/terms/> ;
	dcterms:identifier "dcterms:isPartOf"@en .

dcterms:spatial rdfs:label "spatial coverage"@en ;
	rdfs:comment "The dcterms:spatial property fully represents the RADion relationship of spatial coverage."@en ;
	vann:usageNote "RADion uses this to link to the geographic region or jurisdiction that the Asset or Repository applies to. Note that the range is dcterms:Location."@en ;
	rdfs:isDefinedBy <http://www.w3.org/ns/dublincore.org/documents/dcmi-terms/> ;
	dcterms:identifier "dcterms:spatial"@en .

dcterms:subject rdfs:label "theme, theme taxonomy"@en ;
	rdfs:comment "The dcterms:subject property fully represents the RADion properties of theme and theme taxonomy."@en ;
	vann:usageNote """The theme relationship associates an Asset with a specific Theme and theme taxonomy 
    does the same job for the repository as a whole. Themes are typically, but not necessarily,
    encoded as a skos:Concept, arranged in a skos:ConceptScheme."""@en ;
	rdfs:isDefinedBy <http://www.w3.org/ns/dublincore.org/documents/dcmi-terms/> ;
	dcterms:identifier "dcterms:subject"@en .

dcterms:type rdfs:label "type"@en ;
	rdfs:comment "The dcterms:type property fully represents the RADion property of type."@en ;
	vann:usageNote "Used in RADion to link a Licence or Publisher to its type."@en ;
	rdfs:isDefinedBy <https://joinup.ec.europa.eu/asset/radion/description> ;
	dcterms:identifier "dcterms:type"@en .

:version a rdf:Property ;
	rdfs:label "version"@en ;
	rdfs:comment "The version number or other designation of the Asset; the value should be a free text string"@en ;
	rdfs:isDefinedBy <https://joinup.ec.europa.eu/asset/radion/description> ;
	rdfs:range rdfs:Literal ;
	dcterms:identifier "rad:version"@en .

:versionNotes a rdf:Property ;
	rdfs:label "version notes"@en ;
	rdfs:comment "Notes on the particular version of the Asset."@en ;
	rdfs:isDefinedBy <https://joinup.ec.europa.eu/asset/radion/description> ;
	rdfs:range rdfs:Literal ;
	dcterms:identifier "rad:versionNotes"@en .

<http://www.w3.org/ns/radion#> dcterms:creator _:node17k1l9dmux7 .

_:node17k1l9dmux7 rdfs:seeAlso <http://makxdekkers.com/makxdekkers.rdf#me> ;
	foaf:name "Makx Dekkers"@en ;
	foaf:homepage <http://makxdekkers.com/> .

<http://www.w3.org/ns/radion#> dcterms:creator _:node17k1l9dmux8 .

_:node17k1l9dmux8 rdfs:seeAlso <http://andrea-perego.name/foaf/#me> ;
	foaf:name "Andrea Perego"@en ;
	foaf:homepage <http://andrea-perego.name/> ;
	schema:affiliation _:node17k1l9dmux9 .

_:node17k1l9dmux9 foaf:name "European Commission, JRC-IES"@en .

<http://www.w3.org/ns/radion#> dcterms:creator _:node17k1l9dmux10 .

_:node17k1l9dmux10 rdfs:seeAlso <http://philarcher.org/foaf.rdf#me> ;
	foaf:name "Phil Archer"@en ;
	foaf:homepage <http://philarcher.org/> ;
	schema:affiliation _:node17k1l9dmux11 .

_:node17k1l9dmux11 foaf:name "W3C/ERCIM"@en .

<http://www.w3.org/ns/radion#> foaf:maker _:node17k1l9dmux12 .

_:node17k1l9dmux12 foaf:name "ADMS Working Group"@en ;
	foaf:page <http://joinup.ec.europa.eu/asset/adms/home> .
