@prefix adms:  <http://www.w3.org/ns/adms#> .
@prefix dc:    <http://purl.org/dc/elements/1.1/> .
@prefix rdfs:  <http://www.w3.org/2000/01/rdf-schema#> .
@prefix foaf:  <http://xmlns.com/foaf/0.1/> .
@prefix scsv:  <http://purl.org/NET/schema-org-csv#> .
@prefix owl:   <http://www.w3.org/2002/07/owl#> .
@prefix xsd:   <http://www.w3.org/2001/XMLSchema#> .
@prefix rdf:   <http://www.w3.org/1999/02/22-rdf-syntax-ns#> .
@prefix vann:  <http://purl.org/vocab/vann/> .
@prefix dcterms: <http://purl.org/dc/terms/> .

<http://vocab.deri.ie/scsv#ttl>
        a                   adms:SemanticDistribution ;
        dcterms:FileFormat  <http://vocab.deri.ie/scsv> ;
        adms:accessURL      "http://vocab.deri.ie/scsv.ttl" ;
        adms:status         <http://purl.org/adms/status/Completed> .

scsv:cell  a          rdf:Property ;
        rdfs:comment  "A row has one or more cells (or field as of http://tools.ietf.org/html/rfc4180), each of which is connected to the row with this property." ;
        rdfs:domain   scsv:Row ;
        rdfs:label    "has cell" .

scsv:Row  a           owl:Class , rdfs:Class ;
        rdfs:comment  "A row (or record as of http://tools.ietf.org/html/rfc4180)." ;
        rdfs:label    "row" .

scsv:row  a           rdf:Property ;
        rdfs:comment  "A table has one or more rows, each of which is connected to the table via this property." ;
        rdfs:domain   scsv:Table ;
        rdfs:label    "has row" ;
        rdfs:range    scsv:Row .

<http://vocab.deri.ie/scsv#Michael%20Hausenblas>
        a              foaf:Person ;
        foaf:homepage  <http://sw-app.org/about.html> ;
        foaf:mbox      <mailto:michael.hausenblas@deri.org> ;
        foaf:name      "Michael Hausenblas" .

<http://vocab.deri.ie/scsv>
        a                              adms:SemanticAsset , owl:Ontology ;
        dc:creator                     <http://vocab.deri.ie/scsv#Michael%20Hausenblas> ;
        dcterms:created                "2011-06-10"^^xsd:date ;
        dcterms:description            "Mapping vocabulary for CSV files that use Schema.org terms in the header." ;
        dcterms:modified               "2012-05-22"^^xsd:date ;
        dcterms:partOf                 <http://vocab.deri.ie> ;
        dcterms:publisher              "http://vocab.deri.ie/scsv#LiDRC" ;
        dcterms:status                 <http://purl.org/adms/status/UnderDevelopment> ;
        dcterms:title                  "Schema.org CSV" ;
        dcterms:type                   <http://purl.org/adms/assettype/Ontology> ;
        vann:preferredNamespacePrefix  "scsv" ;
        vann:preferredNamespaceUri     "http://purl.org/NET/schema-org-csv#" ;
        foaf:homepage                  <http://vocab.deri.ie/scsv.html> .

<http://vocab.deri.ie/scsv#rdf>
        a                   adms:SemanticDistribution ;
        dcterms:FileFormat  <http://vocab.deri.ie/scsv> ;
        adms:accessURL      "http://vocab.deri.ie/scsv.rdf" ;
        adms:status         <http://purl.org/adms/status/Completed> .

scsv:Table  a         owl:Class , rdfs:Class ;
        rdfs:comment  "A CSV table as of http://tools.ietf.org/html/rfc4180." ;
        rdfs:label    "table" .

scsv:HeaderRow  a        owl:Class , rdfs:Class ;
        rdfs:comment     "The header row, that is the first row of the table that contains the column heads that are matched against Schema.org terms." ;
        rdfs:label       "header row" ;
        rdfs:subClassOf  scsv:Row .

<http://vocab.deri.ie/scsv#LiDRC>
        a              dcterms:Agent ;
        foaf:homepage  <http://linkeddata.deri.ie/> ;
        foaf:member    <http://vocab.deri.ie/scsv#Michael%20Hausenblas> ;
        foaf:name      "LiDRC" .
