@prefix :      <http://securitytoolbox.appspot.com/securityMain#> .
@prefix rdfs:  <http://www.w3.org/2000/01/rdf-schema#> .
@prefix assurance: <http://www.kim.com/NRLOntologyFiles/securityAssurance.owl#> .
@prefix owl:   <http://www.w3.org/2002/07/owl#> .
@prefix xsd:   <http://www.w3.org/2001/XMLSchema#> .
@prefix rdf:   <http://www.w3.org/1999/02/22-rdf-syntax-ns#> .
@prefix credentials: <http://www.kim.com/NRLOntologyFiles/credentials.owl#> .
@prefix security: <http://securitytoolbox.appspot.com/securityMain#> .
@prefix algorithms: <http://securitytoolbox.appspot.com/securityAlgorithms#> .

security:XML-dsig  a  security:SignatureProtocol .

security:SecurityMechanism
        a                owl:Class ;
        rdfs:subClassOf  security:SecurityConcept .

security:NetworkMechanism
        a                owl:Class ;
        rdfs:subClassOf  security:SecurityMechanism .

security:SecurityProtocol
        a                owl:Class ;
        rdfs:subClassOf  security:SecurityConcept .

security:OnionRouter  a  security:NetworkMechanism ;
        security:supportsSecurityObjectives
                security:Confidentiality , security:Anonymity .

security:MessageAuthentication
        a             security:SecurityObjective ;
        rdfs:comment  "\nProvides guarantee that message came from whoever claimed to have sent it.\n" .

security:reqCredential
        a            owl:ObjectProperty ;
        rdfs:domain  security:SecurityProtocol ;
        rdfs:range   credentials:Credential .

security:hasAlgorithm
        a            owl:ObjectProperty ;
        rdfs:domain  security:SecurityProtocol ;
        rdfs:range   algorithms:Algorithm .

security:ApplicationMechanism
        a                owl:Class ;
        rdfs:subClassOf  security:SecurityMechanism .

security:XML-enc  a  security:EncryptionProtocol .

security:SoapFirewall
        a       security:ServiceMechanism ;
        security:supportsSecurityobjectives
                security:Authorization .

security:Availability
        a             security:SecurityObjective ;
        rdfs:comment  "\nProvides guarantee that resource is available to authorized users at any\nauthorized time.\n" .

security:ReplayPrevention
        a             security:SecurityObjective ;
        rdfs:comment  "\n(Secondary Objective) Protect against replay attacks\n" .

security:EncryptionProtocol
        a                owl:Class ;
        rdfs:subClassOf  security:SecurityProtocol ;
        rdfs:subClassOf  [ a               owl:Restriction ;
                           owl:hasValue    security:Confidentiality ;
                           owl:onProperty  security:supportsSecurityObjectives
                         ] .

security:VMM  a  security:HostMechanism ;
        security:supportsSecurityObjectives
                security:HostTrust .

security:TrafficHiding
        a             security:SecurityObjective ;
        rdfs:comment  "\n(Secondary Objective) Pad traffic with bogus data to hide traffic patterns\n" .

security:SecurityConcept
        a       owl:Class .

security:hasAssurance
        a            owl:ObjectProperty ;
        rdfs:domain  [ a            owl:Class ;
                       owl:unionOf  ( security:SecurityProtocol security:SecurityMechanism )
                     ] ;
        rdfs:range   assurance:Assurance .

security:LoginProtocol
        a       security:AuthenticationProtocol .

security:CovertChannelPrevention
        a             security:SecurityObjective ;
        rdfs:comment  "\n(Secondary Objective) Prevent or limit the existance of covert channels\n" .

security:SecurityObjective
        a       owl:Class .

security:Separation  a  security:SecurityObjective ;
        rdfs:comment  "\n(Secondary Objective)\n" .

security:supportsSecurityObjectives
        a             owl:ObjectProperty ;
        rdfs:comment  "\nAny SecurityConcept can support one or more of the Security Objectives defined\nin the SecurityObjective class\n" ;
        rdfs:domain   security:SecurityConcept ;
        rdfs:range    security:SecurityObjective .

[ a             owl:Ontology ;
  rdfs:comment  "\nA security ontology to annotate resources with security-related information\n"
] .

security:SecurityPolicy
        a                owl:Class ;
        rdfs:subClassOf  security:SecurityConcept ;
        rdfs:subClassOf  [ a               owl:Restriction ;
                           owl:hasValue    <http://securitytoolbox.appspot.com/Authorization> ;
                           owl:onProperty  <http://securitytoolbox.appspot.com/supportsSecurityObjectives>
                         ] .

security:MLSPump  a  security:NetworkMechanism ;
        security:supportsSecurityObjectives
                security:CovertChannelPrevention .

security:AuthenticationProtocol
        a                owl:Class ;
        rdfs:subClassOf  security:SecurityProtocol ;
        rdfs:subClassOf  [ a               owl:Restriction ;
                           owl:hasValue    security:UserAuthentication ;
                           owl:onProperty  security:supportsSecurityObjectives
                         ] .

security:HostTrust  a  security:SecurityObjective ;
        rdfs:comment  "\n(Secondary Objective) How to trust host or platform. Is relevant to Common\ncriteria, etc.\n" .

security:SSH  a  security:NetworkSecurityProtocol ;
        security:supportsSecurityObjectives
                security:MessageAuthentication , security:UserAuthentication , security:Confidentiality , security:Integrity .

security:HostMechanism
        a                owl:Class ;
        rdfs:subClassOf  security:SecurityMechanism .

security:Kerberos  a  security:AuthenticationProtocol .

security:MessageIntegrity
        a             security:SecurityObjective ;
        rdfs:comment  "\nData integrity or Message integrity; data cannot be changed, deleted,\nmodified, etc by unauthorized parties.\n" .

security:Authorization
        a             security:SecurityObjective ;
        rdfs:comment  "\nOnly authorized entities are allowed to access resources in an authorized\nmanner.\n(Aka Access Control). If desired, user may create instance of AccessControl as\nwell.\n" .

security:ChineseWall  a  security:CommercialPolicy .

security:IPSec  a  security:NetworkSecurityProtocol ;
        security:supportsSecurityObjectives
                security:Confidentiality , security:Integrity , security:MessageAuthentication .

security:Anonymity  a  security:SecurityObjective ;
        rdfs:comment  "\n(Secondary Objective) Provides anonymity\n" .

security:VPN  a  security:NetworkMechanism ;
        security:supportsSecurityObjectives
                security:Separation , security:Confidentiality .

security:TLS  a     security:NetworkSecurityProtocol ;
        security:supportsSecurityObjectives
                security:Confidentiality , security:UserAuthentication ;
        owl:sameAs  security:SSL .

security:MilitaryPolicy
        a                owl:Class ;
        rdfs:subClassOf  security:SecurityPolicy .

security:hasEncryptionAlgorithm
        a                   owl:ObjectProperty ;
        rdfs:range          algorithms:EncryptionAlgorithm ;
        rdfs:subPropertyOf  security:hasAlgorithm .

security:SSL  a     security:NetworkSecurityProtocol ;
        security:supportsSecurityObjectives
                security:UserAuthentication , security:Confidentiality ;
        owl:sameAs  security:TLS .

security:CommercialPolicy
        a                owl:Class ;
        rdfs:subClassOf  security:SecurityPolicy .

security:KeyManagementProtocol
        a                owl:Class ;
        rdfs:subClassOf  security:SecurityProtocol ;
        rdfs:subClassOf  [ a               owl:Restriction ;
                           owl:hasValue    security:KeyManagement ;
                           owl:onProperty  security:supportsSecurityObjectives
                         ] .

security:ServiceMechanism
        a                owl:Class ;
        rdfs:subClassOf  security:SecurityMechanism .

security:UserAuthentication
        a             security:SecurityObjective ;
        rdfs:comment  "\nProvides assurance of the identity of a person or entity.\n" .

security:SAML  a  security:AuthenticationProtocol .

security:BLP  a       security:MilitaryPolicy ;
        rdfs:comment  "\nBell La-Padula\n" .

security:KeyManagement
        a             security:SecurityObjective ;
        rdfs:comment  "\n(SecondaryObjective) Securely manages keys for legitimate users.\n" .

security:Confidentiality
        a             security:SecurityObjective ;
        rdfs:comment  "\nProtects against information being disclosed or revealed to unauthorized\nparties.\n" .

security:hasSignatureAlgorithm
        a                   owl:ObjectProperty ;
        rdfs:range          algorithms:SignatureAlgorithm ;
        rdfs:subPropertyOf  security:hasAlgorithm .

security:ClarkWilson  a  security:CommercialPolicy .

security:SignatureProtocol
        a                owl:Class ;
        rdfs:subClassOf  security:SecurityProtocol ;
        rdfs:subClassOf  [ a               owl:Restriction ;
                           owl:hasValue    security:MessageAuthentication ;
                           owl:onProperty  security:supportsSecurityObjectives
                         ] .

security:NetworkSecurityProtocol
        a                owl:Class ;
        rdfs:subClassOf  security:SecurityProtocol .

security:RBAC  a      security:SecurityPolicy ;
        rdfs:comment  "\nRole-based Access Control\n" .

security:XKMS  a  security:KeyManagementProtocol .

security:Trust  a     security:SecurityObjective ;
        rdfs:comment  "\n(Secondary Objective) How to trust entity. Trust not only of identification,\nbut statements, claims, etc.\n" .

security:Safehost  a  security:HostMechanism ;
        security:supportsSecurityObjectives
                security:HostTrust .
