@prefix bbcevent: <http://www.bbc.co.uk/ontologies/event/> .
@prefix geo: <http://www.w3.org/2003/01/geo/wgs84_pos#> .
@prefix tl: <http://purl.org/NET/c4dm/timeline.owl#> .
@prefix foaf: <http://xmlns.com/foaf/0.1/> .
@prefix tag: <http://purl.org/ontology/tag/> .
@prefix geoname: <http://www.geonames.org/ontology#> .
@prefix sport: <http://purl.org/ontology/sport/> .
@prefix ontology: <http://www.bbc.co.uk/ontology/> .
@prefix protons: <http://proton.semanticweb.org/2005/04/protons#> .
@prefix dcterms: <http://purl.org/dc/terms/> .
@prefix rdfs: <http://www.w3.org/2000/01/rdf-schema#> .
@prefix participation: <http://purl.org/vocab/participation/schema#> .
@prefix event: <http://purl.org/NET/c4dm/event.owl#> .
@prefix xsd: <http://www.w3.org/2001/XMLSchema#> .
@prefix owl: <http://www.w3.org/2002/07/owl#> .
@prefix rdf: <http://www.w3.org/1999/02/22-rdf-syntax-ns#> .
@prefix po: <http://purl.org/ontology/po/> .
@prefix skos: <http://www.w3.org/2004/02/skos/core> .

<http://purl.org/ontology/sport/> a owl:Ontology ;
	dcterms:title "Sport Ontology"@en ;
	rdfs:comment "A simple ontology for representing competitive sports events."@en ;
	foaf:maker <http://uk.linkedin.com/pub/jem-rayfield/27/b19/757> , <http://uk.linkedin.com/in/paulwilton> , <http://www.blockslabpillar.com> , <http://uk.linkedin.com/in/brianwmcbride> , <http://uk.linkedin.com/pub/stuart-williams/8/684/351> ;
	dcterms:created "2011-02-17"^^xsd:date .

<http://uk.linkedin.com/pub/jem-rayfield/27/b19/757> a foaf:Person ;
	foaf:name "Jem Rayfield" .

<http://uk.linkedin.com/in/paulwilton> a foaf:Person ;
	foaf:name "Paul Wilton" .

<http://www.blockslabpillar.com> a foaf:Person ;
	foaf:name "Silver Oliver" .

sport:Competition a owl:Class ;
	rdfs:comment "A competitive sporting event."@en ;
	rdfs:label "Competition"@en ;
	rdfs:subClassOf event:Event .

sport:RecurringCompetition a owl:Class ;
	rdfs:comment "A recurring sports competition."@en ;
	rdfs:subClassOf bbcevent:RecurringEvent ;
	rdfs:label "Recurring competition"@en .

sport:CompetitiveSportingOrganisation a owl:Class ;
	rdfs:comment "A sporting organisation that participates in competitive sporting events. For example Manchester United or Great Britain Olympic Team. "@en ;
	rdfs:label "Competitive sporting organisation"@en ;
	rdfs:subClassOf sport:SportingOrganisation .

sport:SportsDiscipline a owl:Class ;
	rdfs:comment "The type of discipline a sporting event involves."@en ;
	rdfs:label "Sports discipline"@en .

sport:DivisionalCompetition a owl:Class ;
	rdfs:label "Divisional competition"@en ;
	rdfs:comment "A DivisionalCompetition is a competition that is divided into a number of divisions each of which is an award. Examples of DivisionalCompetition include the English football league and the annual Wimbledon tennis tournament."@en ;
	rdfs:subClassOf sport:Competition .

sport:EventGender a owl:Class ;
	rdfs:comment "The gender of the sporting event."@en ;
	rdfs:label "Event gender"@en .

sport:GroupCompetition a owl:Class ;
	rdfs:comment "A group competition is a competition organised as a collection of leagues used to select the top N competitors from each league. An example of a group competition would be group stage of the World Cup."@en ;
	rdfs:label "Group competition"@en ;
	rdfs:subClassOf sport:MultiRoundCompetition .

sport:KnockoutCompetition a owl:Class ;
	rdfs:comment "A knockout stage is a competition or stage of a competition that is structured as a knockout competition. Examples of a knockout competition include the last stage of the work cup and the men's tournament at Wimbledon."@en ;
	rdfs:label "Knock out competition"@en ;
	rdfs:subClassOf sport:MultiRoundCompetition .

sport:LeagueCompetition a owl:Class ;
	rdfs:comment "A league competition is a competition or stage in a competition that has a league format. Example of league competition would be the Premier League. "@en ;
	rdfs:label "League competition"@en ;
	rdfs:subClassOf sport:MultiRoundCompetition .

sport:Match a owl:Class ;
	rdfs:comment "A type of unit competition. Example of a match would be a football or tennis match."@en ;
	rdfs:label "Match"@en ;
	rdfs:subClassOf sport:UnitCompetition .

sport:MultiRoundCompetition a owl:Class ;
	rdfs:comment "A multiround competition is a competition that is organised as a sequence of rounds. Example of a multi round competition would be the Premier League or a group stage of the World Cup."@en ;
	rdfs:label "Multiround competition"@en ;
	rdfs:subClassOf sport:Competition .

sport:MultiStageCompetition a owl:Class ;
	rdfs:comment "A multistage competition is a competition that is organised as a sequence of stages. Examples of multistage competitions include the football World Cup."@en ;
	rdfs:label "Multistage competition"@en ;
	rdfs:subClassOf sport:Competition .

sport:Round a owl:Class ;
	rdfs:comment "A round is one or more competitions that are a part of a multiround competition. Examples of a round are the first round of wimbledon and the final round of the FA cup."@en ;
	rdfs:label "Round"@en ;
	rdfs:subClassOf event:Event .

sport:FootballPlayerRole a owl:Class ;
	rdfs:label "Football player role"@en ;
	rdfs:subClassOf participation:Role .

sport:FootballManagerRole a owl:Class ;
	rdfs:label "Football manager role"@en ;
	rdfs:subClassOf participation:Role .

sport:SportGoverningBody a owl:Class ;
	rdfs:comment "A sport governing body is a sports organisation that has a regulatory or sanctioning function. Example of a sport governing body would be FIFA."@en ;
	rdfs:label "Sport governing body"@en ;
	rdfs:subClassOf sport:SportingOrganisation .

sport:SportingOrganisation a owl:Class ;
	rdfs:comment "A sporting organisation includes any organisation that is involved in competitive sports events. This includes competing or organisation. example of a sporting organisation would be Manchester United or FIFA."@en ;
	rdfs:label "Sporting organisation"@en ;
	rdfs:subClassOf foaf:Organisation .

sport:CompetitiveSportingGroup a owl:Class ;
	rdfs:comment "The group of agents that are involved in sporting competitions. Two groups with the same members are not necessarily the same group. Example: The 2010 World Cup England Squad and the 2012 European Championship squad."@en ;
	rdfs:label "Competitive Sporting group"@en ;
	rdfs:subClassOf foaf:Group .

sport:CompetitionType a owl:Class ;
	rdfs:comment "The type of competition the event is. Examples would include domestic league competitions or a European cup competitions."@en ;
	rdfs:label "Competition Type"@en .

sport:UnitCompetition a owl:Class ;
	rdfs:comment "A unit competition is the lowest level of competition with an associated award or result. Examples of unit competition include a 100m race and a football match."@en ;
	rdfs:label "Unit competition"@en ;
	rdfs:subClassOf sport:Competition .

sport:Session a owl:Class ;
	rdfs:comment "A session is a named interval of a competition. For example day 3 of a test match or a session in the track event at the Olympics."@en ;
	rdfs:label "Session"@en ;
	rdfs:subClassOf bbcevent:Event .

sport:awayCompetitor a owl:FunctionalProperty , owl:ObjectProperty ;
	rdfs:comment "associates an agent to the event they are competing in with an away status."@en ;
	rdfs:domain sport:Match ;
	rdfs:label "away competitor"@en ;
	rdfs:range foaf:Agent ;
	rdfs:subPropertyOf sport:hasCompetitor .

sport:competesIn a owl:ObjectProperty ;
	rdfs:comment "associates an agent with the sporting event competed in."@en ;
	rdfs:label "competes in"@en ;
	rdfs:domain foaf:Agent ;
	rdfs:range sport:Competition ;
	owl:inverseOf sport:hasCompetitor ;
	protons:transitiveOver bbcevent:recurringEvent .

sport:firstRound a owl:FunctionalProperty , owl:ObjectProperty ;
	rdfs:comment "associates a multiround competition to the first round in the competition"@en ;
	rdfs:label "first round"@en ;
	rdfs:domain sport:MultiRoundCompetition ;
	rdfs:range sport:Round ;
	rdfs:subPropertyOf sport:hasRound .

sport:firstStage a owl:FunctionalProperty ;
	rdfs:comment "associates a multi staged competition to its first stage."@en ;
	rdfs:domain sport:MultiStageCompetition ;
	rdfs:label "first stage"@en ;
	rdfs:range sport:Competition ;
	rdfs:subPropertyOf sport:hasStage .

sport:firstUnitCompetition a owl:ObjectProperty ;
	rdfs:comment "associates a multiround competition to its first unit competition."@en ;
	rdfs:label "first unit competition"@en ;
	rdfs:domain sport:Competition ;
	rdfs:range sport:UnitCompetition ;
	rdfs:subPropertyOf sport:hasUnitCompetition .

sport:firstSession a owl:ObjectProperty ;
	rdfs:comment "associates a competition to the first session of a series of sessions."@en ;
	rdfs:label "first session"@en ;
	rdfs:domain sport:Competition ;
	rdfs:range sport:Session ;
	rdfs:subPropertyOf sport:hasSession .

sport:hasCompetitor a owl:ObjectProperty ;
	rdfs:comment "associates a competition with those agents competition."@en ;
	rdfs:domain sport:Competition ;
	rdfs:label "has competitor"@en ;
	rdfs:range foaf:Agent ;
	owl:inverseOf sport:competesIn .

sport:hasDivision a rdf:Property ;
	rdfs:comment "associates a DivisionalCompetition to a competition which is a division of that DivisionalCompetition."@en ;
	rdfs:domain sport:DivisionalCompetition ;
	rdfs:range sport:Competition ;
	rdfs:label "has division"@en ;
	rdfs:seeAlso sport:hasDivisionList .

sport:isGroupOf a owl:ObjectProperty ;
	rdfs:domain sport:GroupCompetition ;
	rdfs:comment "associates a group competition with the groups it contains. Example would be associating group stage of World Cup 2010 with Group B."@en ;
	rdfs:label "is group of"@en ;
	rdfs:range sport:LeagueCompetition .

sport:hasGroup a owl:ObjectProperty ;
	owl:inverseOf sport:isGroupOf ;
	rdfs:comment "associates a group with a group competition. Example would be associating Group B of World Cup 2010 with the group stage."@en ;
	rdfs:domain sport:LeagueCompetition ;
	rdfs:label "has group"@en ;
	rdfs:range sport:GroupCompetition .

sport:isCompetitiveSportingOrganisationOf a owl:FunctionalProperty , owl:ObjectProperty ;
	rdfs:comment "associates a group with the competitive sporting organisation it represents. Example would be 2010 England squad associated with the England football team."@en ;
	rdfs:domain sport:CompetitiveSportingGroup ;
	rdfs:label "is competitive sporting organisation of"@en ;
	rdfs:range sport:CompetitiveSportingOrganisation .

sport:hasMatch a owl:ObjectProperty ;
	rdfs:comment "associates a round with a match."@en ;
	rdfs:domain sport:Round ;
	rdfs:label "has match"@en ;
	rdfs:range sport:Match ;
	rdfs:subPropertyOf sport:hasUnitCompetition .

sport:hasRound a owl:ObjectProperty ;
	rdfs:comment "associates a multiround competition to a round in that competition."@en ;
	rdfs:domain sport:MultiRoundCompetition ;
	rdfs:label "has competition"@en ;
	rdfs:range sport:Round .

sport:isRoundOf a owl:ObjectProperty ;
	rdfs:comment "associates a round in that competition with a multiround competition."@en ;
	owl:inverseOf sport:hasRound ;
	rdfs:domain sport:Round ;
	rdfs:label "is round of"@en ;
	rdfs:range sport:MultiRoundCompetition .

sport:hasStage a owl:ObjectProperty ;
	rdfs:comment "associates a multi stage competition to the stages that it contains."@en ;
	rdfs:domain sport:MultiStageCompetition ;
	rdfs:label "has stage"@en ;
	rdfs:range sport:Competition .

sport:isStageOf a owl:ObjectProperty ;
	rdfs:comment "associates a stage to a multi stage competition it is contained in."@en ;
	owl:inverseOf sport:hasStage ;
	rdfs:label "is stage of"@en ;
	rdfs:domain sport:Competition ;
	rdfs:range sport:MultiStageCompetition .

sport:hasSession a owl:ObjectProperty ;
	rdfs:comment "associates a competition with a session."@en ;
	rdfs:domain sport:Competition ;
	rdfs:label "has session"@en ;
	rdfs:range sport:Session .

sport:isSessionOf a owl:ObjectProperty ;
	rdfs:comment "associates a session to a competition."@en ;
	owl:inverseOf sport:hasSession ;
	rdfs:label "is session of"@en ;
	rdfs:domain sport:Session ;
	rdfs:range sport:Competition .

sport:hasUnitCompetition a owl:ObjectProperty ;
	rdfs:comment "associates a round to a unit competition in that round."@en ;
	rdfs:domain sport:Round ;
	rdfs:label "has unit competition"@en ;
	rdfs:range sport:UnitCompetition .

sport:homeCompetitor a owl:FunctionalProperty , owl:ObjectProperty ;
	rdfs:domain sport:Match ;
	rdfs:comment "associates an agent to the event they are competing in with an home status."@en ;
	rdfs:label "home competitor"@en ;
	rdfs:subPropertyOf sport:hasCompetitor .

sport:isMatchOf a owl:ObjectProperty ;
	owl:inverseOf sport:hasMatch ;
	rdfs:comment "associates a match with the round it is contained in."@en ;
	rdfs:domain sport:Match ;
	rdfs:range sport:Round ;
	rdfs:label "is match of"@en ;
	protons:transitiveOver sport:isRoundOf , sport:isGroupOf , sport:isStageOf .

sport:isGroupOf a owl:FunctionalProperty ;
	rdfs:comment "associates a group with competitive sporting organisation it represents."@en ;
	rdfs:domain sport:CompetitiveSportingGroup ;
	rdfs:range sport:CompetitiveSportingOrganisation .

sport:lastRound a owl:FunctionalProperty , owl:ObjectProperty ;
	rdfs:comment "associates a multiround competition to the last round in the competition."@en ;
	rdfs:label "last round"@en ;
	rdfs:domain sport:MultiRoundCompetition ;
	rdfs:range sport:Round ;
	rdfs:subPropertyOf sport:hasRound .

sport:lastStage a owl:FunctionalProperty ;
	rdfs:comment "associates a multistage competition to its last stage."@en ;
	rdfs:label "last Stage"@en ;
	rdfs:domain sport:MultiStageCompetition ;
	rdfs:range sport:MultiRoundCompetition ;
	rdfs:subPropertyOf sport:hasStage .

sport:lastUnitCompetition a owl:ObjectProperty ;
	rdfs:comment "associates a competition to its last unit competition."@en ;
	rdfs:label "last unit competition"@en ;
	rdfs:domain sport:Competition ;
	rdfs:range sport:UnitCompetition ;
	rdfs:subPropertyOf sport:hasUnitCompetition .

sport:lastSession a owl:ObjectProperty ;
	rdfs:comment "associates a competition to the last session of a series of sessions."@en ;
	rdfs:label "last session"@en ;
	rdfs:domain sport:Competition ;
	rdfs:range sport:Session ;
	rdfs:subPropertyOf sport:hasSession .

sport:nextRound a owl:FunctionalProperty ;
	rdfs:comment "associates a round to the next round in a multiround competition."@en ;
	rdfs:domain sport:Round ;
	rdfs:label "next round"@en ;
	rdfs:range sport:Round .

sport:nextStage a owl:FunctionalProperty ;
	rdfs:comment "associates a stage to the next stage in a multistage competition."@en ;
	rdfs:domain sport:Competition ;
	rdfs:label "next stage"@en ;
	rdfs:range sport:Competition .

sport:nextUnitCompetition a owl:ObjectProperty ;
	rdfs:comment "associates a multiround competition to its next unit competition."@en ;
	rdfs:label "next unit competition"@en ;
	rdfs:domain sport:Competition ;
	rdfs:range sport:Competition .

sport:nextSession a owl:ObjectProperty ;
	rdfs:comment "associates a session to its next session."@en ;
	rdfs:label "next session"@en ;
	rdfs:domain sport:Session ;
	rdfs:range sport:Session .

sport:prevRound a owl:FunctionalProperty ;
	rdfs:comment "associates a round to the previous round in a multiround competition."@en ;
	rdfs:domain sport:Round ;
	rdfs:label "previous round"@en ;
	rdfs:range sport:Round .

sport:prevStage a owl:FunctionalProperty ;
	rdfs:comment "associates a stage in a multistage competition to its previous stage."@en ;
	rdfs:domain sport:Competition ;
	rdfs:label "previous stage"@en ;
	rdfs:range sport:Competition .

sport:prevUnitCompetition a owl:ObjectProperty ;
	rdfs:comment "associates a multiround competition to its previous unit competition."@en ;
	rdfs:label "previous unit competition"@en ;
	rdfs:domain sport:Competition ;
	rdfs:range sport:Competition .

sport:prevSession a owl:ObjectProperty ;
	rdfs:comment "associates a session to its previous session."@en ;
	rdfs:label "prev session"@en ;
	rdfs:domain sport:Session ;
	rdfs:range sport:Session .

sport:roundNumber a owl:ObjectProperty ;
	rdfs:comment "associates a round with a round number."@en ;
	rdfs:domain sport:Round ;
	rdfs:label "round number"@en ;
	rdfs:range xsd:int .

sport:discipline a owl:ObjectProperty ;
	rdfs:comment "associates a thing with a sports discipline."@en ;
	rdfs:label "Discipline"@en ;
	rdfs:range sport:SportsDiscipline .

sport:subDiscipline a owl:ObjectProperty ;
	rdfs:domain sport:SportsDiscipline ;
	rdfs:comment "associates a discipline with a a child discipline."@en ;
	rdfs:label "Sub-Discipline"@en ;
	rdfs:range sport:SportsDiscipline .

sport:eventGender a owl:ObjectProperty ;
	rdfs:domain sport:Competition ;
	rdfs:comment "associates an event with a gender type."@en ;
	rdfs:label "Event Gender"@en ;
	rdfs:range sport:EventGender .

sport:competitionType a owl:ObjectProperty ;
	rdfs:label "Competition type"@en ;
	rdfs:comment "associates a competition with a competition type. Examples would include domestic league competitions or European cup competitions."@en ;
	rdfs:range sport:CompetitionType .
