@prefix dc:    <http://purl.org/dc/elements/1.1/> .
@prefix msg0:  <http://web.resource.org/cc/> .
@prefix rdfs:  <http://www.w3.org/2000/01/rdf-schema#> .
@prefix foaf:  <http://xmlns.com/foaf/0.1/> .
@prefix status: <http://www.w3.org/2003/06/sw-vocab-status/ns#> .
@prefix dct:   <http://purl.org/dc/terms/> .
@prefix rdf:   <http://www.w3.org/1999/02/22-rdf-syntax-ns#> .
@prefix vann:  <http://purl.org/vocab/vann/> .
@prefix skos:  <http://www.w3.org/2004/02/skos/core#> .

<http://vocab.org/transit/terms/arrivalTime>
        a                 <http://www.w3.org/2002/07/owl#DatatypeProperty> , rdf:Property ;
        rdfs:comment      "The time of day at which the service arrives at the stop. The time is measured from \"noon minus 12h\" (effectively midnight, except for days on which daylight savings time changes occur) at the beginning of the service date. For times occurring after midnight on the service date, the time will be a value greater than 24:00:00 in HH:MM:SS local time for the day on which the trip schedule begins. Services that span multiple dates will have stop times greater than 24:00:00. For example, if a service begins at 10:30:00 p.m. and ends at 2:15:00 a.m. on the following day, the stop times would be 22:30:00 and 26:15:00. "@en ;
        rdfs:domain       <http://vocab.org/transit/terms/ServiceStop> ;
        rdfs:isDefinedBy  <http://vocab.org/transit/terms/> ;
        rdfs:label        "Arrival Time"@en ;
        dct:issued        "2011-03-28"^^<http://www.w3.org/2001/XMLSchema#date> .

<http://vocab.org/transit/terms/station>
        a                 <http://www.w3.org/2002/07/owl#ObjectProperty> , rdf:Property ;
        rdfs:comment      "The station that this stop is part of."@en ;
        rdfs:domain       <http://vocab.org/transit/terms/Stop> ;
        rdfs:isDefinedBy  <http://vocab.org/transit/terms/> ;
        rdfs:label        "Station"@en ;
        rdfs:range        <http://vocab.org/transit/terms/Station> ;
        dct:issued        "2011-03-28"^^<http://www.w3.org/2001/XMLSchema#date> .

<http://vocab.org/transit/terms/Service>
        a                   <http://www.w3.org/2002/07/owl#Class> ;
        rdfs:comment        "A public transport service that operates a route on a given schedule."@en ;
        rdfs:isDefinedBy    <http://vocab.org/transit/terms/> ;
        rdfs:label          "Service"@en ;
        dct:issued          "2011-03-28"^^<http://www.w3.org/2001/XMLSchema#date> ;
        status:term_status  "unstable" .

<http://vocab.org/transit/terms/BusRoute>
        a                   <http://www.w3.org/2002/07/owl#Class> ;
        rdfs:comment        "A public transportation route utilising buses on roads for short- or long-distance travel."@en ;
        rdfs:isDefinedBy    <http://vocab.org/transit/terms/> ;
        rdfs:label          "Bus Route"@en ;
        rdfs:subClassOf     <http://vocab.org/transit/terms/Route> ;
        dct:issued          "2011-03-28"^^<http://www.w3.org/2001/XMLSchema#date> ;
        status:term_status  "unstable" .

<http://vocab.org/transit/terms/color>
        a                 <http://www.w3.org/2002/07/owl#DatatypeProperty> , rdf:Property ;
        rdfs:comment      "A color associated with this route."@en ;
        rdfs:domain       <http://vocab.org/transit/terms/Route> ;
        rdfs:isDefinedBy  <http://vocab.org/transit/terms/> ;
        rdfs:label        "Color"@en ;
        dct:issued        "2011-03-28"^^<http://www.w3.org/2001/XMLSchema#date> .

<http://vocab.org/transit/terms/InboundService>
        a                   <http://www.w3.org/2002/07/owl#Class> ;
        rdfs:comment        "A service that travels in an inbound direction."@en ;
        rdfs:isDefinedBy    <http://vocab.org/transit/terms/> ;
        rdfs:label          "Inbound Service"@en ;
        dct:issued          "2011-03-28"^^<http://www.w3.org/2001/XMLSchema#date> ;
        status:term_status  "unstable" .

<http://vocab.org/transit/terms/serviceStop>
        a                 <http://www.w3.org/2002/07/owl#ObjectProperty> , rdf:Property ;
        rdfs:comment      "The arrival and departure time of a service at a particular stop."@en ;
        rdfs:isDefinedBy  <http://vocab.org/transit/terms/> ;
        rdfs:label        "Service Stop"@en ;
        rdfs:range        <http://vocab.org/transit/terms/ServiceStop> ;
        dct:issued        "2011-03-28"^^<http://www.w3.org/2001/XMLSchema#date> .

<http://vocab.org/transit/terms/Stop>
        a                   <http://www.w3.org/2002/07/owl#Class> ;
        rdfs:comment        "A location where passengers board or disembark from a transit vehicle."@en ;
        rdfs:isDefinedBy    <http://vocab.org/transit/terms/> ;
        rdfs:label          "Transit Stop"@en ;
        dct:issued          "2011-03-28"^^<http://www.w3.org/2001/XMLSchema#date> ;
        status:term_status  "unstable" .

<http://vocab.org/transit/terms/minTransferTime>
        a                 <http://www.w3.org/2002/07/owl#DatatypeProperty> , rdf:Property ;
        rdfs:comment      "The amount of time (in seconds) that must be available in an itinerary to permit a transfer between routes at this transfer point."@en ;
        rdfs:domain       <http://vocab.org/transit/terms/Transfer> ;
        rdfs:isDefinedBy  <http://vocab.org/transit/terms/> ;
        rdfs:label        "Minimum Transfer Time"@en ;
        rdfs:range        <http://vocab.org/transit/terms/Stop> ;
        dct:issued        "2011-03-28"^^<http://www.w3.org/2001/XMLSchema#date> .

<http://vocab.org/transit/terms/RecommendedTransfer>
        a                   <http://www.w3.org/2002/07/owl#Class> ;
        rdfs:comment        "A point that is recommended for transfer between two routes."@en ;
        rdfs:isDefinedBy    <http://vocab.org/transit/terms/> ;
        rdfs:label          "Timed Transfer"@en ;
        rdfs:subClassOf     <http://vocab.org/transit/terms/Transfer> ;
        dct:issued          "2011-03-28"^^<http://www.w3.org/2001/XMLSchema#date> ;
        status:term_status  "unstable" .

<http://vocab.org/transit/terms/disallowed>
        a             <http://vocab.org/transit/terms/AccessArrangement> ;
        rdfs:comment  "The particular form of access is unavailable."@en ;
        rdfs:label    "Disallowed"@en .

<http://vocab.org/transit/terms/departureTime>
        a                 <http://www.w3.org/2002/07/owl#DatatypeProperty> , rdf:Property ;
        rdfs:comment      "The time of day at which the service departs the stop. The time is measured from \"noon minus 12h\" (effectively midnight, except for days on which daylight savings time changes occur) at the beginning of the service date. For times occurring after midnight on the service date, the time will be a value greater than 24:00:00 in HH:MM:SS local time for the day on which the trip schedule begins. Services that span multiple dates will have stop times greater than 24:00:00. For example, if a service begins at 10:30:00 p.m. and ends at 2:15:00 a.m. on the following day, the stop times would be 22:30:00 and 26:15:00. "@en ;
        rdfs:domain       <http://vocab.org/transit/terms/ServiceStop> ;
        rdfs:isDefinedBy  <http://vocab.org/transit/terms/> ;
        rdfs:label        "Departure Time"@en ;
        dct:issued        "2011-03-28"^^<http://www.w3.org/2001/XMLSchema#date> .

<file:///var/www/vocab.org/www/htdocs/transit/>
        a             msg0:Work ;
        dct:type      <http://purl.org/dc/dcmitype/Text> ;
        msg0:license  <http://creativecommons.org/licenses/by/1.0/> .

<http://vocab.org/transit/terms/FerryRoute>
        a                   <http://www.w3.org/2002/07/owl#Class> ;
        rdfs:comment        "A public transportation route utilising boats for short- or long-distance travel."@en ;
        rdfs:isDefinedBy    <http://vocab.org/transit/terms/> ;
        rdfs:label          "Ferry Route"@en ;
        rdfs:subClassOf     <http://vocab.org/transit/terms/Route> ;
        dct:issued          "2011-03-28"^^<http://www.w3.org/2001/XMLSchema#date> ;
        status:term_status  "unstable" .

<http://vocab.org/transit/terms/sequence>
        a                 <http://www.w3.org/2002/07/owl#DatatypeProperty> , rdf:Property ;
        rdfs:comment      "A sequence number for a stop along a route or service. Sequence values are non-negative integers and increase along the route or service however they need not be consecutive."@en ;
        rdfs:isDefinedBy  <http://vocab.org/transit/terms/> ;
        rdfs:label        "Sequence"@en ;
        dct:issued        "2011-03-28"^^<http://www.w3.org/2001/XMLSchema#date> ;
        skos:historyNote  [ rdf:value    "Relaxed domain" ;
                            dct:creator  "Ian Davis" ;
                            dct:date     "2011-08-06"
                          ] .

<http://vocab.org/transit/terms/prearranged>
        a             <http://vocab.org/transit/terms/AccessArrangement> ;
        rdfs:comment  "The particular form of access must be pre-arranged with the transit agency."@en ;
        rdfs:label    "Pre-arranged"@en .

<http://vocab.org/transit/terms/FunicularRoute>
        a                   <http://www.w3.org/2002/07/owl#Class> ;
        rdfs:comment        "A public transportation route utilising a rail system designed for steep inclines."@en ;
        rdfs:isDefinedBy    <http://vocab.org/transit/terms/> ;
        rdfs:label          "Funicular Route"@en ;
        rdfs:subClassOf     <http://vocab.org/transit/terms/Route> ;
        dct:issued          "2011-03-28"^^<http://www.w3.org/2001/XMLSchema#date> ;
        status:term_status  "unstable" .

<http://vocab.org/transit/terms/TimedTransfer>
        a                   <http://www.w3.org/2002/07/owl#Class> ;
        rdfs:comment        "A transfer point between two routes where the departing vehicle is expected to wait for the arriving one with sufficient time for a passenger to transfer between routes."@en ;
        rdfs:isDefinedBy    <http://vocab.org/transit/terms/> ;
        rdfs:label          "Timed Transfer"@en ;
        rdfs:subClassOf     <http://vocab.org/transit/terms/Transfer> ;
        dct:issued          "2011-03-28"^^<http://www.w3.org/2001/XMLSchema#date> ;
        status:term_status  "unstable" .

<http://vocab.org/transit/terms/.rdf>
        a                  <http://purl.org/dc/dcmitype/Text> , foaf:Document ;
        dct:hasFormat      <http://vocab.org/transit/terms/.turtle> , <http://vocab.org/transit/terms/.json> , <http://vocab.org/transit/terms/.html> ;
        foaf:primaryTopic  <http://vocab.org/transit/terms/> ;
        foaf:topic         <http://vocab.org/transit/terms/> .

<http://vocab.org/transit/terms/scheduleService>
        a                 <http://www.w3.org/2002/07/owl#ObjectProperty> , rdf:Property ;
        rdfs:comment      "A service that operates on this schedule."@en ;
        rdfs:domain       <http://vocab.org/transit/terms/Schedule> ;
        rdfs:isDefinedBy  <http://vocab.org/transit/terms/> ;
        rdfs:label        "Schedule Service"@en ;
        rdfs:range        <http://vocab.org/transit/terms/Service> ;
        dct:issued        "2011-03-28"^^<http://www.w3.org/2001/XMLSchema#date> .

<http://vocab.org/transit/terms/Agency>
        a                   <http://www.w3.org/2002/07/owl#Class> ;
        rdfs:comment        "An organization that oversees public transportation for a city or region."@en ;
        rdfs:isDefinedBy    <http://vocab.org/transit/terms/> ;
        rdfs:label          "Transit Agency"@en ;
        rdfs:subClassOf     foaf:Organization ;
        dct:issued          "2011-03-28"^^<http://www.w3.org/2001/XMLSchema#date> ;
        status:term_status  "unstable" .

<http://vocab.org/transit/terms/RouteStop>
        a                   <http://www.w3.org/2002/07/owl#Class> ;
        rdfs:comment        "A location where passengers board or disembark from a transit vehicle for a specific route."@en ;
        rdfs:isDefinedBy    <http://vocab.org/transit/terms/> ;
        rdfs:label          "Route Stop"@en ;
        dct:issued          "2011-08-06"^^<http://www.w3.org/2001/XMLSchema#date> ;
        status:term_status  "unstable" .

<http://iandavis.com/id/me>
        a          foaf:Person ;
        foaf:name  "Ian Davis" .

<http://vocab.org/transit/terms/.html>
        a           foaf:Document , <http://purl.org/dc/dcmitype/Text> ;
        rdfs:label  "HTML" ;
        dc:format   "text/html" .

<http://vocab.org/transit/terms/iataCode>
        a                   <http://www.w3.org/2002/07/owl#DatatypeProperty> , rdf:Property ;
        rdfs:comment        "The code issued by the International Air Transport Association to identify an airport."@en ;
        rdfs:isDefinedBy    <http://vocab.org/transit/terms/> ;
        rdfs:label          "IATA code"@en ;
        rdfs:subPropertyOf  dct:identifier ;
        dct:issued          "2012-01-25"^^<http://www.w3.org/2001/XMLSchema#date> .

<http://code.google.com/transit/spec/transit_feed_specification.html>
        rdfs:label  "General Transit Feed Specification" .

<http://vocab.org/transit/terms/UnavailableTransfer>
        a                   <http://www.w3.org/2002/07/owl#Class> ;
        rdfs:comment        "A point where transfer between two routes is not possible despite appearing possible by proximity."@en ;
        rdfs:isDefinedBy    <http://vocab.org/transit/terms/> ;
        rdfs:label          "Unavailable Transfer"@en ;
        dct:issued          "2011-03-28"^^<http://www.w3.org/2001/XMLSchema#date> ;
        status:term_status  "unstable" .

<http://vocab.org/transit/terms/SubwayRoute>
        a                   <http://www.w3.org/2002/07/owl#Class> ;
        rdfs:comment        "A public transportation route utilising an underground rail system within a metropolitan area."@en ;
        rdfs:isDefinedBy    <http://vocab.org/transit/terms/> ;
        rdfs:label          "Subway Route"@en ;
        rdfs:subClassOf     <http://vocab.org/transit/terms/Route> ;
        dct:issued          "2011-03-28"^^<http://www.w3.org/2001/XMLSchema#date> ;
        status:term_status  "unstable" .

<http://vocab.org/transit/terms/routeService>
        a                 <http://www.w3.org/2002/07/owl#ObjectProperty> , rdf:Property ;
        rdfs:comment      "A service that operates on this route."@en ;
        rdfs:domain       <http://vocab.org/transit/terms/Route> ;
        rdfs:isDefinedBy  <http://vocab.org/transit/terms/> ;
        rdfs:label        "Route Service"@en ;
        rdfs:range        <http://vocab.org/transit/terms/Service> ;
        dct:issued        "2011-03-28"^^<http://www.w3.org/2001/XMLSchema#date> .

<http://vocab.org/transit/terms/TramRoute>
        a                   <http://www.w3.org/2002/07/owl#Class> ;
        rdfs:comment        "A public transportation route utilising light rail or street level railed vehicles within a metropolitan area."@en ;
        rdfs:isDefinedBy    <http://vocab.org/transit/terms/> ;
        rdfs:label          "Tram Route"@en ;
        rdfs:subClassOf     <http://vocab.org/transit/terms/Route> ;
        dct:issued          "2011-03-28"^^<http://www.w3.org/2001/XMLSchema#date> ;
        status:term_status  "unstable" .

<http://vocab.org/transit/terms/Station>
        a                   <http://www.w3.org/2002/07/owl#Class> ;
        rdfs:comment        "A physical structure or area that contains one or more stops."@en ;
        rdfs:isDefinedBy    <http://vocab.org/transit/terms/> ;
        rdfs:label          "Transit Station"@en ;
        dct:issued          "2011-03-28"^^<http://www.w3.org/2001/XMLSchema#date> ;
        status:term_status  "unstable" .

<http://vocab.org/transit/terms/standard>
        a             <http://vocab.org/transit/terms/AccessArrangement> ;
        rdfs:comment  "The particular form of access has no special arrangement."@en ;
        rdfs:label    "Standard"@en .

<http://vocab.org/transit/terms/>
        a                              <http://www.w3.org/2002/07/owl#Ontology> ;
        rdfs:seeAlso                   <http://code.google.com/transit/spec/transit_feed_specification.html> ;
        dct:abstract                   "This document describes a vocabulary for describing transit systems, routes, stops and schedules."@en ;
        dct:creator                    <http://iandavis.com/id/me> ;
        dct:date                       "2011-03-28"^^<http://www.w3.org/2001/XMLSchema#date> ;
        dct:description                "<div>\n    <p>The TRANSIT schema is based on the General Transit Feed Specification published by Google.</p>\n    <p><figure><img src=\"/transit/core-classes.png\"></img><br></br>Figure: Transit Vocabulary Core Classes (<a href=\"http://vocab.org/transit/core-classes.png\">PNG version</a>, <a href=\"http://vocab.org/transit/core-classes.svg\">SVG version</a>)</figure></p>\n    <p>Please see <a href=\"https://github.com/iand/vocab-transit\">https://github.com/iand/vocab-transit</a> for the master version of this vocabulary.</p>\n    </div>"^^rdf:XMLLiteral ;
        dct:identifier                 "http://vocab.org/transit/terms/" ;
        dct:issued                     "2011-03-28"^^<http://www.w3.org/2001/XMLSchema#date> ;
        dct:rights                     "Copyright 2011 Ian Davis" ;
        dct:title                      "TRANSIT: A vocabulary for describing transit systems and routes"@en ;
        vann:preferredNamespacePrefix  "transit" ;
        vann:preferredNamespaceUri     "http://vocab.org/transit/terms/" .

<http://vocab.org/transit/terms/pickup>
        a                 <http://www.w3.org/2002/07/owl#ObjectProperty> , rdf:Property ;
        rdfs:comment      "The arrangement required for passengers to be picked up at this service stop."@en ;
        rdfs:domain       <http://vocab.org/transit/terms/ServiceStop> ;
        rdfs:isDefinedBy  <http://vocab.org/transit/terms/> ;
        rdfs:label        "Pick Up"@en ;
        rdfs:range        <http://vocab.org/transit/terms/AccessArrangement> ;
        dct:issued        "2011-03-28"^^<http://www.w3.org/2001/XMLSchema#date> .

<http://vocab.org/transit/terms/Fare>
        a                   <http://www.w3.org/2002/07/owl#Class> ;
        rdfs:comment        "A class of fare payable for public transportation."@en ;
        rdfs:isDefinedBy    <http://vocab.org/transit/terms/> ;
        rdfs:label          "Fare"@en ;
        dct:issued          "2011-03-28"^^<http://www.w3.org/2001/XMLSchema#date> ;
        status:term_status  "unstable" .

<http://vocab.org/transit/terms/distance>
        a                 <http://www.w3.org/2002/07/owl#DatatypeProperty> , rdf:Property ;
        rdfs:comment      "The distance of this service stop from the first stop in sequence."@en ;
        rdfs:domain       <http://vocab.org/transit/terms/ServiceStop> ;
        rdfs:isDefinedBy  <http://vocab.org/transit/terms/> ;
        rdfs:label        "Distance"@en ;
        dct:issued        "2011-03-28"^^<http://www.w3.org/2001/XMLSchema#date> .

<http://vocab.org/transit/terms/icaoCode>
        a                   <http://www.w3.org/2002/07/owl#DatatypeProperty> , rdf:Property ;
        rdfs:comment        "The code issued by the International Civil Aviation Authority to identify an airport or airline."@en ;
        rdfs:isDefinedBy    <http://vocab.org/transit/terms/> ;
        rdfs:label          "ICAO code"@en ;
        rdfs:subPropertyOf  dct:identifier ;
        dct:issued          "2012-01-25"^^<http://www.w3.org/2001/XMLSchema#date> .

<http://vocab.org/transit/terms/routeStop>
        a                 <http://www.w3.org/2002/07/owl#ObjectProperty> , rdf:Property ;
        rdfs:comment      "Links a route to a particular stop and the sequence of that stop in the route."@en ;
        rdfs:isDefinedBy  <http://vocab.org/transit/terms/> ;
        rdfs:label        "Route Stop"@en ;
        rdfs:range        <http://vocab.org/transit/terms/RouteStop> ;
        dct:issued        "2011-08-06"^^<http://www.w3.org/2001/XMLSchema#date> .

<http://vocab.org/transit/terms/date>
        a                 <http://www.w3.org/2002/07/owl#DatatypeProperty> , rdf:Property ;
        rdfs:comment      "A date on which this service is scheduled to operate."@en ;
        rdfs:domain       <http://vocab.org/transit/terms/Schedule> ;
        rdfs:isDefinedBy  <http://vocab.org/transit/terms/> ;
        rdfs:label        "Date"@en ;
        dct:issued        "2011-03-28"^^<http://www.w3.org/2001/XMLSchema#date> .

<http://vocab.org/transit/terms/price>
        a                 <http://www.w3.org/2002/07/owl#DatatypeProperty> , rdf:Property ;
        rdfs:comment      "The price of the fare."@en ;
        rdfs:domain       <http://vocab.org/transit/terms/Fare> ;
        rdfs:isDefinedBy  <http://vocab.org/transit/terms/> ;
        rdfs:label        "Price"@en ;
        dct:issued        "2011-03-28"^^<http://www.w3.org/2001/XMLSchema#date> .

<http://vocab.org/transit/terms/service>
        a                 <http://www.w3.org/2002/07/owl#ObjectProperty> , rdf:Property ;
        rdfs:comment      "The service associated with this service stop."@en ;
        rdfs:domain       <http://vocab.org/transit/terms/ServiceStop> ;
        rdfs:isDefinedBy  <http://vocab.org/transit/terms/> ;
        rdfs:label        "Service"@en ;
        rdfs:range        <http://vocab.org/transit/terms/Stop> ;
        dct:issued        "2011-03-28"^^<http://www.w3.org/2001/XMLSchema#date> .

<http://vocab.org/transit/terms/MinimumTimeTransfer>
        a                   <http://www.w3.org/2002/07/owl#Class> ;
        rdfs:comment        "A transfer point between two routes that requires a minimum amount of time between arrival and departure to ensure a connection."@en ;
        rdfs:isDefinedBy    <http://vocab.org/transit/terms/> ;
        rdfs:label          "Minimum Time Transfer"@en ;
        rdfs:subClassOf     <http://vocab.org/transit/terms/Transfer> ;
        dct:issued          "2011-03-28"^^<http://www.w3.org/2001/XMLSchema#date> ;
        status:term_status  "unstable" .

<http://vocab.org/transit/terms/transfer>
        a                 <http://www.w3.org/2002/07/owl#ObjectProperty> , rdf:Property ;
        rdfs:comment      "A transfer point that is associated with this stop."@en ;
        rdfs:domain       <http://vocab.org/transit/terms/Stop> ;
        rdfs:isDefinedBy  <http://vocab.org/transit/terms/> ;
        rdfs:label        "Transfer"@en ;
        rdfs:range        <http://vocab.org/transit/terms/Transfer> ;
        dct:issued        "2011-03-28"^^<http://www.w3.org/2001/XMLSchema#date> .

<http://vocab.org/transit/terms/ServiceStop>
        a                   <http://www.w3.org/2002/07/owl#Class> ;
        rdfs:comment        "A location where passengers board or disembark from a transit vehicle for a specific service."@en ;
        rdfs:isDefinedBy    <http://vocab.org/transit/terms/> ;
        rdfs:label          "Service Stop"@en ;
        dct:issued          "2011-03-28"^^<http://www.w3.org/2001/XMLSchema#date> ;
        status:term_status  "unstable" .

<http://vocab.org/transit/terms/timezone>
        a                 <http://www.w3.org/2002/07/owl#ObjectProperty> , rdf:Property ;
        rdfs:comment      "The timezone where a person or organisation is located."@en ;
        rdfs:domain       foaf:Agent ;
        rdfs:isDefinedBy  <http://vocab.org/transit/terms/> ;
        rdfs:label        "Timezone"@en ;
        dct:issued        "2011-03-28"^^<http://www.w3.org/2001/XMLSchema#date> .

<http://vocab.org/transit/terms/headsign>
        a                 <http://www.w3.org/2002/07/owl#DatatypeProperty> , rdf:Property ;
        rdfs:comment      "Text that appears on a sign that identifies the service's destination to passengers."@en ;
        rdfs:isDefinedBy  <http://vocab.org/transit/terms/> ;
        rdfs:label        "Date"@en ;
        dct:issued        "2011-03-28"^^<http://www.w3.org/2001/XMLSchema#date> .

<http://vocab.org/transit/terms/textColor>
        a                 <http://www.w3.org/2002/07/owl#DatatypeProperty> , rdf:Property ;
        rdfs:comment      "A legible color for text drawn against a background of the color associated with a route."@en ;
        rdfs:domain       <http://vocab.org/transit/terms/Route> ;
        rdfs:isDefinedBy  <http://vocab.org/transit/terms/> ;
        rdfs:label        "Text Color"@en ;
        dct:issued        "2011-03-28"^^<http://www.w3.org/2001/XMLSchema#date> .

<http://vocab.org/transit/terms/OutboundService>
        a                   <http://www.w3.org/2002/07/owl#Class> ;
        rdfs:comment        "A service that travels in an outbound direction."@en ;
        rdfs:isDefinedBy    <http://vocab.org/transit/terms/> ;
        rdfs:label          "Outbound Service"@en ;
        dct:issued          "2011-03-28"^^<http://www.w3.org/2001/XMLSchema#date> ;
        status:term_status  "unstable" .

<http://vocab.org/transit/terms/Schedule>
        a                   <http://www.w3.org/2002/07/owl#Class> ;
        rdfs:comment        "A public transport schedule that applies for one or more routes."@en ;
        rdfs:isDefinedBy    <http://vocab.org/transit/terms/> ;
        rdfs:label          "Schedule"@en ;
        dct:issued          "2011-03-28"^^<http://www.w3.org/2001/XMLSchema#date> ;
        status:term_status  "unstable" .

<http://vocab.org/transit/terms/currency>
        a                 <http://www.w3.org/2002/07/owl#DatatypeProperty> , rdf:Property ;
        rdfs:comment      "The currency of the fare price."@en ;
        rdfs:domain       <http://vocab.org/transit/terms/Fare> ;
        rdfs:isDefinedBy  <http://vocab.org/transit/terms/> ;
        rdfs:label        "Currency"@en ;
        dct:issued        "2011-03-28"^^<http://www.w3.org/2001/XMLSchema#date> .

<http://vocab.org/transit/terms/AccessArrangement>
        a                   <http://www.w3.org/2002/07/owl#Class> ;
        rdfs:comment        "A type of arrangement for picking up or dropping off passengers from a service stop."@en ;
        rdfs:isDefinedBy    <http://vocab.org/transit/terms/> ;
        rdfs:label          "Access Arrangement"@en ;
        rdfs:subClassOf     foaf:Organization ;
        dct:issued          "2011-03-28"^^<http://www.w3.org/2001/XMLSchema#date> ;
        status:term_status  "unstable" .

<http://vocab.org/transit/terms/schedule>
        a                 <http://www.w3.org/2002/07/owl#ObjectProperty> , rdf:Property ;
        rdfs:comment      "The schedule on which this service operates."@en ;
        rdfs:domain       <http://vocab.org/transit/terms/Service> ;
        rdfs:isDefinedBy  <http://vocab.org/transit/terms/> ;
        rdfs:label        "Schedule"@en ;
        rdfs:range        <http://vocab.org/transit/terms/Schedule> ;
        dct:issued        "2011-03-28"^^<http://www.w3.org/2001/XMLSchema#date> .

<http://creativecommons.org/licenses/by/1.0/>
        a              msg0:License ;
        msg0:permits   msg0:DerivativeWorks , msg0:Distribution , msg0:Reproduction ;
        msg0:requires  msg0:Attribution , msg0:Notice .

<http://vocab.org/transit/terms/fromStop>
        a                 <http://www.w3.org/2002/07/owl#ObjectProperty> , rdf:Property ;
        rdfs:comment      "A stop where a connection between routes begins."@en ;
        rdfs:domain       <http://vocab.org/transit/terms/Transfer> ;
        rdfs:isDefinedBy  <http://vocab.org/transit/terms/> ;
        rdfs:label        "From Stop"@en ;
        rdfs:range        <http://vocab.org/transit/terms/Stop> ;
        dct:issued        "2011-03-28"^^<http://www.w3.org/2001/XMLSchema#date> .

<http://vocab.org/transit/terms/RailRoute>
        a                   <http://www.w3.org/2002/07/owl#Class> ;
        rdfs:comment        "A public transportation route utilising a rail system for intercity or long-distance travel."@en ;
        rdfs:isDefinedBy    <http://vocab.org/transit/terms/> ;
        rdfs:label          "Rail Route"@en ;
        rdfs:subClassOf     <http://vocab.org/transit/terms/Route> ;
        dct:issued          "2011-03-28"^^<http://www.w3.org/2001/XMLSchema#date> ;
        status:term_status  "unstable" .

<http://vocab.org/transit/terms/GondalaRoute>
        a                   <http://www.w3.org/2002/07/owl#Class> ;
        rdfs:comment        "A public transportation route utilising aerial cable cars where the car is suspended from the cable."@en ;
        rdfs:isDefinedBy    <http://vocab.org/transit/terms/> ;
        rdfs:label          "Gondala Route"@en ;
        rdfs:subClassOf     <http://vocab.org/transit/terms/Route> ;
        dct:issued          "2011-03-28"^^<http://www.w3.org/2001/XMLSchema#date> ;
        status:term_status  "unstable" .

<http://vocab.org/transit/terms/coordinated>
        a             <http://vocab.org/transit/terms/AccessArrangement> ;
        rdfs:comment  "The particular form of access must be coordinated with the driver."@en ;
        rdfs:label    "Coordinated"@en .

<http://vocab.org/transit/terms/.turtle>
        a           foaf:Document , <http://purl.org/dc/dcmitype/Text> ;
        rdfs:label  "Turtle" ;
        dc:format   "text/plain" .

<http://vocab.org/transit/terms/callsign>
        a                   <http://www.w3.org/2002/07/owl#DatatypeProperty> , rdf:Property ;
        rdfs:comment        "The callsign prefix used by an airline to identify itself to air traffic control."@en ;
        rdfs:isDefinedBy    <http://vocab.org/transit/terms/> ;
        rdfs:label          "Callsign prefix"@en ;
        rdfs:subPropertyOf  dct:identifier ;
        dct:issued          "2012-01-25"^^<http://www.w3.org/2001/XMLSchema#date> ;
        status:term_status  "unstable" .

<http://vocab.org/transit/terms/agency>
        a                 <http://www.w3.org/2002/07/owl#ObjectProperty> , rdf:Property ;
        rdfs:comment      "The agency that operates this public transportation route."@en ;
        rdfs:domain       <http://vocab.org/transit/terms/Route> ;
        rdfs:isDefinedBy  <http://vocab.org/transit/terms/> ;
        rdfs:label        "Agency"@en ;
        rdfs:range        <http://vocab.org/transit/terms/Agency> ;
        dct:issued        "2011-03-28"^^<http://www.w3.org/2001/XMLSchema#date> .

<http://vocab.org/transit/terms/stop>
        a                 <http://www.w3.org/2002/07/owl#ObjectProperty> , rdf:Property ;
        rdfs:comment      "The physical stop associated with this service stop."@en ;
        rdfs:domain       <http://vocab.org/transit/terms/ServiceStop> ;
        rdfs:isDefinedBy  <http://vocab.org/transit/terms/> ;
        rdfs:label        "Stop"@en ;
        rdfs:range        <http://vocab.org/transit/terms/Stop> ;
        dct:issued        "2011-03-28"^^<http://www.w3.org/2001/XMLSchema#date> .

<http://vocab.org/transit/terms/stationStop>
        a                 <http://www.w3.org/2002/07/owl#ObjectProperty> , rdf:Property ;
        rdfs:comment      "A stop that is associated with this station."@en ;
        rdfs:domain       <http://vocab.org/transit/terms/Station> ;
        rdfs:isDefinedBy  <http://vocab.org/transit/terms/> ;
        rdfs:label        "Station Stop"@en ;
        rdfs:range        <http://vocab.org/transit/terms/Stop> ;
        dct:issued        "2011-03-28"^^<http://www.w3.org/2001/XMLSchema#date> .

<http://vocab.org/transit/terms/Transfer>
        a                   <http://www.w3.org/2002/07/owl#Class> ;
        rdfs:comment        "A transfer point between two routes."@en ;
        rdfs:isDefinedBy    <http://vocab.org/transit/terms/> ;
        rdfs:label          "Transfer"@en ;
        dct:issued          "2011-03-28"^^<http://www.w3.org/2001/XMLSchema#date> ;
        status:term_status  "unstable" .

<http://vocab.org/transit/terms/CableCarRoute>
        a                   <http://www.w3.org/2002/07/owl#Class> ;
        rdfs:comment        "A public transportation route utilising street-level cable cars where the cable runs beneath the car."@en ;
        rdfs:isDefinedBy    <http://vocab.org/transit/terms/> ;
        rdfs:label          "Cable Car Route"@en ;
        rdfs:subClassOf     <http://vocab.org/transit/terms/Route> ;
        dct:issued          "2011-03-28"^^<http://www.w3.org/2001/XMLSchema#date> ;
        status:term_status  "unstable" .

<http://vocab.org/transit/terms/.json>
        a           foaf:Document , <http://purl.org/dc/dcmitype/Text> ;
        rdfs:label  "JSON" ;
        dc:format   "application/json" .

<http://vocab.org/transit/terms/language>
        a                 <http://www.w3.org/2002/07/owl#ObjectProperty> , rdf:Property ;
        rdfs:comment      "The primary language used by a person or organisation."@en ;
        rdfs:domain       foaf:Agent ;
        rdfs:isDefinedBy  <http://vocab.org/transit/terms/> ;
        rdfs:label        "Language"@en ;
        dct:issued        "2011-03-28"^^<http://www.w3.org/2001/XMLSchema#date> .

<http://vocab.org/transit/terms/Route>
        a                   <http://www.w3.org/2002/07/owl#Class> ;
        rdfs:comment        "A public transportation route."@en ;
        rdfs:isDefinedBy    <http://vocab.org/transit/terms/> ;
        rdfs:label          "Transit Route"@en ;
        dct:issued          "2011-03-28"^^<http://www.w3.org/2001/XMLSchema#date> ;
        status:term_status  "unstable" .

<http://vocab.org/transit/terms/route>
        a                 <http://www.w3.org/2002/07/owl#ObjectProperty> , rdf:Property ;
        rdfs:comment      "A route associated with the given resource."@en ;
        rdfs:isDefinedBy  <http://vocab.org/transit/terms/> ;
        rdfs:label        "Route"@en ;
        rdfs:range        <http://vocab.org/transit/terms/Route> ;
        dct:issued        "2011-03-28"^^<http://www.w3.org/2001/XMLSchema#date> ;
        skos:historyNote  [ rdf:value    "Relaxed domain" ;
                            dct:creator  "Ian Davis" ;
                            dct:date     "2011-08-06"
                          ] .

<http://vocab.org/transit/terms/toStop>
        a                 <http://www.w3.org/2002/07/owl#ObjectProperty> , rdf:Property ;
        rdfs:comment      "A stop where a connection between routes ends."@en ;
        rdfs:domain       <http://vocab.org/transit/terms/Transfer> ;
        rdfs:isDefinedBy  <http://vocab.org/transit/terms/> ;
        rdfs:label        "To Stop"@en ;
        rdfs:range        <http://vocab.org/transit/terms/Stop> ;
        dct:issued        "2011-03-28"^^<http://www.w3.org/2001/XMLSchema#date> .

<http://vocab.org/transit/terms/dropoff>
        a                 <http://www.w3.org/2002/07/owl#ObjectProperty> , rdf:Property ;
        rdfs:comment      "The arrangement required for passengers to be dropped off at this service stop."@en ;
        rdfs:domain       <http://vocab.org/transit/terms/ServiceStop> ;
        rdfs:isDefinedBy  <http://vocab.org/transit/terms/> ;
        rdfs:label        "Drop Off"@en ;
        rdfs:range        <http://vocab.org/transit/terms/AccessArrangement> ;
        dct:issued        "2011-03-28"^^<http://www.w3.org/2001/XMLSchema#date> .
