@prefix dc: <http://purl.org/dc/elements/1.1/> .
@prefix sit: <http://www.ontologydesignpatterns.org/cp/owl/situation.owl#> .
@prefix : <http://www.essepuntato.it/2013/10/vagueness/> .
@prefix rdfs: <http://www.w3.org/2000/01/rdf-schema#> .
@prefix prov: <http://www.w3.org/ns/prov#> .
@prefix oa: <http://www.w3.org/ns/oa#> .
@prefix xsd: <http://www.w3.org/2001/XMLSchema#> .
@prefix owl: <http://www.w3.org/2002/07/owl#> .
@prefix rdf: <http://www.w3.org/1999/02/22-rdf-syntax-ns#> .

<http://www.essepuntato.it/2013/10/vagueness> a owl:Ontology ;
	rdfs:label "Vagueness Ontology"@en ;
	dc:creator "Panos Alexopoulos" ;
	owl:versionInfo "1.0" ;
	dc:creator "Silvio Peroni" ;
	dc:date "2013-11-28" ;
	dc:title "The Vagueness Ontology (VO)"@en ;
	rdfs:comment "The Vagueness Ontology (VO) allows one to specify vagueness characterisations of the TBox entities of an ontology."@en ;
	dc:description """Vagueness is a common human knowledge and language phenomenon, typically manifested by terms and concepts like High, Expert, Bad, Near etc.

In an OWL ontology vagueness may appear in the definitions of classes, properties, datatypes and individuals. For these entities a more explicit description of the nature and characteristics of their vagueness/non-vagueness is required.

Analyzing and describing the nature of vagueness/non-vagueness in ontological entities is subjective activity, since it is often a personal interpretation of someone (a person or, more generally, an agent).

Vagueness can be described according to at least two complementary types referring to quantitative or qualitative connotations respectively. The quantitative aspect of vagueness concerns the (real or apparent) lack of precise boundaries defining an entity along one or more specific dimensions. The qualitative aspect of vagueness concerns the identification of such other discriminants of which boundaries are not quantifiable in any precise way.

Either a vagueness description, that specifies always a type, or a non-vagueness description provides at least a justification (defined either as natural language text, an entity or a more complex logic formula, or any combination of them) that motivates a specific aspect of why an entity should be intended as vague/non-vague. Multiple justifications are possible for the same description.

The justification of a description of vagueness having quantitative type can include an explicit definition of the dimensions (defined either as natural language text, an entity or a more complex logic formula, or any combination of them) in which the entity is vague.

A description of vagueness/non-vagueness can also be context-dependent. In particular, the context-dependent objects are:

- the descriptions of vagueness/non-vagueness related to entities (i.e. the same entity can be vague in one context and non-vague in another);

- the dimensions related to a description of vagueness having quantitative type (i.e. the same entity can be vague in dimension A in one context and in dimension B in another). Note that it is the relation between a justification and a certain dimension that may specify a particular context, rather than the dimension itself.

The annotation of an entity with information about its vagueness is a particular act of tagging done by someone (i.e., an agent) who associates a description of vagueness/non-vagueness (called the body of the annotation) to the entity in consideration (called the target of the annotation)."""@en ;
	owl:versionIRI <http://www.essepuntato.it/2013/10/vagueness/1.0> ;
	owl:imports <http://www.ontologydesignpatterns.org/cp/owl/situation.owl> .

dc:creator a owl:AnnotationProperty ;
	rdfs:label "has creator"@en ;
	rdfs:isDefinedBy <http://purl.org/dc/elements/1.1/> .

dc:date a owl:AnnotationProperty ;
	rdfs:label "has date"@en ;
	rdfs:isDefinedBy <http://purl.org/dc/elements/1.1/> .

dc:description a owl:AnnotationProperty ;
	rdfs:label "has description"@en ;
	rdfs:isDefinedBy <http://purl.org/dc/elements/1.1/> .

dc:title a owl:AnnotationProperty ;
	rdfs:label "has title"@en ;
	rdfs:isDefinedBy <http://purl.org/dc/elements/1.1/> .

:hasApplicabilityContext a owl:ObjectProperty ;
	rdfs:label "has applicability context"@en ;
	rdfs:comment "This property links either descriptions of vagueness/non-vagueness or dimensions of descriptions of quantitative vagueness to the context to which they apply."@en ;
	rdfs:isDefinedBy <http://www.essepuntato.it/2013/10/vagueness> ;
	rdfs:range :ApplicabilityContext ;
	rdfs:domain _:node18vkkn01mx1 .

_:node18vkkn01mx1 a owl:Class ;
	owl:unionOf _:node18vkkn01mx2 .

_:node18vkkn01mx2 rdf:first :DescriptionOfNonVagueness ;
	rdf:rest _:node18vkkn01mx3 .

_:node18vkkn01mx3 rdf:first :DescriptionOfVagueness ;
	rdf:rest _:node18vkkn01mx4 .

_:node18vkkn01mx4 rdf:first :DimensionInContext ;
	rdf:rest rdf:nil .

:hasDimension a owl:ObjectProperty ;
	rdfs:label "has dimension"@en ;
	rdfs:comment "It links justifications of a description of quantitative vagueness to the dimensions that identify what boundaries are not defined precisely by a particular entity and, thus, are part of the causes of vagueness for the entity itself."@en ;
	rdfs:isDefinedBy <http://www.essepuntato.it/2013/10/vagueness> ;
	rdfs:range :Dimension ;
	owl:propertyChainAxiom _:node18vkkn01mx5 .

_:node18vkkn01mx5 rdf:first :hasDimensionInContext ;
	rdf:rest _:node18vkkn01mx6 .

_:node18vkkn01mx6 rdf:first :withDimension ;
	rdf:rest rdf:nil .

:hasDimension rdfs:domain _:node18vkkn01mx7 .

_:node18vkkn01mx7 a owl:Class ;
	owl:intersectionOf _:node18vkkn01mx8 .

_:node18vkkn01mx8 rdf:first :Justification ;
	rdf:rest _:node18vkkn01mx10 .

_:node18vkkn01mx10 rdf:first _:node18vkkn01mx9 .

_:node18vkkn01mx9 a owl:Restriction ;
	owl:onProperty _:node18vkkn01mx11 .

_:node18vkkn01mx11 owl:inverseOf :hasJustification .

_:node18vkkn01mx9 owl:allValuesFrom _:node18vkkn01mx12 .

_:node18vkkn01mx12 a owl:Class ;
	owl:intersectionOf _:node18vkkn01mx13 .

_:node18vkkn01mx13 rdf:first :DescriptionOfVagueness ;
	rdf:rest _:node18vkkn01mx15 .

_:node18vkkn01mx15 rdf:first _:node18vkkn01mx14 .

_:node18vkkn01mx14 a owl:Restriction ;
	owl:onProperty :hasVaguenessType ;
	owl:hasValue :quantitative-vagueness .

_:node18vkkn01mx15 rdf:rest rdf:nil .

_:node18vkkn01mx10 rdf:rest rdf:nil .

:hasDimensionInContext a owl:ObjectProperty ;
	rdfs:label "has dimension in context"@en ;
	rdfs:comment "It links justifications of a description of quantitative vagueness to situations where a particular dimension, which identifies the boundaries that are not defined precisely by a particular entity, has to be considered within a particular applicability context."@en ;
	rdfs:isDefinedBy <http://www.essepuntato.it/2013/10/vagueness> ;
	rdfs:range :DimensionInContext ;
	rdfs:domain _:node18vkkn01mx16 .

_:node18vkkn01mx16 a owl:Class ;
	owl:intersectionOf _:node18vkkn01mx17 .

_:node18vkkn01mx17 rdf:first :Justification ;
	rdf:rest _:node18vkkn01mx19 .

_:node18vkkn01mx19 rdf:first _:node18vkkn01mx18 .

_:node18vkkn01mx18 a owl:Restriction ;
	owl:onProperty _:node18vkkn01mx20 .

_:node18vkkn01mx20 owl:inverseOf :hasJustification .

_:node18vkkn01mx18 owl:allValuesFrom _:node18vkkn01mx21 .

_:node18vkkn01mx21 a owl:Class ;
	owl:intersectionOf _:node18vkkn01mx22 .

_:node18vkkn01mx22 rdf:first :DescriptionOfVagueness ;
	rdf:rest _:node18vkkn01mx24 .

_:node18vkkn01mx24 rdf:first _:node18vkkn01mx23 .

_:node18vkkn01mx23 a owl:Restriction ;
	owl:onProperty :hasVaguenessType ;
	owl:hasValue :quantitative-vagueness .

_:node18vkkn01mx24 rdf:rest rdf:nil .

_:node18vkkn01mx19 rdf:rest rdf:nil .

:hasEntity a owl:ObjectProperty ;
	rdfs:label "has entity"@en ;
	rdfs:comment "The entity defining the body of either a justification or dimension."@en ;
	rdfs:isDefinedBy <http://www.essepuntato.it/2013/10/vagueness> ;
	rdfs:domain _:node18vkkn01mx25 .

_:node18vkkn01mx25 a owl:Class ;
	owl:unionOf _:node18vkkn01mx26 .

_:node18vkkn01mx26 rdf:first :Dimension ;
	rdf:rest _:node18vkkn01mx27 .

_:node18vkkn01mx27 rdf:first :Justification ;
	rdf:rest rdf:nil .

:hasJustification a owl:ObjectProperty ;
	rdfs:label "has justification"@en ;
	rdfs:comment "It links a particular description of vagueness/non-vagueness to a related justification."@en ;
	rdfs:isDefinedBy <http://www.essepuntato.it/2013/10/vagueness> ;
	rdfs:range :Justification ;
	rdfs:domain _:node18vkkn01mx28 .

_:node18vkkn01mx28 a owl:Class ;
	owl:unionOf _:node18vkkn01mx29 .

_:node18vkkn01mx29 rdf:first :DescriptionOfNonVagueness ;
	rdf:rest _:node18vkkn01mx30 .

_:node18vkkn01mx30 rdf:first :DescriptionOfVagueness ;
	rdf:rest rdf:nil .

:hasLogicFormula a owl:ObjectProperty ;
	rdfs:label "has logic formula"@en ;
	rdfs:comment "The logic formula defining the body of either a justification or dimension."@en ;
	rdfs:isDefinedBy <http://www.essepuntato.it/2013/10/vagueness> ;
	rdfs:domain _:node18vkkn01mx31 .

_:node18vkkn01mx31 a owl:Class ;
	owl:unionOf _:node18vkkn01mx32 .

_:node18vkkn01mx32 rdf:first :Dimension ;
	rdf:rest _:node18vkkn01mx33 .

_:node18vkkn01mx33 rdf:first :Justification ;
	rdf:rest rdf:nil .

:hasVaguenessType a owl:ObjectProperty , owl:FunctionalProperty ;
	rdfs:label "has vagueness type"@en ;
	rdfs:comment "The link between a description of vagueness and the particular type of vagueness it describes."@en ;
	rdfs:isDefinedBy <http://www.essepuntato.it/2013/10/vagueness> ;
	rdfs:domain :DescriptionOfVagueness ;
	rdfs:range :VaguenessType .

:isApplicabilityContextOf a owl:ObjectProperty ;
	rdfs:label "is applicability context of"@en ;
	rdfs:comment "This property links applicability contexts to the related descriptions of vagueness/non-vagueness or dimensions of descriptions of quantitative vagueness."@en ;
	rdfs:isDefinedBy <http://www.essepuntato.it/2013/10/vagueness> ;
	owl:inverseOf :hasApplicabilityContext .

:isDimensionIn a owl:ObjectProperty ;
	rdfs:label "is dimension in"@en ;
	rdfs:comment "It links a dimension to the situations that include related applicability contexts."@en ;
	rdfs:isDefinedBy <http://www.essepuntato.it/2013/10/vagueness> ;
	owl:inverseOf :withDimension ;
	rdfs:subPropertyOf sit:hasSetting .

:isDimensionInContextOf a owl:ObjectProperty ;
	rdfs:label "is dimension in context of"@en ;
	rdfs:comment "It links situations describing a dimension according to a particular context to the justification that involves them."@en ;
	rdfs:isDefinedBy <http://www.essepuntato.it/2013/10/vagueness> ;
	owl:inverseOf :hasDimensionInContext .

:isDimensionOf a owl:ObjectProperty ;
	rdfs:label "is dimension of"@en ;
	rdfs:comment "It links dimensions to the justification that involves them."@en ;
	rdfs:isDefinedBy <http://www.essepuntato.it/2013/10/vagueness> ;
	owl:inverseOf :hasDimension .

:isEntityOf a owl:ObjectProperty ;
	rdfs:label "is entity of"@en ;
	rdfs:comment "It links to the justification/dimension that involves the entity."@en ;
	rdfs:isDefinedBy <http://www.essepuntato.it/2013/10/vagueness> ;
	owl:inverseOf :hasEntity .

:isJustificationOf a owl:ObjectProperty ;
	rdfs:label "is justification of"@en ;
	rdfs:comment "It links to the description of vagueness/non-vagueness supported by the justification."@en ;
	rdfs:isDefinedBy <http://www.essepuntato.it/2013/10/vagueness> ;
	owl:inverseOf :hasJustification .

:isLogicFormulaOf a owl:ObjectProperty ;
	rdfs:label "is logic formula of"@en ;
	rdfs:comment "It links to the justification/dimension that involves the logic formula."@en ;
	rdfs:isDefinedBy <http://www.essepuntato.it/2013/10/vagueness> ;
	owl:inverseOf :hasLogicFormula .

:isVaguenessTypeOf a owl:ObjectProperty ;
	rdfs:label "is vagueness type of"@en ;
	rdfs:comment "It links to the description of vagueness that has the particular vagueness type."@en ;
	rdfs:isDefinedBy <http://www.essepuntato.it/2013/10/vagueness> ;
	owl:inverseOf :hasVaguenessType .

:withDimension a owl:ObjectProperty , owl:FunctionalProperty ;
	rdfs:label "with dimension"@en ;
	rdfs:comment "It links the dimension that is used in a justification according to a particular applicability context."@en ;
	rdfs:isDefinedBy <http://www.essepuntato.it/2013/10/vagueness> ;
	rdfs:range :Dimension ;
	rdfs:domain :DimensionInContext ;
	rdfs:subPropertyOf sit:isSettingFor .

oa:hasBody a owl:ObjectProperty ;
	rdfs:label "has body"@en ;
	rdfs:comment "It links to the description of vagueness/non-vagueness involved in the annotation."@en ;
	dc:description "Note that in the Annotation Ontology the intended meaning of oa:hasBody is broader than what described herein in the entity comment."@en ;
	rdfs:isDefinedBy <http://www.w3.org/ns/oa#> .

oa:hasTarget a owl:ObjectProperty ;
	rdfs:label "has target"@en ;
	rdfs:comment "It links to the entity that has been object of the annotation."@en ;
	dc:description "Note that in the Annotation Ontology the intended meaning of oa:hasTarget is broader than what described herein in the entity comment."@en ;
	rdfs:isDefinedBy <http://www.w3.org/ns/oa#> .

prov:wasAttributedTo a owl:ObjectProperty ;
	rdfs:label "was attributed to"@en ;
	rdfs:comment "It links the annotation of an ontological entity with information about its vagueness to the agent who made the annotation itself."@en ;
	dc:description "Note that in the PROV Ontology the intended meaning of prov:wasAttributedTo is broader than what described herein in the entity comment."@en ;
	rdfs:isDefinedBy <http://www.w3.org/ns/prov#> .

:hasNaturalLanguageText a owl:DatatypeProperty ;
	rdfs:label "has natural language text"@en ;
	rdfs:comment "The natural language text defining the body of either a justification or dimension."@en ;
	rdfs:isDefinedBy <http://www.essepuntato.it/2013/10/vagueness> ;
	rdfs:range rdfs:Literal ;
	rdfs:domain _:node18vkkn01mx34 .

_:node18vkkn01mx34 a owl:Class ;
	owl:unionOf _:node18vkkn01mx35 .

_:node18vkkn01mx35 rdf:first :Dimension ;
	rdf:rest _:node18vkkn01mx36 .

_:node18vkkn01mx36 rdf:first :Justification ;
	rdf:rest rdf:nil .

:ApplicabilityContext a owl:Class ;
	rdfs:label "applicability context of descriptions and related dimensions"@en ;
	rdfs:comment "A context defines precise boundaries of application of descriptions of vagueness/non-vagueness or of the relation between a justification and a certain dimension."@en ;
	rdfs:isDefinedBy <http://www.essepuntato.it/2013/10/vagueness> .

:DescriptionOfNonVagueness a owl:Class ;
	rdfs:label "description of non-vagueness"@en ;
	rdfs:subClassOf _:node18vkkn01mx37 .

_:node18vkkn01mx37 a owl:Restriction ;
	owl:onProperty :hasJustification ;
	owl:minCardinality "1"^^xsd:nonNegativeInteger .

:DescriptionOfNonVagueness rdfs:comment """The descriptive characterisation of non-vagueness to associate to an ontological entity by means of an annotation. It provides at least one justification for considering the target ontological entity non-vague. This description is primarily meant to be used for entities that would typically be considered vague but which, for some reason, in the particular ontology are not. 

A description of non-vagueness is a context-dependent object, which means that it can be applied within the boundaries of a particular context (i.e. the same entity can be vague in one context and non-vague in another)."""@en ;
	rdfs:isDefinedBy <http://www.essepuntato.it/2013/10/vagueness> .

:DescriptionOfVagueness a owl:Class ;
	rdfs:label "description of vagueness"@en ;
	rdfs:subClassOf _:node18vkkn01mx38 .

_:node18vkkn01mx38 a owl:Restriction ;
	owl:onProperty :hasVaguenessType ;
	owl:cardinality "1"^^xsd:nonNegativeInteger .

:DescriptionOfVagueness rdfs:subClassOf _:node18vkkn01mx39 .

_:node18vkkn01mx39 a owl:Restriction ;
	owl:onProperty :hasJustification ;
	owl:minCardinality "1"^^xsd:nonNegativeInteger .

:DescriptionOfVagueness rdfs:comment """The descriptive characterisation of vagueness to associate to an ontological entity by means of an annotation. It specifies a vagueness type and provides at least one justification for considering the target ontological entity vague. 

A description of vagueness is a context-dependent object, which means that it can be applied within the boundaries of a particular context (i.e. the same entity can be vague in one context and non-vague in another)."""@en ;
	rdfs:isDefinedBy <http://www.essepuntato.it/2013/10/vagueness> .

:Dimension a owl:Class ;
	rdfs:label "dimension"@en ;
	rdfs:subClassOf _:node18vkkn01mx40 .

_:node18vkkn01mx40 a owl:Class ;
	owl:unionOf _:node18vkkn01mx42 .

_:node18vkkn01mx42 rdf:first _:node18vkkn01mx41 .

_:node18vkkn01mx41 a owl:Restriction ;
	owl:onProperty :hasEntity ;
	owl:someValuesFrom owl:Thing .

_:node18vkkn01mx42 rdf:rest _:node18vkkn01mx44 .

_:node18vkkn01mx44 rdf:first _:node18vkkn01mx43 .

_:node18vkkn01mx43 a owl:Restriction ;
	owl:onProperty :hasLogicFormula ;
	owl:someValuesFrom owl:Thing .

_:node18vkkn01mx44 rdf:rest _:node18vkkn01mx46 .

_:node18vkkn01mx46 rdf:first _:node18vkkn01mx45 .

_:node18vkkn01mx45 a owl:Restriction ;
	owl:onProperty :hasNaturalLanguageText ;
	owl:someValuesFrom rdfs:Literal .

_:node18vkkn01mx46 rdf:rest rdf:nil .

:Dimension rdfs:comment """A dimension is part of the justification of a description of quantitative vagueness. Dimensions of such a justification are used to identify what boundaries are not defined precisely by a particular entity and, thus, are part of the causes of vagueness for the entity itself. A dimension is defined either as natural language text, an entity, a more complex logic formula, or any combination of them. 

The relation between a justification and a dimension may be context-dependent, which means that it can be applied within the boundaries of a particular context (i.e. the same entity can be vague in dimension A in one context and in dimension B in another). In this case, instances of the classes 'DimensionInContext' should be used to link the justification to the related dimension."""@en ;
	rdfs:isDefinedBy <http://www.essepuntato.it/2013/10/vagueness> .

:DimensionInContext a owl:Class ;
	rdfs:label "dimension in context"@en ;
	rdfs:subClassOf sit:Situation , _:node18vkkn01mx47 .

_:node18vkkn01mx47 a owl:Restriction ;
	owl:onProperty :hasApplicabilityContext ;
	owl:cardinality "1"^^xsd:nonNegativeInteger .

:DimensionInContext rdfs:subClassOf _:node18vkkn01mx48 .

_:node18vkkn01mx48 a owl:Restriction ;
	owl:onProperty :withDimension ;
	owl:cardinality "1"^^xsd:nonNegativeInteger .

:DimensionInContext rdfs:comment "This class describes situations where a particular dimension in considered according to a particular context. In particular, instances of this class are actually specifying that the relation between a justification and a certain dimension must be considered according to a particular applicability context."@en ;
	rdfs:isDefinedBy <http://www.essepuntato.it/2013/10/vagueness> .

:Justification a owl:Class ;
	rdfs:label "justification for vagueness/non-vagueness description"@en ;
	rdfs:subClassOf _:node18vkkn01mx49 .

_:node18vkkn01mx49 a owl:Class ;
	owl:unionOf _:node18vkkn01mx51 .

_:node18vkkn01mx51 rdf:first _:node18vkkn01mx50 .

_:node18vkkn01mx50 a owl:Restriction ;
	owl:onProperty :hasEntity ;
	owl:someValuesFrom owl:Thing .

_:node18vkkn01mx51 rdf:rest _:node18vkkn01mx53 .

_:node18vkkn01mx53 rdf:first _:node18vkkn01mx52 .

_:node18vkkn01mx52 a owl:Restriction ;
	owl:onProperty :hasLogicFormula ;
	owl:someValuesFrom owl:Thing .

_:node18vkkn01mx53 rdf:rest _:node18vkkn01mx55 .

_:node18vkkn01mx55 rdf:first _:node18vkkn01mx54 .

_:node18vkkn01mx54 a owl:Restriction ;
	owl:onProperty :hasNaturalLanguageText ;
	owl:someValuesFrom rdfs:Literal .

_:node18vkkn01mx55 rdf:rest rdf:nil .

:Justification rdfs:comment "A justification that explains one possible reason behind a vagueness/non-vagueness description. It is defined either as natural language text, an entity, a more complex logic formula, or any combination of them."@en ;
	rdfs:isDefinedBy <http://www.essepuntato.it/2013/10/vagueness> .

:VaguenessAnnotation a owl:Class ;
	rdfs:label "annotation of vagueness/non-vagueness"@en ;
	rdfs:subClassOf oa:Annotation , prov:Entity , _:node18vkkn01mx56 .

_:node18vkkn01mx56 a owl:Restriction ;
	owl:onProperty oa:hasTarget ;
	owl:cardinality "1"^^xsd:nonNegativeInteger .

:VaguenessAnnotation rdfs:subClassOf _:node18vkkn01mx57 .

_:node18vkkn01mx57 a owl:Restriction ;
	owl:onProperty prov:wasAttributedTo ;
	owl:someValuesFrom prov:Agent .

:VaguenessAnnotation rdfs:subClassOf _:node18vkkn01mx58 .

_:node18vkkn01mx58 a owl:Restriction ;
	owl:onProperty oa:hasBody ;
	owl:onClass _:node18vkkn01mx59 .

_:node18vkkn01mx59 a owl:Class ;
	owl:unionOf _:node18vkkn01mx60 .

_:node18vkkn01mx60 rdf:first :DescriptionOfNonVagueness ;
	rdf:rest _:node18vkkn01mx61 .

_:node18vkkn01mx61 rdf:first :DescriptionOfVagueness ;
	rdf:rest rdf:nil .

_:node18vkkn01mx58 owl:minQualifiedCardinality "1"^^xsd:nonNegativeInteger .

:VaguenessAnnotation rdfs:comment "The annotation of an ontological entity with information about its vagueness is a particular act of tagging done by someone (i.e., an agent) who associates a description of vagueness/non-vagueness (called the body of the annotation) to the entity in consideration (called the target of the annotation)."@en ;
	rdfs:isDefinedBy <http://www.essepuntato.it/2013/10/vagueness> .

:VaguenessType a owl:Class ;
	rdfs:label "vagueness type"@en ;
	rdfs:comment "A particular kind of vagueness that characterizes the entity."@en ;
	rdfs:isDefinedBy <http://www.essepuntato.it/2013/10/vagueness> .

oa:Annotation a owl:Class ;
	rdfs:label "annotation"@en ;
	rdfs:isDefinedBy <http://www.w3.org/ns/oa#> .

prov:Agent a owl:Class ;
	rdfs:label "agent"@en ;
	dc:description "Note that in the PROV Ontology the intended meaning of prov:Agent is broader than what described herein in the entity comment."@en ;
	rdfs:comment "The agent who tags an ontology entity with a vagueness/non-vagueness description."@en ;
	rdfs:isDefinedBy <http://www.w3.org/ns/prov#> .

prov:Entity a owl:Class ;
	rdfs:label "entity"@en ;
	rdfs:isDefinedBy <http://www.w3.org/ns/prov#> .

:qualitative-vagueness a owl:NamedIndividual , :VaguenessType ;
	rdfs:label "qualitative vagueness"@en ;
	rdfs:comment "A vagueness type that concerns the identification of such other discriminants of which boundaries are not quantifiable in any precise way."@en ;
	rdfs:isDefinedBy <http://www.essepuntato.it/2013/10/vagueness> .

:quantitative-vagueness a owl:NamedIndividual , :VaguenessType ;
	rdfs:label "quantitative vagueness"@en ;
	rdfs:comment "A vagueness type that concerns the (real or apparent) lack of precise boundaries defining an entity along one or more specific dimensions."@en ;
	rdfs:isDefinedBy <http://www.essepuntato.it/2013/10/vagueness> .

_:node18vkkn01mx62 a owl:AllDifferent ;
	owl:distinctMembers _:node18vkkn01mx63 .

_:node18vkkn01mx63 rdf:first :qualitative-vagueness ;
	rdf:rest _:node18vkkn01mx64 .

_:node18vkkn01mx64 rdf:first :quantitative-vagueness ;
	rdf:rest rdf:nil .

_:node18vkkn01mx65 a owl:AllDisjointClasses ;
	owl:members _:node18vkkn01mx66 .

_:node18vkkn01mx66 rdf:first :ApplicabilityContext ;
	rdf:rest _:node18vkkn01mx67 .

_:node18vkkn01mx67 rdf:first :DescriptionOfNonVagueness ;
	rdf:rest _:node18vkkn01mx68 .

_:node18vkkn01mx68 rdf:first :DescriptionOfVagueness ;
	rdf:rest _:node18vkkn01mx69 .

_:node18vkkn01mx69 rdf:first :Dimension ;
	rdf:rest _:node18vkkn01mx70 .

_:node18vkkn01mx70 rdf:first :DimensionInContext ;
	rdf:rest _:node18vkkn01mx71 .

_:node18vkkn01mx71 rdf:first :Justification ;
	rdf:rest _:node18vkkn01mx72 .

_:node18vkkn01mx72 rdf:first :VaguenessAnnotation ;
	rdf:rest _:node18vkkn01mx73 .

_:node18vkkn01mx73 rdf:first :VaguenessType ;
	rdf:rest _:node18vkkn01mx74 .

_:node18vkkn01mx74 rdf:first prov:Agent ;
	rdf:rest rdf:nil .

:hasApplicabilityContext rdfs:domain _:node18vkkn01mx75 .

_:node18vkkn01mx75 a owl:Class ;
	owl:unionOf _:node18vkkn01mx76 .

_:node18vkkn01mx76 rdf:first :DescriptionOfNonVagueness ;
	rdf:rest _:node18vkkn01mx77 .

_:node18vkkn01mx77 rdf:first :DescriptionOfVagueness ;
	rdf:rest _:node18vkkn01mx78 .

_:node18vkkn01mx78 rdf:first :DimensionInContext ;
	rdf:rest rdf:nil .

:hasDimension owl:propertyChainAxiom _:node18vkkn01mx79 .

_:node18vkkn01mx79 rdf:first :hasDimensionInContext ;
	rdf:rest _:node18vkkn01mx80 .

_:node18vkkn01mx80 rdf:first :withDimension ;
	rdf:rest rdf:nil .

:hasDimension rdfs:domain _:node18vkkn01mx81 .

_:node18vkkn01mx81 a owl:Class ;
	owl:intersectionOf _:node18vkkn01mx82 .

_:node18vkkn01mx82 rdf:first :Justification ;
	rdf:rest _:node18vkkn01mx84 .

_:node18vkkn01mx84 rdf:first _:node18vkkn01mx83 .

_:node18vkkn01mx83 a owl:Restriction ;
	owl:onProperty _:node18vkkn01mx85 .

_:node18vkkn01mx85 owl:inverseOf :hasJustification .

_:node18vkkn01mx83 owl:allValuesFrom _:node18vkkn01mx86 .

_:node18vkkn01mx86 a owl:Class ;
	owl:intersectionOf _:node18vkkn01mx87 .

_:node18vkkn01mx87 rdf:first :DescriptionOfVagueness ;
	rdf:rest _:node18vkkn01mx89 .

_:node18vkkn01mx89 rdf:first _:node18vkkn01mx88 .

_:node18vkkn01mx88 a owl:Restriction ;
	owl:onProperty :hasVaguenessType ;
	owl:hasValue :quantitative-vagueness .

_:node18vkkn01mx89 rdf:rest rdf:nil .

_:node18vkkn01mx84 rdf:rest rdf:nil .

:hasDimensionInContext rdfs:domain _:node18vkkn01mx90 .

_:node18vkkn01mx90 a owl:Class ;
	owl:intersectionOf _:node18vkkn01mx91 .

_:node18vkkn01mx91 rdf:first :Justification ;
	rdf:rest _:node18vkkn01mx93 .

_:node18vkkn01mx93 rdf:first _:node18vkkn01mx92 .

_:node18vkkn01mx92 a owl:Restriction ;
	owl:onProperty _:node18vkkn01mx94 .

_:node18vkkn01mx94 owl:inverseOf :hasJustification .

_:node18vkkn01mx92 owl:allValuesFrom _:node18vkkn01mx95 .

_:node18vkkn01mx95 a owl:Class ;
	owl:intersectionOf _:node18vkkn01mx96 .

_:node18vkkn01mx96 rdf:first :DescriptionOfVagueness ;
	rdf:rest _:node18vkkn01mx98 .

_:node18vkkn01mx98 rdf:first _:node18vkkn01mx97 .

_:node18vkkn01mx97 a owl:Restriction ;
	owl:onProperty :hasVaguenessType ;
	owl:hasValue :quantitative-vagueness .

_:node18vkkn01mx98 rdf:rest rdf:nil .

_:node18vkkn01mx93 rdf:rest rdf:nil .

:hasEntity rdfs:domain _:node18vkkn01mx99 .

_:node18vkkn01mx99 a owl:Class ;
	owl:unionOf _:node18vkkn01mx100 .

_:node18vkkn01mx100 rdf:first :Dimension ;
	rdf:rest _:node18vkkn01mx101 .

_:node18vkkn01mx101 rdf:first :Justification ;
	rdf:rest rdf:nil .

:hasJustification rdfs:domain _:node18vkkn01mx102 .

_:node18vkkn01mx102 a owl:Class ;
	owl:unionOf _:node18vkkn01mx103 .

_:node18vkkn01mx103 rdf:first :DescriptionOfNonVagueness ;
	rdf:rest _:node18vkkn01mx104 .

_:node18vkkn01mx104 rdf:first :DescriptionOfVagueness ;
	rdf:rest rdf:nil .

:hasLogicFormula rdfs:domain _:node18vkkn01mx105 .

_:node18vkkn01mx105 a owl:Class ;
	owl:unionOf _:node18vkkn01mx106 .

_:node18vkkn01mx106 rdf:first :Dimension ;
	rdf:rest _:node18vkkn01mx107 .

_:node18vkkn01mx107 rdf:first :Justification ;
	rdf:rest rdf:nil .

:hasNaturalLanguageText rdfs:domain _:node18vkkn01mx108 .

_:node18vkkn01mx108 a owl:Class ;
	owl:unionOf _:node18vkkn01mx109 .

_:node18vkkn01mx109 rdf:first :Dimension ;
	rdf:rest _:node18vkkn01mx110 .

_:node18vkkn01mx110 rdf:first :Justification ;
	rdf:rest rdf:nil .

:DescriptionOfNonVagueness rdfs:subClassOf _:node18vkkn01mx111 .

_:node18vkkn01mx111 a owl:Restriction ;
	owl:onProperty :hasJustification ;
	owl:minCardinality "1"^^xsd:nonNegativeInteger .

:DescriptionOfVagueness rdfs:subClassOf _:node18vkkn01mx112 .

_:node18vkkn01mx112 a owl:Restriction ;
	owl:onProperty :hasVaguenessType ;
	owl:cardinality "1"^^xsd:nonNegativeInteger .

:DescriptionOfVagueness rdfs:subClassOf _:node18vkkn01mx113 .

_:node18vkkn01mx113 a owl:Restriction ;
	owl:onProperty :hasJustification ;
	owl:minCardinality "1"^^xsd:nonNegativeInteger .

:Dimension rdfs:subClassOf _:node18vkkn01mx114 .

_:node18vkkn01mx114 a owl:Class ;
	owl:unionOf _:node18vkkn01mx116 .

_:node18vkkn01mx116 rdf:first _:node18vkkn01mx115 .

_:node18vkkn01mx115 a owl:Restriction ;
	owl:onProperty :hasEntity ;
	owl:someValuesFrom owl:Thing .

_:node18vkkn01mx116 rdf:rest _:node18vkkn01mx118 .

_:node18vkkn01mx118 rdf:first _:node18vkkn01mx117 .

_:node18vkkn01mx117 a owl:Restriction ;
	owl:onProperty :hasLogicFormula ;
	owl:someValuesFrom owl:Thing .

_:node18vkkn01mx118 rdf:rest _:node18vkkn01mx120 .

_:node18vkkn01mx120 rdf:first _:node18vkkn01mx119 .

_:node18vkkn01mx119 a owl:Restriction ;
	owl:onProperty :hasNaturalLanguageText ;
	owl:someValuesFrom rdfs:Literal .

_:node18vkkn01mx120 rdf:rest rdf:nil .

:DimensionInContext rdfs:subClassOf _:node18vkkn01mx121 .

_:node18vkkn01mx121 a owl:Restriction ;
	owl:onProperty :hasApplicabilityContext ;
	owl:cardinality "1"^^xsd:nonNegativeInteger .

:DimensionInContext rdfs:subClassOf _:node18vkkn01mx122 .

_:node18vkkn01mx122 a owl:Restriction ;
	owl:onProperty :withDimension ;
	owl:cardinality "1"^^xsd:nonNegativeInteger .

:Justification rdfs:subClassOf _:node18vkkn01mx123 .

_:node18vkkn01mx123 a owl:Class ;
	owl:unionOf _:node18vkkn01mx125 .

_:node18vkkn01mx125 rdf:first _:node18vkkn01mx124 .

_:node18vkkn01mx124 a owl:Restriction ;
	owl:onProperty :hasEntity ;
	owl:someValuesFrom owl:Thing .

_:node18vkkn01mx125 rdf:rest _:node18vkkn01mx127 .

_:node18vkkn01mx127 rdf:first _:node18vkkn01mx126 .

_:node18vkkn01mx126 a owl:Restriction ;
	owl:onProperty :hasLogicFormula ;
	owl:someValuesFrom owl:Thing .

_:node18vkkn01mx127 rdf:rest _:node18vkkn01mx129 .

_:node18vkkn01mx129 rdf:first _:node18vkkn01mx128 .

_:node18vkkn01mx128 a owl:Restriction ;
	owl:onProperty :hasNaturalLanguageText ;
	owl:someValuesFrom rdfs:Literal .

_:node18vkkn01mx129 rdf:rest rdf:nil .

:VaguenessAnnotation rdfs:subClassOf _:node18vkkn01mx130 .

_:node18vkkn01mx130 a owl:Restriction ;
	owl:onProperty oa:hasTarget ;
	owl:cardinality "1"^^xsd:nonNegativeInteger .

:VaguenessAnnotation rdfs:subClassOf _:node18vkkn01mx131 .

_:node18vkkn01mx131 a owl:Restriction ;
	owl:onProperty prov:wasAttributedTo ;
	owl:someValuesFrom prov:Agent .

:VaguenessAnnotation rdfs:subClassOf _:node18vkkn01mx132 .

_:node18vkkn01mx132 a owl:Restriction ;
	owl:onProperty oa:hasBody ;
	owl:onClass _:node18vkkn01mx133 .

_:node18vkkn01mx133 a owl:Class ;
	owl:unionOf _:node18vkkn01mx134 .

_:node18vkkn01mx134 rdf:first :DescriptionOfNonVagueness ;
	rdf:rest _:node18vkkn01mx135 .

_:node18vkkn01mx135 rdf:first :DescriptionOfVagueness ;
	rdf:rest rdf:nil .

_:node18vkkn01mx132 owl:minQualifiedCardinality "1"^^xsd:nonNegativeInteger .

_:node18vkkn01mx136 a owl:AllDifferent ;
	owl:distinctMembers _:node18vkkn01mx137 .

_:node18vkkn01mx137 rdf:first :qualitative-vagueness ;
	rdf:rest _:node18vkkn01mx138 .

_:node18vkkn01mx138 rdf:first :quantitative-vagueness ;
	rdf:rest rdf:nil .

_:node18vkkn01mx139 a owl:AllDisjointClasses ;
	owl:members _:node18vkkn01mx140 .

_:node18vkkn01mx140 rdf:first :ApplicabilityContext ;
	rdf:rest _:node18vkkn01mx141 .

_:node18vkkn01mx141 rdf:first :DescriptionOfNonVagueness ;
	rdf:rest _:node18vkkn01mx142 .

_:node18vkkn01mx142 rdf:first :DescriptionOfVagueness ;
	rdf:rest _:node18vkkn01mx143 .

_:node18vkkn01mx143 rdf:first :Dimension ;
	rdf:rest _:node18vkkn01mx144 .

_:node18vkkn01mx144 rdf:first :DimensionInContext ;
	rdf:rest _:node18vkkn01mx145 .

_:node18vkkn01mx145 rdf:first :Justification ;
	rdf:rest _:node18vkkn01mx146 .

_:node18vkkn01mx146 rdf:first :VaguenessAnnotation ;
	rdf:rest _:node18vkkn01mx147 .

_:node18vkkn01mx147 rdf:first :VaguenessType ;
	rdf:rest _:node18vkkn01mx148 .

_:node18vkkn01mx148 rdf:first prov:Agent ;
	rdf:rest rdf:nil .
