@prefix dc: <http://purl.org/dc/elements/1.1/> .
@prefix rdfs: <http://www.w3.org/2000/01/rdf-schema#> .
@prefix dctype: <http://purl.org/dc/dcmitype/> .
@prefix dct: <http://purl.org/dc/terms/> .
@prefix xsd: <http://www.w3.org/2001/XMLSchema#> .
@prefix owl: <http://www.w3.org/2002/07/owl#> .
@prefix rdf: <http://www.w3.org/1999/02/22-rdf-syntax-ns#> .
@prefix vann: <http://purl.org/vocab/vann/> .
@prefix aiiso: <http://purl.org/vocab/aiiso/schema#> .
@prefix skos: <http://www.w3.org/2004/02/skos/core#> .
@prefix cc: <http://web.resource.org/cc/> .

<http://www.w3.org/1999/02/22-rdf-syntax-ns> a owl:Ontology ;
	dc:date "2008-05-14" ;
	dc:title "Academic Institution Internal Structure Ontology (AIISO)"@en ;
	rdfs:comment "The Academic Institution Internal Structure Ontology (AIISO) provides classes and properties to describe the internal organisational structure of an academic institution."@en ;
	dc:identifier "http://purl.org/vocab/aiiso/schema" ;
	dct:isVersionOf <http://purl.org/vocab/aiiso/schema#> ;
	dc:creator "Rob Styles" , "Nadeem Shabir" ;
	dc:contributor "Ian Corns" , "Sarah Bartlett" ;
	dc:rights "Copyright Â© 2008 Talis Information Ltd" ;
	vann:preferredNamespaceUri "http://purl.org/vocab/aiiso/schema#" ;
	vann:preferredNamespacePrefix "aiiso" ;
	dct:hasFormat <http://purl.org/vocab/aiiso/schema-20080514.html> .

<http://purl.org/vocab/aiiso/schema-20080514.html> a dctype:Text ;
	dc:format _:node171a4h7blx1 .

_:node171a4h7blx1 a dct:IMT ;
	rdf:value "text/html" ;
	rdfs:label "HTML"@en .

<http://www.w3.org/1999/02/22-rdf-syntax-ns> dct:hasFormat <http://purl.org/vocab/aiiso/schema-20080514.rdf> .

<http://purl.org/vocab/aiiso/schema-20080514.rdf> a dctype:Text ;
	dc:format _:node171a4h7blx2 .

_:node171a4h7blx2 a dct:IMT ;
	rdf:value "application/rdf+xml" ;
	rdfs:label "RDF"@en .

<http://www.w3.org/1999/02/22-rdf-syntax-ns> dct:issued "2008-05-14" ;
	skos:historyNote _:node171a4h7blx3 .

_:node171a4h7blx3 rdf:value "First cut of the ontology published" ;
	dc:date "2008-05-14" ;
	dc:creator "Rob Styles" .

<http://www.w3.org/1999/02/22-rdf-syntax-ns> a cc:Work ;
	cc:license <http://creativecommons.org/licenses/by/2.0/uk/> .

<http://creativecommons.org/licenses/by/2.0/uk/> a cc:License ;
	cc:permits cc:Reproduction , cc:Distribution ;
	cc:requires cc:Notice , cc:Attribution ;
	cc:permits cc:DerivativeWorks .

aiiso:OrganisationalUnit a rdfs:Class ;
	rdfs:label "Organisational Unit"@en ;
	rdfs:comment "An OrganisationalUnit is used to describe a group of people that form a part of an organisations insitutional hierarchy. More specific classes of Institution, Department, Faculty, School, College, Center, Division and Institute exist and are preferred."^^xsd:string ;
	rdfs:isDefinedBy <http://purl.org/vocab/aiiso/schema#> ;
	dct:issued "2008-05-14" .

aiiso:Institution a rdfs:Class ;
	rdfs:label "Institution"@en ;
	rdfs:comment "An Insitution is an OrganisationalUnit that represents the upper most level of an academic institution."^^xsd:string ;
	rdfs:subClassOf aiiso:OrganisationalUnit ;
	rdfs:isDefinedBy <http://purl.org/vocab/aiiso/schema#> ;
	dct:issued "2008-05-14" .

aiiso:Department a rdfs:Class ;
	rdfs:label "Department"@en ;
	rdfs:comment "A Department is an OrganisationalUnit that represents a group of people recognised by an OrganisationalUnit as forming a cohesive group referred to by the organisation as a department."^^xsd:string ;
	rdfs:subClassOf aiiso:OrganisationalUnit ;
	rdfs:isDefinedBy <http://purl.org/vocab/aiiso/schema#> ;
	dct:issued "2008-05-14" .

aiiso:Faculty a rdfs:Class ;
	rdfs:label "Faculty"@en ;
	rdfs:comment "A Faculty is an OrganisationalUnit that represents a group of people recognised by an OrganisationalUnit as forming a cohesive group referred to by the organisation as a faculty."^^xsd:string ;
	rdfs:subClassOf aiiso:OrganisationalUnit ;
	rdfs:isDefinedBy <http://purl.org/vocab/aiiso/schema#> ;
	dct:issued "2008-05-14" .

aiiso:School a rdfs:Class ;
	rdfs:label "School"@en ;
	rdfs:comment "A School is an OrganisationalUnit that represents a group of people recognised by an OrganisationalUnit as forming a cohesive group referred to by the organisation as a school."^^xsd:string ;
	rdfs:subClassOf aiiso:OrganisationalUnit ;
	rdfs:isDefinedBy <http://purl.org/vocab/aiiso/schema#> ;
	dct:issued "2008-05-14" .

aiiso:College a rdfs:Class ;
	rdfs:label "College"@en ;
	rdfs:comment "A College is an OrganisationalUnit that represents a group of people recognised by an OrganisationalUnit as forming a cohesive group referred to by the organisation as a college."^^xsd:string ;
	rdfs:subClassOf aiiso:OrganisationalUnit ;
	rdfs:isDefinedBy <http://purl.org/vocab/aiiso/schema#> ;
	dct:issued "2008-05-14" .

aiiso:Center a rdfs:Class ;
	rdfs:label "Center"@en ;
	rdfs:comment "A Center is an OrganisationalUnit that represents a group of people recognised by an OrganisationalUnit as forming a cohesive group referred to by the organisation as a center."^^xsd:string ;
	rdfs:subClassOf aiiso:OrganisationalUnit ;
	rdfs:isDefinedBy <http://purl.org/vocab/aiiso/schema#> ;
	dct:issued "2008-05-14" .

aiiso:Division a rdfs:Class ;
	rdfs:label "Division"@en ;
	rdfs:comment "A Division is an OrganisationalUnit that represents a group of people recognised by an OrganisationalUnit as forming a cohesive group referred to by the organisation as a division."^^xsd:string ;
	rdfs:subClassOf aiiso:OrganisationalUnit ;
	rdfs:isDefinedBy <http://purl.org/vocab/aiiso/schema#> ;
	dct:issued "2008-05-14" .

aiiso:Institute a rdfs:Class ;
	rdfs:label "Institute"@en ;
	rdfs:comment "An Institute is an OrganisationalUnit that represents a group of people recognised by an OrganisationalUnit as forming a cohesive group referred to by the organisation as an institute."^^xsd:string ;
	rdfs:subClassOf aiiso:OrganisationalUnit ;
	rdfs:isDefinedBy <http://purl.org/vocab/aiiso/schema#> ;
	dct:issued "2008-05-14" .

aiiso:KnowledgeGrouping a rdfs:Class ;
	rdfs:label "KnowledgeGrouping"@en ;
	rdfs:comment "A KnowledgeGrouping represents a collection of resources, learning objectives, timetables, and other materials. The more specific subclasses of Subject, Programme, Course and Module are preferred."^^xsd:string ;
	rdfs:isDefinedBy <http://purl.org/vocab/aiiso/schema#> ;
	dct:issued "2008-05-14" .

aiiso:Programme a rdfs:Class ;
	rdfs:label "Programme"@en ;
	rdfs:comment "A Programme is a KnowledgeGrouping that represents a cohesive collection of educational material referred to by the owning OrganisationalUnit as a programme."^^xsd:string ;
	rdfs:subClassOf aiiso:KnowledgeGrouping ;
	rdfs:isDefinedBy <http://purl.org/vocab/aiiso/schema#> ;
	dct:issued "2008-05-14" .

aiiso:Subject a rdfs:Class ;
	rdfs:label "Subject"@en ;
	rdfs:comment "A Subject is a KnowledgeGrouping that represents a cohesive collection of educational material referred to by the owning OrganisationalUnit as a subject."^^xsd:string ;
	rdfs:subClassOf aiiso:KnowledgeGrouping ;
	rdfs:isDefinedBy <http://purl.org/vocab/aiiso/schema#> ;
	dct:issued "2008-05-14" .

aiiso:Course a rdfs:Class ;
	rdfs:label "Course"@en ;
	rdfs:comment "A Course is a KnowledgeGrouping that represents a cohesive collection of educational material referred to by the owning OrganisationalUnit as a course."^^xsd:string ;
	rdfs:subClassOf aiiso:KnowledgeGrouping ;
	rdfs:isDefinedBy <http://purl.org/vocab/aiiso/schema#> ;
	dct:issued "2008-05-14" .

aiiso:Module a rdfs:Class ;
	rdfs:label "Module"@en ;
	rdfs:comment "A Module is a KnowledgeGrouping that represents a cohesive collection of educational material referred to by the owning OrganisationalUnit as a module."^^xsd:string ;
	rdfs:subClassOf aiiso:KnowledgeGrouping ;
	rdfs:isDefinedBy <http://purl.org/vocab/aiiso/schema#> ;
	dct:issued "2008-05-14" .

aiiso:name a rdf:Property ;
	rdfs:label "name"@en ;
	rdfs:range xsd:string ;
	rdfs:comment "The name given to a KnowledgeGrouping or OrganisationalUnit."^^xsd:string ;
	rdfs:domain aiiso:KnowledgeGrouping , aiiso:OrganisationalUnit ;
	rdfs:subPropertyOf rdfs:Label ;
	rdfs:isDefinedBy <http://purl.org/vocab/aiiso/schema#> ;
	dct:issued "2008-05-14" .

aiiso:code a rdf:Property ;
	rdfs:label "code"@en ;
	rdfs:range xsd:string ;
	rdfs:comment "The code used by an Institution to refer to a KnowledgeGrouping or OrganisationalUnit."^^xsd:string ;
	rdfs:domain aiiso:KnowledgeGrouping , aiiso:OrganisationalUnit ;
	rdfs:isDefinedBy <http://purl.org/vocab/aiiso/schema#> ;
	dct:issued "2008-05-14" .

aiiso:description a rdf:Property ;
	rdfs:label "description"@en ;
	rdfs:range xsd:string ;
	rdfs:comment "A Description of the KnowledgeGrouping or OrganisationalUnit."^^xsd:string ;
	rdfs:domain aiiso:KnowledgeGrouping , aiiso:OrganisationalUnit ;
	rdfs:isDefinedBy <http://purl.org/vocab/aiiso/schema#> ;
	dct:issued "2008-05-14" .

aiiso:organisationalUnit a rdf:Property ;
	rdfs:label "organisationalUnit"@en ;
	rdfs:range aiiso:OrganisationalUnit ;
	rdfs:comment "An OrganisationalUnit may contain other OrganisationalUnits using organisationalUnit."^^xsd:string ;
	rdfs:domain aiiso:OrganisationalUnit ;
	rdfs:isDefinedBy <http://purl.org/vocab/aiiso/schema#> ;
	dct:issued "2008-05-14" .

aiiso:knowledgeGrouping a rdf:Property ;
	rdfs:label "knowledgeGrouping"@en ;
	rdfs:range aiiso:KnowledgeGrouping ;
	rdfs:comment "A KnowledgeGrouping may be contained by another KnowledgeGrouping or an OrganisationalUnit using knowledgeGrouping."^^xsd:string ;
	rdfs:domain aiiso:KnowledgeGrouping , aiiso:OrganisationalUnit ;
	rdfs:isDefinedBy <http://purl.org/vocab/aiiso/schema#> ;
	dct:issued "2008-05-14" .

<http://purl.org/vocab/aiiso/schema-20080514.html> dc:format _:node171a4h7blx4 .

_:node171a4h7blx4 a dct:IMT ;
	rdf:value "text/html" ;
	rdfs:label "HTML"@en .

<http://purl.org/vocab/aiiso/schema-20080514.rdf> dc:format _:node171a4h7blx5 .

_:node171a4h7blx5 a dct:IMT ;
	rdf:value "application/rdf+xml" ;
	rdfs:label "RDF"@en .

<http://www.w3.org/1999/02/22-rdf-syntax-ns> skos:historyNote _:node171a4h7blx6 .

_:node171a4h7blx6 rdf:value "First cut of the ontology published" ;
	dc:date "2008-05-14" ;
	dc:creator "Rob Styles" .
