@prefix wine: <http://www.w3.org/TR/2003/PR-owl-guide-20031209/wine#> .
@prefix foaf: <http://xmlns.com/foaf/0.1/> .
@prefix fowl: <http://www.w3.org/TR/2003/PR-owl-guide-20031209/food#> .
@prefix status: <http://www.w3.org/2003/06/sw-vocab-status/ns#> .
@prefix yago: <http://dbpedia.org/class/yago/> .
@prefix vann: <http://purl.org/vocab/vann/> .
@prefix dcterms: <http://purl.org/dc/terms/> .
@prefix adms: <http://www.w3.org/ns/adms#> .
@prefix rdfs: <http://www.w3.org/2000/01/rdf-schema#> .
@prefix time: <http://www.w3.org/2006/time#> .
@prefix beverage: <http://rdfs.co/bevon/beverage/> .
@prefix container: <http://rdfs.co/bevon/container/> .
@prefix food: <http://data.lirmm.fr/ontologies/food#> .
@prefix xsd: <http://www.w3.org/2001/XMLSchema#> .
@prefix dbpedia: <http://dbpedia.org/ontology/> .
@prefix owl: <http://www.w3.org/2002/07/owl#> .
@prefix whisky: <http://purl.org/vocab/whisky/terms/> .
@prefix rdf: <http://www.w3.org/1999/02/22-rdf-syntax-ns#> .
@prefix pto: <http://www.productontology.org/id/> .
@prefix bevon: <http://rdfs.co/bevon/> .
@prefix gr: <http://purl.org/goodrelations/v1#> .
@prefix skos: <http://www.w3.org/2004/02/skos/core#> .
@prefix cc: <http://creativecommons.org/ns#> .

<http://creativecommons.org/licenses/by/3.0/> cc:permits cc:DerivativeWorks , cc:Distribution , cc:Reproduction ;
	cc:requires cc:Attribution , cc:Notice ;
	a cc:License .

<http://jayg.me/> a foaf:Person ;
	foaf:homepage <http://jayg.org/> ;
	foaf:mbox_sha1sum "a637717b7e34b83694018e8fdd3ff334fffcd4f3" ;
	foaf:name "James G. Kim"@en , "김보람"@ko .

whisky:Distillery rdfs:subClassOf bevon:Distillery .

whisky:abv rdfs:subPropertyOf bevon:abv .

whisky:distillery rdfs:subPropertyOf bevon:distillery .

<http://rdfs.co/bevon/0.6> cc:license <http://creativecommons.org/licenses/by/4.0/> ;
	dcterms:creator <http://jayg.me/> ;
	dcterms:description "\n    Beverage Ontology is a Web vocabulary for describing beverages, mainly\n    alcoholic.\n    "@en ;
	dcterms:hasFormat <http://rdfs.co/bevon/0.6/html> , <http://rdfs.co/bevon/0.6/rdf> , <http://rdfs.co/bevon/0.6/ttl> ;
	dcterms:identifier "http://rdfs.co/bevon/0.6" ;
	dcterms:isVersionOf <http://rdfs.co/bevon/> ;
	dcterms:issued "2013-07-04+09:00"^^xsd:date ;
	dcterms:modified "2014-03-03+09:00"^^xsd:date ;
	dcterms:rights "Copyright © 2013-2014 James G. Kim Some Rights Reserved." ;
	dcterms:title "BEVON: Beverage Ontology"@en ;
	dcterms:type <http://purl.org/adms/assettype/Ontology> ;
	vann:preferredNamespacePrefix "bevon" ;
	vann:preferredNamespaceUri "http://rdfs.co/bevon/" ;
	a cc:Work , owl:Ontology , adms:SemanticAsset ;
	rdfs:comment "\n    <div>\n      The master version of this vocabulary is maintained in <a\n      href=\"https://github.com/jgkim/bevon\">the GitHub repository</a> so others\n      can contribute edits and improvements.\n    </div>\n    "^^rdf:XMLLiteral , "\n    Most of the descriptions given here are from Wikipedia or from the websites\n    of the related products.\n    "@en ;
	rdfs:seeAlso <https://github.com/jgkim/bevon> ;
	owl:versionInfo "0.6" .

_:node18ib1jcplx1 dcterms:creator <http://jayg.me/> ;
	dcterms:date "2014-03-01+09:00"^^xsd:date ;
	rdf:value "Minor revisions for documentation" .

<http://rdfs.co/bevon/0.6> skos:changeNote _:node18ib1jcplx1 .

_:node18ib1jcplx2 dcterms:creator <http://jayg.me/> ;
	dcterms:date "2014-03-03+09:00"^^xsd:date ;
	rdf:value "Added a link to the GitHub repository" .

<http://rdfs.co/bevon/0.6> skos:changeNote _:node18ib1jcplx2 ;
	adms:status <http://purl.org/adms/status/UnderDevelopment> .

_:node18ib1jcplx3 a dcterms:IMT ;
	rdf:value "text/html" ;
	rdfs:label "HTML"@en .

<http://rdfs.co/bevon/0.6/html> dcterms:format _:node18ib1jcplx3 .

_:node18ib1jcplx4 a dcterms:IMT ;
	rdf:value "application/rdf+xml" ;
	rdfs:label "RDF/XML"@en .

<http://rdfs.co/bevon/0.6/rdf> dcterms:format _:node18ib1jcplx4 .

_:node18ib1jcplx5 a dcterms:IMT ;
	rdf:value "text/turtle" ;
	rdfs:label "Turtle"@en .

<http://rdfs.co/bevon/0.6/ttl> dcterms:format _:node18ib1jcplx5 .

bevon:Aging dcterms:issued "2013-07-04+09:00"^^xsd:date ;
	dcterms:modified "2014-03-01+09:00"^^xsd:date ;
	a owl:Class ;
	rdfs:isDefinedBy <http://rdfs.co/bevon/> ;
	status:term_status "unstable"@en ;
	skos:definition "\n    Aging is the process of storing beverages in casks for a specific period of\n    time to remove harsh flavors and add distinct characteristics found in the\n    cask's wood.\n    "@en ;
	skos:prefLabel "Aging"@en , "숙성"@ko .

bevon:AlcoholicBeverage dcterms:issued "2013-07-04+09:00"^^xsd:date ;
	dcterms:modified "2014-03-01+09:00"^^xsd:date ;
	a owl:Class ;
	rdfs:isDefinedBy <http://rdfs.co/bevon/> ;
	rdfs:seeAlso <http://en.wikipedia.org/wiki/Alcoholic_beverage> ;
	rdfs:subClassOf bevon:Beverage , pto:Alcoholic_beverage ;
	owl:disjointWith bevon:NonAlcoholicBeverage ;
	status:term_status "testing"@en ;
	skos:definition "\n     An alcoholic beverage is a drink and psychoactive drug containing\n     ethyl alcohol which is commonly referred to as ethanol.\n     "@en ;
	skos:prefLabel "Alcoholic Beverage"@en , "알코올 음료"@ko .

bevon:Ale dcterms:issued "2013-07-04+09:00"^^xsd:date ;
	dcterms:modified "2014-03-01+09:00"^^xsd:date ;
	a owl:Class ;
	rdfs:comment "\n    The yeast will ferment the beer quickly, giving it a sweet, full bodied and\n    fruity taste.\n    "@en ;
	rdfs:isDefinedBy <http://rdfs.co/bevon/> ;
	rdfs:seeAlso <http://en.wikipedia.org/wiki/Ale> ;
	rdfs:subClassOf bevon:Beer , pto:Ale ;
	status:term_status "unstable"@en ;
	skos:definition "\n    Ale is a type of beer brewed from malted barley using a warm-fermentation\n    with a strain of brewers' yeast.\n    "@en ;
	skos:prefLabel "Ale"@en , "에일"@ko .

bevon:AmericanWhiskey dcterms:issued "2013-07-04+09:00"^^xsd:date ;
	dcterms:modified "2014-03-01+09:00"^^xsd:date ;
	a owl:Class ;
	rdfs:comment "\n    The production and labeling of American whiskey are governed by Title 27 of\n    the U.S. Code of Federal Regulations.\n    "@en ;
	rdfs:isDefinedBy <http://rdfs.co/bevon/> ;
	rdfs:seeAlso <http://en.wikipedia.org/wiki/American_whiskey> ;
	rdfs:subClassOf bevon:Whisky , pto:American_whiskey ;
	status:term_status "unstable"@en ;
	skos:altLabel "American Whisky"@en ;
	skos:definition "\n    American whiskey is a distilled beverage produced in the United States from\n    a fermented mash of cereal grain.\n    "@en ;
	skos:prefLabel "American Whiskey"@en , "아메리칸 위스키"@ko .

bevon:Beer dcterms:issued "2013-07-04+09:00"^^xsd:date ;
	dcterms:modified "2014-03-01+09:00"^^xsd:date ;
	a owl:Class ;
	rdfs:comment "\n    The starch and saccharification enzymes are often derived from malted cereal\n    grains, most commonly malted barley and malted wheat.\n    "@en ;
	rdfs:isDefinedBy <http://rdfs.co/bevon/> ;
	rdfs:seeAlso <http://en.wikipedia.org/wiki/Beer> ;
	rdfs:subClassOf bevon:FermentedBeverages , pto:Beer ;
	owl:disjointWith bevon:NonAlcoholicBeer ;
	status:term_status "testing"@en ;
	skos:definition "\n    Beer is an alcoholic beverage produced by the saccharification of starch and\n    fermentation of the resulting sugar.\n    "@en ;
	skos:prefLabel "Beer"@en , "맥주"@ko .

bevon:BeerBottle dcterms:issued "2013-07-04+09:00"^^xsd:date ;
	dcterms:modified "2014-03-01+09:00"^^xsd:date ;
	a owl:Class ;
	rdfs:comment "\n    Dark amber or brown glass greatly reduces UV light from spoiling the beer.\n    However, lighter colored bottles are often used for marketing reasons.\n    "@en ;
	rdfs:isDefinedBy <http://rdfs.co/bevon/> ;
	rdfs:seeAlso <http://en.wikipedia.org/wiki/Beer_bottle> ;
	rdfs:subClassOf bevon:GlassBottle ;
	status:term_status "unstable"@en ;
	skos:definition "\n    A beer bottle is a bottle made to contain beer, usually made of glass and\n    come in various sizes, shapes and colors.\n    "@en ;
	skos:prefLabel "Beer Bottle"@en , "맥주병"@ko .

bevon:BeerCocktail dcterms:issued "2013-07-04+09:00"^^xsd:date ;
	dcterms:modified "2014-03-01+09:00"^^xsd:date ;
	a owl:Class ;
	rdfs:isDefinedBy <http://rdfs.co/bevon/> ;
	rdfs:seeAlso <http://en.wikipedia.org/wiki/Beer_cocktail> ;
	rdfs:subClassOf bevon:Cocktail , pto:Beer_cocktail ;
	status:term_status "unstable"@en ;
	skos:definition "\n    A beer cocktail is a cocktail that is made by mixing beer with a distilled\n    beverage. In this type of cocktail, the primary ingredient is beer.\n    "@en ;
	skos:prefLabel "Beer Cocktail"@en , "맥주 칵테일"@ko .

bevon:BeerKeg dcterms:issued "2013-07-04+09:00"^^xsd:date ;
	dcterms:modified "2014-03-01+09:00"^^xsd:date ;
	a owl:Class ;
	rdfs:isDefinedBy <http://rdfs.co/bevon/> ;
	rdfs:subClassOf bevon:Keg ;
	status:term_status "unstable"@en ;
	skos:definition "\n    Beer kegs are made of stainless steel, or less commonly, of aluminium.\n    "@en ;
	skos:prefLabel "Beer Keg"@en , "맥주 케그"@ko .

bevon:Beverage dcterms:issued "2013-07-04+09:00"^^xsd:date ;
	dcterms:modified "2014-03-01+09:00"^^xsd:date ;
	a owl:Class ;
	rdfs:isDefinedBy <http://rdfs.co/bevon/> ;
	rdfs:seeAlso <http://en.wikipedia.org/wiki/Beverage> ;
	rdfs:subClassOf food:Food , pto:Drink , fowl:PotableLiquid ;
	status:term_status "testing"@en ;
	skos:altLabel "Drink"@en ;
	skos:definition "\n    A beverage, or drink, is a kind of liquid which is specifically prepared\n    for human consumption.\n    "@en ;
	skos:prefLabel "Beverage"@en , "음료"@ko .

bevon:BeverageCan dcterms:issued "2013-07-04+09:00"^^xsd:date ;
	dcterms:modified "2014-03-01+09:00"^^xsd:date ;
	a owl:Class ;
	rdfs:comment "\n    Beverage cans are made of aluminium (75% of worldwide production) or\n    tin-plated steel (25% worldwide production).\n    "@en ;
	rdfs:isDefinedBy <http://rdfs.co/bevon/> ;
	rdfs:seeAlso <http://en.wikipedia.org/wiki/Beverage_can> ;
	rdfs:subClassOf bevon:Container ;
	status:term_status "unstable"@en ;
	skos:definition "\n    A beverage can is a metal container designed to hold a fixed portion of\n    liquid such as a carbonated soft drinks, alcoholic beverages, fruit juices,\n    teas, tisanes, energy drinks, etc.\n    "@en ;
	skos:prefLabel "Beverage Can"@en , "음료 캔"@ko .

bevon:BourbonWhiskey dcterms:issued "2013-07-04+09:00"^^xsd:date ;
	dcterms:modified "2014-03-01+09:00"^^xsd:date ;
	a owl:Class ;
	rdfs:comment "\n    The name of the spirit derives from its historical association with an area\n    known as Old Bourbon, around what is now Bourbon County, Kentucky (which,\n    in turn, was named after the French House of Bourbon royal family). It has\n    been produced since the 18th century. While it may be made anywhere in the\n    United States, it is strongly associated with the American South in\n    general, and Kentucky in particular.\n    "@en ;
	rdfs:isDefinedBy <http://rdfs.co/bevon/> ;
	rdfs:seeAlso <http://en.wikipedia.org/wiki/Bourbon_whiskey> ;
	rdfs:subClassOf bevon:AmericanWhisky , pto:Bourbon_whiskey ;
	status:term_status "unstable"@en ;
	skos:altLabel "Bourbon Whisky"@en ;
	skos:definition "\n    Bourbon whiskey is a type of American whiskey – a barrel-aged distilled\n    spirit made primarily from corn.\n    "@en ;
	skos:prefLabel "Bourbon Whiskey"@en , "버번 위스키"@ko .

bevon:Brandy dcterms:issued "2013-07-04+09:00"^^xsd:date ;
	dcterms:modified "2014-03-01+09:00"^^xsd:date ;
	a owl:Class ;
	rdfs:comment "\n    Brandy generally contains 35–60% alcohol by volume (70–120 US proof) and is\n    typically taken as an after-dinner drink. Some brandies are aged in wooden\n    casks, some are colored with caramel coloring to imitate the effect of\n    aging, and some brandies are produced using a combination of both aging and\n    coloring.\n    "@en ;
	rdfs:isDefinedBy <http://rdfs.co/bevon/> ;
	rdfs:seeAlso <http://en.wikipedia.org/wiki/Brandy> ;
	rdfs:subClassOf bevon:DistilledBeverage , pto:Brandy ;
	status:term_status "testing"@en ;
	skos:definition "\n    Brandy (from brandywine, derived from Dutch brandewijn—\"burnt wine\") is a\n    spirit produced by distilling wine.\n    "@en ;
	skos:prefLabel "Brandy"@en , "브랜디"@ko .

bevon:Brewery dcterms:issued "2013-07-04+09:00"^^xsd:date ;
	dcterms:modified "2014-03-01+09:00"^^xsd:date ;
	a owl:Class ;
	rdfs:comment "\n    A company that makes beer is called either a brewery or a brewing company.\n    "@en ;
	rdfs:isDefinedBy <http://rdfs.co/bevon/> ;
	rdfs:seeAlso <http://dbpedia.org/resource/Brewery> ;
	status:term_status "unstable"@en ;
	skos:definition "\n    A brewery is a dedicated building for the making of beer, though beer can\n    be made at home, and has been for much of beer's history.\n    "@en ;
	skos:prefLabel "Brewery"@en , "양조장"@ko .

bevon:CanadianWhisky dcterms:issued "2013-07-04+09:00"^^xsd:date ;
	dcterms:modified "2014-03-01+09:00"^^xsd:date ;
	a owl:Class ;
	rdfs:comment "\n    Most Canadian whiskies are blended multi-grain liquors containing a large\n    percentage of corn spirits, and are typically lighter and smoother than\n    other whisky styles.\n    "@en ;
	rdfs:isDefinedBy <http://rdfs.co/bevon/> ;
	rdfs:seeAlso <http://en.wikipedia.org/wiki/Canadian_whisky> ;
	rdfs:subClassOf bevon:Whisky , pto:Canadian_whisky ;
	status:term_status "unstable"@en ;
	skos:altLabel "Canadian Whiskey"@en ;
	skos:definition "\n    Canadian whisky is a type of whisky produced in Canada.\n    "@en ;
	skos:prefLabel "Canadian Whisky"@en , "캐내디언 위스키"@ko .

bevon:CarbonatedWater dcterms:issued "2013-07-04+09:00"^^xsd:date ;
	dcterms:modified "2014-03-01+09:00"^^xsd:date ;
	a owl:Class ;
	rdfs:isDefinedBy <http://rdfs.co/bevon/> ;
	rdfs:seeAlso <http://en.wikipedia.org/wiki/Carbonated_water> ;
	rdfs:subClassOf bevon:Water , pto:Carbonated_water ;
	status:term_status "unstable"@en ;
	skos:altLabel "Club Soda"@en , "Fizzy Water"@en , "Seltzer Water"@en , "Soda Water"@en , "Sparkling Water"@en , "소다수"@ko , "클럽소다"@ko ;
	skos:definition "\n    Carbonated water is water into which carbon dioxide gas under pressure has\n    been dissolved.\n    "@en ;
	skos:prefLabel "Carbonated Water"@en , "탄산수"@ko .

bevon:Cocktail dcterms:issued "2013-07-04+09:00"^^xsd:date ;
	dcterms:modified "2014-03-01+09:00"^^xsd:date ;
	a owl:Class ;
	rdfs:comment "\n    Cocktails were originally a mixture of spirits, sugar, water, and bitters.\n    It is now often used for almost any mixed drink that contains alcohol,\n    including mixers, mixed shots, etc. A cocktail today usually contains one\n    or more kinds of spirit and one or more mixers, such as soda or fruit juice.\n    Additional ingredients may be sugar, honey, milk, cream, and various herbs.\n    "@en ;
	rdfs:isDefinedBy <http://rdfs.co/bevon/> ;
	rdfs:seeAlso <http://en.wikipedia.org/wiki/Cocktail> ;
	rdfs:subClassOf bevon:AlcoholicBeverage , bevon:MixedDrink , pto:Cocktail ;
	owl:disjointWith bevon:Mocktail ;
	status:term_status "unstable"@en ;
	skos:definition "\n    A cocktail is a mixed drink that contains alcohol, including mixers, mixed\n    shots, etc.\n    "@en ;
	skos:prefLabel "Cocktail"@en , "칵테일"@ko .

bevon:Cognac dcterms:issued "2013-07-04+09:00"^^xsd:date ;
	dcterms:modified "2014-03-01+09:00"^^xsd:date ;
	a owl:Class ;
	rdfs:comment "\n    It is produced in the wine-growing region surrounding the town from which\n    it takes its name, in the French Departements of Charente and\n    Charente-Maritime.\n    "@en ;
	rdfs:isDefinedBy <http://rdfs.co/bevon/> ;
	rdfs:seeAlso <http://en.wikipedia.org/wiki/Cognac> ;
	rdfs:subClassOf bevon:Brandy , pto:Cognac ;
	status:term_status "testing"@en ;
	skos:definition "\n    Cognac, named after the town of Cognac in France, is a variety of brandy.\n    "@en ;
	skos:prefLabel "Cognac"@en , "코냑"@ko .

bevon:Container dcterms:issued "2013-07-04+09:00"^^xsd:date ;
	dcterms:modified "2014-03-01+09:00"^^xsd:date ;
	a owl:Class ;
	rdfs:isDefinedBy <http://rdfs.co/bevon/> ;
	rdfs:seeAlso <http://en.wikipedia.org/wiki/Container> ;
	rdfs:subClassOf yago:Containers ;
	status:term_status "unstable"@en ;
	skos:definition "\n    A container is a item used to contain, store, and transport a beverage.\n    "@en ;
	skos:prefLabel "Container"@en , "용기"@ko .

bevon:DilutedSoju dcterms:issued "2013-07-04+09:00"^^xsd:date ;
	dcterms:modified "2014-03-01+09:00"^^xsd:date ;
	a owl:Class ;
	rdfs:isDefinedBy <http://rdfs.co/bevon/> ;
	rdfs:subClassOf bevon:Soju ;
	owl:disjointWith bevon:DistilledSoju ;
	status:term_status "unstable"@en ;
	skos:definition "\n    Diluted Soju is made by mixing pure ethanol distilled from various grains,\n    such as potatoes, wheat, barley, sweet potatoes, or tapioca, with water and\n    flavoring.\n    "@en ;
	skos:prefLabel "Diluted Soju"@en , "희석식 소주"@ko .

bevon:DistilledBeverage dcterms:issued "2013-07-04+09:00"^^xsd:date ;
	dcterms:modified "2014-03-01+09:00"^^xsd:date ;
	a owl:Class ;
	rdfs:comment "\n     This excludes undistilled fermented beverages such as beer, wine, and\n     cider.\n     "@en ;
	rdfs:isDefinedBy <http://rdfs.co/bevon/> ;
	rdfs:seeAlso <http://en.wikipedia.org/wiki/Distilled_beverage> ;
	rdfs:subClassOf bevon:AlcoholicBeverage , pto:Distilled_beverage ;
	status:term_status "testing"@en ;
	skos:altLabel "Liquor"@en , "Spirit"@en ;
	skos:definition "\n     A distilled beverage, spirit, or liquor is an alcoholic beverage\n     containing ethanol that is produced by distilling (i.e., concentrating\n     by distillation) ethanol produced by means of fermenting grain, fruit,\n     or vegetables.\n     "@en ;
	skos:prefLabel "Distilled Beverage"@en , "증류주"@ko .

bevon:DistilledSoju dcterms:issued "2013-07-04+09:00"^^xsd:date ;
	dcterms:modified "2014-03-01+09:00"^^xsd:date ;
	a owl:Class ;
	rdfs:isDefinedBy <http://rdfs.co/bevon/> ;
	rdfs:subClassOf bevon:Soju ;
	owl:disjointWith bevon:DilutedSoju ;
	status:term_status "unstable"@en ;
	skos:definition "\n    Distilled Soju is manufactured traditionally by distillation from grains,\n    mainly rice.\n    "@en ;
	skos:prefLabel "Distilled Soju"@en , "증류식 소주"@ko .

bevon:Distillery dcterms:issued "2013-07-04+09:00"^^xsd:date ;
	dcterms:modified "2014-03-01+09:00"^^xsd:date ;
	a owl:Class ;
	rdfs:isDefinedBy <http://rdfs.co/bevon/> ;
	rdfs:seeAlso <http://en.wikipedia.org/wiki/Distillation> ;
	status:term_status "unstable"@en ;
	skos:definition "\n    A distillery is a premise where distillation takes place, especially\n    distillation of alcohol.\n    "@en ;
	skos:prefLabel "Distillery"@en , "증류소"@ko .

bevon:DryStout dcterms:issued "2013-07-04+09:00"^^xsd:date ;
	dcterms:modified "2014-03-01+09:00"^^xsd:date ;
	a owl:Class ;
	rdfs:isDefinedBy <http://rdfs.co/bevon/> ;
	rdfs:subClassOf bevon:Stout ;
	status:term_status "unstable"@en ;
	skos:altLabel "Irish Stout"@en ;
	skos:definition "\n    Irish stout or dry stout is very dark or rich in color and it often has a\n    \"roasted\" or coffee-like taste.\n    "@en ;
	skos:prefLabel "Dry Stout"@en , "드라이 스타우트"@ko .

bevon:Dunkel dcterms:issued "2013-07-04+09:00"^^xsd:date ;
	dcterms:modified "2014-03-01+09:00"^^xsd:date ;
	a owl:Class ;
	rdfs:comment "\n    Dunkel is the German word meaning dark, and dunkel beers typically range in\n    color from amber to dark reddish brown. They are characterized by their\n    smooth malty flavor.\n    "@en ;
	rdfs:isDefinedBy <http://rdfs.co/bevon/> ;
	rdfs:seeAlso <https://en.wikipedia.org/wiki/Dunkel> ;
	rdfs:subClassOf bevon:Lager , pto:Dunkel ;
	status:term_status "unstable"@en ;
	skos:altLabel "Dunkles"@en ;
	skos:definition "\n    Dunkel, or Dunkles, is a word used for several types of dark German lager.\n    "@en ;
	skos:prefLabel "Dunkel"@en , "둔켈"@ko .

bevon:FermentationBase dcterms:issued "2013-07-04+09:00"^^xsd:date ;
	dcterms:modified "2014-03-01+09:00"^^xsd:date ;
	a owl:Class ;
	rdfs:isDefinedBy <http://rdfs.co/bevon/> ;
	status:term_status "unstable"@en ;
	skos:definition "\n    A fruit or grain which provides the sugar for fermentation from which a\n    alcoholic beverage is made.\n    "@en ;
	skos:prefLabel "Fermentation Base"@en , "발효 주재료"@ko .

bevon:FermentedBeverages dcterms:issued "2013-07-04+09:00"^^xsd:date ;
	dcterms:modified "2014-03-01+09:00"^^xsd:date ;
	a owl:Class ;
	rdfs:isDefinedBy <http://rdfs.co/bevon/> ;
	rdfs:subClassOf bevon:AlcoholicBeverage ;
	status:term_status "testing"@en ;
	skos:altLabel "발효주"@ko ;
	skos:definition "\n    A fermented beverage is a drink produced by fermenting grain, fruit, or\n    vegetables.\n    "@en ;
	skos:prefLabel "Fermented Beverage"@en , "양조주"@ko .

bevon:Gin dcterms:issued "2013-07-04+09:00"^^xsd:date ;
	dcterms:modified "2014-03-01+09:00"^^xsd:date ;
	a owl:Class ;
	rdfs:isDefinedBy <http://rdfs.co/bevon/> ;
	rdfs:seeAlso <http://en.wikipedia.org/wiki/Gin> ;
	rdfs:subClassOf bevon:DistilledBeverage , pto:Gin ;
	status:term_status "testing"@en ;
	skos:definition "\n    Gin is a spirit which derives its predominant flavor from juniper berries\n    (Juniperus communis).\n    "@en ;
	skos:prefLabel "Gin"@en , "진"@ko .

bevon:GlassBottle dcterms:issued "2013-07-04+09:00"^^xsd:date ;
	dcterms:modified "2014-03-01+09:00"^^xsd:date ;
	a owl:Class ;
	rdfs:comment "\n    Glass bottles can vary in size considerably, but are most commonly found in\n    sizes ranging between about 10ml and 5 litres.\n    "@en ;
	rdfs:isDefinedBy <http://rdfs.co/bevon/> ;
	rdfs:seeAlso <http://en.wikipedia.org/wiki/Glass_bottle> ;
	rdfs:subClassOf bevon:Container ;
	status:term_status "unstable"@en ;
	skos:definition "\n    A glass bottle is a bottle created from glass.\n    "@en ;
	skos:prefLabel "Glass Bottle"@en , "유리병"@ko .

bevon:Highball dcterms:issued "2013-07-04+09:00"^^xsd:date ;
	dcterms:modified "2014-03-01+09:00"^^xsd:date ;
	a owl:Class ;
	rdfs:isDefinedBy <http://rdfs.co/bevon/> ;
	rdfs:seeAlso <http://en.wikipedia.org/wiki/Highball> ;
	rdfs:subClassOf bevon:Cocktail , pto:Highball ;
	status:term_status "unstable"@en ;
	skos:definition "\n    Highball is the name for a family of mixed drinks that are composed of an\n    alcoholic base spirit and a larger proportion of a non-alcoholic mixer.\n    "@en ;
	skos:prefLabel "Highball"@en , "하이볼"@ko .

bevon:IrishRedAle dcterms:issued "2013-07-04+09:00"^^xsd:date ;
	dcterms:modified "2014-03-01+09:00"^^xsd:date ;
	a owl:Class ;
	rdfs:isDefinedBy <http://rdfs.co/bevon/> ;
	rdfs:seeAlso <http://en.wikipedia.org/wiki/Irish_red_ale> ;
	rdfs:subClassOf bevon:PaleAle ;
	status:term_status "unstable"@en ;
	skos:definition "\n    Irish red ale, red ale, or Irish ale is a name used by brewers in Ireland.\n    "@en ;
	skos:prefLabel "Irish Red Ale"@en , "아이리쉬 레드 에일"@ko .

bevon:IrishWhiskey dcterms:issued "2013-07-04+09:00"^^xsd:date ;
	dcterms:modified "2014-03-01+09:00"^^xsd:date ;
	a owl:Class ;
	rdfs:comment "\n    Key regulations defining Irish whiskey and its production are established\n    by the Irish Whiskey Act of 1980.\n    "@en ;
	rdfs:isDefinedBy <http://rdfs.co/bevon/> ;
	rdfs:seeAlso <http://en.wikipedia.org/wiki/Irish_whiskey> ;
	rdfs:subClassOf bevon:Whisky , pto:Irish_whiskey ;
	status:term_status "unstable"@en ;
	skos:altLabel "Irish Whisky"@en ;
	skos:definition "\n    Irish whiskey is whisky made in Ireland.\n    "@en ;
	skos:prefLabel "Fuisce"@ga , "Irish Whiskey"@en , "아이리쉬 위스키"@ko .

bevon:JapaneseWhisky dcterms:issued "2013-07-04+09:00"^^xsd:date ;
	dcterms:modified "2014-03-01+09:00"^^xsd:date ;
	a owl:Class ;
	rdfs:commercial "\n    Whisky production in Japan began around 1870, but the first commercial\n    production was in 1924 upon the opening of the country's first distillery,\n    Yamazaki. Broadly speaking the style of Japanese whisky is more similar to\n    that of Scotch whisky than Irish, American, or Canadian styles of whisky,\n    and thus the spelling typically follows the Scottish convention (omitting\n    the letter \"e\").\n    "@en ;
	rdfs:isDefinedBy <http://rdfs.co/bevon/> ;
	rdfs:seeAlso <http://en.wikipedia.org/wiki/Japanese_whisky> ;
	rdfs:subClassOf bevon:Whisky , pto:Japanese_whisky ;
	status:term_status "unstable"@en ;
	skos:altLabel "Japanese Whiskey"@en ;
	skos:definition "\n    Japanese whisky is whisky made in Japan.\n    "@en ;
	skos:prefLabel "Japanese Whisky"@en , "재패니즈 위스키"@ko .

bevon:Keg dcterms:issued "2013-07-04+09:00"^^xsd:date ;
	dcterms:modified "2014-03-01+09:00"^^xsd:date ;
	a owl:Class ;
	rdfs:isDefinedBy <http://rdfs.co/bevon/> ;
	rdfs:seeAlso <http://en.wikipedia.org/wiki/Keg> ;
	rdfs:subClassOf bevon:Container ;
	status:term_status "unstable"@en ;
	skos:definition "\n    A keg is a small barrel.\n    "@en ;
	skos:prefLabel "Keg"@en , "케그"@ko .

bevon:Lager dcterms:issued "2013-07-04+09:00"^^xsd:date ;
	dcterms:modified "2014-03-01+09:00"^^xsd:date ;
	a owl:Class ;
	rdfs:isDefinedBy <http://rdfs.co/bevon/> ;
	rdfs:seeAlso <http://en.wikipedia.org/wiki/Lager> ;
	rdfs:subClassOf bevon:Beer , pto:Lager ;
	status:term_status "unstable"@en ;
	skos:definition "\n    Lager is a type of beer that is fermented and conditioned at low\n    temperatures.\n    "@en ;
	skos:prefLabel "Lager"@en , "라거"@ko .

bevon:Liqueur dcterms:issued "2013-07-04+09:00"^^xsd:date ;
	dcterms:modified "2014-03-01+09:00"^^xsd:date ;
	a owl:Class ;
	rdfs:comment "\n    Liqueurs are typically quite sweet; they are usually not aged for long\n    after the ingredients are mixed, but may have resting periods during their\n    production to allow flavors to marry.\n    "@en ;
	rdfs:isDefinedBy <http://rdfs.co/bevon/> ;
	rdfs:seeAlso <http://en.wikipedia.org/wiki/Liqueur> ;
	rdfs:subClassOf bevon:DistilledBeverage , pto:Liqueur ;
	status:term_status "testing"@en ;
	skos:altLabel "Cordials"@en , "Schnapps"@en ;
	skos:definition "\n    A liqueur is an alcoholic beverage made from a distilled spirit that has\n    been flavored with fruit, cream, herbs, spices, flowers or nuts and bottled\n    with added sugar or other sweetener (such as high-fructose corn syrup).\n    "@en ;
	skos:prefLabel "Liqueur"@en , "리큐어"@ko .

bevon:Longneck dcterms:issued "2013-07-04+09:00"^^xsd:date ;
	dcterms:modified "2014-03-01+09:00"^^xsd:date ;
	a owl:Class ;
	rdfs:comment "\n    It is known as the standard longneck bottle or industry standard bottle\n    (ISB). The ISB longnecks have a uniform capacity, height, weight and\n    diameter and can be reused on average 16 times. The long neck offers a long\n    cushion of air to absorb the pressure of carbonation to reduce the risk of\n    exploding. The longneck also provides a handle for drinking directly from\n    the bottle without transferring body heat to the beer from one's hand.\n    "@en ;
	rdfs:isDefinedBy <http://rdfs.co/bevon/> ;
	rdfs:subClassOf bevon:BeerBottle ;
	status:term_status "unstable"@en ;
	skos:altLabel "Industry Standard Bottle"@en , "North American Longneck"@en ;
	skos:definition "\n    A longneck is a type of beer bottle with a long neck.\n    "@en ;
	skos:prefLabel "Longneck"@en , "긴목 맥주병"@ko .

bevon:MaltWhisky dcterms:issued "2013-07-04+09:00"^^xsd:date ;
	dcterms:modified "2014-03-01+09:00"^^xsd:date ;
	a owl:Class ;
	rdfs:isDefinedBy <http://rdfs.co/bevon/> ;
	rdfs:seeAlso <http://en.wikipedia.org/wiki/Malt_whisky> ;
	rdfs:subClassOf bevon:Whisky , pto:Malt_whisky ;
	status:term_status "unstable"@en ;
	skos:altLabel "Malt Whiskey"@en ;
	skos:definition "\n    Malt whisky is whisky that is made from a fermented mash produced primarily\n    from a malted grain.\n    "@en ;
	skos:prefLabel "Malt Whisky"@en , "몰트 위스키"@ko .

bevon:MineralWater dcterms:issued "2013-07-04+09:00"^^xsd:date ;
	dcterms:modified "2014-03-01+09:00"^^xsd:date ;
	a owl:Class ;
	rdfs:comment "\n    Mineral water may be sparkling due to contained gases.\n    "@en ;
	rdfs:isDefinedBy <http://rdfs.co/bevon/> ;
	rdfs:seeAlso <http://en.wikipedia.org/wiki/Mineral_water> ;
	rdfs:subClassOf bevon:Water , pto:Mineral_water ;
	status:term_status "unstable"@en ;
	skos:definition "\n    Mineral water is water from a mineral spring containing various minerals\n    such as salts and sulfur compounds.\n    "@en ;
	skos:prefLabel "Mineral Water"@en , "광천수"@ko .

bevon:MixedDrink dcterms:issued "2013-07-04+09:00"^^xsd:date ;
	dcterms:modified "2014-03-01+09:00"^^xsd:date ;
	a owl:Class ;
	rdfs:comment "\n    Some mixed drinks are alcoholic beverages that contain liquor; others are\n    non-alcoholic.\n    "@en ;
	rdfs:isDefinedBy <http://rdfs.co/bevon/> ;
	rdfs:seeAlso <http://en.wikipedia.org/wiki/Mixed_drink> ;
	rdfs:subClassOf bevon:Beverage , pto:Mixed_drink ;
	status:term_status "testing"@en ;
	skos:definition "\n    A mixed drink is a beverage in which two or more ingredients are mixed.\n    "@en ;
	skos:prefLabel "Mixed Drink"@en , "혼합 음료"@ko .

bevon:Mocktail dcterms:issued "2013-07-04+09:00"^^xsd:date ;
	dcterms:modified "2014-03-01+09:00"^^xsd:date ;
	a owl:Class ;
	rdfs:isDefinedBy <http://rdfs.co/bevon/> ;
	rdfs:subClassOf bevon:MixedDrink , bevon:NonAlcoholicBeverage ;
	owl:disjointWith bevon:Cocktail ;
	status:term_status "unstable"@en ;
	skos:definition "\n    Mocktails are mock cocktails, or those that do not contain any alcohol.\n    "@en ;
	skos:prefLabel "Mocktail"@en , "목테일"@ko .

bevon:NonAlcoholicBeer dcterms:issued "2013-07-04+09:00"^^xsd:date ;
	dcterms:modified "2014-03-01+09:00"^^xsd:date ;
	a owl:Class ;
	rdfs:isDefinedBy <http://rdfs.co/bevon/> ;
	rdfs:seeAlso <http://en.wikipedia.org/wiki/Low-alcohol_beer> ;
	rdfs:subClassOf bevon:NonAlcoholicBeverage , pto:Low-alcohol_beer ;
	owl:disjointWith bevon:Beer ;
	status:term_status "unstable"@en ;
	skos:altLabel "Low-alcoholic Beer"@en ;
	skos:definition "\n    Non-alcohol beer (also called light beer, low-alcoholic beer, small beer,\n    small ale, or near-beer) is beer with low alcohol content or no alcohol,\n    which aim to reproduce the taste of beer without the inebriating effects of\n    standard alcoholic brews.\n    "@en ;
	skos:prefLabel "Non-alcoholic Beer"@en , "비알코올 맥주"@ko .

bevon:NonAlcoholicBeverage dcterms:issued "2013-07-04+09:00"^^xsd:date ;
	dcterms:modified "2014-03-01+09:00"^^xsd:date ;
	a owl:Class ;
	rdfs:isDefinedBy <http://rdfs.co/bevon/> ;
	rdfs:seeAlso <http://en.wikipedia.org/wiki/Non-alcoholic_beverage> ;
	rdfs:subClassOf bevon:Beverage , pto:Non-alcoholic_beverage ;
	owl:disjointWith bevon:AlcoholicBeverage ;
	status:term_status "testing"@en ;
	skos:definition "\n     A non-alcoholic beverage (also known as a virgin drink) is defined\n     in the U.S. as a beverage that contains less than 0.5% alcohol by volume.\n     "@en ;
	skos:prefLabel "Non-alcoholic Beverage"@en , "비알코올 음료"@ko .

bevon:PaleAle dcterms:issued "2013-07-04+09:00"^^xsd:date ;
	dcterms:modified "2014-03-01+09:00"^^xsd:date ;
	a owl:Class ;
	rdfs:comment "\n    It is one of the world's major beer styles.\n    "@en ;
	rdfs:isDefinedBy <http://rdfs.co/bevon/> ;
	rdfs:seeAlso <http://en.wikipedia.org/wiki/Pale_ale> ;
	rdfs:subClassOf bevon:Ale , pto:Pale_ale ;
	status:term_status "unstable"@en ;
	skos:definition "\n    Pale ale is a beer made by warm fermentation using predominantly pale malt.\n    "@en ;
	skos:prefLabel "Pale Ale"@en , "페일 에일"@ko .

bevon:PaleLager dcterms:issued "2013-07-04+09:00"^^xsd:date ;
	dcterms:modified "2014-03-01+09:00"^^xsd:date ;
	a owl:Class ;
	rdfs:isDefinedBy <http://rdfs.co/bevon/> ;
	rdfs:seeAlso <http://en.wikipedia.org/wiki/Pale_lager> ;
	rdfs:subClassOf bevon:Lager , pto:Pale_lager ;
	status:term_status "unstable"@en ;
	skos:definition "\n    Pale lager is a very pale to golden-colored beer with a well attenuated\n    body and a varying degree of noble hop bitterness.\n    "@en ;
	skos:prefLabel "Pale Lager"@en , "페일 라거"@ko .

bevon:Pilsner dcterms:issued "2013-07-04+09:00"^^xsd:date ;
	dcterms:modified "2014-03-01+09:00"^^xsd:date ;
	a owl:Class ;
	rdfs:comment "\n    It took its name from the city of Pilsen (Plzeň, Bohemia, Czech Republic,\n    where it was first produced in 1842).\n    "@en ;
	rdfs:isDefinedBy <http://rdfs.co/bevon/> ;
	rdfs:seeAlso <http://en.wikipedia.org/wiki/Pilsner> ;
	rdfs:subClassOf bevon:PaleLager , pto:Pilsner ;
	status:term_status "unstable"@en ;
	skos:altLabel "Pils"@en , "Pilsener"@en ;
	skos:definition "\n    Pilsner (also pilsener or simply pils) is a type of pale lager.\n    "@en ;
	skos:prefLabel "Pilsner"@en , "필스너"@ko .

bevon:Pisco dcterms:issued "2013-07-04+09:00"^^xsd:date ;
	dcterms:modified "2014-03-01+09:00"^^xsd:date ;
	a owl:Class ;
	rdfs:isDefinedBy <http://rdfs.co/bevon/> ;
	rdfs:seeAlso <http://en.wikipedia.org/wiki/Pisco> ;
	rdfs:subClassOf bevon:Brandy , pto:Pisco ;
	status:term_status "testing"@en ;
	skos:definition "\n    Pisco is a colorless or yellowish-to-amber colored grape brandy produced\n    in winemaking regions of Peru and Chile.\n    "@en ;
	skos:prefLabel "Pisco"@en , "피스코"@ko .

bevon:PlasticBottle dcterms:issued "2013-07-04+09:00"^^xsd:date ;
	dcterms:modified "2014-03-01+09:00"^^xsd:date ;
	a owl:Class ;
	rdfs:comment "\n    Plastic bottles are typically used to store liquids such as water, soft\n    drinks, motor oil, cooking oil, medicine, shampoo, milk, and ink.\n    "@en ;
	rdfs:isDefinedBy <http://rdfs.co/bevon/> ;
	rdfs:seeAlso <http://en.wikipedia.org/wiki/Plastic_bottle> ;
	rdfs:subClassOf bevon:Container ;
	status:term_status "unstable"@en ;
	skos:definition "\n    A plastic bottle is a bottle constructed of plastic.\n    "@en ;
	skos:prefLabel "Plastic Bottle"@en , "플라스틱 병"@ko .

bevon:Porter dcterms:issued "2013-07-04+09:00"^^xsd:date ;
	dcterms:modified "2014-03-01+09:00"^^xsd:date ;
	a owl:Class ;
	rdfs:comment "\n    The name came about as a result of its popularity with street and river\n    porters.\n    "@en ;
	rdfs:isDefinedBy <http://rdfs.co/bevon/> ;
	rdfs:seeAlso <http://en.wikipedia.org/wiki/English_porter> ;
	rdfs:subClassOf bevon:Ale , pto:English_porter ;
	status:term_status "unstable"@en ;
	skos:altLabel "English Porter"@en ;
	skos:definition "\n    Porter is a dark style of beer originating in London in the 18th century,\n    descended from brown beer, a well hopped beer made from brown malt.\n    "@en ;
	skos:prefLabel "Porter"@en , "포터"@ko .

bevon:Rum dcterms:issued "2013-07-04+09:00"^^xsd:date ;
	dcterms:modified "2014-03-01+09:00"^^xsd:date ;
	a owl:Class ;
	rdfs:comment "\n    The distillate, a clear liquid, is then usually aged in\n    oak barrels.\n    "@en ;
	rdfs:isDefinedBy <http://rdfs.co/bevon/> ;
	rdfs:seeAlso <http://en.wikipedia.org/wiki/Rum> ;
	rdfs:subClassOf bevon:DistilledBeverage , pto:Rum ;
	status:term_status "testing"@en ;
	skos:definition "\n    Rum is a distilled alcoholic beverage made from sugarcane byproducts, such\n    as molasses, or directly from sugarcane juice, by a process of fermentation\n    and distillation.\n    "@en ;
	skos:prefLabel "Ron"@es , "Rum"@en , "럼"@ko .

bevon:Sake dcterms:issued "2013-07-04+09:00"^^xsd:date ;
	dcterms:modified "2014-03-01+09:00"^^xsd:date ;
	a owl:Class ;
	rdfs:isDefinedBy <http://rdfs.co/bevon/> ;
	rdfs:seeAlso <http://en.wikipedia.org/wiki/Sake> ;
	rdfs:subClassOf bevon:FermentedBeverages , pto:Sake ;
	status:term_status "testing"@en ;
	skos:altLabel "Rice Wine"@en ;
	skos:definition "\n    Sake or saké is an alcoholic beverage of Japanese origin that is made from\n    fermented rice.\n    "@en ;
	skos:prefLabel "Sake"@en , "Saké"@fr , "사케"@ko .

bevon:ScotchWhisky dcterms:issued "2013-07-04+09:00"^^xsd:date ;
	dcterms:modified "2014-03-01+09:00"^^xsd:date ;
	a owl:Class ;
	rdfs:comment "\n    All Scotch whisky was originally made from malt barley. Commercial\n    distilleries began introducing whisky made from wheat and rye in the late\n    eighteenth century.\n    "@en ;
	rdfs:isDefinedBy <http://rdfs.co/bevon/> ;
	rdfs:seeAlso <http://en.wikipedia.org/wiki/Scotch_whisky> ;
	rdfs:subClassOf bevon:Whisky , pto:Scotch_whisky ;
	status:term_status "unstable"@en ;
	skos:altLabel "Scotch Whiskey"@en ;
	skos:definition "\n    Scotch whisky (often referred to simply as \"Scotch\") is malt whisky or grain\n    whisky made in Scotland.\n    "@en ;
	skos:prefLabel "Scotch Whisky"@en , "스카치 위스키"@ko .

bevon:Shandy dcterms:issued "2013-07-04+09:00"^^xsd:date ;
	dcterms:modified "2014-03-01+09:00"^^xsd:date ;
	a owl:Class ;
	rdfs:comment "\n    The proportions of the two ingredients are adjusted to taste, usually\n    half-and-half.\n    "@en ;
	rdfs:isDefinedBy <http://rdfs.co/bevon/> ;
	rdfs:seeAlso <http://en.wikipedia.org/wiki/Shandy> ;
	rdfs:subClassOf bevon:Cocktail , pto:Shandy ;
	status:term_status "unstable"@en ;
	skos:definition "\n    A shandy, or shandygaff, is beer mixed with a soft drink, carbonated\n    lemonade, ginger beer, ginger ale, or apple juice.\n    "@en ;
	skos:prefLabel "Shandy"@en , "섄디"@ko .

bevon:SingleMaltScotch dcterms:issued "2013-07-04+09:00"^^xsd:date ;
	dcterms:modified "2014-03-01+09:00"^^xsd:date ;
	a owl:Class ;
	rdfs:comment "\n    As with any Scotch whisky, a single malt Scotch must be distilled in\n    Scotland and matured in oak casks in Scotland for at least three years\n    (most single malts are matured longer).\n    "@en ;
	rdfs:isDefinedBy <http://rdfs.co/bevon/> ;
	rdfs:seeAlso <http://en.wikipedia.org/wiki/Single_malt_Scotch> ;
	rdfs:subClassOf bevon:ScotchWhisky , bevon:SingleMaltWhisky , pto:Single_malt_Scotch ;
	status:term_status "unstable"@en ;
	skos:definition "\n    Single Malt Scotch is single malt whisky made in Scotland using a pot still\n    distillation process at a single distillery, with malted barley as the only\n    grain ingredient.\n    "@en ;
	skos:prefLabel "Single Malt Scotch"@en , "싱글 몰트 스카치"@ko .

bevon:SingleMaltWhisky dcterms:issued "2013-07-04+09:00"^^xsd:date ;
	dcterms:modified "2014-03-01+09:00"^^xsd:date ;
	a owl:Class ;
	rdfs:isDefinedBy <http://rdfs.co/bevon/> ;
	rdfs:seeAlso <http://en.wikipedia.org/wiki/Single_malt_whisky> ;
	rdfs:subClassOf bevon:MaltWhisky , pto:Single_malt_whisky ;
	status:term_status "unstable"@en ;
	skos:altLabel "Single Malt Whiskey"@en ;
	skos:definition "\n    Single malt whisky is a whisky made at one particular distillery from a\n    mash that uses only malted grain, ordinarily barley.\n    "@en ;
	skos:prefLabel "Single Malt Whisky"@en , "싱글 몰트 위스키"@ko .

bevon:Soju dcterms:issued "2013-07-04+09:00"^^xsd:date ;
	dcterms:modified "2014-03-01+09:00"^^xsd:date ;
	a owl:Class ;
	rdfs:comment "\n    Its taste is comparable to vodka, though often slightly sweeter due to\n    sugars added in the manufacturing process.\n    "@en ;
	rdfs:isDefinedBy <http://rdfs.co/bevon/> ;
	rdfs:seeAlso <http://en.wikipedia.org/wiki/Soju> ;
	rdfs:subClassOf bevon:DistilledBeverage , pto:Soju ;
	status:term_status "testing"@en ;
	skos:definition "\n    Soju is a distilled beverage native to Korea.\n    "@en ;
	skos:prefLabel "Soju"@en , "소주"@ko .

bevon:SpeysideSingleMalt dcterms:issued "2013-07-04+09:00"^^xsd:date ;
	dcterms:modified "2014-03-01+09:00"^^xsd:date ;
	a owl:Class ;
	rdfs:isDefinedBy <http://rdfs.co/bevon/> ;
	rdfs:seeAlso <http://en.wikipedia.org/wiki/Speyside_single_malts> ;
	rdfs:subClassOf bevon:SingleMaltScotch , pto:Speyside_single_malts ;
	status:term_status "unstable"@en ;
	skos:definition "\n    Speyside single malts are single malt Scotch whiskies, distilled in\n    Strathspey, the area around the River Spey in Moray and Badenoch and\n    Strathspey, in northeastern Scotland.\n    "@en ;
	skos:prefLabel "Speyside Single Malt"@en , "스페이사이드 싱글 몰트"@ko .

bevon:Stout dcterms:issued "2013-07-04+09:00"^^xsd:date ;
	dcterms:modified "2014-03-01+09:00"^^xsd:date ;
	a owl:Class ;
	rdfs:comment "\n    Stouts were traditionally the generic term for the strongest or stoutest\n    porters, typically 7% or 8%, produced by a brewery.\n    "@en ;
	rdfs:isDefinedBy <http://rdfs.co/bevon/> ;
	rdfs:seeAlso <http://en.wikipedia.org/wiki/Stout> ;
	rdfs:subClassOf bevon:Porter , pto:Stout ;
	status:term_status "unstable"@en ;
	skos:altLabel "Strong Porter"@en ;
	skos:definition "\n    Stout is a dark beer made using roasted malt or roasted barley, hops, water\n    and yeast.\n    "@en ;
	skos:prefLabel "Stout"@en , "스타우트"@ko .

bevon:Tequila dcterms:issued "2013-07-04+09:00"^^xsd:date ;
	dcterms:modified "2014-03-01+09:00"^^xsd:date ;
	a owl:Class ;
	rdfs:isDefinedBy <http://rdfs.co/bevon/> ;
	rdfs:seeAlso <http://en.wikipedia.org/wiki/Tequila> ;
	rdfs:subClassOf bevon:DistilledBeverage , pto:Tequila ;
	status:term_status "testing"@en ;
	skos:definition "\n    Tequila is a distilled beverage made from the blue agave plant, primarily\n    in the area surrounding the city of Tequila, 65 kilometres (40 mi)\n    northwest of Guadalajara, and in the highlands (Los Altos) of the western\n    Mexican state of Jalisco.\n    "@en ;
	skos:prefLabel "Tequila"@en , "테킬라"@ko .

bevon:TequilaBlanco dcterms:issued "2013-07-04+09:00"^^xsd:date ;
	dcterms:modified "2014-03-01+09:00"^^xsd:date ;
	a owl:Class ;
	rdfs:isDefinedBy <http://rdfs.co/bevon/> ;
	rdfs:subClassOf bevon:Tequila ;
	status:term_status "unstable"@en ;
	skos:altLabel "Tequila Plata"@en ;
	skos:definition "\n    Tequila Blanco (\"white\") or Plata (\"silver\") is a white spirit, un-aged and\n    bottled or stored immediately after distillation, or aged less than two\n    months in stainless steel or neutral oak barrels.\n    "@en ;
	skos:prefLabel "Tequila Blanco"@en , "테킬라 블랑코"@ko .

bevon:Vodka dcterms:issued "2013-07-04+09:00"^^xsd:date ;
	dcterms:modified "2014-03-01+09:00"^^xsd:date ;
	a owl:Class ;
	rdfs:comment "\n    Vodka is made by the distillation of fermented substances such as grains,\n    potatoes, or sometimes fruits or sugar.\n    "@en ;
	rdfs:isDefinedBy <http://rdfs.co/bevon/> ;
	rdfs:seeAlso <http://en.wikipedia.org/wiki/Vodka> ;
	rdfs:subClassOf bevon:DistilledBeverage , pto:Vodka ;
	status:term_status "testing"@en ;
	skos:definition "\n    Vodka is a distilled beverage composed primarily of water and ethanol,\n    sometimes with traces of impurities and flavorings.\n    "@en ;
	skos:prefLabel "Vodka"@en , "Wódka"@pl , "водка"@ru , "보드카"@ko .

bevon:Water dcterms:issued "2013-07-04+09:00"^^xsd:date ;
	dcterms:modified "2014-03-01+09:00"^^xsd:date ;
	a owl:Class ;
	rdfs:isDefinedBy <http://rdfs.co/bevon/> ;
	rdfs:seeAlso <http://en.wikipedia.org/wiki/Water> ;
	rdfs:subClassOf bevon:NonAlcoholicBeverage , pto:Water ;
	status:term_status "testing"@en ;
	skos:definition "\n    In the Beverage Ontology, Water means a drinking water.\n    "@en ;
	skos:prefLabel "Water"@en , "물"@ko .

bevon:Whisky dcterms:issued "2013-07-04+09:00"^^xsd:date ;
	dcterms:modified "2014-03-01+09:00"^^xsd:date ;
	a owl:Class ;
	rdfs:comment "\n    Different grains are used for different varieties, including barley, malted\n    barley, rye, malted rye, wheat, and corn. Whisky is typically aged in\n    wooden casks, made generally of charred white oak.\n    "@en ;
	rdfs:isDefinedBy <http://rdfs.co/bevon/> ;
	rdfs:seeAlso <http://en.wikipedia.org/wiki/Whisky> ;
	rdfs:subClassOf bevon:DistilledBeverage , pto:Whisky ;
	owl:sameAs whisky:Whiskey ;
	status:term_status "testing"@en ;
	skos:altLabel "Whiskey"@en ;
	skos:definition "\n    Whisky or whiskey is a type of distilled alcoholic beverage made from\n    fermented grain mash.\n    "@en ;
	skos:prefLabel "Whisky"@en , "위스키"@en .

bevon:Wine dcterms:issued "2013-07-04+09:00"^^xsd:date ;
	dcterms:modified "2014-03-01+09:00"^^xsd:date ;
	a owl:Class ;
	rdfs:isDefinedBy <http://rdfs.co/bevon/> ;
	rdfs:seeAlso <http://en.wikipedia.org/wiki/Wine> ;
	rdfs:subClassOf bevon:FermentedBeverages , pto:Wine ;
	owl:sameAs wine:Wine ;
	status:term_status "testing"@en ;
	skos:definition "\n    Wine is an alcoholic beverage made from fermented grapes or other fruits.\n    "@en ;
	skos:prefLabel "Vin"@fr , "Wine"@en , "와인"@ko .

bevon:abv dcterms:issued "2013-07-04+09:00"^^xsd:date ;
	dcterms:modified "2014-03-01+09:00"^^xsd:date ;
	a owl:DatatypeProperty ;
	rdfs:domain bevon:Beverage ;
	rdfs:isDefinedBy <http://rdfs.co/bevon/> ;
	rdfs:range xsd:decimal ;
	rdfs:seeAlso <http://en.wikipedia.org/wiki/Alcohol_by_volume> ;
	status:term_status "testing"@en ;
	skos:altLabel "alcohol by volume"@en ;
	skos:definition "\n    ABV (Alcohol by Volume) is a standard measure of how much alcohol is\n    contained in the drink.\n    "@en ;
	skos:prefLabel "ABV"@en , "알코올 도수"@ko .

bevon:aging dcterms:issued "2013-07-04+09:00"^^xsd:date ;
	dcterms:modified "2014-03-01+09:00"^^xsd:date ;
	a owl:ObjectProperty ;
	rdfs:domain bevon:AlcoholicBeverage ;
	rdfs:isDefinedBy <http://rdfs.co/bevon/> ;
	rdfs:range bevon:Aging ;
	status:term_status "unstable"@en ;
	skos:definition "\n    This property specifies how the beverage has been aged.\n    "@en ;
	skos:prefLabel "aging"@en , "숙성"@ko .

beverage:Budweiser bevon:abv "5"^^xsd:integer ;
	bevon:container container:330mlLongneck , container:355mlBeverageCan , container:500mlBeverageCan ;
	bevon:description "\n    Budweiser is a pale lager produced by Anheuser–Busch InBev. Introduced in\n    1876 by Adolphus Busch it has grown to become one of the highest selling\n    beers in the United States, and is available in over 80 markets worldwide.\n    "@en ;
	bevon:fermentation_base <http://dbpedia.org/resource/Barley> ;
	bevon:ibu "12"^^xsd:nonNegativeInteger ;
	bevon:launch "1876"^^xsd:gYear ;
	bevon:manufacturer <http://dbpedia.org/resource/Anheuser–Busch_InBev> ;
	bevon:name "Budweiser"@en , "버드와이저"@ko ;
	bevon:origin <http://dbpedia.org/resource/United_States> ;
	bevon:srm "3"^^xsd:nonNegativeInteger ;
	a gr:ProductOrServiceModel , bevon:PaleLager , owl:NamedIndividual ;
	rdfs:seeAlso <https://en.wikipedia.org/wiki/Budweiser_(Anheuser-Busch)> .

beverage:Chamisul bevon:abv "19"^^xsd:integer .

_:node18ib1jcplx6 dcterms:title "Clear"@en ;
	a dbpedia:Colour ;
	owl:sameAs <http://dbpedia.org/resource/Clear_(color)> .

beverage:Chamisul bevon:color _:node18ib1jcplx6 ;
	bevon:container container:1_8lPlasticBottle , container:200mlPlasticBottle , container:360mlGlassBottle , container:640mlPlasticBottle ;
	bevon:description "\n    Chamisul is the diluted soju produced by HITEJiro.\n    "@en ;
	bevon:launch "1998"^^xsd:gYear ;
	bevon:manufacturer <http://dbpedia.org/resource/Jinro> ;
	bevon:name "Chamisul"@en , "참이슬"@ko ;
	bevon:origin <http://dbpedia.org/resource/South_Korea> ;
	a gr:ProductOrServiceModel , bevon:DilutedSoju , owl:NamedIndividual ;
	rdfs:seeAlso <http://ko.wikipedia.org/wiki/참이슬> .

beverage:Chum-Churum bevon:abv "19.5"^^xsd:decimal .

_:node18ib1jcplx7 dcterms:title "Clear"@en ;
	a dbpedia:Colour ;
	owl:sameAs <http://dbpedia.org/resource/Clear_(color)> .

beverage:Chum-Churum bevon:color _:node18ib1jcplx7 ;
	bevon:container container:1_8lPlasticBottle , container:200mlPlasticBottle , container:360mlGlassBottle , container:360mlPlasticBottle , container:640mlPlasticBottle ;
	bevon:description "\n    Chum-Churum is the diluted soju produced by Lotte Liquor.\n    "@en ;
	bevon:launch "2006"^^xsd:gYear .

_:node18ib1jcplx8 a foaf:Organization ;
	rdfs:seeAlso <http://ko.wikipedia.org/wiki/롯데칠성음료> ;
	foaf:homepage <http://www.lotteliquor.com> ;
	foaf:name "Lotte Liquor"@en , "롯데주류"@ko .

beverage:Chum-Churum bevon:manufacturer _:node18ib1jcplx8 ;
	bevon:name "Chum-Churum"@en , "처음처럼"@ko ;
	bevon:origin <http://dbpedia.org/resource/South_Korea> ;
	a gr:ProductOrServiceModel , bevon:DilutedSoju , owl:NamedIndividual ;
	rdfs:seeAlso <http://ko.wikipedia.org/wiki/처음처럼_(주류)> ;
	owl:sameAs <http://dbpedia.org/resource/Chum-Churum> .

beverage:DonJulioBlanco bevon:abv "40"^^xsd:integer .

_:node18ib1jcplx9 dcterms:title "Clear"@en ;
	a dbpedia:Colour ;
	owl:sameAs <http://dbpedia.org/resource/Clear_(color)> .

beverage:DonJulioBlanco bevon:color _:node18ib1jcplx9 ;
	bevon:container container:750mlGlassBottle ;
	bevon:description "\n    Tequila Don Julio Blanco is the base from which all of our other variants\n    are derived. Commonly referred to as \"silver\" tequila, its crisp agave\n    flavor and hints of citrus make it an essential component to a variety of\n    innovative drinks including margaritas. It can also be enjoyed neat or on\n    the rocks.\n    "@en ;
	bevon:fermentation_base <http://dbpedia.org/resource/Agave> ;
	bevon:launch "1942"^^xsd:gYear ;
	bevon:manufacturer <http://dbpedia.org/resource/Diageo> ;
	bevon:name "Don Julio Blanco"@en , "돈 훌리오 블랑코"@ko ;
	bevon:origin <http://dbpedia.org/resource/Mexico> ;
	bevon:proof "80"^^xsd:integer ;
	a gr:ProductOrServiceModel , bevon:TequilaBlanco , owl:NamedIndividual ;
	rdfs:seeAlso <http://www.donjulio.com/blanco.aspx> .

beverage:Glenfiddich12YearOld bevon:abv "40"^^xsd:integer .

_:node18ib1jcplx11 a time:DurationDescription ;
	time:years "12"^^xsd:integer .

_:node18ib1jcplx10 bevon:duration _:node18ib1jcplx11 ;
	bevon:material <http://dbpedia.org/resource/Oak> ;
	bevon:previous_content <http://dbpedia.org/resource/Bourbon_whiskey> , <http://dbpedia.org/resource/Sherry> ;
	a bevon:Aging .

beverage:Glenfiddich12YearOld bevon:aging _:node18ib1jcplx10 .

_:node18ib1jcplx12 dcterms:title "Golden"@en ;
	a dbpedia:Colour ;
	owl:sameAs <http://dbpedia.org/resource/Gold_(color)> , <http://purl.org/colors/rgb/FFD700> .

beverage:Glenfiddich12YearOld bevon:color _:node18ib1jcplx12 ;
	bevon:container container:700mlGlassBottle ;
	bevon:description "\n    Carefully matured in the finest American bourbon and Spanish sherry oak\n    casks for at least 12 years. Married and mellowed in oak marrying tuns for\n    complete harmony of aroma and flavor.\n\n    A single malt Scotch whisky with distinctive fresh pear, creamy with subtle\n    oak flavors and a long smooth and mellow finish.\n    "@en .

_:node18ib1jcplx13 whisky:owner <http://dbpedia.org/resource/William_Grant_%26_Sons> ;
	whisky:region <http://dbpedia.org/resource/Strathspey,_Scotland> .

_:node18ib1jcplx14 dcterms:title "Robbie Dhu Springs"@en , "로비 듀 수원지"@ko ;
	a whisky:WaterSource .

_:node18ib1jcplx13 whisky:waterSource _:node18ib1jcplx14 ;
	a bevon:Distillery ;
	owl:sameAs <http://dbpedia.org/resource/Glenfiddich_distillery> .

beverage:Glenfiddich12YearOld bevon:distillery _:node18ib1jcplx13 ;
	bevon:fermentation_base <http://dbpedia.org/resource/Barley> ;
	bevon:launch "1887"^^xsd:gYear ;
	bevon:manufacturer <http://dbpedia.org/resource/William_Grant_%26_Sons> ;
	bevon:name "Glenfiddich 12 Year Old"@en , "글렌피딕 12년"@ko ;
	bevon:origin <http://dbpedia.org/resource/Strathspey,_Scotland> ;
	a gr:ProductOrServiceModel , bevon:SpeysideSingleMalt , owl:NamedIndividual .

beverage:Guinness bevon:abv "4.2"^^xsd:decimal ;
	bevon:container container:15lBeerKeg , container:30lBeerKeg , container:330mlBeverageCan , container:330mlLongneck ;
	bevon:description "\n    Guinness is a popular Irish dry stout that originated in the brewery of\n    Arthur Guinness (1725–1803) at St. James's Gate, Dublin. Guinness is one\n    of the most successful beer brands worldwide.\n    "@en ;
	bevon:fermentation_base <http://dbpedia.org/resource/Barley> ;
	bevon:ibu "37"^^xsd:nonNegativeInteger ;
	bevon:launch "1759"^^xsd:gYear ;
	bevon:manufacturer <http://dbpedia.org/resource/Diageo> ;
	bevon:name "Guinness Draught"@en , "기네스 드래프트"@ko ;
	bevon:origin <http://dbpedia.org/resource/Dublin> ;
	bevon:srm "32"^^xsd:nonNegativeInteger ;
	a gr:ProductOrServiceModel , bevon:DryStout , owl:NamedIndividual ;
	rdfs:seeAlso <http://en.wikipedia.org/wiki/Guinness> ;
	owl:sameAs <http://dbpedia.org/resource/Guinness> .

beverage:Kilkenny bevon:abv "4.3"^^xsd:decimal ;
	bevon:container container:30lBeerKeg , container:440mlBeverageCan ;
	bevon:description "\n    Kilkenny is a nitrogenated Irish cream ale from the makers of Guinness,\n    which originated in Kilkenny, Ireland. The brand is managed and produced\n    by Diageo. It is available in draught and cans. It is brewed in Ireland\n    and its heritage dates back to the 14th century.\n    "@en ;
	bevon:fermentation_base <http://dbpedia.org/resource/Barley> ;
	bevon:ibu "23"^^xsd:nonNegativeInteger ;
	bevon:launch "1710"^^xsd:gYear ;
	bevon:manufacturer <http://dbpedia.org/resource/Diageo> ;
	bevon:name "Kilkenny Irish Cream Ale"@en , "킬케니 아이리쉬 크림 에일"@ko ;
	bevon:origin <http://dbpedia.org/resource/Kilkenny> ;
	bevon:similar beverage:Smithwicks ;
	bevon:srm "14"^^xsd:nonNegativeInteger ;
	a gr:ProductOrServiceModel , bevon:IrishRedAle , owl:NamedIndividual ;
	rdfs:seeAlso <http://en.wikipedia.org/wiki/Kilkenny_(beer)> ;
	owl:sameAs <http://dbpedia.org/resource/Kilkenny_(beer)> .

beverage:KozelDark bevon:abv "3.8"^^xsd:decimal ;
	bevon:container container:500mlLongneck ;
	bevon:description "\n    Velkopopovický Kozel Dark beer is brewed to the original recipe using a\n    special mix of dark malts, clean water from our own well close to the\n    brewery, and a selection of the best hops. The caramelized malt gives this\n    beer a unique ruby color and sweet flavor, thanks to which it is\n    appreciated and respected all over the world.\n    "@en ;
	bevon:fermentation_base <http://dbpedia.org/resource/Barley> ;
	bevon:launch "1874"^^xsd:gYear ;
	bevon:manufacturer <http://dbpedia.org/resource/SABMiller> ;
	bevon:name "Velkopopovický Kozel Dark"@en , "Velkopopovický Kozel Černý"@cs , "코젤 다크"@ko ;
	bevon:origin <http://dbpedia.org/resource/Velké_Popovice> ;
	a gr:ProductOrServiceModel , bevon:Dunkel , owl:NamedIndividual .

beverage:Smithwicks bevon:abv "3.8"^^xsd:decimal .

_:node18ib1jcplx15 dcterms:title "Ruby Red"@en ;
	a dbpedia:Colour ;
	owl:sameAs <http://dbpedia.org/resource/Ruby_(color)__Ruby_Red__1> , <http://purl.org/colors/rgb/9B111E> .

beverage:Smithwicks bevon:color _:node18ib1jcplx15 ;
	bevon:container container:30lBeerKeg , container:330mlLongneck , container:440mlBeverageCan ;
	bevon:description "\n    Smithwick's is an Irish red ale style beer from Kilkenny, Ireland. It is a\n    clear beer with a rich ruby color and creamy head.\n    "@en ;
	bevon:fermentation_base <http://dbpedia.org/resource/Barley> ;
	bevon:ibu "20"^^xsd:nonNegativeInteger ;
	bevon:launch "1710"^^xsd:gYear ;
	bevon:manufacturer <http://dbpedia.org/resource/Diageo> ;
	bevon:name "Smithwick's Superior Irish Ale"@en , "스미딕스 슈페리어 아이리쉬 에일"@ko ;
	bevon:origin <http://dbpedia.org/resource/Kilkenny> ;
	bevon:similar beverage:Kilkenny ;
	bevon:srm "14"^^xsd:nonNegativeInteger ;
	a gr:ProductOrServiceModel , bevon:IrishRedAle , owl:NamedIndividual ;
	rdfs:seeAlso <http://en.wikipedia.org/wiki/Smithwick%27s> ;
	owl:sameAs <http://dbpedia.org/resource/Smithwick%27s> .

beverage:Tsingtao bevon:abv "4.7"^^xsd:decimal ;
	bevon:brewery <http://dbpedia.org/resource/Tsingtao_Brewery> ;
	bevon:container container:330mlLongneck , container:355mlBeverageCan , container:500mlBeverageCan , container:640mlLongneck ;
	bevon:description "\n    Tsingtao Lager, a well-hopped standard pilsner of 4.7% alcohol, is the\n    flagship brew, accounting for most of the brewery's production.\n    "@en ;
	bevon:fermentation_base <http://dbpedia.org/resource/Barley> ;
	bevon:ibu "20"^^xsd:nonNegativeInteger ;
	bevon:launch "1904"^^xsd:gYear ;
	bevon:manufacturer <http://dbpedia.org/resource/Tsingtao_Brewery> ;
	bevon:name "Tsingtao Lager"@en , "칭타오 라거"@ko ;
	bevon:origin <http://dbpedia.org/resource/Qingdao> ;
	bevon:srm "4"^^xsd:nonNegativeInteger ;
	a gr:ProductOrServiceModel , bevon:Pilsner , owl:NamedIndividual .

beverage:WhiskyAndSoda bevon:description "\n    Whisky & Soda is a kind of mixed drinks that are composed of whisky and\n    carbonated water.\n    "@en .

_:node18ib1jcplx17 dcterms:title "Whisky"@en ;
	a bevon:Whisky ;
	owl:sameAs <http://dbpedia.org/resource/Whisky> .

_:node18ib1jcplx16 bevon:food _:node18ib1jcplx17 .

_:node18ib1jcplx18 gr:hasUnitOfMeasurement "OZA" ;
	gr:hasValue "2"^^xsd:int ;
	a gr:QuantitativeValueInteger .

_:node18ib1jcplx16 bevon:quantity _:node18ib1jcplx18 ;
	a food:Ingredient .

beverage:WhiskyAndSoda bevon:ingredient _:node18ib1jcplx16 .

_:node18ib1jcplx20 dcterms:title "Carbonated Water"@en ;
	a bevon:CarbonatedWater ;
	owl:sameAs <http://dbpedia.org/resource/Carbonated_water> .

_:node18ib1jcplx19 bevon:food _:node18ib1jcplx20 ;
	a food:Ingredient .

beverage:WhiskyAndSoda bevon:ingredient _:node18ib1jcplx19 ;
	bevon:name "Whisky & Soda"@en , "위스키 소다"@ko ;
	a gr:ProductOrServiceModel , bevon:Highball , owl:NamedIndividual .

bevon:brewery dcterms:issued "2013-07-04+09:00"^^xsd:date ;
	dcterms:modified "2014-03-01+09:00"^^xsd:date ;
	a owl:ObjectProperty ;
	rdfs:domain bevon:Beer ;
	rdfs:isDefinedBy <http://rdfs.co/bevon/> ;
	rdfs:range bevon:Brewery ;
	rdfs:seeAlso <http://en.wikipedia.org/wiki/Brewery> ;
	status:term_status "unstable"@en ;
	skos:definition "\n    This property relates a beer to its brewery.\n    "@en ;
	skos:prefLabel "Brewery"@en , "양조장"@ko .

bevon:color dcterms:issued "2013-07-04+09:00"^^xsd:date ;
	dcterms:modified "2014-03-01+09:00"^^xsd:date ;
	a owl:DatatypeProperty ;
	rdfs:domain bevon:Beverage ;
	rdfs:isDefinedBy <http://rdfs.co/bevon/> ;
	rdfs:range dbpedia:Colour ;
	status:term_status "unstable"@en ;
	skos:definition "\n    This property specifies the color of the beverage.\n    "@en ;
	skos:prefLabel "color"@en , "색상"@ko .

bevon:container dcterms:issued "2013-07-04+09:00"^^xsd:date ;
	dcterms:modified "2014-03-01+09:00"^^xsd:date ;
	a owl:ObjectProperty ;
	rdfs:domain bevon:Beverage ;
	rdfs:isDefinedBy <http://rdfs.co/bevon/> ;
	rdfs:range bevon:Container ;
	status:term_status "unstable"@en ;
	skos:definition "\n    This property can be used to indicate that the beverage is available in a\n    type of container.\n    "@en ;
	skos:prefLabel "container"@en , "용기"@ko .

_:node18ib1jcplx21 gr:hasUnitOfMeasurement "LTR" ;
	gr:hasValue "15"^^xsd:int ;
	a gr:QuantitativeValueInteger .

container:15lBeerKeg bevon:volume _:node18ib1jcplx21 ;
	a bevon:BeerKeg , owl:NamedIndividual ;
	skos:prefLabel "15l Beer Keg"@en , "15l 맥주 케그"@ko .

_:node18ib1jcplx22 gr:hasUnitOfMeasurement "LTR" ;
	gr:hasValue "1.8"^^xsd:float ;
	a gr:QuantitativeValueFloat .

container:1_8lPlasticBottle bevon:volume _:node18ib1jcplx22 ;
	a bevon:PlasticBottle , owl:NamedIndividual ;
	skos:prefLabel "1.8l Plastic Bottle"@en , "1.8l 플라스틱 병"@ko .

_:node18ib1jcplx23 gr:hasUnitOfMeasurement "MLT" ;
	gr:hasValue "200"^^xsd:int ;
	a gr:QuantitativeValueInteger .

container:200mlPlasticBottle bevon:volume _:node18ib1jcplx23 ;
	a bevon:PlasticBottle , owl:NamedIndividual ;
	skos:prefLabel "200ml Plastic Bottle"@en , "200ml 플라스틱 병"@ko .

_:node18ib1jcplx24 gr:hasUnitOfMeasurement "LTR" ;
	gr:hasValue "25"^^xsd:int ;
	a gr:QuantitativeValueInteger .

container:25lBeerKeg bevon:volume _:node18ib1jcplx24 ;
	a bevon:BeerKeg , owl:NamedIndividual ;
	skos:prefLabel "25l Beer Keg"@en , "25l 맥주 케그"@ko .

_:node18ib1jcplx25 gr:hasUnitOfMeasurement "LTR" ;
	gr:hasValue "30"^^xsd:int ;
	a gr:QuantitativeValueInteger .

container:30lBeerKeg bevon:volume _:node18ib1jcplx25 ;
	a bevon:BeerKeg , owl:NamedIndividual ;
	skos:prefLabel "30l Beer Keg"@en , "30l 맥주 케그"@ko .

_:node18ib1jcplx26 gr:hasUnitOfMeasurement "MLT" ;
	gr:hasValue "330"^^xsd:int ;
	a gr:QuantitativeValueInteger .

container:330mlBeverageCan bevon:volume _:node18ib1jcplx26 ;
	a bevon:BeverageCan , owl:NamedIndividual ;
	skos:prefLabel "330ml Beverage Can"@en , "330ml 음료 캔"@ko .

_:node18ib1jcplx27 gr:hasUnitOfMeasurement "MLT" ;
	gr:hasValue "330"^^xsd:int ;
	a gr:QuantitativeValueInteger .

container:330mlLongneck bevon:volume _:node18ib1jcplx27 ;
	a bevon:Longneck , owl:NamedIndividual ;
	skos:prefLabel "330ml Longneck Bottle"@en , "330ml 긴목 맥주병"@ko .

_:node18ib1jcplx28 gr:hasUnitOfMeasurement "MLT" ;
	gr:hasValue "355"^^xsd:int ;
	a gr:QuantitativeValueInteger .

container:355mlBeverageCan bevon:volume _:node18ib1jcplx28 ;
	a bevon:BeverageCan , owl:NamedIndividual ;
	skos:prefLabel "355ml Beverage Can"@en , "355ml 음료 캔"@ko .

_:node18ib1jcplx29 gr:hasUnitOfMeasurement "MLT" ;
	gr:hasValue "360"^^xsd:int ;
	a gr:QuantitativeValueInteger .

container:360mlGlassBottle bevon:volume _:node18ib1jcplx29 ;
	a bevon:GlassBottle , owl:NamedIndividual ;
	skos:prefLabel "360ml Glass Bottle"@en , "360ml 유리병"@ko .

_:node18ib1jcplx30 gr:hasUnitOfMeasurement "MLT" ;
	gr:hasValue "360"^^xsd:int ;
	a gr:QuantitativeValueInteger .

container:360mlPlasticBottle bevon:volume _:node18ib1jcplx30 ;
	a bevon:PlasticBottle , owl:NamedIndividual ;
	skos:prefLabel "360ml Plastic Bottle"@en , "360ml 플라스틱 병"@ko .

_:node18ib1jcplx31 gr:hasUnitOfMeasurement "MLT" ;
	gr:hasValue "440"^^xsd:int ;
	a gr:QuantitativeValueInteger .

container:440mlBeverageCan bevon:volume _:node18ib1jcplx31 ;
	a bevon:BeverageCan , owl:NamedIndividual ;
	skos:prefLabel "440ml Beverage Can"@en , "440ml 음료 캔"@ko .

_:node18ib1jcplx32 gr:hasUnitOfMeasurement "MLT" ;
	gr:hasValue "500"^^xsd:int ;
	a gr:QuantitativeValueInteger .

container:500mlBeverageCan bevon:volume _:node18ib1jcplx32 ;
	a bevon:BeverageCan , owl:NamedIndividual ;
	skos:prefLabel "500ml Beverage Can"@en , "500ml 음료 캔"@ko .

_:node18ib1jcplx33 gr:hasUnitOfMeasurement "MLT" ;
	gr:hasValue "500"^^xsd:int ;
	a gr:QuantitativeValueInteger .

container:500mlLongneck bevon:volume _:node18ib1jcplx33 ;
	a bevon:Longneck , owl:NamedIndividual ;
	skos:prefLabel "500ml Longneck Bottle"@en , "500ml 긴목 맥주병"@ko .

_:node18ib1jcplx34 gr:hasUnitOfMeasurement "LTR" ;
	gr:hasValue "50"^^xsd:int ;
	a gr:QuantitativeValueInteger .

container:50lBeerKeg bevon:volume _:node18ib1jcplx34 ;
	a bevon:BeerKeg , owl:NamedIndividual ;
	skos:prefLabel "50l Beer Keg"@en , "50l 맥주 케그"@ko .

_:node18ib1jcplx35 gr:hasUnitOfMeasurement "MLT" ;
	gr:hasValue "640"^^xsd:int ;
	a gr:QuantitativeValueInteger .

container:640mlLongneck bevon:volume _:node18ib1jcplx35 ;
	a bevon:Longneck , owl:NamedIndividual ;
	skos:prefLabel "640ml Longneck Bottle"@en , "640ml 긴목 맥주병"@ko .

_:node18ib1jcplx36 gr:hasUnitOfMeasurement "MLT" ;
	gr:hasValue "640"^^xsd:int ;
	a gr:QuantitativeValueInteger .

container:640mlPlasticBottle bevon:volume _:node18ib1jcplx36 ;
	a bevon:PlasticBottle , owl:NamedIndividual ;
	skos:prefLabel "640ml Plastic Bottle"@en , "640ml 플라스틱 병"@ko .

_:node18ib1jcplx37 gr:hasUnitOfMeasurement "MLT" ;
	gr:hasValue "700"^^xsd:int ;
	a gr:QuantitativeValueInteger .

container:700mlGlassBottle bevon:volume _:node18ib1jcplx37 ;
	a bevon:GlassBottle , owl:NamedIndividual ;
	skos:altLabel "70cl Glass Bottle"@en ;
	skos:prefLabel "700ml Glass Bottle"@en , "700ml 유리병"@ko .

_:node18ib1jcplx38 gr:hasUnitOfMeasurement "MLT" ;
	gr:hasValue "750"^^xsd:int ;
	a gr:QuantitativeValueInteger .

container:750mlGlassBottle bevon:volume _:node18ib1jcplx38 ;
	a bevon:GlassBottle , owl:NamedIndividual ;
	skos:altLabel "75cl Glass Bottle"@en ;
	skos:prefLabel "750ml Glass Bottle"@en , "750ml 유리병"@ko .

bevon:description dcterms:issued "2013-07-04+09:00"^^xsd:date ;
	dcterms:modified "2014-03-01+09:00"^^xsd:date ;
	a owl:DatatypeProperty ;
	rdfs:domain bevon:Beverage ;
	rdfs:isDefinedBy <http://rdfs.co/bevon/> ;
	rdfs:range xsd:string ;
	rdfs:subPropertyOf dcterms:description , gr:description ;
	status:term_status "testing"@en ;
	skos:definition "\n    This property specifies the short text description of the beverage.\n    "@en ;
	skos:prefLabel "description"@en , "설명"@ko .

bevon:distillery dcterms:issued "2013-07-04+09:00"^^xsd:date ;
	dcterms:modified "2014-03-01+09:00"^^xsd:date ;
	a owl:ObjectProperty ;
	rdfs:domain bevon:DistilledBeverage ;
	rdfs:isDefinedBy <http://rdfs.co/bevon/> ;
	rdfs:range bevon:Distillery ;
	rdfs:seeAlso <http://en.wikipedia.org/wiki/Distillation> ;
	status:term_status "unstable"@en ;
	skos:definition "\n    This property relates a distilled beverage to its distillery.\n    "@en ;
	skos:prefLabel "Distillery"@en , "증류소"@ko .

bevon:duration dcterms:issued "2013-07-04+09:00"^^xsd:date ;
	dcterms:modified "2014-03-01+09:00"^^xsd:date ;
	a owl:ObjectProperty ;
	rdfs:domain bevon:Aging ;
	rdfs:isDefinedBy <http://rdfs.co/bevon/> ;
	rdfs:range time:DurationDescription ;
	rdfs:subPropertyOf time:hasDurationDescription ;
	status:term_status "unstable"@en ;
	skos:definition "\n    This property describes how long the beverage was aged in the cask.\n    "@en ;
	skos:prefLabel "duration"@en , "기간"@ko .

bevon:fermentation_base dcterms:issued "2013-07-04+09:00"^^xsd:date ;
	dcterms:modified "2014-03-01+09:00"^^xsd:date ;
	a owl:ObjectProperty ;
	rdfs:domain bevon:AlcoholicBeverage ;
	rdfs:isDefinedBy <http://rdfs.co/bevon/> ;
	rdfs:range bevon:FermentationBase ;
	status:term_status "unstable"@en ;
	skos:definition "\n    This property indicates which fermentation base is used to make the\n    alcoholic beverage.\n    "@en ;
	skos:prefLabel "fermentation base"@en , "발효 주재료"@ko .

bevon:food dcterms:issued "2013-07-04+09:00"^^xsd:date ;
	dcterms:modified "2014-03-01+09:00"^^xsd:date ;
	a owl:ObjectProperty ;
	rdfs:domain food:Ingredient ;
	rdfs:isDefinedBy <http://rdfs.co/bevon/> ;
	rdfs:range food:Food ;
	rdfs:subPropertyOf food:food ;
	status:term_status "unstable"@en ;
	skos:definition "\n    This property describes food that is an ingredient of a mixed drink.\n    "@en ;
	skos:prefLabel "food"@en , "음식"@ko .

bevon:ibu dcterms:issued "2013-07-04+09:00"^^xsd:date ;
	dcterms:modified "2014-03-01+09:00"^^xsd:date ;
	a owl:DatatypeProperty ;
	rdfs:domain bevon:Beer ;
	rdfs:isDefinedBy <http://rdfs.co/bevon/> ;
	rdfs:range xsd:nonNegativeInteger ;
	rdfs:seeAlso <http://en.wikipedia.org/wiki/International_Bitterness_Units_scale> ;
	status:term_status "unstable"@en ;
	skos:altLabel "International Bitterness Unit scale"@en ;
	skos:definition "\n    The International Bittering Units scale, or simply IBU scale, provides a\n    measure of the bitterness of beer, which is provided by the hops used\n    during brewing.\n    "@en ;
	skos:prefLabel "IBU scale"@en , "IBU 척도"@ko .

bevon:ingredient dcterms:issued "2013-07-04+09:00"^^xsd:date ;
	dcterms:modified "2014-03-01+09:00"^^xsd:date ;
	a owl:ObjectProperty ;
	rdfs:domain bevon:MixedDrink ;
	rdfs:isDefinedBy <http://rdfs.co/bevon/> ;
	rdfs:range food:Ingredient ;
	rdfs:subPropertyOf food:containsIngredient ;
	status:term_status "unstable"@en ;
	skos:definition "\n    This property specifies an ingredient of the mixed drink.\n    "@en ;
	skos:prefLabel "ingredient"@en , "재료"@ko .

bevon:launch dcterms:issued "2013-07-04+09:00"^^xsd:date ;
	dcterms:modified "2014-03-01+09:00"^^xsd:date ;
	a owl:DatatypeProperty ;
	rdfs:domain bevon:Beverage ;
	rdfs:isDefinedBy <http://rdfs.co/bevon/> ;
	rdfs:range xsd:gYear ;
	status:term_status "unstable"@en ;
	skos:definition "\n    This property specifies the year when the beverage was first introduced to\n    the market.\n    "@en ;
	skos:prefLabel "launch"@en , "출시년도"@ko .

bevon:manufacturer dcterms:issued "2013-07-04+09:00"^^xsd:date ;
	dcterms:modified "2014-03-01+09:00"^^xsd:date ;
	a owl:ObjectProperty ;
	rdfs:domain bevon:Beverage ;
	rdfs:isDefinedBy <http://rdfs.co/bevon/> ;
	rdfs:range foaf:Agent ;
	rdfs:subPropertyOf gr:hasManufacturer ;
	status:term_status "unstable"@en ;
	skos:definition "\n    This property specifies the manufacturer of the beverage.\n    "@en ;
	skos:prefLabel "manufacturer"@en , "제조사"@ko .

bevon:material dcterms:issued "2013-07-04+09:00"^^xsd:date ;
	dcterms:modified "2014-03-01+09:00"^^xsd:date ;
	a owl:ObjectProperty ;
	rdfs:domain bevon:Aging ;
	rdfs:isDefinedBy <http://rdfs.co/bevon/> ;
	status:term_status "unstable"@en ;
	skos:definition "\n    This property specifies what the aging cask was made of.\n    "@en ;
	skos:prefLabel "material"@en , "소재"@ko .

bevon:name dcterms:issued "2013-07-04+09:00"^^xsd:date ;
	dcterms:modified "2014-03-01+09:00"^^xsd:date ;
	a owl:DatatypeProperty ;
	rdfs:domain bevon:Beverage ;
	rdfs:isDefinedBy <http://rdfs.co/bevon/> ;
	rdfs:range xsd:string ;
	rdfs:subPropertyOf dcterms:title , gr:name , foaf:name ;
	status:term_status "testing"@en ;
	skos:definition "\n    This property indicates the name of the beverage.\n    "@en ;
	skos:prefLabel "name"@en , "이름"@ko .

bevon:non_alcoholic_version dcterms:issued "2013-07-04+09:00"^^xsd:date ;
	dcterms:modified "2014-03-01+09:00"^^xsd:date ;
	a owl:ObjectProperty ;
	rdfs:domain bevon:AlcoholicBeverage ;
	rdfs:isDefinedBy <http://rdfs.co/bevon/> ;
	rdfs:range bevon:NonAlcoholicBeverage ;
	rdfs:subPropertyOf bevon:related ;
	status:term_status "unstable"@en ;
	skos:definition "\n    Some alcoholic beverages have non-alcoholic versions, such as non-alcoholic\n    beer (\"near beer\") and cocktails (\"mocktails\").\n    "@en ;
	skos:prefLabel "non-alcoholic version"@en , "비알코올 버전"@ko .

bevon:origin dcterms:issued "2013-07-04+09:00"^^xsd:date ;
	dcterms:modified "2014-03-01+09:00"^^xsd:date ;
	a owl:ObjectProperty ;
	rdfs:domain bevon:Beverage ;
	rdfs:isDefinedBy <http://rdfs.co/bevon/> ;
	rdfs:range dbpedia:Place ;
	status:term_status "unstable"@en ;
	skos:definition "\n    This property indicates the place where the beverage was first invented.\n    "@en ;
	skos:prefLabel "origin"@en , "원산지"@ko .

bevon:previous_content dcterms:issued "2013-07-04+09:00"^^xsd:date ;
	dcterms:modified "2014-03-01+09:00"^^xsd:date ;
	a owl:ObjectProperty ;
	rdfs:domain bevon:Aging ;
	rdfs:isDefinedBy <http://rdfs.co/bevon/> ;
	rdfs:range fowl:PotableLiquid ;
	status:term_status "unstable"@en ;
	skos:definition "\n    This property specifies what as in the cask before the aging.\n    "@en ;
	skos:prefLabel "previous content"@en , "이전 내용물"@ko .

bevon:proof dcterms:issued "2013-07-04+09:00"^^xsd:date ;
	dcterms:modified "2014-03-01+09:00"^^xsd:date ;
	a owl:DatatypeProperty ;
	rdfs:comment "\n    The term was originally used in the United Kingdom and was defined as 7/4\n    times the alcohol by volume (ABV). The UK now uses the ABV standard instead\n    of alcohol proof. In the United States, alcoholic proof is defined as twice\n    the percentage of ABV.\n    "@en ;
	rdfs:domain bevon:Beverage ;
	rdfs:isDefinedBy <http://rdfs.co/bevon/> ;
	rdfs:range xsd:decimal ;
	rdfs:seeAlso <http://en.wikipedia.org/wiki/Alcohol_proof> ;
	status:term_status "unstable"@en ;
	skos:altLabel "alcohol proof"@en ;
	skos:definition "\n    Alcohol proof is a measure of how much alcohol (ethanol) is contained in an\n    alcoholic beverage.\n    "@en ;
	skos:prefLabel "proof"@en , "프루프"@ko .

bevon:quantity dcterms:issued "2013-07-04+09:00"^^xsd:date ;
	dcterms:modified "2014-03-01+09:00"^^xsd:date ;
	a owl:ObjectProperty ;
	rdfs:domain food:Ingredient ;
	rdfs:isDefinedBy <http://rdfs.co/bevon/> ;
	rdfs:range gr:QuantitativeValue ;
	status:term_status "unstable"@en ;
	skos:definition "\n    This property specifies the quantity of the ingredient with a type\n    in the UN/CEFACT Common Code.\n    "@en ;
	skos:prefLabel "quantity"@en , "양"@ko .

bevon:related dcterms:issued "2013-07-04+09:00"^^xsd:date ;
	dcterms:modified "2014-03-01+09:00"^^xsd:date ;
	a owl:ObjectProperty ;
	rdfs:domain bevon:Beverage ;
	rdfs:isDefinedBy <http://rdfs.co/bevon/> ;
	rdfs:range bevon:Beverage ;
	status:term_status "unstable"@en ;
	skos:definition "\n    This property states that a beverage is related to another beverage.\n    "@en ;
	skos:prefLabel "related"@en , "연관"@ko .

bevon:similar dcterms:issued "2013-07-04+09:00"^^xsd:date ;
	dcterms:modified "2014-03-01+09:00"^^xsd:date ;
	a owl:SymmetricProperty ;
	rdfs:domain bevon:Beverage ;
	rdfs:isDefinedBy <http://rdfs.co/bevon/> ;
	rdfs:range bevon:Beverage ;
	rdfs:subPropertyOf gr:isSimilarTo , bevon:related ;
	status:term_status "unstable"@en ;
	skos:definition "\n    This property states that a beverage is similar to another beverage.\n    "@en ;
	skos:prefLabel "similar"@en , "유사"@ko .

bevon:srm dcterms:issued "2013-07-04+09:00"^^xsd:date ;
	dcterms:modified "2014-03-01+09:00"^^xsd:date ;
	a owl:DatatypeProperty ;
	rdfs:domain bevon:Beer ;
	rdfs:isDefinedBy <http://rdfs.co/bevon/> ;
	rdfs:range xsd:nonNegativeInteger ;
	rdfs:seeAlso <http://en.wikipedia.org/wiki/Standard_Reference_Method> ;
	status:term_status "unstable"@en ;
	skos:altLabel "Standard Reference Method"@en ;
	skos:definition "\n    The Standard Reference Method or SRM is one of several systems modern\n    brewers use to specify beer color.\n    "@en ;
	skos:prefLabel "SRM"@en .

bevon:variant dcterms:issued "2013-07-04+09:00"^^xsd:date ;
	dcterms:modified "2014-03-01+09:00"^^xsd:date ;
	a owl:ObjectProperty ;
	rdfs:domain bevon:Beverage ;
	rdfs:isDefinedBy <http://rdfs.co/bevon/> ;
	rdfs:range bevon:Beverage ;
	rdfs:subPropertyOf bevon:related ;
	owl:inverseOf bevon:variantOf ;
	status:term_status "unstable"@en ;
	skos:definition "\n    This property states that a beverage has a variant.\n    "@en ;
	skos:prefLabel "variant"@en , "변형"@ko .

bevon:variantOf dcterms:issued "2013-07-04+09:00"^^xsd:date ;
	dcterms:modified "2014-03-01+09:00"^^xsd:date ;
	a owl:ObjectProperty ;
	rdfs:domain bevon:Beverage ;
	rdfs:isDefinedBy <http://rdfs.co/bevon/> ;
	rdfs:range bevon:Beverage ;
	rdfs:subPropertyOf dbpedia:variantOf , gr:isVariantOf , bevon:related ;
	owl:inverseOf bevon:variant ;
	status:term_status "unstable"@en ;
	skos:definition "\n    This property states that a beverage is a variant of another beverage.\n    "@en ;
	skos:prefLabel "variant of"@en , "바탕"@ko .

bevon:volume dcterms:issued "2013-07-04+09:00"^^xsd:date ;
	dcterms:modified "2014-03-01+09:00"^^xsd:date ;
	a owl:ObjectProperty ;
	rdfs:domain bevon:Container ;
	rdfs:isDefinedBy <http://rdfs.co/bevon/> ;
	rdfs:range gr:QuantitativeValue ;
	status:term_status "unstable"@en ;
	skos:definition "\n    This property specifies the volume of the container.\n    "@en ;
	skos:prefLabel "volume"@en , "용량"@ko .

_:node18ib1jcplx39 dcterms:creator <http://jayg.me/> ;
	dcterms:date "2014-03-01+09:00"^^xsd:date ;
	rdf:value "Minor revisions for documentation" .

<http://rdfs.co/bevon/0.6> skos:changeNote _:node18ib1jcplx39 .

_:node18ib1jcplx40 dcterms:creator <http://jayg.me/> ;
	dcterms:date "2014-03-03+09:00"^^xsd:date ;
	rdf:value "Added a link to the GitHub repository" .

<http://rdfs.co/bevon/0.6> skos:changeNote _:node18ib1jcplx40 .

_:node18ib1jcplx41 a dcterms:IMT ;
	rdf:value "text/html" ;
	rdfs:label "HTML"@en .

<http://rdfs.co/bevon/0.6/html> dcterms:format _:node18ib1jcplx41 .

_:node18ib1jcplx42 a dcterms:IMT ;
	rdf:value "application/rdf+xml" ;
	rdfs:label "RDF/XML"@en .

<http://rdfs.co/bevon/0.6/rdf> dcterms:format _:node18ib1jcplx42 .

_:node18ib1jcplx43 a dcterms:IMT ;
	rdf:value "text/turtle" ;
	rdfs:label "Turtle"@en .

<http://rdfs.co/bevon/0.6/ttl> dcterms:format _:node18ib1jcplx43 .

_:node18ib1jcplx44 dcterms:title "Clear"@en ;
	a dbpedia:Colour ;
	owl:sameAs <http://dbpedia.org/resource/Clear_(color)> .

beverage:Chamisul bevon:color _:node18ib1jcplx44 .

_:node18ib1jcplx45 dcterms:title "Clear"@en ;
	a dbpedia:Colour ;
	owl:sameAs <http://dbpedia.org/resource/Clear_(color)> .

beverage:Chum-Churum bevon:color _:node18ib1jcplx45 .

_:node18ib1jcplx46 a foaf:Organization ;
	rdfs:seeAlso <http://ko.wikipedia.org/wiki/롯데칠성음료> ;
	foaf:homepage <http://www.lotteliquor.com> ;
	foaf:name "Lotte Liquor"@en , "롯데주류"@ko .

beverage:Chum-Churum bevon:manufacturer _:node18ib1jcplx46 .

_:node18ib1jcplx47 dcterms:title "Clear"@en ;
	a dbpedia:Colour ;
	owl:sameAs <http://dbpedia.org/resource/Clear_(color)> .

beverage:DonJulioBlanco bevon:color _:node18ib1jcplx47 .

_:node18ib1jcplx49 a time:DurationDescription ;
	time:years "12"^^xsd:integer .

_:node18ib1jcplx48 bevon:duration _:node18ib1jcplx49 ;
	bevon:material <http://dbpedia.org/resource/Oak> ;
	bevon:previous_content <http://dbpedia.org/resource/Bourbon_whiskey> , <http://dbpedia.org/resource/Sherry> ;
	a bevon:Aging .

beverage:Glenfiddich12YearOld bevon:aging _:node18ib1jcplx48 .

_:node18ib1jcplx50 dcterms:title "Golden"@en ;
	a dbpedia:Colour ;
	owl:sameAs <http://dbpedia.org/resource/Gold_(color)> , <http://purl.org/colors/rgb/FFD700> .

beverage:Glenfiddich12YearOld bevon:color _:node18ib1jcplx50 .

_:node18ib1jcplx51 whisky:owner <http://dbpedia.org/resource/William_Grant_%26_Sons> ;
	whisky:region <http://dbpedia.org/resource/Strathspey,_Scotland> .

_:node18ib1jcplx52 dcterms:title "Robbie Dhu Springs"@en , "로비 듀 수원지"@ko ;
	a whisky:WaterSource .

_:node18ib1jcplx51 whisky:waterSource _:node18ib1jcplx52 ;
	a bevon:Distillery ;
	owl:sameAs <http://dbpedia.org/resource/Glenfiddich_distillery> .

beverage:Glenfiddich12YearOld bevon:distillery _:node18ib1jcplx51 .

_:node18ib1jcplx53 dcterms:title "Ruby Red"@en ;
	a dbpedia:Colour ;
	owl:sameAs <http://dbpedia.org/resource/Ruby_(color)__Ruby_Red__1> , <http://purl.org/colors/rgb/9B111E> .

beverage:Smithwicks bevon:color _:node18ib1jcplx53 .

_:node18ib1jcplx55 dcterms:title "Whisky"@en ;
	a bevon:Whisky ;
	owl:sameAs <http://dbpedia.org/resource/Whisky> .

_:node18ib1jcplx54 bevon:food _:node18ib1jcplx55 .

_:node18ib1jcplx56 gr:hasUnitOfMeasurement "OZA" ;
	gr:hasValue "2"^^xsd:int ;
	a gr:QuantitativeValueInteger .

_:node18ib1jcplx54 bevon:quantity _:node18ib1jcplx56 ;
	a food:Ingredient .

beverage:WhiskyAndSoda bevon:ingredient _:node18ib1jcplx54 .

_:node18ib1jcplx58 dcterms:title "Carbonated Water"@en ;
	a bevon:CarbonatedWater ;
	owl:sameAs <http://dbpedia.org/resource/Carbonated_water> .

_:node18ib1jcplx57 bevon:food _:node18ib1jcplx58 ;
	a food:Ingredient .

beverage:WhiskyAndSoda bevon:ingredient _:node18ib1jcplx57 .

_:node18ib1jcplx59 gr:hasUnitOfMeasurement "LTR" ;
	gr:hasValue "15"^^xsd:int ;
	a gr:QuantitativeValueInteger .

container:15lBeerKeg bevon:volume _:node18ib1jcplx59 .

_:node18ib1jcplx60 gr:hasUnitOfMeasurement "LTR" ;
	gr:hasValue "1.8"^^xsd:float ;
	a gr:QuantitativeValueFloat .

container:1_8lPlasticBottle bevon:volume _:node18ib1jcplx60 .

_:node18ib1jcplx61 gr:hasUnitOfMeasurement "MLT" ;
	gr:hasValue "200"^^xsd:int ;
	a gr:QuantitativeValueInteger .

container:200mlPlasticBottle bevon:volume _:node18ib1jcplx61 .

_:node18ib1jcplx62 gr:hasUnitOfMeasurement "LTR" ;
	gr:hasValue "25"^^xsd:int ;
	a gr:QuantitativeValueInteger .

container:25lBeerKeg bevon:volume _:node18ib1jcplx62 .

_:node18ib1jcplx63 gr:hasUnitOfMeasurement "LTR" ;
	gr:hasValue "30"^^xsd:int ;
	a gr:QuantitativeValueInteger .

container:30lBeerKeg bevon:volume _:node18ib1jcplx63 .

_:node18ib1jcplx64 gr:hasUnitOfMeasurement "MLT" ;
	gr:hasValue "330"^^xsd:int ;
	a gr:QuantitativeValueInteger .

container:330mlBeverageCan bevon:volume _:node18ib1jcplx64 .

_:node18ib1jcplx65 gr:hasUnitOfMeasurement "MLT" ;
	gr:hasValue "330"^^xsd:int ;
	a gr:QuantitativeValueInteger .

container:330mlLongneck bevon:volume _:node18ib1jcplx65 .

_:node18ib1jcplx66 gr:hasUnitOfMeasurement "MLT" ;
	gr:hasValue "355"^^xsd:int ;
	a gr:QuantitativeValueInteger .

container:355mlBeverageCan bevon:volume _:node18ib1jcplx66 .

_:node18ib1jcplx67 gr:hasUnitOfMeasurement "MLT" ;
	gr:hasValue "360"^^xsd:int ;
	a gr:QuantitativeValueInteger .

container:360mlGlassBottle bevon:volume _:node18ib1jcplx67 .

_:node18ib1jcplx68 gr:hasUnitOfMeasurement "MLT" ;
	gr:hasValue "360"^^xsd:int ;
	a gr:QuantitativeValueInteger .

container:360mlPlasticBottle bevon:volume _:node18ib1jcplx68 .

_:node18ib1jcplx69 gr:hasUnitOfMeasurement "MLT" ;
	gr:hasValue "440"^^xsd:int ;
	a gr:QuantitativeValueInteger .

container:440mlBeverageCan bevon:volume _:node18ib1jcplx69 .

_:node18ib1jcplx70 gr:hasUnitOfMeasurement "MLT" ;
	gr:hasValue "500"^^xsd:int ;
	a gr:QuantitativeValueInteger .

container:500mlBeverageCan bevon:volume _:node18ib1jcplx70 .

_:node18ib1jcplx71 gr:hasUnitOfMeasurement "MLT" ;
	gr:hasValue "500"^^xsd:int ;
	a gr:QuantitativeValueInteger .

container:500mlLongneck bevon:volume _:node18ib1jcplx71 .

_:node18ib1jcplx72 gr:hasUnitOfMeasurement "LTR" ;
	gr:hasValue "50"^^xsd:int ;
	a gr:QuantitativeValueInteger .

container:50lBeerKeg bevon:volume _:node18ib1jcplx72 .

_:node18ib1jcplx73 gr:hasUnitOfMeasurement "MLT" ;
	gr:hasValue "640"^^xsd:int ;
	a gr:QuantitativeValueInteger .

container:640mlLongneck bevon:volume _:node18ib1jcplx73 .

_:node18ib1jcplx74 gr:hasUnitOfMeasurement "MLT" ;
	gr:hasValue "640"^^xsd:int ;
	a gr:QuantitativeValueInteger .

container:640mlPlasticBottle bevon:volume _:node18ib1jcplx74 .

_:node18ib1jcplx75 gr:hasUnitOfMeasurement "MLT" ;
	gr:hasValue "700"^^xsd:int ;
	a gr:QuantitativeValueInteger .

container:700mlGlassBottle bevon:volume _:node18ib1jcplx75 .

_:node18ib1jcplx76 gr:hasUnitOfMeasurement "MLT" ;
	gr:hasValue "750"^^xsd:int ;
	a gr:QuantitativeValueInteger .

container:750mlGlassBottle bevon:volume _:node18ib1jcplx76 .
