@prefix dc: <http://purl.org/dc/elements/1.1/> .
@prefix : <http://purl.org/net/cito/> .
@prefix rdfs: <http://www.w3.org/2000/01/rdf-schema#> .
@prefix owl2xml: <http://www.w3.org/2006/12/owl2-xml#> .
@prefix xsd: <http://www.w3.org/2001/XMLSchema#> .
@prefix owl: <http://www.w3.org/2002/07/owl#> .
@prefix rdf: <http://www.w3.org/1999/02/22-rdf-syntax-ns#> .
@prefix core: <http://purl.org/vocab/frbr/core#> .

<http://purl.org/net/cito/> a owl:Ontology ;
	dc:date "2010-03-26"^^xsd:date ;
	dc:description "CiTO, the Citation Typing Ontology, is an ontology for describing the nature of reference citations in scientific research articles and other scholarly works on the Semantic Web."@en ;
	dc:title "CiTO: A Citation Typing Ontology"@en ;
	owl:versionInfo "Version 1.6"@en ;
	dc:rights "http://creativecommons.org/licenses/by/2.5/" ;
	dc:creator "David Shotton" .

dc:date a owl:AnnotationProperty .

dc:title a owl:AnnotationProperty .

dc:description a owl:AnnotationProperty .

dc:creator a owl:AnnotationProperty .

dc:rights a owl:AnnotationProperty .

:cites a owl:ObjectProperty ;
	rdfs:label "cites"@en ;
	rdfs:comment "A statement of fact that the citing Work cites the cited Work. [This is implicit in human-readable reference lists, and need not be stated when annotating them using CiTO.  However, the statement is useful in machine-readable metadata for construction of citation networks and other purposes.] [For scholarly Works, it is usually the final published Expression of the Work, known to publishers as the 'version of record', which is critical for CiTO, since it is the references within this version of record that are definitive, and it is the version of record itself that is cited by others.  However, for certain items such as a Database or a BlogEntry, it is the on-line Manifestation, i.e. the Web page URI, that is cited.  For this reason, the range of cito:cites is left unconstrained."@en .

:citesAsAuthority a owl:ObjectProperty ;
	rdfs:label "citesAsAuthority"@en ;
	rdfs:comment "The citing work refers to the cited work as providing an authoritative description or definition of the subject under discussion."@en ;
	rdfs:subPropertyOf :cites .

:citesAsMetadataDocument a owl:ObjectProperty ;
	rdfs:label "citesAsMetadataDocument"@en ;
	rdfs:comment "The citing work refers to the cited work as containing metadata about the citing work."@en ;
	rdfs:subPropertyOf :cites .

:citesAsSourceDocument a owl:ObjectProperty ;
	rdfs:label "citesAsSourceDocument"@en ;
	rdfs:comment "The citing work refers to the cited work as the source about which the citing work contains metadata."@en ;
	rdfs:subPropertyOf :cites .

:citesForInformation a owl:ObjectProperty ;
	rdfs:label "citesForInformation"@en ;
	rdfs:comment "The citing work refers the reader to the cited work as a source of information on the subject discussed in the text."@en ;
	rdfs:subPropertyOf :cites .

:confirms a owl:ObjectProperty ;
	rdfs:label "confirms"@en ;
	rdfs:comment "The citing work confirms facts, ideas or statements presented in the cited work."@en ;
	rdfs:subPropertyOf :cites .

:corrects a owl:ObjectProperty ;
	rdfs:label "corrects"@en ;
	rdfs:comment "The citing work corrects ideas or statements presented in the cited work."@en ;
	rdfs:subPropertyOf :cites .

:credits a owl:ObjectProperty ;
	rdfs:label "credits"@en ;
	rdfs:comment "The citing work acknowledges contributions made by the cited work."@en ;
	rdfs:subPropertyOf :cites .

:critiques a owl:ObjectProperty ;
	rdfs:label "critiques"@en ;
	rdfs:comment "The citing work critiques facts, ideas or statements presented in the cited work."@en ;
	rdfs:subPropertyOf :cites .

:disagreesWith a owl:ObjectProperty ;
	rdfs:label "disagreesWith"@en ;
	rdfs:comment "The citing work disagrees with ideas or statements presented in the cited work."@en ;
	rdfs:subPropertyOf :cites .

:discusses a owl:ObjectProperty ;
	rdfs:label "discusses"@en ;
	rdfs:comment "The citing work discusses facts, ideas or statements presented in the cited work."@en ;
	rdfs:subPropertyOf :cites .

:extends a owl:ObjectProperty ;
	rdfs:label "extends"@en ;
	rdfs:comment "The citing work extends facts, ideas or understandings presented in the cited work."@en ;
	rdfs:subPropertyOf :cites .

:globalCitationFrequency a owl:ObjectProperty ;
	rdfs:label "globalCitationFrequency"@en ;
	rdfs:comment "The property linking an Expression of a Work to its Global Citation Count."@en ;
	rdfs:range :GlobalCitationCount .

:globalCountSource a owl:ObjectProperty ;
	rdfs:label "globalCountSource"@en ;
	rdfs:comment "The URI of the bibliographic information source of information providing the Global Citation Count of a Work."@en ;
	rdfs:domain :GlobalCitationCount .

:inTextCitationFrequency a owl:ObjectProperty ;
	rdfs:label "inTextCitationFrequency"@en ;
	rdfs:comment "The property linking an Expression of a cited Work to its In-Text Citation Count within the citing Work."@en ;
	rdfs:range :InTextCitationCount .

:inTextCitationTarget a owl:ObjectProperty ;
	rdfs:label "inTextCitationTarget"@en ;
	rdfs:comment "The URI of the cited Work for which the inTextCitationCount is relevant."@en ;
	rdfs:domain :InTextCitationCount .

:isCitedBy a owl:ObjectProperty ;
	rdfs:label "isCitedBy"@en ;
	rdfs:comment "A statement of fact that the cited Work is cited by the citing Work."@en ;
	owl:inverseOf :cites .

:isEmbodiedIn a owl:ObjectProperty ;
	rdfs:label "isEmbodiedIn"@en ;
	rdfs:comment "As defined by FRBR (http://www.ifla.org/VII/s13/frbr/frbr1.htm), the relationship between an Expression of a Work and its Manifestation."@en ;
	rdfs:domain :Expression ;
	rdfs:range :Manifestation .

:isEmbodimentOf a owl:ObjectProperty ;
	rdfs:label "isEmbodimentOf"@en ;
	rdfs:comment "As defined by FRBR (http://www.ifla.org/VII/s13/frbr/frbr1.htm), the relationship between a Manifestation and the Expression being manifested."@en ;
	rdfs:range :Expression ;
	rdfs:domain :Manifestation ;
	owl:inverseOf :isEmbodiedIn .

:isRealizationOf a owl:ObjectProperty ;
	rdfs:label "isRealizationOf" ;
	rdfs:domain :Expression ;
	rdfs:range :Work ;
	owl:inverseOf :isRealizedThrough .

:isRealizedThrough a owl:ObjectProperty ;
	rdfs:label "isRealizedThrough"@en ;
	rdfs:comment "As defined by FRBR (http://www.ifla.org/VII/s13/frbr/frbr1.htm), the relationship between a Work and its Expression."@en ;
	rdfs:range :Expression ;
	rdfs:domain :Work .

:obtainsBackgroundFrom a owl:ObjectProperty ;
	rdfs:label "obtainsBackgroundFrom"@en ;
	rdfs:comment "The citing work obtains background information from the cited work."@en ;
	rdfs:subPropertyOf :cites .

:obtainsSupportFrom a owl:ObjectProperty ;
	rdfs:label "obtainsSupportFrom"@en ;
	rdfs:comment "The citing work obtains intellectual or factual support from the cited work."@en ;
	rdfs:subPropertyOf :cites .

:qualifies a owl:ObjectProperty ;
	rdfs:label "qualifies"@en ;
	rdfs:comment "The citing work qualifies or places conditions upon facts, ideas or statements presented in the cited work."@en ;
	rdfs:subPropertyOf :cites .

:refutes a owl:ObjectProperty ;
	rdfs:label "refutes"@en ;
	rdfs:comment "The citing work refutes ideas or statements presented in the cited work."@en ;
	rdfs:subPropertyOf :cites .

:reviews a owl:ObjectProperty ;
	rdfs:label "reviews"@en ;
	rdfs:comment "The citing work reviews ideas or statements presented in the cited work."@en ;
	rdfs:subPropertyOf :cites .

:sharesAuthorsWith a owl:ObjectProperty ;
	rdfs:label "sharesAuthorsWith"@en ;
	rdfs:comment "The citing work has at least one author in common with the cited work."@en ;
	rdfs:subPropertyOf :cites .

:supports a owl:ObjectProperty ;
	rdfs:label "supports"@en ;
	rdfs:comment "The citing work provides intellectual or factual support for the cited work." ;
	rdfs:subPropertyOf :cites .

:updates a owl:ObjectProperty ;
	rdfs:label "updates"@en ;
	rdfs:comment "The citing work updates facts, ideas or understandings presented in the cited work."@en ;
	rdfs:subPropertyOf :cites .

:usesDataFrom a owl:ObjectProperty ;
	rdfs:label "usesDataFrom"@en ;
	rdfs:comment "The citing work used data from the cited work."@en ;
	rdfs:subPropertyOf :cites .

:usesMethodIn a owl:ObjectProperty ;
	rdfs:label "usesMethodIn"@en ;
	rdfs:comment "The citing work uses a method described in the cited work."@en ;
	rdfs:subPropertyOf :cites .

:globalCountDate a owl:DatatypeProperty ;
	rdfs:label "globalCountDate"@en ;
	rdfs:comment "The date on which the Global Citation Count of the Work was recorded from a named bibliographic information source."@en ;
	rdfs:domain :GlobalCitationCount ;
	rdfs:range xsd:date .

:globalCountValue a owl:DatatypeProperty ;
	rdfs:label "globalCountValue"@en ;
	rdfs:comment "An integer defining the value of the Global Citation Count of the Work recorded from a named bibliographic information source on a particular date."@en ;
	rdfs:domain :GlobalCitationCount ;
	rdfs:range xsd:integer .

:inTextCountValue a owl:DatatypeProperty ;
	rdfs:label "inTextCountValue"@en ;
	rdfs:comment "An integer defining the value of the In-Text Citation Count of the cited Work within the citing Work."@en ;
	rdfs:domain :InTextCitationCount ;
	rdfs:range xsd:integer .

:peerReviewed a owl:DatatypeProperty ;
	rdfs:label "peerReviewed"@en ;
	rdfs:comment "A Boolean data property having the value 'True' if the cited Work has been peer reviewed, or 'False' if the cited Work has not been peer reviewed.  [When using CiTO, the truth value of cito:peerReviewed may be left unspecified.]"@en ;
	rdfs:domain :Expression ;
	rdfs:range xsd:boolean .

:unpublished a owl:DatatypeProperty ;
	rdfs:label "unpublished"@en ;
	rdfs:comment "A Boolean data property having the value 'True' if the cited Work has not been published, or 'False' if the cited Work has been published.  [When using CiTO, the truth value of cito:Unpublished may be left unspecified.]"@en ;
	rdfs:domain :Expression ;
	rdfs:range xsd:boolean .

:Abstract a owl:Class ;
	rdfs:label "Abstract"@en ;
	rdfs:subClassOf :Document ;
	rdfs:comment "A brief summary of a Work that gives an in-depth description or analysis of a particular subject (typically a Research Paper, Report, Review or Thesis), appearing at the beginning of the Work and designed to act as the point-of-entry that will help the reader quickly to obtain an overview of its contents."@en .

:Algorithm a owl:Class ;
	rdfs:label "Algorithm"@en ;
	rdfs:subClassOf :Specification ;
	rdfs:comment "A precise sequential set of pre-defined logical rules or computational operations to be employed for solving a particular problem in a finite number of steps." .

:AuthorityFile a owl:Class ;
	rdfs:label "AuthorityFile" ;
	rdfs:subClassOf :Specification ;
	rdfs:comment "A controlled vocabulary or official list that establishes, for consistency, the authoritative forms of headings, preferred terms or proper names to be used when creating a catalogue, or when indexing and searching a set of entities within a defined domain."@en .

:BibliographicMetadata a owl:Class ;
	rdfs:label "BibliographicMetadata"@en ;
	rdfs:subClassOf :Metadata ;
	rdfs:comment "Standard bibliographic metadata describing an Expression of a Work, including, to take the example of a JournalArticle, the author(s), the date of publication, the title, the journal name and volume number, the first and last page numbers, and the Digital Object Identifier."@en .

:Biography a owl:Class ;
	rdfs:label "Biography" ;
	rdfs:subClassOf :Work ;
	rdfs:comment "An account of the events, works and achievements, personal and professional, during the life of a person, either living or dead."@en .

:BlogEntry a owl:Class ;
	rdfs:label "BlogEntry"@en ;
	rdfs:subClassOf :WebContent ;
	owl:disjointWith :WikiEntry ;
	rdfs:comment "Information manifested in a Blog, a type of WebPage comprising  periodic sequential entries containing commentary, descriptions of events, or other material such as images or videos, usually displayed in reverse-chronological order and usually maintained by an individual."@en .

:Book a owl:Class ;
	rdfs:label "Book"@en ;
	rdfs:subClassOf :Document ;
	rdfs:comment "A non-serial publication that is complete in one volume or a designated finite number of volumes.  A printed Manifestation of a book is often identified with an ISBN."@en .

:BookChapter a owl:Class ;
	rdfs:label "BookChapter"@en ;
	rdfs:subClassOf :BookSection ;
	rdfs:comment "A defined chapter of a book, usually with a separate title or number."@en .

:BookReview a owl:Class ;
	rdfs:label "BookReview"@en ;
	rdfs:subClassOf :Review ;
	rdfs:comment "A written Work consisting of a review and critical analysis of the content, scope and quality of a book or other monographic work."@en .

:BookSection a owl:Class ;
	rdfs:label "BookSection"@en ;
	rdfs:subClassOf :Document ;
	rdfs:comment "A defined section of a book, such as a preface, chapter or index, usually with a separate title or number."@en .

:CaseForSupport a owl:Class ;
	rdfs:label "CaseForSupport"@en ;
	rdfs:subClassOf :Work ;
	rdfs:comment "An accompaniment to a Grant Application that provides a description of a proposed project and gives reasons why it is worthy of funding. (See also cito:GrantApplication)."@en .

:CaseForSupportDocument a owl:Class ;
	rdfs:label "CaseForSupportDocument"@en ;
	rdfs:subClassOf :Document ;
	rdfs:comment "An Expression of a Case For Support.   (Usually associated with a Grant Application Document.)"@en .

:Catalog a owl:Class ;
	rdfs:label "Catalog" ;
	rdfs:subClassOf :Specification ;
	rdfs:comment "A list of items describing the content of a resource, for example items in an exhibition, offered for sale by a vendor, or contained within a library or collection.  Ideally, Catalogs are created according to specific and uniform principles of construction and are under the control of an Authority File."@en .

:CitationMetadata a owl:Class ;
	rdfs:label "CitationMetadata"@en ;
	rdfs:subClassOf :Metadata ;
	rdfs:comment "Metadata describing the citations made within an Expression of a  Work to Expressions of other Works, and (optionally) some characteristics of the cited Expressions."@en .

:ClinicalCaseReport a owl:Class ;
	rdfs:label "ClinicalCaseReport" ;
	rdfs:subClassOf :Report ;
	owl:disjointWith :ClinicalTrialReport ;
	rdfs:comment "A presentation of findings following a clinical or medical investigation on a human or animal patient, that may contain a diagnosis and proposals for therapeutic treatment and/or epidemiological control measures, or may propose further evaluative studies that will eventually lead to such outcomes."@en .

:ClinicalTrialDesign a owl:Class ;
	rdfs:label "ClinicalTrialDesign"@en ;
	rdfs:subClassOf :Specification ;
	rdfs:comment "A predefined written procedural method, designed to ensure reliability of findings, for undertaking a medical or veterinary clinical study of the safety, efficacy, or optimum dosage schedule of one or more diagnostic, therapeutic or prophylactic drugs or treatments, or of devices or techniques, involving a randomized controlled trial for evidence-based assessment in humans or animals, specifying criteria of eligibility, nature of controls, sampling schedules, data collection parameters, statistical analyses, reporting standards, etc. to be employed in undertaking the clinical trial." .

:ClinicalTrialReport a owl:Class ;
	rdfs:label "ClinicalTrialReport" ;
	rdfs:subClassOf :Report ;
	rdfs:comment "The report of a pre-planned medical or veterinary clinical study of the safety, efficacy, or optimum dosage schedule of one or more diagnostic, therapeutic or prophylactic drugs, or of devices, treatments or techniques, involving a randomized controlled trial for evidence-based assessment in humans or animals selected according to predetermined criteria of eligibility and observed forevidence of favourable and unfavourable effects."@en .

:ComputerFile a owl:Class ;
	rdfs:label "ComputerFile"@en ;
	rdfs:subClassOf :Manifestation ;
	rdfs:comment "A block of digital information created by a computer system and stored electronically on a digital memory device in a form available for re-use, typically encoded in a particular format by a specific software application (e.g. in PDF, plain text, image, video or word processor file format)."@en .

:ConferencePaper a owl:Class ;
	rdfs:label "ConferencePaper"@en ;
	rdfs:subClassOf :Document ;
	rdfs:comment "A Research Paper, Review, Report or other work presented at a conference, seminar, symposium, workshop or similar event."@en .

:ConferencePoster a owl:Class ;
	rdfs:label "ConferencePoster"@en ;
	rdfs:subClassOf :Document ;
	rdfs:comment "A display poster, typically containing text with figures and/or tables, submitted for acceptance to and/or presented at a conference, seminar, symposium, workshop or similar event."@en .

:ConferenceProceedings a owl:Class ;
	rdfs:label "ConferenceProceedings" ;
	rdfs:subClassOf :Document ;
	rdfs:comment "A publication containing the programme and collected Conference Papers presented at a conference, seminar, symposium, workshop or similar event, or their Abstracts."@en .

:Database a owl:Class ;
	rdfs:label "Database"@en ;
	rdfs:subClassOf :Expression ;
	rdfs:comment "A structured collection of logically related records or data stored and retrieved using computer-based means."@en .

:Dataset a owl:Class ;
	rdfs:label "Dataset"@en ;
	rdfs:subClassOf :Work ;
	rdfs:comment "A collection of related facts, often expressed in numerical form and encoded in a defined structure."@en .

:DigitalMediaFile a owl:Class ;
	rdfs:label "DigitalMediaFile"@en ;
	rdfs:subClassOf :ComputerFile ;
	owl:disjointWith :OnlineFile ;
	rdfs:comment "A computer file stored off-line on a removable magnetic, optical, solid state or other digital storage device (e.g. a DVD, CD-ROM, DV tape, or USB flash drive) used to save, transport, distribute and play back such files."@en .

:Document a owl:Class ;
	rdfs:label "Document"@en ;
	rdfs:subClassOf :Expression ;
	rdfs:comment "An Expression of a Work conveying a body of information primarily in textual form.  A Document may contain one or more Figures and Tables in addition to text."@en .

:Editorial a owl:Class ;
	rdfs:label "Editorial"@en ;
	rdfs:subClassOf :PeriodicalItem ;
	rdfs:comment "The Opinions of an editor expressed in a published Periodical Issue."@en .

:Email a owl:Class ;
	rdfs:label "Email"@en ;
	rdfs:subClassOf :Document ;
	rdfs:comment "A Personal Communication transmitted over the Internet as an item of electronic mail, typically based on the Simple Mail Transfer Protocol (SMTP)."@en .

:EntityMetadata a owl:Class ;
	rdfs:label "EntityMetadata"@en ;
	rdfs:subClassOf :Metadata ;
	rdfs:comment "Metadata describing the Work itself, including for example the name of the creator(s), the title, and the data and place of creation."@en .

:ExperimentalProtocol a owl:Class ;
	rdfs:label "ExperimentalProtocol"@en ;
	rdfs:subClassOf :Specification ;
	rdfs:comment "A predefined written procedural method, designed to ensure successful replication of results by others in the same or other laboratories, that describes the overall objectives, organization and implementation of a scientific experiment, and specifies the experimental design, experimental methods, reagents, instrumentation, sampling schedules, data collection parameters, statistical analyses, image processing procedures, safety precautions, reporting standards, etc. employed in undertaking the experiment."@en .

:Expression a owl:Class ;
	rdfs:label "Expression"@en ;
	rdfs:subClassOf core:Expression ;
	owl:disjointWith :Manifestation , :Work ;
	rdfs:comment "As defined by FRBR (http://www.ifla.org/VII/s13/frbr/frbr1.htm), an Expression is the specific form that a Work takes each time it is 'realized' in physical or electronic form.  For scholarly Works, it is usually the final published Expression of the Work, known to publishers as the 'version of record', which is critical for CiTO, since it is the references within this version of record that are definitive, and it is the version of record itself that is cited by others."@en .

:Figure a owl:Class ;
	rdfs:label "Figure"@en ;
	rdfs:subClassOf :Expression ;
	rdfs:comment "A visual communication object comprising one or more StillImages on a related theme.  If included within a publication, a Figure is typically unaligned with the main body of text, having its own descriptive textual figure legend."@en .

:GlobalCitationCount a owl:Class ;
	rdfs:label "GlobalCitationCount"@en ;
	rdfs:subClassOf owl:Thing ;
	owl:disjointWith :InTextCitationCount , core:Expression , core:Manifestation , core:Work ;
	rdfs:comment "The number of times a Work has been cited globally, as determined from a particular bibliographic information source on a particular date."@en .

:GrantApplication a owl:Class ;
	rdfs:label "GrantApplication"@en ;
	rdfs:subClassOf :Work ;
	rdfs:comment "A formal written request for financial support from a grant-giving body in support of a project, for example an academic research project.  (See also cito:CaseForSupport.)"@en .

:GrantApplicationDocument a owl:Class ;
	rdfs:label "GrantApplicationDocument"@en ;
	rdfs:subClassOf :Document ;
	rdfs:comment "An Expression of a Grant Application. (Usually associated with a Case For Support Document.)"@en .

:Image a owl:Class ;
	rdfs:label "Image"@en ;
	rdfs:subClassOf :Work ;
	rdfs:comment "A visual representation other than text, including all types of cito:MovingImage and cito:StillImage, subclass terms that should be used in preference to cito:Image."@en .

:InTextCitationCount a owl:Class ;
	rdfs:label "InTextCitationCount"@en ;
	rdfs:subClassOf owl:Thing ;
	owl:disjointWith core:Expression , core:Manifestation , core:Work ;
	rdfs:comment "The number of times a cited Work has been cited within the text of a citing Work."@en .

:InstructionalWork a owl:Class ;
	rdfs:label "InstructionalWork"@en ;
	rdfs:subClassOf :Work ;
	rdfs:comment "A Work created for the purpose of education or instruction, such as a  text book, lecture, tutorial or instruction manual."@en .

:Journal a owl:Class ;
	rdfs:label "Journal" ;
	rdfs:subClassOf :Periodical ;
	rdfs:comment "A scholarly Periodical primarily devoted to the publication of original Research Papers."@en .

:JournalArticle a owl:Class ;
	rdfs:label "JournalArticle"@en ;
	rdfs:subClassOf :JournalItem ;
	rdfs:comment "A Research Paper, Opinion, Proposition or Review published in a scholarly Journal."@en .

:JournalIssue a owl:Class ;
	rdfs:label "JournalIssue" ;
	rdfs:subClassOf :PeriodicalIssue ;
	rdfs:comment "A particular published  issue of a Journal, one or more of which will constitute a volume of the Journal."@en .

:JournalItem a owl:Class ;
	rdfs:label "JournalItem"@en ;
	rdfs:subClassOf :PeriodicalItem ;
	rdfs:comment "An item in scholarly Journal, for example an Editorial, NewsItem,  Research Paper or Review."@en .

:Letter a owl:Class ;
	rdfs:label "Letter"@en ;
	rdfs:subClassOf :Document ;
	rdfs:comment "A Personal Communication of a personal or professional nature between individuals and/or representatives of corporate bodies, typically in written or printed form and usually transmitted by the postal service or published in a Periodical.  In the latter case, the letter is typically addressed to the editor and comments on or discussed an item previously published by that periodical, or of interest to its readership."@en .

:Magazine a owl:Class ;
	rdfs:label "Magazine" ;
	rdfs:subClassOf :Periodical ;
	rdfs:comment "A periodical, usually devoted to a particular topic or domain of interest, and usually published weekly or monthly, consisting primarily of  non-peer reviewed Editorials, journalistic NewsItems and more substantive Articles, Reviews, BookReviews and Discussions concerning current or recent events and publications, and matters of interest to the domain served by the Magazine.  [Some scientific Journals, notably \"Science\" and \"Nature\", also secondarily serve as science magazines by containing substantive editorials and news reports on vital or controversial issues]."@en .

:MagazineArticle a owl:Class ;
	rdfs:label "MagazineArticle"@en ;
	rdfs:subClassOf :PeriodicalItem ;
	rdfs:comment "An article published in a Magazine, that is typically not peer-reviewed."@en .

:MagazineIssue a owl:Class ;
	rdfs:label "MagazineIssue" ;
	rdfs:subClassOf :PeriodicalIssue ;
	rdfs:comment "A particular published  issue of a Magazine, identified by date, and sometimes also by place (e.g. \"European edition\") or language (e.g. \"Spanish edition\")."@en .

:Manifestation a owl:Class ;
	rdfs:label "Manifestation"@en ;
	rdfs:subClassOf core:Manifestation ;
	owl:disjointWith :Work ;
	rdfs:comment "As defined by FRBR (http://www.ifla.org/VII/s13/frbr/frbr1.htm), a Manifestation of an Expression of a Work defines its particular embodiment. cito:Manifestation specifically applies to electronic (digital) as well as to physical Manifestations of Expressions.  Examples of different Manifestations of a single 'version of record' Expression of a scholarly Work include an Article in a print Journal, the on-line version of that article as an HTML Web Page, and the downloadable PDF version of the same article, which can be seen as alternate 'containers' or 'channels' for the same information."@en .

:Manuscript a owl:Class ;
	rdfs:label "Manuscript"@en ;
	rdfs:subClassOf :Document ;
	rdfs:comment "A textual Work prepared by hand, such as a typescript or word-processed pre-publication draft of a Research Paper or a Report, or a Work not otherwise reproduced in multiple copies. [cito:Manuscript is not intended to describe a handwritten historical document on paper or parchment, for which the distinction between Expression, Manifestation and Copy becomes blurred.]."@en .

:Metadata a owl:Class ;
	rdfs:label "Metadata"@en ;
	rdfs:subClassOf :Work ;
	rdfs:comment "A separate Work that provides information describing one or more characteristics of another Work or of an Expression of that Work."@en .

:MinimalInformationStandard a owl:Class ;
	rdfs:label "MinimalInformationStandard"@en ;
	rdfs:subClassOf :Specification ;
	rdfs:comment "A metadata standard specifying items to be included when creating metadata describing a dataset of a particular type, or when creating a structured digital abstract summarizing the main findings of an article or report in a particular domain of interest, thereby ensuring adequate descriptive information is recorded for subsequent resource discovery and/or interpretation of the information described." .

:Model a owl:Class ;
	rdfs:label "Model"@en ;
	rdfs:subClassOf :Work ;
	rdfs:comment "A mathematical, graphical or physical representation of some physical reality, conceptual idea or theoretical construct."@en .

:MovingImage a owl:Class ;
	rdfs:label "MovingImage"@en ;
	rdfs:subClassOf :Image ;
	owl:disjointWith :StillImage ;
	rdfs:comment "A moving display, either generated dynamically by a computer program or formed from a series of pre-recorded still images imparting an impression of motion when shown in succession.  Examples include animations, movies, videos, and computational simulations. A MovingImage may be accompanied by a synchronized soundtrack."@en .

:NewsItem a owl:Class ;
	rdfs:label "NewsItem"@en ;
	rdfs:subClassOf :Work ;
	rdfs:comment "An item of news."@en .

:Newspaper a owl:Class ;
	rdfs:label "Newspaper" ;
	rdfs:subClassOf :Periodical ;
	rdfs:comment "A non-peer reviewed Periodical, usually published daily or weekly, consisting primarily of Editorials and News Items concerning current or recent events and matters of public interest."@en .

:NewspaperArticle a owl:Class ;
	rdfs:label "NewspaperArticle" ;
	rdfs:subClassOf :PeriodicalItem ;
	rdfs:comment "An article writen by a journalist and published in a Newspaper."@en .

:NewspaperIssue a owl:Class ;
	rdfs:label "NewspaperIssue" ;
	rdfs:subClassOf :PeriodicalIssue ;
	rdfs:comment "A particular published  issue of a Newspaper, identified by date, and sometimes also by place or time (e.g. \"Late London Edition\")."@en .

:OnlineFile a owl:Class ;
	rdfs:label "OnlineFile"@en ;
	rdfs:subClassOf :ComputerFile ;
	rdfs:comment "A Computer File stored on a computer attached to the Internet, available for viewing in a Web browser or for electronic transfer ('uploading' or 'downloading') to a second computer across the Internet." .

:Ontology a owl:Class ;
	rdfs:label "Ontology"@en ;
	rdfs:subClassOf :Specification ;
	rdfs:comment "A formal representation of a set of concepts within a domain of knowledge, and the relationships between those concepts."@en .

:Opinion a owl:Class ;
	rdfs:label "Opinion"@en ;
	rdfs:subClassOf :Work ;
	rdfs:comment "An expression of a personal or professional opinion on an issue or topic."@en .

:Patent a owl:Class ;
	rdfs:label "Patent"@en ;
	rdfs:subClassOf :Specification ;
	rdfs:comment "A formal disclosure of a new invention approved by a government, made to record registration of intellectual property rights, and giving exclusive rights to the inventor or assignee to manufacture, use, licence or sell the invention for a certain number of years."@en .

:PatentApplication a owl:Class ;
	rdfs:label "PatentApplication"@en ;
	rdfs:subClassOf :Specification ;
	rdfs:comment "A formal disclosure of a new invention, made in application for a Patent."@en .

:PatentApplicationDocument a owl:Class ;
	rdfs:label "PatentApplicationDocument"@en ;
	rdfs:subClassOf :Document ;
	rdfs:comment "The physical or electronic Expression of a PatentApplication."@en .

:PatentDocument a owl:Class ;
	rdfs:label "PatentDocument"@en ;
	rdfs:subClassOf :Document ;
	rdfs:comment "The physical or electronic Expression of a Patent."@en .

:Periodical a owl:Class ;
	rdfs:label "Periodical" ;
	rdfs:subClassOf :Expression ;
	rdfs:comment "A publication issued on a regular and ongoing basis, each issue comprising separate Editorials, Articles, NewsItems and/or other writings."@en .

:PeriodicalIssue a owl:Class ;
	rdfs:label "PeriodicalIssue" ;
	rdfs:subClassOf :Document ;
	rdfs:comment "A particular issue of a Periodical, identified and distinguished from other issues of the same publication by date and/or issue number and/or volume number, and comprising separate Editorials, Articles, NewsItems and/or other writings."@en .

:PeriodicalItem a owl:Class ;
	rdfs:label "PeriodicalItem" ;
	rdfs:subClassOf :Document ;
	rdfs:comment "A piece of writing published in a Periodical, typically accompanied by other items by different authors."@en .

:PersonalCommunication a owl:Class ;
	rdfs:label "PersonalCommunication"@en ;
	rdfs:subClassOf :Expression ;
	rdfs:comment "Information communicated personally from one individual to one or more another persons or organizations."@en .

:Preprint a owl:Class ;
	rdfs:label "Preprint"@en ;
	rdfs:subClassOf :Document ;
	rdfs:comment "An author's original scholarly work as submitted to and/or accepted by a Journal for publication.  [For the version of the article published by the Journal and forming the 'version of record', use cito:JournalArticle.  See also cito:Manuscript]"@en .

:Presentation a owl:Class ;
	rdfs:label "Presentation"@en ;
	rdfs:subClassOf :Expression ;
	rdfs:comment "A set of images of text and/or pictures used when communicating ideas or research results to an audience at a meeting, conference, symposium, seminar, lecture, workshop or other gatherings."@en .

:PressRelease a owl:Class ;
	rdfs:label "PressRelease"@en ;
	rdfs:subClassOf :Document ;
	rdfs:comment "A News Item published by an organization to provide information to journalists."@en .

:PrintObject a owl:Class ;
	rdfs:label "PrintObject"@en ;
	rdfs:subClassOf :Manifestation ;
	rdfs:comment "A Manifestation of information in physical printed form, typically on paper."@en .

:ProjectMetadata a owl:Class ;
	rdfs:label "ProjectMetadata"@en ;
	rdfs:subClassOf :Metadata ;
	rdfs:comment "Metadata describing the project that led to the creation of the Work, for example the project name, project institution and project funding information."@en .

:Proposition a owl:Class ;
	rdfs:label "Proposition"@en ;
	rdfs:subClassOf :Work ;
	rdfs:comment "A proposal or proposition of a new conceptualization, hypothesis, idea or theory."@en .

:ReferenceWork a owl:Class ;
	rdfs:label "ReferenceWork"@en ;
	rdfs:subClassOf :Work ;
	rdfs:comment "A work  to which people refer for authoritative factual information, such as a dictionary, encyclopaedia, handbook or field guide, or certain types of informative web page, e.g. an institutional, research group or project home page."@en .

:Report a owl:Class ;
	rdfs:label "Report"@en ;
	rdfs:subClassOf :Work ;
	rdfs:comment "A formal factual, methodological, statistical, technical or research report issued by an individual, group, agency, government body or other institution."@en .

:ReportDocument a owl:Class ;
	rdfs:label "ReportDocument"@en ;
	rdfs:subClassOf :Document ;
	rdfs:comment "The embodiment of a report, usually in printed form. (Use when the Report is not expressed in a Book, Book Section, Journal Item or other more specific form of Expression.)"@en .

:ReportingStandard a owl:Class ;
	rdfs:label "ReportingStandard"@en ;
	rdfs:subClassOf :Specification ;
	rdfs:comment "A set of recommendations for the minimum reporting requirements to be employed when reporting a particular type of investigation or project, for example a randomized clinical trial, that may involve a checklist and a flow diagram, and that offers a standard way for authors to prepare complete and transparent reports of their findings, and aids their critical appraisal and interpretation of their data."@en .

:ResearchPaper a owl:Class ;
	rdfs:label "ResearchPaper"@en ;
	rdfs:subClassOf :Work ;
	rdfs:comment "A report of original research findings."@en .

:Review a owl:Class ;
	rdfs:label "Review"@en ;
	rdfs:subClassOf :Work ;
	rdfs:comment "A scholarly review of others' work."@en .

:Software a owl:Class ;
	rdfs:label "Software"@en ;
	rdfs:subClassOf :Expression ;
	rdfs:comment "A computer program in source or compiled form, employing one or more Algorithms to execute a particular task."@en .

:Specification a owl:Class ;
	rdfs:label "Specification"@en ;
	rdfs:subClassOf :Work ;
	rdfs:comment "An explicit description of, or set of requirements to be satisfied by a material, product resource, service or standard."@en .

:Spreadsheet a owl:Class ;
	rdfs:label "Spreadsheet"@en ;
	rdfs:subClassOf :Expression ;
	rdfs:comment "An electronic form of data storage that displays a grid of rows and columns, in which each cell can contain alphanumeric text, a numeric value, or a formula that defines how the content of that cell is to be calculated from the content of any other cell or cells."@en .

:StandardOperatingProcedure a owl:Class ;
	rdfs:label "StandardOperatingProcedure" ;
	rdfs:subClassOf :Specification ;
	rdfs:comment "Clear and detailed written instructions of a prescribed step-by-step procedure to be routinely followed and decisions to be made when undertaking a specific task, process or function, to achieve consistent performance, ensure safety and/or assure data quality.  (Commonly abbreviated \"SOP\".)"@en .

:StillImage a owl:Class ;
	rdfs:label "StillImage"@en ;
	rdfs:subClassOf :Image ;
	rdfs:comment "A recorded static visual representation. This class includes diagrams, drawings, graphs, graphic designs, plans, maps, photographs and prints."@en .

:SupplementaryInformation a owl:Class ;
	rdfs:label "SupplementaryInformation"@en ;
	rdfs:subClassOf :Document ;
	rdfs:comment "A document accompanying a published JournalArticle, containing additional information of relevance to the article, typically available from the publisher's web site via the JournalArticle itself."@en .

:Table a owl:Class ;
	rdfs:label "Table"@en ;
	rdfs:subClassOf :Expression ;
	rdfs:comment "A graphical means of presenting data in a grid of rows and columns, within which the cells usually contain alphanumeric text or numeric values.  If included within a publication, a table typically appearing unaligned with the main body of text, with its own descriptive title."@en .

:Taxonomy a owl:Class ;
	rdfs:label "Taxonomy"@en ;
	rdfs:subClassOf :Specification ;
	rdfs:comment "A classification arranged in a hierarchical structure of classes and subclasses, showing parent-child isA relationships, or broader_than - narrower_than relationships."@en .

:TechnicalStandard a owl:Class ;
	rdfs:label "TechnicalStandard"@en ;
	rdfs:subClassOf :Specification ;
	rdfs:comment "An official or public specification of or requirement for a technical method, practice, process or protocol involved in, for example, manufacturing, computation, electronic communication, or digital media."@en .

:Thesis a owl:Class ;
	rdfs:label "Thesis"@en ;
	rdfs:subClassOf :Work ;
	rdfs:comment "A Work consisting of formal presentations of research outputs submitted for examination in completion of a course of study at an institution of higher education, to fulfil the requirements for an academic degree. [For the alternative meaning of the word \"Thesis\", namely a formulation of a concept, hypothesis, idea, point of view or theory presented for review and/or discussion, use cito:Proposition.]"@en .

:WebContent a owl:Class ;
	rdfs:label "WebContent"@en ;
	rdfs:subClassOf :Expression ;
	rdfs:comment "Information prepared specifically and primarily for manifestation in a WebPage, comprising Text, Images, Tables and/or other Works." .

:WebPage a owl:Class ;
	rdfs:label "WebPage"@en ;
	rdfs:subClassOf :Manifestation ;
	rdfs:comment "A Manifestation of information on the World Wide Web, usually structured in HTML or XHTML format, identified by a Uniform Resource Identifier (URI), and made accessible to a user by means of the Hypertext Transport Protocol in a Web browser window.  Special software may enable a WebPage to be or to include a Blog or a Wiki.  Several interlinked WebPages hosted together on a Web server and accessed through a single domain name or IP address constitute a Web site."@en .

:WikiEntry a owl:Class ;
	rdfs:label "WikiEntry"@en ;
	rdfs:subClassOf :WebContent ;
	rdfs:comment "Information manifested in a Wiki, a type of WebPage that enables easy editing, usually maintained collaboratively by a project team, group or community to accumulate related information for shared use by the group, and for publication."@en .

:Work a owl:Class ;
	rdfs:label "Work"@en ;
	rdfs:subClassOf core:Work ;
	rdfs:comment "As defined by FRBR (http://www.ifla.org/VII/s13/frbr/frbr1.htm), a Work is a distinct intellectual or artistic creation - an abstract entity that is recognised through its various expressions.  In CiTO, the definition of Work is restricted to Works that cite or are cited, primarily works of scholarship that contain bibliographic references, and excludes artistic works such as plays or photographs that do not.  For this reason cito:Work is a subclass of frbr:Work.  Consequently, cito:Expression and cito:Manifestation are also made subclasses of their respective FRBR classes."@en .

:Workflow a owl:Class ;
	rdfs:label "Workflow"@en ;
	rdfs:subClassOf :Specification ;
	rdfs:comment "A recorded sequence of connected steps, which may be automated, specifying a reliably repeatable sequence of operations to be undertaken when conducting a particular project, for example an in silico investigation that extracts and processes information from a number of bioinformatics databases."@en .

:WorkingPaper a owl:Class ;
	rdfs:label "WorkingPaper"@en ;
	rdfs:subClassOf :Work ;
	rdfs:comment "An unpublished paper, usually circulated privately among a small group of peers, to provide information or with a request for editorial improvement."@en .

core:Expression a owl:Class ;
	rdfs:label "expression"@en ;
	owl:disjointWith core:Manifestation , core:Work ;
	rdfs:isDefinedBy "http://purl.org/vocab/frbr/core"^^xsd:anyURI ;
	rdfs:comment "This class corresponds to the FRBR Group One entity 'Expression'."@en .

core:Manifestation a owl:Class ;
	rdfs:label "manifestation"@en ;
	owl:disjointWith core:Work ;
	rdfs:isDefinedBy "http://purl.org/vocab/frbr/core"^^xsd:anyURI ;
	rdfs:comment "This class corresponds to the FRBR Group One entity 'Manifestation'."@en .

core:Work a owl:Class ;
	rdfs:label "work"@en ;
	rdfs:isDefinedBy "http://purl.org/vocab/frbr/core"^^xsd:anyURI ;
	rdfs:comment "This class corresponds to the FRBR Group One entity 'Work'."@en .

owl:Thing a owl:Class .

_:node171hnm0dix1 a owl:AllDisjointClasses ;
	owl:members _:node171hnm0dix2 .

_:node171hnm0dix2 rdf:first :Journal ;
	rdf:rest _:node171hnm0dix3 .

_:node171hnm0dix3 rdf:first :Magazine ;
	rdf:rest _:node171hnm0dix4 .

_:node171hnm0dix4 rdf:first :Newspaper ;
	rdf:rest rdf:nil .

_:node171hnm0dix5 a owl:AllDisjointClasses ;
	owl:members _:node171hnm0dix6 .

_:node171hnm0dix6 rdf:first :Biography ;
	rdf:rest _:node171hnm0dix7 .

_:node171hnm0dix7 rdf:first :CaseForSupport ;
	rdf:rest _:node171hnm0dix8 .

_:node171hnm0dix8 rdf:first :Dataset ;
	rdf:rest _:node171hnm0dix9 .

_:node171hnm0dix9 rdf:first :GrantApplication ;
	rdf:rest _:node171hnm0dix10 .

_:node171hnm0dix10 rdf:first :Image ;
	rdf:rest _:node171hnm0dix11 .

_:node171hnm0dix11 rdf:first :InstructionalWork ;
	rdf:rest _:node171hnm0dix12 .

_:node171hnm0dix12 rdf:first :Metadata ;
	rdf:rest _:node171hnm0dix13 .

_:node171hnm0dix13 rdf:first :Model ;
	rdf:rest _:node171hnm0dix14 .

_:node171hnm0dix14 rdf:first :NewsItem ;
	rdf:rest _:node171hnm0dix15 .

_:node171hnm0dix15 rdf:first :Opinion ;
	rdf:rest _:node171hnm0dix16 .

_:node171hnm0dix16 rdf:first :Proposition ;
	rdf:rest _:node171hnm0dix17 .

_:node171hnm0dix17 rdf:first :ReferenceWork ;
	rdf:rest _:node171hnm0dix18 .

_:node171hnm0dix18 rdf:first :Report ;
	rdf:rest _:node171hnm0dix19 .

_:node171hnm0dix19 rdf:first :ResearchPaper ;
	rdf:rest _:node171hnm0dix20 .

_:node171hnm0dix20 rdf:first :Review ;
	rdf:rest _:node171hnm0dix21 .

_:node171hnm0dix21 rdf:first :Specification ;
	rdf:rest _:node171hnm0dix22 .

_:node171hnm0dix22 rdf:first :Thesis ;
	rdf:rest _:node171hnm0dix23 .

_:node171hnm0dix23 rdf:first :WorkingPaper ;
	rdf:rest rdf:nil .

_:node171hnm0dix24 a owl:AllDisjointClasses ;
	owl:members _:node171hnm0dix25 .

_:node171hnm0dix25 rdf:first :Algorithm ;
	rdf:rest _:node171hnm0dix26 .

_:node171hnm0dix26 rdf:first :AuthorityFile ;
	rdf:rest _:node171hnm0dix27 .

_:node171hnm0dix27 rdf:first :Catalog ;
	rdf:rest _:node171hnm0dix28 .

_:node171hnm0dix28 rdf:first :ClinicalTrialDesign ;
	rdf:rest _:node171hnm0dix29 .

_:node171hnm0dix29 rdf:first :ExperimentalProtocol ;
	rdf:rest _:node171hnm0dix30 .

_:node171hnm0dix30 rdf:first :MinimalInformationStandard ;
	rdf:rest _:node171hnm0dix31 .

_:node171hnm0dix31 rdf:first :Ontology ;
	rdf:rest _:node171hnm0dix32 .

_:node171hnm0dix32 rdf:first :Patent ;
	rdf:rest _:node171hnm0dix33 .

_:node171hnm0dix33 rdf:first :PatentApplication ;
	rdf:rest _:node171hnm0dix34 .

_:node171hnm0dix34 rdf:first :ReportingStandard ;
	rdf:rest _:node171hnm0dix35 .

_:node171hnm0dix35 rdf:first :StandardOperatingProcedure ;
	rdf:rest _:node171hnm0dix36 .

_:node171hnm0dix36 rdf:first :Taxonomy ;
	rdf:rest _:node171hnm0dix37 .

_:node171hnm0dix37 rdf:first :TechnicalStandard ;
	rdf:rest _:node171hnm0dix38 .

_:node171hnm0dix38 rdf:first :Workflow ;
	rdf:rest rdf:nil .

_:node171hnm0dix39 a owl:AllDisjointProperties ;
	owl:members _:node171hnm0dix40 .

_:node171hnm0dix40 rdf:first :globalCountDate ;
	rdf:rest _:node171hnm0dix41 .

_:node171hnm0dix41 rdf:first :globalCountValue ;
	rdf:rest _:node171hnm0dix42 .

_:node171hnm0dix42 rdf:first :inTextCountValue ;
	rdf:rest _:node171hnm0dix43 .

_:node171hnm0dix43 rdf:first :peerReviewed ;
	rdf:rest _:node171hnm0dix44 .

_:node171hnm0dix44 rdf:first :unpublished ;
	rdf:rest rdf:nil .

_:node171hnm0dix45 a owl:AllDisjointClasses ;
	owl:members _:node171hnm0dix46 .

_:node171hnm0dix46 rdf:first :Database ;
	rdf:rest _:node171hnm0dix47 .

_:node171hnm0dix47 rdf:first :Document ;
	rdf:rest _:node171hnm0dix48 .

_:node171hnm0dix48 rdf:first :Figure ;
	rdf:rest _:node171hnm0dix49 .

_:node171hnm0dix49 rdf:first :Periodical ;
	rdf:rest _:node171hnm0dix50 .

_:node171hnm0dix50 rdf:first :PersonalCommunication ;
	rdf:rest _:node171hnm0dix51 .

_:node171hnm0dix51 rdf:first :Presentation ;
	rdf:rest _:node171hnm0dix52 .

_:node171hnm0dix52 rdf:first :Software ;
	rdf:rest _:node171hnm0dix53 .

_:node171hnm0dix53 rdf:first :Spreadsheet ;
	rdf:rest _:node171hnm0dix54 .

_:node171hnm0dix54 rdf:first :Table ;
	rdf:rest _:node171hnm0dix55 .

_:node171hnm0dix55 rdf:first :WebContent ;
	rdf:rest rdf:nil .

_:node171hnm0dix56 a owl:AllDisjointClasses ;
	owl:members _:node171hnm0dix57 .

_:node171hnm0dix57 rdf:first :Editorial ;
	rdf:rest _:node171hnm0dix58 .

_:node171hnm0dix58 rdf:first :JournalItem ;
	rdf:rest _:node171hnm0dix59 .

_:node171hnm0dix59 rdf:first :MagazineArticle ;
	rdf:rest _:node171hnm0dix60 .

_:node171hnm0dix60 rdf:first :NewspaperArticle ;
	rdf:rest rdf:nil .

_:node171hnm0dix61 a owl:AllDisjointClasses ;
	owl:members _:node171hnm0dix62 .

_:node171hnm0dix62 rdf:first :ComputerFile ;
	rdf:rest _:node171hnm0dix63 .

_:node171hnm0dix63 rdf:first :PrintObject ;
	rdf:rest _:node171hnm0dix64 .

_:node171hnm0dix64 rdf:first :WebPage ;
	rdf:rest rdf:nil .

_:node171hnm0dix65 a owl:AllDisjointProperties ;
	owl:members _:node171hnm0dix66 .

_:node171hnm0dix66 rdf:first :cites ;
	rdf:rest _:node171hnm0dix67 .

_:node171hnm0dix67 rdf:first :globalCitationFrequency ;
	rdf:rest _:node171hnm0dix68 .

_:node171hnm0dix68 rdf:first :globalCountSource ;
	rdf:rest _:node171hnm0dix69 .

_:node171hnm0dix69 rdf:first :inTextCitationFrequency ;
	rdf:rest _:node171hnm0dix70 .

_:node171hnm0dix70 rdf:first :inTextCitationTarget ;
	rdf:rest _:node171hnm0dix71 .

_:node171hnm0dix71 rdf:first :isCitedBy ;
	rdf:rest _:node171hnm0dix72 .

_:node171hnm0dix72 rdf:first :isEmbodiedIn ;
	rdf:rest _:node171hnm0dix73 .

_:node171hnm0dix73 rdf:first :isEmbodimentOf ;
	rdf:rest _:node171hnm0dix74 .

_:node171hnm0dix74 rdf:first :isRealizationOf ;
	rdf:rest _:node171hnm0dix75 .

_:node171hnm0dix75 rdf:first :isRealizedThrough ;
	rdf:rest rdf:nil .

_:node171hnm0dix76 a owl:AllDisjointClasses ;
	owl:members _:node171hnm0dix77 .

_:node171hnm0dix77 rdf:first :BibliographicMetadata ;
	rdf:rest _:node171hnm0dix78 .

_:node171hnm0dix78 rdf:first :CitationMetadata ;
	rdf:rest _:node171hnm0dix79 .

_:node171hnm0dix79 rdf:first :EntityMetadata ;
	rdf:rest _:node171hnm0dix80 .

_:node171hnm0dix80 rdf:first :ProjectMetadata ;
	rdf:rest rdf:nil .

_:node171hnm0dix81 a owl:AllDisjointClasses ;
	owl:members _:node171hnm0dix82 .

_:node171hnm0dix82 rdf:first :JournalIssue ;
	rdf:rest _:node171hnm0dix83 .

_:node171hnm0dix83 rdf:first :MagazineIssue ;
	rdf:rest _:node171hnm0dix84 .

_:node171hnm0dix84 rdf:first :NewspaperIssue ;
	rdf:rest rdf:nil .

_:node171hnm0dix85 a owl:AllDisjointClasses ;
	owl:members _:node171hnm0dix86 .

_:node171hnm0dix86 rdf:first :Abstract ;
	rdf:rest _:node171hnm0dix87 .

_:node171hnm0dix87 rdf:first :Book ;
	rdf:rest _:node171hnm0dix88 .

_:node171hnm0dix88 rdf:first :BookSection ;
	rdf:rest _:node171hnm0dix89 .

_:node171hnm0dix89 rdf:first :CaseForSupportDocument ;
	rdf:rest _:node171hnm0dix90 .

_:node171hnm0dix90 rdf:first :ConferencePaper ;
	rdf:rest _:node171hnm0dix91 .

_:node171hnm0dix91 rdf:first :ConferencePoster ;
	rdf:rest _:node171hnm0dix92 .

_:node171hnm0dix92 rdf:first :ConferenceProceedings ;
	rdf:rest _:node171hnm0dix93 .

_:node171hnm0dix93 rdf:first :Email ;
	rdf:rest _:node171hnm0dix94 .

_:node171hnm0dix94 rdf:first :GrantApplicationDocument ;
	rdf:rest _:node171hnm0dix95 .

_:node171hnm0dix95 rdf:first :Letter ;
	rdf:rest _:node171hnm0dix96 .

_:node171hnm0dix96 rdf:first :Manuscript ;
	rdf:rest _:node171hnm0dix97 .

_:node171hnm0dix97 rdf:first :PatentApplicationDocument ;
	rdf:rest _:node171hnm0dix98 .

_:node171hnm0dix98 rdf:first :PatentDocument ;
	rdf:rest _:node171hnm0dix99 .

_:node171hnm0dix99 rdf:first :PeriodicalIssue ;
	rdf:rest _:node171hnm0dix100 .

_:node171hnm0dix100 rdf:first :PeriodicalItem ;
	rdf:rest _:node171hnm0dix101 .

_:node171hnm0dix101 rdf:first :Preprint ;
	rdf:rest _:node171hnm0dix102 .

_:node171hnm0dix102 rdf:first :PressRelease ;
	rdf:rest _:node171hnm0dix103 .

_:node171hnm0dix103 rdf:first :ReportDocument ;
	rdf:rest _:node171hnm0dix104 .

_:node171hnm0dix104 rdf:first :SupplementaryInformation ;
	rdf:rest rdf:nil .

_:node171hnm0dix105 a owl:AllDisjointClasses ;
	owl:members _:node171hnm0dix106 .

_:node171hnm0dix106 rdf:first :Journal ;
	rdf:rest _:node171hnm0dix107 .

_:node171hnm0dix107 rdf:first :Magazine ;
	rdf:rest _:node171hnm0dix108 .

_:node171hnm0dix108 rdf:first :Newspaper ;
	rdf:rest rdf:nil .

_:node171hnm0dix109 a owl:AllDisjointClasses ;
	owl:members _:node171hnm0dix110 .

_:node171hnm0dix110 rdf:first :Biography ;
	rdf:rest _:node171hnm0dix111 .

_:node171hnm0dix111 rdf:first :CaseForSupport ;
	rdf:rest _:node171hnm0dix112 .

_:node171hnm0dix112 rdf:first :Dataset ;
	rdf:rest _:node171hnm0dix113 .

_:node171hnm0dix113 rdf:first :GrantApplication ;
	rdf:rest _:node171hnm0dix114 .

_:node171hnm0dix114 rdf:first :Image ;
	rdf:rest _:node171hnm0dix115 .

_:node171hnm0dix115 rdf:first :InstructionalWork ;
	rdf:rest _:node171hnm0dix116 .

_:node171hnm0dix116 rdf:first :Metadata ;
	rdf:rest _:node171hnm0dix117 .

_:node171hnm0dix117 rdf:first :Model ;
	rdf:rest _:node171hnm0dix118 .

_:node171hnm0dix118 rdf:first :NewsItem ;
	rdf:rest _:node171hnm0dix119 .

_:node171hnm0dix119 rdf:first :Opinion ;
	rdf:rest _:node171hnm0dix120 .

_:node171hnm0dix120 rdf:first :Proposition ;
	rdf:rest _:node171hnm0dix121 .

_:node171hnm0dix121 rdf:first :ReferenceWork ;
	rdf:rest _:node171hnm0dix122 .

_:node171hnm0dix122 rdf:first :Report ;
	rdf:rest _:node171hnm0dix123 .

_:node171hnm0dix123 rdf:first :ResearchPaper ;
	rdf:rest _:node171hnm0dix124 .

_:node171hnm0dix124 rdf:first :Review ;
	rdf:rest _:node171hnm0dix125 .

_:node171hnm0dix125 rdf:first :Specification ;
	rdf:rest _:node171hnm0dix126 .

_:node171hnm0dix126 rdf:first :Thesis ;
	rdf:rest _:node171hnm0dix127 .

_:node171hnm0dix127 rdf:first :WorkingPaper ;
	rdf:rest rdf:nil .

_:node171hnm0dix128 a owl:AllDisjointClasses ;
	owl:members _:node171hnm0dix129 .

_:node171hnm0dix129 rdf:first :Algorithm ;
	rdf:rest _:node171hnm0dix130 .

_:node171hnm0dix130 rdf:first :AuthorityFile ;
	rdf:rest _:node171hnm0dix131 .

_:node171hnm0dix131 rdf:first :Catalog ;
	rdf:rest _:node171hnm0dix132 .

_:node171hnm0dix132 rdf:first :ClinicalTrialDesign ;
	rdf:rest _:node171hnm0dix133 .

_:node171hnm0dix133 rdf:first :ExperimentalProtocol ;
	rdf:rest _:node171hnm0dix134 .

_:node171hnm0dix134 rdf:first :MinimalInformationStandard ;
	rdf:rest _:node171hnm0dix135 .

_:node171hnm0dix135 rdf:first :Ontology ;
	rdf:rest _:node171hnm0dix136 .

_:node171hnm0dix136 rdf:first :Patent ;
	rdf:rest _:node171hnm0dix137 .

_:node171hnm0dix137 rdf:first :PatentApplication ;
	rdf:rest _:node171hnm0dix138 .

_:node171hnm0dix138 rdf:first :ReportingStandard ;
	rdf:rest _:node171hnm0dix139 .

_:node171hnm0dix139 rdf:first :StandardOperatingProcedure ;
	rdf:rest _:node171hnm0dix140 .

_:node171hnm0dix140 rdf:first :Taxonomy ;
	rdf:rest _:node171hnm0dix141 .

_:node171hnm0dix141 rdf:first :TechnicalStandard ;
	rdf:rest _:node171hnm0dix142 .

_:node171hnm0dix142 rdf:first :Workflow ;
	rdf:rest rdf:nil .

_:node171hnm0dix143 a owl:AllDisjointProperties ;
	owl:members _:node171hnm0dix144 .

_:node171hnm0dix144 rdf:first :globalCountDate ;
	rdf:rest _:node171hnm0dix145 .

_:node171hnm0dix145 rdf:first :globalCountValue ;
	rdf:rest _:node171hnm0dix146 .

_:node171hnm0dix146 rdf:first :inTextCountValue ;
	rdf:rest _:node171hnm0dix147 .

_:node171hnm0dix147 rdf:first :peerReviewed ;
	rdf:rest _:node171hnm0dix148 .

_:node171hnm0dix148 rdf:first :unpublished ;
	rdf:rest rdf:nil .

_:node171hnm0dix149 a owl:AllDisjointClasses ;
	owl:members _:node171hnm0dix150 .

_:node171hnm0dix150 rdf:first :Database ;
	rdf:rest _:node171hnm0dix151 .

_:node171hnm0dix151 rdf:first :Document ;
	rdf:rest _:node171hnm0dix152 .

_:node171hnm0dix152 rdf:first :Figure ;
	rdf:rest _:node171hnm0dix153 .

_:node171hnm0dix153 rdf:first :Periodical ;
	rdf:rest _:node171hnm0dix154 .

_:node171hnm0dix154 rdf:first :PersonalCommunication ;
	rdf:rest _:node171hnm0dix155 .

_:node171hnm0dix155 rdf:first :Presentation ;
	rdf:rest _:node171hnm0dix156 .

_:node171hnm0dix156 rdf:first :Software ;
	rdf:rest _:node171hnm0dix157 .

_:node171hnm0dix157 rdf:first :Spreadsheet ;
	rdf:rest _:node171hnm0dix158 .

_:node171hnm0dix158 rdf:first :Table ;
	rdf:rest _:node171hnm0dix159 .

_:node171hnm0dix159 rdf:first :WebContent ;
	rdf:rest rdf:nil .

_:node171hnm0dix160 a owl:AllDisjointClasses ;
	owl:members _:node171hnm0dix161 .

_:node171hnm0dix161 rdf:first :Editorial ;
	rdf:rest _:node171hnm0dix162 .

_:node171hnm0dix162 rdf:first :JournalItem ;
	rdf:rest _:node171hnm0dix163 .

_:node171hnm0dix163 rdf:first :MagazineArticle ;
	rdf:rest _:node171hnm0dix164 .

_:node171hnm0dix164 rdf:first :NewspaperArticle ;
	rdf:rest rdf:nil .

_:node171hnm0dix165 a owl:AllDisjointClasses ;
	owl:members _:node171hnm0dix166 .

_:node171hnm0dix166 rdf:first :ComputerFile ;
	rdf:rest _:node171hnm0dix167 .

_:node171hnm0dix167 rdf:first :PrintObject ;
	rdf:rest _:node171hnm0dix168 .

_:node171hnm0dix168 rdf:first :WebPage ;
	rdf:rest rdf:nil .

_:node171hnm0dix169 a owl:AllDisjointProperties ;
	owl:members _:node171hnm0dix170 .

_:node171hnm0dix170 rdf:first :cites ;
	rdf:rest _:node171hnm0dix171 .

_:node171hnm0dix171 rdf:first :globalCitationFrequency ;
	rdf:rest _:node171hnm0dix172 .

_:node171hnm0dix172 rdf:first :globalCountSource ;
	rdf:rest _:node171hnm0dix173 .

_:node171hnm0dix173 rdf:first :inTextCitationFrequency ;
	rdf:rest _:node171hnm0dix174 .

_:node171hnm0dix174 rdf:first :inTextCitationTarget ;
	rdf:rest _:node171hnm0dix175 .

_:node171hnm0dix175 rdf:first :isCitedBy ;
	rdf:rest _:node171hnm0dix176 .

_:node171hnm0dix176 rdf:first :isEmbodiedIn ;
	rdf:rest _:node171hnm0dix177 .

_:node171hnm0dix177 rdf:first :isEmbodimentOf ;
	rdf:rest _:node171hnm0dix178 .

_:node171hnm0dix178 rdf:first :isRealizationOf ;
	rdf:rest _:node171hnm0dix179 .

_:node171hnm0dix179 rdf:first :isRealizedThrough ;
	rdf:rest rdf:nil .

_:node171hnm0dix180 a owl:AllDisjointClasses ;
	owl:members _:node171hnm0dix181 .

_:node171hnm0dix181 rdf:first :BibliographicMetadata ;
	rdf:rest _:node171hnm0dix182 .

_:node171hnm0dix182 rdf:first :CitationMetadata ;
	rdf:rest _:node171hnm0dix183 .

_:node171hnm0dix183 rdf:first :EntityMetadata ;
	rdf:rest _:node171hnm0dix184 .

_:node171hnm0dix184 rdf:first :ProjectMetadata ;
	rdf:rest rdf:nil .

_:node171hnm0dix185 a owl:AllDisjointClasses ;
	owl:members _:node171hnm0dix186 .

_:node171hnm0dix186 rdf:first :JournalIssue ;
	rdf:rest _:node171hnm0dix187 .

_:node171hnm0dix187 rdf:first :MagazineIssue ;
	rdf:rest _:node171hnm0dix188 .

_:node171hnm0dix188 rdf:first :NewspaperIssue ;
	rdf:rest rdf:nil .

_:node171hnm0dix189 a owl:AllDisjointClasses ;
	owl:members _:node171hnm0dix190 .

_:node171hnm0dix190 rdf:first :Abstract ;
	rdf:rest _:node171hnm0dix191 .

_:node171hnm0dix191 rdf:first :Book ;
	rdf:rest _:node171hnm0dix192 .

_:node171hnm0dix192 rdf:first :BookSection ;
	rdf:rest _:node171hnm0dix193 .

_:node171hnm0dix193 rdf:first :CaseForSupportDocument ;
	rdf:rest _:node171hnm0dix194 .

_:node171hnm0dix194 rdf:first :ConferencePaper ;
	rdf:rest _:node171hnm0dix195 .

_:node171hnm0dix195 rdf:first :ConferencePoster ;
	rdf:rest _:node171hnm0dix196 .

_:node171hnm0dix196 rdf:first :ConferenceProceedings ;
	rdf:rest _:node171hnm0dix197 .

_:node171hnm0dix197 rdf:first :Email ;
	rdf:rest _:node171hnm0dix198 .

_:node171hnm0dix198 rdf:first :GrantApplicationDocument ;
	rdf:rest _:node171hnm0dix199 .

_:node171hnm0dix199 rdf:first :Letter ;
	rdf:rest _:node171hnm0dix200 .

_:node171hnm0dix200 rdf:first :Manuscript ;
	rdf:rest _:node171hnm0dix201 .

_:node171hnm0dix201 rdf:first :PatentApplicationDocument ;
	rdf:rest _:node171hnm0dix202 .

_:node171hnm0dix202 rdf:first :PatentDocument ;
	rdf:rest _:node171hnm0dix203 .

_:node171hnm0dix203 rdf:first :PeriodicalIssue ;
	rdf:rest _:node171hnm0dix204 .

_:node171hnm0dix204 rdf:first :PeriodicalItem ;
	rdf:rest _:node171hnm0dix205 .

_:node171hnm0dix205 rdf:first :Preprint ;
	rdf:rest _:node171hnm0dix206 .

_:node171hnm0dix206 rdf:first :PressRelease ;
	rdf:rest _:node171hnm0dix207 .

_:node171hnm0dix207 rdf:first :ReportDocument ;
	rdf:rest _:node171hnm0dix208 .

_:node171hnm0dix208 rdf:first :SupplementaryInformation ;
	rdf:rest rdf:nil .
