@prefix dc:    <http://purl.org/dc/elements/1.1/> .
@prefix :      <http://courseware.rkbexplorer.com/ontologies/courseware#> .
@prefix rdfs:  <http://www.w3.org/2000/01/rdf-schema#> .
@prefix dct:   <http://purl.org/dc/terms/> .
@prefix akt:   <http://www.aktors.org/ontology/portal#> .
@prefix xsd:   <http://www.w3.org/2001/XMLSchema#> .
@prefix owl:   <http://www.w3.org/2002/07/owl#> .
@prefix rdf:   <http://www.w3.org/1999/02/22-rdf-syntax-ns#> .
@prefix daml:  <http://www.daml.org/2001/03/daml+oil#> .

:detailed-description
        a                 owl:DatatypeProperty ;
        rdfs:comment      "A detailed description of the content conveyed within the course" ;
        rdfs:domain       :Course ;
        rdfs:isDefinedBy  <http://courseware.rkbexplorer.com/ontologies/courseware> ;
        rdfs:label        "detailed description" ;
        rdfs:range        xsd:string .

:has-instructor  a        owl:ObjectProperty ;
        rdfs:comment      "A person delivering tuition as part of the course" ;
        rdfs:domain       :Course ;
        rdfs:isDefinedBy  <http://courseware.rkbexplorer.com/ontologies/courseware> ;
        rdfs:label        "has instructor" ;
        rdfs:range        akt:Person .

:total-hours-engagement
        a                 owl:DatatypeProperty ;
        rdfs:comment      "The total number of hours of engagement while undertaking this course" ;
        rdfs:domain       :Course ;
        rdfs:isDefinedBy  <http://courseware.rkbexplorer.com/ontologies/courseware> ;
        rdfs:label        "total hours of engagement" ;
        rdfs:range        xsd:float .

:has-language  a          owl:DatatypeProperty ;
        rdfs:comment      "The language in which an item of abstract information is written, expressed or delivered." ;
        rdfs:domain       akt:Abstract-Information ;
        rdfs:isDefinedBy  <http://courseware.rkbexplorer.com/ontologies/courseware> ;
        rdfs:label        "has language" ;
        rdfs:range        xsd:language .

:course-duration  a       owl:DatatypeProperty ;
        rdfs:comment      "The total duration of the course (in hours)" ;
        rdfs:domain       :Course ;
        rdfs:isDefinedBy  <http://courseware.rkbexplorer.com/ontologies/courseware> ;
        rdfs:label        "course duration" ;
        rdfs:range        xsd:integer .

<http://courseware.rkbexplorer.com/ontologies/courseware>
        a                owl:Ontology ;
        rdfs:label       "ReSIST Courseware Ontology" ;
        dc:created       "2006-05-03" ;
        dc:creator       "Ian Millard" , "Bene Rodriguez" ;
        dc:description   "The ReSIST Courseware Ontology represents the various eduacational courses and resources within the ReSIST project"@en ;
        dc:title         "ReSIST Courseware Ontology"@en ;
        owl:imports      <http://www.aktors.org/ontology/portal> ;
        owl:versionInfo  "0.1" .

:Assessment-Method  a     owl:Class ;
        rdfs:comment      "A method by which a student is assessed; instances of this class may include examination, coursework, etc." ;
        rdfs:isDefinedBy  <http://courseware.rkbexplorer.com/ontologies/courseware> ;
        rdfs:label        "Assessment Method" .

:has-infrastructure-requirement
        a                 owl:ObjectProperty ;
        rdfs:comment      "An infrastructure requirement that is needed to carry out the course" ;
        rdfs:domain       :Course ;
        rdfs:isDefinedBy  <http://courseware.rkbexplorer.com/ontologies/courseware> ;
        rdfs:label        "has infrastructure requirement" ;
        rdfs:range        akt:Technology .

:has-rights-description
        a                 owl:DatatypeProperty ;
        rdfs:comment      "Comments on the conditions of use of this learning resource." ;
        rdfs:domain       akt:Abstract-Information ;
        rdfs:isDefinedBy  <http://courseware.rkbexplorer.com/ontologies/courseware> ;
        rdfs:range        xsd:string .

:has-prerequisite  a      owl:ObjectProperty ;
        rdfs:domain       :Course ;
        rdfs:isDefinedBy  <http://courseware.rkbexplorer.com/ontologies/courseware> ;
        rdfs:label        "has pre-requisite" ;
        rdfs:range        :Pre-requisite .

:involves-organization
        a                 owl:ObjectProperty ;
        rdfs:comment      "The association of an organisation which is involved in delivering a course" ;
        rdfs:domain       :Course ;
        rdfs:isDefinedBy  <http://courseware.rkbexplorer.com/ontologies/courseware> ;
        rdfs:label        "involves organisation" ;
        rdfs:range        akt:Organization .

:course-objectives  a     owl:DatatypeProperty ;
        rdfs:comment      "The objectives of this course" ;
        rdfs:domain       :Course ;
        rdfs:isDefinedBy  <http://courseware.rkbexplorer.com/ontologies/courseware> ;
        rdfs:label        "course objectives" ;
        rdfs:range        xsd:string .

:Student-Interaction-Type
        a                 owl:Class ;
        rdfs:comment      "A type of interaction in which a student engages whilst undertaking a course; instances of this class may include lectures, laboratory sessions, and group or individual projects." ;
        rdfs:isDefinedBy  <http://courseware.rkbexplorer.com/ontologies/courseware> ;
        rdfs:label        "Student Interaction Type" .

:has-title  a               owl:DatatypeProperty ;
        rdfs:comment        "The title of this course" ;
        rdfs:domain         :Course ;
        rdfs:isDefinedBy    <http://courseware.rkbexplorer.com/ontologies/courseware> ;
        rdfs:label          "title" ;
        rdfs:range          xsd:string ;
        rdfs:subPropertyOf  rdfs:label .

:has-author  a            owl:ObjectProperty ;
        rdfs:comment      "A person which is involved with the creation of the course" ;
        rdfs:domain       :Course ;
        rdfs:isDefinedBy  <http://courseware.rkbexplorer.com/ontologies/courseware> ;
        rdfs:label        "has author" ;
        rdfs:range        akt:Generic-Agent .

:has-rights  a            owl:ObjectProperty ;
        rdfs:comment      "This property describes the intellectual property rights and conditions of use for this learning object. " ;
        rdfs:domain       akt:Abstract-Information ;
        rdfs:isDefinedBy  <http://courseware.rkbexplorer.com/ontologies/courseware> .

:has-student-interaction-type
        a                 owl:ObjectProperty ;
        rdfs:comment      "Identifies a course as having the prescribed interaction type" ;
        rdfs:domain       :Course ;
        rdfs:isDefinedBy  <http://courseware.rkbexplorer.com/ontologies/courseware> ;
        rdfs:label        "has student interaction type" ;
        rdfs:range        :Student-Interaction-Type .

:hours-of-personal-study
        a                 owl:DatatypeProperty ;
        rdfs:comment      "The total number of hours of personal study in this course" ;
        rdfs:domain       :Course ;
        rdfs:isDefinedBy  <http://courseware.rkbexplorer.com/ontologies/courseware> ;
        rdfs:label        "hours of personal study" ;
        rdfs:range        xsd:float .

:has-rights-copyright
        a                 owl:DatatypeProperty ;
        rdfs:comment      "Whether copyright or other restrictions apply to the use of this learning resource." ;
        rdfs:domain       akt:Abstract-Information ;
        rdfs:isDefinedBy  <http://courseware.rkbexplorer.com/ontologies/courseware> ;
        rdfs:range        [ a          owl:DataRange ;
                            owl:oneOf  ( "false" "true" )
                          ] .

:number-of-credits  a     owl:DatatypeProperty ;
        rdfs:comment      "The number of EU BS/MS program credits" ;
        rdfs:domain       :Course ;
        rdfs:isDefinedBy  <http://courseware.rkbexplorer.com/ontologies/courseware> ;
        rdfs:label        "number of credits" ;
        rdfs:range        xsd:float .

:Pre-requisite  a         owl:Class ;
        rdfs:comment      "This class encapsulates a body of previous knowledge required to undertake a course." ;
        rdfs:isDefinedBy  <http://courseware.rkbexplorer.com/ontologies/courseware> ;
        rdfs:label        "Pre-requisite" .

:has-assessment-method
        a                 owl:ObjectProperty ;
        rdfs:domain       :Course ;
        rdfs:isDefinedBy  <http://courseware.rkbexplorer.com/ontologies/courseware> ;
        rdfs:label        "has assessment method" ;
        rdfs:range        :Assessment-Method .

:is-taught-present  a     owl:DatatypeProperty ;
        rdfs:domain       :Course ;
        rdfs:isDefinedBy  <http://courseware.rkbexplorer.com/ontologies/courseware> ;
        rdfs:range        [ a          owl:DataRange ;
                            owl:oneOf  ( "false" "true" )
                          ] .

:hours-of-labs  a         owl:DatatypeProperty ;
        rdfs:comment      "The total number of hours of laboratory sessions in this course" ;
        rdfs:domain       :Course ;
        rdfs:isDefinedBy  <http://courseware.rkbexplorer.com/ontologies/courseware> ;
        rdfs:label        "hours of labs" ;
        rdfs:range        xsd:float .

:Course  a                owl:Class ;
        rdfs:comment      "This class encapsulates a course that is taught to students" ;
        rdfs:isDefinedBy  <http://courseware.rkbexplorer.com/ontologies/courseware> ;
        rdfs:label        "Course" ;
        rdfs:subClassOf   akt:Abstract-Information .

:hours-of-lectures  a     owl:DatatypeProperty ;
        rdfs:comment      "The total number of hours of lectures delivered in this course" ;
        rdfs:domain       :Course ;
        rdfs:isDefinedBy  <http://courseware.rkbexplorer.com/ontologies/courseware> ;
        rdfs:label        "hours of lectures" ;
        rdfs:range        xsd:float .

:has-courseware  a        owl:ObjectProperty ;
        rdfs:comment      "Courseware used by the Resist-Course (reference texts, personal hand-outs, slides, etc)." ;
        rdfs:domain       :Course ;
        rdfs:isDefinedBy  <http://courseware.rkbexplorer.com/ontologies/courseware> ;
        rdfs:label        "has courseware" ;
        rdfs:range        akt:Publication-Reference .

:submitted-by  a          owl:ObjectProperty ;
        rdfs:comment      "The ReSIST Project member who has submitted and is the point of contact for this course" ;
        rdfs:domain       :Course ;
        rdfs:isDefinedBy  <http://courseware.rkbexplorer.com/ontologies/courseware> ;
        rdfs:label        "submitted by" ;
        rdfs:range        akt:Generic-Agent .

:taught-at  a             owl:ObjectProperty ;
        rdfs:comment      "The organization at which this course is taught" ;
        rdfs:domain       :Course ;
        rdfs:isDefinedBy  <http://courseware.rkbexplorer.com/ontologies/courseware> ;
        rdfs:label        "taught at" ;
        rdfs:range        akt:Organization .

:has-rights-cost  a       owl:DatatypeProperty ;
        rdfs:comment      "Whether use of this learning resource requires payment" ;
        rdfs:domain       akt:Abstract-Information ;
        rdfs:isDefinedBy  <http://courseware.rkbexplorer.com/ontologies/courseware> ;
        rdfs:range        [ a          owl:DataRange ;
                            owl:oneOf  ( "false" "true" )
                          ] .
