@prefix dc:    <http://purl.org/dc/elements/1.1/> .
@prefix rdfs:  <http://www.w3.org/2000/01/rdf-schema#> .
@prefix foaf:  <http://xmlns.com/foaf/0.1/> .
@prefix dct:   <http://purl.org/dc/terms/> .
@prefix owl:   <http://www.w3.org/2002/07/owl#> .
@prefix rdf:   <http://www.w3.org/1999/02/22-rdf-syntax-ns#> .
@prefix vann:  <http://purl.org/vocab/vann/> .
@prefix skos:  <http://www.w3.org/2004/02/skos/core#> .

<http://purl.org/vocab/changeset/schema#subjectOfChange>
        a                 owl:ObjectProperty ;
        rdfs:domain       <http://purl.org/vocab/changeset/schema#ChangeSet> ;
        rdfs:isDefinedBy  <http://purl.org/vocab/changeset/schema> ;
        rdfs:label        "subjectOfChange"@en ;
        rdfs:range        rdfs:Resource ;
        dct:issued        "2005-12-14" ;
        skos:changeNote   [ rdf:value    "Added definitition and documentation" ;
                            dct:creator  "Ian Davis" ;
                            dct:date     "2006-03-21"
                          ] ;
        skos:definition   "the resource to which this set of changes applies"@en ;
        skos:historyNote  [ rdf:value    "Made owl:ObjectProperty" ;
                            dct:creator  "Ian Davis" ;
                            dct:date     "2006-03-21"
                          ] .

<http://purl.org/vocab/changeset/schema#creatorName>
        a                 owl:DatatypeProperty ;
        rdfs:domain       <http://purl.org/vocab/changeset/schema#ChangeSet> ;
        rdfs:isDefinedBy  <http://purl.org/vocab/changeset/schema> ;
        rdfs:label        "creatorName"@en ;
        rdfs:range        rdfs:Literal ;
        dct:issued        "2005-12-14" ;
        skos:definition   "the name of the entity responsible for creating the changeset"@en ;
        skos:historyNote  [ rdf:value    "Made owl:DatatypeProperty" ;
                            dct:creator  "Ian Davis" ;
                            dct:date     "2006-03-21"
                          ] .

<http://purl.org/vocab/changeset/schema#createdDate>
        a                   owl:DatatypeProperty ;
        rdfs:comment        "\n      The date should be in W3CDTF format\n    "@en ;
        rdfs:domain         <http://purl.org/vocab/changeset/schema#ChangeSet> ;
        rdfs:isDefinedBy    <http://purl.org/vocab/changeset/schema> ;
        rdfs:label          "createdDate"@en ;
        rdfs:subPropertyOf  dc:date ;
        dct:issued          "2005-12-14" ;
        skos:definition     "the date that the changeset was created"@en ;
        skos:historyNote    [ rdf:value    "Made owl:DatatypeProperty" ;
                              dct:creator  "Ian Davis" ;
                              dct:date     "2006-03-21"
                            ] .

<http://purl.org/vocab/changeset/schema#statement>
        a                 owl:ObjectProperty ;
        rdfs:domain       <http://purl.org/vocab/changeset/schema#ChangeSet> ;
        rdfs:isDefinedBy  <http://purl.org/vocab/changeset/schema> ;
        rdfs:label        "statement"@en ;
        rdfs:range        rdf:Statement ;
        dct:issued        "2006-03-21" ;
        skos:definition   "a triple included in this set of changes"@en .

<http://vocab.org/changeset/changesets-example3-20060321.html>
        dct:title  "Implementing Undo With ChangeSets" .

<http://iandavis.com/id/me>
        a          foaf:Person ;
        foaf:name  "Ian Davis" .

<http://purl.org/vocab/changeset/schema#precedingChangeSet>
        a                 owl:ObjectProperty ;
        rdfs:comment      "\n      This property can be used to build a history of changes to a particular resource description. The first\n      ChangeSet in the history will have no precedingChangeSet property. Each subsequent ChangeSet added\n      to the history references the preceding one resulting in a singly-linked list of changes.  Care must be taken\n      not to introduce cycles in the history.\n    "@en , "\n      In systems that assume a closed world, the most recent ChangeSet for a particular resource description \n      can be discovered by looking for the ChangeSet that is not the value of a precedingChangeSet property. \n      Conversely, the earliest ChangeSet is the one that is not the subject of a precedingChangeSet property.\n    "@en ;
        rdfs:domain       <http://purl.org/vocab/changeset/schema#ChangeSet> ;
        rdfs:isDefinedBy  <http://purl.org/vocab/changeset/schema> ;
        rdfs:label        "precedingChangeSet"@en ;
        rdfs:range        <http://purl.org/vocab/changeset/schema#ChangeSet> ;
        dct:issued        "2005-12-14" ;
        skos:changeNote   [ rdf:value    "Added definitition and documentation" ;
                            dct:creator  "Ian Davis" ;
                            dct:date     "2006-03-21"
                          ] ;
        skos:definition   "the changeset that immediately precedes this one"@en ;
        skos:historyNote  [ rdf:value    "Made owl:ObjectProperty" ;
                            dct:creator  "Ian Davis" ;
                            dct:date     "2006-03-21"
                          ] .

<http://vocab.org/changeset/schema.html>
        a           foaf:Document , <http://purl.org/dc/dcmitype/Text> ;
        rdfs:label  "HTML" ;
        dc:format   "text/html" .

<http://vocab.org/changeset/changesets-example2-20060321.html>
        dct:title  "Linked ChangeSets" .

<http://purl.org/vocab/changeset/schema>
        a                              owl:Ontology ;
        rdfs:comment                   "\n      The vocabulary introduces the notion of a ChangeSet which encapsulates the delta between two versions of a \n      resource description. In this context a resource description is the set of triples that in some way comprise a \n      description of a resource. The delta is represented by two sets of triples: additions and removals. A ChangeSet can be used to \n      modify a resource description by first removing all triples from the description that are in the removals set and\n      adding the triples in the additions set.\n    "@en , "\n      This vocabulary defines a set of terms for describing changes to resource descriptions.\n    "@en ;
        dct:creator                    "Sam Tunnicliffe" ;
        dct:creator                    <http://iandavis.com/id/me> ;
        dct:date                       "2006-03-21" ;
        dct:identifier                 "http://purl.org/vocab/changeset/schema-20060321" ;
        dct:isVersionOf                <http://purl.org/vocab/changeset/schema#> ;
        dct:issued                     "2005-12-14" ;
        dct:replaces                   <http://purl.org/vocab/changeset/schema-20051214> ;
        dct:rights                     "Copyright Â© 2005 Talis Information Ltd." ;
        dct:title                      "Changeset"@en ;
        vann:example                   <http://vocab.org/changeset/changesets-example-20060321.html> , <http://vocab.org/changeset/changesets-example2-20060321.html> , <http://vocab.org/changeset/changesets-example3-20060321.html> ;
        vann:preferredNamespacePrefix  "cs" ;
        vann:preferredNamespaceUri     "http://purl.org/vocab/changeset/schema#" ;
        skos:changeNote                [ rdfs:label   "Fixed invalid RDF"@en ;
                                         dct:creator  <http://iandavis.com/id/me> ;
                                         dct:date     "2006-06-23"
                                       ] ;
        skos:changeNote                [ rdfs:label   "Improved documentation"@en ;
                                         dct:creator  <http://iandavis.com/id/me> ;
                                         dct:date     "2006-03-21"
                                       ] ;
        skos:historyNote               [ rdfs:label   "Updated dublin core properties to new namespace"@en ;
                                         dct:creator  <http://iandavis.com/id/me> ;
                                         dct:date     "2009-05-18"
                                       ] ;
        skos:historyNote               [ rdfs:label   "Introduced statement property"@en ;
                                         dct:creator  <http://iandavis.com/id/me> ;
                                         dct:date     "2006-03-21"
                                       ] .

<http://purl.org/vocab/changeset/schema#changeReason>
        a                 owl:DatatypeProperty ;
        rdfs:domain       <http://purl.org/vocab/changeset/schema#ChangeSet> ;
        rdfs:isDefinedBy  <http://purl.org/vocab/changeset/schema> ;
        rdfs:label        "changeReason"@en ;
        rdfs:range        rdfs:Literal ;
        dct:issued        "2005-12-14" ;
        skos:definition   "a  short, human readable description of the purpose for the changeset"@en ;
        skos:historyNote  [ rdf:value    "Made owl:DatatypeProperty" ;
                            dct:creator  "Ian Davis" ;
                            dct:date     "2006-03-21"
                          ] .

<http://purl.org/vocab/changeset/schema#addition>
        a                   owl:ObjectProperty ;
        rdfs:comment        "\n      By convention the subject of the triple being added should be the same as the subjectOfChange\n    "@en ;
        rdfs:domain         <http://purl.org/vocab/changeset/schema#ChangeSet> ;
        rdfs:isDefinedBy    <http://purl.org/vocab/changeset/schema> ;
        rdfs:label          "addition"@en ;
        rdfs:range          rdf:Statement ;
        rdfs:subPropertyOf  <http://purl.org/vocab/changeset/schema#statement> ;
        dct:issued          "2005-12-14" ;
        skos:changeNote     [ rdf:value    "Added definitition and documentation" ;
                              dct:creator  "Ian Davis" ;
                              dct:date     "2006-03-21"
                            ] ;
        skos:definition     "a triple to be added to the resource description"@en ;
        skos:historyNote    [ rdf:value    "Made a sub-property of statement" ;
                              dct:creator  "Ian Davis" ;
                              dct:date     "2006-03-21"
                            ] ;
        skos:historyNote    [ rdf:value    "Made owl:ObjectProperty" ;
                              dct:creator  "Ian Davis" ;
                              dct:date     "2006-03-21"
                            ] .

<http://purl.org/vocab/changeset/schema#removal>
        a                   owl:ObjectProperty ;
        rdfs:comment        "\n      By convention the subject of the triple being removed should be the same as the subjectOfChange\n    "@en ;
        rdfs:domain         <http://purl.org/vocab/changeset/schema#ChangeSet> ;
        rdfs:isDefinedBy    <http://purl.org/vocab/changeset/schema> ;
        rdfs:label          "removal"@en ;
        rdfs:range          rdf:Statement ;
        rdfs:subPropertyOf  <http://purl.org/vocab/changeset/schema#statement> ;
        dct:issued          "2005-12-14" ;
        skos:changeNote     [ rdf:value    "Added definitition and documentation" ;
                              dct:creator  "Ian Davis" ;
                              dct:date     "2006-03-21"
                            ] ;
        skos:definition     "a triple to be removed from the resource description"@en ;
        skos:historyNote    [ rdf:value    "Made owl:ObjectProperty" ;
                              dct:creator  "Ian Davis" ;
                              dct:date     "2006-03-21"
                            ] ;
        skos:historyNote    [ rdf:value    "Made a sub-property of statement" ;
                              dct:creator  "Ian Davis" ;
                              dct:date     "2006-03-21"
                            ] .

<http://purl.org/vocab/changeset/schema#ChangeSet>
        a                 owl:Class ;
        rdfs:isDefinedBy  <http://purl.org/vocab/changeset/schema> ;
        rdfs:label        "ChangeSet"@en ;
        rdfs:subClassOf   [ a                   owl:Class ;
                            owl:intersectionOf  ( [ a                   owl:Restriction ;
                                                    owl:minCardinality  "1"^^<http://www.w3.org/2001/XMLSchema#nonNegativeInteger> ;
                                                    owl:onProperty      <http://purl.org/vocab/changeset/schema#statement>
                                                  ] [ a                   owl:Restriction ;
                                                      owl:maxCardinality  "1"^^<http://www.w3.org/2001/XMLSchema#nonNegativeInteger> ;
                                                      owl:onProperty      <http://purl.org/vocab/changeset/schema#previousChangeSet>
                                                    ] [ a                   owl:Restriction ;
                                                        owl:maxCardinality  "1"^^<http://www.w3.org/2001/XMLSchema#nonNegativeInteger> ;
                                                        owl:onProperty      <http://purl.org/vocab/changeset/schema#subjectOfChange>
                                                      ] [ a                   owl:Restriction ;
                                                          owl:maxCardinality  "1"^^<http://www.w3.org/2001/XMLSchema#nonNegativeInteger> ;
                                                          owl:onProperty      <http://purl.org/vocab/changeset/schema#createdDate>
                                                        ] [ a                   owl:Restriction ;
                                                            owl:maxCardinality  "1"^^<http://www.w3.org/2001/XMLSchema#nonNegativeInteger> ;
                                                            owl:onProperty      <http://purl.org/vocab/changeset/schema#creatorName>
                                                          ] [ a                   owl:Restriction ;
                                                              owl:maxCardinality  "1"^^<http://www.w3.org/2001/XMLSchema#nonNegativeInteger> ;
                                                              owl:onProperty      <http://purl.org/vocab/changeset/schema#changeReason>
                                                            ] )
                          ] ;
        dct:issued        "2005-12-14" ;
        skos:changeNote   [ rdf:value    "Improved documentation" ;
                            dct:creator  "Ian Davis" ;
                            dct:date     "2006-03-21"
                          ] ;
        skos:definition   "The encapsulation of a delta between two versions of a resource description"@en ;
        skos:historyNote  [ rdf:value    "Added property cardinality restrictions" ;
                            dct:creator  "Ian Davis" ;
                            dct:date     "2006-03-21"
                          ] .

<http://vocab.org/changeset/schema.turtle>
        a           foaf:Document , <http://purl.org/dc/dcmitype/Text> ;
        rdfs:label  "Turtle" ;
        dc:format   "text/plain" .

<http://vocab.org/changeset/schema.json>
        a           foaf:Document , <http://purl.org/dc/dcmitype/Text> ;
        rdfs:label  "JSON" ;
        dc:format   "application/json" .

<http://vocab.org/changeset/schema.rdf>
        a                  <http://purl.org/dc/dcmitype/Text> , foaf:Document ;
        dct:hasFormat      <http://vocab.org/changeset/schema.turtle> , <http://vocab.org/changeset/schema.json> , <http://vocab.org/changeset/schema.html> ;
        foaf:primaryTopic  <http://purl.org/vocab/changeset/schema> ;
        foaf:topic         <http://purl.org/vocab/changeset/schema> .

<http://vocab.org/changeset/changesets-example-20060321.html>
        dct:title  "A Simple ChangeSet" .
