@prefix dc: <http://purl.org/dc/elements/1.1/> .
@prefix : <http://www.tele.pw.edu.pl/~sims-onto/ConnectivityType.owl#> .
@prefix rdfs: <http://www.w3.org/2000/01/rdf-schema#> .
@prefix owl11: <http://www.w3.org/2006/12/owl11#> .
@prefix owl11xml: <http://www.w3.org/2006/12/owl11-xml#> .
@prefix pc: <http://www.tele.pw.edu.pl/~sims-onto/ParticipantCharacteristic.owl#> .
@prefix owl: <http://www.w3.org/2002/07/owl#> .
@prefix xsd: <http://www.w3.org/2001/XMLSchema#> .
@prefix rdf: <http://www.w3.org/1999/02/22-rdf-syntax-ns#> .
@prefix te: <http://www.tele.pw.edu.pl/~sims-onto/TelecomEntity.owl#> .
@prefix daml: <http://www.daml.org/2001/03/daml+oil#> .

<http://www.tele.pw.edu.pl/~sims-onto/ConnectivityType.owl> a owl:Ontology ;
	rdfs:label "Connectivity types"^^xsd:string ;
	rdfs:comment "Defines types of connectivity used in communication and bearer services accessible in certain connectivity."^^xsd:string ;
	owl:priorVersion "Version 1.0 (2006-10-24), first phase"^^xsd:string ;
	owl:imports <http://www.tele.pw.edu.pl/~sims-onto/ParticipantCharacteristic.owl> ;
	owl:versionInfo "1.4"^^xsd:string .

:hasBearerType a owl:ObjectProperty ;
	rdfs:comment "Defines transmission technology."^^xsd:string ;
	rdfs:range :BearerType ;
	rdfs:domain :NetworkBearerService .

:hasNetworkBearerService a owl:ObjectProperty ;
	rdfs:domain te:ConnectivityType ;
	rdfs:range :NetworkBearerService ;
	rdfs:comment "Defines network bearers supported by connectivity type."^^xsd:string .

:referesToAddress a owl:ObjectProperty ;
	rdfs:domain :NetworkBearerService ;
	rdfs:range :BearerAddressType ;
	rdfs:comment "Defines network address type used by network bearer type."^^xsd:string .

:referesToNetwork a owl:ObjectProperty ;
	rdfs:comment "Defines network which supports bearer."^^xsd:string ;
	rdfs:domain :NetworkBearerService ;
	rdfs:range :Network .

:BearerAddressType a owl:Class ;
	rdfs:subClassOf owl:Thing ;
	rdfs:comment "Defines type of address supported in network and associated with bearer. Specific addresses are modelled as instances e.g. GSM_MSISDN describe type of address used in GSM network."^^xsd:string .

:BearerType a owl:Class ;
	rdfs:subClassOf owl:Thing ;
	rdfs:comment "Defines transmission technology used to transfer voice or data in network."^^xsd:string .

:CellularConnectivityType a owl:Class ;
	rdfs:subClassOf :LongRangeConnectivityType ;
	rdfs:comment "Cellular connectivity, e.g., GSM"^^xsd:string .

:DataBearerService a owl:Class ;
	rdfs:subClassOf :NetworkBearerService ;
	rdfs:comment "Defines bearer capable to transmit data."^^xsd:string .

:LongRangeConnectivityType a owl:Class ;
	rdfs:subClassOf :WirelessConnectivityType ;
	rdfs:comment "Long range wireless connectivity, such as WiMAX or GSM"^^xsd:string .

:Network a owl:Class ;
	rdfs:subClassOf owl:Thing ;
	rdfs:comment "Defines general term for telecommunication network."^^xsd:string .

:NetworkBearerService a owl:Class ;
	rdfs:subClassOf owl:Thing ;
	rdfs:comment "Defines network bearer service that allows transmission of information signals between network interfaces. E.g. transmission of MMS in GSM network is modelled as instance 'GSM_GPRS_IPV4'. Bearer capabilities are modeled as sublasses."^^xsd:string .

:ShortRangeConnectivityType a owl:Class ;
	rdfs:subClassOf :WirelessConnectivityType ;
	rdfs:comment "Short range wireless connectivity type (WiFi, Bluetooth)"^^xsd:string .

:TextBearerService a owl:Class ;
	rdfs:subClassOf :NetworkBearerService ;
	rdfs:comment "Defines bearer capable to transmit text. E.g. bearer responsible for SMS transfer."^^xsd:string .

:VideoBearerService a owl:Class ;
	rdfs:subClassOf :VoiceBearerService ;
	rdfs:comment "Defines bearer capable to transmit video."^^xsd:string .

:VoiceBearerService a owl:Class ;
	rdfs:subClassOf :NetworkBearerService ;
	rdfs:comment "Defines bearer capable to transmit voice."^^xsd:string .

:WirelessConnectivityType a owl:Class ;
	rdfs:subClassOf te:ConnectivityType ;
	rdfs:comment "Wireless connectivity type (e.g., GSM connectivity)"^^xsd:string .

:WirelineConnectivityType a owl:Class ;
	rdfs:subClassOf te:ConnectivityType ;
	rdfs:comment "Fixed, wireline connectivity type (e.g., PSTN)"^^xsd:string .

te:ConnectivityType a owl:Class ;
	rdfs:subClassOf _:node17pmg12fjx1 .

_:node17pmg12fjx1 a owl:Restriction ;
	owl:onProperty :hasNetworkBearerService ;
	owl:allValuesFrom :NetworkBearerService .

te:ConnectivityType rdfs:subClassOf _:node17pmg12fjx2 .

_:node17pmg12fjx2 a owl:Restriction ;
	owl:onProperty :hasNetworkBearerService ;
	owl:someValuesFrom :NetworkBearerService .

owl:Thing a owl:Class .

:BluetoothConnectivity a :ShortRangeConnectivityType ;
	rdfs:comment "Defines Bluetooth connectivity."^^xsd:string .

:CSD a :BearerType ;
	rdfs:comment "Circuit Switched Data (CSD) is the original form of data transmission developed for the time division multiple access (TDMA)-based mobile phone systems like Global System for Mobile Communications (GSM)."^^xsd:string .

:EDGE a :BearerType ;
	rdfs:comment "Defnes Enhanced Data rates for GSM Evolution technology which allows to increase data transmission rate."^^xsd:string .

:GPRS a :BearerType ;
	rdfs:comment "General Packet Radio Service (GPRS) is a Mobile Data Service available to users of Global System for Mobile Communications (GSM) and IS-136 mobile phones."^^xsd:string .

:GSM a :Network ;
	rdfs:comment "The Global System for Mobile communications is the most popular standard for mobile phones in the world. GSM is a cellular network, which means that mobile phones connect to it by searching for cells in the immediate vicinity."^^xsd:string .

:GSMConnectivity a :CellularConnectivityType ;
	:hasNetworkBearerService :GSM_GPRS_IPV4 , :GSM_CSD_IPv4 , :GSM_SMS_MSISDN , :GSM_CSD_MSISDN ;
	rdfs:comment "Defines GSM connectivity."^^xsd:string .

:GSM_CSD_IPv4 a :DataBearerService ;
	:referesToNetwork :GSM ;
	:referesToAddress :IPv4 ;
	:hasBearerType :CSD ;
	rdfs:comment "Defines bearer service in GSM network which use IPv4 address type and CSD bearer. Type of data transfer bearer in GSM network."^^xsd:string .

:GSM_CSD_MSISDN a :VoiceBearerService ;
	:hasBearerType :CSD ;
	:referesToAddress :GSM_MSISDN ;
	rdfs:comment "Defines bearer service in GSM network which use MSISDN address type and CSD bearer. Type of voice transfer bearer in GSM network."^^xsd:string ;
	:referesToNetwork :GSM .

:GSM_EDGE_IPv4 a :DataBearerService ;
	:referesToAddress :IPv4 ;
	rdfs:comment "Defines EDGE bearer service in GSM network with IPv4 address protocol."^^xsd:string ;
	:hasBearerType :EDGE ;
	:referesToNetwork :GSM .

:GSM_GPRS_IPV4 a :DataBearerService ;
	:referesToAddress :IPv4 ;
	rdfs:comment "Defines GPRS bearer service in GSM network using IPv4 address type. Type of data transfer bearer in GSM network."^^xsd:string ;
	:hasBearerType :GPRS ;
	:referesToNetwork :GSM .

:GSM_HSCSD_IPv4 a :DataBearerService ;
	rdfs:comment "Defines HSCSD bearer service in GSM network with IP v4 address protocol."^^xsd:string ;
	:referesToAddress :IPv4 ;
	:hasBearerType :HSCSD ;
	:referesToNetwork :GSM .

:GSM_MSISDN a :BearerAddressType ;
	rdfs:comment "MSISDN (Mobile Subscriber ISDN Number) refers to the telephone number of a mobile subscriber. MSISDN by ITU-T is at most 15 digits long and consists of: * CC - Country Code ( 1-3 digits e.g.\"48\" for Poland), * NDC - National Destination Code (e.g. 3 digits in Poland), * SN - Subscriber Number (e.g. 6 remaining digits (123456))."^^xsd:string .

:GSM_SMS_MSISDN a :TextBearerService ;
	:referesToNetwork :GSM ;
	:hasBearerType :SMS_BearerType ;
	:referesToAddress :GSM_MSISDN ;
	rdfs:comment "Defines SMS bearer service in GSM network using GSM_MSISDN address type."^^xsd:string .

:GSM_USSD a :DataBearerService ;
	:referesToNetwork :GSM ;
	rdfs:comment "USSD is a technology built into the GSM standard for support of transmitting information over the signaling channels of the GSM network. USSD provides session-based communication. Defined within the GSM standard in the documents GSM 02.90 (USSD Stage 1) and GSM 03.90 (USSD Stage 2)."^^xsd:string ;
	:hasBearerType :USSD .

:HSCSD a :BearerType ;
	rdfs:comment "Defines High-Speed Circuit-Switched Data, data transmission mechanism in GSM Network, enhancement of CSD."^^xsd:string .

:IPv4 a :BearerAddressType ;
	rdfs:comment "IP address (Internet Protocol address) is a unique address that certain electronic devices use in order to identify and communicate with each other on a computer network utilizing the Internet Protocol standard (IP). IPv4 uses 32-bit (4 byte) addresses."^^xsd:string .

:IPv6 a :BearerAddressType ;
	rdfs:comment "IP address (Internet Protocol address) is a unique address that certain electronic devices use in order to identify and communicate with each other on a computer network utilizing the Internet Protocol standard (IP). IPv6 uses 128-bit addresses."^^xsd:string .

:IS-95 a :Network ;
	rdfs:comment "Interim Standard 95 (IS-95), is the first CDMA-based digital cellular standard pioneered by Qualcomm. CDMA or \"code division multiple access\" is a digital radio system that transmits streams of bits (PN Sequences)."^^xsd:string .

:IrDAConnectivity a :ShortRangeConnectivityType ;
	rdfs:comment "Defines IrDA connectivity."^^xsd:string .

:SMS_BearerType a :BearerType ;
	rdfs:comment "Defines transmission technology used in GSM network to transmit SMS messages."^^xsd:string .

:UMTS a :Network ;
	rdfs:comment "Universal Mobile Telecommunications System (UMTS) is one of the third-generation (3G) cell phone technologies."^^xsd:string .

:UMTSConnectivity a :CellularConnectivityType ;
	rdfs:comment "Defines UMTS connectivity"^^xsd:string ;
	:hasNetworkBearerService :UMTS_Video_IPv6 .

:UMTS_VideoBearer a :BearerType ;
	rdfs:comment "Defines bearer capable to tansfer video data in UMTS networks."^^xsd:string .

:UMTS_Video_IPv6 a :VideoBearerService ;
	rdfs:comment "Defines video bearer in UMTS network which use IPv6 address type. It is bearer capable to transfer video."^^xsd:string .

:USSD a :BearerType ;
	rdfs:comment "Defines bearer capable to transmit information over the signaling channels of the GSM network."^^xsd:string .

:WLAN a :Network ;
	rdfs:comment "Defines wireless LAN network type."^^xsd:string .

:WLANBearer a :BearerType ;
	rdfs:comment "Defines bearer accessible in wireless LAN networks specified in 802.11 IEEE standars."^^xsd:string .

:WLAN_IPv4 a :DataBearerService ;
	:referesToAddress :IPv4 ;
	rdfs:comment "Defines bearer service in WLAN networks with IPv4 address protocol."^^xsd:string ;
	:hasBearerType :WLANBearer ;
	:referesToNetwork :WLAN .

:WiFiConnectivity a :ShortRangeConnectivityType ;
	rdfs:comment "Defines wi-fi connectivity."^^xsd:string .

:WiMAXConnectivity a :LongRangeConnectivityType ;
	rdfs:comment "Defines WiMax connectivity."^^xsd:string .

te:ConnectivityType rdfs:subClassOf _:node17pmg12fjx3 .

_:node17pmg12fjx3 a owl:Restriction ;
	owl:onProperty :hasNetworkBearerService ;
	owl:allValuesFrom :NetworkBearerService .

te:ConnectivityType rdfs:subClassOf _:node17pmg12fjx4 .

_:node17pmg12fjx4 a owl:Restriction ;
	owl:onProperty :hasNetworkBearerService ;
	owl:someValuesFrom :NetworkBearerService .
