@prefix dc: <http://purl.org/dc/elements/1.1/> .
@prefix : <http://www.w3.org/1999/02/22-rdf-syntax-ns#> .
@prefix rdfs: <http://www.w3.org/2000/01/rdf-schema#> .
@prefix foaf: <http://xmlns.com/foaf/0.1/> .
@prefix status: <http://metadataregistry.org/uri/RegStatus/> .
@prefix reg: <http://metadataregistry.org/uri/profile/RegAp/> .
@prefix dct: <http://purl.org/dc/terms/> .
@prefix owl: <http://www.w3.org/2002/07/owl#> .
@prefix skos: <http://www.w3.org/2004/02/skos/core#> .

<http://iflastandards.info/ns/fr/frad/> dc:title "FRAD model"@en ;
	skos:note "This is the element set of native RDF classes and properties described in the Functional Requirements for Authority Data model. The model also uses elements previously described in the Functional Requirements for Bibliographic Records (FRBR) entity-relationship model."@en .

<http://iflastandards.info/ns/fr/frad/C1008> rdfs:isDefinedBy <http://iflastandards.info/ns/fr/frad/> ;
	reg:status status:1001 ;
	reg:name "Agency"@en ;
	rdfs:label "Agency"@en ;
	skos:definition "An organization responsible for creating or modifying a controlled access point. The agency is responsible for application and interpretation of the rules it creates and/or uses. The agency may also be responsible for the creation and maintenance of identifiers within its domain."@en ;
	a owl:Class ;
	skos:scopeNote "Includes libraries, national bibliographic agencies, bibliographic utilities, consortia, museums, archives, rights management organizations, etc."@en ;
	rdfs:label "Agencia"@es .

<http://iflastandards.info/ns/fr/frad/C1010> rdfs:isDefinedBy <http://iflastandards.info/ns/fr/frad/> ;
	reg:status status:1001 ;
	reg:name "BibliographicEntity"@en ;
	rdfs:label "Bibliographic Entity"@en ;
	a owl:Class ;
	skos:definition "An entity which reflects intellectual constructs or concepts that are integral to the rules used to create library catalogues."@en ;
	skos:scopeNote "What is perceived as a specific instance of a particular entity type may vary from one set of rules to another."@en ;
	reg:hasSubClass <http://iflastandards.info/ns/fr/frad/C1002> , <http://iflastandards.info/ns/fr/frad/C1003> .

<http://iflastandards.info/ns/fr/frad/C1001> rdfs:isDefinedBy <http://iflastandards.info/ns/fr/frad/> ;
	reg:status status:1001 ;
	reg:name "ControlledAccessPoint"@en ;
	rdfs:label "Controlled Access Point"@en ;
	skos:definition "A name, term, code, etc., under which a bibliographic or authority record or reference will be found."@en ;
	a owl:Class ;
	rdfs:comment "Description is modified from: Guidelines for authority records and references / revised by the Working Group on GARE Revision. Second edition.  München : K.G. Saur, 2001."@en ;
	skos:scopeNote "Includes access points designated as authorized (or preferred) forms of names (i.e., authorized access points) as well as those designated as variant forms of name (i.e., variant access points). Includes access points based on personal, family, and corporate names. Includes access points based on titles (i.e., names) for works, expressions, manifestations, and items. Includes access points consisting of a combination of two access points, as in the case of a creator/title access point for a work which consists of an authorized access point for the name of the creator combined with an authorized access point for the name (i.e., the title) of the work. Includes access points based on names and terms for events, objects, concepts, and places. Includes access points based on identifiers, such as standard numbers, classification indicia. Elements added to the name per se (e.g., dates) form an integral part of the controlled access point."@en .

<http://iflastandards.info/ns/fr/frad/C1003> rdfs:isDefinedBy <http://iflastandards.info/ns/fr/frad/> ;
	reg:status status:1001 ;
	reg:name "CorporateBody"@en ;
	rdfs:label "Corporate Body"@en ;
	skos:definition "An organization or group of persons and/or organizations identified by a particular name acting as a unit."@en ;
	a owl:Class ;
	rdfs:comment "Description is modified from that in Functional requirements for bibliographic records : final report, by the IFLA Study Group on the Functional Requirements for Bibliographic Records, published by K.G. Saur, 1998."@en ;
	skos:scopeNote "Includes occasional groups and groups that are constituted as meetings, conferences, congresses, expeditions, exhibitions, festivals, fairs, etc. Includes musical performing groups, groups of visual artists, and dance companies producing collective work. Includes organizations that act as territorial authorities, exercising or claiming to exercise government functions over a certain territory, such as a federation, a state, a region, a local municipality. Includes organizations and groups that are defunct as well as those that continue to operate. Includes fictitious organizations or groups of persons."@en ;
	rdfs:subClassOf <http://iflastandards.info/ns/fr/frad/C1010> .

<http://iflastandards.info/ns/fr/frad/C1002> rdfs:isDefinedBy <http://iflastandards.info/ns/fr/frad/> ;
	reg:status status:1001 ;
	reg:name "Family"@en ;
	rdfs:label "Family"@en ;
	a owl:Class ;
	skos:definition "Two or more persons related by birth, marriage, adoption, civil union, or similar legal status, or who otherwise present themselves as a family."@en ;
	skos:scopeNote "Includes royal families, dynasties, houses of nobility, etc. Includes patriarchies and matriarchies. Includes groups of individuals sharing a common ancestral lineage. Includes family units (parents, children, grandchildren, etc.). Includes the successive holders of a title in a house of nobility, viewed collectively (e.g., Dukes of Norfolk)."@en ;
	rdfs:label "Familia"@es ;
	rdfs:subClassOf <http://iflastandards.info/ns/fr/frad/C1010> .

<http://iflastandards.info/ns/fr/frad/C1009> rdfs:isDefinedBy <http://iflastandards.info/ns/fr/frad/> ;
	reg:status status:1001 ;
	reg:name "Identifier"@en ;
	rdfs:label "Identifier"@en ;
	skos:definition "A number, code, word, phrase, logo, device, etc., that is associated with an entity, and serves to differentiate that entity from other entities within the domain in which the identifier is assigned. An identifier can consist of an identifier string (i.e., a sequence of numeric and/or alphabetic characters assigned to an entity to serve as a unique identifier within the domain to which the identifier is assigned) and a prefix and/or suffix (a character or set of characters (numeric and/or alphabetic) appearing before or after an identifier string)."@en ;
	a owl:Class ;
	skos:scopeNote """Includes identifiers such as social insurance numbers assigned by a government authority. Includes personal identifiers assigned by other registration authorities. Includes business registration numbers, registration numbers for charitable organizations, etc., assigned by a government authority. Includes corporate body identifiers assigned by other registration authorities (e.g., ISBN publisher’s prefix). 
Includes standard identifiers assigned by registration authorities identifying content (e.g., ISRC, ISWC, ISAN). Includes standard identifiers assigned by registration authorities identifying manifestations (e.g., ISBN, ISSN). Includes thematic index numbers assigned to a musical work by the publisher, or a musicologist. Includes catalogue raisonné numbers. Includes identifiers for items assigned by repositories (e.g., shelf number). Includes classification numbers referencing specific entities (e.g., a classification number assigned to a particular painting). Includes registered trademarks."""@en ;
	rdfs:label "Identificador"@es .

<http://iflastandards.info/ns/fr/frad/C1006> rdfs:isDefinedBy <http://iflastandards.info/ns/fr/frad/> ;
	reg:status status:1001 ;
	reg:name "Name"@en ;
	rdfs:label "Name"@en ;
	skos:definition "A character, word, or group of words and/or characters by which an entity is known."@en ;
	a owl:Class ;
	skos:scopeNote "Includes names by which persons, families, and corporate bodies are known. Includes titles by which works, expressions, and manifestations are known. Includes names and terms by which concepts, objects, events, and places are known. Includes real names, pseudonyms, religious names, initials, and separate letters, numerals, or symbols. Includes forenames (or given names), matronymics, patronymics, family names (or surnames), dynastic names, etc. Includes given names of sovereigns, popes, etc., with associated roman numerals. Includes names of families, clans, dynasties, houses of nobility, etc. Includes names representing the successive holders of a title in houses of nobility, etc., viewed collectively (e.g., Dukes of Norfolk). Includes names used by a corporate body at various periods in its history. Includes names of associations, institutions, business firms, not-for-profit enterprises, etc. Includes names of governments, government agencies, projects, programmes, government officials, delegations, legislative bodies, armed forces, etc. Includes names of religious bodies, local churches, etc., religious councils, religious officials, provinces, dioceses, synods, etc., papal diplomatic missions, etc. Includes names of conferences, congresses, meetings, etc. Includes names of exhibitions, athletic contests, expeditions, fairs, festivals, etc. Includes names of subordinate and related bodies. Includes numbers that form an integral part of the name of a corporate body or event. Includes trade names. Includes titles of content, parts of content, compilations of content, etc. Includes titles by which a work has become known. Includes the title proper of the original manifestation of a work. Includes titles by which a work is identified in reference sources. Includes titles under which a work has been published. Includes titles by which manifestations of an expression have become known. Includes the title proper of the original manifestation of an expression. Includes titles by which manifestations of an expression are identified in reference sources. Includes titles under which manifestations of an expression have been published. Includes the title proper of the original edition of a manifestation. Includes titles by which a manifestation is identified in reference sources. Includes variant titles appearing on or in a manifestation. Includes names and terms for events, objects, concepts, and places."@en ;
	rdfs:label "Nombre"@es .

<http://iflastandards.info/ns/fr/frad/C1011> rdfs:isDefinedBy <http://iflastandards.info/ns/fr/frad/> ;
	reg:status status:1001 ;
	reg:name "NameOfACorporateBody"@en ;
	rdfs:label "Name of a Corporate Body"@en ;
	a owl:Class ;
	skos:definition "A name which is the appellation of a corporate body."@en .

<http://iflastandards.info/ns/fr/frad/C1013> rdfs:isDefinedBy <http://iflastandards.info/ns/fr/frad/> ;
	reg:status status:1001 ;
	reg:name "NameOfAFamily"@en ;
	rdfs:label "Name of a Family"@en ;
	a owl:Class ;
	skos:definition "A name which is the appellation of a family."@en .

<http://iflastandards.info/ns/fr/frad/C1012> rdfs:isDefinedBy <http://iflastandards.info/ns/fr/frad/> ;
	reg:status status:1001 ;
	reg:name "NameOfAPerson"@en ;
	rdfs:label "Name of a Person"@en ;
	a owl:Class ;
	skos:definition "A name which is the appellation of a person."@en .

<http://iflastandards.info/ns/fr/frad/C1014> rdfs:isDefinedBy <http://iflastandards.info/ns/fr/frad/> ;
	reg:status status:1001 ;
	reg:name "NameOfAWork"@en ;
	rdfs:label "Name of a Work"@en ;
	a owl:Class ;
	skos:definition "A name which is the appellation of a work."@en .

<http://iflastandards.info/ns/fr/frad/C1007> rdfs:isDefinedBy <http://iflastandards.info/ns/fr/frad/> ;
	reg:status status:1001 ;
	reg:name "Rules"@en ;
	rdfs:label "Rules"@en ;
	skos:definition "A set of instructions relating to the formulation and/or recording of controlled access points (authorized forms, variant forms or references, etc.)."@en ;
	a owl:Class ;
	skos:scopeNote "Includes cataloguing rules and interpretations of those rules. Includes coding conventions."@en ;
	rdfs:label "Reglas"@es .

<http://iflastandards.info/ns/fr/frad/P2002> rdfs:isDefinedBy <http://iflastandards.info/ns/fr/frad/> ;
	reg:status status:1001 ;
	reg:name "applies"@en ;
	rdfs:label "applies"@en ;
	a :Property ;
	rdfs:domain <http://iflastandards.info/ns/fr/frad/C1008> ;
	skos:definition "Relates an agency to rules that it applies when creating or modifying a controlled access point."@en ;
	rdfs:range <http://iflastandards.info/ns/fr/frad/C1007> ;
	rdfs:label "aplica"@es ;
	owl:inverseOf <http://iflastandards.info/ns/fr/frad/P2001> .

<http://iflastandards.info/ns/fr/frad/P2001> rdfs:isDefinedBy <http://iflastandards.info/ns/fr/frad/> ;
	reg:status status:1001 ;
	reg:name "areAppliedBy"@en ;
	rdfs:label "are applied by"@en ;
	a :Property ;
	rdfs:domain <http://iflastandards.info/ns/fr/frad/C1007> ;
	skos:definition "Relates rules to an agency that applies them when creating or modifying a controlled access point."@en ;
	rdfs:range <http://iflastandards.info/ns/fr/frad/C1008> ;
	rdfs:label "son aplicadas por"@es ;
	owl:inverseOf <http://iflastandards.info/ns/fr/frad/P2002> ;
	owl:propertyDisjointWith <http://iflastandards.info/ns/fr/frad/P3019> , <http://iflastandards.info/ns/fr/frad/P3020> .

<http://iflastandards.info/ns/fr/frad/P2006> rdfs:isDefinedBy <http://iflastandards.info/ns/fr/frad/> ;
	reg:status status:1001 ;
	reg:name "creates"@en ;
	rdfs:label "creates"@en ;
	a :Property ;
	rdfs:domain <http://iflastandards.info/ns/fr/frad/C1008> ;
	skos:definition "Relates an agency to a controlled access point that is created by the agency."@en ;
	rdfs:range <http://iflastandards.info/ns/fr/frad/C1001> ;
	rdfs:label "crea"@es ;
	owl:inverseOf <http://iflastandards.info/ns/fr/frad/P2005> .

<http://iflastandards.info/ns/fr/frad/P2004> rdfs:isDefinedBy <http://iflastandards.info/ns/fr/frad/> ;
	reg:status status:1001 ;
	reg:name "govern"@en ;
	rdfs:label "govern"@en ;
	a :Property ;
	rdfs:domain <http://iflastandards.info/ns/fr/frad/C1007> ;
	skos:definition "Relates rules to a controlled access point that they govern."@en ;
	rdfs:range <http://iflastandards.info/ns/fr/frad/C1001> ;
	rdfs:label "regula"@es ;
	owl:inverseOf <http://iflastandards.info/ns/fr/frad/P2003> ;
	owl:propertyDisjointWith <http://iflastandards.info/ns/fr/frad/P3019> , <http://iflastandards.info/ns/fr/frad/P3020> .

<http://iflastandards.info/ns/fr/frad/P2030> rdfs:isDefinedBy <http://iflastandards.info/ns/fr/frad/> ;
	reg:status status:1001 ;
	reg:name "hasAccompanyingRelationship"@en ;
	rdfs:label "has accompanying relationship"@en ;
	skos:definition "Relates a work to another work that is a supplement to that work (i.e., a work that is intended to be used in conjunction with or to augment the related work, such as a teacher’s guide or incidental music to a play; or intended to complement or be a companion to another work, such as a set of maps to a video travelogue, a computer disk to accompany a textbook, a set of coloured plates to accompany a text, the equal parts of a kit)."@en ;
	a :Property ;
	rdfs:domain <http://iflastandards.info/ns/fr/frbr/frbrer/C1001> ;
	rdfs:range <http://iflastandards.info/ns/fr/frbr/frbrer/C1001> .

<http://iflastandards.info/ns/fr/frad/P4027> rdfs:isDefinedBy <http://iflastandards.info/ns/fr/frad/> ;
	reg:status status:1001 ;
	reg:name "hasAcronymOrInitialsOrAbbreviation"@en ;
	rdfs:label "has acronym or initials or abbreviation"@en ;
	skos:definition "Relates a name of a corporate body and an acronym or initials or an abbreviation by which that body is known."@en ;
	a :Property ;
	rdfs:domain <http://iflastandards.info/ns/fr/frad/C1011> ;
	rdfs:range <http://iflastandards.info/ns/fr/frad/C1011> ;
	rdfs:label "tiene acrónimo o iniciales o abreviaturas"@es ;
	owl:inverseOf <http://iflastandards.info/ns/fr/frad/P4026> ;
	owl:propertyDisjointWith <http://iflastandards.info/ns/fr/frad/P4032> , <http://iflastandards.info/ns/fr/frad/P4026> , <http://iflastandards.info/ns/fr/frad/P4025> .

<http://iflastandards.info/ns/fr/frad/P3018> rdfs:isDefinedBy <http://iflastandards.info/ns/fr/frad/> ;
	reg:status status:1001 ;
	reg:name "hasAddition"@en ;
	rdfs:label "has addition"@en ;
	skos:definition "Relates a controlled access point to a name, title, date, place, number, or other designation added to the base access point."@en ;
	a :Property ;
	rdfs:comment "Sometimes referred to as a \"qualifier\"."@en ;
	skos:scopeNote "Includes the fuller form of name added to the base access point. Includes the title of nobility, title of royalty, or ecclesiastical title added to the base access point. Includes dates added to the base access point. Includes the place name associated with a corporate body added to the base access point. Includes a number associated with a corporate body or a musical work added to the base access point. Includes a title of an adaptation or version of a work added to the base access point. Includes the name and/or number of a section or part of a work added to the base access point. Includes a term designating the form of a work added to the base access point. Includes a term designating language of expression added to the base access point. Includes a term designating the key in which a musical work was originally composed added to the base access point. Includes a term designating the medium of performance for which a musical work was originally conceived added to the base access point. Includes other designations associated with persons and corporate bodies added to the base access point."@en ;
	rdfs:domain <http://iflastandards.info/ns/fr/frad/C1001> ;
	rdfs:label "tiene adición"@es .

<http://iflastandards.info/ns/fr/frad/P3041> rdfs:isDefinedBy <http://iflastandards.info/ns/fr/frad/> ;
	reg:status status:1001 ;
	reg:name "hasAddressCorporateBody"@en ;
	rdfs:label "has address (corporate body)"@en ;
	skos:definition "Relates a corporate body to the current or former address of the corporate body's office(s)."@en ;
	a :Property ;
	skos:scopeNote "Includes addresses for the corporate body's headquarters and/or other offices. Includes street address, postal address, telephone number, e-mail address, etc. Includes the address of a World Wide Web site operated by the corporate body, about the corporate body or related to the corporate body."@en ;
	rdfs:domain <http://iflastandards.info/ns/fr/frad/C1003> ;
	owl:propertyDisjointWith <http://iflastandards.info/ns/fr/frad/P3043> , <http://iflastandards.info/ns/fr/frad/P3042> , <http://iflastandards.info/ns/fr/frad/P3040> .

<http://iflastandards.info/ns/fr/frad/P3035> rdfs:isDefinedBy <http://iflastandards.info/ns/fr/frad/> ;
	reg:status status:1001 ;
	reg:name "hasAddressPerson"@en ;
	rdfs:label "has address (person)"@en ;
	skos:definition "Relates a person to the current or former address of the person's place of residence, business, or employer."@en ;
	a :Property ;
	skos:scopeNote "Includes street address, postal address, telephone number, e-mail address, etc. Includes the address of a World Wide Web site operated by the person, about the person or related to the person."@en ;
	rdfs:domain <http://iflastandards.info/ns/fr/frbr/frbrer/C1005> ;
	rdfs:label "tiene dirección (persona)"@es .

<http://iflastandards.info/ns/fr/frad/P3034> rdfs:isDefinedBy <http://iflastandards.info/ns/fr/frad/> ;
	reg:status status:1001 ;
	reg:name "hasAffiliation"@en ;
	rdfs:label "has affiliation"@en ;
	skos:definition "Relates a person to a group with which the person is affiliated or has been affiliated through employment, membership, cultural identity, etc."@en ;
	a :Property ;
	rdfs:domain <http://iflastandards.info/ns/fr/frbr/frbrer/C1005> ;
	rdfs:label "tiene afiliación"@es .

<http://iflastandards.info/ns/fr/frad/P4002> rdfs:isDefinedBy <http://iflastandards.info/ns/fr/frad/> ;
	reg:status status:1001 ;
	reg:name "hasAlternateScriptForm"@en ;
	rdfs:label "has alternate script form"@en ;
	skos:definition "Relates controlled access points that are established as alternate script forms of the access point for the authorized forms of name for the same entity."@en ;
	a :Property ;
	rdfs:domain <http://iflastandards.info/ns/fr/frad/C1001> ;
	rdfs:range <http://iflastandards.info/ns/fr/frad/C1001> ;
	owl:propertyDisjointWith <http://iflastandards.info/ns/fr/frad/P4001> , <http://iflastandards.info/ns/fr/frad/P4003> .

<http://iflastandards.info/ns/fr/frad/P4025> rdfs:isDefinedBy <http://iflastandards.info/ns/fr/frad/> ;
	reg:status status:1001 ;
	reg:name "hasAlternativeLinguisticFormCorporateBody"@en ;
	rdfs:label "has alternative linguistic form (corporate body)"@en ;
	skos:definition "Relates a name of a corporate body and an alternative linguistic form of name by which that body is known."@en ;
	a :Property ;
	skos:scopeNote "Includes translations of the name for the corporate body."@en ;
	rdfs:domain <http://iflastandards.info/ns/fr/frad/C1011> ;
	rdfs:range <http://iflastandards.info/ns/fr/frad/C1011> ;
	rdfs:label "tiene forma lingüística alternativa (entidad corporativa)"@es ;
	owl:propertyDisjointWith <http://iflastandards.info/ns/fr/frad/P4026> , <http://iflastandards.info/ns/fr/frad/P4027> , <http://iflastandards.info/ns/fr/frad/P4032> .

<http://iflastandards.info/ns/fr/frad/P4024> rdfs:isDefinedBy <http://iflastandards.info/ns/fr/frad/> ;
	reg:status status:1001 ;
	reg:name "hasAlternativeLinguisticFormFamily"@en ;
	rdfs:label "has alternative linguistic form (family)"@en ;
	skos:definition "Relates a name of a family and an alternative linguistic form of name by which that family is known."@en ;
	a :Property ;
	rdfs:domain <http://iflastandards.info/ns/fr/frad/C1013> ;
	rdfs:range <http://iflastandards.info/ns/fr/frad/C1013> ;
	rdfs:label "tiene forma lingüística alternativa (familia)"@es .

<http://iflastandards.info/ns/fr/frad/P4034> rdfs:isDefinedBy <http://iflastandards.info/ns/fr/frad/> ;
	reg:status status:1001 ;
	reg:name "hasAlternativeLinguisticFormPerson"@en ;
	rdfs:label "has alternative linguistic form (person)"@en ;
	skos:definition "Relates a name of a person and an alternative linguistic form of name by which that person is known."@en ;
	a :Property ;
	skos:scopeNote "Includes translations of a name into other languages."@en ;
	rdfs:domain <http://iflastandards.info/ns/fr/frad/C1012> ;
	rdfs:range <http://iflastandards.info/ns/fr/frad/C1012> ;
	rdfs:label "tiene forma lingüística alternativa (persona)"@es .

<http://iflastandards.info/ns/fr/frad/P4028> rdfs:isDefinedBy <http://iflastandards.info/ns/fr/frad/> ;
	reg:status status:1001 ;
	reg:name "hasAlternativeLinguisticFormWork"@en ;
	rdfs:label "has alternative linguistic form (work)"@en ;
	skos:definition "Relates a name of a work and an alternative linguistic form of name by which that work is known."@en ;
	a :Property ;
	rdfs:domain <http://iflastandards.info/ns/fr/frad/C1014> ;
	rdfs:range <http://iflastandards.info/ns/fr/frad/C1014> ;
	rdfs:label "tiene forma lingüística alternativa (obra)"@es .

<http://iflastandards.info/ns/fr/frad/P2013> rdfs:isDefinedBy <http://iflastandards.info/ns/fr/frad/> ;
	reg:status status:1001 ;
	reg:name "hasAppellation"@en ;
	rdfs:label "has appellation"@en ;
	a :Property ;
	rdfs:domain <http://iflastandards.info/ns/fr/frad/C1010> ;
	skos:definition "Relates a bibliographic entity to a name."@en ;
	rdfs:range <http://iflastandards.info/ns/fr/frad/C1006> ;
	owl:inverseOf <http://iflastandards.info/ns/fr/frad/P2014> .

<http://iflastandards.info/ns/fr/frad/P4046> rdfs:isDefinedBy <http://iflastandards.info/ns/fr/frad/> ;
	reg:status status:1001 ;
	reg:name "hasAsSubjectFamily"@en ;
	rdfs:label "has as subject (family)"@en ;
	skos:definition "Relates a work to a family that is the subject of the work."@en ;
	a :Property ;
	rdfs:domain <http://iflastandards.info/ns/fr/frbr/frbrer/C1001> ;
	rdfs:range <http://iflastandards.info/ns/fr/frad/C1002> ;
	rdfs:label "tiene como materia (familia)"@es .

<http://iflastandards.info/ns/fr/frad/P4044> rdfs:isDefinedBy <http://iflastandards.info/ns/fr/frad/> ;
	reg:status status:1001 ;
	reg:name "hasAttributedWorksFrom"@en ;
	rdfs:label "has attributed works from"@en ;
	skos:definition "Relates a person (either a \"real\" individual or a persona) or identity to whom one or more works by another person have been attributed, either erroneously or falsely, and that other person."@en ;
	a :Property ;
	rdfs:domain <http://iflastandards.info/ns/fr/frbr/frbrer/C1005> ;
	rdfs:range <http://iflastandards.info/ns/fr/frbr/frbrer/C1005> ;
	owl:inverseOf <http://iflastandards.info/ns/fr/frad/P4043> .

<http://iflastandards.info/ns/fr/frad/P3017> rdfs:isDefinedBy <http://iflastandards.info/ns/fr/frad/> ;
	reg:status status:1001 ;
	reg:name "hasBaseAccessPoint"@en ;
	rdfs:label "has base access point"@en ;
	skos:definition "Relates a controlled access point to all elements in a controlled access point that are integral to the name or identifier that forms the basis for the access point."@en ;
	a :Property ;
	skos:scopeNote "Includes the name element in a controlled access point beginning with the name of a person, family, or corporate body. Includes the phrase element in a controlled access point beginning with a phrase associated with a person that is used in lieu of a name as such when the name of the person is unknown (e.g., A Physician, Author of Early Impressions). Includes the name element for a subordinate or related body in a controlled access point beginning with the name of a superior body. Includes the name element for a government agency, official, legislative body, court, etc., in a controlled access point beginning with the name for the territorial authority. Includes the name element for a religious council, official, province, synod, etc., in a controlled access point beginning with the name for the religious body. Includes the title element in a controlled access point for a work. Includes a term designating form at the beginning of the title element of a controlled access point for a musical work or expression (e.g., Symphony, Concerto). Includes conventional and collective titles at the beginning of the title element of a controlled access point for a work or expression (e.g., Treaties, Laws, Works, Selections, Piano music). Includes the additional  element(s) in a collective title controlled access point (i.e., a subsequent term or terms used to subdivide the collective uniform title)"@en ;
	rdfs:domain <http://iflastandards.info/ns/fr/frad/C1001> ;
	owl:propertyDisjointWith <http://iflastandards.info/ns/fr/frad/P3006> , <http://iflastandards.info/ns/fr/frad/P3007> , <http://iflastandards.info/ns/fr/frad/P3008> , <http://iflastandards.info/ns/fr/frad/P3009> , <http://iflastandards.info/ns/fr/frad/P4018> .

<http://iflastandards.info/ns/fr/frad/P3039> rdfs:isDefinedBy <http://iflastandards.info/ns/fr/frad/> ;
	reg:status status:1001 ;
	reg:name "hasBiographyOrHistory"@en ;
	rdfs:label "has biography or history"@en ;
	skos:definition "Relates a person to information pertaining to the life or history of the person."@en ;
	a :Property ;
	rdfs:domain <http://iflastandards.info/ns/fr/frbr/frbrer/C1005> ;
	rdfs:label "tiene biografía o historia"@es .

<http://iflastandards.info/ns/fr/frad/P4049> rdfs:isDefinedBy <http://iflastandards.info/ns/fr/frad/> ;
	reg:status status:1001 ;
	reg:name "hasChild"@en ;
	rdfs:label "has child"@en ;
	skos:definition "Relates a person to another person who is a \"child\" of that person."@en ;
	a :Property ;
	rdfs:domain <http://iflastandards.info/ns/fr/frbr/frbrer/C1005> ;
	rdfs:range <http://iflastandards.info/ns/fr/frbr/frbrer/C1005> ;
	owl:inverseOf <http://iflastandards.info/ns/fr/frad/P4048> ;
	owl:propertyDisjointWith <http://iflastandards.info/ns/fr/frad/P4048> .

<http://iflastandards.info/ns/fr/frad/P3019> rdfs:isDefinedBy <http://iflastandards.info/ns/fr/frad/> ;
	reg:status status:1001 ;
	reg:name "hasCitationForRules"@en ;
	rdfs:label "has citation for rules"@en ;
	skos:definition "Relates rules to a citation for the cataloguing code, set of rules, instructions, etc."@en ;
	a :Property ;
	skos:scopeNote "Includes the title of the rules, etc., and, as necessary, the name of the body responsible for the rules, the edition designation, date, etc."@en ;
	rdfs:domain <http://iflastandards.info/ns/fr/frad/C1007> ;
	rdfs:label "tiene cita de reglas"@es ;
	owl:propertyDisjointWith <http://iflastandards.info/ns/fr/frad/P3020> , <http://iflastandards.info/ns/fr/frad/P2001> , <http://iflastandards.info/ns/fr/frad/P2004> .

<http://iflastandards.info/ns/fr/frad/P4045> rdfs:isDefinedBy <http://iflastandards.info/ns/fr/frad/> ;
	reg:status status:1001 ;
	reg:name "hasCollaborativeRelationship"@en ;
	rdfs:label "has collaborative relationship"@en ;
	skos:definition "Relates two persons (i.e., individuals) who collaborate in intellectual or artistic endeavours"@en ;
	a :Property ;
	rdfs:domain <http://iflastandards.info/ns/fr/frbr/frbrer/C1005> ;
	rdfs:range <http://iflastandards.info/ns/fr/frbr/frbrer/C1005> ;
	rdfs:label "tiene relación colaborativa con"@es .

<http://iflastandards.info/ns/fr/frad/P4029> rdfs:isDefinedBy <http://iflastandards.info/ns/fr/frad/> ;
	reg:status status:1001 ;
	reg:name "hasConventionalName"@en ;
	rdfs:label "has conventional name"@en ;
	skos:definition "Relates a name of a work and a conventional name by which that work is known"@en ;
	a :Property ;
	rdfs:domain <http://iflastandards.info/ns/fr/frad/C1014> ;
	rdfs:range <http://iflastandards.info/ns/fr/frad/C1014> ;
	rdfs:label "tiene nombre convencional"@es ;
	owl:inverseOf <http://iflastandards.info/ns/fr/frad/P4030> .

<http://iflastandards.info/ns/fr/frad/P4018> rdfs:isDefinedBy <http://iflastandards.info/ns/fr/frad/> ;
	reg:status status:1001 ;
	reg:name "hasCorrespondingSubjectTermOrClassificationNumber"@en ;
	rdfs:label "has corresponding subject term or classification number"@en ;
	skos:definition "Relates a controlled access point for the name of a bibliographic entity and a subject term in a controlled vocabulary or a classification number for that entity."@en ;
	a :Property ;
	skos:scopeNote "The subject term and the classification number may also be viewed as parallel names or identifiers for the name of the same entity."@en ;
	rdfs:domain <http://iflastandards.info/ns/fr/frad/C1001> ;
	owl:propertyDisjointWith <http://iflastandards.info/ns/fr/frad/P3006> , <http://iflastandards.info/ns/fr/frad/P3007> , <http://iflastandards.info/ns/fr/frad/P3008> , <http://iflastandards.info/ns/fr/frad/P3009> , <http://iflastandards.info/ns/fr/frad/P3017> .

<http://iflastandards.info/ns/fr/frad/P3032> rdfs:isDefinedBy <http://iflastandards.info/ns/fr/frad/> ;
	reg:status status:1001 ;
	reg:name "hasCountry"@en ;
	rdfs:label "has country"@en ;
	skos:definition "Relates a person to a country with which the person is identified."@en ;
	a :Property ;
	rdfs:domain <http://iflastandards.info/ns/fr/frbr/frbrer/C1005> ;
	rdfs:label "tiene país"@es .

<http://iflastandards.info/ns/fr/frad/P3048> rdfs:isDefinedBy <http://iflastandards.info/ns/fr/frad/> ;
	reg:status status:1001 ;
	reg:name "hasCustodialHistoryOfItem"@en ;
	rdfs:label "has custodial history of item"@en ;
	skos:definition "Relates an item to the record of previous ownership of an item."@en ;
	a :Property ;
	rdfs:domain <http://iflastandards.info/ns/fr/frbr/frbrer/C1004> .

<http://iflastandards.info/ns/fr/frad/P3002> rdfs:isDefinedBy <http://iflastandards.info/ns/fr/frad/> ;
	reg:status status:1001 ;
	reg:name "hasDatesOfFamily"@en ;
	rdfs:label "has dates of family"@en ;
	skos:definition "Relates a family to dates associated with the family."@en ;
	a :Property ;
	rdfs:domain <http://iflastandards.info/ns/fr/frad/C1002> ;
	owl:propertyDisjointWith <http://iflastandards.info/ns/fr/frad/P3005> , <http://iflastandards.info/ns/fr/frad/P3004> , <http://iflastandards.info/ns/fr/frad/P3003> , <http://iflastandards.info/ns/fr/frad/P3001> .

<http://iflastandards.info/ns/fr/frad/P3025> rdfs:isDefinedBy <http://iflastandards.info/ns/fr/frad/> ;
	reg:status status:1001 ;
	reg:name "hasDatesOfUsage"@en ;
	rdfs:label "has dates of usage"@en ;
	skos:definition "Relates a name to dates associated with the use of a particular name established by a person, corporate body, or family."@en ;
	a :Property ;
	rdfs:domain <http://iflastandards.info/ns/fr/frad/C1006> ;
	rdfs:label "tiene fechas de uso"@es .

<http://iflastandards.info/ns/fr/frad/P2017> rdfs:isDefinedBy <http://iflastandards.info/ns/fr/frad/> ;
	reg:status status:1001 ;
	reg:name "hasDerivative"@en ;
	rdfs:label "has derivative"@en ;
	skos:definition "Relates a work to another work which is an adaptation or modification of the prior work."@en ;
	a :Property ;
	skos:scopeNote "Includes relationships between an original work and a broad range of modifications from the original, including variations or versions of that work, such as editions, revisions, translations, summaries, abstracts, and digests. Includes new works that are adaptations or modifications that become new works but are based on an earlier work (improvisations, etc.); new works that are changes of genre (transformations, dramatizations, novelizations, etc.); and, new works based on the style or thematic content of other works (free translations, paraphrases, imitations, parodies, etc.)."@en ;
	rdfs:domain <http://iflastandards.info/ns/fr/frbr/frbrer/C1001> ;
	rdfs:range <http://iflastandards.info/ns/fr/frbr/frbrer/C1001> ;
	rdfs:label "tiene derivada"@es ;
	owl:inverseOf <http://iflastandards.info/ns/fr/frad/P2018> .

<http://iflastandards.info/ns/fr/frad/P4008> rdfs:isDefinedBy <http://iflastandards.info/ns/fr/frad/> ;
	reg:status status:1001 ;
	reg:name "hasDescendentGenealogicalRelationship"@en ;
	rdfs:label "has (descendent) genealogical relationship"@en ;
	skos:definition "Relates a family to another family that descended from the prior family."@en ;
	a :Property ;
	rdfs:domain <http://iflastandards.info/ns/fr/frad/C1002> ;
	rdfs:range <http://iflastandards.info/ns/fr/frad/C1002> ;
	owl:inverseOf <http://iflastandards.info/ns/fr/frad/P4009> ;
	owl:propertyDisjointWith <http://iflastandards.info/ns/fr/frad/P4009> .

<http://iflastandards.info/ns/fr/frad/P2035> rdfs:isDefinedBy <http://iflastandards.info/ns/fr/frad/> ;
	reg:status status:1001 ;
	reg:name "hasDescriptiveWork"@en ;
	rdfs:label "has descriptive work"@en ;
	skos:definition "Relates a target work or expression or manifestation or item and a new work that refers to that target as its subject."@en ;
	a :Property ;
	skos:scopeNote "Includes criticism, commentary, review, casebook, etc., and the object of that analysis (that is, the target work, expression, or manifestation)."@en ;
	rdfs:range <http://iflastandards.info/ns/fr/frbr/frbrer/C1001> ;
	rdfs:label "tiene obra descriptiva"@es .

<http://iflastandards.info/ns/fr/frad/P3008> rdfs:isDefinedBy <http://iflastandards.info/ns/fr/frad/> ;
	reg:status status:1001 ;
	reg:name "hasDesignatedUsageOfControlledAccessPoint"@en ;
	rdfs:label "has designated usage of controlled access point"@en ;
	skos:definition "Relates a controlled access point to an indication of whether the rules under which the controlled access point was constructed designate it as an authorized (or preferred) form (i.e., authorized access point) or as a variant (or non-preferred) form (i.e., variant access points)."@en ;
	a :Property ;
	rdfs:domain <http://iflastandards.info/ns/fr/frad/C1001> ;
	owl:propertyDisjointWith <http://iflastandards.info/ns/fr/frad/P3006> , <http://iflastandards.info/ns/fr/frad/P3007> , <http://iflastandards.info/ns/fr/frad/P3009> , <http://iflastandards.info/ns/fr/frad/P3017> , <http://iflastandards.info/ns/fr/frad/P4018> .

<http://iflastandards.info/ns/fr/frad/P4003> rdfs:isDefinedBy <http://iflastandards.info/ns/fr/frad/> ;
	reg:status status:1001 ;
	reg:name "hasDifferentRulesForm"@en ;
	rdfs:label "has different rules form"@en ;
	skos:definition "Relates controlled access points for the authorized forms of name for the same entity that have been established according to different sets of rules."@en ;
	a :Property ;
	rdfs:domain <http://iflastandards.info/ns/fr/frad/C1001> ;
	rdfs:range <http://iflastandards.info/ns/fr/frad/C1001> ;
	owl:propertyDisjointWith <http://iflastandards.info/ns/fr/frad/P4002> , <http://iflastandards.info/ns/fr/frad/P4001> .

<http://iflastandards.info/ns/fr/frad/P4021> rdfs:isDefinedBy <http://iflastandards.info/ns/fr/frad/> ;
	reg:status status:1001 ;
	reg:name "hasEarlierName"@en ;
	rdfs:label "has earlier name"@en ;
	a :Property ;
	skos:definition "Relates a name of a person to a name that person used at an earlier stage in life."@en ;
	rdfs:domain <http://iflastandards.info/ns/fr/frad/C1012> ;
	rdfs:range <http://iflastandards.info/ns/fr/frad/C1012> ;
	rdfs:label "tiene nombre anterior"@es ;
	owl:inverseOf <http://iflastandards.info/ns/fr/frad/P4022> .

<http://iflastandards.info/ns/fr/frad/P2037> rdfs:isDefinedBy <http://iflastandards.info/ns/fr/frad/> ;
	reg:status status:1001 ;
	reg:name "hasEquivalenceItemRelationship"@en ;
	rdfs:label "has equivalence (item) relationship"@en ;
	a :Property ;
	skos:definition "Relates an item to another item that exemplifies the same intellectual or artistic content (work or work-expression)."@en ;
	rdfs:domain <http://iflastandards.info/ns/fr/frbr/frbrer/C1004> ;
	rdfs:range <http://iflastandards.info/ns/fr/frbr/frbrer/C1004> .

<http://iflastandards.info/ns/fr/frad/P2019> rdfs:isDefinedBy <http://iflastandards.info/ns/fr/frad/> ;
	reg:status status:1001 ;
	reg:name "hasEquivalenceManifestationRelationship"@en ;
	rdfs:label "has equivalence (manifestation) relationship"@en ;
	skos:definition "Relates a manifestation to another manifestation that embodies the same intellectual or artistic content (work or work-expression)."@en ;
	a :Property ;
	rdfs:domain <http://iflastandards.info/ns/fr/frbr/frbrer/C1003> ;
	rdfs:range <http://iflastandards.info/ns/fr/frbr/frbrer/C1003> .

<http://iflastandards.info/ns/fr/frad/P4026> rdfs:isDefinedBy <http://iflastandards.info/ns/fr/frad/> ;
	reg:status status:1001 ;
	reg:name "hasExpandedName"@en ;
	rdfs:label "has expanded name"@en ;
	skos:definition "Relates a name of a corporate body and the expanded form of name by which that body is known."@en ;
	a :Property ;
	rdfs:domain <http://iflastandards.info/ns/fr/frad/C1011> ;
	rdfs:range <http://iflastandards.info/ns/fr/frad/C1011> ;
	rdfs:label "tiene nombre extenso"@es ;
	owl:inverseOf <http://iflastandards.info/ns/fr/frad/P4027> ;
	owl:propertyDisjointWith <http://iflastandards.info/ns/fr/frad/P4025> , <http://iflastandards.info/ns/fr/frad/P4027> , <http://iflastandards.info/ns/fr/frad/P4032> .

<http://iflastandards.info/ns/fr/frad/P3042> rdfs:isDefinedBy <http://iflastandards.info/ns/fr/frad/> ;
	reg:status status:1001 ;
	reg:name "hasFieldOfActivityCorporateBody"@en ;
	rdfs:label "has field of activity (corporate body)"@en ;
	skos:definition "Relates a corporate body to a field of business in which the corporate body is engaged, its area of competence, responsibility, jurisdiction, etc."@en ;
	a :Property ;
	rdfs:domain <http://iflastandards.info/ns/fr/frad/C1003> ;
	rdfs:label "tiene campo de actividad (entidad corporativa)"@es ;
	owl:propertyDisjointWith <http://iflastandards.info/ns/fr/frad/P3043> , <http://iflastandards.info/ns/fr/frad/P3041> , <http://iflastandards.info/ns/fr/frad/P3040> .

<http://iflastandards.info/ns/fr/frad/P3004> rdfs:isDefinedBy <http://iflastandards.info/ns/fr/frad/> ;
	reg:status status:1001 ;
	reg:name "hasFieldOfActivityFamily"@en ;
	rdfs:label "has field of activity (family)"@en ;
	skos:definition "Relates a family to afield of endeavour, area of expertise, etc., in which the family is engaged or was engaged."@en ;
	a :Property ;
	rdfs:domain <http://iflastandards.info/ns/fr/frad/C1002> ;
	rdfs:label "tiene campo de actividad (familia)"@es ;
	owl:propertyDisjointWith <http://iflastandards.info/ns/fr/frad/P3005> , <http://iflastandards.info/ns/fr/frad/P3003> , <http://iflastandards.info/ns/fr/frad/P3002> , <http://iflastandards.info/ns/fr/frad/P3001> .

<http://iflastandards.info/ns/fr/frad/P3037> rdfs:isDefinedBy <http://iflastandards.info/ns/fr/frad/> ;
	reg:status status:1001 ;
	reg:name "hasFieldOfActivityPerson"@en ;
	rdfs:label "has field of activity (person)"@en ;
	skos:definition "Relates a person to a field of endeavour, area of expertise, etc., in which the person is engaged or was engaged."@en ;
	a :Property ;
	rdfs:domain <http://iflastandards.info/ns/fr/frbr/frbrer/C1005> ;
	rdfs:label "tiene campo de actividad (persona)"@es .

<http://iflastandards.info/ns/fr/frad/P4011> rdfs:isDefinedBy <http://iflastandards.info/ns/fr/frad/> ;
	reg:status status:1001 ;
	reg:name "hasFounder"@en ;
	rdfs:label "has founder"@en ;
	skos:definition "Relates a corporate body to a family which created it."@en ;
	a :Property ;
	rdfs:domain <http://iflastandards.info/ns/fr/frad/C1003> ;
	rdfs:range <http://iflastandards.info/ns/fr/frad/C1002> ;
	owl:inverseOf <http://iflastandards.info/ns/fr/frad/P4010> .

<http://iflastandards.info/ns/fr/frad/P3029> rdfs:isDefinedBy <http://iflastandards.info/ns/fr/frad/> ;
	reg:status status:1001 ;
	reg:name "hasGender"@en ;
	rdfs:label "has gender"@en ;
	skos:definition "Relates a person to a gender by which the person is identified."@en ;
	a :Property ;
	skos:scopeNote "E.g., male, female, unknown, other."@en ;
	rdfs:domain <http://iflastandards.info/ns/fr/frbr/frbrer/C1005> ;
	rdfs:label "tiene género"@es ;
	owl:propertyDisjointWith <http://iflastandards.info/ns/fr/frad/P3030> , <http://iflastandards.info/ns/fr/frad/P3031> , <http://iflastandards.info/ns/fr/frad/P3032> , <http://iflastandards.info/ns/fr/frad/P3033> , <http://iflastandards.info/ns/fr/frad/P3034> , <http://iflastandards.info/ns/fr/frad/P3035> , <http://iflastandards.info/ns/fr/frad/P3036> , <http://iflastandards.info/ns/fr/frad/P3037> , <http://iflastandards.info/ns/fr/frad/P3038> , <http://iflastandards.info/ns/fr/frad/P3039> .

<http://iflastandards.info/ns/fr/frad/P3043> rdfs:isDefinedBy <http://iflastandards.info/ns/fr/frad/> ;
	reg:status status:1001 ;
	reg:name "hasHistoryCorporateBody"@en ;
	rdfs:label "has history (corporate body)"@en ;
	skos:definition "Relates a corporate body to information pertaining to the history of the corporate body."@en ;
	a :Property ;
	skos:scopeNote "Includes historical information pertaining to an organization, institution, etc."@en ;
	rdfs:domain <http://iflastandards.info/ns/fr/frad/C1003> ;
	owl:propertyDisjointWith <http://iflastandards.info/ns/fr/frad/P3040> , <http://iflastandards.info/ns/fr/frad/P3041> , <http://iflastandards.info/ns/fr/frad/P3042> .

<http://iflastandards.info/ns/fr/frad/P3005> rdfs:isDefinedBy <http://iflastandards.info/ns/fr/frad/> ;
	reg:status status:1001 ;
	reg:name "hasHistoryOfFamily"@en ;
	rdfs:label "has history of family"@en ;
	skos:definition "Relates a family to information pertaining to the history of the family."@en ;
	a :Property ;
	rdfs:domain <http://iflastandards.info/ns/fr/frad/C1002> ;
	owl:propertyDisjointWith <http://iflastandards.info/ns/fr/frad/P3001> , <http://iflastandards.info/ns/fr/frad/P3002> , <http://iflastandards.info/ns/fr/frad/P3003> , <http://iflastandards.info/ns/fr/frad/P3004> .

<http://iflastandards.info/ns/fr/frad/P3046> rdfs:isDefinedBy <http://iflastandards.info/ns/fr/frad/> ;
	reg:status status:1001 ;
	reg:name "hasHistoryWork"@en ;
	rdfs:label "has history (work)"@en ;
	skos:definition "Relates a work to information pertaining to the history of the work."@en ;
	a :Property ;
	skos:scopeNote "Includes historical information pertaining to a work, including title changes for continuing resources."@en ;
	rdfs:domain <http://iflastandards.info/ns/fr/frbr/frbrer/C1001> ;
	rdfs:label "tiene historia (obra)"@es .

<http://iflastandards.info/ns/fr/frad/P3049> rdfs:isDefinedBy <http://iflastandards.info/ns/fr/frad/> ;
	reg:status status:1001 ;
	reg:name "hasImmediateSourceOfAcquisitionOfItem"@en ;
	rdfs:label "has immediate source of acquisition of item"@en ;
	skos:definition "Relates an item to the source from which an item was directly acquired and the circumstances under which it was acquired."@en ;
	a :Property ;
	rdfs:domain <http://iflastandards.info/ns/fr/frbr/frbrer/C1004> .

<http://iflastandards.info/ns/fr/frad/P3010> rdfs:isDefinedBy <http://iflastandards.info/ns/fr/frad/> ;
	reg:status status:1001 ;
	reg:name "hasLanguageOfBaseAccessPoint"@en ;
	rdfs:label "has language of base access point"@en ;
	skos:definition "Relates a controlled access point to the language in which the base access point is recorded."@en ;
	a :Property ;
	rdfs:domain <http://iflastandards.info/ns/fr/frad/C1001> .

<http://iflastandards.info/ns/fr/frad/P3011> rdfs:isDefinedBy <http://iflastandards.info/ns/fr/frad/> ;
	reg:status status:1001 ;
	reg:name "hasLanguageOfCataloguing"@en ;
	rdfs:label "has language of cataloguing"@en ;
	skos:definition "Relates a controlled access point to the language in which additions to the base access point are recorded."@en ;
	a :Property ;
	rdfs:domain <http://iflastandards.info/ns/fr/frad/C1001> ;
	rdfs:label "tiene lengua de catalogación"@es .

<http://iflastandards.info/ns/fr/frad/P3052> rdfs:isDefinedBy <http://iflastandards.info/ns/fr/frad/> ;
	reg:status status:1001 ;
	reg:name "hasLanguageOfFamily"@en ;
	rdfs:label "has language of family"@en ;
	skos:definition "Relates a family to a language associated with the family."@en ;
	a :Property ;
	rdfs:domain <http://iflastandards.info/ns/fr/frad/C1002> .

<http://iflastandards.info/ns/fr/frad/P3026> rdfs:isDefinedBy <http://iflastandards.info/ns/fr/frad/> ;
	reg:status status:1001 ;
	reg:name "hasLanguageOfName"@en ;
	rdfs:label "has language of name"@en ;
	skos:definition "Relates a name to the language in which the name is expressed."@en ;
	a :Property ;
	rdfs:domain <http://iflastandards.info/ns/fr/frad/C1006> .

<http://iflastandards.info/ns/fr/frad/P3036> rdfs:isDefinedBy <http://iflastandards.info/ns/fr/frad/> ;
	reg:status status:1001 ;
	reg:name "hasLanguageOfPerson"@en ;
	rdfs:label "has language of person"@en ;
	skos:definition "Relates a person to a language the person uses when creating an expression for publication, broadcasting, etc."@en ;
	a :Property ;
	rdfs:domain <http://iflastandards.info/ns/fr/frbr/frbrer/C1005> .

<http://iflastandards.info/ns/fr/frad/P3040> rdfs:isDefinedBy <http://iflastandards.info/ns/fr/frad/> ;
	reg:status status:1001 ;
	reg:name "hasLanguageOfTheCorporateBody"@en ;
	rdfs:label "has language of the corporate body"@en ;
	skos:definition "Relates a corporate body to a language that the corporate body uses in its communications."@en ;
	a :Property ;
	rdfs:domain <http://iflastandards.info/ns/fr/frad/C1003> ;
	owl:propertyDisjointWith <http://iflastandards.info/ns/fr/frad/P3041> , <http://iflastandards.info/ns/fr/frad/P3042> , <http://iflastandards.info/ns/fr/frad/P3043> .

<http://iflastandards.info/ns/fr/frad/P4022> rdfs:isDefinedBy <http://iflastandards.info/ns/fr/frad/> ;
	reg:status status:1001 ;
	reg:name "hasLaterName"@en ;
	rdfs:label "has later name"@en ;
	skos:definition "Relates a name of a person and a name that person used at a later stage in life."@en ;
	a :Property ;
	rdfs:domain <http://iflastandards.info/ns/fr/frad/C1012> ;
	rdfs:range <http://iflastandards.info/ns/fr/frad/C1012> ;
	rdfs:label "tiene nombre posterior"@es ;
	owl:inverseOf <http://iflastandards.info/ns/fr/frad/P4021> .

<http://iflastandards.info/ns/fr/frad/P3047> rdfs:isDefinedBy <http://iflastandards.info/ns/fr/frad/> ;
	reg:status status:1001 ;
	reg:name "hasLocationOfItem"@en ;
	rdfs:label "has location of item"@en ;
	skos:definition "Relates an item to the collection and/or institution in which the item is held, stored, or made available for access."@en ;
	a :Property ;
	rdfs:domain <http://iflastandards.info/ns/fr/frbr/frbrer/C1004> ;
	rdfs:comment "Scope note not present in original documentation; added to clarify semantic difference with \"is part (item)\" property (http://iflastandards.info/ns/fr/frbr/frbrer/P2092)."@en ;
	skos:scopeNote "E.g. Moir rare book collection, http://www.juilliardmanuscriptcollection.org/, Short loan collection (School of African and Oriental Studies, University of London), Library of Congress. Does not include collections where the item is originally published or manufactured as a component part."@en .

<http://iflastandards.info/ns/fr/frad/P4006> rdfs:isDefinedBy <http://iflastandards.info/ns/fr/frad/> ;
	reg:status status:1001 ;
	reg:name "hasMemberCorporateBody"@en ;
	rdfs:label "has member (corporate body)"@en ;
	skos:definition "Relates a corporate body to a person who is a member of or affiliated with the corporate body."@en ;
	a :Property ;
	rdfs:domain <http://iflastandards.info/ns/fr/frad/C1003> ;
	rdfs:range <http://iflastandards.info/ns/fr/frbr/frbrer/C1005> ;
	owl:inverseOf <http://iflastandards.info/ns/fr/frad/P4007> .

<http://iflastandards.info/ns/fr/frad/P4004> rdfs:isDefinedBy <http://iflastandards.info/ns/fr/frad/> ;
	reg:status status:1001 ;
	reg:name "hasMemberFamily"@en ;
	rdfs:label "has member (family)"@en ;
	skos:definition "Relates a family to a person who is a member of the family."@en ;
	a :Property ;
	rdfs:domain <http://iflastandards.info/ns/fr/frad/C1002> ;
	rdfs:range <http://iflastandards.info/ns/fr/frbr/frbrer/C1005> .

<http://iflastandards.info/ns/fr/frad/P3023> rdfs:isDefinedBy <http://iflastandards.info/ns/fr/frad/> ;
	reg:status status:1001 ;
	reg:name "hasNameString"@en ;
	rdfs:label "has name string"@en ;
	skos:definition "Relates a name to a sequence of numeric and/or alphabetic characters or symbols that represents the name of an entity."@en ;
	a :Property ;
	rdfs:domain <http://iflastandards.info/ns/fr/frad/C1006> ;
	rdfs:label "tiene cadena de caracteres"@es .

<http://iflastandards.info/ns/fr/frad/P3051> rdfs:isDefinedBy <http://iflastandards.info/ns/fr/frad/> ;
	reg:status status:1001 ;
	reg:name "hasNumericDesignation"@en ;
	rdfs:label "has numeric designation"@en ;
	a :Property ;
	skos:definition "Relates a work to a number assigned to it."@en ;
	skos:scopeNote "Includes serial numbers, opus numbers assigned by the composer of a musical work, etc."@en ;
	rdfs:domain <http://iflastandards.info/ns/fr/frbr/frbrer/C1001> ;
	rdfs:label "tiene designación numérica"@es .

<http://iflastandards.info/ns/fr/frad/P4041> rdfs:isDefinedBy <http://iflastandards.info/ns/fr/frad/> ;
	reg:status status:1001 ;
	reg:name "hasOfficialIdentity"@en ;
	rdfs:label "has official identity"@en ;
	skos:definition "Relates a person and an identity that person assumes in an official capacity."@en ;
	a :Property ;
	rdfs:range <http://iflastandards.info/ns/fr/frbr/frbrer/C1005> ;
	rdfs:domain <http://iflastandards.info/ns/fr/frbr/frbrer/C1005> ;
	rdfs:label "tiene identidad oficial"@es ;
	owl:inverseOf <http://iflastandards.info/ns/fr/frad/P4042> .

<http://iflastandards.info/ns/fr/frad/P4032> rdfs:isDefinedBy <http://iflastandards.info/ns/fr/frad/> ;
	reg:status status:1001 ;
	reg:name "hasOtherVariantNameCorporateBody"@en ;
	rdfs:label "has other variant name (corporate body)"@en ;
	skos:definition "Relates a name of a corporate body and a name by which that body is known (other than expanded name, acronym, initials, abbreviation, and alternative linguistic form)."@en ;
	a :Property ;
	skos:scopeNote "Includes orthographic variant names (spelling variations, transliterations, punctuation variations, capitalization variations), word order variant names (inversions, permutations)."@en ;
	rdfs:domain <http://iflastandards.info/ns/fr/frad/C1011> ;
	rdfs:range <http://iflastandards.info/ns/fr/frad/C1011> ;
	owl:propertyDisjointWith <http://iflastandards.info/ns/fr/frad/P4025> , <http://iflastandards.info/ns/fr/frad/P4026> , <http://iflastandards.info/ns/fr/frad/P4027> .

<http://iflastandards.info/ns/fr/frad/P4031> rdfs:isDefinedBy <http://iflastandards.info/ns/fr/frad/> ;
	reg:status status:1001 ;
	reg:name "hasOtherVariantNamePerson"@en ;
	rdfs:label "has other variant name (person)"@en ;
	skos:definition "Relates a name of a person and several other variations on a name (other than earlier name, later name, and alternative linguistic form)."@en ;
	a :Property ;
	skos:scopeNote "Includes orthographic variant names (spelling variations, transliterations, punctuation variations, capitalization variations), word order variant names (inversions, permutations), alternative name/synonym variant names (bynames, nicknames, courtesy names)."@en ;
	rdfs:domain <http://iflastandards.info/ns/fr/frad/C1012> ;
	rdfs:range <http://iflastandards.info/ns/fr/frad/C1012> .

<http://iflastandards.info/ns/fr/frad/P4033> rdfs:isDefinedBy <http://iflastandards.info/ns/fr/frad/> ;
	reg:status status:1001 ;
	reg:name "hasOtherVariantNameWork"@en ;
	rdfs:label "has other variant name (work)"@en ;
	skos:definition "Relates a name of a work and a name by which that work is known (other than conventional name, and alternative linguistic form)."@en ;
	a :Property ;
	skos:scopeNote "Includes orthographic variant names(spelling variations, transliterations, punctuation variations, capitalization variations), word order variant names(inversions, permutations), variant title variant names (titles for the work based on titles found on manifestations or items, including cover title, spine title, caption title, container title, parallel title)."@en ;
	rdfs:domain <http://iflastandards.info/ns/fr/frad/C1014> ;
	rdfs:range <http://iflastandards.info/ns/fr/frad/C1014> .

<http://iflastandards.info/ns/fr/frad/P4013> rdfs:isDefinedBy <http://iflastandards.info/ns/fr/frad/> ;
	reg:status status:1001 ;
	reg:name "hasOwner"@en ;
	rdfs:label "has owner"@en ;
	a :Property ;
	skos:definition "Relates a corporate body to a family which owns it."@en ;
	rdfs:domain <http://iflastandards.info/ns/fr/frad/C1003> ;
	rdfs:range <http://iflastandards.info/ns/fr/frad/C1002> ;
	rdfs:label "tiene propietario"@es ;
	owl:inverseOf <http://iflastandards.info/ns/fr/frad/P4012> .

<http://iflastandards.info/ns/fr/frad/P4001> rdfs:isDefinedBy <http://iflastandards.info/ns/fr/frad/> ;
	reg:status status:1001 ;
	reg:name "hasParallelLanguageForm"@en ;
	rdfs:label "has parallel language form"@en ;
	skos:definition "Relates controlled access points that are established as parallel language forms of access point for the authorized forms of name for the same entity."@en ;
	a :Property ;
	rdfs:domain <http://iflastandards.info/ns/fr/frad/C1001> ;
	rdfs:range <http://iflastandards.info/ns/fr/frad/C1001> ;
	owl:propertyDisjointWith <http://iflastandards.info/ns/fr/frad/P4002> , <http://iflastandards.info/ns/fr/frad/P4003> .

<http://iflastandards.info/ns/fr/frad/P4048> rdfs:isDefinedBy <http://iflastandards.info/ns/fr/frad/> ;
	reg:status status:1001 ;
	reg:name "hasParent"@en ;
	rdfs:label "has parent"@en ;
	skos:definition "Relates a person to another person who is a “parent”  of that person."@en ;
	a :Property ;
	rdfs:domain <http://iflastandards.info/ns/fr/frad/C1003> ;
	rdfs:range <http://iflastandards.info/ns/fr/frad/C1003> ;
	owl:inverseOf <http://iflastandards.info/ns/fr/frad/P4049> ;
	owl:propertyDisjointWith <http://iflastandards.info/ns/fr/frad/P4049> .

<http://iflastandards.info/ns/fr/frad/P3030> rdfs:isDefinedBy <http://iflastandards.info/ns/fr/frad/> ;
	reg:status status:1001 ;
	reg:name "hasPlaceOfBirth"@en ;
	rdfs:label "has place of birth"@en ;
	skos:definition "Relates a person to the town, city, province, state, and/or country in which the person was born."@en ;
	a :Property ;
	rdfs:domain <http://iflastandards.info/ns/fr/frbr/frbrer/C1005> ;
	rdfs:label "tiene lugar de nacimiento"@es ;
	owl:propertyDisjointWith <http://iflastandards.info/ns/fr/frad/P3029> , <http://iflastandards.info/ns/fr/frad/P3032> , <http://iflastandards.info/ns/fr/frad/P3034> , <http://iflastandards.info/ns/fr/frad/P3035> , <http://iflastandards.info/ns/fr/frad/P3036> , <http://iflastandards.info/ns/fr/frad/P3037> , <http://iflastandards.info/ns/fr/frad/P3038> , <http://iflastandards.info/ns/fr/frad/P3039> .

<http://iflastandards.info/ns/fr/frad/P3031> rdfs:isDefinedBy <http://iflastandards.info/ns/fr/frad/> ;
	reg:status status:1001 ;
	reg:name "hasPlaceOfDeath"@en ;
	rdfs:label "has place of death"@en ;
	skos:definition "Relates a person to the town, city, province, state, and/or country in which the person died."@en ;
	a :Property ;
	rdfs:domain <http://iflastandards.info/ns/fr/frbr/frbrer/C1005> ;
	rdfs:label "tiene lugar de fallecimiento"@es ;
	owl:propertyDisjointWith <http://iflastandards.info/ns/fr/frad/P3029> , <http://iflastandards.info/ns/fr/frad/P3032> , <http://iflastandards.info/ns/fr/frad/P3034> , <http://iflastandards.info/ns/fr/frad/P3035> , <http://iflastandards.info/ns/fr/frad/P3036> , <http://iflastandards.info/ns/fr/frad/P3037> , <http://iflastandards.info/ns/fr/frad/P3038> , <http://iflastandards.info/ns/fr/frad/P3039> .

<http://iflastandards.info/ns/fr/frad/P3045> rdfs:isDefinedBy <http://iflastandards.info/ns/fr/frad/> ;
	reg:status status:1001 ;
	reg:name "hasPlaceOfOriginOfTheWork"@en ;
	rdfs:label "has place of origin of the work"@en ;
	skos:definition "Relates a work to the country or other territorial jurisdiction or cultural area from which the work originated."@en ;
	a :Property ;
	skos:scopeNote "Includes area of origin, etc."@en ;
	rdfs:domain <http://iflastandards.info/ns/fr/frbr/frbrer/C1001> ;
	rdfs:label "tiene lugar de origen de la obra"@es .

<http://iflastandards.info/ns/fr/frad/P3033> rdfs:isDefinedBy <http://iflastandards.info/ns/fr/frad/> ;
	reg:status status:1001 ;
	reg:name "hasPlaceOfResidence"@en ;
	rdfs:label "has place of residence"@en ;
	skos:definition "Relates a person to a country, state/province, city, etc., in which the person resides or has resided."@en ;
	a :Property ;
	rdfs:domain <http://iflastandards.info/ns/fr/frbr/frbrer/C1005> ;
	rdfs:label "tiene lugar de residencia"@es .

<http://iflastandards.info/ns/fr/frad/P3003> rdfs:isDefinedBy <http://iflastandards.info/ns/fr/frad/> ;
	reg:status status:1001 ;
	reg:name "hasPlacesAssociatedWithFamily"@en ;
	rdfs:label "has places associated with family"@en ;
	skos:definition "Relates a family to information pertaining to places where the family resides or resided or had some connection."@en ;
	a :Property ;
	rdfs:domain <http://iflastandards.info/ns/fr/frad/C1002> ;
	owl:propertyDisjointWith <http://iflastandards.info/ns/fr/frad/P3001> , <http://iflastandards.info/ns/fr/frad/P3002> , <http://iflastandards.info/ns/fr/frad/P3004> , <http://iflastandards.info/ns/fr/frad/P3005> .

<http://iflastandards.info/ns/fr/frad/P4009> rdfs:isDefinedBy <http://iflastandards.info/ns/fr/frad/> ;
	reg:status status:1001 ;
	reg:name "hasPredecessorGenealogicalRelationship"@en ;
	rdfs:label "has (predecessor) genealogical relationship"@en ;
	skos:definition "Relates a family to another family which is the precursor of the prior family."@en ;
	a :Property ;
	rdfs:domain <http://iflastandards.info/ns/fr/frad/C1002> ;
	rdfs:range <http://iflastandards.info/ns/fr/frad/C1002> ;
	owl:inverseOf <http://iflastandards.info/ns/fr/frad/P4008> ;
	owl:propertyDisjointWith <http://iflastandards.info/ns/fr/frad/P4008> .

<http://iflastandards.info/ns/fr/frad/P3038> rdfs:isDefinedBy <http://iflastandards.info/ns/fr/frad/> ;
	reg:status status:1001 ;
	reg:name "hasProfessionOrOccupation"@en ;
	rdfs:label "has profession or occupation"@en ;
	skos:definition "Relates a person to a profession or occupation in which the person works or worked."@en ;
	a :Property ;
	rdfs:domain <http://iflastandards.info/ns/fr/frbr/frbrer/C1005> .

<http://iflastandards.info/ns/fr/frad/P4035> rdfs:isDefinedBy <http://iflastandards.info/ns/fr/frad/> ;
	reg:status status:1001 ;
	reg:name "hasPseudonymousPersona"@en ;
	rdfs:label "has pseudonymous persona"@en ;
	skos:definition "Relates a \"real\" person (i.e., an individual) and a persona(ae) or identity adopted by that individual through the use of one or more pseudonyms."@en ;
	a :Property ;
	rdfs:range <http://iflastandards.info/ns/fr/frbr/frbrer/C1005> ;
	rdfs:domain <http://iflastandards.info/ns/fr/frbr/frbrer/C1005> ;
	owl:inverseOf <http://iflastandards.info/ns/fr/frad/P4036> .

<http://iflastandards.info/ns/fr/frad/P4019> rdfs:isDefinedBy <http://iflastandards.info/ns/fr/frad/> ;
	reg:status status:1001 ;
	reg:name "hasRelatedIdentifier"@en ;
	rdfs:label "has related identifier"@en ;
	skos:definition "Relates a controlled access point based on an authorized or variant form of name of a bibliographic entity to an identifier for the same bibliographic entity."@en ;
	a :Property ;
	rdfs:domain <http://iflastandards.info/ns/fr/frad/C1001> ;
	rdfs:range <http://iflastandards.info/ns/fr/frad/C1009> ;
	rdfs:label "tiene identificador relacionado"@es .

<http://iflastandards.info/ns/fr/frad/P4039> rdfs:isDefinedBy <http://iflastandards.info/ns/fr/frad/> ;
	reg:status status:1001 ;
	reg:name "hasReligiousIdentity"@en ;
	rdfs:label "has religious identity"@en ;
	skos:definition "Relates a person and an identity that person assumes in a religious capacity."@en ;
	a :Property ;
	rdfs:range <http://iflastandards.info/ns/fr/frbr/frbrer/C1005> ;
	rdfs:domain <http://iflastandards.info/ns/fr/frbr/frbrer/C1005> ;
	rdfs:label "tiene identidad religiosa"@es ;
	owl:equivalentProperty <http://iflastandards.info/ns/fr/frad/P4038> ;
	owl:inverseOf <http://iflastandards.info/ns/fr/frad/P4040> .

<http://iflastandards.info/ns/fr/frad/P3020> rdfs:isDefinedBy <http://iflastandards.info/ns/fr/frad/> ;
	reg:status status:1001 ;
	reg:name "hasRulesIdentifier"@en ;
	rdfs:label "has rules identifier"@en ;
	skos:definition "Relates rules to an acronym or initials or alphanumeric code identifying the rules."@en ;
	a :Property ;
	rdfs:domain <http://iflastandards.info/ns/fr/frad/C1007> ;
	rdfs:label "tiene identificador de reglas"@es ;
	owl:propertyDisjointWith <http://iflastandards.info/ns/fr/frad/P3019> , <http://iflastandards.info/ns/fr/frad/P2001> , <http://iflastandards.info/ns/fr/frad/P2004> .

<http://iflastandards.info/ns/fr/frad/P3024> rdfs:isDefinedBy <http://iflastandards.info/ns/fr/frad/> ;
	reg:status status:1001 ;
	reg:name "hasScopeOfUsage"@en ;
	rdfs:label "has scope of usage"@en ;
	skos:definition "Relates a name to the form of work associated with a particular name for a persona."@en ;
	a :Property ;
	skos:scopeNote "Includes forms, genres, etc., (e.g., literary works, critical works, works on mathematics, detective novels) associated with a name used by an author."@en ;
	rdfs:domain <http://iflastandards.info/ns/fr/frad/C1006> ;
	rdfs:label "tiene alcance de uso"@es .

<http://iflastandards.info/ns/fr/frad/P3012> rdfs:isDefinedBy <http://iflastandards.info/ns/fr/frad/> ;
	reg:status status:1001 ;
	reg:name "hasScriptOfBaseAccessPoint"@en ;
	rdfs:label "has script of base access point"@en ;
	skos:definition "Relates a controlled access point to the form of graphic characters in which the data in the base access point are recorded."@en ;
	a :Property ;
	rdfs:domain <http://iflastandards.info/ns/fr/frad/C1001> .

<http://iflastandards.info/ns/fr/frad/P3013> rdfs:isDefinedBy <http://iflastandards.info/ns/fr/frad/> ;
	reg:status status:1001 ;
	reg:name "hasScriptOfCataloguing"@en ;
	rdfs:label "has script of cataloguing"@en ;
	skos:definition "Relates a controlled access point to the form of graphic characters in which any additions to the base access point are recorded."@en ;
	a :Property ;
	rdfs:domain <http://iflastandards.info/ns/fr/frad/C1001> .

<http://iflastandards.info/ns/fr/frad/P3027> rdfs:isDefinedBy <http://iflastandards.info/ns/fr/frad/> ;
	reg:status status:1001 ;
	reg:name "hasScriptOfName"@en ;
	rdfs:label "has script of name"@en ;
	skos:definition "Relates a name to the script in which the name is rendered"@en ;
	a :Property ;
	rdfs:domain <http://iflastandards.info/ns/fr/frad/C1006> .

<http://iflastandards.info/ns/fr/frad/P4037> rdfs:isDefinedBy <http://iflastandards.info/ns/fr/frad/> ;
	reg:status status:1001 ;
	reg:name "hasSecularIdentity"@en ;
	rdfs:label "has secular identity"@en ;
	skos:definition "Relates a person and an identity that person assumes in a secular capacity."@en ;
	a :Property ;
	rdfs:range <http://iflastandards.info/ns/fr/frbr/frbrer/C1005> ;
	rdfs:domain <http://iflastandards.info/ns/fr/frbr/frbrer/C1005> ;
	rdfs:label "tiene identidad secular"@es ;
	owl:equivalentProperty <http://iflastandards.info/ns/fr/frad/P4040> ;
	owl:inverseOf <http://iflastandards.info/ns/fr/frad/P4038> .

<http://iflastandards.info/ns/fr/frad/P2029> rdfs:isDefinedBy <http://iflastandards.info/ns/fr/frad/> ;
	reg:status status:1001 ;
	reg:name "hasSequentialRelationship"@en ;
	rdfs:label "has sequential relationship"@en ;
	skos:definition "Relates a work to another work of different content that is a successor or a predecessor of that work,"@en ;
	a :Property ;
	skos:scopeNote "E.g. a sequel, a serial or series that has changed title. Excludes derivative works that modify the content of an earlier work."@en ;
	rdfs:domain <http://iflastandards.info/ns/fr/frbr/frbrer/C1001> ;
	rdfs:range <http://iflastandards.info/ns/fr/frbr/frbrer/C1001> .

<http://iflastandards.info/ns/fr/frad/P2032> rdfs:isDefinedBy <http://iflastandards.info/ns/fr/frad/> ;
	reg:status status:1001 ;
	reg:name "hasSharedCharacteristicExpressionRelationship"@en ;
	rdfs:label "has shared characteristic (expression) relationship"@en ;
	skos:definition "Relates two expressions that have some characteristic in common."@en ;
	a :Property ;
	skos:scopeNote "Excludes specific characteristics represented by other properties."@en ;
	rdfs:domain <http://iflastandards.info/ns/fr/frbr/frbrer/C1002> ;
	rdfs:range <http://iflastandards.info/ns/fr/frbr/frbrer/C1002> ;
	rdfs:label "tiene relación de característica compartida (expresión)"@es .

<http://iflastandards.info/ns/fr/frad/P2034> rdfs:isDefinedBy <http://iflastandards.info/ns/fr/frad/> ;
	reg:status status:1001 ;
	reg:name "hasSharedCharacteristicItemRelationship"@en ;
	rdfs:label "has shared characteristic (item) relationship"@en ;
	skos:definition "Relates two items that have some characteristic in common."@en ;
	a :Property ;
	skos:scopeNote "Excludes specific characteristics represented by other properties."@en ;
	rdfs:domain <http://iflastandards.info/ns/fr/frbr/frbrer/C1004> ;
	rdfs:range <http://iflastandards.info/ns/fr/frbr/frbrer/C1004> ;
	rdfs:label "tiene relación de característica compartida (ejemplar)"@es .

<http://iflastandards.info/ns/fr/frad/P2033> rdfs:isDefinedBy <http://iflastandards.info/ns/fr/frad/> ;
	reg:status status:1001 ;
	reg:name "hasSharedCharacteristicManifestationRelationship"@en ;
	rdfs:label "has shared characteristic (manifestation) relationship"@en ;
	skos:definition "Relates two manifestations that have some characteristic in common."@en ;
	a :Property ;
	skos:scopeNote "Excludes specific characteristics represented by other properties."@en ;
	rdfs:domain <http://iflastandards.info/ns/fr/frbr/frbrer/C1003> ;
	rdfs:range <http://iflastandards.info/ns/fr/frbr/frbrer/C1003> ;
	rdfs:label "tiene relación de característica compartida (manifestación)"@es .

<http://iflastandards.info/ns/fr/frad/P2031> rdfs:isDefinedBy <http://iflastandards.info/ns/fr/frad/> ;
	reg:status status:1001 ;
	reg:name "hasSharedCharacteristicWorkRelationship"@en ;
	rdfs:label "has shared characteristic (work) relationship"@en ;
	skos:definition "Relates two works that have some characteristic in common."@en ;
	a :Property ;
	skos:scopeNote "Excludes specific characteristics represented by other properties."@en ;
	rdfs:domain <http://iflastandards.info/ns/fr/frbr/frbrer/C1001> ;
	rdfs:range <http://iflastandards.info/ns/fr/frbr/frbrer/C1001> ;
	rdfs:label "tiene relación de característica compartida (obra)"@es .

<http://iflastandards.info/ns/fr/frad/P4047> rdfs:isDefinedBy <http://iflastandards.info/ns/fr/frad/> ;
	reg:status status:1001 ;
	reg:name "hasSibling"@en ;
	rdfs:label "has sibling"@en ;
	a :Property ;
	skos:definition "Relates two persons who have the same “parent(s)” (in an actual family or within a group)."@en ;
	rdfs:domain <http://iflastandards.info/ns/fr/frad/C1003> ;
	rdfs:range <http://iflastandards.info/ns/fr/frad/C1003> .

<http://iflastandards.info/ns/fr/frad/P3016> rdfs:isDefinedBy <http://iflastandards.info/ns/fr/frad/> ;
	reg:status status:1001 ;
	reg:name "hasSourceOfControlledAccessPoint"@en ;
	rdfs:label "has source of controlled access point"@en ;
	skos:definition "Relates a controlled access point to the publication or reference source used in establishing the form of name or title on which the controlled access point is based."@en ;
	a :Property ;
	skos:scopeNote "Includes the title, publisher, date, etc., of the resource for which the controlled access point was originally created. Includes the title, edition, etc., of the reference source(s) used to establish the conventional name or title."@en ;
	rdfs:domain <http://iflastandards.info/ns/fr/frad/C1001> .

<http://iflastandards.info/ns/fr/frad/P3007> rdfs:isDefinedBy <http://iflastandards.info/ns/fr/frad/> ;
	reg:status status:1001 ;
	reg:name "hasStatusOfControlledAccessPoint"@en ;
	rdfs:label "has status of controlled access point"@en ;
	skos:definition "Relates a controlled access point to an indication of the level of establishment of the authorized access point for the entity (e.g., provisional)."@en ;
	a :Property ;
	rdfs:domain <http://iflastandards.info/ns/fr/frad/C1001> ;
	owl:propertyDisjointWith <http://iflastandards.info/ns/fr/frad/P4018> , <http://iflastandards.info/ns/fr/frad/P3017> , <http://iflastandards.info/ns/fr/frad/P3009> , <http://iflastandards.info/ns/fr/frad/P3008> , <http://iflastandards.info/ns/fr/frad/P3006> .

<http://iflastandards.info/ns/fr/frad/P3050> rdfs:isDefinedBy <http://iflastandards.info/ns/fr/frad/> ;
	reg:status status:1001 ;
	reg:name "hasSubjectOfTheWork"@en ;
	rdfs:label "has subject of the work"@en ;
	skos:definition "Relates a work to the subject aspects of the work and its content."@en ;
	a :Property ;
	skos:scopeNote "Includes information about the subject of the work. Includes classification numbers."@en ;
	rdfs:domain <http://iflastandards.info/ns/fr/frbr/frbrer/C1001> .

<http://iflastandards.info/ns/fr/frad/P4014> rdfs:isDefinedBy <http://iflastandards.info/ns/fr/frad/> ;
	reg:status status:1001 ;
	reg:name "hasSubordinate"@en ;
	rdfs:label "has subordinate"@en ;
	skos:definition "Relates a corporate body to another corporate body which is subordinate to the prior corporate body."@en ;
	a :Property ;
	rdfs:domain <http://iflastandards.info/ns/fr/frad/C1003> ;
	rdfs:range <http://iflastandards.info/ns/fr/frad/C1003> ;
	rdfs:label "tiene subordinado"@es ;
	owl:inverseOf <http://iflastandards.info/ns/fr/frad/P4015> .

<http://iflastandards.info/ns/fr/frad/P3014> rdfs:isDefinedBy <http://iflastandards.info/ns/fr/frad/> ;
	reg:status status:1001 ;
	reg:name "hasTransliterationSchemeOfBaseAccessPoint"@en ;
	rdfs:label "has transliteration scheme of base access point"@en ;
	skos:definition "Relates a controlled access point to an indication of the scheme used in transliterating the base access point."@en ;
	a :Property ;
	rdfs:domain <http://iflastandards.info/ns/fr/frad/C1001> .

<http://iflastandards.info/ns/fr/frad/P3015> rdfs:isDefinedBy <http://iflastandards.info/ns/fr/frad/> ;
	reg:status status:1001 ;
	reg:name "hasTransliterationSchemeOfCataloguing"@en ;
	rdfs:label "has transliteration scheme of cataloguing"@en ;
	skos:definition "Relates a controlled access point to an indication of the scheme used in transliterating any additions to the base access point."@en ;
	a :Property ;
	rdfs:domain <http://iflastandards.info/ns/fr/frad/C1001> .

<http://iflastandards.info/ns/fr/frad/P3028> rdfs:isDefinedBy <http://iflastandards.info/ns/fr/frad/> ;
	reg:status status:1001 ;
	reg:name "hasTransliterationSchemeOfName"@en ;
	rdfs:label "has transliteration scheme of name"@en ;
	skos:definition "Relates a name to the scheme used to produce the transliterated form of the name."@en ;
	a :Property ;
	rdfs:domain <http://iflastandards.info/ns/fr/frad/C1006> ;
	rdfs:label "tiene esquema de transliteración del nombre"@es .

<http://iflastandards.info/ns/fr/frad/P3006> rdfs:isDefinedBy <http://iflastandards.info/ns/fr/frad/> ;
	reg:status status:1001 ;
	reg:name "hasTypeOfControlledAccessPoint"@en ;
	rdfs:label "has type of controlled access point"@en ;
	skos:definition "Relates a controlled access point to a categorization or generic descriptor for the controlled access point."@en ;
	a :Property ;
	skos:scopeNote "Includes terms and/or codes designating the type of access point (e.g., personal name access point, family name access point, corporate name access point, meeting name access point, territorial name access point, title access point, collective title access point or access points consisting of a combination of names, such as creator/title access points)."@en ;
	rdfs:domain <http://iflastandards.info/ns/fr/frad/C1001> ;
	owl:propertyDisjointWith <http://iflastandards.info/ns/fr/frad/P3007> , <http://iflastandards.info/ns/fr/frad/P3008> , <http://iflastandards.info/ns/fr/frad/P3009> , <http://iflastandards.info/ns/fr/frad/P3017> , <http://iflastandards.info/ns/fr/frad/P4018> .

<http://iflastandards.info/ns/fr/frad/P3001> rdfs:isDefinedBy <http://iflastandards.info/ns/fr/frad/> ;
	reg:status status:1001 ;
	reg:name "hasTypeOfFamily"@en ;
	rdfs:label "has type of family"@en ;
	skos:definition "Relates a family to a categorization or generic descriptor for the type of family."@en ;
	a :Property ;
	skos:scopeNote "Includes categorizations, such as clan, dynasty, family unit, patriarchy, matriarchy, etc."@en ;
	rdfs:domain <http://iflastandards.info/ns/fr/frad/C1002> ;
	owl:propertyDisjointWith <http://iflastandards.info/ns/fr/frad/P3002> , <http://iflastandards.info/ns/fr/frad/P3003> , <http://iflastandards.info/ns/fr/frad/P3004> , <http://iflastandards.info/ns/fr/frad/P3005> .

<http://iflastandards.info/ns/fr/frad/P3021> rdfs:isDefinedBy <http://iflastandards.info/ns/fr/frad/> ;
	reg:status status:1001 ;
	reg:name "hasTypeOfIdentifier"@en ;
	rdfs:label "has type of identifier"@en ;
	skos:definition "Relates an identifier to a code or other designation indicating the type of identifier (i.e., the domain in which the identifier is assigned)."@en ;
	a :Property ;
	skos:scopeNote "Includes alphabetic strings identifying the numbering system (e.g., \"ISBN\", \"ISSN\", \"ISRC\"). Includes symbols designating the type of identifier (e.g., registered trademark symbol)"@en ;
	rdfs:domain <http://iflastandards.info/ns/fr/frad/C1009> ;
	rdfs:label "tiene tipo de identificador"@es ;
	owl:propertyDisjointWith <http://iflastandards.info/ns/fr/frad/P2011> , <http://iflastandards.info/ns/fr/frad/P2016> .

<http://iflastandards.info/ns/fr/frad/P3022> rdfs:isDefinedBy <http://iflastandards.info/ns/fr/frad/> ;
	reg:status status:1001 ;
	reg:name "hasTypeOfName"@en ;
	rdfs:label "has type of name"@en ;
	skos:definition "Relates a name to the category of a name."@en ;
	a :Property ;
	skos:scopeNote "Includes personal names, corporate names, names of families, trade names, and titles of works and manifestations. Includes names of concepts, objects, events, and places."@en ;
	rdfs:domain <http://iflastandards.info/ns/fr/frad/C1006> ;
	rdfs:label "tiene tipo de nombre"@es .

<http://iflastandards.info/ns/fr/frad/P3009> rdfs:isDefinedBy <http://iflastandards.info/ns/fr/frad/> ;
	reg:status status:1001 ;
	reg:name "hasUndifferentiatedAccessPoint"@en ;
	rdfs:label "has undifferentiated access point"@en ;
	skos:definition "Relates a controlled access point to an indication that the controlled access point for the authorized form of name (i.e., authorized access point) is insufficiently precise to differentiate between two or more entities identified by the same name."@en ;
	a :Property ;
	rdfs:domain <http://iflastandards.info/ns/fr/frad/C1001> ;
	rdfs:label "tiene punto de acceso no diferenciado"@es ;
	owl:propertyDisjointWith <http://iflastandards.info/ns/fr/frad/P4018> , <http://iflastandards.info/ns/fr/frad/P3017> , <http://iflastandards.info/ns/fr/frad/P3008> , <http://iflastandards.info/ns/fr/frad/P3007> , <http://iflastandards.info/ns/fr/frad/P3006> .

<http://iflastandards.info/ns/fr/frad/P4043> rdfs:isDefinedBy <http://iflastandards.info/ns/fr/frad/> ;
	reg:status status:1001 ;
	reg:name "hasWorksAttributedTo"@en ;
	rdfs:label "has works attributed to"@en ;
	skos:definition "Relates one person and another person (either a \"real\" individual or a persona) or identity to whom one or more works by the former have been attributed, either erroneously or falsely."@en ;
	a :Property ;
	rdfs:range <http://iflastandards.info/ns/fr/frad/C1003> ;
	rdfs:domain <http://iflastandards.info/ns/fr/frad/C1003> ;
	owl:inverseOf <http://iflastandards.info/ns/fr/frad/P4044> .

<http://iflastandards.info/ns/fr/frad/P2014> rdfs:isDefinedBy <http://iflastandards.info/ns/fr/frad/> ;
	reg:status status:1001 ;
	reg:name "isAppellationOf"@en ;
	rdfs:label "is appellation of"@en ;
	skos:definition "Relates a name to a bibliographic entity."@en ;
	a :Property ;
	rdfs:domain <http://iflastandards.info/ns/fr/frad/C1006> ;
	rdfs:range <http://iflastandards.info/ns/fr/frad/C1010> ;
	owl:inverseOf <http://iflastandards.info/ns/fr/frad/P2013> .

<http://iflastandards.info/ns/fr/frad/P2015> rdfs:isDefinedBy <http://iflastandards.info/ns/fr/frad/> ;
	reg:status status:1001 ;
	reg:name "isAssigned"@en ;
	rdfs:label "is assigned"@en ;
	skos:definition "Relates a bibliographic entity to an identifier assigned to the entity."@en ;
	a :Property ;
	rdfs:domain <http://iflastandards.info/ns/fr/frad/C1010> ;
	rdfs:range <http://iflastandards.info/ns/fr/frad/C1009> ;
	owl:inverseOf <http://iflastandards.info/ns/fr/frad/P2016> .

<http://iflastandards.info/ns/fr/frad/P2016> rdfs:isDefinedBy <http://iflastandards.info/ns/fr/frad/> ;
	reg:status status:1001 ;
	reg:name "isAssignedTo"@en ;
	rdfs:label "is assigned to"@en ;
	skos:definition "Relates an identifier to a bibliographic entity to which it is assigned."@en ;
	a :Property ;
	rdfs:domain <http://iflastandards.info/ns/fr/frad/C1009> ;
	rdfs:range <http://iflastandards.info/ns/fr/frad/C1010> ;
	owl:inverseOf <http://iflastandards.info/ns/fr/frad/P2015> ;
	owl:propertyDisjointWith <http://iflastandards.info/ns/fr/frad/P3021> .

<http://iflastandards.info/ns/fr/frad/P2028> rdfs:isDefinedBy <http://iflastandards.info/ns/fr/frad/> ;
	reg:status status:1001 ;
	reg:name "isAssociatedWith"@en ;
	rdfs:label "is associated with"@en ;
	a :Property ;
	skos:definition "Relates a person, a family, or a corporate body to a work, expression, manifestation, or item."@en ;
	reg:hasSubproperty <http://iflastandards.info/ns/fr/frad/P2020> .

<http://iflastandards.info/ns/fr/frad/P2012> rdfs:isDefinedBy <http://iflastandards.info/ns/fr/frad/> ;
	reg:status status:1001 ;
	reg:name "isBasedOnIdentifier"@en ;
	rdfs:label "is based on (identifier)"@en ;
	skos:definition "Relates a controlled access point to an identifier on which it is based."@en ;
	a :Property ;
	rdfs:domain <http://iflastandards.info/ns/fr/frad/C1001> ;
	rdfs:range <http://iflastandards.info/ns/fr/frad/C1009> ;
	rdfs:label "está basado en (identificador)"@es ;
	owl:inverseOf <http://iflastandards.info/ns/fr/frad/P2011> .

<http://iflastandards.info/ns/fr/frad/P2010> rdfs:isDefinedBy <http://iflastandards.info/ns/fr/frad/> ;
	reg:status status:1001 ;
	reg:name "isBasedOnName"@en ;
	rdfs:label "is based on (name)"@en ;
	skos:definition "Relates a controlled access point to a name on which it is based."@en ;
	a :Property ;
	rdfs:domain <http://iflastandards.info/ns/fr/frad/C1001> ;
	rdfs:range <http://iflastandards.info/ns/fr/frad/C1006> ;
	owl:inverseOf <http://iflastandards.info/ns/fr/frad/P2009> .

<http://iflastandards.info/ns/fr/frad/P2011> rdfs:isDefinedBy <http://iflastandards.info/ns/fr/frad/> ;
	reg:status status:1001 ;
	reg:name "isBasisIdentifierFor"@en ;
	rdfs:label "is basis (identifier) for"@en ;
	skos:definition "Relates an identifier to a controlled access point for which it is the basis."@en ;
	a :Property ;
	rdfs:domain <http://iflastandards.info/ns/fr/frad/C1009> ;
	rdfs:range <http://iflastandards.info/ns/fr/frad/C1001> ;
	owl:inverseOf <http://iflastandards.info/ns/fr/frad/P2012> ;
	owl:propertyDisjointWith <http://iflastandards.info/ns/fr/frad/P3021> .

<http://iflastandards.info/ns/fr/frad/P2009> rdfs:isDefinedBy <http://iflastandards.info/ns/fr/frad/> ;
	reg:status status:1001 ;
	reg:name "isBasisNameFor"@en ;
	rdfs:label "is basis (name) for"@en ;
	skos:definition "Relates a name to a controlled access point for which it is the basis."@en ;
	a :Property ;
	rdfs:domain <http://iflastandards.info/ns/fr/frad/C1006> ;
	rdfs:range <http://iflastandards.info/ns/fr/frad/C1001> ;
	owl:inverseOf <http://iflastandards.info/ns/fr/frad/P2010> .

<http://iflastandards.info/ns/fr/frad/P4030> rdfs:isDefinedBy <http://iflastandards.info/ns/fr/frad/> ;
	reg:status status:1001 ;
	reg:name "isConventionalNameOf"@en ;
	rdfs:label "is conventional name of"@en ;
	skos:definition "Relates a conventional name by which a work is known to a name of the same work."@en ;
	a :Property ;
	rdfs:domain <http://iflastandards.info/ns/fr/frad/C1014> ;
	rdfs:range <http://iflastandards.info/ns/fr/frad/C1014> ;
	rdfs:label "es nombre convencional de"@es ;
	owl:inverseOf <http://iflastandards.info/ns/fr/frad/P4029> .

<http://iflastandards.info/ns/fr/frad/P2005> rdfs:isDefinedBy <http://iflastandards.info/ns/fr/frad/> ;
	reg:status status:1001 ;
	reg:name "isCreatedBy"@en ;
	rdfs:label "is created by"@en ;
	a :Property ;
	rdfs:domain <http://iflastandards.info/ns/fr/frad/C1001> ;
	skos:definition "Relates a controlled access point to the agency that creates it."@en ;
	rdfs:range <http://iflastandards.info/ns/fr/frad/C1008> ;
	rdfs:label "es creado por"@es ;
	owl:inverseOf <http://iflastandards.info/ns/fr/frad/P2006> .

<http://iflastandards.info/ns/fr/frad/P2020> rdfs:isDefinedBy <http://iflastandards.info/ns/fr/frad/> ;
	reg:status status:1001 ;
	reg:name "isCreatedByFamily"@en ;
	rdfs:label "is created by (family)"@en ;
	skos:definition "Relates a work to a family which is responsible for the creation of the intellectual or artistic content of the work."@en ;
	a :Property ;
	rdfs:domain <http://iflastandards.info/ns/fr/frbr/frbrer/C1001> ;
	rdfs:range <http://iflastandards.info/ns/fr/frad/C1002> ;
	rdfs:label "es creada por (familia)"@es ;
	rdfs:subPropertyOf <http://iflastandards.info/ns/fr/frad/P2028> .

<http://iflastandards.info/ns/fr/frad/P2021> rdfs:isDefinedBy <http://iflastandards.info/ns/fr/frad/> ;
	reg:status status:1001 ;
	reg:name "isCreatorFamilyOf"@en ;
	rdfs:label "is creator (family) of"@en ;
	skos:definition "Relates a family to a work of which it is responsible for the creation of the intellectual or artistic content."@en ;
	a :Property ;
	rdfs:domain <http://iflastandards.info/ns/fr/frad/C1002> ;
	rdfs:range <http://iflastandards.info/ns/fr/frbr/frbrer/C1001> ;
	rdfs:label "es creadora (familia) de"@es .

<http://iflastandards.info/ns/fr/frad/P2018> rdfs:isDefinedBy <http://iflastandards.info/ns/fr/frad/> ;
	reg:status status:1001 ;
	reg:name "isDerivativeOf"@en ;
	rdfs:label "is derivative of"@en ;
	skos:definition "Relates a work to another work of which it is an adaptation or modification."@en ;
	a :Property ;
	rdfs:range <http://iflastandards.info/ns/fr/frbr/frbrer/C1001> ;
	skos:scopeNote "Includes relationships between an original work and a broad range of modifications from the original, including variations or versions of that work, such as editions, revisions, translations, summaries, abstracts, and digests. Includes new works that are adaptations or modifications that become new works but are based on an earlier work (improvisations, etc.); new works that are changes of genre (transformations, dramatizations, novelizations, etc.); and, new works based on the style or thematic content of other works (free translations, paraphrases, imitations, parodies, etc.)."@en ;
	rdfs:domain <http://iflastandards.info/ns/fr/frbr/frbrer/C1001> ;
	rdfs:label "es derivativa de"@es ;
	owl:inverseOf <http://iflastandards.info/ns/fr/frad/P2017> .

<http://iflastandards.info/ns/fr/frad/P2036> rdfs:isDefinedBy <http://iflastandards.info/ns/fr/frad/> ;
	reg:status status:1001 ;
	reg:name "isDescriptiveWorkOf"@en ;
	rdfs:label "is descriptive work of"@en ;
	skos:definition "Relates a new work to a target work or expression or manifestation or item that it refers to as its subject."@en ;
	a :Property ;
	skos:scopeNote "Includes criticism, commentary, review, casebook, etc., and the object of that analysis (that is, the target work, expression, or manifestation)."@en ;
	rdfs:domain <http://iflastandards.info/ns/fr/frbr/frbrer/C1001> .

<http://iflastandards.info/ns/fr/frad/P4010> rdfs:isDefinedBy <http://iflastandards.info/ns/fr/frad/> ;
	reg:status status:1001 ;
	reg:name "isFounderOf"@en ;
	rdfs:label "is founder of"@en ;
	skos:definition "Relates a family to a corporate body which the family created."@en ;
	a :Property ;
	rdfs:domain <http://iflastandards.info/ns/fr/frad/C1002> ;
	rdfs:range <http://iflastandards.info/ns/fr/frad/C1003> ;
	rdfs:label "es fundador de"@es ;
	owl:inverseOf <http://iflastandards.info/ns/fr/frad/P4011> .

<http://iflastandards.info/ns/fr/frad/P2003> rdfs:isDefinedBy <http://iflastandards.info/ns/fr/frad/> ;
	reg:status status:1001 ;
	reg:name "isGovernedBy"@en ;
	rdfs:label "is governed by"@en ;
	a :Property ;
	rdfs:domain <http://iflastandards.info/ns/fr/frad/C1001> ;
	skos:definition "Relates a controlled access point to the rules that govern it."@en ;
	rdfs:range <http://iflastandards.info/ns/fr/frad/C1007> ;
	rdfs:label "es regulado por"@es ;
	owl:inverseOf <http://iflastandards.info/ns/fr/frad/P2004> .

<http://iflastandards.info/ns/fr/frad/P4007> rdfs:isDefinedBy <http://iflastandards.info/ns/fr/frad/> ;
	reg:status status:1001 ;
	reg:name "isMemberOfCorporateBody"@en ;
	rdfs:label "is member of (corporate body)"@en ;
	skos:definition "Relates a person to a corporate body in which the person is a member or with which the person is affiliated."@en ;
	a :Property ;
	rdfs:domain <http://iflastandards.info/ns/fr/frbr/frbrer/C1005> ;
	rdfs:range <http://iflastandards.info/ns/fr/frad/C1003> ;
	owl:inverseOf <http://iflastandards.info/ns/fr/frad/P4006> .

<http://iflastandards.info/ns/fr/frad/P4005> rdfs:isDefinedBy <http://iflastandards.info/ns/fr/frad/> ;
	reg:status status:1001 ;
	reg:name "isMemberOfFamily"@en ;
	rdfs:label "is member of (family)"@en ;
	skos:definition "Relates a person to a family of which the person is a member."@en ;
	a :Property ;
	rdfs:domain <http://iflastandards.info/ns/fr/frbr/frbrer/C1005> ;
	rdfs:range <http://iflastandards.info/ns/fr/frad/C1002> .

<http://iflastandards.info/ns/fr/frad/P2007> rdfs:isDefinedBy <http://iflastandards.info/ns/fr/frad/> ;
	reg:status status:1001 ;
	reg:name "isModifiedBy"@en ;
	rdfs:label "is modified by"@en ;
	a :Property ;
	rdfs:domain <http://iflastandards.info/ns/fr/frad/C1001> ;
	skos:definition "Relates a controlled access point to the agency that modifies it."@en ;
	rdfs:range <http://iflastandards.info/ns/fr/frad/C1008> ;
	rdfs:label "es modificado por"@es ;
	owl:inverseOf <http://iflastandards.info/ns/fr/frad/P2008> .

<http://iflastandards.info/ns/fr/frad/P4042> rdfs:isDefinedBy <http://iflastandards.info/ns/fr/frad/> ;
	reg:status status:1001 ;
	reg:name "isOfficialIdentityOf"@en ;
	rdfs:label "is official identity of"@en ;
	skos:definition "Relates an identity a person assumes in an official capacity and the person."@en ;
	a :Property ;
	rdfs:range <http://iflastandards.info/ns/fr/frbr/frbrer/C1005> ;
	rdfs:domain <http://iflastandards.info/ns/fr/frbr/frbrer/C1005> ;
	owl:inverseOf <http://iflastandards.info/ns/fr/frad/P4041> .

<http://iflastandards.info/ns/fr/frad/P2022> rdfs:isDefinedBy <http://iflastandards.info/ns/fr/frad/> ;
	reg:status status:1001 ;
	reg:name "isOwnedByFamily"@en ;
	rdfs:label "is owned by (family)"@en ;
	a :Property ;
	skos:definition "Relates an item to a family that is the owner or custodian of the item."@en ;
	rdfs:domain <http://iflastandards.info/ns/fr/frbr/frbrer/C1004> ;
	rdfs:range <http://iflastandards.info/ns/fr/frad/C1002> ;
	rdfs:label "es poseida por (familia)"@es .

<http://iflastandards.info/ns/fr/frad/P2023> rdfs:isDefinedBy <http://iflastandards.info/ns/fr/frad/> ;
	reg:status status:1001 ;
	reg:name "isOwnerFamilyOf"@en ;
	rdfs:label "is owner (family) of"@en ;
	skos:definition "Relates a family to an item of which it is the owner or custodian."@en ;
	a :Property ;
	rdfs:domain <http://iflastandards.info/ns/fr/frad/C1002> ;
	rdfs:range <http://iflastandards.info/ns/fr/frbr/frbrer/C1004> ;
	rdfs:label "es propietaria (familia) de"@es .

<http://iflastandards.info/ns/fr/frad/P4012> rdfs:isDefinedBy <http://iflastandards.info/ns/fr/frad/> ;
	reg:status status:1001 ;
	reg:name "isOwnerOf"@en ;
	rdfs:label "is owner of"@en ;
	skos:definition "Related a family to a corporate body which the family owns."@en ;
	a :Property ;
	rdfs:domain <http://iflastandards.info/ns/fr/frad/C1002> ;
	rdfs:range <http://iflastandards.info/ns/fr/frad/C1003> ;
	rdfs:label "es propietario de"@es ;
	owl:inverseOf <http://iflastandards.info/ns/fr/frad/P4013> .

<http://iflastandards.info/ns/fr/frad/P4016> rdfs:isDefinedBy <http://iflastandards.info/ns/fr/frad/> ;
	reg:status status:1001 ;
	reg:name "isPredecessorOf"@en ;
	rdfs:label "is predecessor of"@en ;
	skos:definition "Relates a corporate body to another corporate body of which it is a predecessor."@en ;
	a :Property ;
	rdfs:domain <http://iflastandards.info/ns/fr/frad/C1003> ;
	rdfs:range <http://iflastandards.info/ns/fr/frad/1003> ;
	skos:scopeNote "Includes splits, mergers, subsequent meetings or conferences."@en ;
	rdfs:label "es predecesora de"@es ;
	owl:inverseOf <http://iflastandards.info/ns/fr/frad/P4017> .

<http://iflastandards.info/ns/fr/frad/P2024> rdfs:isDefinedBy <http://iflastandards.info/ns/fr/frad/> ;
	reg:status status:1001 ;
	reg:name "isProducedByFamily"@en ;
	rdfs:label "is produced by (family)"@en ;
	a :Property ;
	skos:definition "Relates a manifestation to a family that is responsible for publishing, distributing, fabricating or manufacturing the manifestation."@en ;
	rdfs:domain <http://iflastandards.info/ns/fr/frbr/frbrer/C1003> ;
	rdfs:range <http://iflastandards.info/ns/fr/frad/C1002> ;
	rdfs:label "es producida por (familia)"@es .

<http://iflastandards.info/ns/fr/frad/P2025> rdfs:isDefinedBy <http://iflastandards.info/ns/fr/frad/> ;
	reg:status status:1001 ;
	reg:name "isProducerFamilyOf"@en ;
	rdfs:label "is producer (family) of"@en ;
	a :Property ;
	skos:definition "Relates a family to a manifestation of which it is responsible for publishing, distributing, fabricating or manufacturing."@en ;
	rdfs:domain <http://iflastandards.info/ns/fr/frad/C1002> ;
	rdfs:range <http://iflastandards.info/ns/fr/frbr/frbrer/C1003> ;
	rdfs:label "es productora (familia) de"@es .

<http://iflastandards.info/ns/fr/frad/P4036> rdfs:isDefinedBy <http://iflastandards.info/ns/fr/frad/> ;
	reg:status status:1001 ;
	reg:name "isPseudonymousPersonaOf"@en ;
	rdfs:label "is pseudonymous persona of"@en ;
	skos:definition "Relates a persona(ae) or identity adopted by an individual through the use of one or more pseudonyms and the \"real\" person (i.e., the individual)."@en ;
	a :Property ;
	rdfs:range <http://iflastandards.info/ns/fr/frbr/frbrer/C1005> ;
	rdfs:domain <http://iflastandards.info/ns/fr/frbr/frbrer/C1005> ;
	owl:inverseOf <http://iflastandards.info/ns/fr/frad/P4035> .

<http://iflastandards.info/ns/fr/frad/P2026> rdfs:isDefinedBy <http://iflastandards.info/ns/fr/frad/> ;
	reg:status status:1001 ;
	reg:name "isRealizedByFamily"@en ;
	rdfs:label "is realized by (family)"@en ;
	a :Property ;
	skos:definition "Relates an expression to a family that is responsible for the specifics of the intellectual or artistic realization or execution of the expression."@en ;
	rdfs:domain <http://iflastandards.info/ns/fr/frbr/frbrer/C1002> ;
	rdfs:range <http://iflastandards.info/ns/fr/frad/C1002> ;
	rdfs:label "es realizada por (familia)"@es .

<http://iflastandards.info/ns/fr/frad/P2027> rdfs:isDefinedBy <http://iflastandards.info/ns/fr/frad/> ;
	reg:status status:1001 ;
	reg:name "isRealizerFamilyOf"@en ;
	rdfs:label "is realizer (family) of"@en ;
	a :Property ;
	skos:definition "Relates a family to an expression of which it is responsible for the specifics of the intellectual or artistic realization or execution."@en ;
	rdfs:domain <http://iflastandards.info/ns/fr/frad/C1002> ;
	rdfs:range <http://iflastandards.info/ns/fr/frbr/frbrer/C1002> ;
	rdfs:label "es realizadora (familia) de"@es .

<http://iflastandards.info/ns/fr/frad/P4040> rdfs:isDefinedBy <http://iflastandards.info/ns/fr/frad/> ;
	reg:status status:1001 ;
	reg:name "isReligiousIdentityOf"@en ;
	rdfs:label "is religious identity of"@en ;
	skos:definition "Relates an identity a person assumes in a religious capacity and the person."@en ;
	a :Property ;
	rdfs:range <http://iflastandards.info/ns/fr/frbr/frbrer/C1005> ;
	rdfs:domain <http://iflastandards.info/ns/fr/frbr/frbrer/C1005> ;
	owl:equivalentProperty <http://iflastandards.info/ns/fr/frad/P4037> ;
	owl:inverseOf <http://iflastandards.info/ns/fr/frad/P4039> .

<http://iflastandards.info/ns/fr/frad/P4038> rdfs:isDefinedBy <http://iflastandards.info/ns/fr/frad/> ;
	reg:status status:1001 ;
	reg:name "isSecularIdentityOf"@en ;
	rdfs:label "is secular identity of"@en ;
	skos:definition "Relates an identity a person assumes in a secular capacity and the person."@en ;
	a :Property ;
	rdfs:range <http://iflastandards.info/ns/fr/frbr/frbrer/C1005> ;
	rdfs:domain <http://iflastandards.info/ns/fr/frbr/frbrer/C1005> ;
	owl:inverseOf <http://iflastandards.info/ns/fr/frad/P4037> ;
	owl:equivalentProperty <http://iflastandards.info/ns/fr/frad/P4039> .

<http://iflastandards.info/ns/fr/frad/P4015> rdfs:isDefinedBy <http://iflastandards.info/ns/fr/frad/> ;
	reg:status status:1001 ;
	reg:name "isSubordinateOf"@en ;
	rdfs:label "is subordinate of"@en ;
	a :Property ;
	skos:definition "Relates a corporate body to another corporate body to which it is subordinate."@en ;
	rdfs:domain <http://iflastandards.info/ns/fr/frad/C1003> ;
	rdfs:range <http://iflastandards.info/ns/fr/frad/C1003> ;
	rdfs:label "es subordinado de"@es ;
	owl:inverseOf <http://iflastandards.info/ns/fr/frad/P4014> .

<http://iflastandards.info/ns/fr/frad/P4017> rdfs:isDefinedBy <http://iflastandards.info/ns/fr/frad/> ;
	reg:status status:1001 ;
	reg:name "isSuccessorOf"@en ;
	rdfs:label "is successor of"@en ;
	skos:definition "Relates a corporate body to another corporate body of which it is a successor."@en ;
	a :Property ;
	rdfs:domain <http://iflastandards.info/ns/fr/frad/C1003> ;
	rdfs:range <http://iflastandards.info/ns/fr/frad/C1003> ;
	rdfs:label "es sucesora de"@es ;
	owl:inverseOf <http://iflastandards.info/ns/fr/frad/P4016> .

<http://iflastandards.info/ns/fr/frad/P2008> rdfs:isDefinedBy <http://iflastandards.info/ns/fr/frad/> ;
	reg:status status:1001 ;
	reg:name "modifies"@en ;
	rdfs:label "modifies"@en ;
	a :Property ;
	rdfs:domain <http://iflastandards.info/ns/fr/frad/C1008> ;
	skos:definition "Relates an agency to a controlled access point that is modified by the agency."@en ;
	rdfs:range <http://iflastandards.info/ns/fr/frad/C1001> ;
	rdfs:label "modifica"@es ;
	owl:inverseOf <http://iflastandards.info/ns/fr/frad/P2007> .

status:1001 a skos:Concept ;
	skos:prefLabel "Published"@en .
