@prefix : <http://www.w3.org/ns/ldp#> .
@prefix rdfs: <http://www.w3.org/2000/01/rdf-schema#> .
@prefix owl: <http://www.w3.org/2002/07/owl#> .
@prefix rdf: <http://www.w3.org/1999/02/22-rdf-syntax-ns#> .
@prefix vs: <http://www.w3.org/2003/06/sw-vocab-status/ns#> .
@prefix dcterms: <http://purl.org/dc/terms/> .

<http://www.w3.org/ns/ldp#> a owl:Ontology ;
	dcterms:description "All vocabulary URIs defined in the Linked Data Platform (LDP) namespace." ;
	dcterms:title "The W3C Linked Data Platform (LDP) Vocabulary" ;
	rdfs:label "W3C Linked Data Platform (LDP)" ;
	rdfs:comment """This ontology provides an informal representation of the concepts and terms
	as defined in the LDP specification.  Consult the LDP specification for normative reference.""" ;
	rdfs:seeAlso <http://www.w3.org/2012/ldp> , <http://www.w3.org/TR/ldp-ucr/> , <http://www.w3.org/TR/ldp/> , <http://www.w3.org/2011/09/LinkedData/> .

:Resource a rdfs:Class ;
	rdfs:comment "A HTTP-addressable resource with a linked data representation." ;
	vs:term_status "unstable" ;
	rdfs:isDefinedBy <http://www.w3.org/ns/ldp#> ;
	rdfs:label "Resource" .

:Container a rdfs:Class ;
	rdfs:subClassOf :Resource ;
	rdfs:comment """A Linked Data Platform Resource (LDPR) that also conforms to 
	additional patterns and conventions for managing membership.
	Readers should refer to the specification defining this ontology for the list of 
	behaviors associated with it.""" ;
	vs:term_status "unstable" ;
	rdfs:isDefinedBy <http://www.w3.org/ns/ldp#> ;
	rdfs:label "Container" .

:AggregateContainer a rdfs:Class ;
	rdfs:subClassOf :Container ;
	rdfs:comment """A Linked Data Platform Container (LDPC) that also conforms to 
	additional patterns and conventions for managing members.  It is distinguished from
	CompositeContainer by the following behaviors:
	(1) Clients cannot assume that an AggregateContainer, when deleted, deletes its members.
	
	While every attempt is made to be complete in this list, readers should also refer 
	to the specification defining this ontology.""" ;
	vs:term_status "unstable" ;
	rdfs:isDefinedBy <http://www.w3.org/ns/ldp#> ;
	rdfs:label "AggregateContainer" .

:CompositeContainer a rdfs:Class ;
	rdfs:subClassOf :Container ;
	rdfs:comment """A Linked Data Platform Container (LDPC) that also conforms to 
	additional patterns and conventions for managing members.  It is distinguished from
	AggregateContainer by the following behaviors:
	(1) An CompositeContainer, when deleted, must delete all its members.
	
	While every attempt is made to be complete in this list, readers should also
	refer to the specification defining this ontology.""" ;
	vs:term_status "unstable" ;
	rdfs:isDefinedBy <http://www.w3.org/ns/ldp#> ;
	rdfs:label "CompositeContainer" .

:containerSortPredicates a rdf:Property ;
	rdfs:comment "List of predicates that indicate the ascending order of the members in a page." ;
	vs:term_status "unstable" ;
	rdfs:domain :Page ;
	rdfs:isDefinedBy <http://www.w3.org/ns/ldp#> ;
	rdfs:label "containerSortPredicates" ;
	rdfs:range rdf:List .

:membershipPredicate a rdf:Property ;
	rdfs:comment "Indicates which predicate of the container should be used to determine the membership." ;
	vs:term_status "unstable" ;
	rdfs:domain :Container ;
	rdfs:isDefinedBy <http://www.w3.org/ns/ldp#> ;
	rdfs:label "membershipPredicate" ;
	rdfs:range rdf:Property .

:membershipSubject a rdf:Property ;
	rdfs:comment "Indicates which resource is the subject for the members of the container." ;
	vs:term_status "unstable" ;
	rdfs:domain :Container ;
	rdfs:isDefinedBy <http://www.w3.org/ns/ldp#> ;
	rdfs:label "membershipSubject" ;
	rdfs:range rdf:Property .

:nextPage a rdf:Property ;
	rdfs:comment "From a known page, how to indicate the next or last page as rdf:nil." ;
	vs:term_status "unstable" ;
	rdfs:domain :Page ;
	rdfs:isDefinedBy <http://www.w3.org/ns/ldp#> ;
	rdfs:label "nextPage" ;
	rdfs:range rdfs:Resource .

:Page a rdfs:Class ;
	rdfs:comment "A resource that represents a limited set of members of a LDP Container." ;
	vs:term_status "unstable" ;
	rdfs:isDefinedBy <http://www.w3.org/ns/ldp#> ;
	rdfs:label "Page" .

:pageOf a rdf:Property ;
	rdfs:comment "Associated a page with its container." ;
	vs:term_status "unstable" ;
	rdfs:domain :Page ;
	rdfs:isDefinedBy <http://www.w3.org/ns/ldp#> ;
	rdfs:label "pageOf" ;
	rdfs:range :Container .
