@prefix : <http://www.w3.org/1999/xhtml> .
@prefix rdfs: <http://www.w3.org/2000/01/rdf-schema#> .
@prefix xsd: <http://www.w3.org/2001/XMLSchema#> .
@prefix owl: <http://www.w3.org/2002/07/owl#> .
@prefix rdf: <http://www.w3.org/1999/02/22-rdf-syntax-ns#> .
@prefix vs: <http://www.w3.org/2003/06/sw-vocab-status/ns#> .
@prefix xhv: <http://www.w3.org/1999/xhtml/vocab#> .
@prefix cc: <http://creativecommons.org/ns#> .
@prefix dcterms: <http://purl.org/dc/terms/> .

dcterms:type a owl:DatatypeProperty ;
	rdfs:comment """A genre that
            should be associated with the media recording."""@en ;
	vs:term_status "stable"@en .

<http://purl.org/commerce#costs> a owl:DatatypeProperty ;
	rdfs:comment """A link to a
            method of paying for a full version of the media recording."""@en ;
	vs:term_status "stable"@en .

<http://purl.org/media#depiction> a owl:DatatypeProperty ;
	rdfs:comment """An image summary
            of the media recording."""@en ;
	vs:term_status "stable"@en .

dcterms:description a owl:DatatypeProperty ;
	rdfs:comment """The description
            associated with the media recording."""@en ;
	vs:term_status "stable"@en ;
	rdfs:range rdf:XMLLiteral .

<http://purl.org/media/audio> owl:imports <http://www.w3.org/1999/xhtml/vocab#> , <http://purl.org/dc/terms/> .

<http://purl.org/media> a owl:Ontology ;
	dcterms:title "The Media Vocabulary"@en ;
	dcterms:description "The Media RDF vocabulary is not meant to be used by itself if you are marking up audio or video. If the media that you are marking up falls outside of audio/video, you should use the Media RDF Vocabulary if there is no other way to mark up the information. You may want to use the <a xmlns=\"http://www.w3.org/1999/xhtml\" href=\"http://purl.org/media/audio\" xml:lang=\"en\">Audio RDF Vocabulary</a> or <a xmlns=\"http://www.w3.org/1999/xhtml\" href=\"http://purl.org/media/video\" xml:lang=\"en\">Video RDF Vocabulary</a> if you are marking up audio or video."^^rdf:XMLLiteral .

<http://purl.org/media#Recording> a owl:Class ;
	rdfs:subClassOf owl:Thing ;
	rdfs:comment "A recording of an item of interest in any form."@en ;
	vs:term_status "stable"@en ;
	rdfs:label "<a xmlns=\"http://www.w3.org/1999/xhtml\" href=\"http://purl.org/media#Recording\" xml:lang=\"en\">media:Recording</a>"^^rdf:XMLLiteral .

dcterms:title a owl:DatatypeProperty ;
	rdfs:comment """title of the
            media recording"""@en ;
	vs:term_status "stable"@en .

<http://purl.org/media#Collection> a owl:Class ;
	rdfs:subClassOf <http://purl.org/media/media#Recording> , dcterms:Collection ;
	rdfs:comment """A collection of
            one or more media recordings."""@en ;
	vs:term_status "stable"@en ;
	rdfs:label "<a xmlns=\"http://www.w3.org/1999/xhtml\" href=\"http://purl.org/media#Collection\" xml:lang=\"en\">media:Collection</a>"^^rdf:XMLLiteral .

xhv:license a owl:DatatypeProperty ;
	rdfs:comment """The license under
            which the media recording is distributed."""@en ;
	vs:term_status "stable"@en .

<http://purl.org/media#contains> a owl:DatatypeProperty ;
	rdfs:comment """Relationship for
            linking singular media recordings to collections or media recordings. Also used to denote pieces of a media recording that constitute a larger media recording.."""@en ;
	vs:term_status "stable"@en .

<http://purl.org/media#download> a owl:DatatypeProperty ;
	rdfs:comment """A link to a
            complete audio file representation of the media recording."""@en ;
	vs:term_status "stable"@en .

<http://purl.org/media#sample> a owl:DatatypeProperty ;
	rdfs:comment """A link to a
            sample file or stream of the media recording."""@en ;
	vs:term_status "stable"@en .

dcterms:contributor a owl:DatatypeProperty ;
	rdfs:comment """An entity that
            helped create the media recording."""@en ;
	vs:term_status "stable"@en ;
	rdfs:range <http://www.w3.org/2001/vcard-rdf/3.0> , <http://xmlns.com/foaf/0.1/Agent> , <http://xmlns.com/foaf/0.1/Person> .

dcterms:date a owl:DatatypeProperty ;
	rdfs:comment """The date the
            media recording was published."""@en ;
	vs:term_status "stable"@en ;
	rdfs:range xsd:date .

dcterms:creator a owl:DatatypeProperty ;
	rdfs:comment """The primary
            creator or performer of the media recording."""@en ;
	vs:term_status "stable"@en ;
	rdfs:range <http://www.w3.org/2001/vcard-rdf/3.0> , <http://xmlns.com/foaf/0.1/Agent> , <http://xmlns.com/foaf/0.1/Person> .

<http://purl.org/media#position> a owl:DatatypeProperty ;
	rdfs:comment """The position of
            the media recording in an album, LP, playlist, top 10 list,
            podcast history or other ordered list of media recordings."""@en ;
	vs:term_status "stable"@en ;
	rdfs:range xsd:integer .

<http://purl.org/media#rating> a owl:DatatypeProperty ;
	rdfs:comment """A standards-body
            rating such as PG-13, M, 18-SX, 15, AV15+, Explicit Lyrics, 
            etc."""@en ;
	vs:term_status "testing"@en .

<http://purl.org/media#duration> a owl:DatatypeProperty ;
	rdfs:comment """The length of the
            media recording encoded in ISO-8601 time duration format."""@en ;
	vs:term_status "stable"@en ;
	rdfs:range xsd:duration .

<http://purl.org/commerce#payment> a owl:DatatypeProperty ;
	rdfs:comment """A link to a
            method of paying for a full version of the media recording."""@en ;
	vs:term_status "stable"@en .

<http://payswarm.com/vocabs/media> xhv:stylesheet <http://payswarm.com/css/vocabulary.css> ;
	cc:attributionURL <http://digitalbazaar.com/> ;
	cc:attributionName "Digital Bazaar, Inc."@en ;
	xhv:license <http://creativecommons.org/licenses/publicdomain/> .
