@prefix dc: <http://purl.org/dc/elements/1.1/> .
@prefix : <http://rdf.muninn-project.org/ontologies/military#> .
@prefix person: <http://rdf.muninn-project.org/ontologies/person#> .
@prefix foaf: <http://xmlns.com/foaf/spec/> .
@prefix muninn: <http://rdf.muninn-project.org/ontologies/muninn#> .
@prefix vs: <http://www.w3.org/2003/06/sw-vocab-status/ns#> .
@prefix org: <http://rdf.muninn-project.org/ontologies/organization#> .
@prefix rdfs: <http://www.w3.org/2000/01/rdf-schema#> .
@prefix time: <http://www.w3.org/2006/time#> .
@prefix swrl: <http://www.w3.org/2003/11/swrl#> .
@prefix swrlb: <http://www.w3.org/2003/11/swrlb#> .
@prefix dbpedia: <http://dbpedia.org/resource/> .
@prefix owl: <http://www.w3.org/2002/07/owl#> .
@prefix xsd: <http://www.w3.org/2001/XMLSchema#> .
@prefix rdf: <http://www.w3.org/1999/02/22-rdf-syntax-ns#> .

<http://rdf.muninn-project.org/ontologies/military> a owl:Ontology ;
	dc:title "The Muninn Military Ontology" ;
	dc:description "The Muninn Military Ontology is meants to deal with people and organisations." ;
	rdfs:label "The Muninn Military Ontology"@en ;
	rdfs:comment "The Muninn Military Ontology is meants to deal with people and organisations."@en ;
	owl:versionInfo "0.2"^^xsd:decimal .

:Combatant a owl:Class ;
	foaf:name "Combatant" ;
	rdfs:label "Combatant"@en , "Combatant"@fr , ""@de ;
	rdfs:comment "A person engaging in combat and/or war."@en ;
	owl:subClassOf :Person , <org:Role> .

:Non-Combatant a owl:Class ;
	foaf:name "Non-Combatant" ;
	rdfs:label "Non-Combatant"@en , "Non-Combatant"@fr , ""@de ;
	rdfs:comment "A person not engaged in combat and/or war, but which might be involved in a war. This includes nurses, chaplains, medics depending on the era."@en ;
	owl:subClassOf :Person ;
	owl:disjointWith :Combatant ;
	owl:subClassOf <org:Role> .

:PrivilegedCombatant a owl:Class ;
	foaf:name "Privileged Combatant" ;
	rdfs:label "Privileged Combatant"@en , "Combatant privilégié"@fr , "privilegierten Kämpfer"@de ;
	rdfs:comment "A person engaging in combat and/or war as privileged combatants under the rules of war, circa Great War."@en ;
	owl:subClassOf :Combatant ;
	owl:disjointWith :UnprivilegedCombatant .

:UnprivilegedCombatant a owl:Class ;
	foaf:name "Unprivileged Combatant" ;
	rdfs:label "Unprivileged Combatant"@en , "Combatant non-privilégié"@fr , "unprivilegierten Kämpfer"@de ;
	rdfs:comment "A person engaging in combat and/or war as an unprivileged combatants under the rules of war."@en ;
	owl:subClassOf :Combatant .

:Spy a owl:Class ;
	foaf:name "Spy" ;
	rdfs:label "Spy"@en , "Espion"@fr , "Spion"@de ;
	rdfs:comment "A person engaging in combat, war and/or espionage as an unprivileged combatants under the rules of war."@en ;
	owl:subClassOf :UnprivilegedCombatant .

:Civilian a owl:Class ;
	foaf:name "Civilian" ;
	rdfs:label "Civilian"@en , "Civil"@fr , "Zivilist"@de ;
	rdfs:comment "A person uninvolved with the conflict and not working for the conflicting powers."@en ;
	owl:subClassOf :Non-Combatant .

:Soldier a owl:Class ;
	foaf:name "Soldier" ;
	rdfs:label "Soldier"@en , "Soldat"@fr , "Soldat"@de ;
	rdfs:comment "A soldier serving in a political entity' Army."@en ;
	owl:subClassOf :PrivilegedCombatant ;
	owl:sameAs <dbpedia:Soldier> .

:Reservist a owl:Class ;
	foaf:name "Reservist" ;
	rdfs:label "Reservist (Soldier)"@en , "Soldat Réserviste"@fr , "Reservist (Soldat)"@de ;
	rdfs:comment "A soldier which serves on a part-time basis or when called up."@en ;
	owl:subClassOf :Soldier ;
	owl:disjointWith :RegularForceSoldier .

:RegularForceSoldier a owl:Class ;
	foaf:name "Regular Soldier" ;
	rdfs:label "Regular Soldier"@en , "Soldat Régulier"@fr , "regulärer Soldat"@de ;
	rdfs:comment "A soldier which serves on a full-time basis."@en ;
	owl:subClassOf :Soldier .

:DraftedSoldier a owl:Class ;
	foaf:name "Draftee" ;
	rdfs:label "Soldier (Drafted)"@en , "Soldat (Rédigé)"@fr , "Soldat (eingezogen)"@de ;
	rdfs:comment "A soldier which serves on a full-time basis."@en ;
	owl:subClassOf :RegularForceSoldier .

:VolunteerSoldier a owl:Class ;
	foaf:name "Volunteer" ;
	rdfs:label "Soldier (Volunteer)"@en , "Soldat (Volontaire)"@fr , "Soldat (freiwilliger)"@de ;
	rdfs:comment "A soldier which serves on a full-time basis."@en ;
	owl:subClassOf :RegularForceSoldier ;
	owl:disjointWith :DraftedSoldier .

:GeneralOfficer a owl:Class ;
	foaf:name "General Officer" ;
	rdfs:label "General Officer"@en , "Officiers Généraux"@fr , "allgemeinen Offizier"@de ;
	rdfs:comment "General staff officers"@en ;
	owl:subClassOf :Soldier .

:Officer a owl:Class ;
	foaf:name "Officer" ;
	rdfs:label "Officer"@en , "Officier"@fr , "Offizier"@de ;
	rdfs:comment "A commissioned officer, acting, breveted or confirmed."@en ;
	owl:subClassOf :Soldier .

:ExchangeOfficer a owl:Class ;
	foaf:name "Exchange Officer" ;
	rdfs:label "Exchange Officer"@en , "Officier d'échange"@fr , "Austausch-Offizier"@de ;
	rdfs:comment "An officer exchanged for a set period of time."@en ;
	owl:subClassOf :Officer ;
	owl:sameAs <dbpedia:Exchange_officer> .

:LiaisonOfficer a owl:Class ;
	foaf:name "Liaison Officer" ;
	rdfs:label "Liaison Officer"@en , "Officier de Liason"@fr , "Verbindungsoffizier"@de ;
	rdfs:comment "An officer exchanged to another unit for a set purpose."@en ;
	owl:subClassOf :Officer ;
	owl:sameAs <dbpedia:Liaison_officer> .

:Enlisted a owl:Class ;
	foaf:name "Enlisted" ;
	rdfs:label "Enlisted Soldier"@en , "Hommes de Troupes"@fr , "angeworbenen Soldaten"@de ;
	rdfs:comment "A soldier below the rank of Officer or non-commissioned Officer."@en ;
	owl:subClassOf :Soldier .

:NonCommissionedOfficer a owl:Class ;
	foaf:name "Non Commissioned Officer" ;
	rdfs:label "Non Commissioned Officer"@en , "Sous-Officier Subalternes"@fr , "Soldatenlaufbahnverordnung"@de ;
	rdfs:comment "A soldier with a rank of Corporal or above."@en ;
	owl:subClassOf :Soldier .

:WarrantOfficer a owl:Class ;
	foaf:name "Warrant Officer" ;
	rdfs:label "Warrant Officer"@en , "Officiers Mariniers"@fr , "?"@de ;
	rdfs:comment "A senior non-officer ."@en ;
	owl:subClassOf :Soldier .

:MilitaryRank a owl:Class ;
	foaf:name "Rank" ;
	rdfs:label "Rank (Military)"@en , "Grade (Militare)"@fr , "Rang (Militärischen)"@de ;
	rdfs:comment "A military rank."@en ;
	owl:subClassOf <org:Rank> .

:hasUniform a owl:ObjectProperty ;
	rdfs:label "Has Uniform"@en ;
	rdfs:domain <mil:MilitaryRank> ;
	rdfs:range <mil:MilitaryUniform> ;
	owl:inverseOf :CommanderInChiefOf .

:MilitaryUniform a owl:Class ;
	rdfs:label "Military Uniform"@en .

:epauletDepiction a owl:ObjectProperty ;
	rdfs:label "Epaulets"@en ;
	rdfs:domain :MilitaryUniform ;
	rdfs:subPropertyOf <foaf:depiction> .

:inUse a owl:ObjectProperty ;
	rdfs:label "In Use"@en ;
	rdfs:domain :MilitaryUniform ;
	rdfs:range <time:TemporalEntity> .

:ActingRank a owl:Class ;
	rdfs:label "Acting Rank (Military)"@en , "Grade Intérimaire (Militare)"@fr , "Handelnden Rang (Militärischen)"@de ;
	rdfs:comment "An acting military rank."@en ;
	owl:subClassOf <org:Acting_Rank> , :MilitaryRank .

:BrevetRank a owl:Class ;
	rdfs:label "Brevet Rank (Military)"@en , "Grade Brevet (Militare)"@fr , "Brevet Rang (Militärischen)"@de ;
	rdfs:comment "A Brevet military rank."@en ;
	owl:subClassOf :MilitaryRank .

:MilitaryAppointment a owl:Class ;
	rdfs:label "Appointment (Military)"@en , "Appointment (Militare)"@fr , "Appointment (Militärischen)"@de ;
	rdfs:comment "An appointment / function in a Military Organization."@en .

:MilitaryOrganization a owl:Class ;
	rdfs:label "A Military Organization"@en , "Une Organisation Militare"@fr , ""@de ;
	rdfs:comment "An organization that is military."@en ;
	owl:subClassOf <org:Organization> ;
	owl:sameAs <dbpedia:MilitaryUnit> .

:MilitaryServiceBranch a owl:Class ;
	foaf:name "Service Branch" ;
	rdfs:label "Service Branch (Military)"@en , "Branche du service militaire"@fr , "Teilstreitkraft"@de ;
	owl:sameAs <dbpedia:Military_branch> ;
	owl:subClassOf :MilitaryOrganization .

:hasCommanderInChief a owl:ObjectProperty ;
	rdfs:label "Commander In Chief"@en ;
	rdfs:domain :MilitaryOrganization ;
	a <owl:FunctionalProperty> ;
	owl:inverseOf :CommanderInChiefOf .

:commanderInChiefOf a owl:ObjectProperty ;
	rdfs:label "Commander In Chief of"@en ;
	rdfs:range :MilitaryOrganization ;
	a <owl:FunctionalProperty> ;
	owl:inverseOf :hasCommanderInChief .

:Detachment a owl:Class ;
	rdfs:label "Detachment (military)"@en , "Détachement (Militare)"@fr , "Detachement"@de ;
	rdfs:comment "A group of people detached from another larger group for a specific purpose."@en ;
	owl:subClassOf :MilitaryOrganization ;
	owl:sameAs "dbpedia:Detachment_(military)" .

:Garrison a owl:Class ;
	rdfs:label "Garrison (military)"@en , "Garnison (Militaire)"@fr , "Garnison (Militär)"@de ;
	rdfs:comment "A collection of military units housed and occuping a location."@en ;
	owl:sameAs "dbpedia:Garrison" .

:Depot a owl:Class ;
	rdfs:label "Depot (Military)"@en , "Dépot (Military)"@fr , "Depot (Militär)"@de ;
	rdfs:comment "A location where military supplies are stored."@en .

:SupplyTrain a owl:Class ;
	rdfs:label "Supply Train (Military)"@en , "Train D'alimentation (Military)"@fr , "liefern dem Zug (Militär)"@de ;
	rdfs:comment "A supply organization moving military supplies."@en .

:Weapon a owl:Class ;
	rdfs:label "Weapon (Military)"@en , "Arme (Military)"@fr , "Waffe (Militär)"@de ;
	rdfs:comment "A weapon type but not a branch."@en ;
	owl:sameAs <dbpedia:Weapon> .

:ArmsType a owl:Class ;
	rdfs:label "Arms Type(Military)"@en , "Type Armes (Military)"@fr , "?"@de ;
	rdfs:comment "The category of arms in use"@en .

:Infantry a :ArmsType ;
	foaf:name "Infantry" ;
	rdfs:label "Infantry"@en .

:ProtoAirForce a :ArmsType ;
	foaf:name "Proto Air Force" ;
	rdfs:label "Proto Air Force"@en .

:Artillery a :ArmsType ;
	foaf:name "Artillery" ;
	rdfs:label "Artillery"@en .

<http://rdf.muninn-project.org/ontologies/Armor> a :ArmsType ;
	foaf:name "Armor" ;
	rdfs:label "Armor"@en .

:NavyMerchant a owl:Class ;
	owl:subClassOf <org:WaterBasedOrganization> ;
	owl:disjointWith :NavyServiceBranch ;
	owl:sameAs "dbpedia:Merchant_navy" .

<http://rdf.muninn-project.org/ww1/2011/11/11/BattleSpace/FightsPrimarilyOnAndInWater> a :BattleSpace ;
	rdfs:label "Water (Battleground)"@en ;
	rdfs:comment "Fights primarily in and on Water."@en .

:NavyServiceBranch a owl:Class ;
	owl:subClassOf :MilitaryServiceBranch , :FightsPrimarilyOnAndInWater , :WaterBasedOrganization ;
	:member :SeamanMilitary ;
	owl:sameAs "dbpedia:Navy" ;
	:membershipClass <http://rdf.muninn-project.org/ww1/2011/11/11/GroupMemberships/NavyAppointments> .

<http://rdf.muninn-project.org/ww1/2011/11/11/GroupMemberships/NavyAppointments> a owl:Class .

:NavalArtillery a owl:Class ;
	rdfs:label "Navel Artillery"@en , "Artillerie Navale"@fr , "Schiffsartillerie"@de ;
	rdfs:comment "Naval artillery unit operating from the ship on land."@en ;
	owl:subClassOf :Artillery .

:NavalSquadron a owl:Class ;
	rdfs:label "Naval Squadron"@en , "Escadron Naval"@fr , "Geschwader (Marine)"@de ;
	rdfs:comment "A naval squadron of ships."@en ;
	owl:subClass :Squadron , :Navy ;
	owl:sameAs "dbpedia:Squadron_(naval)" .

:NavyBigFleet a owl:Class ;
	rdfs:label "Navy (Named or Numbered)"@en , "Marine (Groupe de batiment naval)"@fr , "Marine (Boot-Gruppe)"@de .

:NavalFleet a owl:Class ;
	rdfs:label "Naval Fleet"@en , "Flotte"@fr , "Flotte (Marine)"@de ;
	owl:sameAs "dbpedia:Naval_fleet" .

:NavalTaskForce a owl:Class ;
	rdfs:label "Task Force (Naval)"@en , "Force opérationnelle (Marine)"@fr , "Task Force"@de .

:CarrierBattleGroup a owl:Class ;
	rdfs:label "Carrier Bettle Group (Naval)"@en , "Groupe aéronaval"@fr , "Flugzeugträgerkampfgruppe"@de ;
	owl:sameAs "dbpedia:Carrier_battle_group" .

:Flotilla a owl:Class ;
	rdfs:label "Flotilla (Navy)"@en , "Flottille (Marine)"@fr , "Flottille"@de ;
	owl:sameAs "dbpedia:Flotilla" .

:DivisionNavalEstablishment a owl:Class ;
	rdfs:label "Division (Navy)"@en , "Division (Marine)"@fr , "Division"@de .

:DivisionNavalUnit a owl:Class ;
	rdfs:label "Ship's Division (Navy)"@en , "Division de Navire (Marine)"@fr , "Division"@de .

:Ship a owl:Class ;
	rdfs:label "Ship"@en , "Navire Militare"@fr , ""@de .

:Warship a owl:Class ;
	rdfs:label "Warship"@en , "Navire Militare"@fr , ""@de ;
	owl:subClassOf :Ship .

:Frigate a owl:Class ;
	rdfs:label "Frigate"@en , "Fregate"@fr , ""@de ;
	owl:subClassOf :Warship .

:ShoreEstablishment a owl:Class ;
	rdfs:label "Shore Establishment (Navy)"@en , "Etablishment de Terre (Marine)"@fr , "Ufer Gründung (Kriegsmarine)"@de ;
	owl:subClassOf :ship ;
	owl:disjointWith :warship .

:SeamanMilitary a owl:Class ;
	rdfs:label "Seaman (Military)"@en , "Matelot (Militare)"@fr , "Matrose (Militär)"@de ;
	rdfs:comment "A Seaman serving in a political entity' Navy."@en ;
	owl:subClassOf :PrivilegedCombatant .

:NavalRating a owl:Class ;
	rdfs:label "Naval Rating"@en , "Maître (Marine de Guerre)"@fr , "Unteroffiziere (Deutsche Marine)"@de ;
	rdfs:comment "A Seaman serving in a political entity' Navy."@en ;
	owl:subClassOf :SeamanMilitary .

:NavalOfficer a owl:Class ;
	rdfs:label "Naval Officer"@en , "Officier (Marine)"@fr , "Offiziere (Deutsche Marine)"@de ;
	rdfs:comment "A Commissioned Officer serving in a political entity' Navy."@en ;
	owl:subClassOf :SeamanMilitary .

:FlagOfficer a owl:Class ;
	rdfs:label "Flag Officer"@en , "????"@fr , "Flaggoffizier"@de ;
	rdfs:comment "A Commissioned Officer serving in a political entity' Navy."@en ;
	owl:subClassOf :NavalOfficer .

<http://rdf.muninn-project.org/ww1/2011/11/11/BattleSpace/FightsPrimarilyOnAndInLand> a :BattleSpace ;
	rdfs:label "Land (Battleground)"@en ;
	rdfs:comment "Fights primarily in and on Water."@en .

:BattleStandard a owl:ObjectProperty ;
	rdfs:label "Battle Standard"@en , "Drapeau de combat(?)"@fr , ""@de ;
	rdfs:comment "Flag used to represent that unit on a battlefield."@en ;
	rdfs:domain :ArmyServiceBranch ;
	rdfs:subPropertyOf <org:flag> .

:RegimentalColours a owl:ObjectProperty ;
	rdfs:label "Regimental Colours"@en , "Drapeau du Regiment"@fr , ""@de ;
	rdfs:comment "Flag used by a regiment on a battlefield or on parade."@en ;
	rdfs:domain :Regiment ;
	rdfs:subPropertyOf <org:flag> .

:ArmyServiceBranch a owl:Class ;
	rdfs:label "Army (Service Branch)"@en , "Armée (Service)"@fr , "Armee (Service)"@de ;
	owl:subClassOf :MilitaryServiceBranch , :FightsPrimarilyOnAndInLand , :GroundBasedOrganization .

:Battalion a owl:Class ;
	rdfs:label "Battalion (Military)"@en , "Bataillon"@de , "Bataillon"@fr ;
	foaf:logo <http://rdf.muninn-project.org/ww1/2011/11/11/image/24> ;
	org:nominalSize "1000" ;
	owl:sameAs "dbpedia:Battalion" .

:Division a owl:Class ;
	rdfs:label "Division (Military)"@en , "Division (Militär)"@de , "Division (Militaire)"@fr ;
	foaf:logo <http://rdf.muninn-project.org/ww1/2011/11/11/image/25> ;
	owl:sameAs "dbpedia:Division_(military)" .

:Regiment a owl:Class ;
	rdfs:label "Regiment"@en , "Regiment"@de , "Régiment"@fr ;
	rdfs:comment "A regiment, be it administrative or historical."@en ;
	foaf:logo <http://rdf.muninn-project.org/ww1/2011/11/11/image/26> ;
	owl:sameAs "dbpedia:Regiment" .

:DemiBrigade a owl:Class ;
	rdfs:label "Half-Brigade"@en , "Demi-brigade"@fr , "Halbbrigade"@de ;
	rdfs:comment "An military organizational unit derived from French Regiments."@en ;
	owl:sameAs "dbpedia:Demi-brigade" ;
	owl:subClassOf :regiment .

:Brigade a owl:Class ;
	rdfs:label "Brigade (Military)"@en , "Brigade (Militare)"@fr , "Brigade"@de ;
	foaf:logo <http://rdf.muninn-project.org/ww1/2011/11/11/image/27> ;
	owl:sameAs "dbpedia:Brigade" .

:CorpsUnit a owl:Class ;
	rdfs:label "Corps (Unit)"@en , "Corps (Unité d'armée)"@fr , "Korps (Unit)"@de ;
	rdfs:comment "A stand-alone administrative military unit with a specialized function, eg: Medical Corps."@en ;
	owl:sameAs "dbpedia:Corps" .

:CorpsFormation a owl:Class ;
	rdfs:label "Corps (Formation)"@en , "Corps d'armée"@fr , "Korps (Großverband)"@de ;
	rdfs:comment "A military formation containing Brigades, Divisions, etc..."@en ;
	foaf:logo <http://rdf.muninn-project.org/ww1/2011/11/11/image/28> ;
	owl:sameAs "dbpedia:Corps" .

:FieldArmy a owl:Class ;
	rdfs:label "Field Army"@en , "Armée (Unité)"@fr , "Armee (Großverband)"@de ;
	rdfs:comment "A field army containing Corps, Brigades, Divisions, etc..."@en ;
	foaf:logo <http://rdf.muninn-project.org/ww1/2011/11/11/image/29> ;
	owl:sameAs "dbpedia:Field_army" .

:WarTheater a owl:Class ;
	rdfs:label "Theater (warfare)"@en , "Théâtre militaire"@fr , "Kriegsschauplatz"@de ;
	rdfs:comment "An army theater of war."@en ;
	owl:sameAs "dbpedia:Theater_(warfare)" .

:ArmyCompany a owl:Class ;
	rdfs:label "Company (Military Unit)"@en , "Compagnie (militaire)"@fr , "Kompanie (Militär)"@de ;
	rdfs:comment "A military company"@en ;
	org:nominalSize "100" ;
	foaf:logo <http://rdf.muninn-project.org/ww1/2011/11/11/Image/86f5d79432849d7059da6460a74ba7fe> ;
	owl:sameAs "dbpedia:Company_(military_unit)" .

:Platoon a owl:Class ;
	rdfs:label "Platoon"@en , "Platoon"@fr , "Peloton (militaire)"@de ;
	rdfs:comment "A platoon"@en ;
	foaf:logo <http://rdf.muninn-project.org/ww1/2011/11/11/image/31> ;
	owl:sameAs "dbpedia:Platoon" ;
	org:isPartOf :ArmyCompany .

:ArmySection a owl:Class ;
	rdfs:label "Section (Military Unit)"@en , "Section (Militaire)"@fr , "Abschnitt (Militär)"@de ;
	foaf:logo <http://rdf.muninn-project.org/ww1/2011/11/11/image/32> ;
	owl:sameAs "dbpedia:Section_(military_unit)" .

:ArmySquad a owl:Class ;
	rdfs:label "Squad (Military Unit)"@en , "Équipe (Militaire)"@fr , "Gruppe (Militär)"@de ;
	foaf:logo <http://rdf.muninn-project.org/ww1/2011/11/11/image/33> ;
	owl:sameAs "dbpedia:Section_(military_unit)" .

:Fireteam a owl:Class ;
	rdfs:label "Fireteam (Military Unit)"@en , "Fireteam?"@fr , "Trupp (Militär)"@de ;
	foaf:logo <http://rdf.muninn-project.org/ww1/2011/11/11/image/34> ;
	owl:sameAs "dbpedia:Section_(military_unit)" .

:ArtilleryBattery a owl:Class ;
	rdfs:label "Artillery Battery"@en , "Batterie (armement)"@fr , "Batterie (Militär)"@de ;
	owl:subClassOf :Artillery ;
	foaf:logo <http://rdf.muninn-project.org/ww1/2011/11/11/image/35> ;
	owl:sameAs "dbpedia:Artillery_battery" .

:HorseArtillery a owl:Class ;
	rdfs:label "Horse Artillery"@en , "Artillerie à cheval"@fr ;
	owl:subClassOf :Artillery ;
	rdfs:label "Berittene Artillerie"@de ;
	rdfs:comment "Field, or foot, artillery where the guns and the gun crewa are transported by horses."@en ;
	owl:sameAs "dbpedia:Horse_artillery" .

:FieldArtillery a owl:Class ;
	rdfs:label "Field Artillery"@en , "Artillerie de campagne"@fr , "Berittene Kampagne"@de ;
	rdfs:comment "Field, or foot, artillery where the guns are pulled by horses but the gun crews are on foot."@en ;
	owl:sameAs "dbpedia:Field_artillery" ;
	owl:subClassOf :Artillery .

:MountainArtillery a owl:Class ;
	rdfs:label "Mountain Artillery"@en , "Artillerie de Montagnecampagne"@fr , "Gebirgsgeschütz"@de ;
	rdfs:comment "Artillery units capable of disassembling and reassembling their guns for mountain transport."@en ;
	owl:subClassOf :Artillery .

:GrandeBatterie a owl:Class ;
	rdfs:label "Grand Battery"@en , "Grande Batterie"@fr , "Grand-Batterie"@de ;
	rdfs:comment "Large unit of all available artillery batteries."@en ;
	owl:sameAs "dbpedia:Grand_Battery" ;
	owl:subClassOf :Artillery .

:ArtilleryBatteryDivision a owl:Class ;
	rdfs:label "Divisional Artillery"@en , "Division de Batterie (armement)"@fr , "Batterie Division (Militär)"@de ;
	owl:subClassOf :Artillery .

:Squadron a owl:Class ;
	rdfs:label "Squadron (unit)"@en , "Escadron"@fr , "Schwadron"@de .

:Cavalry a owl:Class ;
	rdfs:label "Cavalry"@en , "Cavalerie"@fr , "Kavallerie"@de ;
	owl:sameAs "dbpedia:Cavalry" .

:HouseholdCavalry a owl:Class ;
	rdfs:label "Household Cavalry"@en ;
	owl:sameAs "dbpedia:Household_Cavalry" ;
	foaf:membershipClass <http://rdf.muninn-project.org/ontologies/HouseholdCavalryRanks> .

<http://rdf.muninn-project.org/ontologies/HouseholdCavalryRanks> a owl:Class ;
	owl:subClassOf <mil:Rank> .

:HouseholdCavalry foaf:membershipClass <http://rdf.muninn-project.org/ontologies/HouseholdCavalryAppointments> .

<http://rdf.muninn-project.org/ontologies/HouseholdCavalryAppointments> a owl:Class ;
	owl:subClassOf <http://rdf.muninn-project.org/ontologies/Appointment> .

:CavalrySquadron a owl:Class ;
	rdfs:label "Cavalry Squadron"@en , "Escadron de Cavalerie"@fr , "Kavallerie Schwadron"@de ;
	rdfs:comment "A squadron of Cavalrymen."@en ;
	owl:subClass :Squadron , :Cavalry ;
	owl:sameAs "dbpedia:Squadron_(army)" .

:CavalryTroop a owl:Class ;
	rdfs:label "Cavalry Troop"@en , "Troupe de Cavalerie"@fr , "Kavallerie Truppe"@de ;
	rdfs:comment "A troop of Cavalrymen."@en ;
	owl:subClass :ArmyTroop , :Cavalry .

:ArmyTroop a owl:Class ;
	rdfs:label "Troop (Military)"@en , "Troupe (Militare)"@fr , "Truppe (Militär)"@de ;
	rdfs:comment "A generic class for an army troop in the Cavalry or a Corps."@en .

<http://rdf.muninn-project.org/ww1/2011/11/11/BattleSpace/FightsPrimarilyInAir> a :BattleSpace ;
	rdfs:label "Air (Battleground)"@en ;
	rdfs:comment "Fights primarily in Air."@en .

:AirForceServiceBranch a owl:Class ;
	rdfs:label "Air Force (Service Branch)"@en , "Force aérienne (Service Militare)"@fr , "Luftstreitkräfte (Service)"@de ;
	owl:subClassOf :MilitaryServiceBranch , :FightsPrimarilyInAir , <org:AirBasedOrganization> .

:NamedAirForceUnit a owl:Class ;
	rdfs:label "Air Force (Unit)"@en , "Force aérienne (Unitée)"@fr , "Luftstreitkräfte (Einheit)"@de ;
	rdfs:comment "Use this for numbered / named air forces, eg: US 8th Air Force."@en ;
	owl:subClassOf :FightsPrimarilyInair .

:TacticalAirForce a owl:Class ;
	rdfs:label "Tactical Air Force"@en , "Force Aérienne Tactique"@fr , "Luftstreitkräfte (taktisch)"@de ;
	rdfs:comment "Tactical Air Force."@en ;
	owl:subClassOf :FightsPrimarilyInAir .

:ProtoAirForce a owl:Class ;
	rdfs:label "Proto_air_force"@en ;
	rdfs:comment "Use this class for army air corps, naval aviation and army aviation."@en ;
	owl:subClassOf :FightsPrimarilyInAir ;
	owl:disjointWith :AirForce .

:AirForceCommand a owl:Class ;
	rdfs:label "Command (Air Force)"@en , ""@fr , ""@de ;
	rdfs:comment "An air force command. eg: Bomber Command."@en .

:AirForceGroup a owl:Class ;
	rdfs:label "Group (Air Force)"@en , ""@fr , ""@de ;
	rdfs:comment "An air force group."@en .

:AirForceStation a owl:Class ;
	rdfs:label "Station (Air Force)"@en , ""@fr , ""@de ;
	rdfs:comment "An air force station."@en .

:NavyAirStation a owl:Class ;
	rdfs:label "Station (Naval Aircraft)"@en , ""@fr , ""@de ;
	rdfs:comment "An Naval air station."@en .

:AirForceWing a owl:Class ;
	rdfs:label "Wing (Air Force)"@en , ""@fr , ""@de ;
	rdfs:comment "An Air Force Wing."@en .

:AviationSquadron a owl:Class ;
	rdfs:label "Aviation Squadron"@en , "Escadron de l'air"@fr , "Staffel (Militär)"@de ;
	rdfs:comment "An aviation squadron."@en ;
	owl:subClass :Squadron , :air ;
	owl:sameAs "dbpedia:Squadron_(aviation)" .

:MilitaryAirborneFlight a owl:Class ;
	rdfs:label "Aviation Flight (Military Unit)"@en , "Escadrille"@fr , "Schwarm (Luftfahrt)"@de ;
	rdfs:comment "An aviation airborne flight."@en ;
	owl:subClass :flight , :air .

:MilitaryGroundFlight a owl:Class ;
	rdfs:label "Ground Flight (Military Unit)"@en , "Escadrille de terra"@fr , "Schwarm Boden(Luftfahrt)"@de ;
	rdfs:comment "Consists of ground personel for an air force."@en ;
	owl:subClass :flight , :air .

:MilitaryFlightUnit a owl:Class ;
	rdfs:label "Flight (Military Unit)"@en , "Escadrille"@fr , "Schwarm"@de ;
	rdfs:comment "A flight as a group of people."@en .

:AirForceElement a owl:Class ;
	rdfs:label "Element (Air Force)"@en , "Élement"@fr , "Element"@de ;
	rdfs:comment "An element from an Air Force flight."@en .

:AirForceSection a owl:Class ;
	rdfs:label "Section (Air Force)"@en , "Section"@fr , "Section"@de ;
	rdfs:comment "A section from an Air Force flight."@en .

:AirForceDetail a owl:Class ;
	rdfs:label "Detail (Air Force)"@en , ""@de ;
	rdfs:comment "A detail from an Air Force flight."@en .

:BattleSpace a owl:Class ;
	rdfs:label "Battle Space"@en , "Espace de Battaille"@fr , ""@de ;
	rdfs:comment "A detail from an Air Force flight."@en ;
	owl:sameAs "dbpedia:Battlespace" .

<http://rdf.muninn-project.org/ww1/2011/11/11/BattleSpace/information> a :BattleSpace ;
	rdfs:label "Information"@en ;
	rdfs:comment "Fights primarily with information, used for inteliigence outfits."@en .

<http://rdf.muninn-project.org/ww1/2011/11/11/BattleSpace/spacethefinalfrontier> a :BattleSpace ;
	rdfs:label "Space"@en ;
	rdfs:comment "Fights primarily in space."@en .

:NatoRanks a owl:Class ;
	rdfs:label "Ranks of NATO"@en , "NATO Rangcode"@de , "Grades de l'OTAN"@fr ;
	owl:subClassOf :MilitaryRank .

:NatoRankOF-1 a owl:Class ;
	rdfs:label "NATO Officer Rank OF-1"@en ;
	owl:subClassOf :NatoRanks , :Officer ;
	org:rankSeniorTo <http://rdf.muninn-project.org/ontologies/NatoRankOF-1> .

:NatoRankOF-2 a owl:Class ;
	rdfs:label "NATO Officer Rank OF-2"@en ;
	owl:subClassOf :Nato_Ranks , :Officer ;
	org:rankJuniorTo <http://rdf.muninn-project.org/ontologies/NatoRankOF-1> ;
	org:rankSeniorTo <http://rdf.muninn-project.org/ontologies/NatoRankOF-3> .

:NatoRankOF-3 a owl:Class ;
	rdfs:label "NATO Officer Rank OF-3"@en ;
	owl:subClassOf :NatoRanks , :Officer ;
	org:rankJuniorTo <http://rdf.muninn-project.org/ontologies/NatoRankOF-2> ;
	org:rankSeniorTo <http://rdf.muninn-project.org/ontologies/NatoRankOF-4> .

:NatoRankOF-4 a owl:Class ;
	rdfs:label "NATO Officer Rank OF-4"@en ;
	owl:subClassOf :NatoRanks , :Officer ;
	org:rankJuniorTo <http://rdf.muninn-project.org/ontologies/NatoRankOF-3> ;
	org:rankSeniorTo <http://rdf.muninn-project.org/ontologies/NatoRankOF-5> .

:NatoRankOF-5 a owl:Class ;
	rdfs:label "NATO Officer Rank OF-5"@en ;
	owl:subClassOf :NatoRanks , :Officer ;
	org:rankJuniorTo <http://rdf.muninn-project.org/ontologies/NatoRankOF-4> ;
	org:rankSeniorTo <http://rdf.muninn-project.org/ontologies/NatoRankOF-6> .

:NatoRankOF-6 a owl:Class ;
	rdfs:label "NATO Officer Rank OF-6"@en ;
	owl:subClassOf :NatoRanks , :Officer ;
	org:rankJuniorTo <http://rdf.muninn-project.org/ontologies/NatoRankOF-5> ;
	org:rankSeniorTo <http://rdf.muninn-project.org/ontologies/NatoRankOF-7> .

:NatoRankOF-7 a owl:Class ;
	rdfs:label "NATO Officer Rank OF-7"@en ;
	owl:subClassOf :NatoRanks , :Officer ;
	org:rankJuniorTo <http://rdf.muninn-project.org/ontologies/NatoRankOF-6> ;
	org:rankSeniorTo <http://rdf.muninn-project.org/ontologies/NatoRankOF-8> .

:NatoRankOF-8 a owl:Class ;
	rdfs:label "NATO Officer Rank OF-8"@en ;
	owl:subClassOf :NatoRanks , :Officer ;
	org:rankJuniorTo <http://rdf.muninn-project.org/ontologies/NatoRankOF-7> ;
	org:rankSeniorTo <http://rdf.muninn-project.org/ontologies/NatoRankOF-9> .

:NatoRankOF-9 a owl:Class ;
	rdfs:label "NATO Officer Rank OF-9"@en ;
	owl:subClassOf :NatoRanks , :Officer ;
	org:rankJuniorTo <http://rdf.muninn-project.org/ontologies/NatoRankOF-8> ;
	org:rankSeniorTo <http://rdf.muninn-project.org/ontologies/NatoRankOF-10> .

:NatoRankOF-10 a owl:Class ;
	rdfs:label "NATO Officer Rank OF-10"@en ;
	owl:subClassOf :NatoRanks , :Officer ;
	org:rankJuniorTo <http://rdf.muninn-project.org/ontologies/NatoRankOF-10> ;
	org:rankSeniorTo <http://rdf.muninn-project.org/ontologies/NatoRankWO-1> .

:NatoRankWO-1 a owl:Class ;
	rdfs:label "NATO Warrant Officer Rank WO-1"@en ;
	owl:subClassOf :NatoRanks , :WarrantOfficer ;
	org:rankSeniorTo <http://rdf.muninn-project.org/ontologies/NatoRankWO-2> ;
	org:rankJuniorTo <http://rdf.muninn-project.org/ontologies/NatoRankOF-10> .

:NatoRankWO-2 a owl:Class ;
	rdfs:label "NATO Warrant Officer Rank WO-2"@en ;
	owl:subClassOf :NatoRanks , :WarrantOfficer ;
	org:rankSeniorTo <http://rdf.muninn-project.org/ontologies/NatoRankWO-3> ;
	org:rankJuniorTo <http://rdf.muninn-project.org/ontologies/NatoRankWO-1> .

:NatoRankWO-3 a owl:Class ;
	rdfs:label "NATO Warrant Officer Rank WO-3"@en ;
	owl:subClassOf :NatoRanks , :WarrantOfficer ;
	org:rankSeniorTo <http://rdf.muninn-project.org/ontologies/NatoRankWO-4> ;
	org:rankJuniorTo <http://rdf.muninn-project.org/ontologies/NatoRankWO-2> .

:NatoRankWO-4 a owl:Class ;
	rdfs:label "NATO Warrant Officer Rank WO-4"@en ;
	owl:subClassOf :NatoRanks , :WarrantOfficer ;
	org:rankSeniorTo <http://rdf.muninn-project.org/ontologies/NatoRankWO-5> ;
	org:rankJuniorTo <http://rdf.muninn-project.org/ontologies/NatoRankWO-3> .

:NatoRankWO-5 a owl:Class ;
	rdfs:label "NATO Warrant Officer Rank WO-5"@en ;
	owl:subClassOf :NatoRanks , :WarrantOfficer ;
	org:rankJuniorTo <http://rdf.muninn-project.org/ontologies/NatoRankWO-4> ;
	org:rankSeniorTo <http://rdf.muninn-project.org/ontologies/NatoRankOR-1> .

:NatoRankOR-1 a owl:Class ;
	rdfs:label "NATO Other/Enlisted Rank OR-1"@en ;
	owl:subClassOf :NatoRanks , :NonCommissionedOfficer , :Enlisted ;
	org:rankJuniorTo <http://rdf.muninn-project.org/ontologies/NatoRankWO-5> ;
	org:rankSeniorTo <http://rdf.muninn-project.org/ontologies/NatoRankOR-2> .

:NatoRankOR-2 a owl:Class ;
	rdfs:label "NATO Other/Enlisted Rank OR-2"@en ;
	owl:subClassOf :NatoRanks , :NonCommissionedOfficer , :Enlisted ;
	org:rankJuniorTo <http://rdf.muninn-project.org/ontologies/NatoRankOR-1> ;
	org:rankSeniorTo <http://rdf.muninn-project.org/ontologies/NatoRankOR-3> .

:NatoRankOR-3 a owl:Class ;
	rdfs:label "NATO Other/Enlisted Rank OR-3"@en ;
	owl:subClassOf :NatoRanks , :NonCommissionedOfficer , :Enlisted ;
	org:rankJuniorTo <http://rdf.muninn-project.org/ontologies/NatoRankOR-2> ;
	org:rankSeniorTo <http://rdf.muninn-project.org/ontologies/NatoRankOR-4> .

:NatoRankOR-4 a owl:Class ;
	rdfs:label "NATO Other/Enlisted Rank OR-4"@en ;
	owl:subClassOf :NatoRanks , :NonCommissionedOfficer , :Enlisted ;
	org:rankJuniorTo <http://rdf.muninn-project.org/ontologies/NatoRankOR-3> ;
	org:rankSeniorTo <http://rdf.muninn-project.org/ontologies/NatoRankOR-5> .

:NatoRankOR-5 a owl:Class ;
	rdfs:label "NATO Other/Enlisted Rank OR-5"@en ;
	owl:subClassOf :NatoRanks , :NonCommissionedOfficer , :Enlisted ;
	org:rankJuniorTo <http://rdf.muninn-project.org/ontologies/NatoRankOR-4> ;
	org:rankSeniorTo <http://rdf.muninn-project.org/ontologies/NatoRankOR-6> .

:NatoRankOR-6 a owl:Class ;
	rdfs:label "NATO Other/Enlisted Rank OR-6"@en ;
	owl:subClassOf :NatoRanks , :NonCommissionedOfficer , :Enlisted ;
	org:rankJuniorTo <http://rdf.muninn-project.org/ontologies/NatoRankOR-5> ;
	org:rankSeniorTo <http://rdf.muninn-project.org/ontologies/NatoRankOR-7> .

:NatoRankOR-7 a owl:Class ;
	rdfs:label "NATO Other/Enlisted Rank OR-7"@en ;
	owl:subClassOf :NatoRanks , :NonCommissionedOfficer , :Enlisted ;
	org:rankJuniorTo <http://rdf.muninn-project.org/ontologies/NatoRankOR-6> ;
	org:rankSeniorTo <http://rdf.muninn-project.org/ontologies/NatoRankOR-8> .

:NatoRankOR-8 a owl:Class ;
	rdfs:label "NATO Other/Enlisted Rank OR-8"@en ;
	owl:subClassOf :NatoRanks , :NonCommissionedOfficer , :Enlisted ;
	org:rankJuniorTo <http://rdf.muninn-project.org/ontologies/NatoRankOR-7> ;
	org:rankSeniorTo <http://rdf.muninn-project.org/ontologies/NatoRankOR-9> .

:NatoRankOR-9 a owl:Class ;
	rdfs:label "NATO Other/Enlisted Rank OR-9"@en ;
	owl:subClassOf :NatoRanks , :NonCommissionedOfficer , :Enlisted ;
	org:rankJuniorTo <http://rdf.muninn-project.org/ontologies/NatoRankOR-8> .

<dbpedia:Admiral> muninn:wikipedia_version "103794321" .

<dbpedia:Brigadier> muninn:wikipedia_version "102695895" .

<dbpedia:Colonel> muninn:wikipedia_version "88659726" .

<dbpedia:Commander> muninn:wikipedia_version "92206694" .

<dbpedia:Lieutenant> muninn:wikipedia_version "81222307" .

<dbpedia:Major> muninn:wikipedia_version "103728073" .

<dbpedia:Marshal> muninn:wikipedia_version "103489138" .

<dbpedia:Midshipman> muninn:wikipedia_version "104159410" .

<dbpedia:Seaman> muninn:wikipedia_version "91409028" .

<dbpedia:Sergeant> muninn:wikipedia_version "102800259" .

:Rank_Admiral_EnglishTradition a :MilitaryRank ;
	org:rankEquivalentTo :Rank_Air_marshal_EnglishTradition , :Rank_General_officer_EnglishTradition ;
	org:rankJuniorTo_Transitive :Rank_Admiral_of_the_fleet_EnglishTradition ;
	org:rankOf :EnglishTradition , <mil:NavyServiceBranch> ;
	org:rankSeniorTo_Transitive <http://rdf.muninn-project.org/ontologies/military#Rank_Commodore_(rank)_EnglishTradition> ;
	rdfs:comment "Admiral is the rank, or part of the name of the ranks, of the highest naval officers. It is usually considered a full admiral (equivalent to full general) and above vice admiral and below admiral of the fleet. It is usually abbreviated to \"Adm\" or \"ADM\". Where relevant, admiral has a NATO code of OF-9, and is a 4 star rank."@en ;
	rdfs:label "Admiral"@de , "Admiral"@en , "Amiral"@fr ;
	owl:sameAs <dbpedia:Admiral> .

:Rank_Admiral_of_the_fleet_EnglishTradition a :MilitaryRank ;
	org:rankEquivalentTo :Rank_Field_marshal_EnglishTradition , :Rank_Marshal_EnglishTradition , :Rank_Marshal_of_the_air_force_EnglishTradition ;
	org:rankOf :EnglishTradition , <mil:NavyServiceBranch> ;
	org:rankSeniorTo_Transitive :Rank_Admiral_EnglishTradition ;
	rdfs:label "Admiral of the fleet"@en ;
	owl:sameAs <dbpedia:Admiral_of_the_fleet> .

:Rank_Air_commodore_EnglishTradition a :MilitaryRank ;
	org:rankEquivalentTo :Rank_Brigadier_EnglishTradition , <http://rdf.muninn-project.org/ontologies/military#Rank_Commodore_(rank)_EnglishTradition> ;
	org:rankJuniorTo_Transitive :Rank_Air_marshal_EnglishTradition ;
	org:rankOf :EnglishTradition , <mil:AirForceServiceBranch> ;
	org:rankSeniorTo_Transitive :Rank_Group_captain_EnglishTradition ;
	rdfs:label "Air commodore"@en ;
	owl:sameAs <dbpedia:Air_commodore> .

:Rank_Air_marshal_EnglishTradition a :MilitaryRank ;
	org:rankEquivalentTo :Rank_Admiral_EnglishTradition , :Rank_General_officer_EnglishTradition ;
	org:rankJuniorTo_Transitive :Rank_Marshal_of_the_air_force_EnglishTradition ;
	org:rankOf :EnglishTradition , <mil:AirForceServiceBranch> ;
	org:rankSeniorTo_Transitive :Rank_Air_commodore_EnglishTradition ;
	rdfs:label "Air marshal"@en ;
	owl:sameAs <dbpedia:Air_marshal> .

:Rank_Aircraftman_EnglishTradition a :MilitaryRank ;
	org:rankEquivalentTo <http://rdf.muninn-project.org/ontologies/military#Rank_Private_(rank)_EnglishTradition> , :Rank_Seaman_EnglishTradition ;
	org:rankJuniorTo_Transitive :Rank_Corporal_EnglishTradition ;
	org:rankOf :EnglishTradition , <mil:AirForceServiceBranch> ;
	rdfs:comment "Aircraftman (AC), or Aircraftwoman (ACW), is the lowest rank in the Royal Air Force and the air forces of several other Commonwealth countries. Aircraftman ranks below Leading Aircraftman and has a NATO rank code of OR-1. It is presently a training rank only and no airmen in productive service hold this rank. Aircraftman do not wear any rank insignia."@en ;
	rdfs:label "Aircraftman"@en ;
	owl:sameAs <dbpedia:Aircraftman> .

:Rank_Brigadier_EnglishTradition a :MilitaryRank ;
	org:rankEquivalentTo :Rank_Air_commodore_EnglishTradition , <http://rdf.muninn-project.org/ontologies/military#Rank_Commodore_(rank)_EnglishTradition> ;
	org:rankJuniorTo_Transitive :Rank_General_officer_EnglishTradition ;
	org:rankOf :EnglishTradition , <mil:ArmyServiceBranch> ;
	org:rankSeniorTo_Transitive :Rank_Colonel_EnglishTradition ;
	rdfs:comment "Brigadier is a senior military rank, the meaning of which is somewhat different in different military services. The brigadier rank is generally superior to the rank of colonel, and subordinate to major general. A brigadier typically commands a brigade consisting of three battalions (approximately 3,000 troops). Many countries use the rank Brigadier General rather than Brigadier, and prior to the 1920s, so did members of the Commonwealth."@en ;
	rdfs:label "Brigadier"@de , "Brigadier"@en , "Brigadier"@fr ;
	owl:sameAs <dbpedia:Brigadier> .

<http://rdf.muninn-project.org/ontologies/military#Rank_Captain_(OF-2)_EnglishTradition> a :MilitaryRank ;
	org:rankEquivalentTo :Rank_Flight_lieutenant_EnglishTradition , <http://rdf.muninn-project.org/ontologies/military#Rank_Lieutenant_(navy)_EnglishTradition> ;
	org:rankJuniorTo_Transitive <http://rdf.muninn-project.org/ontologies/military#Rank_Commandant_(rank)_EnglishTradition> ;
	org:rankOf :EnglishTradition , <mil:ArmyServiceBranch> ;
	org:rankSeniorTo_Transitive :Rank_Lieutenant_EnglishTradition ;
	owl:sameAs <dbpedia:Captain_(OF-2)> .

<http://rdf.muninn-project.org/ontologies/military#Rank_Captain_(naval)_EnglishTradition> a :MilitaryRank ;
	org:rankEquivalentTo :Rank_Colonel_EnglishTradition , :Rank_Group_captain_EnglishTradition ;
	org:rankJuniorTo_Transitive <http://rdf.muninn-project.org/ontologies/military#Rank_Commodore_(rank)_EnglishTradition> ;
	org:rankOf :EnglishTradition , <mil:NavyServiceBranch> ;
	org:rankSeniorTo_Transitive :Rank_Commander_EnglishTradition ;
	owl:sameAs <dbpedia:Captain_(naval)> .

:Rank_Colonel_EnglishTradition a :MilitaryRank ;
	org:rankEquivalentTo <http://rdf.muninn-project.org/ontologies/military#Rank_Captain_(naval)_EnglishTradition> , :Rank_Group_captain_EnglishTradition ;
	org:rankJuniorTo_Transitive :Rank_Brigadier_EnglishTradition ;
	org:rankOf :EnglishTradition , <mil:ArmyServiceBranch> ;
	org:rankSeniorTo_Transitive :Rank_Lieutenant_colonel_EnglishTradition ;
	rdfs:comment "Colonel, abbreviated as Col or COL, is a military rank of a senior commissioned officer. It or a corresponding rank exists in most armies and in many air forces; the naval equivalent rank is generally \"Captain\". It is also used in some police forces and other paramilitary rank structures. A colonel is typically in charge of a regiment in an army. \"Colonel\" is usually the highest or second-highest field rank, and is below the general ranks."@en ;
	rdfs:label "Colonel"@en , "Colonel"@fr , "Oberst"@de ;
	owl:sameAs <dbpedia:Colonel> .

<http://rdf.muninn-project.org/ontologies/military#Rank_Commandant_(rank)_EnglishTradition> a :MilitaryRank ;
	org:rankEquivalentTo :Rank_Lieutenant_commander_EnglishTradition , :Rank_Squadron_leader_EnglishTradition ;
	org:rankJuniorTo_Transitive :Rank_Lieutenant_colonel_EnglishTradition ;
	org:rankOf :EnglishTradition , <mil:ArmyServiceBranch> ;
	org:rankSeniorTo_Transitive <http://rdf.muninn-project.org/ontologies/military#Rank_Captain_(OF-2)_EnglishTradition> ;
	owl:sameAs <dbpedia:Commandant_(rank)> .

:Rank_Commander_EnglishTradition a :MilitaryRank ;
	org:rankEquivalentTo :Rank_Lieutenant_colonel_EnglishTradition , <http://rdf.muninn-project.org/ontologies/military#Rank_Wing_commander_(rank)_EnglishTradition> ;
	org:rankJuniorTo_Transitive <http://rdf.muninn-project.org/ontologies/military#Rank_Captain_(naval)_EnglishTradition> ;
	org:rankOf :EnglishTradition , <mil:NavyServiceBranch> ;
	org:rankSeniorTo_Transitive :Rank_Lieutenant_commander_EnglishTradition ;
	rdfs:comment "Commander is a naval rank which is also sometimes used as a military title depending on the individual customs of a given military service. Commander is also used as a rank or title in some organizations outside of the armed forces, particularly in police and law enforcement."@en ;
	rdfs:label "Capitaine de frégate"@fr , "Commander"@en , "Fregattenkapitän"@de ;
	owl:sameAs <dbpedia:Commander> .

<http://rdf.muninn-project.org/ontologies/military#Rank_Commodore_(rank)_EnglishTradition> a :MilitaryRank ;
	org:rankEquivalentTo :Rank_Air_commodore_EnglishTradition , :Rank_Brigadier_EnglishTradition ;
	org:rankJuniorTo_Transitive :Rank_Admiral_EnglishTradition ;
	org:rankOf :EnglishTradition , <mil:NavyServiceBranch> ;
	org:rankSeniorTo_Transitive <http://rdf.muninn-project.org/ontologies/military#Rank_Captain_(naval)_EnglishTradition> ;
	owl:sameAs <dbpedia:Commodore_(rank)> .

:Rank_Corporal_EnglishTradition a :MilitaryRank ;
	org:rankEquivalentTo :Rank_Corporal_EnglishTradition , :Rank_Leading_seaman_EnglishTradition ;
	org:rankJuniorTo_Transitive :Rank_Sergeant_EnglishTradition ;
	org:rankOf :EnglishTradition , <mil:AirForceServiceBranch> , <mil:ArmyServiceBranch> ;
	org:rankSeniorTo_Transitive :Rank_Aircraftman_EnglishTradition , <http://rdf.muninn-project.org/ontologies/military#Rank_Private_(rank)_EnglishTradition> ;
	rdfs:comment "Corporal is a rank in use in some form by most militaries and by some police forces or other uniformed organizations. It is usually equivalent to NATO Rank Code OR-4. The rank of corporal nominally corresponds to commanding a section or squad of soldiers. However, in the United States Army, but not the U.S. Marines, a corporal is usually a fire team leader or second-in-command of a squad of soldiers."@en ;
	rdfs:label "Caporal"@fr , "Corporal"@en , "Korporal"@de ;
	owl:sameAs <dbpedia:Corporal> .

<http://rdf.muninn-project.org/ontologies/military#Rank_Ensign_(rank)_EnglishTradition> a :MilitaryRank ;
	org:rankEquivalentTo :Rank_Pilot_officer_EnglishTradition , :Rank_Second_lieutenant_EnglishTradition ;
	org:rankJuniorTo_Transitive :Rank_Sub-lieutenant_EnglishTradition ;
	org:rankOf :EnglishTradition , <mil:NavyServiceBranch> ;
	org:rankSeniorTo_Transitive :Rank_Midshipman_EnglishTradition ;
	owl:sameAs <dbpedia:Ensign_(rank)> .

:Rank_Field_marshal_EnglishTradition a :MilitaryRank ;
	org:rankEquivalentTo :Rank_Admiral_of_the_fleet_EnglishTradition , :Rank_Marshal_of_the_air_force_EnglishTradition ;
	org:rankOf :EnglishTradition , <mil:ArmyServiceBranch> ;
	org:rankSeniorTo_Transitive :Rank_General_officer_EnglishTradition ;
	rdfs:label "Field marshal"@en ;
	owl:sameAs <dbpedia:Field_marshal> .

:Rank_Flight_lieutenant_EnglishTradition a :MilitaryRank ;
	org:rankEquivalentTo <http://rdf.muninn-project.org/ontologies/military#Rank_Captain_(OF-2)_EnglishTradition> , <http://rdf.muninn-project.org/ontologies/military#Rank_Lieutenant_(navy)_EnglishTradition> ;
	org:rankJuniorTo_Transitive :Rank_Squadron_leader_EnglishTradition ;
	org:rankOf :EnglishTradition , <mil:AirForceServiceBranch> ;
	org:rankSeniorTo_Transitive :Rank_Flying_officer_EnglishTradition ;
	rdfs:label "Flight lieutenant"@en ;
	owl:sameAs <dbpedia:Flight_lieutenant> .

:Rank_Flying_officer_EnglishTradition a :MilitaryRank ;
	org:rankEquivalentTo :Rank_Lieutenant_EnglishTradition , :Rank_Sub-lieutenant_EnglishTradition ;
	org:rankJuniorTo_Transitive :Rank_Flight_lieutenant_EnglishTradition ;
	org:rankOf :EnglishTradition , <mil:AirForceServiceBranch> ;
	org:rankSeniorTo_Transitive :Rank_Pilot_officer_EnglishTradition ;
	rdfs:label "Flying officer"@en ;
	owl:sameAs <dbpedia:Flying_officer> .

:Rank_General_officer_EnglishTradition a :MilitaryRank ;
	org:rankEquivalentTo :Rank_Admiral_EnglishTradition , :Rank_Air_marshal_EnglishTradition ;
	org:rankJuniorTo_Transitive :Rank_Field_marshal_EnglishTradition ;
	org:rankOf :EnglishTradition , <mil:ArmyServiceBranch> ;
	org:rankSeniorTo_Transitive :Rank_Brigadier_EnglishTradition ;
	rdfs:comment "A general officer is an officer of high military rank, usually in the army, and in some nations, the air force. The term is widely used by many nations of the world, and when a country uses a different term, there is an equivalent title given. The term General is used in two ways: as the generic title for all grades of general officer; and as a specific rank. Since the late twentieth century, the rank of General is usually the highest active rank of a military not at war."@en ;
	rdfs:label "General"@de , "General officer"@en , "Général"@fr ;
	owl:sameAs <dbpedia:General_officer> .

:Rank_Group_captain_EnglishTradition a :MilitaryRank ;
	org:rankEquivalentTo <http://rdf.muninn-project.org/ontologies/military#Rank_Captain_(naval)_EnglishTradition> , :Rank_Colonel_EnglishTradition ;
	org:rankJuniorTo_Transitive :Rank_Air_commodore_EnglishTradition ;
	org:rankOf :EnglishTradition , <mil:AirForceServiceBranch> ;
	org:rankSeniorTo_Transitive <http://rdf.muninn-project.org/ontologies/military#Rank_Wing_commander_(rank)_EnglishTradition> ;
	rdfs:label "Group captain"@en ;
	owl:sameAs <dbpedia:Group_captain> .

:Rank_Leading_seaman_EnglishTradition a :MilitaryRank ;
	org:rankEquivalentTo :Rank_Corporal_EnglishTradition ;
	org:rankJuniorTo_Transitive :Rank_Petty_officer_EnglishTradition ;
	org:rankOf :EnglishTradition , <mil:NavyServiceBranch> ;
	org:rankSeniorTo_Transitive :Rank_Seaman_EnglishTradition ;
	rdfs:label "Leading seaman"@en ;
	owl:sameAs <dbpedia:Leading_seaman> .

<http://rdf.muninn-project.org/ontologies/military#Rank_Lieutenant_(navy)_EnglishTradition> a :MilitaryRank ;
	org:rankEquivalentTo <http://rdf.muninn-project.org/ontologies/military#Rank_Captain_(OF-2)_EnglishTradition> , :Rank_Flight_lieutenant_EnglishTradition ;
	org:rankJuniorTo_Transitive :Rank_Lieutenant_commander_EnglishTradition ;
	org:rankOf :EnglishTradition , <mil:NavyServiceBranch> ;
	org:rankSeniorTo_Transitive :Rank_Sub-lieutenant_EnglishTradition ;
	owl:sameAs <dbpedia:Lieutenant_(navy)> .

:Rank_Lieutenant_EnglishTradition a :MilitaryRank ;
	org:rankEquivalentTo :Rank_Flying_officer_EnglishTradition , :Rank_Sub-lieutenant_EnglishTradition ;
	org:rankJuniorTo_Transitive <http://rdf.muninn-project.org/ontologies/military#Rank_Captain_(OF-2)_EnglishTradition> ;
	org:rankOf :EnglishTradition , <mil:ArmyServiceBranch> ;
	org:rankSeniorTo_Transitive :Rank_Second_lieutenant_EnglishTradition ;
	rdfs:comment "A Lieutenant is a commissioned officer in many nations' armed forces. Typically, the rank of lieutenant in naval usage is senior to the army rank. It is also used in fire services, emergency medical services, security services and police forces as a rank. Lieutenant may also appear as part of a title used in various other organisations with a codified command structure. It often designates someone who is \"second-in-command,\" and as such, may precede the name of the rank directly above it."@en ;
	rdfs:label "Leutnant"@de , "Lieutenant"@de , "Lieutenant"@en , "Lieutenant (grade militaire)"@fr ;
	owl:sameAs <dbpedia:Lieutenant> .

:Rank_Lieutenant_colonel_EnglishTradition a :MilitaryRank ;
	org:rankEquivalentTo :Rank_Commander_EnglishTradition , <http://rdf.muninn-project.org/ontologies/military#Rank_Wing_commander_(rank)_EnglishTradition> ;
	org:rankJuniorTo_Transitive :Rank_Colonel_EnglishTradition ;
	org:rankOf :EnglishTradition , <mil:ArmyServiceBranch> ;
	org:rankSeniorTo_Transitive <http://rdf.muninn-project.org/ontologies/military#Rank_Commandant_(rank)_EnglishTradition> , :Rank_Major_EnglishTradition ;
	rdfs:label "Lieutenant colonel"@en ;
	owl:sameAs <dbpedia:Lieutenant_colonel> .

:Rank_Lieutenant_commander_EnglishTradition a :MilitaryRank ;
	org:rankEquivalentTo <http://rdf.muninn-project.org/ontologies/military#Rank_Commandant_(rank)_EnglishTradition> , :Rank_Major_EnglishTradition , :Rank_Squadron_leader_EnglishTradition ;
	org:rankJuniorTo_Transitive :Rank_Commander_EnglishTradition ;
	org:rankOf :EnglishTradition , <mil:NavyServiceBranch> ;
	org:rankSeniorTo_Transitive <http://rdf.muninn-project.org/ontologies/military#Rank_Lieutenant_(navy)_EnglishTradition> ;
	rdfs:label "Lieutenant commander"@en ;
	owl:sameAs <dbpedia:Lieutenant_commander> .

:Rank_Major_EnglishTradition a :MilitaryRank ;
	org:rankEquivalentTo :Rank_Lieutenant_commander_EnglishTradition , :Rank_Squadron_leader_EnglishTradition ;
	org:rankJuniorTo_Transitive :Rank_Lieutenant_colonel_EnglishTradition ;
	org:rankOf :EnglishTradition , <mil:ArmyServiceBranch> ;
	rdfs:comment "Major is a rank of commissioned officer, with corresponding ranks existing in almost every military in the world. When used unhyphenated, in conjunction with no other indicator of rank, the term refers to the rank just senior to that of an Army captain and just below the rank of lieutenant colonel. It is considered the most junior of the field ranks. In some militaries, notably France, the rank is referred to as commandant, while in others it is known as \"captain-major\"."@en ;
	rdfs:label "Major"@de , "Major"@en , "Major"@fr ;
	owl:sameAs <dbpedia:Major> .

:Rank_Marshal_EnglishTradition a :MilitaryRank ;
	org:rankEquivalentTo :Rank_Admiral_of_the_fleet_EnglishTradition , :Rank_Marshal_of_the_air_force_EnglishTradition ;
	org:rankOf :EnglishTradition , <mil:ArmyServiceBranch> ;
	rdfs:comment "Marshal (also spelled marshall, more commonly in British English than American English), is a word used in several official titles of various branches of society. The word is an ancient loan word from Old (Norman) French, cf. modern French maréchal, which in turn is a borrowing from Old Frankish *marhskalk \"stable boy, keeper, servant\", still continued by Middle Dutch maerscalc, marscal \"id. \", modern Dutch maarschalk \"military commander\" (the meaning is under French influence)."@en ;
	rdfs:label "Marschall"@de , "Marshal"@en , "Marshal"@fr , "Maréchal (armée)"@fr ;
	owl:sameAs <dbpedia:Marshal> .

:Rank_Marshal_of_the_air_force_EnglishTradition a :MilitaryRank ;
	org:rankEquivalentTo :Rank_Admiral_of_the_fleet_EnglishTradition , :Rank_Field_marshal_EnglishTradition , :Rank_Marshal_EnglishTradition ;
	org:rankOf :EnglishTradition , <mil:AirForceServiceBranch> ;
	org:rankSeniorTo_Transitive :Rank_Air_marshal_EnglishTradition ;
	rdfs:label "Marshal of the air force"@en ;
	owl:sameAs <dbpedia:Marshal_of_the_air_force> .

:Rank_Midshipman_EnglishTradition a :MilitaryRank ;
	org:rankEquivalentTo :Rank_Officer_cadet_EnglishTradition ;
	org:rankJuniorTo_Transitive <http://rdf.muninn-project.org/ontologies/military#Rank_Ensign_(rank)_EnglishTradition> ;
	org:rankOf :EnglishTradition , <mil:NavyServiceBranch> ;
	org:rankSeniorTo_Transitive :Rank_Warrant_officer_EnglishTradition ;
	rdfs:comment "A midshipman is an officer cadet, or a commissioned officer of the lowest rank, in the Royal Navy, United States Navy, and many Commonwealth navies. Commonwealth countries which use the rank include Australia, New Zealand, South Africa, Pakistan, India, Singapore, Sri Lanka and Kenya. The rank was also used, prior to 1968, by the Royal Canadian Navy, but upon the creation of the Canadian Forces the rank of midshipman was replaced with the rank of naval cadet."@en ;
	rdfs:label "Midshipman"@de , "Midshipman"@en , "Seekadett"@de ;
	owl:sameAs <dbpedia:Midshipman> .

:Rank_Officer_cadet_EnglishTradition a :MilitaryRank ;
	org:rankEquivalentTo :Rank_Midshipman_EnglishTradition , :Rank_Officer_cadet_EnglishTradition ;
	org:rankJuniorTo_Transitive :Rank_Pilot_officer_EnglishTradition , :Rank_Second_lieutenant_EnglishTradition ;
	org:rankOf :EnglishTradition , <mil:AirForceServiceBranch> , <mil:ArmyServiceBranch> ;
	org:rankSeniorTo_Transitive :Rank_Sergeant_major_EnglishTradition , :Rank_Warrant_officer_EnglishTradition ;
	rdfs:label "Officer cadet"@en ;
	owl:sameAs <dbpedia:Officer_cadet> .

:Rank_Petty_officer_EnglishTradition a :MilitaryRank ;
	org:rankEquivalentTo :Rank_Sergeant_EnglishTradition ;
	org:rankJuniorTo_Transitive :Rank_Warrant_officer_EnglishTradition ;
	org:rankOf :EnglishTradition , <mil:NavyServiceBranch> ;
	org:rankSeniorTo_Transitive :Rank_Leading_seaman_EnglishTradition ;
	rdfs:comment "A petty officer is a non-commissioned officer in many navies and is given the NATO rank denotion OR-6. They are equal in rank to sergeant, British Army and Royal Air Force. A Petty Officer is superior in rank to Leading Rate and subordinate to Chief Petty Officer, in the case of the British Armed Forces. The modern petty officer dates back to the Age of Sail. Petty officers rank between naval officers and most enlisted sailors."@en ;
	rdfs:label "Maître (grade)"@fr , "Petty Officer"@de , "Petty officer"@en ;
	owl:sameAs <dbpedia:Petty_officer> .

:Rank_Pilot_officer_EnglishTradition a :MilitaryRank ;
	org:rankEquivalentTo <http://rdf.muninn-project.org/ontologies/military#Rank_Ensign_(rank)_EnglishTradition> , :Rank_Second_lieutenant_EnglishTradition ;
	org:rankJuniorTo_Transitive :Rank_Flying_officer_EnglishTradition ;
	org:rankOf :EnglishTradition , <mil:AirForceServiceBranch> ;
	org:rankSeniorTo_Transitive :Rank_Officer_cadet_EnglishTradition ;
	rdfs:label "Pilot officer"@en ;
	owl:sameAs <dbpedia:Pilot_officer> .

<http://rdf.muninn-project.org/ontologies/military#Rank_Private_(rank)_EnglishTradition> a :MilitaryRank ;
	org:rankEquivalentTo :Rank_Aircraftman_EnglishTradition , :Rank_Seaman_EnglishTradition ;
	org:rankJuniorTo_Transitive :Rank_Corporal_EnglishTradition ;
	org:rankOf :EnglishTradition , <mil:ArmyServiceBranch> ;
	owl:sameAs <dbpedia:Private_(rank)> .

:Rank_Seaman_EnglishTradition a :MilitaryRank ;
	org:rankEquivalentTo :Rank_Aircraftman_EnglishTradition , <http://rdf.muninn-project.org/ontologies/military#Rank_Private_(rank)_EnglishTradition> ;
	org:rankJuniorTo_Transitive :Rank_Leading_seaman_EnglishTradition ;
	org:rankOf :EnglishTradition , <mil:NavyServiceBranch> ;
	rdfs:comment "Seaman is one of the lowest ranks in a Navy. In the Commonwealth it is the lowest rank in the Navy, followed by Able Seaman and Leading Seaman, and followed by the Petty Officer ranks. In the United States, it means the lowest three enlisted rates of the U.S. Navy, followed by the higher Petty Officer ranks. The equivalent of the seaman, in French-speaking countries, is the Matelot."@en ;
	rdfs:label "Matelot"@fr , "Seaman"@en , "Seemann"@de ;
	owl:sameAs <dbpedia:Seaman> .

:Rank_Second_lieutenant_EnglishTradition a :MilitaryRank ;
	org:rankEquivalentTo <http://rdf.muninn-project.org/ontologies/military#Rank_Ensign_(rank)_EnglishTradition> , :Rank_Pilot_officer_EnglishTradition ;
	org:rankJuniorTo_Transitive :Rank_Lieutenant_EnglishTradition ;
	org:rankOf :EnglishTradition , <mil:ArmyServiceBranch> ;
	org:rankSeniorTo_Transitive :Rank_Officer_cadet_EnglishTradition ;
	rdfs:label "Second lieutenant"@en ;
	owl:sameAs <dbpedia:Second_lieutenant> .

:Rank_Sergeant_EnglishTradition a :MilitaryRank ;
	org:rankEquivalentTo :Rank_Petty_officer_EnglishTradition , :Rank_Sergeant_EnglishTradition ;
	org:rankJuniorTo_Transitive :Rank_Sergeant_major_EnglishTradition , :Rank_Warrant_officer_EnglishTradition ;
	org:rankOf :EnglishTradition , <mil:AirForceServiceBranch> , <mil:ArmyServiceBranch> ;
	org:rankSeniorTo_Transitive :Rank_Corporal_EnglishTradition ;
	rdfs:comment "Sergeant (normally abbreviated to Sgt) is a rank used in some form by most militaries, police forces, and other uniformed organizations around the world. Its origins are the Latin serviens, \"one who serves\", through the French term Sergent. In most armies the rank of sergeant corresponds to command of a squad. In Commonwealth armies it is a more senior rank, corresponding roughly to a platoon second-in-command."@en ;
	rdfs:label "Sergeant"@de , "Sergeant"@en , "Sergent"@fr ;
	owl:sameAs <dbpedia:Sergeant> .

:Rank_Sergeant_major_EnglishTradition a :MilitaryRank ;
	org:rankEquivalentTo :Rank_Warrant_officer_EnglishTradition ;
	org:rankJuniorTo_Transitive :Rank_Officer_cadet_EnglishTradition ;
	org:rankOf :EnglishTradition , <mil:ArmyServiceBranch> ;
	org:rankSeniorTo_Transitive :Rank_Sergeant_EnglishTradition ;
	rdfs:label "Sergeant major"@en ;
	owl:sameAs <dbpedia:Sergeant_major> .

:Rank_Squadron_leader_EnglishTradition a :MilitaryRank ;
	org:rankEquivalentTo <http://rdf.muninn-project.org/ontologies/military#Rank_Commandant_(rank)_EnglishTradition> , :Rank_Lieutenant_commander_EnglishTradition , :Rank_Major_EnglishTradition ;
	org:rankJuniorTo_Transitive <http://rdf.muninn-project.org/ontologies/military#Rank_Wing_commander_(rank)_EnglishTradition> ;
	org:rankOf :EnglishTradition , <mil:AirForceServiceBranch> ;
	org:rankSeniorTo_Transitive :Rank_Flight_lieutenant_EnglishTradition ;
	rdfs:label "Squadron leader"@en ;
	owl:sameAs <dbpedia:Squadron_leader> .

:Rank_Sub-lieutenant_EnglishTradition a :MilitaryRank ;
	org:rankEquivalentTo :Rank_Flying_officer_EnglishTradition , :Rank_Lieutenant_EnglishTradition ;
	org:rankJuniorTo_Transitive <http://rdf.muninn-project.org/ontologies/military#Rank_Lieutenant_(navy)_EnglishTradition> ;
	org:rankOf :EnglishTradition , <mil:NavyServiceBranch> ;
	org:rankSeniorTo_Transitive <http://rdf.muninn-project.org/ontologies/military#Rank_Ensign_(rank)_EnglishTradition> ;
	rdfs:label "Sub-lieutenant"@en ;
	owl:sameAs <dbpedia:Sub-lieutenant> .

:Rank_Warrant_officer_EnglishTradition a :MilitaryRank ;
	org:rankEquivalentTo :Rank_Sergeant_major_EnglishTradition , :Rank_Warrant_officer_EnglishTradition ;
	org:rankJuniorTo_Transitive :Rank_Midshipman_EnglishTradition , :Rank_Officer_cadet_EnglishTradition ;
	org:rankOf :EnglishTradition , <mil:AirForceServiceBranch> , <mil:NavyServiceBranch> ;
	org:rankSeniorTo_Transitive :Rank_Petty_officer_EnglishTradition , :Rank_Sergeant_EnglishTradition ;
	rdfs:label "Warrant officer"@en ;
	owl:sameAs <dbpedia:Warrant_officer> .

<http://rdf.muninn-project.org/ontologies/military#Rank_Wing_commander_(rank)_EnglishTradition> a :MilitaryRank ;
	org:rankEquivalentTo :Rank_Commander_EnglishTradition , :Rank_Lieutenant_colonel_EnglishTradition ;
	org:rankJuniorTo_Transitive :Rank_Group_captain_EnglishTradition ;
	org:rankOf :EnglishTradition , <mil:AirForceServiceBranch> ;
	org:rankSeniorTo_Transitive :Rank_Squadron_leader_EnglishTradition ;
	owl:sameAs <dbpedia:Wing_commander_(rank)> .

<http://rdf.muninn-project.org/ontologies/military#Rank_Able_seaman_%28rank%29> a :MilitaryRank ;
	foaf:name "Able Seaman" ;
	rdfs:label "Able Seaman"@en ;
	owl:sameAs <dbpedia:Able_seaman_%28rank%29> .

<dbpedia:Able_seaman_%28rank%29> muninn:wikipedia_version "485001067" .

<http://rdf.muninn-project.org/ontologies/military#Rank_Admiral_of_the_Fleet_%28Russia%29> a :MilitaryRank ;
	rdfs:comment "Admiral of the Fleet or Fleet Admiral (Адмирал флoта, Admiral flota) is the highest naval (deck) rank of the Russian Federation. It is the equivalent of the Soviet naval rank of Admiral of the Fleet and the present Russian rank of General of the Army. The rank is roughly equivalent to 4-stars Admiral ranks of other nations. There is only one rank higher than that of Admiral of the Fleet in the Russian armed forces, namely Marshal of the Russian Federation."@en ;
	foaf:name "Admiral of the Fleet" ;
	rdfs:label "Admiral of the Fleet (Russia)"@en , "Ammiraglio della flotta (Russia)"@it ;
	owl:sameAs <dbpedia:Admiral_of_the_Fleet_%28Russia%29> .

<dbpedia:Admiral_of_the_Fleet_%28Russia%29> muninn:wikipedia_version "474375587" .

:Rank_Anthypolochagos a :MilitaryRank ;
	rdfs:comment "Anthypolochagos is used in the Greek language to mean \"Second Lieutenant\". In the modern Hellenic Army the rank is the lowest commissioned officer rank and is inferior to an Ypolochagos. The insignia consists of a single silver star (or a star and a bar for reserve officers). Officers holding this rank should be addressed as \"Kyrie Anthypolochage\" (Κύριε Ανθυπολοχαγέ) by their subordinates, or \"Anthypolochage + family name\" by their superior officers."@en ;
	foaf:name "Anthypolochagos" ;
	rdfs:label "Anthypolochagos"@en ;
	owl:sameAs <dbpedia:Anthypolochagos> .

<dbpedia:Anthypolochagos> muninn:wikipedia_version "485272666" .

:Rank_Antisyntagmatarchis a :MilitaryRank ;
	rdfs:comment "Antisyntagmatarchis is used in the Greek language to mean \"Lieutenant Colonel\". The typical responsibility of an Antisyntagmatarchis is to exercise command of a battalion. Officers holding this rank should be addressed as \"Kyrie Diikita\" (Κύριε διοικητά) (stressed on the last syllable), by their subordinates when they exercise battalion command or \"Kyrie Antisyntagmatarcha\" (Κύριε Αντισυνταγματάρχα) (stressed on the syllable before last) in other cases."@en ;
	foaf:name "Antisyntagmatarchis" ;
	rdfs:label "Antisyntagmatarchis"@en ;
	owl:sameAs <dbpedia:Antisyntagmatarchis> .

<dbpedia:Antisyntagmatarchis> muninn:wikipedia_version "485253360" .

<http://rdf.muninn-project.org/ontologies/military#Rank_Army_General_%28Russia%29> a :MilitaryRank ;
	rdfs:comment "Please see \"Army General\" for other nations which use this rank Army General is the second highest military rank in the Russian Federation, inferior only to a Marshal and superior to a Colonel General. It is a direct counterpart of the Soviet rank, General of the Army (USSR)."@en ;
	foaf:name "Army General" ;
	rdfs:label "Army General (Russia)"@en , "Генерал армии (Россия)"@ru ;
	owl:sameAs <dbpedia:Army_General_%28Russia%29> .

<dbpedia:Army_General_%28Russia%29> muninn:wikipedia_version "474376394" .

:Rank_Aspirant a :MilitaryRank ;
	rdfs:comment "Aspirant is a military rank in the Canadian Navy, French military, Brazilian military, Romanian Navy and Polish Police."@en ;
	foaf:name "Aspirant" ;
	rdfs:label "Aspirant"@en ;
	owl:sameAs <dbpedia:Aspirant> .

<dbpedia:Aspirant> muninn:wikipedia_version "479973767" .

:Rank_Brigade_General a :MilitaryRank ;
	foaf:name "Brigade General" ;
	rdfs:label "Brigade General"@en ;
	owl:sameAs <dbpedia:Brigade_General> .

<dbpedia:Brigade_General> muninn:wikipedia_version "488560485" .

:Rank_Brigadier_general a :MilitaryRank ;
	foaf:name "Brigadier general" ;
	rdfs:label "Brigadier general"@en ;
	owl:sameAs <dbpedia:Brigadier_general> .

<dbpedia:Brigadier_general> muninn:wikipedia_version "498197413" .

<http://rdf.muninn-project.org/ontologies/military#Rank_Buffer_%28navy%29> a :MilitaryRank ;
	rdfs:comment "Buffer is the colloquial title for the senior seaman sailor in a Commonwealth of Nations Navy ship. The formal title is Chief Boatswain's Mate. This person is typically a Chief Petty Officer in frigates or destroyers, and in larger ships may be a Warrant Officer. In smaller ships, such as a patrol boat, the Buffer may be a Petty Officer."@en ;
	foaf:name "Buffer" ;
	rdfs:label "Buffer (navy)"@en ;
	owl:sameAs <dbpedia:Buffer_%28navy%29> .

<dbpedia:Buffer_%28navy%29> muninn:wikipedia_version "332327992" .

<http://rdf.muninn-project.org/ontologies/military#Rank_Captain_%28naval%29> a :MilitaryRank ;
	rdfs:comment "Captain is the name most often given in English-speaking navies to the rank corresponding to command of the largest ships. The NATO rank code is OF-5, equivalent to an army full colonel. The equivalent rank in some navies translates as \"ship captain\" (e.g. French - capitaine de vaisseau), \"captain of sea and war\" (Portuguese capitão de mar e guerra), \"captain at sea\" (e.g. German Kapitän zur See) or \"captain of the first rank\" (Russian - капитан 1-го ранга)."@en ;
	foaf:name "Captain" ;
	rdfs:label "Captain (naval)"@en , "Kommendör"@sv , "Kommodori"@fi , "Capitaine de vaisseau"@fr , "Kapitän zur See"@de , "Capitano di vascello"@it , "Kapitein-ter-zee"@nl , "Kommandør"@no , "Komandor"@pl , "Capitão de mar e guerra"@pt , "Капитан 1-го ранга"@ru , "Capitán de navío"@es ;
	owl:sameAs <dbpedia:Captain_%28naval%29> .

<dbpedia:Captain_%28naval%29> muninn:wikipedia_version "494810123" .

:Rank_Chief_Marshal a :MilitaryRank ;
	rdfs:comment "The ranks of Marshal of a branch and Chief Marshal of a branch were senior military ranks of the Soviet Armed Forces. Immediately above the rank \"Marshal of a branch\" is the rank \"Chief Marshal of a branch\". Both ranks are immediately above the rank \"Colonel General\" and equal to Soviet General of the Army. The ranks were created as an analog to Air Marshal and Air Chief Marshal, though they weren't used just in the Soviet Air Force but also in the several Soviet Army's branch commands."@en ;
	foaf:name "Chief Marshal" ;
	rdfs:label "Chief Marshal"@en , "Главный маршал рода войск"@ru ;
	owl:sameAs <dbpedia:Chief_Marshal> .

<dbpedia:Chief_Marshal> muninn:wikipedia_version "489506259" .

:Rank_Comandarm a :MilitaryRank ;
	rdfs:comment "Comandarm (also Komandarm, Commandarm, Russian \"командарм\" - abbreviated \"командующий армией\", Commander of the Army) was a military rank in the Red Army until the end of the 1930s. Comandarm 2nd rank, with the insignia of four rombs, is graded at 4 ranks above colonel. Comandarm 1st rank, with the insignia of four rombs and a star, is at 5 ranks above colonel."@en ;
	foaf:name "Comandarm" ;
	rdfs:label "Comandarm"@en , "Sowjetische Generalsränge"@de , "Komandarm"@de , "Komandarm av 1. klasse"@no , "Komandarm av 2. klasse"@no , "Komandarm"@pl ;
	owl:sameAs <dbpedia:Comandarm> .

<dbpedia:Comandarm> muninn:wikipedia_version "484165039" .

<http://rdf.muninn-project.org/ontologies/military#Rank_Combat_%28military_rank%29> a :MilitaryRank ;
	rdfs:comment "Combat or Kombat, abbreviated from Командир батальона (\"Commander of a battalion\") was a military rank in the Red Army until the end of the 1930s. At that time it was roughly equivalent to the rank of Captain."@en ;
	foaf:name "Combat" ;
	rdfs:label "Combat (military rank)"@en ;
	owl:sameAs <dbpedia:Combat_%28military_rank%29> .

<dbpedia:Combat_%28military_rank%29> muninn:wikipedia_version "449517873" .

:Rank_Combrig a :MilitaryRank ;
	rdfs:comment "Combrig was a military rank used in the Red Army for commanders of brigades between 1935 and 1940 (with some individuals still holding the rank in 1941). Kombrigs were senior to polkovniks (colonels) and junior to comdivs (commander of the division). When general ranks were reintroduced in July 1940 most kombrigs were transferred to the junior rank of polkovnik, while some received the rank of major general."@en ;
	foaf:name "Combrig" ;
	rdfs:label "Combrig"@en , "Prikaatinkomentaja"@fi , "Kombrig"@de , "Kombrig"@it , "Kombrig"@pl , "Комбриг"@ru , "Kombrig"@es ;
	owl:sameAs <dbpedia:Combrig> .

<dbpedia:Combrig> muninn:wikipedia_version "444403891" .

:Rank_Comcor a :MilitaryRank ;
	rdfs:comment "Comcor (or Comkor, Komkor, abbreviated from Commander of the Corps) was a military rank in the Red Army until the end of the 1930"@en ;
	foaf:name "Comcor" ;
	rdfs:label "Comcor"@en , "Armeijakunnankomentaja"@fi , "Komkor"@de , "Komkor"@no , "Komkor"@pl , "Комкор"@ru , "Komkor"@es ;
	owl:sameAs <dbpedia:Comcor> .

<dbpedia:Comcor> muninn:wikipedia_version "414282347" .

:Rank_Comdiv a :MilitaryRank ;
	rdfs:comment "Comdiv or Komdiv, abbreviated from (\"Commander of the division\") was a military rank in the Red Army until the end of the 1930s."@en ;
	foaf:name "Comdiv" ;
	rdfs:label "Comdiv"@en , "Divisioonankomentaja"@fi , "Komdiv"@de , "Komdiv"@no , "Komdiw"@pl , "Комдив"@ru , "Komdiv"@es ;
	owl:sameAs <dbpedia:Comdiv> .

<dbpedia:Comdiv> muninn:wikipedia_version "466619272" .

<http://rdf.muninn-project.org/ontologies/military#Rank_Commandant_%28rank%29> a :MilitaryRank ;
	rdfs:comment "Commandant is a military or police rank. In the French, Spanish and Irish armed forces it is a rank equivalent to major. In South Africa for most of the second half of the 20th century, commandant was a rank equivalent to lieutenant-colonel in other countries."@en ;
	foaf:name "Commandant" ;
	rdfs:label "Commandant (rank)"@en ;
	owl:sameAs <dbpedia:Commandant_%28rank%29> .

<dbpedia:Commandant_%28rank%29> muninn:wikipedia_version "469176328" .

:Rank_Commandeur a :MilitaryRank ;
	rdfs:comment "Commandeur is a title in French and Dutch (also, now a purism, Kommandeur), usually rendered in English as Commander, with different uses. The literal meaning is he who commands, parallel to Commandant. In most senses the German equivalent is Kommandeur."@en ;
	foaf:name "Commandeur" ;
	rdfs:label "Commandeur"@en , "Commandeur"@fr , "Commandeur (marine)"@nl ;
	owl:sameAs <dbpedia:Commandeur> .

<dbpedia:Commandeur> muninn:wikipedia_version "444183372" .

:Rank_Daejang a :MilitaryRank ;
	rdfs:comment "Daejang is a senior military rank of the Korean Peninsula, used by both North and South Korea. It is considered the combined equivalent of a General and Admiral in other nations. The rank of Daejang is sometimes spelled as Taejang, depending on the transliteration system used (Taejang in McCune-Reischauer, Daejang in official ROK transliteration system)."@en ;
	foaf:name "Daejang" ;
	rdfs:label "Daejang"@en ;
	owl:sameAs <dbpedia:Daejang> .

<dbpedia:Daejang> muninn:wikipedia_version "469177179" .

:Rank_Divisional_Admiral a :MilitaryRank ;
	rdfs:comment "Divisional Admiral or Division Admiral is a commissioned officer rank in several navies. It is a two-star flag rank, equivalent to the rank of Rear Admiral in the Royal Navy and the rank of Rear Admiral (Upper Half) in the United States Navy."@en ;
	foaf:name "Divisional Admiral" ;
	rdfs:label "Divisional Admiral"@en , "Amiral de division"@fr , "Ammiraglio di divisione"@it , "Divisieadmiraal"@nl ;
	owl:sameAs <dbpedia:Divisional_Admiral> .

<dbpedia:Divisional_Admiral> muninn:wikipedia_version "469675599" .

:Rank_Divisional_General a :MilitaryRank ;
	rdfs:comment "Divisional General is a rank used in many armies to denote a rank of general, corresponding to command of a division. For convenience Divisional General is almost always translated into English as Major-General, the equivalent rank used by the UK, USA, etc. , although this translation is, strictly speaking, incorrect. The rank is particularly common in western Europe and Latin America."@en ;
	foaf:name "Divisional General" ;
	rdfs:label "Divisional General"@en , "Divisioonakenraali"@fi , "Général de division"@fr , "Generale di divisione"@it , "General de divisão"@pt ;
	owl:sameAs <dbpedia:Divisional_General> .

<dbpedia:Divisional_General> muninn:wikipedia_version "492101670" .

<http://rdf.muninn-project.org/ontologies/military#Rank_Driver_%28rank%29> a :MilitaryRank ;
	rdfs:comment "Driver (Dvr) was a military rank used in the British Army and the armies of other Commonwealth countries. It was equivalent to the rank of Private. The rank was initially used in the Royal Artillery for the men who drove the teams of horses which pulled the guns. It was phased out after the First World War (when all Royal Artillerymen of the lowest rank were redesignated as Gunners). It was also used in the Royal Australian Artillery and Royal Canadian Artillery."@en ;
	foaf:name "Driver" ;
	rdfs:label "Driver (rank)"@en ;
	owl:sameAs <dbpedia:Driver_%28rank%29> .

<dbpedia:Driver_%28rank%29> muninn:wikipedia_version "366534265" .

:Rank_Epihipparch a :MilitaryRank ;
	rdfs:comment "Epihipparch is an Ancient Greek military title for a cavalry commander of 1,000 horse. This unit was divided into two hipparchiai of 500. Each of these was commanded by a hipparchos."@en ;
	foaf:name "Epihipparch" ;
	rdfs:label "Epihipparch"@en ;
	owl:sameAs <dbpedia:Epihipparch> .

<dbpedia:Epihipparch> muninn:wikipedia_version "444383081" .

:Rank_General-in-Chief a :MilitaryRank ;
	rdfs:comment "General-in-Chief has been a military rank or title in various armed forces around the world."@en ;
	foaf:name "General-in-Chief" ;
	rdfs:label "General-in-Chief"@en , "General en chef"@sv , "Генерал-аншеф"@ru ;
	owl:sameAs <dbpedia:General-in-Chief> .

<dbpedia:General-in-Chief> muninn:wikipedia_version "469172883" .

<http://rdf.muninn-project.org/ontologies/military#Rank_Hasa_%28Korean_military%29> a :MilitaryRank ;
	rdfs:comment "Hasa is a Korean military rank which is used in both the armed forces of North and South Korea. In both countries, the rank is considered the first non-commissioned officer grade and is generally considered the equivalent of a Corporal or Sergeant in western militaries."@en ;
	foaf:name "Hasa" ;
	rdfs:label "Hasa (Korean military)"@en ;
	owl:sameAs <dbpedia:Hasa_%28Korean_military%29> .

<dbpedia:Hasa_%28Korean_military%29> muninn:wikipedia_version "391617597" .

<http://rdf.muninn-project.org/ontologies/military#Rank_Hipparchus_%28cavalry_officer%29> a :MilitaryRank ;
	rdfs:comment "A Hipparchus or Hipparch was the title of an ancient Greek cavalry officer, commanding a hipparchia (unit of about 500 horsemen); two such units were commanded by an Epihipparchos."@en ;
	foaf:name "Hipparchus" ;
	rdfs:label "Hipparchus (cavalry officer)"@en , "Hipparchos"@nl , "Гиппарх (военачальник)"@ru , "Hiparco (oficial de caballería)"@es ;
	owl:sameAs <dbpedia:Hipparchus_%28cavalry_officer%29> .

<dbpedia:Hipparchus_%28cavalry_officer%29> muninn:wikipedia_version "472932397" .

:Rank_Jungsa a :MilitaryRank ;
	rdfs:comment "Jungsa is a Korean military rank used by the armed forces of South and North Koreas. A Jungsa is the equivalent to a Sergeant First Class. The rank of Jungsa is junior to a Sangsa in North and South Korea."@en ;
	foaf:name "Jungsa" ;
	rdfs:label "Jungsa"@en ;
	owl:sameAs <dbpedia:Jungsa> .

<dbpedia:Jungsa> muninn:wikipedia_version "294619203" .

:Rank_Jungwi a :MilitaryRank ;
	rdfs:comment "Chungwi (중위) is the second most junior Korean officer rank in both the militaries of North and South Korea. It is considered the equivalent of a First Lieutenant in most other militaries."@en ;
	foaf:name "Jungwi" ;
	rdfs:label "Jungwi"@en , "Jungwi"@no ;
	owl:sameAs <dbpedia:Jungwi> .

<dbpedia:Jungwi> muninn:wikipedia_version "342301621" .

:Rank_Junior_sergeant a :MilitaryRank ;
	foaf:name "Junior Sergeant" ;
	rdfs:label "Junior Sergeant"@en ;
	owl:sameAs <dbpedia:Junior_sergeant> .

<dbpedia:Junior_sergeant> muninn:wikipedia_version "481658126" .

:Rank_Junjang a :MilitaryRank ;
	foaf:name "Junjang" ;
	rdfs:label "Junjang"@en ;
	owl:sameAs <dbpedia:Junjang> .

<dbpedia:Junjang> muninn:wikipedia_version "450552760" .

:Rank_Kindral a :MilitaryRank ;
	rdfs:comment "Kindral is the Estonian word for General which is also the highest military position in the Republic of Estonia. Both Ground Force and Air Force superior officers ranks share the same names which have been combined with the military rank of general and other senior officer ranks. There are four types of generals in the Estonia Defence Forces."@en ;
	foaf:name "Kindral" ;
	rdfs:label "Kindral"@en ;
	owl:sameAs <dbpedia:Kindral> .

<dbpedia:Kindral> muninn:wikipedia_version "350970761" .

:Rank_Major_general a :MilitaryRank ;
	foaf:name "Major general" ;
	rdfs:label "Major general"@en ;
	owl:sameAs <dbpedia:Major_general> .

<dbpedia:Major_general> muninn:wikipedia_version "498199972" .

:Rank_Marshal_of_the_Soviet_Union a :MilitaryRank ;
	rdfs:comment "Marshal of the Soviet Union was the de facto highest military rank of the Soviet Union. (The highest rank de jure, Generalissimus of the Soviet Union, was created for Joseph Stalin and held by him alone). The rank of Marshal of the Soviet Union was created in 1935 and abolished in 1991. Forty-one people held the rank of Marshal of the Soviet Union. The equivalent naval rank was Admiral of the Fleet of the Soviet Union."@en ;
	foaf:name "Marshal of the Soviet Union" ;
	rdfs:label "Marshal of the Soviet Union"@en , "Marskalk av Sovjetunionen"@sv , "Neuvostoliiton marsalkka"@fi , "Maréchal de l'Union soviétique"@fr , "Marschall der Sowjetunion"@de , "Maresciallo dell'Unione Sovietica"@it , "Maarschalk van de Sovjet-Unie"@nl , "Marskalk av Sovjetunionen"@no , "Marszałkowie ZSRR"@pl , "Marechal da União Soviética"@pt , "Маршал Советского Союза"@ru , "Mariscal de la Unión Soviética"@es ;
	owl:sameAs <dbpedia:Marshal_of_the_Soviet_Union> .

<dbpedia:Marshal_of_the_Soviet_Union> muninn:wikipedia_version "497557208" .

:Rank_Master_warrant_officer a :MilitaryRank ;
	foaf:name "Master Warrant Officer" ;
	rdfs:label "Master Warrant Officer"@en ;
	owl:sameAs <dbpedia:Master_warrant_officer> .

<dbpedia:Master_warrant_officer> muninn:wikipedia_version "452828931" .

:Rank_Obergefreiter a :MilitaryRank ;
	rdfs:comment """Obergefreiter is a rank of the German and Swiss militaries which dates from the 19th century. 	 		 			021-Obergefreiter. png 			 German Army rank insignia (shoulder tab) 			 		 		 			3 - ogefr. GIF 			 German Navy rank insignia (sleeve) 			 		 	 The rank was only used in the German army's heavy artillery branch (Fußartillerie) before 1919 and commonly established with the founding of the Reichswehr."""@en ;
	foaf:name "Obergefreiter" ;
	rdfs:label "Obergefreiter"@en , "Ylikorpraali"@fi , "Obergefreiter"@de ;
	owl:sameAs <dbpedia:Obergefreiter> .

<dbpedia:Obergefreiter> muninn:wikipedia_version "482305142" .

:Rank_Podpraporshchik a :MilitaryRank ;
	rdfs:comment "Podpraporshchik (Sub-Praporshchik) was one of the non-commissioned ranks, originally below the Sergeant and Feldwebel but since 1826 it became the highest non-commissioned rank of the infantry, cavalry and Leib Guard. In 1884, the podpraporshchik rank was renamed Zauryad-praporshchik (Ordinary Praporshchik)."@en ;
	foaf:name "Podpraporshchik" ;
	rdfs:label "Podpraporshchik"@en , "Подпрапорщик"@ru ;
	owl:sameAs <dbpedia:Podpraporshchik> .

<dbpedia:Podpraporshchik> muninn:wikipedia_version "481610330" .

:Rank_Polemarch a :MilitaryRank ;
	rdfs:comment "A polemarch was a senior military title in various ancient Greek city states (poleis). The title is composed out of the polemos (war) and archon (ruler/leader) and translates as \"warleader\" or \"warlord\", one of the nine archontes (ἄρχοντες) appointed annually in Athens. The name indicates that the polemarchos original function was to command the army; presumably the office was created to take over this function from the king."@en ;
	foaf:name "Polemarch" ;
	rdfs:label "Polemarch"@en , "Polemark"@sv , "Polémarque"@fr , "Polemarchos"@nl , "Polemarkos"@no , "Polemarco"@pt , "Полемарх"@ru , "Polemarca"@es ;
	owl:sameAs <dbpedia:Polemarch> .

<dbpedia:Polemarch> muninn:wikipedia_version "480243861" .

:Rank_Praporshchik a :MilitaryRank ;
	rdfs:comment "Praporshchik is a rank in the Russian military."@en ;
	foaf:name "Praporshchik" ;
	rdfs:label "Praporshchik"@en , "Прапорщик"@ru ;
	owl:sameAs <dbpedia:Praporshchik> .

<dbpedia:Praporshchik> muninn:wikipedia_version "491581201" .

:Rank_Rear_admiral a :MilitaryRank ;
	rdfs:comment "Rear admiral is a naval commissioned officer rank above that of a commodore and captain, and below that of a vice admiral. It is generally regarded as the lowest of the \"admiral\" ranks, which are also sometimes referred to as \"flag officers\" or \"flag ranks\". In many navies it is referred to as a two-star rank. It originated from the days of naval sailing squadrons and can trace its origins to the Royal Navy."@en ;
	foaf:name "Rear admiral" ;
	rdfs:label "Rear admiral"@en ;
	owl:sameAs <dbpedia:Rear_admiral> .

<dbpedia:Rear_admiral> muninn:wikipedia_version "494693473" .

:Rank_Sangsa a :MilitaryRank ;
	rdfs:comment "Sangsa is a Korean military rank used by both the armed forces of North and South Korea. A Sangsa is the equivalent to a First Sergeant in most other militaries. The rank of Sangsa is junior to a Wonsa in South Korea and to a Warrant Officer like rank in the North known as Teukmu Sangsa."@en ;
	foaf:name "Sangsa" ;
	rdfs:label "Sangsa"@en ;
	owl:sameAs <dbpedia:Sangsa> .

<dbpedia:Sangsa> muninn:wikipedia_version "294619474" .

:Rank_Skeuophoros a :MilitaryRank ;
	rdfs:comment "A skeuophoros was a slave or servant who carried baggage in Ancient Greece. Herodotus records that every hoplite was followed on campaign by a servant as a skeuophoros. In Aristophanes' play The Frogs, Xanthias, the slave of Dionysus, acts as his skeuophoros: Διόνυσος ἴθι νυν ἐπειδὴ ληματίας κἀνδρεῖος εἶ,σὺ μὲν γενοῦ 'γὼ τὸ ῥόπαλον τουτὶ λαβὼνκαὶ τὴν λεοντῆν, εἴπερ ἀφοβόσπλαγχνος εἶ:ἐγὼ δ᾽ ἔσομαί σοι σκευοφόρος ἐν τῷ μέρει."@en ;
	foaf:name "Skeuophoros" ;
	rdfs:label "Skeuophoros"@en ;
	owl:sameAs <dbpedia:Skeuophoros> .

<dbpedia:Skeuophoros> muninn:wikipedia_version "488522679" .

:Rank_Somatophylakes a :MilitaryRank ;
	rdfs:comment "Somatophylakes, in its literal English translation from Greek, means \"bodyguards\". The most famous body of somatophylakes were those of Philip of Macedon and Alexander the Great. They consisted of seven men, drawn from the Macedonian nobility, who also acted as high-ranking military officers, holding command positions such as general or chiliarch. Alexander the Great appointed Peucestas as eighth somatophylax after the siege of Malli."@en ;
	foaf:name "Somatophylakes" ;
	rdfs:label "Somatophylakes"@en , "Somatofylakes"@fi , "Sômatophylaques"@fr , "Somatophylakes"@de , "Somatofilachie"@it , "Somatophylax"@nl , "Somatophylakes"@es ;
	owl:sameAs <dbpedia:Somatophylakes> .

<dbpedia:Somatophylakes> muninn:wikipedia_version "493685412" .

:Rank_Sowi a :MilitaryRank ;
	rdfs:comment "Sowi (소위) is the junior most Korean officer rank in both the militaries of North and South Korea. It is considered the equivalent of a Second Lieutenant in most other militaries."@en ;
	foaf:name "Sowi" ;
	rdfs:label "Sowi"@en ;
	owl:sameAs <dbpedia:Sowi> .

<dbpedia:Sowi> muninn:wikipedia_version "354997832" .

:Rank_Staabikapten a :MilitaryRank ;
	rdfs:comment "A Staff-Captain (staabikapten in Estonian language), was an Estonian military rank in the Naval forces of Estonia, which existed between 1918 in 1922."@en ;
	foaf:name "Staabikapten" ;
	rdfs:label "Staabikapten"@en ;
	owl:sameAs <dbpedia:Staabikapten> .

<dbpedia:Staabikapten> muninn:wikipedia_version "440079788" .

:Rank_Tetrarch a :MilitaryRank ;
	foaf:name "Tetrarch" ;
	rdfs:label "Tetrarch"@en , "Tetrark"@sv , "Tetrarkki"@fi , "Tetrarch"@de , "Tetrarch"@nl , "Tetrarca"@pt , "Тетрарх (значения)"@ru ;
	owl:sameAs <dbpedia:Tetrarch> .

<dbpedia:Tetrarch> muninn:wikipedia_version "465320704" .

:Rank_Trierarch a :MilitaryRank ;
	rdfs:comment "Trierarch was the title of officers who commanded a trireme (triēres) in the classical Greek world. In Athens and a few other states this officer was also required to pay for the outfitting and maintenance of the ship. Trierarchs thus had to be men of considerable means, since the expenses incurred could run as high as a talent in the course of a year."@en ;
	foaf:name "Trierarch" ;
	rdfs:label "Trierarch"@en , "Triérarchie"@fr , "Trierarchie"@de , "Trierarchia"@it , "Trierark"@no , "Триерархия"@ru , "Trierarca"@es ;
	owl:sameAs <dbpedia:Trierarch> .

<dbpedia:Trierarch> muninn:wikipedia_version "492902890" .

:Rank_Tysyatsky a :MilitaryRank ;
	rdfs:comment "Tysyatsky was a military leader in Ancient Rus, who commanded a people's volunteer army called тысяча (tysyacha, or a thousand). In the Novgorod Republic, the tysyatsky evolved into a judicial or commercial official and was elected from boyars at a veche for a period of one year posadnik."@en ;
	foaf:name "Tysyatsky" ;
	rdfs:label "Tysyatsky"@en , "Tysjackij"@it , "Tysjatski"@nl , "Тысяцкий"@ru ;
	owl:sameAs <dbpedia:Tysyatsky> .

<dbpedia:Tysyatsky> muninn:wikipedia_version "484427552" .

<http://rdf.muninn-project.org/ontologies/military#Rank_V%C3%A4%C3%A4peli> a :MilitaryRank ;
	foaf:name "Vääpeli" ;
	rdfs:label "Vääpeli"@en ;
	owl:sameAs <dbpedia:V%C3%A4%C3%A4peli> .

<dbpedia:V%C3%A4%C3%A4peli> muninn:wikipedia_version "476502911" .

:Rank_Veebel a :MilitaryRank ;
	rdfs:comment "Veebel is an Estonian military rank which has existed since the 20th century. The word veebel is usually, but incorrectly, translated in English as Sergeant. The correct equivalent is Warrant Officer."@en ;
	foaf:name "Veebel" ;
	rdfs:label "Veebel"@en ;
	owl:sameAs <dbpedia:Veebel> .

<dbpedia:Veebel> muninn:wikipedia_version "404975154" .

:Rank_Vice_admiral a :MilitaryRank ;
	foaf:name "Vice admiral" ;
	rdfs:label "Vice admiral"@en ;
	owl:sameAs <dbpedia:Vice_admiral> .

<dbpedia:Vice_admiral> muninn:wikipedia_version "495831034" .

:Rank_Wojski a :MilitaryRank ;
	rdfs:comment "The Wojski was an officer in medieval Poland, responsible for the security of voivodships or districts at times when voivods and castellans had accompanied the szlachta (nobility) to war. With time, the wojski's responsibilities were take over by starostas, and \"wojski\" became an honorary district office in the Polish-Lithuanian Commonwealth."@en ;
	foaf:name "Wojski" ;
	rdfs:label "Wojski"@en , "Wojski"@pl , "Войский"@ru ;
	owl:sameAs <dbpedia:Wojski> .

<dbpedia:Wojski> muninn:wikipedia_version "454605449" .

:Rank_Wonsu a :MilitaryRank ;
	rdfs:comment "Wonsu is a very high military rank of the armed forces of the Republic of Korea and of North Korea."@en ;
	foaf:name "Wonsu" ;
	rdfs:label "Wonsu"@en , "Вонсу"@ru ;
	owl:sameAs <dbpedia:Wonsu> .

<dbpedia:Wonsu> muninn:wikipedia_version "492136047" .

:Rank_Ypolochagos a :MilitaryRank ;
	rdfs:comment "Ypolochagos is used in the modern Greek language to mean \"First Lieutenant\". In the modern Hellenic Army the rank is superior to that of Anthypolochagos and inferior to that of an Lochagos. The insignia consists of two silver stars. Officers holding this rank should be addressed as \"Kyrie Ypolochage\" (Κύριε Υπολοχαγέ) by their subordinates, or \"Ypolochage + family name\" by their superior officers."@en ;
	foaf:name "Ypolochagos" ;
	rdfs:label "Ypolochagos"@en ;
	owl:sameAs <dbpedia:Ypolochagos> .

<dbpedia:Ypolochagos> muninn:wikipedia_version "496047552" .

<http://rdf.muninn-project.org/ontologies/military#Rank_Agha_%28Ottoman_Empire%29> a :MilitaryRank ;
	rdfs:comment "For other uses of the term 'Aga', see Aga. For other uses of the term 'Agha', see Agha. Agha, also Aga, as a title for a civil or military officer, or often part of such title, was placed after the name of certain military functionaries in the Ottoman Empire. At the same time some court functionaries were entitled to the agha title."@en ;
	foaf:name "Agha" ;
	rdfs:label "Agha (Ottoman Empire)"@en , "Agha"@sv , "Agha"@fi , "Agha"@fr , "Agha (Titel)"@de , "Agha"@it , "Agha"@no , "Aga (wojsko)"@pl , "Ага (титул военачальников)"@ru ;
	owl:sameAs <dbpedia:Agha_%28Ottoman_Empire%29> .

<dbpedia:Agha_%28Ottoman_Empire%29> muninn:wikipedia_version "496783931" .

:Rank_Air_chief_marshal a :MilitaryRank ;
	foaf:name "Air chief marshal" ;
	rdfs:label "Air chief marshal"@en ;
	owl:sameAs <dbpedia:Air_chief_marshal> .

<dbpedia:Air_chief_marshal> muninn:wikipedia_version "495804436" .

:Rank_Air_vice-marshal a :MilitaryRank ;
	foaf:name "Air vice-marshal" ;
	rdfs:label "Air vice-marshal"@en ;
	owl:sameAs <dbpedia:Air_vice-marshal> .

<dbpedia:Air_vice-marshal> muninn:wikipedia_version "495806110" .

:Rank_Ataman a :MilitaryRank ;
	rdfs:comment "Ataman was a commander title of the Ukrainian People's Army, Cossack, and haidamak leaders, who were in essence the Cossacks. In the Russia Empire, the term was the official title of the supreme military commanders of the Cossack armies. It had a derogatory suggestion and was also used for the leader of a fisherman artel, a band of robbers or thieves, or leaders of the opposition forces."@en ;
	foaf:name "Ataman" ;
	rdfs:label "Ataman"@en , "Atamaani"@fi , "Ataman / Otaman"@fr , "Ataman"@de , "Atamano"@it , "Ataman"@pl , "Атаман"@ru , "Atamán"@es ;
	owl:sameAs <dbpedia:Ataman> .

<dbpedia:Ataman> muninn:wikipedia_version "470073774" .

:Rank_Birinci_Ferik a :MilitaryRank ;
	rdfs:comment "Birinci Ferik or Ferik-i evvel was a military rank of the Ottoman Army. It is translated as Lieutenant General or General (Orgeneral). The title means \"first Ferik\" and was superior to a Ferik and junior only to the Müşir. The title of Birinci Ferik was abolished with Act No. 2590 of 26 November 1934 on the Abolition of Titles and Appellations such as Efendi, Bey or Pasha."@en ;
	foaf:name "Birinci Ferik" ;
	rdfs:label "Birinci Ferik"@en ;
	owl:sameAs <dbpedia:Birinci_Ferik> .

<dbpedia:Birinci_Ferik> muninn:wikipedia_version "478074487" .

<http://rdf.muninn-project.org/ontologies/military#Rank_Bombardier_%28rank%29> a :MilitaryRank ;
	rdfs:comment "Bombardier is a rank used in artillery units in the armies of Commonwealth countries instead of corporal. Lance-bombardier is used instead of lance-corporal. Bombardier (Bdr) and lance-bombardier (LBdr or L/Bdr) are used by the British Army in the Royal Artillery and Royal Horse Artillery. The same applies to the Royal Australian Artillery, the Royal New Zealand Artillery, the South African Army Artillery and the Armed Forces of Malta (AFM)."@en ;
	foaf:name "Bombardier" ;
	rdfs:label "Bombardier (rank)"@en , "Bombardier (stopień)"@pl , "Бомбардир (воинское звание)"@ru ;
	owl:sameAs <dbpedia:Bombardier_%28rank%29> .

<dbpedia:Bombardier_%28rank%29> muninn:wikipedia_version "492510161" .

:Rank_Bootsmann a :MilitaryRank ;
	rdfs:comment "Bootsmann was a highest-ranking Petty Officer position in German naval forces. A lower-ranking Bootsmann was called Bootsmannsmaat. These names were adopted for the Russian Navy as боцман and боцманмат by Peter the Great, among many other Prussian and Holland military ranks; they were initially treated as positions rather than ranks. The army and air force equivalent is a Feldwebel. In the modern German Navy, Bootsmann is a senior NCO rank."@en ;
	foaf:name "Bootsmann" ;
	rdfs:label "Bootsmann"@en , "Bootsmann"@de , "Боцман"@ru ;
	owl:sameAs <dbpedia:Bootsmann> .

<dbpedia:Bootsmann> muninn:wikipedia_version "339832695" .

<http://rdf.muninn-project.org/ontologies/military#Rank_%C3%87orbac%C4%B1> a :MilitaryRank ;
	rdfs:comment "Çorbacı (sometimes variously transliterated as chorbaji, chorbadzhi, tschorbadji) was a military rank of the corps of Janissaries in the Ottoman Empire, used for the commander of an orta, i.e. , approximately corresponding to the rank of colonel. The word is pronounced tʃoɾbaˈdʒɯ in Turkish and literally means \"soup server\", derived from çorba, \"soup\". However, this word could be connected to an old Turkic word korbashi (head of the unit/campfire)."@en ;
	foaf:name "Çorbacı" ;
	rdfs:label "Çorbacı"@en , "Чорбаджи"@ru ;
	owl:sameAs <dbpedia:%C3%87orbac%C4%B1> .

<dbpedia:%C3%87orbac%C4%B1> muninn:wikipedia_version "482582155" .

:Rank_Captain_Lieutenant a :MilitaryRank ;
	rdfs:comment "Captain Lieutenant or Captain-Lieutenant is a military rank, used in a number of different navies worldwide. It is generally equivalent to the Commonwealth or US rank of Lieutenant, and has the NATO rank code of OF-2, though this can vary."@en ;
	foaf:name "Captain Lieutenant" ;
	rdfs:label "Captain Lieutenant"@en , "Kaptenlöjtnant"@sv , "Kapteeniluutnantti"@fi , "Capitaine-lieutenant"@fr , "Kapitänleutnant"@de , "Kapteinløytnant"@no , "Капитан-лейтенант"@ru ;
	owl:sameAs <dbpedia:Captain_Lieutenant> .

<dbpedia:Captain_Lieutenant> muninn:wikipedia_version "469741486" .

:Rank_Captain_lieutenant a :MilitaryRank ;
	foaf:name "Captain lieutenant" ;
	rdfs:label "Captain lieutenant"@en ;
	owl:sameAs <dbpedia:Captain_lieutenant> .

<dbpedia:Captain_lieutenant> muninn:wikipedia_version "497303881" .

:Rank_Chief_petty_officer a :MilitaryRank ;
	foaf:name "Chief petty officer" ;
	rdfs:label "Chief petty officer"@en ;
	owl:sameAs <dbpedia:Chief_petty_officer> .

<dbpedia:Chief_petty_officer> muninn:wikipedia_version "494987481" .

<http://rdf.muninn-project.org/ontologies/military#Rank_Ferik_%28rank%29> a :MilitaryRank ;
	rdfs:comment "Ferik was a military rank of the Ottoman Army. It is translated as Major General or Lieutenant General (Korgeneral). It was superior to a Mirliva (\"Brigadier\") and junior to a Birinci Ferik (\"First Ferik/General\"). The title of Ferik was abolished with Act No. 2590 of 26 November 1934 on the Abolition of Titles and Appellations such as Efendi, Bey or Pasha."@en ;
	foaf:name "Ferik" ;
	rdfs:label "Ferik (rank)"@en ;
	owl:sameAs <dbpedia:Ferik_%28rank%29> .

<dbpedia:Ferik_%28rank%29> muninn:wikipedia_version "440865120" .

:Rank_Fleet_Board a :MilitaryRank ;
	rdfs:comment "Fleet Board is a term in the Royal Navy for the examination cadet officers take which qualifies them to become commissioned officers. After passing the examination, officers who entered as sub-lieutenants have their commissions backdated to the date when they entered the Royal Navy. Midshipmen are also considered commissioned officers at this point, but are not immediately promoted to sub-lieutenant."@en ;
	foaf:name "Fleet Board" ;
	rdfs:label "Fleet Board"@en ;
	owl:sameAs <dbpedia:Fleet_Board> .

<dbpedia:Fleet_Board> muninn:wikipedia_version "467663769" .

:Rank_Garrison_Sergeant_Major a :MilitaryRank ;
	rdfs:comment "A Garrison Sergeant Major (GSM) in the British Army is the senior warrant officer of a garrison and holds the rank of Warrant Officer Class 1. The GSM London District, always a guardsman, holds one of the four most senior WO1 appointments in the British Army, and has military ceremonial responsibility for important state occasions such as Trooping the Colour."@en ;
	foaf:name "Garrison Sergeant Major" ;
	rdfs:label "Garrison Sergeant Major"@en ;
	owl:sameAs <dbpedia:Garrison_Sergeant_Major> .

<dbpedia:Garrison_Sergeant_Major> muninn:wikipedia_version "462244580" .

:Rank_Gefreiter a :MilitaryRank ;
	rdfs:comment "Gefreiter is the German, Swiss and Austrian equivalent for the military rank Private (NATO Rank Code OR-2). Gefreiter was the lowest rank to which an ordinary soldier could be promoted. As a military rank it has existed since at least the 16th century. From the 1920s on Gefreiter has expanded into several additional ranks, those being Obergefreiter, Hauptgefreiter, Stabsgefreiter and Oberstabsgefreiter (NATO Rank Code OR-3 and OR-4). Gefreiter means \"the exempted\"."@en ;
	foaf:name "Gefreiter" ;
	rdfs:label "Gefreiter"@en , "Gefreiter"@de , "Gefreiter"@no , "Gefrajter"@pl , "Ефрейтор"@ru ;
	owl:sameAs <dbpedia:Gefreiter> .

<dbpedia:Gefreiter> muninn:wikipedia_version "492036845" .

:Rank_General_Admiral a :MilitaryRank ;
	rdfs:comment "General Admiral was a Danish, Dutch, German, Russian, Portuguese, Spanish and Swedish naval rank. Its historic origin is a title high military or naval dignitaries of early modern Europe sometimes held, for example the (nominal) Commander-in-Chief of the Dutch Republic's navy."@en ;
	foaf:name "General Admiral" ;
	rdfs:label "General Admiral"@en , "Kenraaliamiraali"@fi , "Generaladmiral"@de , "Admiraal-generaal"@nl , "Генерал-адмирал"@ru , "Almirante General"@es ;
	owl:sameAs <dbpedia:General_Admiral> .

<dbpedia:General_Admiral> muninn:wikipedia_version "491014584" .

:Rank_Kapudan_Pasha a :MilitaryRank ;
	rdfs:comment "Kapudan Pasha or Kapudan-i Derya were the titles given to the chief commander of the navy in the Ottoman Empire. The title Kapudan-i Derya was first granted during the reign of Bayezid I as an official rank within the state structure. Starting with the reign of Mehmed II, holders of the rank were accorded the status of viziers and held the title of Pasha, thus they were more often called Kapudan Pasha."@en ;
	foaf:name "Kapudan Pasha" ;
	rdfs:label "Kapudan Pasha"@en , "Capitan pacha"@fr , "Kapudan Pascha"@de , "Капудан-паша"@ru ;
	owl:sameAs <dbpedia:Kapudan_Pasha> .

<dbpedia:Kapudan_Pasha> muninn:wikipedia_version "481287970" .

<http://rdf.muninn-project.org/ontologies/military#Rank_Kola%C4%9Fas%C4%B1> a :MilitaryRank ;
	rdfs:comment "Kolağası (also written as Kol Ağsı, Kol Aghasi) was a military rank of the Ottoman Army. It corresponds to a Senior Captain or an Adjutant Major. Kol Ağası is a compound word composed of Kol and Ağa. The rank was junior to the Binbaşı (Major) and superior to the Yüzbaşı (Captain). The rank of Kol Ağası was changed to Önyüzbaşı in Republican period."@en ;
	foaf:name "Kolağası" ;
	rdfs:label "Kolağası"@en ;
	owl:sameAs <dbpedia:Kola%C4%9Fas%C4%B1> .

<dbpedia:Kola%C4%9Fas%C4%B1> muninn:wikipedia_version "491860380" .

:Rank_Lance-corporal_of_horse a :MilitaryRank ;
	foaf:name "Lance Corporal of Horse" ;
	rdfs:label "Lance Corporal of Horse"@en ;
	org:rankOf <mil:HouseholdCavalry> ;
	owl:sameAs <dbpedia:Lance-corporal_of_horse> .

<dbpedia:Lance-corporal_of_horse> muninn:wikipedia_version "450536613" .

:Rank_Leading_aircraftman a :MilitaryRank ;
	foaf:name "Leading aircraftman" ;
	rdfs:label "Leading aircraftman"@en ;
	owl:sameAs <dbpedia:Leading_aircraftman> .

<dbpedia:Leading_aircraftman> muninn:wikipedia_version "460246691" .

:Rank_Lord_High_Admiral_of_the_Wash a :MilitaryRank ;
	rdfs:comment "The position of Lord High Admiral of the Wash is an ancient hereditary naval office of England. In mediaeval times, the Lord High Admiral of the Wash was a nobleman with responsibility for the defence and protection of The Wash coast in north East Anglia. The post was granted to the le Strange family after the Norman Conquest. In the 16th century the post became obsolete and the Royal Navy took over the defence of the area."@en ;
	foaf:name "Lord High Admiral of the Wash" ;
	rdfs:label "Lord High Admiral of the Wash"@en ;
	owl:sameAs <dbpedia:Lord_High_Admiral_of_the_Wash> .

<dbpedia:Lord_High_Admiral_of_the_Wash> muninn:wikipedia_version "462939912" .

<http://rdf.muninn-project.org/ontologies/military#Rank_M%C3%BC%C5%9Fir> a :MilitaryRank ;
	foaf:name "Müşir" ;
	rdfs:label "Müşir"@en ;
	owl:sameAs <dbpedia:M%C3%BC%C5%9Fir> .

:Rank_Mirliva a :MilitaryRank ;
	rdfs:comment "Mirliva or Mîr-i livâ was a military rank of the Ottoman Army. It corresponds to a Brigadier General or Major General (Tümgeneral). Mirliva is a compound word composed of Mir and Liva. The rank was junior to the Ferik and superior to the Miralay (Colonel). The title of Mirliva was abolished with Act No. 2590 of 26 November 1934 on the Abolition of Titles and Appellations such as Efendi, Bey or Pasha."@en ;
	foaf:name "Mirliva" ;
	rdfs:label "Mirliva"@en ;
	owl:sameAs <dbpedia:Mirliva> .

<dbpedia:Mirliva> muninn:wikipedia_version "443324813" .

<http://rdf.muninn-project.org/ontologies/military#Rank_Ordinary_seaman_%28rating%29> a :MilitaryRank ;
	foaf:name "Ordinary Seaman" ;
	rdfs:label "Ordinary Seaman"@en ;
	org:rankOf <mil:NavyServiceBranch> ;
	owl:sameAs <dbpedia:Ordinary_seaman_%28rating%29> .

<dbpedia:Ordinary_seaman_%28rating%29> muninn:wikipedia_version "450538267" .

:Rank_Poruchik a :MilitaryRank ;
	rdfs:comment "Poruchik was a military rank in several Slavic countries, such as the Russian Empire and the Republic of Poland, equivalent to Lieutenant. \"Poruchik\" means \"messenger\", \"officer for orders\". This is a Slavic (Czech) copy of the term \"Lieutenant\" (locum tenens). In Russia this rank was first introduced in Strelets New Regiments, the rank legalised by the Table of Ranks. A podporuchik is simply a Sub-Poruchik."@en ;
	foaf:name "Poruchik" ;
	rdfs:label "Poruchik"@en , "Porutschik"@de , "Poručik"@it , "Poroetsjik"@nl , "Поручик"@ru ;
	owl:sameAs <dbpedia:Poruchik> .

<dbpedia:Poruchik> muninn:wikipedia_version "491662172" .

:Rank_Regimental_sergeant_major a :MilitaryRank ;
	foaf:name "Regimental sergeant major" ;
	rdfs:label "Regimental sergeant major"@en ;
	owl:sameAs <dbpedia:Regimental_sergeant_major> .

<dbpedia:Regimental_sergeant_major> muninn:wikipedia_version "469660582" .

:Rank_Schout-bij-nacht a :MilitaryRank ;
	rdfs:comment "Schout-bij-nacht is a Dutch Naval rank, equivalent to Rear Admiral in the US Navy and Royal Navy. It is the second most junior Admiral position of the Dutch Navy, ranking above Commandeur and below a Vice-admiraal. The rank of Schout-bij-nacht originated between the 15th and 16th century. Translated as Watch-at-night, the Schout-bij-Nacht was the officer who supervised the ship when the Captain was asleep."@en ;
	foaf:name "Schout-bij-nacht" ;
	rdfs:label "Schout-bij-nacht"@en , "Schoutbynacht"@sv , "Schout-bij-nacht"@fr , "Schout-bij-nacht"@nl , "Schoutbynacht"@no , "Шаутбенахт"@ru ;
	owl:sameAs <dbpedia:Schout-bij-nacht> .

<dbpedia:Schout-bij-nacht> muninn:wikipedia_version "469920162" .

:Rank_Second_Corporal a :MilitaryRank ;
	rdfs:comment "Second Corporal was a rank in the Royal Engineers and Army Ordnance Corps of the British Army. Second Corporals wore one rank chevron, but unlike Lance-Corporals they held full non-commissioned officer rank. They were thus equivalent to Bombardiers in the Royal Artillery. The rank was abolished in 1920."@en ;
	foaf:name "Second Corporal" ;
	rdfs:label "Second Corporal"@en ;
	owl:sameAs <dbpedia:Second_Corporal> .

<dbpedia:Second_Corporal> muninn:wikipedia_version "332271219" .

:Rank_Sergeant_Major_Instructor a :MilitaryRank ;
	rdfs:comment "Sergeant Major Instructor (SMI) is a British Army appointment held by Warrant Officers Class 1 in the Small Arms School Corps and the Army Physical Training Corps and by some WO1s in the Royal Engineers."@en ;
	foaf:name "Sergeant Major Instructor" ;
	rdfs:label "Sergeant Major Instructor"@en ;
	owl:sameAs <dbpedia:Sergeant_Major_Instructor> .

<dbpedia:Sergeant_Major_Instructor> muninn:wikipedia_version "345897828" .

:Rank_Sotnik a :MilitaryRank ;
	rdfs:comment "Sotnik or Sotnyk was a military rank among the Cossack starshyna (officers), Strelets Troops (17th century) in Muscovy and Imperial Cossack cavalry (since 1826), the Ukrainian Insurgent Army, the Ukrainian Galician Army, and the Ukrainian People's Army."@en ;
	foaf:name "Sotnik" ;
	rdfs:label "Sotnik"@en , "Sotnik"@fr , "Sotnik"@nl , "Sótnik"@pt , "Сотник"@ru ;
	owl:sameAs <dbpedia:Sotnik> .

<dbpedia:Sotnik> muninn:wikipedia_version "472347025" .

<http://rdf.muninn-project.org/ontologies/military#Rank_Stabskapit%C3%A4n> a :MilitaryRank ;
	rdfs:comment "Stabskapitän (staff captain) is a historic military rank, used in the Prussian and Russian armies. It ranked between the Premierleutnant and Hauptmann/Rittmeister in the Prussian army, and between lieutenant and captain in the Russian army."@en ;
	foaf:name "Stabskapitän" ;
	rdfs:label "Stabskapitän"@en , "Alikapteeni"@fi , "Stabskapitän"@de , "Sztabskapitan"@pl , "Штабс-капитан"@ru ;
	owl:sameAs <dbpedia:Stabskapit%C3%A4n> .

<dbpedia:Stabskapit%C3%A4n> muninn:wikipedia_version "493853501" .

:Rank_Staff_Corporal a :MilitaryRank ;
	rdfs:comment "Staff Corporal (SCpl or S/Cpl) is the equivalent rank to Staff Sergeant in the Household Cavalry, ranking between Corporal of Horse and Warrant Officer Class 2. He may hold an appointment such as Squadron Quartermaster Corporal. A Staff Corporal wears four point-up rank chevrons on his cuff, surmounted by a crown."@en ;
	foaf:name "Staff Corporal" ;
	rdfs:label "Staff Corporal"@en ;
	owl:sameAs <dbpedia:Staff_Corporal> .

<dbpedia:Staff_Corporal> muninn:wikipedia_version "409702884" .

:Rank_Staff_Sergeant_Major a :MilitaryRank ;
	foaf:name "Staff Sergeant Major" ;
	rdfs:label "Staff Sergeant Major"@en ;
	owl:sameAs <dbpedia:Staff_Sergeant_Major> .

<dbpedia:Staff_Sergeant_Major> muninn:wikipedia_version "335788405" .

:Rank_Starshina a :MilitaryRank ;
	rdfs:comment "Starshina, or Starshyna, initially was a Cossacks officership, but in Soviet times was used as the top non-commissioned officer. Among Cossacks and in Ukraine, starshina was a collective noun for categories of officership or a military elite: junior starshina (Молодша старшина), general starshina (Генеральна старшина), military starshina (Військова старшина), substarshina (Підстаршина)."@en ;
	foaf:name "Starshina" ;
	rdfs:label "Starshina"@en , "Старшина"@ru , "Starshiná"@es ;
	owl:sameAs <dbpedia:Starshina> .

<dbpedia:Starshina> muninn:wikipedia_version "492104942" .

:Rank_Stratarches a :MilitaryRank ;
	rdfs:comment "Stratarches, means \"master/ruler of the army\" in Greek, and is a title associated with successful generals. In modern Greek usage, it corresponds to the rank of Field Marshal."@en ;
	foaf:name "Stratarches" ;
	rdfs:label "Stratarches"@en ;
	owl:sameAs <dbpedia:Stratarches> .

<dbpedia:Stratarches> muninn:wikipedia_version "473387231" .

<http://rdf.muninn-project.org/ontologies/military#Rank_Suba%C5%9Fi> a :MilitaryRank ;
	rdfs:comment "Subaşi was an Ottoman gubernatorial title used to describe different positions within Ottoman hierarchy, depending on the context. This title was given to sanjak-beys of Ottoman sanjaks which generated more than 15,000 aspers per annum or to the assistants of the sanjabey. The term was also used for commander of the town or castle in Ottoman Empire, an ancient version of chief of police. A surname found among Balkan families, Subaša or Subašić, is derived from the Subaşi title."@en ;
	foaf:name "Subaşi" ;
	rdfs:label "Subaşi"@en ;
	owl:sameAs <dbpedia:Suba%C5%9Fi> .

<dbpedia:Suba%C5%9Fi> muninn:wikipedia_version "490611693" .

:Rank_Subaltern a :MilitaryRank ;
	rdfs:comment "A subaltern is a chiefly British military term for a junior officer. Literally meaning \"subordinate,\" subaltern is used to describe commissioned officers below the rank of captain and generally comprises the various grades of lieutenant. In the British Army the senior subaltern rank was captain-lieutenant, obsolete since the 18th century."@en ;
	foaf:name "Subaltern" ;
	rdfs:label "Subaltern"@en , "Subalternofficer"@sv , "Subalternoffiser"@no , "Субалтерн-офицер"@ru ;
	owl:sameAs <dbpedia:Subaltern> .

<dbpedia:Subaltern> muninn:wikipedia_version "495224024" .

<http://rdf.muninn-project.org/ontologies/military#Rank_Trooper_%28rank%29> a :MilitaryRank ;
	rdfs:comment "Trooper (abbr. Tpr) from the French \"troupier\" is the equivalent rank to private in a regiment with a cavalry tradition in the British Army and many other Commonwealth armies, including those of Australia, Canada, South Africa and New Zealand. Today, most cavalry units operate in the armoured role, equipped with tanks or other armoured fighting vehicles. Some armoured regiments without a cavalry tradition do not use the rank, although the British Royal Tank Regiment does."@en ;
	foaf:name "Trooper" ;
	rdfs:label "Trooper (rank)"@en ;
	owl:sameAs <dbpedia:Trooper_%28rank%29> .

<dbpedia:Trooper_%28rank%29> muninn:wikipedia_version "486616093" .

:Rank_Vice-Admiral_of_the_Coast a :MilitaryRank ;
	rdfs:comment "The holder of the post Vice-Admiral of the Coast was responsible for the defence of one of the twenty maritime counties of England, the North and South of Wales, or the four provinces of Ireland. As a Vice-Admiral, the post holder was the chief of naval administration for his district. His responsibilities included pressing men for naval service, deciding the lawfulness of prizes (captured by pirate ships), dealing with salvage claims for wrecks and acting as a judge."@en ;
	foaf:name "Vice-Admiral of the Coast" ;
	rdfs:label "Vice-Admiral of the Coast"@en ;
	owl:sameAs <dbpedia:Vice-Admiral_of_the_Coast> .

<dbpedia:Vice-Admiral_of_the_Coast> muninn:wikipedia_version "449897542" .

:Rank_Vice-Admiral_of_the_West a :MilitaryRank ;
	rdfs:comment "The historical title Vice-Admiral of the West is sometimes applied to holders of the crown appointment Vice-Admiral of the Coast of counties in the South West of England. The duties of a Vice-Admiral of the coast were to control the shipping (especially piracy) around a maritime county's coast and organise defense on land and at sea. He also acted as a local judge to deal with maritime matters."@en ;
	foaf:name "Vice-Admiral of the West" ;
	rdfs:label "Vice-Admiral of the West"@en ;
	owl:sameAs <dbpedia:Vice-Admiral_of_the_West> .

<dbpedia:Vice-Admiral_of_the_West> muninn:wikipedia_version "459382951" .

:Rank_Wachtmeister a :MilitaryRank ;
	rdfs:comment "Wachtmeister (German for master-sentinel; watch-master) was a German, Austrian and Swiss military rank of non-commissioned officers. It was also adopted into Russian Army vakhmistr and was used as Sergeant-grade rank in cavalry (until 1826), then Special Corps of Gendarmes and Cossack cavalry and Cossack Leib Guard units. Also, the Polish army used the rank Wachmistrz as a cavalry-specific title for Sergeant. This was similar to calling cavalry Captains Rittmeister."@en ;
	foaf:name "Wachtmeister" ;
	rdfs:label "Wachtmeister"@en , "Wachtmeister"@de , "Wachmistrz"@pl , "Вахмистр"@ru ;
	owl:sameAs <dbpedia:Wachtmeister> .

<dbpedia:Wachtmeister> muninn:wikipedia_version "437735728" .

<http://rdf.muninn-project.org/ontologies/military#Rank_Wing_commander_%28rank%29> a :MilitaryRank ;
	foaf:name "Wing commander" ;
	rdfs:label "Wing commander (rank)"@en ;
	owl:sameAs <dbpedia:Wing_commander_%28rank%29> .

<dbpedia:Wing_commander_%28rank%29> muninn:wikipedia_version "496628941" .

:Rank_Yesaul a :MilitaryRank ;
	rdfs:comment "For the town in Armenia, see Ovuni. Part of a series onCossacksFile:Repin Cossacks."@en ;
	foaf:name "Yesaul" ;
	rdfs:label "Yesaul"@en , "Jesaul"@sv , "Jessaul"@de , "Esauł"@pl , "Есаул"@ru ;
	owl:sameAs <dbpedia:Yesaul> .

<dbpedia:Yesaul> muninn:wikipedia_version "464140973" .

<http://rdf.muninn-project.org/ontologies/military#Rank_Chor%C4%85%C5%BCy> a :MilitaryRank ;
	rdfs:comment "Chorąży is a military rank in Poland and neighboring countries. A chorąży was once a knight who bore a standard — the emblem of an armed troop, a province, a land, a duchy, or the kingdom. This function later evolved into a non-hereditary noble title."@en ;
	foaf:name "Chorąży" ;
	rdfs:label "Chorąży"@en , "Chorąży"@pl , "Хорунжий"@ru ;
	owl:sameAs <dbpedia:Chor%C4%85%C5%BCy> .

<dbpedia:Chor%C4%85%C5%BCy> muninn:wikipedia_version "493459036" .

<http://rdf.muninn-project.org/ontologies/military#Rank_Conductor_%28Army%29> a :MilitaryRank ;
	rdfs:comment "Conductor (Cdr) is an appointment held by a few selected Warrant Officers Class 1 in the Royal Logistic Corps and is the most senior appointment that can be held by a warrant officer in the British Army. The appointment was also reintroduced into the Royal Australian Army Ordnance Corps for selected Warrant Officers Class 1 in 2005."@en ;
	foaf:name "Conductor" ;
	rdfs:label "Conductor (Army)"@en ;
	owl:sameAs <dbpedia:Conductor_%28Army%29> .

<dbpedia:Conductor_%28Army%29> muninn:wikipedia_version "495627480" .

<http://rdf.muninn-project.org/ontologies/military#Rank_Drum_major_%28rank%29> a :MilitaryRank ;
	rdfs:comment "The title Drum Major is an appointment, not a military rank."@en ;
	foaf:name "Drum major" ;
	rdfs:label "Drum major (rank)"@en ;
	owl:sameAs <dbpedia:Drum_major_%28rank%29> .

<dbpedia:Drum_major_%28rank%29> muninn:wikipedia_version "498071860" .

:Rank_Drum_Major_General a :MilitaryRank ;
	rdfs:comment "[edit] Overview The Drum Major General was a royal appointment in the British Army used from the mid-17th century and into the 18th century. Under this appointment, all training and licensing of military drummers took place."@en ;
	foaf:name "Drum Major General" ;
	rdfs:label "Drum Major General"@en ;
	owl:sameAs <dbpedia:Drum_Major_General> .

<dbpedia:Drum_Major_General> muninn:wikipedia_version "488221776" .

:Rank_Flight_sergeant a :MilitaryRank ;
	foaf:name "Flight sergeant" ;
	rdfs:label "Flight sergeant"@en ;
	owl:sameAs <dbpedia:Flight_sergeant> .

<dbpedia:Flight_sergeant> muninn:wikipedia_version "463753770" .

:Rank_Hetman a :MilitaryRank ;
	rdfs:comment "Hetman was the title of the second-highest military commander in 15th- to 18th-century Poland and the Grand Duchy of Lithuania, which together, from 1569 to 1795, comprised the Polish-Lithuanian Commonwealth, or Rzeczpospolita. \"Hetman\" was also the highest military office, and head of state, in Ukraine's Cossack Hetmanate. The title (гетьман) was used by Ukraine's Cossacks from the 16th century, and by the Czechs (hejtman) in Bohemia from the Hussite Wars (15th century) on."@en ;
	foaf:name "Hetman" ;
	rdfs:label "Hetman"@en , "Hetman"@sv , "Hetmani"@fi , "Hetman"@fr , "Hetman"@de , "Hetman"@nl , "Hetman"@no , "Hetman"@pl , "Hetman"@pt , "Гетман"@ru , "Hetman"@es ;
	owl:sameAs <dbpedia:Hetman> .

<dbpedia:Hetman> muninn:wikipedia_version "472297416" .

:Rank_Kolonel a :MilitaryRank ;
	rdfs:comment "Kolonel is a rank of the Belgium, Malaysia, Estonia and Netherlands which corresponds to the rank of Colonel in other countries."@en ;
	foaf:name "Kolonel" ;
	rdfs:label "Kolonel"@en ;
	owl:sameAs <dbpedia:Kolonel> .

<dbpedia:Kolonel> muninn:wikipedia_version "439589790" .

:Rank_Lochagos a :MilitaryRank ;
	rdfs:comment "Lochagos is used in the Greek language to mean \"Captain\". More precisely, it means \"leader of a lochos\"."@en ;
	foaf:name "Lochagos" ;
	rdfs:label "Lochagos"@en ;
	owl:sameAs <dbpedia:Lochagos> .

<dbpedia:Lochagos> muninn:wikipedia_version "485272515" .

:Rank_Navarch a :MilitaryRank ;
	rdfs:comment "Navarch is a Greek word meaning \"leader of the ships\", which in some states became the title of an office equivalent to that of a modern admiral."@en ;
	foaf:name "Navarch" ;
	rdfs:label "Navarch"@en , "Navarque"@fr , "Nauarch"@de , "Nauarch"@pl , "Наварх"@ru , "Navarco"@es ;
	owl:sameAs <dbpedia:Navarch> .

<dbpedia:Navarch> muninn:wikipedia_version "493032839" .

:Rank_Phrourarch a :MilitaryRank ;
	rdfs:comment "Phrourarch or Phrourarchos is a Greek military title, meaning garrison commander. Athenians controlled their overseas empire with the episcopi and phrourarchs . The term was widely used by the Macedonian and later Hellenistic armies. Regarding the Spartans, it is not clear if phrourarch was the specific Spartan term. Phroura (garrison) is reported to be a Spartan term for 'a small mobile or expeditionary force'."@en ;
	foaf:name "Phrourarch" ;
	rdfs:label "Phrourarch"@en ;
	owl:sameAs <dbpedia:Phrourarch> .

<dbpedia:Phrourarch> muninn:wikipedia_version "491704131" .

:Rank_Pipe_Major a :MilitaryRank ;
	rdfs:comment "The Pipe Major is the director of bagpipe music in a Scottish or Irish pipe band. Like Drum Major, the position of Pipe Major is derived from British Army traditions. During the early twentieth century, the term Sergeant Piper was used for the role in place of \"Pipe Major\". Civillian and military pipe bands usually assign a Pipe Major."@en ;
	foaf:name "Pipe Major" ;
	rdfs:label "Pipe Major"@en ;
	owl:sameAs <dbpedia:Pipe_Major> .

<dbpedia:Pipe_Major> muninn:wikipedia_version "484159324" .

:Rank_Podpolkovnik a :MilitaryRank ;
	rdfs:comment "Podpolkovnik is a military rank in Slavic countries which corresponds to a Lieutenant Colonel in English-speaking states. Usually this word is translated as Lieutenant Colonel, however the transliteration is also in common usage, for the sake of the historical context. The exact name of this rank maintains a variety of spellings in different languages: File:Flag of Bulgaria. svg Bulgaria — Подполковник File:Flag of the Czech Republic. svg Czech Republic — Podplukovník File:Flag of Georgia."@en ;
	foaf:name "Podpolkovnik" ;
	rdfs:label "Podpolkovnik"@en , "Podpułkownik"@pl ;
	owl:sameAs <dbpedia:Podpolkovnik> .

<dbpedia:Podpolkovnik> muninn:wikipedia_version "476865824" .

:Rank_Polkovnik a :MilitaryRank ;
	rdfs:comment "Polkovnik is often a military rank in Slavic countries which corresponds to a Colonel in English-speaking states. However, in the History of Ukraine polkovnyk was an administrative rank similar to a governor as well. Usually this word is translated as Colonel, however the transliteration is also in common usage, for the sake of the historical and social context."@en ;
	foaf:name "Polkovnik" ;
	rdfs:label "Polkovnik"@en ;
	owl:sameAs <dbpedia:Polkovnik> .

<dbpedia:Polkovnik> muninn:wikipedia_version "493964196" .

:Rank_Staff_sergeant a :MilitaryRank ;
	foaf:name "Staff sergeant" ;
	rdfs:label "Staff sergeant"@en ;
	owl:sameAs <dbpedia:Staff_sergeant> .

<dbpedia:Staff_sergeant> muninn:wikipedia_version "497529431" .

:Rank_Syntagmatarchis a :MilitaryRank ;
	rdfs:comment "Syntagmatarchis, sometimes anglicized as Syntagmatarch, is used in modern Greek to denote the rank of Colonel. It is translated as \"leader of a regiment (syntagma)\", and dates back to the Classical Age armies. However, the name is misleading in that the Hellenic Army retains very few regiments in its command structure. Thus, the typical responsibilities of Syntagmatarches are in staff positions, or as Executive Officers in brigades."@en ;
	foaf:name "Syntagmatarchis" ;
	rdfs:label "Syntagmatarchis"@en ;
	owl:sameAs <dbpedia:Syntagmatarchis> .

<dbpedia:Syntagmatarchis> muninn:wikipedia_version "485256724" .

:Rank_Tagmatarchis a :MilitaryRank ;
	rdfs:comment "Tagmatarchis, in more archaic context transliterated as Tagmatarches, anglicized as Tagmatarch, is used in the Greek language to mean \"Major\". More precisely, it means \"commander of a tagma\". The rank dates to Antiquity and was also used in the Byzantine Empire. In the modern Hellenic Army, the rank is superior to a Lokhagos and inferior to an Antisyntagmatarchis, and held either usually by battalion (tagma) executive officers (battalions are typically commanded by Lieutenant Colonels)."@en ;
	foaf:name "Tagmatarchis" ;
	rdfs:label "Tagmatarchis"@en ;
	owl:sameAs <dbpedia:Tagmatarchis> .

<dbpedia:Tagmatarchis> muninn:wikipedia_version "485265746" .

:Rank_Trumpet_Major a :MilitaryRank ;
	rdfs:comment "Trumpet Major is an appointment in British Army cavalry regiments or the Royal Horse Artillery, held by a Sergeant or a more senior non-commissioned officer or Warrant Officer. His job is to supervise the training and deployment of trumpeters who blow daily duty and ceremonial calls. Trumpet Majors were first appointed to the establishment in 1811. The trumpet was originally a signalling instrument, but it has become purely ceremonial since the invention of radio."@en ;
	foaf:name "Trumpet Major" ;
	rdfs:label "Trumpet Major"@en ;
	owl:sameAs <dbpedia:Trumpet_Major> .

<dbpedia:Trumpet_Major> muninn:wikipedia_version "261772661" .

:Rank_Chiliarch a :MilitaryRank ;
	rdfs:comment "Chiliarch, in the Greek army of the Hellenistic period, was a commander of a 1,000 men unit, roughly equivalent to a modern battalion. The office was an adaptation by Alexander the Great of the Persian Achaemenid empire's hazarapatish. A chiliarch held duties both martial and civil. Alexander the Great first awarded this rank to Hephaestion Amyntoros, but after Hephaestion's death it was awarded to Perdiccas."@en ;
	foaf:name "Chiliarch" ;
	rdfs:label "Chiliarch"@en , "Chiliarque"@fr , "Chiliarch"@de , "Chiliarca"@it , "Chiliarcha"@pl , "Quiliarca"@es ;
	owl:sameAs <dbpedia:Chiliarch> .

<dbpedia:Chiliarch> muninn:wikipedia_version "493968908" .

:Rank_Company_Quartermaster_Sergeant a :MilitaryRank ;
	rdfs:comment "Company Quartermaster Sergeant is a military rank or appointment."@en ;
	foaf:name "Company Quartermaster Sergeant" ;
	rdfs:label "Company Quartermaster Sergeant"@en ;
	owl:sameAs <dbpedia:Company_Quartermaster_Sergeant> .

<dbpedia:Company_Quartermaster_Sergeant> muninn:wikipedia_version "469636323" .

:Rank_Lance_sergeant a :MilitaryRank ;
	foaf:name "Lance Sergeant" ;
	rdfs:label "Lance Sergeant"@en ;
	owl:sameAs <dbpedia:Lance_sergeant> .

<dbpedia:Lance_sergeant> muninn:wikipedia_version "471580953" .

:Rank_Strategos a :MilitaryRank ;
	rdfs:comment "Strategos, plural strategoi, is used in Greek to mean \"general\". In the Hellenistic and Byzantine Empires the term was also used to describe a military governor. In the modern Hellenic Army, it is the highest officer rank."@en ;
	foaf:name "Strategos" ;
	rdfs:label "Strategos"@en , "Strategos"@fi , "Stratège"@fr , "Strategos"@de , "Strategos"@it , "Strategos"@nl , "Strategos"@no , "Strateg (Grecja)"@pl , "Estratego"@pt , "Стратег"@ru , "Strategos"@es ;
	owl:sameAs <dbpedia:Strategos> .

<dbpedia:Strategos> muninn:wikipedia_version "491977225" .

:Rank_Taxiarch a :MilitaryRank ;
	rdfs:comment "Taxiarch, the anglicized form of taxiarchos or taxiarchēs is used in the Greek language to mean \"brigadier\". The term derives from táxis, \"order\", in military context \"an ordered formation\". In turn, the rank has given rise to the Greek term for brigade, taxiarchia. In Greek Orthodox usage, the term is also applied to the Archangels Michael and Gabriel, as leaders of the heavenly host, and several locations in Greece are named after them."@en ;
	foaf:name "Taxiarch" ;
	rdfs:label "Taxiarch"@en , "Таксиарх"@ru ;
	owl:sameAs <dbpedia:Taxiarch> .

<dbpedia:Taxiarch> muninn:wikipedia_version "498203964" .

:Rank_Under_Officer a :MilitaryRank ;
	rdfs:comment "\"Underofficer\" redirects here, although it can also mean non-commissioned officer when translated from certain other languages. Under Officer is an appointment held by senior cadets at some Commonwealth officer training establishments and in University Officers' Training Corps in the United Kingdom, and also a rank used in some Commonwealth cadet forces."@en ;
	foaf:name "Under Officer" ;
	rdfs:label "Under Officer"@en ;
	owl:sameAs <dbpedia:Under_Officer> .

<dbpedia:Under_Officer> muninn:wikipedia_version "491386869" .

:Rank_Lance_corporal a :MilitaryRank ;
	foaf:name "Lance corporal" ;
	rdfs:label "Lance corporal"@en ;
	owl:sameAs <dbpedia:Lance_corporal> .

<dbpedia:Lance_corporal> muninn:wikipedia_version "498208325" .

<http://rdf.muninn-project.org/ontologies/military#Rank_Private_%28rank%29> a :MilitaryRank ;
	rdfs:comment "A Private is a soldier of the lowest military rank (equivalent to NATO Rank Grades OR-1 to OR-3 depending on the force served in). In modern military parlance, 'Private' is shortened to 'Pte' in the United Kingdom and other Commonwealth countries and to 'Pvt. ' in the United States."@en ;
	foaf:name "Private" ;
	rdfs:label "Private (rank)"@en , "Menig 1kl"@sv , "Menig"@sv , "Sotamies"@fi , "Deuxième classe"@fr , "Soldat (grade)"@fr , "Private (Dienstgrad)"@de , "Soldat (Dienstgrad)"@de , "Menig (grad)"@no , "Menig"@no , "Szeregowy"@pl , "Рядовой"@ru , "Soldado raso"@es ;
	owl:sameAs <dbpedia:Private_%28rank%29> .

<dbpedia:Private_%28rank%29> muninn:wikipedia_version "497378634" .

:Rank_Sergeant_Pilot a :MilitaryRank ;
	rdfs:comment "A Sergeant Pilot was a non-commissioned officer who had undergone flight training and was a qualified pilot in the air forces of several Commonwealth countries and in the United States Army Air Force before, during and after World War II. After World War II, non-commissioned pilots began to be phased out and today all air force pilots are commissioned officers. In the United States, the Flight Officer Act ended enlisted men's chances of undergoing flight training."@en ;
	foaf:name "Sergeant Pilot" ;
	rdfs:label "Sergeant Pilot"@en , "Fältflygare"@sv ;
	owl:sameAs <dbpedia:Sergeant_Pilot> .

<dbpedia:Sergeant_Pilot> muninn:wikipedia_version "491338622" .

<http://rdf.muninn-project.org/ontologies/military#Rank_Warrant_officer_%28United_Kingdom%29> a :MilitaryRank ;
	foaf:name "Warrant Officer" ;
	rdfs:label "Warrant Officer"@en ;
	owl:subClassOf <mil:#Rank_Warrant_officer_EnglishTradition> ;
	owl:sameAs <dbpedia:Warrant_officer_%28United_Kingdom%29> .

<dbpedia:Warrant_officer_%28United_Kingdom%29> muninn:wikipedia_version "496940079" .

<http://rdf.muninn-project.org/ontologies/military#Rank_Captain_%28OF-2%29> a :MilitaryRank ;
	rdfs:comment "The army rank of captain (from the French capitaine) is a commissioned officer rank historically corresponding to command of a company of soldiers. The rank is also used by some air forces and marine forces. Today a captain is typically either the commander or second-in-command of a company or artillery battery. In the Chinese People's Liberation Army, a captain may also command a platoon, or be the second-in-command of a battalion. Captain is one rank above a lieutenant and one below a major."@en ;
	foaf:name "Captain" ;
	rdfs:label "Captain (OF-2)"@en , "Kapten"@sv , "Kapteeni (sotilasarvo)"@fi , "Capitaine"@fr , "Hauptmann (Offizier)"@de , "Capitano"@it , "Kapitein (rang)"@nl , "Kaptein (grad)"@no , "Kapitan (ranga)"@pl , "Capitão (militar)"@pt , "Капитан (воинское звание)"@ru , "Capitán"@es ;
	owl:sameAs <dbpedia:Captain_%28OF-2%29> .

<dbpedia:Captain_%28OF-2%29> muninn:wikipedia_version "495714124" .

:Rank_Company_sergeant_major a :MilitaryRank ;
	foaf:name "Company sergeant major" ;
	rdfs:label "Company sergeant major"@en ;
	owl:sameAs <dbpedia:Company_sergeant_major> .

<dbpedia:Company_sergeant_major> muninn:wikipedia_version "497899716" .

:Rank_Regimental_Quartermaster_Sergeant a :MilitaryRank ;
	rdfs:comment "Regimental Quartermaster Sergeant is a military rank in some militaries, and an appointment in others."@en ;
	foaf:name "Regimental Quartermaster Sergeant" ;
	rdfs:label "Regimental Quartermaster Sergeant"@en ;
	owl:sameAs <dbpedia:Regimental_Quartermaster_Sergeant> .

<dbpedia:Regimental_Quartermaster_Sergeant> muninn:wikipedia_version "495627637" .

:Rank_Oberst a :MilitaryRank ;
	rdfs:comment "Oberst is a military rank in several German-speaking and Scandinavian countries, equivalent to Colonel. It is currently used by both the ground and air forces of Austria, Germany, Switzerland, Denmark and Norway. The Swedish rank överste is a direct translation, as are the Finnish rank eversti and the Icelandic rank ofursti. In the Netherlands the rank overste is used as a synonym for a Lieutenant Colonel"@en ;
	foaf:name "Oberst" ;
	rdfs:label "Oberst"@en , "Oberst"@pt ;
	owl:sameAs <dbpedia:Oberst> .

<dbpedia:Oberst> muninn:wikipedia_version "485029855" .

:Rank_Oberst_Germany a :MilitaryRank ;
	owl:subClass :Rank_Oberst ;
	foaf:name "Oberst"@en ;
	rdfs:label "Oberst (Germany)"@en , "Oberst (Germany)"@pt ;
	rdfs:comment "The specific instance of the Oberst rank in the context of country ."@en ;
	owl:rankOf <dbpedia:Germany> .

<dbpedia:Germany> muninn:wikipedia_version "498342708" .

:Rank_Oberstleutnant_Germany a :MilitaryRank ;
	owl:subClass :Rank_Oberstleutnant ;
	foaf:name "Oberstleutnant"@en ;
	rdfs:label "Oberstleutnant (Germany)"@en , "Oberstleutnant (Germany)"@pt ;
	rdfs:comment "The specific instance of the Oberstleutnant rank in the context of Germany."@en ;
	owl:rankOf <dbpedia:Germany> .

:Rank_Oberst_Sweden a :MilitaryRank ;
	owl:subClass :Rank_Oberst ;
	foaf:name "Oberst"@en ;
	rdfs:label "Oberst (Sweden)"@en , "Oberst (Sverige)"@sv , "Oberst (Ruotsi)"@fi , "Oberst (Suède)"@fr , "Oberst (Schweden)"@de , "Oberst (Svezia)"@it , "Oberst (Zweden)"@nl , "Oberst (Sverige)"@no , "Oberst (Szwecja)"@pl , "Oberst (Suécia)"@pt , "Oberst (Швеция)"@ru , "Oberst (Suecia)"@es ;
	rdfs:comment "The specific instance of the Oberst rank in the context of country Sweden."@en ;
	owl:rankOf <dbpedia:Sweden> .

<dbpedia:Sweden> muninn:wikipedia_version "497805145" .

:Rank_Oberst_Norway a :MilitaryRank ;
	owl:subClass :Rank_Oberst ;
	foaf:name "Oberst"@en ;
	rdfs:label "Oberst (Norway)"@en , "Oberst (Norge)"@sv , "Oberst (Norja)"@fi , "Oberst (Norvège)"@fr , "Oberst (Norwegen)"@de , "Oberst (Norvegia)"@it , "Oberst (Noorwegen)"@nl , "Oberst (Norge)"@no , "Oberst (Norwegia)"@pl , "Oberst (Noruega)"@pt , "Oberst (Норвегия)"@ru , "Oberst (Noruega)"@es ;
	rdfs:comment "The specific instance of the Oberst rank in the context of country Norway."@en ;
	owl:rankOf <dbpedia:Norway> .

<dbpedia:Norway> muninn:wikipedia_version "496844290" .

:Rank_Oberst_Austria a :MilitaryRank ;
	owl:subClass :Rank_Oberst ;
	foaf:name "Oberst"@en ;
	rdfs:label "Oberst (Austria)"@en , "Oberst (Österrike)"@sv , "Oberst (Itävalta)"@fi , "Oberst (Autriche)"@fr , "Oberst (Österreich)"@de , "Oberst (Austria)"@it , "Oberst (Oostenrijk)"@nl , "Oberst (Østerrike)"@no , "Oberst (Austria)"@pl , "Oberst (Áustria)"@pt , "Oberst (Австрия)"@ru , "Oberst (Austria)"@es ;
	rdfs:comment "The specific instance of the Oberst rank in the context of country Austria."@en ;
	owl:rankOf <dbpedia:Austria> .

<dbpedia:Austria> muninn:wikipedia_version "498078721" .

:Rank_Oberst_Finland a :MilitaryRank ;
	owl:subClass :Rank_Oberst ;
	foaf:name "Oberst"@en ;
	rdfs:label "Oberst (Finland)"@en , "Oberst (Finland)"@sv , "Oberst (Suomi)"@fi , "Oberst (Finlande)"@fr , "Oberst (Finnland)"@de , "Oberst (Finlandia)"@it , "Oberst (Finland)"@nl , "Oberst (Finland)"@no , "Oberst (Finlandia)"@pl , "Oberst (Finlândia)"@pt , "Oberst (Финляндия)"@ru , "Oberst (Finlandia)"@es ;
	rdfs:comment "The specific instance of the Oberst rank in the context of country Finland."@en ;
	owl:rankOf <dbpedia:Finland> .

<dbpedia:Finland> muninn:wikipedia_version "498358269" .

:Rank_Oberst_Denmark a :MilitaryRank ;
	owl:subClass :Rank_Oberst ;
	foaf:name "Oberst"@en ;
	rdfs:label "Oberst (Denmark)"@en , "Oberst (Danmark)"@sv , "Oberst (Tanska)"@fi , "Oberst (Danemark)"@fr , "Oberst (Dänemark)"@de , "Oberst (Danimarca)"@it , "Oberst (Denemarken)"@nl , "Oberst (Danmark)"@no , "Oberst (Dania)"@pl , "Oberst (Dinamarca)"@pt , "Oberst (Дания)"@ru , "Oberst (Dinamarca)"@es ;
	rdfs:comment "The specific instance of the Oberst rank in the context of country Denmark."@en ;
	owl:rankOf <dbpedia:Denmark> .

<dbpedia:Denmark> muninn:wikipedia_version "498348760" .

:Rank_Oberst_Kingdom_of_Denmark a :MilitaryRank ;
	owl:subClass :Rank_Oberst ;
	foaf:name "Oberst"@en ;
	rdfs:label "Oberst (Kingdom of Denmark)"@en , "Oberst (Kungariket Danmark)"@sv , "Oberst (Tanskan kuningaskunta)"@fi , "Oberst (Regno Unito di Danimarca)"@it , "Oberst (Reino da Dinamarca)"@pt , "Oberst (Королевство Дания)"@ru , "Oberst (Reino de Dinamarca)"@es ;
	rdfs:comment "The specific instance of the Oberst rank in the context of country Kingdom of Denmark."@en ;
	owl:rankOf <dbpedia:Kingdom_of_Denmark> .

<dbpedia:Kingdom_of_Denmark> muninn:wikipedia_version "472858436" .

:Rank_Oberst_Switzerland a :MilitaryRank ;
	owl:subClass :Rank_Oberst ;
	foaf:name "Oberst"@en ;
	rdfs:label "Oberst (Switzerland)"@en , "Oberst (Schweiz)"@sv , "Oberst (Sveitsi)"@fi , "Oberst (Suisse)"@fr , "Oberst (Schweiz)"@de , "Oberst (Svizzera)"@it , "Oberst (Zwitserland)"@nl , "Oberst (Sveits)"@no , "Oberst (Szwajcaria)"@pl , "Oberst (Suíça)"@pt , "Oberst (Швейцария)"@ru , "Oberst (Suiza)"@es ;
	rdfs:comment "The specific instance of the Oberst rank in the context of country Switzerland."@en ;
	owl:rankOf <dbpedia:Switzerland> .

<dbpedia:Switzerland> muninn:wikipedia_version "498226943" .

<http://rdf.muninn-project.org/ontologies/military#Rank_Able_seaman_%28rank%29_Canada> a :MilitaryRank ;
	owl:subClass <http://rdf.muninn-project.org/ontologies/military#Rank_Able_seaman_%28rank%29> ;
	foaf:name ""@en ;
	rdfs:comment "The specific instance of the  rank in the context of country ."@en ;
	owl:rankOf <dbpedia:Canada> .

<dbpedia:Canada> muninn:wikipedia_version "498337533" .

<http://rdf.muninn-project.org/ontologies/military#Rank_Able_seaman_%28rank%29_Commonwealth_of_Nations> a :MilitaryRank ;
	owl:subClass <http://rdf.muninn-project.org/ontologies/military#Rank_Able_seaman_%28rank%29> ;
	foaf:name ""@en ;
	rdfs:label "(Commonwealth of Nations)"@en , "(Samväldet)"@sv , "(Kansainyhteisö)"@fi , "(Commonwealth of Nations)"@fr , "(Commonwealth of Nations)"@de , "(Commonwealth delle nazioni)"@it , "(Gemenebest van Naties)"@nl , "(Samveldet av nasjoner)"@no , "(Wspólnota Narodów)"@pl , "(Commonwealth)"@pt , "(Содружество наций)"@ru , "(Mancomunidad de Naciones)"@es ;
	rdfs:comment "The specific instance of the  rank in the context of country Commonwealth of Nations."@en ;
	owl:rankOf <dbpedia:Commonwealth_of_Nations> .

<dbpedia:Commonwealth_of_Nations> muninn:wikipedia_version "498034851" .

<http://rdf.muninn-project.org/ontologies/military#Rank_Admiral_of_the_Fleet_%28Russia%29_Russia> a :MilitaryRank ;
	owl:subClass <http://rdf.muninn-project.org/ontologies/military#Rank_Admiral_of_the_Fleet_%28Russia%29> ;
	foaf:name "Admiral of the Fleet"@en ;
	rdfs:label "Admiral of the Fleet (Russia) (Russia)"@en , "Admiral of the Fleet (Russia) (Ryssland)"@sv , "Admiral of the Fleet (Russia) (Venäjä)"@fi , "Admiral of the Fleet (Russia) (Russie)"@fr , "Admiral of the Fleet (Russia) (Russland)"@de , "Ammiraglio della flotta (Russia) (Russia)"@it , "Admiral of the Fleet (Russia) (Rusland)"@nl , "Admiral of the Fleet (Russia) (Russland)"@no , "Admiral of the Fleet (Russia) (Rosja)"@pl , "Admiral of the Fleet (Russia) (Rússia)"@pt , "Admiral of the Fleet (Russia) (Россия)"@ru , "Admiral of the Fleet (Russia) (Rusia)"@es ;
	rdfs:comment "The specific instance of the Admiral of the Fleet (Russia) rank in the context of country Russia."@en ;
	owl:rankOf <dbpedia:Russia> .

<dbpedia:Russia> muninn:wikipedia_version "498219998" .

<http://rdf.muninn-project.org/ontologies/military#Rank_Admiral_of_the_Fleet_%28Russia%29_Soviet_Union> a :MilitaryRank ;
	owl:subClass <http://rdf.muninn-project.org/ontologies/military#Rank_Admiral_of_the_Fleet_%28Russia%29> ;
	foaf:name "Admiral of the Fleet"@en ;
	rdfs:label "Admiral of the Fleet (Russia) (Soviet Union)"@en , "Admiral of the Fleet (Russia) (Sovjetunionen)"@sv , "Admiral of the Fleet (Russia) (Neuvostoliitto)"@fi , "Admiral of the Fleet (Russia) (Union des républiques socialistes soviétiques)"@fr , "Admiral of the Fleet (Russia) (Sowjetunion)"@de , "Ammiraglio della flotta (Russia) (Unione Sovietica)"@it , "Admiral of the Fleet (Russia) (Sovjet-Unie)"@nl , "Admiral of the Fleet (Russia) (Sovjetunionen)"@no , "Admiral of the Fleet (Russia) (Związek Socjalistycznych Republik Radzieckich)"@pl , "Admiral of the Fleet (Russia) (União Soviética)"@pt , "Admiral of the Fleet (Russia) (Союз Советских Социалистических Республик)"@ru , "Admiral of the Fleet (Russia) (Unión Soviética)"@es ;
	rdfs:comment "The specific instance of the Admiral of the Fleet (Russia) rank in the context of country Soviet Union."@en ;
	owl:rankOf <dbpedia:Soviet_Union> .

<dbpedia:Soviet_Union> muninn:wikipedia_version "498351053" .

:Rank_Anthypolochagos_Greece a :MilitaryRank ;
	owl:subClass :Rank_Anthypolochagos ;
	foaf:name "Anthypolochagos"@en ;
	rdfs:label "Anthypolochagos (Greece)"@en , "Anthypolochagos (Grekland)"@sv , "Anthypolochagos (Kreikka)"@fi , "Anthypolochagos (Grèce)"@fr , "Anthypolochagos (Griechenland)"@de , "Anthypolochagos (Grecia)"@it , "Anthypolochagos (Griekenland)"@nl , "Anthypolochagos (Hellas)"@no , "Anthypolochagos (Grecja)"@pl , "Anthypolochagos (Grécia)"@pt , "Anthypolochagos (Греция)"@ru , "Anthypolochagos (Grecia)"@es ;
	rdfs:comment "The specific instance of the Anthypolochagos rank in the context of country Greece."@en ;
	owl:rankOf <dbpedia:Greece> .

<dbpedia:Greece> muninn:wikipedia_version "498205865" .

:Rank_Anthypolochagos_Official_Timocracy_of_Sapinetia a :MilitaryRank ;
	owl:subClass :Rank_Anthypolochagos ;
	foaf:name "Anthypolochagos"@en ;
	rdfs:label "Anthypolochagos (Timocracy of Sapinetia)"@en ;
	rdfs:comment "The specific instance of the Anthypolochagos rank in the context of the Timocracy_of_Sapinetia."@en ;
	owl:rankOf <dbpedia:Official_Timocracy_of_Sapinetia> .

:Rank_Antisyntagmatarchis_Greece a :MilitaryRank ;
	owl:subClass :Rank_Antisyntagmatarchis ;
	foaf:name "Antisyntagmatarchis"@en ;
	rdfs:label "Antisyntagmatarchis (Greece)"@en , "Antisyntagmatarchis (Grekland)"@sv , "Antisyntagmatarchis (Kreikka)"@fi , "Antisyntagmatarchis (Grèce)"@fr , "Antisyntagmatarchis (Griechenland)"@de , "Antisyntagmatarchis (Grecia)"@it , "Antisyntagmatarchis (Griekenland)"@nl , "Antisyntagmatarchis (Hellas)"@no , "Antisyntagmatarchis (Grecja)"@pl , "Antisyntagmatarchis (Grécia)"@pt , "Antisyntagmatarchis (Греция)"@ru , "Antisyntagmatarchis (Grecia)"@es ;
	rdfs:comment "The specific instance of the Antisyntagmatarchis rank in the context of country Greece."@en ;
	owl:rankOf <dbpedia:Greece> .

:Rank_Antisyntagmatarchis_Official_Timocracy_of_Sapinetia a :MilitaryRank ;
	owl:subClass :Rank_Antisyntagmatarchis ;
	foaf:name "Antisyntagmatarchis"@en ;
	rdfs:label "Antisyntagmatarchis (Timocracy_of_Sapinetia)"@en ;
	rdfs:comment "The specific instance of the Antisyntagmatarchis rank in the context of the Timocracy_of_Sapinetia."@en ;
	owl:rankOf <dbpedia:Official_Timocracy_of_Sapinetia> .

:Rank_Appointee_Italy a :MilitaryRank ;
	owl:subClass :Rank_Appointee ;
	foaf:name "Appuntato"@it ;
	rdfs:label "Appointee (Italy)"@en , "Appointee (Italien)"@sv , "Appointee (Italia)"@fi , "Appointé (Italie)"@fr , "Appointee (Italien)"@de , "Appuntato (Italia)"@it , "Appointee (Italië)"@nl , "Appointee (Italia)"@no , "Appointee (Włochy)"@pl , "Appointee (Itália)"@pt , "Appointee (Италия)"@ru , "Appointee (Italia)"@es ;
	rdfs:comment "The specific instance of the Appointee rank in the context of country Italy."@en ;
	owl:rankOf <dbpedia:Italy> .

<dbpedia:Italy> muninn:wikipedia_version "498219654" .

:Rank_Appointee_Switzerland a :MilitaryRank ;
	owl:subClass :Rank_Appointee ;
	foaf:name "Appointé"@fr , "Appuntato"@it ;
	rdfs:label "Appointee (Switzerland)"@en , "Appointee (Schweiz)"@sv , "Appointee (Sveitsi)"@fi , "Appointé (Suisse)"@fr , "Appointee (Schweiz)"@de , "Appuntato (Svizzera)"@it , "Appointee (Zwitserland)"@nl , "Appointee (Sveits)"@no , "Appointee (Szwajcaria)"@pl , "Appointee (Suíça)"@pt , "Appointee (Швейцария)"@ru , "Appointee (Suiza)"@es ;
	rdfs:comment "The specific instance of the Appointee rank in the context of country Switzerland."@en ;
	owl:rankOf <dbpedia:Switzerland> .

<http://rdf.muninn-project.org/ontologies/military#Rank_Army_General_%28Russia%29_Russia> a :MilitaryRank ;
	owl:subClass <http://rdf.muninn-project.org/ontologies/military#Rank_Army_General_%28Russia%29> ;
	foaf:name "Генерал армии"@ru ;
	rdfs:label "Army General (Russia) (Russia)"@en , "Army General (Russia) (Ryssland)"@sv , "Army General (Russia) (Venäjä)"@fi , "Army General (Russia) (Russie)"@fr , "Army General (Russia) (Russland)"@de , "Army General (Russia) (Russia)"@it , "Army General (Russia) (Rusland)"@nl , "Army General (Russia) (Russland)"@no , "Army General (Russia) (Rosja)"@pl , "Army General (Russia) (Rússia)"@pt , "Генерал армии (Россия) (Россия)"@ru , "Army General (Russia) (Rusia)"@es ;
	rdfs:comment "The specific instance of the Army General (Russia) rank in the context of country Russia."@en ;
	owl:rankOf <dbpedia:Russia> .

<http://rdf.muninn-project.org/ontologies/military#Rank_Army_General_%28Russia%29_Soviet_Union> a :MilitaryRank ;
	owl:subClass <http://rdf.muninn-project.org/ontologies/military#Rank_Army_General_%28Russia%29> ;
	foaf:name "Army General"@en ;
	rdfs:label "Army General (Russia) (Soviet Union)"@en , "Army General (Russia) (Sovjetunionen)"@sv , "Army General (Russia) (Neuvostoliitto)"@fi , "Army General (Russia) (Union des républiques socialistes soviétiques)"@fr , "Army General (Russia) (Sowjetunion)"@de , "Army General (Russia) (Unione Sovietica)"@it , "Army General (Russia) (Sovjet-Unie)"@nl , "Army General (Russia) (Sovjetunionen)"@no , "Army General (Russia) (Związek Socjalistycznych Republik Radzieckich)"@pl , "Army General (Russia) (União Soviética)"@pt , "Генерал армии (Россия) (Союз Советских Социалистических Республик)"@ru , "Army General (Russia) (Unión Soviética)"@es ;
	rdfs:comment "The specific instance of the Army General (Russia) rank in the context of country Soviet Union."@en ;
	owl:rankOf <dbpedia:Soviet_Union> .

:Rank_Aspirant_France a :MilitaryRank ;
	owl:subClass :Rank_Aspirant ;
	foaf:name "Aspirant"@en ;
	rdfs:label "Aspirant (France)"@en ;
	rdfs:comment "The specific instance of the Aspirant rank in the context of France."@en ;
	owl:rankOf <dbpedia:France> .

<dbpedia:France> muninn:wikipedia_version "498318960" .

:Rank_Aspirant_Romania a :MilitaryRank ;
	owl:subClass :Rank_Aspirant ;
	foaf:name "Aspirant"@en ;
	rdfs:label "Aspirant (Romania)"@en , "Aspirant (Rumänien)"@sv , "Aspirant (Romania)"@fi , "Aspirant (Roumanie)"@fr , "Aspirant (Rumänien)"@de , "Aspirant (Romania)"@it , "Aspirant (Roemenië)"@nl , "Aspirant (Romania)"@no , "Aspirant (Rumunia)"@pl , "Aspirant (Roménia)"@pt , "Aspirant (Румыния)"@ru , "Aspirant (Rumania)"@es ;
	rdfs:comment "The specific instance of the Aspirant rank in the context of country Romania."@en ;
	owl:rankOf <dbpedia:Romania> .

<dbpedia:Romania> muninn:wikipedia_version "498318250" .

<http://rdf.muninn-project.org/ontologies/military#Rank_Aspirant_%28Romania%29_Romania> a :MilitaryRank ;
	owl:subClass <http://rdf.muninn-project.org/ontologies/military#Rank_Aspirant_%28Romania%29> ;
	foaf:name "Aspirant"@en ;
	rdfs:label "Aspirant (Romania) (Romania)"@en , "Aspirant (Romania) (Rumänien)"@sv , "Aspirant (Romania) (Romania)"@fi , "Aspirant (Romania) (Roumanie)"@fr , "Aspirant (Romania) (Rumänien)"@de , "Aspirant (Romania) (Romania)"@it , "Aspirant (Romania) (Roemenië)"@nl , "Aspirant (Romania) (Romania)"@no , "Aspirant (Romania) (Rumunia)"@pl , "Aspirant (Romania) (Roménia)"@pt , "Aspirant (Romania) (Румыния)"@ru , "Aspirant (Romania) (Rumania)"@es ;
	rdfs:comment "The specific instance of the Aspirant (Romania) rank in the context of country Romania."@en ;
	owl:rankOf <dbpedia:Romania> .

:Rank_Brigade_General_Australia a :MilitaryRank ;
	owl:subClass :Rank_Brigade_General ;
	foaf:name "Brigade General"@en ;
	rdfs:label "Brigade General (Australia)"@en , "Brigade General (Australien)"@sv , "Brigade General (Australia)"@fi , "Brigade General (Australie)"@fr , "Brigade General (Australien)"@de , "Brigade General (Australia)"@it , "Brigade General (Australië (land))"@nl , "Brigade General (Australia)"@no , "Brigade General (Australia)"@pl , "Brigade General (Austrália)"@pt , "Brigade General (Австралия)"@ru , "Brigade General (Australia)"@es ;
	rdfs:comment "The specific instance of the Brigade General rank in the context of country Australia."@en ;
	owl:rankOf <dbpedia:Australia> .

<dbpedia:Australia> muninn:wikipedia_version "498314417" .

:Rank_Brigade_General_Canada a :MilitaryRank ;
	owl:subClass :Rank_Brigade_General ;
	foaf:name "Brigade General"@en ;
	rdfs:label "Brigade General (Canada)"@en ;
	rdfs:comment "The specific instance of the Brigade General rank in the context of Canada."@en ;
	owl:rankOf <dbpedia:Canada> .

:Rank_Brigadier_general_Australia a :MilitaryRank ;
	owl:subClass :Rank_Brigadier_general ;
	foaf:name "Brigadier general"@en ;
	rdfs:label "Brigadier general (Australia)"@en , "Brigadier general (Australien)"@sv , "Brigadier general (Australia)"@fi , "Brigadier general (Australie)"@fr , "Brigadier general (Australien)"@de , "Brigadier general (Australia)"@it , "Brigadier general (Australië (land))"@nl , "Brigadier general (Australia)"@no , "Brigadier general (Australia)"@pl , "Brigadier general (Austrália)"@pt , "Brigadier general (Австралия)"@ru , "Brigadier general (Australia)"@es ;
	rdfs:comment "The specific instance of the Brigadier general rank in the context of country Australia."@en ;
	owl:rankOf <dbpedia:Australia> .

:Rank_Brigadier_general_Canada a :MilitaryRank ;
	owl:subClass :Rank_Brigadier_general ;
	foaf:name "Brigadier general"@en ;
	rdfs:label "Brigadier general (Canada)"@en ;
	rdfs:comment "The specific instance of the Brigadier general rank in the context of Canada."@en ;
	owl:rankOf <dbpedia:Canada> .

<http://rdf.muninn-project.org/ontologies/military#Rank_Buffer_%28navy%29_Australia> a :MilitaryRank ;
	owl:subClass <http://rdf.muninn-project.org/ontologies/military#Rank_Buffer_%28navy%29> ;
	foaf:name "Buffer"@en ;
	rdfs:label "Buffer (navy) (Australia)"@en , "Buffer (navy) (Australien)"@sv , "Buffer (navy) (Australia)"@fi , "Buffer (navy) (Australie)"@fr , "Buffer (navy) (Australien)"@de , "Buffer (navy) (Australia)"@it , "Buffer (navy) (Australië (land))"@nl , "Buffer (navy) (Australia)"@no , "Buffer (navy) (Australia)"@pl , "Buffer (navy) (Austrália)"@pt , "Buffer (navy) (Австралия)"@ru , "Buffer (navy) (Australia)"@es ;
	rdfs:comment "The specific instance of the Buffer (navy) rank in the context of country Australia."@en ;
	owl:rankOf <dbpedia:Australia> .

<http://rdf.muninn-project.org/ontologies/military#Rank_Buffer_%28navy%29_Commonwealth_of_Nations> a :MilitaryRank ;
	owl:subClass <http://rdf.muninn-project.org/ontologies/military#Rank_Buffer_%28navy%29> ;
	foaf:name "Buffer"@en ;
	rdfs:label "Buffer (navy) (Commonwealth of Nations)"@en , "Buffer (navy) (Samväldet)"@sv , "Buffer (navy) (Kansainyhteisö)"@fi , "Buffer (navy) (Commonwealth of Nations)"@fr , "Buffer (navy) (Commonwealth of Nations)"@de , "Buffer (navy) (Commonwealth delle nazioni)"@it , "Buffer (navy) (Gemenebest van Naties)"@nl , "Buffer (navy) (Samveldet av nasjoner)"@no , "Buffer (navy) (Wspólnota Narodów)"@pl , "Buffer (navy) (Commonwealth)"@pt , "Buffer (navy) (Содружество наций)"@ru , "Buffer (navy) (Mancomunidad de Naciones)"@es ;
	rdfs:comment "The specific instance of the Buffer (navy) rank in the context of country Commonwealth of Nations."@en ;
	owl:rankOf <dbpedia:Commonwealth_of_Nations> .

<http://rdf.muninn-project.org/ontologies/military#Rank_Captain_%28naval%29_Australia> a :MilitaryRank ;
	owl:subClass <http://rdf.muninn-project.org/ontologies/military#Rank_Captain_%28naval%29> ;
	foaf:name "Captain"@en ;
	rdfs:label "Captain (naval) (Australia)"@en , "Kommendör (Australien)"@sv , "Kommodori (Australia)"@fi , "Capitaine de vaisseau (Australie)"@fr , "Kapitän zur See (Australien)"@de , "Capitano di vascello (Australia)"@it , "Kapitein-ter-zee (Australië (land))"@nl , "Kommandør (Australia)"@no , "Komandor (Australia)"@pl , "Capitão de mar e guerra (Austrália)"@pt , "Капитан 1-го ранга (Австралия)"@ru , "Capitán de navío (Australia)"@es ;
	rdfs:comment "The specific instance of the Captain (naval) rank in the context of country Australia."@en ;
	owl:rankOf <dbpedia:Australia> .

<http://rdf.muninn-project.org/ontologies/military#Rank_Captain_%28naval%29_Canada> a :MilitaryRank ;
	owl:subClass <http://rdf.muninn-project.org/ontologies/military#Rank_Captain_%28naval%29> ;
	foaf:name "Capitaine de vaisseau"@fr ;
	rdfs:label "Captain (naval, Canada)"@en , "Kommendör (Canada)"@sv , "Kommodori (Canada)"@fi , "Capitaine de vaisseau (Canada)"@fr , "Kapitän zur See (Canada)"@de , "Capitano di vascello (Canada)"@it , "Kapitein-ter-zee (Canada)"@nl , "Kommandør (Canada)"@no , "Komandor (Canada)"@pl , "Capitão de mar e guerra (Canada)"@pt , "Капитан 1-го ранга (Canada)"@ru , "Capitán de navío (Canada)"@es ;
	rdfs:comment "The specific instance of the Captain (naval) rank in the context of Canada."@en ;
	owl:rankOf <dbpedia:Canada> .

:Rank_Chief_Marshal_Russia a :MilitaryRank ;
	owl:subClass :Rank_Chief_Marshal ;
	foaf:name "Главный маршал рода войск"@ru ;
	rdfs:label "Chief Marshal (Russia)"@en , "Chief Marshal (Ryssland)"@sv , "Chief Marshal (Venäjä)"@fi , "Chief Marshal (Russie)"@fr , "Chief Marshal (Russland)"@de , "Chief Marshal (Russia)"@it , "Chief Marshal (Rusland)"@nl , "Chief Marshal (Russland)"@no , "Chief Marshal (Rosja)"@pl , "Chief Marshal (Rússia)"@pt , "Главный маршал рода войск (Россия)"@ru , "Chief Marshal (Rusia)"@es ;
	rdfs:comment "The specific instance of the Chief Marshal rank in the context of country Russia."@en ;
	owl:rankOf <dbpedia:Russia> .

:Rank_Chief_Marshal_Soviet_Union a :MilitaryRank ;
	owl:subClass :Rank_Chief_Marshal ;
	foaf:name "Chief Marshal"@en ;
	rdfs:label "Chief Marshal (Soviet Union)"@en , "Chief Marshal (Sovjetunionen)"@sv , "Chief Marshal (Neuvostoliitto)"@fi , "Chief Marshal (Union des républiques socialistes soviétiques)"@fr , "Chief Marshal (Sowjetunion)"@de , "Chief Marshal (Unione Sovietica)"@it , "Chief Marshal (Sovjet-Unie)"@nl , "Chief Marshal (Sovjetunionen)"@no , "Chief Marshal (Związek Socjalistycznych Republik Radzieckich)"@pl , "Chief Marshal (União Soviética)"@pt , "Главный маршал рода войск (Союз Советских Социалистических Республик)"@ru , "Chief Marshal (Unión Soviética)"@es ;
	rdfs:comment "The specific instance of the Chief Marshal rank in the context of country Soviet Union."@en ;
	owl:rankOf <dbpedia:Soviet_Union> .

:Rank_Comandarm_Russia a :MilitaryRank ;
	owl:subClass :Rank_Comandarm ;
	foaf:name "Comandarm"@en ;
	rdfs:label "Comandarm (Russia)"@en , "Comandarm (Ryssland)"@sv , "Comandarm (Venäjä)"@fi , "Comandarm (Russie)"@fr , "Sowjetische GeneralsrängeKomandarm (Russland)"@de , "Comandarm (Russia)"@it , "Comandarm (Rusland)"@nl , "Komandarm av 1. klasseKomandarm av 2. klasse (Russland)"@no , "Komandarm (Rosja)"@pl , "Comandarm (Rússia)"@pt , "Comandarm (Россия)"@ru , "Comandarm (Rusia)"@es ;
	rdfs:comment "The specific instance of the Comandarm rank in the context of country Russia."@en ;
	owl:rankOf <dbpedia:Russia> .

:Rank_Comandarm_Soviet_Union a :MilitaryRank ;
	owl:subClass :Rank_Comandarm ;
	foaf:name "Comandarm"@en ;
	rdfs:label "Comandarm (Soviet Union)"@en , "Comandarm (Sovjetunionen)"@sv , "Comandarm (Neuvostoliitto)"@fi , "Comandarm (Union des républiques socialistes soviétiques)"@fr , "Sowjetische GeneralsrängeKomandarm (Sowjetunion)"@de , "Comandarm (Unione Sovietica)"@it , "Comandarm (Sovjet-Unie)"@nl , "Komandarm av 1. klasseKomandarm av 2. klasse (Sovjetunionen)"@no , "Komandarm (Związek Socjalistycznych Republik Radzieckich)"@pl , "Comandarm (União Soviética)"@pt , "Comandarm (Союз Советских Социалистических Республик)"@ru , "Comandarm (Unión Soviética)"@es ;
	rdfs:comment "The specific instance of the Comandarm rank in the context of country Soviet Union."@en ;
	owl:rankOf <dbpedia:Soviet_Union> .

<http://rdf.muninn-project.org/ontologies/military#Rank_Combat_%28military_rank%29_Russia> a :MilitaryRank ;
	owl:subClass <http://rdf.muninn-project.org/ontologies/military#Rank_Combat_%28military_rank%29> ;
	foaf:name "Combat"@en ;
	rdfs:label "Combat (military rank) (Russia)"@en , "Combat (military rank) (Ryssland)"@sv , "Combat (military rank) (Venäjä)"@fi , "Combat (military rank) (Russie)"@fr , "Combat (military rank) (Russland)"@de , "Combat (military rank) (Russia)"@it , "Combat (military rank) (Rusland)"@nl , "Combat (military rank) (Russland)"@no , "Combat (military rank) (Rosja)"@pl , "Combat (military rank) (Rússia)"@pt , "Combat (military rank) (Россия)"@ru , "Combat (military rank) (Rusia)"@es ;
	rdfs:comment "The specific instance of the Combat (military rank) rank in the context of country Russia."@en ;
	owl:rankOf <dbpedia:Russia> .

<http://rdf.muninn-project.org/ontologies/military#Rank_Combat_%28military_rank%29_Soviet_Union> a :MilitaryRank ;
	owl:subClass <http://rdf.muninn-project.org/ontologies/military#Rank_Combat_%28military_rank%29> ;
	foaf:name "Combat"@en ;
	rdfs:label "Combat (military rank) (Soviet Union)"@en , "Combat (military rank) (Sovjetunionen)"@sv , "Combat (military rank) (Neuvostoliitto)"@fi , "Combat (military rank) (Union des républiques socialistes soviétiques)"@fr , "Combat (military rank) (Sowjetunion)"@de , "Combat (military rank) (Unione Sovietica)"@it , "Combat (military rank) (Sovjet-Unie)"@nl , "Combat (military rank) (Sovjetunionen)"@no , "Combat (military rank) (Związek Socjalistycznych Republik Radzieckich)"@pl , "Combat (military rank) (União Soviética)"@pt , "Combat (military rank) (Союз Советских Социалистических Республик)"@ru , "Combat (military rank) (Unión Soviética)"@es ;
	rdfs:comment "The specific instance of the Combat (military rank) rank in the context of country Soviet Union."@en ;
	owl:rankOf <dbpedia:Soviet_Union> .

:Rank_Combrig_Russia a :MilitaryRank ;
	owl:subClass :Rank_Combrig ;
	foaf:name "Комбриг"@ru ;
	rdfs:label "Combrig (Russia)"@en , "Combrig (Ryssland)"@sv , "Prikaatinkomentaja (Venäjä)"@fi , "Combrig (Russie)"@fr , "Kombrig (Russland)"@de , "Kombrig (Russia)"@it , "Combrig (Rusland)"@nl , "Combrig (Russland)"@no , "Kombrig (Rosja)"@pl , "Combrig (Rússia)"@pt , "Комбриг (Россия)"@ru , "Kombrig (Rusia)"@es ;
	rdfs:comment "The specific instance of the Combrig rank in the context of country Russia."@en ;
	owl:rankOf <dbpedia:Russia> .

:Rank_Combrig_Soviet_Union a :MilitaryRank ;
	owl:subClass :Rank_Combrig ;
	foaf:name "Combrig"@en ;
	rdfs:label "Combrig (Soviet Union)"@en , "Combrig (Sovjetunionen)"@sv , "Prikaatinkomentaja (Neuvostoliitto)"@fi , "Combrig (Union des républiques socialistes soviétiques)"@fr , "Kombrig (Sowjetunion)"@de , "Kombrig (Unione Sovietica)"@it , "Combrig (Sovjet-Unie)"@nl , "Combrig (Sovjetunionen)"@no , "Kombrig (Związek Socjalistycznych Republik Radzieckich)"@pl , "Combrig (União Soviética)"@pt , "Комбриг (Союз Советских Социалистических Республик)"@ru , "Kombrig (Unión Soviética)"@es ;
	rdfs:comment "The specific instance of the Combrig rank in the context of country Soviet Union."@en ;
	owl:rankOf <dbpedia:Soviet_Union> .

:Rank_Comcor_Russia a :MilitaryRank ;
	owl:subClass :Rank_Comcor ;
	foaf:name "Комкор"@ru ;
	rdfs:label "Comcor (Russia)"@en , "Comcor (Ryssland)"@sv , "Armeijakunnankomentaja (Venäjä)"@fi , "Comcor (Russie)"@fr , "Komkor (Russland)"@de , "Comcor (Russia)"@it , "Comcor (Rusland)"@nl , "Komkor (Russland)"@no , "Komkor (Rosja)"@pl , "Comcor (Rússia)"@pt , "Комкор (Россия)"@ru , "Komkor (Rusia)"@es ;
	rdfs:comment "The specific instance of the Comcor rank in the context of country Russia."@en ;
	owl:rankOf <dbpedia:Russia> .

:Rank_Comcor_Soviet_Union a :MilitaryRank ;
	owl:subClass :Rank_Comcor ;
	foaf:name "Comcor"@en ;
	rdfs:label "Comcor (Soviet Union)"@en , "Comcor (Sovjetunionen)"@sv , "Armeijakunnankomentaja (Neuvostoliitto)"@fi , "Comcor (Union des républiques socialistes soviétiques)"@fr , "Komkor (Sowjetunion)"@de , "Comcor (Unione Sovietica)"@it , "Comcor (Sovjet-Unie)"@nl , "Komkor (Sovjetunionen)"@no , "Komkor (Związek Socjalistycznych Republik Radzieckich)"@pl , "Comcor (União Soviética)"@pt , "Комкор (Союз Советских Социалистических Республик)"@ru , "Komkor (Unión Soviética)"@es ;
	rdfs:comment "The specific instance of the Comcor rank in the context of country Soviet Union."@en ;
	owl:rankOf <dbpedia:Soviet_Union> .

:Rank_Comdiv_Russia a :MilitaryRank ;
	owl:subClass :Rank_Comdiv ;
	foaf:name "Комдив"@ru ;
	rdfs:label "Comdiv (Russia)"@en , "Comdiv (Ryssland)"@sv , "Divisioonankomentaja (Venäjä)"@fi , "Comdiv (Russie)"@fr , "Komdiv (Russland)"@de , "Comdiv (Russia)"@it , "Comdiv (Rusland)"@nl , "Komdiv (Russland)"@no , "Komdiw (Rosja)"@pl , "Comdiv (Rússia)"@pt , "Комдив (Россия)"@ru , "Komdiv (Rusia)"@es ;
	rdfs:comment "The specific instance of the Comdiv rank in the context of country Russia."@en ;
	owl:rankOf <dbpedia:Russia> .

:Rank_Comdiv_Soviet_Union a :MilitaryRank ;
	owl:subClass :Rank_Comdiv ;
	foaf:name "Comdiv"@en ;
	rdfs:label "Comdiv (Soviet Union)"@en , "Comdiv (Sovjetunionen)"@sv , "Divisioonankomentaja (Neuvostoliitto)"@fi , "Comdiv (Union des républiques socialistes soviétiques)"@fr , "Komdiv (Sowjetunion)"@de , "Comdiv (Unione Sovietica)"@it , "Comdiv (Sovjet-Unie)"@nl , "Komdiv (Sovjetunionen)"@no , "Komdiw (Związek Socjalistycznych Republik Radzieckich)"@pl , "Comdiv (União Soviética)"@pt , "Комдив (Союз Советских Социалистических Республик)"@ru , "Komdiv (Unión Soviética)"@es ;
	rdfs:comment "The specific instance of the Comdiv rank in the context of country Soviet Union."@en ;
	owl:rankOf <dbpedia:Soviet_Union> .

<http://rdf.muninn-project.org/ontologies/military#Rank_Commandant_%28rank%29_France> a :MilitaryRank ;
	owl:subClass <http://rdf.muninn-project.org/ontologies/military#Rank_Commandant_%28rank%29> ;
	foaf:name "Commandant"@en ;
	rdfs:label "Commandant (rank) (France)"@en ;
	rdfs:comment "The specific instance of the Commandant (rank) rank in the context of France."@en ;
	owl:rankOf <dbpedia:France> .

<http://rdf.muninn-project.org/ontologies/military#Rank_Commandant_%28rank%29_Republic_of_Ireland> a :MilitaryRank ;
	owl:subClass <http://rdf.muninn-project.org/ontologies/military#Rank_Commandant_%28rank%29> ;
	foaf:name "Commandant"@en ;
	rdfs:label "Commandant (rank) (Republic of Ireland)"@en , "Commandant (rank) (Irland)"@sv , "Commandant (rank) (Irlanti)"@fi , "Commandant (rank) (Irlande (pays))"@fr , "Commandant (rank) (Irland)"@de , "Commandant (rank) (Irlanda)"@it , "Commandant (rank) (Ierland (land))"@nl , "Commandant (rank) (Irland)"@no , "Commandant (rank) (Irlandia)"@pl , "Commandant (rank) (República da Irlanda)"@pt , "Commandant (rank) (Ирландия)"@ru , "Commandant (rank) (Irlanda)"@es ;
	rdfs:comment "The specific instance of the Commandant (rank) rank in the context of country Republic of Ireland."@en ;
	owl:rankOf <dbpedia:Republic_of_Ireland> .

<dbpedia:Republic_of_Ireland> muninn:wikipedia_version "498350287" .

:Rank_Commandeur_France a :MilitaryRank ;
	owl:subClass :Rank_Commandeur ;
	foaf:name "Commandeur"@fr ;
	rdfs:label "Commandeur (France)"@en , "Commandeur (France)"@fr , "Commandeur (marine, France)"@nl ;
	rdfs:comment "The specific instance of the Commandeur rank in the context of France."@en ;
	owl:rankOf <dbpedia:France> .

:Rank_Commandeur_Netherlands a :MilitaryRank ;
	owl:subClass :Rank_Commandeur ;
	foaf:name "Commandeur"@en , "Commandeur"@nl ;
	rdfs:label "Commandeur (Netherlands)"@en , "Commandeur (Nederländerna)"@sv , "Commandeur (Alankomaat)"@fi , "Commandeur (Pays-Bas)"@fr , "Commandeur (Niederlande)"@de , "Commandeur (Paesi Bassi)"@it , "Commandeur (marine) (Nederland)"@nl , "Commandeur (Nederland)"@no , "Commandeur (Holandia)"@pl , "Commandeur (Países Baixos)"@pt , "Commandeur (Нидерланды)"@ru , "Commandeur (Países Bajos)"@es ;
	rdfs:comment "The specific instance of the Commandeur rank in the context of country Netherlands."@en ;
	owl:rankOf <dbpedia:Netherlands> .

<dbpedia:Netherlands> muninn:wikipedia_version "498374388" .

:Rank_Daejang_North_Korea a :MilitaryRank ;
	owl:subClass :Rank_Daejang ;
	foaf:name "Daejang"@en ;
	rdfs:label "Daejang (North Korea)"@en , "Daejang (Nordkorea)"@sv , "Daejang (Korean demokraattinen kansantasavalta)"@fi , "Daejang (Corée du Nord)"@fr , "Daejang (Nordkorea)"@de , "Daejang (Corea del Nord)"@it , "Daejang (Noord-Korea)"@nl , "Daejang (Nord-Korea)"@no , "Daejang (Korea Północna)"@pl , "Daejang (Coreia do Norte)"@pt , "Daejang (Корейская Народно-Демократическая Республика)"@ru , "Daejang (Corea del Norte)"@es ;
	rdfs:comment "The specific instance of the Daejang rank in the context of country North Korea."@en ;
	owl:rankOf <dbpedia:North_Korea> .

<dbpedia:North_Korea> muninn:wikipedia_version "498359658" .

:Rank_Daejang_South_Korea a :MilitaryRank ;
	owl:subClass :Rank_Daejang ;
	foaf:name "Daejang"@en ;
	rdfs:label "Daejang (South Korea)"@en , "Daejang (Sydkorea)"@sv , "Daejang (Korean tasavalta)"@fi , "Daejang (Corée du Sud)"@fr , "Daejang (Südkorea)"@de , "Daejang (Corea del Sud)"@it , "Daejang (Zuid-Korea)"@nl , "Daejang (Sør-Korea)"@no , "Daejang (Korea Południowa)"@pl , "Daejang (Coreia do Sul)"@pt , "Daejang (Республика Корея)"@ru , "Daejang (Corea del Sur)"@es ;
	rdfs:comment "The specific instance of the Daejang rank in the context of country South Korea."@en ;
	owl:rankOf <dbpedia:South_Korea> .

<dbpedia:South_Korea> muninn:wikipedia_version "498171765" .

:Rank_Divisional_Admiral_Italy a :MilitaryRank ;
	owl:subClass :Rank_Divisional_Admiral ;
	foaf:name "Ammiraglio di divisione"@it ;
	rdfs:label "Divisional Admiral (Italy)"@en , "Divisional Admiral (Italien)"@sv , "Divisional Admiral (Italia)"@fi , "Amiral de division (Italie)"@fr , "Divisional Admiral (Italien)"@de , "Ammiraglio di divisione (Italia)"@it , "Divisieadmiraal (Italië)"@nl , "Divisional Admiral (Italia)"@no , "Divisional Admiral (Włochy)"@pl , "Divisional Admiral (Itália)"@pt , "Divisional Admiral (Италия)"@ru , "Divisional Admiral (Italia)"@es ;
	rdfs:comment "The specific instance of the Divisional Admiral rank in the context of country Italy."@en ;
	owl:rankOf <dbpedia:Italy> .

:Rank_Divisional_Admiral_Belgium a :MilitaryRank ;
	owl:subClass :Rank_Divisional_Admiral ;
	foaf:name "Amiral de division"@fr , "Divisieadmiraal"@nl ;
	rdfs:label "Divisional Admiral (Belgium)"@en , "Divisional Admiral (Belgien)"@sv , "Divisional Admiral (Belgia)"@fi , "Amiral de division (Belgique)"@fr , "Divisional Admiral (Belgien)"@de , "Ammiraglio di divisione (Belgio)"@it , "Divisieadmiraal (België)"@nl , "Divisional Admiral (Belgia)"@no , "Divisional Admiral (Belgia)"@pl , "Divisional Admiral (Bélgica)"@pt , "Divisional Admiral (Бельгия)"@ru , "Divisional Admiral (Bélgica)"@es ;
	rdfs:comment "The specific instance of the Divisional Admiral rank in the context of country Belgium."@en ;
	owl:rankOf <dbpedia:Belgium> .

<dbpedia:Belgium> muninn:wikipedia_version "498001232" .

:Rank_Divisional_General_France a :MilitaryRank ;
	owl:subClass :Rank_Divisional_General ;
	foaf:name "Général de division"@fr ;
	rdfs:label "Divisional General (France)"@en , "Divisioonakenraali (France)"@fi , "Général de division (France)"@fr , "Generale di divisione (France)"@it , "General de divisão (France)"@pt ;
	rdfs:comment "The specific instance of the Divisional General rank in the context of France."@en ;
	owl:rankOf <dbpedia:France> .

:Rank_Divisional_General_Poland a :MilitaryRank ;
	owl:subClass :Rank_Divisional_General ;
	foaf:name "Divisional General"@en ;
	rdfs:label "Divisional General (Poland)"@en , "Divisioonakenraali (Poland)"@fi , "Général de division (Poland)"@fr , "Generale di divisione (Poland)"@it , "General de divisão (Poland)"@pt ;
	rdfs:comment "The specific instance of the Divisional General rank in the context of Poland."@en ;
	owl:rankOf <dbpedia:Poland> .

<dbpedia:Poland> muninn:wikipedia_version "497868027" .

<http://rdf.muninn-project.org/ontologies/military#Rank_Driver_%28rank%29_Australia> a :MilitaryRank ;
	owl:subClass <http://rdf.muninn-project.org/ontologies/military#Rank_Driver_%28rank%29> ;
	foaf:name "Driver"@en ;
	rdfs:label "Driver (rank) (Australia)"@en , "Driver (rank) (Australien)"@sv , "Driver (rank) (Australia)"@fi , "Driver (rank) (Australie)"@fr , "Driver (rank) (Australien)"@de , "Driver (rank) (Australia)"@it , "Driver (rank) (Australië (land))"@nl , "Driver (rank) (Australia)"@no , "Driver (rank) (Australia)"@pl , "Driver (rank) (Austrália)"@pt , "Driver (rank) (Австралия)"@ru , "Driver (rank) (Australia)"@es ;
	rdfs:comment "The specific instance of the Driver (rank) rank in the context of country Australia."@en ;
	owl:rankOf <dbpedia:Australia> .

<http://rdf.muninn-project.org/ontologies/military#Rank_Driver_%28rank%29_Canada> a :MilitaryRank ;
	owl:subClass <http://rdf.muninn-project.org/ontologies/military#Rank_Driver_%28rank%29> ;
	foaf:name "Driver"@en ;
	rdfs:label "Driver (rank, Canada)"@en ;
	rdfs:comment "The specific instance of the Driver (rank) rank in the context of Canada."@en ;
	owl:rankOf <dbpedia:Canada> .

<http://rdf.muninn-project.org/ontologies/military#Rank_Epihipparch_Macedonia_%28ancient_kingdom%29> a :MilitaryRank ;
	owl:subClass :Rank_Epihipparch ;
	foaf:name "Epihipparch"@en ;
	rdfs:label "Epihipparch (Macedonia (ancient kingdom))"@en , "Epihipparch (Makedonian valtakunta)"@fi , "Epihipparch (Royaume de Macédoine)"@fr , "Epihipparch (Regno di Macedonia)"@it , "Epihipparch (Macedonië (oudheid))"@nl , "Epihipparch (Oldtidens Makedonia)"@no , "Epihipparch (Starożytna Macedonia)"@pl , "Epihipparch (Macedónia Antiga)"@pt , "Epihipparch (Древняя Македония)"@ru , "Epihipparch (Reino de Macedonia)"@es ;
	rdfs:comment "The specific instance of the Epihipparch rank in the context of country Macedonia (ancient kingdom)."@en ;
	owl:rankOf <dbpedia:Macedonia_%28ancient_kingdom%29> .

<dbpedia:Macedonia_%28ancient_kingdom%29> muninn:wikipedia_version "495202996" .

:Rank_Epihipparch_Achaean_League a :MilitaryRank ;
	owl:subClass :Rank_Epihipparch ;
	foaf:name "Epihipparch"@en ;
	rdfs:label "Epihipparch (Achaean League)"@en , "Epihipparch (Achaiska förbundet)"@sv , "Epihipparch (Akhaian liitto)"@fi , "Epihipparch (Ligue achéenne)"@fr , "Epihipparch (Achaiischer Bund)"@de , "Epihipparch (Lega achea)"@it , "Epihipparch (Achaeïsche Bond)"@nl , "Epihipparch (Det akhaiske forbund)"@no , "Epihipparch (Związek Achajski)"@pl , "Epihipparch (Liga Aqueia)"@pt , "Epihipparch (Ахейский союз)"@ru , "Epihipparch (Liga Aquea)"@es ;
	rdfs:comment "The specific instance of the Epihipparch rank in the context of country Achaean League."@en ;
	owl:rankOf <dbpedia:Achaean_League> .

<dbpedia:Achaean_League> muninn:wikipedia_version "497254384" .

:Rank_General-in-Chief_Russia a :MilitaryRank ;
	owl:subClass :Rank_General-in-Chief ;
	foaf:name "Генерал-аншеф"@ru ;
	rdfs:label "General-in-Chief (Russia)"@en , "General en chef (Ryssland)"@sv , "General-in-Chief (Venäjä)"@fi , "General-in-Chief (Russie)"@fr , "General-in-Chief (Russland)"@de , "General-in-Chief (Russia)"@it , "General-in-Chief (Rusland)"@nl , "General-in-Chief (Russland)"@no , "General-in-Chief (Rosja)"@pl , "General-in-Chief (Rússia)"@pt , "Генерал-аншеф (Россия)"@ru , "General-in-Chief (Rusia)"@es ;
	rdfs:comment "The specific instance of the General-in-Chief rank in the context of country Russia."@en ;
	owl:rankOf <dbpedia:Russia> .

:Rank_General-in-Chief_Soviet_Union a :MilitaryRank ;
	owl:subClass :Rank_General-in-Chief ;
	foaf:name "General-in-Chief"@en ;
	rdfs:label "General-in-Chief (Soviet Union)"@en , "General en chef (Sovjetunionen)"@sv , "General-in-Chief (Neuvostoliitto)"@fi , "General-in-Chief (Union des républiques socialistes soviétiques)"@fr , "General-in-Chief (Sowjetunion)"@de , "General-in-Chief (Unione Sovietica)"@it , "General-in-Chief (Sovjet-Unie)"@nl , "General-in-Chief (Sovjetunionen)"@no , "General-in-Chief (Związek Socjalistycznych Republik Radzieckich)"@pl , "General-in-Chief (União Soviética)"@pt , "Генерал-аншеф (Союз Советских Социалистических Республик)"@ru , "General-in-Chief (Unión Soviética)"@es ;
	rdfs:comment "The specific instance of the General-in-Chief rank in the context of country Soviet Union."@en ;
	owl:rankOf <dbpedia:Soviet_Union> .

<http://rdf.muninn-project.org/ontologies/military#Rank_Hasa_%28Korean_military%29_North_Korea> a :MilitaryRank ;
	owl:subClass <http://rdf.muninn-project.org/ontologies/military#Rank_Hasa_%28Korean_military%29> ;
	foaf:name "Hasa"@en ;
	rdfs:label "Hasa (Korean military) (North Korea)"@en , "Hasa (Korean military) (Nordkorea)"@sv , "Hasa (Korean military) (Korean demokraattinen kansantasavalta)"@fi , "Hasa (Korean military) (Corée du Nord)"@fr , "Hasa (Korean military) (Nordkorea)"@de , "Hasa (Korean military) (Corea del Nord)"@it , "Hasa (Korean military) (Noord-Korea)"@nl , "Hasa (Korean military) (Nord-Korea)"@no , "Hasa (Korean military) (Korea Północna)"@pl , "Hasa (Korean military) (Coreia do Norte)"@pt , "Hasa (Korean military) (Корейская Народно-Демократическая Республика)"@ru , "Hasa (Korean military) (Corea del Norte)"@es ;
	rdfs:comment "The specific instance of the Hasa (Korean military) rank in the context of country North Korea."@en ;
	owl:rankOf <dbpedia:North_Korea> .

<http://rdf.muninn-project.org/ontologies/military#Rank_Hasa_%28Korean_military%29_South_Korea> a :MilitaryRank ;
	owl:subClass <http://rdf.muninn-project.org/ontologies/military#Rank_Hasa_%28Korean_military%29> ;
	foaf:name "Hasa"@en ;
	rdfs:label "Hasa (Korean military) (South Korea)"@en , "Hasa (Korean military) (Sydkorea)"@sv , "Hasa (Korean military) (Korean tasavalta)"@fi , "Hasa (Korean military) (Corée du Sud)"@fr , "Hasa (Korean military) (Südkorea)"@de , "Hasa (Korean military) (Corea del Sud)"@it , "Hasa (Korean military) (Zuid-Korea)"@nl , "Hasa (Korean military) (Sør-Korea)"@no , "Hasa (Korean military) (Korea Południowa)"@pl , "Hasa (Korean military) (Coreia do Sul)"@pt , "Hasa (Korean military) (Республика Корея)"@ru , "Hasa (Korean military) (Corea del Sur)"@es ;
	rdfs:comment "The specific instance of the Hasa (Korean military) rank in the context of country South Korea."@en ;
	owl:rankOf <dbpedia:South_Korea> .

<http://rdf.muninn-project.org/ontologies/military#Rank_Hipparchus_%28cavalry_officer%29_Macedonia_%28ancient_kingdom%29> a :MilitaryRank ;
	owl:subClass <http://rdf.muninn-project.org/ontologies/military#Rank_Hipparchus_%28cavalry_officer%29> ;
	foaf:name "Hipparchus"@en ;
	rdfs:label "Hipparchus (cavalry officer) (Macedonia (ancient kingdom))"@en , "Hipparchus (cavalry officer) (Makedonian valtakunta)"@fi , "Hipparchus (cavalry officer) (Royaume de Macédoine)"@fr , "Hipparchus (cavalry officer) (Regno di Macedonia)"@it , "Hipparchos (Macedonië (oudheid))"@nl , "Hipparchus (cavalry officer) (Oldtidens Makedonia)"@no , "Hipparchus (cavalry officer) (Starożytna Macedonia)"@pl , "Hipparchus (cavalry officer) (Macedónia Antiga)"@pt , "Гиппарх (военачальник) (Древняя Македония)"@ru , "Hiparco (oficial de caballería) (Reino de Macedonia)"@es ;
	rdfs:comment "The specific instance of the Hipparchus (cavalry officer) rank in the context of country Macedonia (ancient kingdom)."@en ;
	owl:rankOf <dbpedia:Macedonia_%28ancient_kingdom%29> .

<http://rdf.muninn-project.org/ontologies/military#Rank_Hipparchus_%28cavalry_officer%29_Achaean_League> a :MilitaryRank ;
	owl:subClass <http://rdf.muninn-project.org/ontologies/military#Rank_Hipparchus_%28cavalry_officer%29> ;
	foaf:name "Hipparchus"@en ;
	rdfs:label "Hipparchus (cavalry officer) (Achaean League)"@en , "Hipparchus (cavalry officer) (Achaiska förbundet)"@sv , "Hipparchus (cavalry officer) (Akhaian liitto)"@fi , "Hipparchus (cavalry officer) (Ligue achéenne)"@fr , "Hipparchus (cavalry officer) (Achaiischer Bund)"@de , "Hipparchus (cavalry officer) (Lega achea)"@it , "Hipparchos (Achaeïsche Bond)"@nl , "Hipparchus (cavalry officer) (Det akhaiske forbund)"@no , "Hipparchus (cavalry officer) (Związek Achajski)"@pl , "Hipparchus (cavalry officer) (Liga Aqueia)"@pt , "Гиппарх (военачальник) (Ахейский союз)"@ru , "Hiparco (oficial de caballería) (Liga Aquea)"@es ;
	rdfs:comment "The specific instance of the Hipparchus (cavalry officer) rank in the context of country Achaean League."@en ;
	owl:rankOf <dbpedia:Achaean_League> .

:Rank_Jungsa_North_Korea a :MilitaryRank ;
	owl:subClass :Rank_Jungsa ;
	foaf:name "Jungsa"@en ;
	rdfs:label "Jungsa (North Korea)"@en , "Jungsa (Nordkorea)"@sv , "Jungsa (Korean demokraattinen kansantasavalta)"@fi , "Jungsa (Corée du Nord)"@fr , "Jungsa (Nordkorea)"@de , "Jungsa (Corea del Nord)"@it , "Jungsa (Noord-Korea)"@nl , "Jungsa (Nord-Korea)"@no , "Jungsa (Korea Północna)"@pl , "Jungsa (Coreia do Norte)"@pt , "Jungsa (Корейская Народно-Демократическая Республика)"@ru , "Jungsa (Corea del Norte)"@es ;
	rdfs:comment "The specific instance of the Jungsa rank in the context of country North Korea."@en ;
	owl:rankOf <dbpedia:North_Korea> .

:Rank_Jungsa_South_Korea a :MilitaryRank ;
	owl:subClass :Rank_Jungsa ;
	foaf:name "Jungsa"@en ;
	rdfs:label "Jungsa (South Korea)"@en , "Jungsa (Sydkorea)"@sv , "Jungsa (Korean tasavalta)"@fi , "Jungsa (Corée du Sud)"@fr , "Jungsa (Südkorea)"@de , "Jungsa (Corea del Sud)"@it , "Jungsa (Zuid-Korea)"@nl , "Jungsa (Sør-Korea)"@no , "Jungsa (Korea Południowa)"@pl , "Jungsa (Coreia do Sul)"@pt , "Jungsa (Республика Корея)"@ru , "Jungsa (Corea del Sur)"@es ;
	rdfs:comment "The specific instance of the Jungsa rank in the context of country South Korea."@en ;
	owl:rankOf <dbpedia:South_Korea> .

:Rank_Jungwi_North_Korea a :MilitaryRank ;
	owl:subClass :Rank_Jungwi ;
	foaf:name "Jungwi"@en ;
	rdfs:label "Jungwi (North Korea)"@en , "Jungwi (Nordkorea)"@sv , "Jungwi (Korean demokraattinen kansantasavalta)"@fi , "Jungwi (Corée du Nord)"@fr , "Jungwi (Nordkorea)"@de , "Jungwi (Corea del Nord)"@it , "Jungwi (Noord-Korea)"@nl , "Jungwi (Nord-Korea)"@no , "Jungwi (Korea Północna)"@pl , "Jungwi (Coreia do Norte)"@pt , "Jungwi (Корейская Народно-Демократическая Республика)"@ru , "Jungwi (Corea del Norte)"@es ;
	rdfs:comment "The specific instance of the Jungwi rank in the context of country North Korea."@en ;
	owl:rankOf <dbpedia:North_Korea> .

:Rank_Jungwi_South_Korea a :MilitaryRank ;
	owl:subClass :Rank_Jungwi ;
	foaf:name "Jungwi"@en ;
	rdfs:label "Jungwi (South Korea)"@en , "Jungwi (Sydkorea)"@sv , "Jungwi (Korean tasavalta)"@fi , "Jungwi (Corée du Sud)"@fr , "Jungwi (Südkorea)"@de , "Jungwi (Corea del Sud)"@it , "Jungwi (Zuid-Korea)"@nl , "Jungwi (Sør-Korea)"@no , "Jungwi (Korea Południowa)"@pl , "Jungwi (Coreia do Sul)"@pt , "Jungwi (Республика Корея)"@ru , "Jungwi (Corea del Sur)"@es ;
	rdfs:comment "The specific instance of the Jungwi rank in the context of country South Korea."@en ;
	owl:rankOf <dbpedia:South_Korea> .

:Rank_Junior_sergeant_Estonia a :MilitaryRank ;
	owl:subClass :Rank_Junior_sergeant ;
	foaf:name ""@en ;
	rdfs:label "(Estonia)"@en , "(Estland)"@sv , "(Viro)"@fi , "(Estonie)"@fr , "(Estland)"@de , "(Estonia)"@it , "(Estland)"@nl , "(Estland)"@no , "(Estonia)"@pl , "(Estónia)"@pt , "(Эстония)"@ru , "(Estonia)"@es ;
	rdfs:comment "The specific instance of the  rank in the context of country Estonia."@en ;
	owl:rankOf <dbpedia:Estonia> .

<dbpedia:Estonia> muninn:wikipedia_version "498355716" .

<http://rdf.muninn-project.org/ontologies/military#Rank_Junior_sergeant_Republic_of_Estonia_%281920-1940%29> a :MilitaryRank ;
	owl:subClass :Rank_Junior_sergeant ;
	foaf:name ""@en ;
	rdfs:comment "The specific instance of the  rank in the context of country ."@en ;
	owl:rankOf <dbpedia:Republic_of_Estonia_%281920-1940%29> .

:Rank_Junjang_North_Korea a :MilitaryRank ;
	owl:subClass :Rank_Junjang ;
	foaf:name "Junjang"@en ;
	rdfs:label "Junjang (North Korea)"@en , "Junjang (Nordkorea)"@sv , "Junjang (Korean demokraattinen kansantasavalta)"@fi , "Junjang (Corée du Nord)"@fr , "Junjang (Nordkorea)"@de , "Junjang (Corea del Nord)"@it , "Junjang (Noord-Korea)"@nl , "Junjang (Nord-Korea)"@no , "Junjang (Korea Północna)"@pl , "Junjang (Coreia do Norte)"@pt , "Junjang (Корейская Народно-Демократическая Республика)"@ru , "Junjang (Corea del Norte)"@es ;
	rdfs:comment "The specific instance of the Junjang rank in the context of country North Korea."@en ;
	owl:rankOf <dbpedia:North_Korea> .

:Rank_Junjang_South_Korea a :MilitaryRank ;
	owl:subClass :Rank_Junjang ;
	foaf:name "Junjang"@en ;
	rdfs:label "Junjang (South Korea)"@en , "Junjang (Sydkorea)"@sv , "Junjang (Korean tasavalta)"@fi , "Junjang (Corée du Sud)"@fr , "Junjang (Südkorea)"@de , "Junjang (Corea del Sud)"@it , "Junjang (Zuid-Korea)"@nl , "Junjang (Sør-Korea)"@no , "Junjang (Korea Południowa)"@pl , "Junjang (Coreia do Sul)"@pt , "Junjang (Республика Корея)"@ru , "Junjang (Corea del Sur)"@es ;
	rdfs:comment "The specific instance of the Junjang rank in the context of country South Korea."@en ;
	owl:rankOf <dbpedia:South_Korea> .

:Rank_Kindral_Estonia a :MilitaryRank ;
	owl:subClass :Rank_Kindral ;
	foaf:name "Kindral"@en ;
	rdfs:label "Kindral (Estonia)"@en , "Kindral (Estland)"@sv , "Kindral (Viro)"@fi , "Kindral (Estonie)"@fr , "Kindral (Estland)"@de , "Kindral (Estonia)"@it , "Kindral (Estland)"@nl , "Kindral (Estland)"@no , "Kindral (Estonia)"@pl , "Kindral (Estónia)"@pt , "Kindral (Эстония)"@ru , "Kindral (Estonia)"@es ;
	rdfs:comment "The specific instance of the Kindral rank in the context of country Estonia."@en ;
	owl:rankOf <dbpedia:Estonia> .

<http://rdf.muninn-project.org/ontologies/military#Rank_Kindral_Republic_of_Estonia_%281920-1940%29> a :MilitaryRank ;
	owl:subClass :Rank_Kindral ;
	foaf:name "Kindral"@en ;
	rdfs:label "Kindral (Republic of Estonia, 1920-1940)"@en ;
	rdfs:comment "The specific instance of the Kindral rank in the context of the Republic of Estonia, 1920-1940."@en ;
	owl:rankOf <dbpedia:Republic_of_Estonia_%281920-1940%29> .

:Rank_Major_general_Australia a :MilitaryRank ;
	owl:subClass :Rank_Major_general ;
	foaf:name "Major general"@en ;
	rdfs:label "Major general (Australia)"@en , "Major general (Australien)"@sv , "Major general (Australia)"@fi , "Major general (Australie)"@fr , "Major general (Australien)"@de , "Major general (Australia)"@it , "Major general (Australië (land))"@nl , "Major general (Australia)"@no , "Major general (Australia)"@pl , "Major general (Austrália)"@pt , "Major general (Австралия)"@ru , "Major general (Australia)"@es ;
	rdfs:comment "The specific instance of the Major general rank in the context of country Australia."@en ;
	owl:rankOf <dbpedia:Australia> .

:Rank_Major_general_Canada a :MilitaryRank ;
	owl:subClass :Rank_Major_general ;
	foaf:name "Major general"@en ;
	rdfs:label "Major general (Canada)"@en ;
	rdfs:comment "The specific instance of the Major general rank in the context of Canada."@en ;
	owl:rankOf <dbpedia:Canada> .

:Rank_Marshal_of_the_Soviet_Union_Soviet_Union a :MilitaryRank ;
	owl:subClass :Rank_Marshal_of_the_Soviet_Union ;
	foaf:name "Marshal of the Soviet Union"@en ;
	rdfs:label "Marshal of the Soviet Union (Soviet Union)"@en , "Marskalk av Sovjetunionen (Sovjetunionen)"@sv , "Neuvostoliiton marsalkka (Neuvostoliitto)"@fi , "Maréchal de l'Union soviétique (Union des républiques socialistes soviétiques)"@fr , "Marschall der Sowjetunion (Sowjetunion)"@de , "Maresciallo dell'Unione Sovietica (Unione Sovietica)"@it , "Maarschalk van de Sovjet-Unie (Sovjet-Unie)"@nl , "Marskalk av Sovjetunionen (Sovjetunionen)"@no , "Marszałkowie ZSRR (Związek Socjalistycznych Republik Radzieckich)"@pl , "Marechal da União Soviética (União Soviética)"@pt , "Маршал Советского Союза (Союз Советских Социалистических Республик)"@ru , "Mariscal de la Unión Soviética (Unión Soviética)"@es ;
	rdfs:comment "The specific instance of the Marshal of the Soviet Union rank in the context of country Soviet Union."@en ;
	owl:rankOf <dbpedia:Soviet_Union> .

:Rank_Master_warrant_officer_Canada a :MilitaryRank ;
	owl:subClass :Rank_Master_warrant_officer ;
	foaf:name "Master Warrant Officer"@en ;
	rdfs:label "Master Warrant Officer (Canada)"@en ;
	rdfs:comment "The specific instance of the  Master Warrant Officerrank in the context of country Canada."@en ;
	owl:rankOf <dbpedia:Canada> .

:Rank_Master_warrant_officer_Singapore a :MilitaryRank ;
	owl:subClass :Rank_Master_warrant_officer ;
	foaf:name "Master Warrant Officer"@en ;
	rdfs:label "Master Warrant Officer (Singapore)"@en , "Master Warrant Officer (Singapore)"@sv , "Master Warrant Officer (Singapore)"@fi , "Master Warrant Officer (Singapour)"@fr , "Master Warrant Officer (Singapur)"@de , "Master Warrant Officer (Singapore)"@it , "Master Warrant Officer (Singapore)"@nl , "Master Warrant Officer (Singapore)"@no , "Master Warrant Officer (Singapur)"@pl , "Master Warrant Officer (Singapura)"@pt , "Master Warrant Officer (Сингапур)"@ru , "Master Warrant Officer (Singapur)"@es ;
	rdfs:comment "The specific instance of the Master Warrant Officer rank in the context of country Singapore."@en ;
	owl:rankOf <dbpedia:Singapore> .

<dbpedia:Singapore> muninn:wikipedia_version "498300526" .

:Rank_Obergefreiter_Germany a :MilitaryRank ;
	owl:subClass :Rank_Obergefreiter ;
	foaf:name "Obergefreiter"@de ;
	rdfs:label "Obergefreiter (Germany)"@en , "Ylikorpraali (Germany)"@fi , "Obergefreiter (Germany)"@de ;
	rdfs:comment "The specific instance of the Obergefreiter rank in the context of Germany."@en ;
	owl:rankOf <dbpedia:Germany> .

:Rank_Obergefreiter_Switzerland a :MilitaryRank ;
	owl:subClass :Rank_Obergefreiter ;
	foaf:name "Obergefreiter"@de ;
	rdfs:label "Obergefreiter (Switzerland)"@en , "Obergefreiter (Schweiz)"@sv , "Ylikorpraali (Sveitsi)"@fi , "Obergefreiter (Suisse)"@fr , "Obergefreiter (Schweiz)"@de , "Obergefreiter (Svizzera)"@it , "Obergefreiter (Zwitserland)"@nl , "Obergefreiter (Sveits)"@no , "Obergefreiter (Szwajcaria)"@pl , "Obergefreiter (Suíça)"@pt , "Obergefreiter (Швейцария)"@ru , "Obergefreiter (Suiza)"@es ;
	rdfs:comment "The specific instance of the Obergefreiter rank in the context of country Switzerland."@en ;
	owl:rankOf <dbpedia:Switzerland> .

:Rank_Podpraporshchik_Russia a :MilitaryRank ;
	owl:subClass :Rank_Podpraporshchik ;
	foaf:name "Подпрапорщик"@ru ;
	rdfs:label "Podpraporshchik (Russia)"@en , "Podpraporshchik (Ryssland)"@sv , "Podpraporshchik (Venäjä)"@fi , "Podpraporshchik (Russie)"@fr , "Podpraporshchik (Russland)"@de , "Podpraporshchik (Russia)"@it , "Podpraporshchik (Rusland)"@nl , "Podpraporshchik (Russland)"@no , "Podpraporshchik (Rosja)"@pl , "Podpraporshchik (Rússia)"@pt , "Подпрапорщик (Россия)"@ru , "Podpraporshchik (Rusia)"@es ;
	rdfs:comment "The specific instance of the Podpraporshchik rank in the context of country Russia."@en ;
	owl:rankOf <dbpedia:Russia> .

:Rank_Podpraporshchik_Soviet_Union a :MilitaryRank ;
	owl:subClass :Rank_Podpraporshchik ;
	foaf:name "Podpraporshchik"@en ;
	rdfs:label "Podpraporshchik (Soviet Union)"@en , "Podpraporshchik (Sovjetunionen)"@sv , "Podpraporshchik (Neuvostoliitto)"@fi , "Podpraporshchik (Union des républiques socialistes soviétiques)"@fr , "Podpraporshchik (Sowjetunion)"@de , "Podpraporshchik (Unione Sovietica)"@it , "Podpraporshchik (Sovjet-Unie)"@nl , "Podpraporshchik (Sovjetunionen)"@no , "Podpraporshchik (Związek Socjalistycznych Republik Radzieckich)"@pl , "Podpraporshchik (União Soviética)"@pt , "Подпрапорщик (Союз Советских Социалистических Республик)"@ru , "Podpraporshchik (Unión Soviética)"@es ;
	rdfs:comment "The specific instance of the Podpraporshchik rank in the context of country Soviet Union."@en ;
	owl:rankOf <dbpedia:Soviet_Union> .

<http://rdf.muninn-project.org/ontologies/military#Rank_Polemarch_Macedonia_%28ancient_kingdom%29> a :MilitaryRank ;
	owl:subClass :Rank_Polemarch ;
	foaf:name "Polemarch"@en ;
	rdfs:label "Polemarch (Macedonia (ancient kingdom))"@en , "Polemark (Macedonia (ancient kingdom))"@sv , "Polemarch (Makedonian valtakunta)"@fi , "Polémarque (Royaume de Macédoine)"@fr , "Polemarch (Regno di Macedonia)"@it , "Polemarchos (Macedonië (oudheid))"@nl , "Polemarkos (Oldtidens Makedonia)"@no , "Polemarch (Starożytna Macedonia)"@pl , "Polemarco (Macedónia Antiga)"@pt , "Полемарх (Древняя Македония)"@ru , "Polemarca (Reino de Macedonia)"@es ;
	rdfs:comment "The specific instance of the Polemarch rank in the context of country Macedonia (ancient kingdom)."@en ;
	owl:rankOf <dbpedia:Macedonia_%28ancient_kingdom%29> .

:Rank_Polemarch_Achaean_League a :MilitaryRank ;
	owl:subClass :Rank_Polemarch ;
	foaf:name "Polemarch"@en ;
	rdfs:label "Polemarch (Achaean League)"@en , "Polemark (Achaiska förbundet)"@sv , "Polemarch (Akhaian liitto)"@fi , "Polémarque (Ligue achéenne)"@fr , "Polemarch (Achaiischer Bund)"@de , "Polemarch (Lega achea)"@it , "Polemarchos (Achaeïsche Bond)"@nl , "Polemarkos (Det akhaiske forbund)"@no , "Polemarch (Związek Achajski)"@pl , "Polemarco (Liga Aqueia)"@pt , "Полемарх (Ахейский союз)"@ru , "Polemarca (Liga Aquea)"@es ;
	rdfs:comment "The specific instance of the Polemarch rank in the context of country Achaean League."@en ;
	owl:rankOf <dbpedia:Achaean_League> .

:Rank_Praporshchik_Russia a :MilitaryRank ;
	owl:subClass :Rank_Praporshchik ;
	foaf:name "Прапорщик"@ru ;
	rdfs:label "Praporshchik (Russia)"@en , "Praporshchik (Ryssland)"@sv , "Praporshchik (Venäjä)"@fi , "Praporshchik (Russie)"@fr , "Praporshchik (Russland)"@de , "Praporshchik (Russia)"@it , "Praporshchik (Rusland)"@nl , "Praporshchik (Russland)"@no , "Praporshchik (Rosja)"@pl , "Praporshchik (Rússia)"@pt , "Прапорщик (Россия)"@ru , "Praporshchik (Rusia)"@es ;
	rdfs:comment "The specific instance of the Praporshchik rank in the context of country Russia."@en ;
	owl:rankOf <dbpedia:Russia> .

:Rank_Praporshchik_Soviet_Union a :MilitaryRank ;
	owl:subClass :Rank_Praporshchik ;
	foaf:name "Praporshchik"@en ;
	rdfs:label "Praporshchik (Soviet Union)"@en , "Praporshchik (Sovjetunionen)"@sv , "Praporshchik (Neuvostoliitto)"@fi , "Praporshchik (Union des républiques socialistes soviétiques)"@fr , "Praporshchik (Sowjetunion)"@de , "Praporshchik (Unione Sovietica)"@it , "Praporshchik (Sovjet-Unie)"@nl , "Praporshchik (Sovjetunionen)"@no , "Praporshchik (Związek Socjalistycznych Republik Radzieckich)"@pl , "Praporshchik (União Soviética)"@pt , "Прапорщик (Союз Советских Социалистических Республик)"@ru , "Praporshchik (Unión Soviética)"@es ;
	rdfs:comment "The specific instance of the Praporshchik rank in the context of country Soviet Union."@en ;
	owl:rankOf <dbpedia:Soviet_Union> .

:Rank_Rear_admiral_Australia a :MilitaryRank ;
	owl:subClass :Rank_Rear_admiral ;
	foaf:name "Rear admiral"@en ;
	rdfs:label "Rear admiral (Australia)"@en , "Rear admiral (Australien)"@sv , "Rear admiral (Australia)"@fi , "Rear admiral (Australie)"@fr , "Rear admiral (Australien)"@de , "Rear admiral (Australia)"@it , "Rear admiral (Australië (land))"@nl , "Rear admiral (Australia)"@no , "Rear admiral (Australia)"@pl , "Rear admiral (Austrália)"@pt , "Rear admiral (Австралия)"@ru , "Rear admiral (Australia)"@es ;
	rdfs:comment "The specific instance of the Rear admiral rank in the context of country Australia."@en ;
	owl:rankOf <dbpedia:Australia> .

:Rank_Rear_admiral_Canada a :MilitaryRank ;
	owl:subClass :Rank_Rear_admiral ;
	foaf:name "Rear admiral"@en ;
	rdfs:label "Rear admiral (Canada)"@en ;
	rdfs:comment "The specific instance of the Rear admiral rank in the context of Canada."@en ;
	owl:rankOf <dbpedia:Canada> .

:Rank_Sangsa_North_Korea a :MilitaryRank ;
	owl:subClass :Rank_Sangsa ;
	foaf:name "Sangsa"@en ;
	rdfs:label "Sangsa (North Korea)"@en , "Sangsa (Nordkorea)"@sv , "Sangsa (Korean demokraattinen kansantasavalta)"@fi , "Sangsa (Corée du Nord)"@fr , "Sangsa (Nordkorea)"@de , "Sangsa (Corea del Nord)"@it , "Sangsa (Noord-Korea)"@nl , "Sangsa (Nord-Korea)"@no , "Sangsa (Korea Północna)"@pl , "Sangsa (Coreia do Norte)"@pt , "Sangsa (Корейская Народно-Демократическая Республика)"@ru , "Sangsa (Corea del Norte)"@es ;
	rdfs:comment "The specific instance of the Sangsa rank in the context of country North Korea."@en ;
	owl:rankOf <dbpedia:North_Korea> .

:Rank_Sangsa_South_Korea a :MilitaryRank ;
	owl:subClass :Rank_Sangsa ;
	foaf:name "Sangsa"@en ;
	rdfs:label "Sangsa (South Korea)"@en , "Sangsa (Sydkorea)"@sv , "Sangsa (Korean tasavalta)"@fi , "Sangsa (Corée du Sud)"@fr , "Sangsa (Südkorea)"@de , "Sangsa (Corea del Sud)"@it , "Sangsa (Zuid-Korea)"@nl , "Sangsa (Sør-Korea)"@no , "Sangsa (Korea Południowa)"@pl , "Sangsa (Coreia do Sul)"@pt , "Sangsa (Республика Корея)"@ru , "Sangsa (Corea del Sur)"@es ;
	rdfs:comment "The specific instance of the Sangsa rank in the context of country South Korea."@en ;
	owl:rankOf <dbpedia:South_Korea> .

<http://rdf.muninn-project.org/ontologies/military#Rank_Skeuophoros_Macedonia_%28ancient_kingdom%29> a :MilitaryRank ;
	owl:subClass :Rank_Skeuophoros ;
	foaf:name "Skeuophoros"@en ;
	rdfs:label "Skeuophoros (Macedonia (ancient kingdom))"@en , "Skeuophoros (Makedonian valtakunta)"@fi , "Skeuophoros (Royaume de Macédoine)"@fr , "Skeuophoros (Regno di Macedonia)"@it , "Skeuophoros (Macedonië (oudheid))"@nl , "Skeuophoros (Oldtidens Makedonia)"@no , "Skeuophoros (Starożytna Macedonia)"@pl , "Skeuophoros (Macedónia Antiga)"@pt , "Skeuophoros (Древняя Македония)"@ru , "Skeuophoros (Reino de Macedonia)"@es ;
	rdfs:comment "The specific instance of the Skeuophoros rank in the context of country Macedonia (ancient kingdom)."@en ;
	owl:rankOf <dbpedia:Macedonia_%28ancient_kingdom%29> .

:Rank_Skeuophoros_Achaean_League a :MilitaryRank ;
	owl:subClass :Rank_Skeuophoros ;
	foaf:name "Skeuophoros"@en ;
	rdfs:label "Skeuophoros (Achaean League)"@en , "Skeuophoros (Achaiska förbundet)"@sv , "Skeuophoros (Akhaian liitto)"@fi , "Skeuophoros (Ligue achéenne)"@fr , "Skeuophoros (Achaiischer Bund)"@de , "Skeuophoros (Lega achea)"@it , "Skeuophoros (Achaeïsche Bond)"@nl , "Skeuophoros (Det akhaiske forbund)"@no , "Skeuophoros (Związek Achajski)"@pl , "Skeuophoros (Liga Aqueia)"@pt , "Skeuophoros (Ахейский союз)"@ru , "Skeuophoros (Liga Aquea)"@es ;
	rdfs:comment "The specific instance of the Skeuophoros rank in the context of country Achaean League."@en ;
	owl:rankOf <dbpedia:Achaean_League> .

:Rank_Somatophylakes_Achaean_League a :MilitaryRank ;
	owl:subClass :Rank_Somatophylakes ;
	foaf:name "Somatophylakes"@en ;
	rdfs:label "Somatophylakes (Achaean League)"@en , "Somatophylakes (Achaiska förbundet)"@sv , "Somatofylakes (Akhaian liitto)"@fi , "Sômatophylaques (Ligue achéenne)"@fr , "Somatophylakes (Achaiischer Bund)"@de , "Somatofilachie (Lega achea)"@it , "Somatophylax (Achaeïsche Bond)"@nl , "Somatophylakes (Det akhaiske forbund)"@no , "Somatophylakes (Związek Achajski)"@pl , "Somatophylakes (Liga Aqueia)"@pt , "Somatophylakes (Ахейский союз)"@ru , "Somatophylakes (Liga Aquea)"@es ;
	rdfs:comment "The specific instance of the Somatophylakes rank in the context of country Achaean League."@en ;
	owl:rankOf <dbpedia:Achaean_League> .

<http://rdf.muninn-project.org/ontologies/military#Rank_Somatophylakes_Macedonia_%28ancient_kingdom%29> a :MilitaryRank ;
	owl:subClass :Rank_Somatophylakes ;
	foaf:name "Somatophylakes"@en ;
	rdfs:label "Somatophylakes (Macedonia (ancient kingdom))"@en , "Somatofylakes (Makedonian valtakunta)"@fi , "Sômatophylaques (Royaume de Macédoine)"@fr , "Somatophylakes (Macedonia (ancient kingdom))"@de , "Somatofilachie (Regno di Macedonia)"@it , "Somatophylax (Macedonië (oudheid))"@nl , "Somatophylakes (Oldtidens Makedonia)"@no , "Somatophylakes (Starożytna Macedonia)"@pl , "Somatophylakes (Macedónia Antiga)"@pt , "Somatophylakes (Древняя Македония)"@ru , "Somatophylakes (Reino de Macedonia)"@es ;
	rdfs:comment "The specific instance of the Somatophylakes rank in the context of country Macedonia (ancient kingdom)."@en ;
	owl:rankOf <dbpedia:Macedonia_%28ancient_kingdom%29> .

:Rank_Sowi_North_Korea a :MilitaryRank ;
	owl:subClass :Rank_Sowi ;
	foaf:name "Sowi"@en ;
	rdfs:label "Sowi (North Korea)"@en , "Sowi (Nordkorea)"@sv , "Sowi (Korean demokraattinen kansantasavalta)"@fi , "Sowi (Corée du Nord)"@fr , "Sowi (Nordkorea)"@de , "Sowi (Corea del Nord)"@it , "Sowi (Noord-Korea)"@nl , "Sowi (Nord-Korea)"@no , "Sowi (Korea Północna)"@pl , "Sowi (Coreia do Norte)"@pt , "Sowi (Корейская Народно-Демократическая Республика)"@ru , "Sowi (Corea del Norte)"@es ;
	rdfs:comment "The specific instance of the Sowi rank in the context of country North Korea."@en ;
	owl:rankOf <dbpedia:North_Korea> .

:Rank_Sowi_South_Korea a :MilitaryRank ;
	owl:subClass :Rank_Sowi ;
	foaf:name "Sowi"@en ;
	rdfs:label "Sowi (South Korea)"@en , "Sowi (Sydkorea)"@sv , "Sowi (Korean tasavalta)"@fi , "Sowi (Corée du Sud)"@fr , "Sowi (Südkorea)"@de , "Sowi (Corea del Sud)"@it , "Sowi (Zuid-Korea)"@nl , "Sowi (Sør-Korea)"@no , "Sowi (Korea Południowa)"@pl , "Sowi (Coreia do Sul)"@pt , "Sowi (Республика Корея)"@ru , "Sowi (Corea del Sur)"@es ;
	rdfs:comment "The specific instance of the Sowi rank in the context of country South Korea."@en ;
	owl:rankOf <dbpedia:South_Korea> .

:Rank_Staabikapten_Estonia a :MilitaryRank ;
	owl:subClass :Rank_Staabikapten ;
	foaf:name "Staabikapten"@en ;
	rdfs:label "Staabikapten (Estonia)"@en , "Staabikapten (Estland)"@sv , "Staabikapten (Viro)"@fi , "Staabikapten (Estonie)"@fr , "Staabikapten (Estland)"@de , "Staabikapten (Estonia)"@it , "Staabikapten (Estland)"@nl , "Staabikapten (Estland)"@no , "Staabikapten (Estonia)"@pl , "Staabikapten (Estónia)"@pt , "Staabikapten (Эстония)"@ru , "Staabikapten (Estonia)"@es ;
	rdfs:comment "The specific instance of the Staabikapten rank in the context of country Estonia."@en ;
	owl:rankOf <dbpedia:Estonia> .

<http://rdf.muninn-project.org/ontologies/military#Rank_Staabikapten_Republic_of_Estonia_%281920-1940%29> a :MilitaryRank ;
	owl:subClass :Rank_Staabikapten ;
	foaf:name "Staabikapten"@en ;
	rdfs:label "Staabikapten (Republic of Estonia, 1920-1940)"@en ;
	rdfs:comment "The specific instance of the Staabikapten rank in the context of the Republic of Estonia, 1920-1940."@en ;
	owl:rankOf <dbpedia:Republic_of_Estonia_%281920-1940%29> .

:Rank_Tetrarch_Achaean_League a :MilitaryRank ;
	owl:subClass :Rank_Tetrarch ;
	foaf:name "Tetrarch"@en ;
	rdfs:label "Tetrarch (Achaean League)"@en , "Tetrark (Achaiska förbundet)"@sv , "Tetrarkki (Akhaian liitto)"@fi , "Tetrarch (Ligue achéenne)"@fr , "Tetrarch (Achaiischer Bund)"@de , "Tetrarch (Lega achea)"@it , "Tetrarch (Achaeïsche Bond)"@nl , "Tetrarch (Det akhaiske forbund)"@no , "Tetrarch (Związek Achajski)"@pl , "Tetrarca (Liga Aqueia)"@pt , "Тетрарх (значения) (Ахейский союз)"@ru , "Tetrarch (Liga Aquea)"@es ;
	rdfs:comment "The specific instance of the Tetrarch rank in the context of country Achaean League."@en ;
	owl:rankOf <dbpedia:Achaean_League> .

<http://rdf.muninn-project.org/ontologies/military#Rank_Tetrarch_Macedonia_%28ancient_kingdom%29> a :MilitaryRank ;
	owl:subClass :Rank_Tetrarch ;
	foaf:name "Tetrarch"@en ;
	rdfs:label "Tetrarch (Macedonia (ancient kingdom))"@en , "Tetrark (Macedonia (ancient kingdom))"@sv , "Tetrarkki (Makedonian valtakunta)"@fi , "Tetrarch (Royaume de Macédoine)"@fr , "Tetrarch (Macedonia (ancient kingdom))"@de , "Tetrarch (Regno di Macedonia)"@it , "Tetrarch (Macedonië (oudheid))"@nl , "Tetrarch (Oldtidens Makedonia)"@no , "Tetrarch (Starożytna Macedonia)"@pl , "Tetrarca (Macedónia Antiga)"@pt , "Тетрарх (значения) (Древняя Македония)"@ru , "Tetrarch (Reino de Macedonia)"@es ;
	rdfs:comment "The specific instance of the Tetrarch rank in the context of country Macedonia (ancient kingdom)."@en ;
	owl:rankOf <dbpedia:Macedonia_%28ancient_kingdom%29> .

<http://rdf.muninn-project.org/ontologies/military#Rank_Trierarch_Macedonia_%28ancient_kingdom%29> a :MilitaryRank ;
	owl:subClass :Rank_Trierarch ;
	foaf:name "Trierarch"@en ;
	rdfs:label "Trierarch (Macedonia (ancient kingdom))"@en , "Trierarch (Makedonian valtakunta)"@fi , "Triérarchie (Royaume de Macédoine)"@fr , "Trierarchie (Macedonia (ancient kingdom))"@de , "Trierarchia (Regno di Macedonia)"@it , "Trierarch (Macedonië (oudheid))"@nl , "Trierark (Oldtidens Makedonia)"@no , "Trierarch (Starożytna Macedonia)"@pl , "Trierarch (Macedónia Antiga)"@pt , "Триерархия (Древняя Македония)"@ru , "Trierarca (Reino de Macedonia)"@es ;
	rdfs:comment "The specific instance of the Trierarch rank in the context of country Macedonia (ancient kingdom)."@en ;
	owl:rankOf <dbpedia:Macedonia_%28ancient_kingdom%29> .

:Rank_Trierarch_Achaean_League a :MilitaryRank ;
	owl:subClass :Rank_Trierarch ;
	foaf:name "Trierarch"@en ;
	rdfs:label "Trierarch (Achaean League)"@en , "Trierarch (Achaiska förbundet)"@sv , "Trierarch (Akhaian liitto)"@fi , "Triérarchie (Ligue achéenne)"@fr , "Trierarchie (Achaiischer Bund)"@de , "Trierarchia (Lega achea)"@it , "Trierarch (Achaeïsche Bond)"@nl , "Trierark (Det akhaiske forbund)"@no , "Trierarch (Związek Achajski)"@pl , "Trierarch (Liga Aqueia)"@pt , "Триерархия (Ахейский союз)"@ru , "Trierarca (Liga Aquea)"@es ;
	rdfs:comment "The specific instance of the Trierarch rank in the context of country Achaean League."@en ;
	owl:rankOf <dbpedia:Achaean_League> .

:Rank_Tysyatsky_Russia a :MilitaryRank ;
	owl:subClass :Rank_Tysyatsky ;
	foaf:name "Тысяцкий"@ru ;
	rdfs:label "Tysyatsky (Russia)"@en , "Tysyatsky (Ryssland)"@sv , "Tysyatsky (Venäjä)"@fi , "Tysyatsky (Russie)"@fr , "Tysyatsky (Russland)"@de , "Tysjackij (Russia)"@it , "Tysjatski (Rusland)"@nl , "Tysyatsky (Russland)"@no , "Tysyatsky (Rosja)"@pl , "Tysyatsky (Rússia)"@pt , "Тысяцкий (Россия)"@ru , "Tysyatsky (Rusia)"@es ;
	rdfs:comment "The specific instance of the Tysyatsky rank in the context of country Russia."@en ;
	owl:rankOf <dbpedia:Russia> .

:Rank_Tysyatsky_Soviet_Union a :MilitaryRank ;
	owl:subClass :Rank_Tysyatsky ;
	foaf:name "Tysyatsky"@en ;
	rdfs:label "Tysyatsky (Soviet Union)"@en , "Tysyatsky (Sovjetunionen)"@sv , "Tysyatsky (Neuvostoliitto)"@fi , "Tysyatsky (Union des républiques socialistes soviétiques)"@fr , "Tysyatsky (Sowjetunion)"@de , "Tysjackij (Unione Sovietica)"@it , "Tysjatski (Sovjet-Unie)"@nl , "Tysyatsky (Sovjetunionen)"@no , "Tysyatsky (Związek Socjalistycznych Republik Radzieckich)"@pl , "Tysyatsky (União Soviética)"@pt , "Тысяцкий (Союз Советских Социалистических Республик)"@ru , "Tysyatsky (Unión Soviética)"@es ;
	rdfs:comment "The specific instance of the Tysyatsky rank in the context of country Soviet Union."@en ;
	owl:rankOf <dbpedia:Soviet_Union> .

<http://rdf.muninn-project.org/ontologies/military#Rank_V%C3%A4%C3%A4peli_Sweden> a :MilitaryRank ;
	owl:subClass <http://rdf.muninn-project.org/ontologies/military#Rank_V%C3%A4%C3%A4peli> ;
	foaf:name "Vääpeli"@en ;
	rdfs:label "Vääpeli (Sweden)"@en , "Vääpeli (Sverige)"@sv , "Vääpeli (Ruotsi)"@fi , "Vääpeli (Suède)"@fr , "Vääpeli (Schweden)"@de , "Vääpeli (Svezia)"@it , "Vääpeli (Zweden)"@nl , "Vääpeli (Sverige)"@no , "Vääpeli (Szwecja)"@pl , "Vääpeli (Suécia)"@pt , "Vääpeli (Швеция)"@ru , "Vääpeli (Suecia)"@es ;
	rdfs:comment "The specific instance of the Vääpeli rank in the context of country Sweden."@en ;
	owl:rankOf <dbpedia:Sweden> .

<http://rdf.muninn-project.org/ontologies/military#Rank_V%C3%A4%C3%A4peli_Finland> a :MilitaryRank ;
	owl:subClass <http://rdf.muninn-project.org/ontologies/military#Rank_V%C3%A4%C3%A4peli> ;
	foaf:name "Vääpeli"@en ;
	rdfs:label "Vääpeli (Finland)"@en , "Vääpeli (Finland)"@sv , "Vääpeli (Suomi)"@fi , "Vääpeli (Finlande)"@fr , "Vääpeli (Finnland)"@de , "Vääpeli (Finlandia)"@it , "Vääpeli (Finland)"@nl , "Vääpeli (Finland)"@no , "Vääpeli (Finlandia)"@pl , "Vääpeli (Finlândia)"@pt , "Vääpeli (Финляндия)"@ru , "Vääpeli (Finlandia)"@es ;
	rdfs:comment "The specific instance of the Vääpeli rank in the context of country Finland."@en ;
	owl:rankOf <dbpedia:Finland> .

:Rank_Veebel_Estonia a :MilitaryRank ;
	owl:subClass :Rank_Veebel ;
	foaf:name "Veebel"@en ;
	rdfs:label "Veebel (Estonia)"@en , "Veebel (Estland)"@sv , "Veebel (Viro)"@fi , "Veebel (Estonie)"@fr , "Veebel (Estland)"@de , "Veebel (Estonia)"@it , "Veebel (Estland)"@nl , "Veebel (Estland)"@no , "Veebel (Estonia)"@pl , "Veebel (Estónia)"@pt , "Veebel (Эстония)"@ru , "Veebel (Estonia)"@es ;
	rdfs:comment "The specific instance of the Veebel rank in the context of country Estonia."@en ;
	owl:rankOf <dbpedia:Estonia> .

<http://rdf.muninn-project.org/ontologies/military#Rank_Veebel_Republic_of_Estonia_%281920-1940%29> a :MilitaryRank ;
	owl:subClass :Rank_Veebel ;
	foaf:name "Veebel"@en ;
	rdfs:label "Veebel (Republic of Estonia, 1920-1940)"@en ;
	rdfs:comment "The specific instance of the Veebel rank in the context of the Republic of Estonia, 1920-1940."@en ;
	owl:rankOf <dbpedia:Republic_of_Estonia_%281920-1940%29> .

:Rank_Vice_admiral_Australia a :MilitaryRank ;
	owl:subClass :Rank_Vice_admiral ;
	foaf:name "Vice admiral"@en ;
	rdfs:label "Vice admiral (Australia)"@en , "Vice admiral (Australien)"@sv , "Vice admiral (Australia)"@fi , "Vice admiral (Australie)"@fr , "Vice admiral (Australien)"@de , "Vice admiral (Australia)"@it , "Vice admiral (Australië (land))"@nl , "Vice admiral (Australia)"@no , "Vice admiral (Australia)"@pl , "Vice admiral (Austrália)"@pt , "Vice admiral (Австралия)"@ru , "Vice admiral (Australia)"@es ;
	rdfs:comment "The specific instance of the Vice admiral rank in the context of country Australia."@en ;
	owl:rankOf <dbpedia:Australia> .

<http://rdf.muninn-project.org/ontologies/military#Rank_Vice_admiral_%28Australia%29_Australia> a :MilitaryRank ;
	owl:subClass <http://rdf.muninn-project.org/ontologies/military#Rank_Vice_admiral_%28Australia%29> ;
	foaf:name ""@en ;
	rdfs:label "(Australia)"@en , "(Australien)"@sv , "(Australia)"@fi , "(Australie)"@fr , "(Australien)"@de , "(Australia)"@it , "(Australië (land))"@nl , "(Australia)"@no , "(Australia)"@pl , "(Austrália)"@pt , "(Австралия)"@ru , "(Australia)"@es ;
	rdfs:comment "The specific instance of the  rank in the context of country Australia."@en ;
	owl:rankOf <dbpedia:Australia> .

:Rank_Vice_admiral_Canada a :MilitaryRank ;
	owl:subClass :Rank_Vice_admiral ;
	foaf:name "Vice admiral"@en ;
	rdfs:label "Vice admiral (Canada)"@en ;
	rdfs:comment "The specific instance of the Vice admiral rank in the context of Canada."@en ;
	owl:rankOf <dbpedia:Canada> .

:Rank_Wojski_Poland a :MilitaryRank ;
	owl:subClass :Rank_Wojski ;
	foaf:name "Wojski"@en ;
	rdfs:label "Wojski (Poland)"@en , "Wojski (Poland)"@pl , "Войский (Poland)"@ru ;
	rdfs:comment "The specific instance of the Wojski rank in the context of Poland."@en ;
	owl:rankOf <dbpedia:Poland> .

:Rank_Wojski_Lithuania a :MilitaryRank ;
	owl:subClass :Rank_Wojski ;
	foaf:name "Wojski"@en ;
	rdfs:label "Wojski (Lithuania)"@en , "Wojski (Litauen)"@sv , "Wojski (Liettua)"@fi , "Wojski (Lituanie)"@fr , "Wojski (Litauen)"@de , "Wojski (Lituania)"@it , "Wojski (Litouwen)"@nl , "Wojski (Litauen)"@no , "Wojski (Litwa)"@pl , "Wojski (Lituânia)"@pt , "Войский (Литва)"@ru , "Wojski (Lituania)"@es ;
	rdfs:comment "The specific instance of the Wojski rank in the context of country Lithuania."@en ;
	owl:rankOf <dbpedia:Lithuania> .

<dbpedia:Lithuania> muninn:wikipedia_version "498142623" .

:Rank_Wonsu_North_Korea a :MilitaryRank ;
	owl:subClass :Rank_Wonsu ;
	foaf:name "Wonsu"@en ;
	rdfs:label "Wonsu (North Korea)"@en , "Wonsu (Nordkorea)"@sv , "Wonsu (Korean demokraattinen kansantasavalta)"@fi , "Wonsu (Corée du Nord)"@fr , "Wonsu (Nordkorea)"@de , "Wonsu (Corea del Nord)"@it , "Wonsu (Noord-Korea)"@nl , "Wonsu (Nord-Korea)"@no , "Wonsu (Korea Północna)"@pl , "Wonsu (Coreia do Norte)"@pt , "Вонсу (Корейская Народно-Демократическая Республика)"@ru , "Wonsu (Corea del Norte)"@es ;
	rdfs:comment "The specific instance of the Wonsu rank in the context of country North Korea."@en ;
	owl:rankOf <dbpedia:North_Korea> .

:Rank_Wonsu_South_Korea a :MilitaryRank ;
	owl:subClass :Rank_Wonsu ;
	foaf:name "Wonsu"@en ;
	rdfs:label "Wonsu (South Korea)"@en , "Wonsu (Sydkorea)"@sv , "Wonsu (Korean tasavalta)"@fi , "Wonsu (Corée du Sud)"@fr , "Wonsu (Südkorea)"@de , "Wonsu (Corea del Sud)"@it , "Wonsu (Zuid-Korea)"@nl , "Wonsu (Sør-Korea)"@no , "Wonsu (Korea Południowa)"@pl , "Wonsu (Coreia do Sul)"@pt , "Вонсу (Республика Корея)"@ru , "Wonsu (Corea del Sur)"@es ;
	rdfs:comment "The specific instance of the Wonsu rank in the context of country South Korea."@en ;
	owl:rankOf <dbpedia:South_Korea> .

:Rank_Ypolochagos_Greece a :MilitaryRank ;
	owl:subClass :Rank_Ypolochagos ;
	foaf:name "Ypolochagos"@en ;
	rdfs:label "Ypolochagos (Greece)"@en , "Ypolochagos (Grekland)"@sv , "Ypolochagos (Kreikka)"@fi , "Ypolochagos (Grèce)"@fr , "Ypolochagos (Griechenland)"@de , "Ypolochagos (Grecia)"@it , "Ypolochagos (Griekenland)"@nl , "Ypolochagos (Hellas)"@no , "Ypolochagos (Grecja)"@pl , "Ypolochagos (Grécia)"@pt , "Ypolochagos (Греция)"@ru , "Ypolochagos (Grecia)"@es ;
	rdfs:comment "The specific instance of the Ypolochagos rank in the context of country Greece."@en ;
	owl:rankOf <dbpedia:Greece> .

:Rank_Ypolochagos_Official_Timocracy_of_Sapinetia a :MilitaryRank ;
	owl:subClass :Rank_Ypolochagos ;
	foaf:name "Ypolochagos"@en ;
	rdfs:label "Ypolochagos (Timocracy_of_Sapinetia)"@en ;
	rdfs:comment "The specific instance of the Ypolochagos rank in the context of the Timocracy_of_Sapinetia."@en ;
	owl:rankOf <dbpedia:Official_Timocracy_of_Sapinetia> .

<http://rdf.muninn-project.org/ontologies/military#Rank_Agha_%28Ottoman_Empire%29_Ottoman_Empire> a :MilitaryRank ;
	owl:subClass <http://rdf.muninn-project.org/ontologies/military#Rank_Agha_%28Ottoman_Empire%29> ;
	foaf:name "Agha"@en ;
	rdfs:label "Agha (Ottoman Empire) (Ottoman Empire)"@en , "Agha (Osmanska riket)"@sv , "Agha (Osmanien valtakunta)"@fi , "Agha (Empire ottoman)"@fr , "Agha (Titel) (Osmanisches Reich)"@de , "Agha (Impero ottomano)"@it , "Agha (Ottoman Empire) (Ottomaanse Rijk)"@nl , "Agha (Det osmanske rike)"@no , "Aga (wojsko) (Imperium osmańskie)"@pl , "Agha (Ottoman Empire) (Império Otomano)"@pt , "Ага (титул военачальников) (Османская империя)"@ru , "Agha (Ottoman Empire) (Imperio otomano)"@es ;
	rdfs:comment "The specific instance of the Agha (Ottoman Empire) rank in the context of country Ottoman Empire."@en ;
	owl:rankOf <dbpedia:Ottoman_Empire> .

<dbpedia:Ottoman_Empire> muninn:wikipedia_version "498292397" .

<http://rdf.muninn-project.org/ontologies/military#Rank_Agha_%28Ottoman_Empire%29_Cossack_Hetmanate> a :MilitaryRank ;
	owl:subClass <http://rdf.muninn-project.org/ontologies/military#Rank_Agha_%28Ottoman_Empire%29> ;
	foaf:name "Agha"@en ;
	rdfs:label "Agha (Ottoman Empire) (Cossack Hetmanate)"@en , "Agha (Cossack Hetmanate)"@sv , "Agha (Cossack Hetmanate)"@fi , "Agha (Hetmanat cosaque)"@fr , "Agha (Titel) (Hetmanat)"@de , "Agha (Cossack Hetmanate)"@it , "Agha (Cossack Hetmanate)"@no , "Aga (wojsko) (Hetmańszczyzna)"@pl , "Ага (титул военачальников) (Гетманщина)"@ru , "Agha (Ottoman Empire) (Hetmanato cosaco)"@es ;
	rdfs:comment "The specific instance of the Agha (Ottoman Empire) rank in the context of country Cossack Hetmanate."@en ;
	owl:rankOf <dbpedia:Cossack_Hetmanate> .

<dbpedia:Cossack_Hetmanate> muninn:wikipedia_version "497147011" .

<http://rdf.muninn-project.org/ontologies/military#Rank_Agha_%28Ottoman_Empire%29_Septinsular_Republic> a :MilitaryRank ;
	owl:subClass <http://rdf.muninn-project.org/ontologies/military#Rank_Agha_%28Ottoman_Empire%29> ;
	foaf:name "Agha"@en ;
	rdfs:label "Agha (Ottoman Empire) (Septinsular Republic)"@en , "Agha (Septinsular Republic)"@sv , "Agha (Septinsular Republic)"@fi , "Agha (République des Sept-Îles)"@fr , "Agha (Titel) (Septinsular Republic)"@de , "Agha (Repubblica delle Sette Isole Unite)"@it , "Agha (Ottoman Empire) (Republiek van de Zeven Eilanden)"@nl , "Agha (Septinsular Republic)"@no , "Aga (wojsko) (Republika Siedmiu Wysp)"@pl , "Ага (титул военачальников) (Республика Семи Островов)"@ru , "Agha (Ottoman Empire) (República de las Islas Jónicas)"@es ;
	rdfs:comment "The specific instance of the Agha (Ottoman Empire) rank in the context of country Septinsular Republic."@en ;
	owl:rankOf <dbpedia:Septinsular_Republic> .

<dbpedia:Septinsular_Republic> muninn:wikipedia_version "496530677" .

:Rank_Air_chief_marshal_Australia a :MilitaryRank ;
	owl:subClass :Rank_Air_chief_marshal ;
	foaf:name "Air chief marshal"@en ;
	rdfs:label "Air chief marshal (Australia)"@en , "Air chief marshal (Australien)"@sv , "Air chief marshal (Australia)"@fi , "Air chief marshal (Australie)"@fr , "Air chief marshal (Australien)"@de , "Air chief marshal (Australia)"@it , "Air chief marshal (Australië (land))"@nl , "Air chief marshal (Australia)"@no , "Air chief marshal (Australia)"@pl , "Air chief marshal (Austrália)"@pt , "Air chief marshal (Австралия)"@ru , "Air chief marshal (Australia)"@es ;
	rdfs:comment "The specific instance of the Air chief marshal rank in the context of country Australia."@en ;
	owl:rankOf <dbpedia:Australia> .

<http://rdf.muninn-project.org/ontologies/military#Rank_Air_chief_marshal_%28Australia%29_Australia> a :MilitaryRank ;
	owl:subClass <http://rdf.muninn-project.org/ontologies/military#Rank_Air_chief_marshal_%28Australia%29> ;
	foaf:name ""@en ;
	rdfs:label "(Australia)"@en , "(Australien)"@sv , "(Australia)"@fi , "(Australie)"@fr , "(Australien)"@de , "(Australia)"@it , "(Australië (land))"@nl , "(Australia)"@no , "(Australia)"@pl , "(Austrália)"@pt , "(Австралия)"@ru , "(Australia)"@es ;
	rdfs:comment "The specific instance of the  rank in the context of country Australia."@en ;
	owl:rankOf <dbpedia:Australia> .

:Rank_Air_chief_marshal_Canada a :MilitaryRank ;
	owl:subClass :Rank_Air_chief_marshal ;
	foaf:name "Air chief marshal"@en ;
	rdfs:label "Air chief marshal (Canada)"@en ;
	rdfs:comment "The specific instance of the Air chief marshal rank in the context of Canada."@en ;
	owl:rankOf <dbpedia:Canada> .

:Rank_Air_chief_marshal_Commonwealth_of_Nations a :MilitaryRank ;
	owl:subClass :Rank_Air_chief_marshal ;
	foaf:name "Air chief marshal"@en ;
	rdfs:label "Air chief marshal (Commonwealth of Nations)"@en , "Air chief marshal (Samväldet)"@sv , "Air chief marshal (Kansainyhteisö)"@fi , "Air chief marshal (Commonwealth of Nations)"@fr , "Air chief marshal (Commonwealth of Nations)"@de , "Air chief marshal (Commonwealth delle nazioni)"@it , "Air chief marshal (Gemenebest van Naties)"@nl , "Air chief marshal (Samveldet av nasjoner)"@no , "Air chief marshal (Wspólnota Narodów)"@pl , "Air chief marshal (Commonwealth)"@pt , "Air chief marshal (Содружество наций)"@ru , "Air chief marshal (Mancomunidad de Naciones)"@es ;
	rdfs:comment "The specific instance of the Air chief marshal rank in the context of country Commonwealth of Nations."@en ;
	owl:rankOf <dbpedia:Commonwealth_of_Nations> .

:Rank_Air_vice-marshal_Australia a :MilitaryRank ;
	owl:subClass :Rank_Air_vice-marshal ;
	foaf:name "Air vice-marshal"@en ;
	rdfs:label "Air vice-marshal (Australia)"@en , "Air vice-marshal (Australien)"@sv , "Air vice-marshal (Australia)"@fi , "Air vice-marshal (Australie)"@fr , "Air vice-marshal (Australien)"@de , "Air vice-marshal (Australia)"@it , "Air vice-marshal (Australië (land))"@nl , "Air vice-marshal (Australia)"@no , "Air vice-marshal (Australia)"@pl , "Air vice-marshal (Austrália)"@pt , "Air vice-marshal (Австралия)"@ru , "Air vice-marshal (Australia)"@es ;
	rdfs:comment "The specific instance of the Air vice-marshal rank in the context of country Australia."@en ;
	owl:rankOf <dbpedia:Australia> .

:Rank_Air_vice-marshal_Canada a :MilitaryRank ;
	owl:subClass :Rank_Air_vice-marshal ;
	foaf:name "Air vice-marshal"@en ;
	rdfs:label "Air vice-marshal (Canada)"@en ;
	rdfs:comment "The specific instance of the Air vice-marshal rank in the context of Canada."@en ;
	owl:rankOf <dbpedia:Canada> .

:Rank_Air_vice-marshal_Commonwealth_of_Nations a :MilitaryRank ;
	owl:subClass :Rank_Air_vice-marshal ;
	foaf:name "Air vice-marshal"@en ;
	rdfs:label "Air vice-marshal (Commonwealth of Nations)"@en , "Air vice-marshal (Samväldet)"@sv , "Air vice-marshal (Kansainyhteisö)"@fi , "Air vice-marshal (Commonwealth of Nations)"@fr , "Air vice-marshal (Commonwealth of Nations)"@de , "Air vice-marshal (Commonwealth delle nazioni)"@it , "Air vice-marshal (Gemenebest van Naties)"@nl , "Air vice-marshal (Samveldet av nasjoner)"@no , "Air vice-marshal (Wspólnota Narodów)"@pl , "Air vice-marshal (Commonwealth)"@pt , "Air vice-marshal (Содружество наций)"@ru , "Air vice-marshal (Mancomunidad de Naciones)"@es ;
	rdfs:comment "The specific instance of the Air vice-marshal rank in the context of country Commonwealth of Nations."@en ;
	owl:rankOf <dbpedia:Commonwealth_of_Nations> .

:Rank_Ataman_Ukraine a :MilitaryRank ;
	owl:subClass :Rank_Ataman ;
	foaf:name "Атаман"@ru ;
	rdfs:label "Ataman (Ukraine)"@en , "Ataman (Ukraina)"@sv , "Atamaani (Ukraina)"@fi , "Ataman / Otaman (Ukraine)"@fr , "Ataman (Ukraine)"@de , "Atamano (Ucraina)"@it , "Ataman (Oekraïne)"@nl , "Ataman (Ukraina)"@no , "Ataman (Ukraina)"@pl , "Ataman (Ucrânia)"@pt , "Атаман (Украина)"@ru , "Atamán (Ucrania)"@es ;
	rdfs:comment "The specific instance of the Ataman rank in the context of country Ukraine."@en ;
	owl:rankOf <dbpedia:Ukraine> .

<dbpedia:Ukraine> muninn:wikipedia_version "497889189" .

:Rank_Ataman_Russia a :MilitaryRank ;
	owl:subClass :Rank_Ataman ;
	foaf:name "Атаман"@ru ;
	rdfs:label "Ataman (Russia)"@en , "Ataman (Ryssland)"@sv , "Atamaani (Venäjä)"@fi , "Ataman / Otaman (Russie)"@fr , "Ataman (Russland)"@de , "Atamano (Russia)"@it , "Ataman (Rusland)"@nl , "Ataman (Russland)"@no , "Ataman (Rosja)"@pl , "Ataman (Rússia)"@pt , "Атаман (Россия)"@ru , "Atamán (Rusia)"@es ;
	rdfs:comment "The specific instance of the Ataman rank in the context of country Russia."@en ;
	owl:rankOf <dbpedia:Russia> .

:Rank_Ataman_Soviet_Union a :MilitaryRank ;
	owl:subClass :Rank_Ataman ;
	foaf:name "Ataman"@en ;
	rdfs:label "Ataman (Soviet Union)"@en , "Ataman (Sovjetunionen)"@sv , "Atamaani (Neuvostoliitto)"@fi , "Ataman / Otaman (Union des républiques socialistes soviétiques)"@fr , "Ataman (Sowjetunion)"@de , "Atamano (Unione Sovietica)"@it , "Ataman (Sovjet-Unie)"@nl , "Ataman (Sovjetunionen)"@no , "Ataman (Związek Socjalistycznych Republik Radzieckich)"@pl , "Ataman (União Soviética)"@pt , "Атаман (Союз Советских Социалистических Республик)"@ru , "Atamán (Unión Soviética)"@es ;
	rdfs:comment "The specific instance of the Ataman rank in the context of country Soviet Union."@en ;
	owl:rankOf <dbpedia:Soviet_Union> .

:Rank_Birinci_Ferik_Ottoman_Empire a :MilitaryRank ;
	owl:subClass :Rank_Birinci_Ferik ;
	foaf:name "Birinci Ferik"@en ;
	rdfs:label "Birinci Ferik (Ottoman Empire)"@en , "Birinci Ferik (Osmanska riket)"@sv , "Birinci Ferik (Osmanien valtakunta)"@fi , "Birinci Ferik (Empire ottoman)"@fr , "Birinci Ferik (Osmanisches Reich)"@de , "Birinci Ferik (Impero ottomano)"@it , "Birinci Ferik (Ottomaanse Rijk)"@nl , "Birinci Ferik (Det osmanske rike)"@no , "Birinci Ferik (Imperium osmańskie)"@pl , "Birinci Ferik (Império Otomano)"@pt , "Birinci Ferik (Османская империя)"@ru , "Birinci Ferik (Imperio otomano)"@es ;
	rdfs:comment "The specific instance of the Birinci Ferik rank in the context of country Ottoman Empire."@en ;
	owl:rankOf <dbpedia:Ottoman_Empire> .

:Rank_Birinci_Ferik_Cossack_Hetmanate a :MilitaryRank ;
	owl:subClass :Rank_Birinci_Ferik ;
	foaf:name "Birinci Ferik"@en ;
	rdfs:label "Birinci Ferik (Cossack Hetmanate)"@en , "Birinci Ferik (Hetmanat cosaque)"@fr , "Birinci Ferik (Hetmanat)"@de , "Birinci Ferik (Hetmańszczyzna)"@pl , "Birinci Ferik (Гетманщина)"@ru , "Birinci Ferik (Hetmanato cosaco)"@es ;
	rdfs:comment "The specific instance of the Birinci Ferik rank in the context of country Cossack Hetmanate."@en ;
	owl:rankOf <dbpedia:Cossack_Hetmanate> .

:Rank_Birinci_Ferik_Septinsular_Republic a :MilitaryRank ;
	owl:subClass :Rank_Birinci_Ferik ;
	foaf:name "Birinci Ferik"@en ;
	rdfs:label "Birinci Ferik (Septinsular Republic)"@en , "Birinci Ferik (République des Sept-Îles)"@fr , "Birinci Ferik (Repubblica delle Sette Isole Unite)"@it , "Birinci Ferik (Republiek van de Zeven Eilanden)"@nl , "Birinci Ferik (Republika Siedmiu Wysp)"@pl , "Birinci Ferik (Республика Семи Островов)"@ru , "Birinci Ferik (República de las Islas Jónicas)"@es ;
	rdfs:comment "The specific instance of the Birinci Ferik rank in the context of country Septinsular Republic."@en ;
	owl:rankOf <dbpedia:Septinsular_Republic> .

<http://rdf.muninn-project.org/ontologies/military#Rank_Bombardier_%28rank%29_Australia> a :MilitaryRank ;
	owl:subClass <http://rdf.muninn-project.org/ontologies/military#Rank_Bombardier_%28rank%29> ;
	foaf:name "Bombardier"@en ;
	rdfs:label "Bombardier (rank) (Australia)"@en , "Bombardier (rank) (Australien)"@sv , "Bombardier (rank) (Australia)"@fi , "Bombardier (rank) (Australie)"@fr , "Bombardier (rank) (Australien)"@de , "Bombardier (rank) (Australia)"@it , "Bombardier (rank) (Australië (land))"@nl , "Bombardier (rank) (Australia)"@no , "Bombardier (stopień) (Australia)"@pl , "Bombardier (rank) (Austrália)"@pt , "Бомбардир (воинское звание) (Австралия)"@ru , "Bombardier (rank) (Australia)"@es ;
	rdfs:comment "The specific instance of the Bombardier (rank) rank in the context of country Australia."@en ;
	owl:rankOf <dbpedia:Australia> .

<http://rdf.muninn-project.org/ontologies/military#Rank_Bombardier_%28rank%29_Canada> a :MilitaryRank ;
	owl:subClass <http://rdf.muninn-project.org/ontologies/military#Rank_Bombardier_%28rank%29> ;
	foaf:name "Bombardier"@en ;
	rdfs:label "Bombardier (rank, Canada)"@en , "Bombardier (stopień, Canada)"@pl , "Бомбардир (воинское звание, Canada)"@ru ;
	rdfs:comment "The specific instance of the Bombardier (rank) rank in the context of Canada."@en ;
	owl:rankOf <dbpedia:Canada> .

<http://rdf.muninn-project.org/ontologies/military#Rank_Bombardier_%28rank%29_Commonwealth_of_Nations> a :MilitaryRank ;
	owl:subClass <http://rdf.muninn-project.org/ontologies/military#Rank_Bombardier_%28rank%29> ;
	foaf:name "Bombardier"@en ;
	rdfs:label "Bombardier (rank) (Commonwealth of Nations)"@en , "Bombardier (rank) (Samväldet)"@sv , "Bombardier (rank) (Kansainyhteisö)"@fi , "Bombardier (rank) (Commonwealth of Nations)"@fr , "Bombardier (rank) (Commonwealth of Nations)"@de , "Bombardier (rank) (Commonwealth delle nazioni)"@it , "Bombardier (rank) (Gemenebest van Naties)"@nl , "Bombardier (rank) (Samveldet av nasjoner)"@no , "Bombardier (stopień) (Wspólnota Narodów)"@pl , "Bombardier (rank) (Commonwealth)"@pt , "Бомбардир (воинское звание) (Содружество наций)"@ru , "Bombardier (rank) (Mancomunidad de Naciones)"@es ;
	rdfs:comment "The specific instance of the Bombardier (rank) rank in the context of country Commonwealth of Nations."@en ;
	owl:rankOf <dbpedia:Commonwealth_of_Nations> .

:Rank_Bootsmann_Germany a :MilitaryRank ;
	owl:subClass :Rank_Bootsmann ;
	foaf:name "Bootsmann"@de ;
	rdfs:label "Bootsmann (Germany)"@en , "Bootsmann (Germany)"@de , "Боцман (Germany)"@ru ;
	rdfs:comment "The specific instance of the Bootsmann rank in the context of Germany."@en ;
	owl:rankOf <dbpedia:Germany> .

:Rank_Bootsmann_Russia a :MilitaryRank ;
	owl:subClass :Rank_Bootsmann ;
	foaf:name "Боцман"@ru ;
	rdfs:label "Bootsmann (Russia)"@en , "Bootsmann (Ryssland)"@sv , "Bootsmann (Venäjä)"@fi , "Bootsmann (Russie)"@fr , "Bootsmann (Russland)"@de , "Bootsmann (Russia)"@it , "Bootsmann (Rusland)"@nl , "Bootsmann (Russland)"@no , "Bootsmann (Rosja)"@pl , "Bootsmann (Rússia)"@pt , "Боцман (Россия)"@ru , "Bootsmann (Rusia)"@es ;
	rdfs:comment "The specific instance of the Bootsmann rank in the context of country Russia."@en ;
	owl:rankOf <dbpedia:Russia> .

:Rank_Bootsmann_Soviet_Union a :MilitaryRank ;
	owl:subClass :Rank_Bootsmann ;
	foaf:name "Bootsmann"@en ;
	rdfs:label "Bootsmann (Soviet Union)"@en , "Bootsmann (Sovjetunionen)"@sv , "Bootsmann (Neuvostoliitto)"@fi , "Bootsmann (Union des républiques socialistes soviétiques)"@fr , "Bootsmann (Sowjetunion)"@de , "Bootsmann (Unione Sovietica)"@it , "Bootsmann (Sovjet-Unie)"@nl , "Bootsmann (Sovjetunionen)"@no , "Bootsmann (Związek Socjalistycznych Republik Radzieckich)"@pl , "Bootsmann (União Soviética)"@pt , "Боцман (Союз Советских Социалистических Республик)"@ru , "Bootsmann (Unión Soviética)"@es ;
	rdfs:comment "The specific instance of the Bootsmann rank in the context of country Soviet Union."@en ;
	owl:rankOf <dbpedia:Soviet_Union> .

<http://rdf.muninn-project.org/ontologies/military#Rank_%C3%87orbac%C4%B1_Ottoman_Empire> a :MilitaryRank ;
	owl:subClass <http://rdf.muninn-project.org/ontologies/military#Rank_%C3%87orbac%C4%B1> ;
	foaf:name "Çorbacı"@en ;
	rdfs:label "Çorbacı (Ottoman Empire)"@en , "Çorbacı (Osmanska riket)"@sv , "Çorbacı (Osmanien valtakunta)"@fi , "Çorbacı (Empire ottoman)"@fr , "Çorbacı (Osmanisches Reich)"@de , "Çorbacı (Impero ottomano)"@it , "Çorbacı (Ottomaanse Rijk)"@nl , "Çorbacı (Det osmanske rike)"@no , "Çorbacı (Imperium osmańskie)"@pl , "Çorbacı (Império Otomano)"@pt , "Чорбаджи (Османская империя)"@ru , "Çorbacı (Imperio otomano)"@es ;
	rdfs:comment "The specific instance of the Çorbacı rank in the context of country Ottoman Empire."@en ;
	owl:rankOf <dbpedia:Ottoman_Empire> .

<http://rdf.muninn-project.org/ontologies/military#Rank_%C3%87orbac%C4%B1_Cossack_Hetmanate> a :MilitaryRank ;
	owl:subClass <http://rdf.muninn-project.org/ontologies/military#Rank_%C3%87orbac%C4%B1> ;
	foaf:name "Çorbacı"@en ;
	rdfs:label "Çorbacı (Cossack Hetmanate)"@en , "Çorbacı (Hetmanat cosaque)"@fr , "Çorbacı (Hetmanat)"@de , "Çorbacı (Hetmańszczyzna)"@pl , "Чорбаджи (Гетманщина)"@ru , "Çorbacı (Hetmanato cosaco)"@es ;
	rdfs:comment "The specific instance of the Çorbacı rank in the context of country Cossack Hetmanate."@en ;
	owl:rankOf <dbpedia:Cossack_Hetmanate> .

<http://rdf.muninn-project.org/ontologies/military#Rank_%C3%87orbac%C4%B1_Septinsular_Republic> a :MilitaryRank ;
	owl:subClass <http://rdf.muninn-project.org/ontologies/military#Rank_%C3%87orbac%C4%B1> ;
	foaf:name "Çorbacı"@en ;
	rdfs:label "Çorbacı (Septinsular Republic)"@en , "Çorbacı (République des Sept-Îles)"@fr , "Çorbacı (Repubblica delle Sette Isole Unite)"@it , "Çorbacı (Republiek van de Zeven Eilanden)"@nl , "Çorbacı (Republika Siedmiu Wysp)"@pl , "Чорбаджи (Республика Семи Островов)"@ru , "Çorbacı (República de las Islas Jónicas)"@es ;
	rdfs:comment "The specific instance of the Çorbacı rank in the context of country Septinsular Republic."@en ;
	owl:rankOf <dbpedia:Septinsular_Republic> .

:Rank_Captain_Lieutenant_Germany a :MilitaryRank ;
	owl:subClass :Rank_Captain_Lieutenant ;
	foaf:name "Kapitänleutnant"@de ;
	rdfs:label "Captain Lieutenant (Germany)"@en , "Kaptenlöjtnant (Germany)"@sv , "Kapteeniluutnantti (Germany)"@fi , "Capitaine-lieutenant (Germany)"@fr , "Kapitänleutnant (Germany)"@de , "Kapteinløytnant (Germany)"@no , "Капитан-лейтенант (Germany)"@ru ;
	rdfs:comment "The specific instance of the Captain Lieutenant rank in the context of Germany."@en ;
	owl:rankOf <dbpedia:Germany> .

:Rank_Captain_Lieutenant_Russia a :MilitaryRank ;
	owl:subClass :Rank_Captain_Lieutenant ;
	foaf:name "Капитан-лейтенант"@ru ;
	rdfs:label "Captain Lieutenant (Russia)"@en , "Kaptenlöjtnant (Ryssland)"@sv , "Kapteeniluutnantti (Venäjä)"@fi , "Capitaine-lieutenant (Russie)"@fr , "Kapitänleutnant (Russland)"@de , "Captain Lieutenant (Russia)"@it , "Captain Lieutenant (Rusland)"@nl , "Kapteinløytnant (Russland)"@no , "Captain Lieutenant (Rosja)"@pl , "Captain Lieutenant (Rússia)"@pt , "Капитан-лейтенант (Россия)"@ru , "Captain Lieutenant (Rusia)"@es ;
	rdfs:comment "The specific instance of the Captain Lieutenant rank in the context of country Russia."@en ;
	owl:rankOf <dbpedia:Russia> .

:Rank_Captain_Lieutenant_Soviet_Union a :MilitaryRank ;
	owl:subClass :Rank_Captain_Lieutenant ;
	foaf:name "Captain Lieutenant"@en ;
	rdfs:label "Captain Lieutenant (Soviet Union)"@en , "Kaptenlöjtnant (Sovjetunionen)"@sv , "Kapteeniluutnantti (Neuvostoliitto)"@fi , "Capitaine-lieutenant (Union des républiques socialistes soviétiques)"@fr , "Kapitänleutnant (Sowjetunion)"@de , "Captain Lieutenant (Unione Sovietica)"@it , "Captain Lieutenant (Sovjet-Unie)"@nl , "Kapteinløytnant (Sovjetunionen)"@no , "Captain Lieutenant (Związek Socjalistycznych Republik Radzieckich)"@pl , "Captain Lieutenant (União Soviética)"@pt , "Капитан-лейтенант (Союз Советских Социалистических Республик)"@ru , "Captain Lieutenant (Unión Soviética)"@es ;
	rdfs:comment "The specific instance of the Captain Lieutenant rank in the context of country Soviet Union."@en ;
	owl:rankOf <dbpedia:Soviet_Union> .

:Rank_Captain_lieutenant_Germany a :MilitaryRank ;
	owl:subClass :Rank_Captain_lieutenant ;
	foaf:name "Captain lieutenant"@en ;
	rdfs:label "Captain lieutenant (Germany)"@en ;
	rdfs:comment "The specific instance of the Captain lieutenant rank in the context of Germany."@en ;
	owl:rankOf <dbpedia:Germany> .

:Rank_Captain_lieutenant_Russia a :MilitaryRank ;
	owl:subClass :Rank_Captain_lieutenant ;
	foaf:name "Captain lieutenant"@en ;
	rdfs:label "Captain lieutenant (Russia)"@en , "Captain lieutenant (Ryssland)"@sv , "Captain lieutenant (Venäjä)"@fi , "Captain lieutenant (Russie)"@fr , "Captain lieutenant (Russland)"@de , "Captain lieutenant (Russia)"@it , "Captain lieutenant (Rusland)"@nl , "Captain lieutenant (Russland)"@no , "Captain lieutenant (Rosja)"@pl , "Captain lieutenant (Rússia)"@pt , "Captain lieutenant (Россия)"@ru , "Captain lieutenant (Rusia)"@es ;
	rdfs:comment "The specific instance of the Captain lieutenant rank in the context of country Russia."@en ;
	owl:rankOf <dbpedia:Russia> .

:Rank_Captain_lieutenant_Soviet_Union a :MilitaryRank ;
	owl:subClass :Rank_Captain_lieutenant ;
	foaf:name "Captain lieutenant"@en ;
	rdfs:label "Captain lieutenant (Soviet Union)"@en , "Captain lieutenant (Sovjetunionen)"@sv , "Captain lieutenant (Neuvostoliitto)"@fi , "Captain lieutenant (Union des républiques socialistes soviétiques)"@fr , "Captain lieutenant (Sowjetunion)"@de , "Captain lieutenant (Unione Sovietica)"@it , "Captain lieutenant (Sovjet-Unie)"@nl , "Captain lieutenant (Sovjetunionen)"@no , "Captain lieutenant (Związek Socjalistycznych Republik Radzieckich)"@pl , "Captain lieutenant (União Soviética)"@pt , "Captain lieutenant (Союз Советских Социалистических Республик)"@ru , "Captain lieutenant (Unión Soviética)"@es ;
	rdfs:comment "The specific instance of the Captain lieutenant rank in the context of country Soviet Union."@en ;
	owl:rankOf <dbpedia:Soviet_Union> .

:Rank_Chief_petty_officer_Australia a :MilitaryRank ;
	owl:subClass :Rank_Chief_petty_officer ;
	foaf:name "Chief petty officer"@en ;
	rdfs:label "Chief petty officer (Australia)"@en , "Chief petty officer (Australien)"@sv , "Chief petty officer (Australia)"@fi , "Chief petty officer (Australie)"@fr , "Chief petty officer (Australien)"@de , "Chief petty officer (Australia)"@it , "Chief petty officer (Australië (land))"@nl , "Chief petty officer (Australia)"@no , "Chief petty officer (Australia)"@pl , "Chief petty officer (Austrália)"@pt , "Chief petty officer (Австралия)"@ru , "Chief petty officer (Australia)"@es ;
	rdfs:comment "The specific instance of the Chief petty officer rank in the context of country Australia."@en ;
	owl:rankOf <dbpedia:Australia> .

:Rank_Chief_petty_officer_Canada a :MilitaryRank ;
	owl:subClass :Rank_Chief_petty_officer ;
	foaf:name "Chief petty officer"@en ;
	rdfs:label "Chief petty officer (Canada)"@en ;
	rdfs:comment "The specific instance of the Chief petty officer rank in the context of Canada."@en ;
	owl:rankOf <dbpedia:Canada> .

<http://rdf.muninn-project.org/ontologies/military#Rank_Chief_petty_officer,_1st_class_Canada> a :MilitaryRank ;
	owl:subClass <http://rdf.muninn-project.org/ontologies/military#Rank_Chief_petty_officer,_1st_class> ;
	foaf:name "Chief petty officer, 1st Class"@en ;
	rdfs:label "Chief petty officer, 1st Class (Canada)"@en ;
	rdfs:comment "The specific instance of the  rank in the context of Canada."@en ;
	owl:rankOf <dbpedia:Canada> .

<http://rdf.muninn-project.org/ontologies/military#Rank_Chief_petty_officer,_2nd_class_Canada> a :MilitaryRank ;
	owl:subClass <http://rdf.muninn-project.org/ontologies/military#Rank_Chief_petty_officer,_2nd_class> ;
	foaf:name "Chief petty officer, 2nd Class"@en ;
	rdfs:label "Chief petty officer, 2nd Class (Canada)"@en ;
	rdfs:comment "The specific instance of the  rank in the context of Canada."@en ;
	owl:rankOf <dbpedia:Canada> .

:Rank_Chief_petty_officer_Commonwealth_of_Nations a :MilitaryRank ;
	owl:subClass :Rank_Chief_petty_officer ;
	foaf:name "Chief petty officer"@en ;
	rdfs:label "Chief petty officer (Commonwealth of Nations)"@en , "Chief petty officer (Samväldet)"@sv , "Chief petty officer (Kansainyhteisö)"@fi , "Chief petty officer (Commonwealth of Nations)"@fr , "Chief petty officer (Commonwealth of Nations)"@de , "Chief petty officer (Commonwealth delle nazioni)"@it , "Chief petty officer (Gemenebest van Naties)"@nl , "Chief petty officer (Samveldet av nasjoner)"@no , "Chief petty officer (Wspólnota Narodów)"@pl , "Chief petty officer (Commonwealth)"@pt , "Chief petty officer (Содружество наций)"@ru , "Chief petty officer (Mancomunidad de Naciones)"@es ;
	rdfs:comment "The specific instance of the Chief petty officer rank in the context of country Commonwealth of Nations."@en ;
	owl:rankOf <dbpedia:Commonwealth_of_Nations> .

<http://rdf.muninn-project.org/ontologies/military#Rank_Ferik_%28rank%29_Ottoman_Empire> a :MilitaryRank ;
	owl:subClass <http://rdf.muninn-project.org/ontologies/military#Rank_Ferik_%28rank%29> ;
	foaf:name "Ferik"@en ;
	rdfs:label "Ferik (rank) (Ottoman Empire)"@en , "Ferik (rank) (Osmanska riket)"@sv , "Ferik (rank) (Osmanien valtakunta)"@fi , "Ferik (rank) (Empire ottoman)"@fr , "Ferik (rank) (Osmanisches Reich)"@de , "Ferik (rank) (Impero ottomano)"@it , "Ferik (rank) (Ottomaanse Rijk)"@nl , "Ferik (rank) (Det osmanske rike)"@no , "Ferik (rank) (Imperium osmańskie)"@pl , "Ferik (rank) (Império Otomano)"@pt , "Ferik (rank) (Османская империя)"@ru , "Ferik (rank) (Imperio otomano)"@es ;
	rdfs:comment "The specific instance of the Ferik (rank) rank in the context of country Ottoman Empire."@en ;
	owl:rankOf <dbpedia:Ottoman_Empire> .

<http://rdf.muninn-project.org/ontologies/military#Rank_Ferik_%28rank%29_Cossack_Hetmanate> a :MilitaryRank ;
	owl:subClass <http://rdf.muninn-project.org/ontologies/military#Rank_Ferik_%28rank%29> ;
	foaf:name "Ferik"@en ;
	rdfs:label "Ferik (rank) (Cossack Hetmanate)"@en , "Ferik (rank) (Hetmanat cosaque)"@fr , "Ferik (rank) (Hetmanat)"@de , "Ferik (rank) (Hetmańszczyzna)"@pl , "Ferik (rank) (Гетманщина)"@ru , "Ferik (rank) (Hetmanato cosaco)"@es ;
	rdfs:comment "The specific instance of the Ferik (rank) rank in the context of country Cossack Hetmanate."@en ;
	owl:rankOf <dbpedia:Cossack_Hetmanate> .

<http://rdf.muninn-project.org/ontologies/military#Rank_Ferik_%28rank%29_Septinsular_Republic> a :MilitaryRank ;
	owl:subClass <http://rdf.muninn-project.org/ontologies/military#Rank_Ferik_%28rank%29> ;
	foaf:name "Ferik"@en ;
	rdfs:label "Ferik (rank) (Septinsular Republic)"@en , "Ferik (rank) (République des Sept-Îles)"@fr , "Ferik (rank) (Repubblica delle Sette Isole Unite)"@it , "Ferik (rank) (Republiek van de Zeven Eilanden)"@nl , "Ferik (rank) (Republika Siedmiu Wysp)"@pl , "Ferik (rank) (Республика Семи Островов)"@ru , "Ferik (rank) (República de las Islas Jónicas)"@es ;
	rdfs:comment "The specific instance of the Ferik (rank) rank in the context of country Septinsular Republic."@en ;
	owl:rankOf <dbpedia:Septinsular_Republic> .

:Rank_Fleet_Board_England a :MilitaryRank ;
	owl:subClass :Rank_Fleet_Board ;
	foaf:name "Fleet Board"@en ;
	rdfs:label "Fleet Board (England)"@en ;
	rdfs:comment "The specific instance of the Fleet Board rank in the context of England."@en ;
	owl:rankOf <dbpedia:England> .

<dbpedia:England> muninn:wikipedia_version "497805822" .

:Rank_Fleet_Board_Scotland a :MilitaryRank ;
	owl:subClass :Rank_Fleet_Board ;
	foaf:name "Fleet Board"@en ;
	rdfs:label "Fleet Board (Scotland)"@en , "Fleet Board (Skottland)"@sv , "Fleet Board (Skotlanti)"@fi , "Fleet Board (Écosse)"@fr , "Fleet Board (Schottland)"@de , "Fleet Board (Scozia)"@it , "Fleet Board (Schotland)"@nl , "Fleet Board (Skottland)"@no , "Fleet Board (Szkocja)"@pl , "Fleet Board (Escócia)"@pt , "Fleet Board (Шотландия)"@ru , "Fleet Board (Escocia)"@es ;
	rdfs:comment "The specific instance of the Fleet Board rank in the context of country Scotland."@en ;
	owl:rankOf <dbpedia:Scotland> .

<dbpedia:Scotland> muninn:wikipedia_version "498376035" .

:Rank_Fleet_Board_Wales a :MilitaryRank ;
	owl:subClass :Rank_Fleet_Board ;
	foaf:name "Fleet Board"@en ;
	rdfs:label "Fleet Board (Wales)"@en , "Fleet Board (Wales)"@sv , "Fleet Board (Wales)"@fi , "Fleet Board (Pays de Galles)"@fr , "Fleet Board (Wales)"@de , "Fleet Board (Galles)"@it , "Fleet Board (Wales)"@nl , "Fleet Board (Wales)"@no , "Fleet Board (Walia)"@pl , "Fleet Board (País de Gales)"@pt , "Fleet Board (Уэльс)"@ru , "Fleet Board (Gales)"@es ;
	rdfs:comment "The specific instance of the Fleet Board rank in the context of country Wales."@en ;
	owl:rankOf <dbpedia:Wales> .

<dbpedia:Wales> muninn:wikipedia_version "497995158" .

:Rank_Garrison_Sergeant_Major_England a :MilitaryRank ;
	owl:subClass :Rank_Garrison_Sergeant_Major ;
	foaf:name "Garrison Sergeant Major"@en ;
	rdfs:label "Garrison Sergeant Major (England)"@en ;
	rdfs:comment "The specific instance of the Garrison Sergeant Major rank in the context of England."@en ;
	owl:rankOf <dbpedia:England> .

:Rank_Garrison_Sergeant_Major_Scotland a :MilitaryRank ;
	owl:subClass :Rank_Garrison_Sergeant_Major ;
	foaf:name "Garrison Sergeant Major"@en ;
	rdfs:label "Garrison Sergeant Major (Scotland)"@en , "Garrison Sergeant Major (Skottland)"@sv , "Garrison Sergeant Major (Skotlanti)"@fi , "Garrison Sergeant Major (Écosse)"@fr , "Garrison Sergeant Major (Schottland)"@de , "Garrison Sergeant Major (Scozia)"@it , "Garrison Sergeant Major (Schotland)"@nl , "Garrison Sergeant Major (Skottland)"@no , "Garrison Sergeant Major (Szkocja)"@pl , "Garrison Sergeant Major (Escócia)"@pt , "Garrison Sergeant Major (Шотландия)"@ru , "Garrison Sergeant Major (Escocia)"@es ;
	rdfs:comment "The specific instance of the Garrison Sergeant Major rank in the context of country Scotland."@en ;
	owl:rankOf <dbpedia:Scotland> .

:Rank_Garrison_Sergeant_Major_Wales a :MilitaryRank ;
	owl:subClass :Rank_Garrison_Sergeant_Major ;
	foaf:name "Garrison Sergeant Major"@en ;
	rdfs:label "Garrison Sergeant Major (Wales)"@en , "Garrison Sergeant Major (Wales)"@sv , "Garrison Sergeant Major (Wales)"@fi , "Garrison Sergeant Major (Pays de Galles)"@fr , "Garrison Sergeant Major (Wales)"@de , "Garrison Sergeant Major (Galles)"@it , "Garrison Sergeant Major (Wales)"@nl , "Garrison Sergeant Major (Wales)"@no , "Garrison Sergeant Major (Walia)"@pl , "Garrison Sergeant Major (País de Gales)"@pt , "Garrison Sergeant Major (Уэльс)"@ru , "Garrison Sergeant Major (Gales)"@es ;
	rdfs:comment "The specific instance of the Garrison Sergeant Major rank in the context of country Wales."@en ;
	owl:rankOf <dbpedia:Wales> .

:Rank_Gefreiter_Germany a :MilitaryRank ;
	owl:subClass :Rank_Gefreiter ;
	foaf:name "Gefreiter"@de ;
	rdfs:label "Gefreiter (Germany)"@en , "Gefreiter (Germany)"@de , "Gefreiter (Germany)"@no , "Gefrajter (Germany)"@pl , "Ефрейтор (Germany)"@ru ;
	rdfs:comment "The specific instance of the Gefreiter rank in the context of Germany."@en ;
	owl:rankOf <dbpedia:Germany> .

:Rank_Gefreiter_Russia a :MilitaryRank ;
	owl:subClass :Rank_Gefreiter ;
	foaf:name "Ефрейтор"@ru ;
	rdfs:label "Gefreiter (Russia)"@en , "Gefreiter (Ryssland)"@sv , "Gefreiter (Venäjä)"@fi , "Gefreiter (Russie)"@fr , "Gefreiter (Russland)"@de , "Gefreiter (Russia)"@it , "Gefreiter (Rusland)"@nl , "Gefreiter (Russland)"@no , "Gefrajter (Rosja)"@pl , "Gefreiter (Rússia)"@pt , "Ефрейтор (Россия)"@ru , "Gefreiter (Rusia)"@es ;
	rdfs:comment "The specific instance of the Gefreiter rank in the context of country Russia."@en ;
	owl:rankOf <dbpedia:Russia> .

<dbpedia:Russia> muninn:wikipedia_version "498382883" .

:Rank_Gefreiter_Soviet_Union a :MilitaryRank ;
	owl:subClass :Rank_Gefreiter ;
	foaf:name "Gefreiter"@en ;
	rdfs:label "Gefreiter (Soviet Union)"@en , "Gefreiter (Sovjetunionen)"@sv , "Gefreiter (Neuvostoliitto)"@fi , "Gefreiter (Union des républiques socialistes soviétiques)"@fr , "Gefreiter (Sowjetunion)"@de , "Gefreiter (Unione Sovietica)"@it , "Gefreiter (Sovjet-Unie)"@nl , "Gefreiter (Sovjetunionen)"@no , "Gefrajter (Związek Socjalistycznych Republik Radzieckich)"@pl , "Gefreiter (União Soviética)"@pt , "Ефрейтор (Союз Советских Социалистических Республик)"@ru , "Gefreiter (Unión Soviética)"@es ;
	rdfs:comment "The specific instance of the Gefreiter rank in the context of country Soviet Union."@en ;
	owl:rankOf <dbpedia:Soviet_Union> .

:Rank_General_Admiral_Germany a :MilitaryRank ;
	owl:subClass :Rank_General_Admiral ;
	foaf:name "Generaladmiral"@de ;
	rdfs:label "General Admiral (Germany)"@en , "Kenraaliamiraali (Germany)"@fi , "Generaladmiral (Germany)"@de , "Admiraal-generaal (Germany)"@nl , "Генерал-адмирал (Germany)"@ru , "Almirante General (Germany)"@es ;
	rdfs:comment "The specific instance of the General Admiral rank in the context of Germany."@en ;
	owl:rankOf <dbpedia:Germany> .

:Rank_General_Admiral_Russia a :MilitaryRank ;
	owl:subClass :Rank_General_Admiral ;
	foaf:name "Генерал-адмирал"@ru ;
	rdfs:label "General Admiral (Russia)"@en , "General Admiral (Ryssland)"@sv , "Kenraaliamiraali (Venäjä)"@fi , "General Admiral (Russie)"@fr , "Generaladmiral (Russland)"@de , "General Admiral (Russia)"@it , "Admiraal-generaal (Rusland)"@nl , "General Admiral (Russland)"@no , "General Admiral (Rosja)"@pl , "General Admiral (Rússia)"@pt , "Генерал-адмирал (Россия)"@ru , "Almirante General (Rusia)"@es ;
	rdfs:comment "The specific instance of the General Admiral rank in the context of country Russia."@en ;
	owl:rankOf <dbpedia:Russia> .

:Rank_General_Admiral_Soviet_Union a :MilitaryRank ;
	owl:subClass :Rank_General_Admiral ;
	foaf:name "General Admiral"@en ;
	rdfs:label "General Admiral (Soviet Union)"@en , "General Admiral (Sovjetunionen)"@sv , "Kenraaliamiraali (Neuvostoliitto)"@fi , "General Admiral (Union des républiques socialistes soviétiques)"@fr , "Generaladmiral (Sowjetunion)"@de , "General Admiral (Unione Sovietica)"@it , "Admiraal-generaal (Sovjet-Unie)"@nl , "General Admiral (Sovjetunionen)"@no , "General Admiral (Związek Socjalistycznych Republik Radzieckich)"@pl , "General Admiral (União Soviética)"@pt , "Генерал-адмирал (Союз Советских Социалистических Республик)"@ru , "Almirante General (Unión Soviética)"@es ;
	rdfs:comment "The specific instance of the General Admiral rank in the context of country Soviet Union."@en ;
	owl:rankOf <dbpedia:Soviet_Union> .

:Rank_Kapudan_Pasha_Ottoman_Empire a :MilitaryRank ;
	owl:subClass :Rank_Kapudan_Pasha ;
	foaf:name "Kapudan Pasha"@en ;
	rdfs:label "Kapudan Pasha (Ottoman Empire)"@en , "Kapudan Pasha (Osmanska riket)"@sv , "Kapudan Pasha (Osmanien valtakunta)"@fi , "Capitan pacha (Empire ottoman)"@fr , "Kapudan Pascha (Osmanisches Reich)"@de , "Kapudan Pasha (Impero ottomano)"@it , "Kapudan Pasha (Ottomaanse Rijk)"@nl , "Kapudan Pasha (Det osmanske rike)"@no , "Kapudan Pasha (Imperium osmańskie)"@pl , "Kapudan Pasha (Império Otomano)"@pt , "Капудан-паша (Османская империя)"@ru , "Kapudan Pasha (Imperio otomano)"@es ;
	rdfs:comment "The specific instance of the Kapudan Pasha rank in the context of country Ottoman Empire."@en ;
	owl:rankOf <dbpedia:Ottoman_Empire> .

:Rank_Kapudan_Pasha_Cossack_Hetmanate a :MilitaryRank ;
	owl:subClass :Rank_Kapudan_Pasha ;
	foaf:name "Kapudan Pasha"@en ;
	rdfs:label "Kapudan Pasha (Cossack Hetmanate)"@en , "Capitan pacha (Hetmanat cosaque)"@fr , "Kapudan Pascha (Hetmanat)"@de , "Kapudan Pasha (Hetmańszczyzna)"@pl , "Капудан-паша (Гетманщина)"@ru , "Kapudan Pasha (Hetmanato cosaco)"@es ;
	rdfs:comment "The specific instance of the Kapudan Pasha rank in the context of country Cossack Hetmanate."@en ;
	owl:rankOf <dbpedia:Cossack_Hetmanate> .

:Rank_Kapudan_Pasha_Septinsular_Republic a :MilitaryRank ;
	owl:subClass :Rank_Kapudan_Pasha ;
	foaf:name "Kapudan Pasha"@en ;
	rdfs:label "Kapudan Pasha (Septinsular Republic)"@en , "Capitan pacha (République des Sept-Îles)"@fr , "Kapudan Pascha (Septinsular Republic)"@de , "Kapudan Pasha (Repubblica delle Sette Isole Unite)"@it , "Kapudan Pasha (Republiek van de Zeven Eilanden)"@nl , "Kapudan Pasha (Republika Siedmiu Wysp)"@pl , "Капудан-паша (Республика Семи Островов)"@ru , "Kapudan Pasha (República de las Islas Jónicas)"@es ;
	rdfs:comment "The specific instance of the Kapudan Pasha rank in the context of country Septinsular Republic."@en ;
	owl:rankOf <dbpedia:Septinsular_Republic> .

<http://rdf.muninn-project.org/ontologies/military#Rank_Kola%C4%9Fas%C4%B1_Ottoman_Empire> a :MilitaryRank ;
	owl:subClass <http://rdf.muninn-project.org/ontologies/military#Rank_Kola%C4%9Fas%C4%B1> ;
	foaf:name "Kolağası"@en ;
	rdfs:label "Kolağası (Ottoman Empire)"@en , "Kolağası (Osmanska riket)"@sv , "Kolağası (Osmanien valtakunta)"@fi , "Kolağası (Empire ottoman)"@fr , "Kolağası (Osmanisches Reich)"@de , "Kolağası (Impero ottomano)"@it , "Kolağası (Ottomaanse Rijk)"@nl , "Kolağası (Det osmanske rike)"@no , "Kolağası (Imperium osmańskie)"@pl , "Kolağası (Império Otomano)"@pt , "Kolağası (Османская империя)"@ru , "Kolağası (Imperio otomano)"@es ;
	rdfs:comment "The specific instance of the Kolağası rank in the context of country Ottoman Empire."@en ;
	owl:rankOf <dbpedia:Ottoman_Empire> .

<http://rdf.muninn-project.org/ontologies/military#Rank_Kola%C4%9Fas%C4%B1_Cossack_Hetmanate> a :MilitaryRank ;
	owl:subClass <http://rdf.muninn-project.org/ontologies/military#Rank_Kola%C4%9Fas%C4%B1> ;
	foaf:name "Kolağası"@en ;
	rdfs:label "Kolağası (Cossack Hetmanate)"@en , "Kolağası (Hetmanat cosaque)"@fr , "Kolağası (Hetmanat)"@de , "Kolağası (Hetmańszczyzna)"@pl , "Kolağası (Гетманщина)"@ru , "Kolağası (Hetmanato cosaco)"@es ;
	rdfs:comment "The specific instance of the Kolağası rank in the context of country Cossack Hetmanate."@en ;
	owl:rankOf <dbpedia:Cossack_Hetmanate> .

<http://rdf.muninn-project.org/ontologies/military#Rank_Kola%C4%9Fas%C4%B1_Septinsular_Republic> a :MilitaryRank ;
	owl:subClass <http://rdf.muninn-project.org/ontologies/military#Rank_Kola%C4%9Fas%C4%B1> ;
	foaf:name "Kolağası"@en ;
	rdfs:label "Kolağası (Septinsular Republic)"@en , "Kolağası (République des Sept-Îles)"@fr , "Kolağası (Repubblica delle Sette Isole Unite)"@it , "Kolağası (Republiek van de Zeven Eilanden)"@nl , "Kolağası (Republika Siedmiu Wysp)"@pl , "Kolağası (Республика Семи Островов)"@ru , "Kolağası (República de las Islas Jónicas)"@es ;
	rdfs:comment "The specific instance of the Kolağası rank in the context of country Septinsular Republic."@en ;
	owl:rankOf <dbpedia:Septinsular_Republic> .

:Rank_Lance-corporal_of_horse_England a :MilitaryRank ;
	owl:subClass :Rank_Lance-corporal_of_horse ;
	foaf:name "Lance Corporal of Horse"@en ;
	rdfs:label "Lance Corporal of Horse (England)"@en ;
	rdfs:comment "The specific instance of the  rank in the context of England."@en ;
	owl:rankOf <dbpedia:England> .

:Rank_Lance-corporal_of_horse_Scotland a :MilitaryRank ;
	owl:subClass :Rank_Lance-corporal_of_horse ;
	foaf:name "Lance Corporal of Horse"@en ;
	rdfs:label "Lance Corporal of Horse (Scotland)"@en , "Lance Corporal of Horse (Skottland)"@sv , "Lance Corporal of Horse (Skotlanti)"@fi , "Lance Corporal of Horse (Écosse)"@fr , "Lance Corporal of Horse (Schottland)"@de , "Lance Corporal of Horse (Scozia)"@it , "Lance Corporal of Horse (Schotland)"@nl , "Lance Corporal of Horse (Skottland)"@no , "Lance Corporal of Horse (Szkocja)"@pl , "Lance Corporal of Horse (Escócia)"@pt , "Lance Corporal of Horse (Шотландия)"@ru , "Lance Corporal of Horse (Escocia)"@es ;
	rdfs:comment "The specific instance of the Lance Corporal of Horse rank in the context of country Scotland."@en ;
	owl:rankOf <dbpedia:Scotland> .

:Rank_Lance-corporal_of_horse_Wales a :MilitaryRank ;
	owl:subClass :Rank_Lance-corporal_of_horse ;
	foaf:name "Lance Corporal of Horse"@en ;
	rdfs:label "Lance Corporal of Horse (Wales)"@en , "Lance Corporal of Horse (Wales)"@sv , "Lance Corporal of Horse (Wales)"@fi , "Lance Corporal of Horse (Pays de Galles)"@fr , "Lance Corporal of Horse (Wales)"@de , "Lance Corporal of Horse (Galles)"@it , "Lance Corporal of Horse (Wales)"@nl , "Lance Corporal of Horse (Wales)"@no , "Lance Corporal of Horse (Walia)"@pl , "Lance Corporal of Horse (País de Gales)"@pt , "Lance Corporal of Horse (Уэльс)"@ru , "Lance Corporal of Horse (Gales)"@es ;
	rdfs:comment "The specific instance of the Lance Corporal of Horse  rank in the context of country Wales."@en ;
	owl:rankOf <dbpedia:Wales> .

:Rank_Leading_aircraftman_Australia a :MilitaryRank ;
	owl:subClass :Rank_Leading_aircraftman ;
	foaf:name "Leading aircraftman"@en ;
	rdfs:label "Leading aircraftman (Australia)"@en , "Leading aircraftman (Australien)"@sv , "Leading aircraftman (Australia)"@fi , "Leading aircraftman (Australie)"@fr , "Leading aircraftman (Australien)"@de , "Leading aircraftman (Australia)"@it , "Leading aircraftman (Australië (land))"@nl , "Leading aircraftman (Australia)"@no , "Leading aircraftman (Australia)"@pl , "Leading aircraftman (Austrália)"@pt , "Leading aircraftman (Австралия)"@ru , "Leading aircraftman (Australia)"@es ;
	rdfs:comment "The specific instance of the Leading aircraftman rank in the context of country Australia."@en ;
	owl:rankOf <dbpedia:Australia> .

:Rank_Leading_aircraftman_Canada a :MilitaryRank ;
	owl:subClass :Rank_Leading_aircraftman ;
	foaf:name "Leading aircraftman"@en ;
	rdfs:label "Leading aircraftman (Canada)"@en ;
	rdfs:comment "The specific instance of the Leading aircraftman rank in the context of Canada."@en ;
	owl:rankOf <dbpedia:Canada> .

:Rank_Leading_aircraftman_Commonwealth_of_Nations a :MilitaryRank ;
	owl:subClass :Rank_Leading_aircraftman ;
	foaf:name "Leading aircraftman"@en ;
	rdfs:label "Leading aircraftman (Commonwealth of Nations)"@en , "Leading aircraftman (Samväldet)"@sv , "Leading aircraftman (Kansainyhteisö)"@fi , "Leading aircraftman (Commonwealth of Nations)"@fr , "Leading aircraftman (Commonwealth of Nations)"@de , "Leading aircraftman (Commonwealth delle nazioni)"@it , "Leading aircraftman (Gemenebest van Naties)"@nl , "Leading aircraftman (Samveldet av nasjoner)"@no , "Leading aircraftman (Wspólnota Narodów)"@pl , "Leading aircraftman (Commonwealth)"@pt , "Leading aircraftman (Содружество наций)"@ru , "Leading aircraftman (Mancomunidad de Naciones)"@es ;
	rdfs:comment "The specific instance of the Leading aircraftman rank in the context of country Commonwealth of Nations."@en ;
	owl:rankOf <dbpedia:Commonwealth_of_Nations> .

:Rank_Lord_High_Admiral_of_the_Wash_England a :MilitaryRank ;
	owl:subClass :Rank_Lord_High_Admiral_of_the_Wash ;
	foaf:name "Lord High Admiral of the Wash"@en ;
	rdfs:label "Lord High Admiral of the Wash (England)"@en ;
	rdfs:comment "The specific instance of the Lord High Admiral of the Wash rank in the context of England."@en ;
	owl:rankOf <dbpedia:England> .

:Rank_Lord_High_Admiral_of_the_Wash_Scotland a :MilitaryRank ;
	owl:subClass :Rank_Lord_High_Admiral_of_the_Wash ;
	foaf:name "Lord High Admiral of the Wash"@en ;
	rdfs:label "Lord High Admiral of the Wash (Scotland)"@en , "Lord High Admiral of the Wash (Skottland)"@sv , "Lord High Admiral of the Wash (Skotlanti)"@fi , "Lord High Admiral of the Wash (Écosse)"@fr , "Lord High Admiral of the Wash (Schottland)"@de , "Lord High Admiral of the Wash (Scozia)"@it , "Lord High Admiral of the Wash (Schotland)"@nl , "Lord High Admiral of the Wash (Skottland)"@no , "Lord High Admiral of the Wash (Szkocja)"@pl , "Lord High Admiral of the Wash (Escócia)"@pt , "Lord High Admiral of the Wash (Шотландия)"@ru , "Lord High Admiral of the Wash (Escocia)"@es ;
	rdfs:comment "The specific instance of the Lord High Admiral of the Wash rank in the context of country Scotland."@en ;
	owl:rankOf <dbpedia:Scotland> .

:Rank_Lord_High_Admiral_of_the_Wash_Wales a :MilitaryRank ;
	owl:subClass :Rank_Lord_High_Admiral_of_the_Wash ;
	foaf:name "Lord High Admiral of the Wash"@en ;
	rdfs:label "Lord High Admiral of the Wash (Wales)"@en , "Lord High Admiral of the Wash (Wales)"@sv , "Lord High Admiral of the Wash (Wales)"@fi , "Lord High Admiral of the Wash (Pays de Galles)"@fr , "Lord High Admiral of the Wash (Wales)"@de , "Lord High Admiral of the Wash (Galles)"@it , "Lord High Admiral of the Wash (Wales)"@nl , "Lord High Admiral of the Wash (Wales)"@no , "Lord High Admiral of the Wash (Walia)"@pl , "Lord High Admiral of the Wash (País de Gales)"@pt , "Lord High Admiral of the Wash (Уэльс)"@ru , "Lord High Admiral of the Wash (Gales)"@es ;
	rdfs:comment "The specific instance of the Lord High Admiral of the Wash rank in the context of country Wales."@en ;
	owl:rankOf <dbpedia:Wales> .

<http://rdf.muninn-project.org/ontologies/military#Rank_M%C3%BC%C5%9Fir_Ottoman_Empire> a :MilitaryRank ;
	owl:subClass <http://rdf.muninn-project.org/ontologies/military#Rank_M%C3%BC%C5%9Fir> ;
	foaf:name "Müşir"@en ;
	rdfs:label "Müşir (Ottoman Empire)"@en , "Müşir (Osmanska riket)"@sv , "Müşir (Osmanien valtakunta)"@fi , "Müşir (Empire ottoman)"@fr , "Müşir (Osmanisches Reich)"@de , "Müşir (Impero ottomano)"@it , "Müşir (Ottomaanse Rijk)"@nl , "Müşir (Det osmanske rike)"@no , "Müşir (Imperium osmańskie)"@pl , "Müşir (Império Otomano)"@pt , "Müşir (Османская империя)"@ru , "Müşir (Imperio otomano)"@es ;
	rdfs:comment "The specific instance of the Müşir rank in the context of country Ottoman Empire."@en ;
	owl:rankOf <dbpedia:Ottoman_Empire> .

<http://rdf.muninn-project.org/ontologies/military#Rank_M%C3%BC%C5%9Fir_Cossack_Hetmanate> a :MilitaryRank ;
	owl:subClass <http://rdf.muninn-project.org/ontologies/military#Rank_M%C3%BC%C5%9Fir> ;
	foaf:name "Müşir"@en ;
	rdfs:label "Müşir (Cossack Hetmanate)"@en , "Müşir (Hetmanat cosaque)"@fr , "Müşir (Hetmanat)"@de , "Müşir (Hetmańszczyzna)"@pl , "Müşir (Гетманщина)"@ru , "Müşir (Hetmanato cosaco)"@es ;
	rdfs:comment "The specific instance of the Müşir rank in the context of country Cossack Hetmanate."@en ;
	owl:rankOf <dbpedia:Cossack_Hetmanate> .

<http://rdf.muninn-project.org/ontologies/military#Rank_M%C3%BC%C5%9Fir_Septinsular_Republic> a :MilitaryRank ;
	owl:subClass <http://rdf.muninn-project.org/ontologies/military#Rank_M%C3%BC%C5%9Fir> ;
	foaf:name "Müşir"@en ;
	rdfs:label "Müşir (Septinsular Republic)"@en , "Müşir (République des Sept-Îles)"@fr , "Müşir (Repubblica delle Sette Isole Unite)"@it , "Müşir (Republiek van de Zeven Eilanden)"@nl , "Müşir (Republika Siedmiu Wysp)"@pl , "Müşir (Республика Семи Островов)"@ru , "Müşir (República de las Islas Jónicas)"@es ;
	rdfs:comment "The specific instance of the Müşir rank in the context of country Septinsular Republic."@en ;
	owl:rankOf <dbpedia:Septinsular_Republic> .

:Rank_Mirliva_Ottoman_Empire a :MilitaryRank ;
	owl:subClass :Rank_Mirliva ;
	foaf:name "Mirliva"@en ;
	rdfs:label "Mirliva (Ottoman Empire)"@en , "Mirliva (Osmanska riket)"@sv , "Mirliva (Osmanien valtakunta)"@fi , "Mirliva (Empire ottoman)"@fr , "Mirliva (Osmanisches Reich)"@de , "Mirliva (Impero ottomano)"@it , "Mirliva (Ottomaanse Rijk)"@nl , "Mirliva (Det osmanske rike)"@no , "Mirliva (Imperium osmańskie)"@pl , "Mirliva (Império Otomano)"@pt , "Mirliva (Османская империя)"@ru , "Mirliva (Imperio otomano)"@es ;
	rdfs:comment "The specific instance of the Mirliva rank in the context of country Ottoman Empire."@en ;
	owl:rankOf <dbpedia:Ottoman_Empire> .

:Rank_Mirliva_Cossack_Hetmanate a :MilitaryRank ;
	owl:subClass :Rank_Mirliva ;
	foaf:name "Mirliva"@en ;
	rdfs:label "Mirliva (Cossack Hetmanate)"@en , "Mirliva (Hetmanat cosaque)"@fr , "Mirliva (Hetmanat)"@de , "Mirliva (Hetmańszczyzna)"@pl , "Mirliva (Гетманщина)"@ru , "Mirliva (Hetmanato cosaco)"@es ;
	rdfs:comment "The specific instance of the Mirliva rank in the context of country Cossack Hetmanate."@en ;
	owl:rankOf <dbpedia:Cossack_Hetmanate> .

:Rank_Mirliva_Septinsular_Republic a :MilitaryRank ;
	owl:subClass :Rank_Mirliva ;
	foaf:name "Mirliva"@en ;
	rdfs:label "Mirliva (Septinsular Republic)"@en , "Mirliva (République des Sept-Îles)"@fr , "Mirliva (Repubblica delle Sette Isole Unite)"@it , "Mirliva (Republiek van de Zeven Eilanden)"@nl , "Mirliva (Republika Siedmiu Wysp)"@pl , "Mirliva (Республика Семи Островов)"@ru , "Mirliva (República de las Islas Jónicas)"@es ;
	rdfs:comment "The specific instance of the Mirliva rank in the context of country Septinsular Republic."@en ;
	owl:rankOf <dbpedia:Septinsular_Republic> .

<http://rdf.muninn-project.org/ontologies/military#Rank_Ordinary_seaman_%28rating%29_Australia> a :MilitaryRank ;
	owl:subClass <http://rdf.muninn-project.org/ontologies/military#Rank_Ordinary_seaman_%28rating%29> ;
	foaf:name ""@en ;
	rdfs:label "(Australia)"@en , "(Australien)"@sv , "(Australia)"@fi , "(Australie)"@fr , "(Australien)"@de , "(Australia)"@it , "(Australië (land))"@nl , "(Australia)"@no , "(Australia)"@pl , "(Austrália)"@pt , "(Австралия)"@ru , "(Australia)"@es ;
	rdfs:comment "The specific instance of the  rank in the context of country Australia."@en ;
	owl:rankOf <dbpedia:Australia> .

<http://rdf.muninn-project.org/ontologies/military#Rank_Ordinary_seaman_%28rating%29_Canada> a :MilitaryRank ;
	owl:subClass <http://rdf.muninn-project.org/ontologies/military#Rank_Ordinary_seaman_%28rating%29> ;
	foaf:name "Ordinary Seaman"@en ;
	rdfs:label "Ordinary Seaman (Canada)"@en ;
	rdfs:comment "The specific instance of the  rank in the context of Canada."@en ;
	owl:rankOf <dbpedia:Canada> .

<http://rdf.muninn-project.org/ontologies/military#Rank_Ordinary_seaman_%28rating%29_Commonwealth_of_Nations> a :MilitaryRank ;
	owl:subClass <http://rdf.muninn-project.org/ontologies/military#Rank_Ordinary_seaman_%28rating%29> ;
	foaf:name "Ordinary Seaman"@en ;
	rdfs:label "Ordinary Seaman (Commonwealth of Nations)"@en , "Ordinary Seaman (Samväldet)"@sv , "Ordinary Seaman (Kansainyhteisö)"@fi , "Ordinary Seaman (Commonwealth of Nations)"@fr , "Ordinary Seaman (Commonwealth of Nations)"@de , "Ordinary Seaman (Commonwealth delle nazioni)"@it , "Ordinary Seaman (Gemenebest van Naties)"@nl , "Ordinary Seaman (Samveldet av nasjoner)"@no , "Ordinary Seaman (Wspólnota Narodów)"@pl , "Ordinary Seaman (Commonwealth)"@pt , "Ordinary Seaman (Содружество наций)"@ru , "Ordinary Seaman (Mancomunidad de Naciones)"@es ;
	rdfs:comment "The specific instance of the  rank in the context of country Commonwealth of Nations."@en ;
	owl:rankOf <dbpedia:Commonwealth_of_Nations> .

:Rank_Poruchik_Poland a :MilitaryRank ;
	owl:subClass :Rank_Poruchik ;
	foaf:name "Poruchik"@en ;
	rdfs:label "Poruchik (Poland)"@en , "Porutschik (Poland)"@de , "Poručik (Poland)"@it , "Poroetsjik (Poland)"@nl , "Поручик (Poland)"@ru ;
	rdfs:comment "The specific instance of the Poruchik rank in the context of Poland."@en ;
	owl:rankOf <dbpedia:Poland> .

:Rank_Poruchik_Russia a :MilitaryRank ;
	owl:subClass :Rank_Poruchik ;
	foaf:name "Поручик"@ru ;
	rdfs:label "Poruchik (Russia)"@en , "Poruchik (Ryssland)"@sv , "Poruchik (Venäjä)"@fi , "Poruchik (Russie)"@fr , "Porutschik (Russland)"@de , "Poručik (Russia)"@it , "Poroetsjik (Rusland)"@nl , "Poruchik (Russland)"@no , "Poruchik (Rosja)"@pl , "Poruchik (Rússia)"@pt , "Поручик (Россия)"@ru , "Poruchik (Rusia)"@es ;
	rdfs:comment "The specific instance of the Poruchik rank in the context of country Russia."@en ;
	owl:rankOf <dbpedia:Russia> .

:Rank_Poruchik_Soviet_Union a :MilitaryRank ;
	owl:subClass :Rank_Poruchik ;
	foaf:name "Poruchik"@en ;
	rdfs:label "Poruchik (Soviet Union)"@en , "Poruchik (Sovjetunionen)"@sv , "Poruchik (Neuvostoliitto)"@fi , "Poruchik (Union des républiques socialistes soviétiques)"@fr , "Porutschik (Sowjetunion)"@de , "Poručik (Unione Sovietica)"@it , "Poroetsjik (Sovjet-Unie)"@nl , "Poruchik (Sovjetunionen)"@no , "Poruchik (Związek Socjalistycznych Republik Radzieckich)"@pl , "Poruchik (União Soviética)"@pt , "Поручик (Союз Советских Социалистических Республик)"@ru , "Poruchik (Unión Soviética)"@es ;
	rdfs:comment "The specific instance of the Poruchik rank in the context of country Soviet Union."@en ;
	owl:rankOf <dbpedia:Soviet_Union> .

:Rank_Regimental_sergeant_major_Australia a :MilitaryRank ;
	owl:subClass :Rank_Regimental_sergeant_major ;
	foaf:name "Regimental sergeant major"@en ;
	rdfs:label "Regimental sergeant major (Australia)"@en , "Regimental sergeant major (Australien)"@sv , "Regimental sergeant major (Australia)"@fi , "Regimental sergeant major (Australie)"@fr , "Regimental sergeant major (Australien)"@de , "Regimental sergeant major (Australia)"@it , "Regimental sergeant major (Australië (land))"@nl , "Regimental sergeant major (Australia)"@no , "Regimental sergeant major (Australia)"@pl , "Regimental sergeant major (Austrália)"@pt , "Regimental sergeant major (Австралия)"@ru , "Regimental sergeant major (Australia)"@es ;
	rdfs:comment "The specific instance of the Regimental sergeant major rank in the context of country Australia."@en ;
	owl:rankOf <dbpedia:Australia> .

:Rank_Regimental_sergeant_major_Singapore a :MilitaryRank ;
	owl:subClass :Rank_Regimental_sergeant_major ;
	foaf:name "Regimental sergeant major"@en ;
	rdfs:label "Regimental sergeant major (Singapore)"@en , "Regimental sergeant major (Singapore)"@sv , "Regimental sergeant major (Singapore)"@fi , "Regimental sergeant major (Singapour)"@fr , "Regimental sergeant major (Singapur)"@de , "Regimental sergeant major (Singapore)"@it , "Regimental sergeant major (Singapore)"@nl , "Regimental sergeant major (Singapore)"@no , "Regimental sergeant major (Singapur)"@pl , "Regimental sergeant major (Singapura)"@pt , "Regimental sergeant major (Сингапур)"@ru , "Regimental sergeant major (Singapur)"@es ;
	rdfs:comment "The specific instance of the Regimental sergeant major rank in the context of country Singapore."@en ;
	owl:rankOf <dbpedia:Singapore> .

:Rank_Regimental_sergeant_major_Commonwealth_of_Nations a :MilitaryRank ;
	owl:subClass :Rank_Regimental_sergeant_major ;
	foaf:name "Regimental sergeant major"@en ;
	rdfs:label "Regimental sergeant major (Commonwealth of Nations)"@en , "Regimental sergeant major (Samväldet)"@sv , "Regimental sergeant major (Kansainyhteisö)"@fi , "Regimental sergeant major (Commonwealth of Nations)"@fr , "Regimental sergeant major (Commonwealth of Nations)"@de , "Regimental sergeant major (Commonwealth delle nazioni)"@it , "Regimental sergeant major (Gemenebest van Naties)"@nl , "Regimental sergeant major (Samveldet av nasjoner)"@no , "Regimental sergeant major (Wspólnota Narodów)"@pl , "Regimental sergeant major (Commonwealth)"@pt , "Regimental sergeant major (Содружество наций)"@ru , "Regimental sergeant major (Mancomunidad de Naciones)"@es ;
	rdfs:comment "The specific instance of the Regimental sergeant major rank in the context of country Commonwealth of Nations."@en ;
	owl:rankOf <dbpedia:Commonwealth_of_Nations> .

:Rank_Schout-bij-nacht_Netherlands a :MilitaryRank ;
	owl:subClass :Rank_Schout-bij-nacht ;
	foaf:name "Schout-bij-nacht"@en , "Schout-bij-nacht"@nl ;
	rdfs:label "Schout-bij-nacht (Netherlands)"@en , "Schoutbynacht (Nederländerna)"@sv , "Schout-bij-nacht (Alankomaat)"@fi , "Schout-bij-nacht (Pays-Bas)"@fr , "Schout-bij-nacht (Niederlande)"@de , "Schout-bij-nacht (Paesi Bassi)"@it , "Schout-bij-nacht (Nederland)"@nl , "Schoutbynacht (Nederland)"@no , "Schout-bij-nacht (Holandia)"@pl , "Schout-bij-nacht (Países Baixos)"@pt , "Шаутбенахт (Нидерланды)"@ru , "Schout-bij-nacht (Países Bajos)"@es ;
	rdfs:comment "The specific instance of the Schout-bij-nacht rank in the context of country Netherlands."@en ;
	owl:rankOf <dbpedia:Netherlands> .

:Rank_Schout-bij-nacht_Russia a :MilitaryRank ;
	owl:subClass :Rank_Schout-bij-nacht ;
	foaf:name "Шаутбенахт"@ru ;
	rdfs:label "Schout-bij-nacht (Russia)"@en , "Schoutbynacht (Ryssland)"@sv , "Schout-bij-nacht (Venäjä)"@fi , "Schout-bij-nacht (Russie)"@fr , "Schout-bij-nacht (Russland)"@de , "Schout-bij-nacht (Russia)"@it , "Schout-bij-nacht (Rusland)"@nl , "Schoutbynacht (Russland)"@no , "Schout-bij-nacht (Rosja)"@pl , "Schout-bij-nacht (Rússia)"@pt , "Шаутбенахт (Россия)"@ru , "Schout-bij-nacht (Rusia)"@es ;
	rdfs:comment "The specific instance of the Schout-bij-nacht rank in the context of country Russia."@en ;
	owl:rankOf <dbpedia:Russia> .

:Rank_Schout-bij-nacht_Soviet_Union a :MilitaryRank ;
	owl:subClass :Rank_Schout-bij-nacht ;
	foaf:name "Schout-bij-nacht"@en ;
	rdfs:label "Schout-bij-nacht (Soviet Union)"@en , "Schoutbynacht (Sovjetunionen)"@sv , "Schout-bij-nacht (Neuvostoliitto)"@fi , "Schout-bij-nacht (Union des républiques socialistes soviétiques)"@fr , "Schout-bij-nacht (Sowjetunion)"@de , "Schout-bij-nacht (Unione Sovietica)"@it , "Schout-bij-nacht (Sovjet-Unie)"@nl , "Schoutbynacht (Sovjetunionen)"@no , "Schout-bij-nacht (Związek Socjalistycznych Republik Radzieckich)"@pl , "Schout-bij-nacht (União Soviética)"@pt , "Шаутбенахт (Союз Советских Социалистических Республик)"@ru , "Schout-bij-nacht (Unión Soviética)"@es ;
	rdfs:comment "The specific instance of the Schout-bij-nacht rank in the context of country Soviet Union."@en ;
	owl:rankOf <dbpedia:Soviet_Union> .

:Rank_Second_Corporal_England a :MilitaryRank ;
	owl:subClass :Rank_Second_Corporal ;
	foaf:name "Second Corporal"@en ;
	rdfs:label "Second Corporal (England)"@en ;
	rdfs:comment "The specific instance of the Second Corporal rank in the context of England."@en ;
	owl:rankOf <dbpedia:England> .

:Rank_Second_Corporal_Scotland a :MilitaryRank ;
	owl:subClass :Rank_Second_Corporal ;
	foaf:name "Second Corporal"@en ;
	rdfs:label "Second Corporal (Scotland)"@en , "Second Corporal (Skottland)"@sv , "Second Corporal (Skotlanti)"@fi , "Second Corporal (Écosse)"@fr , "Second Corporal (Schottland)"@de , "Second Corporal (Scozia)"@it , "Second Corporal (Schotland)"@nl , "Second Corporal (Skottland)"@no , "Second Corporal (Szkocja)"@pl , "Second Corporal (Escócia)"@pt , "Second Corporal (Шотландия)"@ru , "Second Corporal (Escocia)"@es ;
	rdfs:comment "The specific instance of the Second Corporal rank in the context of country Scotland."@en ;
	owl:rankOf <dbpedia:Scotland> .

:Rank_Second_Corporal_Wales a :MilitaryRank ;
	owl:subClass :Rank_Second_Corporal ;
	foaf:name "Second Corporal"@en ;
	rdfs:label "Second Corporal (Wales)"@en , "Second Corporal (Wales)"@sv , "Second Corporal (Wales)"@fi , "Second Corporal (Pays de Galles)"@fr , "Second Corporal (Wales)"@de , "Second Corporal (Galles)"@it , "Second Corporal (Wales)"@nl , "Second Corporal (Wales)"@no , "Second Corporal (Walia)"@pl , "Second Corporal (País de Gales)"@pt , "Second Corporal (Уэльс)"@ru , "Second Corporal (Gales)"@es ;
	rdfs:comment "The specific instance of the Second Corporal rank in the context of country Wales."@en ;
	owl:rankOf <dbpedia:Wales> .

:Rank_Sergeant_Major_Instructor_England a :MilitaryRank ;
	owl:subClass :Rank_Sergeant_Major_Instructor ;
	foaf:name "Sergeant Major Instructor"@en ;
	rdfs:label "Sergeant Major Instructor (England)"@en ;
	rdfs:comment "The specific instance of the Sergeant Major Instructor rank in the context of England."@en ;
	owl:rankOf <dbpedia:England> .

:Rank_Sergeant_Major_Instructor_Scotland a :MilitaryRank ;
	owl:subClass :Rank_Sergeant_Major_Instructor ;
	foaf:name "Sergeant Major Instructor"@en ;
	rdfs:label "Sergeant Major Instructor (Scotland)"@en , "Sergeant Major Instructor (Skottland)"@sv , "Sergeant Major Instructor (Skotlanti)"@fi , "Sergeant Major Instructor (Écosse)"@fr , "Sergeant Major Instructor (Schottland)"@de , "Sergeant Major Instructor (Scozia)"@it , "Sergeant Major Instructor (Schotland)"@nl , "Sergeant Major Instructor (Skottland)"@no , "Sergeant Major Instructor (Szkocja)"@pl , "Sergeant Major Instructor (Escócia)"@pt , "Sergeant Major Instructor (Шотландия)"@ru , "Sergeant Major Instructor (Escocia)"@es ;
	rdfs:comment "The specific instance of the Sergeant Major Instructor rank in the context of country Scotland."@en ;
	owl:rankOf <dbpedia:Scotland> .

:Rank_Sergeant_Major_Instructor_Wales a :MilitaryRank ;
	owl:subClass :Rank_Sergeant_Major_Instructor ;
	foaf:name "Sergeant Major Instructor"@en ;
	rdfs:label "Sergeant Major Instructor (Wales)"@en , "Sergeant Major Instructor (Wales)"@sv , "Sergeant Major Instructor (Wales)"@fi , "Sergeant Major Instructor (Pays de Galles)"@fr , "Sergeant Major Instructor (Wales)"@de , "Sergeant Major Instructor (Galles)"@it , "Sergeant Major Instructor (Wales)"@nl , "Sergeant Major Instructor (Wales)"@no , "Sergeant Major Instructor (Walia)"@pl , "Sergeant Major Instructor (País de Gales)"@pt , "Sergeant Major Instructor (Уэльс)"@ru , "Sergeant Major Instructor (Gales)"@es ;
	rdfs:comment "The specific instance of the Sergeant Major Instructor rank in the context of country Wales."@en ;
	owl:rankOf <dbpedia:Wales> .

:Rank_Sotnik_Ukraine a :MilitaryRank ;
	owl:subClass :Rank_Sotnik ;
	foaf:name "Сотник"@ru ;
	rdfs:label "Sotnik (Ukraine)"@en , "Sotnik (Ukraina)"@sv , "Sotnik (Ukraina)"@fi , "Sotnik (Ukraine)"@fr , "Sotnik (Ukraine)"@de , "Sotnik (Ucraina)"@it , "Sotnik (Oekraïne)"@nl , "Sotnik (Ukraina)"@no , "Sotnik (Ukraina)"@pl , "Sótnik (Ucrânia)"@pt , "Сотник (Украина)"@ru , "Sotnik (Ucrania)"@es ;
	rdfs:comment "The specific instance of the Sotnik rank in the context of country Ukraine."@en ;
	owl:rankOf <dbpedia:Ukraine> .

:Rank_Sotnik_Russia a :MilitaryRank ;
	owl:subClass :Rank_Sotnik ;
	foaf:name "Сотник"@ru ;
	rdfs:label "Sotnik (Russia)"@en , "Sotnik (Ryssland)"@sv , "Sotnik (Venäjä)"@fi , "Sotnik (Russie)"@fr , "Sotnik (Russland)"@de , "Sotnik (Russia)"@it , "Sotnik (Rusland)"@nl , "Sotnik (Russland)"@no , "Sotnik (Rosja)"@pl , "Sótnik (Rússia)"@pt , "Сотник (Россия)"@ru , "Sotnik (Rusia)"@es ;
	rdfs:comment "The specific instance of the Sotnik rank in the context of country Russia."@en ;
	owl:rankOf <dbpedia:Russia> .

:Rank_Sotnik_Soviet_Union a :MilitaryRank ;
	owl:subClass :Rank_Sotnik ;
	foaf:name "Sotnik"@en ;
	rdfs:label "Sotnik (Soviet Union)"@en , "Sotnik (Sovjetunionen)"@sv , "Sotnik (Neuvostoliitto)"@fi , "Sotnik (Union des républiques socialistes soviétiques)"@fr , "Sotnik (Sowjetunion)"@de , "Sotnik (Unione Sovietica)"@it , "Sotnik (Sovjet-Unie)"@nl , "Sotnik (Sovjetunionen)"@no , "Sotnik (Związek Socjalistycznych Republik Radzieckich)"@pl , "Sótnik (União Soviética)"@pt , "Сотник (Союз Советских Социалистических Республик)"@ru , "Sotnik (Unión Soviética)"@es ;
	rdfs:comment "The specific instance of the Sotnik rank in the context of country Soviet Union."@en ;
	owl:rankOf <dbpedia:Soviet_Union> .

<http://rdf.muninn-project.org/ontologies/military#Rank_Stabskapit%C3%A4nleutnant_Germany> a :MilitaryRank ;
	owl:subClass <http://rdf.muninn-project.org/ontologies/military#Rank_Stabskapit%C3%A4nleutnant> ;
	foaf:name "Stabskapitänleutnant"@de ;
	rdfs:label "Stabskapitänleutnant (Germany)"@en , "Stabskapitänleutnant (Germany)"@de ;
	rdfs:comment "The specific instance of the Stabskapitänleutnant rank in the context of Germany."@en ;
	owl:rankOf <dbpedia:Germany> .

<http://rdf.muninn-project.org/ontologies/military#Rank_Stabskapit%C3%A4n_Germany> a :MilitaryRank ;
	owl:subClass <http://rdf.muninn-project.org/ontologies/military#Rank_Stabskapit%C3%A4n> ;
	foaf:name "Stabskapitän"@de ;
	rdfs:label "Stabskapitän (Germany)"@en , "Alikapteeni (Germany)"@fi , "Stabskapitän (Germany)"@de , "Sztabskapitan (Germany)"@pl , "Штабс-капитан (Germany)"@ru ;
	rdfs:comment "The specific instance of the Stabskapitän rank in the context of Germany."@en ;
	owl:rankOf <dbpedia:Germany> .

<http://rdf.muninn-project.org/ontologies/military#Rank_Stabskapit%C3%A4n_Russia> a :MilitaryRank ;
	owl:subClass <http://rdf.muninn-project.org/ontologies/military#Rank_Stabskapit%C3%A4n> ;
	foaf:name "Штабс-капитан"@ru ;
	rdfs:label "Stabskapitän (Russia)"@en , "Stabskapitän (Ryssland)"@sv , "Alikapteeni (Venäjä)"@fi , "Stabskapitän (Russie)"@fr , "Stabskapitän (Russland)"@de , "Stabskapitän (Russia)"@it , "Stabskapitän (Rusland)"@nl , "Stabskapitän (Russland)"@no , "Sztabskapitan (Rosja)"@pl , "Stabskapitän (Rússia)"@pt , "Штабс-капитан (Россия)"@ru , "Stabskapitän (Rusia)"@es ;
	rdfs:comment "The specific instance of the Stabskapitän rank in the context of country Russia."@en ;
	owl:rankOf <dbpedia:Russia> .

<http://rdf.muninn-project.org/ontologies/military#Rank_Stabskapit%C3%A4n_Soviet_Union> a :MilitaryRank ;
	owl:subClass <http://rdf.muninn-project.org/ontologies/military#Rank_Stabskapit%C3%A4n> ;
	foaf:name "Stabskapitän"@en ;
	rdfs:label "Stabskapitän (Soviet Union)"@en , "Stabskapitän (Sovjetunionen)"@sv , "Alikapteeni (Neuvostoliitto)"@fi , "Stabskapitän (Union des républiques socialistes soviétiques)"@fr , "Stabskapitän (Sowjetunion)"@de , "Stabskapitän (Unione Sovietica)"@it , "Stabskapitän (Sovjet-Unie)"@nl , "Stabskapitän (Sovjetunionen)"@no , "Sztabskapitan (Związek Socjalistycznych Republik Radzieckich)"@pl , "Stabskapitän (União Soviética)"@pt , "Штабс-капитан (Союз Советских Социалистических Республик)"@ru , "Stabskapitän (Unión Soviética)"@es ;
	rdfs:comment "The specific instance of the Stabskapitän rank in the context of country Soviet Union."@en ;
	owl:rankOf <dbpedia:Soviet_Union> .

:Rank_Staff_Corporal_England a :MilitaryRank ;
	owl:subClass :Rank_Staff_Corporal ;
	foaf:name "Staff Corporal"@en ;
	rdfs:label "Staff Corporal (England)"@en ;
	rdfs:comment "The specific instance of the Staff Corporal rank in the context of England."@en ;
	owl:rankOf <dbpedia:England> .

:Rank_Staff_Corporal_Scotland a :MilitaryRank ;
	owl:subClass :Rank_Staff_Corporal ;
	foaf:name "Staff Corporal"@en ;
	rdfs:label "Staff Corporal (Scotland)"@en , "Staff Corporal (Skottland)"@sv , "Staff Corporal (Skotlanti)"@fi , "Staff Corporal (Écosse)"@fr , "Staff Corporal (Schottland)"@de , "Staff Corporal (Scozia)"@it , "Staff Corporal (Schotland)"@nl , "Staff Corporal (Skottland)"@no , "Staff Corporal (Szkocja)"@pl , "Staff Corporal (Escócia)"@pt , "Staff Corporal (Шотландия)"@ru , "Staff Corporal (Escocia)"@es ;
	rdfs:comment "The specific instance of the Staff Corporal rank in the context of country Scotland."@en ;
	owl:rankOf <dbpedia:Scotland> .

:Rank_Staff_Corporal_Wales a :MilitaryRank ;
	owl:subClass :Rank_Staff_Corporal ;
	foaf:name "Staff Corporal"@en ;
	rdfs:label "Staff Corporal (Wales)"@en , "Staff Corporal (Wales)"@sv , "Staff Corporal (Wales)"@fi , "Staff Corporal (Pays de Galles)"@fr , "Staff Corporal (Wales)"@de , "Staff Corporal (Galles)"@it , "Staff Corporal (Wales)"@nl , "Staff Corporal (Wales)"@no , "Staff Corporal (Walia)"@pl , "Staff Corporal (País de Gales)"@pt , "Staff Corporal (Уэльс)"@ru , "Staff Corporal (Gales)"@es ;
	rdfs:comment "The specific instance of the Staff Corporal rank in the context of country Wales."@en ;
	owl:rankOf <dbpedia:Wales> .

:Rank_Staff_Sergeant_Major_England a :MilitaryRank ;
	owl:subClass :Rank_Staff_Sergeant_Major ;
	foaf:name "Staff Sergeant Major"@en ;
	rdfs:label "Staff Sergeant Major (England)"@en ;
	rdfs:comment "The specific instance of the Staff Sergeant Major rank in the context of England."@en ;
	owl:rankOf <dbpedia:England> .

:Rank_Staff_Sergeant_Major_Scotland a :MilitaryRank ;
	owl:subClass :Rank_Staff_Sergeant_Major ;
	foaf:name "Staff Sergeant Major"@en ;
	rdfs:label "Staff Sergeant Major (Scotland)"@en , "Staff Sergeant Major (Skottland)"@sv , "Staff Sergeant Major (Skotlanti)"@fi , "Staff Sergeant Major (Écosse)"@fr , "Staff Sergeant Major (Schottland)"@de , "Staff Sergeant Major (Scozia)"@it , "Staff Sergeant Major (Schotland)"@nl , "Staff Sergeant Major (Skottland)"@no , "Staff Sergeant Major (Szkocja)"@pl , "Staff Sergeant Major (Escócia)"@pt , "Staff Sergeant Major (Шотландия)"@ru , "Staff Sergeant Major (Escocia)"@es ;
	rdfs:comment "The specific instance of the Staff Sergeant Major rank in the context of country Scotland."@en ;
	owl:rankOf <dbpedia:Scotland> .

:Rank_Staff_Sergeant_Major_Wales a :MilitaryRank ;
	owl:subClass :Rank_Staff_Sergeant_Major ;
	foaf:name "Staff Sergeant Major"@en ;
	rdfs:label "Staff Sergeant Major (Wales)"@en , "Staff Sergeant Major (Wales)"@sv , "Staff Sergeant Major (Wales)"@fi , "Staff Sergeant Major (Pays de Galles)"@fr , "Staff Sergeant Major (Wales)"@de , "Staff Sergeant Major (Galles)"@it , "Staff Sergeant Major (Wales)"@nl , "Staff Sergeant Major (Wales)"@no , "Staff Sergeant Major (Walia)"@pl , "Staff Sergeant Major (País de Gales)"@pt , "Staff Sergeant Major (Уэльс)"@ru , "Staff Sergeant Major (Gales)"@es ;
	rdfs:comment "The specific instance of the Staff Sergeant Major rank in the context of country Wales."@en ;
	owl:rankOf <dbpedia:Wales> .

:Rank_Starshina_Ukraine a :MilitaryRank ;
	owl:subClass :Rank_Starshina ;
	foaf:name "Старшина"@ru ;
	rdfs:label "Starshina (Ukraine)"@en , "Starshina (Ukraina)"@sv , "Starshina (Ukraina)"@fi , "Starshina (Ukraine)"@fr , "Starshina (Ukraine)"@de , "Starshina (Ucraina)"@it , "Starshina (Oekraïne)"@nl , "Starshina (Ukraina)"@no , "Starshina (Ukraina)"@pl , "Starshina (Ucrânia)"@pt , "Старшина (Украина)"@ru , "Starshiná (Ucrania)"@es ;
	rdfs:comment "The specific instance of the Starshina rank in the context of country Ukraine."@en ;
	owl:rankOf <dbpedia:Ukraine> .

:Rank_Starshina_Russia a :MilitaryRank ;
	owl:subClass :Rank_Starshina ;
	foaf:name "Старшина"@ru ;
	rdfs:label "Starshina (Russia)"@en , "Starshina (Ryssland)"@sv , "Starshina (Venäjä)"@fi , "Starshina (Russie)"@fr , "Starshina (Russland)"@de , "Starshina (Russia)"@it , "Starshina (Rusland)"@nl , "Starshina (Russland)"@no , "Starshina (Rosja)"@pl , "Starshina (Rússia)"@pt , "Старшина (Россия)"@ru , "Starshiná (Rusia)"@es ;
	rdfs:comment "The specific instance of the Starshina rank in the context of country Russia."@en ;
	owl:rankOf <dbpedia:Russia> .

:Rank_Starshina_Soviet_Union a :MilitaryRank ;
	owl:subClass :Rank_Starshina ;
	foaf:name "Starshina"@en ;
	rdfs:label "Starshina (Soviet Union)"@en , "Starshina (Sovjetunionen)"@sv , "Starshina (Neuvostoliitto)"@fi , "Starshina (Union des républiques socialistes soviétiques)"@fr , "Starshina (Sowjetunion)"@de , "Starshina (Unione Sovietica)"@it , "Starshina (Sovjet-Unie)"@nl , "Starshina (Sovjetunionen)"@no , "Starshina (Związek Socjalistycznych Republik Radzieckich)"@pl , "Starshina (União Soviética)"@pt , "Старшина (Союз Советских Социалистических Республик)"@ru , "Starshiná (Unión Soviética)"@es ;
	rdfs:comment "The specific instance of the Starshina rank in the context of country Soviet Union."@en ;
	owl:rankOf <dbpedia:Soviet_Union> .

:Rank_Stratarches_Greece a :MilitaryRank ;
	owl:subClass :Rank_Stratarches ;
	foaf:name "Stratarches"@en ;
	rdfs:label "Stratarches (Greece)"@en , "Stratarches (Grekland)"@sv , "Stratarches (Kreikka)"@fi , "Stratarches (Grèce)"@fr , "Stratarches (Griechenland)"@de , "Stratarches (Grecia)"@it , "Stratarches (Griekenland)"@nl , "Stratarches (Hellas)"@no , "Stratarches (Grecja)"@pl , "Stratarches (Grécia)"@pt , "Stratarches (Греция)"@ru , "Stratarches (Grecia)"@es ;
	rdfs:comment "The specific instance of the Stratarches rank in the context of country Greece."@en ;
	owl:rankOf <dbpedia:Greece> .

:Rank_Stratarches_Official_Timocracy_of_Sapinetia a :MilitaryRank ;
	owl:subClass :Rank_Stratarches ;
	foaf:name "Stratarches"@en ;
	rdfs:label "Stratarches (Timocracy of Sapinetia)"@en ;
	rdfs:comment "The specific instance of the Stratarches rank in the context of country the Timocracy of Sapinetia."@en ;
	owl:rankOf <dbpedia:Official_Timocracy_of_Sapinetia> .

:Rank_Stratarches_Byzantine_Empire a :MilitaryRank ;
	owl:subClass :Rank_Stratarches ;
	foaf:name "Stratarches"@en ;
	rdfs:label "Stratarches (Byzantine Empire)"@en , "Stratarches (Bysantinska riket)"@sv , "Stratarches (Bysantin valtakunta)"@fi , "Stratarches (Empire byzantin)"@fr , "Stratarches (Byzantinisches Reich)"@de , "Stratarches (Impero bizantino)"@it , "Stratarches (Byzantijnse Rijk)"@nl , "Stratarches (Østromerriket)"@no , "Stratarches (Cesarstwo Bizantyńskie)"@pl , "Stratarches (Império Bizantino)"@pt , "Stratarches (Византийская империя)"@ru , "Stratarches (Imperio bizantino)"@es ;
	rdfs:comment "The specific instance of the Stratarches rank in the context of country Byzantine Empire."@en ;
	owl:rankOf <dbpedia:Byzantine_Empire> .

<dbpedia:Byzantine_Empire> muninn:wikipedia_version "498328033" .

<http://rdf.muninn-project.org/ontologies/military#Rank_Suba%C5%9Fi_Ottoman_Empire> a :MilitaryRank ;
	owl:subClass <http://rdf.muninn-project.org/ontologies/military#Rank_Suba%C5%9Fi> ;
	foaf:name "Subaşi"@en ;
	rdfs:label "Subaşi (Ottoman Empire)"@en , "Subaşi (Osmanska riket)"@sv , "Subaşi (Osmanien valtakunta)"@fi , "Subaşi (Empire ottoman)"@fr , "Subaşi (Osmanisches Reich)"@de , "Subaşi (Impero ottomano)"@it , "Subaşi (Ottomaanse Rijk)"@nl , "Subaşi (Det osmanske rike)"@no , "Subaşi (Imperium osmańskie)"@pl , "Subaşi (Império Otomano)"@pt , "Subaşi (Османская империя)"@ru , "Subaşi (Imperio otomano)"@es ;
	rdfs:comment "The specific instance of the Subaşi rank in the context of country Ottoman Empire."@en ;
	owl:rankOf <dbpedia:Ottoman_Empire> .

<http://rdf.muninn-project.org/ontologies/military#Rank_Suba%C5%9Fi_Cossack_Hetmanate> a :MilitaryRank ;
	owl:subClass <http://rdf.muninn-project.org/ontologies/military#Rank_Suba%C5%9Fi> ;
	foaf:name "Subaşi"@en ;
	rdfs:label "Subaşi (Cossack Hetmanate)"@en , "Subaşi (Hetmanat cosaque)"@fr , "Subaşi (Hetmanat)"@de , "Subaşi (Hetmańszczyzna)"@pl , "Subaşi (Гетманщина)"@ru , "Subaşi (Hetmanato cosaco)"@es ;
	rdfs:comment "The specific instance of the Subaşi rank in the context of country Cossack Hetmanate."@en ;
	owl:rankOf <dbpedia:Cossack_Hetmanate> .

<http://rdf.muninn-project.org/ontologies/military#Rank_Suba%C5%9Fi_Septinsular_Republic> a :MilitaryRank ;
	owl:subClass <http://rdf.muninn-project.org/ontologies/military#Rank_Suba%C5%9Fi> ;
	foaf:name "Subaşi"@en ;
	rdfs:label "Subaşi (Septinsular Republic)"@en , "Subaşi (République des Sept-Îles)"@fr , "Subaşi (Repubblica delle Sette Isole Unite)"@it , "Subaşi (Republiek van de Zeven Eilanden)"@nl , "Subaşi (Republika Siedmiu Wysp)"@pl , "Subaşi (Республика Семи Островов)"@ru , "Subaşi (República de las Islas Jónicas)"@es ;
	rdfs:comment "The specific instance of the Subaşi rank in the context of country Septinsular Republic."@en ;
	owl:rankOf <dbpedia:Septinsular_Republic> .

:Rank_Subaltern_England a :MilitaryRank ;
	owl:subClass :Rank_Subaltern ;
	foaf:name "Subaltern"@en ;
	rdfs:label "Subaltern (England)"@en , "Subalternofficer (England)"@sv , "Subalternoffiser (England)"@no , "Субалтерн-офицер (England)"@ru ;
	rdfs:comment "The specific instance of the Subaltern rank in the context of England."@en ;
	owl:rankOf <dbpedia:England> .

:Rank_Subaltern_Scotland a :MilitaryRank ;
	owl:subClass :Rank_Subaltern ;
	foaf:name "Subaltern"@en ;
	rdfs:label "Subaltern (Scotland)"@en , "Subalternofficer (Skottland)"@sv , "Subaltern (Skotlanti)"@fi , "Subaltern (Écosse)"@fr , "Subaltern (Schottland)"@de , "Subaltern (Scozia)"@it , "Subaltern (Schotland)"@nl , "Subalternoffiser (Skottland)"@no , "Subaltern (Szkocja)"@pl , "Subaltern (Escócia)"@pt , "Субалтерн-офицер (Шотландия)"@ru , "Subaltern (Escocia)"@es ;
	rdfs:comment "The specific instance of the Subaltern rank in the context of country Scotland."@en ;
	owl:rankOf <dbpedia:Scotland> .

:Rank_Subaltern_Wales a :MilitaryRank ;
	owl:subClass :Rank_Subaltern ;
	foaf:name "Subaltern"@en ;
	rdfs:label "Subaltern (Wales)"@en , "Subalternofficer (Wales)"@sv , "Subaltern (Wales)"@fi , "Subaltern (Pays de Galles)"@fr , "Subaltern (Wales)"@de , "Subaltern (Galles)"@it , "Subaltern (Wales)"@nl , "Subalternoffiser (Wales)"@no , "Subaltern (Walia)"@pl , "Subaltern (País de Gales)"@pt , "Субалтерн-офицер (Уэльс)"@ru , "Subaltern (Gales)"@es ;
	rdfs:comment "The specific instance of the Subaltern rank in the context of country Wales."@en ;
	owl:rankOf <dbpedia:Wales> .

<http://rdf.muninn-project.org/ontologies/military#Rank_Trooper_%28rank%29_Australia> a :MilitaryRank ;
	owl:subClass <http://rdf.muninn-project.org/ontologies/military#Rank_Trooper_%28rank%29> ;
	foaf:name "Trooper"@en ;
	rdfs:label "Trooper (rank) (Australia)"@en , "Trooper (rank) (Australien)"@sv , "Trooper (rank) (Australia)"@fi , "Trooper (rank) (Australie)"@fr , "Trooper (rank) (Australien)"@de , "Trooper (rank) (Australia)"@it , "Trooper (rank) (Australië (land))"@nl , "Trooper (rank) (Australia)"@no , "Trooper (rank) (Australia)"@pl , "Trooper (rank) (Austrália)"@pt , "Trooper (rank) (Австралия)"@ru , "Trooper (rank) (Australia)"@es ;
	rdfs:comment "The specific instance of the Trooper (rank) rank in the context of country Australia."@en ;
	owl:rankOf <dbpedia:Australia> .

<http://rdf.muninn-project.org/ontologies/military#Rank_Trooper_%28rank%29_Canada> a :MilitaryRank ;
	owl:subClass <http://rdf.muninn-project.org/ontologies/military#Rank_Trooper_%28rank%29> ;
	foaf:name "Trooper"@en ;
	rdfs:label "Trooper (rank, Canada)"@en ;
	rdfs:comment "The specific instance of the Trooper (rank) rank in the context of Canada."@en ;
	owl:rankOf <dbpedia:Canada> .

<http://rdf.muninn-project.org/ontologies/military#Rank_Trooper_%28rank%29_Commonwealth_of_Nations> a :MilitaryRank ;
	owl:subClass <http://rdf.muninn-project.org/ontologies/military#Rank_Trooper_%28rank%29> ;
	foaf:name "Trooper"@en ;
	rdfs:label "Trooper (rank) (Commonwealth of Nations)"@en , "Trooper (rank) (Samväldet)"@sv , "Trooper (rank) (Kansainyhteisö)"@fi , "Trooper (rank) (Commonwealth of Nations)"@fr , "Trooper (rank) (Commonwealth of Nations)"@de , "Trooper (rank) (Commonwealth delle nazioni)"@it , "Trooper (rank) (Gemenebest van Naties)"@nl , "Trooper (rank) (Samveldet av nasjoner)"@no , "Trooper (rank) (Wspólnota Narodów)"@pl , "Trooper (rank) (Commonwealth)"@pt , "Trooper (rank) (Содружество наций)"@ru , "Trooper (rank) (Mancomunidad de Naciones)"@es ;
	rdfs:comment "The specific instance of the Trooper (rank) rank in the context of country Commonwealth of Nations."@en ;
	owl:rankOf <dbpedia:Commonwealth_of_Nations> .

:Rank_Vice-Admiral_of_the_Coast_England a :MilitaryRank ;
	owl:subClass :Rank_Vice-Admiral_of_the_Coast ;
	foaf:name "Vice-Admiral of the Coast"@en ;
	rdfs:label "Vice-Admiral of the Coast (England)"@en ;
	rdfs:comment "The specific instance of the Vice-Admiral of the Coast rank in the context of country England."@en ;
	owl:rankOf <dbpedia:England> .

:Rank_Vice-Admiral_of_the_Coast_Scotland a :MilitaryRank ;
	owl:subClass :Rank_Vice-Admiral_of_the_Coast ;
	foaf:name "Vice-Admiral of the Coast"@en ;
	rdfs:label "Vice-Admiral of the Coast (Scotland)"@en , "Vice-Admiral of the Coast (Skottland)"@sv , "Vice-Admiral of the Coast (Skotlanti)"@fi , "Vice-Admiral of the Coast (Écosse)"@fr , "Vice-Admiral of the Coast (Schottland)"@de , "Vice-Admiral of the Coast (Scozia)"@it , "Vice-Admiral of the Coast (Schotland)"@nl , "Vice-Admiral of the Coast (Skottland)"@no , "Vice-Admiral of the Coast (Szkocja)"@pl , "Vice-Admiral of the Coast (Escócia)"@pt , "Vice-Admiral of the Coast (Шотландия)"@ru , "Vice-Admiral of the Coast (Escocia)"@es ;
	rdfs:comment "The specific instance of the Vice-Admiral of the Coast rank in the context of country Scotland."@en ;
	owl:rankOf <dbpedia:Scotland> .

:Rank_Vice-Admiral_of_the_Coast_Wales a :MilitaryRank ;
	owl:subClass :Rank_Vice-Admiral_of_the_Coast ;
	foaf:name "Vice-Admiral of the Coast"@en ;
	rdfs:label "Vice-Admiral of the Coast (Wales)"@en , "Vice-Admiral of the Coast (Wales)"@sv , "Vice-Admiral of the Coast (Wales)"@fi , "Vice-Admiral of the Coast (Pays de Galles)"@fr , "Vice-Admiral of the Coast (Wales)"@de , "Vice-Admiral of the Coast (Galles)"@it , "Vice-Admiral of the Coast (Wales)"@nl , "Vice-Admiral of the Coast (Wales)"@no , "Vice-Admiral of the Coast (Walia)"@pl , "Vice-Admiral of the Coast (País de Gales)"@pt , "Vice-Admiral of the Coast (Уэльс)"@ru , "Vice-Admiral of the Coast (Gales)"@es ;
	rdfs:comment "The specific instance of the Vice-Admiral of the Coast rank in the context of country Wales."@en ;
	owl:rankOf <dbpedia:Wales> .

:Rank_Vice-Admiral_of_the_West_England a :MilitaryRank ;
	owl:subClass :Rank_Vice-Admiral_of_the_West ;
	foaf:name "Vice-Admiral of the West"@en ;
	rdfs:label "Vice-Admiral of the West (England)"@en ;
	rdfs:comment "The specific instance of the Vice-Admiral of the West rank in the context of England."@en ;
	owl:rankOf <dbpedia:England> .

:Rank_Vice-Admiral_of_the_West_Scotland a :MilitaryRank ;
	owl:subClass :Rank_Vice-Admiral_of_the_West ;
	foaf:name "Vice-Admiral of the West"@en ;
	rdfs:label "Vice-Admiral of the West (Scotland)"@en , "Vice-Admiral of the West (Skottland)"@sv , "Vice-Admiral of the West (Skotlanti)"@fi , "Vice-Admiral of the West (Écosse)"@fr , "Vice-Admiral of the West (Schottland)"@de , "Vice-Admiral of the West (Scozia)"@it , "Vice-Admiral of the West (Schotland)"@nl , "Vice-Admiral of the West (Skottland)"@no , "Vice-Admiral of the West (Szkocja)"@pl , "Vice-Admiral of the West (Escócia)"@pt , "Vice-Admiral of the West (Шотландия)"@ru , "Vice-Admiral of the West (Escocia)"@es ;
	rdfs:comment "The specific instance of the Vice-Admiral of the West rank in the context of country Scotland."@en ;
	owl:rankOf <dbpedia:Scotland> .

:Rank_Vice-Admiral_of_the_West_Wales a :MilitaryRank ;
	owl:subClass :Rank_Vice-Admiral_of_the_West ;
	foaf:name "Vice-Admiral of the West"@en ;
	rdfs:label "Vice-Admiral of the West (Wales)"@en , "Vice-Admiral of the West (Wales)"@sv , "Vice-Admiral of the West (Wales)"@fi , "Vice-Admiral of the West (Pays de Galles)"@fr , "Vice-Admiral of the West (Wales)"@de , "Vice-Admiral of the West (Galles)"@it , "Vice-Admiral of the West (Wales)"@nl , "Vice-Admiral of the West (Wales)"@no , "Vice-Admiral of the West (Walia)"@pl , "Vice-Admiral of the West (País de Gales)"@pt , "Vice-Admiral of the West (Уэльс)"@ru , "Vice-Admiral of the West (Gales)"@es ;
	rdfs:comment "The specific instance of the Vice-Admiral of the West rank in the context of country Wales."@en ;
	owl:rankOf <dbpedia:Wales> .

:Rank_Wachtmeister_Germany a :MilitaryRank ;
	owl:subClass :Rank_Wachtmeister ;
	foaf:name "Wachtmeister"@de ;
	rdfs:label "Wachtmeister (Germany)"@en , "Wachtmeister (Germany)"@de , "Wachmistrz (Germany)"@pl , "Вахмистр (Germany)"@ru ;
	rdfs:comment "The specific instance of the Wachtmeister rank in the context of Germany."@en ;
	owl:rankOf <dbpedia:Germany> .

:Rank_Wachtmeister_Russia a :MilitaryRank ;
	owl:subClass :Rank_Wachtmeister ;
	foaf:name "Вахмистр"@ru ;
	rdfs:label "Wachtmeister (Russia)"@en , "Wachtmeister (Ryssland)"@sv , "Wachtmeister (Venäjä)"@fi , "Wachtmeister (Russie)"@fr , "Wachtmeister (Russland)"@de , "Wachtmeister (Russia)"@it , "Wachtmeister (Rusland)"@nl , "Wachtmeister (Russland)"@no , "Wachmistrz (Rosja)"@pl , "Wachtmeister (Rússia)"@pt , "Вахмистр (Россия)"@ru , "Wachtmeister (Rusia)"@es ;
	rdfs:comment "The specific instance of the Wachtmeister rank in the context of country Russia."@en ;
	owl:rankOf <dbpedia:Russia> .

:Rank_Wachtmeister_Soviet_Union a :MilitaryRank ;
	owl:subClass :Rank_Wachtmeister ;
	foaf:name "Wachtmeister"@en ;
	rdfs:label "Wachtmeister (Soviet Union)"@en , "Wachtmeister (Sovjetunionen)"@sv , "Wachtmeister (Neuvostoliitto)"@fi , "Wachtmeister (Union des républiques socialistes soviétiques)"@fr , "Wachtmeister (Sowjetunion)"@de , "Wachtmeister (Unione Sovietica)"@it , "Wachtmeister (Sovjet-Unie)"@nl , "Wachtmeister (Sovjetunionen)"@no , "Wachmistrz (Związek Socjalistycznych Republik Radzieckich)"@pl , "Wachtmeister (União Soviética)"@pt , "Вахмистр (Союз Советских Социалистических Республик)"@ru , "Wachtmeister (Unión Soviética)"@es ;
	rdfs:comment "The specific instance of the Wachtmeister rank in the context of country Soviet Union."@en ;
	owl:rankOf <dbpedia:Soviet_Union> .

<http://rdf.muninn-project.org/ontologies/military#Rank_Wing_commander_%28rank%29_Australia> a :MilitaryRank ;
	owl:subClass <http://rdf.muninn-project.org/ontologies/military#Rank_Wing_commander_%28rank%29> ;
	foaf:name "Wing commander"@en ;
	rdfs:label "Wing commander (rank) (Australia)"@en , "Wing commander (rank) (Australien)"@sv , "Wing commander (rank) (Australia)"@fi , "Wing commander (rank) (Australie)"@fr , "Wing commander (rank) (Australien)"@de , "Wing commander (rank) (Australia)"@it , "Wing commander (rank) (Australië (land))"@nl , "Wing commander (rank) (Australia)"@no , "Wing commander (rank) (Australia)"@pl , "Wing commander (rank) (Austrália)"@pt , "Wing commander (rank) (Австралия)"@ru , "Wing commander (rank) (Australia)"@es ;
	rdfs:comment "The specific instance of the Wing commander (rank) rank in the context of country Australia."@en ;
	owl:rankOf <dbpedia:Australia> .

<http://rdf.muninn-project.org/ontologies/military#Rank_Wing_commander_%28rank%29_Canada> a :MilitaryRank ;
	owl:subClass <http://rdf.muninn-project.org/ontologies/military#Rank_Wing_commander_%28rank%29> ;
	foaf:name "Wing commander"@en ;
	rdfs:label "Wing commander (rank, Canada)"@en ;
	rdfs:comment "The specific instance of the Wing commander (rank) rank in the context of Canada."@en ;
	owl:rankOf <dbpedia:Canada> .

<http://rdf.muninn-project.org/ontologies/military#Rank_Wing_commander_%28rank%29_Commonwealth_of_Nations> a :MilitaryRank ;
	owl:subClass <http://rdf.muninn-project.org/ontologies/military#Rank_Wing_commander_%28rank%29> ;
	foaf:name "Wing commander"@en ;
	rdfs:label "Wing commander (rank) (Commonwealth of Nations)"@en , "Wing commander (rank) (Samväldet)"@sv , "Wing commander (rank) (Kansainyhteisö)"@fi , "Wing commander (rank) (Commonwealth of Nations)"@fr , "Wing commander (rank) (Commonwealth of Nations)"@de , "Wing commander (rank) (Commonwealth delle nazioni)"@it , "Wing commander (rank) (Gemenebest van Naties)"@nl , "Wing commander (rank) (Samveldet av nasjoner)"@no , "Wing commander (rank) (Wspólnota Narodów)"@pl , "Wing commander (rank) (Commonwealth)"@pt , "Wing commander (rank) (Содружество наций)"@ru , "Wing commander (rank) (Mancomunidad de Naciones)"@es ;
	rdfs:comment "The specific instance of the Wing commander (rank) rank in the context of country Commonwealth of Nations."@en ;
	owl:rankOf <dbpedia:Commonwealth_of_Nations> .

:Rank_Yesaul_Ukraine a :MilitaryRank ;
	owl:subClass :Rank_Yesaul ;
	foaf:name "Есаул"@ru ;
	rdfs:label "Yesaul (Ukraine)"@en , "Jesaul (Ukraina)"@sv , "Yesaul (Ukraina)"@fi , "Yesaul (Ukraine)"@fr , "Jessaul (Ukraine)"@de , "Yesaul (Ucraina)"@it , "Yesaul (Oekraïne)"@nl , "Yesaul (Ukraina)"@no , "Esauł (Ukraina)"@pl , "Yesaul (Ucrânia)"@pt , "Есаул (Украина)"@ru , "Yesaul (Ucrania)"@es ;
	rdfs:comment "The specific instance of the Yesaul rank in the context of country Ukraine."@en ;
	owl:rankOf <dbpedia:Ukraine> .

:Rank_Yesaul_Russia a :MilitaryRank ;
	owl:subClass :Rank_Yesaul ;
	foaf:name "Есаул"@ru ;
	rdfs:label "Yesaul (Russia)"@en , "Jesaul (Ryssland)"@sv , "Yesaul (Venäjä)"@fi , "Yesaul (Russie)"@fr , "Jessaul (Russland)"@de , "Yesaul (Russia)"@it , "Yesaul (Rusland)"@nl , "Yesaul (Russland)"@no , "Esauł (Rosja)"@pl , "Yesaul (Rússia)"@pt , "Есаул (Россия)"@ru , "Yesaul (Rusia)"@es ;
	rdfs:comment "The specific instance of the Yesaul rank in the context of country Russia."@en ;
	owl:rankOf <dbpedia:Russia> .

<dbpedia:Russia> muninn:wikipedia_version "498386672" .

:Rank_Yesaul_Soviet_Union a :MilitaryRank ;
	owl:subClass :Rank_Yesaul ;
	foaf:name "Yesaul"@en ;
	rdfs:label "Yesaul (Soviet Union)"@en , "Jesaul (Sovjetunionen)"@sv , "Yesaul (Neuvostoliitto)"@fi , "Yesaul (Union des républiques socialistes soviétiques)"@fr , "Jessaul (Sowjetunion)"@de , "Yesaul (Unione Sovietica)"@it , "Yesaul (Sovjet-Unie)"@nl , "Yesaul (Sovjetunionen)"@no , "Esauł (Związek Socjalistycznych Republik Radzieckich)"@pl , "Yesaul (União Soviética)"@pt , "Есаул (Союз Советских Социалистических Республик)"@ru , "Yesaul (Unión Soviética)"@es ;
	rdfs:comment "The specific instance of the Yesaul rank in the context of country Soviet Union."@en ;
	owl:rankOf <dbpedia:Soviet_Union> .

<http://rdf.muninn-project.org/ontologies/military#Rank_Chor%C4%85%C5%BCy_Poland> a :MilitaryRank ;
	owl:subClass <http://rdf.muninn-project.org/ontologies/military#Rank_Chor%C4%85%C5%BCy> ;
	foaf:name "Chorąży"@en ;
	rdfs:label "Chorąży (Poland)"@en , "Chorąży (Poland)"@pl , "Хорунжий (Poland)"@ru ;
	rdfs:comment "The specific instance of the Chorąży rank in the context of Poland."@en ;
	owl:rankOf <dbpedia:Poland> .

<http://rdf.muninn-project.org/ontologies/military#Rank_Chor%C4%85%C5%BCy_Ukraine> a :MilitaryRank ;
	owl:subClass <http://rdf.muninn-project.org/ontologies/military#Rank_Chor%C4%85%C5%BCy> ;
	foaf:name "Хорунжий"@ru ;
	rdfs:label "Chorąży (Ukraine)"@en , "Chorąży (Ukraina)"@sv , "Chorąży (Ukraina)"@fi , "Chorąży (Ukraine)"@fr , "Chorąży (Ukraine)"@de , "Chorąży (Ucraina)"@it , "Chorąży (Oekraïne)"@nl , "Chorąży (Ukraina)"@no , "Chorąży (Ukraina)"@pl , "Chorąży (Ucrânia)"@pt , "Хорунжий (Украина)"@ru , "Chorąży (Ucrania)"@es ;
	rdfs:comment "The specific instance of the Chorąży rank in the context of country Ukraine."@en ;
	owl:rankOf <dbpedia:Ukraine> .

<http://rdf.muninn-project.org/ontologies/military#Rank_Chor%C4%85%C5%BCy_Russia> a :MilitaryRank ;
	owl:subClass <http://rdf.muninn-project.org/ontologies/military#Rank_Chor%C4%85%C5%BCy> ;
	foaf:name "Хорунжий"@ru ;
	rdfs:label "Chorąży (Russia)"@en , "Chorąży (Ryssland)"@sv , "Chorąży (Venäjä)"@fi , "Chorąży (Russie)"@fr , "Chorąży (Russland)"@de , "Chorąży (Russia)"@it , "Chorąży (Rusland)"@nl , "Chorąży (Russland)"@no , "Chorąży (Rosja)"@pl , "Chorąży (Rússia)"@pt , "Хорунжий (Россия)"@ru , "Chorąży (Rusia)"@es ;
	rdfs:comment "The specific instance of the Chorąży rank in the context of country Russia."@en ;
	owl:rankOf <dbpedia:Russia> .

<http://rdf.muninn-project.org/ontologies/military#Rank_Chor%C4%85%C5%BCy_Soviet_Union> a :MilitaryRank ;
	owl:subClass <http://rdf.muninn-project.org/ontologies/military#Rank_Chor%C4%85%C5%BCy> ;
	foaf:name "Chorąży"@en ;
	rdfs:label "Chorąży (Soviet Union)"@en , "Chorąży (Sovjetunionen)"@sv , "Chorąży (Neuvostoliitto)"@fi , "Chorąży (Union des républiques socialistes soviétiques)"@fr , "Chorąży (Sowjetunion)"@de , "Chorąży (Unione Sovietica)"@it , "Chorąży (Sovjet-Unie)"@nl , "Chorąży (Sovjetunionen)"@no , "Chorąży (Związek Socjalistycznych Republik Radzieckich)"@pl , "Chorąży (União Soviética)"@pt , "Хорунжий (Союз Советских Социалистических Республик)"@ru , "Chorąży (Unión Soviética)"@es ;
	rdfs:comment "The specific instance of the Chorąży rank in the context of country Soviet Union."@en ;
	owl:rankOf <dbpedia:Soviet_Union> .

<http://rdf.muninn-project.org/ontologies/military#Rank_Conductor_%28Army%29_Australia> a :MilitaryRank ;
	owl:subClass <http://rdf.muninn-project.org/ontologies/military#Rank_Conductor_%28Army%29> ;
	foaf:name "Conductor"@en ;
	rdfs:label "Conductor (Army) (Australia)"@en , "Conductor (Army) (Australien)"@sv , "Conductor (Army) (Australia)"@fi , "Conductor (Army) (Australie)"@fr , "Conductor (Army) (Australien)"@de , "Conductor (Army) (Australia)"@it , "Conductor (Army) (Australië (land))"@nl , "Conductor (Army) (Australia)"@no , "Conductor (Army) (Australia)"@pl , "Conductor (Army) (Austrália)"@pt , "Conductor (Army) (Австралия)"@ru , "Conductor (Army) (Australia)"@es ;
	rdfs:comment "The specific instance of the Conductor (Army) rank in the context of country Australia."@en ;
	owl:rankOf <dbpedia:Australia> .

<http://rdf.muninn-project.org/ontologies/military#Rank_Conductor_%28Army%29_England> a :MilitaryRank ;
	owl:subClass <http://rdf.muninn-project.org/ontologies/military#Rank_Conductor_%28Army%29> ;
	foaf:name "Conductor"@en ;
	rdfs:label "Conductor (Army) (England)"@en ;
	rdfs:comment "The specific instance of the Conductor (Army) rank in the context of England."@en ;
	owl:rankOf <dbpedia:England> .

<http://rdf.muninn-project.org/ontologies/military#Rank_Conductor_%28Army%29_Scotland> a :MilitaryRank ;
	owl:subClass <http://rdf.muninn-project.org/ontologies/military#Rank_Conductor_%28Army%29> ;
	foaf:name "Conductor"@en ;
	rdfs:label "Conductor (Army) (Scotland)"@en , "Conductor (Army) (Skottland)"@sv , "Conductor (Army) (Skotlanti)"@fi , "Conductor (Army) (Écosse)"@fr , "Conductor (Army) (Schottland)"@de , "Conductor (Army) (Scozia)"@it , "Conductor (Army) (Schotland)"@nl , "Conductor (Army) (Skottland)"@no , "Conductor (Army) (Szkocja)"@pl , "Conductor (Army) (Escócia)"@pt , "Conductor (Army) (Шотландия)"@ru , "Conductor (Army) (Escocia)"@es ;
	rdfs:comment "The specific instance of the Conductor (Army) rank in the context of country Scotland."@en ;
	owl:rankOf <dbpedia:Scotland> .

<http://rdf.muninn-project.org/ontologies/military#Rank_Conductor_%28Army%29_Wales> a :MilitaryRank ;
	owl:subClass <http://rdf.muninn-project.org/ontologies/military#Rank_Conductor_%28Army%29> ;
	foaf:name "Conductor"@en ;
	rdfs:label "Conductor (Army) (Wales)"@en , "Conductor (Army) (Wales)"@sv , "Conductor (Army) (Wales)"@fi , "Conductor (Army) (Pays de Galles)"@fr , "Conductor (Army) (Wales)"@de , "Conductor (Army) (Galles)"@it , "Conductor (Army) (Wales)"@nl , "Conductor (Army) (Wales)"@no , "Conductor (Army) (Walia)"@pl , "Conductor (Army) (País de Gales)"@pt , "Conductor (Army) (Уэльс)"@ru , "Conductor (Army) (Gales)"@es ;
	rdfs:comment "The specific instance of the Conductor (Army) rank in the context of country Wales."@en ;
	owl:rankOf <dbpedia:Wales> .

<http://rdf.muninn-project.org/ontologies/military#Rank_Drum_major_%28rank%29_England> a :MilitaryRank ;
	owl:subClass <http://rdf.muninn-project.org/ontologies/military#Rank_Drum_major_%28rank%29> ;
	foaf:name "Drum major"@en ;
	rdfs:label "Drum major (rank, England)"@en ;
	rdfs:comment "The specific instance of the Drum major (rank) rank in the context of England."@en ;
	owl:rankOf <dbpedia:England> .

<http://rdf.muninn-project.org/ontologies/military#Rank_Drum_major_%28rank%29_Scotland> a :MilitaryRank ;
	owl:subClass <http://rdf.muninn-project.org/ontologies/military#Rank_Drum_major_%28rank%29> ;
	foaf:name "Drum major"@en ;
	rdfs:label "Drum major (rank) (Scotland)"@en , "Drum major (rank) (Skottland)"@sv , "Drum major (rank) (Skotlanti)"@fi , "Drum major (rank) (Écosse)"@fr , "Drum major (rank) (Schottland)"@de , "Drum major (rank) (Scozia)"@it , "Drum major (rank) (Schotland)"@nl , "Drum major (rank) (Skottland)"@no , "Drum major (rank) (Szkocja)"@pl , "Drum major (rank) (Escócia)"@pt , "Drum major (rank) (Шотландия)"@ru , "Drum major (rank) (Escocia)"@es ;
	rdfs:comment "The specific instance of the Drum major (rank) rank in the context of country Scotland."@en ;
	owl:rankOf <dbpedia:Scotland> .

<http://rdf.muninn-project.org/ontologies/military#Rank_Drum_major_%28rank%29_Wales> a :MilitaryRank ;
	owl:subClass <http://rdf.muninn-project.org/ontologies/military#Rank_Drum_major_%28rank%29> ;
	foaf:name "Drum major"@en ;
	rdfs:label "Drum major (rank) (Wales)"@en , "Drum major (rank) (Wales)"@sv , "Drum major (rank) (Wales)"@fi , "Drum major (rank) (Pays de Galles)"@fr , "Drum major (rank) (Wales)"@de , "Drum major (rank) (Galles)"@it , "Drum major (rank) (Wales)"@nl , "Drum major (rank) (Wales)"@no , "Drum major (rank) (Walia)"@pl , "Drum major (rank) (País de Gales)"@pt , "Drum major (rank) (Уэльс)"@ru , "Drum major (rank) (Gales)"@es ;
	rdfs:comment "The specific instance of the Drum major (rank) rank in the context of country Wales."@en ;
	owl:rankOf <dbpedia:Wales> .

<http://rdf.muninn-project.org/ontologies/military#Rank_Drum_major_%28rank%29_Commonwealth_of_Nations> a :MilitaryRank ;
	owl:subClass <http://rdf.muninn-project.org/ontologies/military#Rank_Drum_major_%28rank%29> ;
	foaf:name "Drum major"@en ;
	rdfs:label "Drum major (rank) (Commonwealth of Nations)"@en , "Drum major (rank) (Samväldet)"@sv , "Drum major (rank) (Kansainyhteisö)"@fi , "Drum major (rank) (Commonwealth of Nations)"@fr , "Drum major (rank) (Commonwealth of Nations)"@de , "Drum major (rank) (Commonwealth delle nazioni)"@it , "Drum major (rank) (Gemenebest van Naties)"@nl , "Drum major (rank) (Samveldet av nasjoner)"@no , "Drum major (rank) (Wspólnota Narodów)"@pl , "Drum major (rank) (Commonwealth)"@pt , "Drum major (rank) (Содружество наций)"@ru , "Drum major (rank) (Mancomunidad de Naciones)"@es ;
	rdfs:comment "The specific instance of the Drum major (rank) rank in the context of country Commonwealth of Nations."@en ;
	owl:rankOf <dbpedia:Commonwealth_of_Nations> .

:Rank_Drum_Major_General_England a :MilitaryRank ;
	owl:subClass :Rank_Drum_Major_General ;
	foaf:name "Drum Major General"@en ;
	rdfs:label "Drum Major General (England)"@en ;
	rdfs:comment "The specific instance of the Drum Major General rank in the context of England."@en ;
	owl:rankOf <dbpedia:England> .

:Rank_Drum_Major_General_Scotland a :MilitaryRank ;
	owl:subClass :Rank_Drum_Major_General ;
	foaf:name "Drum Major General"@en ;
	rdfs:label "Drum Major General (Scotland)"@en , "Drum Major General (Skottland)"@sv , "Drum Major General (Skotlanti)"@fi , "Drum Major General (Écosse)"@fr , "Drum Major General (Schottland)"@de , "Drum Major General (Scozia)"@it , "Drum Major General (Schotland)"@nl , "Drum Major General (Skottland)"@no , "Drum Major General (Szkocja)"@pl , "Drum Major General (Escócia)"@pt , "Drum Major General (Шотландия)"@ru , "Drum Major General (Escocia)"@es ;
	rdfs:comment "The specific instance of the Drum Major General rank in the context of country Scotland."@en ;
	owl:rankOf <dbpedia:Scotland> .

:Rank_Drum_Major_General_Wales a :MilitaryRank ;
	owl:subClass :Rank_Drum_Major_General ;
	foaf:name "Drum Major General"@en ;
	rdfs:label "Drum Major General (Wales)"@en , "Drum Major General (Wales)"@sv , "Drum Major General (Wales)"@fi , "Drum Major General (Pays de Galles)"@fr , "Drum Major General (Wales)"@de , "Drum Major General (Galles)"@it , "Drum Major General (Wales)"@nl , "Drum Major General (Wales)"@no , "Drum Major General (Walia)"@pl , "Drum Major General (País de Gales)"@pt , "Drum Major General (Уэльс)"@ru , "Drum Major General (Gales)"@es ;
	rdfs:comment "The specific instance of the Drum Major General rank in the context of country Wales."@en ;
	owl:rankOf <dbpedia:Wales> .

:Rank_Drum_Major_General_Commonwealth_of_Nations a :MilitaryRank ;
	owl:subClass :Rank_Drum_Major_General ;
	foaf:name "Drum Major General"@en ;
	rdfs:label "Drum Major General (Commonwealth of Nations)"@en , "Drum Major General (Samväldet)"@sv , "Drum Major General (Kansainyhteisö)"@fi , "Drum Major General (Commonwealth of Nations)"@fr , "Drum Major General (Commonwealth of Nations)"@de , "Drum Major General (Commonwealth delle nazioni)"@it , "Drum Major General (Gemenebest van Naties)"@nl , "Drum Major General (Samveldet av nasjoner)"@no , "Drum Major General (Wspólnota Narodów)"@pl , "Drum Major General (Commonwealth)"@pt , "Drum Major General (Содружество наций)"@ru , "Drum Major General (Mancomunidad de Naciones)"@es ;
	rdfs:comment "The specific instance of the Drum Major General rank in the context of country Commonwealth of Nations."@en ;
	owl:rankOf <dbpedia:Commonwealth_of_Nations> .

:Rank_Flight_sergeant_Australia a :MilitaryRank ;
	owl:subClass :Rank_Flight_sergeant ;
	foaf:name "Flight sergeant"@en ;
	rdfs:label "Flight sergeant (Australia)"@en , "Flight sergeant (Australien)"@sv , "Flight sergeant (Australia)"@fi , "Flight sergeant (Australie)"@fr , "Flight sergeant (Australien)"@de , "Flight sergeant (Australia)"@it , "Flight sergeant (Australië (land))"@nl , "Flight sergeant (Australia)"@no , "Flight sergeant (Australia)"@pl , "Flight sergeant (Austrália)"@pt , "Flight sergeant (Австралия)"@ru , "Flight sergeant (Australia)"@es ;
	rdfs:comment "The specific instance of the Flight sergeant rank in the context of country Australia."@en ;
	owl:rankOf <dbpedia:Australia> .

:Rank_Flight_sergeant_Canada a :MilitaryRank ;
	owl:subClass :Rank_Flight_sergeant ;
	foaf:name "Flight sergeant"@en ;
	rdfs:label "Flight sergeant (Canada)"@en ;
	rdfs:comment "The specific instance of the Flight sergeant rank in the context of Canada."@en ;
	owl:rankOf <dbpedia:Canada> .

:Rank_Flight_sergeant_Commonwealth_of_Nations a :MilitaryRank ;
	owl:subClass :Rank_Flight_sergeant ;
	foaf:name "Flight sergeant"@en ;
	rdfs:label "Flight sergeant (Commonwealth of Nations)"@en , "Flight sergeant (Samväldet)"@sv , "Flight sergeant (Kansainyhteisö)"@fi , "Flight sergeant (Commonwealth of Nations)"@fr , "Flight sergeant (Commonwealth of Nations)"@de , "Flight sergeant (Commonwealth delle nazioni)"@it , "Flight sergeant (Gemenebest van Naties)"@nl , "Flight sergeant (Samveldet av nasjoner)"@no , "Flight sergeant (Wspólnota Narodów)"@pl , "Flight sergeant (Commonwealth)"@pt , "Flight sergeant (Содружество наций)"@ru , "Flight sergeant (Mancomunidad de Naciones)"@es ;
	rdfs:comment "The specific instance of the Flight sergeant rank in the context of country Commonwealth of Nations."@en ;
	owl:rankOf <dbpedia:Commonwealth_of_Nations> .

:Rank_Flight_sergeant_Republic_of_Ireland a :MilitaryRank ;
	owl:subClass :Rank_Flight_sergeant ;
	foaf:name "Flight sergeant"@en ;
	rdfs:label "Flight sergeant (Republic of Ireland)"@en , "Flight sergeant (Irland)"@sv , "Flight sergeant (Irlanti)"@fi , "Flight sergeant (Irlande (pays))"@fr , "Flight sergeant (Irland)"@de , "Flight sergeant (Irlanda)"@it , "Flight sergeant (Ierland (land))"@nl , "Flight sergeant (Irland)"@no , "Flight sergeant (Irlandia)"@pl , "Flight sergeant (República da Irlanda)"@pt , "Flight sergeant (Ирландия)"@ru , "Flight sergeant (Irlanda)"@es ;
	rdfs:comment "The specific instance of the Flight sergeant rank in the context of country Republic of Ireland."@en ;
	owl:rankOf <dbpedia:Republic_of_Ireland> .

:Rank_Hetman_Poland a :MilitaryRank ;
	owl:subClass :Rank_Hetman ;
	foaf:name "Hetman"@en ;
	rdfs:label "Hetman (Poland)"@en , "Hetman (Poland)"@sv , "Hetmani (Poland)"@fi , "Hetman (Poland)"@fr , "Hetman (Poland)"@de , "Hetman (Poland)"@nl , "Hetman (Poland)"@no , "Hetman (Poland)"@pl , "Hetman (Poland)"@pt , "Гетман (Poland)"@ru , "Hetman (Poland)"@es ;
	rdfs:comment "The specific instance of the Hetman rank in the context of Poland."@en ;
	owl:rankOf <dbpedia:Poland> .

:Rank_Hetman_Belarus a :MilitaryRank ;
	owl:subClass :Rank_Hetman ;
	foaf:name "Гетман"@ru ;
	rdfs:label "Hetman (Belarus)"@en , "Hetman (Vitryssland)"@sv , "Hetmani (Valko-Venäjä)"@fi , "Hetman (Biélorussie)"@fr , "Hetman (Weißrussland)"@de , "Hetman (Bielorussia)"@it , "Hetman (Wit-Rusland)"@nl , "Hetman (Hviterussland)"@no , "Hetman (Białoruś)"@pl , "Hetman (Bielorrússia)"@pt , "Гетман (Белоруссия)"@ru , "Hetman (Bielorrusia)"@es ;
	rdfs:comment "The specific instance of the Hetman rank in the context of country Belarus."@en ;
	owl:rankOf <dbpedia:Belarus> .

<dbpedia:Belarus> muninn:wikipedia_version "498368216" .

:Rank_Hetman_Lithuania a :MilitaryRank ;
	owl:subClass :Rank_Hetman ;
	foaf:name "Hetman"@en ;
	rdfs:label "Hetman (Lithuania)"@en , "Hetman (Litauen)"@sv , "Hetmani (Liettua)"@fi , "Hetman (Lituanie)"@fr , "Hetman (Litauen)"@de , "Hetman (Lituania)"@it , "Hetman (Litouwen)"@nl , "Hetman (Litauen)"@no , "Hetman (Litwa)"@pl , "Hetman (Lituânia)"@pt , "Гетман (Литва)"@ru , "Hetman (Lituania)"@es ;
	rdfs:comment "The specific instance of the Hetman rank in the context of country Lithuania."@en ;
	owl:rankOf <dbpedia:Lithuania> .

:Rank_Hetman_Ukraine a :MilitaryRank ;
	owl:subClass :Rank_Hetman ;
	foaf:name "Гетман"@ru ;
	rdfs:label "Hetman (Ukraine)"@en , "Hetman (Ukraina)"@sv , "Hetmani (Ukraina)"@fi , "Hetman (Ukraine)"@fr , "Hetman (Ukraine)"@de , "Hetman (Ucraina)"@it , "Hetman (Oekraïne)"@nl , "Hetman (Ukraina)"@no , "Hetman (Ukraina)"@pl , "Hetman (Ucrânia)"@pt , "Гетман (Украина)"@ru , "Hetman (Ucrania)"@es ;
	rdfs:comment "The specific instance of the Hetman rank in the context of country Ukraine."@en ;
	owl:rankOf <dbpedia:Ukraine> .

:Rank_Kolonel_Netherlands a :MilitaryRank ;
	owl:subClass :Rank_Kolonel ;
	foaf:name "Kolonel"@en ;
	rdfs:label "Kolonel (Netherlands)"@en , "Kolonel (Nederländerna)"@sv , "Kolonel (Alankomaat)"@fi , "Kolonel (Pays-Bas)"@fr , "Kolonel (Niederlande)"@de , "Kolonel (Paesi Bassi)"@it , "Kolonel (Nederland)"@nl , "Kolonel (Nederland)"@no , "Kolonel (Holandia)"@pl , "Kolonel (Países Baixos)"@pt , "Kolonel (Нидерланды)"@ru , "Kolonel (Países Bajos)"@es ;
	rdfs:comment "The specific instance of the Kolonel rank in the context of country Netherlands."@en ;
	owl:rankOf <dbpedia:Netherlands> .

:Rank_Kolonel_Belgium a :MilitaryRank ;
	owl:subClass :Rank_Kolonel ;
	foaf:name "Kolonel"@en ;
	rdfs:label "Kolonel (Belgium)"@en , "Kolonel (Belgien)"@sv , "Kolonel (Belgia)"@fi , "Kolonel (Belgique)"@fr , "Kolonel (Belgien)"@de , "Kolonel (Belgio)"@it , "Kolonel (België)"@nl , "Kolonel (Belgia)"@no , "Kolonel (Belgia)"@pl , "Kolonel (Bélgica)"@pt , "Kolonel (Бельгия)"@ru , "Kolonel (Bélgica)"@es ;
	rdfs:comment "The specific instance of the Kolonel rank in the context of country Belgium."@en ;
	owl:rankOf <dbpedia:Belgium> .

:Rank_Kolonel_Estonia a :MilitaryRank ;
	owl:subClass :Rank_Kolonel ;
	foaf:name "Kolonel"@en ;
	rdfs:label "Kolonel (Estonia)"@en , "Kolonel (Estland)"@sv , "Kolonel (Viro)"@fi , "Kolonel (Estonie)"@fr , "Kolonel (Estland)"@de , "Kolonel (Estonia)"@it , "Kolonel (Estland)"@nl , "Kolonel (Estland)"@no , "Kolonel (Estonia)"@pl , "Kolonel (Estónia)"@pt , "Kolonel (Эстония)"@ru , "Kolonel (Estonia)"@es ;
	rdfs:comment "The specific instance of the Kolonel rank in the context of country Estonia."@en ;
	owl:rankOf <dbpedia:Estonia> .

<http://rdf.muninn-project.org/ontologies/military#Rank_Kolonel_Republic_of_Estonia_%281920-1940%29> a :MilitaryRank ;
	owl:subClass :Rank_Kolonel ;
	foaf:name "Kolonel"@en ;
	rdfs:label "Kolonel (Republic of Estonia, 1920-1940)"@en ;
	rdfs:comment "The specific instance of the Kolonel rank in the context of the Republic of Estonia, 1920-1940."@en ;
	owl:rankOf <dbpedia:Republic_of_Estonia_%281920-1940%29> .

:Rank_Lochagos_Greece a :MilitaryRank ;
	owl:subClass :Rank_Lochagos ;
	foaf:name "Lochagos"@en ;
	rdfs:label "Lochagos (Greece)"@en , "Lochagos (Grekland)"@sv , "Lochagos (Kreikka)"@fi , "Lochagos (Grèce)"@fr , "Lochagos (Griechenland)"@de , "Lochagos (Grecia)"@it , "Lochagos (Griekenland)"@nl , "Lochagos (Hellas)"@no , "Lochagos (Grecja)"@pl , "Lochagos (Grécia)"@pt , "Lochagos (Греция)"@ru , "Lochagos (Grecia)"@es ;
	rdfs:comment "The specific instance of the Lochagos rank in the context of country Greece."@en ;
	owl:rankOf <dbpedia:Greece> .

:Rank_Lochagos_Official_Timocracy_of_Sapinetia a :MilitaryRank ;
	owl:subClass :Rank_Lochagos ;
	foaf:name "Lochagos"@en ;
	rdfs:label "Lochagos (Timocracy of Sapinetia)"@en ;
	rdfs:comment "The specific instance of the Lochagos rank in the context of the Timocracy of Sapinetia."@en ;
	owl:rankOf <dbpedia:Official_Timocracy_of_Sapinetia> .

<http://rdf.muninn-project.org/ontologies/military#Rank_Lochagos_Macedonia_%28ancient_kingdom%29> a :MilitaryRank ;
	owl:subClass :Rank_Lochagos ;
	foaf:name "Lochagos"@en ;
	rdfs:label "Lochagos (Macedonia (ancient kingdom))"@en , "Lochagos (Makedonian valtakunta)"@fi , "Lochagos (Royaume de Macédoine)"@fr , "Lochagos (Regno di Macedonia)"@it , "Lochagos (Macedonië (oudheid))"@nl , "Lochagos (Oldtidens Makedonia)"@no , "Lochagos (Starożytna Macedonia)"@pl , "Lochagos (Macedónia Antiga)"@pt , "Lochagos (Древняя Македония)"@ru , "Lochagos (Reino de Macedonia)"@es ;
	rdfs:comment "The specific instance of the Lochagos rank in the context of country Macedonia (ancient kingdom)."@en ;
	owl:rankOf <dbpedia:Macedonia_%28ancient_kingdom%29> .

:Rank_Lochagos_Achaean_League a :MilitaryRank ;
	owl:subClass :Rank_Lochagos ;
	foaf:name "Lochagos"@en ;
	rdfs:label "Lochagos (Achaean League)"@en , "Lochagos (Achaiska förbundet)"@sv , "Lochagos (Akhaian liitto)"@fi , "Lochagos (Ligue achéenne)"@fr , "Lochagos (Achaiischer Bund)"@de , "Lochagos (Lega achea)"@it , "Lochagos (Achaeïsche Bond)"@nl , "Lochagos (Det akhaiske forbund)"@no , "Lochagos (Związek Achajski)"@pl , "Lochagos (Liga Aqueia)"@pt , "Lochagos (Ахейский союз)"@ru , "Lochagos (Liga Aquea)"@es ;
	rdfs:comment "The specific instance of the Lochagos rank in the context of country Achaean League."@en ;
	owl:rankOf <dbpedia:Achaean_League> .

:Rank_Navarch_Greece a :MilitaryRank ;
	owl:subClass :Rank_Navarch ;
	foaf:name "Navarch"@en ;
	rdfs:label "Navarch (Greece)"@en , "Navarch (Grekland)"@sv , "Navarch (Kreikka)"@fi , "Navarque (Grèce)"@fr , "Nauarch (Griechenland)"@de , "Navarch (Grecia)"@it , "Navarch (Griekenland)"@nl , "Navarch (Hellas)"@no , "Nauarch (Grecja)"@pl , "Navarch (Grécia)"@pt , "Наварх (Греция)"@ru , "Navarco (Grecia)"@es ;
	rdfs:comment "The specific instance of the Navarch rank in the context of country Greece."@en ;
	owl:rankOf <dbpedia:Greece> .

:Rank_Navarch_Official_Timocracy_of_Sapinetia a :MilitaryRank ;
	owl:subClass :Rank_Navarch ;
	foaf:name "Navarch"@en ;
	rdfs:label "Navarch (Timocracy of Sapinetia)"@en , "Navarque (Timocracy of Sapinetia)"@fr , "Nauarch (Timocracy of Sapinetia)"@de , "Nauarch (Timocracy of Sapinetia)"@pl , "Наварх (Timocracy of Sapinetia)"@ru , "Navarco (Timocracy of Sapinetia)"@es ;
	rdfs:comment "The specific instance of the Navarch rank in the context of the Timocracy of Sapinetia."@en ;
	owl:rankOf <dbpedia:Official_Timocracy_of_Sapinetia> .

<http://rdf.muninn-project.org/ontologies/military#Rank_Navarch_Macedonia_%28ancient_kingdom%29> a :MilitaryRank ;
	owl:subClass :Rank_Navarch ;
	foaf:name "Navarch"@en ;
	rdfs:label "Navarch (Macedonia (ancient kingdom))"@en , "Navarch (Makedonian valtakunta)"@fi , "Navarque (Royaume de Macédoine)"@fr , "Nauarch (Macedonia (ancient kingdom))"@de , "Navarch (Regno di Macedonia)"@it , "Navarch (Macedonië (oudheid))"@nl , "Navarch (Oldtidens Makedonia)"@no , "Nauarch (Starożytna Macedonia)"@pl , "Navarch (Macedónia Antiga)"@pt , "Наварх (Древняя Македония)"@ru , "Navarco (Reino de Macedonia)"@es ;
	rdfs:comment "The specific instance of the Navarch rank in the context of country Macedonia (ancient kingdom)."@en ;
	owl:rankOf <dbpedia:Macedonia_%28ancient_kingdom%29> .

:Rank_Navarch_Achaean_League a :MilitaryRank ;
	owl:subClass :Rank_Navarch ;
	foaf:name "Navarch"@en ;
	rdfs:label "Navarch (Achaean League)"@en , "Navarch (Achaiska förbundet)"@sv , "Navarch (Akhaian liitto)"@fi , "Navarque (Ligue achéenne)"@fr , "Nauarch (Achaiischer Bund)"@de , "Navarch (Lega achea)"@it , "Navarch (Achaeïsche Bond)"@nl , "Navarch (Det akhaiske forbund)"@no , "Nauarch (Związek Achajski)"@pl , "Navarch (Liga Aqueia)"@pt , "Наварх (Ахейский союз)"@ru , "Navarco (Liga Aquea)"@es ;
	rdfs:comment "The specific instance of the Navarch rank in the context of country Achaean League."@en ;
	owl:rankOf <dbpedia:Achaean_League> .

:Rank_Phrourarch_Greece a :MilitaryRank ;
	owl:subClass :Rank_Phrourarch ;
	foaf:name "Phrourarch"@en ;
	rdfs:label "Phrourarch (Greece)"@en , "Phrourarch (Grekland)"@sv , "Phrourarch (Kreikka)"@fi , "Phrourarch (Grèce)"@fr , "Phrourarch (Griechenland)"@de , "Phrourarch (Grecia)"@it , "Phrourarch (Griekenland)"@nl , "Phrourarch (Hellas)"@no , "Phrourarch (Grecja)"@pl , "Phrourarch (Grécia)"@pt , "Phrourarch (Греция)"@ru , "Phrourarch (Grecia)"@es ;
	rdfs:comment "The specific instance of the Phrourarch rank in the context of country Greece."@en ;
	owl:rankOf <dbpedia:Greece> .

:Rank_Phrourarch_Official_Timocracy_of_Sapinetia a :MilitaryRank ;
	owl:subClass :Rank_Phrourarch ;
	foaf:name "Phrourarch"@en ;
	rdfs:label "Phrourarch (Timocracy of Sapinetia)"@en ;
	rdfs:comment "The specific instance of the Phrourarch rank in the context of the Timocracy of Sapinetia."@en ;
	owl:rankOf <dbpedia:Official_Timocracy_of_Sapinetia> .

<http://rdf.muninn-project.org/ontologies/military#Rank_Phrourarch_Macedonia_%28ancient_kingdom%29> a :MilitaryRank ;
	owl:subClass :Rank_Phrourarch ;
	foaf:name "Phrourarch"@en ;
	rdfs:label "Phrourarch (Macedonia (ancient kingdom))"@en , "Phrourarch (Makedonian valtakunta)"@fi , "Phrourarch (Royaume de Macédoine)"@fr , "Phrourarch (Regno di Macedonia)"@it , "Phrourarch (Macedonië (oudheid))"@nl , "Phrourarch (Oldtidens Makedonia)"@no , "Phrourarch (Starożytna Macedonia)"@pl , "Phrourarch (Macedónia Antiga)"@pt , "Phrourarch (Древняя Македония)"@ru , "Phrourarch (Reino de Macedonia)"@es ;
	rdfs:comment "The specific instance of the Phrourarch rank in the context of country Macedonia (ancient kingdom)."@en ;
	owl:rankOf <dbpedia:Macedonia_%28ancient_kingdom%29> .

:Rank_Phrourarch_Achaean_League a :MilitaryRank ;
	owl:subClass :Rank_Phrourarch ;
	foaf:name "Phrourarch"@en ;
	rdfs:label "Phrourarch (Achaean League)"@en , "Phrourarch (Achaiska förbundet)"@sv , "Phrourarch (Akhaian liitto)"@fi , "Phrourarch (Ligue achéenne)"@fr , "Phrourarch (Achaiischer Bund)"@de , "Phrourarch (Lega achea)"@it , "Phrourarch (Achaeïsche Bond)"@nl , "Phrourarch (Det akhaiske forbund)"@no , "Phrourarch (Związek Achajski)"@pl , "Phrourarch (Liga Aqueia)"@pt , "Phrourarch (Ахейский союз)"@ru , "Phrourarch (Liga Aquea)"@es ;
	rdfs:comment "The specific instance of the Phrourarch rank in the context of country Achaean League."@en ;
	owl:rankOf <dbpedia:Achaean_League> .

:Rank_Pipe_Major_England a :MilitaryRank ;
	owl:subClass :Rank_Pipe_Major ;
	foaf:name "Pipe Major"@en ;
	rdfs:label "Pipe Major (England)"@en ;
	rdfs:comment "The specific instance of the Pipe Major rank in the context of England."@en ;
	owl:rankOf <dbpedia:England> .

:Rank_Pipe_Major_Scotland a :MilitaryRank ;
	owl:subClass :Rank_Pipe_Major ;
	foaf:name "Pipe Major"@en ;
	rdfs:label "Pipe Major (Scotland)"@en , "Pipe Major (Skottland)"@sv , "Pipe Major (Skotlanti)"@fi , "Pipe Major (Écosse)"@fr , "Pipe Major (Schottland)"@de , "Pipe Major (Scozia)"@it , "Pipe Major (Schotland)"@nl , "Pipe Major (Skottland)"@no , "Pipe Major (Szkocja)"@pl , "Pipe Major (Escócia)"@pt , "Pipe Major (Шотландия)"@ru , "Pipe Major (Escocia)"@es ;
	rdfs:comment "The specific instance of the Pipe Major rank in the context of country Scotland."@en ;
	owl:rankOf <dbpedia:Scotland> .

:Rank_Pipe_Major_Wales a :MilitaryRank ;
	owl:subClass :Rank_Pipe_Major ;
	foaf:name "Pipe Major"@en ;
	rdfs:label "Pipe Major (Wales)"@en , "Pipe Major (Wales)"@sv , "Pipe Major (Wales)"@fi , "Pipe Major (Pays de Galles)"@fr , "Pipe Major (Wales)"@de , "Pipe Major (Galles)"@it , "Pipe Major (Wales)"@nl , "Pipe Major (Wales)"@no , "Pipe Major (Walia)"@pl , "Pipe Major (País de Gales)"@pt , "Pipe Major (Уэльс)"@ru , "Pipe Major (Gales)"@es ;
	rdfs:comment "The specific instance of the Pipe Major rank in the context of country Wales."@en ;
	owl:rankOf <dbpedia:Wales> .

:Rank_Pipe_Major_Commonwealth_of_Nations a :MilitaryRank ;
	owl:subClass :Rank_Pipe_Major ;
	foaf:name "Pipe Major"@en ;
	rdfs:label "Pipe Major (Commonwealth of Nations)"@en , "Pipe Major (Samväldet)"@sv , "Pipe Major (Kansainyhteisö)"@fi , "Pipe Major (Commonwealth of Nations)"@fr , "Pipe Major (Commonwealth of Nations)"@de , "Pipe Major (Commonwealth delle nazioni)"@it , "Pipe Major (Gemenebest van Naties)"@nl , "Pipe Major (Samveldet av nasjoner)"@no , "Pipe Major (Wspólnota Narodów)"@pl , "Pipe Major (Commonwealth)"@pt , "Pipe Major (Содружество наций)"@ru , "Pipe Major (Mancomunidad de Naciones)"@es ;
	rdfs:comment "The specific instance of the Pipe Major rank in the context of country Commonwealth of Nations."@en ;
	owl:rankOf <dbpedia:Commonwealth_of_Nations> .

:Rank_Podpolkovnik_Poland a :MilitaryRank ;
	owl:subClass :Rank_Podpolkovnik ;
	foaf:name "Podpolkovnik"@en ;
	rdfs:label "Podpolkovnik (Poland)"@en , "Podpułkownik (Poland)"@pl ;
	rdfs:comment "The specific instance of the Podpolkovnik rank in the context of Poland."@en ;
	owl:rankOf <dbpedia:Poland> .

:Rank_Podpolkovnik_Ukraine a :MilitaryRank ;
	owl:subClass :Rank_Podpolkovnik ;
	foaf:name "Podpolkovnik"@en ;
	rdfs:label "Podpolkovnik (Ukraine)"@en , "Podpolkovnik (Ukraina)"@sv , "Podpolkovnik (Ukraina)"@fi , "Podpolkovnik (Ukraine)"@fr , "Podpolkovnik (Ukraine)"@de , "Podpolkovnik (Ucraina)"@it , "Podpolkovnik (Oekraïne)"@nl , "Podpolkovnik (Ukraina)"@no , "Podpułkownik (Ukraina)"@pl , "Podpolkovnik (Ucrânia)"@pt , "Podpolkovnik (Украина)"@ru , "Podpolkovnik (Ucrania)"@es ;
	rdfs:comment "The specific instance of the Podpolkovnik rank in the context of country Ukraine."@en ;
	owl:rankOf <dbpedia:Ukraine> .

:Rank_Podpolkovnik_Russia a :MilitaryRank ;
	owl:subClass :Rank_Podpolkovnik ;
	foaf:name "Podpolkovnik"@en ;
	rdfs:label "Podpolkovnik (Russia)"@en , "Podpolkovnik (Ryssland)"@sv , "Podpolkovnik (Venäjä)"@fi , "Podpolkovnik (Russie)"@fr , "Podpolkovnik (Russland)"@de , "Podpolkovnik (Russia)"@it , "Podpolkovnik (Rusland)"@nl , "Podpolkovnik (Russland)"@no , "Podpułkownik (Rosja)"@pl , "Podpolkovnik (Rússia)"@pt , "Podpolkovnik (Россия)"@ru , "Podpolkovnik (Rusia)"@es ;
	rdfs:comment "The specific instance of the Podpolkovnik rank in the context of country Russia."@en ;
	owl:rankOf <dbpedia:Russia> .

:Rank_Podpolkovnik_Soviet_Union a :MilitaryRank ;
	owl:subClass :Rank_Podpolkovnik ;
	foaf:name "Podpolkovnik"@en ;
	rdfs:label "Podpolkovnik (Soviet Union)"@en , "Podpolkovnik (Sovjetunionen)"@sv , "Podpolkovnik (Neuvostoliitto)"@fi , "Podpolkovnik (Union des républiques socialistes soviétiques)"@fr , "Podpolkovnik (Sowjetunion)"@de , "Podpolkovnik (Unione Sovietica)"@it , "Podpolkovnik (Sovjet-Unie)"@nl , "Podpolkovnik (Sovjetunionen)"@no , "Podpułkownik (Związek Socjalistycznych Republik Radzieckich)"@pl , "Podpolkovnik (União Soviética)"@pt , "Podpolkovnik (Союз Советских Социалистических Республик)"@ru , "Podpolkovnik (Unión Soviética)"@es ;
	rdfs:comment "The specific instance of the Podpolkovnik rank in the context of country Soviet Union."@en ;
	owl:rankOf <dbpedia:Soviet_Union> .

:Rank_Polkovnik_Poland a :MilitaryRank ;
	owl:subClass :Rank_Polkovnik ;
	foaf:name "Polkovnik"@en ;
	rdfs:label "Polkovnik (Poland)"@en ;
	rdfs:comment "The specific instance of the Polkovnik rank in the context of Poland."@en ;
	owl:rankOf <dbpedia:Poland> .

:Rank_Polkovnik_Ukraine a :MilitaryRank ;
	owl:subClass :Rank_Polkovnik ;
	foaf:name "Polkovnik"@en ;
	rdfs:label "Polkovnik (Ukraine)"@en , "Polkovnik (Ukraina)"@sv , "Polkovnik (Ukraina)"@fi , "Polkovnik (Ukraine)"@fr , "Polkovnik (Ukraine)"@de , "Polkovnik (Ucraina)"@it , "Polkovnik (Oekraïne)"@nl , "Polkovnik (Ukraina)"@no , "Polkovnik (Ukraina)"@pl , "Polkovnik (Ucrânia)"@pt , "Polkovnik (Украина)"@ru , "Polkovnik (Ucrania)"@es ;
	rdfs:comment "The specific instance of the Polkovnik rank in the context of country Ukraine."@en ;
	owl:rankOf <dbpedia:Ukraine> .

:Rank_Polkovnik_Russia a :MilitaryRank ;
	owl:subClass :Rank_Polkovnik ;
	foaf:name "Polkovnik"@en ;
	rdfs:label "Polkovnik (Russia)"@en , "Polkovnik (Ryssland)"@sv , "Polkovnik (Venäjä)"@fi , "Polkovnik (Russie)"@fr , "Polkovnik (Russland)"@de , "Polkovnik (Russia)"@it , "Polkovnik (Rusland)"@nl , "Polkovnik (Russland)"@no , "Polkovnik (Rosja)"@pl , "Polkovnik (Rússia)"@pt , "Polkovnik (Россия)"@ru , "Polkovnik (Rusia)"@es ;
	rdfs:comment "The specific instance of the Polkovnik rank in the context of country Russia."@en ;
	owl:rankOf <dbpedia:Russia> .

:Rank_Polkovnik_Soviet_Union a :MilitaryRank ;
	owl:subClass :Rank_Polkovnik ;
	foaf:name "Polkovnik"@en ;
	rdfs:label "Polkovnik (Soviet Union)"@en , "Polkovnik (Sovjetunionen)"@sv , "Polkovnik (Neuvostoliitto)"@fi , "Polkovnik (Union des républiques socialistes soviétiques)"@fr , "Polkovnik (Sowjetunion)"@de , "Polkovnik (Unione Sovietica)"@it , "Polkovnik (Sovjet-Unie)"@nl , "Polkovnik (Sovjetunionen)"@no , "Polkovnik (Związek Socjalistycznych Republik Radzieckich)"@pl , "Polkovnik (União Soviética)"@pt , "Polkovnik (Союз Советских Социалистических Республик)"@ru , "Polkovnik (Unión Soviética)"@es ;
	rdfs:comment "The specific instance of the Polkovnik rank in the context of country Soviet Union."@en ;
	owl:rankOf <dbpedia:Soviet_Union> .

:Rank_Staff_sergeant_Australia a :MilitaryRank ;
	owl:subClass :Rank_Staff_sergeant ;
	foaf:name "Staff sergeant"@en ;
	rdfs:label "Staff sergeant (Australia)"@en , "Staff sergeant (Australien)"@sv , "Staff sergeant (Australia)"@fi , "Staff sergeant (Australie)"@fr , "Staff sergeant (Australien)"@de , "Staff sergeant (Australia)"@it , "Staff sergeant (Australië (land))"@nl , "Staff sergeant (Australia)"@no , "Staff sergeant (Australia)"@pl , "Staff sergeant (Austrália)"@pt , "Staff sergeant (Австралия)"@ru , "Staff sergeant (Australia)"@es ;
	rdfs:comment "The specific instance of the Staff sergeant rank in the context of country Australia."@en ;
	owl:rankOf <dbpedia:Australia> .

:Rank_Staff_sergeant_Canada a :MilitaryRank ;
	owl:subClass :Rank_Staff_sergeant ;
	foaf:name "Staff sergeant"@en ;
	rdfs:label "Staff sergeant (Canada)"@en ;
	rdfs:comment "The specific instance of the Staff sergeant rank in the context of Canada."@en ;
	owl:rankOf <dbpedia:Canada> .

:Rank_Staff_sergeant_Singapore a :MilitaryRank ;
	owl:subClass :Rank_Staff_sergeant ;
	foaf:name "Staff sergeant"@en ;
	rdfs:label "Staff sergeant (Singapore)"@en , "Staff sergeant (Singapore)"@sv , "Staff sergeant (Singapore)"@fi , "Staff sergeant (Singapour)"@fr , "Staff sergeant (Singapur)"@de , "Staff sergeant (Singapore)"@it , "Staff sergeant (Singapore)"@nl , "Staff sergeant (Singapore)"@no , "Staff sergeant (Singapur)"@pl , "Staff sergeant (Singapura)"@pt , "Staff sergeant (Сингапур)"@ru , "Staff sergeant (Singapur)"@es ;
	rdfs:comment "The specific instance of the Staff sergeant rank in the context of country Singapore."@en ;
	owl:rankOf <dbpedia:Singapore> .

:Rank_Staff_sergeant_Commonwealth_of_Nations a :MilitaryRank ;
	owl:subClass :Rank_Staff_sergeant ;
	foaf:name "Staff sergeant"@en ;
	rdfs:label "Staff sergeant (Commonwealth of Nations)"@en , "Staff sergeant (Samväldet)"@sv , "Staff sergeant (Kansainyhteisö)"@fi , "Staff sergeant (Commonwealth of Nations)"@fr , "Staff sergeant (Commonwealth of Nations)"@de , "Staff sergeant (Commonwealth delle nazioni)"@it , "Staff sergeant (Gemenebest van Naties)"@nl , "Staff sergeant (Samveldet av nasjoner)"@no , "Staff sergeant (Wspólnota Narodów)"@pl , "Staff sergeant (Commonwealth)"@pt , "Staff sergeant (Содружество наций)"@ru , "Staff sergeant (Mancomunidad de Naciones)"@es ;
	rdfs:comment "The specific instance of the Staff sergeant rank in the context of country Commonwealth of Nations."@en ;
	owl:rankOf <dbpedia:Commonwealth_of_Nations> .

:Rank_Syntagmatarchis_Greece a :MilitaryRank ;
	owl:subClass :Rank_Syntagmatarchis ;
	foaf:name "Syntagmatarchis"@en ;
	rdfs:label "Syntagmatarchis (Greece)"@en , "Syntagmatarchis (Grekland)"@sv , "Syntagmatarchis (Kreikka)"@fi , "Syntagmatarchis (Grèce)"@fr , "Syntagmatarchis (Griechenland)"@de , "Syntagmatarchis (Grecia)"@it , "Syntagmatarchis (Griekenland)"@nl , "Syntagmatarchis (Hellas)"@no , "Syntagmatarchis (Grecja)"@pl , "Syntagmatarchis (Grécia)"@pt , "Syntagmatarchis (Греция)"@ru , "Syntagmatarchis (Grecia)"@es ;
	rdfs:comment "The specific instance of the Syntagmatarchis rank in the context of country Greece."@en ;
	owl:rankOf <dbpedia:Greece> .

:Rank_Syntagmatarchis_Official_Timocracy_of_Sapinetia a :MilitaryRank ;
	owl:subClass :Rank_Syntagmatarchis ;
	foaf:name "Syntagmatarchis"@en ;
	rdfs:label "Syntagmatarchis (Timocracy of Sapinetia)"@en ;
	rdfs:comment "The specific instance of the Syntagmatarchis rank in the context of the Timocracy of Sapinetia."@en ;
	owl:rankOf <dbpedia:Official_Timocracy_of_Sapinetia> .

<http://rdf.muninn-project.org/ontologies/military#Rank_Syntagmatarchis_Macedonia_%28ancient_kingdom%29> a :MilitaryRank ;
	owl:subClass :Rank_Syntagmatarchis ;
	foaf:name "Syntagmatarchis"@en ;
	rdfs:label "Syntagmatarchis (Macedonia (ancient kingdom))"@en , "Syntagmatarchis (Makedonian valtakunta)"@fi , "Syntagmatarchis (Royaume de Macédoine)"@fr , "Syntagmatarchis (Regno di Macedonia)"@it , "Syntagmatarchis (Macedonië (oudheid))"@nl , "Syntagmatarchis (Oldtidens Makedonia)"@no , "Syntagmatarchis (Starożytna Macedonia)"@pl , "Syntagmatarchis (Macedónia Antiga)"@pt , "Syntagmatarchis (Древняя Македония)"@ru , "Syntagmatarchis (Reino de Macedonia)"@es ;
	rdfs:comment "The specific instance of the Syntagmatarchis rank in the context of country Macedonia (ancient kingdom)."@en ;
	owl:rankOf <dbpedia:Macedonia_%28ancient_kingdom%29> .

:Rank_Syntagmatarchis_Achaean_League a :MilitaryRank ;
	owl:subClass :Rank_Syntagmatarchis ;
	foaf:name "Syntagmatarchis"@en ;
	rdfs:label "Syntagmatarchis (Achaean League)"@en , "Syntagmatarchis (Achaiska förbundet)"@sv , "Syntagmatarchis (Akhaian liitto)"@fi , "Syntagmatarchis (Ligue achéenne)"@fr , "Syntagmatarchis (Achaiischer Bund)"@de , "Syntagmatarchis (Lega achea)"@it , "Syntagmatarchis (Achaeïsche Bond)"@nl , "Syntagmatarchis (Det akhaiske forbund)"@no , "Syntagmatarchis (Związek Achajski)"@pl , "Syntagmatarchis (Liga Aqueia)"@pt , "Syntagmatarchis (Ахейский союз)"@ru , "Syntagmatarchis (Liga Aquea)"@es ;
	rdfs:comment "The specific instance of the Syntagmatarchis rank in the context of country Achaean League."@en ;
	owl:rankOf <dbpedia:Achaean_League> .

:Rank_Tagmatarchis_Greece a :MilitaryRank ;
	owl:subClass :Rank_Tagmatarchis ;
	foaf:name "Tagmatarchis"@en ;
	rdfs:label "Tagmatarchis (Greece)"@en , "Tagmatarchis (Grekland)"@sv , "Tagmatarchis (Kreikka)"@fi , "Tagmatarchis (Grèce)"@fr , "Tagmatarchis (Griechenland)"@de , "Tagmatarchis (Grecia)"@it , "Tagmatarchis (Griekenland)"@nl , "Tagmatarchis (Hellas)"@no , "Tagmatarchis (Grecja)"@pl , "Tagmatarchis (Grécia)"@pt , "Tagmatarchis (Греция)"@ru , "Tagmatarchis (Grecia)"@es ;
	rdfs:comment "The specific instance of the Tagmatarchis rank in the context of country Greece."@en ;
	owl:rankOf <dbpedia:Greece> .

:Rank_Tagmatarchis_Official_Timocracy_of_Sapinetia a :MilitaryRank ;
	owl:subClass :Rank_Tagmatarchis ;
	foaf:name "Tagmatarchis"@en ;
	rdfs:label "Tagmatarchis (Timocracy of Sapinetia)"@en ;
	rdfs:comment "The specific instance of the Tagmatarchis rank in the context of the Timocracy of Sapinetia."@en ;
	owl:rankOf <dbpedia:Official_Timocracy_of_Sapinetia> .

<http://rdf.muninn-project.org/ontologies/military#Rank_Tagmatarchis_Macedonia_%28ancient_kingdom%29> a :MilitaryRank ;
	owl:subClass :Rank_Tagmatarchis ;
	foaf:name "Tagmatarchis"@en ;
	rdfs:label "Tagmatarchis (Macedonia (ancient kingdom))"@en , "Tagmatarchis (Makedonian valtakunta)"@fi , "Tagmatarchis (Royaume de Macédoine)"@fr , "Tagmatarchis (Regno di Macedonia)"@it , "Tagmatarchis (Macedonië (oudheid))"@nl , "Tagmatarchis (Oldtidens Makedonia)"@no , "Tagmatarchis (Starożytna Macedonia)"@pl , "Tagmatarchis (Macedónia Antiga)"@pt , "Tagmatarchis (Древняя Македония)"@ru , "Tagmatarchis (Reino de Macedonia)"@es ;
	rdfs:comment "The specific instance of the Tagmatarchis rank in the context of country Macedonia (ancient kingdom)."@en ;
	owl:rankOf <dbpedia:Macedonia_%28ancient_kingdom%29> .

:Rank_Tagmatarchis_Achaean_League a :MilitaryRank ;
	owl:subClass :Rank_Tagmatarchis ;
	foaf:name "Tagmatarchis"@en ;
	rdfs:label "Tagmatarchis (Achaean League)"@en , "Tagmatarchis (Achaiska förbundet)"@sv , "Tagmatarchis (Akhaian liitto)"@fi , "Tagmatarchis (Ligue achéenne)"@fr , "Tagmatarchis (Achaiischer Bund)"@de , "Tagmatarchis (Lega achea)"@it , "Tagmatarchis (Achaeïsche Bond)"@nl , "Tagmatarchis (Det akhaiske forbund)"@no , "Tagmatarchis (Związek Achajski)"@pl , "Tagmatarchis (Liga Aqueia)"@pt , "Tagmatarchis (Ахейский союз)"@ru , "Tagmatarchis (Liga Aquea)"@es ;
	rdfs:comment "The specific instance of the Tagmatarchis rank in the context of country Achaean League."@en ;
	owl:rankOf <dbpedia:Achaean_League> .

:Rank_Trumpet_Major_England a :MilitaryRank ;
	owl:subClass :Rank_Trumpet_Major ;
	foaf:name "Trumpet Major"@en ;
	rdfs:label "Trumpet Major (England)"@en ;
	rdfs:comment "The specific instance of the Trumpet Major rank in the context of England."@en ;
	owl:rankOf <dbpedia:England> .

:Rank_Trumpet_Major_Scotland a :MilitaryRank ;
	owl:subClass :Rank_Trumpet_Major ;
	foaf:name "Trumpet Major"@en ;
	rdfs:label "Trumpet Major (Scotland)"@en , "Trumpet Major (Skottland)"@sv , "Trumpet Major (Skotlanti)"@fi , "Trumpet Major (Écosse)"@fr , "Trumpet Major (Schottland)"@de , "Trumpet Major (Scozia)"@it , "Trumpet Major (Schotland)"@nl , "Trumpet Major (Skottland)"@no , "Trumpet Major (Szkocja)"@pl , "Trumpet Major (Escócia)"@pt , "Trumpet Major (Шотландия)"@ru , "Trumpet Major (Escocia)"@es ;
	rdfs:comment "The specific instance of the Trumpet Major rank in the context of country Scotland."@en ;
	owl:rankOf <dbpedia:Scotland> .

:Rank_Trumpet_Major_Wales a :MilitaryRank ;
	owl:subClass :Rank_Trumpet_Major ;
	foaf:name "Trumpet Major"@en ;
	rdfs:label "Trumpet Major (Wales)"@en , "Trumpet Major (Wales)"@sv , "Trumpet Major (Wales)"@fi , "Trumpet Major (Pays de Galles)"@fr , "Trumpet Major (Wales)"@de , "Trumpet Major (Galles)"@it , "Trumpet Major (Wales)"@nl , "Trumpet Major (Wales)"@no , "Trumpet Major (Walia)"@pl , "Trumpet Major (País de Gales)"@pt , "Trumpet Major (Уэльс)"@ru , "Trumpet Major (Gales)"@es ;
	rdfs:comment "The specific instance of the Trumpet Major rank in the context of country Wales."@en ;
	owl:rankOf <dbpedia:Wales> .

:Rank_Trumpet_Major_Commonwealth_of_Nations a :MilitaryRank ;
	owl:subClass :Rank_Trumpet_Major ;
	foaf:name "Trumpet Major"@en ;
	rdfs:label "Trumpet Major (Commonwealth of Nations)"@en , "Trumpet Major (Samväldet)"@sv , "Trumpet Major (Kansainyhteisö)"@fi , "Trumpet Major (Commonwealth of Nations)"@fr , "Trumpet Major (Commonwealth of Nations)"@de , "Trumpet Major (Commonwealth delle nazioni)"@it , "Trumpet Major (Gemenebest van Naties)"@nl , "Trumpet Major (Samveldet av nasjoner)"@no , "Trumpet Major (Wspólnota Narodów)"@pl , "Trumpet Major (Commonwealth)"@pt , "Trumpet Major (Содружество наций)"@ru , "Trumpet Major (Mancomunidad de Naciones)"@es ;
	rdfs:comment "The specific instance of the Trumpet Major rank in the context of country Commonwealth of Nations."@en ;
	owl:rankOf <dbpedia:Commonwealth_of_Nations> .

:Rank_Chiliarch_Greece a :MilitaryRank ;
	owl:subClass :Rank_Chiliarch ;
	foaf:name "Chiliarch"@en ;
	rdfs:label "Chiliarch (Greece)"@en , "Chiliarch (Grekland)"@sv , "Chiliarch (Kreikka)"@fi , "Chiliarque (Grèce)"@fr , "Chiliarch (Griechenland)"@de , "Chiliarca (Grecia)"@it , "Chiliarch (Griekenland)"@nl , "Chiliarch (Hellas)"@no , "Chiliarcha (Grecja)"@pl , "Chiliarch (Grécia)"@pt , "Chiliarch (Греция)"@ru , "Quiliarca (Grecia)"@es ;
	rdfs:comment "The specific instance of the Chiliarch rank in the context of country Greece."@en ;
	owl:rankOf <dbpedia:Greece> .

:Rank_Chiliarch_Official_Timocracy_of_Sapinetia a :MilitaryRank ;
	owl:subClass :Rank_Chiliarch ;
	foaf:name "Chiliarch"@en ;
	rdfs:label "Chiliarch (Timocracy of Sapinetia)"@en , "Chiliarque (Timocracy of Sapinetia)"@fr , "Chiliarch (Timocracy of Sapinetia)"@de , "Chiliarca (Timocracy of Sapinetia)"@it , "Chiliarcha (Timocracy of Sapinetia)"@pl , "Quiliarca (Timocracy of Sapinetia)"@es ;
	rdfs:comment "The specific instance of the Chiliarch rank in the context of the Timocracy of Sapinetia."@en ;
	owl:rankOf <dbpedia:Official_Timocracy_of_Sapinetia> .

<http://rdf.muninn-project.org/ontologies/military#Rank_Chiliarch_Macedonia_%28ancient_kingdom%29> a :MilitaryRank ;
	owl:subClass :Rank_Chiliarch ;
	foaf:name "Chiliarch"@en ;
	rdfs:label "Chiliarch (Macedonia (ancient kingdom))"@en , "Chiliarch (Makedonian valtakunta)"@fi , "Chiliarque (Royaume de Macédoine)"@fr , "Chiliarch (Macedonia (ancient kingdom))"@de , "Chiliarca (Regno di Macedonia)"@it , "Chiliarch (Macedonië (oudheid))"@nl , "Chiliarch (Oldtidens Makedonia)"@no , "Chiliarcha (Starożytna Macedonia)"@pl , "Chiliarch (Macedónia Antiga)"@pt , "Chiliarch (Древняя Македония)"@ru , "Quiliarca (Reino de Macedonia)"@es ;
	rdfs:comment "The specific instance of the Chiliarch rank in the context of country Macedonia (ancient kingdom)."@en ;
	owl:rankOf <dbpedia:Macedonia_%28ancient_kingdom%29> .

:Rank_Chiliarch_Achaean_League a :MilitaryRank ;
	owl:subClass :Rank_Chiliarch ;
	foaf:name "Chiliarch"@en ;
	rdfs:label "Chiliarch (Achaean League)"@en , "Chiliarch (Achaiska förbundet)"@sv , "Chiliarch (Akhaian liitto)"@fi , "Chiliarque (Ligue achéenne)"@fr , "Chiliarch (Achaiischer Bund)"@de , "Chiliarca (Lega achea)"@it , "Chiliarch (Achaeïsche Bond)"@nl , "Chiliarch (Det akhaiske forbund)"@no , "Chiliarcha (Związek Achajski)"@pl , "Chiliarch (Liga Aqueia)"@pt , "Chiliarch (Ахейский союз)"@ru , "Quiliarca (Liga Aquea)"@es ;
	rdfs:comment "The specific instance of the Chiliarch rank in the context of country Achaean League."@en ;
	owl:rankOf <dbpedia:Achaean_League> .

:Rank_Chiliarch_Byzantine_Empire a :MilitaryRank ;
	owl:subClass :Rank_Chiliarch ;
	foaf:name "Chiliarch"@en ;
	rdfs:label "Chiliarch (Byzantine Empire)"@en , "Chiliarch (Bysantinska riket)"@sv , "Chiliarch (Bysantin valtakunta)"@fi , "Chiliarque (Empire byzantin)"@fr , "Chiliarch (Byzantinisches Reich)"@de , "Chiliarca (Impero bizantino)"@it , "Chiliarch (Byzantijnse Rijk)"@nl , "Chiliarch (Østromerriket)"@no , "Chiliarcha (Cesarstwo Bizantyńskie)"@pl , "Chiliarch (Império Bizantino)"@pt , "Chiliarch (Византийская империя)"@ru , "Quiliarca (Imperio bizantino)"@es ;
	rdfs:comment "The specific instance of the Chiliarch rank in the context of country Byzantine Empire."@en ;
	owl:rankOf <dbpedia:Byzantine_Empire> .

:Rank_Company_Quartermaster_Sergeant_England a :MilitaryRank ;
	owl:subClass :Rank_Company_Quartermaster_Sergeant ;
	foaf:name "Company Quartermaster Sergeant"@en ;
	rdfs:label "Company Quartermaster Sergeant (England)"@en ;
	rdfs:comment "The specific instance of the Company Quartermaster Sergeant rank in the context of England."@en ;
	owl:rankOf <dbpedia:England> .

:Rank_Company_Quartermaster_Sergeant_Scotland a :MilitaryRank ;
	owl:subClass :Rank_Company_Quartermaster_Sergeant ;
	foaf:name "Company Quartermaster Sergeant"@en ;
	rdfs:label "Company Quartermaster Sergeant (Scotland)"@en , "Company Quartermaster Sergeant (Skottland)"@sv , "Company Quartermaster Sergeant (Skotlanti)"@fi , "Company Quartermaster Sergeant (Écosse)"@fr , "Company Quartermaster Sergeant (Schottland)"@de , "Company Quartermaster Sergeant (Scozia)"@it , "Company Quartermaster Sergeant (Schotland)"@nl , "Company Quartermaster Sergeant (Skottland)"@no , "Company Quartermaster Sergeant (Szkocja)"@pl , "Company Quartermaster Sergeant (Escócia)"@pt , "Company Quartermaster Sergeant (Шотландия)"@ru , "Company Quartermaster Sergeant (Escocia)"@es ;
	rdfs:comment "The specific instance of the Company Quartermaster Sergeant rank in the context of country Scotland."@en ;
	owl:rankOf <dbpedia:Scotland> .

:Rank_Company_Quartermaster_Sergeant_Wales a :MilitaryRank ;
	owl:subClass :Rank_Company_Quartermaster_Sergeant ;
	foaf:name "Company Quartermaster Sergeant"@en ;
	rdfs:label "Company Quartermaster Sergeant (Wales)"@en , "Company Quartermaster Sergeant (Wales)"@sv , "Company Quartermaster Sergeant (Wales)"@fi , "Company Quartermaster Sergeant (Pays de Galles)"@fr , "Company Quartermaster Sergeant (Wales)"@de , "Company Quartermaster Sergeant (Galles)"@it , "Company Quartermaster Sergeant (Wales)"@nl , "Company Quartermaster Sergeant (Wales)"@no , "Company Quartermaster Sergeant (Walia)"@pl , "Company Quartermaster Sergeant (País de Gales)"@pt , "Company Quartermaster Sergeant (Уэльс)"@ru , "Company Quartermaster Sergeant (Gales)"@es ;
	rdfs:comment "The specific instance of the Company Quartermaster Sergeant rank in the context of country Wales."@en ;
	owl:rankOf <dbpedia:Wales> .

:Rank_Company_Quartermaster_Sergeant_Commonwealth_of_Nations a :MilitaryRank ;
	owl:subClass :Rank_Company_Quartermaster_Sergeant ;
	foaf:name "Company Quartermaster Sergeant"@en ;
	rdfs:label "Company Quartermaster Sergeant (Commonwealth of Nations)"@en , "Company Quartermaster Sergeant (Samväldet)"@sv , "Company Quartermaster Sergeant (Kansainyhteisö)"@fi , "Company Quartermaster Sergeant (Commonwealth of Nations)"@fr , "Company Quartermaster Sergeant (Commonwealth of Nations)"@de , "Company Quartermaster Sergeant (Commonwealth delle nazioni)"@it , "Company Quartermaster Sergeant (Gemenebest van Naties)"@nl , "Company Quartermaster Sergeant (Samveldet av nasjoner)"@no , "Company Quartermaster Sergeant (Wspólnota Narodów)"@pl , "Company Quartermaster Sergeant (Commonwealth)"@pt , "Company Quartermaster Sergeant (Содружество наций)"@ru , "Company Quartermaster Sergeant (Mancomunidad de Naciones)"@es ;
	rdfs:comment "The specific instance of the Company Quartermaster Sergeant rank in the context of country Commonwealth of Nations."@en ;
	owl:rankOf <dbpedia:Commonwealth_of_Nations> .

:Rank_Company_Quartermaster_Sergeant_Republic_of_Ireland a :MilitaryRank ;
	owl:subClass :Rank_Company_Quartermaster_Sergeant ;
	foaf:name "Company Quartermaster Sergeant"@en ;
	rdfs:label "Company Quartermaster Sergeant (Republic of Ireland)"@en , "Company Quartermaster Sergeant (Irland)"@sv , "Company Quartermaster Sergeant (Irlanti)"@fi , "Company Quartermaster Sergeant (Irlande (pays))"@fr , "Company Quartermaster Sergeant (Irland)"@de , "Company Quartermaster Sergeant (Irlanda)"@it , "Company Quartermaster Sergeant (Ierland (land))"@nl , "Company Quartermaster Sergeant (Irland)"@no , "Company Quartermaster Sergeant (Irlandia)"@pl , "Company Quartermaster Sergeant (República da Irlanda)"@pt , "Company Quartermaster Sergeant (Ирландия)"@ru , "Company Quartermaster Sergeant (Irlanda)"@es ;
	rdfs:comment "The specific instance of the Company Quartermaster Sergeant rank in the context of country Republic of Ireland."@en ;
	owl:rankOf <dbpedia:Republic_of_Ireland> .

:Rank_Lance_sergeant_Australia a :MilitaryRank ;
	owl:subClass :Rank_Lance_sergeant ;
	foaf:name ""@en ;
	rdfs:label "(Australia)"@en , "(Australien)"@sv , "(Australia)"@fi , "(Australie)"@fr , "(Australien)"@de , "(Australia)"@it , "(Australië (land))"@nl , "(Australia)"@no , "(Australia)"@pl , "(Austrália)"@pt , "(Австралия)"@ru , "(Australia)"@es ;
	rdfs:comment "The specific instance of the  rank in the context of country Australia."@en ;
	owl:rankOf <dbpedia:Australia> .

:Rank_Lance_sergeant_England a :MilitaryRank ;
	owl:subClass :Rank_Lance_sergeant ;
	foaf:name "Lance Sergeant"@en ;
	rdfs:label "Lance Sergeant (England)"@en ;
	rdfs:comment "The specific instance of the  rank in the context of England."@en ;
	owl:rankOf <dbpedia:England> .

:Rank_Lance_sergeant_Scotland a :MilitaryRank ;
	owl:subClass :Rank_Lance_sergeant ;
	foaf:name "Lance Sergeant"@en ;
	rdfs:label "Lance Sergeant (Scotland)"@en , "Lance Sergeant (Skottland)"@sv , "Lance Sergeant (Skotlanti)"@fi , "Lance Sergeant (Écosse)"@fr , "Lance Sergeant (Schottland)"@de , "Lance Sergeant (Scozia)"@it , "Lance Sergeant (Schotland)"@nl , "Lance Sergeant (Skottland)"@no , "Lance Sergeant (Szkocja)"@pl , "Lance Sergeant (Escócia)"@pt , "Lance Sergeant (Шотландия)"@ru , "Lance Sergeant (Escocia)"@es ;
	rdfs:comment "The specific instance of the Lance Sergeant rank in the context of country Scotland."@en ;
	owl:rankOf <dbpedia:Scotland> .

:Rank_Lance_sergeant_Wales a :MilitaryRank ;
	owl:subClass :Rank_Lance_sergeant ;
	foaf:name "Lance Sergeant"@en ;
	rdfs:label "Lance Sergeant (Wales)"@en , "Lance Sergeant (Wales)"@sv , "Lance Sergeant (Wales)"@fi , "Lance Sergeant (Pays de Galles)"@fr , "Lance Sergeant (Wales)"@de , "Lance Sergeant (Galles)"@it , "Lance Sergeant (Wales)"@nl , "Lance Sergeant (Wales)"@no , "Lance Sergeant (Walia)"@pl , "Lance Sergeant (País de Gales)"@pt , "Lance Sergeant (Уэльс)"@ru , "Lance Sergeant (Gales)"@es ;
	rdfs:comment "The specific instance of the Lance Sergeant rank in the context of country Wales."@en ;
	owl:rankOf <dbpedia:Wales> .

:Rank_Lance_sergeant_Commonwealth_of_Nations a :MilitaryRank ;
	owl:subClass :Rank_Lance_sergeant ;
	foaf:name "Lance Sergeant"@en ;
	rdfs:label "Lance Sergeant (Commonwealth of Nations)"@en , "Lance Sergeant (Samväldet)"@sv , "Lance Sergeant (Kansainyhteisö)"@fi , "Lance Sergeant (Commonwealth of Nations)"@fr , "Lance Sergeant (Commonwealth of Nations)"@de , "Lance Sergeant (Commonwealth delle nazioni)"@it , "Lance Sergeant (Gemenebest van Naties)"@nl , "Lance Sergeant (Samveldet av nasjoner)"@no , "Lance Sergeant (Wspólnota Narodów)"@pl , "Lance Sergeant (Commonwealth)"@pt , "Lance Sergeant (Содружество наций)"@ru , "Lance Sergeant (Mancomunidad de Naciones)"@es ;
	rdfs:comment "The specific instance of the Lance Sergeant  rank in the context of country Commonwealth of Nations."@en ;
	owl:rankOf <dbpedia:Commonwealth_of_Nations> .

:Rank_Strategos_Greece a :MilitaryRank ;
	owl:subClass :Rank_Strategos ;
	foaf:name "Strategos"@en ;
	rdfs:label "Strategos (Greece)"@en , "Strategos (Grekland)"@sv , "Strategos (Kreikka)"@fi , "Stratège (Grèce)"@fr , "Strategos (Griechenland)"@de , "Strategos (Grecia)"@it , "Strategos (Griekenland)"@nl , "Strategos (Hellas)"@no , "Strateg (Grecja) (Grecja)"@pl , "Estratego (Grécia)"@pt , "Стратег (Греция)"@ru , "Strategos (Grecia)"@es ;
	rdfs:comment "The specific instance of the Strategos rank in the context of country Greece."@en ;
	owl:rankOf <dbpedia:Greece> .

:Rank_Strategos_Official_Timocracy_of_Sapinetia a :MilitaryRank ;
	owl:subClass :Rank_Strategos ;
	foaf:name "Strategos"@en ;
	rdfs:label "Strategos (Timocracy of Sapinetia)"@en , "Strategos (Timocracy of Sapinetia)"@fi , "Stratège (Timocracy of Sapinetia)"@fr , "Strategos (Timocracy of Sapinetia)"@de , "Strategos (Timocracy of Sapinetia)"@it , "Strategos (Timocracy of Sapinetia)"@nl , "Strategos (Timocracy of Sapinetia)"@no , "Strateg (Grecja) (Timocracy of Sapinetia)"@pl , "Estratego (Timocracy of Sapinetia)"@pt , "Стратег (Timocracy of Sapinetia)"@ru , "Strategos (Timocracy of Sapinetia)"@es ;
	rdfs:comment "The specific instance of the Strategos rank in the context of the Timocracy of Sapinetia."@en ;
	owl:rankOf <dbpedia:Official_Timocracy_of_Sapinetia> .

<http://rdf.muninn-project.org/ontologies/military#Rank_Strategos_Macedonia_%28ancient_kingdom%29> a :MilitaryRank ;
	owl:subClass :Rank_Strategos ;
	foaf:name "Strategos"@en ;
	rdfs:label "Strategos (Macedonia (ancient kingdom))"@en , "Strategos (Makedonian valtakunta)"@fi , "Stratège (Royaume de Macédoine)"@fr , "Strategos (Macedonia (ancient kingdom))"@de , "Strategos (Regno di Macedonia)"@it , "Strategos (Macedonië (oudheid))"@nl , "Strategos (Oldtidens Makedonia)"@no , "Strateg (Grecja) (Starożytna Macedonia)"@pl , "Estratego (Macedónia Antiga)"@pt , "Стратег (Древняя Македония)"@ru , "Strategos (Reino de Macedonia)"@es ;
	rdfs:comment "The specific instance of the Strategos rank in the context of country Macedonia (ancient kingdom)."@en ;
	owl:rankOf <dbpedia:Macedonia_%28ancient_kingdom%29> .

:Rank_Strategos_Achaean_League a :MilitaryRank ;
	owl:subClass :Rank_Strategos ;
	foaf:name "Strategos"@en ;
	rdfs:label "Strategos (Achaean League)"@en , "Strategos (Achaiska förbundet)"@sv , "Strategos (Akhaian liitto)"@fi , "Stratège (Ligue achéenne)"@fr , "Strategos (Achaiischer Bund)"@de , "Strategos (Lega achea)"@it , "Strategos (Achaeïsche Bond)"@nl , "Strategos (Det akhaiske forbund)"@no , "Strateg (Grecja) (Związek Achajski)"@pl , "Estratego (Liga Aqueia)"@pt , "Стратег (Ахейский союз)"@ru , "Strategos (Liga Aquea)"@es ;
	rdfs:comment "The specific instance of the Strategos rank in the context of country Achaean League."@en ;
	owl:rankOf <dbpedia:Achaean_League> .

:Rank_Strategos_Byzantine_Empire a :MilitaryRank ;
	owl:subClass :Rank_Strategos ;
	foaf:name "Strategos"@en ;
	rdfs:label "Strategos (Byzantine Empire)"@en , "Strategos (Bysantinska riket)"@sv , "Strategos (Bysantin valtakunta)"@fi , "Stratège (Empire byzantin)"@fr , "Strategos (Byzantinisches Reich)"@de , "Strategos (Impero bizantino)"@it , "Strategos (Byzantijnse Rijk)"@nl , "Strategos (Østromerriket)"@no , "Strateg (Grecja) (Cesarstwo Bizantyńskie)"@pl , "Estratego (Império Bizantino)"@pt , "Стратег (Византийская империя)"@ru , "Strategos (Imperio bizantino)"@es ;
	rdfs:comment "The specific instance of the Strategos rank in the context of country Byzantine Empire."@en ;
	owl:rankOf <dbpedia:Byzantine_Empire> .

:Rank_Strategos_autokrator_Byzantine_Empire a :MilitaryRank ;
	owl:subClass :Rank_Strategos_autokrator ;
	foaf:name "Strategos autokrator"@en ;
	rdfs:label "Strategos autokrator (Byzantine Empire)"@en , "Strategos autokrator (Bysantinska riket)"@sv , "Strategos autokrator (Bysantin valtakunta)"@fi , "Strategos autokrator (Empire byzantin)"@fr , "Strategos autokrator (Byzantinisches Reich)"@de , "Strategos autokrator (Impero bizantino)"@it , "Strategos autokrator (Byzantijnse Rijk)"@nl , "Strategos autokrator (Østromerriket)"@no , "Strategos autokrator (Cesarstwo Bizantyńskie)"@pl , "Strategos autokrator (Império Bizantino)"@pt , "Strategos autokrator (Византийская империя)"@ru , "Strategos autokrator (Imperio bizantino)"@es ;
	rdfs:comment "The specific instance of the Strategos autokrator rank in the context of country Byzantine Empire."@en ;
	owl:rankOf <dbpedia:Byzantine_Empire> .

:Rank_Taxiarch_Greece a :MilitaryRank ;
	owl:subClass :Rank_Taxiarch ;
	foaf:name "Taxiarch"@en ;
	rdfs:label "Taxiarch (Greece)"@en , "Taxiarch (Grekland)"@sv , "Taxiarch (Kreikka)"@fi , "Taxiarch (Grèce)"@fr , "Taxiarch (Griechenland)"@de , "Taxiarch (Grecia)"@it , "Taxiarch (Griekenland)"@nl , "Taxiarch (Hellas)"@no , "Taxiarch (Grecja)"@pl , "Taxiarch (Grécia)"@pt , "Таксиарх (Греция)"@ru , "Taxiarch (Grecia)"@es ;
	rdfs:comment "The specific instance of the Taxiarch rank in the context of country Greece."@en ;
	owl:rankOf <dbpedia:Greece> .

:Rank_Taxiarch_Official_Timocracy_of_Sapinetia a :MilitaryRank ;
	owl:subClass :Rank_Taxiarch ;
	foaf:name "Taxiarch"@en ;
	rdfs:label "Taxiarch (Timocracy of Sapinetia)"@en , "Таксиарх (Timocracy of Sapinetia)"@ru ;
	rdfs:comment "The specific instance of the Taxiarch rank in the context of the Timocracy of Sapinetia."@en ;
	owl:rankOf <dbpedia:Official_Timocracy_of_Sapinetia> .

<http://rdf.muninn-project.org/ontologies/military#Rank_Taxiarch_Macedonia_%28ancient_kingdom%29> a :MilitaryRank ;
	owl:subClass :Rank_Taxiarch ;
	foaf:name "Taxiarch"@en ;
	rdfs:label "Taxiarch (Macedonia (ancient kingdom))"@en , "Taxiarch (Makedonian valtakunta)"@fi , "Taxiarch (Royaume de Macédoine)"@fr , "Taxiarch (Regno di Macedonia)"@it , "Taxiarch (Macedonië (oudheid))"@nl , "Taxiarch (Oldtidens Makedonia)"@no , "Taxiarch (Starożytna Macedonia)"@pl , "Taxiarch (Macedónia Antiga)"@pt , "Таксиарх (Древняя Македония)"@ru , "Taxiarch (Reino de Macedonia)"@es ;
	rdfs:comment "The specific instance of the Taxiarch rank in the context of country Macedonia (ancient kingdom)."@en ;
	owl:rankOf <dbpedia:Macedonia_%28ancient_kingdom%29> .

:Rank_Taxiarch_Achaean_League a :MilitaryRank ;
	owl:subClass :Rank_Taxiarch ;
	foaf:name "Taxiarch"@en ;
	rdfs:label "Taxiarch (Achaean League)"@en , "Taxiarch (Achaiska förbundet)"@sv , "Taxiarch (Akhaian liitto)"@fi , "Taxiarch (Ligue achéenne)"@fr , "Taxiarch (Achaiischer Bund)"@de , "Taxiarch (Lega achea)"@it , "Taxiarch (Achaeïsche Bond)"@nl , "Taxiarch (Det akhaiske forbund)"@no , "Taxiarch (Związek Achajski)"@pl , "Taxiarch (Liga Aqueia)"@pt , "Таксиарх (Ахейский союз)"@ru , "Taxiarch (Liga Aquea)"@es ;
	rdfs:comment "The specific instance of the Taxiarch rank in the context of country Achaean League."@en ;
	owl:rankOf <dbpedia:Achaean_League> .

:Rank_Taxiarch_Byzantine_Empire a :MilitaryRank ;
	owl:subClass :Rank_Taxiarch ;
	foaf:name "Taxiarch"@en ;
	rdfs:label "Taxiarch (Byzantine Empire)"@en , "Taxiarch (Bysantinska riket)"@sv , "Taxiarch (Bysantin valtakunta)"@fi , "Taxiarch (Empire byzantin)"@fr , "Taxiarch (Byzantinisches Reich)"@de , "Taxiarch (Impero bizantino)"@it , "Taxiarch (Byzantijnse Rijk)"@nl , "Taxiarch (Østromerriket)"@no , "Taxiarch (Cesarstwo Bizantyńskie)"@pl , "Taxiarch (Império Bizantino)"@pt , "Таксиарх (Византийская империя)"@ru , "Taxiarch (Imperio bizantino)"@es ;
	rdfs:comment "The specific instance of the Taxiarch rank in the context of country Byzantine Empire."@en ;
	owl:rankOf <dbpedia:Byzantine_Empire> .

:Rank_Under_Officer_Australia a :MilitaryRank ;
	owl:subClass :Rank_Under_Officer ;
	foaf:name "Under Officer"@en ;
	rdfs:label "Under Officer (Australia)"@en , "Under Officer (Australien)"@sv , "Under Officer (Australia)"@fi , "Under Officer (Australie)"@fr , "Under Officer (Australien)"@de , "Under Officer (Australia)"@it , "Under Officer (Australië (land))"@nl , "Under Officer (Australia)"@no , "Under Officer (Australia)"@pl , "Under Officer (Austrália)"@pt , "Under Officer (Австралия)"@ru , "Under Officer (Australia)"@es ;
	rdfs:comment "The specific instance of the Under Officer rank in the context of country Australia."@en ;
	owl:rankOf <dbpedia:Australia> .

:Rank_Under_Officer_England a :MilitaryRank ;
	owl:subClass :Rank_Under_Officer ;
	foaf:name "Under Officer"@en ;
	rdfs:label "Under Officer (England)"@en ;
	rdfs:comment "The specific instance of the Under Officer rank in the context of England."@en ;
	owl:rankOf <dbpedia:England> .

:Rank_Under_Officer_Scotland a :MilitaryRank ;
	owl:subClass :Rank_Under_Officer ;
	foaf:name "Under Officer"@en ;
	rdfs:label "Under Officer (Scotland)"@en , "Under Officer (Skottland)"@sv , "Under Officer (Skotlanti)"@fi , "Under Officer (Écosse)"@fr , "Under Officer (Schottland)"@de , "Under Officer (Scozia)"@it , "Under Officer (Schotland)"@nl , "Under Officer (Skottland)"@no , "Under Officer (Szkocja)"@pl , "Under Officer (Escócia)"@pt , "Under Officer (Шотландия)"@ru , "Under Officer (Escocia)"@es ;
	rdfs:comment "The specific instance of the Under Officer rank in the context of country Scotland."@en ;
	owl:rankOf <dbpedia:Scotland> .

:Rank_Under_Officer_Wales a :MilitaryRank ;
	owl:subClass :Rank_Under_Officer ;
	foaf:name "Under Officer"@en ;
	rdfs:label "Under Officer (Wales)"@en , "Under Officer (Wales)"@sv , "Under Officer (Wales)"@fi , "Under Officer (Pays de Galles)"@fr , "Under Officer (Wales)"@de , "Under Officer (Galles)"@it , "Under Officer (Wales)"@nl , "Under Officer (Wales)"@no , "Under Officer (Walia)"@pl , "Under Officer (País de Gales)"@pt , "Under Officer (Уэльс)"@ru , "Under Officer (Gales)"@es ;
	rdfs:comment "The specific instance of the Under Officer rank in the context of country Wales."@en ;
	owl:rankOf <dbpedia:Wales> .

:Rank_Under_Officer_Commonwealth_of_Nations a :MilitaryRank ;
	owl:subClass :Rank_Under_Officer ;
	foaf:name "Under Officer"@en ;
	rdfs:label "Under Officer (Commonwealth of Nations)"@en , "Under Officer (Samväldet)"@sv , "Under Officer (Kansainyhteisö)"@fi , "Under Officer (Commonwealth of Nations)"@fr , "Under Officer (Commonwealth of Nations)"@de , "Under Officer (Commonwealth delle nazioni)"@it , "Under Officer (Gemenebest van Naties)"@nl , "Under Officer (Samveldet av nasjoner)"@no , "Under Officer (Wspólnota Narodów)"@pl , "Under Officer (Commonwealth)"@pt , "Under Officer (Содружество наций)"@ru , "Under Officer (Mancomunidad de Naciones)"@es ;
	rdfs:comment "The specific instance of the Under Officer rank in the context of country Commonwealth of Nations."@en ;
	owl:rankOf <dbpedia:Commonwealth_of_Nations> .

:Rank_Lance_corporal_Australia a :MilitaryRank ;
	owl:subClass :Rank_Lance_corporal ;
	foaf:name "Lance corporal"@en ;
	rdfs:label "Lance corporal (Australia)"@en , "Lance corporal (Australien)"@sv , "Lance corporal (Australia)"@fi , "Lance corporal (Australie)"@fr , "Lance corporal (Australien)"@de , "Lance corporal (Australia)"@it , "Lance corporal (Australië (land))"@nl , "Lance corporal (Australia)"@no , "Lance corporal (Australia)"@pl , "Lance corporal (Austrália)"@pt , "Lance corporal (Австралия)"@ru , "Lance corporal (Australia)"@es ;
	rdfs:comment "The specific instance of the Lance corporal rank in the context of country Australia."@en ;
	owl:rankOf <dbpedia:Australia> .

:Rank_Lance_corporal_England a :MilitaryRank ;
	owl:subClass :Rank_Lance_corporal ;
	foaf:name "Lance corporal"@en ;
	rdfs:label "Lance corporal (England)"@en ;
	rdfs:comment "The specific instance of the Lance corporal rank in the context of England"@en ;
	owl:rankOf <dbpedia:England> .

:Rank_Lance_corporal_Scotland a :MilitaryRank ;
	owl:subClass :Rank_Lance_corporal ;
	foaf:name "Lance corporal"@en ;
	rdfs:label "Lance corporal (Scotland)"@en , "Lance corporal (Skottland)"@sv , "Lance corporal (Skotlanti)"@fi , "Lance corporal (Écosse)"@fr , "Lance corporal (Schottland)"@de , "Lance corporal (Scozia)"@it , "Lance corporal (Schotland)"@nl , "Lance corporal (Skottland)"@no , "Lance corporal (Szkocja)"@pl , "Lance corporal (Escócia)"@pt , "Lance corporal (Шотландия)"@ru , "Lance corporal (Escocia)"@es ;
	rdfs:comment "The specific instance of the Lance corporal rank in the context of country Scotland."@en ;
	owl:rankOf <dbpedia:Scotland> .

:Rank_Lance_corporal_Wales a :MilitaryRank ;
	owl:subClass :Rank_Lance_corporal ;
	foaf:name "Lance corporal"@en ;
	rdfs:label "Lance corporal (Wales)"@en , "Lance corporal (Wales)"@sv , "Lance corporal (Wales)"@fi , "Lance corporal (Pays de Galles)"@fr , "Lance corporal (Wales)"@de , "Lance corporal (Galles)"@it , "Lance corporal (Wales)"@nl , "Lance corporal (Wales)"@no , "Lance corporal (Walia)"@pl , "Lance corporal (País de Gales)"@pt , "Lance corporal (Уэльс)"@ru , "Lance corporal (Gales)"@es ;
	rdfs:comment "The specific instance of the Lance corporal rank in the context of country Wales."@en ;
	owl:rankOf <dbpedia:Wales> .

:Rank_Lance_corporal_Singapore a :MilitaryRank ;
	owl:subClass :Rank_Lance_corporal ;
	foaf:name "Lance corporal"@en ;
	rdfs:label "Lance corporal (Singapore)"@en , "Lance corporal (Singapore)"@sv , "Lance corporal (Singapore)"@fi , "Lance corporal (Singapour)"@fr , "Lance corporal (Singapur)"@de , "Lance corporal (Singapore)"@it , "Lance corporal (Singapore)"@nl , "Lance corporal (Singapore)"@no , "Lance corporal (Singapur)"@pl , "Lance corporal (Singapura)"@pt , "Lance corporal (Сингапур)"@ru , "Lance corporal (Singapur)"@es ;
	rdfs:comment "The specific instance of the Lance corporal rank in the context of country Singapore."@en ;
	owl:rankOf <dbpedia:Singapore> .

:Rank_Lance_corporal_Commonwealth_of_Nations a :MilitaryRank ;
	owl:subClass :Rank_Lance_corporal ;
	foaf:name "Lance corporal"@en ;
	rdfs:label "Lance corporal (Commonwealth of Nations)"@en , "Lance corporal (Samväldet)"@sv , "Lance corporal (Kansainyhteisö)"@fi , "Lance corporal (Commonwealth of Nations)"@fr , "Lance corporal (Commonwealth of Nations)"@de , "Lance corporal (Commonwealth delle nazioni)"@it , "Lance corporal (Gemenebest van Naties)"@nl , "Lance corporal (Samveldet av nasjoner)"@no , "Lance corporal (Wspólnota Narodów)"@pl , "Lance corporal (Commonwealth)"@pt , "Lance corporal (Содружество наций)"@ru , "Lance corporal (Mancomunidad de Naciones)"@es ;
	rdfs:comment "The specific instance of the Lance corporal rank in the context of country Commonwealth of Nations."@en ;
	owl:rankOf <dbpedia:Commonwealth_of_Nations> .

<http://rdf.muninn-project.org/ontologies/military#Rank_Private_%28rank%29_Australia> a :MilitaryRank ;
	owl:subClass <http://rdf.muninn-project.org/ontologies/military#Rank_Private_%28rank%29> ;
	foaf:name "Private"@en ;
	rdfs:label "Private (rank) (Australia)"@en , "Menig 1klMenig (Australien)"@sv , "Sotamies (Australia)"@fi , "Deuxième classeSoldat (grade) (Australie)"@fr , "Private (Dienstgrad)Soldat (Dienstgrad) (Australien)"@de , "Private (rank) (Australia)"@it , "Private (rank) (Australië (land))"@nl , "Menig (grad)Menig (Australia)"@no , "Szeregowy (Australia)"@pl , "Private (rank) (Austrália)"@pt , "Рядовой (Австралия)"@ru , "Soldado raso (Australia)"@es ;
	rdfs:comment "The specific instance of the Private (rank) rank in the context of country Australia."@en ;
	owl:rankOf <dbpedia:Australia> .

<http://rdf.muninn-project.org/ontologies/military#Rank_Private_%28rank%29_England> a :MilitaryRank ;
	owl:subClass <http://rdf.muninn-project.org/ontologies/military#Rank_Private_%28rank%29> ;
	foaf:name "Private"@en ;
	rdfs:label "Private (rank, England)"@en , "Menig 1klMenig (England)"@sv , "Sotamies (England)"@fi , "Deuxième classeSoldat (grade) (England)"@fr , "Private (Dienstgrad)Soldat (Dienstgrad, England)"@de , "Menig (grad, England)"@no , "Szeregowy (England)"@pl , "Рядовой (England)"@ru , "Soldado raso (England)"@es ;
	rdfs:comment "The specific instance of the Private (rank) rank in the context of England."@en ;
	owl:rankOf <dbpedia:England> .

<http://rdf.muninn-project.org/ontologies/military#Rank_Private_%28rank%29_Scotland> a :MilitaryRank ;
	owl:subClass <http://rdf.muninn-project.org/ontologies/military#Rank_Private_%28rank%29> ;
	foaf:name "Private"@en ;
	rdfs:label "Private (rank) (Scotland)"@en , "Menig 1klMenig (Skottland)"@sv , "Sotamies (Skotlanti)"@fi , "Deuxième classeSoldat (grade) (Écosse)"@fr , "Private (Dienstgrad)Soldat (Dienstgrad) (Schottland)"@de , "Private (rank) (Scozia)"@it , "Private (rank) (Schotland)"@nl , "Menig (grad)Menig (Skottland)"@no , "Szeregowy (Szkocja)"@pl , "Private (rank) (Escócia)"@pt , "Рядовой (Шотландия)"@ru , "Soldado raso (Escocia)"@es ;
	rdfs:comment "The specific instance of the Private (rank) rank in the context of country Scotland."@en ;
	owl:rankOf <dbpedia:Scotland> .

<http://rdf.muninn-project.org/ontologies/military#Rank_Private_%28rank%29_Wales> a :MilitaryRank ;
	owl:subClass <http://rdf.muninn-project.org/ontologies/military#Rank_Private_%28rank%29> ;
	foaf:name "Private"@en ;
	rdfs:label "Private (rank) (Wales)"@en , "Menig 1klMenig (Wales)"@sv , "Sotamies (Wales)"@fi , "Deuxième classeSoldat (grade) (Pays de Galles)"@fr , "Private (Dienstgrad)Soldat (Dienstgrad) (Wales)"@de , "Private (rank) (Galles)"@it , "Private (rank) (Wales)"@nl , "Menig (grad)Menig (Wales)"@no , "Szeregowy (Walia)"@pl , "Private (rank) (País de Gales)"@pt , "Рядовой (Уэльс)"@ru , "Soldado raso (Gales)"@es ;
	rdfs:comment "The specific instance of the Private (rank) rank in the context of country Wales."@en ;
	owl:rankOf <dbpedia:Wales> .

<http://rdf.muninn-project.org/ontologies/military#Rank_Private_%28rank%29_Canada> a :MilitaryRank ;
	owl:subClass <http://rdf.muninn-project.org/ontologies/military#Rank_Private_%28rank%29> ;
	foaf:name "Private"@en , "Soldat, Deuxième classe"@fr ;
	rdfs:label "Private (rank, Canada)"@en , "Menig 1klMenig (Canada)"@sv , "Sotamies (Canada)"@fi , "Deuxième classeSoldat (grade, Canada)"@fr , "Soldat (Dienstgrad, Canada)"@de , "Menig (grad, Canada)"@no , "Szeregowy (Canada)"@pl , "Рядовой (Canada)"@ru , "Soldado raso (Canada)"@es ;
	rdfs:comment "The specific instance of the Private (rank) rank in the context of Canada."@en ;
	owl:rankOf <dbpedia:Canada> .

<http://rdf.muninn-project.org/ontologies/military#Rank_Private_%28rank%29_Republic_of_Ireland> a :MilitaryRank ;
	owl:subClass <http://rdf.muninn-project.org/ontologies/military#Rank_Private_%28rank%29> ;
	foaf:name "Private"@en ;
	rdfs:label "Private (rank) (Republic of Ireland)"@en , "Menig 1klMenig (Irland)"@sv , "Sotamies (Irlanti)"@fi , "Deuxième classeSoldat (grade) (Irlande (pays))"@fr , "Private (Dienstgrad)Soldat (Dienstgrad) (Irland)"@de , "Private (rank) (Irlanda)"@it , "Private (rank) (Ierland (land))"@nl , "Menig (grad)Menig (Irland)"@no , "Szeregowy (Irlandia)"@pl , "Private (rank) (República da Irlanda)"@pt , "Рядовой (Ирландия)"@ru , "Soldado raso (Irlanda)"@es ;
	rdfs:comment "The specific instance of the Private (rank) rank in the context of country Republic of Ireland."@en ;
	owl:rankOf <dbpedia:Republic_of_Ireland> .

:Rank_Sergeant_Pilot_Australia a :MilitaryRank ;
	owl:subClass :Rank_Sergeant_Pilot ;
	foaf:name "Sergeant Pilot"@en ;
	rdfs:label "Sergeant Pilot (Australia)"@en , "Fältflygare (Australien)"@sv , "Sergeant Pilot (Australia)"@fi , "Sergeant Pilot (Australie)"@fr , "Sergeant Pilot (Australien)"@de , "Sergeant Pilot (Australia)"@it , "Sergeant Pilot (Australië (land))"@nl , "Sergeant Pilot (Australia)"@no , "Sergeant Pilot (Australia)"@pl , "Sergeant Pilot (Austrália)"@pt , "Sergeant Pilot (Австралия)"@ru , "Sergeant Pilot (Australia)"@es ;
	rdfs:comment "The specific instance of the Sergeant Pilot rank in the context of country Australia."@en ;
	owl:rankOf <dbpedia:Australia> .

:Rank_Sergeant_Pilot_England a :MilitaryRank ;
	owl:subClass :Rank_Sergeant_Pilot ;
	foaf:name "Sergeant Pilot"@en ;
	rdfs:label "Sergeant Pilot (England)"@en , "Fältflygare (England)"@sv ;
	rdfs:comment "The specific instance of the Sergeant Pilot rank in the context of England."@en ;
	owl:rankOf <dbpedia:England> .

:Rank_Sergeant_Pilot_Scotland a :MilitaryRank ;
	owl:subClass :Rank_Sergeant_Pilot ;
	foaf:name "Sergeant Pilot"@en ;
	rdfs:label "Sergeant Pilot (Scotland)"@en , "Fältflygare (Skottland)"@sv , "Sergeant Pilot (Skotlanti)"@fi , "Sergeant Pilot (Écosse)"@fr , "Sergeant Pilot (Schottland)"@de , "Sergeant Pilot (Scozia)"@it , "Sergeant Pilot (Schotland)"@nl , "Sergeant Pilot (Skottland)"@no , "Sergeant Pilot (Szkocja)"@pl , "Sergeant Pilot (Escócia)"@pt , "Sergeant Pilot (Шотландия)"@ru , "Sergeant Pilot (Escocia)"@es ;
	rdfs:comment "The specific instance of the Sergeant Pilot rank in the context of country Scotland."@en ;
	owl:rankOf <dbpedia:Scotland> .

:Rank_Sergeant_Pilot_Wales a :MilitaryRank ;
	owl:subClass :Rank_Sergeant_Pilot ;
	foaf:name "Sergeant Pilot"@en ;
	rdfs:label "Sergeant Pilot (Wales)"@en , "Fältflygare (Wales)"@sv , "Sergeant Pilot (Wales)"@fi , "Sergeant Pilot (Pays de Galles)"@fr , "Sergeant Pilot (Wales)"@de , "Sergeant Pilot (Galles)"@it , "Sergeant Pilot (Wales)"@nl , "Sergeant Pilot (Wales)"@no , "Sergeant Pilot (Walia)"@pl , "Sergeant Pilot (País de Gales)"@pt , "Sergeant Pilot (Уэльс)"@ru , "Sergeant Pilot (Gales)"@es ;
	rdfs:comment "The specific instance of the Sergeant Pilot rank in the context of country Wales."@en ;
	owl:rankOf <dbpedia:Wales> .

:Rank_Sergeant_Pilot_Canada a :MilitaryRank ;
	owl:subClass :Rank_Sergeant_Pilot ;
	foaf:name "Sergeant Pilot"@en ;
	rdfs:label "Sergeant Pilot (Canada)"@en , "Fältflygare (Canada)"@sv ;
	rdfs:comment "The specific instance of the Sergeant Pilot rank in the context of Canada."@en ;
	owl:rankOf <dbpedia:Canada> .

:Rank_Sergeant_Pilot_Commonwealth_of_Nations a :MilitaryRank ;
	owl:subClass :Rank_Sergeant_Pilot ;
	foaf:name "Sergeant Pilot"@en ;
	rdfs:label "Sergeant Pilot (Commonwealth of Nations)"@en , "Fältflygare (Samväldet)"@sv , "Sergeant Pilot (Kansainyhteisö)"@fi , "Sergeant Pilot (Commonwealth of Nations)"@fr , "Sergeant Pilot (Commonwealth of Nations)"@de , "Sergeant Pilot (Commonwealth delle nazioni)"@it , "Sergeant Pilot (Gemenebest van Naties)"@nl , "Sergeant Pilot (Samveldet av nasjoner)"@no , "Sergeant Pilot (Wspólnota Narodów)"@pl , "Sergeant Pilot (Commonwealth)"@pt , "Sergeant Pilot (Содружество наций)"@ru , "Sergeant Pilot (Mancomunidad de Naciones)"@es ;
	rdfs:comment "The specific instance of the Sergeant Pilot rank in the context of country Commonwealth of Nations."@en ;
	owl:rankOf <dbpedia:Commonwealth_of_Nations> .

<http://rdf.muninn-project.org/ontologies/military#Rank_Warrant_officer_%28United_Kingdom%29_Australia> a :MilitaryRank ;
	owl:subClass <http://rdf.muninn-project.org/ontologies/military#Rank_Warrant_officer_%28United_Kingdom%29> ;
	foaf:name "Warrant Officer"@en ;
	rdfs:label "Warrant Officer (Australia)"@en , "Warrant Officer (Australien)"@sv , "Warrant Officer (Australia)"@fi , "Warrant Officer (Australie)"@fr , "Warrant Officer (Australien)"@de , "Warrant Officer (Australia)"@it , "Warrant Officer (Australië (land))"@nl , "Warrant Officer (Australia)"@no , "Warrant Officer (Australia)"@pl , "Warrant Officer (Austrália)"@pt , "Warrant Officer (Австралия)"@ru , "Warrant Officer (Australia)"@es ;
	rdfs:comment "The specific instance of the Warrant Officer rank in the context of country Australia."@en ;
	owl:rankOf <dbpedia:Australia> .

<http://rdf.muninn-project.org/ontologies/military#Rank_Warrant_officer_%28United_Kingdom%29_England> a :MilitaryRank ;
	owl:subClass <http://rdf.muninn-project.org/ontologies/military#Rank_Warrant_officer_%28United_Kingdom%29> ;
	foaf:name "Warrant Officer"@en ;
	rdfs:label "Warrant Officer (England)"@en ;
	rdfs:comment "The specific instance of the  rank in the context of England."@en ;
	owl:rankOf <dbpedia:England> .

<http://rdf.muninn-project.org/ontologies/military#Rank_Warrant_officer_%28United_Kingdom%29_Scotland> a :MilitaryRank ;
	owl:subClass <http://rdf.muninn-project.org/ontologies/military#Rank_Warrant_officer_%28United_Kingdom%29> ;
	foaf:name "Warrant Officer"@en ;
	rdfs:label "Warrant Officer (Scotland)"@en , "Warrant Officer (Skottland)"@sv , "Warrant Officer (Skotlanti)"@fi , "Warrant Officer (Écosse)"@fr , "Warrant Officer (Schottland)"@de , "Warrant Officer (Scozia)"@it , "Warrant Officer (Schotland)"@nl , "Warrant Officer (Skottland)"@no , "Warrant Officer (Szkocja)"@pl , "Warrant Officer (Escócia)"@pt , "Warrant Officer (Шотландия)"@ru , "Warrant Officer (Escocia)"@es ;
	rdfs:comment "The specific instance of the Warrant Officer rank in the context of country Scotland."@en ;
	owl:rankOf <dbpedia:Scotland> .

<http://rdf.muninn-project.org/ontologies/military#Rank_Warrant_officer_%28United_Kingdom%29_Wales> a :MilitaryRank ;
	owl:subClass <http://rdf.muninn-project.org/ontologies/military#Rank_Warrant_officer_%28United_Kingdom%29> ;
	foaf:name "Warrant Officer"@en ;
	rdfs:label "Warrant Officer (Wales)"@en , "Warrant Officer (Wales)"@sv , "Warrant Officer (Wales)"@fi , "Warrant Officer (Pays de Galles)"@fr , "Warrant Officer (Wales)"@de , "Warrant Officer (Galles)"@it , "Warrant Officer (Wales)"@nl , "Warrant Officer (Wales)"@no , "Warrant Officer (Walia)"@pl , "Warrant Officer (País de Gales)"@pt , "Warrant Officer (Уэльс)"@ru , "Warrant Officer (Gales)"@es ;
	rdfs:comment "The specific instance of the Warrant Officer rank in the context of country Wales."@en ;
	owl:rankOf <dbpedia:Wales> .

<http://rdf.muninn-project.org/ontologies/military#Rank_Warrant_officer_%28United_Kingdom%29_Canada> a :MilitaryRank ;
	owl:subClass <http://rdf.muninn-project.org/ontologies/military#Rank_Warrant_officer_%28United_Kingdom%29> ;
	foaf:name "Warrant Officer"@en ;
	rdfs:label "Warrant Officer (Canada)"@en ;
	rdfs:comment "The specific instance of the  rank in the context of Canada"@en ;
	owl:rankOf <dbpedia:Canada> .

<http://rdf.muninn-project.org/ontologies/military#Rank_Warrant_officer_%28United_Kingdom%29_Commonwealth_of_Nations> a :MilitaryRank ;
	owl:subClass <http://rdf.muninn-project.org/ontologies/military#Rank_Warrant_officer_%28United_Kingdom%29> ;
	foaf:name "Warrant Officer"@en ;
	rdfs:label "Warrant Officer (Commonwealth of Nations)"@en , "Warrant Officer (Samväldet)"@sv , "Warrant Officer (Kansainyhteisö)"@fi , "Warrant Officer (Commonwealth of Nations)"@fr , "Warrant Officer (Commonwealth of Nations)"@de , "Warrant Officer (Commonwealth delle nazioni)"@it , "Warrant Officer (Gemenebest van Naties)"@nl , "Warrant Officer (Samveldet av nasjoner)"@no , "Warrant Officer (Wspólnota Narodów)"@pl , "Warrant Officer (Commonwealth)"@pt , "Warrant Officer (Содружество наций)"@ru , "Warrant Officer (Mancomunidad de Naciones)"@es ;
	rdfs:comment "The specific instance of the  rank in the context of country Commonwealth of Nations."@en ;
	owl:rankOf <dbpedia:Commonwealth_of_Nations> .

<http://rdf.muninn-project.org/ontologies/military#Rank_Captain_%28OF-2%29_Australia> a :MilitaryRank ;
	owl:subClass <http://rdf.muninn-project.org/ontologies/military#Rank_Captain_%28OF-2%29> ;
	foaf:name "Captain"@en ;
	rdfs:label "Captain (OF-2) (Australia)"@en , "Kapten (Australien)"@sv , "Kapteeni (sotilasarvo) (Australia)"@fi , "Capitaine (Australie)"@fr , "Hauptmann (Offizier) (Australien)"@de , "Capitano (Australia)"@it , "Kapitein (rang) (Australië (land))"@nl , "Kaptein (grad) (Australia)"@no , "Kapitan (ranga) (Australia)"@pl , "Capitão (militar) (Austrália)"@pt , "Капитан (воинское звание) (Австралия)"@ru , "Capitán (Australia)"@es ;
	rdfs:comment "The specific instance of the Captain (OF-2) rank in the context of country Australia."@en ;
	owl:rankOf <dbpedia:Australia> .

<http://rdf.muninn-project.org/ontologies/military#Rank_Captain_%28OF-2%29_Canada> a :MilitaryRank ;
	owl:subClass <http://rdf.muninn-project.org/ontologies/military#Rank_Captain_%28OF-2%29> ;
	foaf:name "Capitaine"@fr ;
	rdfs:label "Captain (OF-2, Canada)"@en , "Kapten (Canada)"@sv , "Kapteeni (sotilasarvo, Canada)"@fi , "Capitaine (Canada)"@fr , "Hauptmann (Offizier, Canada)"@de , "Capitano (Canada)"@it , "Kapitein (rang, Canada)"@nl , "Kaptein (grad, Canada)"@no , "Kapitan (ranga, Canada)"@pl , "Capitão (militar, Canada)"@pt , "Капитан (воинское звание, Canada)"@ru , "Capitán (Canada)"@es ;
	rdfs:comment "The specific instance of the Captain (OF-2) rank in the context of Canada."@en ;
	owl:rankOf <dbpedia:Canada> .

<http://rdf.muninn-project.org/ontologies/military#Rank_Captain_%28OF-2%29_Singapore> a :MilitaryRank ;
	owl:subClass <http://rdf.muninn-project.org/ontologies/military#Rank_Captain_%28OF-2%29> ;
	foaf:name "Captain"@en ;
	rdfs:label "Captain (OF-2) (Singapore)"@en , "Kapten (Singapore)"@sv , "Kapteeni (sotilasarvo) (Singapore)"@fi , "Capitaine (Singapour)"@fr , "Hauptmann (Offizier) (Singapur)"@de , "Capitano (Singapore)"@it , "Kapitein (rang) (Singapore)"@nl , "Kaptein (grad) (Singapore)"@no , "Kapitan (ranga) (Singapur)"@pl , "Capitão (militar) (Singapura)"@pt , "Капитан (воинское звание) (Сингапур)"@ru , "Capitán (Singapur)"@es ;
	rdfs:comment "The specific instance of the Captain (OF-2) rank in the context of country Singapore."@en ;
	owl:rankOf <dbpedia:Singapore> .

<http://rdf.muninn-project.org/ontologies/military#Rank_Captain_%28OF-2%29_Republic_of_Ireland> a :MilitaryRank ;
	owl:subClass <http://rdf.muninn-project.org/ontologies/military#Rank_Captain_%28OF-2%29> ;
	foaf:name "Captain"@en ;
	rdfs:label "Captain (OF-2) (Republic of Ireland)"@en , "Kapten (Irland)"@sv , "Kapteeni (sotilasarvo) (Irlanti)"@fi , "Capitaine (Irlande (pays))"@fr , "Hauptmann (Offizier) (Irland)"@de , "Capitano (Irlanda)"@it , "Kapitein (rang) (Ierland (land))"@nl , "Kaptein (grad) (Irland)"@no , "Kapitan (ranga) (Irlandia)"@pl , "Capitão (militar) (República da Irlanda)"@pt , "Капитан (воинское звание) (Ирландия)"@ru , "Capitán (Irlanda)"@es ;
	rdfs:comment "The specific instance of the Captain (OF-2) rank in the context of country Republic of Ireland."@en ;
	owl:rankOf <dbpedia:Republic_of_Ireland> .

<http://rdf.muninn-project.org/ontologies/military#Rank_Captain_%28OF-2%29_Sweden> a :MilitaryRank ;
	owl:subClass <http://rdf.muninn-project.org/ontologies/military#Rank_Captain_%28OF-2%29> ;
	foaf:name "Kapten"@sv ;
	rdfs:label "Captain (OF-2) (Sweden)"@en , "Kapten (Sverige)"@sv , "Kapteeni (sotilasarvo) (Ruotsi)"@fi , "Capitaine (Suède)"@fr , "Hauptmann (Offizier) (Schweden)"@de , "Capitano (Svezia)"@it , "Kapitein (rang) (Zweden)"@nl , "Kaptein (grad) (Sverige)"@no , "Kapitan (ranga) (Szwecja)"@pl , "Capitão (militar) (Suécia)"@pt , "Капитан (воинское звание) (Швеция)"@ru , "Capitán (Suecia)"@es ;
	rdfs:comment "The specific instance of the Captain (OF-2) rank in the context of country Sweden."@en ;
	owl:rankOf <dbpedia:Sweden> .

<http://rdf.muninn-project.org/ontologies/military#Rank_Captain_%28OF-2%29_Russia> a :MilitaryRank ;
	owl:subClass <http://rdf.muninn-project.org/ontologies/military#Rank_Captain_%28OF-2%29> ;
	foaf:name "Капитан"@ru ;
	rdfs:label "Captain (OF-2) (Russia)"@en , "Kapten (Ryssland)"@sv , "Kapteeni (sotilasarvo) (Venäjä)"@fi , "Capitaine (Russie)"@fr , "Hauptmann (Offizier) (Russland)"@de , "Capitano (Russia)"@it , "Kapitein (rang) (Rusland)"@nl , "Kaptein (grad) (Russland)"@no , "Kapitan (ranga) (Rosja)"@pl , "Capitão (militar) (Rússia)"@pt , "Капитан (воинское звание) (Россия)"@ru , "Capitán (Rusia)"@es ;
	rdfs:comment "The specific instance of the Captain (OF-2) rank in the context of country Russia."@en ;
	owl:rankOf <dbpedia:Russia> .

<http://rdf.muninn-project.org/ontologies/military#Rank_Captain_%28OF-2%29_Soviet_Union> a :MilitaryRank ;
	owl:subClass <http://rdf.muninn-project.org/ontologies/military#Rank_Captain_%28OF-2%29> ;
	foaf:name "Captain"@en ;
	rdfs:label "Captain (OF-2) (Soviet Union)"@en , "Kapten (Sovjetunionen)"@sv , "Kapteeni (sotilasarvo) (Neuvostoliitto)"@fi , "Capitaine (Union des républiques socialistes soviétiques)"@fr , "Hauptmann (Offizier) (Sowjetunion)"@de , "Capitano (Unione Sovietica)"@it , "Kapitein (rang) (Sovjet-Unie)"@nl , "Kaptein (grad) (Sovjetunionen)"@no , "Kapitan (ranga) (Związek Socjalistycznych Republik Radzieckich)"@pl , "Capitão (militar) (União Soviética)"@pt , "Капитан (воинское звание) (Союз Советских Социалистических Республик)"@ru , "Capitán (Unión Soviética)"@es ;
	rdfs:comment "The specific instance of the Captain (OF-2) rank in the context of country Soviet Union."@en ;
	owl:rankOf <dbpedia:Soviet_Union> .

:Rank_Company_sergeant_major_Australia a :MilitaryRank ;
	owl:subClass :Rank_Company_sergeant_major ;
	foaf:name "Company sergeant major"@en ;
	rdfs:label "Company sergeant major (Australia)"@en , "Company sergeant major (Australien)"@sv , "Company sergeant major (Australia)"@fi , "Company sergeant major (Australie)"@fr , "Company sergeant major (Australien)"@de , "Company sergeant major (Australia)"@it , "Company sergeant major (Australië (land))"@nl , "Company sergeant major (Australia)"@no , "Company sergeant major (Australia)"@pl , "Company sergeant major (Austrália)"@pt , "Company sergeant major (Австралия)"@ru , "Company sergeant major (Australia)"@es ;
	rdfs:comment "The specific instance of the Company sergeant major rank in the context of country Australia."@en ;
	owl:rankOf <dbpedia:Australia> .

:Rank_Company_sergeant_major_England a :MilitaryRank ;
	owl:subClass :Rank_Company_sergeant_major ;
	foaf:name "Company sergeant major"@en ;
	rdfs:label "Company sergeant major (England)"@en ;
	rdfs:comment "The specific instance of the Company sergeant major rank in the context of England."@en ;
	owl:rankOf <dbpedia:England> .

:Rank_Company_sergeant_major_Scotland a :MilitaryRank ;
	owl:subClass :Rank_Company_sergeant_major ;
	foaf:name "Company sergeant major"@en ;
	rdfs:label "Company sergeant major (Scotland)"@en , "Company sergeant major (Skottland)"@sv , "Company sergeant major (Skotlanti)"@fi , "Company sergeant major (Écosse)"@fr , "Company sergeant major (Schottland)"@de , "Company sergeant major (Scozia)"@it , "Company sergeant major (Schotland)"@nl , "Company sergeant major (Skottland)"@no , "Company sergeant major (Szkocja)"@pl , "Company sergeant major (Escócia)"@pt , "Company sergeant major (Шотландия)"@ru , "Company sergeant major (Escocia)"@es ;
	rdfs:comment "The specific instance of the Company sergeant major rank in the context of country Scotland."@en ;
	owl:rankOf <dbpedia:Scotland> .

:Rank_Company_sergeant_major_Wales a :MilitaryRank ;
	owl:subClass :Rank_Company_sergeant_major ;
	foaf:name "Company sergeant major"@en ;
	rdfs:label "Company sergeant major (Wales)"@en , "Company sergeant major (Wales)"@sv , "Company sergeant major (Wales)"@fi , "Company sergeant major (Pays de Galles)"@fr , "Company sergeant major (Wales)"@de , "Company sergeant major (Galles)"@it , "Company sergeant major (Wales)"@nl , "Company sergeant major (Wales)"@no , "Company sergeant major (Walia)"@pl , "Company sergeant major (País de Gales)"@pt , "Company sergeant major (Уэльс)"@ru , "Company sergeant major (Gales)"@es ;
	rdfs:comment "The specific instance of the Company sergeant major rank in the context of country Wales."@en ;
	owl:rankOf <dbpedia:Wales> .

:Rank_Company_sergeant_major_Canada a :MilitaryRank ;
	owl:subClass :Rank_Company_sergeant_major ;
	foaf:name "Company sergeant major"@en ;
	rdfs:label "Company sergeant major (Canada)"@en ;
	rdfs:comment "The specific instance of the Company sergeant major rank in the context of Canada."@en ;
	owl:rankOf <dbpedia:Canada> .

:Rank_Company_sergeant_major_Singapore a :MilitaryRank ;
	owl:subClass :Rank_Company_sergeant_major ;
	foaf:name "Company sergeant major"@en ;
	rdfs:label "Company sergeant major (Singapore)"@en , "Company sergeant major (Singapore)"@sv , "Company sergeant major (Singapore)"@fi , "Company sergeant major (Singapour)"@fr , "Company sergeant major (Singapur)"@de , "Company sergeant major (Singapore)"@it , "Company sergeant major (Singapore)"@nl , "Company sergeant major (Singapore)"@no , "Company sergeant major (Singapur)"@pl , "Company sergeant major (Singapura)"@pt , "Company sergeant major (Сингапур)"@ru , "Company sergeant major (Singapur)"@es ;
	rdfs:comment "The specific instance of the Company sergeant major rank in the context of country Singapore."@en ;
	owl:rankOf <dbpedia:Singapore> .

:Rank_Company_sergeant_major_Commonwealth_of_Nations a :MilitaryRank ;
	owl:subClass :Rank_Company_sergeant_major ;
	foaf:name "Company sergeant major"@en ;
	rdfs:label "Company sergeant major (Commonwealth of Nations)"@en , "Company sergeant major (Samväldet)"@sv , "Company sergeant major (Kansainyhteisö)"@fi , "Company sergeant major (Commonwealth of Nations)"@fr , "Company sergeant major (Commonwealth of Nations)"@de , "Company sergeant major (Commonwealth delle nazioni)"@it , "Company sergeant major (Gemenebest van Naties)"@nl , "Company sergeant major (Samveldet av nasjoner)"@no , "Company sergeant major (Wspólnota Narodów)"@pl , "Company sergeant major (Commonwealth)"@pt , "Company sergeant major (Содружество наций)"@ru , "Company sergeant major (Mancomunidad de Naciones)"@es ;
	rdfs:comment "The specific instance of the Company sergeant major rank in the context of country Commonwealth of Nations."@en ;
	owl:rankOf <dbpedia:Commonwealth_of_Nations> .

:Rank_Regimental_Quartermaster_Sergeant_Australia a :MilitaryRank ;
	owl:subClass :Rank_Regimental_Quartermaster_Sergeant ;
	foaf:name "Regimental Quartermaster Sergeant"@en ;
	rdfs:label "Regimental Quartermaster Sergeant (Australia)"@en , "Regimental Quartermaster Sergeant (Australien)"@sv , "Regimental Quartermaster Sergeant (Australia)"@fi , "Regimental Quartermaster Sergeant (Australie)"@fr , "Regimental Quartermaster Sergeant (Australien)"@de , "Regimental Quartermaster Sergeant (Australia)"@it , "Regimental Quartermaster Sergeant (Australië (land))"@nl , "Regimental Quartermaster Sergeant (Australia)"@no , "Regimental Quartermaster Sergeant (Australia)"@pl , "Regimental Quartermaster Sergeant (Austrália)"@pt , "Regimental Quartermaster Sergeant (Австралия)"@ru , "Regimental Quartermaster Sergeant (Australia)"@es ;
	rdfs:comment "The specific instance of the Regimental Quartermaster Sergeant rank in the context of country Australia."@en ;
	owl:rankOf <dbpedia:Australia> .

:Rank_Regimental_Quartermaster_Sergeant_England a :MilitaryRank ;
	owl:subClass :Rank_Regimental_Quartermaster_Sergeant ;
	foaf:name "Regimental Quartermaster Sergeant"@en ;
	rdfs:label "Regimental Quartermaster Sergeant (England)"@en ;
	rdfs:comment "The specific instance of the Regimental Quartermaster Sergeant rank in the context of England."@en ;
	owl:rankOf <dbpedia:England> .

:Rank_Regimental_Quartermaster_Sergeant_Scotland a :MilitaryRank ;
	owl:subClass :Rank_Regimental_Quartermaster_Sergeant ;
	foaf:name "Regimental Quartermaster Sergeant"@en ;
	rdfs:label "Regimental Quartermaster Sergeant (Scotland)"@en , "Regimental Quartermaster Sergeant (Skottland)"@sv , "Regimental Quartermaster Sergeant (Skotlanti)"@fi , "Regimental Quartermaster Sergeant (Écosse)"@fr , "Regimental Quartermaster Sergeant (Schottland)"@de , "Regimental Quartermaster Sergeant (Scozia)"@it , "Regimental Quartermaster Sergeant (Schotland)"@nl , "Regimental Quartermaster Sergeant (Skottland)"@no , "Regimental Quartermaster Sergeant (Szkocja)"@pl , "Regimental Quartermaster Sergeant (Escócia)"@pt , "Regimental Quartermaster Sergeant (Шотландия)"@ru , "Regimental Quartermaster Sergeant (Escocia)"@es ;
	rdfs:comment "The specific instance of the Regimental Quartermaster Sergeant rank in the context of country Scotland."@en ;
	owl:rankOf <dbpedia:Scotland> .

:Rank_Regimental_Quartermaster_Sergeant_Wales a :MilitaryRank ;
	owl:subClass :Rank_Regimental_Quartermaster_Sergeant ;
	foaf:name "Regimental Quartermaster Sergeant"@en ;
	rdfs:label "Regimental Quartermaster Sergeant (Wales)"@en , "Regimental Quartermaster Sergeant (Wales)"@sv , "Regimental Quartermaster Sergeant (Wales)"@fi , "Regimental Quartermaster Sergeant (Pays de Galles)"@fr , "Regimental Quartermaster Sergeant (Wales)"@de , "Regimental Quartermaster Sergeant (Galles)"@it , "Regimental Quartermaster Sergeant (Wales)"@nl , "Regimental Quartermaster Sergeant (Wales)"@no , "Regimental Quartermaster Sergeant (Walia)"@pl , "Regimental Quartermaster Sergeant (País de Gales)"@pt , "Regimental Quartermaster Sergeant (Уэльс)"@ru , "Regimental Quartermaster Sergeant (Gales)"@es ;
	rdfs:comment "The specific instance of the Regimental Quartermaster Sergeant rank in the context of country Wales."@en ;
	owl:rankOf <dbpedia:Wales> .

:Rank_Regimental_Quartermaster_Sergeant_Canada a :MilitaryRank ;
	owl:subClass :Rank_Regimental_Quartermaster_Sergeant ;
	foaf:name "Regimental Quartermaster Sergeant"@en ;
	rdfs:label "Regimental Quartermaster Sergeant (Canada)"@en ;
	rdfs:comment "The specific instance of the Regimental Quartermaster Sergeant rank in the context of Canada."@en ;
	owl:rankOf <dbpedia:Canada> .

:Rank_Regimental_Quartermaster_Sergeant_Commonwealth_of_Nations a :MilitaryRank ;
	owl:subClass :Rank_Regimental_Quartermaster_Sergeant ;
	foaf:name "Regimental Quartermaster Sergeant"@en ;
	rdfs:label "Regimental Quartermaster Sergeant (Commonwealth of Nations)"@en , "Regimental Quartermaster Sergeant (Samväldet)"@sv , "Regimental Quartermaster Sergeant (Kansainyhteisö)"@fi , "Regimental Quartermaster Sergeant (Commonwealth of Nations)"@fr , "Regimental Quartermaster Sergeant (Commonwealth of Nations)"@de , "Regimental Quartermaster Sergeant (Commonwealth delle nazioni)"@it , "Regimental Quartermaster Sergeant (Gemenebest van Naties)"@nl , "Regimental Quartermaster Sergeant (Samveldet av nasjoner)"@no , "Regimental Quartermaster Sergeant (Wspólnota Narodów)"@pl , "Regimental Quartermaster Sergeant (Commonwealth)"@pt , "Regimental Quartermaster Sergeant (Содружество наций)"@ru , "Regimental Quartermaster Sergeant (Mancomunidad de Naciones)"@es ;
	rdfs:comment "The specific instance of the Regimental Quartermaster Sergeant rank in the context of country Commonwealth of Nations."@en ;
	owl:rankOf <dbpedia:Commonwealth_of_Nations> .

:Rank_Regimental_Quartermaster_Sergeant_Republic_of_Ireland a :MilitaryRank ;
	owl:subClass :Rank_Regimental_Quartermaster_Sergeant ;
	foaf:name "Regimental Quartermaster Sergeant"@en ;
	rdfs:label "Regimental Quartermaster Sergeant (Republic of Ireland)"@en , "Regimental Quartermaster Sergeant (Irland)"@sv , "Regimental Quartermaster Sergeant (Irlanti)"@fi , "Regimental Quartermaster Sergeant (Irlande (pays))"@fr , "Regimental Quartermaster Sergeant (Irland)"@de , "Regimental Quartermaster Sergeant (Irlanda)"@it , "Regimental Quartermaster Sergeant (Ierland (land))"@nl , "Regimental Quartermaster Sergeant (Irland)"@no , "Regimental Quartermaster Sergeant (Irlandia)"@pl , "Regimental Quartermaster Sergeant (República da Irlanda)"@pt , "Regimental Quartermaster Sergeant (Ирландия)"@ru , "Regimental Quartermaster Sergeant (Irlanda)"@es ;
	rdfs:comment "The specific instance of the Regimental Quartermaster Sergeant rank in the context of country Republic of Ireland."@en ;
	owl:rankOf <dbpedia:Republic_of_Ireland> .

:Rank_Oberst_Germany rdfs:comment "The specific instance of the Oberst rank in the context of country Germany."@en .

:Rank_Oberstleutnant_Germany rdfs:comment "The specific instance of the Oberstleutnant rank in the context of country Germany."@en .
