@prefix rdfs: <http://www.w3.org/2000/01/rdf-schema#> .
@prefix foaf: <http://xmlns.com/foaf/0.1/> .
@prefix opdm: <http://purl.org/opdm/utility#> .
@prefix owl: <http://www.w3.org/2002/07/owl#> .
@prefix rdf: <http://www.w3.org/1999/02/22-rdf-syntax-ns#> .
@prefix gr: <http://purl.org/goodrelations/v1#> .
@prefix skos: <http://www.w3.org/2004/02/skos/core#> .
@prefix dcterms: <http://purl.org/dc/terms/> .

<http://purl.org/opdm/refrigerator#FridgeFreezer> rdfs:label "Frigorífico/Congelador"@es ;
	opdm:category <http://purl.org/opdm/category/google#Home_and_Garden_Kitchen_and_Dining_KitchenAppliances_Refrigerators> , <http://purl.org/opdm/category/google#Home_and_Garden_Kitchen_and_Dining_KitchenAppliances_Freezers> ;
	a owl:Class ;
	foaf:depiction <http://upload.wikimedia.org/wikipedia/commons/2/21/2011-05-09_14-56-45_407.jpg> ;
	skos:altLabel "Refrigerator/Freezer"@en ;
	rdfs:comment "A generic Fridge/Freezer as a product type"@en ;
	skos:altLabel "Heladera/Congelador"@es , "Refrigerador/Congelador"@es ;
	rdfs:label "Kühlschrank"@de ;
	skos:altLabel "Nevera/Congelador"@es ;
	rdfs:isDefinedBy <http://purl.org/opdm/refrigerator#> ;
	rdfs:label "FridgeFreezer"@en ;
	rdfs:subClassOf gr:ProductOrService .

_:node18vkiok0kx1 opdm:exampleOfUsage "The value of this property is an individual of the gr:QuantitativeValue class."^^<http://www.w3.org/2001/XMLSchema#string> ;
	opdm:inProfile opdm:DefaultProfile ;
	opdm:priority "0"^^<http://www.w3.org/2001/XMLSchema#integer> ;
	opdm:attributePosition "0"^^<http://www.w3.org/2001/XMLSchema#integer> ;
	a opdm:MetadataContainer ;
	opdm:rankingDirection "DESC"^^<http://www.w3.org/2001/XMLSchema#string> .

<http://purl.org/opdm/refrigerator#Right> rdfs:label "Right"@en ;
	rdfs:isDefinedBy <http://purl.org/opdm/refrigerator#> ;
	a <http://purl.org/opdm/refrigerator#RelativeDirection> ;
	rdfs:comment "It represents the relative direction: right."@en .

<http://purl.org/opdm/refrigerator#numberOfFrontDrawers> opdm:isConfiguredBy _:node18vkiok0kx2 ;
	rdfs:isDefinedBy <http://purl.org/opdm/refrigerator#> ;
	opdm:minCardinality "0"^^<http://www.w3.org/2001/XMLSchema#string> ;
	rdfs:label "Number of front drawers"@en ;
	opdm:maxCardinality "1"^^<http://www.w3.org/2001/XMLSchema#string> ;
	rdfs:comment "This property specifies the number of front drawers that the fridge is equipped with."@en ;
	rdfs:domain <http://purl.org/opdm/refrigerator#FridgeFreezer> ;
	rdfs:range <http://www.w3.org/2001/XMLSchema#integer> ;
	a owl:DatatypeProperty ;
	opdm:recommendedRangeOfMeasure _:node18vkiok0kx3 ;
	rdfs:subPropertyOf gr:datatypeProductOrServiceProperty .

_:node18vkiok0kx4 opdm:inProfile opdm:DefaultProfile ;
	opdm:attributePosition "0"^^<http://www.w3.org/2001/XMLSchema#integer> ;
	opdm:exampleOfUsage "The value of this property is an individual of the gr:QuantitativeValue class."^^<http://www.w3.org/2001/XMLSchema#string> ;
	opdm:priority "0"^^<http://www.w3.org/2001/XMLSchema#integer> ;
	opdm:rankingDirection "DESC"^^<http://www.w3.org/2001/XMLSchema#string> ;
	a opdm:MetadataContainer .

_:node18vkiok0kx5 gr:hasMinValue "0"^^<http://www.w3.org/2001/XMLSchema#integer> ;
	a gr:QuantitativeValue ;
	gr:hasMaxValue "0"^^<http://www.w3.org/2001/XMLSchema#integer> .

<http://purl.org/opdm/refrigerator#ratingOfStars> rdfs:domain <http://purl.org/opdm/refrigerator#FridgeFreezer> ;
	rdfs:comment "This property specifies the maximum temperature that the freezer unit can reach. The temperature is indicated using a number of stars. Each star corresponds to a -6 degree celsius increment."@en ;
	opdm:minCardinality "0"^^<http://www.w3.org/2001/XMLSchema#string> ;
	rdfs:isDefinedBy <http://purl.org/opdm/refrigerator#> ;
	opdm:maxCardinality "1"^^<http://www.w3.org/2001/XMLSchema#string> ;
	rdfs:range <http://www.w3.org/2001/XMLSchema#integer> ;
	rdfs:label "Rating of stars"@en ;
	opdm:isConfiguredBy _:node18vkiok0kx6 ;
	a owl:DatatypeProperty ;
	opdm:recommendedRangeOfMeasure _:node18vkiok0kx7 ;
	rdfs:subPropertyOf gr:datatypeProductOrServiceProperty .

<http://purl.org/opdm/refrigerator#Left> rdfs:isDefinedBy <http://purl.org/opdm/refrigerator#> ;
	rdfs:comment "It represents the relative direction: left."@en ;
	rdfs:label "Left"@en ;
	a <http://purl.org/opdm/refrigerator#RelativeDirection> .

_:node18vkiok0kx8 opdm:rankingDirection "DESC"^^<http://www.w3.org/2001/XMLSchema#string> ;
	opdm:attributePosition "0"^^<http://www.w3.org/2001/XMLSchema#integer> ;
	opdm:priority "0"^^<http://www.w3.org/2001/XMLSchema#integer> ;
	opdm:exampleOfUsage "The value of this property is a boolean (true/false - xsd:boolean)."^^<http://www.w3.org/2001/XMLSchema#string> ;
	a opdm:MetadataContainer ;
	opdm:inProfile opdm:DefaultProfile .

<http://purl.org/opdm/refrigerator#EnergyF> a <http://purl.org/opdm/refrigerator#EnergyRatingEU> ;
	rdfs:label "F Rating"@en ;
	rdfs:isDefinedBy <http://purl.org/opdm/refrigerator#> ;
	rdfs:comment "This concept represents the F energy efficiency rating in the European Union labelling scheme"@en .

_:node18vkiok0kx9 a gr:QuantitativeValue ;
	gr:hasMaxValue "0"^^<http://www.w3.org/2001/XMLSchema#integer> ;
	gr:hasMinValue "0"^^<http://www.w3.org/2001/XMLSchema#integer> .

<http://purl.org/opdm/refrigerator#ratingOfEnergyEU> rdfs:range <http://purl.org/opdm/refrigerator#EnergyRatingEU> ;
	opdm:maxCardinality "1"^^<http://www.w3.org/2001/XMLSchema#string> ;
	a owl:ObjectProperty ;
	rdfs:isDefinedBy <http://purl.org/opdm/refrigerator#> ;
	rdfs:domain <http://purl.org/opdm/refrigerator#FridgeFreezer> ;
	rdfs:subPropertyOf gr:qualitativeProductOrServiceProperty ;
	opdm:isConfiguredBy _:node18vkiok0kx10 ;
	rdfs:comment "The rating of energy efficiency in the European Union that the fridge/freezer operates at."@en ;
	rdfs:label "Rating of energy EU"@en ;
	opdm:minCardinality "0"^^<http://www.w3.org/2001/XMLSchema#string> .

<http://purl.org/opdm/refrigerator#volumeOfUnitGross> opdm:isConfiguredBy _:node18vkiok0kx1 ;
	opdm:recommendedRangeOfMeasure _:node18vkiok0kx9 ;
	rdfs:comment "The gross volume in liters of the total unit."@en ;
	opdm:minCardinality "0"^^<http://www.w3.org/2001/XMLSchema#string> ;
	opdm:maxCardinality "1"^^<http://www.w3.org/2001/XMLSchema#string> ;
	a owl:ObjectProperty ;
	rdfs:isDefinedBy <http://purl.org/opdm/refrigerator#> ;
	rdfs:range gr:QuantitativeValue ;
	opdm:recommendedUnitOfMeasure "LTR"^^<http://www.w3.org/2001/XMLSchema#string> ;
	rdfs:domain <http://purl.org/opdm/refrigerator#FridgeFreezer> ;
	rdfs:label "Volume of unit gross"@en ;
	rdfs:subPropertyOf gr:quantitativeProductOrServiceProperty .

_:node18vkiok0kx11 opdm:priority "0"^^<http://www.w3.org/2001/XMLSchema#integer> ;
	opdm:rankingDirection "DESC"^^<http://www.w3.org/2001/XMLSchema#string> ;
	a opdm:MetadataContainer ;
	opdm:attributePosition "0"^^<http://www.w3.org/2001/XMLSchema#integer> ;
	opdm:inProfile opdm:DefaultProfile ;
	opdm:exampleOfUsage "The value of this property is an individual of the ofrd:StyleOfUnit class."^^<http://www.w3.org/2001/XMLSchema#string> .

<http://purl.org/opdm/refrigerator#EnergyA3> a <http://purl.org/opdm/refrigerator#EnergyRatingEU> ;
	rdfs:isDefinedBy <http://purl.org/opdm/refrigerator#> ;
	rdfs:comment "This concept represents the A+++ energy efficiency rating in the European Union labelling scheme"@en ;
	rdfs:label "A+++ Rating"@en .

<http://purl.org/opdm/refrigerator#> dcterms:creator "Laszlo Torok" , <http://opdm-project.org/> ;
	rdfs:label "Fridge and Freezer Vocabulary"@en ;
	owl:imports <http://purl.org/goodrelations/v1> ;
	rdfs:comment "Vocabulary to describe fridges and freezers"@en ;
	dcterms:contributor <http://www.wikipedia.org> ;
	dcterms:creator <http://www.unibw.de/ebusiness/> , "Bene Rodriguez-Castro" ;
	dcterms:contributor <http://www.consumer.es/web/es/economia_domestica/servicios-y-hogar/2005/11/04/146650.php> ;
	owl:imports <http://purl.org/opdm/utility#> ;
	a owl:Ontology ;
	dcterms:subject "refrigerator fridge freezer"@en ;
	dcterms:creator "Martin Hepp" .

<http://purl.org/opdm/refrigerator#SingleDoor> rdfs:isDefinedBy <http://purl.org/opdm/refrigerator#> ;
	a <http://purl.org/opdm/refrigerator#StyleOfUnit> ;
	rdfs:comment "It represents a freezer-less door type of fridge."@en ;
	rdfs:label "FreezerlessDoor"@en .

<http://purl.org/opdm/refrigerator#BuiltIn> rdfs:isDefinedBy <http://purl.org/opdm/refrigerator#> ;
	a <http://purl.org/opdm/refrigerator#TypeOfBody> ;
	rdfs:label "BuiltIn"@en ;
	rdfs:comment "It represents a bult-in type of body frame for a fridge/freezer."@en .

_:node18vkiok0kx12 opdm:inProfile opdm:DefaultProfile ;
	opdm:rankingDirection "DESC"^^<http://www.w3.org/2001/XMLSchema#string> ;
	a opdm:MetadataContainer ;
	opdm:priority "0"^^<http://www.w3.org/2001/XMLSchema#integer> ;
	opdm:exampleOfUsage "The value of this property is a boolean (true/false - xsd:boolean)."^^<http://www.w3.org/2001/XMLSchema#string> ;
	opdm:attributePosition "0"^^<http://www.w3.org/2001/XMLSchema#integer> .

<http://purl.org/opdm/refrigerator#EnergyA1> rdfs:comment "This concept represents the A+ energy efficiency rating in the European Union labelling scheme"@en ;
	a <http://purl.org/opdm/refrigerator#EnergyRatingEU> ;
	rdfs:isDefinedBy <http://purl.org/opdm/refrigerator#> ;
	rdfs:label "A+ Rating"@en .

_:node18vkiok0kx13 opdm:attributePosition "0"^^<http://www.w3.org/2001/XMLSchema#integer> ;
	a opdm:MetadataContainer ;
	opdm:rankingDirection "DESC"^^<http://www.w3.org/2001/XMLSchema#string> ;
	opdm:inProfile opdm:DefaultProfile ;
	opdm:priority "0"^^<http://www.w3.org/2001/XMLSchema#integer> ;
	opdm:exampleOfUsage "The value of this property is a boolean (true/false - xsd:boolean)."^^<http://www.w3.org/2001/XMLSchema#string> .

foaf:depiction a owl:AnnotationProperty .

<http://purl.org/opdm/refrigerator#ClimateST> rdfs:isDefinedBy <http://purl.org/opdm/refrigerator#> ;
	rdfs:label "ST Rating"@en ;
	rdfs:comment "This concept represents the ST climate class rating. The fridge/freezer can operate between 18 - 38 degree celsius of room temperature"@en ;
	a <http://purl.org/opdm/refrigerator#ClimateClass> .

<http://purl.org/opdm/refrigerator#EnergyC> rdfs:comment "This concept represents the C energy efficiency rating in the European Union labelling scheme"@en ;
	rdfs:isDefinedBy <http://purl.org/opdm/refrigerator#> ;
	rdfs:label "C Rating"@en ;
	a <http://purl.org/opdm/refrigerator#EnergyRatingEU> .

<http://purl.org/opdm/refrigerator#display> rdfs:subPropertyOf gr:datatypeProductOrServiceProperty ;
	opdm:isConfiguredBy _:node18vkiok0kx12 ;
	a owl:DatatypeProperty ;
	opdm:minCardinality "0"^^<http://www.w3.org/2001/XMLSchema#string> ;
	rdfs:label "Display"@en ;
	rdfs:domain <http://purl.org/opdm/refrigerator#FridgeFreezer> ;
	rdfs:comment "This property specifies whether the fridge/freezer is equipped with an electronic display system or not."@en ;
	rdfs:isDefinedBy <http://purl.org/opdm/refrigerator#> ;
	rdfs:range <http://www.w3.org/2001/XMLSchema#boolean> ;
	opdm:maxCardinality "1"^^<http://www.w3.org/2001/XMLSchema#string> .

_:node18vkiok0kx14 opdm:priority "0"^^<http://www.w3.org/2001/XMLSchema#integer> ;
	opdm:inProfile opdm:DefaultProfile ;
	opdm:rankingDirection "DESC"^^<http://www.w3.org/2001/XMLSchema#string> ;
	a opdm:MetadataContainer ;
	opdm:exampleOfUsage "The value of this property is an individual of the gr:QuantitativeValue class."^^<http://www.w3.org/2001/XMLSchema#string> ;
	opdm:attributePosition "0"^^<http://www.w3.org/2001/XMLSchema#integer> .

<http://purl.org/opdm/refrigerator#powerSupply> opdm:minCardinality "0"^^<http://www.w3.org/2001/XMLSchema#string> ;
	rdfs:isDefinedBy <http://purl.org/opdm/refrigerator#> ;
	rdfs:range gr:QuantitativeValue ;
	a owl:ObjectProperty ;
	rdfs:comment "The power supply requirements in volts of the fridge/freezer unit (UN/CEFACT common code: VLT). Optionally, this property can be complemented with a gr:valueReference property to indicate the frecuency that the power supply operates at in Hertz (UN/CEFACT common code: HTZ)."@en ;
	rdfs:label "Power supply"@en ;
	opdm:recommendedUnitOfMeasure "VLT"^^<http://www.w3.org/2001/XMLSchema#string> ;
	rdfs:domain <http://purl.org/opdm/refrigerator#FridgeFreezer> ;
	opdm:isConfiguredBy _:node18vkiok0kx14 ;
	opdm:recommendedRangeOfMeasure _:node18vkiok0kx15 ;
	rdfs:subPropertyOf gr:quantitativeProductOrServiceProperty ;
	opdm:maxCardinality "1"^^<http://www.w3.org/2001/XMLSchema#string> .

<http://purl.org/opdm/refrigerator#typeOfBody> rdfs:range <http://purl.org/opdm/refrigerator#TypeOfBody> ;
	rdfs:subPropertyOf gr:qualitativeProductOrServiceProperty ;
	rdfs:isDefinedBy <http://purl.org/opdm/refrigerator#> ;
	opdm:minCardinality "0"^^<http://www.w3.org/2001/XMLSchema#string> ;
	opdm:maxCardinality "1"^^<http://www.w3.org/2001/XMLSchema#string> ;
	rdfs:comment "The type of body frame that the fridge/freezer is equipped with."@en ;
	opdm:isConfiguredBy _:node18vkiok0kx16 ;
	rdfs:domain <http://purl.org/opdm/refrigerator#FridgeFreezer> ;
	a owl:ObjectProperty ;
	rdfs:label "Type of body"@en .

<http://purl.org/opdm/refrigerator#ClimateT> a <http://purl.org/opdm/refrigerator#ClimateClass> ;
	rdfs:isDefinedBy <http://purl.org/opdm/refrigerator#> ;
	rdfs:comment "This concept represents the T climate class rating. The fridge/freezer can operate between 18 - 43 degree celsius of room temperature"@en ;
	rdfs:label "T Rating"@en .

_:node18vkiok0kx17 opdm:rankingDirection "DESC"^^<http://www.w3.org/2001/XMLSchema#string> ;
	opdm:attributePosition "0"^^<http://www.w3.org/2001/XMLSchema#integer> ;
	opdm:priority "0"^^<http://www.w3.org/2001/XMLSchema#integer> ;
	opdm:exampleOfUsage "The value of this property is a boolean (true/false - xsd:boolean)."^^<http://www.w3.org/2001/XMLSchema#string> ;
	a opdm:MetadataContainer ;
	opdm:inProfile opdm:DefaultProfile .

<http://purl.org/opdm/refrigerator#positionOfDoorHinge> rdfs:range <http://purl.org/opdm/refrigerator#RelativeDirection> ;
	rdfs:isDefinedBy <http://purl.org/opdm/refrigerator#> ;
	opdm:maxCardinality "1"^^<http://www.w3.org/2001/XMLSchema#string> ;
	rdfs:comment "The position of the door hinge of the fridge/freezer unit."@en ;
	rdfs:subPropertyOf gr:qualitativeProductOrServiceProperty ;
	a owl:ObjectProperty ;
	rdfs:label "Position of door hinge"@en ;
	opdm:minCardinality "0"^^<http://www.w3.org/2001/XMLSchema#string> ;
	opdm:isConfiguredBy _:node18vkiok0kx18 ;
	rdfs:domain <http://purl.org/opdm/refrigerator#FridgeFreezer> .

_:node18vkiok0kx2 opdm:rankingDirection "DESC"^^<http://www.w3.org/2001/XMLSchema#string> ;
	opdm:exampleOfUsage "The value of this property is an integer (xsd:integer)."^^<http://www.w3.org/2001/XMLSchema#string> ;
	opdm:priority "0"^^<http://www.w3.org/2001/XMLSchema#integer> ;
	a opdm:MetadataContainer ;
	opdm:attributePosition "0"^^<http://www.w3.org/2001/XMLSchema#integer> ;
	opdm:inProfile opdm:DefaultProfile .

_:node18vkiok0kx10 a opdm:MetadataContainer ;
	opdm:attributePosition "0"^^<http://www.w3.org/2001/XMLSchema#integer> ;
	opdm:rankingDirection "DESC"^^<http://www.w3.org/2001/XMLSchema#string> ;
	opdm:exampleOfUsage "The value of this property is an individual of the ofrd:EnergyRatingEU class."^^<http://www.w3.org/2001/XMLSchema#string> ;
	opdm:inProfile opdm:DefaultProfile ;
	opdm:priority "0"^^<http://www.w3.org/2001/XMLSchema#integer> .

_:node18vkiok0kx19 opdm:priority "0"^^<http://www.w3.org/2001/XMLSchema#integer> ;
	opdm:inProfile opdm:DefaultProfile ;
	opdm:rankingDirection "DESC"^^<http://www.w3.org/2001/XMLSchema#string> ;
	a opdm:MetadataContainer ;
	opdm:exampleOfUsage "The value of this property is an individual of the ofrd:ClimateClass class."^^<http://www.w3.org/2001/XMLSchema#string> ;
	opdm:attributePosition "0"^^<http://www.w3.org/2001/XMLSchema#integer> .

dcterms:creator a owl:AnnotationProperty .

<http://purl.org/opdm/refrigerator#Chest> rdfs:isDefinedBy <http://purl.org/opdm/refrigerator#> ;
	rdfs:comment "It represents a chest type of body frame for a fridge/freezer."@en ;
	a <http://purl.org/opdm/refrigerator#TypeOfBody> ;
	rdfs:label "Chest"@en .

_:node18vkiok0kx20 opdm:inProfile opdm:DefaultProfile ;
	a opdm:MetadataContainer ;
	opdm:priority "0"^^<http://www.w3.org/2001/XMLSchema#integer> ;
	opdm:rankingDirection "DESC"^^<http://www.w3.org/2001/XMLSchema#string> ;
	opdm:attributePosition "0"^^<http://www.w3.org/2001/XMLSchema#integer> ;
	opdm:exampleOfUsage "The value of this property is an integer (xsd:integer)."^^<http://www.w3.org/2001/XMLSchema#string> .

_:node18vkiok0kx3 a gr:QuantitativeValue ;
	gr:hasMaxValue "3"^^<http://www.w3.org/2001/XMLSchema#integer> ;
	gr:hasMinValue "0"^^<http://www.w3.org/2001/XMLSchema#integer> .

<http://purl.org/opdm/refrigerator#iceDispenser> rdfs:domain <http://purl.org/opdm/refrigerator#FridgeFreezer> ;
	rdfs:label "Ice dispenser"@en ;
	a owl:DatatypeProperty ;
	opdm:isConfiguredBy _:node18vkiok0kx21 ;
	rdfs:comment "This property specifies whether the fridge/freezer is equipped with an ice dispenser system or not."@en ;
	opdm:maxCardinality "1"^^<http://www.w3.org/2001/XMLSchema#string> ;
	rdfs:isDefinedBy <http://purl.org/opdm/refrigerator#> ;
	rdfs:range <http://www.w3.org/2001/XMLSchema#boolean> ;
	opdm:minCardinality "0"^^<http://www.w3.org/2001/XMLSchema#string> ;
	rdfs:subPropertyOf gr:datatypeProductOrServiceProperty .

_:node18vkiok0kx22 a opdm:MetadataContainer ;
	opdm:exampleOfUsage "The value of this property is an individual of the gr:QuantitativeValue class."^^<http://www.w3.org/2001/XMLSchema#string> ;
	opdm:rankingDirection "DESC"^^<http://www.w3.org/2001/XMLSchema#string> ;
	opdm:attributePosition "0"^^<http://www.w3.org/2001/XMLSchema#integer> ;
	opdm:inProfile opdm:DefaultProfile ;
	opdm:priority "0"^^<http://www.w3.org/2001/XMLSchema#integer> .

<http://purl.org/opdm/refrigerator#styleOfUnit> rdfs:subPropertyOf gr:qualitativeProductOrServiceProperty ;
	rdfs:label "Style of unit"@en ;
	opdm:isConfiguredBy _:node18vkiok0kx11 ;
	opdm:maxCardinality "1"^^<http://www.w3.org/2001/XMLSchema#string> ;
	rdfs:range <http://purl.org/opdm/refrigerator#StyleOfUnit> ;
	rdfs:comment "The type of door that the fridge/freezer is equipped with."@en ;
	rdfs:isDefinedBy <http://purl.org/opdm/refrigerator#> ;
	a owl:ObjectProperty ;
	opdm:minCardinality "0"^^<http://www.w3.org/2001/XMLSchema#string> ;
	rdfs:domain <http://purl.org/opdm/refrigerator#FridgeFreezer> .

_:node18vkiok0kx23 a gr:QuantitativeValue ;
	gr:hasMinValue "1"^^<http://www.w3.org/2001/XMLSchema#integer> ;
	gr:hasMaxValue "4"^^<http://www.w3.org/2001/XMLSchema#integer> .

_:node18vkiok0kx24 opdm:exampleOfUsage "The value of this property is an individual of the gr:QuantitativeValue class."^^<http://www.w3.org/2001/XMLSchema#string> ;
	opdm:attributePosition "0"^^<http://www.w3.org/2001/XMLSchema#integer> ;
	opdm:priority "0"^^<http://www.w3.org/2001/XMLSchema#integer> ;
	opdm:inProfile opdm:DefaultProfile ;
	a opdm:MetadataContainer ;
	opdm:rankingDirection "DESC"^^<http://www.w3.org/2001/XMLSchema#string> .

<http://purl.org/opdm/refrigerator#waterDispenser> rdfs:label "Water dispenser"@en ;
	a owl:DatatypeProperty ;
	opdm:isConfiguredBy _:node18vkiok0kx8 ;
	rdfs:subPropertyOf gr:datatypeProductOrServiceProperty ;
	rdfs:domain <http://purl.org/opdm/refrigerator#FridgeFreezer> ;
	rdfs:range <http://www.w3.org/2001/XMLSchema#boolean> ;
	opdm:minCardinality "0"^^<http://www.w3.org/2001/XMLSchema#string> ;
	rdfs:isDefinedBy <http://purl.org/opdm/refrigerator#> ;
	rdfs:comment "This property specifies whether the fridge/freezer is equipped with a water dispenser system or not."@en ;
	opdm:maxCardinality "1"^^<http://www.w3.org/2001/XMLSchema#string> .

<http://purl.org/opdm/refrigerator#FrenchDoor> rdfs:label "FrenchDoor"@en ;
	rdfs:isDefinedBy <http://purl.org/opdm/refrigerator#> ;
	a <http://purl.org/opdm/refrigerator#StyleOfUnit> ;
	rdfs:comment "It represents a french-door type of fridge."@en .

<http://purl.org/opdm/refrigerator#remoteControl> rdfs:isDefinedBy <http://purl.org/opdm/refrigerator#> ;
	rdfs:range <http://www.w3.org/2001/XMLSchema#boolean> ;
	opdm:minCardinality "0"^^<http://www.w3.org/2001/XMLSchema#string> ;
	rdfs:label "Remote control"@en ;
	opdm:maxCardinality "1"^^<http://www.w3.org/2001/XMLSchema#string> ;
	a owl:DatatypeProperty ;
	rdfs:domain <http://purl.org/opdm/refrigerator#FridgeFreezer> ;
	opdm:isConfiguredBy _:node18vkiok0kx25 ;
	rdfs:subPropertyOf gr:datatypeProductOrServiceProperty ;
	rdfs:comment "This property specifies whether the fridge/freezer can be controlled remotely via an external electronic device (smartphone, computer, etc.) system or not."@en .

_:node18vkiok0kx6 opdm:priority "0"^^<http://www.w3.org/2001/XMLSchema#integer> ;
	opdm:rankingDirection "DESC"^^<http://www.w3.org/2001/XMLSchema#string> ;
	a opdm:MetadataContainer ;
	opdm:exampleOfUsage "The value of this property is an integer (xsd:integer)."^^<http://www.w3.org/2001/XMLSchema#string> ;
	opdm:attributePosition "0"^^<http://www.w3.org/2001/XMLSchema#integer> ;
	opdm:inProfile opdm:DefaultProfile .

<http://purl.org/opdm/refrigerator#Freezer> rdfs:subClassOf <http://purl.org/opdm/refrigerator#FridgeFreezer> ;
	opdm:category <http://purl.org/opdm/category/google#Home_and_Garden_Kitchen_and_Dining_KitchenAppliances_Freezers> ;
	a owl:Class ;
	rdfs:isDefinedBy <http://purl.org/opdm/refrigerator#> ;
	foaf:depiction <http://upload.wikimedia.org/wikipedia/commons/2/21/2011-05-09_14-56-45_407.jpg> ;
	rdfs:comment "A generic dedicated Freezer (with no Fridge unit) as a product type"@en ;
	rdfs:label "Freezer"@en , "Congelador"@es .

_:node18vkiok0kx26 gr:hasMaxValue "0"^^<http://www.w3.org/2001/XMLSchema#integer> ;
	a gr:QuantitativeValue ;
	gr:hasMinValue "0"^^<http://www.w3.org/2001/XMLSchema#integer> .

_:node18vkiok0kx27 opdm:attributePosition "0"^^<http://www.w3.org/2001/XMLSchema#integer> ;
	opdm:exampleOfUsage "The value of this property is an integer (xsd:integer)."^^<http://www.w3.org/2001/XMLSchema#string> ;
	opdm:inProfile opdm:DefaultProfile ;
	opdm:rankingDirection "DESC"^^<http://www.w3.org/2001/XMLSchema#string> ;
	opdm:priority "0"^^<http://www.w3.org/2001/XMLSchema#integer> ;
	a opdm:MetadataContainer .

_:node18vkiok0kx28 opdm:exampleOfUsage "The value of this property is a boolean (true/false - xsd:boolean)."^^<http://www.w3.org/2001/XMLSchema#string> ;
	a opdm:MetadataContainer ;
	opdm:inProfile opdm:DefaultProfile ;
	opdm:rankingDirection "DESC"^^<http://www.w3.org/2001/XMLSchema#string> ;
	opdm:attributePosition "0"^^<http://www.w3.org/2001/XMLSchema#integer> ;
	opdm:priority "0"^^<http://www.w3.org/2001/XMLSchema#integer> .

_:node18vkiok0kx29 opdm:rankingDirection "DESC"^^<http://www.w3.org/2001/XMLSchema#string> ;
	opdm:attributePosition "0"^^<http://www.w3.org/2001/XMLSchema#integer> ;
	opdm:priority "0"^^<http://www.w3.org/2001/XMLSchema#integer> ;
	opdm:exampleOfUsage "The value of this property is a boolean (true/false - xsd:boolean)."^^<http://www.w3.org/2001/XMLSchema#string> ;
	a opdm:MetadataContainer ;
	opdm:inProfile opdm:DefaultProfile .

dcterms:contributor a owl:AnnotationProperty .

_:node18vkiok0kx30 gr:hasMinValue "0"^^<http://www.w3.org/2001/XMLSchema#integer> ;
	gr:hasMaxValue "0"^^<http://www.w3.org/2001/XMLSchema#integer> ;
	a gr:QuantitativeValue .

_:node18vkiok0kx31 gr:hasMinValue "0"^^<http://www.w3.org/2001/XMLSchema#integer> ;
	a gr:QuantitativeValue ;
	gr:hasMaxValue "0"^^<http://www.w3.org/2001/XMLSchema#integer> .

skos:altLabel a owl:AnnotationProperty .

<http://purl.org/opdm/refrigerator#frostFree> opdm:minCardinality "0"^^<http://www.w3.org/2001/XMLSchema#string> ;
	a owl:DatatypeProperty ;
	rdfs:label "Frost free"@en ;
	opdm:maxCardinality "1"^^<http://www.w3.org/2001/XMLSchema#string> ;
	rdfs:subPropertyOf gr:datatypeProductOrServiceProperty ;
	rdfs:domain <http://purl.org/opdm/refrigerator#FridgeFreezer> ;
	opdm:isConfiguredBy _:node18vkiok0kx13 ;
	rdfs:isDefinedBy <http://purl.org/opdm/refrigerator#> ;
	rdfs:range <http://www.w3.org/2001/XMLSchema#boolean> ;
	rdfs:comment "This property specifies whether the fridge/freezer is equipped with a frost-free system or not."@en .

_:node18vkiok0kx7 gr:hasMinValue "1"^^<http://www.w3.org/2001/XMLSchema#integer> ;
	gr:hasMaxValue "4"^^<http://www.w3.org/2001/XMLSchema#integer> ;
	a gr:QuantitativeValue .

<http://purl.org/opdm/refrigerator#BottomFreezer> rdfs:label "BottomFreezerDoor"@en ;
	rdfs:comment "It represents a bottom freezer door type of fridge."@en ;
	rdfs:isDefinedBy <http://purl.org/opdm/refrigerator#> ;
	a <http://purl.org/opdm/refrigerator#StyleOfUnit> .

<http://purl.org/opdm/refrigerator#waterFiltration> rdfs:domain <http://purl.org/opdm/refrigerator#FridgeFreezer> ;
	a owl:DatatypeProperty ;
	opdm:maxCardinality "1"^^<http://www.w3.org/2001/XMLSchema#string> ;
	rdfs:label "Water filtration"@en ;
	opdm:isConfiguredBy _:node18vkiok0kx17 ;
	rdfs:isDefinedBy <http://purl.org/opdm/refrigerator#> ;
	rdfs:range <http://www.w3.org/2001/XMLSchema#boolean> ;
	opdm:minCardinality "0"^^<http://www.w3.org/2001/XMLSchema#string> ;
	rdfs:comment "This property specifies whether the fridge/freezer is equipped with a water filtration system or not."@en ;
	rdfs:subPropertyOf gr:datatypeProductOrServiceProperty .

_:node18vkiok0kx25 opdm:rankingDirection "DESC"^^<http://www.w3.org/2001/XMLSchema#string> ;
	opdm:priority "0"^^<http://www.w3.org/2001/XMLSchema#integer> ;
	a opdm:MetadataContainer ;
	opdm:attributePosition "0"^^<http://www.w3.org/2001/XMLSchema#integer> ;
	opdm:exampleOfUsage "The value of this property is a boolean (true/false - xsd:boolean)."^^<http://www.w3.org/2001/XMLSchema#string> ;
	opdm:inProfile opdm:DefaultProfile .

<http://purl.org/opdm/refrigerator#RelativeDirection> dcterms:contributor <http://en.wikipedia.org/wiki/Relative_direction> ;
	rdfs:isDefinedBy <http://purl.org/opdm/refrigerator#> ;
	rdfs:comment "Class to represent the most common relative directions. Possible values include: left, right, forward, backward, up, down."@en ;
	rdfs:label "RelativeDirection"@en ;
	a owl:Class ;
	rdfs:subClassOf gr:QualitativeValue .

_:node18vkiok0kx18 opdm:inProfile opdm:DefaultProfile ;
	opdm:exampleOfUsage "The value of this property is an individual of the ofrd:RelativeDirection class."^^<http://www.w3.org/2001/XMLSchema#string> ;
	a opdm:MetadataContainer ;
	opdm:priority "0"^^<http://www.w3.org/2001/XMLSchema#integer> ;
	opdm:rankingDirection "DESC"^^<http://www.w3.org/2001/XMLSchema#string> ;
	opdm:attributePosition "0"^^<http://www.w3.org/2001/XMLSchema#integer> .

<http://purl.org/opdm/refrigerator#EnergyG> rdfs:isDefinedBy <http://purl.org/opdm/refrigerator#> ;
	rdfs:comment "This concept represents the G energy efficiency rating in the European Union labelling scheme"@en ;
	a <http://purl.org/opdm/refrigerator#EnergyRatingEU> ;
	rdfs:label "G Rating"@en .

<http://purl.org/opdm/refrigerator#consumptionOfEnergy> rdfs:isDefinedBy <http://purl.org/opdm/refrigerator#> ;
	rdfs:subPropertyOf gr:quantitativeProductOrServiceProperty ;
	opdm:maxCardinality "1"^^<http://www.w3.org/2001/XMLSchema#string> ;
	rdfs:label "Consumption of energy"@en ;
	opdm:minCardinality "0"^^<http://www.w3.org/2001/XMLSchema#string> ;
	opdm:recommendedRangeOfMeasure _:node18vkiok0kx31 ;
	a owl:ObjectProperty ;
	opdm:recommendedUnitOfMeasure "KWH"^^<http://www.w3.org/2001/XMLSchema#string> ;
	opdm:isConfiguredBy _:node18vkiok0kx32 ;
	rdfs:domain <http://purl.org/opdm/refrigerator#FridgeFreezer> ;
	rdfs:range gr:QuantitativeValue ;
	rdfs:comment "The consumption of energy of the fridge/freezer in kilowatt hour (in a year) - UN/CEFACT common code: KWH."@en .

<http://purl.org/opdm/refrigerator#ClimateSN> rdfs:isDefinedBy <http://purl.org/opdm/refrigerator#> ;
	rdfs:label "SN Rating"@en ;
	a <http://purl.org/opdm/refrigerator#ClimateClass> ;
	rdfs:comment "This concept represents the SN climate class rating. The fridge/freezer can operate between 10 - 32 degree celsius of room temperature"@en .

<http://purl.org/opdm/refrigerator#antibacterial> rdfs:label "Antibacterial"@en ;
	rdfs:isDefinedBy <http://purl.org/opdm/refrigerator#> ;
	rdfs:comment "This property specifies whether the fridge/freezer is equipped with an antibacterial detector system or not."@en ;
	rdfs:domain <http://purl.org/opdm/refrigerator#FridgeFreezer> ;
	rdfs:subPropertyOf gr:datatypeProductOrServiceProperty ;
	opdm:minCardinality "0"^^<http://www.w3.org/2001/XMLSchema#string> ;
	opdm:maxCardinality "1"^^<http://www.w3.org/2001/XMLSchema#string> ;
	opdm:isConfiguredBy _:node18vkiok0kx33 ;
	a owl:DatatypeProperty ;
	rdfs:range <http://www.w3.org/2001/XMLSchema#boolean> .

<http://purl.org/opdm/refrigerator#Fridge> rdfs:label "Frigorífico"@es ;
	rdfs:comment "A generic Fridge with no Freezer unit as a product type"@en ;
	rdfs:subClassOf <http://purl.org/opdm/refrigerator#FridgeFreezer> ;
	foaf:depiction <http://upload.wikimedia.org/wikipedia/commons/2/21/2011-05-09_14-56-45_407.jpg> ;
	rdfs:label "Fridge"@en ;
	skos:altLabel "Nevera"@es ;
	a owl:Class ;
	skos:altLabel "Refrigerator"@en , "Heladera"@es ;
	rdfs:isDefinedBy <http://purl.org/opdm/refrigerator#> ;
	rdfs:label "Kühlschrank"@de ;
	opdm:category <http://purl.org/opdm/category/google#Home_and_Garden_Kitchen_and_Dining_KitchenAppliances_Refrigerators> ;
	skos:altLabel "Refrigerador"@es .

<http://purl.org/opdm/refrigerator#FreeStanding> a <http://purl.org/opdm/refrigerator#TypeOfBody> ;
	rdfs:label "FreeStanding"@en ;
	rdfs:isDefinedBy <http://purl.org/opdm/refrigerator#> ;
	rdfs:comment "It represents a free-standing type of body frame for a fridge/freezer."@en .

_:node18vkiok0kx32 opdm:attributePosition "0"^^<http://www.w3.org/2001/XMLSchema#integer> ;
	opdm:exampleOfUsage "The value of this property is an individual of the gr:QuantitativeValue class."^^<http://www.w3.org/2001/XMLSchema#string> ;
	a opdm:MetadataContainer ;
	opdm:rankingDirection "DESC"^^<http://www.w3.org/2001/XMLSchema#string> ;
	opdm:inProfile opdm:DefaultProfile ;
	opdm:priority "0"^^<http://www.w3.org/2001/XMLSchema#integer> .

dcterms:subject a owl:AnnotationProperty .

_:node18vkiok0kx15 gr:hasMinValue "100"^^<http://www.w3.org/2001/XMLSchema#integer> ;
	gr:hasMaxValue "300"^^<http://www.w3.org/2001/XMLSchema#integer> ;
	a gr:QuantitativeValue .

_:node18vkiok0kx16 a opdm:MetadataContainer ;
	opdm:attributePosition "0"^^<http://www.w3.org/2001/XMLSchema#integer> ;
	opdm:exampleOfUsage "The value of this property is an individual of the ofrd:TypeOfBody class."^^<http://www.w3.org/2001/XMLSchema#string> ;
	opdm:priority "0"^^<http://www.w3.org/2001/XMLSchema#integer> ;
	opdm:inProfile opdm:DefaultProfile ;
	opdm:rankingDirection "DESC"^^<http://www.w3.org/2001/XMLSchema#string> .

<http://purl.org/opdm/refrigerator#volumeOfUnitNet> rdfs:subPropertyOf gr:quantitativeProductOrServiceProperty ;
	rdfs:isDefinedBy <http://purl.org/opdm/refrigerator#> ;
	opdm:recommendedRangeOfMeasure _:node18vkiok0kx30 ;
	rdfs:label "Volume of unit net"@en ;
	opdm:maxCardinality "1"^^<http://www.w3.org/2001/XMLSchema#string> ;
	opdm:isConfiguredBy _:node18vkiok0kx24 ;
	rdfs:domain <http://purl.org/opdm/refrigerator#FridgeFreezer> ;
	rdfs:comment "The net volume in liters of the total unit. The value of this property usually is equal to the sum of the value of the properties ofrd:volumeOfFridge and ofrd:volumeOfFreezer"@en ;
	a owl:ObjectProperty ;
	opdm:recommendedUnitOfMeasure "LTR"^^<http://www.w3.org/2001/XMLSchema#string> ;
	opdm:minCardinality "0"^^<http://www.w3.org/2001/XMLSchema#string> ;
	rdfs:range gr:QuantitativeValue .

_:node18vkiok0kx34 opdm:rankingDirection "DESC"^^<http://www.w3.org/2001/XMLSchema#string> ;
	opdm:attributePosition "0"^^<http://www.w3.org/2001/XMLSchema#integer> ;
	opdm:priority "0"^^<http://www.w3.org/2001/XMLSchema#integer> ;
	opdm:exampleOfUsage "The value of this property is a boolean (true/false - xsd:boolean)."^^<http://www.w3.org/2001/XMLSchema#string> ;
	a opdm:MetadataContainer ;
	opdm:inProfile opdm:DefaultProfile .

<http://purl.org/opdm/refrigerator#EnergyA2> rdfs:isDefinedBy <http://purl.org/opdm/refrigerator#> ;
	rdfs:label "A++ Rating"@en ;
	rdfs:comment "This concept represents the A++ energy efficiency rating in the European Union labelling scheme"@en ;
	a <http://purl.org/opdm/refrigerator#EnergyRatingEU> .

<http://purl.org/opdm/refrigerator#EnergyB> rdfs:comment "This concept represents the B energy efficiency rating in the European Union labelling scheme"@en ;
	a <http://purl.org/opdm/refrigerator#EnergyRatingEU> ;
	rdfs:isDefinedBy <http://purl.org/opdm/refrigerator#> ;
	rdfs:label "B Rating"@en .

<http://purl.org/opdm/refrigerator#doorOpenAlarm> rdfs:subPropertyOf gr:datatypeProductOrServiceProperty ;
	a owl:DatatypeProperty ;
	opdm:isConfiguredBy _:node18vkiok0kx29 ;
	rdfs:comment "This property specifies whether the fridge/freezer is equipped with a door-open alarm system or not."@en ;
	opdm:maxCardinality "1"^^<http://www.w3.org/2001/XMLSchema#string> ;
	opdm:minCardinality "0"^^<http://www.w3.org/2001/XMLSchema#string> ;
	rdfs:isDefinedBy <http://purl.org/opdm/refrigerator#> ;
	rdfs:range <http://www.w3.org/2001/XMLSchema#boolean> ;
	rdfs:domain <http://purl.org/opdm/refrigerator#FridgeFreezer> ;
	rdfs:label "Door open alarm"@en .

<http://purl.org/opdm/refrigerator#EnergyRatingEU> rdfs:subClassOf gr:QualitativeValue ;
	rdfs:comment "Class to represent the European Union energy label codas of a fridge. Possible values go from A+++ to G."@en ;
	rdfs:isDefinedBy <http://purl.org/opdm/refrigerator#> ;
	a owl:Class ;
	rdfs:label "EnergyRatingEU"@en .

<http://purl.org/opdm/refrigerator#energyStarUS> rdfs:domain <http://purl.org/opdm/refrigerator#FridgeFreezer> ;
	a owl:DatatypeProperty ;
	opdm:isConfiguredBy _:node18vkiok0kx28 ;
	opdm:maxCardinality "1"^^<http://www.w3.org/2001/XMLSchema#string> ;
	rdfs:label "Energy Star US"@en ;
	rdfs:comment "This property specifies whether the fridge/freezer is certified with the Energy Star label awarded by the Department of Energy and Enviromental Protection Agency of the US, or not."@en ;
	rdfs:isDefinedBy <http://purl.org/opdm/refrigerator#> ;
	rdfs:range <http://www.w3.org/2001/XMLSchema#boolean> ;
	opdm:minCardinality "0"^^<http://www.w3.org/2001/XMLSchema#string> ;
	rdfs:subPropertyOf gr:datatypeProductOrServiceProperty .

_:node18vkiok0kx35 opdm:priority "0"^^<http://www.w3.org/2001/XMLSchema#integer> ;
	opdm:inProfile opdm:DefaultProfile ;
	a opdm:MetadataContainer ;
	opdm:rankingDirection "DESC"^^<http://www.w3.org/2001/XMLSchema#string> ;
	opdm:attributePosition "0"^^<http://www.w3.org/2001/XMLSchema#integer> ;
	opdm:exampleOfUsage "The value of this property is a boolean (true/false - xsd:boolean)."^^<http://www.w3.org/2001/XMLSchema#string> .

<http://purl.org/opdm/refrigerator#ClimateClass> a owl:Class ;
	rdfs:comment "Class to represent the range of room temperatures that a fridge/freezer can operate. Possible values include: N, SN, ST, T."@en ;
	rdfs:subClassOf gr:QualitativeValue ;
	rdfs:label "ClimateClass"@en ;
	rdfs:isDefinedBy <http://purl.org/opdm/refrigerator#> .

<http://purl.org/opdm/refrigerator#SideBySide> rdfs:isDefinedBy <http://purl.org/opdm/refrigerator#> ;
	rdfs:label "SideBySideDoor"@en ;
	a <http://purl.org/opdm/refrigerator#StyleOfUnit> ;
	rdfs:comment "It represents a side-by-side door type of fridge."@en .

_:node18vkiok0kx36 gr:hasMinValue "0"^^<http://www.w3.org/2001/XMLSchema#integer> ;
	a gr:QuantitativeValue ;
	gr:hasMaxValue "0"^^<http://www.w3.org/2001/XMLSchema#integer> .

<http://purl.org/opdm/refrigerator#childLock> rdfs:domain <http://purl.org/opdm/refrigerator#FridgeFreezer> ;
	rdfs:comment "This property specifies whether the fridge/freezer is equipped with a child lock system or not."@en ;
	rdfs:label "Child lock"@en ;
	opdm:maxCardinality "1"^^<http://www.w3.org/2001/XMLSchema#string> ;
	rdfs:subPropertyOf gr:datatypeProductOrServiceProperty ;
	rdfs:isDefinedBy <http://purl.org/opdm/refrigerator#> ;
	rdfs:range <http://www.w3.org/2001/XMLSchema#boolean> ;
	opdm:minCardinality "0"^^<http://www.w3.org/2001/XMLSchema#string> ;
	opdm:isConfiguredBy _:node18vkiok0kx37 ;
	a owl:DatatypeProperty .

<http://purl.org/opdm/refrigerator#EnergyD> rdfs:comment "This concept represents the D energy efficiency rating in the European Union labelling scheme"@en ;
	a <http://purl.org/opdm/refrigerator#EnergyRatingEU> ;
	rdfs:label "D Rating"@en ;
	rdfs:isDefinedBy <http://purl.org/opdm/refrigerator#> .

_:node18vkiok0kx38 opdm:priority "0"^^<http://www.w3.org/2001/XMLSchema#integer> ;
	opdm:exampleOfUsage "The value of this property is a boolean (true/false - xsd:boolean)."^^<http://www.w3.org/2001/XMLSchema#string> ;
	a opdm:MetadataContainer ;
	opdm:rankingDirection "DESC"^^<http://www.w3.org/2001/XMLSchema#string> ;
	opdm:attributePosition "0"^^<http://www.w3.org/2001/XMLSchema#integer> ;
	opdm:inProfile opdm:DefaultProfile .

<http://purl.org/opdm/refrigerator#reversibleDoor> rdfs:label "Reversible door"@en ;
	rdfs:isDefinedBy <http://purl.org/opdm/refrigerator#> ;
	rdfs:range <http://www.w3.org/2001/XMLSchema#boolean> ;
	rdfs:comment "This property specifies whether the fridge/freezer is equipped with doors that can be mounted on either side of the unit or not."@en ;
	opdm:minCardinality "0"^^<http://www.w3.org/2001/XMLSchema#string> ;
	rdfs:subPropertyOf gr:datatypeProductOrServiceProperty ;
	rdfs:domain <http://purl.org/opdm/refrigerator#FridgeFreezer> ;
	opdm:isConfiguredBy _:node18vkiok0kx35 ;
	a owl:DatatypeProperty ;
	opdm:maxCardinality "1"^^<http://www.w3.org/2001/XMLSchema#string> .

_:node18vkiok0kx39 opdm:attributePosition "0"^^<http://www.w3.org/2001/XMLSchema#integer> ;
	opdm:inProfile opdm:DefaultProfile ;
	opdm:priority "0"^^<http://www.w3.org/2001/XMLSchema#integer> ;
	a opdm:MetadataContainer ;
	opdm:exampleOfUsage "The value of this property is an integer (xsd:integer)."^^<http://www.w3.org/2001/XMLSchema#string> ;
	opdm:rankingDirection "DESC"^^<http://www.w3.org/2001/XMLSchema#string> .

<http://purl.org/opdm/refrigerator#numberOfFreezerCompartments> opdm:minCardinality "0"^^<http://www.w3.org/2001/XMLSchema#string> ;
	opdm:maxCardinality "1"^^<http://www.w3.org/2001/XMLSchema#string> ;
	rdfs:domain <http://purl.org/opdm/refrigerator#FridgeFreezer> ;
	rdfs:isDefinedBy <http://purl.org/opdm/refrigerator#> ;
	rdfs:comment "This property specifies the number of compartments that the freezer is equipped with."@en ;
	rdfs:label "Number of freezer compartments"@en ;
	rdfs:subPropertyOf gr:datatypeProductOrServiceProperty ;
	rdfs:range <http://www.w3.org/2001/XMLSchema#integer> ;
	a owl:DatatypeProperty ;
	opdm:isConfiguredBy _:node18vkiok0kx27 .

_:node18vkiok0kx37 opdm:attributePosition "0"^^<http://www.w3.org/2001/XMLSchema#integer> ;
	a opdm:MetadataContainer ;
	opdm:rankingDirection "DESC"^^<http://www.w3.org/2001/XMLSchema#string> ;
	opdm:inProfile opdm:DefaultProfile ;
	opdm:priority "0"^^<http://www.w3.org/2001/XMLSchema#integer> ;
	opdm:exampleOfUsage "The value of this property is a boolean (true/false - xsd:boolean)."^^<http://www.w3.org/2001/XMLSchema#string> .

<http://purl.org/opdm/refrigerator#TypeOfBody> rdfs:subClassOf gr:QualitativeValue ;
	rdfs:comment "Class to represent the different types of body frames of a fridge/freezer. Possible values include: built-in, free-standing."@en ;
	rdfs:isDefinedBy <http://purl.org/opdm/refrigerator#> ;
	a owl:Class ;
	rdfs:label "TypeOfBody"@en .

<http://purl.org/opdm/refrigerator#volumeOfFridge> rdfs:domain <http://purl.org/opdm/refrigerator#FridgeFreezer> ;
	rdfs:label "Volume of fridge"@en ;
	rdfs:subPropertyOf gr:quantitativeProductOrServiceProperty ;
	a owl:ObjectProperty ;
	opdm:maxCardinality "1"^^<http://www.w3.org/2001/XMLSchema#string> ;
	rdfs:comment "The volume in liters of the fresh goods compartment built-into the full fridge/freezer unit."@en ;
	opdm:isConfiguredBy _:node18vkiok0kx4 ;
	rdfs:isDefinedBy <http://purl.org/opdm/refrigerator#> ;
	rdfs:range gr:QuantitativeValue ;
	opdm:recommendedUnitOfMeasure "LTR"^^<http://www.w3.org/2001/XMLSchema#string> ;
	opdm:minCardinality "0"^^<http://www.w3.org/2001/XMLSchema#string> ;
	opdm:recommendedRangeOfMeasure _:node18vkiok0kx36 .

<http://purl.org/opdm/refrigerator#volumeOfFreezer> a owl:ObjectProperty ;
	rdfs:domain <http://purl.org/opdm/refrigerator#FridgeFreezer> ;
	opdm:recommendedUnitOfMeasure "LTR"^^<http://www.w3.org/2001/XMLSchema#string> ;
	rdfs:subPropertyOf gr:quantitativeProductOrServiceProperty ;
	rdfs:isDefinedBy <http://purl.org/opdm/refrigerator#> ;
	rdfs:range gr:QuantitativeValue ;
	rdfs:comment "The volume in liters of the frozen goods compartment built-into the full fridge/freezer unit."@en ;
	opdm:recommendedRangeOfMeasure _:node18vkiok0kx26 ;
	rdfs:label "Volume of freezer"@en ;
	opdm:maxCardinality "1"^^<http://www.w3.org/2001/XMLSchema#string> ;
	opdm:isConfiguredBy _:node18vkiok0kx40 ;
	opdm:minCardinality "0"^^<http://www.w3.org/2001/XMLSchema#string> .

<http://purl.org/opdm/refrigerator#levelOfNoise> a owl:ObjectProperty ;
	rdfs:isDefinedBy <http://purl.org/opdm/refrigerator#> ;
	rdfs:range gr:QuantitativeValue ;
	opdm:recommendedUnitOfMeasure "2N"^^<http://www.w3.org/2001/XMLSchema#string> ;
	rdfs:label "Level of noise"@en ;
	opdm:recommendedRangeOfMeasure _:node18vkiok0kx5 ;
	opdm:minCardinality "0"^^<http://www.w3.org/2001/XMLSchema#string> ;
	opdm:isConfiguredBy _:node18vkiok0kx22 ;
	rdfs:comment "The level of noise in decibels of the fridge/freezer (UN/CEFACT common code: 2N)."@en ;
	rdfs:subPropertyOf gr:quantitativeProductOrServiceProperty ;
	opdm:maxCardinality "1"^^<http://www.w3.org/2001/XMLSchema#string> ;
	rdfs:domain <http://purl.org/opdm/refrigerator#FridgeFreezer> .

_:node18vkiok0kx21 a opdm:MetadataContainer ;
	opdm:inProfile opdm:DefaultProfile ;
	opdm:priority "0"^^<http://www.w3.org/2001/XMLSchema#integer> ;
	opdm:exampleOfUsage "The value of this property is a boolean (true/false - xsd:boolean)."^^<http://www.w3.org/2001/XMLSchema#string> ;
	opdm:attributePosition "0"^^<http://www.w3.org/2001/XMLSchema#integer> ;
	opdm:rankingDirection "DESC"^^<http://www.w3.org/2001/XMLSchema#string> .

<http://purl.org/opdm/refrigerator#ClimateN> rdfs:isDefinedBy <http://purl.org/opdm/refrigerator#> ;
	rdfs:label "N Rating"@en ;
	rdfs:comment "This concept represents the N climate class rating. The fridge/freezer can operate between 16 - 32 degree celsius of room temperature"@en ;
	a <http://purl.org/opdm/refrigerator#ClimateClass> .

<http://purl.org/opdm/refrigerator#ratingOfClimateClass> opdm:maxCardinality "1"^^<http://www.w3.org/2001/XMLSchema#string> ;
	opdm:isConfiguredBy _:node18vkiok0kx19 ;
	rdfs:domain <http://purl.org/opdm/refrigerator#FridgeFreezer> ;
	rdfs:subPropertyOf gr:qualitativeProductOrServiceProperty ;
	rdfs:range <http://purl.org/opdm/refrigerator#ClimateClass> ;
	rdfs:comment "The climate class rating that the fridge/freezer can operate at."@en ;
	a owl:ObjectProperty ;
	rdfs:label "Rating of climate class"@en ;
	opdm:minCardinality "0"^^<http://www.w3.org/2001/XMLSchema#string> ;
	rdfs:isDefinedBy <http://purl.org/opdm/refrigerator#> .

<http://purl.org/opdm/refrigerator#iceMaker> opdm:maxCardinality "1"^^<http://www.w3.org/2001/XMLSchema#string> ;
	rdfs:comment "This property specifies whether the fridge/freezer is equipped with an ice-maker system or not."@en ;
	opdm:minCardinality "0"^^<http://www.w3.org/2001/XMLSchema#string> ;
	rdfs:isDefinedBy <http://purl.org/opdm/refrigerator#> ;
	rdfs:range <http://www.w3.org/2001/XMLSchema#boolean> ;
	rdfs:domain <http://purl.org/opdm/refrigerator#FridgeFreezer> ;
	opdm:isConfiguredBy _:node18vkiok0kx34 ;
	rdfs:subPropertyOf gr:datatypeProductOrServiceProperty ;
	rdfs:label "Ice maker"@en ;
	a owl:DatatypeProperty .

<http://purl.org/opdm/refrigerator#capableOfACS> rdfs:isDefinedBy <http://purl.org/opdm/refrigerator#> ;
	rdfs:label "Capable of ACS"@en ;
	rdfs:comment "This property specifies whether the fridge/freezer is equipped with an Advanced Control System (ACS) or not. ACS allows the fridge/freezer to maintain the desired internal temperature safe from variations in the external termperature."@en ;
	rdfs:domain <http://purl.org/opdm/refrigerator#FridgeFreezer> ;
	rdfs:subPropertyOf gr:datatypeProductOrServiceProperty ;
	opdm:minCardinality "0"^^<http://www.w3.org/2001/XMLSchema#string> ;
	opdm:maxCardinality "1"^^<http://www.w3.org/2001/XMLSchema#string> ;
	a owl:DatatypeProperty ;
	rdfs:range <http://www.w3.org/2001/XMLSchema#boolean> ;
	opdm:isConfiguredBy _:node18vkiok0kx38 .

<http://purl.org/opdm/refrigerator#StyleOfUnit> rdfs:label "StyleOfUnit"@en ;
	rdfs:isDefinedBy <http://purl.org/opdm/refrigerator#> ;
	rdfs:comment "Class to represent the different styles of fridge/freezers. Possible values include: french-door, side-by-side, top-freezer, bottom-freezer, single-door."@en ;
	a owl:Class ;
	rdfs:subClassOf gr:QualitativeValue .

_:node18vkiok0kx40 opdm:exampleOfUsage "The value of this property is an individual of the gr:QuantitativeValue class."^^<http://www.w3.org/2001/XMLSchema#string> ;
	opdm:attributePosition "0"^^<http://www.w3.org/2001/XMLSchema#integer> ;
	opdm:inProfile opdm:DefaultProfile ;
	opdm:priority "0"^^<http://www.w3.org/2001/XMLSchema#integer> ;
	a opdm:MetadataContainer ;
	opdm:rankingDirection "DESC"^^<http://www.w3.org/2001/XMLSchema#string> .

<http://purl.org/opdm/refrigerator#TopFreezer> rdfs:isDefinedBy <http://purl.org/opdm/refrigerator#> ;
	rdfs:label "TopFreezerDoor"@en ;
	rdfs:comment "It represents a top freezer door type of fridge."@en ;
	a <http://purl.org/opdm/refrigerator#StyleOfUnit> .

<http://purl.org/opdm/refrigerator#numberOfFridgeShelves> rdfs:subPropertyOf gr:datatypeProductOrServiceProperty ;
	opdm:isConfiguredBy _:node18vkiok0kx39 ;
	rdfs:label "Number of fridge shelves"@en ;
	rdfs:range <http://www.w3.org/2001/XMLSchema#integer> ;
	rdfs:isDefinedBy <http://purl.org/opdm/refrigerator#> ;
	opdm:maxCardinality "1"^^<http://www.w3.org/2001/XMLSchema#string> ;
	rdfs:comment "This property specifies the number of shelves or levels that the fridge is equipped with."@en ;
	a owl:DatatypeProperty ;
	opdm:minCardinality "0"^^<http://www.w3.org/2001/XMLSchema#string> ;
	rdfs:domain <http://purl.org/opdm/refrigerator#FridgeFreezer> .

<http://purl.org/opdm/refrigerator#EnergyA> a <http://purl.org/opdm/refrigerator#EnergyRatingEU> ;
	rdfs:comment "This concept represents the A energy efficiency rating in the European Union labelling scheme"@en ;
	rdfs:isDefinedBy <http://purl.org/opdm/refrigerator#> ;
	rdfs:label "A Rating"@en .

_:node18vkiok0kx33 opdm:rankingDirection "DESC"^^<http://www.w3.org/2001/XMLSchema#string> ;
	opdm:priority "0"^^<http://www.w3.org/2001/XMLSchema#integer> ;
	a opdm:MetadataContainer ;
	opdm:attributePosition "0"^^<http://www.w3.org/2001/XMLSchema#integer> ;
	opdm:exampleOfUsage "The value of this property is a boolean (true/false - xsd:boolean)."^^<http://www.w3.org/2001/XMLSchema#string> ;
	opdm:inProfile opdm:DefaultProfile .

<http://purl.org/opdm/refrigerator#numberOfFrontDoors> rdfs:domain <http://purl.org/opdm/refrigerator#FridgeFreezer> ;
	rdfs:label "Number of front doors"@en ;
	opdm:minCardinality "0"^^<http://www.w3.org/2001/XMLSchema#string> ;
	rdfs:isDefinedBy <http://purl.org/opdm/refrigerator#> ;
	rdfs:comment "This property specifies the number of front doors that the fridge is equipped with."@en ;
	opdm:maxCardinality "1"^^<http://www.w3.org/2001/XMLSchema#string> ;
	rdfs:range <http://www.w3.org/2001/XMLSchema#integer> ;
	rdfs:subPropertyOf gr:datatypeProductOrServiceProperty ;
	opdm:recommendedRangeOfMeasure _:node18vkiok0kx23 ;
	a owl:DatatypeProperty ;
	opdm:isConfiguredBy _:node18vkiok0kx20 .

<http://purl.org/opdm/refrigerator#EnergyE> rdfs:label "E Rating"@en ;
	rdfs:comment "This concept represents the E energy efficiency rating in the European Union labelling scheme"@en ;
	a <http://purl.org/opdm/refrigerator#EnergyRatingEU> ;
	rdfs:isDefinedBy <http://purl.org/opdm/refrigerator#> .

_:node18vkiok0kx41 opdm:exampleOfUsage "The value of this property is an individual of the gr:QuantitativeValue class."^^<http://www.w3.org/2001/XMLSchema#string> ;
	opdm:inProfile opdm:DefaultProfile ;
	opdm:priority "0"^^<http://www.w3.org/2001/XMLSchema#integer> ;
	opdm:attributePosition "0"^^<http://www.w3.org/2001/XMLSchema#integer> ;
	a opdm:MetadataContainer ;
	opdm:rankingDirection "DESC"^^<http://www.w3.org/2001/XMLSchema#string> .

<http://purl.org/opdm/refrigerator#numberOfFrontDrawers> opdm:isConfiguredBy _:node18vkiok0kx42 ;
	opdm:recommendedRangeOfMeasure _:node18vkiok0kx43 .

_:node18vkiok0kx44 opdm:inProfile opdm:DefaultProfile ;
	opdm:attributePosition "0"^^<http://www.w3.org/2001/XMLSchema#integer> ;
	opdm:exampleOfUsage "The value of this property is an individual of the gr:QuantitativeValue class."^^<http://www.w3.org/2001/XMLSchema#string> ;
	opdm:priority "0"^^<http://www.w3.org/2001/XMLSchema#integer> ;
	opdm:rankingDirection "DESC"^^<http://www.w3.org/2001/XMLSchema#string> ;
	a opdm:MetadataContainer .

_:node18vkiok0kx45 gr:hasMinValue "0"^^<http://www.w3.org/2001/XMLSchema#integer> ;
	a gr:QuantitativeValue ;
	gr:hasMaxValue "0"^^<http://www.w3.org/2001/XMLSchema#integer> .

<http://purl.org/opdm/refrigerator#ratingOfStars> opdm:isConfiguredBy _:node18vkiok0kx46 ;
	opdm:recommendedRangeOfMeasure _:node18vkiok0kx47 .

_:node18vkiok0kx48 opdm:rankingDirection "DESC"^^<http://www.w3.org/2001/XMLSchema#string> ;
	opdm:attributePosition "0"^^<http://www.w3.org/2001/XMLSchema#integer> ;
	opdm:priority "0"^^<http://www.w3.org/2001/XMLSchema#integer> ;
	opdm:exampleOfUsage "The value of this property is a boolean (true/false - xsd:boolean)."^^<http://www.w3.org/2001/XMLSchema#string> ;
	a opdm:MetadataContainer ;
	opdm:inProfile opdm:DefaultProfile .

_:node18vkiok0kx49 a gr:QuantitativeValue ;
	gr:hasMaxValue "0"^^<http://www.w3.org/2001/XMLSchema#integer> ;
	gr:hasMinValue "0"^^<http://www.w3.org/2001/XMLSchema#integer> .

<http://purl.org/opdm/refrigerator#ratingOfEnergyEU> opdm:isConfiguredBy _:node18vkiok0kx50 .

<http://purl.org/opdm/refrigerator#volumeOfUnitGross> opdm:isConfiguredBy _:node18vkiok0kx41 ;
	opdm:recommendedRangeOfMeasure _:node18vkiok0kx49 .

_:node18vkiok0kx51 opdm:priority "0"^^<http://www.w3.org/2001/XMLSchema#integer> ;
	opdm:rankingDirection "DESC"^^<http://www.w3.org/2001/XMLSchema#string> ;
	a opdm:MetadataContainer ;
	opdm:attributePosition "0"^^<http://www.w3.org/2001/XMLSchema#integer> ;
	opdm:inProfile opdm:DefaultProfile ;
	opdm:exampleOfUsage "The value of this property is an individual of the ofrd:StyleOfUnit class."^^<http://www.w3.org/2001/XMLSchema#string> .

_:node18vkiok0kx52 opdm:inProfile opdm:DefaultProfile ;
	opdm:rankingDirection "DESC"^^<http://www.w3.org/2001/XMLSchema#string> ;
	a opdm:MetadataContainer ;
	opdm:priority "0"^^<http://www.w3.org/2001/XMLSchema#integer> ;
	opdm:exampleOfUsage "The value of this property is a boolean (true/false - xsd:boolean)."^^<http://www.w3.org/2001/XMLSchema#string> ;
	opdm:attributePosition "0"^^<http://www.w3.org/2001/XMLSchema#integer> .

_:node18vkiok0kx53 opdm:attributePosition "0"^^<http://www.w3.org/2001/XMLSchema#integer> ;
	a opdm:MetadataContainer ;
	opdm:rankingDirection "DESC"^^<http://www.w3.org/2001/XMLSchema#string> ;
	opdm:inProfile opdm:DefaultProfile ;
	opdm:priority "0"^^<http://www.w3.org/2001/XMLSchema#integer> ;
	opdm:exampleOfUsage "The value of this property is a boolean (true/false - xsd:boolean)."^^<http://www.w3.org/2001/XMLSchema#string> .

<http://purl.org/opdm/refrigerator#display> opdm:isConfiguredBy _:node18vkiok0kx52 .

_:node18vkiok0kx54 opdm:priority "0"^^<http://www.w3.org/2001/XMLSchema#integer> ;
	opdm:inProfile opdm:DefaultProfile ;
	opdm:rankingDirection "DESC"^^<http://www.w3.org/2001/XMLSchema#string> ;
	a opdm:MetadataContainer ;
	opdm:exampleOfUsage "The value of this property is an individual of the gr:QuantitativeValue class."^^<http://www.w3.org/2001/XMLSchema#string> ;
	opdm:attributePosition "0"^^<http://www.w3.org/2001/XMLSchema#integer> .

<http://purl.org/opdm/refrigerator#powerSupply> opdm:isConfiguredBy _:node18vkiok0kx54 ;
	opdm:recommendedRangeOfMeasure _:node18vkiok0kx55 .

<http://purl.org/opdm/refrigerator#typeOfBody> opdm:isConfiguredBy _:node18vkiok0kx56 .

_:node18vkiok0kx57 opdm:rankingDirection "DESC"^^<http://www.w3.org/2001/XMLSchema#string> ;
	opdm:attributePosition "0"^^<http://www.w3.org/2001/XMLSchema#integer> ;
	opdm:priority "0"^^<http://www.w3.org/2001/XMLSchema#integer> ;
	opdm:exampleOfUsage "The value of this property is a boolean (true/false - xsd:boolean)."^^<http://www.w3.org/2001/XMLSchema#string> ;
	a opdm:MetadataContainer ;
	opdm:inProfile opdm:DefaultProfile .

<http://purl.org/opdm/refrigerator#positionOfDoorHinge> opdm:isConfiguredBy _:node18vkiok0kx58 .

_:node18vkiok0kx42 opdm:rankingDirection "DESC"^^<http://www.w3.org/2001/XMLSchema#string> ;
	opdm:exampleOfUsage "The value of this property is an integer (xsd:integer)."^^<http://www.w3.org/2001/XMLSchema#string> ;
	opdm:priority "0"^^<http://www.w3.org/2001/XMLSchema#integer> ;
	a opdm:MetadataContainer ;
	opdm:attributePosition "0"^^<http://www.w3.org/2001/XMLSchema#integer> ;
	opdm:inProfile opdm:DefaultProfile .

_:node18vkiok0kx50 a opdm:MetadataContainer ;
	opdm:attributePosition "0"^^<http://www.w3.org/2001/XMLSchema#integer> ;
	opdm:rankingDirection "DESC"^^<http://www.w3.org/2001/XMLSchema#string> ;
	opdm:exampleOfUsage "The value of this property is an individual of the ofrd:EnergyRatingEU class."^^<http://www.w3.org/2001/XMLSchema#string> ;
	opdm:inProfile opdm:DefaultProfile ;
	opdm:priority "0"^^<http://www.w3.org/2001/XMLSchema#integer> .

_:node18vkiok0kx59 opdm:priority "0"^^<http://www.w3.org/2001/XMLSchema#integer> ;
	opdm:inProfile opdm:DefaultProfile ;
	opdm:rankingDirection "DESC"^^<http://www.w3.org/2001/XMLSchema#string> ;
	a opdm:MetadataContainer ;
	opdm:exampleOfUsage "The value of this property is an individual of the ofrd:ClimateClass class."^^<http://www.w3.org/2001/XMLSchema#string> ;
	opdm:attributePosition "0"^^<http://www.w3.org/2001/XMLSchema#integer> .

_:node18vkiok0kx60 opdm:inProfile opdm:DefaultProfile ;
	a opdm:MetadataContainer ;
	opdm:priority "0"^^<http://www.w3.org/2001/XMLSchema#integer> ;
	opdm:rankingDirection "DESC"^^<http://www.w3.org/2001/XMLSchema#string> ;
	opdm:attributePosition "0"^^<http://www.w3.org/2001/XMLSchema#integer> ;
	opdm:exampleOfUsage "The value of this property is an integer (xsd:integer)."^^<http://www.w3.org/2001/XMLSchema#string> .

_:node18vkiok0kx43 a gr:QuantitativeValue ;
	gr:hasMaxValue "3"^^<http://www.w3.org/2001/XMLSchema#integer> ;
	gr:hasMinValue "0"^^<http://www.w3.org/2001/XMLSchema#integer> .

<http://purl.org/opdm/refrigerator#iceDispenser> opdm:isConfiguredBy _:node18vkiok0kx61 .

_:node18vkiok0kx62 a opdm:MetadataContainer ;
	opdm:exampleOfUsage "The value of this property is an individual of the gr:QuantitativeValue class."^^<http://www.w3.org/2001/XMLSchema#string> ;
	opdm:rankingDirection "DESC"^^<http://www.w3.org/2001/XMLSchema#string> ;
	opdm:attributePosition "0"^^<http://www.w3.org/2001/XMLSchema#integer> ;
	opdm:inProfile opdm:DefaultProfile ;
	opdm:priority "0"^^<http://www.w3.org/2001/XMLSchema#integer> .

<http://purl.org/opdm/refrigerator#styleOfUnit> opdm:isConfiguredBy _:node18vkiok0kx51 .

_:node18vkiok0kx63 a gr:QuantitativeValue ;
	gr:hasMinValue "1"^^<http://www.w3.org/2001/XMLSchema#integer> ;
	gr:hasMaxValue "4"^^<http://www.w3.org/2001/XMLSchema#integer> .

_:node18vkiok0kx64 opdm:exampleOfUsage "The value of this property is an individual of the gr:QuantitativeValue class."^^<http://www.w3.org/2001/XMLSchema#string> ;
	opdm:attributePosition "0"^^<http://www.w3.org/2001/XMLSchema#integer> ;
	opdm:priority "0"^^<http://www.w3.org/2001/XMLSchema#integer> ;
	opdm:inProfile opdm:DefaultProfile ;
	a opdm:MetadataContainer ;
	opdm:rankingDirection "DESC"^^<http://www.w3.org/2001/XMLSchema#string> .

<http://purl.org/opdm/refrigerator#waterDispenser> opdm:isConfiguredBy _:node18vkiok0kx48 .

<http://purl.org/opdm/refrigerator#remoteControl> opdm:isConfiguredBy _:node18vkiok0kx65 .

_:node18vkiok0kx46 opdm:priority "0"^^<http://www.w3.org/2001/XMLSchema#integer> ;
	opdm:rankingDirection "DESC"^^<http://www.w3.org/2001/XMLSchema#string> ;
	a opdm:MetadataContainer ;
	opdm:exampleOfUsage "The value of this property is an integer (xsd:integer)."^^<http://www.w3.org/2001/XMLSchema#string> ;
	opdm:attributePosition "0"^^<http://www.w3.org/2001/XMLSchema#integer> ;
	opdm:inProfile opdm:DefaultProfile .

_:node18vkiok0kx66 gr:hasMaxValue "0"^^<http://www.w3.org/2001/XMLSchema#integer> ;
	a gr:QuantitativeValue ;
	gr:hasMinValue "0"^^<http://www.w3.org/2001/XMLSchema#integer> .

_:node18vkiok0kx67 opdm:attributePosition "0"^^<http://www.w3.org/2001/XMLSchema#integer> ;
	opdm:exampleOfUsage "The value of this property is an integer (xsd:integer)."^^<http://www.w3.org/2001/XMLSchema#string> ;
	opdm:inProfile opdm:DefaultProfile ;
	opdm:rankingDirection "DESC"^^<http://www.w3.org/2001/XMLSchema#string> ;
	opdm:priority "0"^^<http://www.w3.org/2001/XMLSchema#integer> ;
	a opdm:MetadataContainer .

_:node18vkiok0kx68 opdm:exampleOfUsage "The value of this property is a boolean (true/false - xsd:boolean)."^^<http://www.w3.org/2001/XMLSchema#string> ;
	a opdm:MetadataContainer ;
	opdm:inProfile opdm:DefaultProfile ;
	opdm:rankingDirection "DESC"^^<http://www.w3.org/2001/XMLSchema#string> ;
	opdm:attributePosition "0"^^<http://www.w3.org/2001/XMLSchema#integer> ;
	opdm:priority "0"^^<http://www.w3.org/2001/XMLSchema#integer> .

_:node18vkiok0kx69 opdm:rankingDirection "DESC"^^<http://www.w3.org/2001/XMLSchema#string> ;
	opdm:attributePosition "0"^^<http://www.w3.org/2001/XMLSchema#integer> ;
	opdm:priority "0"^^<http://www.w3.org/2001/XMLSchema#integer> ;
	opdm:exampleOfUsage "The value of this property is a boolean (true/false - xsd:boolean)."^^<http://www.w3.org/2001/XMLSchema#string> ;
	a opdm:MetadataContainer ;
	opdm:inProfile opdm:DefaultProfile .

_:node18vkiok0kx70 gr:hasMinValue "0"^^<http://www.w3.org/2001/XMLSchema#integer> ;
	gr:hasMaxValue "0"^^<http://www.w3.org/2001/XMLSchema#integer> ;
	a gr:QuantitativeValue .

_:node18vkiok0kx71 gr:hasMinValue "0"^^<http://www.w3.org/2001/XMLSchema#integer> ;
	a gr:QuantitativeValue ;
	gr:hasMaxValue "0"^^<http://www.w3.org/2001/XMLSchema#integer> .

<http://purl.org/opdm/refrigerator#frostFree> opdm:isConfiguredBy _:node18vkiok0kx53 .

_:node18vkiok0kx47 gr:hasMinValue "1"^^<http://www.w3.org/2001/XMLSchema#integer> ;
	gr:hasMaxValue "4"^^<http://www.w3.org/2001/XMLSchema#integer> ;
	a gr:QuantitativeValue .

<http://purl.org/opdm/refrigerator#waterFiltration> opdm:isConfiguredBy _:node18vkiok0kx57 .

_:node18vkiok0kx65 opdm:rankingDirection "DESC"^^<http://www.w3.org/2001/XMLSchema#string> ;
	opdm:priority "0"^^<http://www.w3.org/2001/XMLSchema#integer> ;
	a opdm:MetadataContainer ;
	opdm:attributePosition "0"^^<http://www.w3.org/2001/XMLSchema#integer> ;
	opdm:exampleOfUsage "The value of this property is a boolean (true/false - xsd:boolean)."^^<http://www.w3.org/2001/XMLSchema#string> ;
	opdm:inProfile opdm:DefaultProfile .

_:node18vkiok0kx58 opdm:inProfile opdm:DefaultProfile ;
	opdm:exampleOfUsage "The value of this property is an individual of the ofrd:RelativeDirection class."^^<http://www.w3.org/2001/XMLSchema#string> ;
	a opdm:MetadataContainer ;
	opdm:priority "0"^^<http://www.w3.org/2001/XMLSchema#integer> ;
	opdm:rankingDirection "DESC"^^<http://www.w3.org/2001/XMLSchema#string> ;
	opdm:attributePosition "0"^^<http://www.w3.org/2001/XMLSchema#integer> .

<http://purl.org/opdm/refrigerator#consumptionOfEnergy> opdm:recommendedRangeOfMeasure _:node18vkiok0kx71 ;
	opdm:isConfiguredBy _:node18vkiok0kx72 .

<http://purl.org/opdm/refrigerator#antibacterial> opdm:isConfiguredBy _:node18vkiok0kx73 .

_:node18vkiok0kx72 opdm:attributePosition "0"^^<http://www.w3.org/2001/XMLSchema#integer> ;
	opdm:exampleOfUsage "The value of this property is an individual of the gr:QuantitativeValue class."^^<http://www.w3.org/2001/XMLSchema#string> ;
	a opdm:MetadataContainer ;
	opdm:rankingDirection "DESC"^^<http://www.w3.org/2001/XMLSchema#string> ;
	opdm:inProfile opdm:DefaultProfile ;
	opdm:priority "0"^^<http://www.w3.org/2001/XMLSchema#integer> .

_:node18vkiok0kx55 gr:hasMinValue "100"^^<http://www.w3.org/2001/XMLSchema#integer> ;
	gr:hasMaxValue "300"^^<http://www.w3.org/2001/XMLSchema#integer> ;
	a gr:QuantitativeValue .

_:node18vkiok0kx56 a opdm:MetadataContainer ;
	opdm:attributePosition "0"^^<http://www.w3.org/2001/XMLSchema#integer> ;
	opdm:exampleOfUsage "The value of this property is an individual of the ofrd:TypeOfBody class."^^<http://www.w3.org/2001/XMLSchema#string> ;
	opdm:priority "0"^^<http://www.w3.org/2001/XMLSchema#integer> ;
	opdm:inProfile opdm:DefaultProfile ;
	opdm:rankingDirection "DESC"^^<http://www.w3.org/2001/XMLSchema#string> .

<http://purl.org/opdm/refrigerator#volumeOfUnitNet> opdm:recommendedRangeOfMeasure _:node18vkiok0kx70 ;
	opdm:isConfiguredBy _:node18vkiok0kx64 .

_:node18vkiok0kx74 opdm:rankingDirection "DESC"^^<http://www.w3.org/2001/XMLSchema#string> ;
	opdm:attributePosition "0"^^<http://www.w3.org/2001/XMLSchema#integer> ;
	opdm:priority "0"^^<http://www.w3.org/2001/XMLSchema#integer> ;
	opdm:exampleOfUsage "The value of this property is a boolean (true/false - xsd:boolean)."^^<http://www.w3.org/2001/XMLSchema#string> ;
	a opdm:MetadataContainer ;
	opdm:inProfile opdm:DefaultProfile .

<http://purl.org/opdm/refrigerator#doorOpenAlarm> opdm:isConfiguredBy _:node18vkiok0kx69 .

<http://purl.org/opdm/refrigerator#energyStarUS> opdm:isConfiguredBy _:node18vkiok0kx68 .

_:node18vkiok0kx75 opdm:priority "0"^^<http://www.w3.org/2001/XMLSchema#integer> ;
	opdm:inProfile opdm:DefaultProfile ;
	a opdm:MetadataContainer ;
	opdm:rankingDirection "DESC"^^<http://www.w3.org/2001/XMLSchema#string> ;
	opdm:attributePosition "0"^^<http://www.w3.org/2001/XMLSchema#integer> ;
	opdm:exampleOfUsage "The value of this property is a boolean (true/false - xsd:boolean)."^^<http://www.w3.org/2001/XMLSchema#string> .

_:node18vkiok0kx76 gr:hasMinValue "0"^^<http://www.w3.org/2001/XMLSchema#integer> ;
	a gr:QuantitativeValue ;
	gr:hasMaxValue "0"^^<http://www.w3.org/2001/XMLSchema#integer> .

<http://purl.org/opdm/refrigerator#childLock> opdm:isConfiguredBy _:node18vkiok0kx77 .

_:node18vkiok0kx78 opdm:priority "0"^^<http://www.w3.org/2001/XMLSchema#integer> ;
	opdm:exampleOfUsage "The value of this property is a boolean (true/false - xsd:boolean)."^^<http://www.w3.org/2001/XMLSchema#string> ;
	a opdm:MetadataContainer ;
	opdm:rankingDirection "DESC"^^<http://www.w3.org/2001/XMLSchema#string> ;
	opdm:attributePosition "0"^^<http://www.w3.org/2001/XMLSchema#integer> ;
	opdm:inProfile opdm:DefaultProfile .

<http://purl.org/opdm/refrigerator#reversibleDoor> opdm:isConfiguredBy _:node18vkiok0kx75 .

_:node18vkiok0kx79 opdm:attributePosition "0"^^<http://www.w3.org/2001/XMLSchema#integer> ;
	opdm:inProfile opdm:DefaultProfile ;
	opdm:priority "0"^^<http://www.w3.org/2001/XMLSchema#integer> ;
	a opdm:MetadataContainer ;
	opdm:exampleOfUsage "The value of this property is an integer (xsd:integer)."^^<http://www.w3.org/2001/XMLSchema#string> ;
	opdm:rankingDirection "DESC"^^<http://www.w3.org/2001/XMLSchema#string> .

<http://purl.org/opdm/refrigerator#numberOfFreezerCompartments> opdm:isConfiguredBy _:node18vkiok0kx67 .

_:node18vkiok0kx77 opdm:attributePosition "0"^^<http://www.w3.org/2001/XMLSchema#integer> ;
	a opdm:MetadataContainer ;
	opdm:rankingDirection "DESC"^^<http://www.w3.org/2001/XMLSchema#string> ;
	opdm:inProfile opdm:DefaultProfile ;
	opdm:priority "0"^^<http://www.w3.org/2001/XMLSchema#integer> ;
	opdm:exampleOfUsage "The value of this property is a boolean (true/false - xsd:boolean)."^^<http://www.w3.org/2001/XMLSchema#string> .

<http://purl.org/opdm/refrigerator#volumeOfFridge> opdm:isConfiguredBy _:node18vkiok0kx44 ;
	opdm:recommendedRangeOfMeasure _:node18vkiok0kx76 .

<http://purl.org/opdm/refrigerator#volumeOfFreezer> opdm:recommendedRangeOfMeasure _:node18vkiok0kx66 ;
	opdm:isConfiguredBy _:node18vkiok0kx80 .

<http://purl.org/opdm/refrigerator#levelOfNoise> opdm:recommendedRangeOfMeasure _:node18vkiok0kx45 ;
	opdm:isConfiguredBy _:node18vkiok0kx62 .

_:node18vkiok0kx61 a opdm:MetadataContainer ;
	opdm:inProfile opdm:DefaultProfile ;
	opdm:priority "0"^^<http://www.w3.org/2001/XMLSchema#integer> ;
	opdm:exampleOfUsage "The value of this property is a boolean (true/false - xsd:boolean)."^^<http://www.w3.org/2001/XMLSchema#string> ;
	opdm:attributePosition "0"^^<http://www.w3.org/2001/XMLSchema#integer> ;
	opdm:rankingDirection "DESC"^^<http://www.w3.org/2001/XMLSchema#string> .

<http://purl.org/opdm/refrigerator#ratingOfClimateClass> opdm:isConfiguredBy _:node18vkiok0kx59 .

<http://purl.org/opdm/refrigerator#iceMaker> opdm:isConfiguredBy _:node18vkiok0kx74 .

<http://purl.org/opdm/refrigerator#capableOfACS> opdm:isConfiguredBy _:node18vkiok0kx78 .

_:node18vkiok0kx80 opdm:exampleOfUsage "The value of this property is an individual of the gr:QuantitativeValue class."^^<http://www.w3.org/2001/XMLSchema#string> ;
	opdm:attributePosition "0"^^<http://www.w3.org/2001/XMLSchema#integer> ;
	opdm:inProfile opdm:DefaultProfile ;
	opdm:priority "0"^^<http://www.w3.org/2001/XMLSchema#integer> ;
	a opdm:MetadataContainer ;
	opdm:rankingDirection "DESC"^^<http://www.w3.org/2001/XMLSchema#string> .

<http://purl.org/opdm/refrigerator#numberOfFridgeShelves> opdm:isConfiguredBy _:node18vkiok0kx79 .

_:node18vkiok0kx73 opdm:rankingDirection "DESC"^^<http://www.w3.org/2001/XMLSchema#string> ;
	opdm:priority "0"^^<http://www.w3.org/2001/XMLSchema#integer> ;
	a opdm:MetadataContainer ;
	opdm:attributePosition "0"^^<http://www.w3.org/2001/XMLSchema#integer> ;
	opdm:exampleOfUsage "The value of this property is a boolean (true/false - xsd:boolean)."^^<http://www.w3.org/2001/XMLSchema#string> ;
	opdm:inProfile opdm:DefaultProfile .

<http://purl.org/opdm/refrigerator#numberOfFrontDoors> opdm:recommendedRangeOfMeasure _:node18vkiok0kx63 ;
	opdm:isConfiguredBy _:node18vkiok0kx60 .
