@prefix legal: <http://www.w3.org/ns/legal#> .
@prefix : <http://purl.org/oslo/ns/localgov#> .
@prefix person: <http://www.w3.org/ns/person#> .
@prefix olca: <http://www.lingvoj.org/olca#> .
@prefix vann: <http://purl.org/vocab/vann/> .
@prefix org: <http://www.w3.org/ns/org#> .
@prefix cpsv: <http://purl.org/vocab/cpsv#> .
@prefix dcterms: <http://purl.org/dc/terms/> .
@prefix schema: <http://schema.org/> .
@prefix adms: <http://www.w3.org/ns/adms#> .
@prefix sioc: <http://rdfs.org/sioc/ns#> .
@prefix rdfs: <http://www.w3.org/2000/01/rdf-schema#> .
@prefix time: <http://www.w3.org/2006/time#> .
@prefix ogc: <http://www.opengis.net/rdf#> .
@prefix spin: <http://spinrdf.org/spin#> .
@prefix rdf: <http://www.w3.org/1999/02/22-rdf-syntax-ns#> .
@prefix wdrs: <http://www.w3.org/2007/05/powder-s#> .
@prefix foaf: <http://xmlns.com/foaf/0.1/> .
@prefix locn: <http://www.w3.org/ns/locn#> .
@prefix rov: <http://www.w3.org/ns/regorg#> .
@prefix vcard: <http://www.w3.org/2006/vcard/ns#> .
@prefix voaf: <http://purl.org/vocommons/voaf#> .
@prefix xsd: <http://www.w3.org/2001/XMLSchema#> .
@prefix owl: <http://www.w3.org/2002/07/owl#> .
@prefix xhv: <http://www.w3.org/1999/xhtml/vocab#> .
@prefix skos: <http://www.w3.org/2004/02/skos/core#> .
@prefix cc: <http://creativecommons.org/ns#> .

<http://purl.org/oslo/ns/localgov> a owl:Ontology ;
	vann:preferredNamespaceUri "http://purl.org/oslo/ns/localgov#" ;
	spin:imports <http://topbraid.org/spin/owlrl-all> ;
	rdfs:label "OSLO Exchange Standard"^^xsd:string ;
	xhv:last <http://purl.org/oslo/ns/localgov> ;
	foaf:depiction <http://www.w3.org/ns/Core_Vocabularies_1.0.png> ;
	dcterms:description "This is the RDF encoding of the OSLO Vocabulary developed under the OSLO (Open Standards for Local Administrations) Programme."^^xsd:string ;
	spin:imports <http://topbraid.org/spin/rdfsplus> ;
	dcterms:creator _:node186aoaf8qx1 .

_:node186aoaf8qx1 foaf:name "Laurens De Vocht" ;
	foaf:homepage <http://be.linkedin.com/pub/laurensdv/> ;
	schema:affiliation _:node186aoaf8qx2 .

_:node186aoaf8qx2 foaf:name "Ghent University - iMinds - Multimedialab" .

<http://purl.org/oslo/ns/localgov> dcterms:rights "Copyright © 2013 V-ICT-OR." ;
	dcterms:conformsTo <https://joinup.ec.europa.eu/elibrary/document/isa-deliverable-process-and-methodology-developing-core-vocabularies> .

<https://joinup.ec.europa.eu/elibrary/document/isa-deliverable-process-and-methodology-developing-core-vocabularies> dcterms:title "Process and Methodology for Developing Core Vocabularies" .

<http://purl.org/oslo/ns/localgov> dcterms:modified "2013-09-30Z"^^xsd:date ;
	dcterms:license <https://joinup.ec.europa.eu/category/licence/isa-open-metadata-licence-v11> .

<https://joinup.ec.europa.eu/category/licence/isa-open-metadata-licence-v11> dcterms:title "ISA Open Metadata Licence v1.1" ;
	cc:attributionName "European Commission" ;
	cc:attributionURL <http://ec.europa.eu/> .

<http://purl.org/oslo/ns/localgov> rdfs:comment "This file specifies the set of RDF classes and properties used in the OSLO exchange standard for local administrations in Flanders."^^xsd:string ;
	cc:attributionURL <http://www.v-ict-or.be> ;
	wdrs:describedby <https://joinup.ec.europa.eu/system/files/project/Core_Vocabularies-Business_Location_Person-Specification-v0.3_0.zip> .

<https://joinup.ec.europa.eu/system/files/project/Core_Vocabularies-Business_Location_Person-Specification-v0.3_0.zip> dcterms:title "Person Core Vocabulary" .

<http://purl.org/oslo/ns/localgov> voaf:reliesOn <http://www.opengis.net/rdf#> ;
	foaf:depiction <http://purl.org/oslo/model> ;
	owl:versionInfo "Version 1.0.1 30 September 2013"^^xsd:string ;
	cc:attributionName "V-ICT-OR"^^xsd:string ;
	dcterms:abstract "This version of the OSLO Exchange Standard provides a minimum set of classes and properties for describing a natural person, i.e. the individual as opposed to any role they may play in society or the relationships they have to other people, organisations and property; all of which contribute significantly to the broader concept of identity. The vocabulary is closely integrated with the Person, Organisation and Location Vocabularies published by the W3C in the Gov Linked Data Project."^^xsd:string ;
	voaf:reliesOn <http://purl.org/dc/terms/> ;
	dcterms:relation <http://joinup.ec.europa.eu/asset/core_person/topic/public-comments-core-person-vocabulary-v02> .

<http://joinup.ec.europa.eu/asset/core_person/topic/public-comments-core-person-vocabulary-v02> a sioc:Forum ;
	dcterms:title "Public comments on the Core Person Vocabulary v0.2" .

<http://purl.org/oslo/ns/localgov> foaf:maker _:node186aoaf8qx3 .

_:node186aoaf8qx3 foaf:name "Core Vocabularies Working Group (Business Task Force)" ;
	foaf:page <http://joinup.ec.europa.eu/asset/core_business/home> .

<http://purl.org/oslo/ns/localgov> vann:preferredNamespacePrefix "oslo" , "oslo"@en ;
	a <http://labs.mondeca.com/vocab/voaf#Vocabulary> ;
	dcterms:creator _:node186aoaf8qx4 .

_:node186aoaf8qx4 foaf:name "Raf Buyle" ;
	foaf:homepage <http://be.linkedin.com/pub/raf-buyle/3/86/959/> ;
	schema:affiliation _:node186aoaf8qx5 .

_:node186aoaf8qx5 foaf:name "V-ICT-OR/OSLO" .

<http://purl.org/oslo/ns/localgov> dcterms:rights "Copyright © 2013 V-ICT-OR"^^xsd:string ;
	cc:attributionURL <http://purl.org/oslo> .

:ResidenceObject a rdfs:Class ;
	rdfs:label "ResidenceObject"@en ;
	rdfs:comment "This class represents any object that has an address."@en ;
	vann:usageNote "This is the key class for the Location Core Vocabulary and represents any location that has an address, a building and a parcel."@en ;
	rdfs:isDefinedBy <http://purl.org/oslo/ns/localgov> ;
	rdfs:subClassOf dcterms:Location .

dcterms:Location a rdfs:Class .

:ResidenceObject dcterms:identifier "oslo:ResidenceObject" .

:ExtendedAddress a rdfs:Class ;
	rdfs:label "ExtendedAddress"@en ;
	rdfs:comment "An \"address representation\" as defined in the <a xmlns=\"http://purl.org/oslo/ns/localgov#\" href=\"https://inspire-twg.jrc.ec.europa.eu/inspire-fc.html#_C2538\">data specifications</a> of the EU INSPIRE Directive. The <a xmlns=\"http://purl.org/oslo/ns/localgov#\" href=\"#locn:addressId\">locn:addressId</a> property may be used to link this Address to other representations. This address extends the address with additional information"^^rdf:XMLLiteral ;
	rdfs:isDefinedBy <http://purl.org/oslo/ns/localgov> ;
	wdrs:describedby <https://joinup.ec.europa.eu/system/files/project/Core_Vocabularies-Business_Location_Person-Specification-v0.3_0.zip> ;
	dcterms:identifier "oslo:ExtendedAddress" ;
	rdfs:subClassOf locn:Address .

locn:Address a rdfs:Class .

adms:Identifier a rdfs:Class ;
	rdfs:label "Identifier"@en ;
	rdfs:comment "The ADMS class of Identifier fully represents the Business Core Vocabulary term of the same name"@en ;
	vann:usageNote """<p xmlns=\"http://purl.org/oslo/ns/localgov#\">The Identifier class represents any identifier issued by any authority, whether a 
      government agency or not. It captures the identifier itself and details of the issuing authority, 
      the date on which the identifier was issued and so on.</p>
      <p xmlns=\"http://purl.org/oslo/ns/localgov#\">This class is based on the UN/CEFACT Identifier complex type defined in See Section 5.8 of 
        <a xmlns=\"http://purl.org/oslo/ns/localgov#\" href=\"http://www.unece.org/fileadmin/DAM/cefact/codesfortrade/CCTS/CCTS-DTCatalogueVersion3p1.pdf\">Core Components Data Type Catalogue Version 3.1</a></p>
      <p xmlns=\"http://purl.org/oslo/ns/localgov#\">The various conceptual properties can be fulfilled as follows:</p><ul xmlns=\"http://purl.org/oslo/ns/localgov#\">
        <li xmlns=\"http://purl.org/oslo/ns/localgov#\">use <a xmlns=\"http://purl.org/oslo/ns/localgov#\" href=\"http://www.w3.org/2004/02/skos/core##notation\">skos:notation</a> to provide the actual identifier (the 
          Identifier class is effectively meaningless without this property and conceptually it is mandatory);</li>
        <li xmlns=\"http://purl.org/oslo/ns/localgov#\">use <a xmlns=\"http://purl.org/oslo/ns/localgov#\" href=\"http://purl.org/dc/terms/type\">dcterms:type</a> to provide an identifier for the type of identifier issued;</li>
        <li xmlns=\"http://purl.org/oslo/ns/localgov#\">use <a xmlns=\"http://purl.org/oslo/ns/localgov#\" href=\"http://purl.org/dc/terms/created\">dcterms:created</a> to provide the date on which the identifier was issued.</li>
        <li xmlns=\"http://purl.org/oslo/ns/localgov#\">use <a xmlns=\"http://purl.org/oslo/ns/localgov#\" href=\"#schemeagency\">adms:schemeAgency</a> to provide the name of the agency that created the identifier (as an rdfs:Literal).</li>
        <li xmlns=\"http://purl.org/oslo/ns/localgov#\">use <a xmlns=\"http://purl.org/oslo/ns/localgov#\" href=\"http://purl.org/dc/terms/creator\">dcterms:creator</a> to link to a URI of an Agent class describing the issuing Agency;</li></ul>"""^^rdf:XMLLiteral ;
	rdfs:isDefinedBy <http://www.w3.org/ns/legal#> ;
	dcterms:identifier "adms:Identifier" .

dcterms:Location rdfs:label "Location"@en ;
	rdfs:comment "dcterms:Location class fully represents the Location Core Vocabulary class of Location."@en ;
	vann:usageNote "This is the key class for the Location Core Vocabulary and represents any location, irrespective of size or other restriction."@en ;
	rdfs:isDefinedBy <http://purl.org/dc/terms/> ;
	dcterms:identifier "dcterms:Location" .

:Membership a rdfs:Class ;
	dcterms:identifier "oslo:Membership" ;
	rdfs:subClassOf org:Membership ;
	rdfs:isDefinedBy <http://purl.org/oslo/ns/localgov> ;
	rdfs:comment """This is the key class for the Business Core Vocabulary and represents a 
    business that is legally registered. In many countries there is a single registry although in others, 
    such as Spain and Germany, multiple registries exist. A Legal Entity is able to trade, is 
    legally liable for its actions, accounts, tax affairs etc. It is a sub class of org:FormalOrganization
    which covers a wider range of entities, such as charities."""@en ;
	rdfs:label "Membership"@en .

locn:Geometry a rdfs:Class ;
	rdfs:label "Geometry"@en ;
	rdfs:comment "The Geometry Class provides the means to identify a Location as a point, line, polygon, etc. expressed using coordinates in some coordinate reference system."@en ;
	vann:usageNote """This class defines the notion of \"geometry\" at the conceptual level, and it shall be encoded by using different formats. For interoperability reasons, it is recommended using one of the following:
      <ul xmlns=\"http://purl.org/oslo/ns/localgov#\">
        <li xmlns=\"http://purl.org/oslo/ns/localgov#\"><p xmlns=\"http://purl.org/oslo/ns/localgov#\">Any geometry:</p>
          <ul xmlns=\"http://purl.org/oslo/ns/localgov#\">
            <li xmlns=\"http://purl.org/oslo/ns/localgov#\">WKT, GML, and RDF+WKT/GML, as per the <a xmlns=\"http://purl.org/oslo/ns/localgov#\" href=\"http://www.w3.org/2011/02/GeoSPARQL.pdf\">GeoSPARQL specification</a>.</li>
            <li xmlns=\"http://purl.org/oslo/ns/localgov#\"><a xmlns=\"http://purl.org/oslo/ns/localgov#\" href=\"http://www.opengeospatial.org/standards/kml\">KML (Keyhole Markup Language)</a> - note that KML supports the following geometries only: point, line string, linear ring, and polygon.</li>
            <li xmlns=\"http://purl.org/oslo/ns/localgov#\">RDF as per the <a xmlns=\"http://purl.org/oslo/ns/localgov#\" href=\"http://schema.org/\">schema.org</a> vocabulary (see classes <a xmlns=\"http://purl.org/oslo/ns/localgov#\" href=\"http://schema.org/GeoCoordinates\">schema:GeoCoordinates</a> and <a xmlns=\"http://purl.org/oslo/ns/localgov#\" href=\"http://schema.org/GeoShape\">schema:GeoShape</a>).</li>
          </ul>
        </li>
        <li xmlns=\"http://purl.org/oslo/ns/localgov#\"><p xmlns=\"http://purl.org/oslo/ns/localgov#\">Points: one of the above, or:</p>
          <ul xmlns=\"http://purl.org/oslo/ns/localgov#\">
            <li xmlns=\"http://purl.org/oslo/ns/localgov#\">RDF as per the <a xmlns=\"http://purl.org/oslo/ns/localgov#\" href=\"http://www.w3.org/2003/01/geo/wgs84_pos#\">W3C Basic Geo (WGS84 lat/long) vocabulary</a>.</li>
            <li xmlns=\"http://purl.org/oslo/ns/localgov#\"><a xmlns=\"http://purl.org/oslo/ns/localgov#\" href=\"http://geohash.org/\">GeoHash</a> URI references.</li>
          </ul>
        </li>
      </ul>
    """^^rdf:XMLLiteral ;
	rdfs:isDefinedBy <http://www.w3.org/ns/locn#> ;
	dcterms:identifier "locn:Geometry" .

_:node186aoaf8qx6 a rdfs:Class ;
	dcterms:identifier "oslo:ResidenceObject" ;
	rdfs:subClassOf locn:location .

locn:location a rdf:Property .

_:node186aoaf8qx6 rdfs:comment """This is the key class for the OSLO Location Vocabulary and represents a 
      location that is linked with an address and/or a building with parcel(s)."""@en ;
	rdfs:label "Residence Object"@en ;
	rdfs:ID "ResidenceObject" .

:BasicAddress a rdfs:Class ;
	wdrs:describedby <https://joinup.ec.europa.eu/system/files/project/Core_Vocabularies-Business_Location_Person-Specification-v0.3_0.zip> ;
	rdfs:isDefinedBy <http://purl.org/oslo/ns/localgov> ;
	rdfs:label "BasicAddress"@en ;
	rdfs:comment "An \"address representation\" as defined in the <a xmlns=\"http://purl.org/oslo/ns/localgov#\" href=\"https://inspire-twg.jrc.ec.europa.eu/inspire-fc.html#_C2538\">data specifications</a> of the EU INSPIRE Directive. The <a xmlns=\"http://purl.org/oslo/ns/localgov#\" href=\"#locn:addressId\">locn:addressId</a> property may be used to link this Address to other representations. This address extends the address with additional information"^^rdf:XMLLiteral ;
	dcterms:identifier "oslo:BasicAddress" ;
	rdfs:subClassOf locn:Address .

:Organization a rdfs:Class ;
	dcterms:identifier "oslo:Organization" ;
	rdfs:subClassOf legal:LegalEntity , rov:RegisteredOrganization ;
	rdfs:isDefinedBy <http://purl.org/oslo/ns/localgov> ;
	rdfs:comment """This is the key class for the Business Core Vocabulary and represents a 
    business that is legally registered. In many countries there is a single registry although in others, 
    such as Spain and Germany, multiple registries exist. A Legal Entity is able to trade, is 
    legally liable for its actions, accounts, tax affairs etc. It is a sub class of org:FormalOrganization
    which covers a wider range of entities, such as charities."""@en ;
	rdfs:label "Organization"@en .

:Parcel a rdfs:Class ;
	rdfs:label "Parcel"@en ;
	rdfs:comment "Information related to a Parcel Address or Label"@en ;
	vann:usageNote "Use this class to contain the parcels in."@en ;
	rdfs:isDefinedBy <http://purl.org/oslo/ns/localgov> ;
	rdfs:subClassOf vcard:Parcel ;
	dcterms:identifier "oslo:Parcel" .

locn:Address rdfs:label "Address"@en ;
	rdfs:comment "An \"address representation\" as defined in the <a xmlns=\"http://purl.org/oslo/ns/localgov#\" href=\"https://inspire-twg.jrc.ec.europa.eu/inspire-fc.html#_C2538\">data specifications</a> of the EU INSPIRE Directive. The <a xmlns=\"http://purl.org/oslo/ns/localgov#\" href=\"#locn:addressId\">locn:addressId</a> property may be used to link this Address to other representations."^^rdf:XMLLiteral ;
	rdfs:isDefinedBy <http://www.w3.org/ns/locn#> ;
	wdrs:describedby <https://joinup.ec.europa.eu/system/files/project/Core_Vocabularies-Business_Location_Person-Specification-v0.3_0.zip> ;
	dcterms:identifier "locn:Address" .

:Building a rdfs:Class ;
	rdfs:label "Building"@en ;
	rdfs:comment "Information related to a Building"@en ;
	vann:usageNote "Use this class to represent information about a building."@en ;
	rdfs:isDefinedBy <http://purl.org/oslo/ns/localgov> ;
	rdfs:subClassOf owl:Thing ;
	dcterms:identifier "oslo:Building" .

:Code a rdfs:Class ;
	rdfs:label "Code"@en ;
	rdfs:comment """<p xmlns=\"http://purl.org/oslo/ns/localgov#\">The Conceptual Model includes a 'Code' datatype that 
      is used for the types of relation and membership properties. This is expressed using the <a xmlns=\"http://purl.org/oslo/ns/localgov#\" href=\"http://www.w3.org/TR/skos-primer/\">SKOS vocabulary</a> with
      a particular 'code' usually being a oslo:Code which is a skos:Concept that is part of a scheme. 
      The intention is that the oslo:Code class be used as follows;</p><ul xmlns=\"http://purl.org/oslo/ns/localgov#\">
        <li xmlns=\"http://purl.org/oslo/ns/localgov#\">for the content property, use skos:notation</li>
        <li xmlns=\"http://purl.org/oslo/ns/localgov#\">the 'list' property will be taken care of by means of the skos:inScheme property;</li>
        <li xmlns=\"http://purl.org/oslo/ns/localgov#\">the list agency property is likely to be applied to the scheme as a whole for which dcterms:creator is appropriate;</li>
        <li xmlns=\"http://purl.org/oslo/ns/localgov#\">the list version property can be fulfilled using schema:version (see <a xmlns=\"http://purl.org/oslo/ns/localgov#\" href=\"http://schema.org/CreativeWork\">http://schema.org/CreativeWork</a>)</li></ul>
    """^^rdf:XMLLiteral ;
	rdfs:isDefinedBy <http://www.w3.org/TR/skos-primer/> ;
	rdfs:subClassOf skos:Concept ;
	dcterms:identifier "oslo:Code" .

person:Person a rdfs:Class ;
	rdfs:label "Person"@en ;
	rdfs:comment """An individual person who may be dead or alive, 
    but not imaginary. It is that restriction that makes person:Person a
    sub class of both foaf:Person and schema:Person which both cover imaginary
    characters as well as real people."""@en ;
	rdfs:isDefinedBy <http://www.w3.org/ns/person#> ;
	rdfs:subClassOf foaf:Person , schema:Person ;
	dcterms:identifier "person:Person" .

cpsv:PublicService a owl:Class ;
	rdfs:comment "This class represents the service itself. As noted in the scope (section 1.4), a public service is the capacity to carry out a procedure and exists whether it is used or not. It is a set of deeds and acts performed by or on behalf of a public agency for the benefit of a citizen, a business or another public agency."@en ;
	rdfs:label "Public Service"@en ;
	a rdfs:Class .

cpsv:Input a owl:Class ;
	rdfs:comment "Inputs can by any resource - document, artefact - anything. In a specific context it is likely to be useful to either define a sub class or declare the particular resource to also be of another type as well. A general case might be a foaf:Document but where possible, it is better to refer to a controlled vocabulary of types. dcterms:type should be used to use to provide this information linking to a SKOS Concept."@en ;
	rdfs:label "Input"@en ;
	a rdfs:Class .

cpsv:Output a owl:Class ;
	rdfs:comment "Outputs can by any resource - document, artefact - anything. In a specific context it is likely to be useful to either define a sub class or declare the particular resource to also be of another type as well. A general case might be a foaf:Document but where possible, it is better to refer to a controlled vocabulary of types. dcterms:type should be used to use to provide this information linking to a SKOS Concept."@en ;
	rdfs:label "Output"@en ;
	a rdfs:Class .

:Permission a owl:Class ;
	dcterms:identifier "oslo:Permission" ;
	rdfs:comment "Denotes a the permission of a role. Should be linked with a formal rule."@en ;
	rdfs:isDefinedBy <http://purl.org/oslo/ns/localgov> ;
	rdfs:label "Permission"@en ;
	a rdfs:Class .

:PersonRelation a owl:Class ;
	dcterms:identifier "oslo:PersonRelation" ;
	rdfs:comment "A relation between two persons"@en ;
	rdfs:subClassOf :Relation .

:Relation a owl:Class .

:PersonRelation rdfs:isDefinedBy <http://purl.org/oslo/ns/localgov> ;
	rdfs:label "PersonRelation"@en ;
	a rdfs:Class .

:Role a owl:Class ;
	dcterms:identifier "oslo:Role" ;
	rdfs:comment "Denotes a role that a Person or other Agent can take in an public service. Instances of this class describe the abstract role; to denote a specific instance of a person playing that role in a specific public service use an instance of `Permission` that is linked with the formal rules `Rule`."@en ;
	rdfs:isDefinedBy <http://purl.org/oslo/ns/localgov> ;
	rdfs:label "Role"@en ;
	a rdfs:Class .

:Status a owl:Class ;
	dcterms:identifier "oslo:Status" ;
	rdfs:comment "Status of Public Service"@en ;
	rdfs:isDefinedBy <http://purl.org/oslo/ns/localgov> ;
	rdfs:label "Status"@en ;
	a rdfs:Class .

cpsv:Rule a owl:Class ;
	rdfs:comment "The Rule class represents the specific rules, guidelines or procedures that the Public Service follows. Instances of the Rule class are FRBR Expressions, that is, a concrete expression, such as a document, of the more abstract concept of the rules themselves."@en ;
	rdfs:label "Rule"@en ;
	rdfs:subClassOf <http://purl.org/vocab/frbr/core#Expression> ;
	a rdfs:Class .

:Relation dcterms:identifier "oslo:Relation" ;
	rdfs:comment "A relation between two agents"@en ;
	rdfs:isDefinedBy <http://purl.org/oslo/ns/localgov> ;
	rdfs:label "Relation"@en ;
	a rdfs:Class .

:OrganizationRelation a owl:Class ;
	dcterms:identifier "oslo:OrganizationRelation" ;
	rdfs:comment "A relation between two organizations"@en ;
	rdfs:subClassOf :Relation ;
	rdfs:isDefinedBy <http://purl.org/oslo/ns/localgov> ;
	rdfs:label "OrganizationnRelation"@en ;
	a rdfs:Class .

rov:registration a owl:ObjectProperty ;
	dcterms:identifier "rov:registration" ;
	rdfs:subPropertyOf adms:identifier ;
	rdfs:domain rov:RegisteredOrganization ;
	rdfs:isDefinedBy <http://www.w3.org/ns/regorg#> ;
	rdfs:comment """The legal status of a registered organization is conferred on it by an authority within a given 
      jurisdiction. The registration is therefore a fundamental relationship between a the organization and the authority with 
      which it is registered. The details of the registration are provided as properties of the Identifier class which is 
      defined by ADMS. The vocabulary sets no restriction on the type of legal identifier. In many countries, the business register's 
      identifier is the relevant data point. The tax number often fulfils this function in Spain and elsewhere.
      Although there is no formal cardinality constraint on any property in the Registered Organization Vocabulary, it is 
      questionable whether a description of a registered organization without this property and an associated Identifier class will 
      be of any value."""@en ;
	rdfs:label "registration"@en ;
	a rdf:Property .

rov:companyStatus a owl:ObjectProperty ;
	dcterms:identifier "rov:companyStatus" ;
	rdfs:subPropertyOf org:classification ;
	rdfs:isDefinedBy <http://www.w3.org/TR/vocab-regorg/> ;
	rdfs:comment """Terms like insolvent, bankrupt and in receivership are likely to have 
      different legal implications in different jurisdictions. Best Practice for recording various 
      other status levels is to use the relevant jurisdiction's terms and to do so in a 
      consistent manner using a SKOS Concept Scheme. rov:companyStatus is a sub class of org:classification
      which has a range of skos:Concept."""@en ;
	rdfs:label "company status"@en ;
	a rdf:Property .

cpsv:produces a owl:ObjectProperty ;
	rdfs:range cpsv:Output ;
	rdfs:comment "The produces property links a Public Service to one or more instances of the Output class which is its range."@en ;
	rdfs:label "produces"@en ;
	a rdf:Property .

org:member a owl:ObjectProperty ;
	rdfs:label "member"@en , "membre"@fr ;
	a owl:FunctionalProperty ;
	rdfs:range foaf:Agent ;
	owl:inverseOf org:hasMembership .

org:hasMembership a owl:ObjectProperty .

org:member rdfs:comment "Indicates the Person (or other Agent including Organization) involved in the Membership relationship. Inverse of `org:hasMembership`"@en ;
	rdfs:isDefinedBy <http://www.w3.org/ns/org> ;
	rdfs:domain org:Membership ;
	a rdf:Property ;
	rdfs:comment "Indique une personne (ou tout autre Agent, y compris une Organisation) impliqué dans la relation d'Engagement. Inverse de `org:hasMembership`"@fr .

cpsv:hasInput a owl:ObjectProperty ;
	rdfs:range cpsv:Input ;
	rdfs:comment "The hasInput property links a Public Service to one or more instances of the Input class (see below). A specific service may require the presence of certain inputs or combinations of inputs in order to operate. These should be described in an application profile for a given service."@en ;
	rdfs:label "has input"@en ;
	a rdf:Property .

rov:companyActivity a owl:ObjectProperty ;
	dcterms:identifier "rov:companyActivity" ;
	rdfs:subPropertyOf org:classification ;
	rdfs:isDefinedBy <http://www.w3.org/TR/vocab-regorg/> ;
	rdfs:comment """The activity of a company should be 
      recorded using a controlled vocabulary expressed as a SKOS concept scheme. Several such 
      vocabularies exist, many of which map to the UN's ISIC codes. Where a particular controlled vocabulary is in use 
      within a given context, such as SIC codes in the UK, it is acceptable to use these, however, the preferred 
      choice for European interoperability is NACE. rov:companyActivity is a sub class of org:classification which has a range of skos:Concept."""@en ;
	rdfs:label "company activity"@en ;
	a rdf:Property .

cpsv:follows a owl:ObjectProperty ;
	rdfs:range cpsv:Rule ;
	rdfs:comment "The follows property links a service to the Rule(s) under which it operates."@en ;
	rdfs:label "follows"@en ;
	a rdf:Property .

rov:companyType a owl:ObjectProperty ;
	dcterms:identifier "rov:companyType" ;
	rdfs:subPropertyOf org:classification ;
	rdfs:isDefinedBy <http://www.w3.org/TR/vocab-regorg/> ;
	rdfs:comment """This property records the type of company. Familiar types are SA, PLC, LLC, GmbH etc. Each 
      jurisdiction will have a limited set of recognized company types and these should be used in a consistent manner
      using a SKOS Concept Scheme. rov:companyType is a sub class of org:classification which has a range of skos:Concept."""@en ;
	rdfs:label "company type"@en ;
	a rdf:Property .

:extended_address a rdf:Property ;
	dcterms:identifier "locn:address" ;
	rdfs:range :ExtendedAddress ;
	rdfs:label "extended address"@en ;
	rdfs:isDefinedBy <http://purl.org/oslo/ns/localgov> ;
	rdfs:comment "The oslo:extended_address property relationship associates an <a xmlns=\"http://purl.org/oslo/ns/localgov#\" href=\"#oslo:ExtendedAddress\">Extended Address</a> with a <a xmlns=\"http://purl.org/oslo/ns/localgov#\" href=\"#locn:Address\">Address</a> Class "^^rdf:XMLLiteral ;
	rdfs:domain :BasicAddress .

person:countryOfBirth a rdf:Property ;
	rdfs:label "country of birth"@en ;
	rdfs:comment "The range of country of birth is dcterms:Location and schema:Place."@en ;
	rdfs:range schema:Place , dcterms:Location , locn:Location ;
	rdfs:isDefinedBy <http://www.w3.org/ns/person#> ;
	dcterms:identifier "person:countryOfBirth" .

:validityPeriod a rdf:Property ;
	rdfs:label "validity period"@en ;
	rdfs:comment "Points to a time interval"@en ;
	rdfs:isDefinedBy <http://purl.org/oslo/ns/localgov> ;
	rdfs:range <http://www.w3.org/2006/time#> ;
	dcterms:identifier "oslo:validityPeriod" .

:parcelId a rdf:Property ;
	dcterms:identifier "oslo:parcelId" ;
	rdfs:range adms:Identifier ;
	rdfs:domain :Parcel ;
	rdfs:isDefinedBy <http://purl.org/oslo/ns/localgov> ;
	rdfs:comment "The concept of adding a globally unique identifier for each instance of a parcel is a crucial part of the OSLO data spec. The domain of oslo:parcelId is oslo:Parcel."@en ;
	rdfs:label "parcel ID"@en .

dcterms:identifier a rdf:Property ;
	rdfs:label "identifer"@en ;
	rdfs:comment "dcterms:identifier fully represents the Core Vocabulary property of the same name"@en ;
	vann:usageNote "The identifier relation links a resource to any formally issued identifier for that resource other than one that confers legal status upon it. The range is adms:Identifier."@en ;
	rdfs:isDefinedBy <http://dublincore.org/documents/dcmi-terms/> ;
	dcterms:identifier "dcterms:identifier" ;
	vann:usageNote "The identifier relation is used to link a person to any formally issued identifier for that person."@en .

foaf:givenName a rdf:Property ;
	rdfs:label "given name"@en ;
	rdfs:comment "The foaf:givenName property fully represents the Person Core Vocabulary term of given name"@en ;
	vann:usageNote """A given name, or multiple given names, are the denominator(s) that identify an individual 
    within a family. These are given to a person by his or her parents at birth or may be legally recognised 
    for example, the given name for Johan Sebastian Bach is 'Johan Sebastian.'"""@en ;
	rdfs:isDefinedBy <http://xmlns.com/foaf/spec/> ;
	dcterms:identifier "foaf:givenName" .

:establishmentDate a rdf:Property ;
	rdfs:label "date of establishment"@en ;
	rdfs:comment "Date of establishment of an organization"@en ;
	rdfs:isDefinedBy <http://purl.org/oslo/ns/localgov> ;
	rdfs:domain :Organization ;
	rdfs:range rdfs:Literal ;
	dcterms:identifier "oslo:establishmentDate" .

:country a rdf:Property ;
	rdfs:label "country"@en ;
	rdfs:comment "The uppermost administrative unit for the address, almost always a country. The domain of locn:adminUnitL1 is locn:Address and the range is a literal, conceptually defined by the <a xmlns=\"http://purl.org/oslo/ns/localgov#\" href=\"https://inspire-twg.jrc.ec.europa.eu/inspire-fc.html#_C2612\">INSPIRE Geographical Name data type</a>."^^rdf:XMLLiteral ;
	vann:usageNote "Best practice is to use the ISO 3166-1 code but if this is inappropriate for the context, country names should be provided in a consistent manner to reduce ambiguity. For example, either write 'United Kingdom' or 'UK' consistently throughout the data set and avoid mixing the two."@en ;
	rdfs:isDefinedBy <http://www.w3.org/ns/locn#> ;
	rdfs:domain locn:Address ;
	rdfs:subPropertyOf locn:adminUnitL1 ;
	dcterms:identifier "oslo:country" , "urn:x-inspire:specification:gmlas:BaseTypes:3.2:adminUnit" .

:buildingId a rdf:Property ;
	dcterms:identifier "oslo:buldingId" ;
	rdfs:range adms:Identifier ;
	rdfs:domain :Building ;
	rdfs:isDefinedBy <http://purl.org/oslo/ns/localgov> ;
	rdfs:comment "The concept of adding a globally unique identifier for each instance of a building is a crucial part of the OSLO data spec. The domain of oslo:buildingId is oslo:Building."@en ;
	rdfs:label "building ID"@en .

:nobelityTitle a rdf:Property ;
	rdfs:label "nobelity title"@en ;
	rdfs:comment "Nobelity title of a person"@en ;
	rdfs:isDefinedBy <http://purl.org/oslo/ns/localgov> ;
	rdfs:domain person:Person ;
	rdfs:range rdfs:Literal ;
	dcterms:identifier "oslo:nobelityTitle" .

:civilClass a rdf:Property ;
	rdfs:label "civil classs"@en ;
	rdfs:comment "The range of place of death is a code."@en ;
	rdfs:domain person:Person ;
	rdfs:range :Code ;
	rdfs:isDefinedBy <http://purl.org/oslo/ns/localgov> ;
	dcterms:identifier "oslo:civilClass" .

:function a rdf:Property ;
	rdfs:label "KBO function"@en ;
	rdfs:comment "A KBO Funtion"@en ;
	rdfs:isDefinedBy <http://purl.org/oslo/ns/localgov> ;
	rdfs:domain :Organization ;
	rdfs:range :Code ;
	dcterms:identifier "oslo:function" .

:poBox a rdf:Property ;
	rdfs:label "po box"@en ;
	rdfs:comment "The Post Office Box number. The domain of oslo:poBox is oslo:ExtendedAddress."@en ;
	rdfs:isDefinedBy <http://www.w3.org/ns/locn#> ;
	rdfs:domain :ExtendedAddress ;
	rdfs:range rdfs:Literal ;
	rdfs:subPropertyOf locn:poBox ;
	dcterms:identifier "oslo:poBox" .

:result a rdf:Property ;
	rdfs:label "Public Service Result"@en ;
	rdfs:comment "Result of the public service process."@en ;
	rdfs:isDefinedBy <http://purl.org/oslo/ns/localgov> ;
	rdfs:domain cpsv:PublicService ;
	rdfs:range :Code ;
	dcterms:identifier "oslo:result" .

locn:address a rdf:Property ;
	rdfs:label "address"@en ;
	rdfs:comment "The locn:address property relationship associates any resource with the <a xmlns=\"http://purl.org/oslo/ns/localgov#\" href=\"#locn:Address\">Address</a> Class "^^rdf:XMLLiteral ;
	rdfs:isDefinedBy <http://www.w3.org/ns/locn#> ;
	rdfs:range locn:Address ;
	dcterms:identifier "locn:address" .

:address a rdf:Property ;
	dcterms:identifier "oslo:address" ;
	rdfs:domain :ResidenceObject ;
	rdfs:range :BasicAddress ;
	rdfs:isDefinedBy <http://purl.org/oslo/ns/localgov> ;
	rdfs:comment "Parcel linked to a building or a residence object."@en ;
	rdfs:label "addres"@en .

foaf:name a rdf:Property ;
	rdfs:label "name"@en ;
	rdfs:comment "The foaf:name property fully represents the Person Core Vocabulary term of full name"@en ;
	vann:usageNote """The full name contains the complete name of a person 
    as one string. In addition to the content of given name, family name and, in some 
    systems, patronymic name, this can carry additional parts of a person's name 
    such as titles, middle names or suffixes like \"the third\" or names which are neither 
    a given nor a family name."""@en ;
	rdfs:isDefinedBy <http://xmlns.com/foaf/spec/> ;
	dcterms:identifier "foaf:name" .

:fromPerson a rdf:Property ;
	rdfs:range :Person ;
	rdfs:domain :PersonRelation ;
	rdfs:comment "from relation"@en ;
	rdfs:label "from"@en .

:companyStatus a rdf:Property ;
	rdfs:label "KBO Company status"@en ;
	rdfs:comment "A KBO Company status"@en ;
	rdfs:isDefinedBy <http://purl.org/oslo/ns/localgov> ;
	rdfs:domain :Organization ;
	rdfs:range :Code ;
	dcterms:identifier "oslo:companyStatus" .

:providesRole a rdf:Property ;
	rdfs:range :Role ;
	rdfs:domain cpsv:PublicService ;
	rdfs:comment "This very general property links an Public Service to a Role."@en ;
	rdfs:label "provides role"@en .

:productType a rdf:Property ;
	rdfs:label "type of product"@en ;
	rdfs:comment "Type of a product"@en ;
	rdfs:isDefinedBy <http://purl.org/oslo/ns/localgov> ;
	rdfs:domain :Product ;
	rdfs:range :Code ;
	rdfs:subPropertyOf <http://purl.org/dc/elements/1.1/type> ;
	dcterms:identifier "oslo:productType" .

schema:gender a rdf:Property ;
	rdfs:label "gender"@en ;
	rdfs:comment "The schema:gender property fully represents the Person Core Vocabulary term of the same name."@en ;
	vann:usageNote """The gender of an individual should be recorded using a controlled vocabulary 
    that is appropriate for the specific context. In some cases the chromosomal or physical state of an 
    individual will be more important than the gender that they express, in others the reverse will be true. 
    What is always important is that the controlled vocabulary used to describe an individual's gender 
    is stated explicitly. To do this use a skos:Concept as described in the <a xmlns=\"http://purl.org/oslo/ns/localgov#\" href=\"#skos:Concept\">Code</a> class.
    The <a xmlns=\"http://purl.org/oslo/ns/localgov#\" href=\"https://joinup.ec.europa.eu/system/files/project/Core_Vocabularies-Business_Location_Person-Specification-v0.3_0.zip\">Person Core Vocabulary</a> includes an example of such a SKOS concept scheme."""^^rdf:XMLLiteral ;
	rdfs:isDefinedBy <http://schema.org/docs/schemaorg.owl> ;
	dcterms:identifier "schema:gender" .

:membershipFunction a rdf:Property ;
	rdfs:label "membership function"@en ;
	rdfs:comment "Function label of a membership"@en ;
	rdfs:isDefinedBy <http://purl.org/oslo/ns/localgov> ;
	rdfs:domain :Membership ;
	rdfs:range rdfs:Literal ;
	dcterms:identifier "oslo:membershipFunction" .

person:birthName a rdf:Property ;
	rdfs:label "birth name"@en ;
	rdfs:comment """All data associated with an individual are subject to change. Names can change for 
    a variety of reasons, either formally or informally, and new information may come to light that means that 
    a correction or clarification can be made to an existing record. Birth names tend to be persistent 
    however and for this reason they are recorded by some public sector information systems. There is 
    no granularity for birth name - the full name should be recorded in a single field."""@en ;
	rdfs:isDefinedBy <http://www.w3.org/ns/person#> ;
	dcterms:identifier "person:birthName" .

:statusCode a rdf:Property ;
	rdfs:label "Statuscode"@en ;
	rdfs:comment "Statuscode"@en ;
	rdfs:isDefinedBy <http://purl.org/oslo/ns/localgov> ;
	rdfs:domain :Status ;
	rdfs:range :Code ;
	rdfs:subPropertyOf <http://purl.org/dc/elements/1.1/type> ;
	dcterms:identifier "oslo:statusCode" .

legal:legalIdentifier a rdf:Property ;
	rdfs:label "legal identifer"@en ;
	rdfs:comment """The legal identifier is a fundamental relationship between a legal entity and the 
    authority with which it is registered and that confers legal status upon it. legal:legalIdentifier is 
    a sub property of dcterms:identifier. legal:legalIdentifier has a
    defined domain of legal:LegalEntity and a range of adms:Identifier"""@en ;
	rdfs:isDefinedBy <http://www.w3.org/ns/legal#> ;
	rdfs:domain legal:LegalEntity ;
	rdfs:range adms:Identifier ;
	rdfs:subPropertyOf dcterms:identifier ;
	dcterms:identifier "legal:legalIdentifier" .

:residence a rdf:Property ;
	rdfs:label "residence"@en ;
	rdfs:comment "The range of residence is ResidenceObject."@en ;
	rdfs:range :ResidenceObject ;
	rdfs:domain person:Person ;
	rdfs:isDefinedBy <http://purl.org/oslo/ns/localgov> ;
	dcterms:identifier "oslo:residence" .

legal:companyActivity a rdf:Property ;
	rdfs:label "company activity"@en ;
	rdfs:comment """The activity of a company should be recorded using a controlled vocabulary expressed
    as a SKOS concept scheme (see <a xmlns=\"http://purl.org/oslo/ns/localgov#\" href=\"#skos:Concept\">Code</a>. Several such 
    vocabularies exist, many of which map to the UN's ISIC codes. Where a particular controlled vocabulary is in use 
    within a given context, such as SIC codes in the UK, it is acceptable to use these, however, the preferred 
    choice for European interoperability is NACE."""^^rdf:XMLLiteral ;
	rdfs:isDefinedBy <http://www.w3.org/ns/legal#> ;
	rdfs:subPropertyOf org:classification ;
	rdfs:range skos:Concept ;
	dcterms:identifier "legal:companyActivity" .

person:citizenship a rdf:Property ;
	rdfs:label "citizenship"@en ;
	rdfs:comment "The range of citizenship is dcterms:Jurisdiction."@en ;
	rdfs:range dcterms:Jurisdiction ;
	rdfs:isDefinedBy <http://www.w3.org/ns/person#> ;
	dcterms:identifier "person:citizenship" .

rdfs:seeAlso a rdf:Property ;
	rdfs:label "geographic identifier"@en ;
	rdfs:comment "rdfs:seeAlso fully represents the Location Core Vocabulary concept of a geographic identifier."@en ;
	vann:usageNote """Used in the Location Core vocabulary to provide a URI that identifies the location. 
    This should be expressed using the rdfs:seeAlso property unless the identifier is already the subject of the description. 
    Examples include URIs from <a xmlns=\"http://purl.org/oslo/ns/localgov#\" href=\"http://www.geonames.org/\">GeoNames.org</a> and <a xmlns=\"http://purl.org/oslo/ns/localgov#\" href=\"http://dbpedia.org/\">DBpedia</a> 
    such as http://dbpedia.org/resource/ISO_3166-2:XX where XX is the ISO 3166 two character code for a country."""^^rdf:XMLLiteral ;
	rdfs:isDefinedBy <http://purl.org/oslo/ns/localgov> ;
	dcterms:identifier "rdfs:seeAlso" .

:legalFormCode a rdf:Property ;
	rdfs:label "legal form code"@en ;
	rdfs:comment "A Legal Form Code"@en ;
	rdfs:isDefinedBy <http://purl.org/oslo/ns/localgov> ;
	rdfs:domain :Organization ;
	rdfs:range :Code ;
	rdfs:subPropertyOf rov:companyType ;
	dcterms:identifier "oslo:legalFormCode" .

:hasActor a rdf:Property ;
	olca:rangeIncludes :Membership , :Organization , person:Person ;
	rdfs:domain :Role ;
	rdfs:comment "This very general property links an Public Service to a Role."@en ;
	rdfs:label "provides role"@en .

legal:companyType a rdf:Property ;
	rdfs:label "company type"@en ;
	rdfs:comment """This property records the type of company. Familiar types are SA, PLC, LLC, GmbH etc. Each 
    jurisdiction will have a limited set of recognised company types and these should be used in a consistent manner
    using a oslo:Code as described in the <a xmlns=\"http://purl.org/oslo/ns/localgov#\" href=\"#oslo:Code\">Code</a> Class."""^^rdf:XMLLiteral ;
	rdfs:isDefinedBy <http://www.w3.org/ns/legal#> ;
	rdfs:range :Code ;
	rdfs:subPropertyOf org:classification ;
	dcterms:identifier "legal:companyType" .

:isBranch a rdf:Property ;
	rdfs:label "organization is a branch or not"@en ;
	rdfs:comment "Depicts if organization is branch of another organization"@en ;
	rdfs:isDefinedBy <http://purl.org/oslo/ns/localgov> ;
	rdfs:domain :Organization ;
	rdfs:range rdfs:Literal ;
	dcterms:identifier "oslo:isBranch" .

:locatorName a rdf:Property ;
	rdfs:label "locator name"@en ;
	rdfs:comment "Proper noun(s) applied to the real world entity identified by the locator. The locator name could be the name of the property or complex, of the building or part of the building, or it could be the name of a room inside a building. The domain of oslo:locatorName is oslo:ExtendedAddress."@en ;
	rdfs:isDefinedBy <http://purl.org/oslo/ns/localgov> ;
	rdfs:domain :ExtendedAddress ;
	rdfs:range rdfs:Literal ;
	rdfs:subPropertyOf <http://www.w3.org/ns/locn#locn;locatorName> ;
	dcterms:identifier "oslo:locatorName" .

:functionPhase a rdf:Property ;
	rdfs:label "KBO function phase"@en ;
	rdfs:comment "A KBO Funtionphase"@en ;
	rdfs:isDefinedBy <http://purl.org/oslo/ns/localgov> ;
	rdfs:domain :Organization ;
	rdfs:range :Code ;
	dcterms:identifier "oslo:functionPhase" .

legal:legalEntity a rdf:Property ;
	rdfs:label "legal entity"@en ;
	rdfs:comment "The legal entity relationship can be used to link any resource to a Legal Entity Class. This is useful, for example, where an organisation includes one or more legal entities. The Dublin Core term isPartOf is a suitable inverse of this relationship. legal:legalEntity has a range of legal:LegalEntity."@en ;
	rdfs:isDefinedBy <http://www.w3.org/ns/legal#> ;
	rdfs:range legal:LegalEntity ;
	dcterms:identifier "legal:legalEntity" .

:legalIncompetence a rdf:Property ;
	rdfs:label "legal incompetence"@en ;
	rdfs:comment "Legal Incompetence"@en ;
	rdfs:isDefinedBy <http://purl.org/oslo/ns/localgov> ;
	rdfs:domain person:Person ;
	rdfs:range :Code ;
	dcterms:identifier "oslo:legalIncompetence" .

:hasPermission a rdf:Property ;
	rdfs:range :Permission ;
	rdfs:domain :Role ;
	rdfs:comment "Permission belonging to a Role."@en ;
	rdfs:label "has permission"@en .

:contact a rdf:Property ;
	olca:domainIncludes :Membership , :Organization , person:Person ;
	rdfs:comment "Depicts the contact information for a person, organizaton or membership"@en ;
	rdfs:label "contact information"@en ;
	rdfs:isDefinedBy <http://purl.org/oslo/ns/localgov> ;
	rdfs:range vcard:VCard ;
	dcterms:identifier "oslo:contact" .

legal:registeredAddress a rdf:Property ;
	rdfs:label "registered address"@en ;
	rdfs:comment "Links a Legal Entity to its registered address. This may or may not be the actual address at which the legal entity does its business, it is commonly the address of their lawyer or accountant, but it is the address to which formal communications can be sent. legal:registeredAddress is a sub property of locn:address that has a domain of legal:LegalEntity and a range of locn:Address."@en ;
	rdfs:isDefinedBy <http://www.w3.org/ns/legal#> ;
	rdfs:domain legal:LegalEntity ;
	rdfs:range locn:Address ;
	rdfs:subPropertyOf locn:address ;
	dcterms:identifier "legal:registeredAddress" .

schema:deathDate a rdf:Property ;
	rdfs:label "date of death"@en ;
	rdfs:comment "The schema:deathDate property fully represents the Person Core Vocabulary term of date of death."@en ;
	vann:usageNote """A date that specifies the death date of a person. The date should be 
    provided as a literal and data typed if applicable."""@en ;
	rdfs:isDefinedBy <http://schema.org/docs/schemaorg.owl> ;
	dcterms:identifier "schema:deathDate" .

:addressId a rdf:Property ;
	dcterms:identifier "oslo:addressId" ;
	rdfs:range adms:Identifier ;
	rdfs:domain locn:Address ;
	rdfs:isDefinedBy <http://purl.org/oslo/ns/localgov> ;
	rdfs:comment "The concept of adding a globally unique identifier for each instance of an address is a crucial part of the INSPIRE data spec. The domain of oslo:addressId is locn:Address."@en ;
	rdfs:label "address ID"@en .

:extended_addressId a rdf:Property ;
	dcterms:identifier "oslo:extended_addressId" ;
	rdfs:range adms:Identifier ;
	rdfs:domain :ExtendedAddress ;
	rdfs:isDefinedBy <http://purl.org/oslo/ns/localgov> ;
	rdfs:comment "The concept of adding a globally unique identifier for each instance of an address is a crucial part of the INSPIRE data spec. The domain of oslo:extended_addressId is oslo:ExtendedAddress."@en ;
	rdfs:label "extended address ID"@en .

schema:birthDate a rdf:Property ;
	rdfs:label "date of birth"@en ;
	rdfs:comment "The schema:birthDate property fully represents the Person Core Vocabulary term of date of birth"@en ;
	vann:usageNote """A date that specifies the birth date of a person. The date 
    should be provided as a literal and data typed if applicable."""@en ;
	rdfs:isDefinedBy <http://schema.org/docs/schemaorg.owl> ;
	dcterms:identifier "schema:birthDate" .

:building a rdf:Property ;
	dcterms:identifier "oslo:building" ;
	rdfs:domain :ResidenceObject ;
	rdfs:range :Building ;
	rdfs:isDefinedBy <http://purl.org/oslo/ns/localgov> ;
	rdfs:comment "Building linked to a residence object."@en ;
	rdfs:label "building"@en .

:invoiceLocation a rdf:Property ;
	rdfs:label "invoice location"@en ;
	rdfs:comment "Points to a invoice location"@en ;
	rdfs:isDefinedBy <http://purl.org/oslo/ns/localgov> ;
	rdfs:domain :Organization ;
	rdfs:range :ResidenceObject ;
	rdfs:subPropertyOf rov:registration ;
	dcterms:identifier "oslo:invoiceLocation" .

:targetDate a rdf:Property ;
	rdfs:label "Target date"@en ;
	rdfs:comment "Targetdate for a public service to process its input and produce output"@en ;
	rdfs:isDefinedBy <http://purl.org/oslo/ns/localgov> ;
	rdfs:domain cpsv:PublicService ;
	rdfs:range rdfs:Literal ;
	dcterms:identifier "oslo:targetDate" .

locn:postCode a rdf:Property ;
	rdfs:label "post code"@en ;
	rdfs:comment "The post code (a.k.a postal code, zip code etc.). Post codes are common elements in many countries' postal address systems. The domain of locn:postCode is locn:Address."@en ;
	rdfs:isDefinedBy <http://www.w3.org/ns/locn#> ;
	rdfs:domain locn:Address ;
	rdfs:range rdfs:Literal ;
	dcterms:identifier "locn:postCode" .

locn:geographicName a rdf:Property ;
	rdfs:label "geographic name"@en ;
	rdfs:comment """<p xmlns=\"http://purl.org/oslo/ns/localgov#\">A geographic name is a proper noun applied to a spatial object. Taking the example used in the <a xmlns=\"http://purl.org/oslo/ns/localgov#\" href=\"http://inspire.jrc.ec.europa.eu/documents/Data_Specifications/INSPIRE_DataSpecification_GN_v3.0.1.pdf\">INSPIRE document</a> (page 18), the following are all valid geographic names for the Greek capital:</p>
    <ul xmlns=\"http://purl.org/oslo/ns/localgov#\"><li xmlns=\"http://purl.org/oslo/ns/localgov#\">A?n?a (the Greek endonym written in the Greek script)</li><li xmlns=\"http://purl.org/oslo/ns/localgov#\">Athina (the standard Romanisation of the endonym)</li><li xmlns=\"http://purl.org/oslo/ns/localgov#\">Athens (the English language exonym)</li></ul>
    <p xmlns=\"http://purl.org/oslo/ns/localgov#\">For INSPIRE-conformant data, provide the metadata for the geographic name using a skos:Concept as a datatype.</p>"""^^rdf:XMLLiteral ;
	rdfs:isDefinedBy <http://www.w3.org/ns/locn#> ;
	wdrs:describedby <https://joinup.ec.europa.eu/system/files/project/Core_Vocabularies-Business_Location_Person-Specification-v0.3_0.zip> ;
	rdfs:domain dcterms:Location ;
	rdfs:range rdf:Literal ;
	dcterms:identifier "locn:geographicName" .

person:patronymicName a rdf:Property ;
	rdfs:label "patronymic name"@en ;
	rdfs:comment """Patronymic names are important in some countries. Iceland 
    does not have a concept of family name in the way that many other European countries 
    do, for example. In Bulgaria and Russia, patronymic names are in every day usage, 
    for example, the \"Sergeyevich\" (?????????) in \"Mikhail Sergeyevich Gorbachev\" 
    (?????? ????????? ????????)."""@en ;
	rdfs:isDefinedBy <http://www.w3.org/ns/person#> ;
	dcterms:identifier "person:patronymicName" .

:mailingLocation a rdf:Property ;
	olca:domainIncludes :Membership , :Organization ;
	rdfs:isDefinedBy <http://purl.org/oslo/ns/localgov> ;
	rdfs:label "mailing location"@en ;
	rdfs:comment "Points to a mailing location"@en ;
	rdfs:range :ResidenceObject ;
	dcterms:identifier "oslo:mailingLocation" .

:reasonShutDown a rdf:Property ;
	rdfs:label "reason shutdown"@en ;
	rdfs:comment "Reason for shutdown of an organization"@en ;
	rdfs:isDefinedBy <http://purl.org/oslo/ns/localgov> ;
	rdfs:domain :Organization ;
	rdfs:range rdfs:Literal ;
	dcterms:identifier "oslo:reasonShutDown" .

:toPerson a rdf:Property ;
	rdfs:range :Person ;
	rdfs:domain :PersonRelation ;
	rdfs:comment "to relation"@en ;
	rdfs:label "to"@en .

:deliveryLocation a rdf:Property ;
	rdfs:label "delivery location"@en ;
	rdfs:comment "Points to a delivery location"@en ;
	rdfs:isDefinedBy <http://purl.org/oslo/ns/localgov> ;
	rdfs:domain :Organization ;
	rdfs:range :ResidenceObject ;
	rdfs:subPropertyOf rov:registration ;
	dcterms:identifier "oslo:deliveryLocation" .

legal:companyStatus a rdf:Property ;
	rdfs:label "company status"@en ;
	rdfs:comment """Terms like insolvent, bankrupt and in receivership are likely to have 
    different legal implications in different jurisdictions. Best Practice for recording various 
    other status levels is to use the relevant jurisdiction's terms and to do so in a 
    consistent manner using a oslo:Code as described in the <a xmlns=\"http://purl.org/oslo/ns/localgov#\" href=\"#oslo:Code\">Code</a> Class. 
    The term \"Normal Activity\" appears to have cross-border usefulness 
    and this should be used in preference to terms like trading or operating."""^^rdf:XMLLiteral ;
	rdfs:isDefinedBy <http://www.w3.org/ns/legal#> ;
	rdfs:range <http://purl.org/oslo/ns/Code> ;
	rdfs:subPropertyOf org:classification ;
	dcterms:identifier "legal:companyStatus" .

:locatorDesignator a rdf:Property ;
	dcterms:identifier "oslo:locatorDesignator" ;
	rdfs:subPropertyOf locn:locatorDesignator ;
	rdfs:range rdfs:Literal ;
	rdfs:domain :ExtendedAddress ;
	rdfs:isDefinedBy <http://purl.org/oslo/ns/localgov> ;
	rdfs:comment "A number or a sequence of characters that uniquely identifies the locator within the relevant scope(s). The full identification of the locator could include one or more locator designators. The domain of oslo:locatorDesignator is oslo:Address."@en ;
	rdfs:label "locator designator"@en .

person:placeOfDeath a rdf:Property ;
	rdfs:label "place of death"@en ;
	rdfs:comment "The range of place of death is dcterms:Location and schema:Place."@en ;
	rdfs:range schema:Place , dcterms:Location ;
	rdfs:isDefinedBy <http://www.w3.org/ns/person#> ;
	dcterms:identifier "person:placeOfDeath" .

:status a rdf:Property ;
	rdfs:label "Public Service Status"@en ;
	rdfs:comment "Status of the public service process."@en ;
	rdfs:isDefinedBy <http://purl.org/oslo/ns/localgov> ;
	rdfs:domain cpsv:PublicService ;
	rdfs:range :Status ;
	dcterms:identifier "oslo:result" .

:toOrganization a rdf:Property ;
	rdfs:range :Organization ;
	rdfs:domain :OrganizationRelation ;
	rdfs:comment "to relation"@en ;
	rdfs:label "to"@en .

:kind a rdf:Property ;
	rdfs:label "kind"@en ;
	rdfs:comment "Kind of organization, natural person or legal person"@en ;
	rdfs:isDefinedBy <http://purl.org/oslo/ns/localgov> ;
	rdfs:domain :Organization ;
	rdfs:range rdfs:Literal ;
	dcterms:identifier "oslo:kind" .

:adminUnit a rdf:Property ;
	dcterms:identifier "oslo:adminUnit" ;
	rdfs:domain :BasicAddress ;
	rdfs:range :Code ;
	rdfs:isDefinedBy <http://purl.org/oslo/ns/localgov> ;
	rdfs:comment "Admin Unit linked to an address"@en ;
	rdfs:label "Administrative Unit"@en .

person:placeOfBirth a rdf:Property ;
	rdfs:label "place of birth"@en ;
	rdfs:comment "The range of place of birth is dcterms:Location and schema:Place."@en ;
	rdfs:range schema:Place , dcterms:Location ;
	rdfs:isDefinedBy <http://www.w3.org/ns/person#> ;
	dcterms:identifier "person:placeOfBirth" .

:fullAddress a rdf:Property ;
	rdfs:label "full address"@en ;
	rdfs:comment "The complete address written as a string, with or without formatting. The domain of locn:fullAddress is locn:Address."@en ;
	rdfs:isDefinedBy <http://www.w3.org/ns/locn#> ;
	rdfs:domain :ExtendedAddress ;
	rdfs:range rdfs:Literal ;
	rdfs:subPropertyOf locn:fullAddress ;
	dcterms:identifier "oslo:fullAddress" .

locn:location rdfs:label "location"@en ;
	rdfs:comment """The location property links any resource to the Location Class. 
    Asserting the location relationship implies only that the domain has some connection to a 
    Location in time or space. It does not imply that the resource is necessarily at that location 
    at the time when the assertion is made."""@en ;
	rdfs:isDefinedBy <http://www.w3.org/ns/locn#> ;
	rdfs:range dcterms:Location ;
	dcterms:identifier "locn:location" .

foaf:familyName a rdf:Property ;
	rdfs:label "family name"@en ;
	rdfs:comment "The foaf:familyName property fully represents the Person Core Vocabulary term of family name"@en ;
	vann:usageNote "A family name is usually shared by members of a family. This attribute also carries prefixes or suffixes which are part of the Family Name, e.g. \"de Boer\", \"van de Putte\", \"von und zu Orlow\". Multiple family names, such as are commonly found in Hispanic countries, are recorded in the single Family Name field so that, for example, Miguel de Cervantes Saavedra's Family Name would be recorded as \"Cervantes Saavedra.\""@en ;
	rdfs:isDefinedBy <http://xmlns.com/foaf/spec/> ;
	dcterms:identifier "foaf:familyName" .

:locatorNumber a rdf:Property ;
	rdfs:label "locator number"@en ;
	rdfs:comment "A number or a sequence of characters that uniquely identifies the locator within the relevant scope(s). This is typically an identification for the locator in the thoroughfare (most of the times a street or square)."@en ;
	rdfs:isDefinedBy <http://purl.org/oslo/ns/localgov> ;
	rdfs:domain locn:Address ;
	rdfs:range rdfs:Literal ;
	rdfs:subPropertyOf locn:locatorDesignator ;
	dcterms:identifier "oslo:locatorNumber" .

locn:postName a rdf:Property ;
	rdfs:label "post name"@en ;
	rdfs:comment "The key postal division of the address, usually the city. (INSPIRE's definition is \"One or more names created and maintained for postal purposes to identify a subdivision of addresses and postal delivery points.\") The domain of locn:postName is locn:Address."@en ;
	rdfs:isDefinedBy <http://www.w3.org/ns/locn#> ;
	rdfs:domain locn:Address ;
	rdfs:range rdfs:Literal ;
	dcterms:identifier "locn:postName" .

locn:thoroughfare a rdf:Property ;
	rdfs:label "thoroughfare"@en ;
	rdfs:comment "An address component that represents the name of a passage or way through from one location to another. A thoroughfare is not necessarily a road, it might be a waterway or some other feature. The domain of locn:thoroughfare is locn:Address."@en ;
	rdfs:isDefinedBy <http://www.w3.org/ns/locn#> ;
	rdfs:domain locn:Address ;
	rdfs:range rdfs:Literal ;
	dcterms:identifier "locn:thoroughfare" .

:shutDownDate a rdf:Property ;
	rdfs:label "date of shutdown"@en ;
	rdfs:comment "Date of shutdown of an organization"@en ;
	rdfs:isDefinedBy <http://purl.org/oslo/ns/localgov> ;
	rdfs:domain :Organization ;
	rdfs:range rdfs:Literal ;
	dcterms:identifier "oslo:shutDownDate" .

:statusType a rdf:Property ;
	rdfs:label "type of status"@en ;
	rdfs:comment "Type of a status"@en ;
	rdfs:isDefinedBy <http://purl.org/oslo/ns/localgov> ;
	rdfs:domain :Status ;
	rdfs:range :Code ;
	rdfs:subPropertyOf <http://purl.org/dc/elements/1.1/type> ;
	dcterms:identifier "oslo:statusType" .

:parcel a rdf:Property ;
	olca:domainIncludes :Building , :ResidenceObject ;
	dcterms:identifier "oslo:parcel" ;
	rdfs:range :Parcel ;
	rdfs:isDefinedBy <http://purl.org/oslo/ns/localgov> ;
	rdfs:comment "Parcel linked to a building or a residence object."@en ;
	rdfs:label "parcel"@en .

:fromOrganization a rdf:Property ;
	rdfs:range :Person ;
	rdfs:domain :OrganizationRelation ;
	rdfs:comment "from relation"@en ;
	rdfs:label "from"@en .

:addressArea a rdf:Property ;
	rdfs:label "address area"@en ;
	rdfs:comment "The name or names of a geographic area or locality that groups a number of addressable objects for addressing purposes, without being an administrative unit. This would typically be part of a city, a neighbourhood or village. The domain of oslo:addressArea is oslo:Address."@en ;
	rdfs:isDefinedBy <http://purl.org/oslo/ns/localgov> ;
	rdfs:domain :ExtendedAddress ;
	rdfs:range rdfs:Literal ;
	rdfs:subPropertyOf locn:addressArea ;
	dcterms:identifier "oslo:addressArea" .

:availableAt a rdf:Property ;
	rdfs:label "availableAt"@en ;
	rdfs:comment "Points to a residence"@en ;
	rdfs:isDefinedBy <http://purl.org/oslo/ns/localgov> ;
	rdfs:domain :Membership ;
	rdfs:range :ResidenceObject ;
	rdfs:subPropertyOf rov:registration ;
	dcterms:identifier "oslo:availableAt" .

locn:geometry a rdf:Property ;
	rdfs:comment "Associates any <a xmlns=\"http://purl.org/oslo/ns/localgov#\" href=\"#dcterms:Location\">Location</a> with the locn:Geometry class."^^rdf:XMLLiteral ;
	dcterms:identifier "locn:geometry" ;
	rdfs:domain :Building , dcterms:Location ;
	rdfs:label "geometry"@en ;
	rdfs:range locn:Geometry ;
	rdfs:isDefinedBy <http://www.w3.org/ns/locn#> ;
	vann:usageNote "\n      <p xmlns=\"http://purl.org/oslo/ns/localgov#\">Depending on how a geometry is encoded (see usage note of the <a xmlns=\"http://purl.org/oslo/ns/localgov#\" href=\"#locn:Geometry\">locn:Geometry</a> class), the range of this property may be either a literal (e.g., WKT - string literal -, GML, KML - XML literal) or a geometry class, as those defined in the OGC's <a xmlns=\"http://purl.org/oslo/ns/localgov#\" href=\"http://www.w3.org/2011/02/GeoSPARQL.pdf\">GeoSPARQL specification</a>, in the W3C's <a xmlns=\"http://purl.org/oslo/ns/localgov#\" href=\"http://www.w3.org/2003/01/geo/wgs84_pos#\">Basic Geo (WGS84 lat/long) vocabulary</a>, and at <a xmlns=\"http://purl.org/oslo/ns/localgov#\" href=\"http://schema.org/\">schema.org</a>, or even the <a xmlns=\"http://purl.org/oslo/ns/localgov#\" href=\"http://geohash.org/\">GeoHash</a> URI references.</p>\n      <p xmlns=\"http://purl.org/oslo/ns/localgov#\">The following are examples of equivalent statements using different geometry encodings:</p>\n      <ul xmlns=\"http://purl.org/oslo/ns/localgov#\">\n        <li xmlns=\"http://purl.org/oslo/ns/localgov#\"><p xmlns=\"http://purl.org/oslo/ns/localgov#\">WKT (GeoSPARQL)</p>\n          <pre xmlns=\"http://purl.org/oslo/ns/localgov#\">&lt;ex:a&gt; locn:geometry\n  \"&lt;http://www.opengis.net/def/crs/OGC/1.3/CRS84&gt; Point(-0.001475 51.477811)\"^^ogc:WKTLiteral .</pre>\n        </li>\n        <li xmlns=\"http://purl.org/oslo/ns/localgov#\"><p xmlns=\"http://purl.org/oslo/ns/localgov#\">GML</p>\n          <pre xmlns=\"http://purl.org/oslo/ns/localgov#\">&lt;ex:a&gt; locn:geometry\n  \"&lt;gml:Point srsName='http://www.opengis.net/def/crs/OGC/1.3/CRS84'&gt;\n  &lt;gml:coordinates&gt;-0.001475, 51.477811&lt;/gml:coordinates&gt;&lt;/gml:Point&gt;\"^^ogc:GMLLiteral .</pre>\n        </li>\n        <li xmlns=\"http://purl.org/oslo/ns/localgov#\"><p xmlns=\"http://purl.org/oslo/ns/localgov#\">RDF+WKT (GeoSPARQL)</p>\n          <pre xmlns=\"http://purl.org/oslo/ns/localgov#\">&lt;ex:a&gt; locn:geometry\n  [ a ogc:Point; ogc:asWKT \"&lt;http://www.opengis.net/def/crs/OGC/1.3/CRS84&gt; Point(-0.001475 51.477811)\"^^ogc:WKTLiteral ] .</pre>\n        </li>\n        <li xmlns=\"http://purl.org/oslo/ns/localgov#\"><p xmlns=\"http://purl.org/oslo/ns/localgov#\">RDF+GML (GeoSPARQL)</p>\n          <pre xmlns=\"http://purl.org/oslo/ns/localgov#\">&lt;ex:a&gt; locn:geometry\n  [ a ogc:Point; ogc:asGML\n     \"&lt;gml:Point srsName='http://www.opengis.net/def/crs/OGC/1.3/CRS84'&gt;\n      &lt;gml:coordinates&gt;-0.001475, 51.477811&lt;/gml:coordinates&gt;&lt;/gml:Point&gt;\"^^ogc:GMLLiteral ] .</pre>\n        </li>\n        <li xmlns=\"http://purl.org/oslo/ns/localgov#\"><p xmlns=\"http://purl.org/oslo/ns/localgov#\">RDF (WGS84 lat/long)</p>\n          <pre xmlns=\"http://purl.org/oslo/ns/localgov#\">&lt;ex:a&gt; locn:geometry [ a geo:Point; geo:lat \"51.477811\"; geo:long \"-0.001475\" ] .</pre>\n        </li>\n        <li xmlns=\"http://purl.org/oslo/ns/localgov#\"><p xmlns=\"http://purl.org/oslo/ns/localgov#\">RDF (schema.org)</p>\n          <pre xmlns=\"http://purl.org/oslo/ns/localgov#\">&lt;ex:a&gt; locn:geometry [ a schema:GeoCoordinates; schema:latitude \"51.477811\"; schema:longitude \"-0.001475\" ] .</pre>\n        </li>\n        <li xmlns=\"http://purl.org/oslo/ns/localgov#\"><p xmlns=\"http://purl.org/oslo/ns/localgov#\">URI reference (GeoHash)</p>\n          <pre xmlns=\"http://purl.org/oslo/ns/localgov#\">&lt;ex:a&gt; locn:geometry &lt;<a xmlns=\"http://purl.org/oslo/ns/localgov#\" href=\"http://geohash.org/gcpuzgnzvxkp\">http://geohash.org/gcpuzgnzvxkp</a>&gt; .</pre>\n        </li>\n      </ul>\n    "^^rdf:XMLLiteral ;
	wdrs:describedby <https://joinup.ec.europa.eu/system/files/project/Core_Vocabularies-Business_Location_Person-Specification-v0.3_0.zip> ;
	rdfs:domain :Parcel .

:membershipType a rdf:Property ;
	rdfs:label "type of membership"@en ;
	rdfs:comment "Type of a membership"@en ;
	rdfs:isDefinedBy <http://purl.org/oslo/ns/localgov> ;
	rdfs:domain :Membership ;
	rdfs:range :Code ;
	rdfs:subPropertyOf <http://purl.org/dc/elements/1.1/type> ;
	dcterms:identifier "oslo:membershipType" .

person:countryOfDeath a rdf:Property ;
	rdfs:label "country of death"@en ;
	rdfs:comment "The range of country of death is dcterms:Location and schema:Place."@en ;
	rdfs:range schema:Place , dcterms:Location ;
	rdfs:isDefinedBy <http://www.w3.org/ns/person#> ;
	wdrs:describedby <https://joinup.ec.europa.eu/system/files/project/Core_Vocabularies-Business_Location_Person-Specification-v0.3_0.zip> ;
	dcterms:identifier "person:countryOfDeath" .

:province a rdf:Property ;
	dcterms:identifier "oslo:province" ;
	rdfs:subPropertyOf locn:adminUnitL2 ;
	rdfs:range rdfs:Literal ;
	rdfs:domain :ExtendedAddress ;
	rdfs:isDefinedBy <http://www.w3.org/ns/locn#> ;
	rdfs:comment """The province of the address. The domain of 
    oslo:province is oslo:ExtendedAddress and the range is a literal, conceptually 
  defined by the <a xmlns=\"http://purl.org/oslo/ns/localgov#\" href=\"https://inspire-twg.jrc.ec.europa.eu/inspire-fc.html#_C2612\">INSPIRE Geographical Name data type</a>."""^^rdf:XMLLiteral ;
	rdfs:label "province"@en .

dcterms:alternative a rdf:Property ;
	vann:usage "Any name by which an individual is known. Many individuals use a short form of their name, a \"middle\" name as a \"first\" name or a professional name. For example, the British politician and former UN High Representative for Bosnia and Herzegovina, Jeremy John Durham Ashdown, Baron Ashdown of Norton-sub-Hamdon, is usually referred to simply as Paddy Ashdown or Lord Ashdown."@en ;
	rdfs:label "alternative name"@en ;
	rdfs:comment """The dcterms:alternative property fully represents the 
      Registered Organization vocabulary property of alternative name. Some jurisdictions recognize concepts such as 
      a trading name or alternative forms of a legal entity's name. The alternative name property can be 
      used to record such names but should not be used to record translations of the primary legal name. 
      Where more than one legal name exists and where they have equal standing but are expressed in 
      different languages, identify the language used in each of the multiple legal names."""@en ;
	vann:usageNote """It is not the role of the alternative name field to record nick names, 
    pet names or other 'familiar names' that will be of no consequence in public sector data exchange (foaf:nick would be appropriate for that)."""@en ;
	dcterms:identifier "dcterms:alternative" ;
	rdfs:isDefinedBy <http://dublincore.org/documents/dcmi-terms/> , <http://purl.org/oslo/ns/dublincore.org/documents/dcmi-terms/> ;
	vann:usageNote "Some jurisdictions recognise concepts such as a trading name or alternative forms of a legal entity's name. The Alternative Name property can be used to record such names but should not be used to record translations of the primary legal name. Where more than one legal name exists and where they have equal standing but are expressed in different languages, identify the language used in each of the multiple legal names."@en ;
	rdfs:isDefinedBy <http://www.w3.org/ns/person#> ;
	rdfs:comment "The dcterms:alternative property fully represents the Person Core Vocabulary property of alternative name."@en , "The dcterms:alternative property fully represents the Business Core Vocabulary property of alternative name."@en ;
	wdrs:describedby <https://joinup.ec.europa.eu/system/files/project/Core_Vocabularies-Business_Location_Person-Specification-v0.3_0.zip> .

:domicile a rdf:Property ;
	rdfs:label "domicle"@en ;
	rdfs:comment "The range of domicile is ResidenceObject."@en ;
	rdfs:range :ResidenceObject ;
	rdfs:domain person:Person ;
	rdfs:isDefinedBy <http://purl.org/oslo/ns/localgov> ;
	dcterms:identifier "oslo:domicile" .

adms:identifies a rdf:Property ;
	rdfs:label "identifies"@en ;
	rdfs:comment "adms:identifies fully represents the Core Vocabulary property of the same name"@en ;
	vann:usageNote "The identifies relation is used to link an adms:Identifier class to whatever resource it identifies (such as a business or a person)."@en ;
	rdfs:isDefinedBy <http://www.w3.org/ns/adms#> ;
	dcterms:identifier "adms:identifies" .

:legalCohabetation a rdf:Property ;
	rdfs:label "nobelity title"@en ;
	rdfs:comment "Legal Cohabetitation"@en ;
	rdfs:isDefinedBy <http://purl.org/oslo/ns/localgov> ;
	rdfs:domain person:Person ;
	rdfs:range rdfs:Literal ;
	dcterms:identifier "oslo:legalCohabetation" .

rov:legalName a owl:DatatypeProperty ;
	rdfs:isDefinedBy <http://www.w3.org/TR/vocab-regorg/> ;
	rdfs:range rdfs:Literal ;
	rdfs:comment """The legal name of the business. A business might have more than one 
      legal name, particularly in countries with more than one official language. In such cases the 
      language of the string should be identified."""@en ;
	rdfs:label "legal name"@en ;
	rdfs:comment """The legal name of the business. A business might have more than one 
    legal name, particularly in countries with more than one official language. In such cases the 
    language of the string should be identified."""@en ;
	rdfs:isDefinedBy <http://www.w3.org/ns/regorg#> ;
	dcterms:identifier "rov:legalName" ;
	a rdf:Property .

org:organization a owl:FunctionalProperty ;
	rdfs:range org:Organization ;
	rdfs:comment "Indique l'Organization dont l'agent est membre."@fr ;
	rdfs:domain org:Membership ;
	rdfs:comment "Indicates Organization in which the Agent is a member."@en ;
	a rdf:Property ;
	rdfs:label "organization"@en ;
	rdfs:isDefinedBy <http://www.w3.org/ns/org> ;
	a owl:ObjectProperty ;
	rdfs:label "organisation"@fr .

<http://purl.org/oslo/ns/OSLO_0.8.png> rdfs:label "OSLO Vocabulary Combined UML Class Diagram" .

<http://purl.org/oslo/ns/localgov> dcterms:creator _:node186aoaf8qx7 .

_:node186aoaf8qx7 foaf:name "Laurens De Vocht" ;
	foaf:homepage <http://be.linkedin.com/pub/laurensdv/> ;
	schema:affiliation _:node186aoaf8qx8 .

_:node186aoaf8qx8 foaf:name "Ghent University - iMinds - Multimedialab" .

<http://purl.org/oslo/ns/localgov> foaf:maker _:node186aoaf8qx9 .

_:node186aoaf8qx9 foaf:name "Core Vocabularies Working Group (Business Task Force)" ;
	foaf:page <http://joinup.ec.europa.eu/asset/core_business/home> .

<http://purl.org/oslo/ns/localgov> dcterms:creator _:node186aoaf8qx10 .

_:node186aoaf8qx10 foaf:name "Raf Buyle" ;
	foaf:homepage <http://be.linkedin.com/pub/raf-buyle/3/86/959/> ;
	schema:affiliation _:node186aoaf8qx11 .

_:node186aoaf8qx11 foaf:name "V-ICT-OR/OSLO" .

_:node186aoaf8qx12 a rdfs:Class ;
	dcterms:identifier "oslo:ResidenceObject" ;
	rdfs:subClassOf locn:location ;
	rdfs:comment """This is the key class for the OSLO Location Vocabulary and represents a 
      location that is linked with an address and/or a building with parcel(s)."""@en ;
	rdfs:label "Residence Object"@en ;
	rdfs:ID "ResidenceObject" .
