@prefix dc: <http://purl.org/dc/elements/1.1/> .
@prefix : <http://www.w3.org/1999/02/22-rdf-syntax-ns#> .
@prefix rdfs: <http://www.w3.org/2000/01/rdf-schema#> .
@prefix foaf: <http://xmlns.com/foaf/0.1/> .
@prefix status: <http://metadataregistry.org/uri/RegStatus/> .
@prefix reg: <http://metadataregistry.org/uri/profile/RegAp/> .
@prefix dct: <http://purl.org/dc/terms/> .
@prefix owl: <http://www.w3.org/2002/07/owl#> .
@prefix skos: <http://www.w3.org/2004/02/skos/core#> .

<http://rdvocab.info/roles> dc:title "RDA Roles"@en ;
	foaf:homepage <http://dublincore.org/dcmirdataskgroup/> .

<http://rdvocab.info/roles/abridger> rdfs:isDefinedBy <http://rdvocab.info/roles> ;
	reg:status <http://metadataregistry.org/uri/RegStatus/1002> ;
	reg:name "abridger"@en ;
	rdfs:label "Abridger"@en ;
	a :Property ;
	reg:hasSubproperty <http://rdvocab.info/roles/abridgerExpression> ;
	rdfs:label "Abridger"@de .

<http://rdvocab.info/roles/abridgerExpression> rdfs:isDefinedBy <http://rdvocab.info/roles> ;
	reg:status <http://metadataregistry.org/uri/RegStatus/1002> ;
	reg:name "abridgerExpression"@en ;
	rdfs:label "Abridger (Expression)"@en ;
	skos:definition "A person, family, or corporate body contributing to an expression of a work by shortening or condensing the original work but leaving the nature and content of the original work substantially unchanged."@en ;
	a :Property ;
	rdfs:domain <http://rdvocab.info/uri/schema/FRBRentitiesRDA/Expression> ;
	rdfs:subPropertyOf <http://rdvocab.info/roles/contributor> ;
	rdfs:label "Abridger (Expression)"@de ;
	skos:definition "Eine Person, Familie oder Körperschaft, die eine Expression eines Werkes kürzt oder zusammenfasst, dabei aber das Wesen des Originalwerkes unverändert lässt."@de .

<http://rdvocab.info/roles/actor> rdfs:isDefinedBy <http://rdvocab.info/roles> ;
	reg:status <http://metadataregistry.org/uri/RegStatus/1002> ;
	reg:name "actor"@en ;
	rdfs:label "Actor"@en ;
	a :Property ;
	rdfs:subPropertyOf <http://rdvocab.info/roles/performer> ;
	rdfs:label "Schauspieler"@de .

<http://rdvocab.info/roles/actorExpression> rdfs:isDefinedBy <http://rdvocab.info/roles> ;
	reg:status <http://metadataregistry.org/uri/RegStatus/1002> ;
	reg:name "actorExpression"@en ;
	rdfs:label "Actor (Expression)"@en ;
	skos:definition "A performer contributing to an expression of a work by acting as a cast member or player in a musical or dramatic presentation, etc."@en ;
	a :Property ;
	rdfs:subPropertyOf <http://rdvocab.info/roles/performerExpression> ;
	rdfs:domain <http://rdvocab.info/uri/schema/FRBRentitiesRDA/Expression> ;
	rdfs:label "Schauspieler (Expression)"@de ;
	skos:definition "Ein Darsteller, der zu einer Expression eines Werkes als Ensemble-Mitglied oder Darsteller in einer musikalischen oder dramatischen Darbietung usw. beiträgt."@de .

<http://rdvocab.info/roles/addressee> rdfs:isDefinedBy <http://rdvocab.info/roles> ;
	reg:status <http://metadataregistry.org/uri/RegStatus/1002> ;
	reg:name "addressee"@en ;
	rdfs:label "addressee"@en ;
	a :Property ;
	reg:hasSubproperty <http://rdvocab.info/roles/addresseeWork> ;
	rdfs:label "Adressat"@de .

<http://rdvocab.info/roles/addresseeWork> rdfs:isDefinedBy <http://rdvocab.info/roles> ;
	reg:status <http://metadataregistry.org/uri/RegStatus/1002> ;
	reg:name "addresseeWork"@en ;
	rdfs:label "addressee (Work)"@en ;
	skos:definition "A person, family, or corporate body to whom the work or part of the work is addressed."@en ;
	a :Property ;
	rdfs:domain <http://rdvocab.info/uri/schema/FRBRentitiesRDA/Work> ;
	rdfs:subPropertyOf <http://rdvocab.info/roles/addressee> ;
	rdfs:label "Adressat (Werk)"@de ;
	skos:definition "Eine Person, Familie oder Körperschaft, an die Korrespondenz in einem Werk adressiert ist."@de .

<http://rdvocab.info/roles/animator> rdfs:isDefinedBy <http://rdvocab.info/roles> ;
	reg:status <http://metadataregistry.org/uri/RegStatus/1002> ;
	reg:name "animator"@en ;
	rdfs:label "Animator"@en ;
	a :Property ;
	reg:hasSubproperty <http://rdvocab.info/roles/animatorExpression> ;
	rdfs:label "Animator"@de .

<http://rdvocab.info/roles/animatorExpression> rdfs:isDefinedBy <http://rdvocab.info/roles> ;
	reg:status <http://metadataregistry.org/uri/RegStatus/1002> ;
	reg:name "animatorExpression"@en ;
	rdfs:label "Animator (Expression)"@en ;
	skos:definition "A person, family, or corporate body contributing to an expression of a moving image work or computer program by giving apparent movement to inanimate objects or drawings."@en ;
	a :Property ;
	rdfs:domain <http://rdvocab.info/uri/schema/FRBRentitiesRDA/Expression> ;
	rdfs:subPropertyOf <http://rdvocab.info/roles/contributor> ;
	rdfs:label "Animator (Expression)"@de ;
	skos:definition "Eine Person, Familie oder Körperschaft, an die Korrespondenz in einem Werk adressiert ist."@de .

<http://rdvocab.info/roles/annotator> rdfs:isDefinedBy <http://rdvocab.info/roles> ;
	reg:status <http://metadataregistry.org/uri/RegStatus/1002> ;
	reg:name "annotator"@en ;
	rdfs:label "Annotator"@en ;
	a :Property ;
	reg:hasSubproperty <http://rdvocab.info/roles/annotatorItem> ;
	rdfs:label "Annotator"@de .

<http://rdvocab.info/roles/annotatorItem> rdfs:isDefinedBy <http://rdvocab.info/roles> ;
	reg:status <http://metadataregistry.org/uri/RegStatus/1002> ;
	reg:name "annotatorItem"@en ;
	rdfs:label "Annotator (Item)"@en ;
	skos:definition "A person who makes manuscript annotations on a specific item."@en ;
	a :Property ;
	rdfs:subPropertyOf <http://rdvocab.info/roles/annotator> ;
	rdfs:domain <http://rdvocab.info/uri/schema/FRBRentitiesRDA/Item> ;
	rdfs:label "Annotator (Exemplar)"@de ;
	skos:definition "Eine Person, die handschriftlich Anmerkungen in ein spezifisches Exemplar schreibt."@de .

<http://rdvocab.info/roles/appellant> rdfs:isDefinedBy <http://rdvocab.info/roles> ;
	reg:status <http://metadataregistry.org/uri/RegStatus/1002> ;
	reg:name "appellant"@en ;
	rdfs:label "Appellant"@en ;
	a :Property ;
	reg:hasSubproperty <http://rdvocab.info/roles/appellantWork> ;
	rdfs:label "Berufungskläger / Revisionskläger"@de ;
	skos:definition "Eine natürliche oder juristische Person, die gegen ein Gerichtsurteil einer unteren Instanz Rechtsmittel (Berufung / Revision) einlegt."@de .

<http://rdvocab.info/roles/appellantWork> rdfs:isDefinedBy <http://rdvocab.info/roles> ;
	reg:status <http://metadataregistry.org/uri/RegStatus/1002> ;
	reg:name "appellantWork"@en ;
	rdfs:label "Appellant (Work)"@en ;
	skos:definition "A person or corporate body who appeals a lower court's decision."@en ;
	a :Property ;
	rdfs:domain <http://rdvocab.info/uri/schema/FRBRentitiesRDA/Work> ;
	rdfs:subPropertyOf <http://rdvocab.info/roles/appellant> ;
	skos:definition "Eine natürliche oder juristische Person, die gegen ein Gerichtsurteil einer unteren Instanz Rechtsmittel (Berufung / Revision) einlegt."@de ;
	rdfs:label "Berufungskläger / Revisionskläger (Werk)"@de .

<http://rdvocab.info/roles/appellee> rdfs:isDefinedBy <http://rdvocab.info/roles> ;
	reg:status <http://metadataregistry.org/uri/RegStatus/1002> ;
	reg:name "appellee"@en ;
	rdfs:label "Appellee"@en ;
	a :Property ;
	reg:hasSubproperty <http://rdvocab.info/roles/appelleeWork> ;
	rdfs:label "Berufungsbeklagter / Revisionsbeklagter"@de ;
	skos:definition "Eine natürliche oder juristische Person, gegen die Rechtsmittel (Berufung / Revision) eingelegt wurde."@de .

<http://rdvocab.info/roles/appelleeWork> rdfs:isDefinedBy <http://rdvocab.info/roles> ;
	reg:status <http://metadataregistry.org/uri/RegStatus/1002> ;
	reg:name "appelleeWork"@en ;
	rdfs:label "Appellee (Work)"@en ;
	skos:definition "A person or corporate body against whom an appeal is taken."@en ;
	a :Property ;
	rdfs:domain <http://rdvocab.info/uri/schema/FRBRentitiesRDA/Work> ;
	rdfs:subPropertyOf <http://rdvocab.info/roles/appellee> ;
	rdfs:label "Berufungsbeklagter / Revisionsbeklagter (Werk)"@de ;
	skos:definition "Eine natürliche oder juristische Person, gegen die Rechtsmittel (Berufung / Revision) eingelegt wurde."@de .

<http://rdvocab.info/roles/architect> rdfs:isDefinedBy <http://rdvocab.info/roles> ;
	reg:status <http://metadataregistry.org/uri/RegStatus/1002> ;
	reg:name "architect"@en ;
	rdfs:label "Architect"@en ;
	a :Property ;
	reg:hasSubproperty <http://rdvocab.info/roles/landscapeArchitect> ;
	rdfs:label "Architekt"@de .

<http://rdvocab.info/roles/architectWork> rdfs:isDefinedBy <http://rdvocab.info/roles> ;
	reg:status <http://metadataregistry.org/uri/RegStatus/1002> ;
	reg:name "architectWork"@en ;
	rdfs:label "Architect (Work)"@en ;
	skos:definition "A person, family, or corporate body responsible for creating an architectural design, including a pictorial representation intended to show how a building, etc., will look when completed."@en ;
	a :Property ;
	rdfs:subPropertyOf <http://rdvocab.info/roles/creator> ;
	rdfs:domain <http://rdvocab.info/uri/schema/FRBRentitiesRDA/Work> ;
	rdfs:label "Architekt (Werk)"@de ;
	skos:definition "Eine Person, Familie oder Körperschaft, die für eine architektonische Gestaltung verantwortlich ist, einschließlich einer bildlichen Darstellung, die zeigt, wie ein Gebäude o. ä. aussieht, wenn es fertig gebaut sein wird."@de .

<http://rdvocab.info/roles/arrangerOfMusic> rdfs:isDefinedBy <http://rdvocab.info/roles> ;
	reg:status <http://metadataregistry.org/uri/RegStatus/1002> ;
	reg:name "arrangerOfMusic"@en ;
	rdfs:label "Arranger of music"@en ;
	a :Property ;
	rdfs:label "Arrangeur"@de .

<http://rdvocab.info/roles/arrangerOfMusicExpression> rdfs:isDefinedBy <http://rdvocab.info/roles> ;
	reg:status <http://metadataregistry.org/uri/RegStatus/1002> ;
	reg:name "arrangerOfMusicExpression"@en ;
	rdfs:label "Arranger of music (Expression)"@en ;
	skos:definition "A person, family, or corporate body contributing to an expression of a musical work by rewriting the composition for a medium of performance different from that for which the work was originally intended, modifying the work for the same medium of performance, etc., such that the musical substance of the original composition remains essentially unchanged."@en ;
	a :Property ;
	rdfs:domain <http://rdvocab.info/uri/schema/FRBRentitiesRDA/Expression> ;
	rdfs:subPropertyOf <http://rdvocab.info/roles/contributor> ;
	rdfs:label "Arrangeur (Expression)"@de ;
	skos:definition "Eine Person, Familie oder Körperschaft, die zu einer Expression eines Musikwerkes beiträgt, indem sie eine Komposition mit einer bestimmen Originalbesetzung für eine andere Besetzung umschreibt oder das Werk für die Originalbesetzung modifiziert. Das Wesen des originären Musikstückes bleibt dabei unverändert."@de .

<http://rdvocab.info/roles/artDirector> rdfs:isDefinedBy <http://rdvocab.info/roles> ;
	reg:status <http://metadataregistry.org/uri/RegStatus/1002> ;
	reg:name "artDirector"@en ;
	rdfs:label "Art director"@en ;
	a :Property ;
	rdfs:label "Art Director"@de .

<http://rdvocab.info/roles/artDirectorExpression> rdfs:isDefinedBy <http://rdvocab.info/roles> ;
	reg:status <http://metadataregistry.org/uri/RegStatus/1002> ;
	reg:name "artDirectorExpression"@en ;
	rdfs:label "Art director (Expression)"@en ;
	skos:definition "A person, family or corporate body responsible for overseeing the artists and craftspeople who build the sets for moving image productions."@en ;
	a :Property ;
	rdfs:subPropertyOf <http://rdvocab.info/roles/contributor> ;
	rdfs:domain <http://rdvocab.info/uri/schema/FRBRentitiesRDA/Expression> ;
	rdfs:label "Art Director (Expression)"@de ;
	skos:definition "Eine Person, Familie oder Körperschaft, die für die Künstler und Kunsthandwerker, die ein Set für eine Bewegtbildproduktion aufbauen, verantwortlich ist."@de .

<http://rdvocab.info/roles/artist> rdfs:isDefinedBy <http://rdvocab.info/roles> ;
	reg:status <http://metadataregistry.org/uri/RegStatus/1002> ;
	reg:name "artist"@en ;
	rdfs:label "Artist"@en ;
	a :Property ;
	reg:hasSubproperty <http://rdvocab.info/roles/sculptor> ;
	rdfs:label "Künstler"@de .

<http://rdvocab.info/roles/artistWork> rdfs:isDefinedBy <http://rdvocab.info/roles> ;
	reg:status <http://metadataregistry.org/uri/RegStatus/1002> ;
	reg:name "artistWork"@en ;
	rdfs:label "Artist (Work)"@en ;
	skos:definition "A person, family, or corporate body responsible for creating a work by conceiving, and often implementing, an original graphic design, drawing, painting, etc."@en ;
	a :Property ;
	rdfs:subPropertyOf <http://rdvocab.info/roles/creator> ;
	rdfs:domain <http://rdvocab.info/uri/schema/FRBRentitiesRDA/Work> ;
	rdfs:label "Künstler (Werk)"@de ;
	skos:definition "Eine Person, Familie oder Körperschaft, die für die Idee und meist auch Umsetzung eines Werkes in Form einer Grafik, einer Zeichnung oder eines Gemäldes verantwortlich ist."@de .

<http://rdvocab.info/roles/author> rdfs:isDefinedBy <http://rdvocab.info/roles> ;
	reg:status <http://metadataregistry.org/uri/RegStatus/1002> ;
	reg:name "author"@en ;
	rdfs:label "Author"@en ;
	a :Property ;
	reg:hasSubproperty <http://rdvocab.info/roles/librettist> , <http://rdvocab.info/roles/lyricist> , <http://rdvocab.info/roles/screenwriter> ;
	rdfs:label "Verfasser"@de ;
	skos:definition "Eine Person, Familie oder Körperschaft, die verantwortlich für die Erstellung eines Werkes ist, das im Wesentlichen aus Text besteht, unabhängig vom Medientyp (gedruckter Text, gesprochenes Wort, elektronischer Text, taktiler Text usw.) oder von der Gattung (Gedichte, Romane, Drehbücher, Blogs usw.). Die Rolle wird auch für Personen verwendet, die den Charakter und den Inhalt eines Originalwerkes wesentlich durch Paraphrasieren, Umschreiben oder Adaption verändern und so ein neues Werk erschaffen, oder den Medientyp einer Expression ändern."@de .

<http://rdvocab.info/roles/authorWork> rdfs:isDefinedBy <http://rdvocab.info/roles> ;
	reg:status <http://metadataregistry.org/uri/RegStatus/1002> ;
	reg:name "authorWork"@en ;
	rdfs:label "Author (Work)"@en ;
	a :Property ;
	skos:definition "A person, family, or corporate body responsible for creating a work that is primarily textual in content, regardless of media type (e.g., printed text, spoken word, electronic text, tactile text) or genre (e.g., poems, novels, screenplays, blogs). Use also for persons, etc., creating a new work by paraphrasing, rewriting, or adapting works by another creator such that the modification has substantially changed the nature and content of the original or changed the medium of expression."@en ;
	reg:hasSubproperty <http://rdvocab.info/roles/librettistWork> ;
	rdfs:domain <http://rdvocab.info/uri/schema/FRBRentitiesRDA/Work> ;
	rdfs:subPropertyOf <http://rdvocab.info/roles/creator> ;
	rdfs:label "Verfasser (Werk)"@de ;
	skos:definition "Eine Person, Familie oder Körperschaft, die verantwortlich für die Erstellung eines Werkes ist, das im Wesentlichen aus Text besteht, unabhängig vom Medientyp (gedruckter Text, gesprochenes Wort, elektronischer Text, taktiler Text usw.) oder von der Gattung (Gedichte, Romane, Drehbücher, Blogs usw.). Die Rolle wird auch für Personen verwendet, die den Charakter und den Inhalt eines Originalwerkes wesentlich durch Paraphrasieren, Umschreiben oder Adaption verändern und so ein neues Werk erschaffen, oder den Medientyp einer Expression ändern."@de ;
	reg:hasSubproperty <http://rdvocab.info/roles/screenwriterWork> , <http://rdvocab.info/roles/lyricistWork> .

<http://rdvocab.info/roles/autographer> rdfs:isDefinedBy <http://rdvocab.info/roles> ;
	reg:status <http://metadataregistry.org/uri/RegStatus/1002> ;
	reg:name "autographer"@en ;
	rdfs:label "Autographer"@en ;
	a :Property ;
	reg:hasSubproperty <http://rdvocab.info/roles/autographerItem> ;
	rdfs:label "Unterzeichner"@de .

<http://rdvocab.info/roles/autographerItem> rdfs:isDefinedBy <http://rdvocab.info/roles> ;
	reg:status <http://metadataregistry.org/uri/RegStatus/1002> ;
	reg:name "autographerItem"@en ;
	rdfs:label "Autographer (item)"@en ;
	skos:definition "A person whose manuscript signature appears on an item."@en ;
	a :Property ;
	rdfs:domain <http://rdvocab.info/uri/schema/FRBRentitiesRDA/Item> ;
	rdfs:subPropertyOf <http://rdvocab.info/roles/autographer> ;
	rdfs:label "Unterzeichner (Exemplar)"@de ;
	skos:definition "Eine Person, deren handschriftliche Unterschrift auf einem Exemplar steht."@de .

<http://rdvocab.info/roles/binder> rdfs:isDefinedBy <http://rdvocab.info/roles> ;
	reg:status <http://metadataregistry.org/uri/RegStatus/1002> ;
	reg:name "binder"@en ;
	rdfs:label "Binder"@en ;
	a :Property ;
	reg:hasSubproperty <http://rdvocab.info/roles/binderItem> ;
	rdfs:label "Buchbinder"@de ;
	skos:definition "Eine Person, die ein Exemplar bindet."@de .

<http://rdvocab.info/roles/binderItem> rdfs:isDefinedBy <http://rdvocab.info/roles> ;
	reg:status <http://metadataregistry.org/uri/RegStatus/1002> ;
	reg:name "binderItem"@en ;
	rdfs:label "Binder (Item)"@en ;
	skos:definition "A person who binds a specific item."@en ;
	a :Property ;
	rdfs:domain <http://rdvocab.info/uri/schema/FRBRentitiesRDA/Item> ;
	rdfs:subPropertyOf <http://rdvocab.info/roles/binder> ;
	rdfs:label "Buchbinder (Exemplar)"@de , "Eine Person, die ein Exemplar bindet."@de .

<http://rdvocab.info/roles/bookDesigner> rdfs:isDefinedBy <http://rdvocab.info/roles> ;
	reg:status <http://metadataregistry.org/uri/RegStatus/1002> ;
	reg:name "bookDesigner"@en ;
	rdfs:label "Book designer"@en ;
	a :Property ;
	rdfs:subPropertyOf <http://rdvocab.info/roles/manufacturer> ;
	rdfs:label "Buchgestalter"@de .

<http://rdvocab.info/roles/bookDesignerManifestation> rdfs:isDefinedBy <http://rdvocab.info/roles> ;
	reg:status <http://metadataregistry.org/uri/RegStatus/1002> ;
	reg:name "bookDesignerManifestation"@en ;
	rdfs:label "Book designer (Manifestation)"@en ;
	skos:definition "A person, family, or corporate body involved in manufacturing a manifestation by being responsible for the entire graphic design of a book, including arrangement of type and illustration, choice of materials, and process used."@en ;
	a :Property ;
	rdfs:domain <http://rdvocab.info/uri/schema/FRBRentitiesRDA/Manifestation> ;
	rdfs:subPropertyOf <http://rdvocab.info/roles/manufacturerManifestation> ;
	rdfs:label "Buchgestalter (Manifestation)"@de ;
	skos:definition "Eine Person, Familie oder Körperschaft, die für das gesamte grafische Design eines Buches verantwortlich ist, einschließlich Schriftbild, Bildgestaltung, Materialwahl und der angewandten Verfahren."@de .

<http://rdvocab.info/roles/brailleEmbosser> rdfs:isDefinedBy <http://rdvocab.info/roles> ;
	reg:status <http://metadataregistry.org/uri/RegStatus/1002> ;
	reg:name "brailleEmbosser"@en ;
	rdfs:label "Braille embosser"@en ;
	a :Property ;
	rdfs:subPropertyOf <http://rdvocab.info/roles/manufacturer> ;
	rdfs:label "Brailleschriftpräger"@de .

<http://rdvocab.info/roles/brailleEmbosserManifestation> rdfs:isDefinedBy <http://rdvocab.info/roles> ;
	reg:status <http://metadataregistry.org/uri/RegStatus/1002> ;
	reg:name "brailleEmbosserManifestation"@en ;
	rdfs:label "Braille embosser (Manifestation)"@en ;
	skos:definition "A person, family, or corporate body involved in producing a manifestation by embossing Braille cells using a stylus, special embossing printer, or other device."@en ;
	a :Property ;
	rdfs:domain <http://rdvocab.info/uri/schema/FRBRentitiesRDA/Manifestation> ;
	rdfs:subPropertyOf <http://rdvocab.info/roles/manufacturerManifestation> ;
	rdfs:label "Brailleschriftpräger (Manifestation)"@de ;
	skos:definition "Eine Person, Familie oder Körperschaft, die im Herstellungsprozess einer Manifestation in Form von Braillezeichen involviert ist. Für das Prägen wird ein Griffel, ein spezieller Brailledrucker oder ein anderes Gerät verwendet."@de .

<http://rdvocab.info/roles/broadcaster> rdfs:isDefinedBy <http://rdvocab.info/roles> ;
	reg:status <http://metadataregistry.org/uri/RegStatus/1002> ;
	reg:name "broadcaster"@en ;
	rdfs:label "Broadcaster"@en ;
	a :Property ;
	rdfs:subPropertyOf <http://rdvocab.info/roles/publisher> ;
	skos:definition "Eine Person, eine Familie oder eine Körperschaft, die für Ausstrahlung einer Manifestation über Hörfunk, Fernsehen oder Webcast usw. verantwortlich ist."@de ;
	rdfs:label "Broadcaster"@de .

<http://rdvocab.info/roles/broadcasterManifestation> rdfs:isDefinedBy <http://rdvocab.info/roles> ;
	reg:status <http://metadataregistry.org/uri/RegStatus/1002> ;
	reg:name "broadcasterManifestation"@en ;
	rdfs:label "Broadcaster (Manifestation)"@en ;
	skos:definition "A person, family, or corporate body responsible for broadcasting a manifestation to an audience via radio, television, webcast, etc."@en ;
	a :Property ;
	rdfs:domain <http://rdvocab.info/uri/schema/FRBRentitiesRDA/Manifestation> ;
	rdfs:subPropertyOf <http://rdvocab.info/roles/publisherManifestation> ;
	rdfs:label "Broadcaster (Manifestation)"@de ;
	skos:definition "Eine Person, eine Familie oder eine Körperschaft, die für Ausstrahlung einer Manifestation über Hörfunk, Fernsehen oder Webcast usw. verantwortlich ist."@de .

<http://rdvocab.info/roles/cartographer> rdfs:isDefinedBy <http://rdvocab.info/roles> ;
	reg:status <http://metadataregistry.org/uri/RegStatus/1002> ;
	reg:name "cartographer"@en ;
	rdfs:label "Cartographer"@en ;
	a :Property ;
	rdfs:label "Kartograf"@de .

<http://rdvocab.info/roles/cartographerWork> rdfs:isDefinedBy <http://rdvocab.info/roles> ;
	reg:status <http://metadataregistry.org/uri/RegStatus/1002> ;
	reg:name "cartographerWork"@en ;
	rdfs:label "Cartographer (Work)"@en ;
	skos:definition "A person, family, or corporate body responsible for creating a map, atlase, globe, or other cartographic work."@en ;
	a :Property ;
	rdfs:subPropertyOf <http://rdvocab.info/roles/creator> ;
	rdfs:domain <http://rdvocab.info/uri/schema/FRBRentitiesRDA/Work> ;
	rdfs:label "Kartograf (Werk)"@de ;
	skos:definition "Eine Person, Familie oder Körperschaft, die für das Erstellen einer Karte, eines Atlasses, eines Globusses oder eines anderen kartografischen Werkes verantwortlich ist."@de .

<http://rdvocab.info/roles/caster> rdfs:isDefinedBy <http://rdvocab.info/roles> ;
	reg:status <http://metadataregistry.org/uri/RegStatus/1002> ;
	reg:name "caster"@en ;
	rdfs:label "Caster"@en ;
	a :Property ;
	rdfs:subPropertyOf <http://rdvocab.info/roles/manufacturer> ;
	rdfs:label "Formgießer"@de .

<http://rdvocab.info/roles/casterManifestation> rdfs:isDefinedBy <http://rdvocab.info/roles> ;
	reg:status <http://metadataregistry.org/uri/RegStatus/1002> ;
	reg:name "casterManifestation"@en ;
	rdfs:label "Caster (Manifestation)"@en ;
	skos:definition "A person, family, or corporate body involved in producing a manifestation by pouring a liquid or molten substance into a mold and leaving it to solidify to take the shape of the mold."@en ;
	a :Property ;
	rdfs:domain <http://rdvocab.info/uri/schema/FRBRentitiesRDA/Manifestation> ;
	rdfs:subPropertyOf <http://rdvocab.info/roles/manufacturerManifestation> ;
	rdfs:label "Formgießer (Manifestation)"@de ;
	skos:definition """Eine Person, Familie oder Körperschaft, die in den Herstellungsprozess einer Manifestation durch das Gießen einer Flüssigkeit oder einer geschmolzenen Substanz in eine Form involviert ist.
Die Substanz verbleibt in der Gießform, bis sie ausgehärtet ist."""@de .

<http://rdvocab.info/roles/choreographer> rdfs:isDefinedBy <http://rdvocab.info/roles> ;
	reg:status <http://metadataregistry.org/uri/RegStatus/1002> ;
	reg:name "choreographer"@en ;
	rdfs:label "Choreographer"@en ;
	a :Property ;
	rdfs:label "Choreograf"@de .

<http://rdvocab.info/roles/choreographerExpression> rdfs:isDefinedBy <http://rdvocab.info/roles> ;
	reg:status <http://metadataregistry.org/uri/RegStatus/1002> ;
	reg:name "choreographerExpression"@en ;
	rdfs:label "Choreographer (Expression)"@en ;
	skos:definition "A person, family, or corporate body contributing to an expression of a work by providing additional choreography, or by modifying the previous choreography."@en ;
	a :Property ;
	rdfs:subPropertyOf <http://rdvocab.info/roles/contributor> ;
	rdfs:domain <http://rdvocab.info/uri/schema/FRBRentitiesRDA/Expression> ;
	rdfs:label "Choreograph (Expression)"@de ;
	skos:definition "Eine Person, Familie oder Körperschaft, die für ein aus Bewegung bestehendes Werk verantwortlich ist."@de .

<http://rdvocab.info/roles/choreographerWork> rdfs:isDefinedBy <http://rdvocab.info/roles> ;
	reg:status <http://metadataregistry.org/uri/RegStatus/1002> ;
	reg:name "choreographerWork"@en ;
	rdfs:label "Choreographer (Work)"@en ;
	skos:definition "A person, family, or corporate body responsible for creating a work of movement."@en ;
	a :Property ;
	rdfs:subPropertyOf <http://rdvocab.info/roles/creator> ;
	rdfs:domain <http://rdvocab.info/uri/schema/FRBRentitiesRDA/Work> ;
	rdfs:label "Choreograf (Werk)"@de ;
	skos:definition "Eine Person, Familie oder Körperschaft, die für ein aus Bewegung bestehendes Werk verantwortlich ist."@de .

<http://rdvocab.info/roles/cinematographer> rdfs:isDefinedBy <http://rdvocab.info/roles> ;
	reg:status <http://metadataregistry.org/uri/RegStatus/1002> ;
	reg:name "cinematographer"@en ;
	rdfs:label "Cinematographer"@en ;
	skos:definition "A person, family, or corporate body contributing to an expression of a moving image work by capturing images either electronically or on film or video stock using a visual recording device, and often the selection and arrangement of lighting. The chief cinematographer for a movie is also called the director of photography. Use this designation also for videographers."@en ;
	a :Property ;
	rdfs:label "Kameramann"@de ;
	skos:definition "Eine Person, eine Familie oder eine Körperschaft, die zu einer Expression eines Bewegtbildwerkes  beiträgt, indem sie die Bilder mit einem Aufzeichnungsgerät aufnimmt, entweder in elektronischer Form oder auf Film oder Video. Häufig gehört auch die Auswahl der Bilder und die Beleuchtung dazu. Der leitende Kameramann wird auch verantwortlicher Kameramann genannt. Die Bezeichnung „Kameramann\" wird auch für einen Videografen verwendet."@de .

<http://rdvocab.info/roles/collectionRegistrar> rdfs:isDefinedBy <http://rdvocab.info/roles> ;
	reg:status <http://metadataregistry.org/uri/RegStatus/1002> ;
	reg:name "collectionRegistrar"@en ;
	rdfs:label "Collection registrar"@en ;
	a :Property ;
	rdfs:subPropertyOf <http://rdvocab.info/roles/curator> ;
	rdfs:label "Registrar"@de .

<http://rdvocab.info/roles/collectionRegistrarItem> rdfs:isDefinedBy <http://rdvocab.info/roles> ;
	reg:status <http://metadataregistry.org/uri/RegStatus/1002> ;
	reg:name "collectionRegistrarItem"@en ;
	rdfs:label "Collection registrar (Item)"@en ;
	skos:definition "A type of curator who lists or inventories the items in an aggregate work such as a collection of items or works."@en ;
	a :Property ;
	rdfs:domain <http://rdvocab.info/uri/schema/FRBRentitiesRDA/Item> ;
	rdfs:label "Registrar (Exemplar)"@de ;
	skos:definition "Jemand, der die Exemplare eines zusammengestellten Werkes, wie beispielsweise eine Sammlung von Exemplaren oder Werken, verzeichnet und inventarisiert."@de .

<http://rdvocab.info/roles/collector> rdfs:isDefinedBy <http://rdvocab.info/roles> ;
	reg:status <http://metadataregistry.org/uri/RegStatus/1002> ;
	reg:name "collector"@en ;
	rdfs:label "Collector"@en ;
	a :Property ;
	rdfs:subPropertyOf <http://rdvocab.info/roles/curator> ;
	rdfs:label "Sammler"@de .

<http://rdvocab.info/roles/collectorItem> rdfs:isDefinedBy <http://rdvocab.info/roles> ;
	reg:status <http://metadataregistry.org/uri/RegStatus/1002> ;
	reg:name "collectorItem"@en ;
	rdfs:label "Collector (Item)"@en ;
	skos:definition "A curator who brings together material from various sources that are then arranged, described, and cataloged as a collection."@en ;
	a :Property ;
	rdfs:domain <http://rdvocab.info/uri/schema/FRBRentitiesRDA/Item> ;
	rdfs:label "Sammler (Exemplar)"@de ;
	skos:definition "Jemand, der Materialien aus unterschiedlichen Quellen zusammenträgt, die zu einer Sammlung zusammengestellt, beschrieben und katalogisiert werden."@de .

<http://rdvocab.info/roles/collotyper> rdfs:isDefinedBy <http://rdvocab.info/roles> ;
	reg:status <http://metadataregistry.org/uri/RegStatus/1002> ;
	reg:name "collotyper"@en ;
	rdfs:label "Collotyper"@en ;
	a :Property ;
	rdfs:subPropertyOf <http://rdvocab.info/roles/manufacturer> ;
	rdfs:label "Drucker (im Lichtdruckverfahren)"@de .

<http://rdvocab.info/roles/collotyperManifestation> rdfs:isDefinedBy <http://rdvocab.info/roles> ;
	reg:status <http://metadataregistry.org/uri/RegStatus/1002> ;
	reg:name "collotyperManifestation"@en ;
	rdfs:label "Collotyper (Manifestation)"@en ;
	skos:definition "A person, family, or corporate body involved in producing a manifestation of photographic prints from film or other colloid that has ink-receptive and ink-repellent surfaces."@en ;
	a :Property ;
	rdfs:domain <http://rdvocab.info/uri/schema/FRBRentitiesRDA/Manifestation> ;
	rdfs:subPropertyOf <http://rdvocab.info/roles/manufacturerManifestation> ;
	rdfs:label "Drucker (im Lichtdruckverfahren) (Manifestation)"@de ;
	skos:definition "Eine Person, Familie oder Körperschaft, die an der Produktion einer Manifestation aus Fotodrucken von Film oder einem anderem Kolloiden, der Druckerfarbe anziehende und abstoßende Flächen aufweist, beteiligt ist."@de .

<http://rdvocab.info/roles/commentator> rdfs:isDefinedBy <http://rdvocab.info/roles> ;
	reg:status <http://metadataregistry.org/uri/RegStatus/1002> ;
	reg:name "commentator"@en ;
	rdfs:label "Commentator"@en ;
	a :Property ;
	rdfs:subPropertyOf <http://rdvocab.info/roles/performer> ;
	rdfs:label "Kommentator (mündlich)"@de .

<http://rdvocab.info/roles/commentatorExpression> rdfs:isDefinedBy <http://rdvocab.info/roles> ;
	reg:status <http://metadataregistry.org/uri/RegStatus/1002> ;
	reg:name "commentatorExpression"@en ;
	rdfs:label "Commentator (Expression)"@en ;
	skos:definition "A performer contributing to an expression of a work by providing interpretation, analysis, or a discussion of the subject matter on a recording, film, or other audiovisual medium."@en ;
	a :Property ;
	rdfs:domain <http://rdvocab.info/uri/schema/FRBRentitiesRDA/Expression> ;
	rdfs:label "Kommentator (mündlich) (Expression)"@de ;
	skos:definition "Jemand, der zu einer Expression eines Werkes in einer Aufnahme, in einem Film oder in einem anderen audiovisuellen Medium in Form einer Interpretation, einer Analyse oder einer Diskussion des Themas beiträgt."@de .

<http://rdvocab.info/roles/compiler> rdfs:isDefinedBy <http://rdvocab.info/roles> ;
	reg:status <http://metadataregistry.org/uri/RegStatus/1002> ;
	reg:name "compiler"@en ;
	rdfs:label "Compiler"@en ;
	a :Property ;
	rdfs:label "Compiler"@de .

<http://rdvocab.info/roles/compilerWork> rdfs:isDefinedBy <http://rdvocab.info/roles> ;
	reg:status <http://metadataregistry.org/uri/RegStatus/1002> ;
	reg:name "compilerWork"@en ;
	rdfs:label "Compiler (Work)"@en ;
	skos:definition "A person, family, or corporate body responsible for creating a new work (e.g., a bibliography, a directory) through the act of compilation, e.g., selecting, arranging, aggregating, and editing data, information, etc."@en ;
	a :Property ;
	rdfs:subPropertyOf <http://rdvocab.info/roles/creator> ;
	rdfs:domain <http://rdvocab.info/uri/schema/FRBRentitiesRDA/Work> ;
	skos:definition "Eine Person, Familie oder Körperschaft, die für das Erstellen eines Werkes durch eine Zusammenstellung verantwortlich ist, beispielsweise durch Selektieren, Gliedern, Zusammenstellen und Editieren von Daten, Information, usw."@de ;
	rdfs:label "Compiler (Werk)"@de .

<http://rdvocab.info/roles/composer> rdfs:isDefinedBy <http://rdvocab.info/roles> ;
	reg:status <http://metadataregistry.org/uri/RegStatus/1002> ;
	reg:name "composer"@en ;
	rdfs:label "Composer"@en ;
	a :Property ;
	rdfs:label "Komponist"@de .

<http://rdvocab.info/roles/composerExpression> rdfs:isDefinedBy <http://rdvocab.info/roles> ;
	reg:status <http://metadataregistry.org/uri/RegStatus/1002> ;
	reg:name "composerExpression"@en ;
	rdfs:label "Composer (Expression)"@en ;
	skos:definition "A person, family, or corporate body contributing to an expression by composing new music to substitute for the original music, or by composing new music to supplement the existing music."@en ;
	a :Property ;
	rdfs:subPropertyOf <http://rdvocab.info/roles/contributor> ;
	rdfs:domain <http://rdvocab.info/uri/schema/FRBRentitiesRDA/Expression> ;
	rdfs:label "Komponist (Expression)"@de ;
	skos:definition "Eine Person, Familie oder Körperschaft, die zu einer Expression eines Werkes beiträgt, indem sie als Ersatz für die Originalmusik neue Musik komponiert oder neue Musik komponiert, die die existierende Musik ergänzt."@de .

<http://rdvocab.info/roles/composerOfAdditionalMusic> rdfs:isDefinedBy <http://rdvocab.info/roles> ;
	reg:status <http://metadataregistry.org/uri/RegStatus/1002> ;
	reg:name "composerOfAdditionalMusic"@en ;
	rdfs:label "Composer of Additional Music"@en ;
	skos:definition "A person, family, or corporate body contributing to an expression of a musical work by composing accompaniments or additional parts (e.g., vocal/instrumental parts, musical numbers) that supplement the music written by the original composer."@en ;
	a :Property ;
	rdfs:label "Komponist eines zusätzlichen Musikstückes"@de ;
	skos:definition "Eine Person, Familie oder Körperschaft, die zu einer Expression eines Musikwerkes durch Begleitkompositionen oder Zusätze (wie zusätzliche Parts für Stimmen/Instrumente oder weitere Musikstücke) beiträgt, welche die Musik des ursprünglichen Komponisten ergänzen."@de ;
	reg:hasSubproperty <http://rdvocab.info/roles/composerOfAdditionalMusicExpression> .

<http://rdvocab.info/roles/composerOfAdditionalMusicExpression> rdfs:isDefinedBy <http://rdvocab.info/roles> ;
	reg:status <http://metadataregistry.org/uri/RegStatus/1002> ;
	reg:name "composerOfAdditionalMusicExpression"@en ;
	rdfs:label "Composer of Additional Music (Expression)"@en ;
	skos:definition "A person, family, or corporate body contributing to an expression of a musical work by composing accompaniments or additional parts (e.g., vocal/instrumental parts, musical numbers) that supplement the music written by the original composer."@en ;
	a :Property ;
	rdfs:subPropertyOf <http://rdvocab.info/roles/composerOfAdditionalMusic> .

<http://rdvocab.info/roles/composerOfIncidentalMusic> rdfs:isDefinedBy <http://rdvocab.info/roles> ;
	reg:status <http://metadataregistry.org/uri/RegStatus/1002> ;
	reg:name "composerOfIncidentalMusic"@en ;
	rdfs:label "Composer of Incidental Music"@en ;
	skos:definition "A person, family, or corporate body contributing to an expression of a work by composing music for a pre-existing, usually textual, work."@en ;
	a :Property ;
	rdfs:label "Komponist von Begleitmusik"@de ;
	skos:definition "Eine Person, Familie oder Körperschaft, die zu einer Expression eines Werkes durch die Komposition von Musik für ein bereits bestehendes, meist textliches, Werk beiträgt."@de ;
	reg:hasSubproperty <http://rdvocab.info/roles/composerOfIncidentalMusicExpression> .

<http://rdvocab.info/roles/composerOfIncidentalMusicExpression> rdfs:isDefinedBy <http://rdvocab.info/roles> ;
	reg:status <http://metadataregistry.org/uri/RegStatus/1002> ;
	reg:name "composerOfIncidentalMusicExpression"@en ;
	rdfs:label "Composer of Incidental Music (Expression)"@en ;
	skos:definition "A person, family, or corporate body contributing to an expression of a work by composing music for a pre-existing, usually textual, work."@en ;
	a :Property ;
	rdfs:subPropertyOf <http://rdvocab.info/roles/composerOfIncidentalMusic> .

<http://rdvocab.info/roles/composerOfMusicForSilentFilm> rdfs:isDefinedBy <http://rdvocab.info/roles> ;
	reg:status <http://metadataregistry.org/uri/RegStatus/1002> ;
	reg:name "composerOfMusicForSilentFilm"@en ;
	rdfs:label "Composer of Music for Silent Film"@en ;
	skos:definition "A person, family, or corporate body responsible for contributing compositions to accompany the presentation of a moving image work produced in the silent film era and recorded without a synchronized, integrated soundtrack. These musical works may be originally written for the moving image or may consist of or incorporate pre-existing works in a manner that is intended to complement the moving image."@en ;
	a :Property ;
	rdfs:label "Komponist von Stummfilm-Musik"@de ;
	skos:definition "Eine Person, Familie oder Körperschaft, die für Kompositionen zur Begleitung von Bewegtbildwerken aus der Stummfilmzeit, die ohne synchronisierten und integrierten Ton aufgenommen wurden, verantwortlich ist. Diese Musikwerke können entweder eigens für das bewegte Bild geschrieben sein oder aber aus bereits existierenden Werken bestehen bzw. sich zusammensetzen, die vorgesehen sind, das bewegte Bild zu ergänzen."@de ;
	reg:hasSubproperty <http://rdvocab.info/roles/composerOfMusicForSilentFilmExpression> .

<http://rdvocab.info/roles/composerOfMusicForSilentFilmExpression> rdfs:isDefinedBy <http://rdvocab.info/roles> ;
	reg:status <http://metadataregistry.org/uri/RegStatus/1002> ;
	reg:name "composerOfMusicForSilentFilmExpression"@en ;
	rdfs:label "Composer of Music for Silent Film (Expression)"@en ;
	skos:definition "A person, family, or corporate body responsible for contributing compositions to accompany the presentation of a moving image work produced in the silent film era and recorded without a synchronized, integrated soundtrack. These musical works may be originally written for the moving image or may consist of or incorporate pre-existing works in a manner that is intended to complement the moving image."@en ;
	a :Property ;
	rdfs:subPropertyOf <http://rdvocab.info/roles/composerOfMusicForSilentFilm> .

<http://rdvocab.info/roles/composerOfMusicForSoundFilm> rdfs:isDefinedBy <http://rdvocab.info/roles> ;
	reg:status <http://metadataregistry.org/uri/RegStatus/1002> ;
	reg:name "composerOfMusicForSoundFilm"@en ;
	rdfs:label "Composer of Music for Sound Film"@en ;
	skos:definition "A person, family, or corporate body responsible for contributing compositions that form part of the presentation of a moving image work recorded with a synchronized, integrated soundtrack. These musical works may be originally written for the moving image or be pre-existing works that are incorporated into the moving image soundtrack."@en ;
	a :Property ;
	rdfs:label "Filmkomponist"@de ;
	reg:hasSubproperty <http://rdvocab.info/roles/composerOfMusicForSoundFilmExpression> ;
	skos:definition "Eine Person, Familie oder Körperschaft, die für Kompositionen verantwortlich ist, die einen Teil eines Bewegtbildwerkes  bilden, das mit synchronisiertem und integriertem Ton aufgenommen wurde. Diese Musikwerke können entweder eigens für das bewegte Bild geschriebene oder bereits bestehende Werke sein, die in den Bewegtbildsoundtrack eingebunden wurden."@de .

<http://rdvocab.info/roles/composerOfMusicForSoundFilmExpression> rdfs:isDefinedBy <http://rdvocab.info/roles> ;
	reg:status <http://metadataregistry.org/uri/RegStatus/1002> ;
	reg:name "composerOfMusicForSoundFilmExpression"@en ;
	rdfs:label "Composer of Music for Sound Film (Expression)"@en ;
	skos:definition "A person, family, or corporate body responsible for contributing compositions that form part of the presentation of a moving image work recorded with a synchronized, integrated soundtrack. These musical works may be originally written for the moving image or be pre-existing works that are incorporated into the moving image soundtrack."@en ;
	a :Property ;
	rdfs:subPropertyOf <http://rdvocab.info/roles/composerOfMusicForSoundFilm> ;
	rdfs:label "Filmkomponist (Expression)"@de ;
	skos:definition "Eine Person, Familie oder Körperschaft, die für Kompositionen verantwortlich ist, die einen Teil eines Bewegtbildwerkes  bilden, das mit synchronisiertem und integriertem Ton aufgenommen wurde. Diese Musikwerke können entweder eigens für das bewegte Bild geschriebene oder bereits bestehende Werke sein, die in den Bewegtbildsoundtrack eingebunden wurden."@de .

<http://rdvocab.info/roles/composerWork> rdfs:isDefinedBy <http://rdvocab.info/roles> ;
	reg:status <http://metadataregistry.org/uri/RegStatus/1002> ;
	reg:name "composerWork"@en ;
	rdfs:label "Composer (Work)"@en ;
	skos:definition "A person, family, or corporate body responsible for creating a musical work. Use also for persons, etc., adapting another musical work to form a distinct alteration (e.g., free transcription), paraphrasing a work or creating a work in the general style of another composer, or creating a work that is based on the music of another composer (e.g., variations on a theme)."@en ;
	a :Property ;
	rdfs:subPropertyOf <http://rdvocab.info/roles/creator> ;
	rdfs:domain <http://rdvocab.info/uri/schema/FRBRentitiesRDA/Work> ;
	rdfs:label "Komponist (Werk)"@de ;
	skos:definition "Eine Person, Familie oder Körperschaft, die für ein Musikwerk verantwortlich ist. Die Bezeichnung wird auch für Personen usw. verwendet, die ein anderes Musikwerk adaptiert haben, das sich deutlich vom Original unterscheidet, beispielsweise eine freie Bearbeitung. Oder die ein Werk im Stil eines anderen Komponisten umgeschrieben oder erschaffen hat oder ein Werk, das auf der Musik eines anderen Komponisten basiert, wie beispielsweise Variationen eines Themas."@de .

<http://rdvocab.info/roles/conductor> rdfs:isDefinedBy <http://rdvocab.info/roles> ;
	reg:status <http://metadataregistry.org/uri/RegStatus/1002> ;
	reg:name "conductor"@en ;
	rdfs:label "Conductor"@en ;
	a :Property ;
	rdfs:subPropertyOf <http://rdvocab.info/roles/performer> ;
	rdfs:label "Dirigent"@de .

<http://rdvocab.info/roles/conductorExpression> rdfs:isDefinedBy <http://rdvocab.info/roles> ;
	reg:status <http://metadataregistry.org/uri/RegStatus/1002> ;
	reg:name "conductorExpression"@en ;
	rdfs:label "Conductor (Expression)"@en ;
	skos:definition "A performer contributing to an expression of a musical work by leading a performing group (orchestra, chorus, opera, etc.) in a musical or dramatic presentation, etc."@en ;
	a :Property ;
	rdfs:domain <http://rdvocab.info/uri/schema/FRBRentitiesRDA/Expression> ;
	rdfs:label "Dirigent (Expression)"@de ;
	skos:definition "Jemand, der zu einer Expression eines Musikwerkes beiträgt, indem er ein aufführendes Ensemble (Orchester, Chor, Oper usw.) in einer musikalischen oder darstellenden Vorführung leitet."@de .

<http://rdvocab.info/roles/contributor> rdfs:isDefinedBy <http://rdvocab.info/roles> ;
	reg:status <http://metadataregistry.org/uri/RegStatus/1002> ;
	reg:name "contributor"@en ;
	rdfs:label "Contributor"@en ;
	skos:definition "A person, family, or corporate body contributing to the realization of a work through an expression. Contributors include editors, translators, arrangers of music, performers, etc."@en ;
	a :Property ;
	rdfs:domain <http://rdvocab.info/uri/schema/FRBRentitiesRDA/Expression> ;
	reg:hasSubproperty <http://rdvocab.info/roles/abridgerExpression> , <http://rdvocab.info/roles/animatorExpression> , <http://rdvocab.info/roles/arrangerOfMusicExpression> , <http://rdvocab.info/roles/artDirectorExpression> , <http://rdvocab.info/roles/choreographerExpression> , <http://rdvocab.info/roles/composerExpression> , <http://rdvocab.info/roles/courtReporterExpression> , <http://rdvocab.info/roles/costumeDesignerExpression> , <http://rdvocab.info/roles/draftsmanExpression> , <http://rdvocab.info/roles/editorExpression> , <http://rdvocab.info/roles/editorOfCompilationExpression> , <http://rdvocab.info/roles/editorOfMovingImageWorkExpression> , <http://rdvocab.info/roles/illustratorExpression> , <http://rdvocab.info/roles/intervieweeExpression> , <http://rdvocab.info/roles/interviewerExpression> , <http://rdvocab.info/roles/musicalDirectorExpression> , <http://rdvocab.info/roles/performerExpression> , <http://rdvocab.info/roles/presenterExpression> , <http://rdvocab.info/roles/productionDesignerExpression> , <http://rdvocab.info/roles/recordingEngineerExpression> , <http://rdvocab.info/roles/recordistExpression> , <http://rdvocab.info/roles/stageDirectorExpression> , <http://rdvocab.info/roles/surveyorExpression> , <http://rdvocab.info/roles/transcriberExpression> , <http://rdvocab.info/roles/translatorExpression> , <http://rdvocab.info/roles/writerOfAddedCommentaryExpression> , <http://rdvocab.info/roles/writerOfAddedTextExpression> ;
	rdfs:label "Mitwirkender"@de ;
	skos:definition "Eine Person, Familie oder Körperschaft, die an der Realisierung eines Werkes durch eine Expression mitwirkt. Zu den Mitwirkenden gehören Herausgeber, Übersetzer, Arrangeure/Bearbeiter für Musik, Darsteller, usw."@de .

<http://rdvocab.info/roles/costumeDesigner> rdfs:isDefinedBy <http://rdvocab.info/roles> ;
	reg:status <http://metadataregistry.org/uri/RegStatus/1002> ;
	reg:name "costumeDesigner"@en ;
	rdfs:label "Costume designer"@en ;
	a :Property ;
	rdfs:label "Kostümbildner"@de .

<http://rdvocab.info/roles/costumeDesignerExpression> rdfs:isDefinedBy <http://rdvocab.info/roles> ;
	reg:status <http://metadataregistry.org/uri/RegStatus/1002> ;
	reg:name "costumeDesignerExpression"@en ;
	rdfs:label "Costume designer (Expression)"@en ;
	skos:definition "A person, family, or corporate body responsible for designing the costumes for a moving image production or for a musical or dramatic presentation or entertainment."@en ;
	a :Property ;
	rdfs:subPropertyOf <http://rdvocab.info/roles/contributor> ;
	rdfs:domain <http://rdvocab.info/uri/schema/FRBRentitiesRDA/Expression> ;
	rdfs:label "Kostümbildner (Expression)"@de ;
	skos:definition "Eine Person, Familie oder Körperschaft, die für das Design der Kostüme für eine Bewegtbildproduktion, ein Musical, eine Theateraufführung oder Entertainment verantwortlich ist."@de .

<http://rdvocab.info/roles/courtGoverned> rdfs:isDefinedBy <http://rdvocab.info/roles> ;
	reg:status <http://metadataregistry.org/uri/RegStatus/1002> ;
	reg:name "courtGoverned"@en ;
	rdfs:label "Court governed"@en ;
	a :Property ;
	reg:hasSubproperty <http://rdvocab.info/roles/courtGovernedWork> ;
	rdfs:label "Court governed"@de ;
	skos:definition "Ein Gericht geregelt von der Prozessordnung (unabhängig von deren förmlicher Rechtsnatur, zum Beispiel Gesetze, Verwaltungsvorschriften)."@de .

<http://rdvocab.info/roles/courtGovernedWork> rdfs:isDefinedBy <http://rdvocab.info/roles> ;
	reg:status <http://metadataregistry.org/uri/RegStatus/1002> ;
	reg:name "courtGovernedWork"@en ;
	rdfs:label "Court governed (Work)"@en ;
	skos:definition "A court governed by court rules (regardless of their official nature, e.g., laws, administrative regulations)."@en ;
	a :Property ;
	rdfs:domain <http://rdvocab.info/uri/schema/FRBRentitiesRDA/Work> ;
	rdfs:subPropertyOf <http://rdvocab.info/roles/courtGoverned> ;
	rdfs:label "Court governed"@de ;
	skos:definition "Ein Gericht geregelt von der Prozessordnung (unabhängig von deren förmlicher Rechtsnatur, zum Beispiel Gesetze, Verwaltungsvorschriften)."@de .

<http://rdvocab.info/roles/courtReporter> rdfs:isDefinedBy <http://rdvocab.info/roles> ;
	reg:status <http://metadataregistry.org/uri/RegStatus/1002> ;
	reg:name "courtReporter"@en ;
	rdfs:label "Court reporter"@en ;
	a :Property ;
	rdfs:label "Gerichtsstenograf"@de ;
	skos:definition "Eine Person, Familie oder Körperschaft, die zu einer Expression eines Werkes beiträgt, indem sie die Auffassung eines Gerichts zur Veröffentlichung vorbereitet."@de .

<http://rdvocab.info/roles/courtReporterExpression> rdfs:isDefinedBy <http://rdvocab.info/roles> ;
	reg:status <http://metadataregistry.org/uri/RegStatus/1002> ;
	reg:name "courtReporterExpression"@en ;
	rdfs:label "Court reporter (Expression)"@en ;
	skos:definition "The person, family, or corporate body contributing to an expression of a work by preparing a court’s opinions for publication."@en ;
	a :Property ;
	rdfs:subPropertyOf <http://rdvocab.info/roles/contributor> ;
	rdfs:domain <http://rdvocab.info/uri/schema/FRBRentitiesRDA/Expression> ;
	rdfs:label "Gerichtsstenograf (Expression)"@de ;
	skos:definition "Eine Person, Familie oder Körperschaft, die zu einer Expression eines Werkes beiträgt, indem sie die Auffassung eines Gerichts zur Veröffentlichung vorbereitet."@de .

<http://rdvocab.info/roles/creator> rdfs:isDefinedBy <http://rdvocab.info/roles> ;
	reg:status <http://metadataregistry.org/uri/RegStatus/1002> ;
	reg:name "creator"@en ;
	rdfs:label "Creator"@en ;
	skos:definition "A person, family, or corporate body responsible for the creation of a work."@en ;
	a :Property ;
	rdfs:domain <http://rdvocab.info/uri/schema/FRBRentitiesRDA/Work> ;
	reg:hasSubproperty <http://rdvocab.info/roles/architectWork> , <http://rdvocab.info/roles/artistWork> , <http://rdvocab.info/roles/authorWork> , <http://rdvocab.info/roles/cartographerWork> , <http://rdvocab.info/roles/choreographerWork> , <http://rdvocab.info/roles/compilerWork> , <http://rdvocab.info/roles/composerWork> , <http://rdvocab.info/roles/designerWork> , <http://rdvocab.info/roles/enactingJurisdictionWork> , <http://rdvocab.info/roles/filmmakerWork> , <http://rdvocab.info/roles/intervieweeWork> , <http://rdvocab.info/roles/interviewerWork> , <http://rdvocab.info/roles/inventorWork> , <http://rdvocab.info/roles/photographerWork> , <http://rdvocab.info/roles/praesesWork> , <http://rdvocab.info/roles/programmerWork> , <http://rdvocab.info/roles/respondentWork> ;
	rdfs:label "geistiger Schöpfer"@de ;
	skos:definition "Eine Person, Familie oder Körperschaft, die für die Schaffung eines Werkes verantwortlich ist."@de .

<http://rdvocab.info/roles/curator> rdfs:isDefinedBy <http://rdvocab.info/roles> ;
	reg:status <http://metadataregistry.org/uri/RegStatus/1002> ;
	reg:name "curator"@en ;
	rdfs:label "Curator"@en ;
	a :Property ;
	reg:hasSubproperty <http://rdvocab.info/roles/curatorItem> , <http://rdvocab.info/roles/collector> , <http://rdvocab.info/roles/collectionRegistrar> ;
	rdfs:label "Kurator"@de .

<http://rdvocab.info/roles/curatorItem> rdfs:isDefinedBy <http://rdvocab.info/roles> ;
	reg:status <http://metadataregistry.org/uri/RegStatus/1002> ;
	reg:name "curatorItem"@en ;
	rdfs:label "Curator (Item)"@en ;
	skos:definition "A person, family, or corporate body conceiving, aggregating, and/or organizing an exhibition, collection, or other item."@en ;
	a :Property ;
	rdfs:domain <http://rdvocab.info/uri/schema/FRBRentitiesRDA/Item> ;
	rdfs:subPropertyOf <http://rdvocab.info/roles/curator> ;
	rdfs:label "Kurator (Exemplar)"@de ;
	skos:definition "Eine Person, Familie oder Körperschaft, die Zusammenstellungen entwirft und/oder eine Ausstellung, eine Sammlung oder andere Exemplare organisiert."@de .

<http://rdvocab.info/roles/currentOwner> rdfs:isDefinedBy <http://rdvocab.info/roles> ;
	reg:status <http://metadataregistry.org/uri/RegStatus/1002> ;
	reg:name "currentOwner"@en ;
	rdfs:label "Current owner"@en ;
	a :Property ;
	rdfs:subPropertyOf <http://rdvocab.info/roles/owner> ;
	reg:hasSubproperty <http://rdvocab.info/roles/depositor> ;
	rdfs:label "Derzeitiger Besitzer"@de .

<http://rdvocab.info/roles/currentOwnerItem> rdfs:isDefinedBy <http://rdvocab.info/roles> ;
	reg:status <http://metadataregistry.org/uri/RegStatus/1002> ;
	reg:name "currentOwnerItem"@en ;
	rdfs:label "Current owner (Item)"@en ;
	skos:definition "A person, family, or corporate body currently having legal possession of an item (i.e., a specific copy or instance of a resource)."@en ;
	a :Property ;
	rdfs:subPropertyOf <http://rdvocab.info/roles/ownerItem> ;
	rdfs:domain <http://rdvocab.info/uri/schema/FRBRentitiesRDA/Item> ;
	rdfs:label "Derzeitiger Besitzer (Exemplar)"@de ;
	skos:definition "Eine Person, Familie oder Körperschaft, die derzeit rechtmäßig im Besitz eines Exemplars ist (z. B. einer bestimmten Kopie oder eines bestimmten Exemplars einer Ressource)."@de .

<http://rdvocab.info/roles/custodian> rdfs:isDefinedBy <http://rdvocab.info/roles> ;
	reg:status <http://metadataregistry.org/uri/RegStatus/1002> ;
	reg:name "custodian"@en ;
	rdfs:label "Custodian"@en ;
	a :Property ;
	reg:hasSubproperty <http://rdvocab.info/roles/custodianItem> ;
	rdfs:label "Besitzer"@de ;
	skos:definition "Eine Person, Familie oder Körperschaft, die der rechtmäßige Besitzer eines Objekts ist (d.h., einer bestimmten Kopie oder Instanz einer Ressource)."@de .

<http://rdvocab.info/roles/custodianItem> rdfs:isDefinedBy <http://rdvocab.info/roles> ;
	reg:status <http://metadataregistry.org/uri/RegStatus/1002> ;
	reg:name "custodianItem"@en ;
	rdfs:label "Custodian (Item)"@en ;
	skos:definition "A person, family, or corporate body having legal custody of an item (i.e., a specific copy or instance of a resource)."@en ;
	a :Property ;
	rdfs:domain <http://rdvocab.info/uri/schema/FRBRentitiesRDA/Item> ;
	rdfs:subPropertyOf <http://rdvocab.info/roles/custodian> ;
	rdfs:label "Besitzer (Exemplar)"@de ;
	skos:definition "Eine Person, Familie oder Körperschaft, die der rechtmäßige Besitzer eines Objekts ist (d.h., einer bestimmten Kopie oder Instanz einer Ressource)."@de .

<http://rdvocab.info/roles/dancer> rdfs:isDefinedBy <http://rdvocab.info/roles> ;
	reg:status <http://metadataregistry.org/uri/RegStatus/1002> ;
	reg:name "dancer"@en ;
	rdfs:label "Dancer"@en ;
	a :Property ;
	rdfs:subPropertyOf <http://rdvocab.info/roles/performer> ;
	rdfs:label "Tänzer"@de .

<http://rdvocab.info/roles/dancerExpression> rdfs:isDefinedBy <http://rdvocab.info/roles> ;
	reg:status <http://metadataregistry.org/uri/RegStatus/1002> ;
	reg:name "dancerExpression"@en ;
	rdfs:label "Dancer (Expression)"@en ;
	skos:definition "A performer contributing to an expression of a work by dancing in a musical, dramatic, etc., presentation."@en ;
	a :Property ;
	rdfs:subPropertyOf <http://rdvocab.info/roles/performerExpression> ;
	rdfs:domain <http://rdvocab.info/uri/schema/FRBRentitiesRDA/Expression> ;
	rdfs:label "Tänzer (Expression)"@de ;
	skos:definition "Ein Darsteller, der durch Tanzen in einer musikalischen, dramatischen oder ähnlichen Darbietung an einer Expression eines Werkes mitwirkt."@de .

<http://rdvocab.info/roles/dedicatee> rdfs:isDefinedBy <http://rdvocab.info/roles> ;
	reg:status <http://metadataregistry.org/uri/RegStatus/1002> ;
	reg:name "dedicatee"@en ;
	rdfs:label "Dedicatee"@en ;
	a :Property ;
	reg:hasSubproperty <http://rdvocab.info/roles/dedicateeWork> , <http://rdvocab.info/roles/dedicateeOfItem> ;
	rdfs:label "Person, der ein Werk gewidmet ist"@de .

<http://rdvocab.info/roles/dedicateeOfItem> rdfs:isDefinedBy <http://rdvocab.info/roles> ;
	reg:status <http://metadataregistry.org/uri/RegStatus/1002> ;
	reg:name "dedicateeOfItem"@en ;
	rdfs:label "Dedicatee of Item"@en ;
	skos:definition "A person, family, or corporate body to whom an item is dedicated."@en ;
	a :Property ;
	rdfs:domain <http://rdvocab.info/uri/schema/FRBRentitiesRDA/Item> ;
	rdfs:subPropertyOf <http://rdvocab.info/roles/dedicatee> ;
	rdfs:label "Person, der ein Exemplar gewidmet ist"@de ;
	skos:definition "Eine Person, Familie oder Körperschaft, der ein Exemplar gewidmet ist."@de .

<http://rdvocab.info/roles/dedicateeWork> rdfs:isDefinedBy <http://rdvocab.info/roles> ;
	reg:status <http://metadataregistry.org/uri/RegStatus/1002> ;
	reg:name "dedicateeWork"@en ;
	rdfs:label "Dedicatee (Work)"@en ;
	skos:definition "A person, family, or corporate body to whom the work is dedicated."@en ;
	a :Property ;
	rdfs:domain <http://rdvocab.info/uri/schema/FRBRentitiesRDA/Work> ;
	rdfs:subPropertyOf <http://rdvocab.info/roles/dedicatee> ;
	rdfs:label "Person, der ein Werk gewidmet ist"@de ;
	skos:definition "Eine Person, Familie oder Körperschaft, der das Werk gewidmet ist."@de .

<http://rdvocab.info/roles/defendant> rdfs:isDefinedBy <http://rdvocab.info/roles> ;
	reg:status <http://metadataregistry.org/uri/RegStatus/1002> ;
	reg:name "defendant"@en ;
	rdfs:label "Defendant"@en ;
	a :Property ;
	reg:hasSubproperty <http://rdvocab.info/roles/defendantWork> ;
	rdfs:label "Angeklagter/Beklagter (Werk)"@de .

<http://rdvocab.info/roles/defendantWork> rdfs:isDefinedBy <http://rdvocab.info/roles> ;
	reg:status <http://metadataregistry.org/uri/RegStatus/1002> ;
	reg:name "defendantWork"@en ;
	rdfs:label "Defendant (Work)"@en ;
	skos:definition "A person or corporate body who is accused in a criminal proceeding or sued in a civil proceeding."@en ;
	a :Property ;
	rdfs:domain <http://rdvocab.info/uri/schema/FRBRentitiesRDA/Work> ;
	rdfs:subPropertyOf <http://rdvocab.info/roles/defendant> ;
	rdfs:label "Angeklagter/Beklagter (Werk)"@de ;
	skos:definition "Eine Person oder Körperschaft, die in einem Strafverfahren angeklagt oder in einem Zivilprozess verklagt ist."@de .

<http://rdvocab.info/roles/degreeGrantingInstitution> rdfs:isDefinedBy <http://rdvocab.info/roles> ;
	reg:status <http://metadataregistry.org/uri/RegStatus/1002> ;
	reg:name "degreeGrantingInstitution"@en ;
	rdfs:label "Degree granting institution"@en ;
	a :Property ;
	reg:hasSubproperty <http://rdvocab.info/roles/degreeGrantingInstitutionWork> ;
	rdfs:label "Institution, die einen akademischen Grad verleiht"@de ;
	skos:definition "Eine Körperschaft, die einen akademischen Grad verleiht, z.T. basierend auf der Einreichung einer Hochschulschrift o.ä."@de .

<http://rdvocab.info/roles/degreeGrantingInstitutionWork> rdfs:isDefinedBy <http://rdvocab.info/roles> ;
	reg:status <http://metadataregistry.org/uri/RegStatus/1002> ;
	reg:name "degreeGrantingInstitutionWork"@en ;
	rdfs:label "Degree granting institution (Work)"@en ;
	skos:definition "A corporate body granting an academic degree, based in part on the submission of a thesis, dissertation, etc."@en ;
	a :Property ;
	rdfs:domain <http://rdvocab.info/uri/schema/FRBRentitiesRDA/Work> ;
	rdfs:subPropertyOf <http://rdvocab.info/roles/degreeGrantingInstitution> ;
	rdfs:label "Institution, die einen akademischen Grad verleiht (Werk)"@de ;
	skos:definition "Eine Körperschaft, die einen akademischen Grad verleiht, z.T. basierend auf der Einreichung einer Hochschulschrift o.ä."@de .

<http://rdvocab.info/roles/depositor> rdfs:isDefinedBy <http://rdvocab.info/roles> ;
	reg:status <http://metadataregistry.org/uri/RegStatus/1002> ;
	reg:name "depositor"@en ;
	rdfs:label "Depositor"@en ;
	a :Property ;
	rdfs:subPropertyOf <http://rdvocab.info/roles/currentOwner> ;
	rdfs:label "Leihgeber"@de .

<http://rdvocab.info/roles/depositorItem> rdfs:isDefinedBy <http://rdvocab.info/roles> ;
	reg:status <http://metadataregistry.org/uri/RegStatus/1002> ;
	reg:name "depositorItem"@en ;
	rdfs:label "Depositor (Item)"@en ;
	skos:definition "A current owner of an item who deposited the item into the custody of another person, family, or corporate body, while still retaining ownership."@en ;
	a :Property ;
	rdfs:domain <http://rdvocab.info/uri/schema/FRBRentitiesRDA/Item> ;
	rdfs:label "Leihgeber (Exemplar)"@de ;
	skos:definition "Der gegenwärtige Eigentümer eines Exemplars, der das Exemplar in die Obhut einer anderen Person, Familie oder Körperschaft gegeben hat, während er weiterhin der Eigentümer bleibt."@de .

<http://rdvocab.info/roles/designer> rdfs:isDefinedBy <http://rdvocab.info/roles> ;
	reg:status <http://metadataregistry.org/uri/RegStatus/1002> ;
	reg:name "designer"@en ;
	rdfs:label "Designer"@en ;
	a :Property ;
	rdfs:label "Designer"@de .

<http://rdvocab.info/roles/designerWork> rdfs:isDefinedBy <http://rdvocab.info/roles> ;
	reg:status <http://metadataregistry.org/uri/RegStatus/1002> ;
	reg:name "designerWork"@en ;
	rdfs:label "Designer (Work)"@en ;
	skos:definition "A person, family, or corporate body responsible for creating a design for an object."@en ;
	a :Property ;
	rdfs:subPropertyOf <http://rdvocab.info/roles/creator> ;
	rdfs:domain <http://rdvocab.info/uri/schema/FRBRentitiesRDA/Work> ;
	rdfs:label "Designer (Werk)"@de ;
	skos:definition "Eine Person, Familie oder Körperschaft, die für die Gestaltung des Designs eines Objekts verantwortlich ist."@de .

<http://rdvocab.info/roles/director> rdfs:isDefinedBy <http://rdvocab.info/roles> ;
	reg:status <http://metadataregistry.org/uri/RegStatus/1002> ;
	reg:name "director"@en ;
	rdfs:label "Director"@en ;
	a :Property ;
	reg:hasSubproperty <http://rdvocab.info/roles/directorWork> , <http://rdvocab.info/roles/filmDirector> , <http://rdvocab.info/roles/radioDirector> , <http://rdvocab.info/roles/televisionDirector> ;
	rdfs:label "Director"@de ;
	skos:definition "Eine Person, Familie oder Körperschaft, die für die allgemeine Leitung und Betreuung einer verfilmten Aufführung, einer Radio- oder Fernsehsendung usw. verantwortlich ist."@de .

<http://rdvocab.info/roles/directorOfPhotography> rdfs:isDefinedBy <http://rdvocab.info/roles> ;
	reg:status <http://metadataregistry.org/uri/RegStatus/1002> ;
	reg:name "directorOfPhotography"@en ;
	rdfs:label "Director of photography"@en ;
	a :Property ;
	reg:hasSubproperty <http://rdvocab.info/roles/directorOfPhotographyWork> ;
	rdfs:label "Verantwortlicher Kameramann"@de .

<http://rdvocab.info/roles/directorOfPhotographyWork> rdfs:isDefinedBy <http://rdvocab.info/roles> ;
	reg:status <http://metadataregistry.org/uri/RegStatus/1002> ;
	reg:name "directorOfPhotographyWork"@en ;
	rdfs:label "Director of photography (Work)"@en ;
	skos:definition "A person, family, or corporate body that captures images, either electronically or on film or video stock, and often selects and arranges the lighting. The director of photography for a movie is also called the chief cinematographer."@en ;
	a :Property ;
	rdfs:comment "Use this designation also for videographers."@en ;
	rdfs:domain <http://rdvocab.info/uri/schema/FRBRentitiesRDA/Work> ;
	rdfs:subPropertyOf <http://rdvocab.info/roles/directorOfPhotography> ;
	rdfs:label "Verantwortlicher Kameramann (Werk)"@de ;
	skos:definition "Eine Person, Familie oder Körperschaft, die Bilder festhält, entweder elektronisch oder auf Film- oder Videomaterial, und häufig die Belichtung auswählt und arrangiert. Der verantwortliche Kameramann für einen Film wird auch als \"Leitender Kamermann\" bezeichnet. Diese Bezeichnung wird auch für \"Videograph\" verwendet."@de .

<http://rdvocab.info/roles/directorWork> rdfs:isDefinedBy <http://rdvocab.info/roles> ;
	reg:status <http://metadataregistry.org/uri/RegStatus/1002> ;
	reg:name "directorWork"@en ;
	rdfs:label "Director (Work)"@en ;
	skos:definition "A person, family, or corporate body responsible for the general management and supervision of a filmed performance, a radio or television program, etc."@en ;
	a :Property ;
	rdfs:subPropertyOf <http://rdvocab.info/roles/director> ;
	rdfs:domain <http://rdvocab.info/uri/schema/FRBRentitiesRDA/Work> ;
	reg:hasSubproperty <http://rdvocab.info/roles/filmDirectorWork> , <http://rdvocab.info/roles/radioDirectorWork> , <http://rdvocab.info/roles/televisionDirectorWork> .

<http://rdvocab.info/roles/distributor> rdfs:isDefinedBy <http://rdvocab.info/roles> ;
	reg:status <http://metadataregistry.org/uri/RegStatus/1002> ;
	reg:name "distributor"@en ;
	rdfs:label "Distributor"@en ;
	a :Property ;
	reg:hasSubproperty <http://rdvocab.info/roles/distributorManifestation> , <http://rdvocab.info/roles/filmDistributor> ;
	rdfs:label "Vertrieb"@de ;
	skos:definition "Eine Person, Familie oder Körperschaft, die für den Vertrieb einer Ressource verantwortlich ist."@de .

<http://rdvocab.info/roles/distributorManifestation> rdfs:isDefinedBy <http://rdvocab.info/roles> ;
	reg:status <http://metadataregistry.org/uri/RegStatus/1002> ;
	reg:name "distributorManifestation"@en ;
	rdfs:label "Distributor (Manifestation)"@en ;
	skos:definition "A person, family, or corporate body responsible for distributing a resource."@en ;
	a :Property ;
	rdfs:subPropertyOf <http://rdvocab.info/roles/distributor> ;
	rdfs:domain <http://rdvocab.info/uri/schema/FRBRentitiesRDA/Manifestation> ;
	reg:hasSubproperty <http://rdvocab.info/roles/filmDistributorManifestation> ;
	skos:definition "Eine Person, Familie oder Körperschaft, die für den Vertrieb einer Ressource verantwortlich ist."@de ;
	rdfs:label "Vertrieb (Manifestation)"@de .

<http://rdvocab.info/roles/donor> rdfs:isDefinedBy <http://rdvocab.info/roles> ;
	reg:status <http://metadataregistry.org/uri/RegStatus/1002> ;
	reg:name "donor"@en ;
	rdfs:label "Donor"@en ;
	a :Property ;
	rdfs:subPropertyOf <http://rdvocab.info/roles/formerOwner> ;
	rdfs:label "Stifter"@de .

<http://rdvocab.info/roles/donorItem> rdfs:isDefinedBy <http://rdvocab.info/roles> ;
	reg:status <http://metadataregistry.org/uri/RegStatus/1002> ;
	reg:name "donorItem"@en ;
	rdfs:label "Donor (Item)"@en ;
	skos:definition "A former owner of an item who donated that item to the another owner."@en ;
	a :Property ;
	rdfs:subPropertyOf <http://rdvocab.info/roles/formerOwnerItem> ;
	rdfs:domain <http://rdvocab.info/uri/schema/FRBRentitiesRDA/Item> ;
	rdfs:label "Stifter (Exemplar)"@de ;
	skos:definition "Ein ehemaliger Eigentümer eines Exemplars, der dieses Exemplar jemand anderem überlassen hat."@de .

<http://rdvocab.info/roles/draftsman> rdfs:isDefinedBy <http://rdvocab.info/roles> ;
	reg:status <http://metadataregistry.org/uri/RegStatus/1002> ;
	reg:name "draftsman"@en ;
	rdfs:label "Draftsman"@en ;
	a :Property ;
	rdfs:label "Technischer Zeichner"@de .

<http://rdvocab.info/roles/draftsmanExpression> rdfs:isDefinedBy <http://rdvocab.info/roles> ;
	reg:status <http://metadataregistry.org/uri/RegStatus/1002> ;
	reg:name "draftsmanExpression"@en ;
	rdfs:label "Draftsman (Expression)"@en ;
	skos:definition "A person, family, or corporate body contributing to an expression of a work by an architect, inventor, etc., by making detailed plans or drawings for buildings, ships, aircraft, machines, objects, etc."@en ;
	a :Property ;
	rdfs:subPropertyOf <http://rdvocab.info/roles/contributor> ;
	rdfs:domain <http://rdvocab.info/uri/schema/FRBRentitiesRDA/Expression> ;
	rdfs:label "Technischer Zeichner (Expression)"@de ;
	skos:definition "Eine Person, Familie oder Körperschaft, die an einer Expression eines Werkes eines Architekten, Erfinders oder ähnlichen mitwirkt, indem sie detaillierte Pläne oder Zeichnungen für Gebäude, Schiffe, Flugzeuge, Maschinen, Objekte o.ä. erstellt."@de .

<http://rdvocab.info/roles/editor> rdfs:isDefinedBy <http://rdvocab.info/roles> ;
	reg:status <http://metadataregistry.org/uri/RegStatus/1002> ;
	reg:name "editor"@en ;
	rdfs:label "Editor"@en ;
	a :Property ;
	rdfs:label "Herausgeber"@de .

<http://rdvocab.info/roles/editorExpression> rdfs:isDefinedBy <http://rdvocab.info/roles> ;
	reg:status <http://metadataregistry.org/uri/RegStatus/1002> ;
	reg:name "editorExpression"@en ;
	rdfs:label "Editor (Expression)"@en ;
	skos:definition "A person, family, or corporate body contributing to an expression of a work by revising or elucidating the content, e.g., adding an introduction, notes, or other critical matter. An editor may also prepare an expression of a work for production, publication, or distribution."@en ;
	a :Property ;
	rdfs:subPropertyOf <http://rdvocab.info/roles/contributor> ;
	rdfs:domain <http://rdvocab.info/uri/schema/FRBRentitiesRDA/Expression> ;
	rdfs:label "Herausgeber (Expression)"@de ;
	skos:definition "Eine Person, Familie oder Körperschaft, die an einer Expression eines Werkes mitwirkt, indem sie den Inhalt überarbeitet oder erläutert, beispielsweise indem sie eine Einleitung oder Anmerkungen oder anderes kritisches Material hinzufügt. Ein Herausgeber kann ebenso eine Expression eines Werkes für die Produktion, die Herausgabe oder den Vertrieb vorbereiten."@de .

<http://rdvocab.info/roles/editorOfCompilation> rdfs:isDefinedBy <http://rdvocab.info/roles> ;
	reg:status <http://metadataregistry.org/uri/RegStatus/1002> ;
	reg:name "editorOfCompilation"@en ;
	rdfs:label "Editor of compilation"@en ;
	a :Property ;
	rdfs:label "Compilation Editor"@de .

<http://rdvocab.info/roles/editorOfCompilationExpression> rdfs:isDefinedBy <http://rdvocab.info/roles> ;
	reg:status <http://metadataregistry.org/uri/RegStatus/1002> ;
	reg:name "editorOfCompilationExpression"@en ;
	rdfs:label "Editor of compilation (Expression)"@en ;
	skos:definition "A person, family, or corporate body contributing to an expression of a collective or aggregate work by selecting and putting together works, or parts of works, by one or more creators. The editor of compilation may also be involved in elucidating the content, e.g., adding an introduction, notes, or other critical matter, of the compilation.  For compilations of data, information, etc., that result in new works, see Compiler."@en ;
	a :Property ;
	rdfs:subPropertyOf <http://rdvocab.info/roles/contributor> ;
	rdfs:domain <http://rdvocab.info/uri/schema/FRBRentitiesRDA/Expression> ;
	rdfs:label "Compilation Editor"@de ;
	skos:definition "Eine Person, Familie oder Körperschaft, die an einem gemeinschaftlichen oder gesammelten Werk mitwirken, indem sie die Werke oder Teile von Werken von einem oder mehreren Schöpfern auswählen und zusammenstellen."@de ;
	skos:scopeNote "For compilations of data, information, etc., that result in new works, see Compiler."@en .

<http://rdvocab.info/roles/editorOfMovingImageWork> rdfs:isDefinedBy <http://rdvocab.info/roles> ;
	reg:status <http://metadataregistry.org/uri/RegStatus/1002> ;
	reg:name "editorOfMovingImageWork"@en ;
	rdfs:label "Editor of moving image work"@en ;
	a :Property ;
	rdfs:label "Cutter"@de .

<http://rdvocab.info/roles/editorOfMovingImageWorkExpression> rdfs:isDefinedBy <http://rdvocab.info/roles> ;
	reg:status <http://metadataregistry.org/uri/RegStatus/1002> ;
	reg:name "editorOfMovingImageWorkExpression"@en ;
	rdfs:label "Editor of moving image work (Expression)"@en ;
	skos:definition "A person, family, or corporate body responsible for assembling, arranging, and trimming film, video, or other moving image formats, including both visual and audio aspects."@en ;
	a :Property ;
	rdfs:subPropertyOf <http://rdvocab.info/roles/contributor> ;
	rdfs:domain <http://rdvocab.info/uri/schema/FRBRentitiesRDA/Expression> ;
	rdfs:label "Cutter (Expression)"@de ;
	skos:definition "Eine Person, Familie oder Körperschaft, die für das Zusammensetzen, Arrangieren und Nachschneiden von Film-, Video- oder anderen Bewegtbildformaten zuständig ist, sowohl Video- als auch Audio-Aspekte umfassend."@de .

<http://rdvocab.info/roles/enactingJurisdiction> rdfs:isDefinedBy <http://rdvocab.info/roles> ;
	reg:status <http://metadataregistry.org/uri/RegStatus/1002> ;
	reg:name "enactingJurisdiction"@en ;
	rdfs:label "Enacting jurisdiction"@en ;
	a :Property ;
	rdfs:label "Normerlassender Rechtsträger"@de .

<http://rdvocab.info/roles/enactingJurisdictionWork> rdfs:isDefinedBy <http://rdvocab.info/roles> ;
	reg:status <http://metadataregistry.org/uri/RegStatus/1002> ;
	reg:name "enactingJurisdictionWork"@en ;
	rdfs:label "Enacting jurisdiction (Work)"@en ;
	skos:definition "A jurisdiction enacting a law, regulation, constitution, court rule, etc."@en ;
	a :Property ;
	rdfs:subPropertyOf <http://rdvocab.info/roles/creator> ;
	rdfs:domain <http://rdvocab.info/uri/schema/FRBRentitiesRDA/Work> ;
	rdfs:label "Normerlassender Rechtsträger (Werk)"@de ;
	skos:definition "Ein Rechtsträger, der Gesetze, Verordnungen, eine Satzung, gerichtliche Anordnungen usw. erlassen kann."@de .

<http://rdvocab.info/roles/engraver> rdfs:isDefinedBy <http://rdvocab.info/roles> ;
	reg:status <http://metadataregistry.org/uri/RegStatus/1002> ;
	reg:name "engraver"@en ;
	rdfs:label "Engraver"@en ;
	a :Property ;
	rdfs:subPropertyOf <http://rdvocab.info/roles/manufacturer> ;
	rdfs:label "Graveur"@de .

<http://rdvocab.info/roles/engraverManifestation> rdfs:isDefinedBy <http://rdvocab.info/roles> ;
	reg:status <http://metadataregistry.org/uri/RegStatus/1002> ;
	reg:name "engraverManifestation"@en ;
	rdfs:label "Engraver (Manifestation)"@en ;
	skos:definition "A person, family, or corporate body involved in manufacturing a manifestation by cutting letters, figures, etc., on a surface such as a wooden or metal plate used for printing."@en ;
	a :Property ;
	rdfs:domain <http://rdvocab.info/uri/schema/FRBRentitiesRDA/Manifestation> ;
	rdfs:subPropertyOf <http://rdvocab.info/roles/manufacturerManifestation> ;
	rdfs:label "Graveur (Manifestation)"@de ;
	skos:definition "Eine Person, Familie oder Körperschaft, die in die Produktion einer Manifestation eingebunden ist, indem sie Buchstaben, Zahlen usw. in eine Oberfläche, wie z.B. eine Holz- oder Metallplatte, die zum Drucken benutzt wird, schneidet."@de .

<http://rdvocab.info/roles/etcher> rdfs:isDefinedBy <http://rdvocab.info/roles> ;
	reg:status <http://metadataregistry.org/uri/RegStatus/1002> ;
	reg:name "etcher"@en ;
	rdfs:label "Etcher"@en ;
	a :Property ;
	rdfs:subPropertyOf <http://rdvocab.info/roles/manufacturer> ;
	rdfs:label "Radierer"@de .

<http://rdvocab.info/roles/etcherManifestation> rdfs:isDefinedBy <http://rdvocab.info/roles> ;
	reg:status <http://metadataregistry.org/uri/RegStatus/1002> ;
	reg:name "etcherManifestation"@en ;
	rdfs:label "Etcher (Manifestation)"@en ;
	skos:definition "A person, family, or corporate body involved in manufacturing a manifestation by subjecting metal, glass, or some other surface used for printing, to acid or another corrosive substance."@en ;
	a :Property ;
	rdfs:domain <http://rdvocab.info/uri/schema/FRBRentitiesRDA/Manifestation> ;
	rdfs:subPropertyOf <http://rdvocab.info/roles/manufacturerManifestation> ;
	rdfs:label "Radierer (Manifestation)"@de ;
	skos:definition "Eine Person, Familie oder Körperschaft, die in die Produktion einer Manifestation eingebunden ist, indem sie Metall, Glas oder eine andere Oberfläche, die zum Drucken benutzt wird, mit Säure oder einer anderen ätzenden Substanz behandelt."@de .

<http://rdvocab.info/roles/filmDirector> rdfs:isDefinedBy <http://rdvocab.info/roles> ;
	reg:status <http://metadataregistry.org/uri/RegStatus/1002> ;
	reg:name "filmDirector"@en ;
	rdfs:label "Film director"@en ;
	a :Property ;
	rdfs:subPropertyOf <http://rdvocab.info/roles/director> ;
	rdfs:label "Filmregisseur"@de .

<http://rdvocab.info/roles/filmDirectorWork> rdfs:isDefinedBy <http://rdvocab.info/roles> ;
	reg:status <http://metadataregistry.org/uri/RegStatus/1002> ;
	reg:name "filmDirectorWork"@en ;
	rdfs:label "Film director (Work)"@en ;
	skos:definition "A director responsible for the general management and supervision of a filmed performance."@en ;
	a :Property ;
	rdfs:subPropertyOf <http://rdvocab.info/roles/directorWork> ;
	rdfs:domain <http://rdvocab.info/uri/schema/FRBRentitiesRDA/Work> ;
	rdfs:label "Filmregisseur (Werk)"@de ;
	skos:definition "Eine Person, Familie oder Körperschaft, die für das allgemeine Management und die Leitung einer verfilmten Darbietung verantwortlich ist."@de .

<http://rdvocab.info/roles/filmDistributor> rdfs:isDefinedBy <http://rdvocab.info/roles> ;
	reg:status <http://metadataregistry.org/uri/RegStatus/1002> ;
	reg:name "filmDistributor"@en ;
	rdfs:label "Film distributor"@en ;
	a :Property ;
	rdfs:subPropertyOf <http://rdvocab.info/roles/distributor> ;
	rdfs:label "Filmverleiher"@de .

<http://rdvocab.info/roles/filmDistributorManifestation> rdfs:isDefinedBy <http://rdvocab.info/roles> ;
	reg:status <http://metadataregistry.org/uri/RegStatus/1002> ;
	reg:name "filmDistributorManifestation"@en ;
	rdfs:label "Film distributor (Manifestation)"@en ;
	skos:definition "A person, family, or corporate body responsible for distributing a moving image manifestation to theatres or other distribution channels."@en ;
	a :Property ;
	rdfs:domain <http://rdvocab.info/uri/schema/FRBRentitiesRDA/Manifestation> ;
	rdfs:subPropertyOf <http://rdvocab.info/roles/distributorManifestation> ;
	rdfs:label "Filmverleiher (Manifestation)"@de ;
	skos:definition "Eine Person, Familie oder Körperschaft, die für den Vertrieb einer verfilmten Bewegtbildmanifestation an Kinos oder andere Vertriebskanäle verantwortlich ist."@de .

<http://rdvocab.info/roles/Filmmaker> rdfs:isDefinedBy <http://rdvocab.info/roles> ;
	reg:status <http://metadataregistry.org/uri/RegStatus/1002> ;
	reg:name "Filmmaker"@en ;
	rdfs:label "Filmmaker"@en ;
	skos:definition "A person, family, or corporate body responsible for creating an independent or personal film. A filmmaker is individually responsible for the conception, and execution of all aspects of the film."@en ;
	a :Property .

<http://rdvocab.info/roles/filmmakerWork> rdfs:isDefinedBy <http://rdvocab.info/roles> ;
	reg:status <http://metadataregistry.org/uri/RegStatus/1002> ;
	reg:name "filmmakerWork"@en ;
	rdfs:label "Filmmaker (Work)"@en ;
	skos:definition "A person, family, or corporate body responsible for creating an independent or personal film. A filmmaker is individually responsible for the conception, and execution of all aspects of the film."@en ;
	a :Property ;
	rdfs:subPropertyOf <http://rdvocab.info/roles/creator> ;
	rdfs:domain <http://rdvocab.info/uri/schema/FRBRentitiesRDA/Work> ;
	rdfs:label "Filmemacher (Werk)"@de ;
	skos:definition "Eine Person, Familie oder Körperschaft, die für die Erstellung eines unabhängigen oder privaten Films verantwortlich ist. Ein Filmemacher ist individuell verantwortlich für das Konzept und die Ausführung aller Aspekte des Films."@de .

<http://rdvocab.info/roles/filmProducer> rdfs:isDefinedBy <http://rdvocab.info/roles> ;
	reg:status <http://metadataregistry.org/uri/RegStatus/1002> ;
	reg:name "filmProducer"@en ;
	rdfs:label "Film producer"@en ;
	a :Property ;
	rdfs:subPropertyOf <http://rdvocab.info/roles/producer> ;
	rdfs:label "Filmproduzent"@de .

<http://rdvocab.info/roles/filmProducerWork> rdfs:isDefinedBy <http://rdvocab.info/roles> ;
	reg:status <http://metadataregistry.org/uri/RegStatus/1002> ;
	reg:name "filmProducerWork"@en ;
	rdfs:label "Film producer (Work)"@en ;
	skos:definition "A producer responsible for most of the business aspects of a film."@en ;
	a :Property ;
	rdfs:subPropertyOf <http://rdvocab.info/roles/producerWork> ;
	rdfs:domain <http://rdvocab.info/uri/schema/FRBRentitiesRDA/Work> ;
	rdfs:label "Filmproduzent (Werk)"@de ;
	skos:definition "Eine Person, Familie oder Körperschaft, die für einen Film die Verantwortung für die meisten geschäftlichen Aspekte übernimmt. Der Produzent ist hauptsächlich verantwortlich für die Geldbeschaffung, das Produktionsmanagement, die Einstellung der Kompetenzträger, die Organisation des Vertriebs, die Absicherung des kommerziellen Erfolges usw."@de .

<http://rdvocab.info/roles/formerOwner> rdfs:isDefinedBy <http://rdvocab.info/roles> ;
	reg:status <http://metadataregistry.org/uri/RegStatus/1002> ;
	reg:name "formerOwner"@en ;
	rdfs:label "Former owner"@en ;
	a :Property ;
	rdfs:subPropertyOf <http://rdvocab.info/roles/owner> ;
	reg:hasSubproperty <http://rdvocab.info/roles/donor> , <http://rdvocab.info/roles/seller> ;
	rdfs:label "Früherer Besitzer"@de .

<http://rdvocab.info/roles/formerOwnerItem> rdfs:isDefinedBy <http://rdvocab.info/roles> ;
	reg:status <http://metadataregistry.org/uri/RegStatus/1002> ;
	reg:name "formerOwnerItem"@en ;
	rdfs:label "Former owner (Item)"@en ;
	skos:definition "A person, family, or corporate body formerly having legal possession of an item (i.e., a specific copy or instance of a resource)."@en ;
	a :Property ;
	reg:hasSubproperty <http://rdvocab.info/roles/donorItem> , <http://rdvocab.info/roles/sellerItem> ;
	rdfs:subPropertyOf <http://rdvocab.info/roles/ownerItem> ;
	rdfs:domain <http://rdvocab.info/uri/schema/FRBRentitiesRDA/Item> ;
	rdfs:label "Früherer Besitzer (Exemplar)"@de ;
	skos:definition "Eine Person, Familie oder Körperschaft, die früher rechtmäßiger Besitzer eines Exemplars war (d.h. einer bestimmten Kopie oder eines Exemplars einer Ressource)"@de .

<http://rdvocab.info/roles/honouree> rdfs:isDefinedBy <http://rdvocab.info/roles> ;
	reg:status <http://metadataregistry.org/uri/RegStatus/1002> ;
	reg:name "honouree"@en ;
	rdfs:label "Honouree"@en ;
	a :Property ;
	reg:hasSubproperty <http://rdvocab.info/roles/honoureeWork> , <http://rdvocab.info/roles/honoureeOfItem> ;
	rdfs:label "Gefeierte Person"@de .

<http://rdvocab.info/roles/honoureeOfItem> rdfs:isDefinedBy <http://rdvocab.info/roles> ;
	reg:status <http://metadataregistry.org/uri/RegStatus/1002> ;
	reg:name "honoureeOfItem"@en ;
	rdfs:label "Honouree of item"@en ;
	skos:definition "A person, family, or corporate body honoured by an item, e.g., a person to whom a copy is presented."@en ;
	a :Property ;
	rdfs:domain <http://rdvocab.info/uri/schema/FRBRentitiesRDA/Item> ;
	rdfs:subPropertyOf <http://rdvocab.info/roles/honouree> ;
	rdfs:label "Mit einem Exemplar geehrte Person."@de ;
	skos:definition "Eine Person, Familie oder Körperschaft, die durch ein Exemplar geehrt wird, z.B. die Person, der ein Exemplar gewidmet wird."@de .

<http://rdvocab.info/roles/honoureeWork> rdfs:isDefinedBy <http://rdvocab.info/roles> ;
	reg:status <http://metadataregistry.org/uri/RegStatus/1002> ;
	reg:name "honoureeWork"@en ;
	rdfs:label "Honouree (Work)"@en ;
	skos:definition "A person, family, or corporate body honoured by a work, e.g., the honouree of a festschrift."@en ;
	a :Property ;
	rdfs:domain <http://rdvocab.info/uri/schema/FRBRentitiesRDA/Work> ;
	rdfs:subPropertyOf <http://rdvocab.info/roles/honouree> ;
	rdfs:label "Gefeierte Person (Werk)"@de ;
	skos:definition "Eine Person, Familie oder Körperschaft, die durch ein Werk geehrt wird, z.B. die mit einer Festschrift gefeierte Person."@de .

<http://rdvocab.info/roles/host> rdfs:isDefinedBy <http://rdvocab.info/roles> ;
	reg:status <http://metadataregistry.org/uri/RegStatus/1002> ;
	reg:name "host"@en ;
	rdfs:label "Host"@en ;
	a :Property ;
	rdfs:subPropertyOf <http://rdvocab.info/roles/performer> ;
	rdfs:label "Gastgeber"@de .

<http://rdvocab.info/roles/hostExpression> rdfs:isDefinedBy <http://rdvocab.info/roles> ;
	reg:status <http://metadataregistry.org/uri/RegStatus/1002> ;
	reg:name "hostExpression"@en ;
	rdfs:label "Host (Expression)"@en ;
	skos:definition "A performer contributing to an expression of a work by leading a program (often broadcast) that includes other guests, performers, etc. (e.g., talk show host)."@en ;
	a :Property ;
	rdfs:domain <http://rdvocab.info/uri/schema/FRBRentitiesRDA/Expression> ;
	skos:definition "Ein Darsteller, der an einer Expression eines Werkes mitwirkt, indem er ein Programm leitet, häufig im Rundfunk, an dem auch andere Gäste, Darsteller usw. teilnehmen (z.B. der Gastgeber einer Talkshow)."@de ;
	rdfs:label "Gastgeber (Expression)"@de .

<http://rdvocab.info/roles/hostInstitution> rdfs:isDefinedBy <http://rdvocab.info/roles> ;
	reg:status <http://metadataregistry.org/uri/RegStatus/1002> ;
	reg:name "hostInstitution"@en ;
	rdfs:label "Host institution"@en ;
	a :Property ;
	reg:hasSubproperty <http://rdvocab.info/roles/hostInstitutionWork> ;
	rdfs:label "Veranstalter"@de .

<http://rdvocab.info/roles/hostInstitutionWork> rdfs:isDefinedBy <http://rdvocab.info/roles> ;
	reg:status <http://metadataregistry.org/uri/RegStatus/1002> ;
	reg:name "hostInstitutionWork"@en ;
	rdfs:label "Host institution (Work)"@en ;
	skos:definition "A corporate body hosting an event, exhibit, conference, etc., which gave rise to the work, but having little or no responsibility for the content of the work."@en ;
	a :Property ;
	rdfs:domain <http://rdvocab.info/uri/schema/FRBRentitiesRDA/Work> ;
	rdfs:subPropertyOf <http://rdvocab.info/roles/hostInstitution> ;
	rdfs:label "Veranstalter (Werk)"@de ;
	skos:definition "Eine Körperschaft, die eine Veranstaltung, eine Ausstellung, einen Kongress usw. ausrichtet, die/der ein Werk zur Folge hat, die aber für den Inhalt des Werkes wenig oder gar keine Verantwortung für trägt."@de .

<http://rdvocab.info/roles/illuminator> rdfs:isDefinedBy <http://rdvocab.info/roles> ;
	reg:status <http://metadataregistry.org/uri/RegStatus/1002> ;
	reg:name "illuminator"@en ;
	rdfs:label "Illuminator"@en ;
	a :Property ;
	reg:hasSubproperty <http://rdvocab.info/roles/illuminatorItem> ;
	rdfs:label "Illuminator"@de .

<http://rdvocab.info/roles/illuminatorItem> rdfs:isDefinedBy <http://rdvocab.info/roles> ;
	reg:status <http://metadataregistry.org/uri/RegStatus/1002> ;
	reg:name "illuminatorItem"@en ;
	rdfs:label "Illuminator (Item)"@en ;
	skos:definition "A person providing decoration to a specific item using precious metals or color, often with elaborate designs and motifs."@en ;
	a :Property ;
	rdfs:domain <http://rdvocab.info/uri/schema/FRBRentitiesRDA/Item> ;
	rdfs:subPropertyOf <http://rdvocab.info/roles/illuminator> ;
	rdfs:label "Illuminator (Exemplar)"@de ;
	skos:definition "Eine Person, die ein bestimmtes Exemplar durch Edelmetalle oder Farben (aus-)gestaltet, häufig mit kunstvollen Mustern und Motiven."@de .

<http://rdvocab.info/roles/illustrator> rdfs:isDefinedBy <http://rdvocab.info/roles> ;
	reg:status <http://metadataregistry.org/uri/RegStatus/1002> ;
	reg:name "illustrator"@en ;
	rdfs:label "Illustrator"@en ;
	a :Property ;
	rdfs:label "Illustrator"@de .

<http://rdvocab.info/roles/illustratorExpression> rdfs:isDefinedBy <http://rdvocab.info/roles> ;
	reg:status <http://metadataregistry.org/uri/RegStatus/1002> ;
	reg:name "illustratorExpression"@en ;
	rdfs:label "Illustrator (Expression)"@en ;
	skos:definition "A person, family, or corporate body contributing to an expression of a work by supplementing the primary content with drawings, diagrams, photographs, etc."@en ;
	a :Property ;
	rdfs:subPropertyOf <http://rdvocab.info/roles/contributor> ;
	rdfs:domain <http://rdvocab.info/uri/schema/FRBRentitiesRDA/Expression> ;
	rdfs:label "Illustrator (Expression)"@de ;
	skos:definition "Eine Person, Familie oder Körperschaft, die an einer Expression eines Werkes mitwirkt, indem sie den primären Inhalt mit Zeichnungen, Diagrammen, Fotografien usw. ausschmückt / ergänzt."@de .

<http://rdvocab.info/roles/inscriber> rdfs:isDefinedBy <http://rdvocab.info/roles> ;
	reg:status <http://metadataregistry.org/uri/RegStatus/1002> ;
	reg:name "inscriber"@en ;
	rdfs:label "Inscriber"@en ;
	a :Property ;
	reg:hasSubproperty <http://rdvocab.info/roles/inscriberItem> ;
	rdfs:label "Person, deren handschriftliche Anmerkungen in einem Exemplar erscheinen"@de .

<http://rdvocab.info/roles/inscriberItem> rdfs:isDefinedBy <http://rdvocab.info/roles> ;
	reg:status <http://metadataregistry.org/uri/RegStatus/1002> ;
	reg:name "inscriberItem"@en ;
	rdfs:label "Inscriber (Item)"@en ;
	skos:definition "A person whose manuscript notes appear on an item."@en ;
	a :Property ;
	rdfs:domain <http://rdvocab.info/uri/schema/FRBRentitiesRDA/Item> ;
	rdfs:subPropertyOf <http://rdvocab.info/roles/inscriber> ;
	skos:definition "Eine Person, deren handschriftliche Anmerkungen in einem Exemplar erkennbar sind."@de ;
	rdfs:label "Person, deren handschriftliche Anmerkungen in einem Exemplar erscheinen (Exemplar)"@de .

<http://rdvocab.info/roles/instrumentalist> rdfs:isDefinedBy <http://rdvocab.info/roles> ;
	reg:status <http://metadataregistry.org/uri/RegStatus/1002> ;
	reg:name "instrumentalist"@en ;
	rdfs:label "Instrumentalist"@en ;
	a :Property ;
	rdfs:subPropertyOf <http://rdvocab.info/roles/performer> ;
	rdfs:label "Instrumentalmusiker"@de .

<http://rdvocab.info/roles/instrumentalistExpression> rdfs:isDefinedBy <http://rdvocab.info/roles> ;
	reg:status <http://metadataregistry.org/uri/RegStatus/1002> ;
	reg:name "instrumentalistExpression"@en ;
	rdfs:label "Instrumentalist (Expression)"@en ;
	skos:definition "A performer contributing to an expression of a work by playing a musical instrument."@en ;
	a :Property ;
	rdfs:subPropertyOf <http://rdvocab.info/roles/performerExpression> ;
	rdfs:domain <http://rdvocab.info/uri/schema/FRBRentitiesRDA/Expression> ;
	rdfs:label "Instrumentalmusiker (Expression)"@de ;
	skos:definition "Ein Darsteller, der durch das Spielen eines Musikinstruments an einer Expression eines Werkes mitwirkt."@de .

<http://rdvocab.info/roles/interviewee> rdfs:isDefinedBy <http://rdvocab.info/roles> ;
	reg:status <http://metadataregistry.org/uri/RegStatus/1002> ;
	reg:name "interviewee"@en ;
	rdfs:label "Interviewee"@en ;
	a :Property ;
	rdfs:label "Interviewter"@de ;
	skos:definition "Eine Person, Familie oder Körperschaft, die für die Erschaffung eines Werkes verantwortlich ist, indem sie einem Interviewer antwortet, normalerweise einem Reporter, einem Meinungsforscher oder einem anderen, der Informationen zusammenträgt."@de .

<http://rdvocab.info/roles/intervieweeExpression> rdfs:isDefinedBy <http://rdvocab.info/roles> ;
	reg:status <http://metadataregistry.org/uri/RegStatus/1002> ;
	reg:name "intervieweeExpression"@en ;
	rdfs:label "Interviewee (Expression)"@en ;
	skos:definition "A person, family, or corporate body contributing to an expression of a work by responding to an interviewer, usually a reporter, pollster, or some other information gathering agent."@en ;
	a :Property ;
	rdfs:subPropertyOf <http://rdvocab.info/roles/contributor> ;
	rdfs:domain <http://rdvocab.info/uri/schema/FRBRentitiesRDA/Expression> ;
	rdfs:label "Interviewter (Expression)"@de ;
	skos:definition "Eine Person, Familie oder Körperschaft, die für die Erschaffung eines Werkes verantwortlich ist, indem sie einem Interviewer antwortet, normalerweise einem Reporter, einem Meinungsforscher oder einem anderen, der Informationen zusammenträgt."@de .

<http://rdvocab.info/roles/intervieweeWork> rdfs:isDefinedBy <http://rdvocab.info/roles> ;
	reg:status <http://metadataregistry.org/uri/RegStatus/1002> ;
	reg:name "intervieweeWork"@en ;
	rdfs:label "Interviewee (Work)"@en ;
	skos:definition "A person, family, or corporate body responsible for creating a work by responding to an interviewer, usually a reporter, pollster, or some other information gathering agent."@en ;
	a :Property ;
	rdfs:subPropertyOf <http://rdvocab.info/roles/creator> ;
	rdfs:domain <http://rdvocab.info/uri/schema/FRBRentitiesRDA/Work> ;
	skos:definition "Eine Person, Familie oder Körperschaft, die für die Erschaffung eines Werkes verantwortlich ist, indem sie einem Interviewer antwortet, normalerweise einem Reporter, einem Meinungsforscher oder einem anderen, der Informationen zusammenträgt."@de ;
	rdfs:label "Interviewer (Werk)"@de .

<http://rdvocab.info/roles/interviewer> rdfs:isDefinedBy <http://rdvocab.info/roles> ;
	reg:status <http://metadataregistry.org/uri/RegStatus/1002> ;
	reg:name "interviewer"@en ;
	rdfs:label "Interviewer"@en ;
	a :Property ;
	rdfs:label "Interviewer"@de ;
	skos:definition "Eine Person, Familie oder Körperschaft, die für die Erschaffung eines Werkes verantwortlich ist, indem sie als Interviewer, Reporter, Meinungsforscher oder anderer Informationssammler tätig ist."@de .

<http://rdvocab.info/roles/interviewerExpression> rdfs:isDefinedBy <http://rdvocab.info/roles> ;
	reg:status <http://metadataregistry.org/uri/RegStatus/1002> ;
	reg:name "interviewerExpression"@en ;
	rdfs:label "Interviewer (Expression)"@en ;
	skos:definition "A person, family, or corporate body contributing to an expression of a work by acting as an interviewer, reporter, pollster, or some other information gathering agent."@en ;
	a :Property ;
	rdfs:subPropertyOf <http://rdvocab.info/roles/contributor> ;
	rdfs:domain <http://rdvocab.info/uri/schema/FRBRentitiesRDA/Expression> ;
	rdfs:label "Interviewer (Expression)"@de ;
	skos:definition "Eine Person, Familie oder Körperschaft, die für die Erschaffung eines Werkes verantwortlich ist, indem sie als Interviewer, Reporter, Meinungsforscher oder anderer Informationssammler tätig ist."@de .

<http://rdvocab.info/roles/interviewerWork> rdfs:isDefinedBy <http://rdvocab.info/roles> ;
	reg:status <http://metadataregistry.org/uri/RegStatus/1002> ;
	reg:name "interviewerWork"@en ;
	rdfs:label "Interviewer (Work)"@en ;
	skos:definition "A person, family, or corporate body responsible for creating a work by acting as an interviewer, reporter, pollster, or some other information gathering agent."@en ;
	a :Property ;
	rdfs:subPropertyOf <http://rdvocab.info/roles/creator> ;
	rdfs:domain <http://rdvocab.info/uri/schema/FRBRentitiesRDA/Work> ;
	skos:definition "Eine Person, Familie oder Körperschaft, die für die Erschaffung eines Werkes verantwortlich ist, indem sie einem Interviewer antwortet, normalerweise einem Reporter, einem Meinungsforscher oder einem anderen, der Informationen zusammenträgt."@de ;
	rdfs:label "Interviewter (Werk)"@de .

<http://rdvocab.info/roles/inventor> rdfs:isDefinedBy <http://rdvocab.info/roles> ;
	reg:status <http://metadataregistry.org/uri/RegStatus/1002> ;
	reg:name "inventor"@en ;
	rdfs:label "Inventor"@en ;
	a :Property ;
	rdfs:label "Erfinder"@de .

<http://rdvocab.info/roles/inventorWork> rdfs:isDefinedBy <http://rdvocab.info/roles> ;
	reg:status <http://metadataregistry.org/uri/RegStatus/1002> ;
	reg:name "inventorWork"@en ;
	rdfs:label "Inventor (Work)"@en ;
	skos:definition "A person, family, or corporate body responsible for creating a new device or process."@en ;
	a :Property ;
	rdfs:subPropertyOf <http://rdvocab.info/roles/creator> ;
	rdfs:domain <http://rdvocab.info/uri/schema/FRBRentitiesRDA/Work> ;
	rdfs:label "Erfinder (Werk)"@de ;
	skos:definition "Eine Person, Familie oder Körperschaft, die für die Erschaffung eines neuen Gerätes oder Prozesses verantwortlich ist."@de .

<http://rdvocab.info/roles/issuingBody> rdfs:isDefinedBy <http://rdvocab.info/roles> ;
	reg:status <http://metadataregistry.org/uri/RegStatus/1002> ;
	reg:name "issuingBody"@en ;
	rdfs:label "Issuing body"@en ;
	a :Property ;
	reg:hasSubproperty <http://rdvocab.info/roles/issuingBodyWork> ;
	rdfs:label "Veröffentlichendes Organ"@de .

<http://rdvocab.info/roles/issuingBodyWork> rdfs:isDefinedBy <http://rdvocab.info/roles> ;
	reg:status <http://metadataregistry.org/uri/RegStatus/1002> ;
	reg:name "issuingBodyWork"@en ;
	rdfs:label "Issuing body (Work)"@en ;
	skos:definition "A person, family or corporate body issuing the work, such as an official organ of the body."@en ;
	a :Property ;
	rdfs:domain <http://rdvocab.info/uri/schema/FRBRentitiesRDA/Work> ;
	rdfs:subPropertyOf <http://rdvocab.info/roles/issuingBody> ;
	rdfs:label "Veröffentlichendes Organ (Werk)"@de ;
	skos:definition "Eine Person, Familie oder Körperschaft, die ein Werk herausgibt, wie z.B. ein offizielles Organ der Körperschaft."@de .

<http://rdvocab.info/roles/judge> rdfs:isDefinedBy <http://rdvocab.info/roles> ;
	reg:status <http://metadataregistry.org/uri/RegStatus/1002> ;
	reg:name "judge"@en ;
	rdfs:label "Judge"@en ;
	a :Property ;
	reg:hasSubproperty <http://rdvocab.info/roles/judgeWork> ;
	rdfs:label "Richter"@de .

<http://rdvocab.info/roles/judgeWork> rdfs:isDefinedBy <http://rdvocab.info/roles> ;
	reg:status <http://metadataregistry.org/uri/RegStatus/1002> ;
	reg:name "judgeWork"@en ;
	rdfs:label "Judge (Work)"@en ;
	skos:definition "A person who hears and decides on legal matters in court."@en ;
	a :Property ;
	rdfs:domain <http://rdvocab.info/uri/schema/FRBRentitiesRDA/Work> ;
	rdfs:subPropertyOf <http://rdvocab.info/roles/judge> ;
	rdfs:label "Richter (Werk)"@de ;
	skos:definition "Eine Person, die bei Gericht gesetzliche Angelegenheiten anhört und darüber entscheidet."@de .

<http://rdvocab.info/roles/jurisdictionGoverned> rdfs:isDefinedBy <http://rdvocab.info/roles> ;
	reg:status <http://metadataregistry.org/uri/RegStatus/1002> ;
	reg:name "jurisdictionGoverned"@en ;
	rdfs:label "Jurisdiction governed"@en ;
	a :Property ;
	reg:hasSubproperty <http://rdvocab.info/roles/jurisdictionGovernedWork> ;
	rdfs:label "Normunterworfener Rechtsträger"@de .

<http://rdvocab.info/roles/jurisdictionGovernedWork> rdfs:isDefinedBy <http://rdvocab.info/roles> ;
	reg:status <http://metadataregistry.org/uri/RegStatus/1002> ;
	reg:name "jurisdictionGovernedWork"@en ;
	rdfs:label "Jurisdiction governed (Work)"@en ;
	skos:definition "A jurisdiction governed by a law, regulation, etc., that was enacted by another jurisdiction."@en ;
	a :Property ;
	rdfs:domain <http://rdvocab.info/uri/schema/FRBRentitiesRDA/Work> ;
	rdfs:subPropertyOf <http://rdvocab.info/roles/jurisdictionGoverned> ;
	rdfs:label "Normunterworfener Rechtsträger (Werk)"@de ;
	skos:definition "Ein Rechtsträger, der Gesetzen, Verordnungen o. ä. unterworfen ist, die von einem anderen Rechtsträger erlassen wurden."@de .

<http://rdvocab.info/roles/landscapeArchitect> rdfs:isDefinedBy <http://rdvocab.info/roles> ;
	reg:status <http://metadataregistry.org/uri/RegStatus/1002> ;
	reg:name "landscapeArchitect"@en ;
	rdfs:label "Landscape architect"@en ;
	a :Property ;
	rdfs:subPropertyOf <http://rdvocab.info/roles/architect> ;
	rdfs:label "Landschaftsarchitekt"@de .

<http://rdvocab.info/roles/landscapeArchitectWork> rdfs:isDefinedBy <http://rdvocab.info/roles> ;
	reg:status <http://metadataregistry.org/uri/RegStatus/1002> ;
	reg:name "landscapeArchitectWork"@en ;
	rdfs:label "Landscape architect (Work)"@en ;
	skos:definition "An architect responsible for creating landscape works."@en ;
	a :Property ;
	rdfs:domain <http://rdvocab.info/uri/schema/FRBRentitiesRDA/Work> ;
	rdfs:label "Landschaftsarchitekt (Werk)"@de ;
	skos:definition "Ein Architekt, der für die Erschaffung landschaftlicher Werke verantwortlich ist."@de .

<http://rdvocab.info/roles/librettist> rdfs:isDefinedBy <http://rdvocab.info/roles> ;
	reg:status <http://metadataregistry.org/uri/RegStatus/1002> ;
	reg:name "librettist"@en ;
	rdfs:label "Librettist"@en ;
	a :Property ;
	rdfs:subPropertyOf <http://rdvocab.info/roles/author> ;
	rdfs:label "Librettist"@de .

<http://rdvocab.info/roles/librettistWork> rdfs:isDefinedBy <http://rdvocab.info/roles> ;
	reg:status <http://metadataregistry.org/uri/RegStatus/1002> ;
	reg:name "librettistWork"@en ;
	rdfs:label "Librettist (Work)"@en ;
	skos:definition "An author of a libretto of an opera or other stage work, or an oratorio."@en ;
	a :Property ;
	rdfs:subPropertyOf <http://rdvocab.info/roles/authorWork> ;
	rdfs:domain <http://rdvocab.info/uri/schema/FRBRentitiesRDA/Work> ;
	rdfs:label "Librettist (Werk)"@de ;
	skos:definition "Ein Verfasser eines Librettos einer Oper oder anderer Bühnenwerke oder eines Oratoriums."@de .

<http://rdvocab.info/roles/lithographer> rdfs:isDefinedBy <http://rdvocab.info/roles> ;
	reg:status <http://metadataregistry.org/uri/RegStatus/1002> ;
	reg:name "lithographer"@en ;
	rdfs:label "Lithographer"@en ;
	a :Property ;
	rdfs:subPropertyOf <http://rdvocab.info/roles/manufacturer> ;
	rdfs:label "Lithograf"@de .

<http://rdvocab.info/roles/lithographerManifestation> rdfs:isDefinedBy <http://rdvocab.info/roles> ;
	reg:status <http://metadataregistry.org/uri/RegStatus/1002> ;
	reg:name "lithographerManifestation"@en ;
	rdfs:label "Lithographer (Manifestation)"@en ;
	skos:definition "A person, family, or corporate body involved in producing a manifestation by preparing a stone or plate for lithographic printing, including a graphic artist creating a design directly on the surface from which printing will be done."@en ;
	a :Property ;
	rdfs:domain <http://rdvocab.info/uri/schema/FRBRentitiesRDA/Manifestation> ;
	rdfs:subPropertyOf <http://rdvocab.info/roles/manufacturerManifestation> ;
	rdfs:label "Lithograf (Manifestation)"@de ;
	skos:definition "Eine Person, Familie oder Körperschaft, die in die Erstellung einer Manifestation eingebunden ist, indem sie einen Stein oder eine Platte für lithografischen Druck vorbereitet, einschließlich eines Grafikers, der ein Muster direkt auf der Oberfläche erstellt, von der aus gedruckt werden wird."@de .

<http://rdvocab.info/roles/lyricist> rdfs:isDefinedBy <http://rdvocab.info/roles> ;
	reg:status <http://metadataregistry.org/uri/RegStatus/1002> ;
	reg:name "lyricist"@en ;
	rdfs:label "Lyricist"@en ;
	a :Property ;
	rdfs:subPropertyOf <http://rdvocab.info/roles/author> ;
	rdfs:label "Textdichter"@de .

<http://rdvocab.info/roles/lyricistWork> rdfs:isDefinedBy <http://rdvocab.info/roles> ;
	reg:status <http://metadataregistry.org/uri/RegStatus/1002> ;
	reg:name "lyricistWork"@en ;
	rdfs:label "Lyricist (Work)"@en ;
	skos:definition "An author of the words of a non-dramatic musical work, except for oratorios."@en ;
	a :Property ;
	rdfs:domain <http://rdvocab.info/uri/schema/FRBRentitiesRDA/Work> ;
	rdfs:label "Textdichter (Werk)"@de ;
	skos:definition "Ein Verfasser des Textes eines nicht-dramatischen musikalischen Werkes, ausgenommen für Oratorien."@de ;
	rdfs:subPropertyOf <http://rdvocab.info/roles/authorWork> .

<http://rdvocab.info/roles/manufacturer> rdfs:isDefinedBy <http://rdvocab.info/roles> ;
	reg:status <http://metadataregistry.org/uri/RegStatus/1002> ;
	reg:name "manufacturer"@en ;
	rdfs:label "Manufacturer"@en ;
	a :Property ;
	reg:hasSubproperty <http://rdvocab.info/roles/manufacturerManifestation> , <http://rdvocab.info/roles/bookDesigner> , <http://rdvocab.info/roles/brailleEmbosser> , <http://rdvocab.info/roles/caster> , <http://rdvocab.info/roles/collotyper> , <http://rdvocab.info/roles/engraver> , <http://rdvocab.info/roles/etcher> , <http://rdvocab.info/roles/lithographer> , <http://rdvocab.info/roles/platemaker> , <http://rdvocab.info/roles/printer> , <http://rdvocab.info/roles/printmaker> ;
	rdfs:label "Hersteller"@de ;
	skos:definition "Eine Person, Familie oder Körperschaft, die für den Druck, die Vervielfältigung, Auswahl etc. einer Ressource in einer veröffentlichten Form verantwortlich ist."@de .

<http://rdvocab.info/roles/manufacturerManifestation> rdfs:isDefinedBy <http://rdvocab.info/roles> ;
	reg:status <http://metadataregistry.org/uri/RegStatus/1002> ;
	reg:name "manufacturerManifestation"@en ;
	rdfs:label "Manufacturer (Manifestation)"@en ;
	skos:definition "A person, family, or corporate body responsible for printing, duplicating, casting, etc., a resource in a published form."@en ;
	a :Property ;
	rdfs:subPropertyOf <http://rdvocab.info/roles/manufacturer> ;
	rdfs:domain <http://rdvocab.info/uri/schema/FRBRentitiesRDA/Manifestation> ;
	reg:hasSubproperty <http://rdvocab.info/roles/bookDesignerManifestation> , <http://rdvocab.info/roles/brailleEmbosserManifestation> , <http://rdvocab.info/roles/casterManifestation> , <http://rdvocab.info/roles/collotyperManifestation> , <http://rdvocab.info/roles/engraverManifestation> , <http://rdvocab.info/roles/etcherManifestation> , <http://rdvocab.info/roles/lithographerManifestation> , <http://rdvocab.info/roles/platemakerManifestation> , <http://rdvocab.info/roles/printerManifestation> , <http://rdvocab.info/roles/printmakerManifestation> ;
	skos:definition "Eine Person, Familie oder Körperschaft, die für den Druck, die Vervielfältigung, Auswahl etc. einer Ressource in einer veröffentlichten Form verantwortlich ist."@de ;
	rdfs:label "Hersteller (Manifestation)"@de .

<http://rdvocab.info/roles/moderator> rdfs:isDefinedBy <http://rdvocab.info/roles> ;
	reg:status <http://metadataregistry.org/uri/RegStatus/1002> ;
	reg:name "moderator"@en ;
	rdfs:label "Moderator"@en ;
	a :Property ;
	rdfs:subPropertyOf <http://rdvocab.info/roles/performer> ;
	rdfs:label "Moderator"@de .

<http://rdvocab.info/roles/moderatorExpression> rdfs:isDefinedBy <http://rdvocab.info/roles> ;
	reg:status <http://metadataregistry.org/uri/RegStatus/1002> ;
	reg:name "moderatorExpression"@en ;
	rdfs:label "Moderator (Expression)"@en ;
	skos:definition "A performer contributing to an expression of a work by leading a program (often broadcast) where topics are discussed, usually with participation of experts in fields related to the discussion."@en ;
	a :Property ;
	rdfs:domain <http://rdvocab.info/uri/schema/FRBRentitiesRDA/Expression> ;
	skos:definition "Ein Darsteller, der an einer Expression eines Werkes mitwirkt, indem er ein Programm leitet (oft eine Rundfunk-Sendung), in dem Themen diskutiert werden, normalerweise mit Teilnahme von Experten auf den diskutierten Gebieten."@de ;
	rdfs:label "Moderator (Expression)"@de .

<http://rdvocab.info/roles/musicalDirector> rdfs:isDefinedBy <http://rdvocab.info/roles> ;
	reg:status <http://metadataregistry.org/uri/RegStatus/1002> ;
	reg:name "musicalDirector"@en ;
	rdfs:label "Musical director"@en ;
	a :Property ;
	rdfs:label "Musikalischer Leiter"@de .

<http://rdvocab.info/roles/musicalDirectorExpression> rdfs:isDefinedBy <http://rdvocab.info/roles> ;
	reg:status <http://metadataregistry.org/uri/RegStatus/1002> ;
	reg:name "musicalDirectorExpression"@en ;
	rdfs:label "Musical director (Expression)"@en ;
	skos:definition "A person, family, or corporate body responsible for coordinating the work of the composer, the sound editor, and sound mixers for a moving image production or for a musical or dramatic presentation or entertainment."@en ;
	a :Property ;
	rdfs:subPropertyOf <http://rdvocab.info/roles/contributor> ;
	rdfs:domain <http://rdvocab.info/uri/schema/FRBRentitiesRDA/Expression> ;
	rdfs:label "Musikalischer Leiter (Expression)"@de ;
	skos:definition "Eine Person, Familie oder Körperschaft, die für die Koordinierung der Arbeit des Komponisten, des Tonbearbeiters und Tonmeisters für eine Bewegtbildproduktion oder eine musikalische oder dramatische Darbietung oder Aufführung verantwortlich ist."@de .

<http://rdvocab.info/roles/narrator> rdfs:isDefinedBy <http://rdvocab.info/roles> ;
	reg:status <http://metadataregistry.org/uri/RegStatus/1002> ;
	reg:name "narrator"@en ;
	rdfs:label "Narrator"@en ;
	a :Property ;
	rdfs:subPropertyOf <http://rdvocab.info/roles/performer> ;
	rdfs:label "Erzähler"@de .

<http://rdvocab.info/roles/narratorExpression> rdfs:isDefinedBy <http://rdvocab.info/roles> ;
	reg:status <http://metadataregistry.org/uri/RegStatus/1002> ;
	reg:name "narratorExpression"@en ;
	rdfs:label "Narrator (Expression)"@en ;
	skos:definition "A performer contributing to an expression of a work by reading or speaking in order to give an account of an act, occurrence, course of events, etc."@en ;
	a :Property ;
	rdfs:subPropertyOf <http://rdvocab.info/roles/performerExpression> ;
	rdfs:domain <http://rdvocab.info/uri/schema/FRBRentitiesRDA/Expression> ;
	rdfs:label "Erzähler (Expression)"@de ;
	skos:definition "Ein Darsteller, der eine Expression eines Werkes liest oder spricht, um einen Akt, ein Geschehnis, einen Ereignisablauf usw. darzustellen."@de .

<http://rdvocab.info/roles/onScreenPresenter> rdfs:isDefinedBy <http://rdvocab.info/roles> ;
	reg:status <http://metadataregistry.org/uri/RegStatus/1002> ;
	reg:name "onScreenPresenter"@en ;
	rdfs:label "On-screen presenter"@en ;
	a :Property ;
	rdfs:subPropertyOf <http://rdvocab.info/roles/performer> ;
	rdfs:label "On-screen Presenter"@de .

<http://rdvocab.info/roles/onScreenPresenterExpression> rdfs:isDefinedBy <http://rdvocab.info/roles> ;
	reg:status <http://metadataregistry.org/uri/RegStatus/1002> ;
	reg:name "onScreenPresenterExpression"@en ;
	rdfs:label "On-screen presenter (Expression)"@en ;
	skos:definition "A performer contributing to an expression of a work by appearing on screen in nonfiction moving image materials or introductions to fiction moving image materials to provide contextual or background information."@en ;
	a :Property ;
	rdfs:comment "Use when a more specific term (e.g., Narrator or Host) is either not applicable or not desired."@en ;
	rdfs:domain <http://rdvocab.info/uri/schema/FRBRentitiesRDA/Expression> ;
	rdfs:label "On-screen Presenter (Expression)"@de ;
	skos:definition "Ein Darsteller, der an einer Expression eines Werkes mitwirkt, indem er über den Bildschirm Kontext- und Hintergrundinformationen zu nicht-fiktiven Bewegtbildmaterialien oder zu Einleitungen zu fiktivenBewegtbildmaterialien beisteuert. Die Funktionsbezeichnung wird verwendet, wenn ein spezifischerer Begriff (z. B. Erzähler oder Gastgeber) nicht anwendbar ist."@de .

<http://rdvocab.info/roles/owner> rdfs:isDefinedBy <http://rdvocab.info/roles> ;
	reg:status <http://metadataregistry.org/uri/RegStatus/1002> ;
	reg:name "owner"@en ;
	rdfs:label "Owner"@en ;
	a :Property ;
	reg:hasSubproperty <http://rdvocab.info/roles/ownerItem> , <http://rdvocab.info/roles/currentOwner> , <http://rdvocab.info/roles/formerOwner> ;
	rdfs:label "Besitzer"@de ;
	skos:definition "Eine Person, Familie oder Körperschaft, die im rechtmäßigen Besitz eines Exemplars ist (z.B. einer bestimmten Kopie oder einer bestimmten Instanz einer Ressource)."@de .

<http://rdvocab.info/roles/ownerItem> rdfs:isDefinedBy <http://rdvocab.info/roles> ;
	reg:status <http://metadataregistry.org/uri/RegStatus/1002> ;
	reg:name "ownerItem"@en ;
	rdfs:label "Owner (Item)"@en ;
	skos:definition "A person, family, or corporate body having legal possession of an item (i.e., a specific copy or instance of a resource)."@en ;
	a :Property ;
	rdfs:domain <http://rdvocab.info/uri/schema/FRBRentitiesRDA/Item> ;
	reg:hasSubproperty <http://rdvocab.info/roles/currentOwnerItem> , <http://rdvocab.info/roles/formerOwnerItem> ;
	rdfs:subPropertyOf <http://rdvocab.info/roles/owner> ;
	rdfs:label "Besitzer (Exemplar)"@de ;
	skos:definition "Eine Person, Familie oder Körperschaft, die im rechtmäßigen Besitz eines Exemplars ist (z.B. einer bestimmten Kopie oder einer bestimmten Instanz einer Ressource)."@de .

<http://rdvocab.info/roles/panelist> rdfs:isDefinedBy <http://rdvocab.info/roles> ;
	reg:status <http://metadataregistry.org/uri/RegStatus/1002> ;
	reg:name "panelist"@en ;
	rdfs:label "Panelist"@en ;
	a :Property ;
	rdfs:subPropertyOf <http://rdvocab.info/roles/performer> ;
	rdfs:label "Diskussionsteilnehmer"@de .

<http://rdvocab.info/roles/panelistExpression> rdfs:isDefinedBy <http://rdvocab.info/roles> ;
	reg:status <http://metadataregistry.org/uri/RegStatus/1002> ;
	reg:name "panelistExpression"@en ;
	rdfs:label "Panelist (Expression)"@en ;
	skos:definition "A performer contributing to an expression of a work by participating in a program (often broadcast) where topics are discussed, usually with participation of experts in fields related to the discussion."@en ;
	a :Property ;
	rdfs:domain <http://rdvocab.info/uri/schema/FRBRentitiesRDA/Expression> ;
	rdfs:label "Diskussionsteilnehmer (Expression)"@de ;
	skos:definition "Ein Darsteller, der an einem Programm (oft einer Rundfunk-Sendung) teilnimmt, in dem Themen diskutiert werden, normalerweise mit Experten auf den diskutierten Gebieten."@de .

<http://rdvocab.info/roles/performer> rdfs:isDefinedBy <http://rdvocab.info/roles> ;
	reg:status <http://metadataregistry.org/uri/RegStatus/1002> ;
	reg:name "performer"@en ;
	rdfs:label "Performer"@en ;
	a :Property ;
	reg:hasSubproperty <http://rdvocab.info/roles/actor> , <http://rdvocab.info/roles/commentator> , <http://rdvocab.info/roles/conductor> , <http://rdvocab.info/roles/dancer> , <http://rdvocab.info/roles/host> , <http://rdvocab.info/roles/instrumentalist> , <http://rdvocab.info/roles/moderator> , <http://rdvocab.info/roles/narrator> , <http://rdvocab.info/roles/onScreenPresenter> , <http://rdvocab.info/roles/panelist> , <http://rdvocab.info/roles/puppeteer> , <http://rdvocab.info/roles/singer> , <http://rdvocab.info/roles/speaker> , <http://rdvocab.info/roles/storyteller> , <http://rdvocab.info/roles/teacher> ;
	rdfs:label "Darsteller"@de .

<http://rdvocab.info/roles/performerExpression> rdfs:isDefinedBy <http://rdvocab.info/roles> ;
	reg:status <http://metadataregistry.org/uri/RegStatus/1002> ;
	reg:name "performerExpression"@en ;
	rdfs:label "Performer (Expression)"@en ;
	skos:definition "A person, family, or corporate body contributing to an expression of a work by performing music, acting, dancing, speaking, etc., often in a musical or dramatic presentation, etc."@en ;
	a :Property ;
	reg:hasSubproperty <http://rdvocab.info/roles/actorExpression> , <http://rdvocab.info/roles/dancerExpression> , <http://rdvocab.info/roles/instrumentalistExpression> , <http://rdvocab.info/roles/narratorExpression> , <http://rdvocab.info/roles/singerExpression> , <http://rdvocab.info/roles/storytellerExpression> ;
	rdfs:subPropertyOf <http://rdvocab.info/roles/contributor> ;
	rdfs:domain <http://rdvocab.info/uri/schema/FRBRentitiesRDA/Expression> ;
	reg:hasSubproperty <http://rdvocab.info/roles/speakerExpression> ;
	rdfs:label "Darsteller (Expression)"@de ;
	skos:definition "Eine Person, Familie oder Körperschaft, die für die Expression eines Werkes Musik aufführen, auftreten, tanzen, sprechen usw., oft in einer musikalischen oder dramatischen Darbietung usw."@de .

<http://rdvocab.info/roles/photographer> rdfs:isDefinedBy <http://rdvocab.info/roles> ;
	reg:status <http://metadataregistry.org/uri/RegStatus/1002> ;
	reg:name "photographer"@en ;
	rdfs:label "Photographer"@en ;
	a :Property ;
	rdfs:label "Fotograf"@de ;
	skos:definition "Eine Person, Familie oder Körperschaft, die für die Erstellung eines fotografischen Werks verantwortlich ist."@de .

<http://rdvocab.info/roles/photographerWork> rdfs:isDefinedBy <http://rdvocab.info/roles> ;
	reg:status <http://metadataregistry.org/uri/RegStatus/1002> ;
	reg:name "photographerWork"@en ;
	rdfs:label "Photographer (Work)"@en ;
	skos:definition "A person, family, or corporate body responsible for creating a photographic work."@en ;
	a :Property ;
	rdfs:subPropertyOf <http://rdvocab.info/roles/creator> ;
	rdfs:domain <http://rdvocab.info/uri/schema/FRBRentitiesRDA/Work> ;
	rdfs:label "Fotograf (Werk)"@de ;
	skos:definition "Eine Person, Familie oder Körperschaft, die für die Erstellung eines fotografischen Werks verantwortlich ist."@de .

<http://rdvocab.info/roles/plaintiff> rdfs:isDefinedBy <http://rdvocab.info/roles> ;
	reg:status <http://metadataregistry.org/uri/RegStatus/1002> ;
	reg:name "plaintiff"@en ;
	rdfs:label "Plaintiff"@en ;
	a :Property ;
	reg:hasSubproperty <http://rdvocab.info/roles/plaintiffWork> ;
	rdfs:label "Zivilkläger"@de .

<http://rdvocab.info/roles/plaintiffWork> rdfs:isDefinedBy <http://rdvocab.info/roles> ;
	reg:status <http://metadataregistry.org/uri/RegStatus/1002> ;
	reg:name "plaintiffWork"@en ;
	rdfs:label "Plaintiff (Work)"@en ;
	skos:definition "A person or corporate body who brings a suit in a civil proceeding."@en ;
	a :Property ;
	rdfs:domain <http://rdvocab.info/uri/schema/FRBRentitiesRDA/Work> ;
	rdfs:subPropertyOf <http://rdvocab.info/roles/plaintiff> ;
	rdfs:label "Zivilkläger"@de ;
	skos:definition "Eine Person oder Körperschaft, die eine Klage in ein Zivilverfahren einbringt."@de .

<http://rdvocab.info/roles/platemaker> rdfs:isDefinedBy <http://rdvocab.info/roles> ;
	reg:status <http://metadataregistry.org/uri/RegStatus/1002> ;
	reg:name "platemaker"@en ;
	rdfs:label "Platemaker"@en ;
	a :Property ;
	rdfs:subPropertyOf <http://rdvocab.info/roles/manufacturer> ;
	rdfs:label "Druckformhersteller"@de .

<http://rdvocab.info/roles/platemakerManifestation> rdfs:isDefinedBy <http://rdvocab.info/roles> ;
	reg:status <http://metadataregistry.org/uri/RegStatus/1002> ;
	reg:name "platemakerManifestation"@en ;
	rdfs:label "Platemaker (Manifestation)"@en ;
	skos:definition "A person, family, or corporate body involved in producing a manifestation by preparing plates used in the production of printed images and/or text."@en ;
	a :Property ;
	rdfs:domain <http://rdvocab.info/uri/schema/FRBRentitiesRDA/Manifestation> ;
	rdfs:subPropertyOf <http://rdvocab.info/roles/manufacturerManifestation> ;
	rdfs:label "Druckformhersteller (Manifestation)"@de ;
	skos:definition "Eine Person, Familie oder Körperschaft, die an der Produktion einer Manifestation beteiligt ist, indem sie Druckformen für die Produktion von gedruckten Bildern und/oder Text anfertigt."@de .

<http://rdvocab.info/roles/praeses> rdfs:isDefinedBy <http://rdvocab.info/roles> ;
	reg:status <http://metadataregistry.org/uri/RegStatus/1002> ;
	reg:name "praeses"@en ;
	rdfs:label "Praeses"@en ;
	a :Property ;
	rdfs:label "Disputationsleiter"@de .

<http://rdvocab.info/roles/praesesWork> rdfs:isDefinedBy <http://rdvocab.info/roles> ;
	reg:status <http://metadataregistry.org/uri/RegStatus/1002> ;
	reg:name "praesesWork"@en ;
	rdfs:label "Praeses (Work)"@en ;
	skos:definition "A person who is the faculty moderator of an academic disputation, normally proposing a thesis and participating in the ensuing disputation."@en ;
	a :Property ;
	rdfs:subPropertyOf <http://rdvocab.info/roles/creator> ;
	rdfs:domain <http://rdvocab.info/uri/schema/FRBRentitiesRDA/Work> ;
	rdfs:label "Disputationsleiter (Werk)"@de ;
	skos:definition "Angehöriger des Lehrpersonals, der eine akademische Disputation moderiert, normalerweise indem er eine These aufstellt und an der folgenden Disputation teilnimmt, aber nur indirekte Verbindung mit dem Inhalt der These hat."@de .

<http://rdvocab.info/roles/presenter> rdfs:isDefinedBy <http://rdvocab.info/roles> ;
	reg:status <http://metadataregistry.org/uri/RegStatus/1002> ;
	reg:name "presenter"@en ;
	rdfs:label "Presenter"@en ;
	a :Property ;
	rdfs:label "Presenter"@de .

<http://rdvocab.info/roles/presenterExpression> rdfs:isDefinedBy <http://rdvocab.info/roles> ;
	reg:status <http://metadataregistry.org/uri/RegStatus/1002> ;
	reg:name "presenterExpression"@en ;
	rdfs:label "Presenter (Expression)"@en ;
	skos:definition "A person, family, or corporate body mentioned in an “X presents” credit for moving image materials and who is probably associated with production, finance, or distribution in some way. In the early years of film production, this was often used as a vanity credit."@en ;
	a :Property ;
	rdfs:subPropertyOf <http://rdvocab.info/roles/contributor> ;
	rdfs:domain <http://rdvocab.info/uri/schema/FRBRentitiesRDA/Expression> ;
	rdfs:label "Presenter (Expression)"@de ;
	skos:definition "Eine Person, Familie oder Körperschaft, die in einem \"X präsentiert\"-Vorspann für Bewegtbildmaterialien erwähnt wird und die wahrscheinlich in gewisser Weise mit Produktion, Finanzierung oder Vertrieb in Zusammenhang steht. In den frühen Jahren der Filmproduktion wurde dies häufig  als \"vanity credit\" verwendet."@de .

<http://rdvocab.info/roles/printer> rdfs:isDefinedBy <http://rdvocab.info/roles> ;
	reg:status <http://metadataregistry.org/uri/RegStatus/1002> ;
	reg:name "printer"@en ;
	rdfs:label "Printer"@en ;
	a :Property ;
	rdfs:subPropertyOf <http://rdvocab.info/roles/manufacturer> ;
	rdfs:label "Drucker"@de .

<http://rdvocab.info/roles/printerManifestation> rdfs:isDefinedBy <http://rdvocab.info/roles> ;
	reg:status <http://metadataregistry.org/uri/RegStatus/1002> ;
	reg:name "printerManifestation"@en ;
	rdfs:label "Printer (Manifestation)"@en ;
	skos:definition "A person, family, or corporate body involved in producing a manifestation of printed text, notated music, etc., from type or plates, such as a book, newspaper, magazine, broadside, score, etc."@en ;
	a :Property ;
	rdfs:domain <http://rdvocab.info/uri/schema/FRBRentitiesRDA/Manifestation> ;
	rdfs:subPropertyOf <http://rdvocab.info/roles/manufacturerManifestation> ;
	rdfs:label "Drucker (Manifestation)"@de ;
	skos:definition "Eine Person, Familie oder Körperschaft, die an der Produktion einer Manifestation von gedrucktem Text, notierter Musik usw. durch Drucktypen oder Druckformen, wie z.B. ein Buch, eine Zeitung, ein Magazin, ein Einblattdruck, eine Partitur o.ä. beteiligt ist."@de .

<http://rdvocab.info/roles/printmaker> rdfs:isDefinedBy <http://rdvocab.info/roles> ;
	reg:status <http://metadataregistry.org/uri/RegStatus/1002> ;
	reg:name "printmaker"@en ;
	rdfs:label "Printmaker"@en ;
	a :Property ;
	rdfs:subPropertyOf <http://rdvocab.info/roles/manufacturer> ;
	rdfs:label "Druckgrafiker"@de .

<http://rdvocab.info/roles/printmakerManifestation> rdfs:isDefinedBy <http://rdvocab.info/roles> ;
	reg:status <http://metadataregistry.org/uri/RegStatus/1002> ;
	reg:name "printmakerManifestation"@en ;
	rdfs:label "Printmaker (Manifestation)"@en ;
	skos:definition "A person, family, or corporate body involved in manufacturing a manifestation by making a relief, intaglio, or planographic printing surface."@en ;
	a :Property ;
	rdfs:domain <http://rdvocab.info/uri/schema/FRBRentitiesRDA/Manifestation> ;
	rdfs:subPropertyOf <http://rdvocab.info/roles/manufacturerManifestation> ;
	rdfs:label "Druckgrafiker (Manifestation)"@de ;
	skos:definition "Eine Person, Familie oder Körperschaft, die an der Produktion einer Manifestation durch die Erstellung einer Hochdruck-, Tiefdruck- oder Flachdruckoberfläche beteiligt ist."@de .

<http://rdvocab.info/roles/producer> rdfs:isDefinedBy <http://rdvocab.info/roles> ;
	reg:status <http://metadataregistry.org/uri/RegStatus/1002> ;
	reg:name "producer"@en ;
	rdfs:label "Producer"@en ;
	a :Property ;
	reg:hasSubproperty <http://rdvocab.info/roles/producerWork> , <http://rdvocab.info/roles/televisionProducer> , <http://rdvocab.info/roles/radioProducer> , <http://rdvocab.info/roles/filmProducer> ;
	rdfs:label "Produzent"@de .

<http://rdvocab.info/roles/producerWork> rdfs:isDefinedBy <http://rdvocab.info/roles> ;
	reg:status <http://metadataregistry.org/uri/RegStatus/1002> ;
	reg:name "producerWork"@en ;
	rdfs:label "Producer (Work)"@en ;
	skos:definition "A person, family, or corporate body responsible for most of the business aspects of a production for screen, sound recording, television, webcast, etc. The producer is generally responsible for fund raising, managing the production, hiring key personnel, arranging for distributors, etc."@en ;
	a :Property ;
	rdfs:domain <http://rdvocab.info/uri/schema/FRBRentitiesRDA/Work> ;
	rdfs:subPropertyOf <http://rdvocab.info/roles/producer> ;
	reg:hasSubproperty <http://rdvocab.info/roles/televisionProducerWork> , <http://rdvocab.info/roles/radioProducerWork> , <http://rdvocab.info/roles/filmProducerWork> ;
	skos:definition "Eine Person, Familie oder Körperschaft,  die Verantwortung für die meisten geschäftlichen Aspekte einer Darbietung für die Bühne, die Leinwand, eine Tonaufnahme, das Fernsehen, eine Internetübertragung usw. übernimmt. Der Produzent ist allgemein verantwortlich für die Geldbeschaffung, das Produktionsmanagement, die Einstellung der Kompetenzträger, die Organisation des Vertriebs, o.ä."@de ;
	rdfs:label "Produzent (Werk)"@de .

<http://rdvocab.info/roles/productionCompany> rdfs:isDefinedBy <http://rdvocab.info/roles> ;
	reg:status <http://metadataregistry.org/uri/RegStatus/1002> ;
	reg:name "productionCompany"@en ;
	rdfs:label "Production company"@en ;
	a :Property ;
	reg:hasSubproperty <http://rdvocab.info/roles/productionCompanyWork> ;
	rdfs:label "Produktionsunternehmen"@de ;
	skos:definition "Eine Körperschaft, die für das finanzielle, technische und organisatorische Management einer Produktion für Bühne, Leinwand, Tonaufnahme, Fernsehen, Internetübertragung o.ä. verantwortlich ist."@de .

<http://rdvocab.info/roles/productionCompanyWork> rdfs:isDefinedBy <http://rdvocab.info/roles> ;
	reg:status <http://metadataregistry.org/uri/RegStatus/1002> ;
	reg:name "productionCompanyWork"@en ;
	rdfs:label "Production company (Work)"@en ;
	skos:definition "A corporate body that is responsible for financial, technical, and organizational management of a production for stage, screen, sound recording, television, webcast, etc."@en ;
	a :Property ;
	rdfs:domain <http://rdvocab.info/uri/schema/FRBRentitiesRDA/Work> ;
	rdfs:subPropertyOf <http://rdvocab.info/roles/productionCompany> ;
	rdfs:label "Produktionsunternehmen (Werk)"@de ;
	skos:definition "Eine Körperschaft, die für das finanzielle, technische und organisatorische Management einer Produktion für Bühne, Leinwand, Tonaufnahme, Fernsehen, Internetübertragung o.ä. verantwortlich ist."@de .

<http://rdvocab.info/roles/productionDesigner> rdfs:isDefinedBy <http://rdvocab.info/roles> ;
	reg:status <http://metadataregistry.org/uri/RegStatus/1002> ;
	reg:name "productionDesigner"@en ;
	rdfs:label "Production designer"@en ;
	a :Property ;
	rdfs:label "Production Designer"@de .

<http://rdvocab.info/roles/productionDesignerExpression> rdfs:isDefinedBy <http://rdvocab.info/roles> ;
	reg:status <http://metadataregistry.org/uri/RegStatus/1002> ;
	reg:name "productionDesignerExpression"@en ;
	rdfs:label "Production designer (Expression)"@en ;
	skos:definition "A person, family, or corporate body responsible for designing the overall visual appearance of a moving image production."@en ;
	a :Property ;
	rdfs:subPropertyOf <http://rdvocab.info/roles/contributor> ;
	rdfs:domain <http://rdvocab.info/uri/schema/FRBRentitiesRDA/Expression> ;
	skos:definition "Eine Person, Familie oder Körperschaft, die für die Gestaltung des gesamten visuellen Erscheinungsbildes einer Bewegtbildproduktion verantwortlich ist."@de ;
	rdfs:label "Production Designer (Expression)"@de .

<http://rdvocab.info/roles/programmer> rdfs:isDefinedBy <http://rdvocab.info/roles> ;
	reg:status <http://metadataregistry.org/uri/RegStatus/1002> ;
	reg:name "programmer"@en ;
	rdfs:label "Programmer"@en ;
	a :Property ;
	rdfs:label "Programmierer"@de .

<http://rdvocab.info/roles/programmerWork> rdfs:isDefinedBy <http://rdvocab.info/roles> ;
	reg:status <http://metadataregistry.org/uri/RegStatus/1002> ;
	reg:name "programmerWork"@en ;
	rdfs:label "Programmer (Work)"@en ;
	skos:definition "A person, family, or corporate body responsible for creating a computer program."@en ;
	a :Property ;
	rdfs:subPropertyOf <http://rdvocab.info/roles/creator> ;
	rdfs:domain <http://rdvocab.info/uri/schema/FRBRentitiesRDA/Work> ;
	rdfs:label "Programmierer (Werk)"@de ;
	skos:definition "Eine Person, Familie oder Körperschaft, die für die Erstellung eines Computerprogramms verantwortlich ist."@de .

<http://rdvocab.info/roles/publisher> rdfs:isDefinedBy <http://rdvocab.info/roles> ;
	reg:status <http://metadataregistry.org/uri/RegStatus/1002> ;
	reg:name "publisher"@en ;
	rdfs:label "Publisher"@en ;
	a :Property ;
	reg:hasSubproperty <http://rdvocab.info/roles/publisherManifestation> , <http://rdvocab.info/roles/broadcaster> ;
	rdfs:label "Verlag"@de ;
	skos:definition "Eine Person, Familie oder Körperschaft, die für das Veröffentlichen, die Freigabe oder die Herausgabe einer Ressource verantwortlich ist."@de .

<http://rdvocab.info/roles/publisherManifestation> rdfs:isDefinedBy <http://rdvocab.info/roles> ;
	reg:status <http://metadataregistry.org/uri/RegStatus/1002> ;
	reg:name "publisherManifestation"@en ;
	rdfs:label "Publisher (Manifestation)"@en ;
	a :Property ;
	rdfs:subPropertyOf <http://rdvocab.info/roles/publisher> ;
	rdfs:domain <http://rdvocab.info/uri/schema/FRBRentitiesRDA/Manifestation> ;
	reg:hasSubproperty <http://rdvocab.info/roles/broadcasterManifestation> ;
	rdfs:label "Verlag (Manifestation)"@de ;
	skos:definition "Eine Person, Familie oder Körperschaft, die für das Veröffentlichen, die Freigabe oder die Herausgabe einer Ressource verantwortlich ist."@de .

<http://rdvocab.info/roles/puppeteer> rdfs:isDefinedBy <http://rdvocab.info/roles> ;
	reg:status <http://metadataregistry.org/uri/RegStatus/1002> ;
	reg:name "puppeteer"@en ;
	rdfs:label "Puppeteer"@en ;
	a :Property ;
	rdfs:subPropertyOf <http://rdvocab.info/roles/performer> ;
	rdfs:label "Puppenspieler"@de .

<http://rdvocab.info/roles/puppeteerExpression> rdfs:isDefinedBy <http://rdvocab.info/roles> ;
	reg:status <http://metadataregistry.org/uri/RegStatus/1002> ;
	reg:name "puppeteerExpression"@en ;
	rdfs:label "Puppeteer (Expression)"@en ;
	skos:definition "A performer contributing to an expression of a work by manipulating, controlling, or directing puppets or marionettes in a moving image production or a musical or dramatic presentation or entertainment."@en ;
	a :Property ;
	rdfs:domain <http://rdvocab.info/uri/schema/FRBRentitiesRDA/Expression> ;
	rdfs:label "Puppenspieler (Expression)"@de ;
	skos:definition "Ein Darsteller, der an einer Expression eines Werkes mitwirkt, indem er Puppen oder Marionetten in einer Bewegtbildproduktion oder einer musikalischen oder dramatischen Darbietung oder Aufführung bewegt, kontrolliert oder lenkt."@de .

<http://rdvocab.info/roles/radioDirector> rdfs:isDefinedBy <http://rdvocab.info/roles> ;
	reg:status <http://metadataregistry.org/uri/RegStatus/1002> ;
	reg:name "radioDirector"@en ;
	rdfs:label "Radio director"@en ;
	a :Property ;
	rdfs:subPropertyOf <http://rdvocab.info/roles/director> ;
	rdfs:label "Hörfunkintendant"@de .

<http://rdvocab.info/roles/radioDirectorWork> rdfs:isDefinedBy <http://rdvocab.info/roles> ;
	reg:status <http://metadataregistry.org/uri/RegStatus/1002> ;
	reg:name "radioDirectorWork"@en ;
	rdfs:label "Radio director (Work)"@en ;
	skos:definition "A director responsible for the general management and supervision of a radio program."@en ;
	a :Property ;
	rdfs:subPropertyOf <http://rdvocab.info/roles/directorWork> ;
	rdfs:domain <http://rdvocab.info/uri/schema/FRBRentitiesRDA/Work> ;
	rdfs:label "Hörfunkintendant (Werk)"@de ;
	skos:definition "Eine Person, Familie oder Körperschaft, die für das allgemeine Management und die Leitung eines Radioprogramms verantwortlich ist."@de .

<http://rdvocab.info/roles/radioProducer> rdfs:isDefinedBy <http://rdvocab.info/roles> ;
	reg:status <http://metadataregistry.org/uri/RegStatus/1002> ;
	reg:name "radioProducer"@en ;
	rdfs:label "Radio producer"@en ;
	a :Property ;
	rdfs:subPropertyOf <http://rdvocab.info/roles/producer> ;
	rdfs:label "Hörfunkproduzent"@de .

<http://rdvocab.info/roles/radioProducerWork> rdfs:isDefinedBy <http://rdvocab.info/roles> ;
	reg:status <http://metadataregistry.org/uri/RegStatus/1002> ;
	reg:name "radioProducerWork"@en ;
	rdfs:label "Radio producer (Work)"@en ;
	skos:definition "A producer responsible for most of the business aspects of a radio program."@en ;
	a :Property ;
	rdfs:subPropertyOf <http://rdvocab.info/roles/producerWork> ;
	rdfs:domain <http://rdvocab.info/uri/schema/FRBRentitiesRDA/Work> ;
	rdfs:label "Hörfunkproduzent (Werk)"@de ;
	skos:definition """Eine Person, Familie oder Körperschaft, die die Verantwortung für die meisten geschäftlichen Aspekte eines Radioprogramms übernimmt.
Der Radioproduzent ist hauptsächlich verantwortlich für die Geldbeschaffung, das Produktionsmanagement, die Einstellung der Kompetenzträger, die Organisation des Vertriebs, die Absicherung des kommerziellen Erfolges usw."""@de .

<http://rdvocab.info/roles/recordingEngineer> rdfs:isDefinedBy <http://rdvocab.info/roles> ;
	reg:status <http://metadataregistry.org/uri/RegStatus/1002> ;
	reg:name "recordingEngineer"@en ;
	rdfs:label "Recording engineer"@en ;
	a :Property ;
	rdfs:label "Toningenieur"@de .

<http://rdvocab.info/roles/recordingEngineerExpression> rdfs:isDefinedBy <http://rdvocab.info/roles> ;
	reg:status <http://metadataregistry.org/uri/RegStatus/1002> ;
	reg:name "recordingEngineerExpression"@en ;
	rdfs:label "Recording engineer (Expression)"@en ;
	skos:definition "A person, family, or corporate body contributing to an expression of a work by supervising the technical aspects of a sound or video recording session."@en ;
	a :Property ;
	rdfs:subPropertyOf <http://rdvocab.info/roles/contributor> ;
	rdfs:domain <http://rdvocab.info/uri/schema/FRBRentitiesRDA/Expression> ;
	rdfs:label "Toningenieur (Expression)"@de ;
	skos:definition "Eine Person, Familie oder Körperschaft, die an einer Expression eines Werkes mitwirkt, indem sie die technischen Aspekte einer Ton- oder Videoaufnahme überwacht"@de .

<http://rdvocab.info/roles/recordist> rdfs:isDefinedBy <http://rdvocab.info/roles> ;
	reg:status <http://metadataregistry.org/uri/RegStatus/1002> ;
	reg:name "recordist"@en ;
	rdfs:label "Recordist"@en ;
	a :Property ;
	rdfs:label "Recordist"@de .

<http://rdvocab.info/roles/recordistExpression> rdfs:isDefinedBy <http://rdvocab.info/roles> ;
	reg:status <http://metadataregistry.org/uri/RegStatus/1002> ;
	reg:name "recordistExpression"@en ;
	rdfs:label "Recordist (Expression)"@en ;
	skos:definition "A person, family, or corporate body contributing to an expression of a work by using a recording device to capture sound and/or video during a recording session, including field recordings of natural sounds, folkloric events, music, etc."@en ;
	a :Property ;
	rdfs:subPropertyOf <http://rdvocab.info/roles/contributor> ;
	rdfs:domain <http://rdvocab.info/uri/schema/FRBRentitiesRDA/Expression> ;
	rdfs:label "Recordist (Expression)"@de ;
	skos:definition "Eine Person, Familie oder Körperschaft, die an einer Expression eines Werkes mitwirkt, indem sie mit einem Aufzeichnungsgerät Ton und/oder Bild aufnimmt, einschließlich Außenaufnahmen natürlicher Geräusche, folkloristischer Veranstaltungen, Musik o.ä."@de .

<http://rdvocab.info/roles/respondent> rdfs:isDefinedBy <http://rdvocab.info/roles> ;
	reg:status <http://metadataregistry.org/uri/RegStatus/1002> ;
	reg:name "respondent"@en ;
	rdfs:label "Respondent"@en ;
	a :Property ;
	rdfs:label "Respondent"@de .

<http://rdvocab.info/roles/respondentWork> rdfs:isDefinedBy <http://rdvocab.info/roles> ;
	reg:status <http://metadataregistry.org/uri/RegStatus/1002> ;
	reg:name "respondentWork"@en ;
	rdfs:label "Respondent (Work)"@en ;
	skos:definition "A candidate for a degree who defends or opposes a theses provided by the praeses in an academic disputation. Also called defendant."@en ;
	a :Property ;
	rdfs:subPropertyOf <http://rdvocab.info/roles/creator> ;
	rdfs:domain <http://rdvocab.info/uri/schema/FRBRentitiesRDA/Work> ;
	rdfs:label "Respondent (Werk)"@de ;
	skos:definition "Ein Kandidat für einen akademischen Grad, der eine These, die von dem Disputationsleiter in einer akademischen Disputation aufgestellt wurde, verteidigt oder ablehnt. Auch Proponent / Opponent genannt."@de .

<http://rdvocab.info/roles/restorationist> rdfs:isDefinedBy <http://rdvocab.info/roles> ;
	reg:status <http://metadataregistry.org/uri/RegStatus/1002> ;
	reg:name "restorationist"@en ;
	rdfs:label "Restorationist"@en ;
	a :Property ;
	reg:hasSubproperty <http://rdvocab.info/roles/restorationistItem> ;
	rdfs:label "Restaurator"@de .

<http://rdvocab.info/roles/restorationistItem> rdfs:isDefinedBy <http://rdvocab.info/roles> ;
	reg:status <http://metadataregistry.org/uri/RegStatus/1002> ;
	reg:name "restorationistItem"@en ;
	rdfs:label "Restorationist (Item)"@en ;
	skos:definition "A person, family, or corporate body responsible for the set of technical, editorial and intellectual procedures aimed at compensating for the degradation of an artifact, such as bringing it back to a state as close as possible to its original condition."@en ;
	a :Property ;
	rdfs:domain <http://rdvocab.info/uri/schema/FRBRentitiesRDA/Item> ;
	rdfs:subPropertyOf <http://rdvocab.info/roles/restorationist> ;
	rdfs:label "Restaurator"@de ;
	skos:definition "Eine Person, Familie oder Körperschaft, die für den Vertrieb einer Bewegtbildmanifestation an Kinos oder andere Vertriebskanäle verantwortlich ist."@de .

<http://rdvocab.info/roles/screenwriter> rdfs:isDefinedBy <http://rdvocab.info/roles> ;
	reg:status <http://metadataregistry.org/uri/RegStatus/1002> ;
	reg:name "screenwriter"@en ;
	rdfs:label "Screenwriter"@en ;
	a :Property ;
	rdfs:subPropertyOf <http://rdvocab.info/roles/author> ;
	rdfs:label "Drehbuchautor"@de .

<http://rdvocab.info/roles/screenwriterWork> rdfs:isDefinedBy <http://rdvocab.info/roles> ;
	reg:status <http://metadataregistry.org/uri/RegStatus/1002> ;
	reg:name "screenwriterWork"@en ;
	rdfs:label "Screenwriter (Work)"@en ;
	skos:definition "An author of a screenplay, script, or scene."@en ;
	a :Property ;
	rdfs:domain <http://rdvocab.info/uri/schema/FRBRentitiesRDA/Work> ;
	rdfs:label "Drehbuchautor (Werk)"@de ;
	skos:definition "Ein Autor eines Drehbuchs, eines Manuskripts oder einer Szene."@de ;
	rdfs:subPropertyOf <http://rdvocab.info/roles/authorWork> .

<http://rdvocab.info/roles/sculptor> rdfs:isDefinedBy <http://rdvocab.info/roles> ;
	reg:status <http://metadataregistry.org/uri/RegStatus/1002> ;
	reg:name "sculptor"@en ;
	rdfs:label "Sculptor"@en ;
	a :Property ;
	rdfs:subPropertyOf <http://rdvocab.info/roles/artist> ;
	rdfs:label "Bildhauer"@de .

<http://rdvocab.info/roles/sculptorWork> rdfs:isDefinedBy <http://rdvocab.info/roles> ;
	reg:status <http://metadataregistry.org/uri/RegStatus/1002> ;
	reg:name "sculptorWork"@en ;
	rdfs:label "Sculptor (Work)"@en ;
	skos:definition "An artist responsible for creating a three-dimensional work by modeling, carving, or similar technique."@en ;
	a :Property ;
	rdfs:domain <http://rdvocab.info/uri/schema/FRBRentitiesRDA/Work> ;
	rdfs:label "Bildhauer (Werk)"@de ;
	skos:definition "Ein Künstler, der für die Erstellung eines dreidimensionalen Werkes durch Modellierung, Schnitzen oder ähnliche Techniken verantwortlich ist."@de .

<http://rdvocab.info/roles/seller> rdfs:isDefinedBy <http://rdvocab.info/roles> ;
	reg:status <http://metadataregistry.org/uri/RegStatus/1002> ;
	reg:name "seller"@en ;
	rdfs:label "Seller"@en ;
	a :Property ;
	rdfs:subPropertyOf <http://rdvocab.info/roles/formerOwner> ;
	rdfs:label "Verkäufer"@de .

<http://rdvocab.info/roles/sellerItem> rdfs:isDefinedBy <http://rdvocab.info/roles> ;
	reg:status <http://metadataregistry.org/uri/RegStatus/1002> ;
	reg:name "sellerItem"@en ;
	rdfs:label "Seller (Item)"@en ;
	skos:definition "A former owner of an item who sold that item to another owner."@en ;
	a :Property ;
	rdfs:subPropertyOf <http://rdvocab.info/roles/formerOwnerItem> ;
	rdfs:domain <http://rdvocab.info/uri/schema/FRBRentitiesRDA/Item> ;
	rdfs:label "Verkäufer (Exemplar)"@de ;
	skos:definition "Ein ehemaliger Eigentümer eines Exemplars, der dieses Exemplar an einen anderen Eigentümer verkauft hat."@de .

<http://rdvocab.info/roles/singer> rdfs:isDefinedBy <http://rdvocab.info/roles> ;
	reg:status <http://metadataregistry.org/uri/RegStatus/1002> ;
	reg:name "singer"@en ;
	rdfs:label "Singer"@en ;
	a :Property ;
	rdfs:subPropertyOf <http://rdvocab.info/roles/performer> ;
	rdfs:label "Sänger"@de .

<http://rdvocab.info/roles/singerExpression> rdfs:isDefinedBy <http://rdvocab.info/roles> ;
	reg:status <http://metadataregistry.org/uri/RegStatus/1002> ;
	reg:name "singerExpression"@en ;
	rdfs:label "Singer (Expression)"@en ;
	skos:definition "A performer contributing to an expression of a work by using his/her/their voice, with or without instrumental accompaniment, to produce music. A singer’s performance may or may not include actual words."@en ;
	a :Property ;
	rdfs:subPropertyOf <http://rdvocab.info/roles/performerExpression> ;
	rdfs:domain <http://rdvocab.info/uri/schema/FRBRentitiesRDA/Expression> ;
	rdfs:label "Sänger (Expression)"@de ;
	skos:definition "Ein Darsteller, der an einer Expression eines Werkes mitwirkt, indem er durch seine Stimme mit oder ohne instrumentale Begleitung Musik erzeugt. Die Darbietung eines Sängers kann Worte enthalten oder nicht."@de .

<http://rdvocab.info/roles/speaker> rdfs:isDefinedBy <http://rdvocab.info/roles> ;
	reg:status <http://metadataregistry.org/uri/RegStatus/1002> ;
	reg:name "speaker"@en ;
	rdfs:label "Speaker"@en ;
	a :Property ;
	rdfs:subPropertyOf <http://rdvocab.info/roles/performer> ;
	rdfs:label "Sprecher"@de .

<http://rdvocab.info/roles/speakerExpression> rdfs:isDefinedBy <http://rdvocab.info/roles> ;
	reg:status <http://metadataregistry.org/uri/RegStatus/1002> ;
	reg:name "speakerExpression"@en ;
	rdfs:label "Speaker (Expression)"@en ;
	skos:definition "A performer contributing to an expression of a work by speaking words, such as a lecture, speech, etc."@en ;
	a :Property ;
	rdfs:subPropertyOf <http://rdvocab.info/roles/performerExpression> ;
	rdfs:domain <http://rdvocab.info/uri/schema/FRBRentitiesRDA/Expression> ;
	rdfs:label "Sprecher (Expression)"@de ;
	skos:definition "Ein Darsteller, der an einer Expression eines Werkes durch das Sprechen von Worten, wie z.B. einen Vortrag, eine Rede o.ä. mitwirkt."@de .

<http://rdvocab.info/roles/sponsoringBody> rdfs:isDefinedBy <http://rdvocab.info/roles> ;
	reg:status <http://metadataregistry.org/uri/RegStatus/1002> ;
	reg:name "sponsoringBody"@en ;
	rdfs:label "Sponsoring body"@en ;
	a :Property ;
	reg:hasSubproperty <http://rdvocab.info/roles/sponsoringBodyWork> ;
	rdfs:label "Sponsor"@de .

<http://rdvocab.info/roles/sponsoringBodyWork> rdfs:isDefinedBy <http://rdvocab.info/roles> ;
	reg:status <http://metadataregistry.org/uri/RegStatus/1002> ;
	reg:name "sponsoringBodyWork"@en ;
	rdfs:label "Sponsoring body (Work)"@en ;
	skos:definition "A person, family, or corporate body sponsoring some aspect of the work, e.g., funding research, sponsoring an event."@en ;
	a :Property ;
	rdfs:domain <http://rdvocab.info/uri/schema/FRBRentitiesRDA/Work> ;
	rdfs:subPropertyOf <http://rdvocab.info/roles/sponsoringBody> ;
	rdfs:label "Sponsor (Werk)"@de ;
	skos:definition "Eine Person, Familie oder Körperschaft, die einzelne Aspekte des Werks finanziell unterstützt, z. B. Forschungsförderung, finanzielle Unterstützung einer Veranstaltung."@de .

<http://rdvocab.info/roles/stageDirector> rdfs:isDefinedBy <http://rdvocab.info/roles> ;
	reg:status <http://metadataregistry.org/uri/RegStatus/1002> ;
	reg:name "stageDirector"@en ;
	rdfs:label "Stage director"@en ;
	a :Property ;
	rdfs:label "Theaterregisseur"@de .

<http://rdvocab.info/roles/stageDirectorExpression> rdfs:isDefinedBy <http://rdvocab.info/roles> ;
	reg:status <http://metadataregistry.org/uri/RegStatus/1002> ;
	reg:name "stageDirectorExpression"@en ;
	rdfs:label "Stage director (Expression)"@en ;
	skos:definition "A person, family, or corporate body contributing to an expression of a stage work through the general management and supervision of a performance."@en ;
	a :Property ;
	rdfs:subPropertyOf <http://rdvocab.info/roles/contributor> ;
	rdfs:domain <http://rdvocab.info/uri/schema/FRBRentitiesRDA/Expression> ;
	rdfs:label "Theaterregisseur"@de ;
	skos:definition "Eine Person, Familie oder Körperschaft, die an der Expression eines Bühnenwerks durch die allgemeine Betreuung und Leitung einer Darbietung mitwirken."@de .

<http://rdvocab.info/roles/storyteller> rdfs:isDefinedBy <http://rdvocab.info/roles> ;
	reg:status <http://metadataregistry.org/uri/RegStatus/1002> ;
	reg:name "storyteller"@en ;
	rdfs:label "Storyteller"@en ;
	a :Property ;
	rdfs:subPropertyOf <http://rdvocab.info/roles/performer> ;
	rdfs:label "Geschichtenerzähler"@de .

<http://rdvocab.info/roles/storytellerExpression> rdfs:isDefinedBy <http://rdvocab.info/roles> ;
	reg:status <http://metadataregistry.org/uri/RegStatus/1002> ;
	reg:name "storytellerExpression"@en ;
	rdfs:label "Storyteller (Expression)"@en ;
	skos:definition "A performer contributing to an expression of a work by relaying a creator’s original story with dramatic or theatrical interpretation."@en ;
	a :Property ;
	rdfs:subPropertyOf <http://rdvocab.info/roles/performerExpression> ;
	rdfs:domain <http://rdvocab.info/uri/schema/FRBRentitiesRDA/Expression> ;
	rdfs:label "Geschichtenerzähler (Expression)"@de ;
	skos:definition "Ein Darsteller, der an einer Expression eines Werks mitwirkt, indem er die ursprüngliche Geschichte eines geistigen Schöpfers mit dramatischer oder theatralischer Interpretation weitergibt."@de .

<http://rdvocab.info/roles/surveyor> rdfs:isDefinedBy <http://rdvocab.info/roles> ;
	reg:status <http://metadataregistry.org/uri/RegStatus/1002> ;
	reg:name "surveyor"@en ;
	rdfs:label "Surveyor"@en ;
	a :Property ;
	rdfs:label "Vermesser"@de .

<http://rdvocab.info/roles/surveyorExpression> rdfs:isDefinedBy <http://rdvocab.info/roles> ;
	reg:status <http://metadataregistry.org/uri/RegStatus/1002> ;
	reg:name "surveyorExpression"@en ;
	rdfs:label "Surveyor (Expression)"@en ;
	skos:definition "A person, family, or corporate body contributing to an expression of a cartographic work by providing measurements or dimensional relationships for the geographic area represented."@en ;
	a :Property ;
	rdfs:subPropertyOf <http://rdvocab.info/roles/contributor> ;
	rdfs:domain <http://rdvocab.info/uri/schema/FRBRentitiesRDA/Expression> ;
	rdfs:label "Vermesser (Expression)"@de ;
	skos:definition """Eine Person, Familie oder Körperschaft, die an der Expression eines kartografischen Werkes mitwirkt, indem sie Messwerte oder Abmessungsverhältnisse
für den dargestellten geografischen Bereich zur Verfügung stellt."""@de .

<http://rdvocab.info/roles/teacher> rdfs:isDefinedBy <http://rdvocab.info/roles> ;
	reg:status <http://metadataregistry.org/uri/RegStatus/1002> ;
	reg:name "teacher"@en ;
	rdfs:label "Teacher"@en ;
	a :Property ;
	rdfs:subPropertyOf <http://rdvocab.info/roles/performer> ;
	rdfs:label "Lehrer"@de .

<http://rdvocab.info/roles/teacherExpression> rdfs:isDefinedBy <http://rdvocab.info/roles> ;
	reg:status <http://metadataregistry.org/uri/RegStatus/1002> ;
	reg:name "teacherExpression"@en ;
	rdfs:label "Teacher (Expression)"@en ;
	skos:definition "A performer contributing to an expression of a work by giving instruction or providing a demonstration."@en ;
	a :Property ;
	rdfs:domain <http://rdvocab.info/uri/schema/FRBRentitiesRDA/Expression> ;
	rdfs:label "Lehrer (Expression)"@de ;
	skos:definition "Ein Darsteller, der im Zusammenhang mit einer Expression eines Werkes Anleitungen gibt oder Demonstrationen bietet."@de .

<http://rdvocab.info/roles/televisionDirector> rdfs:isDefinedBy <http://rdvocab.info/roles> ;
	reg:status <http://metadataregistry.org/uri/RegStatus/1002> ;
	reg:name "televisionDirector"@en ;
	rdfs:label "Television director"@en ;
	a :Property ;
	rdfs:subPropertyOf <http://rdvocab.info/roles/director> ;
	rdfs:label "Fernsehintendant"@de .

<http://rdvocab.info/roles/televisionDirectorWork> rdfs:isDefinedBy <http://rdvocab.info/roles> ;
	reg:status <http://metadataregistry.org/uri/RegStatus/1002> ;
	reg:name "televisionDirectorWork"@en ;
	rdfs:label "Television director (Work)"@en ;
	skos:definition "A director responsible for the general management and supervision of a television program."@en ;
	a :Property ;
	rdfs:subPropertyOf <http://rdvocab.info/roles/directorWork> ;
	rdfs:domain <http://rdvocab.info/uri/schema/FRBRentitiesRDA/Work> ;
	rdfs:label "Fernsehintendant (Werk)"@de ;
	skos:definition "Eine Person, Familie oder Körperschaft, die für das allgemeine Management und die Leitung eines Fernsehprogramms verantwortlich ist."@de .

<http://rdvocab.info/roles/televisionProducer> rdfs:isDefinedBy <http://rdvocab.info/roles> ;
	reg:status <http://metadataregistry.org/uri/RegStatus/1002> ;
	reg:name "televisionProducer"@en ;
	rdfs:label "Television producer"@en ;
	a :Property ;
	reg:hasSubproperty <http://rdvocab.info/roles/televisionProducerWork> ;
	rdfs:subPropertyOf <http://rdvocab.info/roles/producer> ;
	rdfs:label "Fernsehproduzent"@de .

<http://rdvocab.info/roles/televisionProducerWork> rdfs:isDefinedBy <http://rdvocab.info/roles> ;
	reg:status <http://metadataregistry.org/uri/RegStatus/1002> ;
	reg:name "televisionProducerWork"@en ;
	rdfs:label "Television producer (Work)"@en ;
	skos:definition "A producer responsible for most of the business aspects of a television program."@en ;
	a :Property ;
	rdfs:domain <http://rdvocab.info/uri/schema/FRBRentitiesRDA/Work> ;
	rdfs:subPropertyOf <http://rdvocab.info/roles/producerWork> ;
	rdfs:label "Fernsehproduzent (Werk)"@de ;
	skos:definition """Eine Person, Familie oder Körperschaft, die die Verantwortung für die meisten geschäftlichen Aspekte eines Fernsehprogramms übernimmt.
Der Fernsehproduzent ist hauptsächlich verantwortlich für die Geldbeschaffung, das Produktionsmanagement, die Einstellung der Kompetenzträger, die Organisation des Vertriebs, die Absicherung des kommerziellen Erfolges usw."""@de .

<http://rdvocab.info/roles/thesisAdvisor> rdfs:isDefinedBy <http://rdvocab.info/roles> ;
	reg:status <http://metadataregistry.org/uri/RegStatus/1002> ;
	reg:name "thesisAdvisor"@en ;
	rdfs:label "Thesis Advisor"@en ;
	a :Property .

<http://rdvocab.info/roles/transcriber> rdfs:isDefinedBy <http://rdvocab.info/roles> ;
	reg:status <http://metadataregistry.org/uri/RegStatus/1002> ;
	reg:name "transcriber"@en ;
	rdfs:label "Transcriber"@en ;
	a :Property ;
	rdfs:label "Transkribierer"@de .

<http://rdvocab.info/roles/transcriberExpression> rdfs:isDefinedBy <http://rdvocab.info/roles> ;
	reg:status <http://metadataregistry.org/uri/RegStatus/1002> ;
	reg:name "transcriberExpression"@en ;
	rdfs:label "Transcriber (Expression)"@en ;
	skos:definition "A person, family, or corporate body contributing to an expression of a work by changing it from one system of notation to another."@en ;
	a :Property ;
	rdfs:subPropertyOf <http://rdvocab.info/roles/contributor> ;
	rdfs:domain <http://rdvocab.info/uri/schema/FRBRentitiesRDA/Expression> ;
	skos:definition "Eine Person, Familie oder Körperschaft, die an einer Expression eines Werkes mitwirkt, indem sie es von einem Notationssystem in ein anderes überträgt."@de ;
	rdfs:label "Transkribierer (Expression)"@de .

<http://rdvocab.info/roles/translator> rdfs:isDefinedBy <http://rdvocab.info/roles> ;
	reg:status <http://metadataregistry.org/uri/RegStatus/1002> ;
	reg:name "translator"@en ;
	rdfs:label "Translator"@en ;
	a :Property ;
	rdfs:label "Übersetzer"@de .

<http://rdvocab.info/roles/translatorExpression> rdfs:isDefinedBy <http://rdvocab.info/roles> ;
	reg:status <http://metadataregistry.org/uri/RegStatus/1002> ;
	reg:name "translatorExpression"@en ;
	rdfs:label "Translator (Expression)"@en ;
	skos:definition "A person, family, or corporate body contributing to an expression of a work by rendering one language into another, or from an older form of a language into the modern form, that more or less closely follows the original text of the work."@en ;
	a :Property ;
	rdfs:subPropertyOf <http://rdvocab.info/roles/contributor> ;
	rdfs:domain <http://rdvocab.info/uri/schema/FRBRentitiesRDA/Expression> ;
	rdfs:label "Übersetzer (Expression)"@de ;
	skos:definition "Eine Person, Familie oder Körperschaft, die an einer Expression eines Werkes mitwirkt, indem sie eine Sprache in eine andere übersetzt, oder aus einer älteren Sprachform in die moderne Form, die mehr oder weniger eng dem Originaltext des Werkes folgt."@de .

<http://rdvocab.info/roles/writerOfAddedCommentary> rdfs:isDefinedBy <http://rdvocab.info/roles> ;
	reg:status <http://metadataregistry.org/uri/RegStatus/1002> ;
	reg:name "writerOfAddedCommentary"@en ;
	rdfs:label "Writer of added commentary"@en ;
	a :Property ;
	rdfs:label "Kommentator (schriftlich)"@de .

<http://rdvocab.info/roles/writerOfAddedCommentaryExpression> rdfs:isDefinedBy <http://rdvocab.info/roles> ;
	reg:status <http://metadataregistry.org/uri/RegStatus/1002> ;
	reg:name "writerOfAddedCommentaryExpression"@en ;
	rdfs:label "Writer of added commentary (Expression)"@en ;
	skos:definition "A person, family, or corporate body contributing to an expression of a work by providing an interpretation or critical explanation of the original work."@en ;
	a :Property ;
	rdfs:subPropertyOf <http://rdvocab.info/roles/contributor> ;
	rdfs:domain <http://rdvocab.info/uri/schema/FRBRentitiesRDA/Expression> ;
	rdfs:label "Kommentator (schriftlich) (Eypression)"@de ;
	skos:definition "Eine Person, Familie oder Körperschaft, die an einer Expression eines Werkes mitwirkt, indem sie eine Interpretation oder kritische Erläuterung des Originalwerkes verfasst."@de .

<http://rdvocab.info/roles/writerOfAddedLyrics> rdfs:isDefinedBy <http://rdvocab.info/roles> ;
	reg:status <http://metadataregistry.org/uri/RegStatus/1002> ;
	reg:name "writerOfAddedLyrics"@en ;
	rdfs:label "Writer of added lyrics"@en ;
	a :Property ;
	rdfs:subPropertyOf <http://rdvocab.info/roles/writerOfAddedText> ;
	rdfs:label "Verfasser eines Textes, der nachträglich einem Musikwerk unterlegt wird"@de .

<http://rdvocab.info/roles/writerOfAddedLyricsExpression> rdfs:isDefinedBy <http://rdvocab.info/roles> ;
	reg:status <http://metadataregistry.org/uri/RegStatus/1002> ;
	reg:name "writerOfAddedLyricsExpression"@en ;
	rdfs:label "Writer of added lyrics (Expression)"@en ;
	skos:definition "A writer of words added to an expression of a musical work."@en ;
	a :Property ;
	rdfs:domain <http://rdvocab.info/uri/schema/FRBRentitiesRDA/Expression> ;
	rdfs:label "Verfasser eines Textes, der nachträglich einem Musikwerk unterlegt wird (Expression)."@de ;
	skos:definition "Ein Verfasser eines Textes, der einer Expression eines Musikwerkes beigefügt wird."@de .

<http://rdvocab.info/roles/writerOfAddedText> rdfs:isDefinedBy <http://rdvocab.info/roles> ;
	reg:status <http://metadataregistry.org/uri/RegStatus/1002> ;
	reg:name "writerOfAddedText"@en ;
	rdfs:label "Writer of added text"@en ;
	a :Property ;
	reg:hasSubproperty <http://rdvocab.info/roles/writerOfAddedLyrics> ;
	rdfs:label "Verfasser von Zusatztexten"@de .

<http://rdvocab.info/roles/writerOfAddedTextExpression> rdfs:isDefinedBy <http://rdvocab.info/roles> ;
	reg:status <http://metadataregistry.org/uri/RegStatus/1002> ;
	reg:name "writerOfAddedTextExpression"@en ;
	rdfs:label "Writer of added text (Expression)"@en ;
	skos:definition "A person, family, or corporate body contributing to an expression of a primarily non-textual work by providing text for the non-textual work (e.g., writing captions for photographs, descriptions of maps)."@en ;
	a :Property ;
	rdfs:subPropertyOf <http://rdvocab.info/roles/contributor> ;
	rdfs:domain <http://rdvocab.info/uri/schema/FRBRentitiesRDA/Expression> ;
	rdfs:label "Verfasser von Zusatztexten (Expression)"@de ;
	skos:definition "Eine Person, Familie oder Körperschaft, die an einer Expression eines primär nicht-textlichen Werkes mitwirkt, indem sie Texte für das nicht-textliche Werk eines anderen Schöpfers verfasst (z.B. Bildunterschriften für Fotografien, Beschreibungen von Karten)."@de .

<http://metadataregistry.org/uri/RegStatus/1002> a skos:Concept ;
	skos:prefLabel "New-Proposed"@en .
