@prefix : <http://purl.org/imbi/ru-meta.owl#> .
@prefix rdfs: <http://www.w3.org/2000/01/rdf-schema#> .
@prefix owl: <http://www.w3.org/2002/07/owl#> .
@prefix xsd: <http://www.w3.org/2001/XMLSchema#> .
@prefix rdf: <http://www.w3.org/1999/02/22-rdf-syntax-ns#> .

<http://purl.org/imbi/ru-meta.owl> a owl:Ontology ;
	rdfs:comment """This is the dirst draft for a recommendation for metadata on Representational Units (RU) which appear in ontologies. It is so far harmonized for implementation through owl annotation properties.
Comments to: OBI discussion list, metadata wiki or to  schober at ebi.ac.uk"""^^xsd:string ;
	rdfs:label "RU_metadata_ontology"^^xsd:string ;
	owl:versionInfo "0.1"^^xsd:float .

:_deleted a owl:Class ;
	rdfs:comment "This residual category holds deleted classes"^^xsd:string ;
	rdfs:subClassOf owl:Thing .

owl:Thing a owl:Class .

:_inclusion_list a owl:Class ;
	rdfs:comment "This residual category holds yet to be classified (mass-)imported terms as a simple list."^^xsd:string ;
	rdfs:subClassOf owl:Thing .

:_temp_orphan a owl:Class ;
	rdfs:comment "A temporal store for classes that are being worked on."^^xsd:string ;
	rdfs:subClassOf owl:Thing .

:scope_note a owl:AnnotationProperty ;
	rdfs:comment "Any general formless remark or note about the scope of the RU (was: rem, note)."^^xsd:string .

:cls_expl a owl:AnnotationProperty ;
	rdfs:comment "A prototypical example subclass for the class."^^xsd:string .

:prpty_name a owl:AnnotationProperty ;
	rdfs:comment "A name of the property, analogously as a cls_name."^^xsd:string .

:cls_prov a owl:AnnotationProperty ;
	rdfs:comment """The class name provenance. It can be a source publication, a database or ontology entry, a group,  person name or a URL (dbxref in obo)
A database cross reference. ???"""^^xsd:string .

:unresolved_issue a owl:AnnotationProperty ;
	rdfs:comment "An important problematic issue that has to be tackled by the editors."^^xsd:string .

:del_date a owl:AnnotationProperty ;
	rdfs:comment "The date a RU was deleted."^^xsd:string .

:old_cls_state a owl:AnnotationProperty ;
	rdfs:comment "State wheather a class was defined or primitive when deleted."^^xsd:string .

:pref_cls_name a owl:AnnotationProperty ;
	rdfs:comment "The preferred name for a class, usually the one used to display in the Hierarchy-browser. As now captured in the rdf:label ???"^^xsd:string .

:prpty_prov a owl:AnnotationProperty ;
	rdfs:comment """The property name provenance. It can be a source publication, a database or ontology entry, a group,  person name or a URL (dbxref in obo)
A database cross reference. ???"""^^xsd:string .

:cls_del a owl:AnnotationProperty ;
	rdfs:comment "Allows to state the reason why a RU has been deleted."^^xsd:string .

:prpty_expl a owl:AnnotationProperty ;
	rdfs:comment "A prototypic example od a sub-property of this property )when property hierarchies are allowed."^^xsd:string .

:UMLS_connect a owl:AnnotationProperty ;
	rdfs:comment "A link to a UMLS semantic Type CUI."^^xsd:string .

:pref_propty_name a owl:AnnotationProperty ;
	rdfs:comment "The preferred name for a class, usually the one used to display in the Hierarchy-browser."^^xsd:string .

:action_item a owl:AnnotationProperty ;
	rdfs:comment "A description of a task / action for the RU editor to solve an issue related to the RU."^^xsd:string .

:temp_def a owl:AnnotationProperty ;
	rdfs:comment "Indicates definitions which need to be refined."^^xsd:string .

:curation_status a owl:AnnotationProperty ;
	rdfs:comment "The status (stability level) of the class. Specifies tracking information. E.g. unstable, experimental, stable."^^xsd:string .

:editor a owl:AnnotationProperty ;
	rdfs:comment "The name of a specific editior/curator who is responsible for and edits this RU."^^xsd:string .

:prpty_del a owl:AnnotationProperty ;
	rdfs:comment "State the reason why a property was deleted, analogously as for cla_del."^^xsd:string .

:def a owl:AnnotationProperty ;
	rdfs:comment "The arestotelian, formalized and normalized class definition layed out according to IFOMIS-best practice, explanaining the meaning of a class."^^xsd:string .

:formal_cls_name a owl:AnnotationProperty ;
	rdfs:comment "A name for the class that is formaly controlled through linguistical rules and axioms. E.G. OBOL normalized ones that adhere to defined principles of word/morpheme/affix order and form. ???"^^xsd:string .

:cls_name a owl:AnnotationProperty ;
	rdfs:comment "Any name of the class. ??? Will change according to Synonym implementation..."^^xsd:string .

:short_cls_name a owl:AnnotationProperty ;
	rdfs:comment "A short class name suitable for graph visualisations etc."^^xsd:string .

:axiom a owl:AnnotationProperty ;
	rdfs:comment "General axioms to be fulfilled by instances of the class can be captured in an informal way in natural language here."^^xsd:string .

:acronym a owl:AnnotationProperty ;
	rdfs:comment "A common accepted acronyn for the RU-name."^^xsd:string .

:short_prpty_name a owl:AnnotationProperty ;
	rdfs:comment "A shortproperty name suitable for graph visualisations etc."^^xsd:string .

:def_prov a owl:AnnotationProperty ;
	rdfs:comment "The definition provenance (was: Defsource). It can be a source publication, a database or ontology entry, a group or person name or a URL (dbxref in obo)"^^xsd:string .

:editor_note a owl:AnnotationProperty ;
	rdfs:comment "A note related to the RU intended for its editor."^^xsd:string .

:creation_date a owl:AnnotationProperty ;
	rdfs:comment "The date when a RU was first created. (Will be provided automatically by Protege 4)."^^xsd:string .

:alt_def a owl:AnnotationProperty ;
	rdfs:comment "An alternative definition. Usually the non-aristotelian natural language definition initially provided by domain specialists."^^xsd:string .

:context_keyword a owl:AnnotationProperty ;
	rdfs:comment "The main usage contexts can be stated, e.g. for text mining purposes or translation purposes."^^xsd:string .

:inst_expl a owl:AnnotationProperty ;
	rdfs:comment "An example  value or instance for the class or Database entry which will be annotated through this RU."^^xsd:string .

:synonym a owl:AnnotationProperty ;
	rdfs:comment "An alternative name for the RU used as synonym (can be used in the same manner as the name in different contexts)."^^xsd:string .

:replace a owl:AnnotationProperty ;
	rdfs:comment "When a new RU-name replaces an old one, state here which one was replaced. ???"^^xsd:string .

:refact a owl:AnnotationProperty ;
	rdfs:comment "When a class has been refactored into more atomic classes, then the original compound class is made obsolete and this deleted source class which gave birth to the new atomic child classes is mentioned here for all new atomic classes."^^xsd:string .

:rights a owl:AnnotationProperty ;
	rdfs:comment "Indicate access rights for a RU. The security policy should be compliant with the rule-based access control standards,INCITS, InterNational Committee for Information Technology Standards (formerly NCITS). (2003). Role Based Access Control. INCITS 359 DRAF, 4/4/2003. http://csrc.nist.gov/rbac/ Those offer, in at the same time, a consistent layered approach for security policy definition and management and for compliance with a growing set of supporting tools."^^xsd:string .

:old_sub_cls a owl:AnnotationProperty ;
	rdfs:comment "For deleted classes state their last position within the ontology, state the old subclasses."^^xsd:string .

:change_note a owl:AnnotationProperty ;
	rdfs:comment """A note that indicates what was modified or changed concerning the RU. 
Might become RU specific, i.e. cls_change_note AND prpty_change_note"""^^xsd:string .

:cls_id a owl:AnnotationProperty ;
	rdfs:comment "A unique Identifyer for the class, consisting of a groups prefix, underscore and unique number."^^xsd:string .

:abbrev a owl:AnnotationProperty ;
	rdfs:comment "A common accepted abbreviation for the RU-name. A word formed from the initials of one or more words describing the name, that is pronounceable like a normal word."^^xsd:string .

:alt_spr_cls a owl:AnnotationProperty ;
	rdfs:comment "An alternative superclass assertion. Used to capture multiple parenthood."^^xsd:string .

:modif_date a owl:AnnotationProperty ;
	rdfs:comment "The date on which the RU was last modified."^^xsd:string .

:ont_imp a owl:AnnotationProperty ;
	rdfs:comment "To mark from where on in the Class-hierarchy we want to import / refer to a complete subclass hierarchy from an other ontology (was: refer to) ??? Maybe better: cls_imp"^^xsd:string .

:source a owl:AnnotationProperty ;
	rdfs:comment """??? rel to ont_imp
??? rel to def_prov or cls_prov ?
Do we need this separately for diff RUs? Eg. cls_src, prprty_src,â€¦?"""^^xsd:string .

:old_spr_cls a owl:AnnotationProperty ;
	rdfs:comment "For deleted classes state their last position within the ontology, state the old superclasses."^^xsd:string .

:prpty_id a owl:AnnotationProperty ;
	rdfs:comment "A unique formal identifyer for the property, analogously to the cls_id."^^xsd:string .
