@prefix : <http://www.w3.org/1999/02/22-rdf-syntax-ns#> .
@prefix dc: <http://purl.org/dc/elements/1.1/> .
@prefix irw: <http://www.ontologydesignpatterns.org/ont/web/irw.owl#> .
@prefix foaf: <http://xmlns.com/foaf/0.1/> .
@prefix isicil: <http://ns.inria.fr/isicil#> .
@prefix vann: <http://purl.org/vocab/vann/> .
@prefix scot: <http://scot-project.org/scot/ns#> .
@prefix vs: <http://www.w3.org/2003/06/sw-vocab-status/ns#> .
@prefix nicetag: <http://ns.inria.fr/nicetag/2010/09/09/voc> .
@prefix dcterms: <http://purl.org/dc/terms/> .
@prefix sioc: <http://rdfs.org/sioc/ns#> .
@prefix rdfs: <http://www.w3.org/2000/01/rdf-schema#> .
@prefix ma: <http://www.w3.org/ns/ma-ont> .
@prefix owl: <http://www.w3.org/2002/07/owl#> .
@prefix xsd: <http://www.w3.org/2001/XMLSchema#> .
@prefix ademe: <http://www.ademe.fr/2009/svic-schema.rdfs#> .
@prefix skos: <http://www.w3.org/2004/02/skos/core#> .
@prefix cc: <http://creativecommons.org/ns#> .

<http://ns.inria.fr/s4ac/v1> a owl:Ontology ;
	dc:title "Social Semantic SPARQL Security For Access Control (S4AC) Ontology"@en ;
	dc:description "A vocabulary to describe the access policies which protect an RDF data store."@en ;
	dc:issued "2011-06-28"^^xsd:date ;
	owl:versionInfo "0.1"^^xsd:decimal ;
	cc:license <http://creativecommons.org/licenses/by/3.0/> ;
	dc:publisher <http://dbpedia.org/resource/National_Institute_for_Research_in_Computer_Science_and_Control> .

<http://dbpedia.org/resource/National_Institute_for_Research_in_Computer_Science_and_Control> a foaf:Organization .

<http://ns.inria.fr/s4ac/v1> foaf:page <http://ns.inria.fr/s4ac/v1/s4ac_v1.html> ;
	vann:preferredNamespacePrefix "s4ac" ;
	vann:preferredNamespaceUri "http://ns.inria.fr/s4ac/v1#" .

<http://ns.inria.fr/s4ac/v1#Condition> a owl:Class ;
	rdfs:label "Condition"@en ;
	rdfs:comment "This class is used to manage the AccessCondition, and the ExceptionAccess."@en ;
	rdfs:isDefinedBy <http://ns.inria.fr/s4ac/v1#> .

<http://ns.inria.fr/s4ac/v1#hasSpatialValidity> a owl:ObjectProperty ;
	rdfs:domain <http://ns.inria.fr/s4ac/v1#AccessCondition> ;
	rdfs:range <http://www.w3.org/2003/01/geo/wgs84_pos#SpatialThing> ;
	rdfs:label "hasSpatialValidity"@en ;
	rdfs:comment "The property defines the location constraints under which an AccessCondition is valid."@en ;
	rdfs:isDefinedBy <http://ns.inria.fr/s4ac/v1#> .

<http://ns.inria.fr/s4ac/v1#hasValidity> a owl:ObjectProperty ;
	rdfs:domain <http://ns.inria.fr/s4ac/v1#AccessCondition> ;
	rdfs:range <http://www.w3.org/2006/time#TemporalEntity> ;
	rdfs:label "hasValidity"@en ;
	rdfs:comment "The property defines the temporal constraints under which an AccessCondition is valid. The validity can be expressed as a specific date, or as a time interval."@en ;
	rdfs:isDefinedBy <http://ns.inria.fr/s4ac/v1#> .

<http://ns.inria.fr/s4ac/v1#hasParameter> a owl:ObjectProperty ;
	rdfs:domain <http://ns.inria.fr/s4ac/v1#AccessCondition> ;
	rdfs:range <http://ns.inria.fr/s4ac/v1#Variable> ;
	rdfs:label "hasParameter"@en ;
	rdfs:comment "The property defines the variables used in the Access Condition, and a comment explaining their use."@en ;
	rdfs:isDefinedBy <http://ns.inria.fr/s4ac/v1#> .

<http://ns.inria.fr/s4ac/v1#Variable> a owl:Class ;
	rdfs:label "Variable"@en ;
	rdfs:comment "This class is used to describe the variables used in the Access Condition."@en ;
	rdfs:isDefinedBy <http://ns.inria.fr/s4ac/v1#> .

<http://ns.inria.fr/s4ac/v1#hasComment> a owl:ObjectProperty ;
	rdfs:domain <http://ns.inria.fr/s4ac/v1#Variable> ;
	rdfs:range rdfs:Literal ;
	rdfs:label "hasComment"@en ;
	rdfs:comment "This property associates a comment to the variable used in the Access Condition to explain their use in the definition of the policies."@en ;
	rdfs:isDefinedBy <http://ns.inria.fr/s4ac/v1#> .

<http://ns.inria.fr/s4ac/v1#hasName> a owl:ObjectProperty ;
	rdfs:domain <http://ns.inria.fr/s4ac/v1#Variable> ;
	rdfs:range rdfs:Literal ;
	rdfs:label "hasValue"@en ;
	rdfs:comment "This property associates a name to the variable used in the Access Condition."@en ;
	rdfs:isDefinedBy <http://ns.inria.fr/s4ac/v1#> .

<http://ns.inria.fr/s4ac/v1#AccessPrivilege> a owl:Class ;
	rdfs:label "AccessPrivilege"@en ;
	rdfs:comment "This class represents the kind of access privileges which is granted to the user (Create, Read, Update, Delete)."@en ;
	rdfs:isDefinedBy <http://ns.inria.fr/s4ac/v1#> .

<http://ns.inria.fr/s4ac/v1#hasAccessPrivilege> a owl:ObjectProperty ;
	rdfs:domain <http://ns.inria.fr/s4ac/v1#AccessTaggingRule> ;
	rdfs:range <http://ns.inria.fr/s4ac/v1#AccessPrivilege> ;
	rdfs:label "hasAccessPrivilege"@en ;
	rdfs:comment "This property adds the access privileges to the access tagging rules."@en ;
	rdfs:isDefinedBy <http://ns.inria.fr/s4ac/v1#> .

<http://ns.inria.fr/s4ac/v1#hasPriorityOn> a owl:ObjectProperty ;
	rdfs:domain <http://ns.inria.fr/s4ac/v1#AccessPrivilege> ;
	rdfs:range <http://ns.inria.fr/s4ac/v1#AccessPrivilege> ;
	rdfs:label "hasPriorityOn"@en ;
	rdfs:comment "This property represents the pre-order among the access privileges."@en .

<http://ns.inria.fr/s4ac/v1#Create> a owl:Class ;
	owl:equivalentClass <http://www.w3.org/ns/auth/acl#Append> ;
	rdfs:subClassOf <http://ns.inria.fr/s4ac/v1#AccessPrivilege> ;
	rdfs:label "Create"@en ;
	rdfs:comment "This class represents a create access on the resource. This class is equivalent to acl:Append."@en ;
	rdfs:isDefinedBy <http://ns.inria.fr/s4ac/v1#> .

<http://ns.inria.fr/s4ac/v1#Read> a owl:Class ;
	owl:equivalentClass <http://www.w3.org/ns/auth/acl#Read> ;
	rdfs:subClassOf <http://ns.inria.fr/s4ac/v1#AccessPrivilege> ;
	rdfs:label "Read"@en ;
	rdfs:comment "This class represents a read access on the resource. This class is equivalent to acl:Read."@en ;
	rdfs:isDefinedBy <http://ns.inria.fr/s4ac/v1#> .

<http://ns.inria.fr/s4ac/v1#Update> a owl:Class ;
	rdfs:subClassOf <http://ns.inria.fr/s4ac/v1#AccessPrivilege> ;
	rdfs:label "Update"@en ;
	rdfs:comment "This class represents an update access on the resource."@en ;
	rdfs:isDefinedBy <http://ns.inria.fr/s4ac/v1#> .

<http://ns.inria.fr/s4ac/v1#Delete> a owl:Class ;
	rdfs:subClassOf <http://ns.inria.fr/s4ac/v1#AccessPrivilege> ;
	rdfs:label "Delete"@en ;
	rdfs:comment "This class represents a delete access on the resource."@en ;
	rdfs:isDefinedBy <http://ns.inria.fr/s4ac/v1#> .

<http://ns.inria.fr/s4ac/v1#AccessCondition> a owl:Class ;
	rdfs:subClassOf <http://ns.inria.fr/s4ac/v1#Condition> ;
	rdfs:label "AccessCondition"@en ;
	rdfs:comment "The AC allows the users to access specific resources. An Access Condition (AC) is a SPARQL 1.1 ASK query. If a solution exists, the ASK query returns true, and the AC is said to be verified. If no solution exists, the ASK query returns false, and the AC is said not to be verified."@en ;
	rdfs:isDefinedBy <http://ns.inria.fr/s4ac/v1#> .

<http://ns.inria.fr/s4ac/v1#hasCategoryLabel> a owl:ObjectProperty ;
	rdfs:domain <http://ns.inria.fr/s4ac/v1#AccessCondition> ;
	rdfs:range skos:prefLabel ;
	rdfs:label "hasCategoryLabel"@en ;
	rdfs:comment "This property is used to add a label in natural language to the AccessCondition."@en ;
	rdfs:isDefinedBy <http://ns.inria.fr/s4ac/v1#> .

<http://ns.inria.fr/s4ac/v1#AccessConditionSet> a owl:Class ;
	rdfs:subClassOf <http://ns.inria.fr/s4ac/v1#Condition> ;
	rdfs:label "AccessConditionSet"@en ;
	rdfs:comment "An Access Condition Set (ACS) represents a set of Access Conditions which can be either Conjunctive or Disjunctive."@en ;
	rdfs:isDefinedBy <http://ns.inria.fr/s4ac/v1#> .

<http://ns.inria.fr/s4ac/v1#DisjunctiveAccessConditionSet> a owl:Class ;
	rdfs:subClassOf <http://ns.inria.fr/s4ac/v1#AccessConditionSet> ;
	owl:disjointWith <http://ns.inria.fr/s4ac/v1#ConjunctiveAccessConditionSet> ;
	rdfs:label "DisjontiveAccessConditionSet"@en ;
	rdfs:comment ": A Disjunctive ACS (DACS) is a logical disjunction of Access Conditions, and it is said to be verified if and only if at least one Access Condition it contains is verified."@en ;
	rdfs:isDefinedBy <http://ns.inria.fr/s4ac/v1#> .

<http://ns.inria.fr/s4ac/v1#ConjunctiveAccessConditionSet> a owl:Class ;
	rdfs:subClassOf <http://ns.inria.fr/s4ac/v1#AccessConditionSet> ;
	owl:disjointWith <http://ns.inria.fr/s4ac/v1#DisjunctiveAccessConditionSet> ;
	rdfs:label "ConjontiveAccessConditionSet"@en ;
	rdfs:comment "A Conjunctive ACS (CACS) is a logical conjunction of Access Conditions, and it is said to be verified if and only if every Access Condition it contains is verified."@en ;
	rdfs:isDefinedBy <http://ns.inria.fr/s4ac/v1#> .

<http://ns.inria.fr/s4ac/v1#hasAccessCondition> a owl:ObjectProperty ;
	owl:inverseOf <http://ns.inria.fr/s4ac/isAccessConditionOf> .

<http://ns.inria.fr/s4ac/isAccessConditionOf> a owl:ObjectProperty .

<http://ns.inria.fr/s4ac/v1#hasAccessCondition> rdfs:domain <http://ns.inria.fr/s4ac/v1#AccessConditionSet> ;
	rdfs:range <http://ns.inria.fr/s4ac/v1#AccessCondition> ;
	rdfs:label "hasAccessCondition"@en ;
	rdfs:comment "This property adds an Access Condition to an Access Condition Set."@en ;
	rdfs:isDefinedBy <http://ns.inria.fr/s4ac/v1#> .

<http://ns.inria.fr/s4ac/v1#isAccessConditionOf> a owl:ObjectProperty ;
	owl:inverseOf <http://ns.inria.fr/s4ac/hasAccessCondition> .

<http://ns.inria.fr/s4ac/hasAccessCondition> a owl:ObjectProperty .

<http://ns.inria.fr/s4ac/v1#isAccessConditionOf> rdfs:domain <http://ns.inria.fr/s4ac/v1#AccessCondition> ;
	rdfs:range <http://ns.inria.fr/s4ac/v1#AccessConditionSet> ;
	rdfs:label "isAccessConditionOf"@en ;
	rdfs:comment "This property says that an Access Condition is part of an Access Condition Set."@en ;
	rdfs:isDefinedBy <http://ns.inria.fr/s4ac/v1#> .

<http://ns.inria.fr/s4ac/v1#AccessTag> a owl:Class ;
	rdfs:subClassOf scot:Tag ;
	rdfs:label "TagSet"@en ;
	rdfs:comment "This class is used to define the set of tags such that the Access Conditions apply to any resource tagged with one or more tags form AccessTag."@en ;
	rdfs:isDefinedBy <http://ns.inria.fr/s4ac/v1#> .

<http://ns.inria.fr/s4ac/v1#scopedBy> a owl:ObjectProperty ;
	rdfs:domain <http://ns.inria.fr/s4ac/v1#AccessConditionSet> ;
	rdfs:range <http://ns.inria.fr/s4ac/v1#AccessTag> ;
	owl:inverseOf <http://ns.inria.fr/s4ac/scopes> .

<http://ns.inria.fr/s4ac/scopes> a owl:ObjectProperty .

<http://ns.inria.fr/s4ac/v1#scopedBy> rdfs:label "scopedBy"@en ;
	rdfs:comment "This property defines when an Access Condition Set is scoped by a tag."@en ;
	rdfs:isDefinedBy <http://ns.inria.fr/s4ac/v1#> .

<http://ns.inria.fr/s4ac/v1#scopes> a owl:ObjectProperty ;
	rdfs:domain <http://ns.inria.fr/s4ac/v1#AccessTag> ;
	rdfs:range <http://ns.inria.fr/s4ac/v1#AccessConditionSet> ;
	owl:inverseOf <http://ns.inria.fr/s4ac/scopedBy> .

<http://ns.inria.fr/s4ac/scopedBy> a owl:ObjectProperty .

<http://ns.inria.fr/s4ac/v1#scopes> rdfs:label "scopes"@en ;
	rdfs:comment "This property defines when a tag scopes an Access Condition Set."@en ;
	rdfs:isDefinedBy <http://ns.inria.fr/s4ac/v1#> .

<http://ns.inria.fr/s4ac/v1#hasQueryAsk> a owl:ObjectProperty ;
	rdfs:domain <http://ns.inria.fr/s4ac/v1#AccessCondition> ;
	rdfs:range rdfs:Literal ;
	rdfs:label "SPARQL 1.1 ASK query"@en ;
	rdfs:comment "This property defines the SPARQL 1.1 ASK queries of the Access Conditions."@en ;
	rdfs:isDefinedBy <http://ns.inria.fr/s4ac/v1#> .

<http://ns.inria.fr/s4ac/v1#ExceptionAccess> a owl:Class ;
	rdfs:subClassOf <http://ns.inria.fr/s4ac/v1#AccessCondition> , _:node17aev3fskx1 .

_:node17aev3fskx1 a owl:Restriction ;
	owl:onProperty <http://ns.inria.fr/s4ac/v1#isAccessConditionOf> ;
	owl:allValuesFrom <http://ns.inria.fr/s4ac/v1#ConjunctiveAccessConditionSet> .

<http://ns.inria.fr/s4ac/v1#ExceptionAccess> rdfs:label "ExceptionAccess"@en ;
	rdfs:comment "This class is used to forbid or authorize a specific user to access a resource."@en ;
	rdfs:isDefinedBy <http://ns.inria.fr/s4ac/v1#> .

<http://ns.inria.fr/s4ac/v1#PositiveExceptionAccess> a owl:Class ;
	rdfs:subClassOf <http://ns.inria.fr/s4ac/v1#ExceptionAccess> ;
	rdfs:label "PositiveExceptionAccess"@en ;
	rdfs:comment "This class is used to add an exception to an Access Condition Set, in order to authorize a specific user to access."@en ;
	rdfs:isDefinedBy <http://ns.inria.fr/s4ac/v1#> .

<http://ns.inria.fr/s4ac/v1#NegativeExceptionAccess> a owl:Class ;
	rdfs:subClassOf <http://ns.inria.fr/s4ac/v1#ExceptionAccess> ;
	rdfs:label "NegativeExceptionAccess"@en ;
	rdfs:comment "This class is used to add an exception to an Access Condition Set, in order to unauthorize a specific user to access."@en ;
	rdfs:isDefinedBy <http://ns.inria.fr/s4ac/v1#> .

<http://ns.inria.fr/s4ac/v1#hasNegativeException> a owl:ObjectProperty ;
	rdfs:domain <http://ns.inria.fr/s4ac/v1#AccessConditionSet> ;
	rdfs:range <http://ns.inria.fr/s4ac/v1#NegativeExceptionAccess> ;
	rdfs:label "hasNegativeException"@en ;
	rdfs:comment "This property associates an Access Condition Set with a Negative Exception Access."@en ;
	rdfs:isDefinedBy <http://ns.inria.fr/s4ac/v1#> .

<http://ns.inria.fr/s4ac/v1#hasPositiveException> a owl:ObjectProperty ;
	rdfs:domain <http://ns.inria.fr/s4ac/v1#AccessConditionSet> ;
	rdfs:range <http://ns.inria.fr/s4ac/v1#PositiveExceptionAccess> ;
	rdfs:label "hasPositiveException"@en ;
	rdfs:comment "This property associates an Access Condition Set with a Positive Exception Access."@en ;
	rdfs:isDefinedBy <http://ns.inria.fr/s4ac/v1#> .

<http://ns.inria.fr/s4ac/v1#AccessTaggingRule> a owl:Class ;
	rdfs:label "AccessTaggingRule"@en ;
	rdfs:comment "An Access Tagging Rule (ATR) is a triple (ACS, TagSet, Binding) where ACS is an Access Condition Set, TagSet is as set of Access Tags, and Binding is an Access Evaluation Context."@en ;
	rdfs:isDefinedBy <http://ns.inria.fr/s4ac/v1#> .

<http://ns.inria.fr/s4ac/v1#hasAccessConditionSet> a owl:ObjectProperty ;
	rdfs:domain <http://ns.inria.fr/s4ac/v1#AccessTaggingRule> ;
	rdfs:range <http://ns.inria.fr/s4ac/v1#AccessConditionSet> ;
	rdfs:label "hasAccessConditionSet"@en ;
	rdfs:comment "This property defines whether the ACS of an Access Tagging Rule is a Conjunctive ACS, or a Disjunctive ACS."@en ;
	rdfs:isDefinedBy <http://ns.inria.fr/s4ac/v1#> .

<http://ns.inria.fr/s4ac/v1#hasTag> a owl:ObjectProperty ;
	rdfs:domain <http://ns.inria.fr/s4ac/v1#AccessTaggingRule> ;
	rdfs:range <http://ns.inria.fr/s4ac/v1#AccessTag> ;
	rdfs:label "hasTag"@en ;
	rdfs:comment "This property associates an Access Tagging Rule with the set of Access Tags which constrain it."@en ;
	rdfs:isDefinedBy <http://ns.inria.fr/s4ac/v1#> .

<http://ns.inria.fr/s4ac/v1#hasAccessEvaluationContext> a owl:ObjectProperty ;
	rdfs:domain <http://ns.inria.fr/s4ac/v1#AccessTaggingRule> ;
	rdfs:range <http://ns.inria.fr/s4ac/v1#AccessEvaluationContext> ;
	rdfs:label "hasAccessEvaluationContext"@en ;
	rdfs:comment "This property associates an Access Tagging Rule with an Access Evaluation Context."@en ;
	rdfs:isDefinedBy <http://ns.inria.fr/s4ac/v1#> .

<http://ns.inria.fr/s4ac/v1#AccessEvaluationContext> a owl:Class ;
	rdfs:label "AccessEvaluationContext"@en ;
	rdfs:comment "An Access Evaluation Context (AEC) is a list L of predetermined bound variables names of the form (var1, val1) for which a SPARQL 1.1 Binding Clause constrains the ASK query evaluation when verifying the Access Conditions."@en ;
	rdfs:isDefinedBy <http://ns.inria.fr/s4ac/v1#> .

<http://ns.inria.fr/s4ac/v1#hasVariable> a owl:ObjectProperty ;
	rdfs:domain <http://ns.inria.fr/s4ac/v1#AccessEvaluationContext> ;
	rdfs:range rdfs:Literal ;
	rdfs:label "hasVariable"@en ;
	rdfs:comment "This property associates a name of the variable used in the SPARQL 1.1 Bindings to an Access Evaluation Context."@en ;
	rdfs:isDefinedBy <http://ns.inria.fr/s4ac/v1#> .

<http://ns.inria.fr/s4ac/v1#hasValue> a owl:ObjectProperty ;
	rdfs:domain <http://ns.inria.fr/s4ac/v1#AccessEvaluationContext> ;
	rdfs:range rdfs:Literal ;
	rdfs:label "hasValue"@en ;
	rdfs:comment "This property associates the value associated to the variable used in the SPARQL 1.1 Bindings to an Access Evaluation Context."@en ;
	rdfs:isDefinedBy <http://ns.inria.fr/s4ac/v1#> .

<http://ns.inria.fr/s4ac/v1#MaxResource> a owl:Class ;
	rdfs:label "MaxResource"@en ;
	rdfs:comment "This class defines a maximum number of accesses on one or more resources."@en ;
	rdfs:isDefinedBy <http://ns.inria.fr/s4ac/v1#> .

<http://ns.inria.fr/s4ac/v1#hasMaxResource> a owl:ObjectProperty ;
	rdfs:domain <http://ns.inria.fr/s4ac/v1#MaxResource> ;
	rdfs:range rdfs:Literal ;
	rdfs:label "hasMaxResource"@en ;
	rdfs:comment "This property provides the number of times a user can consult one or all the resources."@en ;
	rdfs:isDefinedBy <http://ns.inria.fr/s4ac/v1#> .

<http://ns.inria.fr/s4ac/v1#maxOnResource> a owl:ObjectProperty ;
	rdfs:domain <http://ns.inria.fr/s4ac/v1#MaxResource> ;
	rdfs:label "MaxResource for one resource"@en ;
	rdfs:comment "This property is used to precise which resource is accessible by a limited number of accesses."@en ;
	rdfs:isDefinedBy <http://ns.inria.fr/s4ac/v1#> .

<http://ns.inria.fr/s4ac/v1#ExceptionAccess> rdfs:subClassOf _:node17aev3fskx2 .

_:node17aev3fskx2 a owl:Restriction ;
	owl:onProperty <http://ns.inria.fr/s4ac/v1#isAccessConditionOf> ;
	owl:allValuesFrom <http://ns.inria.fr/s4ac/v1#ConjunctiveAccessConditionSet> .
