@prefix dc: <http://purl.org/dc/elements/1.1/> .
@prefix adms: <http://www.w3.org/ns/adms#> .
@prefix : <http://www.ics.forth.gr/isl/VoIDWarehouse/VoID_Extension_Schema.owl> .
@prefix rdfs: <http://www.w3.org/2000/01/rdf-schema#> .
@prefix ns: <http://www.w3.org/2003/06/sw-vocab-status/ns#> .
@prefix foaf: <http://xmlns.com/foaf/0.1/> .
@prefix terms: <http://purl.org/dc/terms/> .
@prefix xsd: <http://www.w3.org/2001/XMLSchema#> .
@prefix owl: <http://www.w3.org/2002/07/owl#> .
@prefix rdf: <http://www.w3.org/1999/02/22-rdf-syntax-ns#> .

<http://www.ics.forth.gr/isl/VoIDWarehouse/VoID_Extension_Schema.owl> a owl:Ontology ;
	owl:versionInfo "1.0"^^xsd:decimal ;
	terms:issued "2014-05-21"^^xsd:date ;
	terms:creator "Carlo Allocca" ;
	terms:contributor "Carlo Allocca" , "Michalis Mountantonakis" , "Christina Lantzaki" ;
	terms:description "An extension of W3C VoID that is able to represent these metrics for expressing the Connectivity Metrics of a Semantic Warehouse." ;
	terms:creator "Nikos Minadakis" ;
	terms:title "Void Warehouse Ontology" ;
	terms:creator "Michalis Mountantonakis" ;
	terms:rights "Copyright Â© FORTH ICS" ;
	terms:contributor "Nikos Minadakis" ;
	terms:creator "Christina Lantzaki" ;
	terms:license <http://creativecommons.org/licenses/by/3.0/> ;
	terms:creator <http://users.ics.forth.gr/~fafalios/> ;
	terms:contributor <http://users.ics.forth.gr/~fafalios/> ;
	terms:creator <http://users.ics.forth.gr/~marketak/pages/aboutme.html> ;
	terms:contributor <http://users.ics.forth.gr/~marketak/pages/aboutme.html> , <http://users.ics.forth.gr/~tzitzik/> ;
	terms:creator <http://users.ics.forth.gr/~tzitzik/> ;
	terms:publisher <http://www.ics.forth.gr/isl> .

dc:publisher a owl:AnnotationProperty .

ns:term_status a owl:AnnotationProperty .

terms:hasVersion a owl:AnnotationProperty .

dc:description a owl:AnnotationProperty .

terms:modified a owl:AnnotationProperty .

terms:requires a owl:AnnotationProperty .

dc:language a owl:AnnotationProperty .

dc:type a owl:AnnotationProperty .

terms:issued a owl:AnnotationProperty .

dc:source a owl:AnnotationProperty .

terms:isReferencedBy a owl:AnnotationProperty .

adms:status a owl:AnnotationProperty .

dc:title a owl:AnnotationProperty .

<http://www.ics.forth.gr/isl/VoIDWarehouse/VoID_Extension_Schema.owl#accordingTo> a owl:ObjectProperty ;
	rdfs:label "according To" ;
	rdfs:comment "A measurement is carried out by an agent using a specific metric accordingTo one (or more) configurations over one (or more) datasets. Therefore, this property links an instance of measurement class with an instance of configuation class." ;
	rdfs:isDefinedBy "http://www.ics.forth.gr/isl/VoIDWarehouse/v1/voidwarehouse.owl" ;
	ns:term_status "Stable" ;
	rdfs:range <http://www.ics.forth.gr/isl/VoIDWarehouse/VoID_Extension_Schema.owl#Configuration> ;
	rdfs:domain <http://www.ics.forth.gr/isl/VoIDWarehouse/VoID_Extension_Schema.owl#Measurement> .

<http://www.ics.forth.gr/isl/VoIDWarehouse/VoID_Extension_Schema.owl#carriedOutBy> a owl:ObjectProperty ;
	rdfs:isDefinedBy "http://www.ics.forth.gr/isl/VoIDWarehouse/v1/voidwarehouse.owl" ;
	rdfs:comment """A measurement is carried out by an agent using a specific metric according to one (or more) configurations over one (or more) datasets (atomic or composite) and produces a value (i.e. literal).
Therefore, this property links an instance of measurement class with an instance of the Agent class.""" ;
	ns:term_status "Stable" ;
	rdfs:range terms:Agent ;
	rdfs:domain <http://www.ics.forth.gr/isl/VoIDWarehouse/VoID_Extension_Schema.owl#Measurement> .

<http://www.ics.forth.gr/isl/VoIDWarehouse/VoID_Extension_Schema.owl#over> a owl:ObjectProperty ;
	rdfs:label "over" ;
	ns:term_status "Stable" ;
	rdfs:comment "A measurement is carried out by an agent using a specific metric according to one (or more) configurations over one (or more) datasets (atomic or composite) and produces a value (i.e. literal). Therefore, this property links instances of Measurement class with instances of dataset class." ;
	rdfs:isDefinedBy "http://www.ics.forth.gr/isl/VoIDWarehouse/v1/voidwarehouse.owl" ;
	rdfs:range <http://rdfs.org/ns/void#Dataset> ;
	rdfs:domain <http://www.ics.forth.gr/isl/VoIDWarehouse/VoID_Extension_Schema.owl#Measurement> .

<http://www.ics.forth.gr/isl/VoIDWarehouse/VoID_Extension_Schema.owl#usesMetrics> a owl:ObjectProperty ;
	rdfs:label "uses Metrics" ;
	ns:term_status "Stable" ;
	rdfs:comment "A measurement is carried out by an agent using a specific metric according to one (or more) configurations over one (or more) datasets. Therefore, this property links an instance of measurement class with an instance of metrics class." ;
	rdfs:isDefinedBy "http://www.ics.forth.gr/isl/VoIDWarehouse/v1/voidwarehouse.owl" ;
	rdfs:domain <http://www.ics.forth.gr/isl/VoIDWarehouse/VoID_Extension_Schema.owl#Measurement> ;
	rdfs:range <http://www.ics.forth.gr/isl/VoIDWarehouse/VoID_Extension_Schema.owl#Metrics> .

rdfs:isDefinedBy a owl:ObjectProperty ;
	rdfs:domain <http://www.ics.forth.gr/isl/VoIDWarehouse/VoID_Extension_Schema.owl#Configuration> , <http://www.ics.forth.gr/isl/VoIDWarehouse/VoID_Extension_Schema.owl#Measurement> ;
	rdfs:range rdf:resource .

<http://www.ics.forth.gr/isl/VoIDWarehouse/VoID_Extension_Schema.owl#producesValue> a owl:DatatypeProperty ;
	rdfs:label "produces Value" ;
	rdfs:isDefinedBy "http://www.ics.forth.gr/isl/VoIDWarehouse/v1/voidwarehouse.owl" ;
	ns:term_status "Stable" ;
	rdfs:comment "A measurement is carried out by an agent using a specific metric according to one (or more) configurations over one (or more) datasets. Therefore, this property indicates the value produced by the measurement." ;
	rdfs:domain <http://www.ics.forth.gr/isl/VoIDWarehouse/VoID_Extension_Schema.owl#Measurement> ;
	rdfs:range rdfs:Literal .

<http://www.ics.forth.gr/isl/VoIDWarehouse/VoID_Extension_Schema.owl#usesSPARQLquery> a owl:DatatypeProperty ;
	rdfs:label "uses SPARQL query" ;
	ns:term_status "Stable" ;
	rdfs:comment "This property specifies the entities of interest involved in a configuration by providing a SPARQL query that returns them." ;
	rdfs:isDefinedBy "http://www.ics.forth.gr/isl/VoIDWarehouse/v1/voidwarehouse.owl" ;
	rdfs:domain <http://www.ics.forth.gr/isl/VoIDWarehouse/VoID_Extension_Schema.owl#EntityConfiguration> ;
	rdfs:range rdfs:Literal .

<http://purl.org/dc/dcmitype/Collection> a owl:Class ;
	rdfs:label "Collection"@en-us ;
	terms:issued "2000-07-11" ;
	rdfs:comment """A collection is an aggregation of items. The term 
		collection means that the resource is described as a 
		group; its parts may be separately described and navigated."""@en-us ;
	dc:type <http://dublincore.org/usage/documents/principles/#vocabulary-term> ;
	terms:hasVersion <http://dublincore.org/usage/terms/history/#Collection-001> .

<http://purl.org/dc/dcmitype/Dataset> a owl:Class ;
	rdfs:label "Dataset"@en-us ;
	terms:issued "2000-07-11" ;
	rdfs:comment """A dataset is information encoded in a defined structure 
		(for example, lists, tables, and databases), intended to 
		be useful for direct machine processing."""@en-us ;
	dc:type <http://dublincore.org/usage/documents/principles/#vocabulary-term> ;
	terms:hasVersion <http://dublincore.org/usage/terms/history/#Dataset-001> .

<http://purl.org/dc/dcmitype/Event> a owl:Class ;
	rdfs:label "Event"@en-us ;
	terms:issued "2000-07-11" ;
	rdfs:comment """An event is a non-persistent, time-based occurrence. 
		Metadata for an event provides descriptive
		information that is the basis for discovery of the
		purpose, location, duration, responsible agents, and
		links to related events and resources.  The resource
		of type event may not be retrievable if the described
		instantiation has expired or is yet to occur.
		Examples - exhibition, web-cast, conference,
		workshop, open-day, performance, battle, trial,
		wedding, tea-party, conflagration."""@en-us ;
	dc:type <http://dublincore.org/usage/documents/principles/#vocabulary-term> ;
	terms:hasVersion <http://dublincore.org/usage/terms/history/#Event-001> .

<http://purl.org/dc/dcmitype/Image> a owl:Class ;
	rdfs:label "Image"@en-us ;
	terms:issued "2000-07-11" ;
	rdfs:comment """An image is a primarily symbolic visual representation 
		other than text. For example - images and photographs of 
		physical objects, paintings, prints, drawings, other 
		images and graphics, animations and moving pictures, 
		film, diagrams, maps, musical notation. Note that image 
		may include both electronic and physical representations."""@en-us ;
	dc:type <http://dublincore.org/usage/documents/principles/#vocabulary-term> ;
	terms:hasVersion <http://dublincore.org/usage/terms/history/#Image-002> .

<http://purl.org/dc/dcmitype/InteractiveResource> a owl:Class ;
	rdfs:label "Interactive Resource"@en-us ;
	terms:issued "2000-07-11" ;
	rdfs:comment """An interactive resource is a resource which requires 
		interaction from the user to be understood, executed, 
		or experienced. For example - forms on web pages, applets, 
		multimedia learning objects, chat services, virtual 
		reality."""@en-us ;
	dc:type <http://dublincore.org/usage/documents/principles/#vocabulary-term> ;
	terms:hasVersion <http://dublincore.org/usage/terms/history/#InteractiveResource-001> .

<http://purl.org/dc/dcmitype/MovingImage> a owl:Class ;
	rdfs:label "Moving Image"@en-us ;
	rdfs:subClassOf <http://purl.org/dc/dcmitype/Image> ;
	terms:issued "2003-11-18" ;
	rdfs:comment """A series of visual representations that,
        when shown in succession, impart an impression
        of motion.  Examples of moving images are:
        animations, movies, television programs,
        videos, zoetropes, or visual output from
        a simulation."""@en-us ;
	dc:type <http://dublincore.org/usage/documents/principles/#vocabulary-term> ;
	terms:hasVersion <http://dublincore.org/usage/terms/history/#MovingImage-001> .

<http://purl.org/dc/dcmitype/PhysicalObject> a owl:Class ;
	rdfs:label "Physical Object"@en-us ;
	terms:issued "2002-07-13" ;
	rdfs:comment """An inanimate, three-dimensional object or substance.  
		For example -- a computer, the great pyramid, a 
		sculpture.  Note that digital representations 
		of, or surrogates for, these things should use Image, 
		Text or one of the other types."""@en-us ;
	dc:type <http://dublincore.org/usage/documents/principles/#vocabulary-term> ;
	terms:hasVersion <http://dublincore.org/usage/terms/history/#PhysicalObject-001> .

<http://purl.org/dc/dcmitype/Service> a owl:Class ;
	rdfs:label "Service"@en-us ;
	terms:issued "2000-07-11" ;
	rdfs:comment """A service is a system that provides one or more 
		functions of value to the end-user. Examples include: 
		a photocopying service, a banking service, an 
		authentication service, interlibrary loans, a Z39.50 
		or Web server."""@en-us ;
	dc:type <http://dublincore.org/usage/documents/principles/#vocabulary-term> ;
	terms:hasVersion <http://dublincore.org/usage/terms/history/#Service-001> .

<http://purl.org/dc/dcmitype/Software> a owl:Class ;
	rdfs:label "Software"@en-us ;
	terms:issued "2000-07-11" ;
	rdfs:comment """Software is a computer program in source or 
		compiled form which may be available for installation 
		non-transiently on another machine. For software which 
		exists only to create an interactive environment, use 
		interactive instead."""@en-us ;
	dc:type <http://dublincore.org/usage/documents/principles/#vocabulary-term> ;
	terms:hasVersion <http://dublincore.org/usage/terms/history/#Software-001> .

<http://purl.org/dc/dcmitype/Sound> a owl:Class ;
	rdfs:label "Sound"@en-us ;
	terms:issued "2000-07-11" ;
	rdfs:comment """A sound is a resource whose content is primarily 
		intended to be rendered as audio. For example - a 
		music playback file format, an audio compact disc, 
		and recorded speech or sounds."""@en-us ;
	dc:type <http://dublincore.org/usage/documents/principles/#vocabulary-term> ;
	terms:hasVersion <http://dublincore.org/usage/terms/history/#Sound-001> .

<http://purl.org/dc/dcmitype/StillImage> a owl:Class ;
	rdfs:label "Still Image"@en-us ;
	rdfs:subClassOf <http://purl.org/dc/dcmitype/Image> ;
	terms:issued "2003-11-18" ;
	rdfs:comment """A static visual representation. Examples of
        still images are: paintings, drawings, graphic designs,
        plans and maps."""@en-us ;
	dc:type <http://dublincore.org/usage/documents/principles/#vocabulary-term> ;
	terms:hasVersion <http://dublincore.org/usage/terms/history/#StillImage-001> .

<http://purl.org/dc/dcmitype/Text> a owl:Class ;
	rdfs:label "Text"@en-us ;
	terms:issued "2000-07-11" ;
	rdfs:comment """A text is a resource whose content is primarily 
		words for reading. For example - books, letters, 
		dissertations, poems, newspapers, articles, 
		archives of mailing lists. Note that facsimiles 
		or images of texts are still of the genre text."""@en-us ;
	dc:type <http://dublincore.org/usage/documents/principles/#vocabulary-term> ;
	terms:hasVersion <http://dublincore.org/usage/terms/history/#Text-001> .

terms:Agent a owl:Class .

terms:DCMIType a owl:Class ;
	terms:issued "2000-07-11" ;
	dc:description """The DCMI Type Vocabulary provides a general, cross-domain list of
	    approved terms that may be used as values for the Resource Type
	    element to identify the genre of a resource.""" .

terms:TypeScheme a owl:Class .

<http://rdfs.org/ns/void#Dataset> a owl:Class .

<http://www.ics.forth.gr/isl/VoIDWarehouse/VoID_Extension_Schema.owl#Configuration> a owl:Class ;
	rdfs:label "Configuration"^^xsd:string ;
	ns:term_status "Stable"^^xsd:string ;
	rdfs:comment "Based on the fact that a measurement is carried out by an agent using a specific metric according to one (or more) configurations over one (or more) datasets (atomic or composite) and produces a value (i.e. literal). The Configuration defines the polices with respect to a measurement is carried out. It defines polices about how to compare URIs and the configuration of an entity." ;
	rdfs:isDefinedBy "http://www.ics.forth.gr/isl/VoIDWarehouse/v1/voidwarehouse.owl" .

<http://www.ics.forth.gr/isl/VoIDWarehouse/VoID_Extension_Schema.owl#EntityConfiguration> a owl:Class ;
	rdfs:label "Entity Configuration" ;
	rdfs:subClassOf <http://www.ics.forth.gr/isl/VoIDWarehouse/VoID_Extension_Schema.owl#Configuration> ;
	rdfs:comment "The notion of Configuration concerns issues that explain how the measurement was done. At this point, and for the requirements at hand, we need two subclasses: the first concerns the way URI equivalence is defined (see URIEquivalence class), while the second (the EntityConfiguration class) concerns how the entities of interest are defined. Regarding the latter the current modeling allows someone to specify the desired set of entities by providing a SPARQL query that returns them." ;
	ns:term_status "Stable" ;
	rdfs:isDefinedBy "http://www.ics.forth.gr/isl/VoIDWarehouse/v1/voidwarehouse.owl" .

<http://www.ics.forth.gr/isl/VoIDWarehouse/VoID_Extension_Schema.owl#Measurement> a owl:Class ;
	rdfs:label "Measurement" ;
	rdfs:subClassOf <http://purl.org/dc/dcmitype/Event> , _:node18rr3ageox1 .

_:node18rr3ageox1 a owl:Restriction ;
	owl:onProperty <http://www.ics.forth.gr/isl/VoIDWarehouse/VoID_Extension_Schema.owl#producesValue> ;
	owl:minCardinality "1"^^xsd:nonNegativeInteger .

<http://www.ics.forth.gr/isl/VoIDWarehouse/VoID_Extension_Schema.owl#Measurement> rdfs:subClassOf _:node18rr3ageox2 .

_:node18rr3ageox2 a owl:Restriction ;
	owl:onProperty <http://www.ics.forth.gr/isl/VoIDWarehouse/VoID_Extension_Schema.owl#over> ;
	owl:onClass <http://rdfs.org/ns/void#Dataset> ;
	owl:minQualifiedCardinality "1"^^xsd:nonNegativeInteger .

<http://www.ics.forth.gr/isl/VoIDWarehouse/VoID_Extension_Schema.owl#Measurement> rdfs:isDefinedBy "http://www.ics.forth.gr/isl/VoIDWarehouse/v1/voidwarehouse.owl" ;
	rdfs:comment "The notion of Measurement is actually a specialization of dc:Event and therefore inherits the property date. A measurement is carried out by an agent using a specific metric according to one (or more) configurations over one (or more) datasets (atomic or composite) and produces a value (i.e. literal)." ;
	adms:status "Stable" .

<http://www.ics.forth.gr/isl/VoIDWarehouse/VoID_Extension_Schema.owl#Metrics> a owl:Class ;
	rdfs:label "Metrics" ;
	ns:term_status "stable" ;
	rdfs:isDefinedBy "http://www.ics.forth.gr/isl/VoIDWarehouse/v1/voidwarehouse.owl" ;
	rdfs:comment "A metric is an individual with a URI and is defined by a resource (e.g. the DOI of the scientific paper that defined that metric)." .

<http://www.ics.forth.gr/isl/VoIDWarehouse/VoID_Extension_Schema.owl#URIEquivalence> a owl:Class ;
	rdfs:label "URI Equivalence" ;
	rdfs:subClassOf <http://www.ics.forth.gr/isl/VoIDWarehouse/VoID_Extension_Schema.owl#Configuration> ;
	rdfs:comment "The notion of Configuration concerns issues that explain how the measurement was done. At this point, and for the requirements at hand, we need two subclasses: the first concerns the way URI equivalence is defined (see URIEquivalence class), while the second (the EntityConfiguration class) concerns how the entities of interest are defined. Regarding the latter the current modeling allows someone to specify the desired set of entities by providing a SPARQL query that returns them." ;
	rdfs:isDefinedBy "http://www.ics.forth.gr/isl/VoIDWarehouse/v1/voidwarehouse.owl" ;
	ns:term_status "Stable" .

rdf:resource a owl:Class .

foaf:Person a owl:Class .

<http://purl.org/dc/dcmitype/> terms:modified "2002-05-22" ;
	terms:issued "2000-07-11" ;
	dc:language "English"@en-us ;
	dc:title "The DCMI Types namespace providing access to its content by means of an RDF Schema"@en-us ;
	dc:publisher "The Dublin Core Metadata Initiative"@en-us ;
	dc:description "The Dublin Core Types namespace provides URIs for the entries of the DCMI Type Vocabulary. Entries are declared using RDF Schema language to support RDF applications. The Schema will be updated according to dc-usage decisions."@en-us ;
	terms:requires <http://dublincore.org/documents/dcmi-type-vocabulary/> ;
	dc:source <http://dublincore.org/documents/dcmi-type-vocabulary/> , <http://dublincore.org/usage/terms/> ;
	terms:requires <http://purl.org/dc/elements/1.1/> ;
	terms:isReferencedBy <http://purl.org/dc/terms/> .

<http://purl.org/dc/dcmitype/Collection> a owl:NamedIndividual , terms:DCMIType ;
	rdfs:isDefinedBy <http://purl.org/dc/dcmitype/> .

<http://purl.org/dc/dcmitype/Dataset> a owl:NamedIndividual , terms:DCMIType ;
	rdfs:isDefinedBy <http://purl.org/dc/dcmitype/> .

<http://purl.org/dc/dcmitype/Event> a owl:NamedIndividual , terms:DCMIType ;
	rdfs:isDefinedBy <http://purl.org/dc/dcmitype/> .

<http://purl.org/dc/dcmitype/Image> a owl:NamedIndividual , terms:DCMIType ;
	rdfs:isDefinedBy <http://purl.org/dc/dcmitype/> .

<http://purl.org/dc/dcmitype/InteractiveResource> a owl:NamedIndividual , terms:DCMIType ;
	rdfs:isDefinedBy <http://purl.org/dc/dcmitype/> .

<http://purl.org/dc/dcmitype/MovingImage> a owl:NamedIndividual , terms:DCMIType ;
	rdfs:isDefinedBy <http://purl.org/dc/dcmitype/> .

<http://purl.org/dc/dcmitype/PhysicalObject> a owl:NamedIndividual , terms:DCMIType ;
	rdfs:isDefinedBy <http://purl.org/dc/dcmitype/> .

<http://purl.org/dc/dcmitype/Service> a owl:NamedIndividual , terms:DCMIType ;
	rdfs:isDefinedBy <http://purl.org/dc/dcmitype/> .

<http://purl.org/dc/dcmitype/Software> a owl:NamedIndividual , terms:DCMIType ;
	rdfs:isDefinedBy <http://purl.org/dc/dcmitype/> .

<http://purl.org/dc/dcmitype/Sound> a owl:NamedIndividual , terms:DCMIType ;
	rdfs:isDefinedBy <http://purl.org/dc/dcmitype/> .

<http://purl.org/dc/dcmitype/StillImage> a owl:NamedIndividual , terms:DCMIType ;
	rdfs:isDefinedBy <http://purl.org/dc/dcmitype/> .

<http://purl.org/dc/dcmitype/Text> a owl:NamedIndividual , terms:DCMIType ;
	rdfs:isDefinedBy <http://purl.org/dc/dcmitype/> .

terms:DCMIType a owl:NamedIndividual , terms:TypeScheme .

<http://users.ics.forth.gr/~fafalios/> a owl:NamedIndividual , foaf:Person .

<http://users.ics.forth.gr/~marketak/pages/aboutme.html> a owl:NamedIndividual , foaf:Person .

<http://users.ics.forth.gr/~tzitzik/> a owl:NamedIndividual , foaf:Person .

<http://www.ics.forth.gr/isl/VoIDWarehouse/VoID_Extension_Schema.owl#EntityMatching> a owl:NamedIndividual , <http://www.ics.forth.gr/isl/VoIDWarehouse/VoID_Extension_Schema.owl#URIEquivalence> .

<http://www.ics.forth.gr/isl/VoIDWarehouse/VoID_Extension_Schema.owl#ExactStringEquality> a owl:NamedIndividual , <http://www.ics.forth.gr/isl/VoIDWarehouse/VoID_Extension_Schema.owl#URIEquivalence> .

<http://www.ics.forth.gr/isl/VoIDWarehouse/VoID_Extension_Schema.owl#averageDegreeIncrement> a owl:NamedIndividual , <http://www.ics.forth.gr/isl/VoIDWarehouse/VoID_Extension_Schema.owl#Metrics> .

<http://www.ics.forth.gr/isl/VoIDWarehouse/VoID_Extension_Schema.owl#commonLiterals> a owl:NamedIndividual , <http://www.ics.forth.gr/isl/VoIDWarehouse/VoID_Extension_Schema.owl#Metrics> .

<http://www.ics.forth.gr/isl/VoIDWarehouse/VoID_Extension_Schema.owl#commonLiteralsPercentage> a owl:NamedIndividual , <http://www.ics.forth.gr/isl/VoIDWarehouse/VoID_Extension_Schema.owl#Metrics> .

<http://www.ics.forth.gr/isl/VoIDWarehouse/VoID_Extension_Schema.owl#commonUris> a owl:NamedIndividual , <http://www.ics.forth.gr/isl/VoIDWarehouse/VoID_Extension_Schema.owl#Metrics> .

<http://www.ics.forth.gr/isl/VoIDWarehouse/VoID_Extension_Schema.owl#commonUrisPercentage> a owl:NamedIndividual , <http://www.ics.forth.gr/isl/VoIDWarehouse/VoID_Extension_Schema.owl#Metrics> .

<http://www.ics.forth.gr/isl/VoIDWarehouse/VoID_Extension_Schema.owl#complementarityFactor> a owl:NamedIndividual , <http://www.ics.forth.gr/isl/VoIDWarehouse/VoID_Extension_Schema.owl#Metrics> .

<http://www.ics.forth.gr/isl/VoIDWarehouse/VoID_Extension_Schema.owl#suffixCanonicalization> a owl:NamedIndividual , <http://www.ics.forth.gr/isl/VoIDWarehouse/VoID_Extension_Schema.owl#URIEquivalence> .

<http://www.ics.forth.gr/isl/VoIDWarehouse/VoID_Extension_Schema.owl#uniqueTriples> a owl:NamedIndividual , <http://www.ics.forth.gr/isl/VoIDWarehouse/VoID_Extension_Schema.owl#Metrics> .

<http://www.ics.forth.gr/isl/VoIDWarehouse/VoID_Extension_Schema.owl#uniqueTriplesPercentage> a owl:NamedIndividual , <http://www.ics.forth.gr/isl/VoIDWarehouse/VoID_Extension_Schema.owl#Metrics> .

<http://www.ics.forth.gr/isl/VoIDWarehouse/VoID_Extension_Schema.owl#Measurement> rdfs:subClassOf _:node18rr3ageox3 .

_:node18rr3ageox3 a owl:Restriction ;
	owl:onProperty <http://www.ics.forth.gr/isl/VoIDWarehouse/VoID_Extension_Schema.owl#producesValue> ;
	owl:minCardinality "1"^^xsd:nonNegativeInteger .

<http://www.ics.forth.gr/isl/VoIDWarehouse/VoID_Extension_Schema.owl#Measurement> rdfs:subClassOf _:node18rr3ageox4 .

_:node18rr3ageox4 a owl:Restriction ;
	owl:onProperty <http://www.ics.forth.gr/isl/VoIDWarehouse/VoID_Extension_Schema.owl#over> ;
	owl:onClass <http://rdfs.org/ns/void#Dataset> ;
	owl:minQualifiedCardinality "1"^^xsd:nonNegativeInteger .
