@prefix :      <http://www.w3.org/2007/05/powder-s#> .
@prefix rdfs:  <http://www.w3.org/2000/01/rdf-schema#> .
@prefix wdrs:  <http://www.w3.org/2007/05/powder-s#> .
@prefix xsd:   <http://www.w3.org/2001/XMLSchema#> .
@prefix owl:   <http://www.w3.org/2002/07/owl#> .
@prefix base:  <http://www.w3.org/2007/05/powder-s#> .
@prefix rdf:   <http://www.w3.org/1999/02/22-rdf-syntax-ns#> .

base:authenticate  a      rdf:Property ;
        rdfs:comment      "A pointer to a document that describes how Description Resources created by a FOAF Agent or a DC Terms Agent may be authenticated"@en ;
        rdfs:isDefinedBy  <http://www.w3.org/TR/powder-dr/#discover> ;
        rdfs:label        "authenticate"@en .

base:issuedby  a          owl:AnnotationProperty , rdf:Property ;
        rdfs:comment      "This property denotes the author of a POWDER document."@en ;
        rdfs:isDefinedBy  <http://www.w3.org/TR/powder-dr/#line3> ;
        rdfs:label        "issued by"@en .

base:sha1sum  a           rdf:Property ;
        rdfs:comment      "Links to a Base64-encoded binary SHA-1 hash of the described resource. May be used by POWDER Processors when assessing trustworthiness of a DR."@en ;
        rdfs:isDefinedBy  <http://www.w3.org/TR/powder-dr/#certification> ;
        rdfs:label        "SHA-1 sum"@en ;
        rdfs:range        xsd:base64Binary .

base:proc_error  a        rdf:Property ;
        rdfs:comment      "A property denoting a description of the specific software error."@en ;
        rdfs:domain       base:Processor ;
        rdfs:isDefinedBy  <http://www.w3.org/TR/powder-dr/#ppErrorhandling> ;
        rdfs:label        "processing error"@en .

base:error_code  a        rdf:Property ;
        rdfs:comment      "A property denoting the code of any error encountered by the POWDER processor."@en ;
        rdfs:isDefinedBy  <http://www.w3.org/TR/powder-dr/#ppErrorhandling> ;
        rdfs:label        "error code"@en ;
        rdfs:range        xsd:nonNegativeInteger .

base:notknownto  a        rdf:Property ;
        rdfs:comment      "Property used in results returned from a POWDER Processor that has no data about the candidate resource. The value is the IRI of the processor."@en ;
        rdfs:isDefinedBy  <http://www.w3.org/TR/powder-dr/#powderprocessor> ;
        rdfs:label        "not known to"@en ;
        rdfs:range        base:Processor .

base:hasIRI  a            owl:DatatypeProperty , rdf:Property ;
        rdfs:comment      "This property is meant to be used in OWL2 instead of wdrs:matchesregex. It denotes the string data range corresponding to a set of IRIs."@en ;
        rdfs:domain       rdfs:Resource ;
        rdfs:isDefinedBy  <http://www.w3.org/TR/powder-formal/#oxRegexSemantics> ;
        rdfs:label        "has IRI"@en ;
        rdfs:range        xsd:anyURI .

base:supportedby  a       owl:AnnotationProperty , rdf:Property ;
        rdfs:comment      "A property that links a POWDER document to some other data source that supports the descriptions provided."@en ;
        rdfs:isDefinedBy  <http://www.w3.org/TR/powder-dr/#supportedBy> ;
        rdfs:label        "supported by"@en .

base:validuntil  a        owl:AnnotationProperty , rdf:Property ;
        rdfs:comment      "Provides a timestamp that a POWDER Processor may use when assessing trustworthiness of a POWDER document. Informally, a POWDER Processor should normally ignore data in the document after the given date."@en ;
        rdfs:isDefinedBy  <http://www.w3.org/TR/powder-dr/#certification> ;
        rdfs:label        "valid until"@en .

base:matchesregex  a      owl:DatatypeProperty , rdf:Property ;
        rdfs:comment      "This is the key 'include' property for IRI set definitions in POWDER-S. It is necessary to take account of the POWDER Semantic Extension to process this fully. The value is a regular expression that is matched against an IRI."@en ;
        rdfs:domain       rdfs:Resource ;
        rdfs:isDefinedBy  <http://www.w3.org/TR/powder-formal/#regexSemantics> ;
        rdfs:label        "matches regular expression"@en ;
        rdfs:range        xsd:string ;
        rdfs:seeAlso      <http://www.w3.org/TR/xpath-functions/#regex-syntax> .

base:certifiedby  a       owl:AnnotationProperty , rdf:Property ;
        rdfs:comment      "A property that links a resource to a POWDER document that certifies it."@en ;
        rdfs:isDefinedBy  <http://www.w3.org/TR/powder-dr/#certification> ;
        rdfs:label        "certified by"@en .

base:logo  a              owl:AnnotationProperty , rdf:Property ;
        rdfs:comment      "Points to a graphic summary for the resources in a given class. Typically, it is a logo denoting conformance of a given (set of) resource(s) to a given set of criteria."@en ;
        rdfs:isDefinedBy  <http://www.w3.org/TR/powder-dr/#line13> ;
        rdfs:label        "logo"@en .

base:text  a              owl:AnnotationProperty , rdf:Property ;
        rdfs:comment      "This property provides a summary of the descriptorset that it annotates, suitable for display to end users."@en ;
        rdfs:isDefinedBy  <http://www.w3.org/TR/powder-dr/#line13> ;
        rdfs:label        "text that may be displayed"@en .

base:data_error  a        rdf:Property ;
        rdfs:comment      "A property denoting a description of the specific error found in a given POWDER document."@en ;
        rdfs:domain       base:Document ;
        rdfs:isDefinedBy  <http://www.w3.org/TR/powder-dr/#ppErrorhandling> ;
        rdfs:label        "data error"@en .

base:tag  a               owl:DatatypeProperty , rdf:Property ;
        rdfs:comment      "Property linking to a free-text tag which may include spaces."@en ;
        rdfs:isDefinedBy  <http://www.w3.org/TR/powder-dr/#tags> ;
        rdfs:label        "tag"@en ;
        rdfs:range        xsd:token .

base:certified  a         rdf:Property ;
        rdfs:comment      "A property that takes a Boolean value to declare whether the author of the data certifies the described resource."@en ;
        rdfs:isDefinedBy  <http://www.w3.org/TR/powder-dr/#certification> ;
        rdfs:label        "certified"@en ;
        rdfs:range        xsd:boolean .

base:notmatchesregex  a   owl:DatatypeProperty , rdf:Property ;
        rdfs:comment      "This is the key 'exclude' property for IRI set definitions in POWDER-S. It is necessary to take account of the POWDER Semantic Extension to process this fully. The value is a regular expression that is matched against an IRI."@en ;
        rdfs:domain       rdfs:Resource ;
        rdfs:isDefinedBy  <http://www.w3.org/TR/powder-formal/#regexSemantics> ;
        rdfs:label        "matches regular expression"@en ;
        rdfs:range        xsd:string ;
        rdfs:seeAlso      <http://www.w3.org/TR/xpath-functions/#regex-syntax> .

base:describedby  a       rdf:Property ;
        rdfs:comment      "An RDF property to exactly match the describedby relationship type introduced in http://www.w3.org/TR/powder-dr/#assoc-linking and formally defined in appendix D of the same document, i.e. the relationship A 'describedby' B asserts that resource B provides a description of resource A. There are no constraints on the format or representation of either A or B, neither are there any further constraints on either resource."@en ;
        rdfs:isDefinedBy  <http://www.w3.org/TR/powder-dr/#semlink> ;
        rdfs:label        "described by"@en .

base:Document  a          rdfs:Class ;
        rdfs:comment      "A POWDER document."@en ;
        rdfs:isDefinedBy  <http://www.w3.org/TR/powder-dr/#structure> ;
        rdfs:label        "POWDER document"@en ;
        rdfs:subClassOf   owl:Ontology .

base:Processor  a         rdfs:Class ;
        rdfs:comment      "A software agent able to process POWDER documents."@en ;
        rdfs:isDefinedBy  <http://www.w3.org/TR/powder-dr/#powderprocessor> ;
        rdfs:label        "POWDER processor"@en ;
        rdfs:subClassOf   <http://purl.org/dc/terms/Agent> .

base:validfrom  a         owl:AnnotationProperty , rdf:Property ;
        rdfs:comment      "Provides a timestamp that a POWDER Processor may use when assessing trustworthiness of a POWDER document. Informally, a POWDER Processor should normally ignore data in the document before the given date."@en ;
        rdfs:isDefinedBy  <http://www.w3.org/TR/powder-dr/#certification> ;
        rdfs:label        "valid from"@en .

<http://www.w3.org/2007/05/powder-s>
        a                 owl:Ontology ;
        rdfs:comment      "This file specifies the set of classes and properties used in the RDF/OWL version of POWDER documents." ;
        rdfs:label        "POWDER-S Vocabulary" ;
        owl:priorVersion  <http://www.w3.org/2007/05/powder-s> ;
        owl:versionInfo   "8 November 2010" .
