@prefix dc: <http://purl.org/dc/elements/1.1/> .
@prefix rdfs: <http://www.w3.org/2000/01/rdf-schema#> .
@prefix rev: <http://purl.org/stuff/rev#> .
@prefix foaf: <http://xmlns.com/foaf/0.1/> .
@prefix ao: <http://purl.org/ontology/ao/core#> .
@prefix event: <http://purl.org/NET/c4dm/event.owl#> .
@prefix xsd: <http://www.w3.org/2001/XMLSchema#> .
@prefix owl: <http://www.w3.org/2002/07/owl#> .
@prefix sim: <http://purl.org/ontology/similarity/> .
@prefix rdf: <http://www.w3.org/1999/02/22-rdf-syntax-ns#> .
@prefix vs: <http://www.w3.org/2003/06/sw-vocab-status/ns#> .
@prefix dcterms: <http://purl.org/dc/terms/> .

<http://purl.org/ontology/ao/core#> a owl:Ontology ;
	dc:creator <http://foaf.me/zazi#me> , <http://tobyinkster.co.uk/#i> ;
	dc:date "2010-09-13T13:59:52+01:00"^^xsd:dateTime ;
	dc:description """The Association Ontology specification provides basic properties 
for describing specific associations to something, e.g. a context, an occasion, a genre or a mood, and enables furthermore, a mechanism to 
like/rate and feedback these associations in context to something on/ for the Semantic Web. This document contains a RDF description 
of the Association Ontology."""@en ;
	dc:title "The Association Ontology"@en ;
	owl:imports <http://purl.org/NET/c4dm/event.owl> , <http://purl.org/dc/elements/1.1/> , <http://purl.org/dc/terms/> , <http://purl.org/ontology/similarity/> , <http://purl.org/stuff/rev> , <http://www.w3.org/2003/06/sw-vocab-status/ns> , <http://xmlns.com/foaf/0.1/> ;
	owl:versionInfo "0.4"^^xsd:decimal .

ao:LikeableAssociation a owl:Class ;
	rdfs:comment """A likeable association. That means this association type is intended to be used for voting (ao:likeminded), 
feedbacking (rev:Feedback), reviewing (e.g. rev:rating) an association statement (related by ao:included_association) in the 
context of something."""@en ;
	rdfs:isDefinedBy <http://purl.org/ontology/ao/core#> ;
	rdfs:label "Likeable Association"@en ;
	rdfs:subClassOf sim:Association , rev:Review ;
	vs:term_status "testing"@en .

ao:activity a rdf:Property ;
	rdfs:comment "An activity, which is associated to an individual, e.g. dancing, sleeping, driving."@en ;
	rdfs:isDefinedBy <http://purl.org/ontology/ao/core#> ;
	rdfs:label "has activity"@en ;
	rdfs:subPropertyOf ao:context ;
	vs:term_status "testing"@en .

ao:application a rdf:Property ;
	rdfs:comment "An application, which is associated to an individual, e.g. a music player to a music track it's currently playing back."@en ;
	rdfs:isDefinedBy <http://purl.org/ontology/ao/core#> ;
	rdfs:label "has application"@en ;
	rdfs:subPropertyOf ao:context ;
	vs:term_status "testing"@en .

ao:context a rdf:Property ;
	rdfs:comment "A property to associate any environmental context to an individual, e.g. a location, a time or an activity. Hence, this property is intended that sub properties should be created from it."@en ;
	rdfs:domain owl:Thing ;
	rdfs:isDefinedBy <http://purl.org/ontology/ao/core#> ;
	rdfs:label "has context"@en ;
	vs:term_status "testing"@en .

ao:device a rdf:Property ;
	rdfs:comment "A device, which is associated with an individual, e.g. a CD player with a CD it's currently playing back."@en ;
	rdfs:isDefinedBy <http://purl.org/ontology/ao/core#> ;
	rdfs:label "has device"@en ;
	rdfs:subPropertyOf ao:context ;
	vs:term_status "testing"@en .

ao:genre a rdf:Property ;
	rdfs:comment "An genre of something."@en ;
	rdfs:domain owl:Thing ;
	rdfs:isDefinedBy <http://purl.org/ontology/ao/core#> ;
	rdfs:label "has genre"@en ;
	rdfs:subPropertyOf dcterms:subject ;
	vs:term_status "unstable"@en .

ao:included_association a owl:ObjectProperty ;
	rdfs:comment """This property could be used to compose association statements or to reuse them, e.g. to make them likeable 
in a specific context."""@en ;
	rdfs:domain sim:Association ;
	rdfs:isDefinedBy <http://purl.org/ontology/ao/core#> ;
	rdfs:label "has included association"@en ;
	rdfs:range sim:Association ;
	owl:inverseOf _:node17168lpjtx3 .

_:node17168lpjtx3 a owl:ObjectProperty ;
	rdfs:label "is included association of" .

ao:included_association vs:term_status "testing"@en .

ao:likeminded a owl:ObjectProperty ;
	rdfs:comment "Associates likeminded people to an association, which they like/ agree with."^^xsd:string ;
	rdfs:domain sim:Association ;
	rdfs:isDefinedBy <http://purl.org/ontology/ao/core#> ;
	rdfs:label "has likeminded"^^xsd:string ;
	rdfs:range foaf:Agent ;
	owl:inverseOf _:node17168lpjtx4 .

_:node17168lpjtx4 a owl:ObjectProperty ;
	rdfs:label "is likeminded of" .

ao:likeminded vs:term_status "testing"^^xsd:string .

ao:location a rdf:Property ;
	rdfs:comment "A location, which is associated to an individual, e.g. my house, my country, my current whereabouts."@en ;
	rdfs:isDefinedBy <http://purl.org/ontology/ao/core#> ;
	rdfs:label "has location"@en ;
	rdfs:subPropertyOf ao:context ;
	vs:term_status "testing"@en .

ao:mood a rdf:Property ;
	rdfs:comment "A mood that should be created by something."@en ;
	rdfs:domain owl:Thing ;
	rdfs:isDefinedBy <http://purl.org/ontology/ao/core#> ;
	rdfs:label "has mood"@en ;
	rdfs:subPropertyOf dcterms:subject ;
	vs:term_status "unstable"@en .

ao:occasion a rdf:Property ;
	rdfs:comment "An occasion for which something was created."@en ;
	rdfs:domain owl:Thing ;
	rdfs:isDefinedBy <http://purl.org/ontology/ao/core#> ;
	rdfs:label "has occassion"@en ;
	rdfs:subPropertyOf dcterms:subject ;
	vs:term_status "unstable"@en .

ao:time a rdf:Property ;
	rdfs:comment "A time, which is associated to an individual, e.g. morning, afternoon, evening."@en ;
	rdfs:isDefinedBy <http://purl.org/ontology/ao/core#> ;
	rdfs:label "has time"@en ;
	rdfs:subPropertyOf ao:context ;
	owl:equivalentProperty dc:date ;
	vs:term_status "testing"@en .

ao:used_application a rdf:Property , owl:ObjectProperty ;
	rdfs:comment "An application that is related to an event, e.g. a iTunes to a play back event of a music track."@en ;
	rdfs:isDefinedBy <http://purl.org/ontology/ao/core#> ;
	rdfs:label "has used application"@en ;
	rdfs:subPropertyOf event:factor , ao:application ;
	vs:term_status "unstable"@en .

ao:used_device a rdf:Property , owl:ObjectProperty ;
	rdfs:comment "A device that is related to an event, e.g. a MP3 player to a play back event of a music track."@en ;
	rdfs:isDefinedBy <http://purl.org/ontology/ao/core#> ;
	rdfs:label "has used device"@en ;
	rdfs:subPropertyOf event:factor , ao:device ;
	vs:term_status "unstable"@en .
