@prefix dc:    <http://purl.org/dc/elements/1.1/> .
@prefix :      <http://www.ebusiness-unibw.org/ontologies/consumerelectronics/v1#> .
@prefix rdfs:  <http://www.w3.org/2000/01/rdf-schema#> .
@prefix xsd:   <http://www.w3.org/2001/XMLSchema#> .
@prefix owl:   <http://www.w3.org/2002/07/owl#> .
@prefix rdf:   <http://www.w3.org/1999/02/22-rdf-syntax-ns#> .
@prefix gr:    <http://purl.org/goodrelations/v1#> .

:JVC    a                 gr:BusinessEntity ;
        rdfs:comment      "The business entity Victor Company of Japan, Limited."@en ;
        rdfs:label        "JVC"^^xsd:string ;
        rdfs:seeAlso      <http://jdl.jvc-europe.com/> ;
        gr:legalName      "Victor Company of Japan, limited"^^xsd:string ;
        :belongsToModule  "MP3Player, TV, Camcorder"@en .

:YPbPr  a                 :Connectivity ;
        rdfs:comment      "YPbPR is the analog video signal carried by component video cable in consumer electronics. The green cable carries Y, the blue cable carries PB and the red cable carries PR.\n\n(This description is partly based on or reuses content from the Wikipedia article \"YPbPr\" (http://en.wikipedia.org/wiki/YPbPr) and is licensed under the GNU Free Documentation License (http://www.gnu.org/copyleft/fdl.html).)"@en ;
        rdfs:label        "YPbPr"@en , "YPbPr"@de ;
        :belongsToModule  "TV"@en .

:hasOpticalZoomFactor
        a                   owl:ObjectProperty ;
        rdfs:comment        "Defines the stages an object can be zoomed optically."@en ;
        rdfs:isDefinedBy    <http://www.ebusiness-unibw.org/ontologies/consumerelectronics/v1> ;
        rdfs:label          "optical zoom factor"@en , "optischer Zoomfaktor"@de ;
        rdfs:range          gr:QuantitativeValueFloat ;
        rdfs:subPropertyOf  gr:quantitativeProductOrServiceProperty ;
        :belongsToModule    "DigitalCamera, Camcorder"@en .

:LaserPrinter  a          owl:Class ;
        rdfs:comment      "A laser printer is a common type of computer printer that rapidly produces high quality text and graphics on plain paper.\n\n(This description is partly based on or reuses content from the Wikipedia article \"Laser printer\" (http://en.wikipedia.org/wiki/Laser_printer) and is licensed under the GNU Free Documentation License (http://www.gnu.org/copyleft/fdl.html).)"@en ;
        rdfs:isDefinedBy  <http://www.ebusiness-unibw.org/ontologies/consumerelectronics/v1> ;
        rdfs:label        "Laserdrucker"@de , "Laser printer"@en ;
        rdfs:subClassOf   :Printer ;
        :belongsToModule  "Printer"@en .

:ProcessorType  a         owl:Class ;
        rdfs:comment      "The type of central processing unit (CPU) as an electronic circuit that can execute printing tasks or programs."@en ;
        rdfs:isDefinedBy  <http://www.ebusiness-unibw.org/ontologies/consumerelectronics/v1> ;
        rdfs:label        "Prozessorart"@de , "Processor type"@en ;
        rdfs:subClassOf   gr:QualitativeValue ;
        :belongsToModule  "Printer"@en .

:NTSC   a                 :SignalFormat ;
        rdfs:comment      "NTSC (National Television Standard Conversion) is the analog television system used in most of the Americas, Japan, South Korea, Taiwan, the Philippines, Burma, and some Pacific island nations and territories.\n\n(This description is partly based on or reuses content from the Wikipedia article \"NTSC\" (http://en.wikipedia.org/wiki/NTSC) and is licensed under the GNU Free Documentation License (http://www.gnu.org/copyleft/fdl.html).)"@en ;
        rdfs:label        "NTSC"@de , "NTSC"@en ;
        :belongsToModule  "TV"@en .

:MP3Player  a             owl:Class ;
        rdfs:comment      "Playback equipment for certain data formats, especially audio data. Product is often equipped with some scope of delivery. Especially earphones, booklet, sotwareCD, charger and datacable."@en ;
        rdfs:isDefinedBy  <http://www.ebusiness-unibw.org/ontologies/consumerelectronics/v1> ;
        rdfs:label        "MP3-Player"@de , "MP3-Player"@en ;
        rdfs:subClassOf   gr:ProductOrService ;
        :belongsToModule  "MP3Player"@en .

:Vivitar  a               gr:BusinessEntity ;
        rdfs:comment      "The business entity Vivitar Corporation."@en ;
        rdfs:label        "Vivitar"^^xsd:string ;
        rdfs:seeAlso      <http://www.syntaxbrillian.com/> ;
        gr:legalName      "Vivitar Corporation"^^xsd:string ;
        :belongsToModule  "DigitalCamera"@en .

:LG     a                 gr:BusinessEntity ;
        rdfs:comment      "The business entity LG Group."@en ;
        rdfs:label        "LG"^^xsd:string ;
        rdfs:seeAlso      <http://www.lge.com/> ;
        gr:legalName      "LG Group"^^xsd:string ;
        :belongsToModule  "MP3Player, TV"@en .

:hasDigitalFrequency  a     owl:ObjectProperty ;
        rdfs:comment        "Digital frequency is the analogue for discrete signals as frequency is to continuous signals (Common unit of measurement hertz, HTZ).\n\n(This description is partly based on or reuses content from the Wikipedia article \"Digital frequency\" (http://en.wikipedia.org/wiki/Digital_frequency) and is licensed under the GNU Free Documentation License (http://www.gnu.org/copyleft/fdl.html).)"@en ;
        rdfs:isDefinedBy    <http://www.ebusiness-unibw.org/ontologies/consumerelectronics/v1> ;
        rdfs:label          "digital frequency"@en , "Digitale Frequenz"@de ;
        rdfs:range          gr:QuantitativeValueFloat ;
        rdfs:subPropertyOf  gr:quantitativeProductOrServiceProperty ;
        :belongsToModule    "TV"@en .

:hasOpticalSensorResolution
        a                   owl:ObjectProperty ;
        rdfs:comment        "Describes the ability of an imaging system to resolve detail in the object that is being imaged."@en ;
        rdfs:isDefinedBy    <http://www.ebusiness-unibw.org/ontologies/consumerelectronics/v1> ;
        rdfs:label          "optical sensor resolution"@en , "Auflösung optischer Sensor"@de ;
        rdfs:range          gr:QuantitativeValueFloat ;
        rdfs:subPropertyOf  gr:quantitativeProductOrServiceProperty ;
        :belongsToModule    "Camcorder"@en .

:MP4_Audio  a             :DataFormatAudio ;
        rdfs:comment      "A collection of methods defining compression of audio digital data."@en ;
        rdfs:label        "MP4 Audio"@de , "MP4 Audio"@en ;
        :belongsToModule  "MP3Player, DigitalCamera, Camcorder"@en .

:hasWarmupTime  a           owl:ObjectProperty ;
        rdfs:comment        "Defines the amount of time the device needs to be ready."@en ;
        rdfs:isDefinedBy    <http://www.ebusiness-unibw.org/ontologies/consumerelectronics/v1> ;
        rdfs:label          "warmup time"@en , "Warmlaufzeit"@de ;
        rdfs:range          gr:QuantitativeValueFloat ;
        rdfs:subPropertyOf  gr:quantitativeProductOrServiceProperty ;
        :belongsToModule    "Printer"@en .

:Green  a                 :Color ;
        rdfs:comment      "RGB Value 0,128,0"@en ;
        rdfs:label        "Grün"@de , "Green"@en ;
        :belongsToModule  "MP3Player, TV, Printer, DigitalCamera, Camcorder"@en .

:hasStorageMedia  a         owl:ObjectProperty ;
        rdfs:comment        "Defines the type of storage media the object uses to store data."@en ;
        rdfs:isDefinedBy    <http://www.ebusiness-unibw.org/ontologies/consumerelectronics/v1> ;
        rdfs:label          "storage media"@en , "Speichermedium"@de ;
        rdfs:range          :StorageMedia ;
        rdfs:subPropertyOf  gr:qualitativeProductOrServiceProperty ;
        :belongsToModule    "MP3Player, DigitalCamera, Camcorder"@en .

:Radio  a                 :Features ;
        rdfs:comment      "Ability to recieve radiosignal."@en ;
        rdfs:label        "Radio"@de , "Radio"@en ;
        :belongsToModule  "MP3Player"@en .

:Navy   a                 :Color ;
        rdfs:comment      "RGB Value 0,0,128"@en ;
        rdfs:label        "Marineblau"@de , "Navy"@en ;
        :belongsToModule  "MP3Player, TV, Printer, DigitalCamera, Camcorder"@en .

:MacOSXTiger  a           :CompatibleOperatingSystems ;
        rdfs:comment      "Mac OS is the trademarked name for a series of graphical user interface-based operating systems developed by Apple Inc. for their Macintosh line of computer systems."@en ;
        rdfs:label        "Mac OS X Tiger"@de , "Mac OS X Tiger"@en ;
        :belongsToModule  "MP3Player, Printer, DigitalCamera, Camcorder"@en .

:hasNumberOfHyptertextPages
        a                   owl:ObjectProperty ;
        rdfs:comment        "Defines the number of hypertext pages that can be displayed on the main screen of a device."@en ;
        rdfs:isDefinedBy    <http://www.ebusiness-unibw.org/ontologies/consumerelectronics/v1> ;
        rdfs:label          "number of hypertext pages"@en , "Anzahl von Teletextseiten"@de ;
        rdfs:range          gr:QuantitativeValueInteger ;
        rdfs:subPropertyOf  gr:quantitativeProductOrServiceProperty ;
        :belongsToModule    "TV"@en .

:IBM    a                 gr:BusinessEntity ;
        rdfs:comment      "The business entity IBM."@en ;
        rdfs:label        "IBM"^^xsd:string ;
        rdfs:seeAlso      <http://www.ibm.com/> ;
        gr:legalName      "International Business Machines Corporation"^^xsd:string ;
        :belongsToModule  "Printer"@en .

:SmartSoundControl  a     :AudioFeatures ;
        rdfs:comment      "SmartSound’s technology benefits television producers and editors by giving enhanced creative options through special music technology that delivers multiple musical variations for different moods."@en ;
        rdfs:label        "SmartSound control"@de , "SmartSound control"@en ;
        :belongsToModule  "TV"@en .

:hasDepthWithStand  a       owl:ObjectProperty ;
        rdfs:comment        "Defines the distance from side to side, measuring across the object with its stand at right angles to the width (Common unit of measurement centimetre, CMT).\n\n(This description is partly based on or reuses content from the Wikipedia article \"Length\" (http://en.wikipedia.org/wiki/Length) and is licensed under the GNU Free Documentation License (http://www.gnu.org/copyleft/fdl.html).)"@en ;
        rdfs:isDefinedBy    <http://www.ebusiness-unibw.org/ontologies/consumerelectronics/v1> ;
        rdfs:label          "depth with stand"@en , "Tiefe mit Standfuß"@de ;
        rdfs:range          gr:QuantitativeValueFloat ;
        rdfs:subPropertyOf  gr:quantitativeProductOrServiceProperty ;
        :belongsToModule    "TV"@en .

:Xerox  a                 gr:BusinessEntity ;
        rdfs:comment      "The business entity Xerox."@en ;
        rdfs:label        "Xerox"^^xsd:string ;
        rdfs:seeAlso      <http://www.xerox.com/> ;
        gr:legalName      "Xerox Corporation"^^xsd:string ;
        :belongsToModule  "Printer"@en .

:TV     a                 owl:Class ;
        rdfs:comment      "Television (TV) is a widely used telecommunication medium for transmitting and receiving moving images, either monochromatic (\"black and white\") or color, usually accompanied by sound. Is often deliverd with a remote control and a manual.\n\n(This description is partly based on or reuses content from the Wikipedia article \"TV\" (http://en.wikipedia.org/wiki/Tv) and is licensed under the GNU Free Documentation License (http://www.gnu.org/copyleft/fdl.html).)"@en ;
        rdfs:isDefinedBy  <http://www.ebusiness-unibw.org/ontologies/consumerelectronics/v1> ;
        rdfs:label        "TV"@de , "TV"@en ;
        rdfs:subClassOf   gr:ProductOrService ;
        :belongsToModule  "Printer"@en .

:Zoom   a                 owl:Class ;
        rdfs:comment      "Zoom is a method of decreasing (narrowing) the apparent angle of view of a photographic or video image.\n\n(This description is partly based on or reuses content from the Wikipedia article \"Digital zoom\" (http://en.wikipedia.org/wiki/Digital_zoom) and is licensed under the GNU Free Documentation License (http://www.gnu.org/copyleft/fdl.html).)"@en ;
        rdfs:isDefinedBy  <http://www.ebusiness-unibw.org/ontologies/consumerelectronics/v1> ;
        rdfs:label        "Zoom"@en , "Zoom"@de ;
        rdfs:subClassOf   gr:QualitativeValue ;
        :belongsToModule  "DigitalCamera, Camcorder"@en .

:MSI    a                 gr:BusinessEntity ;
        rdfs:comment      "The business entity Micro-Star Int'l Co., Ltd."@en ;
        rdfs:label        "MSI"^^xsd:string ;
        rdfs:seeAlso      <http://www.msi.com.tw/> ;
        gr:legalName      "Micro-Star Int'l Co., Ltd."^^xsd:string ;
        :belongsToModule  "MP3Player, TV"@en .

:DataFormatVideo  a       owl:Class ;
        rdfs:comment      "A data format is a particular way to encode information for storage in a computer file (refers to video data).\n\n(This description is partly based on or reuses content from the Wikipedia article \"File Format\" (http://en.wikipedia.org/wiki/File_format) and is licensed under the GNU Free Documentation License (http://www.gnu.org/copyleft/fdl.html).)"@en ;
        rdfs:isDefinedBy  <http://www.ebusiness-unibw.org/ontologies/consumerelectronics/v1> ;
        rdfs:label        "Data Format Video"@en , "Video Datenformat"@de ;
        rdfs:subClassOf   :DataFormat ;
        :belongsToModule  "MP3Player, DigitalCamera, Camcorder"@en .

:CVBS_out  a              :Connectivity ;
        rdfs:comment      "Composite video is often designated by the CVBS acronym, meaning any of \"Color, Video, Blank and Sync\", \"Composite Video Baseband Signal\", \"Composite Video Burst Signal\", or \"Composite Video with Burst and Sync\". Here the output is meant."@en ;
        rdfs:label        "CVBS out"@de , "CVBS out"@en ;
        :belongsToModule  "TV"@en .

:B9     a                 :MediaFormat ;
        rdfs:comment      "Format of the german institute for standardization: 44 x 62 mm."@en ;
        rdfs:label        "B9"@en , "B9"@de ;
        :belongsToModule  "Printer"@en .

:ASF    a                 :DataFormatAudio ;
        rdfs:comment      "Advanced Systems Format (formerly Advanced Streaming Format, Active Streaming Format) is Microsoft's proprietary digital audio/digital video container format, especially meant for streaming media. ASF is part of the Windows Media framework.\n\n(This description is partly based on or reuses content from the Wikipedia article \"Advanced Systems Format\" (http://en.wikipedia.org/wiki/Advanced_Systems_Format) and is licensed under the GNU Free Documentation License (http://www.gnu.org/copyleft/fdl.html).)"@en ;
        rdfs:label        "ASF"@de , "ASF"@en ;
        :belongsToModule  "MP3Player, DigitalCamera, Camcorder"@en .

:hasDisplayResolutionHorizontal
        a                   owl:ObjectProperty ;
        rdfs:comment        "Defines the digital resolution of the horizontal axe (Common unit of measurement pixel, E37)."@en ;
        rdfs:isDefinedBy    <http://www.ebusiness-unibw.org/ontologies/consumerelectronics/v1> ;
        rdfs:label          "display resolution horizontal"@en , "horizontale Bildschirmauflösung"@de ;
        rdfs:range          gr:QuantitativeValueInteger ;
        rdfs:subPropertyOf  gr:quantitativeProductOrServiceProperty ;
        :belongsToModule    "MP3Player, TV, DigitalCamera, Camcorder"@en .

:hasPhotographicFilterSize
        a                   owl:ObjectProperty ;
        rdfs:comment        "Size of a camera accessory consisting of an optical filter that can be inserted in the optical path.\n\n(This description is partly based on or reuses content from the Wikipedia article \"Photographic filter\" (http://en.wikipedia.org/wiki/Photographic_filter) and is licensed under the GNU Free Documentation License (http://www.gnu.org/copyleft/fdl.html).)"@en ;
        rdfs:isDefinedBy    <http://www.ebusiness-unibw.org/ontologies/consumerelectronics/v1> ;
        rdfs:label          "filter size"@en , "Filtergröße"@de ;
        rdfs:range          gr:QuantitativeValueFloat ;
        rdfs:subPropertyOf  gr:quantitativeProductOrServiceProperty ;
        :belongsToModule    "Camcorder"@en .

:Anti-ReflectionCoatedScreen
        a                 :GeneralFeatures ;
        rdfs:comment      "The screen has a short persistence phosphor with an anti-reflection and anti-static coating."@en ;
        rdfs:label        "Anti-reflection coated screen"@en , "Antireflektierende Bildschirmbeschichtung"@de ;
        :belongsToModule  "TV"@en .

:Dell   a                 gr:BusinessEntity ;
        rdfs:comment      "The business entity Dell."@en ;
        rdfs:label        "Dell"^^xsd:string ;
        rdfs:seeAlso      <http://www.dell.com/> ;
        gr:legalName      "Dell Inc."^^xsd:string ;
        :belongsToModule  "Printer"@en .

:PictBridge  a            :DataInterfaceType ;
        rdfs:comment      "Is an industry standard from the Camera & Imaging Products Association (CIPA) for direct printing."@en ;
        rdfs:label        "PictBridge"@en , "PictBridge"@de ;
        :belongsToModule  "Camcorder"@en .

:Pendrive  a              gr:BusinessEntity ;
        rdfs:comment      "The business entity dynaTRON Electronics GmbH & Co KG."@en ;
        rdfs:label        "Pendrive"^^xsd:string ;
        rdfs:seeAlso      <http://www.pendrive.com/> ;
        gr:legalName      "dynaTRON Electronics GmbH & Co. KG "^^xsd:string ;
        :belongsToModule  "MP3Player, DigitalCamera"@en .

:IEEE_802.11  a           :DataInterfaceType ;
        rdfs:comment      "IEEE 802.11 is a set of standards for wireless local area network (WLAN) computer communication, developed by the IEEE LAN/MAN Standards Committee (IEEE 802) in the 5 GHz and 2.4 GHz public spectrum bands.\n\n(This description is partly based on or reuses content from the Wikipedia article \"802.11\" (http://en.wikipedia.org/wiki/802.11) and is licensed under the GNU Free Documentation License (http://www.gnu.org/copyleft/fdl.html).)"@en ;
        rdfs:label        "IEEE 802.11"@de , "IEEE 802.11"@en ;
        :belongsToModule  "MP3Player, Printer, DigitalCamera, Camcorder"@en .

:VideoFeatures  a         owl:Class ;
        rdfs:comment      "Additional video equipment and abilities."@en ;
        rdfs:isDefinedBy  <http://www.ebusiness-unibw.org/ontologies/consumerelectronics/v1> ;
        rdfs:label        "Video Features"@en , "Video Eigenschaften"@de ;
        rdfs:subClassOf   :Features ;
        :belongsToModule  "TV"@en .

:Salora  a                gr:BusinessEntity ;
        rdfs:comment      "The business entity Salora."@en ;
        rdfs:label        "Salora"^^xsd:string ;
        rdfs:seeAlso      <http://www.salora.com/> ;
        gr:legalName      "SALORA"^^xsd:string ;
        :belongsToModule  "TV"@en .

:hasSleepModePowerConsumption
        a                   owl:ObjectProperty ;
        rdfs:comment        "Defines the ability to use a mode that saves significant electrical consumption compared to leaving a device fully on and idle but allows the user to avoid having to reset programming codes (Common unit of measurement Watt, WTT).\n\n(This description is partly based on or reuses content from the Wikipedia article \"Sleep mode\" (http://en.wikipedia.org/wiki/Sleep_mode) and is licensed under the GNU Free Documentation License (http://www.gnu.org/copyleft/fdl.html).)"@en ;
        rdfs:isDefinedBy    <http://www.ebusiness-unibw.org/ontologies/consumerelectronics/v1> ;
        rdfs:label          "sleep mode power consumption"@en , "Stromverbrauch im Ruhezustand"@de ;
        rdfs:range          gr:QuantitativeValueFloat ;
        rdfs:subPropertyOf  gr:quantitativeProductOrServiceProperty ;
        :belongsToModule    "TV"@en .

:A1     a                 :MediaFormat ;
        rdfs:comment      "Format of the german institute for standardization: 594 x 841 mm."@en ;
        rdfs:label        "A1"@en , "A1"@de ;
        :belongsToModule  "Printer"@en .

:hasDisplaySize  a          owl:ObjectProperty ;
        rdfs:comment        "Defines the diagonal length from the upper left to the lower right angle (Common unit of measurement centimetre, CMT; or inch, INH)."@en ;
        rdfs:isDefinedBy    <http://www.ebusiness-unibw.org/ontologies/consumerelectronics/v1> ;
        rdfs:label          "display size"@en , "Bildschirmgröße"@de ;
        rdfs:range          gr:QuantitativeValueFloat ;
        rdfs:subPropertyOf  gr:quantitativeProductOrServiceProperty ;
        :belongsToModule    "MP3Player, TV, Printer, DigitalCamera, Camcorder"@en .

:hasSpeakerQuantity  a      owl:ObjectProperty ;
        rdfs:comment        "Defines the number of integrated speakers an object includes."@en ;
        rdfs:isDefinedBy    <http://www.ebusiness-unibw.org/ontologies/consumerelectronics/v1> ;
        rdfs:label          "speaker quantity"@en , "Anzahl an Lautsprecher"@de ;
        rdfs:range          gr:QuantitativeValueInteger ;
        rdfs:subPropertyOf  gr:quantitativeProductOrServiceProperty ;
        :belongsToModule    "TV"@en .

:hasOperatingTime  a        owl:ObjectProperty ;
        rdfs:comment        "Average time the object operates (Common unit of measurement hour, HUR)."@en ;
        rdfs:isDefinedBy    <http://www.ebusiness-unibw.org/ontologies/consumerelectronics/v1> ;
        rdfs:label          "operating time"@en , "Betriebsdauer"@de ;
        rdfs:range          gr:QuantitativeValueFloat ;
        rdfs:subPropertyOf  gr:quantitativeProductOrServiceProperty ;
        :belongsToModule    "MP3Player, DigitalCamera, Camcorder"@en .

:Pink   a                 :Color ;
        rdfs:comment      "RGB Value 255,192,203"@en ;
        rdfs:label        "Pink"@de , "Pink"@en ;
        :belongsToModule  "MP3Player, TV, Printer, DigitalCamera, Camcorder"@en .

:RF     a             :Connectivity ;
        rdfs:comment  "An RF connector is an electrical connector designed to work at radio frequencies in the multi-megahertz range. RF connectors are typically used with coaxial cables and are designed to maintain the shielding that the coaxial design offers. Better models also minimize the change in transmission line impedance at the connection. Mechanically they provide a fastening mechanism (thread, bayonet, braces, push pull) and springs for a low ohmic electric contact while sparing the gold surface thus allowing above 1000 reconnects and reducing the insertion force. Research activity in the area of radio-frequency (RF) circuit design has surged in the last decade in direct response to the enormous market demand for inexpensive, high data rate wireless transceivers.\n\n(This description is partly based on or reuses content from the Wikipedia article \"RF connector\" (http://en.wikipedia.org/wiki/RF_connector) and is licensed under the GNU Free Documentation License (http://www.gnu.org/copyleft/fdl.html).)"@en ;
        rdfs:label    "RF"@en , "RF"@de .

:hasPrintBorderRight  a     owl:ObjectProperty ;
        rdfs:comment        "Defines the area which can not be printed on the right side of a paper (A4) (Common unit of measurement millimetre, MMT)."@en ;
        rdfs:isDefinedBy    <http://www.ebusiness-unibw.org/ontologies/consumerelectronics/v1> ;
        rdfs:label          "print border right"@en , "Druckgrenze rechts"@de ;
        rdfs:range          gr:QuantitativeValueFloat ;
        rdfs:subPropertyOf  gr:quantitativeProductOrServiceProperty ;
        :belongsToModule    "Printer"@en .

:Equalizer  a             :AudioFeatures ;
        rdfs:comment      "Equalization, equalisation or EQ is the process of using passive or active electronic elements or digital algorithms for the purpose of altering (originally flattening) the frequency response characteristics of a system.\n\n(This description is partly based on or reuses content from the Wikipedia article \"Equalization\" (http://en.wikipedia.org/wiki/Equalization) and is licensed under the GNU Free Documentation License (http://www.gnu.org/copyleft/fdl.html).)"@en ;
        rdfs:label        "Equalizer"@de , "Equalizer"@en ;
        :belongsToModule  "TV"@en .

:Hyperband  a             :SignalFormat ;
        rdfs:comment      "Hyperband designates a range (band) of electromagnetic waves with frequencies between 300 MHz and 470 MHz. This is designated for kable TV especially to recieve digital TV normed for DVB-C."@en ;
        rdfs:label        "Hyperband"@de , "Hyperband"@en ;
        :belongsToModule  "TV"@en .

:ComponentVideoOut  a  :Connectivity ;
        rdfs:comment  "Component video is a video signal that has been split into two or more components. In popular use, it refers to a type of analog video information that is transmitted or stored as three separate signals. Component video can be contrasted with composite video (NTSC, PAL or SECAM) in which all the video information is combined into a single line-level signal. Like composite, component video cables do not carry audio and are often paired with audio cables. Here the output is meant.\n\n(This description is partly based on or reuses content from the Wikipedia article \"Component video\" (http://en.wikipedia.org/wiki/Component_video) and is licensed under the GNU Free Documentation License (http://www.gnu.org/copyleft/fdl.html).)"@en ;
        rdfs:label    "Component video out"@de , "Component video out"@en .

:LightExposureControl
        a                 :Features ;
        rdfs:comment      "Is the total amount of light allowed to fall on the photographic medium during the process of taking a photograph."@en ;
        rdfs:label        "Belichtungsregelung"@de , "Light exposure control"@en ;
        :belongsToModule  "Camcorder"@en .

:Postcard  a              :MediaType ;
        rdfs:comment      "Rectangular piece of thick paper or thin cardboard intended for writing and mailing without an envelope."@en ;
        rdfs:label        "Postcard"@en , "Postkarte"@de ;
        :belongsToModule  "Printer"@en .

:iRiver  a                gr:BusinessEntity ;
        rdfs:comment      "The business entity iriver Europe GmbH."@en ;
        rdfs:label        "iriver"^^xsd:string ;
        rdfs:seeAlso      <http://www.iriver.de/> ;
        gr:legalName      "iriver Europe GmbH"^^xsd:string ;
        :belongsToModule  "MP3Player"@en .

:BeachAndSnow  a          :SceneMode ;
        rdfs:comment      "Ability of the camcorder to adapt to special environments."@en ;
        rdfs:label        "Strand und Schnee"@de , "Beach and snow"@en ;
        :belongsToModule  "Camcorder"@en .

:hasViewingAngleHorizontal
        a                   owl:ObjectProperty ;
        rdfs:comment        "Defines the angle in a horizontal axe where a viewer is still able to see the picture on a screen (Common unit of measurement degree, DD)."@en ;
        rdfs:isDefinedBy    <http://www.ebusiness-unibw.org/ontologies/consumerelectronics/v1> ;
        rdfs:label          "viewing angle horizontal"@en , "horizontaler Betrachtungswinkel"@de ;
        rdfs:range          gr:QuantitativeValueFloat ;
        rdfs:subPropertyOf  gr:quantitativeProductOrServiceProperty ;
        :belongsToModule    "TV"@en .

:hasDraftPrintableResolutionBlackWhiteHorizontal
        a                   owl:ObjectProperty ;
        rdfs:comment        "Defines the digital resolution of the horizontal axe (Common unit of measurement pixel, E37) for black/white prints for draft prints."@en ;
        rdfs:isDefinedBy    <http://www.ebusiness-unibw.org/ontologies/consumerelectronics/v1> ;
        rdfs:label          "draft printable resolution black white horizontal"@en , "horizontale druckbare Auflösung Schwarz/Weiß Entwurf"@de ;
        rdfs:range          gr:QuantitativeValueInteger ;
        rdfs:subPropertyOf  gr:quantitativeProductOrServiceProperty ;
        :belongsToModule    "Printer"@en .

:DocumentViewing  a       :Features ;
        rdfs:comment      "Ability to display documents."@en ;
        rdfs:label        "Dokumentdarstellung"@de , "Document viewing"@en ;
        :belongsToModule  "MP3Player, DigitalCamera, Camcorder"@en .

:DataFormatOffice  a      owl:Class ;
        rdfs:comment      "A data format is a particular way to encode information for storage in a computer file (refers to office data).\n\n(This description is partly based on or reuses content from the Wikipedia article \"File Format\" (http://en.wikipedia.org/wiki/File_format) and is licensed under the GNU Free Documentation License (http://www.gnu.org/copyleft/fdl.html).)"@en ;
        rdfs:isDefinedBy  <http://www.ebusiness-unibw.org/ontologies/consumerelectronics/v1> ;
        rdfs:label        "Data Format Office"@en , "Büro Datenformat"@de ;
        rdfs:subClassOf   :DataFormat ;
        :belongsToModule  "MP3Player, DigitalCamera"@en .

:ComputerDisplayResolution
        a                 owl:Class ;
        rdfs:comment      "The display resolution of a computer display typically refers to the number of distinct pixels in each dimension that can be displayed.\n\n(This description is partly based on or reuses content from the Wikipedia article \"Display resolution\" (http://en.wikipedia.org/wiki/Display_resolution) and is licensed under the GNU Free Documentation License (http://www.gnu.org/copyleft/fdl.html).)"@en ;
        rdfs:isDefinedBy  <http://www.ebusiness-unibw.org/ontologies/consumerelectronics/v1> ;
        rdfs:label        "Computer display resolution"@en , "Computerbildschirmauflösung"@de ;
        rdfs:subClassOf   :SupportedResolution ;
        :belongsToModule  "TV"@en .

:Microsoft  a             gr:BusinessEntity ;
        rdfs:comment      "The business entity Microsoft Corporation."@en ;
        rdfs:label        "Microsoft"^^xsd:string ;
        rdfs:seeAlso      <http://www.microsoft.com/> ;
        gr:legalName      "Microsoft Corporation"^^xsd:string ;
        :belongsToModule  "MP3Player"@en .

:AmbilightSpectraActiveFrame
        a                 :VideoFeatures ;
        rdfs:comment      "Active Frame is a single soft halo of light powered by 126 LEDs."@en ;
        rdfs:label        "Ambilight Spectra Active Frame"@de , "Ambilight Spectra Active Frame"@en ;
        :belongsToModule  "TV"@en .

:DVB_COFDM  a             :SignalFormat ;
        rdfs:comment      "Digital Video Broadcasting (DVB) is a suite of internationally accepted open standards for digital television. Coded OFDM (COFDM) and Discrete multi-tone modulation (DMT) is a frequency-division multiplexing (FDM) scheme utilized as a digital multi-carrier modulation method. A large number of closely-spaced orthogonal sub-carriers are used to carry data. The data is divided into several parallel data streams or channels, one for each sub-carrier. Each sub-carrier is modulated with a conventional modulation scheme (such as quadrature amplitude modulation or phase shift keying) at a low symbol rate, maintaining total data rates similar to conventional single-carrier modulation schemes in the same bandwidth.\n\n(This description is partly based on or reuses content from the Wikipedia article \"Digital Video Broadcasting\" (http://en.wikipedia.org/wiki/Digital_Video_Broadcasting) and is licensed under the GNU Free Documentation License (http://www.gnu.org/copyleft/fdl.html).)"@en ;
        rdfs:label        "DVB COFDM"@de , "DVB COFDM"@en ;
        :belongsToModule  "TV"@en .

:B4     a                 :MediaFormat ;
        rdfs:comment      "Format of the german institute for standardization: 250 x 353 mm."@en ;
        rdfs:label        "B4"@en , "B4"@de ;
        :belongsToModule  "Printer"@en .

:SensorType  a            owl:Class ;
        rdfs:comment      "Type of device that measures a physical quantity and converts it into a signal which can be read by an observer or by an instrument.\n\n(This description is partly based on or reuses content from the Wikipedia article \"Sensor\" (http://en.wikipedia.org/wiki/Sensor) and is licensed under the GNU Free Documentation License (http://www.gnu.org/copyleft/fdl.html).)"@en ;
        rdfs:isDefinedBy  <http://www.ebusiness-unibw.org/ontologies/consumerelectronics/v1> ;
        rdfs:label        "Sensorart"@de , "Sensor type"@en ;
        rdfs:subClassOf   gr:QualitativeValue ;
        :belongsToModule  "Camcorder"@en .

:BuiltInSpeakers  a       :AudioFeatures ;
        rdfs:comment      "Speakers that are integrated in the hull of a electronical device, that is able to play audio signals."@en ;
        rdfs:label        "Built in speakers"@en , "Eingebaute Lautsprecher"@de ;
        :belongsToModule  "TV, Camcorder"@en .

:StandbyLED  a            :GeneralFeatures ;
        rdfs:comment      "It is a semiconductor diode that emits light when an electric current is applied in the forward direction of the device used to show the standby status of an electrical device.\n\n(This description is partly based on or reuses content from the Wikipedia article \"LED\" (http://en.wikipedia.org/wiki/Led) and is licensed under the GNU Free Documentation License (http://www.gnu.org/copyleft/fdl.html).)"@en ;
        rdfs:label        "Standby LED"@en , "Standby Ledanzeige"@de ;
        :belongsToModule  "TV"@en .

:hasPowerRequirementsAC
        a                   owl:ObjectProperty ;
        rdfs:comment        "Defines the requirements of power an electronical device needs to operate (Common unit of measurement Ampere, AMP)."@en ;
        rdfs:isDefinedBy    <http://www.ebusiness-unibw.org/ontologies/consumerelectronics/v1> ;
        rdfs:label          "power requirements AC"@en , "Strombedarf AC"@de ;
        rdfs:range          gr:QuantitativeValueFloat ;
        rdfs:subPropertyOf  gr:quantitativeProductOrServiceProperty ;
        :belongsToModule    "TV"@en .

:SIGMA  a                 gr:BusinessEntity ;
        rdfs:comment      "The business entity SIGMA GmbH."@en ;
        rdfs:label        "SIGMA"^^xsd:string ;
        rdfs:seeAlso      <http://www.sigma-foto.de/> ;
        gr:legalName      "SIGMA GmbH"^^xsd:string ;
        :belongsToModule  "DigitalCamera"@en .

:SCART  a                 :Connectivity ;
        rdfs:comment      "SCART (from Syndicat des Constructeurs d'Appareils Radiorécepteurs et Téléviseurs, Radio and Television Receiver Manufacturer's Association) is a French-originated standard and associated 21-pin connector for connecting audio-visual (AV) equipment together.\n\n(This description is partly based on or reuses content from the Wikipedia article \"SCART\" (http://en.wikipedia.org/wiki/SCART) and is licensed under the GNU Free Documentation License (http://www.gnu.org/copyleft/fdl.html).)"@en ;
        rdfs:label        "SCART"@de , "SCART"@en ;
        :belongsToModule  "TV"@en .

:SubwooferOut  a          :Connectivity ;
        rdfs:comment      "A connection port for a subwoover. Subwoofer is a woofer, or a complete loudspeaker dedicated to the reproduction of bass audio frequencies, from perhaps 150 Hz down as far as 20 Hz, or in rare cases lower.\n\n(This description is partly based on or reuses content from the Wikipedia article \"Subwoofer\" (http://en.wikipedia.org/wiki/Subwoofer) and is licensed under the GNU Free Documentation License (http://www.gnu.org/copyleft/fdl.html).)"@en ;
        rdfs:label        "Subwoofer out"@de , "Subwoofer out"@en ;
        :belongsToModule  "TV"@en .

:Yusmart  a               gr:BusinessEntity ;
        rdfs:comment      "The business entity Yusmart."@en ;
        rdfs:label        "Yusmart"^^xsd:string ;
        rdfs:seeAlso      <http://www.yusmart-lcd.co.uk/> ;
        gr:legalName      "Yusmart B.V."^^xsd:string ;
        :belongsToModule  "TV"@en .

:hasBodyColor  a            owl:ObjectProperty ;
        rdfs:comment        "Defines the major color of an objects body."@en ;
        rdfs:isDefinedBy    <http://www.ebusiness-unibw.org/ontologies/consumerelectronics/v1> ;
        rdfs:label          "body color"@en , "Farbe"@de ;
        rdfs:range          :Color ;
        rdfs:subPropertyOf  gr:qualitativeProductOrServiceProperty ;
        :belongsToModule    "MP3Player, TV, Printer, DigitalCamera, Camcorder"@en .

:Archos  a                gr:BusinessEntity ;
        rdfs:comment      "The business entity Archos GmbH."@en ;
        rdfs:label        "Archos"^^xsd:string ;
        rdfs:seeAlso      <http://www.archos.com/> ;
        gr:legalName      "Archos GmbH"^^xsd:string ;
        :belongsToModule  "MP3Player, Camcorder"@en .

:Lenco  a                 gr:BusinessEntity ;
        rdfs:comment      "The business entity Lenco Audio-Video."@en ;
        rdfs:label        "Lenco"^^xsd:string ;
        rdfs:seeAlso      <http://www.lenco-audiovideo.com/> ;
        gr:legalName      "Lenco Audio-Video"^^xsd:string ;
        :belongsToModule  "MP3Player, TV"@en .

:MacOSXSnowLeopard  a     :CompatibleOperatingSystems ;
        rdfs:comment      "Mac OS is the trademarked name for a series of graphical user interface-based operating systems developed by Apple Inc. for their Macintosh line of computer systems."@en ;
        rdfs:label        "Mac OS X Snow Leopard"@de , "Mac OS X Snow Leopard"@en ;
        :belongsToModule  "MP3Player, Printer, DigitalCamera, Camcorder"@en .

:Differo  a               gr:BusinessEntity ;
        rdfs:comment      "The business entity Differo Ltd."@en ;
        rdfs:label        "Differo"^^xsd:string ;
        rdfs:seeAlso      <http://www.differo.es/> ;
        gr:legalName      "Differo Ltd."^^xsd:string ;
        :belongsToModule  "MP3Player"@en .

:has35mmCameraLensEquivalentRange
        a                   owl:DatatypeProperty ;
        rdfs:comment        "Defines an optical lens or assembly of lenses used in conjunction with a camera body and mechanism to make images of objects either on photographic film or on other media capable of storing an image chemically or electronically."@en ;
        rdfs:isDefinedBy    <http://www.ebusiness-unibw.org/ontologies/consumerelectronics/v1> ;
        rdfs:label          "35mm camera lens equivalent range"@en , "35mm Kameraobjektiv"@de ;
        rdfs:range          xsd:boolean ;
        rdfs:subPropertyOf  gr:datatypeProductOrServiceProperty ;
        :belongsToModule    "Camcorder"@en .

:AutoWhiteBalance  a      :WhiteBalance ;
        rdfs:comment      "Ability to adapt of different adjustments of the intensities of the colors."@en ;
        rdfs:label        "Auto white balance"@en , "Automatischer Weißabgleich"@de ;
        :belongsToModule  "Camcorder"@en .

:Kyocera  a               gr:BusinessEntity ;
        rdfs:comment      "The business entity Kyocera."@en ;
        rdfs:label        "Kyocera"^^xsd:string ;
        rdfs:seeAlso      <http://global.kyocera.com/> ;
        gr:legalName      "Kyocera Corporation"^^xsd:string ;
        :belongsToModule  "Printer"@en .

:Kodak  a                 gr:BusinessEntity ;
        rdfs:comment      "The business entity Eastman Kodak Company."@en ;
        rdfs:label        "Kodak"^^xsd:string ;
        rdfs:seeAlso      <http://www.kodak.com/> ;
        gr:legalName      "Eastman Kodak Company"^^xsd:string ;
        :belongsToModule  "DigitalCamera, Camcorder"@en .

:FocusFixed  a            :Focus ;
        rdfs:comment      "A photographic lens for which the focus is not adjustable is called a fixed-focus lens.\n\n(This description is partly based on or reuses content from the Wikipedia article \"Fixed focus\" (http://en.wikipedia.org/wiki/Fixed_focus) and is licensed under the GNU Free Documentation License (http://www.gnu.org/copyleft/fdl.html).)"@en ;
        rdfs:label        "Focus fixed"@en , "Starrer Fokus"@de ;
        :belongsToModule  "DigitalCamera, Camcorder"@en .

:Epson  a                 gr:BusinessEntity ;
        rdfs:comment      "The business entity Seiko Epson Corporation."@en ;
        rdfs:label        "Epson"^^xsd:string ;
        rdfs:seeAlso      <http://www.epson.co.jp/e/> ;
        gr:legalName      "Seiko Epson Corporation"^^xsd:string ;
        :belongsToModule  "MP3Player, Printer, DigitalCamera"@en .

:Bitmap  a                :DataFormatImage ;
        rdfs:comment      "In computer graphics, a bitmap or pixmap is a type of memory organization or image file format used to store digital images.\n\n(This description is partly based on or reuses content from the Wikipedia article \"Bitmap\" (http://en.wikipedia.org/wiki/Bitmap) and is licensed under the GNU Free Documentation License (http://www.gnu.org/copyleft/fdl.html).)"@en ;
        rdfs:label        "Bitmap"@de , "Bitmap"@en ;
        :belongsToModule  "MP3Player, DigitalCamera, Camcorder"@en .

:Sagem  a                 gr:BusinessEntity ;
        rdfs:comment      "The business entity Sagem."@en ;
        rdfs:label        "Sagem"^^xsd:string ;
        rdfs:seeAlso      <http://www.sagem.com/> ;
        gr:legalName      "Sagem Télécommunications"^^xsd:string ;
        :belongsToModule  "TV, Printer"@en .

:hasMediaWeightTray2  a     owl:ObjectProperty ;
        rdfs:comment        "Describes the weight of the media format (Common unit of measurement gram per square metre, GM) hold in tray 2."@en ;
        rdfs:isDefinedBy    <http://www.ebusiness-unibw.org/ontologies/consumerelectronics/v1> ;
        rdfs:label          "media weight tray 2"@en , "Mediengewicht Kassette 1"@de ;
        rdfs:range          gr:QuantitativeValueFloat ;
        rdfs:subPropertyOf  gr:quantitativeProductOrServiceProperty ;
        :belongsToModule    "Printer"@en .

:TallyGenicom  a          gr:BusinessEntity ;
        rdfs:comment      "The business entity TallyGenicom."@en ;
        rdfs:label        "TallyGenicom"^^xsd:string ;
        rdfs:seeAlso      <http://www.tallygenicom.com/> ;
        gr:legalName      "TallyGenicom"^^xsd:string ;
        :belongsToModule  "Printer"@en .

:Gembird  a               gr:BusinessEntity ;
        rdfs:comment      "The business entity GEMBIRD ® Deutschland GmbH."@en ;
        rdfs:label        "Gembird"^^xsd:string ;
        rdfs:seeAlso      <http://www.gembird.com/> ;
        gr:legalName      "GEMBIRD ® Deutschland GmbH "^^xsd:string ;
        :belongsToModule  "MP3Player"@en .

:hasFocus  a                owl:ObjectProperty ;
        rdfs:comment        "A focus, also called an image point, is the point where light rays originating from a point on the object converge.\n\n(This description is partly based on or reuses content from the Wikipedia article \"Focus (optics)\" (http://en.wikipedia.org/wiki/Focus_(optics)) and is licensed under the GNU Free Documentation License (http://www.gnu.org/copyleft/fdl.html).)"@en ;
        rdfs:isDefinedBy    <http://www.ebusiness-unibw.org/ontologies/consumerelectronics/v1> ;
        rdfs:label          "focus"@en , "Fokus"@de ;
        rdfs:range          :Focus ;
        rdfs:subPropertyOf  gr:qualitativeProductOrServiceProperty ;
        :belongsToModule    "DigitalCamera, Camcorder"@en .

:HDTV_1080i  a            :TVDisplayResolution ;
        rdfs:comment      "1080i is the shorthand name of a format of high-definition video modes. 1080 denotes the number of horizontal scan lines - also known as vertical resolution - and the letter i stands for interlaced.\n\n(This description is partly based on or reuses content from the Wikipedia article \"1080i\" (http://en.wikipedia.org/wiki/1080i) and is licensed under the GNU Free Documentation License (http://www.gnu.org/copyleft/fdl.html).)"@en ;
        rdfs:label        "HDTV 1080i"@en , "HDTV 1080i"@de ;
        :belongsToModule  "TV"@en .

:Hyundai  a               gr:BusinessEntity ;
        rdfs:comment      "The business entity Hyundai."@en ;
        rdfs:label        "Hyundai"^^xsd:string ;
        rdfs:seeAlso      <http://www.hyundaiit.eu/> ;
        gr:legalName      "Hyundai IT Europe GmbH"^^xsd:string ;
        :belongsToModule  "TV"@en .

:SD     a                 :StorageMedia ;
        rdfs:comment      "A flash memory card format used in portable device."@en ;
        rdfs:label        "SD"@de , "SD"@en ;
        :belongsToModule  "MP3Player, DigitalCamera, Camcorder"@en .

:iDream  a                gr:BusinessEntity ;
        rdfs:comment      "The business entity iDream Production Pvt. Ltd."@en ;
        rdfs:label        "iDream"^^xsd:string ;
        rdfs:seeAlso      <http://www.idream.be/> ;
        gr:legalName      "iDream Production Pvt. Ltd."^^xsd:string ;
        :belongsToModule  "MP3Player"@en .

:SDTV_576i  a             :TVDisplayResolution ;
        rdfs:comment      "576i is a standard-definition video mode used in (former) PAL and SECAM countries. In digital applications it's usually referred to as \"576i\", in analogue contexts it's often quoted as \"625 lines\". The 576 identifies a vertical resolution of 576 lines (usually with a horizontal resolution of 720 or 704 pixels), and the i identifies it as an interlaced resolution.\n\n(This description is partly based on or reuses content from the Wikipedia article \"576ii\" (http://en.wikipedia.org/wiki/576i) and is licensed under the GNU Free Documentation License (http://www.gnu.org/copyleft/fdl.html).)"@en ;
        rdfs:label        "SDTV 576i"@de , "SDTV 576i"@en ;
        :belongsToModule  "TV"@en .

:Gold   a                 :Color ;
        rdfs:comment      "RGB Value 255,215,0"@en ;
        rdfs:label        "Gold"@de , "Gold"@en ;
        :belongsToModule  "MP3Player, TV, Printer, DigitalCamera, Camcorder"@en .

:ViewSonic  a             gr:BusinessEntity ;
        rdfs:comment      "The business entity ViewSonic."@en ;
        rdfs:label        "ViewSonic"^^xsd:string ;
        rdfs:seeAlso      <http://www.viewsonic.com/> ;
        gr:legalName      "ViewSonic Corporation"^^xsd:string ;
        :belongsToModule  "TV"@en .

:Polaroid  a              gr:BusinessEntity ;
        rdfs:comment      "The business entity Polaroid."@en ;
        rdfs:label        "Polaroid"^^xsd:string ;
        rdfs:seeAlso      <http://www.polaroid.com/> ;
        gr:legalName      "Polaroid Corporation"^^xsd:string ;
        :belongsToModule  "TV, DigitalCamera"@en .

:RoHS   a                 :Certificate ;
        rdfs:comment      "The Directive on the restriction of the use of certain hazardous substances in electrical and electronic equipment 2002/95/EC.\n\n(This description is partly based on or reuses content from the Wikipedia article \"ROHS\" (http://en.wikipedia.org/wiki/ROHS) and is licensed under the GNU Free Documentation License (http://www.gnu.org/copyleft/fdl.html).)"@en ;
        rdfs:label        "RoHS"@de , "RoHS"@en ;
        :belongsToModule  "TV"@en .

:AutoVolumeLeveller  a    :AudioFeatures ;
        rdfs:comment      "Levels the audio volume of televisions automatically so that undesired peaks in the sound can be reduced."@en ;
        rdfs:label        "Auto volume leveller"@en , "Automatische Lautstärkenanpassung"@de ;
        :belongsToModule  "TV"@en .

:Accessory  a             owl:Class ;
        rdfs:comment      "A subordinate or supplementary item; an adjunct."@en ;
        rdfs:isDefinedBy  <http://www.ebusiness-unibw.org/ontologies/consumerelectronics/v1> ;
        rdfs:label        "Zubehör"@de , "Accessory"@en ;
        rdfs:subClassOf   gr:QualitativeValue ;
        :belongsToModule  "Camcorder"@en .

:VideoRecording  a        :Features ;
        rdfs:comment      "Ability to record videos."@en ;
        rdfs:label        "Video recording"@en , "Videoaufnahme"@de ;
        :belongsToModule  "DigitalCamera"@en .

:UHF    a                 :SignalFormat ;
        rdfs:comment      "Ultra high frequency (UHF) designates a range (band) of electromagnetic waves with frequencies between 300 MHz and 3 GHz (3,000 MHz).\n\n(This description is partly based on or reuses content from the Wikipedia article \"UHF\" (http://en.wikipedia.org/wiki/UHF) and is licensed under the GNU Free Documentation License (http://www.gnu.org/copyleft/fdl.html).)"@en ;
        rdfs:label        "VHF"@de , "UHF"@en ;
        :belongsToModule  "TV"@en .

:Yuraku  a                gr:BusinessEntity ;
        rdfs:comment      "The business entity Yuraku."@en ;
        rdfs:label        "Yuraku"^^xsd:string ;
        rdfs:seeAlso      <http://www.yuraku.com.sg/> ;
        gr:legalName      "YURAKU Pte Ltd."^^xsd:string ;
        :belongsToModule  "TV"@en .

:A8     a                 :MediaFormat ;
        rdfs:comment      "Format of the german institute for standardization: 52 x 74 mm."@en ;
        rdfs:label        "A8"@en , "A8"@de ;
        :belongsToModule  "Printer"@en .

:Playlist  a              :Features ;
        rdfs:comment      "Ability to put audiofiles in a playlist."@en ;
        rdfs:label        "Playlist"@en , "Wiedergabeliste"@de ;
        :belongsToModule  "MP3Player"@en .

:hasMinRelativeHumidity
        a                   owl:ObjectProperty ;
        rdfs:comment        "Defines the minimum level of relative humidity, non-condensing, within which the product can operate."@en ;
        rdfs:isDefinedBy    <http://www.ebusiness-unibw.org/ontologies/consumerelectronics/v1> ;
        rdfs:label          "min relative humidity"@en , "minimale Luftfeuchtigkeit"@de ;
        rdfs:range          gr:QuantitativeValueFloat ;
        rdfs:subPropertyOf  gr:quantitativeProductOrServiceProperty ;
        :belongsToModule    "TV, Printer"@en .

:AOC    a             gr:BusinessEntity ;
        rdfs:comment  "The business entity AOC."@en ;
        rdfs:label    "AOC"^^xsd:string ;
        rdfs:seeAlso  <http://www.aoc-europe.com/> ;
        gr:legalName  "AOC"^^xsd:string .

:hasPackageDepth  a         owl:ObjectProperty ;
        rdfs:comment        "Defines the distance from side to side, measuring across the object with its package at right angles to the width (Common unit of measurement centimetre, CMT).\n\n(This description is partly based on or reuses content from the Wikipedia article \"Length\" (http://en.wikipedia.org/wiki/Length) and is licensed under the GNU Free Documentation License (http://www.gnu.org/copyleft/fdl.html).)"@en ;
        rdfs:isDefinedBy    <http://www.ebusiness-unibw.org/ontologies/consumerelectronics/v1> ;
        rdfs:label          "package depth"@en , "Verpackungstiefe"@de ;
        rdfs:range          gr:QuantitativeValueFloat ;
        rdfs:subPropertyOf  gr:quantitativeProductOrServiceProperty ;
        :belongsToModule    "TV"@en .

:TechniSat  a             gr:BusinessEntity ;
        rdfs:comment      "The business entity TechniSat."@en ;
        rdfs:label        "TechniSat"^^xsd:string ;
        rdfs:seeAlso      <http://www.technisat.com/> ;
        gr:legalName      "TechniSat Digital GmbH "^^xsd:string ;
        :belongsToModule  "MP3Player, TV"@en .

:hasStandardOutputCapacityForEnvelopes
        a                   owl:ObjectProperty ;
        rdfs:comment        "Defines the maximum amount of envelopes the product is able to print."@en ;
        rdfs:isDefinedBy    <http://www.ebusiness-unibw.org/ontologies/consumerelectronics/v1> ;
        rdfs:label          "standard output capacity for envelopes"@en , "Standard Ausgabekapazität für Briefkuvert"@de ;
        rdfs:range          gr:QuantitativeValueInteger ;
        rdfs:subPropertyOf  gr:quantitativeProductOrServiceProperty ;
        :belongsToModule    "Printer"@en .

:FullHD  a                :VideoFeatures ;
        rdfs:comment      "Usually assumes a widescreen aspect ratio of 16:9, implying a horizontal resolution of 1920 pixels. This creates a frame resolution of 1920×1080, or 2,073,600 pixels in total.\n\n(This description is partly based on or reuses content from the Wikipedia article \"1080p\" (http://en.wikipedia.org/wiki/1080p) and is licensed under the GNU Free Documentation License (http://www.gnu.org/copyleft/fdl.html).)"@en ;
        rdfs:label        "Full HD"@de , "Full HD"@en ;
        :belongsToModule  "TV"@en .

:Axago  a                 gr:BusinessEntity ;
        rdfs:comment      "The business entity Axago."@en ;
        rdfs:label        "Axago"^^xsd:string ;
        rdfs:seeAlso      <http://www.axago.cz/> ;
        gr:legalName      "Axago"^^xsd:string ;
        :belongsToModule  "MP3Player"@en .

:MediaFormaPostcard  a    :MediaFormat ;
        rdfs:comment      "Media format that is able to assume different shapes."@en ;
        rdfs:label        "Media format postcard"@en , "Medienformat Postkarte"@de ;
        :belongsToModule  "Printer"@en .

:Pacific_Digital  a       gr:BusinessEntity ;
        rdfs:comment      "The business entity Pacific Digital Home."@en ;
        rdfs:label        "Pacific Digital"^^xsd:string ;
        rdfs:seeAlso      <http://www.pacificdigitalhome.com/> ;
        gr:legalName      "Pacific Digital Home"^^xsd:string ;
        :belongsToModule  "MP3Player"@en .

:RISC   a                 :ProcessorType ;
        rdfs:comment      "Reduced instruction set computing, represents a CPU design strategy emphasizing the insight that simplified instructions that \"do less\" may still provide for higher performance if this simplicity can be utilized to make instructions execute very quickly."@en ;
        rdfs:label        "RISC"@en , "RISC"@de ;
        :belongsToModule  "Printer"@en .

:ComputerDisplayResolution_800x600_60_72_75_85Hz
        a                 :ComputerDisplayResolution ;
        rdfs:comment      "Display resolution specified as the width and height in pixels, color depth measured in bits, and refresh rate expressed in hertz; here Super Video Graphics Array.\n\n(This description is partly based on or reuses content from the Wikipedia article \"Display resolution\" (http://en.wikipedia.org/wiki/Display_resolution) and is licensed under the GNU Free Documentation License (http://www.gnu.org/copyleft/fdl.html).)"@en ;
        rdfs:label        "Computerbildschirmauflösung 800x600 60 72 75 85Hz"@de , "Computer display resolution 800x600 60 72 75 85Hz"@en ;
        :belongsToModule  "TV"@en .

:Features  a              owl:Class ;
        rdfs:comment      "Additional equipment and abilities."@en ;
        rdfs:isDefinedBy  <http://www.ebusiness-unibw.org/ontologies/consumerelectronics/v1> ;
        rdfs:label        "Eigenschaften"@de , "Features"@en ;
        rdfs:subClassOf   gr:QualitativeValue ;
        :belongsToModule  "MP3Player, TV, DigitalCamera, Camcorder"@en .

:hasPackageWidth  a         owl:ObjectProperty ;
        rdfs:comment        "Defines the distance between the ends of an object, its linear extent as measured from end to end with its package (Common unit of measurement centimetre, CMT)."@en ;
        rdfs:isDefinedBy    <http://www.ebusiness-unibw.org/ontologies/consumerelectronics/v1> ;
        rdfs:label          "package width"@en , "Verpackungsbreite"@de ;
        rdfs:range          gr:QuantitativeValueFloat ;
        rdfs:subPropertyOf  gr:quantitativeProductOrServiceProperty ;
        :belongsToModule    "TV"@en .

:Windows98  a             :CompatibleOperatingSystems ;
        rdfs:comment      "A version of a Microsoft operating system."@en ;
        rdfs:label        "Windows 98"@de , "Windows 98"@en ;
        :belongsToModule  "MP3Player, Printer, DigitalCamera, Camcorder"@en .

:hasNormalPrintableResolutionColorVertical
        a                   owl:ObjectProperty ;
        rdfs:comment        "Defines the digital resolution of the vertical axe (Common unit of measurement pixel, E37)  for color prints for normal prints."@en ;
        rdfs:isDefinedBy    <http://www.ebusiness-unibw.org/ontologies/consumerelectronics/v1> ;
        rdfs:label          "normal printable resolution color vertical"@en , "vertikale durckbare Aufslösung Farbe normal"@de ;
        rdfs:range          gr:QuantitativeValueInteger ;
        rdfs:subPropertyOf  gr:quantitativeProductOrServiceProperty ;
        :belongsToModule    "Printer"@en .

:CompositeVideoIn  a      :Connectivity ;
        rdfs:comment      "Composite video is the format of an analog television (picture only) signal before it is combined with a sound signal and modulated onto an RF carrier. It is usually in a standard format such as NTSC, PAL, or SECAM. It is a composite of three source signals called Y, U and V (together referred to as YUV) with sync pulses. Here the input is meant.\n\n(This description is partly based on or reuses content from the Wikipedia article \"Composite video\" (http://en.wikipedia.org/wiki/Composite_video) and is licensed under the GNU Free Documentation License (http://www.gnu.org/copyleft/fdl.html).)"@en ;
        rdfs:label        "Composite video in"@de , "Composite video in"@en ;
        :belongsToModule  "TV"@en .

:PAL-B_G  a               :SignalFormat ;
        rdfs:comment      "PAL, short for Phase Alternating Line, is a colour-encoding system used in broadcast television systems in large parts of the world. This is used in western europe.\n\n(This description is partly based on or reuses content from the Wikipedia article \"PAL\" (http://en.wikipedia.org/wiki/PAL) and is licensed under the GNU Free Documentation License (http://www.gnu.org/copyleft/fdl.html).)"@en ;
        rdfs:label        "PAL-B G"@de , "PAL-B G"@en ;
        :belongsToModule  "TV"@en .

:AmbilightSpectra3  a     :VideoFeatures ;
        rdfs:comment      "Enlarges the screen further by projecting a glow of light from the back of the screen onto the surrounding wall. Ambilight adjusts automatically the colour and brightness of the light surrounding the TV to match with the picture."@en ;
        rdfs:label        "Ambilight Spectra 3"@en , "Ambilight Spectra 3"@de ;
        :belongsToModule  "TV"@en .

:SECAM  a                 :SignalFormat ;
        rdfs:comment      "SECAM, also written SÉCAM (Séquentiel couleur à mémoire, French for \"Sequential Color with Memory\"), is an analog color television system first used in France.\n\n(This description is partly based on or reuses content from the Wikipedia article \"SECAM\" (http://en.wikipedia.org/wiki/SECAM) and is licensed under the GNU Free Documentation License (http://www.gnu.org/copyleft/fdl.html).)"@en ;
        rdfs:label        "SECAM"@de , "SECAM"@en ;
        :belongsToModule  "TV"@en .

:XDPictureCard  a         :StorageMedia ;
        rdfs:comment      "The xD-Picture Card is a type of flash memory card."@en ;
        rdfs:label        "XDPictureCard"@en , "XDPictureCard"@de ;
        :belongsToModule  "MP3Player, DigitalCamera, Camcorder"@en .

:Palm   a                 gr:BusinessEntity ;
        rdfs:comment      "The business entity Palm Inc."@en ;
        rdfs:label        "Palm"^^xsd:string ;
        rdfs:seeAlso      <http://www.palm.com/> ;
        gr:legalName      "Palm Inc"^^xsd:string ;
        :belongsToModule  "MP3Player"@en .

:DigitalAudioOpticalOut
        a                 :Connectivity ;
        rdfs:comment      "Digital audio uses digital signals for sound reproduction. This includes analog-to-digital conversion, digital-to-analog conversion, storage, and transmission. TOSLINK or Optical Cable is a standardized optical fiber connection system.\n\n(This description is partly based on or reuses content from the Wikipedia article \"Digital audio\" (http://en.wikipedia.org/wiki/Digital_audio) and is licensed under the GNU Free Documentation License (http://www.gnu.org/copyleft/fdl.html).)"@en ;
        rdfs:label        "Digital audio optical out"@de , "Digital audio optical out"@en ;
        :belongsToModule  "TV"@en .

:NIH2   a                 :RechargeableEnergySource ;
        rdfs:comment      "A nickel hydrogen battery (NIH2 or Ni-H2) is a rechargeable electrochemical power source based on nickel and hydrogen."@en ;
        rdfs:label        "NIH2"@de , "NIH2"@en ;
        :belongsToModule  "MP3Player, DigitalCamera, Camcorder"@en .

:Harwa  a                 gr:BusinessEntity ;
        rdfs:comment      "The business entity Harwa."@en ;
        rdfs:label        "Harwa"^^xsd:string ;
        gr:legalName      "Harwa Electronics GmbH"^^xsd:string ;
        :belongsToModule  "TV"@en .

:Memorex  a               gr:BusinessEntity ;
        rdfs:comment      "The business entity Memorex Products, Inc."@en ;
        rdfs:label        "Memorex"^^xsd:string ;
        rdfs:seeAlso      <http://www.memorex.com/> ;
        gr:legalName      "Memorex Products, Inc."^^xsd:string ;
        :belongsToModule  "MP3Player, TV"@en .

:hasMaxPrintCapacity  a     owl:ObjectProperty ;
        rdfs:comment        "Describes the maximum printed sites per month."@en ;
        rdfs:isDefinedBy    <http://www.ebusiness-unibw.org/ontologies/consumerelectronics/v1> ;
        rdfs:label          "max print capacity"@en , "maximale Druckkapazität"@de ;
        rdfs:range          gr:QuantitativeValueInteger ;
        rdfs:subPropertyOf  gr:quantitativeProductOrServiceProperty ;
        :belongsToModule    "Printer"@en .

:PQI    a                 gr:BusinessEntity ;
        rdfs:comment      "The business entity Power Quotient International Co., Ltd."@en ;
        rdfs:label        "PQI"^^xsd:string ;
        rdfs:seeAlso      <http://www.pqi.com.tw/> ;
        gr:legalName      "Power Quotient International Co., Ltd."^^xsd:string ;
        :belongsToModule  "MP3Player"@en .

:Orion  a                 gr:BusinessEntity ;
        rdfs:comment      "The business entity Orion."@en ;
        rdfs:label        "Orion"^^xsd:string ;
        rdfs:seeAlso      <http://www.orion-europa.de/> ;
        gr:legalName      "ORION - ISP Kommanditgesellschaft Dieter Lather"^^xsd:string ;
        :belongsToModule  "TV"@en .

:SECAM-L  a               :SignalFormat ;
        rdfs:comment      "SECAM, also written SÉCAM (Séquentiel couleur à mémoire, French for \"Sequential Color with Memory\"), is an analog color television system first used in France. French SECAM (SECAM-L) is used only in France, Luxembourg (only RTL9 on CH 21 from Dudelange) and Tele Monte-Carlo Transmitters in the south of France.\n\n(This description is partly based on or reuses content from the Wikipedia article \"SECAM\" (http://en.wikipedia.org/wiki/SECAM) and is licensed under the GNU Free Documentation License (http://www.gnu.org/copyleft/fdl.html).)"@en ;
        rdfs:label        "SECAM-L"@de , "SECAM-L"@en ;
        :belongsToModule  "TV"@en .

:PNG    a                 :DataFormatImage ;
        rdfs:comment      "The PNG (Portable Network Graphics) file format was created as the free, open-source successor to the GIF.\n\n(This description is partly based on or reuses content from the Wikipedia article \"Graphics file format\" (http://en.wikipedia.org/wiki/Graphics_file_format) and is licensed under the GNU Free Documentation License (http://www.gnu.org/copyleft/fdl.html).)"@en ;
        rdfs:label        "PNG"@de , "PNG"@en ;
        :belongsToModule  "MP3Player, DigitalCamera, Camcorder"@en .

:hasChannelQuantity  a      owl:ObjectProperty ;
        rdfs:comment        "Defines the number of channels of a television that can be used to save specific transmitted signals."@en ;
        rdfs:isDefinedBy    <http://www.ebusiness-unibw.org/ontologies/consumerelectronics/v1> ;
        rdfs:label          "channel quantity"@en , "Anzahl von Kanäle"@de ;
        rdfs:range          gr:QuantitativeValueInteger ;
        rdfs:subPropertyOf  gr:quantitativeProductOrServiceProperty ;
        :belongsToModule    "TV"@en .

:PCIn   a                 :Connectivity ;
        rdfs:comment      "Port to connect a PC with the electronical device."@en ;
        rdfs:label        "PC in"@de , "PC in"@en ;
        :belongsToModule  "TV"@en .

:hasDraftPrintableResolutionColorHorizontal
        a                   owl:ObjectProperty ;
        rdfs:comment        "Defines the digital resolution of the horizontal axe (Common unit of measurement pixel, E37) for black/white prints for draft prints."@en ;
        rdfs:isDefinedBy    <http://www.ebusiness-unibw.org/ontologies/consumerelectronics/v1> ;
        rdfs:label          "draft printable resolution color horizontal"@en , "horizontale druckbare Auflösung Farbe Entwurf"@de ;
        rdfs:range          gr:QuantitativeValueInteger ;
        rdfs:subPropertyOf  gr:quantitativeProductOrServiceProperty ;
        :belongsToModule    "Printer"@en .

:MacOSXJaguar  a          :CompatibleOperatingSystems ;
        rdfs:comment      "Mac OS is the trademarked name for a series of graphical user interface-based operating systems developed by Apple Inc. for their Macintosh line of computer systems."@en ;
        rdfs:label        "Mac OS X Jaguar"@de , "Mac OS X Jaguar"@en ;
        :belongsToModule  "MP3Player, Printer, DigitalCamera, Camcorder"@en .

:Yellow  a                :Color ;
        rdfs:comment      "RGB Value 255,255,0"@en ;
        rdfs:label        "Gelb"@de , "Yellow"@en ;
        :belongsToModule  "MP3Player, TV, Printer, DigitalCamera, Camcorder"@en .

:HP     a                 gr:BusinessEntity ;
        rdfs:comment      "The business entity Hewlett-Packard Company."@en ;
        rdfs:label        "HP"^^xsd:string ;
        rdfs:seeAlso      <http://www.hp.com/> ;
        gr:legalName      "Hewlett-Packard Company"^^xsd:string ;
        :belongsToModule  "MP3Player, Printer, DigitalCamera"@en .

:A3     a                 :MediaFormat ;
        rdfs:comment      "Format of the german institute for standardization: 297 x 420 mm."@en ;
        rdfs:label        "A3"@en , "A3"@de ;
        :belongsToModule  "Printer"@en .

:hasPaperFormat  a          owl:ObjectProperty ;
        rdfs:comment        "Defines the supported paper formats."@en ;
        rdfs:isDefinedBy    <http://www.ebusiness-unibw.org/ontologies/consumerelectronics/v1> ;
        rdfs:label          "paper format"@en , "Papierformat"@de ;
        rdfs:range          :MediaFormat ;
        rdfs:subPropertyOf  gr:qualitativeProductOrServiceProperty ;
        :belongsToModule    "Printer"@en .

:USB3.0  a                :DataInterfaceType ;
        rdfs:comment      "Maximum speed of 4,8 Gbit/s."@en ;
        rdfs:label        "USB 3.0"@de , "USB 3.0"@en ;
        :belongsToModule  "MP3Player, TV, Printer, DigitalCamera, Camcorder"@en .

:hasMaxRelativeHumidity
        a                   owl:ObjectProperty ;
        rdfs:comment        "Defines the maximum level of relative humidity, non-condensing, within which the product can operate."@en ;
        rdfs:isDefinedBy    <http://www.ebusiness-unibw.org/ontologies/consumerelectronics/v1> ;
        rdfs:label          "max relative humidity"@en , "maximale Luftfeuchtigkeit"@de ;
        rdfs:range          gr:QuantitativeValueFloat ;
        rdfs:subPropertyOf  gr:quantitativeProductOrServiceProperty ;
        :belongsToModule    "TV, Printer"@en .

:RGB    a                 :Connectivity ;
        rdfs:comment      "The RGB color model is an additive color model in which red, green, and blue light are added together in various ways to reproduce a broad array of colors. The name of the model comes from the initials of the three additive primary colors, red, green, and blue. Typical RGB input devices are color TV and video cameras, image scanners, and digital cameras. Typical RGB output devices are TV sets of various technologies (CRT, LCD, plasma, etc.), computer and mobile phone displays, video projectors, multicolor LED displays, and large screens as JumboTron, etc. Color printers, on the other hand, are usually not RGB devices, but subtractive color devices (typically CMYK color model).\n\n(This description is partly based on or reuses content from the Wikipedia article \"RGB\" (http://en.wikipedia.org/wiki/RGB) and is licensed under the GNU Free Documentation License (http://www.gnu.org/copyleft/fdl.html).)"@en ;
        rdfs:label        "RGB"@de , "RGB"@en ;
        :belongsToModule  "TV"@en .

:Memup  a                 gr:BusinessEntity ;
        rdfs:comment      "The business entity Modul Burotic SAS."@en ;
        rdfs:label        "Memup"^^xsd:string ;
        rdfs:seeAlso      <http://www.memup.de/> ;
        gr:legalName      "Modul Burotic SAS "^^xsd:string ;
        :belongsToModule  "MP3Player"@en .

:Asus   a                 gr:BusinessEntity ;
        rdfs:comment      "The business entity Asus."@en ;
        rdfs:label        "Asus"^^xsd:string ;
        rdfs:seeAlso      <http://www.asus.com/> ;
        gr:legalName      "ASUSTeK Computer Inc."^^xsd:string ;
        :belongsToModule  "TV"@en .

:Clock  a                 :Features ;
        rdfs:comment      "Can display the current time."@en ;
        rdfs:label        "Uhr"@de , "Clock"@en ;
        :belongsToModule  "MP3Player"@en .

dc:subject  a   owl:AnnotationProperty .

:PixelPlusHD  a           :VideoFeatures ;
        rdfs:comment      "Pixel Plus HD is a picture processing technology that enables viewers to watch content that is vivid, natural and real."@en ;
        rdfs:label        "Pixel Plus HD"@de , "Pixel Plus HD"@en ;
        :belongsToModule  "TV"@en .

:TVDisplayResolution  a   owl:Class ;
        rdfs:comment      "The display resolution of a digital television or display typically refers to the number of distinct pixels in each dimension that can be displayed.\n\n(This description is partly based on or reuses content from the Wikipedia article \"Display resolution\" (http://en.wikipedia.org/wiki/Display_resolution) and is licensed under the GNU Free Documentation License (http://www.gnu.org/copyleft/fdl.html).)"^^xsd:string ;
        rdfs:isDefinedBy  <http://www.ebusiness-unibw.org/ontologies/consumerelectronics/v1> ;
        rdfs:label        "TV display resolution"@en , "Fernsehbildschirmauflösung"@de ;
        rdfs:subClassOf   :SupportedResolution ;
        :belongsToModule  "TV"@en .

:PackardBell  a           gr:BusinessEntity ;
        rdfs:comment      "The business entity Packard Bell."@en ;
        rdfs:label        "Packard Bell"^^xsd:string ;
        rdfs:seeAlso      <http://www.packardbell.com/> ;
        gr:legalName      "Packard Bell"^^xsd:string ;
        :belongsToModule  "MP3Player, TV"@en .

:Nokia  a                 gr:BusinessEntity ;
        rdfs:comment      "The business entity Nokia Corporation."@en ;
        rdfs:label        "Nokia"^^xsd:string ;
        rdfs:seeAlso      <http://www.nokia.com/> ;
        gr:legalName      "Nokia Corporation"^^xsd:string ;
        :belongsToModule  "DigitalCamera"@en .

:hasMaxColorPrintSpeedBestQuality
        a                   owl:ObjectProperty ;
        rdfs:comment        "Amount of pages per minute the product is able to print in the mode of color-printig best quality."@en ;
        rdfs:isDefinedBy    <http://www.ebusiness-unibw.org/ontologies/consumerelectronics/v1> ;
        rdfs:label          "max color print speed best quality"@en , "maximale Druckgeschwindigkeit Farbe beste Qualität"@de ;
        rdfs:range          gr:QuantitativeValueFloat ;
        rdfs:subPropertyOf  gr:quantitativeProductOrServiceProperty ;
        :belongsToModule    "Printer"@en .

:NiCd   a                 :RechargeableEnergySource ;
        rdfs:comment      "A type of rechargeable battery using nickel oxide hydroxide and metallic cadmium as electrodes.\n\n(This description is partly based on or reuses content from the Wikipedia article \"Nickel-cadmium battery\" (http://en.wikipedia.org/wiki/Nickel-cadmium_battery) and is licensed under the GNU Free Documentation License (http://www.gnu.org/copyleft/fdl.html).)"@en ;
        rdfs:label        "NiCd"@de , "NiCd"@en ;
        :belongsToModule  "MP3Player, DigitalCamera, Camcorder"@en .

:MP3    a                 :DataFormatAudio ;
        rdfs:comment      "A digital audio encoding format using a form of lossy data compression."@en ;
        rdfs:label        "MP3"@de , "MP3"@en ;
        :belongsToModule  "MP3Player, DigitalCamera, Camcorder"@en .

:DVB-T  a                 :GeneralFeatures ;
        rdfs:comment      "DVB-T is an abbreviation for Digital Video Broadcasting - Terrestrial; it is the DVB European-based consortium standard for the broadcast transmission of digital terrestrial television. This system transmits compressed digital audio, video and other data in an MPEG transport stream, using COFDM modulation.\n\n(This description is partly based on or reuses content from the Wikipedia article \"DVB-T\" (http://en.wikipedia.org/wiki/DVB-T) and is licensed under the GNU Free Documentation License (http://www.gnu.org/copyleft/fdl.html).)"@en ;
        rdfs:label        "DVB-T"@de , "DVB-T"@en ;
        :belongsToModule  "TV"@en .

:TeletextFunction  a      :GeneralFeatures ;
        rdfs:comment      "Teletext (or \"broadcast Teletext\") is a television information retrieval service developed in the United Kingdom in the early 1970s. It offers a range of text-based information, typically including national, international and sporting news, weather and TV schedules.\n\n(This description is partly based on or reuses content from the Wikipedia article \"Teletext\" (http://en.wikipedia.org/wiki/Teletext) and is licensed under the GNU Free Documentation License (http://www.gnu.org/copyleft/fdl.html).)"@en ;
        rdfs:label        "Teletext function"@en , "Teletext Funktion"@de ;
        :belongsToModule  "TV"@en .

:Spotlight  a             :SceneMode ;
        rdfs:comment      "Ability of the camcorder to adapt to special environments."@en ;
        rdfs:label        "Spotlight"@en , "Spotlight"@de ;
        :belongsToModule  "Camcorder"@en .

:Hitachi  a               gr:BusinessEntity ;
        rdfs:comment      "The business entity Hitachi."@en ;
        rdfs:label        "Hitachi"^^xsd:string ;
        rdfs:seeAlso      <http://www.hitachidigitalmedia.com/> ;
        gr:legalName      "HITACHI Digital Media"^^xsd:string ;
        :belongsToModule  "TV, DigitalCamera, Camcorder"@en .

:hasSelfTimer  a            owl:DatatypeProperty ;
        rdfs:comment        "Defines whether the product is able  to give a delay between the pressing of the shutter release and the shutter firing."@en ;
        rdfs:isDefinedBy    <http://www.ebusiness-unibw.org/ontologies/consumerelectronics/v1> ;
        rdfs:label          "self-timer"@en , "Selbstauslöser"@de ;
        rdfs:range          xsd:boolean ;
        rdfs:subPropertyOf  gr:datatypeProductOrServiceProperty ;
        :belongsToModule    "DigitalCamera"@en .

:Sharp  a                 gr:BusinessEntity ;
        rdfs:comment      "The business entity Sharp."@en ;
        rdfs:label        "Sharp"^^xsd:string ;
        rdfs:seeAlso      <http://www.sharp-world.com/> ;
        gr:legalName      "Sharp Corporation"^^xsd:string ;
        :belongsToModule  "TV"@en .

:Yukai  a                 gr:BusinessEntity ;
        rdfs:comment      "The business entity Yukai."@en ;
        rdfs:label        "Yukai"^^xsd:string ;
        rdfs:seeAlso      <http://www.yukai.eu/> ;
        gr:legalName      "Mustek Optic-Computer and Communication International GmbH"^^xsd:string ;
        :belongsToModule  "Camcorder"@en .

:VoiceRecording  a        :Features ;
        rdfs:comment      "Ability to record sounds with a micro."@en ;
        rdfs:label        "Voicerecorder"@en , "Voicerekorder"@de ;
        :belongsToModule  "MP3Player, DigitalCamera"@en .

:Pioneer  a               gr:BusinessEntity ;
        rdfs:comment      "The business entity Pioneer."@en ;
        rdfs:label        "Pioneer"^^xsd:string ;
        rdfs:seeAlso      <http://pioneer.jp/> ;
        gr:legalName      "Pioneer Corporation"^^xsd:string ;
        :belongsToModule  "TV"@en .

:HDTV_1080p  a            :TVDisplayResolution ;
        rdfs:comment      "1080p is the shorthand name for a category of HDTV video modes. The number \"1080\" represents 1,080 lines of vertical resolution (1080 horizontal scan lines), while the letter p stands for progressive scan (meaning the image is not interlaced). 1080p can be referred to as full HD or full high definition to differentiate it from other HDTV video modes.\n\n(This description is partly based on or reuses content from the Wikipedia article \"1080p\" (http://en.wikipedia.org/wiki/1080p) and is licensed under the GNU Free Documentation License (http://www.gnu.org/copyleft/fdl.html).)"@en ;
        rdfs:label        "HDTV 1080p"@en , "HDTV 1080p"@de ;
        :belongsToModule  "TV"@en .

:B6     a                 :MediaFormat ;
        rdfs:comment      "Format of the german institute for standardization: 125 x 176 mm."@en ;
        rdfs:label        "B6"@en , "B6"@de ;
        :belongsToModule  "Printer"@en .

:hasMaxOutputCapacity
        a                   owl:ObjectProperty ;
        rdfs:comment        "Maximum number of sheets the product can hold in all available standard and optional output trays."@en ;
        rdfs:isDefinedBy    <http://www.ebusiness-unibw.org/ontologies/consumerelectronics/v1> ;
        rdfs:label          "max output capacity"@en , "maximale Größe Ausgabefach"@de ;
        rdfs:range          gr:QuantitativeValueInteger ;
        rdfs:subPropertyOf  gr:quantitativeProductOrServiceProperty ;
        :belongsToModule    "Printer"@en .

:RechargeableEnergySource
        a                 owl:Class ;
        rdfs:comment      "A rechargeable battery is a kind of energy source that is able to be reused by refilling it with a charger."@en ;
        rdfs:isDefinedBy  <http://www.ebusiness-unibw.org/ontologies/consumerelectronics/v1> ;
        rdfs:label        "Rechargeable Energy Source"@en , "Wiederaufladbare Energiequelle"@de ;
        rdfs:subClassOf   :EnergySource ;
        :belongsToModule  "MP3Player, DigitalCamera, Camcorder"@en .

:hasProcessorType  a        owl:ObjectProperty ;
        rdfs:comment        "The type of central processing unit (CPU) as an electronic circuit that can execute printing tasks or programs."@en ;
        rdfs:isDefinedBy    <http://www.ebusiness-unibw.org/ontologies/consumerelectronics/v1> ;
        rdfs:label          "processor type"@en , "Prozessorart"@de ;
        rdfs:range          :ProcessorType ;
        rdfs:subPropertyOf  gr:qualitativeProductOrServiceProperty ;
        :belongsToModule    "Printer"@en .

:FLAC   a                 :DataFormatAudio ;
        rdfs:comment      "Free Lossless Audio Codec (FLAC) is a file format for lossless audio data compression.\n\n(This description is partly based on or reuses content from the Wikipedia article \"Free Lossless Audio Codec\" (http://en.wikipedia.org/wiki/Free_Lossless_Audio_Codec) and is licensed under the GNU Free Documentation License (http://www.gnu.org/copyleft/fdl.html).)"@en ;
        rdfs:label        "FLAC"@de , "FLAC"@en ;
        :belongsToModule  "MP3Player, DigitalCamera, Camcorder"@en .

:FaceIdendification  a    :Features ;
        rdfs:comment      "Ability to identify the face and to justify the picture to it."@en ;
        rdfs:label        "Face identification"@en , "Gesichtserkennung"@de ;
        :belongsToModule  "DigitalCamera, Camcorder"@en .

:hasZoom  a                 owl:ObjectProperty ;
        rdfs:comment        "Zoom is a method of decreasing (narrowing) the apparent angle of view of a photographic or video image.\n\n(This description is partly based on or reuses content from the Wikipedia article \"Digital zoom\" (http://en.wikipedia.org/wiki/Digital_zoom) and is licensed under the GNU Free Documentation License (http://www.gnu.org/copyleft/fdl.html).)"@en ;
        rdfs:isDefinedBy    <http://www.ebusiness-unibw.org/ontologies/consumerelectronics/v1> ;
        rdfs:label          "zoom"@en , "Zoom"@de ;
        rdfs:range          :Zoom ;
        rdfs:subPropertyOf  gr:qualitativeProductOrServiceProperty ;
        :belongsToModule    "DigitalCamera, Camcorder"@en .

:Linux  a                 :CompatibleOperatingSystems ;
        rdfs:comment      "Linux is a generic term commonly used to refer to Unix-like computer operating systems which use the Linux kernel."@en ;
        rdfs:label        "Linux"@de , "Linux"@en ;
        :belongsToModule  "MP3Player, Printer, DigitalCamera, Camcorder"@en .

:DVI_in  a                :DataInterfaceType ;
        rdfs:comment      "A digital video format created by Sony, JVC, Panasonic and other video camera producers."@en ;
        rdfs:label        "DV in"@en , "DV in"@de ;
        :belongsToModule  "Camcorder"@en .

:InternalHDD  a           :StorageMedia ;
        rdfs:comment      "Hard disk drive, a computer device which stores digitally encoded data."@en ;
        rdfs:label        "Internal HDD"@en , "Interne HDD"@de ;
        :belongsToModule  "MP3Player, DigitalCamera, Camcorder"@en .

:Sapphire  a              gr:BusinessEntity ;
        rdfs:comment      "The business entity Sapphire Technology Limited"@en ;
        rdfs:label        "Sapphire"^^xsd:string ;
        rdfs:seeAlso      <http://www.sapphiretech.com/> ;
        gr:legalName      "Sapphire Technology Limited"^^xsd:string ;
        :belongsToModule  "MP3Player"@en .

dc:creator  a   owl:AnnotationProperty .

:hasPackageWeight  a        owl:ObjectProperty ;
        rdfs:comment        "Defines the measurement of the gravitational force acting on an object with its package (Common unit of measurement gramm, GRM)."@en ;
        rdfs:isDefinedBy    <http://www.ebusiness-unibw.org/ontologies/consumerelectronics/v1> ;
        rdfs:label          "package weight"@en , "Verpackungsgewicht"@de ;
        rdfs:range          gr:QuantitativeValueFloat ;
        rdfs:subPropertyOf  gr:quantitativeProductOrServiceProperty ;
        :belongsToModule    "TV"@en .

:MacOSXPanther  a         :CompatibleOperatingSystems ;
        rdfs:comment      "Mac OS is the trademarked name for a series of graphical user interface-based operating systems developed by Apple Inc. for their Macintosh line of computer systems."@en ;
        rdfs:label        "Mac OS X Panther"@de , "Mac OS X Panther"@en ;
        :belongsToModule  "MP3Player, Printer, DigitalCamera, Camcorder"@en .

:MulticoloredBody  a      :Color ;
        rdfs:comment      "The body of the Product has more than one color."@en ;
        rdfs:label        "multicolored"@en , "Mehrfarbig"@de ;
        :belongsToModule  "MP3Player, TV, Printer, DigitalCamera, Camcorder"@en .

:hasMaxBlackWhitePrintSpeedNormal
        a                   owl:ObjectProperty ;
        rdfs:comment        "Amount of pages per minute the product is able to print in the mode of black-printig normal quality."@en ;
        rdfs:isDefinedBy    <http://www.ebusiness-unibw.org/ontologies/consumerelectronics/v1> ;
        rdfs:label          "max black white print speed draft"@en , "maximale Druckgeschwindigkeit Schwarz/Weiß normal"@de ;
        rdfs:range          gr:QuantitativeValueFloat ;
        rdfs:subPropertyOf  gr:quantitativeProductOrServiceProperty ;
        :belongsToModule    "Printer"@en .

:LCD    a                 :DisplayType ;
        rdfs:comment      "A liquid crystal display (LCD) is an electronically-modulated optical device shaped into a thin, flat panel made up of any number of color or monochrome pixels filled with liquid crystals and arrayed in front of a light source (backlight) or reflector.\n\n(This description is partly based on or reuses content from the Wikipedia article \"Liquid crystal display\" (http://en.wikipedia.org/wiki/Liquid_crystal_display) and is licensed under the GNU Free Documentation License (http://www.gnu.org/copyleft/fdl.html).)"@en ;
        rdfs:label        "LCD"@de , "LCD"@en ;
        :belongsToModule  "TV, Camcorder"@en .

:hasEconomicPrintMode
        a                   owl:DatatypeProperty ;
        rdfs:comment        "Describes whether or not the product is equipped with features that allow economical printing."@en ;
        rdfs:isDefinedBy    <http://www.ebusiness-unibw.org/ontologies/consumerelectronics/v1> ;
        rdfs:label          "economic print mode"@en , "Energiespardruckmodus"@de ;
        rdfs:range          xsd:boolean ;
        rdfs:subPropertyOf  gr:datatypeProductOrServiceProperty ;
        :belongsToModule    "Printer"@en .

:V7     a                 gr:BusinessEntity ;
        rdfs:comment      "The business entity Videoseven."@en ;
        rdfs:label        "V7"^^xsd:string ;
        rdfs:seeAlso      <http://www.v7-world.com/> ;
        gr:legalName      "V7"^^xsd:string ;
        :belongsToModule  "TV"@en .

:hasNumberOfOnScreenLanguages
        a                   owl:ObjectProperty ;
        rdfs:comment        "Defines the available languages that can be chosen to be displayed on the main screen of a device."@en ;
        rdfs:isDefinedBy    <http://www.ebusiness-unibw.org/ontologies/consumerelectronics/v1> ;
        rdfs:label          "number of on screen languages"@en , "Anzahl von verfügbaren Sprachen"@de ;
        rdfs:range          gr:QuantitativeValueInteger ;
        rdfs:subPropertyOf  gr:quantitativeProductOrServiceProperty ;
        :belongsToModule    "TV"@en .

:Orange  a                :Color ;
        rdfs:comment      "RGB Value 255,165,0"@en ;
        rdfs:label        "Orange"@de , "Orange"@en ;
        :belongsToModule  "MP3Player, TV, Printer, DigitalCamera, Camcorder"@en .

:WindowsME  a             :CompatibleOperatingSystems ;
        rdfs:comment      "A version of a Microsoft operating system."@en ;
        rdfs:label        "Windows ME"@de , "Windows ME"@en ;
        :belongsToModule  "MP3Player, Printer, DigitalCamera, Camcorder"@en .

:Acuity  a                :VideoFeatures ;
        rdfs:comment      "Is acuteness or clearness of vision, especially form vision, which is dependent on the sharpness of the retinal focus within the eye and the sensitivity of the interpretative faculty of the brain.\n\n(This description is partly based on or reuses content from the Wikipedia article \"Visual acuity\" (http://en.wikipedia.org/wiki/Visual_acuity) and is licensed under the GNU Free Documentation License (http://www.gnu.org/copyleft/fdl.html).)"@en ;
        rdfs:label        "Acuity"@en , "Acuity"@de ;
        :belongsToModule  "TV"@en .

:IncredibleSurround  a    :AudioFeatures ;
        rdfs:comment      "Psycho-acoustic method of widening the stereo spatial image especially suited for applications with limited separation of left and right speakers."@en ;
        rdfs:label        "Incredible Surround"@de , "Incredible Surround"@en ;
        :belongsToModule  "TV"@en .

:CompactFlash  a          :StorageMedia ;
        rdfs:comment      "CompactFlash (CF) is a mass storage device format used in portable electronic devices. For storage, CompactFlash typically uses flash memory in a standardized enclosure.\n\n(This description is partly based on or reuses content from the Wikipedia article \"CompactFlash\" (http://en.wikipedia.org/wiki/CompactFlash) and is licensed under the GNU Free Documentation License (http://www.gnu.org/copyleft/fdl.html).)"@en ;
        rdfs:label        "CompactFlash"@en , "CompactFlash"@de ;
        :belongsToModule  "MP3Player, DigitalCamera, Camcorder"@en .

:MacOSXCheetah  a         :CompatibleOperatingSystems ;
        rdfs:comment      "Mac OS is the trademarked name for a series of graphical user interface-based operating systems developed by Apple Inc. for their Macintosh line of computer systems."@en ;
        rdfs:label        "Mac OS X Cheetah"@de , "Mac OS X Cheetah"@en ;
        :belongsToModule  "MP3Player, Printer, DigitalCamera, Camcorder"@en .

:AutoChannelSearch  a     :GeneralFeatures ;
        rdfs:comment      "Gives an indication of preprogrammed channels for the user of a television so that he does not need to programm it himself."@en ;
        rdfs:label        "Auto channel search"@en , "Automatischer Sendersuchlauf"@de ;
        :belongsToModule  "TV"@en .

:DisplayType  a           owl:Class ;
        rdfs:comment      "A display device is an output device for presentation of information for visual, tactile or auditive reception, acquired, stored, or transmitted in various forms.\n\n(This description is partly based on or reuses content from the Wikipedia article \"Display device\" (http://en.wikipedia.org/wiki/Display_device) and is licensed under the GNU Free Documentation License (http://www.gnu.org/copyleft/fdl.html).)"@en ;
        rdfs:isDefinedBy  <http://www.ebusiness-unibw.org/ontologies/consumerelectronics/v1> ;
        rdfs:label        "Bildschirmtyp"@de , "Display Type"@en ;
        rdfs:subClassOf   gr:QualitativeValue ;
        :belongsToModule  "MP3Player, TV, Printer, Camcorder"@en .

:Silver  a                :Color ;
        rdfs:comment      "RGB Value 192,192,192"@en ;
        rdfs:label        "Silver"@en , "Silber"@de ;
        :belongsToModule  "MP3Player, TV, Printer, DigitalCamera, Camcorder"@en .

:SECAM-B_G  a             :SignalFormat ;
        rdfs:comment      "SECAM, also written SÉCAM (Séquentiel couleur à mémoire, French for \"Sequential Color with Memory\"), is an analog color television system first used in France. SECAM-B/G is used in the Middle East, former East Germany and Greece.\n\n(This description is partly based on or reuses content from the Wikipedia article \"SECAM\" (http://en.wikipedia.org/wiki/SECAM) and is licensed under the GNU Free Documentation License (http://www.gnu.org/copyleft/fdl.html).)"@en ;
        rdfs:label        "SECAM-B G"@de , "SECAM-B G"@en ;
        :belongsToModule  "TV"@en .

:hasBatterySize  a          owl:DatatypeProperty ;
        rdfs:comment        "Defines the size of used energy source. (Use ASIN code here. For more information we refer to http://en.wikipedia.org/wiki/List_of_battery_sizes)"@en ;
        rdfs:isDefinedBy    <http://www.ebusiness-unibw.org/ontologies/consumerelectronics/v1> ;
        rdfs:label          "battery size"@en , "Batteriegröße"@de ;
        rdfs:range          xsd:string ;
        rdfs:subPropertyOf  gr:datatypeProductOrServiceProperty ;
        :belongsToModule    "MP3Player, DigitalCamera, Camcorder"@en .

:MediaFormat  a           owl:Class ;
        rdfs:comment      "Sizes and shapes of the paper."@en ;
        rdfs:isDefinedBy  <http://www.ebusiness-unibw.org/ontologies/consumerelectronics/v1> ;
        rdfs:label        "Medienformat"@de , "Media format"@en ;
        rdfs:subClassOf   gr:QualitativeValue ;
        :belongsToModule  "Printer"@en .

:Focus  a                 owl:Class ;
        rdfs:comment      "A focus, also called an image point, is the point where light rays originating from a point on the object converge.\n\n(This description is partly based on or reuses content from the Wikipedia article \"Focus (optics)\" (http://en.wikipedia.org/wiki/Focus_(optics)) and is licensed under the GNU Free Documentation License (http://www.gnu.org/copyleft/fdl.html).)"@en ;
        rdfs:isDefinedBy  <http://www.ebusiness-unibw.org/ontologies/consumerelectronics/v1> ;
        rdfs:label        "Focus"@en , "Fokus"@de ;
        rdfs:subClassOf   gr:QualitativeValue ;
        :belongsToModule  "DigitalCamera, Camcorder"@en .

:B1     a                 :MediaFormat ;
        rdfs:comment      "Format of the german institute for standardization: 707 x 1000 mm."@en ;
        rdfs:label        "B1"@en , "B1"@de ;
        :belongsToModule  "Printer"@en .

:SMS    a                 gr:BusinessEntity ;
        rdfs:comment      "The business entity SMS."@en ;
        rdfs:label        "SMS"^^xsd:string ;
        rdfs:seeAlso      <http://www.smsprintingngraphics.com/> ;
        gr:legalName      "SMS Printing Graphics"^^xsd:string ;
        :belongsToModule  "Printer"@en .

:Agfa   a                 gr:BusinessEntity ;
        rdfs:comment      "The business entity Agfa-Gevaert N.V."@en ;
        rdfs:label        "Agfa"^^xsd:string ;
        rdfs:seeAlso      <http://www.agfa.com/> ;
        gr:legalName      "Agfa-Gevaert N.V."^^xsd:string ;
        :belongsToModule  "DigitalCamera"@en .

:Ricatech  a              gr:BusinessEntity ;
        rdfs:comment      "The business entity Ricatech B.V."@en ;
        rdfs:label        "Ricatech"^^xsd:string ;
        rdfs:seeAlso      <http://www.ricatech.com/> ;
        gr:legalName      "Ricatech B.V."^^xsd:string ;
        :belongsToModule  "MP3Player"@en .

:hasEqualizer  a            owl:DatatypeProperty ;
        rdfs:comment        "Defines the possibility to vary the audio presentation of sound."@en ;
        rdfs:isDefinedBy    <http://www.ebusiness-unibw.org/ontologies/consumerelectronics/v1> ;
        rdfs:label          "Equalizer"@en , "Equalizer"@de ;
        rdfs:range          xsd:boolean ;
        rdfs:subPropertyOf  gr:datatypeProductOrServiceProperty ;
        :belongsToModule    "MP3Player"@en .

:Acer   a                 gr:BusinessEntity ;
        rdfs:comment      "The business entity Acer, Inc."@en ;
        rdfs:label        "Acer"^^xsd:string ;
        rdfs:seeAlso      <http://www.acer.com/> ;
        gr:legalName      "Acer, Inc"^^xsd:string ;
        :belongsToModule  "MP3Player, TV, DigitalCamera"@en .

:PAL-L  a                 :SignalFormat ;
        rdfs:comment      "PAL, short for Phase Alternating Line, is a colour-encoding system used in broadcast television systems in large parts of the world. PAL L is used on some hotel internal distribution systems, as well as other public display and plant television systems.\n\n(This description is partly based on or reuses content from the Wikipedia article \"PAL\" (http://en.wikipedia.org/wiki/PAL) and is licensed under the GNU Free Documentation License (http://www.gnu.org/copyleft/fdl.html).)"@en ;
        rdfs:label        "PAL-L"@de , "PAL-L"@en ;
        :belongsToModule  "TV"@en .

:ColorPrint  a            :Features ;
        rdfs:comment      "The reproduction of an image or text in color on a paper."@en ;
        rdfs:label        "Farbdruck"@de , "Color print"@en ;
        :belongsToModule  "Printer"@en .

:Techsolo  a              gr:BusinessEntity ;
        rdfs:comment      "The business entity Techsolo Europe B.V."@en ;
        rdfs:label        "Techsolo"^^xsd:string ;
        rdfs:seeAlso      <http://www.techsolo.com/> ;
        gr:legalName      "Techsolo Europe B.V."^^xsd:string ;
        :belongsToModule  "MP3Player"@en .

:TXT    a                 :DataFormatOffice ;
        rdfs:comment      "Is a filename extension for files consisting of text usually contain very little formatting."@en ;
        rdfs:label        "TXT"@de , "TXT"@en ;
        :belongsToModule  "MP3Player, DigitalCamera"@en .

:TakeMS  a                gr:BusinessEntity ;
        rdfs:comment      "The business entity takeMS International AG."@en ;
        rdfs:label        "takeMS"^^xsd:string ;
        rdfs:seeAlso      <http://www.takems.de/> ;
        gr:legalName      "takeMS International AG"^^xsd:string ;
        :belongsToModule  "MP3Player"@en .

:LineInRecorder  a        :Features ;
        rdfs:comment      "Ability to record sounds via cable connection."@en ;
        rdfs:label        "Audioaufnahme"@de , "Line in recorder"@en ;
        :belongsToModule  "MP3Player"@en .

:hasNetworkAbility  a       owl:DatatypeProperty ;
        rdfs:comment        "Ability to connect the product to a network."@en ;
        rdfs:isDefinedBy    <http://www.ebusiness-unibw.org/ontologies/consumerelectronics/v1> ;
        rdfs:label          "network ability"@en , "Netzwerkfähigkeit"@de ;
        rdfs:range          xsd:boolean ;
        rdfs:subPropertyOf  gr:datatypeProductOrServiceProperty .

:hasEnvelopeFeeder  a       owl:DatatypeProperty ;
        rdfs:comment        "Indicates wheter this feature is available on this product."@en ;
        rdfs:isDefinedBy    <http://www.ebusiness-unibw.org/ontologies/consumerelectronics/v1> ;
        rdfs:label          "envelope feeder"@en , "Kuvertzuführeinrichtung"@de ;
        rdfs:range          xsd:boolean ;
        rdfs:subPropertyOf  gr:datatypeProductOrServiceProperty ;
        :belongsToModule    "Printer"@en .

:AudioInterfaceType  a    owl:Class ;
        rdfs:comment      "Interface generally refers to an abstraction that an entity provides of itself to the outside (refers to audio output).\n\n(This description is partly based on or reuses content from the Wikipedia article \"Interface (computer science)\" (http://en.wikipedia.org/wiki/Interface_(computer_science)) and is licensed under the GNU Free Documentation License (http://www.gnu.org/copyleft/fdl.html).)"@en ;
        rdfs:isDefinedBy  <http://www.ebusiness-unibw.org/ontologies/consumerelectronics/v1> ;
        rdfs:label        "Audioschnittstellentyp"@de , "Audio Interface Type"@en ;
        rdfs:subClassOf   gr:QualitativeValue ;
        :belongsToModule  "MP3Player"@en .

:OnScreenDisplay  a       :GeneralFeatures ;
        rdfs:comment      "An on-screen display (abbreviated OSD) is an image superimposed on a screen picture, commonly used by modern televisions, VCRs, and DVD players to display information such as volume, channel, and time.\n\n(This description is partly based on or reuses content from the Wikipedia article \"On-screen display\" (http://en.wikipedia.org/wiki/On-screen_display) and is licensed under the GNU Free Documentation License (http://www.gnu.org/copyleft/fdl.html).)"@en ;
        rdfs:label        "Bildschirmanzeige"@de , "on screen display"@en ;
        :belongsToModule  "TV"@en .

:Bluetooth  a             :DataInterfaceType ;
        rdfs:comment      "Bluetooth is a wireless protocol utilizing short-range communications technology facilitating data transmission over short distances from fixed and mobile devices, creating wireless personal area networks."@en ;
        rdfs:label        "Bluetooth"@de , "Bluetooth"@en ;
        :belongsToModule  "MP3Player, Printer, DigitalCamera, Camcorder"@en .

:hasNormalPrintableResolutionColorHorizontal
        a                   owl:ObjectProperty ;
        rdfs:comment        "Defines the digital resolution of the horizontal axe (Common unit of measurement pixel, E37) for color prints for normal prints."@en ;
        rdfs:isDefinedBy    <http://www.ebusiness-unibw.org/ontologies/consumerelectronics/v1> ;
        rdfs:label          "normal printable resolution color horizontal"@en , "horizontale druckbare Auflösung Farbe normal"@de ;
        rdfs:range          gr:QuantitativeValueInteger ;
        rdfs:subPropertyOf  gr:quantitativeProductOrServiceProperty ;
        :belongsToModule    "Printer"@en .

:Esselte  a               gr:BusinessEntity ;
        rdfs:comment      "The business entity Esselte."@en ;
        rdfs:label        "Esselte"^^xsd:string ;
        rdfs:seeAlso      <http://www.esselte.com/> ;
        gr:legalName      "Esselte Corporation"^^xsd:string ;
        :belongsToModule  "Printer"@en .

:DigitalCrystalClear  a   :VideoFeatures ;
        rdfs:comment      "Digital Crystal Clear is a package of picture innovations that digitally adjusts and optimises picture quality to optimal contrast, colour and sharpness levels."@en ;
        rdfs:label        "Digital Crystal Clear"@de , "Digital Crystal Clear"@en ;
        :belongsToModule  "TV"@en .

:GNR    a                 gr:BusinessEntity ;
        rdfs:comment      "The business entity GNR."@en ;
        rdfs:label        "GNR"^^xsd:string ;
        rdfs:seeAlso      <http://www.gnr.co.uk/> ;
        gr:legalName      "GNR"^^xsd:string ;
        :belongsToModule  "TV"@en .

:FocusAuto  a             :Focus ;
        rdfs:comment      "Autofocus (or AF) is a feature of some optical systems that allows them to obtain (and in some systems to also continuously maintain) correct focus on a subject, instead of requiring the operator to adjust focus manually.\n\n(This description is partly based on or reuses content from the Wikipedia article \"Autofocus\" (http://en.wikipedia.org/wiki/Autofocus) and is licensed under the GNU Free Documentation License (http://www.gnu.org/copyleft/fdl.html).)"@en ;
        rdfs:label        "Focus auto"@en , "Autofokus"@de ;
        :belongsToModule  "DigitalCamera, Camcorder"@en .

:USB1.0  a                :DataInterfaceType ;
        rdfs:comment      "Specified data rates of 1.5 Mbit/s and 12 Mbit/s."@en ;
        rdfs:label        "USB 1.0"@de , "USB 1.0"@en ;
        :belongsToModule  "MP3Player, TV, Printer, DigitalCamera, Camcorder"@en .

:hasWeightWithStand  a      owl:ObjectProperty ;
        rdfs:comment        "Defines the measurement of the gravitational force acting on an object with its stand (Common unit of measurement gramm, GRM)."@en ;
        rdfs:isDefinedBy    <http://www.ebusiness-unibw.org/ontologies/consumerelectronics/v1> ;
        rdfs:label          "weight with stand"@en , "Gewicht mit Standfuß"@de ;
        rdfs:range          gr:QuantitativeValueFloat ;
        rdfs:subPropertyOf  gr:quantitativeProductOrServiceProperty ;
        :belongsToModule    "TV"@en .

:Difrnce  a               gr:BusinessEntity ;
        rdfs:comment      "The business entity DIFRNCE B.V."@en ;
        rdfs:label        "Difrnce"^^xsd:string ;
        rdfs:seeAlso      <http://www.difrnce.nl/> ;
        gr:legalName      "DIFRNCE B.V."^^xsd:string ;
        :belongsToModule  "MP3Player"@en .

:hasNumberOfInputPaperTrays
        a                   owl:ObjectProperty ;
        rdfs:comment        "Counts the trays which feed the printer with paper."@en ;
        rdfs:isDefinedBy    <http://www.ebusiness-unibw.org/ontologies/consumerelectronics/v1> ;
        rdfs:label          "number of input paper trays"@en , "Anzahl an Papierkassetten Zuführung"@de ;
        rdfs:range          gr:QuantitativeValueInteger ;
        rdfs:subPropertyOf  gr:quantitativeProductOrServiceProperty ;
        :belongsToModule    "Printer"@en .

:VIVOTEK  a               gr:BusinessEntity ;
        rdfs:comment      "The business entity VIVOTEK Inc."@en ;
        rdfs:label        "VIVOTEK"^^xsd:string ;
        rdfs:seeAlso      <http://www.vivotek.com/> ;
        gr:legalName      "VIVOTEK Inc."^^xsd:string ;
        :belongsToModule  "DigitalCamera"@en .

:Lit-Ion  a               :RechargeableEnergySource ;
        rdfs:comment      "Type of rechargeable battery in which a lithium ion moves between the anode and cathode.\n\n(This description is partly based on or reuses content from the Wikipedia article \"Lithium ion battery\" (http://en.wikipedia.org/wiki/Lithium_ion_battery) and is licensed under the GNU Free Documentation License (http://www.gnu.org/copyleft/fdl.html).)"@en ;
        rdfs:label        "Lit-Ion"@de , "Lit-Ion"@en ;
        :belongsToModule  "MP3Player, DigitalCamera, Camcorder"@en .

:Creative_Labs  a         gr:BusinessEntity ;
        rdfs:comment      "The business entity Creative Technology Limited."@en ;
        rdfs:label        "Creative Labs"^^xsd:string ;
        rdfs:seeAlso      <http://www.creative.com/> ;
        gr:legalName      "Creative Technology Limited"^^xsd:string ;
        :belongsToModule  "MP3Player, DigitalCamera, Camcorder"@en .

:CompatibleOperatingSystems
        a                 owl:Class ;
        rdfs:comment      "Ability to communicate with different kinds of operating systems."@en ;
        rdfs:isDefinedBy  <http://www.ebusiness-unibw.org/ontologies/consumerelectronics/v1> ;
        rdfs:label        "Compatible Operating Systems"@en , "Kompatible Betriebssyteme"@de ;
        rdfs:subClassOf   gr:QualitativeValue ;
        :belongsToModule  "MP3Player, Printer, DigitalCamera, Camcorder"@en .

:CombFilter  a            :VideoFeatures ;
        rdfs:comment      "In signal processing, a comb filter adds a delayed version of a signal to itself, causing constructive and destructive interference. The frequency response of a comb filter consists of a series of regularly-spaced spikes, giving the appearance of a comb.\n\n(This description is partly based on or reuses content from the Wikipedia article \"Comb filter\" (http://en.wikipedia.org/wiki/Comb_filter) and is licensed under the GNU Free Documentation License (http://www.gnu.org/copyleft/fdl.html).)"@en ;
        rdfs:label        "Comb Filter"@de , "Comb filter"@en ;
        :belongsToModule  "TV"@en .

:USBEnergyInterface  a    :USB ;
        rdfs:comment      "USB-interface used to provide power to low-consumption devices without the need for an external power supply."@en ;
        rdfs:label        "USB Stromschnittstelle"@de , "USB energy interface"@en ;
        :belongsToModule  "MP3Player, Printer, DigitalCamera"@en .

:MPMAN  a                 gr:BusinessEntity ;
        rdfs:comment      "The business entity MPMAN Europe."@en ;
        rdfs:label        "MPAN"^^xsd:string ;
        rdfs:seeAlso      <http://www.mpmaneurope.com/> ;
        gr:legalName      "MPMAN Europe"^^xsd:string ;
        :belongsToModule  "MP3Player"@en .

:Sports  a                :SceneMode ;
        rdfs:comment      "Ability of the camcorder to adapt to special environments."@en ;
        rdfs:label        "Sports"@en , "Sport"@en ;
        :belongsToModule  "Camcorder"@en .

:PowerSupplyUnit  a       owl:Class ;
        rdfs:comment      "A Power Supply Adapter is used to convert 120 or 240 volt AC supplied by a utility company to a well-regulated lower voltage DC for electronic devices.\n\n(This description is partly based on or reuses content from the Wikipedia article \"Power supply\" (http://en.wikipedia.org/wiki/Power_supply) and is licensed under the GNU Free Documentation License (http://www.gnu.org/copyleft/fdl.html).)"@en ;
        rdfs:isDefinedBy  <http://www.ebusiness-unibw.org/ontologies/consumerelectronics/v1> ;
        rdfs:label        "Netzgerät"@de , "Power Supply Unit"@en ;
        rdfs:subClassOf   :EnergySource ;
        :belongsToModule  "MP3Player, Printer, DigitalCamera, Camcorder"@en .

:AudioInput  a            :Features ;
        rdfs:comment      "Defines the support of a computer soundcard driver protocol for digital audio specified by Steinberg, providing a low-latency and high fidelity interface between a software application and a computer's sound card."@en ;
        rdfs:label        "Audioeingang"@de , "Audio input"@en ;
        :belongsToModule  "Camcorder"@en .

:Transcend  a             gr:BusinessEntity ;
        rdfs:comment      "The business entity Transcend Information, Inc."@en ;
        rdfs:label        "Transcend"^^xsd:string ;
        rdfs:seeAlso      <http://www.transcendusa.com/> ;
        gr:legalName      "Transcend Information, Inc. "^^xsd:string ;
        :belongsToModule  "MP3Player"@en .

:ATEC   a                 gr:BusinessEntity ;
        rdfs:comment      "The business entity ATEC."@en ;
        rdfs:label        "ATEC"^^xsd:string ;
        gr:legalName      "ATEC"^^xsd:string ;
        :belongsToModule  "TV"@en .

:hasNumberOfStandardInputTrays
        a                   owl:ObjectProperty ;
        rdfs:comment        "Defines the number of trays able to hold sheets of paper to be printed."@en ;
        rdfs:isDefinedBy    <http://www.ebusiness-unibw.org/ontologies/consumerelectronics/v1> ;
        rdfs:label          "number of standard input trays"@en , "Anzahl an Standard Papierkassetten"@de ;
        rdfs:range          gr:QuantitativeValueInteger ;
        rdfs:subPropertyOf  gr:quantitativeProductOrServiceProperty ;
        :belongsToModule    "Printer"@en .

:Sony   a                 gr:BusinessEntity ;
        rdfs:comment      "The business entity Sony Corporation"@en ;
        rdfs:label        "Sony"^^xsd:string ;
        rdfs:seeAlso      <http://www.sony.com/> ;
        gr:legalName      "Sony Corporation "^^xsd:string ;
        :belongsToModule  "MP3Player, TV, DigitalCamera, Camcorder"@en .

:EconomicalMode  a        :Features ;
        rdfs:comment      "Equipment that allows economical printing."@en ;
        rdfs:label        "Energiesparmodus"@de , "Economical mode"@en ;
        :belongsToModule  "Printer"@en .

:DataInterfaceType  a     owl:Class ;
        rdfs:comment      "Interface generally refers to an abstraction that an entity provides of itself to the outside.\n\n(This description is partly based on or reuses content from the Wikipedia article \"Interface (computer science)\" (http://en.wikipedia.org/wiki/Interface_(computer_science)) and is licensed under the GNU Free Documentation License (http://www.gnu.org/copyleft/fdl.html).)"@en ;
        rdfs:isDefinedBy  <http://www.ebusiness-unibw.org/ontologies/consumerelectronics/v1> ;
        rdfs:label        "Datenschnittstellentyp"@de , "Data Interface Type"@en ;
        rdfs:subClassOf   gr:QualitativeValue ;
        :belongsToModule  "MP3Player, Printer, DigitalCamera, Camcorder"@en .

:VideoComponent_Cable
        a                 :Accessory ;
        rdfs:comment      "A video signal that has been split into two or more components."@en ;
        rdfs:label        "Video component cable"@en , "Videokomponentenkabel"@de ;
        :belongsToModule  "Camcorder"@en .

:hasMaxBlackWhitePrintSpeedDraft
        a                   owl:ObjectProperty ;
        rdfs:comment        "Amount of pages per minute the product is able to print in the mode of black-printig of drafts."@en ;
        rdfs:isDefinedBy    <http://www.ebusiness-unibw.org/ontologies/consumerelectronics/v1> ;
        rdfs:label          "max black white print speed draft"@en , "maximale Druckgeschwindigkeit schwarz/weiß Entwurf"@de ;
        rdfs:range          gr:QuantitativeValueFloat ;
        rdfs:subPropertyOf  gr:quantitativeProductOrServiceProperty ;
        :belongsToModule    "Printer"@en .

:TIFF   a                 :DataFormatImage ;
        rdfs:comment      "The TIFF (Tagged Image File Format) is a flexible format that normally saves 8 bits or 16 bits per color (red, green, blue) for 24-bit and 48-bit totals, respectively, using either the TIFF or the TIF filenames.\n\n(This description is partly based on or reuses content from the Wikipedia article \"Graphics file format\" (http://en.wikipedia.org/wiki/Graphics_file_format) and is licensed under the GNU Free Documentation License (http://www.gnu.org/copyleft/fdl.html).)"@en ;
        rdfs:label        "TIFF"@de , "TIFF"@en ;
        :belongsToModule  "MP3Player, DigitalCamera, Camcorder"@en .

:hasExpansionSlot  a        owl:DatatypeProperty ;
        rdfs:comment        "Defines the ability to add devices (e.g. cards) to maximize the storage capacity."@en ;
        rdfs:isDefinedBy    <http://www.ebusiness-unibw.org/ontologies/consumerelectronics/v1> ;
        rdfs:label          "expansion slot"@en , "Erweiterungsplätze"@de ;
        rdfs:range          xsd:boolean ;
        rdfs:subPropertyOf  gr:datatypeProductOrServiceProperty ;
        :belongsToModule    "Camcorder"@en .

dc:contributor  a  owl:AnnotationProperty .

:hasMaxPrintableResolutionColorHorizontal
        a                   owl:ObjectProperty ;
        rdfs:comment        "Defines the maximum digital resolution of the horizontal axe (Common unit of measurement pixel, E37) for color prints."@en ;
        rdfs:isDefinedBy    <http://www.ebusiness-unibw.org/ontologies/consumerelectronics/v1> ;
        rdfs:label          "max printable resolution color horizontal"@en , "maximale horizontale druckbare Auflösung Farbe"@de ;
        rdfs:range          gr:QuantitativeValueInteger ;
        rdfs:subPropertyOf  gr:quantitativeProductOrServiceProperty ;
        :belongsToModule    "Printer"@en .

:Typhoon  a               gr:BusinessEntity ;
        rdfs:comment      "The business entity COS Distribution GmbH"@en ;
        rdfs:label        "Typhoon"^^xsd:string ;
        rdfs:seeAlso      <http://www.typhoon.de/> ;
        gr:legalName      "COS Distribution GmbH"^^xsd:string ;
        :belongsToModule  "MP3Player"@en .

:A5     a                 :MediaFormat ;
        rdfs:comment      "Format of the german institute for standardization: 148 x 210 mm."@en ;
        rdfs:label        "A5"@en , "A5"@de ;
        :belongsToModule  "Printer"@en .

:hasFocusSize  a            owl:ObjectProperty ;
        rdfs:comment        "Focus, also called an image point, is the point where light rays originating from a point on the object converge.\n\n(This description is partly based on or reuses content from the Wikipedia article \"Focus (optics)\" (http://en.wikipedia.org/wiki/Focus_(optics)) and is licensed under the GNU Free Documentation License (http://www.gnu.org/copyleft/fdl.html).)"@en ;
        rdfs:isDefinedBy    <http://www.ebusiness-unibw.org/ontologies/consumerelectronics/v1> ;
        rdfs:label          "focus size"@en , "Fokusgröße"@de ;
        rdfs:range          gr:QuantitativeValueFloat ;
        rdfs:subPropertyOf  gr:quantitativeProductOrServiceProperty ;
        :belongsToModule    "Camcorder"@en .

:Lavod  a                 gr:BusinessEntity ;
        rdfs:comment      "The business entity LAVOD CORPORATION."@en ;
        rdfs:label        "Lavod"^^xsd:string ;
        rdfs:seeAlso      <http://www.lavod.com/> ;
        gr:legalName      "LAVOD CORPOPATION"^^xsd:string ;
        :belongsToModule  "MP3Player"@en .

:hasMaxInternalMemoryCapacity
        a                   owl:ObjectProperty ;
        rdfs:comment        "Defines the maximum amount of memory that can be installed in the systems hardware (common unit of measurement: megabyte(MB): 4L)."@en ;
        rdfs:isDefinedBy    <http://www.ebusiness-unibw.org/ontologies/consumerelectronics/v1> ;
        rdfs:label          "max internal memory capacity"@en , "maximaler interner Speicherplatz"@de ;
        rdfs:range          gr:QuantitativeValueFloat ;
        rdfs:subPropertyOf  gr:quantitativeProductOrServiceProperty ;
        :belongsToModule    "Printer"@en .

:Haier  a                 gr:BusinessEntity ;
        rdfs:comment      "The business entity Haier."@en ;
        rdfs:label        "Haier"^^xsd:string ;
        rdfs:seeAlso      <http://www.haier.com/> ;
        gr:legalName      "Haier Group"^^xsd:string ;
        :belongsToModule  "TV"@en .

:Verbatim  a              gr:BusinessEntity ;
        rdfs:comment      "The business entity Verbatim Corporation."@en ;
        rdfs:label        "Verbatim"^^xsd:string ;
        rdfs:seeAlso      <http://www.verbatim.com/> ;
        gr:legalName      "Verbatim Corporation "^^xsd:string ;
        :belongsToModule  "MP3Player"@en .

:VideoPlayBack  a         :Features ;
        rdfs:comment      "Ability to display video files."@en ;
        rdfs:label        "Videowiedergabe"@de , "Video play back"@en ;
        :belongsToModule  "MP3Player"@en .

:WindowsNT  a             :CompatibleOperatingSystems ;
        rdfs:comment      "A version of a Microsoft operating system."@en ;
        rdfs:label        "Windows NT"@de , "Windows NT"@en ;
        :belongsToModule  "MP3Player, Printer, DigitalCamera, Camcorder"@en .

:Akai   a                 gr:BusinessEntity ;
        rdfs:comment      "The business entity Akai."@en ;
        rdfs:label        "Akai"^^xsd:string ;
        rdfs:seeAlso      <http://www.akai.com/> ;
        gr:legalName      "Akai"^^xsd:string ;
        :belongsToModule  "MP3Player, TV"@en .

:Vestel  a                gr:BusinessEntity ;
        rdfs:comment      "The business entity Vestel."@en ;
        rdfs:label        "Vestel"^^xsd:string ;
        rdfs:seeAlso      <http://www.vestel.com/> ;
        gr:legalName      "Vestel Electronics"^^xsd:string ;
        :belongsToModule  "TV"@en .

:hasMaxMediaFormat  a       owl:ObjectProperty ;
        rdfs:comment        "Defines the maximum size of the printed media format."@en ;
        rdfs:isDefinedBy    <http://www.ebusiness-unibw.org/ontologies/consumerelectronics/v1> ;
        rdfs:label          "max media format"@en , "maximale Mediengröße"@de ;
        rdfs:range          :MediaFormat ;
        rdfs:subPropertyOf  gr:qualitativeProductOrServiceProperty ;
        :belongsToModule    "Printer"@en .

:SleepTimer  a            :GeneralFeatures ;
        rdfs:comment      "A sleep timer is a function on many modern televisions that shut off the power after a preset amount of time. The setting is usually made either from the remote control or the television menus. They are intended to allow viewers to watch as they fall asleep.\n\n(This description is partly based on or reuses content from the Wikipedia article \"Sleep timer\" (http://en.wikipedia.org/wiki/Sleep_timer) and is licensed under the GNU Free Documentation License (http://www.gnu.org/copyleft/fdl.html).)"@en ;
        rdfs:label        "Schlafzeitgeber"@de , "Sleep timer"@en ;
        :belongsToModule  "TV"@en .

:hasPowerRequirementsHTZ
        a                   owl:ObjectProperty ;
        rdfs:comment        "Defines the power requirements of an electronical device (Common unit of measurement hertz, HTZ)."@en ;
        rdfs:isDefinedBy    <http://www.ebusiness-unibw.org/ontologies/consumerelectronics/v1> ;
        rdfs:label          "power requirements HTZ"@en , "Strombedarf HTZ"@de ;
        rdfs:range          gr:QuantitativeValueFloat ;
        rdfs:subPropertyOf  gr:quantitativeProductOrServiceProperty .

:hasDraftPrintableResolutionBlackWhiteVertical
        a                   owl:ObjectProperty ;
        rdfs:comment        "Defines the digital resolution of the vertical axe (Common unit of measurement pixel, E37) for black/white prints for draft prints."@en ;
        rdfs:isDefinedBy    <http://www.ebusiness-unibw.org/ontologies/consumerelectronics/v1> ;
        rdfs:label          "draft printable resolution black white vertical"@en , "vertikale druckbare Auflösung Schwarz/Weiß Entwurf"@de ;
        rdfs:range          gr:QuantitativeValueInteger ;
        rdfs:subPropertyOf  gr:quantitativeProductOrServiceProperty ;
        :belongsToModule    "Printer"@en .

:Blue   a                 :Color ;
        rdfs:comment      "RGB Value 0,0,255"@en ;
        rdfs:label        "Blau"@de , "Blue"@en ;
        :belongsToModule  "MP3Player, TV, Printer, DigitalCamera, Camcorder"@en .

:JPEG   a                 :DataFormatImage ;
        rdfs:comment      "JPEG compression is used in a number of image file formats. JPEG/Exif is the most common image format used by digital cameras and other photographic image capture devices; along with JPEG/JFIF, it is the most common format for storing and transmitting photographic images on the World Wide Web.\n\n(This description is partly based on or reuses content from the Wikipedia article \"JPEG\" (http://en.wikipedia.org/wiki/JPEG) and is licensed under the GNU Free Documentation License (http://www.gnu.org/copyleft/fdl.html).)"@en ;
        rdfs:label        "JPEG"@de , "JPEG"@en ;
        :belongsToModule  "MP3Player, DigitalCamera, Camcorder"@en .

:hasResolution  a           owl:ObjectProperty ;
        rdfs:comment        "Defines the type of resolution a screen is able to display."@en ;
        rdfs:isDefinedBy    <http://www.ebusiness-unibw.org/ontologies/consumerelectronics/v1> ;
        rdfs:label          "resolution"@en , "Auflösung"@de ;
        rdfs:range          :SupportedResolution ;
        rdfs:subPropertyOf  gr:qualitativeProductOrServiceProperty ;
        :belongsToModule    "TV"^^xsd:string .

:Windows95  a             :CompatibleOperatingSystems ;
        rdfs:comment      "A version of a Microsoft operating system."@en ;
        rdfs:label        "Windows 95"@de , "Windows 95"@en ;
        :belongsToModule  "MP3Player, Printer, DigitalCamera, Camcorder"@en .

:TVTuner  a               owl:Class ;
        rdfs:comment      "A television tuner converts an RF television transmission into audio and video signals which can be further processed to produce sound and a picture.\n\n(This description is partly based on or reuses content from the Wikipedia article \"Tuner (electronics)\" (http://en.wikipedia.org/wiki/Tuner_(electronics)) and is licensed under the GNU Free Documentation License (http://www.gnu.org/copyleft/fdl.html).)"^^xsd:string ;
        rdfs:isDefinedBy  <http://www.ebusiness-unibw.org/ontologies/consumerelectronics/v1> ;
        rdfs:label        "TV Tuner"@de , "TV Tuner"@en ;
        rdfs:subClassOf   gr:QualitativeValue ;
        :belongsToModule  "TV"@en .

:hasAccessory  a            owl:ObjectProperty ;
        rdfs:comment        "Defines subordinate or supplementary items."@en ;
        rdfs:isDefinedBy    <http://www.ebusiness-unibw.org/ontologies/consumerelectronics/v1> ;
        rdfs:label          "accessory"@en , "Zubehör"@de ;
        rdfs:range          :Accessory ;
        rdfs:subPropertyOf  gr:qualitativeProductOrServiceProperty ;
        :belongsToModule    "Camcorder"@en .

:Canon  a                 gr:BusinessEntity ;
        rdfs:comment      "The business entity Canon."@en ;
        rdfs:label        "Canon"^^xsd:string ;
        rdfs:seeAlso      <http://www.canon.com/> ;
        gr:legalName      "Canon Inc."^^xsd:string ;
        :belongsToModule  "Printer, DigitalCamera, Camcorder"@en .

:hasApertureRange  a        owl:ObjectProperty ;
        rdfs:comment        "Defines the hole or an opening through which light is admitted."@en ;
        rdfs:isDefinedBy    <http://www.ebusiness-unibw.org/ontologies/consumerelectronics/v1> ;
        rdfs:label          "aperture range"@en , "Blendenbereich"@de ;
        rdfs:range          gr:QuantitativeValueFloat ;
        rdfs:subPropertyOf  gr:quantitativeProductOrServiceProperty ;
        :belongsToModule    "Camcorder"@en .

:PlainPaper  a            :MediaType ;
        rdfs:comment      "Thin material mainly used for writing upon, printing upon or packaging."@en ;
        rdfs:label        "Plain paper"@en , "Normalpapier"@de ;
        :belongsToModule  "Printer"@en .

:hasMaxPrintableResolutionColorVertical
        a                   owl:ObjectProperty ;
        rdfs:comment        "Defines the maximum digital resolution of the vertical axe (Common unit of measurement pixel, E37)  for color prints."@en ;
        rdfs:isDefinedBy    <http://www.ebusiness-unibw.org/ontologies/consumerelectronics/v1> ;
        rdfs:label          "max printable resolution color vertical"@en , "maximale vertikale druckbare Auflösung Farbe"@de ;
        rdfs:range          gr:QuantitativeValueInteger ;
        rdfs:subPropertyOf  gr:quantitativeProductOrServiceProperty ;
        :belongsToModule    "Printer"@en .

:Red    a                 :Color ;
        rdfs:comment      "RGB Value 255,0,0"@en ;
        rdfs:label        "Rot"@de , "Red"@en ;
        :belongsToModule  "MP3Player, TV, Printer, DigitalCamera, Camcorder"@en .

:Ricoh  a                 gr:BusinessEntity ;
        rdfs:comment      "The business entity Ricoh."@en ;
        rdfs:label        "Ricoh"^^xsd:string ;
        rdfs:seeAlso      <http://www.ebusiness-unibw.org/ontologies/consumerelectronics/v1> ;
        gr:legalName      "Ricoh Company, Ltd."^^xsd:string ;
        :belongsToModule  "Printer, DigitalCamera"@en .

:DataFormatAudio  a       owl:Class ;
        rdfs:comment      "A data format is a particular way to encode information for storage in a computer file (refers to audiodata).\n\n(This description is partly based on or reuses content from the Wikipedia article \"File Format\" (http://en.wikipedia.org/wiki/File_format) and is licensed under the GNU Free Documentation License (http://www.gnu.org/copyleft/fdl.html).)"@en ;
        rdfs:isDefinedBy  <http://www.ebusiness-unibw.org/ontologies/consumerelectronics/v1> ;
        rdfs:label        "Data Format Audio"@en , "Audio Datenformat"@de ;
        rdfs:subClassOf   :DataFormat ;
        :belongsToModule  "MP3Player, DigitalCamera, Camcorder"@en .

:WindFilter  a            :Features ;
        rdfs:comment      "Ability to filter out wind noises."@en ;
        rdfs:label        "Wind filter"@en , "Windfilter"@de ;
        :belongsToModule  "Camcorder"@en .

:Samsung  a               gr:BusinessEntity ;
        rdfs:comment      "The business entity Samsung Group."@en ;
        rdfs:label        "Samsung"^^xsd:string ;
        rdfs:seeAlso      <http://www.samsung.com/> ;
        gr:legalName      "Samsung Group"^^xsd:string ;
        :belongsToModule  "MP3Player, TV, Printer, DigitalCamera, Camcorder"@en .

:B8     a                 :MediaFormat ;
        rdfs:comment      "Format of the german institute for standardization: 62 x 88 mm."@en ;
        rdfs:label        "B8"@en , "B8"@de ;
        :belongsToModule  "Printer"@en .

:WMA    a                 :DataFormatAudio ;
        rdfs:comment      "An audio data compression technology developed by Microsoft."@en ;
        rdfs:label        "WMA"@de , "WMA"@en ;
        :belongsToModule  "MP3Player, DigitalCamera, Camcorder"@en .

:Belkin  a                gr:BusinessEntity ;
        rdfs:comment      "The business entity Belkin International Inc."@en ;
        rdfs:label        "Belkin"^^xsd:string ;
        rdfs:seeAlso      <http://www.belkin.com/> ;
        gr:legalName      "Belkin International Inc"^^xsd:string ;
        :belongsToModule  "MP3Player"@en .

:Finlux  a                gr:BusinessEntity ;
        rdfs:comment      "The business entity Finlux."@en ;
        rdfs:label        "Finlux"^^xsd:string ;
        rdfs:seeAlso      <http://www.finlux.fi/> ;
        gr:legalName      "Finlux Inc."^^xsd:string ;
        :belongsToModule  "TV"@en .

:A0     a                 :MediaFormat ;
        rdfs:comment      "Format of the german institute for standardization: 841 x 1189 mm."@en ;
        rdfs:label        "A0"@en , "A0"@de ;
        :belongsToModule  "Printer"@en .

:NiMH   a                 :RechargeableEnergySource ;
        rdfs:comment      "A nickel-metal hydride battery, abbreviated NiMH, is a type of rechargeable battery similar to a nickel-cadmium (NiCd) battery but using a hydrogen-absorbing alloy for the negative electrode instead of cadmium.\n\n(This description is partly based on or reuses content from the Wikipedia article \"Nickel metal hydride battery\" (http://en.wikipedia.org/wiki/Nickel_metal_hydride_battery) and is licensed under the GNU Free Documentation License (http://www.gnu.org/copyleft/fdl.html).)"@en ;
        rdfs:label        "NiMH"@de , "NiMH"@en ;
        :belongsToModule  "MP3Player, DigitalCamera, Camcorder"@en .

:Solar  a                 :RechargeableEnergySource ;
        rdfs:comment      "Solar cell or photovoltaic cell is a wide area electronic device that converts solar energy into electricity by the photovoltaic effect.\n\n(This description is partly based on or reuses content from the Wikipedia article \"Solar cell\" (http://en.wikipedia.org/wiki/Solar_cell) and is licensed under the GNU Free Documentation License (http://www.gnu.org/copyleft/fdl.html).)"@en ;
        rdfs:label        "Solar"@de , "Solar"@en ;
        :belongsToModule  "MP3Player, DigitalCamera, Camcorder"@en .

:SDTV_480i  a             :TVDisplayResolution ;
        rdfs:comment      "480i is the shorthand name for a video mode, namely the U.S. NTSC television system or digital television systems with the same characteristics. The i, which is sometimes uppercase, stands for interlaced, the 480 for a vertical frame resolution of 480 lines containing picture information; while NTSC has a total of 525 lines, only 480 of these are used to display the image.\n\n(This description is partly based on or reuses content from the Wikipedia article \"480i\" (http://en.wikipedia.org/wiki/480i) and is licensed under the GNU Free Documentation License (http://www.gnu.org/copyleft/fdl.html).)"@en ;
        rdfs:label        "SDTV 480i"@en , "SDTV 480i"@de ;
        :belongsToModule  "TV"@en .

:PixelPlus2  a            :VideoFeatures ;
        rdfs:comment      "Pixelplus 2 is a technology which allows motion reinterpolation on 480p and 576p material."@en ;
        rdfs:label        "Pixelplus 2"@en , "Pixelplus 2"@de ;
        :belongsToModule  "TV"@en .

:Lexmark  a               gr:BusinessEntity ;
        rdfs:comment      "The business entity Lexmark."@en ;
        rdfs:label        "Lexmark."^^xsd:string ;
        rdfs:seeAlso      <http://www.lexmark.com/> ;
        gr:legalName      "Lexmark International, Inc."^^xsd:string ;
        :belongsToModule  "Printer"@en .

:hasMaxInputCapacity  a     owl:ObjectProperty ;
        rdfs:comment        "Maximum number of sheets the device can hold in all available standard and optional output trays."@en ;
        rdfs:isDefinedBy    <http://www.ebusiness-unibw.org/ontologies/consumerelectronics/v1> ;
        rdfs:label          "max input capacity"@en , "maximale Medienkapazität"@de ;
        rdfs:range          gr:QuantitativeValueInteger ;
        rdfs:subPropertyOf  gr:quantitativeProductOrServiceProperty ;
        :belongsToModule    "Printer"@en .

:hasPrintBorderLeft  a      owl:ObjectProperty ;
        rdfs:comment        "Defines the area which can not be printed on the left side of a paper (DIN A4) (Common unit of measurement millimetre, MMT)."@en ;
        rdfs:isDefinedBy    <http://www.ebusiness-unibw.org/ontologies/consumerelectronics/v1> ;
        rdfs:label          "print border left"@en , "Druckgrenze links"@de ;
        rdfs:range          gr:QuantitativeValueFloat ;
        rdfs:subPropertyOf  gr:quantitativeProductOrServiceProperty .

:GE     a                 gr:BusinessEntity ;
        rdfs:comment      "The business entity General Electric Company."@en ;
        rdfs:label        "GE"^^xsd:string ;
        rdfs:seeAlso      <http://www.ge.com/> ;
        gr:legalName      "General Electric Company"^^xsd:string ;
        :belongsToModule  "DigitalCamera"@en .

:DisposableBattery  a     :DisposableEnergySource ;
        rdfs:comment      "Is any kind of electrochemical cell in which the electrochemical reaction of interest is not reversible."@en ;
        rdfs:label        "Disposable battery"@en , "Batterie"@de ;
        :belongsToModule  "MP3Player, DigitalCamera, Camcorder"@en .

:DataFormat  a            owl:Class ;
        rdfs:comment      "A data format is a particular way to encode information for storage in a computer file.\n\n(This description is partly based on or reuses content from the Wikipedia article \"File Format\" (http://en.wikipedia.org/wiki/File_format) and is licensed under the GNU Free Documentation License (http://www.gnu.org/copyleft/fdl.html).)"@en ;
        rdfs:isDefinedBy  <http://www.ebusiness-unibw.org/ontologies/consumerelectronics/v1> ;
        rdfs:label        "Data Format"@en , "Datenformat"@de ;
        rdfs:subClassOf   gr:QualitativeValue ;
        :belongsToModule  "MP3Player, DigitalCamera, Camcorder"@en .

:Microphon  a             :Features ;
        rdfs:comment      "Ability to record voices and sounds."@en ;
        rdfs:label        "Microphon"@en , "Mikrofon"@de ;
        :belongsToModule  "DigitalCamera, Camcorder"@en .

:CMOS   a                 :SensorType ;
        rdfs:comment      "Complementary metal-oxide-semiconductor (CMOS) (pronounced \"see-moss\", IPA: /ˈsiːmɒs/), is a major class of integrated circuits. CMOS technology is used in microprocessors, microcontrollers, static RAM, and other digital logic circuits. CMOS technology is also used for a wide variety of analog circuits such as image sensors, data converters, and highly integrated transceivers for many types of communication. Frank Wanlass successfully patented CMOS in 1967 (US Patent 3,356,858).\n\n(This description is partly based on or reuses content from the Wikipedia article \"CMOS\" (http://en.wikipedia.org/wiki/CMOS) and is licensed under the GNU Free Documentation License (http://www.gnu.org/copyleft/fdl.html).)"@en ;
        rdfs:label        "CMOS"@de , "CMOS"@en ;
        :belongsToModule  "Camcorder"@en .

:hasMaxOperatingTemperature
        a                   owl:ObjectProperty ;
        rdfs:comment        "Defines the maximum temperature the product is able to operate (Common unit of measurement grad celsius, CEL)."@en ;
        rdfs:isDefinedBy    <http://www.ebusiness-unibw.org/ontologies/consumerelectronics/v1> ;
        rdfs:label          "max operating temperatur"@en , "maximale Betriebstemperatur"@de ;
        rdfs:range          gr:QuantitativeValueFloat ;
        rdfs:subPropertyOf  gr:quantitativeProductOrServiceProperty ;
        :belongsToModule    "TV, Printer"@en .

:Mustek  a                gr:BusinessEntity ;
        rdfs:comment      "The business entity Mustek Ltd."@en ;
        rdfs:label        "Mustek"^^xsd:string ;
        rdfs:seeAlso      <http://www.mustek.com/> ;
        gr:legalName      "Mustek Ltd."^^xsd:string ;
        :belongsToModule  "MP3Player, Camcorder"@en .

:hasMaxPrintableResolutionBlackWhiteHorizontal
        a                   owl:ObjectProperty ;
        rdfs:comment        "Defines the maximum digital resolution of the horizontal axe (Common unit of measurement pixel, E37) for black/white prints."@en ;
        rdfs:isDefinedBy    <http://www.ebusiness-unibw.org/ontologies/consumerelectronics/v1> ;
        rdfs:label          "max printable resolution black white horizontal"@en , "maximale horizontale druckbare Auflösung Schwarz/Weiß"@de ;
        rdfs:range          gr:QuantitativeValueInteger ;
        rdfs:subPropertyOf  gr:quantitativeProductOrServiceProperty ;
        :belongsToModule    "Printer"@en .

:PictureViewing  a        :Features ;
        rdfs:comment      "Ability to display digital pictures."@en ;
        rdfs:label        "Picture viewing"@en , "Bildbetrachtung"@de ;
        :belongsToModule  "MP3Player"@en .

:Connectivity  a          owl:Class ;
        rdfs:comment      "A generic term for linking devices to each other and allow sending data in one or both directions."@en ;
        rdfs:isDefinedBy  <http://www.ebusiness-unibw.org/ontologies/consumerelectronics/v1> ;
        rdfs:label        "Verbindungsmöglichkeit"@de , "Connectivity"@en ;
        rdfs:subClassOf   gr:QualitativeValue ;
        :belongsToModule  "TV"@en .

:ComponentVideoIn  a      :Connectivity ;
        rdfs:comment      "Component video is a video signal that has been split into two or more components. In popular use, it refers to a type of analog video information that is transmitted or stored as three separate signals. Component video can be contrasted with composite video (NTSC, PAL or SECAM) in which all the video information is combined into a single line-level signal. Like composite, component video cables do not carry audio and are often paired with audio cables. Here the input is meant.\n\n(This description is partly based on or reuses content from the Wikipedia article \"Component video\" (http://en.wikipedia.org/wiki/Component_video) and is licensed under the GNU Free Documentation License (http://www.gnu.org/copyleft/fdl.html).)"@en ;
        rdfs:label        "Component video in"@de , "Component video in"@en ;
        :belongsToModule  "TV"@en .

:DC_Cable  a              :Accessory ;
        rdfs:comment      "The mean amplitude of a waveform."@en ;
        rdfs:label        "DC cable"@en , "DC Kabel"@de ;
        :belongsToModule  "Camcorder"@en .

:Pentax  a                gr:BusinessEntity ;
        rdfs:comment      "The business entity Pentax Corporation."@en ;
        rdfs:label        "Pentax"^^xsd:string ;
        rdfs:seeAlso      <http://www.pentax.jp/english/> ;
        gr:legalName      "Pentax Corporation"^^xsd:string ;
        :belongsToModule  "DigitalCamera"@en .

:FocusManual  a           :Focus ;
        rdfs:comment      "A manual focus allows the operator to adjust the focus of the lens by hand.\n\n(This description is partly based on or reuses content from the Wikipedia article \"Manual focus\" (http://en.wikipedia.org/wiki/Manual_focus) and is licensed under the GNU Free Documentation License (http://www.gnu.org/copyleft/fdl.html).)"@en ;
        rdfs:label        "Focus manual"@en , "Manueller Fokus"@de ;
        :belongsToModule  "DigitalCamera, Camcorder"@en .

:DOC    a                 :DataFormatOffice ;
        rdfs:comment      "A file extension for word processing documents."@en ;
        rdfs:label        "DOC"@de , "DOC"@en ;
        :belongsToModule  "MP3Player, DigitalCamera"@en .

dc:rights  a    owl:AnnotationProperty .

:hasAnalogVideoSignal
        a                   owl:DatatypeProperty ;
        rdfs:comment        "Defines whether an analog video signal is supported."@en ;
        rdfs:isDefinedBy    <http://www.ebusiness-unibw.org/ontologies/consumerelectronics/v1> ;
        rdfs:label          "analog video signal"@en , "analoges Videosignal"@de ;
        rdfs:range          xsd:boolean ;
        rdfs:subPropertyOf  gr:datatypeProductOrServiceProperty ;
        :belongsToModule    "DigitalCamera"@en .

:Tatung  a                gr:BusinessEntity ;
        rdfs:comment      "The business entity Tatung Co."@en ;
        rdfs:label        "Tatung"^^xsd:string ;
        rdfs:seeAlso      <http://www.tatung.com/> ;
        gr:legalName      "Tatung Co."^^xsd:string ;
        :belongsToModule  "MP3Player, TV"@en .

:DynamicBassEnhancement
        a                 :AudioFeatures ;
        rdfs:comment      "Dynamic settlement of bass audiosignals."@en ;
        rdfs:label        "Dynamic bass enhancement"@en , "Dynamischer Bass"@de ;
        :belongsToModule  "TV"@en .

:Black  a                 :Color ;
        rdfs:comment      "RGB Value 0,0,0"@en ;
        rdfs:label        "Schwarz"@de , "Black"@en ;
        :belongsToModule  "MP3Player, TV, Printer, DigitalCamera, Camcorder"@en .

:SensorType_3CCD  a       :SensorType ;
        rdfs:comment      "3CCD is a term used to describe an imaging system employed by some still cameras, video cameras, telecine and camcorders.\n\n(This description is partly based on or reuses content from the Wikipedia article \"Three-CCD\" (http://en.wikipedia.org/wiki/Three-CCD) and is licensed under the GNU Free Documentation License (http://www.gnu.org/copyleft/fdl.html).)"@en ;
        rdfs:label        "Three-CCD"@de , "Three-CCD"@en ;
        :belongsToModule  "Camcorder"@en .

:hasStandbyPowerConsumption
        a                   owl:ObjectProperty ;
        rdfs:comment        "Defines the amount of consumed energy while the device is in the standby mode (Common unit of measurement Watt, WTT)."@en ;
        rdfs:isDefinedBy    <http://www.ebusiness-unibw.org/ontologies/consumerelectronics/v1> ;
        rdfs:label          "standby power consumption"@en , "Standby Stromverbrauch"@de ;
        rdfs:range          gr:QuantitativeValueFloat ;
        rdfs:subPropertyOf  gr:quantitativeProductOrServiceProperty ;
        :belongsToModule    "TV, Printer"@en .

:Apacer  a                gr:BusinessEntity ;
        rdfs:comment      "The business entity Apacer Technology, Inc."@en ;
        rdfs:label        "Apacer"^^xsd:string ;
        rdfs:seeAlso      <http://www.apacer.com/> ;
        gr:legalName      "Apacer Technology, Inc."^^xsd:string ;
        :belongsToModule  "MP3Player"@en .

:hasWallMountability  a     owl:DatatypeProperty ;
        rdfs:comment        "Defines if an object can be installed at a wall."@en ;
        rdfs:isDefinedBy    <http://www.ebusiness-unibw.org/ontologies/consumerelectronics/v1> ;
        rdfs:label          "wall mountability"@en , "Wandmontagemöglichkeit"@de ;
        rdfs:range          xsd:boolean ;
        rdfs:subPropertyOf  gr:datatypeProductOrServiceProperty ;
        :belongsToModule    "TV"@en .

:PerfectPixelHD  a        :VideoFeatures ;
        rdfs:comment      "Perfect Pixel HD Engine offers the unique combination of ultimate sharpness, natural detail, vivid colours and smooth natural motion on all qualities of HD, standard TV signals and multimedia content, for high definition displays. Each pixel of the incoming picture is enhanced to better match the surrounding pixels, resulting in a more natural picture."@en ;
        rdfs:label        "Perfect Pixel HD"@de , "Perfect Pixel HD"@en ;
        :belongsToModule  "TV"@en .

:B3     a                 :MediaFormat ;
        rdfs:comment      "Format of the german institute for standardization: 353 x 500 mm."@en ;
        rdfs:label        "B3"@en , "B3"@de ;
        :belongsToModule  "Printer"@en .

:DataFormatImage  a       owl:Class ;
        rdfs:comment      "A data format is a particular way to encode information for storage in a computer file (refers to image data).\n\n(This description is partly based on or reuses content from the Wikipedia article \"File Format\" (http://en.wikipedia.org/wiki/File_format) and is licensed under the GNU Free Documentation License (http://www.gnu.org/copyleft/fdl.html).)"@en ;
        rdfs:isDefinedBy  <http://www.ebusiness-unibw.org/ontologies/consumerelectronics/v1> ;
        rdfs:label        "Graphik Datenformat"@de , "Data Format Image"@en ;
        rdfs:subClassOf   :DataFormat ;
        :belongsToModule  "MP3Player, DigitalCamera, Camcorder"@en .

:hasDigitalZoom  a          owl:DatatypeProperty ;
        rdfs:comment        "Zoom is a method of decreasing (narrowing) the apparent angle of view of a photographic or video image.\n\n(This description is partly based on or reuses content from the Wikipedia article \"Digital zoom\" (http://en.wikipedia.org/wiki/Digital_zoom) and is licensed under the GNU Free Documentation License (http://www.gnu.org/copyleft/fdl.html).)"@en ;
        rdfs:isDefinedBy    <http://www.ebusiness-unibw.org/ontologies/consumerelectronics/v1> ;
        rdfs:label          "digital zoom"@en , "digitaler Zoom"@de ;
        rdfs:range          xsd:boolean ;
        rdfs:subPropertyOf  gr:datatypeProductOrServiceProperty ;
        :belongsToModule    "DigitalCamera, Camcorder"@en .

:SDHC   a                 :StorageMedia ;
        rdfs:comment      "SDHC (Secure Digital High Capacity, SD 2.0) is an extension of the SD standard that appeared in June 2006.\n\n(This description is partly based on or reuses content from the Wikipedia article \"Secure Digital card\" (http://en.wikipedia.org/wiki/Secure_Digital_card) and is licensed under the GNU Free Documentation License (http://www.gnu.org/copyleft/fdl.html).)"@en ;
        rdfs:label        "SDHC"@en , "SDHC"@de ;
        :belongsToModule  "Camcorder"@en .

:hasBatteryRechargeTime
        a                   owl:ObjectProperty ;
        rdfs:comment        "Total time needed to fully recharge a completely discharged rechargeable energy source for this mp3 player (Common unit of measurement hour, HUR)."@en ;
        rdfs:isDefinedBy    <http://www.ebusiness-unibw.org/ontologies/consumerelectronics/v1> ;
        rdfs:label          "battery recharge time"@en , "Akkuladezeit"@de ;
        rdfs:range          gr:QuantitativeValueFloat ;
        rdfs:subPropertyOf  gr:quantitativeProductOrServiceProperty ;
        :belongsToModule    "MP3Player, DigitalCamera, Camcorder"@en .

:Oppo   a                 gr:BusinessEntity ;
        rdfs:comment      "The business entity Oppo."@en ;
        rdfs:label        "Oppo"^^xsd:string ;
        rdfs:seeAlso      <http://www.oppo.nl/> ;
        gr:legalName      "Elmarc BV"^^xsd:string ;
        :belongsToModule  "TV"@en .

:hasDataFormat  a           owl:ObjectProperty ;
        rdfs:comment        "Defines the supported data formats."@en ;
        rdfs:isDefinedBy    <http://www.ebusiness-unibw.org/ontologies/consumerelectronics/v1> ;
        rdfs:label          "data format"@en , "Datenformat"@de ;
        rdfs:range          :DataFormat ;
        rdfs:subPropertyOf  gr:qualitativeProductOrServiceProperty ;
        :belongsToModule    "MP3Player, DigitalCamera, Camcorder"@en .

:hasFeature  a              owl:ObjectProperty ;
        rdfs:comment        "Defines the type of special functions the object is capable of."@en ;
        rdfs:isDefinedBy    <http://www.ebusiness-unibw.org/ontologies/consumerelectronics/v1> ;
        rdfs:label          "feature"@en , "Eigenschaft"@de ;
        rdfs:range          :Features ;
        rdfs:subPropertyOf  gr:qualitativeProductOrServiceProperty ;
        :belongsToModule    "MP3Player, TV, DigitalCamera, Camcorder"@en .

:hasID3Support  a           owl:DatatypeProperty ;
        rdfs:comment        "Defines the support of information such as the title, artist, album, track number, or other information about the file to be stored in the file itself."@en ;
        rdfs:isDefinedBy    <http://www.ebusiness-unibw.org/ontologies/consumerelectronics/v1> ;
        rdfs:label          "ID3 support"@en , "ID3 Unterstützung"@de ;
        rdfs:range          xsd:boolean ;
        rdfs:subPropertyOf  gr:datatypeProductOrServiceProperty ;
        :belongsToModule    "MP3Player"@de .

dc:title  a     owl:AnnotationProperty .

:IR_Remote  a             :Accessory ;
        rdfs:comment      "Remote control with a electromagnetic radiation whose wavelength is longer than that of visible light (400-700 nm), but shorter than that of terahertz radiation (3-300 µm) and microwaves (~30,000 µm). Infrared radiation spans roughly three orders of magnitude (750 nm and 1000 µm)"@en ;
        rdfs:label        "IR remote control"@en , "Infrarotfernbedienung"@de ;
        :belongsToModule  "Camcorder"@en .

:CE_Mark  a               :Certificate ;
        rdfs:comment      "The CE marking (also known as CE mark) is a mandatory conformity mark on many products placed on the single market in the European Economic Area (EEA).\n\n(This description is partly based on or reuses content from the Wikipedia article \"CE mark\" (http://en.wikipedia.org/wiki/CE_mark) and is licensed under the GNU Free Documentation License (http://www.gnu.org/copyleft/fdl.html).)"@en ;
        rdfs:label        "CE Mark"@de , "CE Mark"@en ;
        :belongsToModule  "TV"@en .

:hasResponseTime  a         owl:ObjectProperty ;
        rdfs:comment        "Defines the time an electronical device needs to react on a signal (Common unit of measurement millisecond, C26)."@en ;
        rdfs:isDefinedBy    <http://www.ebusiness-unibw.org/ontologies/consumerelectronics/v1> ;
        rdfs:label          "response time"@en , "Reaktionszeit"@de ;
        rdfs:range          gr:QuantitativeValueFloat ;
        rdfs:subPropertyOf  gr:quantitativeProductOrServiceProperty ;
        :belongsToModule    "TV"@en .

:AC_Cable  a              :Accessory ;
        rdfs:comment      "A net transfer of energy over a complete cycle of the alternating current waveform."@en ;
        rdfs:label        "AC Kabel"@de , "AC cable"@en ;
        :belongsToModule  "Camcorder"@en .

:Yakumo  a                gr:BusinessEntity ;
        rdfs:comment      "The business entity Yakumo GmbH."@en ;
        rdfs:label        "Yakumo"^^xsd:string ;
        gr:legalName      "Yakumo GmbH"^^xsd:string ;
        :belongsToModule  "DigitalCamera"@en .

:Flash  a                 :Features ;
        rdfs:comment      "Is a device used in photography that produces an instantaneous flash of artificial light."@en ;
        rdfs:label        "Flash"@en , "Blitz"@de ;
        :belongsToModule  "Camcorder"@en .

:hasLensSystem  a           owl:ObjectProperty ;
        rdfs:comment        "Defines the perfect or approximate axial symmetry which transmits and refracts light."@en ;
        rdfs:isDefinedBy    <http://www.ebusiness-unibw.org/ontologies/consumerelectronics/v1> ;
        rdfs:label          "lens system"@en , "Objektivsystem"@de ;
        rdfs:range          :LensSystem ;
        rdfs:subPropertyOf  gr:qualitativeProductOrServiceProperty ;
        :belongsToModule    "Camcorder"@en .

:Certificate  a           owl:Class ;
        rdfs:comment      "A certificate is an official document affirming some fact like quality standards.\n\n(This description is partly based on or reuses content from the Wikipedia article \"Certificate\" (http://en.wikipedia.org/wiki/Certificate) and is licensed under the GNU Free Documentation License (http://www.gnu.org/copyleft/fdl.html).)"@en ;
        rdfs:isDefinedBy  <http://www.ebusiness-unibw.org/ontologies/consumerelectronics/v1> ;
        rdfs:label        "Zertifikat"@de , "Certificate"@en ;
        rdfs:subClassOf   gr:QualitativeValue ;
        :belongsToModule  "TV"@en .

:TEAC   a                 gr:BusinessEntity ;
        rdfs:comment      "The business entity TEAC Europe GmbH."@en ;
        rdfs:label        "TEAC"^^xsd:string ;
        rdfs:seeAlso      <http://www.teac.de/> ;
        gr:legalName      "TEAC Europe GmbH "^^xsd:string ;
        :belongsToModule  "MP3Player, TV"@en .

:Fujitsu_Siemens  a       gr:BusinessEntity ;
        rdfs:comment      "The business entity Fujitsu Siemens."@en ;
        rdfs:label        "Fujitsu Siemens"^^xsd:string ;
        rdfs:seeAlso      <http://www.fujitsu.com/> ;
        gr:legalName      "Fujitsu Siemens Computers"^^xsd:string ;
        :belongsToModule  "TV, Printer, DigitalCamera"@en .

:hasEnergySource  a         owl:ObjectProperty ;
        rdfs:comment        "Defines the used energy source."@en ;
        rdfs:isDefinedBy    <http://www.ebusiness-unibw.org/ontologies/consumerelectronics/v1> ;
        rdfs:label          "energy source"@en , "Energiequelle"@de ;
        rdfs:range          :EnergySource ;
        rdfs:subPropertyOf  gr:qualitativeProductOrServiceProperty ;
        :belongsToModule    "MP3Player, Printer, DigitalCamera, Camcorder"@en .

:hasPictureInPicture  a     owl:DatatypeProperty ;
        rdfs:comment        "Defines that an electronical screen can display minimum two pictures on one screen."@en ;
        rdfs:isDefinedBy    <http://www.ebusiness-unibw.org/ontologies/consumerelectronics/v1> ;
        rdfs:label          "picture in picture"@en , "Bild-in-Bild Funktion"@de ;
        rdfs:range          xsd:boolean ;
        rdfs:subPropertyOf  gr:datatypeProductOrServiceProperty ;
        :belongsToModule    "TV"@en .

:NEC    a                 gr:BusinessEntity ;
        rdfs:comment      "The business entity NEC Corporation."@en ;
        rdfs:label        "NEC"^^xsd:string ;
        rdfs:seeAlso      <http://www.necel.com/> ;
        gr:legalName      "NEC Corporation"^^xsd:string ;
        :belongsToModule  "MP3Player, TV"@en .

:MiniUSB  a               :DataInterfaceType ;
        rdfs:comment      "The non-standard Mini-USB's, official Mini-B, Micro-A, and Micro-B connectors are used for smaller devices such as PDAs, mobile phones or digital cameras. The Standard-A plug is approximately 4 by 12 mm, the Standard-B approximately 7 by 8 mm, and the Mini-A and Mini-B plugs approximately 2 by 7 mm.\n\n(This description is partly based on or reuses content from the Wikipedia article \"Universial Serial Bus\" (http://en.wikipedia.org/wiki/Universal_Serial_Bus) and is licensed under the GNU Free Documentation License (http://www.gnu.org/copyleft/fdl.html).)"@en ;
        rdfs:label        "Mini USB"^^xsd:string , "Mini USB"@en ;
        :belongsToModule  "MP3Player, Printer, DigitalCamera, Camcorder"@en .

:ALE    a                 :DataFormatAudio ;
        rdfs:comment      "Apple Lossless (also known as Apple Lossless Encoder, ALE, or Apple Lossless Audio Codec, ALAC) is an audio codec developed by Apple Inc. for lossless data compression of digital music.\n\n(This description is partly based on or reuses content from the Wikipedia article \"Apple Lossless\" (http://en.wikipedia.org/wiki/Apple_Lossless) and is licensed under the GNU Free Documentation License (http://www.gnu.org/copyleft/fdl.html).)"@en ;
        rdfs:label        "ALE"@de , "ALE"@en ;
        :belongsToModule  "MP3Player, DigitalCamera, Camcorder"@en .

:G4_Class_Processor  a    :ProcessorType ;
        rdfs:comment      "A designation used by Apple Computer to describe a fourth generation of 32-bit PowerPC microprocessors.\n\n(This description is partly based on or reuses content from the Wikipedia article \"PowerPC_G4\" (http://en.wikipedia.org/wiki/PowerPC_G4) and is licensed under the GNU Free Documentation License (http://www.gnu.org/copyleft/fdl.html).)"@en ;
        rdfs:label        "G4 Class Processor"@en , "G4 Class Processor"@de ;
        :belongsToModule  "Printer"@en .

:hasMediaWeightTray1  a     owl:ObjectProperty ;
        rdfs:comment        "Describes the weight of the media format (Common unit of measurement gram per square metre, GM) hold in tray 1."@en ;
        rdfs:isDefinedBy    <http://www.ebusiness-unibw.org/ontologies/consumerelectronics/v1> ;
        rdfs:label          "media weight tray 1"@en , "Mediengewicht Kassette 1"@de ;
        rdfs:range          gr:QuantitativeValueFloat ;
        rdfs:subPropertyOf  gr:quantitativeProductOrServiceProperty ;
        :belongsToModule    "Printer"@en .

:Alert  a                 :Features ;
        rdfs:comment      "Has wakeup-function."@en ;
        rdfs:label        "Alarm"@de , "Alert"@en ;
        :belongsToModule  "MP3Player"@en .

:SECAM-D_K  a             :SignalFormat ;
        rdfs:comment      "SECAM, also written SÉCAM (Séquentiel couleur à mémoire, French for \"Sequential Color with Memory\"), is an analog color television system first used in France. SECAM D/K is used in the Commonwealth of Independent States and Eastern Europe (this is simply SECAM used with the D and K monochrome TV transmission standards).\n\n(This description is partly based on or reuses content from the Wikipedia article \"SECAM\" (http://en.wikipedia.org/wiki/SECAM) and is licensed under the GNU Free Documentation License (http://www.gnu.org/copyleft/fdl.html).)"@en ;
        rdfs:label        "SECAM-D K"@de , "SECAM-D K"@en ;
        :belongsToModule  "TV"@en .

:Nintendo  a              gr:BusinessEntity ;
        rdfs:comment      "The business entity Nintendo Company Ltd."@en ;
        rdfs:label        "Nintendo"^^xsd:string ;
        rdfs:seeAlso      <http://www.nintendo.com/> ;
        gr:legalName      "Nintendo Company Ltd."^^xsd:string ;
        :belongsToModule  "MP3Player"@en .

:PCAudioIn  a             :Connectivity ;
        rdfs:comment      "Port to connect the audio cables for a PC with the electronical device."@en ;
        rdfs:label        "PC Audio out"@en , "PC Audio in"@de ;
        :belongsToModule  "TV"@en .

:hasAspectRatioVertical
        a                   owl:DatatypeProperty ;
        rdfs:comment        "The aspect ratio of a shape is the ratio of its longer dimension to its shorter dimension. The vertical dimension is the shorter one.\n\n(This description is partly based on or reuses content from the Wikipedia article \"Aspect ratio\" (http://en.wikipedia.org/wiki/Aspect_ratio) and is licensed under the GNU Free Documentation License (http://www.gnu.org/copyleft/fdl.html).)"@en ;
        rdfs:isDefinedBy    <http://www.ebusiness-unibw.org/ontologies/consumerelectronics/v1> ;
        rdfs:label          "aspect ratio vertical"^^xsd:string , "vertikales Bildseitenverhältnis"@de ;
        rdfs:range          xsd:float ;
        rdfs:subPropertyOf  gr:datatypeProductOrServiceProperty ;
        :belongsToModule    "TV"@en .

:EPG    a                 :GeneralFeatures ;
        rdfs:comment      "An electronic program(me) guide (EPG) or interactive program(me) guide (IPG) or electronic service guide (ESG) is an digital guide to scheduled broadcast television or radio programs, typically displayed on-screen with functions allowing a viewer to navigate, select, and discover content by time, title, channel, genre, etc. by use of their remote control, a keyboard, or other input devices such as a phone keypad.\n\n(This description is partly based on or reuses content from the Wikipedia article \"Electronic program guide\" (http://en.wikipedia.org/wiki/Electronic_program_guide) and is licensed under the GNU Free Documentation License (http://www.gnu.org/copyleft/fdl.html).)"@en ;
        rdfs:label        "EPG"@de , "EPG"@en ;
        :belongsToModule  "TV"@en .

:ViewFinder  a            owl:Class ;
        rdfs:comment      "A viewfinder is what the photographer looks through to compose, and in many cases to focus, the picture.\n\n(This description is partly based on or reuses content from the Wikipedia article \"Viewfinder\" (http://en.wikipedia.org/wiki/Viewfinder) and is licensed under the GNU Free Documentation License (http://www.gnu.org/copyleft/fdl.html).)"@en ;
        rdfs:isDefinedBy  <http://www.ebusiness-unibw.org/ontologies/consumerelectronics/v1> ;
        rdfs:label        "Viewfinder"@en , "Bildsucher"@de ;
        rdfs:subClassOf   gr:QualitativeValue ;
        :belongsToModule  "DigitalCamera, Camcorder"@en .

:DisposableEnergySource
        a                 owl:Class ;
        rdfs:comment      "Disposable batteries are non-rechargeable batteries. When they are out of power you have to dispose them."@en ;
        rdfs:isDefinedBy  <http://www.ebusiness-unibw.org/ontologies/consumerelectronics/v1> ;
        rdfs:label        "Einweg-Energiequelle"@de , "Disposable Energy Source"@en ;
        rdfs:subClassOf   :EnergySource ;
        :belongsToModule  "MP3Player, DigitalCamera, Camcorder"@en .

:Purple  a                :Color ;
        rdfs:comment      "RGB Value 128,0,128"@en ;
        rdfs:label        "Purpurrot"@de , "Purple"@en ;
        :belongsToModule  "MP3Player, TV, Printer, DigitalCamera, Camcorder"@en .

:PlugAndPlay  a       :GeneralFeatures ;
        rdfs:comment  "Describes any hardware specification that alleviates the need for user configuration of device resources.\n\n(This description is partly based on or reuses content from the Wikipedia article \"Legacy Plug and Play\" (http://en.wikipedia.org/wiki/Legacy_Plug_and_Play) and is licensed under the GNU Free Documentation License (http://www.gnu.org/copyleft/fdl.html).)"@en ;
        rdfs:label    "Plug and Play"@de , "Plug and Play"@en .

:Audio2.5mm  a            :AudioInterfaceType ;
        rdfs:comment      "Audio interface type of a specific diameter."@en ;
        rdfs:label        "Audio 2.5mm"@de , "Audio 2.5mm"@en ;
        :belongsToModule  "MP3Player"@en .

:Victory  a               gr:BusinessEntity ;
        rdfs:comment      "The business entity Victory Niederland B.V."@en ;
        rdfs:label        "Victory"^^xsd:string ;
        rdfs:seeAlso      <http://www.123victory.eu/> ;
        gr:legalName      "Victory Niederland B.V."^^xsd:string ;
        :belongsToModule  "MP3Player"@en .

:Olympus  a               gr:BusinessEntity ;
        rdfs:comment      "The business entity Olympus Europa Holding GmbH."@en ;
        rdfs:label        "Olympus"^^xsd:string ;
        rdfs:seeAlso      <http://www.olympus.de/> ;
        gr:legalName      "Olympus Europa Holding GmbH Corporate Communications"^^xsd:string ;
        :belongsToModule  "MP3Player, DigitalCamera"@en .

:PAL-I  a                 :SignalFormat ;
        rdfs:comment      "PAL, short for Phase Alternating Line, is a colour-encoding system used in broadcast television systems in large parts of the world. This is only used in Ireland, the UK, Hongkong and Macau.\n\n(This description is partly based on or reuses content from the Wikipedia article \"PAL\" (http://en.wikipedia.org/wiki/PAL) and is licensed under the GNU Free Documentation License (http://www.gnu.org/copyleft/fdl.html).)"@en ;
        rdfs:label        "PAL-L"@de , "PAL-I"@en ;
        :belongsToModule  "TV"@en .

:Casio  a                 gr:BusinessEntity ;
        rdfs:comment      "The business entity Casio Computer Co., Ltd."@en ;
        rdfs:label        "Casio"^^xsd:string ;
        rdfs:seeAlso      <http://world.casio.com/> ;
        gr:legalName      "Casio Computer Co., Ltd"^^xsd:string ;
        :belongsToModule  "DigitalCamera"@en .

:WAV    a                 :DataFormatAudio ;
        rdfs:comment      "WAV (or WAVE), short for Waveform audio format, is a Microsoft and IBM audio file format standard for storing an audio bitstream on PCs.\n\n(This description is partly based on or reuses content from the Wikipedia article \"WAV\" (http://en.wikipedia.org/wiki/WAV) and is licensed under the GNU Free Documentation License (http://www.gnu.org/copyleft/fdl.html).)"@en ;
        rdfs:label        "WAV"@de , "WAV"@en ;
        :belongsToModule  "MP3Player, DigitalCamera, Camcorder"@en .

:hasProcessorClockSpeed
        a                   owl:ObjectProperty ;
        rdfs:comment        "Defines the frequency of the clock in any synchronous circuit (common unit of measurement: hertz, HTZ)."@en ;
        rdfs:isDefinedBy    <http://www.ebusiness-unibw.org/ontologies/consumerelectronics/v1> ;
        rdfs:label          "processor clock speed"@en , "Prozessortaktrate"@de ;
        rdfs:range          gr:QuantitativeValueFloat ;
        rdfs:subPropertyOf  gr:quantitativeProductOrServiceProperty ;
        :belongsToModule    "Printer"@en .

:Hisense  a               gr:BusinessEntity ;
        rdfs:comment      "The business entity Hisense."@en ;
        rdfs:label        "Hisense"^^xsd:string ;
        rdfs:seeAlso      <http://www.hisense.com/> ;
        gr:legalName      "Hisense Group"^^xsd:string ;
        :belongsToModule  "TV"@en .

:hasDisplayResolutionVertical
        a                   owl:ObjectProperty ;
        rdfs:comment        "Defines the digital resolution of the vertical axe (Common unit of measurement pixel, E37)."@en ;
        rdfs:isDefinedBy    <http://www.ebusiness-unibw.org/ontologies/consumerelectronics/v1> ;
        rdfs:label          "display resolution vertical"@en , "vertikale Bildschirmauflösung"@de ;
        rdfs:range          gr:QuantitativeValueInteger ;
        rdfs:subPropertyOf  gr:quantitativeProductOrServiceProperty ;
        :belongsToModule    "MP3Player, TV, DigitalCamera, Camcorder"@en .

:MicroDrive  a            :StorageMedia ;
        rdfs:comment      "A miniature, 1-inch hard disk designed to fit in a CompactFlash (CF) Type II slot."@en ;
        rdfs:label        "MicroDrive"@en , "MicroDrive"@de ;
        :belongsToModule  "MP3Player, DigitalCamera, Camcorder"@en .

:hasDraftPrintableResolutionColorVertical
        a                   owl:ObjectProperty ;
        rdfs:comment        "Defines the digital resolution of the vertical axe (Common unit of measurement pixel, E37) for black/white prints for draft prints."@en ;
        rdfs:isDefinedBy    <http://www.ebusiness-unibw.org/ontologies/consumerelectronics/v1> ;
        rdfs:label          "draft printable resolution color vertical"@en , "vertikale druckbare Auflösung Farbe Entwurf"@de ;
        rdfs:range          gr:QuantitativeValueInteger ;
        rdfs:subPropertyOf  gr:quantitativeProductOrServiceProperty ;
        :belongsToModule    "Printer"@en .

:AV_Cable  a              :Accessory ;
        rdfs:comment      "A cable to carry video and audio signals from a device, to a tv; in digital or analog format."@en ;
        rdfs:label        "AV Kabel"@de , "AV cable"@en ;
        :belongsToModule  "Camcorder"@en .

:hasOutputPower  a          owl:ObjectProperty ;
        rdfs:comment        "Defines the rate of energy conversion (Common unit of Measurement milliwatt, C31)."@en ;
        rdfs:isDefinedBy    <http://www.ebusiness-unibw.org/ontologies/consumerelectronics/v1> ;
        rdfs:label          "output power"@en , "Ausgangsleistung"@de ;
        rdfs:range          gr:QuantitativeValueFloat ;
        rdfs:subPropertyOf  gr:quantitativeProductOrServiceProperty ;
        :belongsToModule    "MP3Player, Printer"@en .

:LaserPrintingPaper  a    :MediaType ;
        rdfs:comment      "Special sort of paper used in laser printers."@en ;
        rdfs:label        "Laser printing paper"@en , "Laserdruckpapier"@de ;
        :belongsToModule  "Printer"@en .

:hasUsagePowerConsumption
        a                   owl:ObjectProperty ;
        rdfs:comment        "Defines the necessary power for an electronical object while the device is used (Common unit of measurement Watt, WTT)."@en ;
        rdfs:isDefinedBy    <http://www.ebusiness-unibw.org/ontologies/consumerelectronics/v1> ;
        rdfs:label          "usage power consumption"@en , "Stromverbrauch in Betrieb"@de ;
        rdfs:range          gr:QuantitativeValueFloat ;
        rdfs:subPropertyOf  gr:quantitativeProductOrServiceProperty ;
        :belongsToModule    "TV, Printer"@en .

:RedEyeReduction  a       :Features ;
        rdfs:comment      "Defines the ability to precede the flash with a series of short, low-power flashes, or a continuous piercing bright light triggering the iris to contract."@en ;
        rdfs:label        "Red eye reduction"@en , "Rote-Augen-Effekt Reduktion"@de ;
        :belongsToModule  "Camcorder"@en .

:hasSwivel  a               owl:ObjectProperty ;
        rdfs:comment        "Defines the possibilty to rotate or turn an object into different directions (Common unit of measurement degree, DD)."@en ;
        rdfs:isDefinedBy    <http://www.ebusiness-unibw.org/ontologies/consumerelectronics/v1> ;
        rdfs:label          "swivel"@en , "Schwenkarm"@de ;
        rdfs:range          gr:QuantitativeValueFloat ;
        rdfs:subPropertyOf  gr:quantitativeProductOrServiceProperty ;
        :belongsToModule    "TV"@en .

:EnergySource  a          owl:Class ;
        rdfs:comment      "Methods of energy storage have been developed, which transform electrical energy into forms of potential energy.\n\n(This description is partly based on or reuses content from the Wikipedia article \"Energy development\" (http://en.wikipedia.org/wiki/Energy_development) and is licensed under the GNU Free Documentation License (http://www.gnu.org/copyleft/fdl.html).)"@en ;
        rdfs:isDefinedBy  <http://www.ebusiness-unibw.org/ontologies/consumerelectronics/v1> ;
        rdfs:label        "Energiequelle"@de , "Energy Source"@en ;
        rdfs:subClassOf   gr:QualitativeValue ;
        :belongsToModule  "MP3Player, Printer, DigitalCamera, Camcorder"@en .

:hasWidth  a                owl:ObjectProperty ;
        rdfs:comment        "Defines the distance between the ends of an object, its linear extent as measured from end to end (Common unit of measurement centimetre, CMT)."@en ;
        rdfs:isDefinedBy    <http://www.ebusiness-unibw.org/ontologies/consumerelectronics/v1> ;
        rdfs:label          "width"@en , "Breite"@de ;
        rdfs:range          gr:QuantitativeValueFloat ;
        rdfs:subPropertyOf  gr:quantitativeProductOrServiceProperty ;
        :belongsToModule    "MP3Player, TV, Printer, DigitalCamera, Camcorder"@en .

:hasMaxPrintableResolutionBlackWhiteVertical
        a                   owl:ObjectProperty ;
        rdfs:comment        "Defines the maximum digital resolution of the vertical axe (Common unit of measurement pixel, E37) for black/white prints."@en ;
        rdfs:isDefinedBy    <http://www.ebusiness-unibw.org/ontologies/consumerelectronics/v1> ;
        rdfs:label          "maximale vertikale druckbare Auflösung Schwarz/Weiß"@de , "max printable resolution black white vertical"@en ;
        rdfs:range          gr:QuantitativeValueInteger ;
        rdfs:subPropertyOf  gr:quantitativeProductOrServiceProperty ;
        :belongsToModule    "Printer"@en .

:FirmwareUpgradable  a    :GeneralFeatures ;
        rdfs:comment      "The term upgrade refers to the replacement of a product with a newer version of that same product, here it is the replacement of the firmware with a newer version of it."@en ;
        rdfs:label        "Firmware upgradable"@en , "Firmware aufrüstbar"@de ;
        :belongsToModule  "TV"@en .

:HDMI   a                 :Connectivity ;
        rdfs:comment      "HDMI (High-Definition Multimedia Interface) is a compact audio/video interface for transmitting uncompressed digital data. It represents a digital alternative to consumer analog standards such as Radio Frequency (RF) coaxial cable, composite video, S-Video, SCART, component video, D-Terminal, and VGA. HDMI connects digital audio/video sources such as set-top boxes, Blu-ray Disc players, personal computers (PCs), video game consoles, and AV receivers to compatible digital audio devices, computer monitors, and digital televisions.\n\n(This description is partly based on or reuses content from the Wikipedia article \"HDMI\" (http://en.wikipedia.org/wiki/HDMI) and is licensed under the GNU Free Documentation License (http://www.gnu.org/copyleft/fdl.html).)"@en ;
        rdfs:label        "HDMI"@en , "HDMI"@de ;
        :belongsToModule  "TV"@en .

:hasAudioInterfaceType
        a                   owl:ObjectProperty ;
        rdfs:comment        "Defines the type of interfaces used to transfer audio signals."@en ;
        rdfs:isDefinedBy    <http://www.ebusiness-unibw.org/ontologies/consumerelectronics/v1> ;
        rdfs:label          "audio interface type"@en , "Audioschnittstellentyp"@de ;
        rdfs:range          :AudioInterfaceType ;
        rdfs:subPropertyOf  gr:qualitativeProductOrServiceProperty ;
        :belongsToModule    "MP3Player"@en .

:SignalFormat  a          owl:Class ;
        rdfs:comment      "Type of the transmitted video format signal that is displayed by a monitor or TV panel."@en ;
        rdfs:isDefinedBy  <http://www.ebusiness-unibw.org/ontologies/consumerelectronics/v1> ;
        rdfs:label        "Signalformat"@de , "Signal format"@en ;
        rdfs:subClassOf   :TVTuner ;
        :belongsToModule  "TV"@en .

:AutomaticPictureStabilizer
        a                 :Features ;
        rdfs:comment      "A device used to stabilize a picture in order to keep it in a steady position."@en ;
        rdfs:label        "Automatic picture stabilizer"@en , "Automatischer Bildstabilisator"@de ;
        :belongsToModule  "DigitalCamera, Camcorder"@en .

:A7     a                 :MediaFormat ;
        rdfs:comment      "Format of the german institute for standardization: 74 x 105 mm."@en ;
        rdfs:label        "A7"@en , "A7"@de ;
        :belongsToModule  "Printer"@en .

:ATMT   a                 gr:BusinessEntity ;
        rdfs:comment      "ATMT"@en ;
        rdfs:label        "ATMT"^^xsd:string ;
        rdfs:seeAlso      <http://www.atmt.co.uk/> ;
        gr:legalName      "ATMT Group"^^xsd:string ;
        :belongsToModule  "MP3Player"@en .

:Netgear  a               gr:BusinessEntity ;
        rdfs:comment      "The business entity NETGEAR, Inc."@en ;
        rdfs:label        "Netgear"^^xsd:string ;
        rdfs:seeAlso      <http://www.netgear.de/> ;
        gr:legalName      "NETGEAR, Inc."^^xsd:string ;
        :belongsToModule  "MP3Player"@en .

:hasWidthWithStand  a       owl:ObjectProperty ;
        rdfs:comment        "Defines the distance between the ends of an object, its linear extent as measured from end to end with its stand (Common unit of measurement centimetre, CMT)."@en ;
        rdfs:isDefinedBy    <http://www.ebusiness-unibw.org/ontologies/consumerelectronics/v1> ;
        rdfs:label          "width with stand"@en , "Breite mit Standfuß"@de ;
        rdfs:range          gr:QuantitativeValueFloat ;
        rdfs:subPropertyOf  gr:quantitativeProductOrServiceProperty ;
        :belongsToModule    "TV"@en .

:hasHeightWithStand  a      owl:ObjectProperty ;
        rdfs:comment        "Defines the measurement of vertical distance of an object with its stand (Common unit of measurement centimetre, CMT)."@en ;
        rdfs:isDefinedBy    <http://www.ebusiness-unibw.org/ontologies/consumerelectronics/v1> ;
        rdfs:label          "height with stand"@en , "Höhe mit Standfuß"@de ;
        rdfs:range          gr:QuantitativeValueFloat ;
        rdfs:subPropertyOf  gr:quantitativeProductOrServiceProperty ;
        :belongsToModule    "TV"@en .

:Nikon  a                 gr:BusinessEntity ;
        rdfs:comment      "The business entity Nikon Corporation."@en ;
        rdfs:label        "Nikon"^^xsd:string ;
        rdfs:seeAlso      <http://www.nikon.com/> ;
        gr:legalName      "Nikon Corporation"^^xsd:string ;
        :belongsToModule  "DigitalCamera"@en .

:hasViewFinder  a           owl:ObjectProperty ;
        rdfs:comment        "A viewfinder is what the photographer looks through to compose, and in many cases to focus, the picture.\n\n(This description is partly based on or reuses content from the Wikipedia article \"Viewfinder\" (http://en.wikipedia.org/wiki/Viewfinder) and is licensed under the GNU Free Documentation License (http://www.gnu.org/copyleft/fdl.html).)"@en ;
        rdfs:isDefinedBy    <http://www.ebusiness-unibw.org/ontologies/consumerelectronics/v1> ;
        rdfs:label          "viewfinder"@en , "Bildsucher"@de ;
        rdfs:range          :ViewFinder ;
        rdfs:subPropertyOf  gr:qualitativeProductOrServiceProperty ;
        :belongsToModule    "DigitalCamera, Camcorder"@en .

:ComputerDisplayResolution_640x480_60_72_75_85Hz
        a                 :ComputerDisplayResolution ;
        rdfs:comment      "Display resolution specified as the width and height in pixels, color depth measured in bits, and refresh rate expressed in hertz; here Video Graphics Array.\n\n(This description is partly based on or reuses content from the Wikipedia article \"Display resolution\" (http://en.wikipedia.org/wiki/Display_resolution) and is licensed under the GNU Free Documentation License (http://www.gnu.org/copyleft/fdl.html).)"@en ;
        rdfs:label        "Computerbildschirmauflösung 640x480 60 72 75 85Hz"@de , "Computer display resolution 640x480 60 72 75 85Hz"@en ;
        :belongsToModule  "TV"@en .

:LabelPrinter  a          owl:Class ;
        rdfs:comment      "A label printer is a computer peripheral that prints on self-adhesive label material and sometimes card-stock (also called tags)."@en ;
        rdfs:isDefinedBy  <http://www.ebusiness-unibw.org/ontologies/consumerelectronics/v1> ;
        rdfs:label        "Label printer"@en , "Etikettendrucker"@de ;
        rdfs:subClassOf   :Printer ;
        :belongsToModule  "Printer"@en .

:Thomson  a               gr:BusinessEntity ;
        rdfs:comment      "The business entity The Thomson Corporation."@en ;
        rdfs:label        "Thomson"^^xsd:string ;
        rdfs:seeAlso      <http://www.thomson.net/> ;
        gr:legalName      "The Thomson Corporation"^^xsd:string ;
        :belongsToModule  "MP3Player, TV"@en .

:Viewpia  a               gr:BusinessEntity ;
        rdfs:comment      "The business entity Viewpia."@en ;
        rdfs:label        "Viewpia"^^xsd:string ;
        rdfs:seeAlso      <http://www.gt-24.de/> ;
        gr:legalName      "Global-Tech 24 Ltd."^^xsd:string ;
        :belongsToModule  "TV"@en .

:ODYS   a                 gr:BusinessEntity ;
        rdfs:comment      "The business entity ODYS."@en ;
        rdfs:label        "ODYS"^^xsd:string ;
        rdfs:seeAlso      <http://www.odys.de/> ;
        gr:legalName      "ODYS"^^xsd:string ;
        :belongsToModule  "MP3Player, TV, DigitalCamera, Camcorder"@en .

:MOV    a                 :DataFormatVideo ;
        rdfs:comment      "The QuickTime (.mov) file format functions as a multimedia container file that contains one or more tracks, each of which stores a particular type of data: audio, video, effects, or text (e.g. for subtitles).\n\n(This description is partly based on or reuses content from the Wikipedia article \"QuickTime\" (http://en.wikipedia.org/wiki/QuickTime) and is licensed under the GNU Free Documentation License (http://www.gnu.org/copyleft/fdl.html).)"@en ;
        rdfs:label        "MOV"@de , "MOV"@en ;
        :belongsToModule  "MP3Player, DigitalCamera, Camcorder"@en .

:MP4_Video  a             :DataFormatVideo ;
        rdfs:comment      "A collection of methods defining compression of video digital data."@en ;
        rdfs:label        "MP4 Video"@de , "MP4 Video"@en ;
        :belongsToModule  "MP3Player, DigitalCamera, Camcorder"@en .

:PhotoPrinter  a          owl:Class ;
        rdfs:comment      "A photo printer is a printer that is specifically designed to print high quality digital photos on photo paper.\n\n(This description is partly based on or reuses content from the Wikipedia article \"Photo printer\" (http://en.wikipedia.org/wiki/Photo_printer) and is licensed under the GNU Free Documentation License (http://www.gnu.org/copyleft/fdl.html).)"@en ;
        rdfs:isDefinedBy  <http://www.ebusiness-unibw.org/ontologies/consumerelectronics/v1> ;
        rdfs:label        "Fotodrucker"@de , "Photo printer"@en ;
        rdfs:subClassOf   :Printer ;
        :belongsToModule  "Printer"@en .

:VHF    a                 :SignalFormat ;
        rdfs:comment      "VHF (Very high frequency) is the radio frequency range from 30 MHz to 300 MHz.\n\n(This description is partly based on or reuses content from the Wikipedia article \"VHF\" (http://en.wikipedia.org/wiki/VHF) and is licensed under the GNU Free Documentation License (http://www.gnu.org/copyleft/fdl.html).)"@en ;
        rdfs:label        "VHF"@de , "VHF"@en ;
        :belongsToModule  "TV"@en .

:PowerLED  a              :GeneralFeatures ;
        rdfs:comment      "It is a semiconductor diode that emits light when an electric current is applied in the forward direction of the device used to show the power status of an electrical device.\n\n(This description is partly based on or reuses content from the Wikipedia article \"LED\" (http://en.wikipedia.org/wiki/Led) and is licensed under the GNU Free Documentation License (http://www.gnu.org/copyleft/fdl.html).)"@en ;
        rdfs:label        "Power LED"@en , "In-Betrieb Ledanzeige"@de ;
        :belongsToModule  "TV, Camcorder"@en .

:Windows2003  a           :CompatibleOperatingSystems ;
        rdfs:comment      "A version of a Microsoft operating system."@en ;
        rdfs:label        "Windows 2003"@de , "Windows 2003"@en ;
        :belongsToModule  "MP3Player, Printer, DigitalCamera, Camcorder"@en .

:Printer  a               owl:Class ;
        rdfs:comment      "A peripheral which produces a hard copy (permanent human-readable text and/or graphics) of documents stored in electronic form, usually on physical print media such as paper or transparencies.\n\n(This description is partly based on or reuses content from the Wikipedia article \"Printer\" (http://en.wikipedia.org/wiki/Computer_printer) and is licensed under the GNU Free Documentation License (http://www.gnu.org/copyleft/fdl.html).)"@en ;
        rdfs:isDefinedBy  <http://www.ebusiness-unibw.org/ontologies/consumerelectronics/v1> ;
        rdfs:label        "Drucker"@de , "Printer"@en ;
        rdfs:subClassOf   gr:ProductOrService ;
        :belongsToModule  "Printer"@en .

:Prestigio  a             gr:BusinessEntity ;
        rdfs:comment      "The business entity Prestigio."@en ;
        rdfs:label        "Prestigio"^^xsd:string ;
        rdfs:seeAlso      <http://www.prestigio.com/> ;
        gr:legalName      "Prestigio Plaza Ltd."^^xsd:string ;
        :belongsToModule  "TV"@en .

:DPOF   a                 :DataFormatImage ;
        rdfs:comment      "DPOF (Digital Print Order format) is a format which allows the user of a digital camera or other device such as a Mobile Phone or PDA to define which captured images on the storage card are to be printed, together with information on the number of copies or other image information such as paper size, image title text, image orientation, contact information and more.\n\n(This description is partly based on or reuses content from the Wikipedia article \"DPOF\" (http://en.wikipedia.org/wiki/DPOF) and is licensed under the GNU Free Documentation License (http://www.gnu.org/copyleft/fdl.html).)"@en ;
        rdfs:label        "DPOF"@en , "DPOF"@de ;
        :belongsToModule  "DigitalCamera, Camcorder"@en .

:AmbilightSpectra2  a     :VideoFeatures ;
        rdfs:comment      "Ambilight Spectra 2 generates reactive ambient lighting on both sides of a Flat TV."@en ;
        rdfs:label        "Ambilight Spectra 2"@de , "Ambilight Spectra 2"@en ;
        :belongsToModule  "TV"@en .

:hasDigitalVideoCaptureSpeed
        a                   owl:ObjectProperty ;
        rdfs:comment        "Speed of the process of converting an analog video signal—such as that produced by a video camera or DVD player—to digital form."@en ;
        rdfs:isDefinedBy    <http://www.ebusiness-unibw.org/ontologies/consumerelectronics/v1> ;
        rdfs:label          "digital video capture speed"@en , "digitale Videoaufnahmgeschwindigkeit"@de ;
        rdfs:range          gr:QuantitativeValueFloat ;
        rdfs:subPropertyOf  gr:quantitativeProductOrServiceProperty ;
        :belongsToModule    "Camcorder"@en .

:Phillar  a               gr:BusinessEntity ;
        rdfs:comment      "The business entity Phillar."@en ;
        rdfs:label        "Phillar"^^xsd:string ;
        gr:legalName      "Phillar electronics b. V."^^xsd:string ;
        :belongsToModule  "TV"@en .

:Envelope  a              :MediaType ;
        rdfs:comment      "Is a packaging product, usually made of flat material such as paper or cardboard."@en ;
        rdfs:label        "Briefkuvert"@de , "Envelope"@en ;
        :belongsToModule  "Printer"@en .

:Shuffle  a               :Features ;
        rdfs:comment      "Ability to play files in random order."@en ;
        rdfs:label        "Zufällige Wiedergabe"@de , "Shuffle"@en ;
        :belongsToModule  "MP3Player"@en .

:Actebis  a               gr:BusinessEntity ;
        rdfs:comment      "The business entity Actebis Peacock GmbH."@en ;
        rdfs:label        "Actebis"^^xsd:string ;
        rdfs:seeAlso      <http://www.actebis.com/> ;
        gr:legalName      "Actebis Peacock GmbH "^^xsd:string ;
        :belongsToModule  "MP3Player"@en .

:Brother  a               gr:BusinessEntity ;
        rdfs:comment      "The business entity Brother."@en ;
        rdfs:label        "Brother"^^xsd:string ;
        rdfs:seeAlso      <http://www.brother.de/> ;
        gr:legalName      "Brother International GmbH"^^xsd:string ;
        :belongsToModule  "Printer"@en .

:AVI    a                 :DataFormatVideo ;
        rdfs:comment      "A multimedia container format introduced by Microsoft."@en ;
        rdfs:label        "AVI"^^xsd:string , "AVI"@en ;
        :belongsToModule  "MP3Player, DigitalCamera, Camcorder"@en .

:ChildSafetyLock  a       :GeneralFeatures ;
        rdfs:comment      "A child safety lock is a special-purpose lock that is designed to help prevent children from getting at any dangerous contents.\n\n(This description is partly based on or reuses content from the Wikipedia article \"Child safety lock\" (http://en.wikipedia.org/wiki/Child_safety_lock) and is licensed under the GNU Free Documentation License (http://www.gnu.org/copyleft/fdl.html).)"@en ;
        rdfs:label        "Child safety lock"@en , "Kindersicherung"@de ;
        :belongsToModule  "TV"@en .

:MediaFormatEnvelope  a   :MediaFormat ;
        rdfs:comment      "Media format that is able to assume different shapes."@en ;
        rdfs:label        "Medienformat Briefkuvert"@de , "Media format Envelope"@en ;
        :belongsToModule  "Printer"@en .

:PAL    a                 :SignalFormat ;
        rdfs:comment      "PAL, short for Phase Alternating Line, is a colour-encoding system used in broadcast television systems in large parts of the world.\n\n(This description is partly based on or reuses content from the Wikipedia article \"PAL\" (http://en.wikipedia.org/wiki/PAL) and is licensed under the GNU Free Documentation License (http://www.gnu.org/copyleft/fdl.html).)"@en ;
        rdfs:label        "PAL"@de , "PAL"@en ;
        :belongsToModule  "TV"@en .

:hasSoundEmission  a        owl:ObjectProperty ;
        rdfs:comment        "Level of sound power during the printing (Common unit of measurement decibel, 2N)."@en ;
        rdfs:isDefinedBy    <http://www.ebusiness-unibw.org/ontologies/consumerelectronics/v1> ;
        rdfs:label          "sound emission"@en , "Geräuschentwicklung"@de ;
        rdfs:range          gr:QuantitativeValueFloat ;
        rdfs:subPropertyOf  gr:quantitativeProductOrServiceProperty ;
        :belongsToModule    "Printer"@en .

:Audio3.5mm  a            :AudioInterfaceType ;
        rdfs:comment      "Audio interface type of a specific diameter."@en ;
        rdfs:label        "Audio 3.5mm"@de , "Audio 3.5mm"@en ;
        :belongsToModule  "MP3Player"@en .

:DVI_out  a               :DataInterfaceType ;
        rdfs:comment      "A digital video format created by Sony, JVC, Panasonic and other video camera producers."@en ;
        rdfs:label        "DVI out"@en , "DVI out"@de ;
        :belongsToModule  "Camcorder"@en .

:NightMode  a             :SceneMode ;
        rdfs:comment      "Ability of the camcorder to adapt to special environments."@en ;
        rdfs:label        "Night mode"@en , "Nachtmodus"@de ;
        :belongsToModule  "Camcorder"@en .

:hasMaxInputCapacityForEnvelopes
        a                   owl:ObjectProperty ;
        rdfs:comment        "Defines the maximum ability to hold for envelopes."@en ;
        rdfs:isDefinedBy    <http://www.ebusiness-unibw.org/ontologies/consumerelectronics/v1> ;
        rdfs:label          "max input capacity for envelopes"@en , "maximale Menge an Briefkuvert"@de ;
        rdfs:range          gr:QuantitativeValueInteger ;
        rdfs:subPropertyOf  gr:quantitativeProductOrServiceProperty ;
        :belongsToModule    "Printer"@en .

:StorageMedia  a          owl:Class ;
        rdfs:comment      "A data storage device is a device for recording (storing) information (data).\n \n(This description is partly based on or reuses content from the Wikipedia article \"Data Storage Device\" (http://en.wikipedia.org/wiki/Data_storage_device) and is licensed under the GNU Free Documentation License (http://www.gnu.org/copyleft/fdl.html).)"@en ;
        rdfs:isDefinedBy  <http://www.ebusiness-unibw.org/ontologies/consumerelectronics/v1> ;
        rdfs:label        "Speichermedium"@de , "Storage Media"@en ;
        rdfs:subClassOf   gr:QualitativeValue ;
        :belongsToModule  "MP3Player, DigitalCamera, Camcorder"@en .

:hasEqualizerBandsQuantity
        a                   owl:ObjectProperty ;
        rdfs:comment        "Defines the number of supported equalizers."@en ;
        rdfs:isDefinedBy    <http://www.ebusiness-unibw.org/ontologies/consumerelectronics/v1> ;
        rdfs:label          "equalizer bands qunatity"@en , "Anzahl von Equalizer"@de ;
        rdfs:range          gr:QuantitativeValueInteger ;
        rdfs:subPropertyOf  gr:quantitativeProductOrServiceProperty ;
        :belongsToModule    "MP3Player, TV"@en .

:A2     a                 :MediaFormat ;
        rdfs:comment      "Format of the german institute for standardization: 420 x 594 mm."@en ;
        rdfs:label        "A2"@en , "A2"@de ;
        :belongsToModule  "Printer"@en .

:AIFF   a                 :DataFormatAudio ;
        rdfs:comment      "Audio Interchange File Format (AIFF) is an audio file format standard used for storing sound data for personal computers and other electronic audio devices.\n\n(This description is partly based on or reuses content from the Wikipedia article \"Audio Interchange File Format\" (http://en.wikipedia.org/wiki/Audio_Interchange_File_Format) and is licensed under the GNU Free Documentation License (http://www.gnu.org/copyleft/fdl.html).)"@en ;
        rdfs:label        "AIFF"@de , "AIFF"@en ;
        :belongsToModule  "MP3Player, DigitalCamera, Camcorder"@en .

:Chimei  a                gr:BusinessEntity ;
        rdfs:comment      "The business entity Chimei."@en ;
        rdfs:label        "Chimei"^^xsd:string ;
        rdfs:seeAlso      <http://www.chimei.com.tw/> ;
        gr:legalName      "CHIE MEI Optoelectronics Corp(CMO)"^^xsd:string ;
        :belongsToModule  "TV"@en .

:Konica_Minolta  a        gr:BusinessEntity ;
        rdfs:comment      "The business entity Konica Minolta."@en ;
        rdfs:label        "Konica Minolta"^^xsd:string ;
        rdfs:seeAlso      <http://www.konicaminolta.com/> ;
        gr:legalName      "Konica Minolta Holdings, Inc."^^xsd:string ;
        :belongsToModule  "Printer, DigitalCamera"@en .

:Cowon  a                 gr:BusinessEntity ;
        rdfs:comment      "The business entity COWON SYSTEMS, Inc."@en ;
        rdfs:label        "Cowon"^^xsd:string ;
        rdfs:seeAlso      <http://www.cowonglobal.com/> ;
        gr:legalName      "COWON SYSTEMS, Inc. "^^xsd:string ;
        :belongsToModule  "MP3Player"@en .

:hasVideoResolution  a      owl:DatatypeProperty ;
        rdfs:comment        "Defines the digital resolution of the videos (Common unit of measurement pixel, E37). (Example: 1024x768)"@en ;
        rdfs:isDefinedBy    <http://www.ebusiness-unibw.org/ontologies/consumerelectronics/v1> ;
        rdfs:label          "video resolution"@en , "Videoauflösung"@de ;
        rdfs:range          xsd:string ;
        rdfs:subPropertyOf  gr:datatypeProductOrServiceProperty ;
        :belongsToModule    "DigitalCamera, Camcorder"@en .

:ACAdapter  a             :PowerSupplyUnit ;
        rdfs:comment      "A linear or switched-mode power supply (or in some cases just a transformer) that is built into the top of a plug and needed for the conversion of one form of electrical power to another desired form and voltage.\n\n(This description is partly based on or reuses content from the Wikipedia article \"Power supply\" (http://en.wikipedia.org/wiki/Power_supply) and is licensed under the GNU Free Documentation License (http://www.gnu.org/copyleft/fdl.html).)"@en ;
        rdfs:label        "AC Adapter"@de , "AC Adapter"@en ;
        :belongsToModule  "MP3Player, Printer, DigitalCamera, Camcorder"@en .

:NICAM  a                 :SignalFormat ;
        rdfs:comment      "NICAM stands for Near Instantaneous Companded Audio Multiplex. It is an early form of lossy compression for digital audio.\n\n(This description is partly based on or reuses content from the Wikipedia article \"NICAM\" (http://en.wikipedia.org/wiki/NICAM) and is licensed under the GNU Free Documentation License (http://www.gnu.org/copyleft/fdl.html).)"@en ;
        rdfs:label        "NICAM"@de , "NICAM"@en ;
        :belongsToModule  "TV"@en .

:GameMode  a              :GeneralFeatures ;
        rdfs:comment      "A special mode providing more performance of the television to optimize pictures when games are played on a LCD or plasma panel."@en ;
        rdfs:label        "Game mode"@en , "Spielemodus"@de ;
        :belongsToModule  "TV"@en .

:OutdoorWhiteBalance  a   :WhiteBalance ;
        rdfs:comment      "Ability to adapt of different adjustments of the intensities of the colors."@en ;
        rdfs:label        "Outdoor white balance"@en , "Weißabgleich außen"@de ;
        :belongsToModule  "Camcorder"@en .

:RS-232  a                :Connectivity ;
        rdfs:comment      "In telecommunications, RS-232 (Recommended Standard 232) is a standard for serial binary data signals connecting between a DTE (Data Terminal Equipment) and a DCE (Data Circuit-terminating Equipment). It is commonly used in computer serial ports.\n\n(This description is partly based on or reuses content from the Wikipedia article \"RS-232\" (http://en.wikipedia.org/wiki/RS-232) and is licensed under the GNU Free Documentation License (http://www.gnu.org/copyleft/fdl.html).)"@en ;
        rdfs:label        "RS-232"@de , "RS-232"@en ;
        :belongsToModule  "TV"@en .

:Daewoo  a                gr:BusinessEntity ;
        rdfs:comment      "The business entity Daewoo."@en ;
        rdfs:label        "Daewoo"^^xsd:string ;
        rdfs:seeAlso      <http://www.daewoo-electronics.de/> ;
        gr:legalName      "Daewoo Electronics"^^xsd:string ;
        :belongsToModule  "TV"@en .

:hasDRMSupport  a           owl:DatatypeProperty ;
        rdfs:comment        "Defines the support of a generic term that refers to access control technologies used by hardware manufacturers."@en ;
        rdfs:isDefinedBy    <http://www.ebusiness-unibw.org/ontologies/consumerelectronics/v1> ;
        rdfs:label          "DRM support"@en , "DRM Unterstützung"@de ;
        rdfs:range          xsd:boolean ;
        rdfs:subPropertyOf  gr:datatypeProductOrServiceProperty ;
        :belongsToModule    "MP3Player"@en .

:SceneMode  a             owl:Class ;
        rdfs:comment      "A projection of information from any physical environment into any sensory system."@en ;
        rdfs:isDefinedBy  <http://www.ebusiness-unibw.org/ontologies/consumerelectronics/v1> ;
        rdfs:label        "Scene mode"@en , "Szenenmodus"@de ;
        rdfs:subClassOf   gr:QualitativeValue ;
        :belongsToModule  "Camcorder"@en .

:SanDisk  a               gr:BusinessEntity ;
        rdfs:comment      "The business entity SanDisk Corporation."@en ;
        rdfs:label        "Sandisk"^^xsd:string ;
        rdfs:seeAlso      <http://sandisk.de/> ;
        gr:legalName      "SanDisk Corporation"^^xsd:string ;
        :belongsToModule  "MP3Player"@en .

:PictureInPicture  a      :VideoFeatures ;
        rdfs:comment      "Picture in Picture (PiP) is a feature of some television receivers and similar devices. One program (channel) is displayed on the full TV screen at the same time as one or more other programs are displayed in inset windows. Sound is usually from the main program only.\n\n(This description is partly based on or reuses content from the Wikipedia article \"Picture in picture\" (http://en.wikipedia.org/wiki/Picture-in-picture) and is licensed under the GNU Free Documentation License (http://www.gnu.org/copyleft/fdl.html).)"@en ;
        rdfs:label        "Bild in Bild Funktion"@de , "Picture in Picture"@en ;
        :belongsToModule  "TV"@en .

:MediaType  a             owl:Class ;
        rdfs:comment      "The type of paper a device is able to handle."@en ;
        rdfs:isDefinedBy  <http://www.ebusiness-unibw.org/ontologies/consumerelectronics/v1> ;
        rdfs:label        "Mediumart"@en , "Media type"^^xsd:string ;
        rdfs:subClassOf   gr:QualitativeValue ;
        :belongsToModule  "Printer"@en .

:Panasonic  a             gr:BusinessEntity ;
        rdfs:comment      "The business entity Panasonic Corporation."@en ;
        rdfs:label        "Panasonic"^^xsd:string ;
        rdfs:seeAlso      <http://www.panasonic.com/> ;
        gr:legalName      "Panasonic Corporation"^^xsd:string ;
        :belongsToModule  "MP3Player, TV, Printer, DigitalCamera, Camcorder"@en .

:AVCH   a                 :DataFormatVideo ;
        rdfs:comment      "A high-definition and standard-definition recording format for use in digital tapeless camcorders. The format is comparable to other handheld video camera recording formats, particularly HDV and TOD.\n\n(This description is partly based on or reuses content from the Wikipedia article \"HDV\" (http://en.wikipedia.org/wiki/HDV) and is licensed under the GNU Free Documentation License (http://www.gnu.org/copyleft/fdl.html).)"@en ;
        rdfs:label        "AVCH"@en , "AVCH"@de ;
        :belongsToModule  "Camcorder"@en .

:hasColorBalance  a         owl:DatatypeProperty ;
        rdfs:comment        "In photography and image processing, color balance is the global adjustment of the intensities of the colors (typically red, green, and blue primary colors).\n\n(This description is partly based on or reuses content from the Wikipedia article \"White balance\" (http://en.wikipedia.org/wiki/White_balance) and is licensed under the GNU Free Documentation License (http://www.gnu.org/copyleft/fdl.html).)"@en ;
        rdfs:isDefinedBy    <http://creativecommons.org/licenses/by/3.0/> ;
        rdfs:label          "color balance"@en , "Farbabgleich"@de ;
        rdfs:range          xsd:boolean ;
        rdfs:subPropertyOf  gr:datatypeProductOrServiceProperty ;
        :belongsToModule    "DigitalCamera"@en .

:Beige  a                 :Color ;
        rdfs:comment      "RGB Value 245,245,220"@en ;
        rdfs:label        "Beige"@de , "Beige"@en ;
        :belongsToModule  "MP3Player, TV, Printer, DigitalCamera, Camcorder"@en .

:White  a                 :Color ;
        rdfs:comment      "RGB Value 255,255,255"@en ;
        rdfs:label        "Weiß"@de , "White"@en ;
        :belongsToModule  "MP3Player, TV, Printer, DigitalCamera, Camcorder"@en .

:DV     a                 :DataFormatVideo ;
        rdfs:comment      "Digital Video (DV) is a digital video format created by Sony, JVC, Panasonic and other video camera producers, and launched in 1995. The DV specification (originally known as the Blue Book, current official name IEC 61834) defines both the codec and the tape format.\n\n(This description is partly based on or reuses content from the Wikipedia article \"DV\" (http://en.wikipedia.org/wiki/DV) and is licensed under the GNU Free Documentation License (http://www.gnu.org/copyleft/fdl.html).)"@en ;
        rdfs:label        "DV"@en , "DV"@de ;
        :belongsToModule  "DigitalCamera, Camcorder"@en .

:DigitalCamera  a         owl:Class ;
        rdfs:comment      "A digital camera (or digicam for short) is a camera that takes video or still photographs, or both, digitally by recording images via an electronic image sensor.\n\n(This description is partly based on or reuses content from the Wikipedia article \"Digital camera\" (http://en.wikipedia.org/wiki/Digital_camera) and is licensed under the GNU Free Documentation License (http://www.gnu.org/copyleft/fdl.html).)"@en ;
        rdfs:isDefinedBy  <http://www.ebusiness-unibw.org/ontologies/consumerelectronics/v1> ;
        rdfs:label        "Digital camera"@en , "Digitalkamera"@de ;
        rdfs:subClassOf   gr:ProductOrService ;
        :belongsToModule  "DigitalCamera"^^xsd:string .

:BluetoothAudio  a        :AudioInterfaceType ;
        rdfs:comment      "Bluetooth is a wireless protocol utilizing short-range communications technology facilitating data transmission over short distances from fixed and mobile devices, creating wireless personal area networks (refers to audio)."@en ;
        rdfs:label        "Bluetooth Audio"@de , "Bluetooth audio"@en ;
        :belongsToModule  "MP3Player"@en .

:B5     a                 :MediaFormat ;
        rdfs:comment      "Format of the german institute for standardization: 176 x 250 mm."@en ;
        rdfs:label        "B5"@en , "B5"@de ;
        :belongsToModule  "Printer"@en .

:S-Video_in  a            :DataInterfaceType ;
        rdfs:comment      "Is an analog video signal that carries the video data as two separate signals, lumen (luminance) and chroma (color).\n\n(This description is partly based on or reuses content from the Wikipedia article \"S-Video\" (http://en.wikipedia.org/wiki/S-Video) and is licensed under the GNU Free Documentation License (http://www.gnu.org/copyleft/fdl.html).)"@en ;
        rdfs:label        "S-Video in"@en , "S-Video in"@de ;
        :belongsToModule  "TV, Camcorder"@en .

:S-Video_out  a           :DataInterfaceType ;
        rdfs:comment      "Is an analog video signal that carries the video data as two separate signals, lumen (luminance) and chroma (color).\n\n(This description is partly based on or reuses content from the Wikipedia article \"S-Video\" (http://en.wikipedia.org/wiki/S-Video) and is licensed under the GNU Free Documentation License (http://www.gnu.org/copyleft/fdl.html).)"@en ;
        rdfs:label        "S-Video out"@en , "S-Video out"@de ;
        :belongsToModule  "Camcorder"@en .

:hasTVTuner  a              owl:ObjectProperty ;
        rdfs:comment        "Defines the type of included TV tuner."@en ;
        rdfs:domain         :TV ;
        rdfs:isDefinedBy    <http://www.ebusiness-unibw.org/ontologies/consumerelectronics/v1> ;
        rdfs:label          "TV Tuner"^^xsd:string , "TV Tuner"@de ;
        rdfs:range          :TVTuner ;
        rdfs:subPropertyOf  gr:qualitativeProductOrServiceProperty ;
        :belongsToModule    "TV"@en .

:Lexar  a                 gr:BusinessEntity ;
        rdfs:comment      "The business entity Lexar Media, Inc."@en ;
        rdfs:label        "Lexar"^^xsd:string ;
        rdfs:seeAlso      <http://www.lexar.com/> ;
        gr:legalName      "Lexar Media, Inc. "^^xsd:string ;
        :belongsToModule  "MP3Player"@en .

:BenQ   a                 gr:BusinessEntity ;
        rdfs:comment      "The business entity BenQ Corporation."@en ;
        rdfs:label        "BenQ"^^xsd:string ;
        rdfs:seeAlso      <http://www.aoc-europe.com/> ;
        gr:legalName      "BenQ Corporation"^^xsd:string ;
        :belongsToModule  "MP3Player, TV, DigitalCamera"@en .

:Timer  a                 :GeneralFeatures ;
        rdfs:comment      "A timer is a specialized type of clock counting backwards to a predefined end.\n\n(This description is partly based on or reuses content from the Wikipedia article \"Timer\" (http://en.wikipedia.org/wiki/Timer) and is licensed under the GNU Free Documentation License (http://www.gnu.org/copyleft/fdl.html).)"@en ;
        rdfs:label        "Timer"@en , "Zeitgeber"@de ;
        :belongsToModule  "TV"@en .

:TRSConnector  a          :Connectivity ;
        rdfs:comment      "A TRS connector (tip, ring, sleeve) also called an audio jack, phone plug, jack plug, stereo plug, mini-jack, or mini-stereo, is a common audio connector. It is cylindrical in shape, typically with three contacts, although sometimes with two (a TS connector) or four (a TRRS connector).\n\n(This description is partly based on or reuses content from the Wikipedia article \"TRS connector\" (http://en.wikipedia.org/wiki/TRS_connector) and is licensed under the GNU Free Documentation License (http://www.gnu.org/copyleft/fdl.html).)"@en ;
        rdfs:label        "TRS Verbindungsstecker"@de , "TRS connector"@en ;
        :belongsToModule  "TV"@en .

:MemoryStick  a           :StorageMedia ;
        rdfs:comment      "Memory Stick is a removable flash memory card format."@en ;
        rdfs:label        "MemoryStick"@en , "MemoryStick"@de ;
        :belongsToModule  "MP3Player, DigitalCamera, Camcorder"@en .

:hasPrintBorderTop  a       owl:ObjectProperty ;
        rdfs:comment        "Defines the area which can not be printed on the top side of a paper (A4) (Common unit of measurement millimetre, MMT)."@en ;
        rdfs:isDefinedBy    <http://www.ebusiness-unibw.org/ontologies/consumerelectronics/v1> ;
        rdfs:label          "print border top"@en , "Druckgrenze oben"@de ;
        rdfs:range          gr:QuantitativeValueFloat ;
        rdfs:subPropertyOf  gr:quantitativeProductOrServiceProperty ;
        :belongsToModule    "Printer"@en .

:PhotoMode  a             :SceneMode ;
        rdfs:comment      "Ability of the camcorder to adapt to special environments."@en ;
        rdfs:label        "Photo mode"@en , "Photo modus"@de ;
        :belongsToModule  "Camcorder"@en .

:InternalFlashMemory  a   :StorageMedia ;
        rdfs:comment      "Flash memory is non-volatile computer memory that can be electrically erased and reprogrammed."@en ;
        rdfs:label        "Internal flash memory"@en , "Interner Flashspeicher"@de ;
        :belongsToModule  "MP3Player, DigitalCamera, Camcorder"@en .

:SVG    a                 :DataFormatImage ;
        rdfs:comment      "SVG (Scalable Vector Graphics) is an open standard created and developed by the World Wide Web Consortium to address the need (and attempts of several corporations) for a versatile, scriptable and all-purpose vector format for the web and otherwise.\n\n(This description is partly based on or reuses content from the Wikipedia article \"Vector graphics\" (http://en.wikipedia.org/wiki/Vector_graphics) and is licensed under the GNU Free Documentation License (http://www.gnu.org/copyleft/fdl.html).)"@en ;
        rdfs:label        "SVG"@de , "SVG"@en ;
        :belongsToModule  "MP3Player, , DigitalCamera, Camcorder"@en .

:Label  a                 :MediaType ;
        rdfs:comment      "Media type that can be printed on one side and has a glued area on the other side."@en ;
        rdfs:label        "Label"@en , "Etikett"@de ;
        :belongsToModule  "Printer"@en .

:Iiyama  a                gr:BusinessEntity ;
        rdfs:comment      "The business entity Iiyama."@en ;
        rdfs:label        "Iiyama"^^xsd:string ;
        rdfs:seeAlso      <http://www.iiyama.com/> ;
        gr:legalName      "Iiyama"^^xsd:string ;
        :belongsToModule  "TV"@en .

:New_Universe  a          gr:BusinessEntity ;
        rdfs:comment      "The business entity New Universe B.V."@en ;
        rdfs:label        "New Universe"^^xsd:string ;
        rdfs:seeAlso      <http://www.nu-europe.com/> ;
        gr:legalName      "New Universe B.V."^^xsd:string ;
        :belongsToModule  "MP3Player, TV"@en .

:hasWhiteBalance  a         owl:ObjectProperty ;
        rdfs:comment        "Defines the global adjustment of the intensities of the colors."@en ;
        rdfs:isDefinedBy    <http://www.ebusiness-unibw.org/ontologies/consumerelectronics/v1> ;
        rdfs:label          "white balance"@en , "Weißabgleich"@de ;
        rdfs:range          :WhiteBalance ;
        rdfs:subPropertyOf  gr:qualitativeProductOrServiceProperty ;
        :belongsToModule    "Camcorder"@en .

:MPIO   a                 gr:BusinessEntity ;
        rdfs:comment      "The business entity MPIO Inc."@en ;
        rdfs:label        "MPIO"^^xsd:string ;
        rdfs:seeAlso      <http://www.mpio.com/> ;
        gr:legalName      "MPIO Inc."^^xsd:string ;
        :belongsToModule  "MP3Player"@en .

:Dane-Elec  a             gr:BusinessEntity ;
        rdfs:comment      "The business entity Dane-Elec GmbH."@en ;
        rdfs:label        "Dane-Elec"^^xsd:string ;
        rdfs:seeAlso      <http://www.dane-elec.com/> ;
        gr:legalName      "Dane-Elec GmbH"^^xsd:string ;
        :belongsToModule  "MP3Player"@en .

:Oki    a                 gr:BusinessEntity ;
        rdfs:comment      "The business entity Oki."@en ;
        rdfs:label        "Oki"^^xsd:string ;
        rdfs:seeAlso      <http://www.oki.com/> ;
        gr:legalName      "Oki Electric Industry Co., Ltd."^^xsd:string ;
        :belongsToModule  "TV, Printer"@en .

:Hannspree  a             gr:BusinessEntity ;
        rdfs:comment      "The business entity Hannspree."@en ;
        rdfs:label        "Hannspree"^^xsd:string ;
        rdfs:seeAlso      <http://www.hannspree.com/> ;
        gr:legalName      "Hannspree Inc."^^xsd:string ;
        :belongsToModule  "TV"@en .

:DigitalImageScalingTechnology
        a                 :VideoFeatures ;
        rdfs:comment      "Seamlessly up-scales any video source to display at full high definition 1080p."@en ;
        rdfs:label        "Digital Image Scaling Technology"@de , "Digital Image Scaling Technology"@en ;
        :belongsToModule  "TV"@en .

:hasSensorType  a           owl:ObjectProperty ;
        rdfs:comment        "Defines type of device that measures a physical quantity and converts it into a signal which can be read by an observer or by an instrument."@en ;
        rdfs:isDefinedBy    <http://www.ebusiness-unibw.org/ontologies/consumerelectronics/v1> ;
        rdfs:label          "sensor type"@en , "Sensorart"@de ;
        rdfs:range          :SensorType ;
        rdfs:subPropertyOf  gr:qualitativeProductOrServiceProperty ;
        :belongsToModule    "Camcorder"@en .

:Aigo   a                 gr:BusinessEntity ;
        rdfs:comment      "The business entity Beijing Huaqi Information Digital Technology Co., Ltd."@en ;
        rdfs:label        "Aigo"^^xsd:string ;
        rdfs:seeAlso      <http://www.aigo.com/> ;
        gr:legalName      "Beijing Huaqi Information Digital Technology Co., Ltd."^^xsd:string ;
        :belongsToModule  "MP3Player"@en .

:hasAspectRatioHorizontal
        a                   owl:DatatypeProperty ;
        rdfs:comment        "The aspect ratio of a shape is the ratio of its longer dimension to its shorter dimension. The vertical dimension is the longer one.\n\n(This description is partly based on or reuses content from the Wikipedia article \"Aspect ratio\" (http://en.wikipedia.org/wiki/Aspect_ratio) and is licensed under the GNU Free Documentation License (http://www.gnu.org/copyleft/fdl.html).)"@en ;
        rdfs:isDefinedBy    <http://www.ebusiness-unibw.org/ontologies/consumerelectronics/v1> ;
        rdfs:label          "aspect ratio horizontal"@en , "horizontales Bildseitenverhältnis"@de ;
        rdfs:range          xsd:float ;
        rdfs:subPropertyOf  gr:datatypeProductOrServiceProperty ;
        :belongsToModule    "TV"@en .

:TunerType  a             owl:Class ;
        rdfs:comment      "Type of TV tuner that is used to convert RF television transmissions into audio and video signals.\n\n(This description is partly based on or reuses content from the Wikipedia article \"Tuner (electronics)\" (http://en.wikipedia.org/wiki/Tuner_(electronics)) and is licensed under the GNU Free Documentation License (http://www.gnu.org/copyleft/fdl.html).)"@en ;
        rdfs:isDefinedBy  <http://www.ebusiness-unibw.org/ontologies/consumerelectronics/v1> ;
        rdfs:label        "Tuner Typ"@de , "Tuner type"@en ;
        rdfs:subClassOf   :TVTuner ;
        :belongsToModule  "TV"@en .

:hasFocalLength  a          owl:ObjectProperty ;
        rdfs:comment        "Defines a measure of how strongly it converges (focuses) or diverges (diffuses) light.\n\n(This description is partly based on or reuses content from the Wikipedia article \"Focal length\" (http://en.wikipedia.org/wiki/Focal_length) and is licensed under the GNU Free Documentation License (http://www.gnu.org/copyleft/fdl.html).)"@en ;
        rdfs:isDefinedBy    <http://www.ebusiness-unibw.org/ontologies/consumerelectronics/v1> ;
        rdfs:label          "focal length"@en , "Brennweite"@de ;
        rdfs:range          gr:QuantitativeValueFloat ;
        rdfs:subPropertyOf  gr:quantitativeProductOrServiceProperty ;
        :belongsToModule    "Camcorder"@en .

:hasMinMediaWeight  a       owl:ObjectProperty ;
        rdfs:comment        "Describes the minimum weight of the media format (Common unit of measurement gram per square metre, GM)."@en ;
        rdfs:isDefinedBy    <http://www.ebusiness-unibw.org/ontologies/consumerelectronics/v1> ;
        rdfs:label          "min media weight"@en , "minimales Mediengewicht"@de ;
        rdfs:range          gr:QuantitativeValueFloat ;
        rdfs:subPropertyOf  gr:quantitativeProductOrServiceProperty ;
        :belongsToModule    "Printer"@en .

:DuplexPrint  a           :Features ;
        rdfs:comment      "A feature of computer printers and MFPs that allows the automatic printing of a sheet of paper on both sides."@en ;
        rdfs:label        "Duplex print"@en , "Duplexdruck"@de ;
        :belongsToModule  "Printer"@en .

:Fujifilm  a              gr:BusinessEntity ;
        rdfs:comment      "The business entity Fujifilm Holdings Corporation."@en ;
        rdfs:label        "Fujifilm"^^xsd:string ;
        rdfs:seeAlso      <http://www.fujifilm.com/> ;
        gr:legalName      "Fujifilm Holdings Corporation"^^xsd:string ;
        :belongsToModule  "DigitalCamera"@en .

<http://www.ebusiness-unibw.org/ontologies/consumerelectronics/v1>
        a             owl:Ontology ;
        rdfs:comment  "The CEO: Consumer Electronics Ontology is a vocabulary for describing typical consumer electronics products and services and their features, e.g. digital cameras, camcorders, etc.\nIt can be used in combination with GoodRelations, http://purl.org/goodrelations/ for making your e-commerce offerings available in the new Web of Data.\n\nSeveral descriptions of conceptual elements in this ontology are partly based on or reuse content from respective Wikipedia articles in the English Wikipedia http://en.wikipedia.org/wiki/. Thus, this ontology is also licensed under the GNU Free Documentation License, http://www.gnu.org/copyleft/fdl.html."@en ;
        rdfs:label    "CEO: Consumer Electronics Ontology - An Ontology for Consumer Electronics Products and Services"@en ;
        rdfs:seeAlso  <http://www.rdf4ecommerce.org/> ;
        dc:creator    "Xaver Brandl, Christian Deckert, Felix Frommer, Daniel Karl, Daniel Koslowski, Daniel Schley, David Sonntag, Andreas Wechselberger, and Martin Hepp"@en ;
        dc:rights     "http://creativecommons.org/licenses/by/3.0/"@en ;
        dc:subject    "E-Commerce, E-Business, GoodRelations, Ontology, MP3 player, TV, Printer, DigitalCamera, Camcorder"@en ;
        dc:title      "CEO: Consumer Electronics Ontology - An Ontology for Consumer Electronics Products and Services"@en ;
        owl:imports   <http://purl.org/goodrelations/v1> .

:HDTV_720p  a             :TVDisplayResolution ;
        rdfs:comment      "720p is the shorthand name for a category of HDTV video modes. The number 720 stands for the 720 vertical scan lines of display resolution (also known as 720 pixels of vertical resolution), while the letter p stands for progressive scan or non-interlaced.\n\n(This description is partly based on or reuses content from the Wikipedia article \"720p\" (http://en.wikipedia.org/wiki/720p) and is licensed under the GNU Free Documentation License (http://www.gnu.org/copyleft/fdl.html).)"@en ;
        rdfs:label        "HDTV 720p"@de , "HDTV 720p"@en ;
        :belongsToModule  "TV"@en .

:AIPTEK  a                gr:BusinessEntity ;
        rdfs:comment      "The business entity AIPTEK, Inc."@en ;
        rdfs:label        "AIPTEK"^^xsd:string ;
        rdfs:seeAlso      <http://www.aiptek.com/> ;
        gr:legalName      "AIPTEK, Inc."^^xsd:string ;
        :belongsToModule  "DigitalCamera, Camcorder"@en .

:B0     a                 :MediaFormat ;
        rdfs:comment      "Format of the german institute for standardization: 1000 x 1414 mm."@en ;
        rdfs:label        "B0"@en , "B0"@de ;
        :belongsToModule  "Printer"@en .

:hasTouchscreen  a          owl:DatatypeProperty ;
        rdfs:comment        "Defines the ability to operate an object by touching its screen."@en ;
        rdfs:isDefinedBy    <http://www.ebusiness-unibw.org/ontologies/consumerelectronics/v1> ;
        rdfs:label          "touch screen"@en , "Sensorbildschirm"@de ;
        rdfs:range          xsd:boolean ;
        rdfs:subPropertyOf  gr:datatypeProductOrServiceProperty ;
        :belongsToModule    "MP3Player, Printer, DigitalCamera, Camcorder"@en .

:Cardstock  a             :MediaType ;
        rdfs:comment      "A paper stock that is thicker and more durable than normal writing or printing paper, but thinner and more flexible than other forms of paperboard.\n\n(This description is partly based on or reuses content from the Wikipedia article \"Cardstock\" (http://en.wikipedia.org/wiki/Card_stock) and is licensed under the GNU Free Documentation License (http://www.gnu.org/copyleft/fdl.html).)"@en ;
        rdfs:label        "cardstock"@en , "Fotokarton"@de ;
        :belongsToModule  "Printer"@en .

:hasOpticalZoom  a          owl:DatatypeProperty ;
        rdfs:comment        "Defines a method of decreasing (narrowing) the apparent angle of view of a digital photographic or video image with a higher optical resolution than the digital zoom."@en ;
        rdfs:isDefinedBy    <http://www.ebusiness-unibw.org/ontologies/consumerelectronics/v1> ;
        rdfs:label          "optical zoom"@en , "optischer Zoom"@de ;
        rdfs:range          xsd:boolean ;
        rdfs:subPropertyOf  gr:datatypeProductOrServiceProperty ;
        :belongsToModule    "DigitalCamera"@en .

:Sitecom  a               gr:BusinessEntity ;
        rdfs:comment      "The business entity Sitecom"@en ;
        rdfs:label        "Sitecom"^^xsd:string ;
        rdfs:seeAlso      <http://www.sitecom.com/> ;
        gr:legalName      "Sitecom"^^xsd:string ;
        :belongsToModule  "MP3Player"@en .

:GeneralFeatures  a       owl:Class ;
        rdfs:comment      "Additional general equipment and abilities."@en ;
        rdfs:isDefinedBy  <http://www.ebusiness-unibw.org/ontologies/consumerelectronics/v1> ;
        rdfs:label        "General Features"@en , "Allgemeine Eigenschaften"@de ;
        rdfs:subClassOf   :Features ;
        :belongsToModule  "TV"@en .

:PowerPC_32_bit  a        :ProcessorType ;
        rdfs:comment      "A RISC instruction set architecture created by the 1991 Apple-IBM-Motorola alliance, known as AIM. Originally intended for personal computers, PowerPC CPUs have since become popular embedded and high-performance processors."@en ;
        rdfs:label        "PowerPC 32 bit"@en , "PowerPC 32 bit"@de ;
        :belongsToModule  "Printer"@en .

:HeadphoneLineOut_2.5mm
        a                 :Connectivity ;
        rdfs:comment      "Port to connect headphones with an electronical device. Here the port has the diameter of 2,5 millimetres."@en ;
        rdfs:label        "Kopfhörerausgang 2.5 mm"@de , "Headphone line out 2.5mm"@en ;
        :belongsToModule  "TV"@en .

:Brown  a                 :Color ;
        rdfs:comment      "RGB Value 165,42,42"@en ;
        rdfs:label        "Braun"@de , "Brown"@en ;
        :belongsToModule  "MP3Player, TV, Printer, DigitalCamera, Camcorder"@en .

:WhiteBalance  a          owl:Class ;
        rdfs:comment      "Is the global adjustment of the intensities of the colors (typically red, green, and blue primary colors). An important goal of this adjustment is to render specific colors - particularly neutral colors - correctly; hence, the general method is sometimes called gray balance, neutral balance, or white balance.\n\n(This description is partly based on or reuses content from the Wikipedia article \"White Balance\" (http://en.wikipedia.org/wiki/White_Balance) and is licensed under the GNU Free Documentation License (http://www.gnu.org/copyleft/fdl.html).)"@en ;
        rdfs:isDefinedBy  <http://www.ebusiness-unibw.org/ontologies/consumerelectronics/v1> ;
        rdfs:label        "Weißabgleich"@de , "White balance"@en ;
        rdfs:subClassOf   gr:QualitativeValue ;
        :belongsToModule  "Camcorder"@en .

:Canyon  a                gr:BusinessEntity ;
        rdfs:comment      "The business entity Canyon."@en ;
        rdfs:label        "Canyon"^^xsd:string ;
        rdfs:seeAlso      <http://www.canyon-tech.it/> ;
        gr:legalName      "Canyon"^^xsd:string ;
        :belongsToModule  "MP3Player"@en .

:hasFrequencyRange  a       owl:ObjectProperty ;
        rdfs:comment        "Defines the range of supported frequency signals (Common unit of measurement megahertz, MHZ)."@en ;
        rdfs:isDefinedBy    <http://www.ebusiness-unibw.org/ontologies/consumerelectronics/v1> ;
        rdfs:label          "frequency range"@en , "Frequenzberich"@de ;
        rdfs:range          gr:QuantitativeValueFloat ;
        rdfs:subPropertyOf  gr:quantitativeProductOrServiceProperty ;
        :belongsToModule    "MP3Player"@en .

:hasNumberOfDisplayColors
        a                   owl:ObjectProperty ;
        rdfs:comment        "Defines the number of colors an electronical device is able to display on a screen."@en ;
        rdfs:isDefinedBy    <http://www.ebusiness-unibw.org/ontologies/consumerelectronics/v1> ;
        rdfs:label          "number of display colors"@en , "Anzahl von Bildschirmfarben"@de ;
        rdfs:range          gr:QuantitativeValueInteger ;
        rdfs:subPropertyOf  gr:quantitativeProductOrServiceProperty ;
        :belongsToModule    "MP3Player, TV, Printer, DigitalCamera, Camcorder"@en .

:Headphones  a            :Accessory ;
        rdfs:comment      "A pair of small loudspeakers, or less commonly a single speaker, with a way of holding them close to a user's ears and a means of connecting them to a signal source such as an audio amplifier, radio or CD player."@en ;
        rdfs:label        "Headphones"@en , "Kopfhörer"@de ;
        :belongsToModule  "Camcorder"@en .

:Griffin  a               gr:BusinessEntity ;
        rdfs:comment      "The business entity Griffin Technology."@en ;
        rdfs:label        "Griffin"^^xsd:string ;
        rdfs:seeAlso      <http://www.griffintechnology.com/> ;
        gr:legalName      "Griffin Technology"^^xsd:string ;
        :belongsToModule  "MP3Player"@en .

:Guillemot  a             gr:BusinessEntity ;
        rdfs:comment      "The business entity Guillemot Corporation."@en ;
        rdfs:label        "Guillemot"^^xsd:string ;
        rdfs:seeAlso      <http://www.guillemot.biz/> ;
        gr:legalName      "Guillemot Corporation"^^xsd:string ;
        :belongsToModule  "MP3Player"@en .

:Medion  a                gr:BusinessEntity ;
        rdfs:comment      "The business entity Medion AG."@en ;
        rdfs:label        "Medion"^^xsd:string ;
        rdfs:seeAlso      <http://www.medion.com/> ;
        gr:legalName      "Medion AG"^^xsd:string ;
        :belongsToModule  "MP3Player, TV"@en .

:belongsToModule  a       owl:AnnotationProperty ;
        rdfs:comment      "Describes to which product categories the property or concept belongs (comma seperated, e.g. \"MP3Player, TV\")."@en ;
        rdfs:isDefinedBy  <http://www.ebusiness-unibw.org/ontologies/consumerelectronics/v1> .

:OnOffTimer  a            :GeneralFeatures ;
        rdfs:comment      "Describes the possibility to maintain a designated  time when the television or electrical device should be switched off or on automatically."@en ;
        rdfs:label        "On off timer"@en , "Ein- und Ausschalttimer"@de ;
        :belongsToModule  "TV"@en .

:hasInternalMemoryCapacity
        a                   owl:ObjectProperty ;
        rdfs:comment        "Defines the capacity to store data on internal memory (Common unit of measurement Megabyte, 4L)."@en ;
        rdfs:isDefinedBy    <http://www.ebusiness-unibw.org/ontologies/consumerelectronics/v1> ;
        rdfs:label          "internal memory capacity"@en , "interner Speicherplatz"@de ;
        rdfs:range          gr:QuantitativeValueFloat ;
        rdfs:subPropertyOf  gr:quantitativeProductOrServiceProperty ;
        :belongsToModule    "MP3Player, Printer, DigitalCamera, Camcorder"@en .

:A9     a                 :MediaFormat ;
        rdfs:comment      "Format of the german institute for standardization: 37 x 52 mm."@en ;
        rdfs:label        "A9"@en , "A9"@de ;
        :belongsToModule  "Printer"@en .

:hasFlash  a                owl:DatatypeProperty ;
        rdfs:comment        "Device for instantaneous illumination for picture taking."@en ;
        rdfs:isDefinedBy    <http://www.ebusiness-unibw.org/ontologies/consumerelectronics/v1> ;
        rdfs:label          "flash"@en , "Blitz"@de ;
        rdfs:range          xsd:boolean ;
        rdfs:subPropertyOf  gr:datatypeProductOrServiceProperty ;
        :belongsToModule    "DigitalCamera"@en .

:hasMaxMediaWeight  a       owl:ObjectProperty ;
        rdfs:comment        "Describes the maximum weight of the media format (Common unit of measurement gram per square metre, GM)."@en ;
        rdfs:isDefinedBy    <http://www.ebusiness-unibw.org/ontologies/consumerelectronics/v1> ;
        rdfs:label          "max media weight"@en , "maximales Mediengewicht"@de ;
        rdfs:range          gr:QuantitativeValueFloat ;
        rdfs:subPropertyOf  gr:quantitativeProductOrServiceProperty ;
        :belongsToModule    "Printer"@en .

:CGM    a                 :DataFormatImage ;
        rdfs:comment      "CGM (Computer Graphics Metafile) is a file format for 2D vector graphics, raster graphics, and text, and is defined by ISO/IEC 8632.\n\n(This description is partly based on or reuses content from the Wikipedia article \"Computer Graphics Metafile\" (http://en.wikipedia.org/wiki/Computer_Graphics_Metafile) and is licensed under the GNU Free Documentation License (http://www.gnu.org/copyleft/fdl.html).)"@en ;
        rdfs:label        "CGM"@de , "CGM"@en ;
        :belongsToModule  "MP3Player, DigitalCamera, Camcorder"@en .

:TrekStor  a              gr:BusinessEntity ;
        rdfs:comment      "The business entity TrekStore GmbH & Co. KG"@en ;
        rdfs:label        "Trekstor"^^xsd:string ;
        rdfs:seeAlso      <http://www.trekstor.de/> ;
        gr:legalName      "TrekStor GmbH & Co. KG"^^xsd:string ;
        :belongsToModule  "MP3Player"@en .

:Seiko  a                 gr:BusinessEntity ;
        rdfs:comment      "The business entity Seiko."@en ;
        rdfs:label        "Seiko"^^xsd:string ;
        rdfs:seeAlso      <http://www.seikoinstruments.com/> ;
        gr:legalName      "Seiko Holdings Corporation"^^xsd:string ;
        :belongsToModule  "Printer"@en .

:hasNumberOfHDMIPorts
        a                   owl:ObjectProperty ;
        rdfs:comment        "Number of compact audio/video interface ports for transmitting uncompressed digital data."@en ;
        rdfs:isDefinedBy    <http://www.ebusiness-unibw.org/ontologies/consumerelectronics/v1> ;
        rdfs:label          "number of HDMI ports"@en , "Anzahl HDMI Anschlussmöglichkeiten"@de ;
        rdfs:range          gr:QuantitativeValueInteger ;
        rdfs:subPropertyOf  gr:quantitativeProductOrServiceProperty ;
        :belongsToModule    "Camcorder"@en .

:AudioFeatures  a         owl:Class ;
        rdfs:comment      "Additional audio equipment and abilities."@en ;
        rdfs:isDefinedBy  <http://www.ebusiness-unibw.org/ontologies/consumerelectronics/v1> ;
        rdfs:label        "Audio Features"@en , "Audio Eigenschaften"@de ;
        rdfs:subClassOf   :Features ;
        :belongsToModule  "TV"@en .

:hasWeight  a               owl:ObjectProperty ;
        rdfs:comment        "Defines the measurement of the gravitational force acting on an object (Common unit of measurement gramm, GRM)."@en ;
        rdfs:isDefinedBy    <http://www.ebusiness-unibw.org/ontologies/consumerelectronics/v1> ;
        rdfs:label          "weight"@en , "Gewicht"@de ;
        rdfs:range          gr:QuantitativeValueFloat ;
        rdfs:subPropertyOf  gr:quantitativeProductOrServiceProperty ;
        :belongsToModule    "MP3Player, TV, Printer, DigitalCamera, Camcorder"@en .

:Logitech  a              gr:BusinessEntity ;
        rdfs:comment      "The business entity Logitech International S.A."@en ;
        rdfs:label        "Logitech"^^xsd:string ;
        rdfs:seeAlso      <http://www.logitech.com/> ;
        gr:legalName      "Logitech International S.A."^^xsd:string ;
        :belongsToModule  "DigitalCamera"@en .

:WindowsXP  a             :CompatibleOperatingSystems ;
        rdfs:comment      "A version of a Microsoft operating system."@en ;
        rdfs:label        "Windows XP"@de , "Windows XP"@en ;
        :belongsToModule  "MP3Player, Printer, DigitalCamera, Camcorder"@en .

:DL     a                 :MediaFormat ;
        rdfs:comment      "Format of the german institute for standardization: 110 x 220 mm."@en ;
        rdfs:label        "DL"@en , "DL"@de ;
        :belongsToModule  "Printer"@en .

:TwinMOS  a               gr:BusinessEntity ;
        rdfs:comment      "The business entity TwinMOS Technologies Inc"@en ;
        rdfs:label        "TwinMOS"^^xsd:string ;
        rdfs:seeAlso      <http://www.twinmos.com/> ;
        gr:legalName      "TwinMOS Technologies Inc"^^xsd:string ;
        :belongsToModule  "MP3Player"@en .

:hasDisplayType  a          owl:ObjectProperty ;
        rdfs:comment        "Defines the type of the display like LCD or Plasma."@en ;
        rdfs:isDefinedBy    <http://www.ebusiness-unibw.org/ontologies/consumerelectronics/v1> ;
        rdfs:label          "display type"@en , "Bildschirmtyp"@de ;
        rdfs:range          :DisplayType ;
        rdfs:subPropertyOf  gr:qualitativeProductOrServiceProperty ;
        :belongsToModule    "MP3Player, TV, Printer, Camcorder"@en .

:Freecom  a               gr:BusinessEntity ;
        rdfs:comment      "The business entity Freecom Technologies GmbH."@en ;
        rdfs:label        "Freecom"^^xsd:string ;
        rdfs:seeAlso      <http://www.freecom.de/> ;
        gr:legalName      "Freecom Technologies GmbH"^^xsd:string ;
        :belongsToModule  "MP3Player"@en .

:ProgressiveScan  a       :VideoFeatures ;
        rdfs:comment      "Progressive or noninterlaced scanning is a method for displaying, storing or transmitting moving images in which all the lines of each frame are drawn in sequence.\n\n(This description is partly based on or reuses content from the Wikipedia article \"Progressive scan\" (http://en.wikipedia.org/wiki/Progressive_scan) and is licensed under the GNU Free Documentation License (http://www.gnu.org/copyleft/fdl.html).)"@en ;
        rdfs:label        "Progressive Scan"@de , "Progressive Scan"@en ;
        :belongsToModule  "TV"@en .

:Snapshot  a              :Features ;
        rdfs:comment      "Is a shot that is aimed and fired very quickly at a target that appears suddenly and for a very short period of time."@en ;
        rdfs:label        "Snapshot"@en , "Snapshot"@de ;
        :belongsToModule  "Camcorder"@en .

:hasMaxColorPrintSpeedDraft
        a                   owl:ObjectProperty ;
        rdfs:comment        "Amount of pages per minute the product is able to print in the mode of color-printig of drafts."@en ;
        rdfs:isDefinedBy    <http://www.ebusiness-unibw.org/ontologies/consumerelectronics/v1> ;
        rdfs:label          "max color print speed draft"@en , "maximale Druckgeschwindigkeit Farbe Entwurf"@de ;
        rdfs:range          gr:QuantitativeValueFloat ;
        rdfs:subPropertyOf  gr:quantitativeProductOrServiceProperty ;
        :belongsToModule    "Printer"@en .

:Eaconn  a                gr:BusinessEntity ;
        rdfs:comment      "The business entity EACONN B.V."@en ;
        rdfs:label        "Eaconn"^^xsd:string ;
        rdfs:seeAlso      <http://www.eaconn.com/> ;
        gr:legalName      "EACONN B.V."^^xsd:string ;
        :belongsToModule  "MP3Player"@en .

:hasMaxMemoryCapacity
        a                   owl:ObjectProperty ;
        rdfs:comment        "Defines the maxium capacity that can be provided by using external memory (Common unit of measurement megabyte, 4L)."@en ;
        rdfs:isDefinedBy    <http://www.ebusiness-unibw.org/ontologies/consumerelectronics/v1> ;
        rdfs:label          "maximale memory capacity"@en , "maximale Speicherkapazität"@de ;
        rdfs:range          gr:QuantitativeValueFloat ;
        rdfs:subPropertyOf  gr:quantitativeProductOrServiceProperty ;
        :belongsToModule    "MP3Player, DigitalCamera, Camcorder"@en .

:PrintResolution  a       owl:Class ;
        rdfs:comment      "Defines the maximum digital resolution the device is able to print."@en ;
        rdfs:isDefinedBy  <http://www.ebusiness-unibw.org/ontologies/consumerelectronics/v1> ;
        rdfs:label        "Print resolution"@en , "Druckauflösung"@de ;
        rdfs:subClassOf   :SupportedResolution ;
        :belongsToModule  "Printer"@en .

:hasNumberOfComponentVideoPorts
        a                   owl:DatatypeProperty ;
        rdfs:comment        "Defines the number of component video ports a device offers."@en ;
        rdfs:isDefinedBy    <http://www.ebusiness-unibw.org/ontologies/consumerelectronics/v1> ;
        rdfs:label          "number of component video ports"@en , "Anzahl an Component Vido Ports"@de ;
        rdfs:range          xsd:int ;
        rdfs:subPropertyOf  gr:datatypeProductOrServiceProperty ;
        :belongsToModule    "Camcorder"@en .

:NoiseReduction  a        :AudioFeatures ;
        rdfs:comment      "Noise reduction is the process of removing noise from a signal."@en ;
        rdfs:label        "Geräuschunterdrückung"@de , "Noise reduction"@en ;
        :belongsToModule  "TV"@en .

:hasMinOperatingTemperature
        a                   owl:ObjectProperty ;
        rdfs:comment        "Defines the minimum temperature the product is able to operate (Common unit of measurement grad celsius, CEL)."@en ;
        rdfs:isDefinedBy    <http://www.ebusiness-unibw.org/ontologies/consumerelectronics/v1> ;
        rdfs:label          "min operating temperature"@en , "minimale Betriebstemperatur"@de ;
        rdfs:range          gr:QuantitativeValueFloat ;
        rdfs:subPropertyOf  gr:quantitativeProductOrServiceProperty ;
        :belongsToModule    "TV, Printer"@en .

:CTX    a                 gr:BusinessEntity ;
        rdfs:comment      "The business entity CTX."@en ;
        rdfs:label        "CTX"^^xsd:string ;
        rdfs:seeAlso      <http://www.ctxeurope.com/> ;
        gr:legalName      "CTX Technology Corporation"^^xsd:string ;
        :belongsToModule  "TV"@en .

:IntegratedClock  a       :GeneralFeatures ;
        rdfs:comment      "Clock integrated in a device."@en ;
        rdfs:label        "Integrated clock"@en , "Integrierte Uhr"@de ;
        :belongsToModule  "TV"@en .

:Digital  a               :TunerType ;
        rdfs:comment      "A digital system uses discrete (discontinuous) values, usually but not always symbolized numerically (hence called \"digital\") to represent information for input, processing, transmission, storage.\n\n(This description is partly based on or reuses content from the Wikipedia article \"Digital\" (http://en.wikipedia.org/wiki/Digital) and is licensed under the GNU Free Documentation License (http://www.gnu.org/copyleft/fdl.html).)"@en ;
        rdfs:label        "Digital"@en , "Digital"@de ;
        :belongsToModule  "TV"@en .

:MacOSXLeopard  a         :CompatibleOperatingSystems ;
        rdfs:comment      "Mac OS is the trademarked name for a series of graphical user interface-based operating systems developed by Apple Inc. for their Macintosh line of computer systems."@en ;
        rdfs:label        "Mac OS X Leopard"@de , "Mac OS X Leopard"@en ;
        :belongsToModule  "MP3Player, Printer, DigitalCamera, Camcorder"@en .

:hasStandardOutputCapacity
        a                   owl:ObjectProperty ;
        rdfs:comment        "Number of sheets the product can hold in all available output trays as a standard."@en ;
        rdfs:isDefinedBy    <http://www.ebusiness-unibw.org/ontologies/consumerelectronics/v1> ;
        rdfs:label          "standard output capacity"@en , "Standard Ausgabkapazität"@de ;
        rdfs:range          gr:QuantitativeValueInteger ;
        rdfs:subPropertyOf  gr:quantitativeProductOrServiceProperty .

:Sanyo  a                 gr:BusinessEntity ;
        rdfs:comment      "The business entity Sanyo."@en ;
        rdfs:label        "Sanyo"^^xsd:string ;
        rdfs:seeAlso      <http://sanyo.com/> ;
        gr:legalName      "SANYO Electric Co., Ltd."^^xsd:string ;
        :belongsToModule  "TV, DigitalCamera, Camcorder"@en .

:ScreenFormatAdjustments
        a                 :VideoFeatures ;
        rdfs:comment      "Includes the possibility to switch between different screen formats."@en ;
        rdfs:label        "Bildschirmformatanpassung"@de , "Screen format adjustments"@en ;
        :belongsToModule  "TV"@en .

:Photopaper  a            :MediaType ;
        rdfs:comment      "Kind of paper that is specifically designed to print high quality digital photos."@en ;
        rdfs:label        "Photo paper"@en , "Fotopapier"@de ;
        :belongsToModule  "Printer"@en .

:Color  a                 owl:Class ;
        rdfs:comment      "Color derives from the spectrum of light interacting in the eye with the spectral sensitivities of the light receptors.\n\n(This description is partly based on or reuses content from the Wikipedia article \"Color\" (http://en.wikipedia.org/wiki/Color) and is licensed under the GNU Free Documentation License (http://www.gnu.org/copyleft/fdl.html).)"@en ;
        rdfs:isDefinedBy  <http://www.ebusiness-unibw.org/ontologies/consumerelectronics/v1> ;
        rdfs:label        "Color"@en , "Farbe"@de ;
        rdfs:subClassOf   gr:QualitativeValue ;
        :belongsToModule  "MP3Player, TV, Printer, DigitalCamera, Camcorder"@en .

:USB2.0  a                :DataInterfaceType ;
        rdfs:comment      "Maximum speed of 480 Mbit/s."@en ;
        rdfs:label        "USB 2.0"@de , "USB 2.0"@en ;
        :belongsToModule  "MP3Player, TV, Printer, DigitalCamera, Camcorder"@en .

:EDTV_480p  a             :TVDisplayResolution ;
        rdfs:comment      "480p is the shorthand name for a video display resolution. The p stands for progressive scan, i.e. non-interlaced. The 480 denotes a vertical resolution of 480 vertically scanning lines, usually with a horizontal resolution of 640 pixels and 4:3 aspect ratio or a horizontal resolution of 854 pixels and 16:9 aspect ratio.\n\n(This description is partly based on or reuses content from the Wikipedia article \"480p\" (http://en.wikipedia.org/wiki/480p) and is licensed under the GNU Free Documentation License (http://www.gnu.org/copyleft/fdl.html).)"@en ;
        rdfs:label        "EDTV 480p"@en , "EDTV 480p"@de ;
        :belongsToModule  "TV"@en .

:hasPictureResolution
        a                   owl:ObjectProperty ;
        rdfs:comment        "Defines the digital resolution of the pictures (Common unit of measurement pixel, E37)."@en ;
        rdfs:isDefinedBy    <http://www.ebusiness-unibw.org/ontologies/consumerelectronics/v1> ;
        rdfs:label          "picture resolution"@en , "Fotoauflösung"@de ;
        rdfs:range          gr:QuantitativeValueFloat ;
        rdfs:subPropertyOf  gr:quantitativeProductOrServiceProperty ;
        :belongsToModule    "DigitalCamera, Camcorder"@en .

:PDP    a             :DisplayType ;
        rdfs:comment  "A plasma display panel (PDP) is a type of flat panel display common to large TV displays (37in. [940mm]). Many tiny cells between two panels of glass hold an inert mixture of noble gases. The gas in the cells is electrically turned into a plasma which then excites phosphors to emit light.\n\n(This description is partly based on or reuses content from the Wikipedia article \"Digital newspaper technology - Plasma\" (http://en.wikipedia.org/wiki/Digital_newspaper_technology#Plasma) and is licensed under the GNU Free Documentation License (http://www.gnu.org/copyleft/fdl.html).)"@en ;
        rdfs:label    "PDP"@de , "PDP"@en .

:DVB    a                 :SignalFormat ;
        rdfs:comment      "Digital Video Broadcasting (DVB) is a suite of internationally accepted open standards for digital television. DVB systems distribute data using a variety of approaches, including by satellite (DVB-S, DVB-S2 and DVB-SH; also DVB-SMATV for distribution via SMATV); cable (DVB-C); terrestrial television (DVB-T, DVB-T2) and digital terrestrial television for handhelds (DVB-H,DVB-SH); and via microwave using DTT (DVB-MT), the MMDS (DVB-MC), and/or MVDS standards (DVB-MS).\n\n(This description is partly based on or reuses content from the Wikipedia article \"Digital Video Broadcasting\" (http://en.wikipedia.org/wiki/Digital_Video_Broadcasting) and is licensed under the GNU Free Documentation License (http://www.gnu.org/copyleft/fdl.html).)"@en ;
        rdfs:label        "DVB"@de , "DVB"@en ;
        :belongsToModule  "TV"@en .

:ViewFinderOptical  a     :ViewFinder ;
        rdfs:comment      "An optical viewfinder is simply a reversed telescope mounted to see what the camera will see.\n\n(This description is partly based on or reuses content from the Wikipedia article \"Viewfinder\" (http://en.wikipedia.org/wiki/Viewfinder) and is licensed under the GNU Free Documentation License (http://www.gnu.org/copyleft/fdl.html).)"@en ;
        rdfs:label        "Optischer Bildsucher"@de , "Viewfinder optical"@en ;
        :belongsToModule  "DigitalCamera"@en .

:hasOpticalSensorSize
        a                   owl:ObjectProperty ;
        rdfs:comment        "Size of the device that measures a physical quantity and converts it into a signal which can be read by an observer or by an instrument (common unit of measurement: inch; INH)."@en ;
        rdfs:label          "optical sensor size"@en , "optischer Sensorgröße"@de ;
        rdfs:range          gr:QuantitativeValueFloat ;
        rdfs:seeAlso        <http://www.ebusiness-unibw.org/ontologies/consumerelectronics/v1> ;
        rdfs:subPropertyOf  gr:quantitativeProductOrServiceProperty ;
        :belongsToModule    "Camcorder"@en .

:USB    a                 owl:Class ;
        rdfs:comment      "Universal Serial Bus (USB) is a serial bus standard to connect devices to a host computer.\n\n(This description is partly based on or reuses content from the Wikipedia article \"Universal Serial Bus\" (http://en.wikipedia.org/wiki/Universal_Serial_Bus) and is licensed under the GNU Free Documentation License (http://www.gnu.org/copyleft/fdl.html).)"@en ;
        rdfs:isDefinedBy  <http://www.ebusiness-unibw.org/ontologies/consumerelectronics/v1> ;
        rdfs:label        "USB"@de , "USB"@en ;
        rdfs:subClassOf   :EnergySource ;
        :belongsToModule  "MP3Player, Printer, DigitalCamera, Camcorder"@en .

:Portrait  a              :SceneMode ;
        rdfs:comment      "Ability of the camcorder to adapt to special environments."@en ;
        rdfs:label        "Portrait"@de , "Portrait"@en ;
        :belongsToModule  "Camcorder"@en .

:hasContrastRatio  a        owl:DatatypeProperty ;
        rdfs:comment        "The contrast ratio is a measure of a display system, defined as the ratio of the luminance of the brightest color (white) to that of the darkest color (black) that the system is capable of producing.\n\n(This description is partly based on or reuses content from the Wikipedia article \"Contrast ratio\" (http://en.wikipedia.org/wiki/Contrast_ratio) and is licensed under the GNU Free Documentation License (http://www.gnu.org/copyleft/fdl.html).)"@en ;
        rdfs:isDefinedBy    <http://www.ebusiness-unibw.org/ontologies/consumerelectronics/v1> ;
        rdfs:label          "contrast ratio"@en , "Kontrastverhältnis"@de ;
        rdfs:range          xsd:string ;
        rdfs:subPropertyOf  gr:datatypeProductOrServiceProperty ;
        :belongsToModule    "TV"@en .

:ComputerDisplayResolution_1024x768_60_70_75_85Hz
        a                 :ComputerDisplayResolution ;
        rdfs:comment      "Display resolution specified as the width and height in pixels, color depth measured in bits, and refresh rate expressed in hertz; here Extended Graphics Array.\n\n(This description is partly based on or reuses content from the Wikipedia article \"Display resolution\" (http://en.wikipedia.org/wiki/Display_resolution) and is licensed under the GNU Free Documentation License (http://www.gnu.org/copyleft/fdl.html).)"@en ;
        rdfs:label        "Computerbildschirmauflösung 1024x768 60 70 75 85Hz"@de , "Computer display resolution 1024x768 60 70 75 85Hz"@en ;
        :belongsToModule  "TV"@en .

:Mirai  a                 gr:BusinessEntity ;
        rdfs:comment      "The business entity Mirai."@en ;
        rdfs:label        "Mirai"^^xsd:string ;
        rdfs:seeAlso      <http://www.mirai.eu/> ;
        gr:legalName      "Mirai"^^xsd:string ;
        :belongsToModule  "TV"@en .

:PSD    a                 :DataFormatImage ;
        rdfs:comment      "The .PSD (Photoshop Document) format stores an image with support for most imaging options available in Photoshop. These include layers with masks, color spaces, ICC profiles, transparency, text, alpha channels and spot colors, clipping paths, and duotone settings.\n\n(This description is partly based on or reuses content from the Wikipedia article \"Adobe Photoshop\" (http://en.wikipedia.org/wiki/Adobe_Photoshop) and is licensed under the GNU Free Documentation License (http://www.gnu.org/copyleft/fdl.html).)"@en ;
        rdfs:label        "PSD"@de , "PSD"@en ;
        :belongsToModule  "MP3Player, DigitalCamera, Camcorder"@en .

:Olivetti  a              gr:BusinessEntity ;
        rdfs:comment      "The business entity Olivetti."@en ;
        rdfs:label        "Olivetti"^^xsd:string ;
        rdfs:seeAlso      <http://www.olivetti.com/> ;
        gr:legalName      "Olivetti Tecnost"^^xsd:string ;
        :belongsToModule  "Printer"@en .

:HeadphoneLineOut_3.5mm
        a                 :Connectivity ;
        rdfs:comment      "Port to connect headphones with an electronical device. Here the port has the diameter of 3,5 millimetres."@en ;
        rdfs:label        "Kopfhörerausgang 3,5 mm"@de , "Headphone line out 3,5 mm"@en ;
        :belongsToModule  "TV"@en .

:Aiwa   a                 gr:BusinessEntity ;
        rdfs:comment      "The business entity Sony Corporation."@en ;
        rdfs:label        "Aiwa"^^xsd:string ;
        rdfs:seeAlso      <http://www.aiwa.com/> ;
        gr:legalName      "Sony Corporation  "^^xsd:string ;
        :belongsToModule  "MP3Player"@en .

:A4     a                 :MediaFormat ;
        rdfs:comment      "Format of the german institute for standardization: 210 x 297 mm."@en ;
        rdfs:label        "A4"@en , "A4"@de ;
        :belongsToModule  "Printer"@en .

:AAC-LC  a                :DataFormatAudio ;
        rdfs:comment      "Advanced Audio Coding (AAC) is a standardized, lossy compression and encoding scheme for digital audio.\n\n(This description is partly based on or reuses content from the Wikipedia article \"Advanced Audio Coding\" (http://en.wikipedia.org/wiki/Advanced_Audio_Coding) and is licensed under the GNU Free Documentation License (http://www.gnu.org/copyleft/fdl.html).)"@en ;
        rdfs:label        "AAC-LC"@de , "AAC-LC"@en ;
        :belongsToModule  "MP3Player, DigitalCamera, Camcorder"@en .

:hasPrintBorderBottom
        a                   owl:ObjectProperty ;
        rdfs:comment        "Defines the area which can not be printed on the bottom side of a paper (A4) (Common unit of measurement millimetre, MMT)."@en ;
        rdfs:isDefinedBy    <http://www.ebusiness-unibw.org/ontologies/consumerelectronics/v1> ;
        rdfs:label          "print border bottom"@en , "Druckgrenze unten"@de ;
        rdfs:range          gr:QuantitativeValueFloat ;
        rdfs:subPropertyOf  gr:quantitativeProductOrServiceProperty ;
        :belongsToModule    "Printer"@en .

:H.264  a                 :DataFormatVideo ;
        rdfs:comment      "H.264 is a standard for video compression, and is equivalent to MPEG-4 Part 10, or MPEG-4 AVC (for Advanced Video Coding). As of 2008, it is the latest block-oriented motion-compensation-based codec standard developed by the ITU-T Video Coding Experts Group (VCEG) together with the ISO/IEC Moving Picture Experts Group (MPEG), and it was the product of a partnership effort known as the Joint Video Team (JVT).\n\n(This description is partly based on or reuses content from the Wikipedia article \"H.264\" (http://en.wikipedia.org/wiki/H.264) and is licensed under the GNU Free Documentation License (http://www.gnu.org/copyleft/fdl.html).)"@en ;
        rdfs:label        "H.264"@de , "H.264"@en ;
        :belongsToModule  "MP3Player, DigitalCamera, Camcorder"@en .

:Apple  a                 gr:BusinessEntity ;
        rdfs:comment      "The business entity Apple, Inc."@en ;
        rdfs:label        "Apple"^^xsd:string ;
        rdfs:seeAlso      <http://www.apple.com/> ;
        gr:legalName      "Apple Inc."^^xsd:string ;
        :belongsToModule  "MP3Player"@en .

:MacOSXPuma  a            :CompatibleOperatingSystems ;
        rdfs:comment      "Mac OS is the trademarked name for a series of graphical user interface-based operating systems developed by Apple Inc. for their Macintosh line of computer systems."@en ;
        rdfs:label        "Mac OS X Puma"@de , "Mac OS X Puma"@en ;
        :belongsToModule  "MP3Player, Printer, DigitalCamera, Camcorder"@en .

:WMV    a                 :DataFormatVideo ;
        rdfs:comment      "A compressed video file format for several proprietary codecs developed by Microsoft."@en ;
        rdfs:label        "WMV"@de , "WMV"@en ;
        :belongsToModule  "MP3Player, DigitalCamera, Camcorder"@en .

:hasNumberOfPrintCartridges
        a                   owl:ObjectProperty ;
        rdfs:comment        "Number of replaceable components of a printer that contains the ink that is spread on paper during printing."@en ;
        rdfs:isDefinedBy    <http://www.ebusiness-unibw.org/ontologies/consumerelectronics/v1> ;
        rdfs:label          "number of print cartridges"@en , "Anzahl von Druckerkassetten"@de ;
        rdfs:range          gr:QuantitativeValueInteger ;
        rdfs:subPropertyOf  gr:quantitativeProductOrServiceProperty ;
        :belongsToModule    "Printer"@en .

:Windows2000  a           :CompatibleOperatingSystems ;
        rdfs:comment      "A version of a Microsoft operating system."@en ;
        rdfs:label        "Windows 2000"@de , "Windows 2000"@en ;
        :belongsToModule  "MP3Player, Printer, DigitalCamera, Camcorder"@en .

:hasPackageHeight  a        owl:ObjectProperty ;
        rdfs:comment        "Defines the measurement of vertical distance of an object with its package (Common unit of measurement centimetre, CMT)."@en ;
        rdfs:isDefinedBy    <http://www.ebusiness-unibw.org/ontologies/consumerelectronics/v1> ;
        rdfs:label          "package height"@en , "Verpackungshöhe"@de ;
        rdfs:range          gr:QuantitativeValueFloat ;
        rdfs:subPropertyOf  gr:quantitativeProductOrServiceProperty ;
        :belongsToModule    "TV"@en .

:hasMaxBlackWhitePrintSpeedBestQuality
        a                   owl:ObjectProperty ;
        rdfs:comment        "Amount of pages per minute the product is able to print in the mode of black-printig best quality."@en ;
        rdfs:isDefinedBy    <http://www.ebusiness-unibw.org/ontologies/consumerelectronics/v1> ;
        rdfs:label          "max black white print speed best quality"@en , "maximale Druckgeschwindigkeit Schwarz/Weiß beste Qualität"@de ;
        rdfs:range          gr:QuantitativeValueFloat ;
        rdfs:subPropertyOf  gr:quantitativeProductOrServiceProperty ;
        :belongsToModule    "Printer"@en .

:Coby   a                 gr:BusinessEntity ;
        rdfs:comment      "The business entity Coby Electronics Corporation."@en ;
        rdfs:label        "Coby"^^xsd:string ;
        rdfs:seeAlso      <http://www.cobyusa.com/> ;
        gr:legalName      "Coby Electronics Corporation"^^xsd:string ;
        :belongsToModule  "MP3Player, TV"@en .

:Decktron  a              gr:BusinessEntity ;
        rdfs:comment      "The business entity Decktron Europe GmbH."@en ;
        rdfs:label        "Decktron"^^xsd:string ;
        rdfs:seeAlso      <http://decktron.de/> ;
        gr:legalName      "Decktron Europe GmbH"^^xsd:string ;
        :belongsToModule  "MP3Player"@en .

:hasDisplay  a              owl:DatatypeProperty ;
        rdfs:comment        "Defines if object includes a screen."@en ;
        rdfs:isDefinedBy    <http://www.ebusiness-unibw.org/ontologies/consumerelectronics/v1> ;
        rdfs:label          "display"@en , "Bildschirm"@de ;
        rdfs:range          xsd:boolean ;
        rdfs:subPropertyOf  gr:datatypeProductOrServiceProperty ;
        :belongsToModule    "MP3Player, Printer, DigitalCamera, Camcorder"@en .

:Humax  a                 gr:BusinessEntity ;
        rdfs:comment      "The business entity Humax."@en ;
        rdfs:label        "Humax"^^xsd:string ;
        rdfs:seeAlso      <http://www.humaxdigital.com/> ;
        gr:legalName      "HUMAX Electronics Co Ltd."^^xsd:string ;
        :belongsToModule  "TV"^^xsd:string .

:hasRedEyeReduction  a      owl:DatatypeProperty ;
        rdfs:comment        "The red-eye effect in photography is the common appearance of red pupils in color photographs of eyes. The red-eye reduction feature reduces the red-eye effect."@en ;
        rdfs:isDefinedBy    <http://www.ebusiness-unibw.org/ontologies/consumerelectronics/v1> ;
        rdfs:label          "red eye reduction"@en , "Rote-Augen-Effekt Reduktion"@de ;
        rdfs:range          xsd:boolean ;
        rdfs:subPropertyOf  gr:datatypeProductOrServiceProperty ;
        :belongsToModule    "DigitalCamera"@en .

:Multicolor  a            :DisplayType ;
        rdfs:comment      "Ability to display more than two different kinds of color."@en ;
        rdfs:label        "Mehrfarbig"@de , "Multicolor"@en ;
        :belongsToModule  "MP3Player"@en .

:Eizo   a                 gr:BusinessEntity ;
        rdfs:comment      "The business entity Eizo."@en ;
        rdfs:label        "Eizo"^^xsd:string ;
        rdfs:seeAlso      <http://www.eizo.com/> ;
        gr:legalName      "Eizo Nano Technologies Inc."^^xsd:string ;
        :belongsToModule  "TV"@en .

:ZoomDigital  a           :Zoom ;
        rdfs:comment      "Zoom is a method of decreasing (narrowing) the apparent angle of view of a photographic or video image.\n\n(This description is partly based on or reuses content from the Wikipedia article \"Digital zoom\" (http://en.wikipedia.org/wiki/Digital_zoom) and is licensed under the GNU Free Documentation License (http://www.gnu.org/copyleft/fdl.html).)"@en ;
        rdfs:label        "Zoom digital"@en , "Digitaler Zoom"@de ;
        :belongsToModule  "DigitalCamera"@en .

:hasDataInterfaceType
        a                   owl:ObjectProperty ;
        rdfs:comment        "Defines the type of interfaces used to exchange data."@en ;
        rdfs:isDefinedBy    <http://www.ebusiness-unibw.org/ontologies/consumerelectronics/v1> ;
        rdfs:label          "data interface type"@en , "Datenschnittstellentyp"@de ;
        rdfs:range          :DataInterfaceType ;
        rdfs:subPropertyOf  gr:qualitativeProductOrServiceProperty ;
        :belongsToModule    "MP3Player, DigitalCamera, Camcorder"@en .

:B7     a                 :MediaFormat ;
        rdfs:comment      "Format of the german institute for standardization: 88 x 125 mm."@en ;
        rdfs:label        "B7"@en , "B7"@de ;
        :belongsToModule  "Printer"@en .

:AV     a                 :Connectivity ;
        rdfs:comment      "Audio connectors and video connectors are electrical connectors for carrying an audio signal or video signal, either in an analog or digital format. Analog A/V connectors often use shielded cable to inhibit RF interference and noise.\n\n(This description is partly based on or reuses content from the Wikipedia article \"Audio and video connector\" (http://en.wikipedia.org/wiki/Audio_and_video_connector) and is licensed under the GNU Free Documentation License (http://www.gnu.org/copyleft/fdl.html).)"@en ;
        rdfs:label        "AV"@de , "AV"@en ;
        :belongsToModule  "TV"@en .

:MMC    a                 :StorageMedia ;
        rdfs:comment      "A solid state disk or flash memory data storage device."@en ;
        rdfs:label        "MMC"@de , "MMC"@en ;
        :belongsToModule  "MP3Player, DigitalCamera, Camcorder"@en .

:Kye_Genius  a            gr:BusinessEntity ;
        rdfs:comment      "The business entity Genius, KYE Systems Corp."@en ;
        rdfs:label        "Kye Genius"^^xsd:string ;
        rdfs:seeAlso      <http://www.geniusnet.com/> ;
        gr:legalName      "Genius, KYE Systems Corp."^^xsd:string ;
        :belongsToModule  "MP3Player, Camcorder"@en .

:hasConnectivity  a         owl:ObjectProperty ;
        rdfs:comment        "Defines the possibilities to connect different kinds of electronical devices."@en ;
        rdfs:isDefinedBy    <http://www.ebusiness-unibw.org/ontologies/consumerelectronics/v1> ;
        rdfs:label          "connectivity"@en , "Verbindungsmöglichkeit"@de ;
        rdfs:range          :Connectivity ;
        rdfs:subPropertyOf  gr:qualitativeProductOrServiceProperty ;
        :belongsToModule    "TV"@en .

:Olive  a                 :Color ;
        rdfs:comment      "RGB Value 128,128,0"@en ;
        rdfs:label        "Olivgrün"@de , "Olive"@en ;
        :belongsToModule  "MP3Player, TV, Printer, DigitalCamera, Camcorder"@en .

:hasAudioOutputPower  a     owl:ObjectProperty ;
        rdfs:comment        "Defines the rate of energy conversion (Common unit of Measurement milliwatt, C31)."@en ;
        rdfs:isDefinedBy    <http://www.ebusiness-unibw.org/ontologies/consumerelectronics/v1> ;
        rdfs:label          "audio output power"@en , "Audioausgangsleistung"@de ;
        rdfs:subPropertyOf  :hasOutputPower ;
        :belongsToModule    "TV"^^xsd:string .

:hasNormalPrintableResolutionBlackWhiteVertical
        a                   owl:ObjectProperty ;
        rdfs:comment        "Defines the  digital resolution of the vertical axe (Common unit of measurement pixel, E37) for black/white prints for normal prints."@en ;
        rdfs:isDefinedBy    <http://www.ebusiness-unibw.org/ontologies/consumerelectronics/v1> ;
        rdfs:label          "normal printable resolution black white vertical"@en , "vertikale druckbare Auflösung Schwarz/Weiß normal"@de ;
        rdfs:range          gr:QuantitativeValueInteger ;
        rdfs:subPropertyOf  gr:quantitativeProductOrServiceProperty ;
        :belongsToModule    "Printer"@en .

:Li-Ion_Polymer  a        :RechargeableEnergySource ;
        rdfs:comment      "Lithium polymer batteries (abbreviated Li-poly, Li-Pol, LiPo, LIP, PLI or LiP) are rechargeable batteries which have technologically evolved from lithium-ion batteries.\n\n(This description is partly based on or reuses content from the Wikipedia article \"Lithium-polymer\" (http://en.wikipedia.org/wiki/Lithium-polymer) and is licensed under the GNU Free Documentation License (http://www.gnu.org/copyleft/fdl.html).)"@en ;
        rdfs:label        "Li-ion Polymer"@de , "Li-ion Polymer"@en ;
        :belongsToModule  "MP3Player, DigitalCamera, Camcorder"@en .

:BacklightMode  a         :Features ;
        rdfs:comment      "Ability to photograph against a light source."@en ;
        rdfs:label        "Backlight mode"@en , "Hintergrundbeleuchtungsmodus"@de ;
        :belongsToModule  "DigitalCamera, Camcorder"@en .

:hasDurationToPrintFirstPage
        a                   owl:ObjectProperty ;
        rdfs:comment        "Amount of time the printer needs to start printing the first page."@en ;
        rdfs:isDefinedBy    <http://www.ebusiness-unibw.org/ontologies/consumerelectronics/v1> ;
        rdfs:label          "duration to print first page"@en , "Zeitspanne bis Druck erster Seite"@de ;
        rdfs:range          gr:QuantitativeValueFloat ;
        rdfs:subPropertyOf  gr:quantitativeProductOrServiceProperty ;
        :belongsToModule    "Printer"@en .

:hasLightExposureControl
        a                   owl:DatatypeProperty ;
        rdfs:comment        "Defines the total amount of light allowed to fall on the photographic medium (photographic film or image sensor) during the process of taking a photograph."@en ;
        rdfs:isDefinedBy    <http://www.ebusiness-unibw.org/ontologies/consumerelectronics/v1> ;
        rdfs:label          "light exposure control"@en , "Belichtungsregelung"@de ;
        rdfs:range          xsd:boolean ;
        rdfs:subPropertyOf  gr:datatypeProductOrServiceProperty ;
        :belongsToModule    "Camcorder"@en .

:hasNormalPrintableResolutionBlackWhiteHorizontal
        a                   owl:ObjectProperty ;
        rdfs:comment        "Defines the digital resolution of the horizontal axe (Common unit of measurement pixel, E37) for black/white prints for normal prints."@en ;
        rdfs:isDefinedBy    <http://www.ebusiness-unibw.org/ontologies/consumerelectronics/v1> ;
        rdfs:label          "normal printable resolution black white horizontal"@en , "horizontale druckbare Auflösung Schwarz/Weiß normal"@de ;
        rdfs:range          gr:QuantitativeValueInteger ;
        rdfs:subPropertyOf  gr:quantitativeProductOrServiceProperty ;
        :belongsToModule    "Printer"@en .

:Grundig  a               gr:BusinessEntity ;
        rdfs:comment      "The business entity GRUNDIG Intermedia GmbH."@en ;
        rdfs:label        "Grundig"^^xsd:string ;
        rdfs:seeAlso      <http://www.grundig.de/> ;
        gr:legalName      "GRUNDIG Intermedia GmbH "^^xsd:string ;
        :belongsToModule  "MP3Player, TV"@en .

:OGG    a                 :DataFormatAudio ;
        rdfs:comment      "Ogg is a free, open standard container format maintained by the Xiph.Org Foundation."@en ;
        rdfs:label        "OGG"@de , "OGG"@en ;
        :belongsToModule  "MP3Player, DigitalCamera, Camcorder"@en .

:ContrastPlus  a          :VideoFeatures ;
        rdfs:comment      "Ensures that, according to the scene, the screen always displays the best possible contrast. This results in a depth of focus, which lends an extraordinary power to the television image, making it appear almost touchable."@en ;
        rdfs:label        "Contrast Plus"@de , "Contrast Plus"@en ;
        :belongsToModule  "TV"@en .

:DolbyDigital  a          :DataFormatAudio ;
        rdfs:comment      "The marketing name for a series of lossy audio compression technologies developed by Dolby Laboratories.\n\n(This description is partly based on or reuses content from the Wikipedia article \"Dolby Digital\" (http://en.wikipedia.org/wiki/Dolby_Digital) and is licensed under the GNU Free Documentation License (http://www.gnu.org/copyleft/fdl.html).)"@en ;
        rdfs:label        "DolbyDigital"@en , "DolbyDigital"@de ;
        :belongsToModule  "Camcorder"@en .

:PixelPlus3HD  a          :VideoFeatures ;
        rdfs:comment      "Pixel Plus 3 HD offers the unique combination of ultimate sharpness, natural detail, vivid colours and smooth natural motion on all qualities of HD, standard TV signals and multimedia content for high definition displays. Each pixel of the incoming picture is enhanced to better match the surrounding pixels, resulting in a more natural picture. Artefacts and noise in all sources from multimedia to standard TV and also in highly compressed HD are detected and reduced."@en ;
        rdfs:label        "Pixel Plus 3 HD"@de , "Pixel Plus 3 HD"@en ;
        :belongsToModule  "TV"@en .

:USB_Cable  a             :Accessory ;
        rdfs:comment      "A serial bus standard to connect devices to a host computer."@en ;
        rdfs:label        "USB Kabel"@de , "USB cable"@en ;
        :belongsToModule  "Camcorder"@en .

:ZoomOptical  a           :Zoom ;
        rdfs:comment      "An optical zoom is a mechanical assembly of lens elements with the ability to vary its focal length (and thus angle of view), as opposed to a fixed focal length (FFL) lens (see prime lens).\n\n(This description is partly based on or reuses content from the Wikipedia article \"Zoom lens\" (http://en.wikipedia.org/wiki/Zoom_lens) and is licensed under the GNU Free Documentation License (http://www.gnu.org/copyleft/fdl.html).)"@en ;
        rdfs:label        "Zoom optical"@en , "Optischer Zoom"@de ;
        :belongsToModule  "DigitalCamera"@en .

:InfoPrint  a             gr:BusinessEntity ;
        rdfs:comment      "The business entity InfoPrint."@en ;
        rdfs:label        "InfoPrint"^^xsd:string ;
        rdfs:seeAlso      <http://www.infoprintsolutionscompany.com/> ;
        gr:legalName      "InfoPrint Solutions Company"^^xsd:string ;
        :belongsToModule  "Printer"@en .

:Intenso  a               gr:BusinessEntity ;
        rdfs:comment      "The business entity Intenso GmbH."@en ;
        rdfs:label        "Intenso"^^xsd:string ;
        rdfs:seeAlso      <http://www.intenso.de/> ;
        gr:legalName      "Intenso GmbH"^^xsd:string ;
        :belongsToModule  "MP3Player"@en .

:hasStandardInputCapacity
        a                   owl:ObjectProperty ;
        rdfs:comment        "Amount of sheets the product can hold as standard."@en ;
        rdfs:isDefinedBy    <http://www.ebusiness-unibw.org/ontologies/consumerelectronics/v1> ;
        rdfs:label          "standard input capacity"@en , "Standard Eingabekapazität"@de ;
        rdfs:range          gr:QuantitativeValueInteger ;
        rdfs:subPropertyOf  gr:quantitativeProductOrServiceProperty ;
        :belongsToModule    "Printer"@en .

:Ambilight1  a            :VideoFeatures ;
        rdfs:comment      "Ambilight, which is short for Ambient Lighting Technology, is a feature invented by Philips Electronics, generating light effects around the TV that correspond to the video content.\n\n(This description is partly based on or reuses content from the Wikipedia article \"Ambilight\" (http://en.wikipedia.org/wiki/Ambilight) and is licensed under the GNU Free Documentation License (http://www.gnu.org/copyleft/fdl.html).)"@en ;
        rdfs:label        "Ambilight 1"^^xsd:string , "Ambilight 1"@en ;
        :belongsToModule  "TV"@en .

:MPEG   a                 :DataFormatVideo ;
        rdfs:comment      "Includes all kinds of MPEG formats."@en ;
        rdfs:label        "MPEG"@de , "MPEG"@en ;
        :belongsToModule  "MP3Player, DigitalCamera, Camcorder"@en .

:hasStandardOutputCapacityForTransperancies
        a                   owl:ObjectProperty ;
        rdfs:comment        "Defines the maximum amount of transparancies the product is able to print."@en ;
        rdfs:isDefinedBy    <http://www.ebusiness-unibw.org/ontologies/consumerelectronics/v1> ;
        rdfs:label          "standard output capacity for transperancies"@en , "Standard Ausgabekapazität für Folien"@de ;
        rdfs:range          gr:QuantitativeValueInteger ;
        rdfs:subPropertyOf  gr:quantitativeProductOrServiceProperty ;
        :belongsToModule    "Printer"@en .

:PDF    a                 :DataFormatOffice ;
        rdfs:comment      "Portable Document Format (PDF) is a file format created by Adobe Systems in 1993 for document exchange.\n\n(This description is partly based on or reuses content from the Wikipedia article \"Pdf\" (http://en.wikipedia.org/wiki/Pdf) and is licensed under the GNU Free Documentation License (http://www.gnu.org/copyleft/fdl.html).)"@en ;
        rdfs:label        "PDF"@de , "PDF"@en ;
        :belongsToModule  "MP3Player, DigitalCamera"@en .

:InFocus  a               gr:BusinessEntity ;
        rdfs:comment      "The business entity InFocus."@en ;
        rdfs:label        "InFocus"^^xsd:string ;
        rdfs:seeAlso      <http://www.infocus.com/> ;
        gr:legalName      "InFocus Co"^^xsd:string ;
        :belongsToModule  "TV"@en .

:PCMCIA  a                :Connectivity ;
        rdfs:comment      "The Personal Computer Memory Card International Association is an international standards body that defines and promotes the PC Card (formerly known as \"PCMCIA card\") and ExpressCard standards. Although the organization's name refers to memory cards, their standards are not limited to memory devices. These cards can be used for wireless connectivity, modem and other functions in laptop/notebook PCs that may be lacking them natively.\n\n(This description is partly based on or reuses content from the Wikipedia article \"PCMCIA\" (http://en.wikipedia.org/wiki/PCMCIA) and is licensed under the GNU Free Documentation License (http://www.gnu.org/copyleft/fdl.html).)"@en ;
        rdfs:label        "PCMCIA"@de , "PCMCIA"@en ;
        :belongsToModule  "TV"@en .

:DLNA_Ethernet  a         :Connectivity ;
        rdfs:comment      "The Digital Living Network Alliance is an international, cross-industry collaboration of consumer electronics, computing industry and mobile device companies. Members of DLNA develop a concept of wired and wireless interoperable networks where digital content such as photos, music, and videos can be shared through consumer electronics (CE), personal computers (PCs), and mobile devices in and beyond the home.\n\n(This description is partly based on or reuses content from the Wikipedia article \"Digital Living Network Alliance\" (http://en.wikipedia.org/wiki/Digital_Living_Network_Alliance) and is licensed under the GNU Free Documentation License (http://www.gnu.org/copyleft/fdl.html).)"@en ;
        rdfs:label        "DLNA Ethernet"@de , "DLNA Ethernet"@en ;
        :belongsToModule  "TV"@en .

:Monochrome  a            :DisplayType ;
        rdfs:comment      "Ability to display just two colors (black/white)."@en ;
        rdfs:label        "Monochrom"@de , "Monochrome"@en ;
        :belongsToModule  "MP3Player"@en .

:hasHeight  a               owl:ObjectProperty ;
        rdfs:comment        "Defines the measurement of vertical distance (Common unit of measurement centimetre, CMT)."@en ;
        rdfs:isDefinedBy    <http://www.ebusiness-unibw.org/ontologies/consumerelectronics/v1> ;
        rdfs:label          "height"@en , "Höhe"@de ;
        rdfs:range          gr:QuantitativeValueFloat ;
        rdfs:subPropertyOf  gr:quantitativeProductOrServiceProperty ;
        :belongsToModule    "MP3Player, TV, Printer, DigitalCamera, Camcorder"@en .

:IndoorWhiteBalance  a    :WhiteBalance ;
        rdfs:comment      "Ability to adapt of different adjustments of the intensities of the colors."@en ;
        rdfs:label        "Indoor white balance"@en , "Weißabgleich innen"@de ;
        :belongsToModule  "Camcorder"@en .

:Infrared  a              :DataInterfaceType ;
        rdfs:comment      "Infrared (IR) radiation is electromagnetic radiation whose wavelength is longer than that of visible light, but shorter than that of terahertz radiation and microwaves.\n\n(This description is partly based on or reuses content from the Wikipedia article \"Infrared\" (http://en.wikipedia.org/wiki/Infrared) and is licensed under the GNU Free Documentation License (http://www.gnu.org/copyleft/fdl.html).)"@en ;
        rdfs:label        "Infrarot"@de , "Infrared"@en ;
        :belongsToModule  "MP3Player, Printer, DigitalCamera, Camcorder"@en .

:B2     a                 :MediaFormat ;
        rdfs:comment      "Format of the german institute for standardization: 500 x 707 mm."@en ;
        rdfs:label        "B2"@en , "B2"@de ;
        :belongsToModule  "Printer"@en .

:LensSystem  a            owl:Class ;
        rdfs:comment      "A lens is an optical device with perfect or approximate axial symmetry which transmits and refracts light, converging or diverging the beam.\n\n(This description is partly based on or reuses content from the Wikipedia article \"Lens (optics)\" (http://en.wikipedia.org/wiki/Lens_(optics)) and is licensed under the GNU Free Documentation License (http://www.gnu.org/copyleft/fdl.html).)"@en ;
        rdfs:isDefinedBy  <http://www.ebusiness-unibw.org/ontologies/consumerelectronics/v1> ;
        rdfs:label        "Objektivsystem"@de , "Lens system"@en ;
        rdfs:subClassOf   gr:QualitativeValue ;
        :belongsToModule  "Camcorder"@en .

:Smartdisk  a             gr:BusinessEntity ;
        rdfs:comment      "The business entity Verbatim Corporation."@en ;
        rdfs:label        "Smartdisk"^^xsd:string ;
        rdfs:seeAlso      <http://www.smartdisk.com/> ;
        gr:legalName      "Verbatim Corporation "^^xsd:string ;
        :belongsToModule  "MP3Player"@en .

:IEEE_1394  a             :DataInterfaceType ;
        rdfs:comment      "The IEEE 1394 interface is a serial bus interface standard for high-speed communications and isochronous real-time data transfer, frequently used by personal computers, as well as in digital audio, digital video, automotive, and aeronautics applications.  \n\n(This description is partly based on or reuses content from the Wikipedia article \"firewire\" (http://en.wikipedia.org/wiki/FireWire) and is licensed under the GNU Free Documentation License (http://www.gnu.org/copyleft/fdl.html).)"@en ;
        rdfs:label        "IEEE_1394"@en , "IEEE_1394"@de ;
        :belongsToModule  "Printer, Printer, DigitalCamera, Camcorder"@en .

:Transparency  a          :MediaType ;
        rdfs:comment      "A thin sheet of transparent flexible material, typically cellulose acetate, onto which you can print."@en ;
        rdfs:label        "Transparency"@en , "Folie"@de ;
        :belongsToModule  "Printer"@en .

:hasUSBPortsQuantity  a     owl:ObjectProperty ;
        rdfs:comment        "Number of serial bus standard ports to connect devices to a host computer."@en ;
        rdfs:isDefinedBy    <http://www.ebusiness-unibw.org/ontologies/consumerelectronics/v1> ;
        rdfs:label          "number of USB ports"@en , "Anzahl USB Anschlussmöglichkeiten"@de ;
        rdfs:range          gr:QuantitativeValueInteger ;
        rdfs:subPropertyOf  gr:quantitativeProductOrServiceProperty ;
        :belongsToModule    "Camcorder"@en .

:HDMI_Interface  a        :DataInterfaceType ;
        rdfs:comment      "HDMI (High-Definition Multimedia Interface) is a compact audio/video interface for transmitting uncompressed digital data.\n\n(This description is partly based on or reuses content from the Wikipedia article \"HDMI\" (http://en.wikipedia.org/wiki/HDMI) and is licensed under the GNU Free Documentation License (http://www.gnu.org/copyleft/fdl.html).)"@en ;
        rdfs:label        "HDMI interface"@en , "HDMI Schnittstelle"@de ;
        :belongsToModule  "DigitalCamera, Camcorder"@en .

:hasSceneMode  a            owl:ObjectProperty ;
        rdfs:comment        "Defines a projection of information from any physical environment into any sensory system."@en ;
        rdfs:isDefinedBy    <http://www.ebusiness-unibw.org/ontologies/consumerelectronics/v1> ;
        rdfs:label          "scene mode"@en , "Szenenmodus"@de ;
        rdfs:range          :SceneMode ;
        rdfs:subPropertyOf  gr:qualitativeProductOrServiceProperty ;
        :belongsToModule    "Camcorder"@en .

:Energy_Sistem  a         gr:BusinessEntity ;
        rdfs:comment      "The business entity Energy Sistem Soyntec S.A."@en ;
        rdfs:label        "Energy Sistem"^^xsd:string ;
        rdfs:seeAlso      <http://www.energysistem.com/> ;
        gr:legalName      "Energy Sistem Soyntec S.A."^^xsd:string ;
        :belongsToModule  "MP3Player"@en .

:Analog  a                :TunerType ;
        rdfs:comment      "An analog or analogue signal is any continuous signal for which the time varying feature (variable) of the signal is a representation of some other time varying quantity, i.e analogous to another time varying signal.\n\n(This description is partly based on or reuses content from the Wikipedia article \"Analog signal\" (http://en.wikipedia.org/wiki/Analog_signal) and is licensed under the GNU Free Documentation License (http://www.gnu.org/copyleft/fdl.html).)"@en ;
        rdfs:label        "Digital"@de , "Analog"@en ;
        :belongsToModule  "TV"@en .

:DVI    a                 :Connectivity ;
        rdfs:comment      "The Digital Visual Interface (DVI) is a video interface standard designed to maximize the visual quality of digital display devices such as flat panel LCD computer displays and digital projectors. It is designed for carrying uncompressed digital video data to a display. It is partially compatible with the High-Definition Multimedia Interface (HDMI) standard in digital mode (DVI-D), and VGA in analog mode (DVI-A).\n\n(This description is partly based on or reuses content from the Wikipedia article \"Digital Visual Interface\" (http://en.wikipedia.org/wiki/Digital_Visual_Interface) and is licensed under the GNU Free Documentation License (http://www.gnu.org/copyleft/fdl.html).)"@en ;
        rdfs:label        "DVI"@de , "DVI"@en ;
        :belongsToModule  "TV"@en .

:GIF    a                 :DataFormatImage ;
        rdfs:comment      "The format supports up to 8 bits per pixel, allowing a single image to reference a palette of up to 256 distinct colors chosen from the 24-bit RGB color space.\n\n(This description is partly based on or reuses content from the Wikipedia article \"Graphics Interchange Format\" (http://en.wikipedia.org/wiki/Graphics_Interchange_Format) and is licensed under the GNU Free Documentation License (http://www.gnu.org/copyleft/fdl.html).)"@en ;
        rdfs:label        "GIF"@de , "GIF"@en ;
        :belongsToModule  "MP3Player, DigitalCamera, Camcorder"@en .

:hasDisplayBrightness
        a                   owl:DatatypeProperty ;
        rdfs:comment        "Defines the brightness of a display or screen. Brightness is an attribute of visual perception in which a source appears to be radiating or reflecting light.\n\n(This description is partly based on or reuses content from the Wikipedia article \"Brightness\" (http://en.wikipedia.org/wiki/Brightness) and is licensed under the GNU Free Documentation License (http://www.gnu.org/copyleft/fdl.html).)"@en ;
        rdfs:isDefinedBy    <http://www.ebusiness-unibw.org/ontologies/consumerelectronics/v1> ;
        rdfs:label          "display brightness"@en , "Bildhelligkeit"@de ;
        rdfs:range          xsd:float ;
        rdfs:subPropertyOf  gr:datatypeProductOrServiceProperty ;
        :belongsToModule    "TV"@en .

:SupportedResolution  a   owl:Class ;
        rdfs:comment      "Resolution supported by an electronical device."@en ;
        rdfs:isDefinedBy  <http://www.ebusiness-unibw.org/ontologies/consumerelectronics/v1> ;
        rdfs:label        "Unterstützte Auflösung"@en , "Supported resolution"@en ;
        rdfs:subClassOf   gr:QualitativeValue ;
        :belongsToModule  "TV"@en .

:Grey   a                 :Color ;
        rdfs:comment      "RGB Value 128,128,128"@en ;
        rdfs:label        "Grau"@de , "Grey"@en ;
        :belongsToModule  "MP3Player, TV, Printer, DigitalCamera, Camcorder"@en .

:hasMaxColorPrintSpeedNormal
        a                   owl:ObjectProperty ;
        rdfs:comment        "Amount of pages per minute the product is able to print in the mode of color-printig normal quality."@en ;
        rdfs:isDefinedBy    <http://www.ebusiness-unibw.org/ontologies/consumerelectronics/v1> ;
        rdfs:label          "max color print speed normal"@en , "maximale Druckgeschwindigkeit Farbe normal"@de ;
        rdfs:range          gr:QuantitativeValueFloat ;
        rdfs:subPropertyOf  gr:quantitativeProductOrServiceProperty ;
        :belongsToModule    "Printer"@en .

:Phoenix  a               gr:BusinessEntity ;
        rdfs:comment      "The business entity Phoenix."@en ;
        rdfs:label        "Phoenix"^^xsd:string ;
        rdfs:seeAlso      <http://www.phoenixcontact.com/> ;
        gr:legalName      "Phoenix Contact GmbH Co. KG"^^xsd:string ;
        :belongsToModule  "Camcorder"@en .

:Intuix  a                gr:BusinessEntity ;
        rdfs:comment      "The business entity Intuix LLC."@en ;
        rdfs:label        "Intuix"^^xsd:string ;
        rdfs:seeAlso      <http://www.intuix.net/> ;
        gr:legalName      "Intuix LLC"^^xsd:string ;
        :belongsToModule  "MP3Player"@en .

:DigitalAudioCoaxialOut
        a                 :Connectivity ;
        rdfs:comment      "Digital audio uses digital signals for sound reproduction. This includes analog-to-digital conversion, digital-to-analog conversion, storage and transmission. From the signal point of view, a connector can be viewed as a short, rigid cable. The connector usually has the same impedance as the related cable and probably has a similar cutoff frequency although its dielectric may be different. Some connectors are gold or rhodium plated, while some connectors use nickel or tin plating. Silver is also used due to its excellent conductivity. Although silver tends to oxidize rather quickly, the silver oxide that is produced is still conductive. This may pose a cosmetic issue but it does not degrade the performance of the connector. Here the output is meant.\n\n(This description is partly based on or reuses content from the Wikipedia article \"Digital audio\" (http://en.wikipedia.org/wiki/Digital_audio) and is licensed under the GNU Free Documentation License (http://www.gnu.org/copyleft/fdl.html).)"@en ;
        rdfs:label        "Digital audio coaxial out"@de , "Digital audio coaxial out"@en ;
        :belongsToModule  "TV"@en .

:CommonInterface  a       :GeneralFeatures ;
        rdfs:comment      "The Common Interface is an extensible digital interconnect found in the digital TV market.\n\n(This description is partly based on or reuses content from the Wikipedia article \"Common Interface\" (http://en.wikipedia.org/wiki/Common_Interface) and is licensed under the GNU Free Documentation License (http://www.gnu.org/copyleft/fdl.html).)"@en ;
        rdfs:label        "Common interface"@de , "Common interface"@en ;
        :belongsToModule  "TV"@en .

:TRUST  a                 gr:BusinessEntity ;
        rdfs:comment      "The business entity TRUST International B.V."@en ;
        rdfs:label        "TRUST"^^xsd:string ;
        rdfs:seeAlso      <http://www.trust.com/> ;
        gr:legalName      "TRUST International B.V."^^xsd:string ;
        :belongsToModule  "MP3Player, DigitalCamera, Camcorder"@en .

:hasViewingAngleVertical
        a                   owl:ObjectProperty ;
        rdfs:comment        "Defines the angle in a vertical axe where a viewer is still able to see the picture on a screen (Common unit of measurement degree, DD)."@en ;
        rdfs:isDefinedBy    <http://www.ebusiness-unibw.org/ontologies/consumerelectronics/v1> ;
        rdfs:label          "viewing angle vertical"@en , "vertikaler Betrachtungswinkel"@de ;
        rdfs:range          gr:QuantitativeValueFloat ;
        rdfs:subPropertyOf  gr:quantitativeProductOrServiceProperty ;
        :belongsToModule    "TV"@en .

:Format5.1ch  a           :DataFormatAudio ;
        rdfs:comment      "Encompasses a range of techniques for enriching (expanding and deepening) the sound reproduction quality, of an audio source, with additional audio channels reproduced via additional, discrete speakers."@en ;
        rdfs:label        "Format 5.1ch"@en , "Format 5.1ch"@de ;
        :belongsToModule  "Camcorder"@en .

:HP_FastRes_1200_DPI  a   :PrintResolution ;
        rdfs:comment      "Special printing technology invented and used by HP."@en ;
        rdfs:label        "HP FastRes 1200 DPI"@en , "HP FastRes 1200 DPI"@de ;
        :belongsToModule  "Printer"@en .

:Toshiba  a               gr:BusinessEntity ;
        rdfs:comment      "The business entity Toshiba Corporation."@en ;
        rdfs:label        "Toshiba"^^xsd:string ;
        rdfs:seeAlso      <http://www.toshiba.com/> ;
        gr:legalName      "Toshiba Corporation"^^xsd:string ;
        :belongsToModule  "MP3Player, TV, DigitalCamera, Camcorder"@en .

:WindowsVista  a          :CompatibleOperatingSystems ;
        rdfs:comment      "A version of a Microsoft operating system."@en ;
        rdfs:label        "Windows Vista"@de , "Windows Vista"@en ;
        :belongsToModule  "MP3Player, Printer, DigitalCamera, Camcorder"@en .

:Maxfield  a              gr:BusinessEntity ;
        rdfs:comment      "The business entity Maxfield GmbH."@en ;
        rdfs:label        "Maxfield"^^xsd:string ;
        rdfs:seeAlso      <http://www.maxfield.de/> ;
        gr:legalName      "Maxfield GmbH"^^xsd:string ;
        :belongsToModule  "MP3Player"@en .

:hasDigitalZoomFactor
        a                   owl:ObjectProperty ;
        rdfs:comment        "Defines the stages an object can be zoomed digitally."@en ;
        rdfs:isDefinedBy    <http://www.ebusiness-unibw.org/ontologies/consumerelectronics/v1> ;
        rdfs:label          "digital zoom factor"@en , "digitaler Zoomfaktor"@de ;
        rdfs:range          gr:QuantitativeValueFloat ;
        rdfs:subPropertyOf  gr:quantitativeProductOrServiceProperty ;
        :belongsToModule    "DigitalCamera, Camcorder"@en .

:CVBS_in  a               :Connectivity ;
        rdfs:comment      "Composite video is often designated by the CVBS acronym, meaning any of \"Color, Video, Blank and Sync\", \"Composite Video Baseband Signal\", \"Composite Video Burst Signal\", or \"Composite Video with Burst and Sync\". Here the input is meant."@en ;
        rdfs:label        "CVBS in"@en , "CVBS in"@de ;
        :belongsToModule  "TV"@en .

:Nanopoint  a             gr:BusinessEntity ;
        rdfs:comment      "The business entity Nanopoint Technology Inc."@en ;
        rdfs:label        "Nanopoint"^^xsd:string ;
        rdfs:seeAlso      <http://www.nanopoint.co.uk/> ;
        gr:legalName      "Nanopoint Technology Inc."^^xsd:string ;
        :belongsToModule  "MP3Player"@en .

:ViewFinderElectronic
        a                 :ViewFinder ;
        rdfs:comment      "An electronic viewfinder or EVF is a viewfinder where the image captured by the lens is projected electronically onto a miniature display. The image on this display is used to assist in aiming the camera at the scene to be photographed.\n\n(This description is partly based on or reuses content from the Wikipedia article \"Electronic viewfinder\" (http://en.wikipedia.org/wiki/Electronic_viewfinder) and is licensed under the GNU Free Documentation License (http://www.gnu.org/copyleft/fdl.html).)"@en ;
        rdfs:label        "Elektronischer Bildsucher"@de , "Viewfinder electronic"@en ;
        :belongsToModule  "DigitalCamera"@en .

:Sweex  a                 gr:BusinessEntity ;
        rdfs:comment      "The business entity Sweex."@en ;
        rdfs:label        "Sweex"^^xsd:string ;
        rdfs:seeAlso      <http://www.sweex.com/> ;
        gr:legalName      "Sweex"^^xsd:string ;
        :belongsToModule  "TV"@en .

:hasMinIllumination  a      owl:ObjectProperty ;
        rdfs:comment        "Minimum deliberate application of light to achieve some aesthetic or practical effect (common unit of measurement: Lux; LUX)."@en ;
        rdfs:isDefinedBy    <http://www.ebusiness-unibw.org/ontologies/consumerelectronics/v1> ;
        rdfs:label          "min illumination"@en , "minimale Belichtung"@de ;
        rdfs:range          gr:QuantitativeValueFloat ;
        rdfs:subPropertyOf  gr:quantitativeProductOrServiceProperty ;
        :belongsToModule    "Camcorder"@en .

:HP_REt  a                :PrintResolution ;
        rdfs:comment      "Special printing technology invented and used by HP."@en ;
        rdfs:label        "HP REt"@en , "HP REt"@de ;
        :belongsToModule  "Printer"@en .

:hasShutterLag  a           owl:ObjectProperty ;
        rdfs:comment        "Defines the delay between triggering the shutter and when the photograph is actually recorded (Common unit of measurement seconds, SEC)."@en ;
        rdfs:isDefinedBy    <http://www.ebusiness-unibw.org/ontologies/consumerelectronics/v1> ;
        rdfs:label          "shutter lag"@en , "Auslöseverzögerung"@de ;
        rdfs:range          gr:QuantitativeValueFloat ;
        rdfs:subPropertyOf  gr:quantitativeProductOrServiceProperty ;
        :belongsToModule    "DigitalCamera, Camcorder"@en .

:TextViewing  a           :Features ;
        rdfs:comment      "Ability to display text."@en ;
        rdfs:label        "Text viewing"@en , "Textdarstellung"@de ;
        :belongsToModule  "MP3Player"@en .

:SmartMediaCard  a        :StorageMedia ;
        rdfs:comment      "SmartMedia is a flash memory card standard."@en ;
        rdfs:label        "SmartMediaCard"@en , "SmartMediaCard"@de ;
        :belongsToModule  "MP3Player, DigitalCamera, Camcorder"@en .

:Denver  a                gr:BusinessEntity ;
        rdfs:comment      "The business entity Denver."@en ;
        rdfs:label        "Denver"^^xsd:string ;
        rdfs:seeAlso      <http://www.denver-electronics.com/> ;
        gr:legalName      "Denver Electronics"^^xsd:string ;
        :belongsToModule  "TV"@en .

:Philips  a               gr:BusinessEntity ;
        rdfs:comment      "The business entity Koninklijke Philips Electronics N.V."@en ;
        rdfs:label        "Philips"^^xsd:string ;
        rdfs:seeAlso      <http://www.philips.com/> ;
        gr:legalName      "Koninklijke Philips Electronics N.V."^^xsd:string ;
        :belongsToModule  "MP3Player, TV, DigitalCamera"@en .

:OneStepFixed  a          :LensSystem ;
        rdfs:comment      "A special lens system."@en ;
        rdfs:label        "One step fixed"@en , "One step fixed"@de ;
        :belongsToModule  "Camcorder"@en .

:hasDepth  a                owl:ObjectProperty ;
        rdfs:comment        "Defines the distance from side to side, measuring across the object at right angles to the width (Common unit of measurement centimetre, CMT).\n\n(This description is partly based on or reuses content from the Wikipedia article \"Length\" (http://en.wikipedia.org/wiki/Length) and is licensed under the GNU Free Documentation License (http://www.gnu.org/copyleft/fdl.html).)"@en ;
        rdfs:isDefinedBy    <http://www.ebusiness-unibw.org/ontologies/consumerelectronics/v1> ;
        rdfs:label          "depth"@en , "Tiefe"@de ;
        rdfs:range          gr:QuantitativeValueFloat ;
        rdfs:subPropertyOf  gr:quantitativeProductOrServiceProperty ;
        :belongsToModule    "MP3Player, TV, Printer, DigitalCamera, Camcorder"@en .

:hasAudioInputSource  a     owl:DatatypeProperty ;
        rdfs:comment        "Defines which audio input devices can be used with this object."@en ;
        rdfs:isDefinedBy    <http://www.ebusiness-unibw.org/ontologies/consumerelectronics/v1> ;
        rdfs:label          "audio input source"@en , "Audioeingang"@de ;
        rdfs:range          xsd:boolean ;
        rdfs:subPropertyOf  gr:datatypeProductOrServiceProperty ;
        :belongsToModule    "DigitalCamera"@en .

:InkjetPrinter  a         owl:Class ;
        rdfs:comment      "Inkjet printers operate by propelling variably-sized droplets of liquid or molten material (ink) onto almost any sized page.\n\n(This description is partly based on or reuses content from the Wikipedia article \"Inkjet printer\" (http://en.wikipedia.org/wiki/Inkjet_printer) and is licensed under the GNU Free Documentation License (http://www.gnu.org/copyleft/fdl.html).)"@en ;
        rdfs:isDefinedBy  <http://www.ebusiness-unibw.org/ontologies/consumerelectronics/v1> ;
        rdfs:label        "Inkjet printer"@en , "Tintenstrahldrucker"@de ;
        rdfs:subClassOf   :Printer ;
        :belongsToModule  "Printer"@en .

:DK_digital  a            gr:BusinessEntity ;
        rdfs:comment      "The business entity DK digital GmbH."@en ;
        rdfs:label        "DK digital"^^xsd:string ;
        rdfs:seeAlso      <http://www.dk-digital.com/> ;
        gr:legalName      "DK digital GmbH"^^xsd:string ;
        :belongsToModule  "MP3Player"@en .

:Camcorder  a             owl:Class ;
        rdfs:comment      "A camcorder is a portable consumer electronics device for recording video and audio using a built-in recorder unit."@en ;
        rdfs:isDefinedBy  <http://www.ebusiness-unibw.org/ontologies/consumerelectronics/v1> ;
        rdfs:label        "Camcorder"@de , "Camcorder"@en ;
        rdfs:subClassOf   gr:ProductOrService ;
        :belongsToModule  "Camcorder"@en .

:hasCompatibleOperatingSystem
        a                   owl:ObjectProperty ;
        rdfs:comment        "Defines the possible external operating systems to communicate with."@en ;
        rdfs:isDefinedBy    <http://www.ebusiness-unibw.org/ontologies/consumerelectronics/v1> ;
        rdfs:label          "compatible operating system"@en , "kompatibles Betriebssystem"@de ;
        rdfs:range          :CompatibleOperatingSystems ;
        rdfs:subPropertyOf  gr:qualitativeProductOrServiceProperty ;
        :belongsToModule    "MP3Player, Printer, DigitalCamera, Camcorder"@en .

:Sharkoon  a              gr:BusinessEntity ;
        rdfs:comment      "The business entity SHARKOON Technologies GmbH."@en ;
        rdfs:label        "Sharkoon"^^xsd:string ;
        rdfs:seeAlso      <http://www.sharkoon.com/> ;
        gr:legalName      "SHARKOON Technologies GmbH "^^xsd:string ;
        :belongsToModule  "MP3Player"@en .

:SelfTimer  a             :Features ;
        rdfs:comment      "Ability to give a delay between the pressing of the shutter release and the shutter firing."@en ;
        rdfs:label        "Self-timer"@en , "Selbstauslöser"@de ;
        :belongsToModule  "DigitalCamera, Camcorder"@en .

:A6     a                 :MediaFormat ;
        rdfs:comment      "Format of the german institute for standardization: 105 x 148 mm."@en ;
        rdfs:label        "A6"@en , "A6"@de ;
        :belongsToModule  "Printer"@en .

:hasCertificate  a          owl:ObjectProperty ;
        rdfs:comment        "Defines the type of certificate of a product used to attest quality standards."@en ;
        rdfs:isDefinedBy    <http://www.ebusiness-unibw.org/ontologies/consumerelectronics/v1> ;
        rdfs:label          "certificate"@en , "Zertifikat"@de ;
        rdfs:range          :Certificate ;
        rdfs:subPropertyOf  gr:qualitativeProductOrServiceProperty ;
        :belongsToModule    "TV"@en .

:Tektronix  a             gr:BusinessEntity ;
        rdfs:comment      "The business entity Tektronix."@en ;
        rdfs:label        "Tektronix"^^xsd:string ;
        rdfs:seeAlso      <http://www.tek.com/> ;
        gr:legalName      "Tektronix, Inc."^^xsd:string ;
        :belongsToModule  "Printer"@en .
