@prefix dc: <http://purl.org/dc/elements/1.1/> .
@prefix rdfs: <http://www.w3.org/2000/01/rdf-schema#> .
@prefix ome: <http://contextus.net/ontology/ontomedia/core/expression#> .
@prefix omt: <http://contextus.net/ontology/ontomedia/ext/common/trait#> .
@prefix dct: <http://purl.org/dc/terms/> .
@prefix omb: <http://contextus.net/ontology/ontomedia/ext/common/being#> .
@prefix owl: <http://www.w3.org/2002/07/owl#> .
@prefix xsd: <http://www.w3.org/2001/XMLSchema#> .
@prefix rdf: <http://www.w3.org/1999/02/22-rdf-syntax-ns#> .
@prefix omk: <http://contextus.net/ontology/ontomedia/ext/detail/know#> .

<http://contextus.net/ontology/ontomedia/misc/date#> a owl:Ontology ;
	rdfs:label "OntoMedia Date Part Representation" ;
	dc:title "OntoMedia Date-Component Part Representation"@en ;
	dc:description "OntoMedia (Ontology for Media) Date Component has been designed to describe the different ways of marking time in media."@en ;
	dc:creator "Michael O. Jewell (mailto:moj@ecs.soton.ac.uk)" , "K Faith Lawrence (mailto:kf03r@ecs.soton.ac.uk)" , "Mischa M Tuffield (mailto:mmt04r@ecs.soton.ac.uk)" ;
	dct:created "2005-05-11" ;
	owl:versionInfo "0.21" .

<http://contextus.net/ontology/ontomedia/misc/date#Calendar> a owl:Class ;
	rdfs:subClassOf omk:Culture ;
	rdfs:comment "This class represents a system of representing time" ;
	rdfs:label "Calendar" .

<http://contextus.net/ontology/ontomedia/misc/date#Date> a owl:Class ;
	rdfs:subClassOf omt:Value ;
	rdfs:comment "This class represents a value representing time" ;
	rdfs:label "Date" .

<http://contextus.net/ontology/ontomedia/misc/date#CalendarReferencePoint> a owl:Class ;
	rdfs:subClassOf <http://contextus.net/ontology/ontomedia/misc/date#Date> ;
	rdfs:comment "This class represents a reference point which a calendar measures other dates relative to" ;
	rdfs:label "Calendar Reference Point" .

<http://contextus.net/ontology/ontomedia/misc/date#Date-Component> a owl:Class ;
	rdfs:subClassOf omt:AbstractComponent ;
	rdfs:comment "This class represents the parts of a date" ;
	rdfs:label "Date Component" .

<http://contextus.net/ontology/ontomedia/misc/date#Date-Ordering> a owl:Class ;
	rdfs:subClassOf omt:Ordering ;
	rdfs:comment "This class represents the order in which components describing a date should be displayed" ;
	rdfs:label "Date Ordering" .

<http://contextus.net/ontology/ontomedia/misc/date#Second> a owl:Class ;
	rdfs:subClassOf <http://contextus.net/ontology/ontomedia/misc/date#Date-Component> ;
	rdfs:comment "This class represents the part of a date which is the second designaition" ;
	rdfs:label "Second" .

<http://contextus.net/ontology/ontomedia/misc/date#Minute> a owl:Class ;
	rdfs:subClassOf <http://contextus.net/ontology/ontomedia/misc/date#Date-Component> ;
	rdfs:comment "This class represents the part of a date which is the minute designaition" ;
	rdfs:label "Minute" .

<http://contextus.net/ontology/ontomedia/misc/date#Hour> a owl:Class ;
	rdfs:subClassOf <http://contextus.net/ontology/ontomedia/misc/date#Date-Component> ;
	rdfs:comment "This class represents the part of a date which is the hour designaition" ;
	rdfs:label "Hour" .

<http://contextus.net/ontology/ontomedia/misc/date#Day> a owl:Class ;
	rdfs:subClassOf <http://contextus.net/ontology/ontomedia/misc/date#Date-Component> ;
	rdfs:comment "This class represents the part of a date which is the day designaition" ;
	rdfs:label "Day" .

<http://contextus.net/ontology/ontomedia/misc/date#Month> a owl:Class ;
	rdfs:subClassOf <http://contextus.net/ontology/ontomedia/misc/date#Date-Component> ;
	rdfs:comment "This class represents the part of a date which is the month designaition" ;
	rdfs:label "Month" .

<http://contextus.net/ontology/ontomedia/misc/date#Year> a owl:Class ;
	rdfs:subClassOf <http://contextus.net/ontology/ontomedia/misc/date#Date-Component> ;
	rdfs:comment "This class represents the part of a date which is the year designaition" ;
	rdfs:label "Year" .

<http://contextus.net/ontology/ontomedia/misc/date#Qualifier> a owl:Class ;
	rdfs:subClassOf <http://contextus.net/ontology/ontomedia/misc/date#Date-Component> ;
	rdfs:comment "This class represents the textual qualifier that may be part of the data i.e. AD, BCE etc" ;
	rdfs:label "Qualifier" .

<http://contextus.net/ontology/ontomedia/misc/date#Standard> a owl:Class ;
	rdfs:subClassOf <http://contextus.net/ontology/ontomedia/misc/date#Date-Ordering> ;
	rdfs:comment "This class represents the International Standard form of the date" ;
	rdfs:label "International Standard" .

<http://contextus.net/ontology/ontomedia/misc/date#has-date-component> a owl:ObjectProperty ;
	rdfs:label "Has Date Component" ;
	rdfs:comment "This property specifies the name represented by the component" ;
	rdfs:domain <http://contextus.net/ontology/ontomedia/misc/date#Date> ;
	rdfs:range <http://contextus.net/ontology/ontomedia/misc/date#Date-Component> .

<http://contextus.net/ontology/ontomedia/misc/date#abstracted-from-occurrence> a owl:ObjectProperty ;
	rdfs:label "Abstracted From Occurrence" ;
	rdfs:comment "The occurrance of an event from which the reference point was abstracted" ;
	rdfs:domain <http://contextus.net/ontology/ontomedia/misc/date#Date> ;
	rdfs:range ome:Occurrence .

<http://contextus.net/ontology/ontomedia/misc/date#before-reference-point> a owl:ObjectProperty ;
	rdfs:label "Before Reference Point" ;
	rdfs:comment "The relative reference point before which the desired point of time occurs" ;
	rdfs:domain <http://contextus.net/ontology/ontomedia/misc/date#Date> ;
	rdfs:range <http://contextus.net/ontology/ontomedia/misc/date#CalendarReferencePoint> .

<http://contextus.net/ontology/ontomedia/misc/date#after-reference-point> a owl:ObjectProperty ;
	rdfs:label "After Reference Point" ;
	rdfs:comment "The relative reference point after which the desired point of time occurs" ;
	rdfs:domain <http://contextus.net/ontology/ontomedia/misc/date#Date> ;
	rdfs:range <http://contextus.net/ontology/ontomedia/misc/date#CalendarReferencePoint> .

<http://contextus.net/ontology/ontomedia/misc/date#uses-calendar> a owl:ObjectProperty ;
	rdfs:label "Uses Calendar" ;
	rdfs:comment "The calandar which the date uses" ;
	rdfs:domain <http://contextus.net/ontology/ontomedia/misc/date#Date> ;
	rdfs:range <http://contextus.net/ontology/ontomedia/misc/date#Calendar> .

<http://contextus.net/ontology/ontomedia/misc/date#has-reference-point> a owl:ObjectProperty ;
	rdfs:label "Has Reference Point" ;
	rdfs:comment "This property specifies a point of reference in a Calendar" ;
	rdfs:domain <http://contextus.net/ontology/ontomedia/misc/date#Calendar> ;
	rdfs:range <http://contextus.net/ontology/ontomedia/misc/date#CalendarReferencePoint> .

<http://contextus.net/ontology/ontomedia/misc/date#reference-point-minus-one> a owl:ObjectProperty ;
	rdfs:label "Reference Point Minus One" ;
	rdfs:comment "The Year Preceeding the Reference Point Year" ;
	rdfs:domain <http://contextus.net/ontology/ontomedia/misc/date#CalendarReferencePoint> ;
	rdfs:range <http://contextus.net/ontology/ontomedia/misc/date#Year> .

<http://contextus.net/ontology/ontomedia/misc/date#reference-point-plus-one> a owl:ObjectProperty ;
	rdfs:label "Reference Point Plus One" ;
	rdfs:comment "The Year Following the Reference Point Year" ;
	rdfs:domain <http://contextus.net/ontology/ontomedia/misc/date#CalendarReferencePoint> ;
	rdfs:range <http://contextus.net/ontology/ontomedia/misc/date#Year> .
