@prefix dc:    <http://purl.org/dc/elements/1.1/> .
@prefix rdfs:  <http://www.w3.org/2000/01/rdf-schema#> .
@prefix geo:   <http://www.opengis.net/ont/geosparql#> .
@prefix owl:   <http://www.w3.org/2002/07/owl#> .
@prefix xsd:   <http://www.w3.org/2001/XMLSchema#> .
@prefix rdf:   <http://www.w3.org/1999/02/22-rdf-syntax-ns#> .
@prefix skos:  <http://www.w3.org/2004/02/skos/core#> .

geo:ehEquals  a           owl:ObjectProperty ;
        rdfs:comment      "\n      Exists if the subject SpatialObject spatially equals the \n      object SpatialObject. DE-9IM: TFFFTFFFT\n    "@en ;
        rdfs:domain       geo:SpatialObject ;
        rdfs:isDefinedBy  <http://www.opengis.net/ont/geosparql> , <http://www.opengis.net/spec/geosparql/1.0> ;
        rdfs:label        "equals"@en ;
        rdfs:range        geo:SpatialObject ;
        dc:contributor    "Matthew Perry" ;
        dc:creator        "OGC GeoSPARQL 1.0 Standard Working Group" ;
        dc:date           "2011-06-16"^^xsd:date ;
        dc:description    "\n      Exists if the subject SpatialObject spatially equals the \n      object SpatialObject. DE-9IM: TFFFTFFFT\n    "@en ;
        skos:definition   "\n      Exists if the subject SpatialObject spatially equals the \n      object SpatialObject. DE-9IM: TFFFTFFFT\n    "@en ;
        skos:prefLabel    "equals"@en .

geo:rcc8tppi  a           owl:ObjectProperty ;
        rdfs:comment      "\n      Exists if the subject SpatialObject spatially covers the \n      object SpatialObject. DE-9IM: TTTFTTFFT\n    "@en ;
        rdfs:domain       geo:SpatialObject ;
        rdfs:isDefinedBy  <http://www.opengis.net/spec/geosparql/1.0> , <http://www.opengis.net/ont/geosparql> ;
        rdfs:label        "tangential proper part inverse"@en ;
        rdfs:range        geo:SpatialObject ;
        dc:contributor    "Matthew Perry" ;
        dc:creator        "OGC GeoSPARQL 1.0 Standard Working Group" ;
        dc:date           "2011-06-16"^^xsd:date ;
        dc:description    "\n      Exists if the subject SpatialObject spatially covers the \n      object SpatialObject. DE-9IM: TTTFTTFFT\n    "@en ;
        skos:definition   "\n      Exists if the subject SpatialObject spatially covers the \n      object SpatialObject. DE-9IM: TTTFTTFFT\n    "@en ;
        skos:prefLabel    "tangential proper part inverse"@en .

geo:sfWithin  a           owl:ObjectProperty ;
        rdfs:comment      "\n      Exists if the subject SpatialObject is spatially within the \n      object SpatialObject. DE-9IM: T*F**F***\n    "@en ;
        rdfs:domain       geo:SpatialObject ;
        rdfs:isDefinedBy  <http://www.opengis.net/ont/geosparql> , <http://www.opengis.net/spec/geosparql/1.0> ;
        rdfs:label        "within"@en ;
        rdfs:range        geo:SpatialObject ;
        dc:contributor    "Matthew Perry" ;
        dc:creator        "OGC GeoSPARQL 1.0 Standard Working Group" ;
        dc:date           "2011-06-16"^^xsd:date ;
        dc:description    "\n      Exists if the subject SpatialObject is spatially within the \n      object SpatialObject. DE-9IM: T*F**F***\n    "@en ;
        skos:definition   "\n      Exists if the subject SpatialObject is spatially within the \n      object SpatialObject. DE-9IM: T*F**F***\n    "@en ;
        skos:prefLabel    "within"@en .

geo:gmlLiteral  a         rdfs:Datatype ;
        rdfs:comment      "\n      A GML serialization of a geometry object.\n    "@en ;
        rdfs:isDefinedBy  <http://www.opengis.net/spec/geosparql/1.0> , <http://www.opengis.net/ont/geosparql> ;
        rdfs:label        "GML Literal"@en ;
        dc:contributor    "Matthew Perry" ;
        dc:creator        "OGC GeoSPARQL 1.0 Standard Working Group" ;
        dc:date           "2011-06-16"^^xsd:date ;
        dc:description    "\n      A GML serialization of a geometry object.\n    "@en ;
        skos:definition   "\n      A GML serialization of a geometry object.\n    "@en ;
        skos:prefLabel    "GML Literal"@en .

geo:ehDisjoint  a         owl:ObjectProperty ;
        rdfs:comment      "\n      Exists if the subject SpatialObject is spatially disjoint\n      from the object SpatialObject. DE-9IM: FF*FF****\n    "@en ;
        rdfs:domain       geo:SpatialObject ;
        rdfs:isDefinedBy  <http://www.opengis.net/ont/geosparql> , <http://www.opengis.net/spec/geosparql/1.0> ;
        rdfs:label        "disjoint"@en ;
        rdfs:range        geo:SpatialObject ;
        dc:contributor    "Matthew Perry" ;
        dc:creator        "OGC GeoSPARQL 1.0 Standard Working Group" ;
        dc:date           "2011-06-16"^^xsd:date ;
        dc:description    "\n      Exists if the subject SpatialObject is spatially disjoint\n      from the object SpatialObject. DE-9IM: FF*FF****\n    "@en ;
        skos:definition   "\n      Exists if the subject SpatialObject is spatially disjoint\n      from the object SpatialObject. DE-9IM: FF*FF****\n    "@en ;
        skos:prefLabel    "disjoint"@en .

geo:sfIntersects  a       owl:ObjectProperty ;
        rdfs:comment      "\n      Exists if the subject SpatialObject is not spatially disjoint \n      from the object SpatialObject.\n      DE-9IM: T******** ^ *T******* ^ ***T***** ^ ****T**** \n    "@en ;
        rdfs:domain       geo:SpatialObject ;
        rdfs:isDefinedBy  <http://www.opengis.net/ont/geosparql> , <http://www.opengis.net/spec/geosparql/1.0> ;
        rdfs:label        "intersects"@en ;
        rdfs:range        geo:SpatialObject ;
        dc:contributor    "Matthew Perry" ;
        dc:creator        "OGC GeoSPARQL 1.0 Standard Working Group" ;
        dc:date           "2011-06-16"^^xsd:date ;
        dc:description    "\n      Exists if the subject SpatialObject is not spatially disjoint \n      from the object SpatialObject.\n      DE-9IM: T******** ^ *T******* ^ ***T***** ^ ****T**** \n    "@en ;
        skos:definition   "\n      Exists if the subject SpatialObject is not spatially disjoint \n      from the object SpatialObject.\n      DE-9IM: T******** ^ *T******* ^ ***T***** ^ ****T**** \n    "@en ;
        skos:prefLabel    "intersects"@en .

geo:rcc8ntpp  a           owl:ObjectProperty ;
        rdfs:comment      "\n      Exists if the subject SpatialObject is spatially inside \n      the object SpatialObject. DE-9IM: TFFTFFTTT\n    "@en ;
        rdfs:domain       geo:SpatialObject ;
        rdfs:isDefinedBy  <http://www.opengis.net/spec/geosparql/1.0> , <http://www.opengis.net/ont/geosparql> ;
        rdfs:label        "non-tangential proper part"@en ;
        rdfs:range        geo:SpatialObject ;
        dc:contributor    "Matthew Perry" ;
        dc:creator        "OGC GeoSPARQL 1.0 Standard Working Group" ;
        dc:date           "2011-06-16"^^xsd:date ;
        dc:description    "\n      Exists if the subject SpatialObject is spatially inside \n      the object SpatialObject. DE-9IM: TFFTFFTTT\n    "@en ;
        skos:definition   "\n      Exists if the subject SpatialObject is spatially inside \n      the object SpatialObject. DE-9IM: TFFTFFTTT\n    "@en ;
        skos:prefLabel    "non-tangential proper part"@en .

geo:sfTouches  a          owl:ObjectProperty ;
        rdfs:comment      "\n      Exists if the subject SpatialObject spatially touches the \n      object SpatialObject.\n      DE-9IM: FT******* ^ F**T***** ^ F***T****\n    "@en ;
        rdfs:domain       geo:SpatialObject ;
        rdfs:isDefinedBy  <http://www.opengis.net/spec/geosparql/1.0> , <http://www.opengis.net/ont/geosparql> ;
        rdfs:label        "touches"@en ;
        rdfs:range        geo:SpatialObject ;
        dc:contributor    "Matthew Perry" ;
        dc:creator        "OGC GeoSPARQL 1.0 Standard Working Group" ;
        dc:date           "2011-06-16"^^xsd:date ;
        dc:description    "\n      Exists if the subject SpatialObject spatially touches the \n      object SpatialObject.\n      DE-9IM: FT******* ^ F**T***** ^ F***T****\n    "@en ;
        skos:definition   "\n      Exists if the subject SpatialObject spatially touches the \n      object SpatialObject.\n      DE-9IM: FT******* ^ F**T***** ^ F***T****\n    "@en ;
        skos:prefLabel    "touches"@en .

geo:ehInside  a           owl:ObjectProperty ;
        rdfs:comment      "\n      Exists if the subject SpatialObject is spatially inside \n      the object SpatialObject. DE-9IM: TFF*FFT**\n    "@en ;
        rdfs:domain       geo:SpatialObject ;
        rdfs:isDefinedBy  <http://www.opengis.net/ont/geosparql> , <http://www.opengis.net/spec/geosparql/1.0> ;
        rdfs:label        "inside"@en ;
        rdfs:range        geo:SpatialObject ;
        dc:contributor    "Matthew Perry" ;
        dc:creator        "OGC GeoSPARQL 1.0 Standard Working Group" ;
        dc:date           "2011-06-16"^^xsd:date ;
        dc:description    "\n      Exists if the subject SpatialObject is spatially inside \n      the object SpatialObject. DE-9IM: TFF*FFT**\n    "@en ;
        skos:definition   "\n      Exists if the subject SpatialObject is spatially inside \n      the object SpatialObject. DE-9IM: TFF*FFT**\n    "@en ;
        skos:prefLabel    "inside"@en .

geo:Feature  a            owl:Class ;
        rdfs:comment      "\n      This class represents the top-level feature type. This class is \n      equivalent to GFI_Feature defined in ISO 19156:2011, and it is \n      superclass of all feature types.\n    "@en ;
        rdfs:isDefinedBy  <http://www.opengis.net/ont/geosparql> , <http://www.opengis.net/spec/geosparql/1.0> ;
        rdfs:label        "Feature"@en ;
        rdfs:subClassOf   geo:SpatialObject ;
        dc:contributor    "Matthew Perry" ;
        dc:creator        "OGC GeoSPARQL 1.0 Standard Working Group" ;
        dc:date           "2011-06-16"^^xsd:date ;
        dc:description    "\n      This class represents the top-level feature type. This class is \n      equivalent to GFI_Feature defined in ISO 19156:2011, and it is \n      superclass of all feature types.\n    "@en ;
        owl:disjointWith  geo:Geometry ;
        skos:definition   "\n      This class represents the top-level feature type. This class is \n      equivalent to GFI_Feature defined in ISO 19156:2011, and it is \n      superclass of all feature types.\n    "@en ;
        skos:prefLabel    "Feature"@en .

geo:ehContains  a         owl:ObjectProperty ;
        rdfs:comment      "\n      Exists if the subject SpatialObject spatially contains the \n      object SpatialObject. DE-9IM: T*TFF*FF*\n    "@en ;
        rdfs:domain       geo:SpatialObject ;
        rdfs:isDefinedBy  <http://www.opengis.net/spec/geosparql/1.0> , <http://www.opengis.net/ont/geosparql> ;
        rdfs:label        "contains"@en ;
        rdfs:range        geo:SpatialObject ;
        dc:contributor    "Matthew Perry" ;
        dc:creator        "OGC GeoSPARQL 1.0 Standard Working Group" ;
        dc:date           "2011-06-16"^^xsd:date ;
        dc:description    "\n      Exists if the subject SpatialObject spatially contains the \n      object SpatialObject. DE-9IM: T*TFF*FF*\n    "@en ;
        skos:definition   "\n      Exists if the subject SpatialObject spatially contains the \n      object SpatialObject. DE-9IM: T*TFF*FF*\n    "@en ;
        skos:prefLabel    "contains"@en .

geo:isEmpty  a            owl:DatatypeProperty ;
        rdfs:comment      "\n      (true) if this geometric object is the empty Geometry. If \n      true, then this geometric object represents the empty point \n      set for the coordinate space.\n    "@en ;
        rdfs:domain       geo:Geometry ;
        rdfs:isDefinedBy  <http://www.opengis.net/spec/geosparql/1.0> , <http://www.opengis.net/ont/geosparql> ;
        rdfs:label        "isEmpty"@en ;
        rdfs:range        xsd:boolean ;
        dc:contributor    "Matthew Perry" ;
        dc:creator        "OGC GeoSPARQL 1.0 Standard Working Group" ;
        dc:date           "2011-06-16"^^xsd:date ;
        dc:description    "\n      (true) if this geometric object is the empty Geometry. If \n      true, then this geometric object represents the empty point \n      set for the coordinate space.\n    "@en ;
        skos:definition   "\n      (true) if this geometric object is the empty Geometry. If \n      true, then this geometric object represents the empty point \n      set for the coordinate space.\n    "@en ;
        skos:prefLabel    "isEmpty"@en .

geo:sfDisjoint  a         owl:ObjectProperty ;
        rdfs:comment      "\n      Exists if the subject SpatialObject is spatially disjoint \n      from the object SpatialObject. DE-9IM: FF*FF****\n    "@en ;
        rdfs:domain       geo:SpatialObject ;
        rdfs:isDefinedBy  <http://www.opengis.net/ont/geosparql> , <http://www.opengis.net/spec/geosparql/1.0> ;
        rdfs:label        "disjoint"@en ;
        rdfs:range        geo:SpatialObject ;
        dc:contributor    "Matthew Perry" ;
        dc:creator        "OGC GeoSPARQL 1.0 Standard Working Group" ;
        dc:date           "2011-06-16"^^xsd:date ;
        dc:description    "\n      Exists if the subject SpatialObject is spatially disjoint \n      from the object SpatialObject. DE-9IM: FF*FF****\n    "@en ;
        skos:definition   "\n      Exists if the subject SpatialObject is spatially disjoint \n      from the object SpatialObject. DE-9IM: FF*FF****\n    "@en ;
        skos:prefLabel    "disjoint"@en .

geo:sfCrosses  a          owl:ObjectProperty ;
        rdfs:comment      "\n      Exists if the subject SpatialObject spatially crosses the \n      object SpatialObject. DE-9IM: T*T******\n    "@en ;
        rdfs:domain       geo:SpatialObject ;
        rdfs:isDefinedBy  <http://www.opengis.net/ont/geosparql> , <http://www.opengis.net/spec/geosparql/1.0> ;
        rdfs:label        "crosses"@en ;
        rdfs:range        geo:SpatialObject ;
        dc:contributor    "Matthew Perry" ;
        dc:creator        "OGC GeoSPARQL 1.0 Standard Working Group" ;
        dc:date           "2011-06-16"^^xsd:date ;
        dc:description    "\n      Exists if the subject SpatialObject spatially crosses the \n      object SpatialObject. DE-9IM: T*T******\n    "@en ;
        skos:definition   "\n      Exists if the subject SpatialObject spatially crosses the \n      object SpatialObject. DE-9IM: T*T******\n    "@en ;
        skos:prefLabel    "crosses"@en .

geo:dimension  a          owl:DatatypeProperty ;
        rdfs:comment      "\n      The topological dimension of this geometric object, which \n      must be less than or equal to the coordinate dimension. \n      In non-homogeneous collections, this will return the largest \n      topological dimension of the contained objects.\n    "@en ;
        rdfs:domain       geo:Geometry ;
        rdfs:isDefinedBy  <http://www.opengis.net/ont/geosparql> , <http://www.opengis.net/spec/geosparql/1.0> ;
        rdfs:label        "dimension"@en ;
        rdfs:range        xsd:integer ;
        dc:contributor    "Matthew Perry" ;
        dc:creator        "OGC GeoSPARQL 1.0 Standard Working Group" ;
        dc:date           "2011-06-16"^^xsd:date ;
        dc:description    "\n      The topological dimension of this geometric object, which \n      must be less than or equal to the coordinate dimension. \n      In non-homogeneous collections, this will return the largest \n      topological dimension of the contained objects.\n    "@en ;
        skos:definition   "\n      The topological dimension of this geometric object, which \n      must be less than or equal to the coordinate dimension. \n      In non-homogeneous collections, this will return the largest \n      topological dimension of the contained objects.\n    "@en ;
        skos:prefLabel    "dimension"@en .

geo:rcc8dc  a             owl:ObjectProperty ;
        rdfs:comment      "\n      Exists if the subject SpatialObject is spatially disjoint\n      from the object SpatialObject. DE-9IM: FFTFFTTTT\n    "@en ;
        rdfs:domain       geo:SpatialObject ;
        rdfs:isDefinedBy  <http://www.opengis.net/ont/geosparql> , <http://www.opengis.net/spec/geosparql/1.0> ;
        rdfs:label        "disconnected"@en ;
        rdfs:range        geo:SpatialObject ;
        dc:contributor    "Matthew Perry" ;
        dc:creator        "OGC GeoSPARQL 1.0 Standard Working Group" ;
        dc:date           "2011-06-16"^^xsd:date ;
        dc:description    "\n      Exists if the subject SpatialObject is spatially disjoint\n      from the object SpatialObject. DE-9IM: FFTFFTTTT\n    "@en ;
        skos:definition   "\n      Exists if the subject SpatialObject is spatially disjoint\n      from the object SpatialObject. DE-9IM: FFTFFTTTT\n    "@en ;
        skos:prefLabel    "disconnected"@en .

geo:hasGeometry  a        owl:ObjectProperty ;
        rdfs:comment      "\n      A spatial representation for a given feature.\n    "@en ;
        rdfs:domain       geo:Feature ;
        rdfs:isDefinedBy  <http://www.opengis.net/ont/geosparql> , <http://www.opengis.net/spec/geosparql/1.0> ;
        rdfs:label        "hasGeometry"@en ;
        rdfs:range        geo:Geometry ;
        dc:contributor    "Matthew Perry" ;
        dc:creator        "OGC GeoSPARQL 1.0 Standard Working Group" ;
        dc:date           "2011-06-16"^^xsd:date ;
        dc:description    "\n      A spatial representation for a given feature.\n    "@en ;
        skos:definition   "\n      A spatial representation for a given feature.\n    "@en ;
        skos:prefLabel    "hasGeometry"@en .

geo:sfContains  a         owl:ObjectProperty ;
        rdfs:comment      "\n      Exists if the subject SpatialObject spatially contains the \n      object SpatialObject. DE-9IM: T*****FF*\n    "@en ;
        rdfs:domain       geo:SpatialObject ;
        rdfs:isDefinedBy  <http://www.opengis.net/spec/geosparql/1.0> , <http://www.opengis.net/ont/geosparql> ;
        rdfs:label        "contains"@en ;
        rdfs:range        geo:SpatialObject ;
        dc:contributor    "Matthew Perry" ;
        dc:creator        "OGC GeoSPARQL 1.0 Standard Working Group" ;
        dc:date           "2011-06-16"^^xsd:date ;
        dc:description    "\n      Exists if the subject SpatialObject spatially contains the \n      object SpatialObject. DE-9IM: T*****FF*\n    "@en ;
        skos:definition   "\n      Exists if the subject SpatialObject spatially contains the \n      object SpatialObject. DE-9IM: T*****FF*\n    "@en ;
        skos:prefLabel    "contains"@en .

geo:coordinateDimension
        a                 owl:DatatypeProperty ;
        rdfs:comment      "\n      The number of measurements or axes needed to describe the position of this\n      geometry in a coordinate system.\n    "@en ;
        rdfs:domain       geo:Geometry ;
        rdfs:isDefinedBy  <http://www.opengis.net/spec/geosparql/1.0> , <http://www.opengis.net/ont/geosparql> ;
        rdfs:label        "coordinateDimension"@en ;
        rdfs:range        xsd:integer ;
        dc:contributor    "Matthew Perry" ;
        dc:creator        "OGC GeoSPARQL 1.0 Standard Working Group" ;
        dc:date           "2011-06-16"^^xsd:date ;
        dc:description    "\n      The number of measurements or axes needed to describe the position of this\n      geometry in a coordinate system.\n    "@en ;
        skos:definition   "\n      The number of measurements or axes needed to describe the position of this\n      geometry in a coordinate system.\n    "@en ;
        skos:prefLabel    "coordinateDimension"@en .

geo:asWKT  a                owl:DatatypeProperty ;
        rdfs:comment        "\n      The WKT serialization of a geometry\n    "@en ;
        rdfs:domain         geo:Geometry ;
        rdfs:isDefinedBy    <http://www.opengis.net/spec/geosparql/1.0> , <http://www.opengis.net/ont/geosparql> ;
        rdfs:label          "asWKT"@en ;
        rdfs:range          geo:wktLiteral ;
        rdfs:subPropertyOf  geo:hasSerialization ;
        dc:contributor      "Matthew Perry" ;
        dc:creator          "OGC GeoSPARQL 1.0 Standard Working Group" ;
        dc:date             "2011-06-16"^^xsd:date ;
        dc:description      "\n      The WKT serialization of a geometry\n    "@en ;
        skos:definition     "\n      The WKT serialization of a geometry\n    "@en ;
        skos:prefLabel      "asWKT"@en .

geo:rcc8eq  a             owl:ObjectProperty ;
        rdfs:comment      "\n      Exists if the subject SpatialObject spatially equals the \n      object SpatialObject. DE-9IM: TFFFTFFFT\n    "@en ;
        rdfs:domain       geo:SpatialObject ;
        rdfs:isDefinedBy  <http://www.opengis.net/spec/geosparql/1.0> , <http://www.opengis.net/ont/geosparql> ;
        rdfs:label        "equals"@en ;
        rdfs:range        geo:SpatialObject ;
        dc:contributor    "Matthew Perry" ;
        dc:creator        "OGC GeoSPARQL 1.0 Standard Working Group" ;
        dc:date           "2011-06-16"^^xsd:date ;
        dc:description    "\n      Exists if the subject SpatialObject spatially equals the \n      object SpatialObject. DE-9IM: TFFFTFFFT\n    "@en ;
        skos:definition   "\n      Exists if the subject SpatialObject spatially equals the \n      object SpatialObject. DE-9IM: TFFFTFFFT\n    "@en ;
        skos:prefLabel    "equals"@en .

geo:ehMeet  a             owl:ObjectProperty ;
        rdfs:comment      "\n      Exists if the subject SpatialObject spatially meets the \n      object SpatialObject. \n      DE-9IM: FT******* ^ F**T***** ^ F***T****\n    "@en ;
        rdfs:domain       geo:SpatialObject ;
        rdfs:isDefinedBy  <http://www.opengis.net/ont/geosparql> , <http://www.opengis.net/spec/geosparql/1.0> ;
        rdfs:label        "meet"@en ;
        rdfs:range        geo:SpatialObject ;
        dc:contributor    "Matthew Perry" ;
        dc:creator        "OGC GeoSPARQL 1.0 Standard Working Group" ;
        dc:date           "2011-06-16"^^xsd:date ;
        dc:description    "\n      Exists if the subject SpatialObject spatially meets the \n      object SpatialObject. \n      DE-9IM: FT******* ^ F**T***** ^ F***T****\n    "@en ;
        skos:definition   "\n      Exists if the subject SpatialObject spatially meets the \n      object SpatialObject. \n      DE-9IM: FT******* ^ F**T***** ^ F***T****\n    "@en ;
        skos:prefLabel    "meet"@en .

geo:asGML  a                owl:DatatypeProperty ;
        rdfs:comment        "\n      The GML serialization of a geometry\n    "@en ;
        rdfs:domain         geo:Geometry ;
        rdfs:isDefinedBy    <http://www.opengis.net/spec/geosparql/1.0> , <http://www.opengis.net/ont/geosparql> ;
        rdfs:label          "asGML"@en ;
        rdfs:range          geo:gmlLiteral ;
        rdfs:subPropertyOf  geo:hasSerialization ;
        dc:contributor      "Matthew Perry" ;
        dc:creator          "OGC GeoSPARQL 1.0 Standard Working Group" ;
        dc:date             "2011-06-16"^^xsd:date ;
        dc:description      "\n      The GML serialization of a geometry\n    "@en ;
        skos:definition     "\n      The GML serialization of a geometry\n    "@en ;
        skos:prefLabel      "asGML"@en .

<http://www.opengis.net/ont/geosparql>
        a                owl:Ontology ;
        rdfs:seeAlso     <http://www.opengis.net/doc/IS/geosparql/1.0> , <http://www.opengis.net/def/rule/ogc-geosparql/1.0> , <http://www.opengis.net/def/function/ogc-geosparql/1.0> ;
        dc:creator       "Open Geospatial Consortium"^^xsd:string ;
        dc:date          "2012-04-30"^^xsd:date ;
        dc:description   "An RDF/OWL vocabulary for representing spatial information"^^xsd:string ;
        dc:source        "OGC GeoSPARQL – A Geographic Query Language for RDF Data OGC 11-052r5"^^xsd:string ;
        dc:source        <http://www.opengis.net/doc/IS/geosparql/1.0> ;
        owl:imports      <http://www.opengis.net/ont/gml> , <http://www.opengis.net/ont/sf> , dc: , <http://www.w3.org/2004/02/skos/core> ;
        owl:versionInfo  "OGC GeoSPARQL 1.0"^^xsd:string .

geo:hasSerialization  a   owl:DatatypeProperty ;
        rdfs:comment      "\n      Connects a geometry object with its text-based serialization.\n    "@en ;
        rdfs:domain       geo:Geometry ;
        rdfs:isDefinedBy  <http://www.opengis.net/spec/geosparql/1.0> , <http://www.opengis.net/ont/geosparql> ;
        rdfs:label        "has serialization"@en ;
        rdfs:range        rdfs:Literal ;
        dc:contributor    "Matthew Perry" ;
        dc:creator        "OGC GeoSPARQL 1.0 Standard Working Group" ;
        dc:date           "2011-06-16"^^xsd:date ;
        dc:description    "\n      Connects a geometry object with its text-based serialization.\n    "@en ;
        skos:definition   "\n      Connects a geometry object with its text-based serialization.\n    "@en ;
        skos:prefLabel    "has serialization"@en .

geo:sfOverlaps  a         owl:ObjectProperty ;
        rdfs:comment      "\n      Exists if the subject SpatialObject spatially overlaps the \n      object SpatialObject. DE-9IM: T*T***T** \n    "@en ;
        rdfs:domain       geo:SpatialObject ;
        rdfs:isDefinedBy  <http://www.opengis.net/spec/geosparql/1.0> , <http://www.opengis.net/ont/geosparql> ;
        rdfs:label        "overlaps"@en ;
        rdfs:range        geo:SpatialObject ;
        dc:contributor    "Matthew Perry" ;
        dc:creator        "OGC GeoSPARQL 1.0 Standard Working Group" ;
        dc:date           "2011-06-16"^^xsd:date ;
        dc:description    "\n      Exists if the subject SpatialObject spatially overlaps the \n      object SpatialObject. DE-9IM: T*T***T** \n    "@en ;
        skos:definition   "\n      Exists if the subject SpatialObject spatially overlaps the \n      object SpatialObject. DE-9IM: T*T***T** \n    "@en ;
        skos:prefLabel    "overlaps"@en .

geo:defaultGeometry  a      owl:ObjectProperty ;
        rdfs:comment        "\n      The default geometry to be used in spatial calculations.\n      It is Usually the most detailed geometry.\n    "@en ;
        rdfs:domain         geo:Feature ;
        rdfs:isDefinedBy    <http://www.opengis.net/ont/geosparql> , <http://www.opengis.net/spec/geosparql/1.0> ;
        rdfs:label          "defaultGeometry"@en ;
        rdfs:range          geo:Geometry ;
        rdfs:subPropertyOf  geo:hasGeometry ;
        dc:contributor      "Matthew Perry" ;
        dc:creator          "OGC GeoSPARQL 1.0 Standard Working Group" ;
        dc:date             "2011-06-16"^^xsd:date ;
        dc:description      "\n      The default geometry to be used in spatial calculations.\n      It is Usually the most detailed geometry.\n    "@en ;
        skos:definition     "\n      The default geometry to be used in spatial calculations.\n      It is Usually the most detailed geometry.\n    "@en ;
        skos:prefLabel      "defaultGeometry"@en .

geo:spatialDimension  a   owl:DatatypeProperty ;
        rdfs:comment      "\n      The number of measurements or axes needed to describe the spatial position of \n      this geometry in a coordinate system.\n    "@en ;
        rdfs:domain       geo:Geometry ;
        rdfs:isDefinedBy  <http://www.opengis.net/ont/geosparql> , <http://www.opengis.net/spec/geosparql/1.0> ;
        rdfs:label        "spatialDimension"@en ;
        rdfs:range        xsd:integer ;
        dc:contributor    "Matthew Perry" ;
        dc:creator        "OGC GeoSPARQL 1.0 Standard Working Group" ;
        dc:date           "2011-06-16"^^xsd:date ;
        dc:description    "\n      The number of measurements or axes needed to describe the spatial position of \n      this geometry in a coordinate system.\n    "@en ;
        skos:definition   "\n      The number of measurements or axes needed to describe the spatial position of \n      this geometry in a coordinate system.\n    "@en ;
        skos:prefLabel    "spatialDimension"@en .

geo:rcc8ntppi  a          owl:ObjectProperty ;
        rdfs:comment      "\n      Exists if the subject SpatialObject spatially contains the \n      object SpatialObject. DE-9IM: TTTFFTFFT\n    "@en ;
        rdfs:domain       geo:SpatialObject ;
        rdfs:isDefinedBy  <http://www.opengis.net/spec/geosparql/1.0> , <http://www.opengis.net/ont/geosparql> ;
        rdfs:label        "non-tangential proper part inverse"@en ;
        rdfs:range        geo:SpatialObject ;
        dc:contributor    "Matthew Perry" ;
        dc:creator        "OGC GeoSPARQL 1.0 Standard Working Group" ;
        dc:date           "2011-06-16"^^xsd:date ;
        dc:description    "\n      Exists if the subject SpatialObject spatially contains the \n      object SpatialObject. DE-9IM: TTTFFTFFT\n    "@en ;
        skos:definition   "\n      Exists if the subject SpatialObject spatially contains the \n      object SpatialObject. DE-9IM: TTTFFTFFT\n    "@en ;
        skos:prefLabel    "non-tangential proper part inverse"@en .

geo:sfEquals  a           owl:ObjectProperty ;
        rdfs:comment      "\n      Exists if the subject SpatialObject spatially equals the \n      object SpatialObject. DE-9IM: TFFFTFFFT\n    "@en ;
        rdfs:domain       geo:SpatialObject ;
        rdfs:isDefinedBy  <http://www.opengis.net/ont/geosparql> , <http://www.opengis.net/spec/geosparql/1.0> ;
        rdfs:label        "equals"@en ;
        rdfs:range        geo:SpatialObject ;
        dc:contributor    "Matthew Perry" ;
        dc:creator        "OGC GeoSPARQL 1.0 Standard Working Group" ;
        dc:date           "2011-06-16"^^xsd:date ;
        dc:description    "\n      Exists if the subject SpatialObject spatially equals the \n      object SpatialObject. DE-9IM: TFFFTFFFT\n    "@en ;
        skos:definition   "\n      Exists if the subject SpatialObject spatially equals the \n      object SpatialObject. DE-9IM: TFFFTFFFT\n    "@en ;
        skos:prefLabel    "equals"@en .

geo:wktLiteral  a         rdfs:Datatype ;
        rdfs:comment      "\n      A Well-known Text serialization of a geometry object.\n    "@en ;
        rdfs:isDefinedBy  <http://www.opengis.net/ont/geosparql> , <http://www.opengis.net/spec/geosparql/1.0> ;
        rdfs:label        "Well-known Text Literal"@en ;
        dc:contributor    "Matthew Perry" ;
        dc:creator        "OGC GeoSPARQL 1.0 Standard Working Group" ;
        dc:date           "2011-06-16"^^xsd:date ;
        dc:description    "\n      A Well-known Text serialization of a geometry object.\n    "@en ;
        skos:definition   "\n      A Well-known Text serialization of a geometry object.\n    "@en ;
        skos:prefLabel    "Well-known Text Literal"@en .

geo:ehCovers  a           owl:ObjectProperty ;
        rdfs:comment      "\n      Exists if the subject SpatialObject spatially covers the \n      object SpatialObject. DE-9IM: T*TFT*FF*\n    "@en ;
        rdfs:domain       geo:SpatialObject ;
        rdfs:isDefinedBy  <http://www.opengis.net/ont/geosparql> , <http://www.opengis.net/spec/geosparql/1.0> ;
        rdfs:label        "covers"@en ;
        rdfs:range        geo:SpatialObject ;
        dc:contributor    "Matthew Perry" ;
        dc:creator        "OGC GeoSPARQL 1.0 Standard Working Group" ;
        dc:date           "2011-06-16"^^xsd:date ;
        dc:description    "\n      Exists if the subject SpatialObject spatially covers the \n      object SpatialObject. DE-9IM: T*TFT*FF*\n    "@en ;
        skos:definition   "\n      Exists if the subject SpatialObject spatially covers the \n      object SpatialObject. DE-9IM: T*TFT*FF*\n    "@en ;
        skos:prefLabel    "covers"@en .

geo:isSimple  a           owl:DatatypeProperty ;
        rdfs:comment      "\n      (true) if this geometric object has no anomalous geometric \n      points, such as self intersection or self tangency.\n    "@en ;
        rdfs:domain       geo:Geometry ;
        rdfs:isDefinedBy  <http://www.opengis.net/ont/geosparql> , <http://www.opengis.net/spec/geosparql/1.0> ;
        rdfs:label        "isSimple"@en ;
        rdfs:range        xsd:boolean ;
        dc:contributor    "Matthew Perry" ;
        dc:creator        "OGC GeoSPARQL 1.0 Standard Working Group" ;
        dc:date           "2011-06-16"^^xsd:date ;
        dc:description    "\n      (true) if this geometric object has no anomalous geometric \n      points, such as self intersection or self tangency.\n    "@en ;
        skos:definition   "\n      (true) if this geometric object has no anomalous geometric \n      points, such as self intersection or self tangency.\n    "@en ;
        skos:prefLabel    "isSimple"@en .

geo:rcc8po  a             owl:ObjectProperty ;
        rdfs:comment      "\n      Exists if the subject SpatialObject spatially overlaps the \n      object SpatialObject. DE-9IM: TTTTTTTTT\n    "@en ;
        rdfs:domain       geo:SpatialObject ;
        rdfs:isDefinedBy  <http://www.opengis.net/spec/geosparql/1.0> , <http://www.opengis.net/ont/geosparql> ;
        rdfs:label        "partially overlapping"@en ;
        rdfs:range        geo:SpatialObject ;
        dc:contributor    "Matthew Perry" ;
        dc:creator        "OGC GeoSPARQL 1.0 Standard Working Group" ;
        dc:date           "2011-06-16"^^xsd:date ;
        dc:description    "\n      Exists if the subject SpatialObject spatially overlaps the \n      object SpatialObject. DE-9IM: TTTTTTTTT\n    "@en ;
        skos:definition   "\n      Exists if the subject SpatialObject spatially overlaps the \n      object SpatialObject. DE-9IM: TTTTTTTTT\n    "@en ;
        skos:prefLabel    "partially overlapping"@en .

geo:rcc8tpp  a            owl:ObjectProperty ;
        rdfs:comment      "\n      Exists if the subject SpatialObject is spatially covered \n      by the object SpatialObject. DE-9IM: TFFTTFTTT\n    "@en ;
        rdfs:domain       geo:SpatialObject ;
        rdfs:isDefinedBy  <http://www.opengis.net/ont/geosparql> , <http://www.opengis.net/spec/geosparql/1.0> ;
        rdfs:label        "tangential proper part"@en ;
        rdfs:range        geo:SpatialObject ;
        dc:contributor    "Matthew Perry" ;
        dc:creator        "OGC GeoSPARQL 1.0 Standard Working Group" ;
        dc:date           "2011-06-16"^^xsd:date ;
        dc:description    "\n      Exists if the subject SpatialObject is spatially covered \n      by the object SpatialObject. DE-9IM: TFFTTFTTT\n    "@en ;
        skos:definition   "\n      Exists if the subject SpatialObject is spatially covered \n      by the object SpatialObject. DE-9IM: TFFTTFTTT\n    "@en ;
        skos:prefLabel    "tangential proper part"@en .

geo:Geometry  a           owl:Class ;
        rdfs:comment      "\n      The class represents the top-level geometry type. This class is \n      equivalent to the UML class GM_Object defined in ISO 19107, and \n      it is superclass of all geometry types.\n    "@en ;
        rdfs:isDefinedBy  <http://www.opengis.net/spec/geosparql/1.0> , <http://www.opengis.net/ont/geosparql> ;
        rdfs:label        "Geometry"@en ;
        rdfs:subClassOf   geo:SpatialObject ;
        dc:contributor    "Matthew Perry" ;
        dc:creator        "OGC GeoSPARQL 1.0 Standard Working Group" ;
        dc:date           "2011-06-16"^^xsd:date ;
        dc:description    "\n      The class represents the top-level geometry type. This class is \n      equivalent to the UML class GM_Object defined in ISO 19107, and \n      it is superclass of all geometry types.\n    "@en ;
        owl:disjointWith  geo:Feature ;
        skos:definition   "\n      The class represents the top-level geometry type. This class is \n      equivalent to the UML class GM_Object defined in ISO 19107, and \n      it is superclass of all geometry types.\n    "@en ;
        skos:prefLabel    "Geometry"@en .

geo:rcc8ec  a             owl:ObjectProperty ;
        rdfs:comment      "\n      Exists if the subject SpatialObject spatially meets the \n      object SpatialObject. DE-9IM: FFTFTTTTT\n    "@en ;
        rdfs:domain       geo:SpatialObject ;
        rdfs:isDefinedBy  <http://www.opengis.net/spec/geosparql/1.0> , <http://www.opengis.net/ont/geosparql> ;
        rdfs:label        "externally connected"@en ;
        rdfs:range        geo:SpatialObject ;
        dc:contributor    "Matthew Perry" ;
        dc:creator        "OGC GeoSPARQL 1.0 Standard Working Group" ;
        dc:date           "2011-06-16"^^xsd:date ;
        dc:description    "\n      Exists if the subject SpatialObject spatially meets the \n      object SpatialObject. DE-9IM: FFTFTTTTT\n    "@en ;
        skos:definition   "\n      Exists if the subject SpatialObject spatially meets the \n      object SpatialObject. DE-9IM: FFTFTTTTT\n    "@en ;
        skos:prefLabel    "externally connected"@en .

geo:SpatialObject  a      owl:Class ;
        rdfs:comment      "\n      The class spatial-object represents everything that can have \n      a spatial representation. It is superclass of feature and geometry.\n    "@en ;
        rdfs:isDefinedBy  <http://www.opengis.net/spec/geosparql/1.0> , <http://www.opengis.net/ont/geosparql> ;
        rdfs:label        "SpatialObject"@en ;
        dc:contributor    "Matthew Perry" ;
        dc:creator        "OGC GeoSPARQL 1.0 Standard Working Group" ;
        dc:date           "2011-06-16"^^xsd:date ;
        dc:description    "\n      The class spatial-object represents everything that can have \n      a spatial representation. It is superclass of feature and geometry.\n    "@en ;
        skos:definition   "\n      The class spatial-object represents everything that can have \n      a spatial representation. It is superclass of feature and geometry.\n    "@en ;
        skos:prefLabel    "SpatialObject"@en .

geo:ehCoveredBy  a        owl:ObjectProperty ;
        rdfs:comment      "\n      Exists if the subject SpatialObject is spatially covered \n      by the object SpatialObject. DE-9IM: TFF*TFT**\n    "@en ;
        rdfs:domain       geo:SpatialObject ;
        rdfs:isDefinedBy  <http://www.opengis.net/spec/geosparql/1.0> , <http://www.opengis.net/ont/geosparql> ;
        rdfs:label        "coveredBy"@en ;
        rdfs:range        geo:SpatialObject ;
        dc:contributor    "Matthew Perry" ;
        dc:creator        "OGC GeoSPARQL 1.0 Standard Working Group" ;
        dc:date           "2011-06-16"^^xsd:date ;
        dc:description    "\n      Exists if the subject SpatialObject is spatially covered \n      by the object SpatialObject. DE-9IM: TFF*TFT**\n    "@en ;
        skos:definition   "\n      Exists if the subject SpatialObject is spatially covered \n      by the object SpatialObject. DE-9IM: TFF*TFT**\n    "@en ;
        skos:prefLabel    "coveredBy"@en .

geo:ehOverlap  a          owl:ObjectProperty ;
        rdfs:comment      "\n      Exists if the subject SpatialObject spatially overlaps the \n      object SpatialObject. DE-9IM: T*T***T**\n    "@en ;
        rdfs:domain       geo:SpatialObject ;
        rdfs:isDefinedBy  <http://www.opengis.net/spec/geosparql/1.0> , <http://www.opengis.net/ont/geosparql> ;
        rdfs:label        "overlap"@en ;
        rdfs:range        geo:SpatialObject ;
        dc:contributor    "Matthew Perry" ;
        dc:creator        "OGC GeoSPARQL 1.0 Standard Working Group" ;
        dc:date           "2011-06-16"^^xsd:date ;
        dc:description    "\n      Exists if the subject SpatialObject spatially overlaps the \n      object SpatialObject. DE-9IM: T*T***T**\n    "@en ;
        skos:definition   "\n      Exists if the subject SpatialObject spatially overlaps the \n      object SpatialObject. DE-9IM: T*T***T**\n    "@en ;
        skos:prefLabel    "overlap"@en .
