@prefix : <http://purl.oclc.org/NET/ldr/ns#> .
@prefix lkif: <http://www.estrellaproject.org/lkif-core/lkif-core.owl> .
@prefix dc: <http://purl.org/dc/elements/1.1/> .
@prefix prov: <http://www.w3.org/ns/prov#> .
@prefix foaf: <http://xmlns.com/foaf/0.1/> .
@prefix frbr: <http://purl.org/vocab/frbr/core#> .
@prefix acl: <http://www.w3.org/ns/auth/acl#> .
@prefix vann: <http://purl.org/vocab/vann/> .
@prefix void: <http://rdfs.org/ns/void#> .
@prefix voaf: <http://purl.org/vocommons/voaf#> .
@prefix rdfs: <http://www.w3.org/2000/01/rdf-schema#> .
@prefix cpannotationschema: <http://www.ontologydesignpatterns.org/schemas/cpannotationschema.owl#> .
@prefix dct: <http://purl.org/dc/terms/> .
@prefix xsd: <http://www.w3.org/2001/XMLSchema#> .
@prefix owl: <http://www.w3.org/2002/07/owl#> .
@prefix rdf: <http://www.w3.org/1999/02/22-rdf-syntax-ns#> .
@prefix skos: <http://www.w3.org/2004/02/skos/core#> .
@prefix cc: <http://creativecommons.org/ns#> .
@prefix odrl: <http://www.w3.org/ns/odrl/2/> .

<http://purl.oclc.org/NET/ldr/ns#> a owl:Ontology ;
	rdfs:label "Linked Data Rights"@en ;
	voaf:propertyNumber "11"^^xsd:int ;
	dct:issued "2013-09-20"^^xsd:date ;
	voaf:classNumber "27"^^xsd:int ;
	dc:contributor "Victor Rodriguez" ;
	vann:preferredNamespaceUri "http://purl.oclc.org/NET/ldr/ns#" ;
	owl:versionInfo "1.0"@en ;
	dc:contributor "Mari Carmen Suarez" , "Asuncion Gomez" ;
	vann:preferredNamespacePrefix "ldr" ;
	cpannotationschema:scenarios "Declaring rights on both Linked Open Data and Linked Closed Data"@en ;
	dc:title "Linked Data Rights (LDR)"@en ;
	dc:creator "Ontology Engineering Group - Universidad Polit√©cnica de Madrid" ;
	dc:contributor "Maria Poveda" ;
	dc:description "he Linked Data Rights ontology provides the vocabulary for creating rights expressions for Linked Data resources. Linked Data assets (RDF triples, graphs, datasets, mappings...) can be object of protection by the intellectual property law, the database law or its access or publication be restricted by other legal reasons (personal data pro- tection, security reasons, etc.). Publishing a rights expression along with the digital asset, allows the rightsholder waiving some or all of the IP and database rights (leaving the work in the public domain), permitting some operations if certain conditions are satisfied (like giving attribution to the author) or simply reminding the audience that some rights are reserved."@en ;
	cpannotationschema:hasComponent "http://www.w3.org/TR/swbp-n-aryRelations/"@en ;
	cc:license <http://creativecommons.org/licenses/by/3.0/> ;
	voaf:reliesOn cc:null ;
	voaf:specializes cc:null ;
	voaf:hasEquivalencesWith cc:null ;
	voaf:similar <http://data.opendataday.it/LiMo> ;
	dc:creator <http://delicias.dia.fi.upm.es/~vrodriguez/> ;
	voaf:similar <http://ns.inria.fr/l4lod/v2/l4lod_v2.rdf> ;
	cpannotationschema:hasIntent <http://oeg-dev.dia.fi.upm.es/licensius/static/ldr/pattern.html#int> ;
	cpannotationschema:coversRequirements <http://oeg-dev.dia.fi.upm.es/licensius/static/ldr/pattern.html#reqs> ;
	prov:wasDerivedFrom <http://oeg-dev.dia.fi.upm.es/licensius/static/lldr/lldr-2013.07.18.owl> ;
	voaf:reliesOn dc:null ;
	voaf:similar <http://schema.theodi.org/odrs/> ;
	voaf:specializes odrl:null ;
	voaf:hasEquivalencesWith odrl:null ;
	voaf:reliesOn odrl:null ;
	voaf:similar odrl:null ;
	voaf:hasEquivalencesWith foaf:null .

skos:narrowMatch a owl:AnnotationProperty .

skos:exactMatch a owl:AnnotationProperty .

skos:example a owl:AnnotationProperty .

:hasClaim a owl:ObjectProperty ;
	rdfs:comment "Declares a claim asserted about a rights expression"@en ;
	rdfs:range :Proposition ;
	rdfs:domain :RightsExpression .

:hasObject a owl:ObjectProperty ;
	rdfs:comment "Declares which object is referred in a rights expression"@en ;
	rdfs:domain :RightsExpression ;
	rdfs:range :RightsObject ;
	skos:exactMatch odrl:target .

:hasPart a owl:ObjectProperty ;
	rdfs:comment "Declares that which rights expression is part of a composite rights expression"@en ;
	rdfs:domain :ComplexRightsExpression ;
	rdfs:range :RightsExpression .

:hasRequirement a owl:ObjectProperty ;
	rdfs:comment "Declares which requirements have to be fulfilled for the rights expression to be valid"@en ;
	rdfs:range :Proposition ;
	rdfs:domain :RightsExpression .

:hasRight a owl:ObjectProperty ;
	rdfs:comment "Declares the right of a right expression"@en ;
	rdfs:range :Right ;
	rdfs:domain :RightsExpression ;
	skos:exactMatch odrl:action .

:hasSubject a owl:ObjectProperty ;
	rdfs:comment "Declares which agent can exercise the right granted in a rights expression"@en ;
	rdfs:range :Agent ;
	rdfs:domain :RightsExpression ;
	skos:exactMatch odrl:assignee .

:hasAttributionText a owl:DatatypeProperty ;
	rdfs:comment "Text that has to be included as requested by a condition"@en ;
	rdfs:domain :Proposition ;
	rdfs:range rdfs:Literal .

:hasCopyrightNotice a owl:DatatypeProperty ;
	rdfs:comment "Text that has to be attached imposed as a condition"@en ;
	rdfs:domain :Proposition ;
	rdfs:range rdfs:Literal .

:issuedOn a owl:DatatypeProperty ;
	rdfs:comment "Date on which the rights expression is issued, with legal consequences on the copyright or database right expiration."@en ;
	rdfs:domain :RightsExpression ;
	rdfs:range xsd:dateTime .

:jurisdiction a owl:DatatypeProperty ;
	rdfs:comment "legal system under which the rights expression has to be interpreted"@en ;
	skos:exactMatch cc:jurisdiction ;
	rdfs:subPropertyOf owl:topDataProperty .

:truthValue a owl:DatatypeProperty ;
	rdfs:comment "Truth value"@en ;
	rdfs:domain :Proposition ;
	rdfs:range xsd:boolean .

cc:Permission a owl:Class ;
	rdfs:subClassOf :RightsExpression ;
	rdfs:comment "Deontic proposition allowing an action"@en ;
	skos:exactMatch odrl:Permission .

cc:Prohibition a owl:Class ;
	rdfs:subClassOf :RightsExpression ;
	rdfs:comment "Deontic proposition not permitting an action"@en ;
	skos:exactMatch odrl:Prohibition .

:Access a owl:Class ;
	rdfs:subClassOf :Right ;
	rdfs:comment "Right of access, which can be legally granted (e.g. public sector information) or expressely restricted (e.g. secrets compromising national security)"@en ;
	skos:exactMatch acl:Access .

:Agent a owl:Class ;
	rdfs:comment "Agent related to a Linked Data resource" ;
	skos:exactMatch odrl:Party , foaf:Agent .

:ComplexRightsExpression a owl:Class ;
	rdfs:subClassOf :RightsExpression ;
	rdfs:comment "A right expression made up of more than one rights expressions"@en ;
	skos:exactMatch odrl:Policy .

:Contract a owl:Class ;
	rdfs:subClassOf :ComplexRightsExpression ;
	rdfs:comment "Set of rights expressions binding two agents"@en .

:CopyrightException a owl:Class ;
	rdfs:subClassOf :Proposition ;
	rdfs:comment "Reason which can be invoked to make an exception to the intellectual property or database law"@en .

:DatabaseRight a owl:Class ;
	rdfs:subClassOf :Right ;
	rdfs:comment "Sui generis right for databases, recognized in European countries and others"@en .

:Derivation a owl:Class ;
	rdfs:subClassOf :IPRight ;
	rdfs:comment "Transformation of the work, including translation adaptation or any other form modification"@en ;
	skos:exactMatch cc:DerivativeWorks .

:Distribution a owl:Class ;
	rdfs:subClassOf :IPRight ;
	rdfs:comment "Make available the original work or its copies, in a physical medium"@en ;
	skos:exactMatch cc:Distribution .

:Extraction a owl:Class ;
	rdfs:subClassOf :DatabaseRight ;
	rdfs:comment "Right to permanent or temporary transfer of all or a substantial part of the contents of a database to another medium by any means or in any form"@en .

:IPRight a owl:Class ;
	rdfs:subClassOf :Right ;
	rdfs:comment "Intellectual Property right"@en .

:KnownLicense a owl:Class ;
	rdfs:subClassOf :License ;
	rdfs:comment "License publicly available and known to the public"@en .

:License a owl:Class ;
	rdfs:subClassOf :ComplexRightsExpression ;
	rdfs:comment "Set of rights expressions offered to the public, which grant one or more rights, possibly conditioned to the fulfillment of one or more conditions (propositions)"@en .

:LinkedDataResource a owl:Class ;
	rdfs:subClassOf :RightsObject ;
	rdfs:comment "A Linked Data resource, object of some rights"@en .

:Obligation a owl:Class ;
	rdfs:subClassOf :RightsExpression ;
	rdfs:comment "Deontic proposition not permitting not doing an action"@en ;
	skos:exactMatch odrl:Duty .

:Proposition a owl:Class ;
	rdfs:comment "A veritative statement"@en .

:PublicCommunication a owl:Class ;
	rdfs:subClassOf :IPRight ;
	rdfs:comment "Granting a number of people access to the work without existing distribution"@en .

:Reproduction a owl:Class ;
	rdfs:subClassOf :IPRight ;
	rdfs:comment "Direct or indirect fixation, allowing its communication and/or making copies of it"@en ;
	skos:exactMatch cc:Reproduction .

:ResourceLegalStatus a owl:Class ;
	rdfs:subClassOf :Proposition ;
	rdfs:comment "Attribute of a resource regarding its legal status"@en .

:Reutilization a owl:Class ;
	rdfs:subClassOf :DatabaseRight ;
	rdfs:comment "Right to make available to the public all or a substantial part of the contents of a database by the distribution of copies, by renting, by on-line or other forms of transmission"@en .

:Right a owl:Class ;
	rdfs:comment "Action legally granted as allowable"@en .

:RightsExpression a owl:Class ;
	rdfs:comment "Deontic expression declaring what is permitted, prohibited or obligated to act"@en ;
	skos:narrowMatch cc:License ;
	skos:exactMatch odrl:Rule .

:RightsObject a owl:Class ;
	rdfs:comment "Object over which a right is execised"@en ;
	skos:exactMatch odrl:Asset .

void:Dataset a owl:Class ;
	rdfs:subClassOf :LinkedDataResource .

void:Linkset a owl:Class ;
	rdfs:subClassOf :LinkedDataResource .

rdf:Statement a owl:Class ;
	rdfs:subClassOf :LinkedDataResource .

<http://creativecommons.org/publicdomain/zero/1.0/> a owl:NamedIndividual , :KnownLicense ;
	rdfs:label "CC0"@en ;
	rdfs:comment "Creative Commons public domain waiver"@en .

<http://opendatacommons.org/licenses/by/> a owl:NamedIndividual , :KnownLicense ;
	rdfs:label "Open Data Commons Attribution"@en ;
	rdfs:comment "Attribution for data/databases"@en .

<http://opendatacommons.org/licenses/odbl/> a owl:NamedIndividual , :KnownLicense ;
	rdfs:label "Open Database License"@en ;
	rdfs:comment "Attribution Share-Alike for data/databases"@en .

<http://opendatacommons.org/licenses/pddl/1-0/> a owl:NamedIndividual , :KnownLicense ;
	rdfs:label "ODC Public Domain Dedication and Licence (PDDL)"@en ;
	rdfs:comment "Public Domain for data/databases"@en .

:LinkedDataAccess a owl:NamedIndividual , :Access ;
	rdfs:label "Retrieval of Linked Data resources"@en .

:attribution a owl:NamedIndividual , :Proposition ;
	rdfs:comment "credit be given to copyright holder and/or author"@en ;
	skos:exactMatch cc:Attribution .

:commercialUse a owl:NamedIndividual , :Proposition ;
	rdfs:comment "exercising rights for commercial purposes"@en ;
	skos:exactMatch cc:Commercialuse .

:copyDatabase a owl:NamedIndividual , :Extraction ;
	rdfs:comment "Coyping a dataset, for other purposes than private use"@en .

:copyWork a owl:NamedIndividual , :Reproduction ;
	rdfs:comment "copying the work for purposes other than private"@en .

:copyleft a owl:NamedIndividual , :Proposition ;
	rdfs:comment "derivative and combined works must be licensed under specified terms, similar to those on the original work"@en ;
	skos:exactMatch cc:Copyleft .

:derivation a owl:NamedIndividual , :Derivation ;
	rdfs:comment "General transformation of the work"@en .

:disclaimer a owl:NamedIndividual , :Proposition ;
	rdfs:comment "The publisher is not responsible or liable, directly or indirectly, for any damage or loss caused by the use of the published piece of information, which may be not accurate or error free. Also, the publisher does not endorse the information obtained by following the outlinks or mappings."@en .

:distribution a owl:NamedIndividual , :Distribution ;
	rdfs:comment "General act of making available the original work or its copies, in a physical medium"@en .

:downloadDatabase a owl:NamedIndividual , :Extraction ;
	rdfs:comment "Downloading a dataset, for other purposes than private use"@en .

:downloadWork a owl:NamedIndividual , :Reproduction ;
	rdfs:comment "downloading the work for purposes other than private"@en .

:extract a owl:NamedIndividual , :Extraction ;
	rdfs:comment "General right of extraction"@en .

:hasAllRightsReserved a owl:NamedIndividual , :ResourceLegalStatus ;
	rdfs:comment "Declares that the referred resource is protected under copyright or database rights, and none of them is waived"@en .

:hasCopyrightExpired a owl:NamedIndividual , :ResourceLegalStatus ;
	rdfs:comment "Declares that the referred resource has its copyright expired"@en .

:hasDatabaseRightsExpired a owl:NamedIndividual , :ResourceLegalStatus ;
	rdfs:comment "Declares that the referred resource has the database rights expired"@en .

:hasIndustrialSecret a owl:NamedIndividual , :ResourceLegalStatus ;
	rdfs:comment "The referred resource containts an Industrial Secret"@en .

:hasNationalSecurityInfo a owl:NamedIndividual , :ResourceLegalStatus ;
	rdfs:comment "Declares that the referred resource has information whose disclosure might harm the national security"@en .

:hasPersonalData a owl:NamedIndividual , :ResourceLegalStatus ;
	rdfs:comment "Declares that the referred resource has personal data"@en .

:hasTopSecret a owl:NamedIndividual , :ResourceLegalStatus ;
	rdfs:comment "Declares that the referred resource contains top secret information of military nature or other"@en .

:isInPublicDomain a owl:NamedIndividual , :ResourceLegalStatus ;
	rdfs:comment "Declares that the declared resource is in the public domain"@en .

:judicialProcess a owl:NamedIndividual , :CopyrightException ;
	rdfs:comment "if the action is carried out for the purposes of an administrative or judicial procedure"@en .

:lesserCopyleft a owl:NamedIndividual , :Proposition ;
	rdfs:comment "derivative works must be licensed under specified terms, with at least the same conditions as the original work; combinations with the work may be licensed under different terms"@en ;
	skos:exactMatch cc:LesserCopyleft .

:nationalSecurity a owl:NamedIndividual , :CopyrightException ;
	rdfs:comment "if the action is carried out in the interests of public security"@en .

:notice a owl:NamedIndividual , :Proposition ;
	rdfs:comment "copyright and license notices be kept intact"@en ;
	skos:exactMatch cc:Notice .

:publicCommunication a owl:NamedIndividual , :PublicCommunication ;
	rdfs:comment "General right of public communication"@en .

:publishDatabase a owl:NamedIndividual , :Reutilization ;
	rdfs:comment "Make available a database in internet or by other means"@en .

:rent a owl:NamedIndividual , :Distribution ;
	rdfs:comment "Renting a copy of the work"@en .

:reproduction a owl:NamedIndividual , :Reproduction ;
	rdfs:comment "General right of public reproduction"@en .

:research a owl:NamedIndividual , :CopyrightException ;
	rdfs:comment "illustration for teaching or scientific research, provided the source, including the author's name, is acknowledged"@en .

:reutilization a owl:NamedIndividual , :Reutilization ;
	rdfs:comment "General right of re-utilization"@en .

:sell a owl:NamedIndividual , :Distribution ;
	rdfs:comment "Selling a copy of the work"@en .

:sellAccess a owl:NamedIndividual , :Distribution ;
	rdfs:comment "Offering for meny the access to a copy of the work"@en .

:shareAlike a owl:NamedIndividual , :Proposition ;
	rdfs:comment "derivative works be licensed under the same terms or compatible terms as the original work"@en ;
	skos:exactMatch cc:ShareAlike .

:sourceCode a owl:NamedIndividual , :Proposition ;
	rdfs:comment "source code (the preferred form for making modifications) must be provided when exercising some rights granted by the license"@en ;
	skos:exactMatch cc:SourceCode .

:transcodeWork a owl:NamedIndividual , :Derivation ;
	skos:example "Having permission to publish a dataset as NTRIPLES, does not entitle the grantee the act of publishing the dataset as Turtle"@en ;
	rdfs:comment "Transcoding the work"@en .

:translateWork a owl:NamedIndividual , :Derivation ;
	skos:example "Having permission to publish a dataset, does not entitle the grantee the act of publishing a tanslated version of it"@en ;
	rdfs:comment "Translating the work"@en .

<http://www.nationalarchives.gov.uk/doc/open-government-licence/version/2/> a owl:NamedIndividual , :KnownLicense ;
	rdfs:label "UK Open Government License"@en , "UK Open Government License for public sector information"@en .

owl:topObjectProperty rdfs:comment "hasIssuer"@en .
