@prefix : <http://reference.data.gov.uk/def/organogram/> .
@prefix opmv: <http://purl.org/net/opmv/ns#> .
@prefix foaf: <http://xmlns.com/foaf/0.1/> .
@prefix profession: <http://reference.data.gov.uk/def/civil-service-profession/> .
@prefix void: <http://rdfs.org/ns/void#> .
@prefix sdmx-concept: <http://purl.org/linked-data/sdmx/2009/concept#> .
@prefix job: <http://reference.data.gov.uk/def/civil-service-job/> .
@prefix intervals: <http://reference.data.gov.uk/def/intervals/> .
@prefix org: <http://www.w3.org/ns/org#> .
@prefix qb: <http://purl.org/linked-data/cube#> .
@prefix rdfs: <http://www.w3.org/2000/01/rdf-schema#> .
@prefix time: <http://www.w3.org/2006/time#> .
@prefix dct: <http://purl.org/dc/terms/> .
@prefix xsd: <http://www.w3.org/2001/XMLSchema#> .
@prefix owl: <http://www.w3.org/2002/07/owl#> .
@prefix grade: <http://reference.data.gov.uk/def/civil-service-grade/> .
@prefix rdf: <http://www.w3.org/1999/02/22-rdf-syntax-ns#> .
@prefix skos: <http://www.w3.org/2004/02/skos/core#> .
@prefix gov: <http://reference.data.gov.uk/def/central-government/> .

<http://reference.data.gov.uk/def/organogram> a owl:Ontology ;
	dct:contributor _:node182kglarkx21 .

_:node182kglarkx21 foaf:mbox "jeni@jenitennison.com" ;
	foaf:name "Jeni Tennison" .

<http://reference.data.gov.uk/def/organogram> dct:created "2010-10-17"^^xsd:date ;
	dct:license <http://www.opendatacommons.org/licenses/pddl/1.0/> ;
	dct:modified "2011-06-11"^^xsd:date ;
	dct:title "Organogram Data Vocabulary"@en ;
	void:vocabulary <http://purl.org/linked-data/cube#> , <http://purl.org/net/opmv/ns#> , <http://reference.data.gov.uk/def/central-government/> , <http://reference.data.gov.uk/def/organogram/> , <http://www.w3.org/2000/01/rdf-schema#> , <http://www.w3.org/2002/07/owl#> , <http://www.w3.org/2004/02/skos/core#> , <http://www.w3.org/2006/time#> , <http://www.w3.org/ns/org#> , <http://xmlns.com/foaf/0.1/> ;
	a void:Dataset ;
	rdfs:label "Organogram Data Vocabulary"@en .

:currency a qb:AttributeProperty ;
	qb:concept sdmx-concept:currency ;
	rdfs:comment "Currency in which the salary is paid, typically attached to the dataset for single currency datasets."@en ;
	rdfs:isDefinedBy <http://reference.data.gov.uk/def/organogram/> ;
	rdfs:label "currency"@en .

:date a rdf:Property , qb:DimensionProperty , owl:ObjectProperty ;
	rdfs:comment "The date that the observation relates to."@en ;
	rdfs:domain qb:Observation ;
	rdfs:isDefinedBy <http://reference.data.gov.uk/def/organogram/> ;
	rdfs:label "Date"@en ;
	rdfs:range intervals:CalendarDay .

:grade a rdf:Property , qb:DimensionProperty , owl:ObjectProperty ;
	rdfs:comment "The grade of the junior posts."@en ;
	rdfs:domain qb:Observation ;
	rdfs:isDefinedBy <http://reference.data.gov.uk/def/organogram/> ;
	rdfs:label "Grade"@en ;
	rdfs:range grade:Grade .

:job a rdf:Property , qb:DimensionProperty , owl:ObjectProperty ;
	rdfs:comment "The job performed by the junior posts."@en ;
	rdfs:domain qb:Observation ;
	rdfs:isDefinedBy <http://reference.data.gov.uk/def/organogram/> ;
	rdfs:label "Job"@en ;
	rdfs:range job:Job .

:junior-posts a qb:DataStructureDefinition ;
	qb:component _:node182kglarkx22 .

_:node182kglarkx22 qb:dimension :unit .

:junior-posts qb:component _:node182kglarkx23 .

_:node182kglarkx23 qb:dimension :reportingTo .

:junior-posts qb:component _:node182kglarkx24 .

_:node182kglarkx24 qb:dimension :grade .

:junior-posts qb:component _:node182kglarkx25 .

_:node182kglarkx25 qb:dimension :job .

:junior-posts qb:component _:node182kglarkx26 .

_:node182kglarkx26 qb:dimension :profession .

:junior-posts qb:component _:node182kglarkx27 .

_:node182kglarkx27 qb:dimension :date .

:junior-posts qb:component _:node182kglarkx28 .

_:node182kglarkx28 qb:measure :fullTimeEquivalent .

:junior-posts a rdfs:Resource ;
	rdfs:comment "The structure of a cube containing data about the number of junior staff of different grades that report to a particular post from within a particular unit, with a particular job and a particular profession, on a particular day." ;
	rdfs:isDefinedBy <http://reference.data.gov.uk/def/organogram/> ;
	rdfs:label "Junior Posts Data Structure"@en .

:number-of-posts a qb:DataStructureDefinition ;
	qb:component _:node182kglarkx29 .

_:node182kglarkx29 qb:dimension :post .

:number-of-posts qb:component _:node182kglarkx30 .

_:node182kglarkx30 qb:dimension :grade .

:number-of-posts qb:component _:node182kglarkx31 .

_:node182kglarkx31 qb:dimension :date .

:number-of-posts qb:component _:node182kglarkx32 .

_:node182kglarkx32 qb:measure :numberOfPosts .

:number-of-posts a rdfs:Resource ;
	rdfs:comment "The structure of a cube containing data about the number of posts of different grades that report to a particular post on a particular day." ;
	rdfs:isDefinedBy <http://reference.data.gov.uk/def/organogram/> ;
	rdfs:label "Number of Posts Data Structure"@en .

:numberOfPosts a rdf:Property , qb:MeasureProperty , owl:DatatypeProperty ;
	rdfs:comment "The number of posts with this grade that report to the given post, as a full-time equivalent."@en ;
	rdfs:domain qb:Observation ;
	rdfs:isDefinedBy <http://reference.data.gov.uk/def/organogram/> ;
	rdfs:label "Number of Posts"@en ;
	rdfs:range xsd:decimal .

:post a rdf:Property , qb:DimensionProperty , owl:ObjectProperty ;
	rdfs:comment "The post whose subordinates this statistic relates to."@en ;
	rdfs:domain qb:Observation ;
	rdfs:isDefinedBy <http://reference.data.gov.uk/def/organogram/> ;
	rdfs:label "Post"@en ;
	rdfs:range gov:Post .

:profession a rdf:Property , qb:DimensionProperty , owl:ObjectProperty ;
	rdfs:comment "The profession of the junior posts."@en ;
	rdfs:domain qb:Observation ;
	rdfs:isDefinedBy <http://reference.data.gov.uk/def/organogram/> ;
	rdfs:label "Profession"@en ;
	rdfs:range profession:Profession .

:reportingTo a rdf:Property , qb:DimensionProperty , owl:ObjectProperty ;
	rdfs:comment "The post to which the junior posts report."@en ;
	rdfs:domain qb:Observation ;
	rdfs:isDefinedBy <http://reference.data.gov.uk/def/organogram/> ;
	rdfs:label "Reporting To"@en ;
	rdfs:range gov:Post .

:salary-costs-of-reports a qb:DataStructureDefinition ;
	qb:component _:node182kglarkx33 .

_:node182kglarkx33 qb:dimension :post .

:salary-costs-of-reports qb:component _:node182kglarkx34 .

_:node182kglarkx34 qb:dimension :date .

:salary-costs-of-reports qb:component _:node182kglarkx35 .

_:node182kglarkx35 qb:measure :salaryCostOfReports .

:salary-costs-of-reports qb:component _:node182kglarkx36 .

_:node182kglarkx36 qb:attribute :currency .

:salary-costs-of-reports a rdfs:Resource ;
	rdfs:comment "The structure of a cube containing data about the salary costs of the reports to a particular post on a particular day." ;
	rdfs:isDefinedBy <http://reference.data.gov.uk/def/organogram/> ;
	rdfs:label "Salary Costs Data Structure"@en .

:salaryCostOfReports a rdf:Property , qb:MeasureProperty , owl:DatatypeProperty ;
	rdfs:comment "The total salary cost of each Deputy Director/SCS Pay Band 1 and 1A member and the non-SCS staff that report to this post. Salary costs are base pay (excluding bonuses and allowances) as at the date of the observation. To ensure that individual salaries cannot be identified from this information (for Deputy Director/SCS Pay Band 1 and 1A level and non-SCS grades), where the team is less than five people, the cost is rounded to the nearest £100,000. Where the team is one person only, the salary cost may be rounded to the nearest £100,000 or merged with the costs of another team."@en ;
	rdfs:domain qb:Observation ;
	rdfs:isDefinedBy <http://reference.data.gov.uk/def/organogram/> ;
	rdfs:label "Salary Cost of Reports"@en ;
	rdfs:range xsd:integer .

:tenure a rdf:Property , qb:DimensionProperty , owl:ObjectProperty ;
	rdfs:comment "The tenure through which pay was given."@en ;
	rdfs:domain qb:Observation ;
	rdfs:isDefinedBy <http://reference.data.gov.uk/def/organogram/> ;
	rdfs:label "Tenure"@en ;
	rdfs:range gov:Tenure .

:total-pay a qb:DataStructureDefinition ;
	qb:component _:node182kglarkx37 .

_:node182kglarkx37 qb:dimension :tenure .

:total-pay qb:component _:node182kglarkx38 .

_:node182kglarkx38 qb:dimension :date .

:total-pay qb:component _:node182kglarkx39 .

_:node182kglarkx39 qb:measure :totalPay .

:total-pay qb:component _:node182kglarkx40 .

_:node182kglarkx40 qb:attribute :currency .

:total-pay a rdfs:Resource ;
	rdfs:comment "The structure of a cube containing data about the total pay received for a particular tenure (a person in a post) on a particular day." ;
	rdfs:isDefinedBy <http://reference.data.gov.uk/def/organogram/> ;
	rdfs:label "Total Pay Data Structure"@en .

:totalPay a rdf:Property , qb:MeasureProperty , owl:DatatypeProperty ;
	rdfs:comment "The total pay received."@en ;
	rdfs:domain qb:Observation ;
	rdfs:isDefinedBy <http://reference.data.gov.uk/def/organogram/> ;
	rdfs:label "Total Pay"@en ;
	rdfs:range xsd:decimal .

:unit a rdf:Property , qb:DimensionProperty , owl:ObjectProperty ;
	rdfs:comment "The unit to which the junior posts belong."@en ;
	rdfs:domain qb:Observation ;
	rdfs:isDefinedBy <http://reference.data.gov.uk/def/organogram/> ;
	rdfs:label "Unit"@en ;
	rdfs:range org:OrganizationalUnit .
