@prefix dc: <http://purl.org/dc/elements/1.1/> .
@prefix rdfs: <http://www.w3.org/2000/01/rdf-schema#> .
@prefix foaf: <http://xmlns.com/foaf/0.1/> .
@prefix owl: <http://www.w3.org/2002/07/owl#> .
@prefix vann: <http://purl.org/vocab/vann/> .
@prefix rdf: <http://www.w3.org/1999/02/22-rdf-syntax-ns#> .
@prefix vs: <http://www.w3.org/2003/06/sw-vocab-status/ns#> .
@prefix cc: <http://creativecommons.org/ns#> .

<http://ns.inria.fr/prissma/v1> a owl:Ontology ;
	dc:title "PRISSMA: Presentation of Resources for Interoperable Semantic and Shareable Mobile Adaptability" ;
	foaf:page <http://ns.inria.fr/prissma/v1/prissma.html> ;
	dc:creator <http://www-sop.inria.fr/members/Luca.Costabello/foaf.rdf#me> ;
	dc:description "A vocabulary to model context-aware presentation knowledge for RDF User Interfaces."@en ;
	dc:issued "2011-06-22"^^<http://www.w3.org/2001/XMLSchema#date> ;
	dc:modified "2011-06-22"^^<http://www.w3.org/2001/XMLSchema#date> ;
	owl:versionInfo "1.0"^^<http://www.w3.org/2001/XMLSchema#decimal> ;
	cc:license <http://creativecommons.org/licenses/by/3.0/> ;
	dc:publisher <http://dbpedia.org/resource/National_Institute_for_Research_in_Computer_Science_and_Control> .

<http://dbpedia.org/resource/National_Institute_for_Research_in_Computer_Science_and_Control> a foaf:Organization .

<http://ns.inria.fr/prissma/v1> vann:preferredNamespacePrefix "prissma" ;
	vann:preferredNamespaceUri "http://ns.inria.fr/prissma/v1#" .

<http://ns.inria.fr/prissma/v1#User> a rdfs:Class , owl:Class ;
	rdfs:label "User" ;
	rdfs:comment "Represents the target mobile user associated to a fresnel:Purpose. To provide more flexibility, the class can be used to model both user stereotypes and specific users." ;
	rdfs:subClassOf foaf:Person ;
	rdfs:isDefinedBy <http://ns.inria.fr/prissma/v1#> ;
	vs:term_status "stable" .

<http://ns.inria.fr/prissma/v1#Device> a rdfs:Class , owl:Class ;
	rdfs:label "Device" ;
	rdfs:comment "The Device represents the mobile device on which Web of Data resource consumption takes place. It enables device-specific data representation." ;
	rdfs:subClassOf <http://www.w3.org/2007/uwa/context/deliveryContext.owl#Device> ;
	rdfs:isDefinedBy <http://ns.inria.fr/prissma/v1#> ;
	vs:term_status "stable" .

<http://ns.inria.fr/prissma/v1#Environment> a rdfs:Class , owl:Class ;
	rdfs:label "Environment" ;
	rdfs:comment "The class Environment models the user context in which the resource consumption takes place, therefore enabling customized resource presentation according to specific situations." ;
	rdfs:isDefinedBy <http://ns.inria.fr/prissma/v1#> ;
	vs:term_status "stable" .

<http://ns.inria.fr/prissma/v1#Activity> a rdfs:Class , owl:Class ;
	rdfs:label "Activity" ;
	rdfs:comment "The Activity class consists in a placemark aimed at modeling a high-level representation of an user action, such as 'running', 'driving', 'working', 'shopping', etc." ;
	rdfs:isDefinedBy <http://ns.inria.fr/prissma/v1#> ;
	vs:term_status "stable" .

<http://ns.inria.fr/prissma/v1#POI> a rdfs:Class , owl:Class ;
	rdfs:label "POI" ;
	rdfs:comment "The class models a Point of Interest (POI) and consists in a simplified version of W3C Point of Interest Core specifications. POIs are defined as entities that \"describe information about locations such as name, category, unique identifier, or civic address\"." ;
	rdfs:subClassOf <http://www.w3.org/2003/01/geo/wgs84_pos#SpatialThing> ;
	rdfs:isDefinedBy <http://ns.inria.fr/prissma/v1#> ;
	vs:term_status "stable" .

<http://ns.inria.fr/prissma/v1#Time> a rdfs:Class , owl:Class ;
	rdfs:label "Time" ;
	rdfs:comment "Time class models temporal dimension." ;
	rdfs:subClassOf <http://www.w3.org/2006/time#TemporalEntity> ;
	rdfs:isDefinedBy <http://ns.inria.fr/prissma/v1#> ;
	vs:term_status "testing" .

<http://ns.inria.fr/prissma/v1#Paradigm> a rdfs:Class , owl:Class ;
	rdfs:label "Paradigm" ;
	rdfs:comment """The original Fresnel proposition does not specify the representation paradigm adopted by the user agent. The designer depends therefore on the representation paradigm adopted by the target application. Being able to address this aspect in a declarative way is important in a context-aware environment, where the representation paradigm might vary dynamically.

The class prissma:Paradigm models therefore an instance of the Fresnel abstract box model, and it is associated to a given fresnel:Purpose.""" ;
	rdfs:isDefinedBy <http://ns.inria.fr/prissma/v1#> ;
	vs:term_status "testing" .

<http://ns.inria.fr/prissma/v1#user> a rdf:Property ;
	rdfs:label "user" ;
	rdfs:comment "The property associates a User to a Purpose" ;
	rdfs:domain <http://www.w3.org/2004/09/fresnel#Purpose> ;
	rdfs:range <http://ns.inria.fr/prissma/v1#User> ;
	rdfs:isDefinedBy <http://ns.inria.fr/prissma/v1#> ;
	vs:term_status "stable" .

<http://ns.inria.fr/prissma/v1#device> a rdf:Property ;
	rdfs:label "device" ;
	rdfs:comment "The property associates a Device to a Purpose" ;
	rdfs:domain <http://www.w3.org/2004/09/fresnel#Purpose> ;
	rdfs:range <http://ns.inria.fr/prissma/v1#Device> ;
	rdfs:isDefinedBy <http://ns.inria.fr/prissma/v1#> ;
	vs:term_status "stable" .

<http://ns.inria.fr/prissma/v1#environment> a rdf:Property ;
	rdfs:label "environment" ;
	rdfs:comment "The property associates an Environment to a Purpose" ;
	rdfs:domain <http://www.w3.org/2004/09/fresnel#Purpose> ;
	rdfs:range <http://ns.inria.fr/prissma/v1#Environment> ;
	rdfs:isDefinedBy <http://ns.inria.fr/prissma/v1#> ;
	vs:term_status "stable" .

<http://ns.inria.fr/prissma/v1#currentPOI> a rdf:Property ;
	rdfs:label "currentPOI" ;
	rdfs:comment "The property associates a POI to a prissma:Environment" ;
	rdfs:domain <http://ns.inria.fr/prissma/v1#Environment> ;
	rdfs:range <http://ns.inria.fr/prissma/v1#POI> ;
	rdfs:isDefinedBy <http://ns.inria.fr/prissma/v1#> ;
	vs:term_status "stable" .

<http://ns.inria.fr/prissma/v1#nearbyEntity> a rdf:Property ;
	rdfs:label "nearbyObject" ;
	rdfs:comment "The environmental proximity of a generic object can trigger different resource representations. The property is therefore used to associate nearby objects to the Environment model." ;
	rdfs:domain <http://ns.inria.fr/prissma/v1#Environment> ;
	rdfs:range owl:Thing ;
	rdfs:isDefinedBy <http://ns.inria.fr/prissma/v1#> ;
	vs:term_status "stable" .

<http://ns.inria.fr/prissma/v1#nearbyPerson> a rdf:Property ;
	rdfs:label "nearbyPerson" ;
	rdfs:domain <http://ns.inria.fr/prissma/v1#Environment> ;
	rdfs:subPropertyOf <http://ns.inria.fr/prissma/v1#nearbyObject> ;
	rdfs:isDefinedBy <http://ns.inria.fr/prissma/v1#> ;
	vs:term_status "testing" .

<http://ns.inria.fr/prissma/v1#motion> a rdf:Property ;
	rdfs:label "motion" ;
	rdfs:comment "Associates any given high-level representation of motion to a prissma:Environment" ;
	rdfs:domain <http://ns.inria.fr/prissma/v1#Environment> ;
	rdfs:isDefinedBy <http://ns.inria.fr/prissma/v1#> ;
	vs:term_status "testing" .

<http://ns.inria.fr/prissma/v1#disability> a rdf:Property ;
	rdfs:label "disability" ;
	rdfs:comment "Refers to user disabilities that drive resource presentation on mobile." ;
	rdfs:domain <http://ns.inria.fr/prissma/v1#User> ;
	rdfs:isDefinedBy <http://ns.inria.fr/prissma/v1#> ;
	vs:term_status "testing" .

<http://ns.inria.fr/prissma/v1#poiLabel> a rdf:Property ;
	rdfs:label "poiLabel" ;
	rdfs:comment "Associates an identifying resource to a POI (e.g. a given monument, a specific restaurant, etc.)" ;
	rdfs:domain <http://ns.inria.fr/prissma/v1#POI> ;
	rdfs:isDefinedBy <http://ns.inria.fr/prissma/v1#> ;
	vs:term_status "testing" .

<http://ns.inria.fr/prissma/v1#poiCategory> a rdf:Property ;
	rdfs:label "poiCategory" ;
	rdfs:comment "Associates a category to a POI (e.g. monument, restaurant, etc.)" ;
	rdfs:domain <http://ns.inria.fr/prissma/v1#POI> ;
	rdfs:isDefinedBy <http://ns.inria.fr/prissma/v1#> ;
	vs:term_status "testing" .

<http://ns.inria.fr/prissma/v1#descriptivePeriod> a rdf:Property ;
	rdfs:label "descriptivePeriod" ;
	rdfs:comment "Property used to refer to a descriptive and rather generic period of time, such as 'morning', 'summer', 'weekend', etc." ;
	rdfs:domain <http://ns.inria.fr/prissma/v1#Time> ;
	rdfs:isDefinedBy <http://ns.inria.fr/prissma/v1#> ;
	vs:term_status "testing" .

<http://ns.inria.fr/prissma/v1#usedParadigm> a rdf:Property ;
	rdfs:label "usedParadigm" ;
	rdfs:comment "Specifies the desired representation paradigm associated to a given fresnel:Purpose" ;
	rdfs:domain <http://ns.inria.fr/prissma/v1#Paradigm> ;
	rdfs:range <http://www.w3.org/2004/09/fresnel#Purpose> ;
	rdfs:isDefinedBy <http://ns.inria.fr/prissma/v1#> ;
	vs:term_status "testing" .

<http://ns.inria.fr/prissma/v1#extension> a rdf:Property , owl:DatatypeProperty ;
	rdfs:label "Specifies the geographic extension of a POI. Value is expressed in metres." ;
	rdfs:domain <http://ns.inria.fr/prissma/v1#POI> ;
	rdfs:range <http://www.w3.org/2001/XMLSchema#nonNegativeInteger> ;
	rdfs:isDefinedBy <http://ns.inria.fr/prissma/v1#> ;
	vs:term_status "testing" .
