@prefix prv: <http://purl.org/net/provenance/ns#> .
@prefix : <http://www.w3.org/1999/xhtml> .
@prefix rdfs: <http://www.w3.org/2000/01/rdf-schema#> .
@prefix wot: <http://xmlns.com/wot/0.1/> .
@prefix foaf: <http://xmlns.com/foaf/0.1/> .
@prefix owl: <http://www.w3.org/2002/07/owl#> .
@prefix xsd: <http://www.w3.org/2001/XMLSchema#> .
@prefix rdf: <http://www.w3.org/1999/02/22-rdf-syntax-ns#> .
@prefix xhv: <http://www.w3.org/1999/xhtml/vocab#> .
@prefix dcterms: <http://purl.org/dc/terms/> .

<http://trdf.sourceforge.net/provenance/ns.html> a foaf:Document ;
	wot:assurance <http://trdf.sourceforge.net/provenance/ns.html.sig> .

<http://trdf.sourceforge.net/provenance/ns.html.sig> a wot:Endorsement ;
	wot:endorser <http://www.informatik.hu-berlin.de/~hartig/foaf.rdf#pubkey> .

<http://www.informatik.hu-berlin.de/~hartig/foaf.rdf#pubkey> a wot:PubKey .

<http://trdf.sourceforge.net/provenance/ns.html.sig> dcterms:title "Detached signature"@en .

dcterms:creator a owl:ObjectProperty .

foaf:Organization a owl:Class ;
	rdfs:subClassOf prv:HumanActor .

prv:HumanActor a owl:Class ;
	rdfs:comment "HumanActor is a general class that represents actors who are social beings such as persons, organizations, companies."@en ;
	rdfs:label "Human Actor"@en ;
	owl:disjointWith prv:NonHumanActor .

prv:NonHumanActor a owl:Class ;
	rdfs:comment "NonHumanActor is a general class that represents actors who are not social beings."@en ;
	rdfs:label "Non-Human Actor"@en ;
	owl:disjointWith prv:HumanActor ;
	rdfs:isDefinedBy <http://purl.org/net/provenance/ns> ;
	rdfs:subClassOf prv:Actor .

prv:Actor a owl:Class ;
	rdfs:isDefinedBy <http://purl.org/net/provenance/ns> ;
	rdfs:comment "Actor is a general class that represents actors which usually performed the execution (see the class <a xmlns=\"http://www.w3.org/1999/xhtml\" href=\"#Execution\" xml:lang=\"en\">Execution</a>) of an action or a process."^^rdf:XMLLiteral ;
	rdfs:label "Actor"@en ;
	owl:equivalentClass foaf:Agent .

foaf:Agent a owl:Class .

prv:HumanActor owl:disjointWith prv:Artifact .

prv:Artifact a owl:Class ;
	rdfs:isDefinedBy <http://purl.org/net/provenance/ns> ;
	rdfs:comment "Artifact is a general class that represents artifacts which can be used during the execution (see the class <a xmlns=\"http://www.w3.org/1999/xhtml\" href=\"#Execution\" xml:lang=\"en\">Execution</a>) of an action or a process and which can also be the result of such an execution."^^rdf:XMLLiteral ;
	rdfs:label "Artifact"@en ;
	owl:disjointWith prv:Execution .

prv:Execution a owl:Class ;
	rdfs:isDefinedBy <http://purl.org/net/provenance/ns> ;
	rdfs:comment "Execution is a general class that represents completed executions of actions or processes. An execution is usually performed by an actor (see the class <a xmlns=\"http://www.w3.org/1999/xhtml\" href=\"#Actor\" xml:lang=\"en\">Actor</a>) and an execution, in most cases, yielded an artifact (see the class <a xmlns=\"http://www.w3.org/1999/xhtml\" href=\"#Artifact\" xml:lang=\"en\">Artifact</a>)."^^rdf:XMLLiteral ;
	rdfs:label "Execution"@en ;
	owl:disjointWith prv:Artifact , prv:Actor .

prv:Artifact owl:disjointWith prv:Actor .

prv:HumanActor owl:disjointWith prv:Execution ;
	rdfs:isDefinedBy <http://purl.org/net/provenance/ns> ;
	rdfs:subClassOf prv:Actor .

foaf:name a owl:DatatypeProperty .

prv:performedAt a owl:DatatypeProperty ;
	rdfs:range xsd:dateTime ;
	rdfs:comment "This property refers to the time an execution has been performed at."@en ;
	rdfs:label "executed at"@en ;
	rdfs:isDefinedBy <http://purl.org/net/provenance/ns> ;
	rdfs:domain prv:Execution .

dcterms:conformsTo a owl:ObjectProperty .

dcterms:created a owl:DatatypeProperty .

wot:assurance a owl:ObjectProperty .

foaf:homepage a owl:ObjectProperty .

prv:createdBy a owl:ObjectProperty ;
	rdfs:subPropertyOf prv:yieldedBy .

prv:yieldedBy a owl:ObjectProperty ;
	rdfs:range prv:Execution ;
	rdfs:comment "This is an abstract property that refers to the execution by which an artifact was yielded."@en ;
	rdfs:label "yielded by"@en ;
	rdfs:isDefinedBy <http://purl.org/net/provenance/ns> ;
	rdfs:domain prv:Artifact .

prv:createdBy rdfs:range prv:DataCreation .

prv:DataCreation a owl:Class ;
	rdfs:comment "DataCreation is a class that represents the completed creation of a data item."@en ;
	rdfs:label "Data Creation"@en ;
	owl:disjointWith prv:DataAccess .

prv:DataAccess a owl:Class ;
	rdfs:comment "DataAccess is a class that represents the completed execution of accessing a data item on the Web."@en ;
	rdfs:label "Data Access"@en ;
	owl:disjointWith prv:DataCreation ;
	rdfs:isDefinedBy <http://purl.org/net/provenance/ns> ;
	rdfs:subClassOf prv:Execution .

prv:DataCreation rdfs:isDefinedBy <http://purl.org/net/provenance/ns> ;
	rdfs:subClassOf prv:Execution .

prv:createdBy rdfs:comment "This property refers to the creation of a data item."@en ;
	rdfs:label "created by"@en ;
	rdfs:isDefinedBy <http://purl.org/net/provenance/ns> ;
	rdfs:domain prv:DataItem .

prv:DataItem a owl:Class ;
	rdfs:comment "DataItem is a general class that represents data items of any kind."@en ;
	rdfs:label "Data Item"@en ;
	owl:disjointWith prv:Document .

prv:Document a owl:Class ;
	rdfs:comment "Document is a general class that represents a Web representation (i.e. a document) with which a data item has been retrieved from the Web."@en ;
	rdfs:label "Web Document"@en ;
	owl:disjointWith prv:DataItem ;
	rdfs:isDefinedBy <http://purl.org/net/provenance/ns> ;
	rdfs:subClassOf prv:Artifact , <http://sw.nokia.com/WebArch-1/Representation> .

<http://sw.nokia.com/WebArch-1/Representation> a owl:Class .

prv:Document rdfs:subClassOf <http://www.ontologydesignpatterns.org/ont/web/irw.owl#WebRepresentation> .

<http://www.ontologydesignpatterns.org/ont/web/irw.owl#WebRepresentation> a owl:Class .

prv:DataItem rdfs:isDefinedBy <http://purl.org/net/provenance/ns> ;
	rdfs:subClassOf prv:Artifact , <http://www.ontologydesignpatterns.org/ont/web/irw.owl#InformationResource> .

<http://www.ontologydesignpatterns.org/ont/web/irw.owl#InformationResource> a owl:Class .

<http://sw.nokia.com/WebArch-1/Service> a owl:Class ;
	rdfs:subClassOf prv:DataProvidingService .

prv:DataProvidingService a owl:Class ;
	rdfs:isDefinedBy <http://purl.org/net/provenance/ns> ;
	rdfs:comment "DataProvidingService is a class that represents a non-human actor - usually a Web service or a server - that processes data access requests and actually sends the requested Web representations (i.e. <a xmlns=\"http://www.w3.org/1999/xhtml\" href=\"#Document\" xml:lang=\"en\">prv:Document</a>) over the Web."^^rdf:XMLLiteral ;
	rdfs:label "Data Providing Service"@en ;
	rdfs:subClassOf prv:NonHumanActor .

xhv:license a owl:ObjectProperty .

wot:endorser a owl:ObjectProperty .

dcterms:title a owl:DatatypeProperty .

<http://sw.nokia.com/WebArch-1/Server> a owl:Class ;
	rdfs:subClassOf prv:DataProvidingService .

prv:retrievedBy a owl:ObjectProperty ;
	rdfs:subPropertyOf prv:yieldedBy ;
	rdfs:range prv:DataAccess ;
	rdfs:comment "This property refers to the data access by which a document that contains a data item has been retrieved from the Web."@en ;
	rdfs:label "retrieved by"@en ;
	rdfs:isDefinedBy <http://purl.org/net/provenance/ns> ;
	rdfs:domain prv:Document .

xhv:alternate a owl:ObjectProperty .

prv:usedBy a owl:ObjectProperty ;
	rdfs:range prv:DataPublisher .

prv:DataPublisher a owl:Class ;
	rdfs:isDefinedBy <http://purl.org/net/provenance/ns> ;
	rdfs:comment "DataPublisher is a class that represents entities such as persons, groups, or organizations who use a data providing service (see class <a xmlns=\"http://www.w3.org/1999/xhtml\" href=\"#DataProvidingService\" xml:lang=\"en\">prv:DataProvidingService</a>) to publish data on the Web."^^rdf:XMLLiteral ;
	rdfs:label "Data Publisher"@en ;
	rdfs:subClassOf prv:HumanActor .

prv:usedBy rdfs:comment "This property refers to a data publisher who used a data providing services."@en ;
	rdfs:label "used by"@en ;
	rdfs:isDefinedBy <http://purl.org/net/provenance/ns> ;
	rdfs:domain prv:DataProvidingService .

<http://www.ontologydesignpatterns.org/ont/web/irw.owl#WebServer> a owl:Class ;
	rdfs:subClassOf prv:DataProvidingService .

dcterms:description a owl:DatatypeProperty .

prv:precededBy a owl:ObjectProperty ;
	rdfs:subPropertyOf dcterms:replaces .

dcterms:replaces a owl:ObjectProperty .

prv:precededBy rdfs:range prv:DataItem ;
	rdfs:comment "This property refers to an immediately preceding version of a data item; hence, the new version (i.e. the subject) has been created using the old version (i.e. the object). We strongly encourage to also describe this creation of the new version explicitly."@en ;
	rdfs:label "immediately preceded by"@en ;
	rdfs:isDefinedBy <http://purl.org/net/provenance/ns> ;
	rdfs:domain prv:DataItem .

<http://purl.org/net/provenance/ns.rdf> a foaf:Document .

prv:performedBy a owl:ObjectProperty ;
	rdfs:subPropertyOf prv:involvedActor .

prv:involvedActor a owl:ObjectProperty ;
	rdfs:range prv:Actor ;
	rdfs:comment "This is an abstract property that refers to an actor involved in an execution."@en ;
	rdfs:label "involved"@en ;
	rdfs:isDefinedBy <http://purl.org/net/provenance/ns> ;
	rdfs:domain prv:Execution .

prv:performedBy rdfs:range prv:Actor ;
	rdfs:comment "This property refers to an actor that/who performed an execution."@en ;
	rdfs:label "performed by"@en ;
	rdfs:isDefinedBy <http://purl.org/net/provenance/ns> ;
	rdfs:domain prv:Execution .

<http://trdf.sourceforge.net/provenance/ns-20090825.html> a foaf:Document ;
	foaf:primaryTopic <http://purl.org/net/provenance/ns#> .

<http://purl.org/net/provenance/ns#> a owl:Ontology ;
	prv:createdBy _:node183fu4jtnx1 .

_:node183fu4jtnx1 a prv:DataCreation ;
	prv:performedBy <http://users.ox.ac.uk/~zool0770/foaf.rdf#me> .

<http://users.ox.ac.uk/~zool0770/foaf.rdf#me> a foaf:Person ;
	foaf:name "Jun Zhao"@en ;
	foaf:homepage <http://users.ox.ac.uk/~zool0770/> .

<http://users.ox.ac.uk/~zool0770/> a foaf:Document .

_:node183fu4jtnx1 prv:performedBy <http://www.informatik.hu-berlin.de/~hartig/foaf.rdf#olaf> .

<http://www.informatik.hu-berlin.de/~hartig/foaf.rdf#olaf> a foaf:Person ;
	foaf:name "Olaf Hartig"@en ;
	foaf:homepage <http://olafhartig.de/> .

<http://olafhartig.de/> a foaf:Document .

_:node183fu4jtnx1 prv:performedAt "2009-08-25T12:00:00Z"^^xsd:dateTime .

<http://purl.org/net/provenance/ns#> dcterms:creator <http://users.ox.ac.uk/~zool0770/foaf.rdf#me> , <http://www.informatik.hu-berlin.de/~hartig/foaf.rdf#olaf> ;
	dcterms:title "Provenance Vocabulary Core Ontology namespace"@en ;
	a prv:DataItem ;
	dcterms:created "2009-08-25T12:00:00Z"^^xsd:dateTime ;
	dcterms:description "The Provenance Vocabulary enables providers of Web data to publish provenance-related metadata about their data. The Provenance Vocabulary Core Ontology provides the main classes and properties required to describe provenance of data on the Web."@en .

<http://trdf.sourceforge.net/provenance/ns-20090825.html> xhv:license <http://creativecommons.org/licenses/by/1.0/> .

<http://creativecommons.org/licenses/by/1.0/> a owl:Thing .

<http://trdf.sourceforge.net/provenance/ns-20090825.html> rdfs:label "Document that defines the core ontology of the Provenance Vocabulary"@en ;
	dcterms:title "Provenance Vocabulary Core Ontology Specification"@en ;
	dcterms:description "This documents specifies the classes and properties introduced by the Provenance Vocabulary Core Ontology."@en ;
	dcterms:conformsTo <http://www.w3.org/TR/rdfa-syntax> .

<http://www.w3.org/TR/rdfa-syntax> a owl:Thing .

<http://trdf.sourceforge.net/provenance/ns-20090825.html> xhv:alternate <http://trdf.sourceforge.net/provenance/ns.rdf> .

foaf:Group a owl:Class ;
	rdfs:subClassOf prv:HumanActor .

foaf:primaryTopic a owl:ObjectProperty .

prv:operatedBy a owl:ObjectProperty ;
	rdfs:range prv:HumanActor ;
	rdfs:comment "This property refers to a human actor who was operating a non-human actor. For instance, a service provider operates a data providing service (see class <a xmlns=\"http://www.w3.org/1999/xhtml\" href=\"#DataProvidingService\" xml:lang=\"en\">prv:DataProvidingService</a>). Another example is a human actor who operates a non-human data creating actor."^^rdf:XMLLiteral ;
	rdfs:label "operated by"@en ;
	rdfs:isDefinedBy <http://purl.org/net/provenance/ns> ;
	rdfs:domain prv:NonHumanActor .

prv:accessedService a owl:ObjectProperty ;
	rdfs:subPropertyOf prv:involvedActor ;
	rdfs:range prv:DataProvidingService ;
	rdfs:comment "This property refers to the service that provided the document during the execution of a data access."@en ;
	rdfs:label "accessed"@en ;
	rdfs:isDefinedBy <http://purl.org/net/provenance/ns> ;
	rdfs:domain prv:DataAccess .

prv:usedGuideline a owl:ObjectProperty ;
	rdfs:subPropertyOf prv:usedData .

prv:usedData a owl:ObjectProperty ;
	rdfs:subPropertyOf prv:employedArtifact .

prv:employedArtifact a owl:ObjectProperty ;
	rdfs:range prv:Artifact ;
	rdfs:comment "This is an abstract property that refers to an artifact which was used during an execution."@en ;
	rdfs:label "used"@en ;
	rdfs:isDefinedBy <http://purl.org/net/provenance/ns> ;
	rdfs:domain prv:Execution .

prv:usedData rdfs:range prv:DataItem ;
	rdfs:comment "This property refers to a source data item that has been used during the creation of a data item. Examples for source data are the content of a document used for machine learning, the statements in a knowledge base used to entail a new statement, and the entries in a database used to answer a query. Notice, all source data has provenance; we strongly encourage to describe this provenance as well, at least as far as available information permits."@en ;
	rdfs:label "used"@en ;
	rdfs:isDefinedBy <http://purl.org/net/provenance/ns> ;
	rdfs:domain prv:DataCreation .

prv:usedGuideline rdfs:range prv:CreationGuideline .

prv:CreationGuideline a owl:Class ;
	rdfs:isDefinedBy <http://purl.org/net/provenance/ns> ;
	rdfs:comment "CreationGuideline is a class that represents a guideline used to guide the execution of a data creation. Examples for creation guidelines are transformation rules, mapping definitions, entailment rules, and database queries."@en ;
	rdfs:label "Creation Guideline"@en ;
	rdfs:subClassOf prv:DataItem .

prv:usedGuideline rdfs:comment "This property refers to a creation guideline which guided the execution of a data creation. Examples for creation guidelines are transformation rules, mapping definitions, entailment rules, and database queries. Notice, all creation guidelines have provenance; we strongly encourage to describe this provenance as well, at least as far as available information permits."@en ;
	rdfs:label "guided by"@en ;
	rdfs:isDefinedBy <http://purl.org/net/provenance/ns> ;
	rdfs:domain prv:DataCreation .

prv:containedBy a owl:ObjectProperty ;
	rdfs:range prv:Artifact ;
	rdfs:comment "This property refers to an artifact that contained a data item. This artifact can either be a host document (see class <a xmlns=\"http://www.w3.org/1999/xhtml\" href=\"#Document\" xml:lang=\"en\">prv:Document</a>) or it can be another data item of a larger granularity (e.g. an RDF statement is usually contained in an RDF graph)."^^rdf:XMLLiteral ;
	rdfs:label "contained in"@en ;
	rdfs:isDefinedBy <http://purl.org/net/provenance/ns> ;
	rdfs:domain prv:DataItem .

foaf:Document a owl:Class .

foaf:Person a owl:Class ;
	rdfs:subClassOf prv:HumanActor .

wot:Endorsement a owl:Class .

wot:PubKey a owl:Class .

<http://purl.org/net/provenance/ns#> prv:createdBy _:node183fu4jtnx2 .

_:node183fu4jtnx2 a prv:DataCreation ;
	prv:performedBy <http://users.ox.ac.uk/~zool0770/foaf.rdf#me> , <http://www.informatik.hu-berlin.de/~hartig/foaf.rdf#olaf> ;
	prv:performedAt "2009-08-25T12:00:00Z"^^xsd:dateTime .

<http://purl.org/net/provenance/ns#> prv:createdBy _:node183fu4jtnx3 .

_:node183fu4jtnx3 a prv:DataCreation ;
	prv:performedBy <http://users.ox.ac.uk/~zool0770/foaf.rdf#me> , <http://www.informatik.hu-berlin.de/~hartig/foaf.rdf#olaf> ;
	prv:performedAt "2009-08-25T12:00:00Z"^^xsd:dateTime .

<http://purl.org/net/provenance/ns#> prv:createdBy _:node183fu4jtnx4 .

_:node183fu4jtnx4 a prv:DataCreation ;
	prv:performedBy <http://users.ox.ac.uk/~zool0770/foaf.rdf#me> , <http://www.informatik.hu-berlin.de/~hartig/foaf.rdf#olaf> ;
	prv:performedAt "2009-08-25T12:00:00Z"^^xsd:dateTime .
