@prefix : <http://www.w3.org/ns/regorg#> .
@prefix wdrs: <http://www.w3.org/2007/05/powder-s#> .
@prefix foaf: <http://xmlns.com/foaf/0.1/> .
@prefix vann: <http://purl.org/vocab/vann/> .
@prefix org: <http://www.w3.org/ns/org#> .
@prefix dcterms: <http://purl.org/dc/terms/> .
@prefix sioc: <http://rdfs.org/sioc/ns#> .
@prefix schema: <http://schema.org/> .
@prefix adms: <http://www.w3.org/ns/adms#> .
@prefix rdfs: <http://www.w3.org/2000/01/rdf-schema#> .
@prefix xsd: <http://www.w3.org/2001/XMLSchema#> .
@prefix owl: <http://www.w3.org/2002/07/owl#> .
@prefix rdf: <http://www.w3.org/1999/02/22-rdf-syntax-ns#> .
@prefix skos: <http://www.w3.org/2004/02/skos/core#> .

<http://www.w3.org/ns/regorg#> a owl:Ontology ;
	rdfs:label "Registered Organization Vocabulary"@en ;
	rdfs:comment "This file specifies the set of RDF classes and properties used in the Registered Organization Vocabulary"@en ;
	owl:versionInfo "First version in w3.org/ns"@en ;
	dcterms:created "2012-07-03"^^xsd:date ;
	dcterms:modified "2013-01-08"^^xsd:date ;
	vann:preferredNamespaceUri "http://www.w3.org/ns/regorg#"@en ;
	vann:preferredNamespacePrefix "rov"@en ;
	dcterms:creator _:node17kgo8026x1 .

_:node17kgo8026x1 rdfs:seeAlso <http://philarcher.org/foaf.rdf#me> ;
	foaf:name "Phil Archer"@en ;
	foaf:homepage <http://philarcher.org/> ;
	schema:affiliation _:node17kgo8026x2 .

_:node17kgo8026x2 foaf:name "W3C/ERCIM"@en .

<http://www.w3.org/ns/regorg#> dcterms:creator _:node17kgo8026x3 .

_:node17kgo8026x3 rdfs:seeAlso <http://andrea-perego.name/foaf/#me> ;
	foaf:name "Andrea Perego"@en ;
	foaf:homepage <http://andrea-perego.name/> ;
	schema:affiliation _:node17kgo8026x4 .

_:node17kgo8026x4 foaf:name "European Commission, Joint Research Centre (JRC)"@en .

<http://www.w3.org/ns/regorg#> foaf:maker _:node17kgo8026x5 .

_:node17kgo8026x5 foaf:name "Government Linked Data WG"@en ;
	foaf:page <http://www.w3.org/2011/gld/> .

<http://www.w3.org/ns/regorg#> dcterms:abstract "This is a vocabulary for describing organizations that gain legal entity status through a formal registration process, typically in a national or regional register. This schema is defined in the Recommendations Track document at http://www.w3.org/TR/vocab-regorg"@en ;
	dcterms:description "This is the RDF schema of the Registered Organization vocabulary, originally developed under the European Commission's ISA Programme as the Core Business Vocabulary."@en ;
	wdrs:describedby <http://www.w3.org/TR/vocab-regorg/> .

<http://www.w3.org/TR/vocab-regorg/> dcterms:title "Registered Organization Vocabulary"@en .

<http://www.w3.org/ns/regorg#> dcterms:relation <http://lists.w3.org/Archives/Public/public-gld-comments/> .

<http://lists.w3.org/Archives/Public/public-gld-comments/> a sioc:Forum ;
	dcterms:title "Public GLD comments"@en .

<http://www.w3.org/ns/regorg#> dcterms:rights "Original Copyright Â© 2012 European Commission."@en .

:RegisteredOrganization a rdfs:Class , owl:Class ;
	rdfs:label "Registered Organization"@en ;
	rdfs:comment """rov:RegisteredOrganization is the key class for the Registered Organization vocabulary and represents an organization that is legally registered. In many countries there is a single registry although in others, such as Spain and Germany, multiple registries exist. A Registered Organization is able to trade, is legally liable for its actions, accounts, tax affairs etc. Legal entity status is conferred by the act of registration cf. org:FormalOrganization that applies to any legal entity, including those created by other legal means.
    This makes registered organizations distinct from the broader concept of organizations, groups or, in some jurisdictions, sole traders. Many organizations exist that are not legal entities yet to the outside world they have staff, hierarchies, locations etc. Other organizations exist that are an umbrella for several legal entities (universities are often good examples of this). This vocabulary is concerned solely with registered organizations.
    In RDF, Registered Organization is a sub class of the Organization Ontology's org:FormalOrganization which is itself a sub class of the more general 'Agent' class found in FOAF and Dublin Core that does encompass organizations, natural persons, groups etc. - i.e. an Agent is any entity that is able to carry out actions."""@en ;
	rdfs:isDefinedBy <http://www.w3.org/TR/vocab-regorg/> ;
	rdfs:subClassOf org:FormalOrganization ;
	dcterms:identifier "rov:RegisteredOrganization"@en .

:legalName a rdf:Property , owl:DatatypeProperty ;
	rdfs:label "legal name"@en ;
	rdfs:comment """The legal name of the business. A business might have more than one 
    legal name, particularly in countries with more than one official language. In such cases the 
    language of the string should be identified."""@en ;
	rdfs:range rdfs:Literal ;
	rdfs:isDefinedBy <http://www.w3.org/TR/vocab-regorg/> ;
	dcterms:identifier "rov:legalName"@en .

dcterms:alternative rdfs:label "alternative name"@en ;
	rdfs:comment """The dcterms:alternative property fully represents the 
    Registered Organization vocabulary property of alternative name. Some jurisdictions recognize concepts such as 
    a trading name or alternative forms of a legal entity's name. The alternative name property can be 
    used to record such names but should not be used to record translations of the primary legal name. 
    Where more than one legal name exists and where they have equal standing but are expressed in 
    different languages, identify the language used in each of the multiple legal names."""@en ;
	rdfs:isDefinedBy <http://www.w3.org/ns/dublincore.org/documents/dcmi-terms/> ;
	dcterms:identifier "dcterms:alternative"@en .

:companyType a rdf:Property , owl:ObjectProperty ;
	rdfs:label "company type"@en ;
	rdfs:comment """This property records the type of company. Familiar types are SA, PLC, LLC, GmbH etc. Each 
    jurisdiction will have a limited set of recognized company types and these should be used in a consistent manner
    using a SKOS Concept Scheme. rov:companyType is a sub class of org:classification which has a range of skos:Concept."""@en ;
	rdfs:isDefinedBy <http://www.w3.org/TR/vocab-regorg/> ;
	rdfs:subPropertyOf org:classification ;
	dcterms:identifier "rov:companyType"@en .

:companyStatus a rdf:Property , owl:ObjectProperty ;
	rdfs:label "company status"@en ;
	rdfs:comment """Terms like insolvent, bankrupt and in receivership are likely to have 
    different legal implications in different jurisdictions. Best Practice for recording various 
    other status levels is to use the relevant jurisdiction's terms and to do so in a 
    consistent manner using a SKOS Concept Scheme. rov:companyStatus is a sub class of org:classification
    which has a range of skos:Concept."""@en ;
	rdfs:isDefinedBy <http://www.w3.org/TR/vocab-regorg/> ;
	rdfs:subPropertyOf org:classification ;
	dcterms:identifier "rov:companyStatus"@en .

:companyActivity a rdf:Property , owl:ObjectProperty ;
	rdfs:label "company activity"@en ;
	rdfs:comment """The activity of a company should be 
    recorded using a controlled vocabulary expressed as a SKOS concept scheme. Several such 
    vocabularies exist, many of which map to the UN's ISIC codes. Where a particular controlled vocabulary is in use 
    within a given context, such as SIC codes in the UK, it is acceptable to use these, however, the preferred 
    choice for European interoperability is NACE. rov:companyActivity is a sub class of org:classification which has a range of skos:Concept."""@en ;
	rdfs:isDefinedBy <http://www.w3.org/TR/vocab-regorg/> ;
	rdfs:subPropertyOf org:classification ;
	dcterms:identifier "rov:companyActivity"@en .

:registration a rdf:Property , owl:ObjectProperty ;
	rdfs:label "registration"@en ;
	rdfs:comment """The legal status of a registered organization is conferred on it by an authority within a given 
    jurisdiction. The registration is therefore a fundamental relationship between a the organization and the authority with 
    which it is registered. The details of the registration are provided as properties of the Identifier class which is 
    defined by ADMS. The vocabulary sets no restriction on the type of legal identifier. In many countries, the business register's 
    identifier is the relevant data point. The tax number often fulfils this function in Spain and elsewhere.
    Although there is no formal cardinality constraint on any property in the Registered Organization Vocabulary, it is 
    questionable whether a description of a registered organization without this property and an associated Identifier class will 
    be of any value."""@en ;
	rdfs:isDefinedBy <http://www.w3.org/ns/regorg#> ;
	rdfs:domain :RegisteredOrganization ;
	rdfs:subPropertyOf adms:identifier ;
	dcterms:identifier "rov:registration"@en .

:registeredOrganization a rdf:Property , owl:ObjectProperty ;
	rdfs:label "registered organization"@en ;
	rdfs:comment """The registered organization relationship can be used to link any dcterms:Agent (equivalent class foaf:Agent)
    to a Registered Organization that in some way acts as a registered legal entity for it. This is useful, for example, 
    where an organization includes one or more legal entities, or where a natural person is also registered as a legal entity.
    rov:registeredOrganization has a range of rov:RegisteredOrganization."""@en ;
	rdfs:isDefinedBy <http://www.w3.org/TR/vocab-regorg/> ;
	rdfs:domain dcterms:Agent ;
	rdfs:range :RegisteredOrganization ;
	dcterms:identifier "rov:registeredOrganization"@en .

<http://www.w3.org/ns/regorg#> dcterms:creator _:node17kgo8026x6 .

_:node17kgo8026x6 rdfs:seeAlso <http://philarcher.org/foaf.rdf#me> ;
	foaf:name "Phil Archer"@en ;
	foaf:homepage <http://philarcher.org/> ;
	schema:affiliation _:node17kgo8026x7 .

_:node17kgo8026x7 foaf:name "W3C/ERCIM"@en .

<http://www.w3.org/ns/regorg#> dcterms:creator _:node17kgo8026x8 .

_:node17kgo8026x8 rdfs:seeAlso <http://andrea-perego.name/foaf/#me> ;
	foaf:name "Andrea Perego"@en ;
	foaf:homepage <http://andrea-perego.name/> ;
	schema:affiliation _:node17kgo8026x9 .

_:node17kgo8026x9 foaf:name "European Commission, Joint Research Centre (JRC)"@en .

<http://www.w3.org/ns/regorg#> foaf:maker _:node17kgo8026x10 .

_:node17kgo8026x10 foaf:name "Government Linked Data WG"@en ;
	foaf:page <http://www.w3.org/2011/gld/> .
