@prefix adms:  <http://www.w3.org/ns/adms#> .
@prefix dc:    <http://purl.org/dc/elements/1.1/> .
@prefix rdfs:  <http://www.w3.org/2000/01/rdf-schema#> .
@prefix foaf:  <http://xmlns.com/foaf/0.1/> .
@prefix search: <http://sindice.com/vocab/search#> .
@prefix owl:   <http://www.w3.org/2002/07/owl#> .
@prefix xsd:   <http://www.w3.org/2001/XMLSchema#> .
@prefix rdf:   <http://www.w3.org/1999/02/22-rdf-syntax-ns#> .
@prefix vann:  <http://purl.org/vocab/vann/> .
@prefix dcterms: <http://purl.org/dc/terms/> .

<http://vocab.deri.ie/search#Digital%20Enterprise%20Research%20Institute%2C%20NUI%20Galway>
        a              dcterms:Agent ;
        foaf:homepage  <http://www.deri.ie/> ;
        foaf:member    <http://vocab.deri.ie/search#cygri> ;
        foaf:name      "Digital Enterprise Research Institute, NUI Galway" .

search:page  a        rdf:Property ;
        rdfs:comment  "A link from a paged list of search results to one page within that list" ;
        rdfs:domain   rdfs:Resource ;
        rdfs:label    "Page" ;
        rdfs:range    rdfs:Resource .

search:startIndex  a  owl:DatatypeProperty , rdf:Property ;
        rdfs:comment  "The rank (or index) of the first result on a page of search results" ;
        rdfs:domain   rdfs:Resource ;
        rdfs:label    "Start Index" ;
        rdfs:range    xsd:integer .

search:previous  a    rdf:Property ;
        rdfs:comment  "A link from one page of a paged search result to the preceding page" ;
        rdfs:domain   rdfs:Resource ;
        rdfs:label    "Previous" ;
        rdfs:range    rdfs:Resource .

search:itemsPerPage  a  owl:DatatypeProperty , rdf:Property ;
        rdfs:comment  "The number of items found on each page in a paged list of search results" ;
        rdfs:domain   rdfs:Resource ;
        rdfs:label    "Items per Page" ;
        rdfs:range    xsd:integer .

<http://vocab.deri.ie/search#cygri>
        a              foaf:Person ;
        foaf:homepage  <http://richard.cyganiak.de/> ;
        foaf:mbox      <mailto:richard.cyganiak@deri.org> ;
        foaf:name      "Richard Cyganiak" .

search:openSearchDescription
        a             rdf:Property ;
        rdfs:comment  "A link to an OpenSearch XML description of a search service" ;
        rdfs:domain   rdfs:Resource ;
        rdfs:label    "OpenSearch Description" ;
        rdfs:range    rdfs:Resource .

search:first  a       rdf:Property ;
        rdfs:comment  "A link to the first page of results to a search query" ;
        rdfs:domain   rdfs:Resource ;
        rdfs:label    "First" ;
        rdfs:range    rdfs:Resource .

search:link  a        rdf:Property ;
        rdfs:comment  "A link to a resource that was found as a search result" ;
        rdfs:domain   rdfs:Resource ;
        rdfs:label    "Link" ;
        rdfs:range    rdfs:Resource .

<http://vocab.deri.ie/search#rdf>
        a                   adms:SemanticDistribution ;
        dcterms:FileFormat  <http://vocab.deri.ie/search> ;
        adms:accessURL      "http://vocab.deri.ie/search.rdf" ;
        adms:status         <http://purl.org/adms/status/Completed> .

search:totalResults  a  owl:DatatypeProperty , rdf:Property ;
        rdfs:comment  "The total number of results of a search query" ;
        rdfs:domain   rdfs:Resource ;
        rdfs:label    "Total Results" ;
        rdfs:range    xsd:integer .

search:last  a        rdf:Property ;
        rdfs:comment  "A link to the last page of results to a search query" ;
        rdfs:domain   rdfs:Resource ;
        rdfs:label    "Last" ;
        rdfs:range    rdfs:Resource .

<http://vocab.deri.ie/search#ttl>
        a                   adms:SemanticDistribution ;
        dcterms:FileFormat  <http://vocab.deri.ie/search> ;
        adms:accessURL      "http://vocab.deri.ie/search.ttl" ;
        adms:status         <http://purl.org/adms/status/Completed> .

search:cache  a       rdf:Property ;
        rdfs:comment  "Link to a cached copy of a search result" ;
        rdfs:domain   rdfs:Resource ;
        rdfs:label    "Cache" ;
        rdfs:range    rdfs:Resource .

search:searchTerms  a  owl:DatatypeProperty , rdf:Property ;
        rdfs:comment  "The search terms used in a search query" ;
        rdfs:domain   rdfs:Resource ;
        rdfs:label    "Search Terms" ;
        rdfs:range    rdfs:Literal .

search:rank  a        owl:DatatypeProperty , rdf:Property ;
        rdfs:comment  "The rank (or index) of an individual search result item within the list of search results" ;
        rdfs:domain   rdfs:Resource ;
        rdfs:label    "Rank" ;
        rdfs:range    xsd:integer .

search:Result  a      owl:Class , rdfs:Class ;
        rdfs:comment  "An individual result in a list of ranked search results to a search query" ;
        rdfs:label    "Result" .

search:Page  a        owl:Class , rdfs:Class ;
        rdfs:comment  "A page in a paged list of search results" ;
        rdfs:label    "Page" .

search:result  a      rdf:Property ;
        rdfs:comment  "A link from a search query to an individual search result of that query" ;
        rdfs:domain   rdfs:Resource ;
        rdfs:label    "Result" ;
        rdfs:range    rdfs:Resource .

<http://vocab.deri.ie/search>
        a                              owl:Ontology , adms:SemanticAsset ;
        dc:creator                     <http://vocab.deri.ie/search#cygri> ;
        dcterms:created                "2010-09-26"^^xsd:date ;
        dcterms:description            "A vocabulary for ranked search results, for use in the Sindice API." ;
        dcterms:modified               "2010-09-26"^^xsd:date ;
        dcterms:partOf                 <http://vocab.deri.ie> ;
        dcterms:publisher              "http://vocab.deri.ie/search#Digital%20Enterprise%20Research%20Institute%2C%20NUI%20Galway" ;
        dcterms:status                 <http://purl.org/adms/status/UnderDevelopment> ;
        dcterms:title                  "Sindice Search Vocabulary" ;
        dcterms:type                   <http://purl.org/adms/assettype/Ontology> ;
        vann:preferredNamespacePrefix  "search" ;
        vann:preferredNamespaceUri     "http://sindice.com/vocab/search#" ;
        foaf:homepage                  <http://vocab.deri.ie/search.html> .

search:Query  a       owl:Class , rdfs:Class ;
        rdfs:comment  "A search query" ;
        rdfs:label    "Query" .

search:next  a        rdf:Property ;
        rdfs:comment  "A link from one page of a paged search result to the following page" ;
        rdfs:domain   rdfs:Resource ;
        rdfs:label    "Next" ;
        rdfs:range    rdfs:Resource .
