@prefix rdfs:  <http://www.w3.org/2000/01/rdf-schema#> .
@prefix swp:   <http://www.w3.org/2004/03/trix/swp-1/> .
@prefix xsd:   <http://www.w3.org/2001/XMLSchema#> .
@prefix rdf:   <http://www.w3.org/1999/02/22-rdf-syntax-ns#> .
@prefix rdfg:  <http://www.w3.org/2004/03/trix/rdfg-1/> .

swp:signatureMethod  a  rdf:Property ;
        rdfs:comment  "\nThe object is the signature method by which  the signature specified for the\nwarrant subject was constructed.\n      " ;
        rdfs:domain   swp:Warrant ;
        rdfs:label    "signature method" ;
        rdfs:range    swp:SignatureMethod .

swp:Warrant  a        rdfs:Class ;
        rdfs:comment  "\nA relationship between an authority and a graph, in which the authority is in\nsome way an origin of that graph. Warrants may include a digital signature of\nthe graph by the authority.\n      " ;
        rdfs:label    "Warrant" .

swp:signature  a      rdf:Property ;
        rdfs:comment  "\nThe object is the signature to be used to authenticate the graph with which the\nsubject warrant is associated.\n      " ;
        rdfs:domain   swp:Warrant ;
        rdfs:label    "signature" ;
        rdfs:range    xsd:base64Binary .

swp:Authority  a      rdfs:Class ;
        rdfs:comment  "\nAn authority, or origin, of a graph; such as a person or company.\n      " ;
        rdfs:label    "Authority" .

swp:authority  a      rdf:Property ;
        rdfs:comment  "\nThe object authority is the origin of the graph with which the subject warrant\nis associated.\n      " ;
        rdfs:domain   swp:Warrant ;
        rdfs:label    "authority" ;
        rdfs:range    swp:Authority .

swp:assertedBy  a     rdf:Property ;
        rdfs:comment  "\nThe subject graph originates from and is asserted by the authority specified\nfor the object warrant. The statements expressed in the graph are taken to be\nclaims made by that authority. This property has performative semantics.\n      " ;
        rdfs:domain   rdfg:Graph ;
        rdfs:label    "asserted by" ;
        rdfs:range    swp:Warrant .

swp:certificate  a    rdf:Property ;
        rdfs:comment  "\nThe object is a certificate by which the authority specified for the warrant\ncan be authenticated.\n      " ;
        rdfs:domain   swp:Warrant ;
        rdfs:label    "certificate" ;
        rdfs:range    xsd:base64Binary .

swp:SignatureMethod  a  rdfs:Class ;
        rdfs:comment  "\nA method used to construct a signature used to authenticate a graph.\n      " ;
        rdfs:label    "Signature Method" .

swp:quotedBy  a       rdf:Property ;
        rdfs:comment  "\nThe subject graph originates from the authority specified for the object warrant.\nThe statements expressed in the graph are not taken to be claims made by that\nauthority, insofar as any statement using this property is concerned.\n      " ;
        rdfs:domain   rdfg:Graph ;
        rdfs:label    "quoted by" ;
        rdfs:range    swp:Warrant .
